@prefix owl:   <http://www.w3.org/2002/07/owl#> .
@prefix rdf:   <http://www.w3.org/1999/02/22-rdf-syntax-ns#> .
@prefix cap-iacs-basecode: <http://lpis.ec.europa.eu/registry/applicationschema/cap-iacs-base/code#> .
@prefix xsd:   <http://www.w3.org/2001/XMLSchema#> .
@prefix skos:  <http://www.w3.org/2004/02/skos/core#> .
@prefix rdfs:  <http://www.w3.org/2000/01/rdf-schema#> .
@prefix cap-iacs-base: <http://lpis.ec.europa.eu/registry/applicationschema/cap-iacs-base#> .
@prefix foaf:  <http://xmlns.com/foaf/0.1/> .
@prefix dct:   <http://purl.org/dc/terms/> .
@prefix schema: <http://schema.org/> .


<http://lpis.ec.europa.eu/registry/applicationschema/cap-iacs-base/code#CropItemCodeValue/redCurrants>
        a                cap-iacs-base:CropItemCodeValue ;
        rdfs:label       "Red currants"@en ;
        skos:definition  "-- Definition --\r\n||||Red currants.\r\n-- Description --\r\nCereals and main crops - C\r\nNOTE. Initial value:C2275"@en ;
        skos:inScheme    cap-iacs-basecode:CropItemCodeValue .

<http://lpis.ec.europa.eu/registry/applicationschema/cap-iacs-base/code#ConformanceRequirementClassValue/conditional>
        a                cap-iacs-base:ConformanceRequirementClassValue ;
        rdfs:label       "Conditional requirement"@en ;
        skos:definition  "--Name--\r\nConditional\r\n\r\n--Definition--\r\nRequirement that shall be observed if the conditions set out in the specification apply."@en ;
        skos:inScheme    cap-iacs-basecode:ConformanceRequirementClassValue .

<http://lpis.ec.europa.eu/registry/applicationschema/cap-iacs-base/code#CropItemCodeValue/commonSpringWheat>
        a                cap-iacs-base:CropItemCodeValue ;
        rdfs:label       "Common spring wheat"@en ;
        skos:definition  "-- Definition --\r\n|||||Common spring wheat.\r\n-- Description --\r\nCereals and main crops - C\r\nNOTE. Initial value:C1124"@en ;
        skos:inScheme    cap-iacs-basecode:CropItemCodeValue .

<http://lpis.ec.europa.eu/registry/applicationschema/cap-iacs-base/code#SpecieCodeValue/alliumPorrumLLeek>
        a                cap-iacs-base:SpecieCodeValue ;
        rdfs:label       "Allium porrum L. Leek"@en ;
        skos:definition  "-- Definition --\r\nAllium porrum L. Leek.\r\n-- Description --\r\nList of vegetable specie -H\r\nNOTE. Initial value: H - 3."@en ;
        skos:inScheme    cap-iacs-basecode:SpecieCodeValue .

<http://lpis.ec.europa.eu/registry/applicationschema/cap-iacs-base/code#SpecieCodeValue/apiumGraveolensLCelery>
        a                cap-iacs-base:SpecieCodeValue ;
        rdfs:label       "Apium graveolens L. Celery"@en ;
        skos:definition  "-- Definition --\r\nApium graveolens L. Celery.\r\n-- Description --\r\nList of vegetable specie -H\r\nNOTE. Initial value: H - 7.1"@en ;
        skos:inScheme    cap-iacs-basecode:SpecieCodeValue .

<http://lpis.ec.europa.eu/registry/applicationschema/cap-iacs-base/code#StatusOfIssueValue/open>
        a                cap-iacs-base:StatusOfIssueValue ;
        rdfs:label       "Open"@en ;
        skos:definition  "--Name--\r\nOpen\r\n\r\n-- Definition --\r\nStatus of issue after recording it in the information system."@en ;
        skos:inScheme    cap-iacs-basecode:StatusOfIssueValue .

<http://lpis.ec.europa.eu/registry/applicationschema/cap-iacs-base/code#CropItemCodeValue/cerealsHarvestedGreen>
        a                cap-iacs-base:CropItemCodeValue ;
        rdfs:label       "Cereals harvested green"@en ;
        skos:definition  "-- Definition --\r\n|||Cereals harvested green.\r\n-- Description --\r\nCereals and main crops - C\r\nNOTE. Initial value:C2626"@en ;
        skos:inScheme    cap-iacs-basecode:CropItemCodeValue .

<http://lpis.ec.europa.eu/registry/applicationschema/cap-iacs-base/code#SpecieCodeValue/alliumSativumLGarlic>
        a                cap-iacs-base:SpecieCodeValue ;
        rdfs:label       "Allium sativum L. Garlic"@en ;
        skos:definition  "-- Definition --\r\nAllium sativum L. Garlic.\r\n-- Description --\r\nList of vegetable specie -H\r\nNOTE. Initial value: H - 4."@en ;
        skos:inScheme    cap-iacs-basecode:SpecieCodeValue .

<http://lpis.ec.europa.eu/registry/applicationschema/cap-iacs-base/code#SpecieCodeValue/carumCarviLCaraway>
        a                cap-iacs-base:SpecieCodeValue ;
        rdfs:label       "Carum carvi L. Caraway"@en ;
        skos:definition  "-- Definition --\r\nCarum carvi L. Caraway.\r\n-- Description --\r\nList of agricultural species -A\r\nIII. Oil and fibre plants\r\nNOTE. Initial value: A - 65."@en ;
        skos:inScheme    cap-iacs-basecode:SpecieCodeValue .

<http://lpis.ec.europa.eu/registry/applicationschema/cap-iacs-base/code#SpecieCodeValue/cucumisSativusLGherkin>
        a                cap-iacs-base:SpecieCodeValue ;
        rdfs:label       "Cucumis sativus L. Gherkin"@en ;
        skos:definition  "-- Definition --\r\nCucumis sativus L. Gherkin.\r\n-- Description --\r\nList of vegetable specie -H\r\nNOTE. Initial value: H - 17.2"@en ;
        skos:inScheme    cap-iacs-basecode:SpecieCodeValue .

<http://lpis.ec.europa.eu/registry/applicationschema/cap-iacs-base/code#SpecieCodeValue/trifoliumAlexandrinumLBerseemEgyptian>
        a                cap-iacs-base:SpecieCodeValue ;
        rdfs:label       "Trifolium alexandrinum L. Berseem/Egyptian"@en ;
        skos:definition  "-- Definition --\r\nTrifolium alexandrinum L. Berseem/Egyptian.\r\n-- Description --\r\nList of agricultural species -A\r\nII. Fodder plants\r\nNOTE. Initial value: A - 43."@en ;
        skos:inScheme    cap-iacs-basecode:SpecieCodeValue .

<http://lpis.ec.europa.eu/registry/applicationschema/cap-iacs-base/code#FarmStructureSurveyNumberValue/plantsHarvestedGreen>
        a                cap-iacs-base:FarmStructureSurveyNumberValue ;
        rdfs:label       "Plants harvested green"@en ;
        skos:definition  "-- Definition --\r\nPlants harvested green.\r\n-- Description --\r\nAll ‘green’ arable crops intended mainly for animal feed, grown in rotation with other crops and occupying the same parcel for less than five years (annual or multiannual fodder crops).\r\nGreen crops used for renewable energy production are included.\r\nCrops not used on the holding but sold, either for direct use on other agricultural holdings or to industry, are included.\r\nNOTE. Initial value:2.01.09"@en ;
        skos:inScheme    cap-iacs-basecode:FarmStructureSurveyNumberValue .

<http://lpis.ec.europa.eu/registry/applicationschema/cap-iacs-base/code#CropItemCodeValue/strawberriesUnderGlassOrHighAccessibleCoverC2261>
        a                cap-iacs-base:CropItemCodeValue ;
        rdfs:label       "Strawberries under glass or high accessible cover C2261 "@en ;
        skos:definition  "-- Definition --\r\n|||Strawberries under glass or high accessible cover C2261.\r\n-- Description --\r\nCereals and main crops - C\r\nNOTE. Initial value:C2261"@en ;
        skos:inScheme    cap-iacs-basecode:CropItemCodeValue .

cap-iacs-basecode:ConformanceStatementValue
        a                skos:ConceptScheme ;
        rdfs:label       "List of conformance statement values"@en ;
        dct:isFormatOf   cap-iacs-base:ConformanceStatementValue ;
        skos:definition  "--Name--\r\nConformance Statement Value\r\n\r\n-- Definition --\r\nEnumeration of conformance statement values.\r\n\r\n-- Description --\r\nList of possible conformance verdicts whether the subject of testing (e.g. SUT, schema element, source data, etc.) conforms to the specified rules."@en .

<http://lpis.ec.europa.eu/registry/applicationschema/cap-iacs-base/code#SpecieCodeValue/lactucaSativaLLettuce>
        a                cap-iacs-base:SpecieCodeValue ;
        rdfs:label       "Lactuca sativa L. Lettuce"@en ;
        skos:definition  "-- Definition --\r\nLactuca sativa L. Lettuce.\r\n-- Description --\r\nList of vegetable specie -H\r\nNOTE. Initial value: H - 23."@en ;
        skos:inScheme    cap-iacs-basecode:SpecieCodeValue .

<http://lpis.ec.europa.eu/registry/applicationschema/cap-iacs-base/code#MonthValue/march>
        a                cap-iacs-base:MonthValue ;
        rdfs:label       "March"@en ;
        skos:definition  "-- Definition --\r\nMarch.\r\n-- Description --\r\nItem description."@en ;
        skos:inScheme    cap-iacs-basecode:MonthValue .

<http://lpis.ec.europa.eu/registry/applicationschema/cap-iacs-base/code#SpecieCodeValue/solanumTuberosumLPotato>
        a                cap-iacs-base:SpecieCodeValue ;
        rdfs:label       "Solanum tuberosum L. Potato"@en ;
        skos:definition  "-- Definition --\r\nSolanum tuberosum L. Potato.\r\n-- Description --\r\nList of agricultural species -A   \r\nV. Potatoes\r\nNOTE. Initial value: A - 87."@en ;
        skos:inScheme    cap-iacs-basecode:SpecieCodeValue .

<http://lpis.ec.europa.eu/registry/applicationschema/cap-iacs-base/code#CropItemCodeValue/hazelnuts>
        a                cap-iacs-base:CropItemCodeValue ;
        rdfs:label       "Hazelnuts"@en ;
        skos:definition  "-- Definition --\r\n|||Hazelnuts.\r\n-- Description --\r\nCereals and main crops - C\r\nNOTE. Initial value:C2232"@en ;
        skos:inScheme    cap-iacs-basecode:CropItemCodeValue .

<http://lpis.ec.europa.eu/registry/applicationschema/cap-iacs-base/code#CropItemCodeValue/triticale>
        a                cap-iacs-base:CropItemCodeValue ;
        rdfs:label       "Triticale"@en ;
        skos:definition  "-- Definition --\r\n|||Triticale.\r\n-- Description --\r\nCereals and main crops - C\r\nNOTE. Initial value:C1212"@en ;
        skos:inScheme    cap-iacs-basecode:CropItemCodeValue .

<http://lpis.ec.europa.eu/registry/applicationschema/cap-iacs-base/code#CropItemCodeValue/otherAnnualPlantsHarvestedGreenNecC2612>
        a                cap-iacs-base:CropItemCodeValue ;
        rdfs:label       "Other annual plants harvested green n.e.c. C2612"@en ;
        skos:definition  "-- Definition --\r\n|||Other annual plants harvested green n.e.c. C2612.\r\n-- Description --\r\nCereals and main crops - C\r\nNOTE. Initial value:C2612"@en ;
        skos:inScheme    cap-iacs-basecode:CropItemCodeValue .

<http://lpis.ec.europa.eu/registry/applicationschema/cap-iacs-base/code#SpecieCodeValue/arrhenatherumElatiusLTallOatgrass>
        a                cap-iacs-base:SpecieCodeValue ;
        rdfs:label       "Arrhenatherum elatius L. Tall oatgrass "@en ;
        skos:definition  "-- Definition --\r\nArrhenatherum elatius L. Tall oatgrass.\r\n-- Description --\r\nList of agricultural species -A\r\nII. Fodder plants\r\nNOTE. Initial value: A - 8."@en ;
        skos:inScheme    cap-iacs-basecode:SpecieCodeValue .

<http://lpis.ec.europa.eu/registry/applicationschema/cap-iacs-base/code#CropItemCodeValue/pomelosAndGrapefruitC2380>
        a                cap-iacs-base:CropItemCodeValue ;
        rdfs:label       "Pomelos and grapefruit C2380"@en ;
        skos:definition  "-- Definition --\r\n|||Pomelos and grapefruit C2380.\r\n-- Description --\r\nCereals and main crops - C\r\nNOTE. Initial value:C2380"@en ;
        skos:inScheme    cap-iacs-basecode:CropItemCodeValue .

cap-iacs-basecode:StatusOfAnomalyValue
        a                skos:ConceptScheme ;
        rdfs:label       "Anomaly status value list"@en ;
        dct:isFormatOf   cap-iacs-base:StatusOfAnomalyValue ;
        skos:definition  "--Name--\r\nStatus of anomaly value\r\n\r\n-- Definition --\r\nCode list of possible anomaly status values.\r\n\r\n-- Description --\r\nList of possible anomaly status values used for documentation of anomaly in the information system.\r\n\r\nNOTE. Under information system IACS is understood. Most probably anomalies are registered in the Integrated control systems or in the quality assessment leaf of LPIS QA."@en .

<http://lpis.ec.europa.eu/registry/applicationschema/cap-iacs-base/code#CropItemCodeValue/fibreFlax>
        a                cap-iacs-base:CropItemCodeValue ;
        rdfs:label       "Fibre flax"@en ;
        skos:definition  "-- Definition --\r\n|||Fibre flax.\r\n-- Description --\r\nCereals and main crops - C\r\nNOTE. Initial value:C1520"@en ;
        skos:inScheme    cap-iacs-basecode:CropItemCodeValue .

cap-iacs-basecode:WeekdayValue
        a                skos:ConceptScheme ;
        rdfs:label       "List of weekday values"@en ;
        dct:isFormatOf   cap-iacs-base:WeekdayValue ;
        skos:definition  "-- Definition --\r\nList of possible weekdays.\r\n-- Description --\r\nList of possible weekdays."@en .

<http://lpis.ec.europa.eu/registry/applicationschema/cap-iacs-base/code#SpecieCodeValue/rheumRhabarbarumLRhubarb>
        a                cap-iacs-base:SpecieCodeValue ;
        rdfs:label       "Rheum rhabarbarum L. Rhubarb"@en ;
        skos:definition  "-- Definition --\r\nRheum rhabarbarum L. Rhubarb.\r\n-- Description --\r\nList of vegetable specie -H\r\nNOTE. Initial value: H - 30."@en ;
        skos:inScheme    cap-iacs-basecode:SpecieCodeValue .

<http://lpis.ec.europa.eu/registry/applicationschema/cap-iacs-base/code#FarmStructureSurveyNumberValue/otherCerealsForTheProductionOfGrain>
        a                cap-iacs-base:FarmStructureSurveyNumberValue ;
        rdfs:label       "Other cereals for the production of grain"@en ;
        skos:definition  "-- Definition --\r\nOther cereals for the production of grain.\r\n-- Description --\r\nCereals sown in pure crops, harvested dry for grain, and that are not recorded elsewhere under the previous items.\r\nNOTE. Initial value:2.01.01.99"@en ;
        skos:inScheme    cap-iacs-basecode:FarmStructureSurveyNumberValue .

<http://lpis.ec.europa.eu/registry/applicationschema/cap-iacs-base/code#VarietalNameValue/accent>
        a                cap-iacs-base:VarietalNameValue ;
        rdfs:label       "H - 1.2  Accent"@en ;
        skos:definition  "-- Definition --\r\nH - 1.2  Accent\r\n-- Description --\r\nH - 1.2 Allium cepa L. Cepa group - Onion, Echalion /  Accent.\r\nNOTE. Initial value: Accent\r\nNOTE. MS - NL (Netherlands)."@en ;
        skos:inScheme    cap-iacs-basecode:VarietalNameValue .

<http://lpis.ec.europa.eu/registry/applicationschema/cap-iacs-base/code#SpecieCodeValue/festucaArundinaceaSchreberTallFescue>
        a                cap-iacs-base:SpecieCodeValue ;
        rdfs:label       "Festuca arundinacea Schreber Tall fescue"@en ;
        skos:definition  "-- Definition --\r\nFestuca arundinacea Schreber Tall fescue.\r\n-- Description --\r\nList of agricultural species -A\r\nII. Fodder plants\r\nNOTE. Initial value: A - 13."@en ;
        skos:inScheme    cap-iacs-basecode:SpecieCodeValue .

<http://lpis.ec.europa.eu/registry/applicationschema/cap-iacs-base/code#CropItemCodeValue/walnuts>
        a                cap-iacs-base:CropItemCodeValue ;
        rdfs:label       "Walnuts"@en ;
        skos:definition  "-- Definition --\r\n|||Walnuts.\r\n-- Description --\r\nCereals and main crops - C\r\nNOTE. Initial value:C2231"@en ;
        skos:inScheme    cap-iacs-basecode:CropItemCodeValue .

<http://lpis.ec.europa.eu/registry/applicationschema/cap-iacs-base/code#FarmStructureSurveyNumberValue/normallyProducingOlivesForOilProduction>
        a                cap-iacs-base:FarmStructureSurveyNumberValue ;
        rdfs:label       "Normally producing olives for oil production"@en ;
        skos:definition  "-- Definition --\r\nNormally producing olives for oil production.\r\n-- Description --\r\nPlantations of varieties normally grown for producing olive oil.\r\nNOTE. Initial value:2.04.03.02"@en ;
        skos:inScheme    cap-iacs-basecode:FarmStructureSurveyNumberValue .

<http://lpis.ec.europa.eu/registry/applicationschema/cap-iacs-base/code#CropItemCodeValue/asparagus>
        a                cap-iacs-base:CropItemCodeValue ;
        rdfs:label       "Asparagus"@en ;
        skos:definition  "-- Definition --\r\n|||Asparagus.\r\n-- Description --\r\nCereals and main crops - C\r\nNOTE. Initial value:C1700"@en ;
        skos:inScheme    cap-iacs-basecode:CropItemCodeValue .

<http://lpis.ec.europa.eu/registry/applicationschema/cap-iacs-base/code#FarmStructureSurveyNumberValue/permanentCrops>
        a                cap-iacs-base:FarmStructureSurveyNumberValue ;
        rdfs:label       "Permanent crops"@en ;
        skos:definition  "-- Definition --\r\nPermanent crops.\r\n-- Description --\r\nCrops not grown in rotation, other than permanent grassland, which occupy the soil for a long period and yield crops over several years.\r\nNOTE. Initial value:2.04"@en ;
        skos:inScheme    cap-iacs-basecode:FarmStructureSurveyNumberValue .

<http://lpis.ec.europa.eu/registry/applicationschema/cap-iacs-base/code#NotificationGroupValue/notificationsRelatingToSapsDecisionsOnTransitionalNationalAid>
        a                cap-iacs-base:NotificationGroupValue ;
        rdfs:label       "Notifications relating to SAPS decisions on transitional national aid"@en ;
        skos:definition  "-- Definition --\r\nNotifications relating to SAPS decisions on transitional national aid.\r\n-- Description --\r\nNOTE.74"@en ;
        skos:inScheme    cap-iacs-basecode:NotificationGroupValue .

<http://lpis.ec.europa.eu/registry/applicationschema/cap-iacs-base/code#NotificationGroupValue/notificationsRelatingToDefinitionsAndRelatedProvisions>
        a                cap-iacs-base:NotificationGroupValue ;
        rdfs:label       "Notifications relating to definitions and related provisions"@en ;
        skos:definition  "-- Definition --\r\nNotifications relating to definitions and related provisions.\r\n-- Description --\r\nNOTE.61"@en ;
        skos:inScheme    cap-iacs-basecode:NotificationGroupValue .

<http://lpis.ec.europa.eu/registry/applicationschema/cap-iacs-base/code#CropItemCodeValue/nectarines>
        a                cap-iacs-base:CropItemCodeValue ;
        rdfs:label       "Nectarines"@en ;
        skos:definition  "-- Definition --\r\n|||Nectarines.\r\n-- Description --\r\nCereals and main crops - C\r\nNOTE. Initial value:C2221"@en ;
        skos:inScheme    cap-iacs-basecode:CropItemCodeValue .

<http://lpis.ec.europa.eu/registry/applicationschema/cap-iacs-base/code#CropItemCodeValue/leguminousPlants>
        a                cap-iacs-base:CropItemCodeValue ;
        rdfs:label       "Leguminous plants"@en ;
        skos:definition  "-- Definition --\r\n||Leguminous plants.\r\n-- Description --\r\nCereals and main crops - C\r\nNOTE. Initial value:C2670"@en ;
        skos:inScheme    cap-iacs-basecode:CropItemCodeValue .

<http://lpis.ec.europa.eu/registry/applicationschema/cap-iacs-base/code#StatusOfAnomalyValue/open>
        a                cap-iacs-base:StatusOfAnomalyValue ;
        rdfs:label       "Open"@en ;
        skos:definition  "--Name--\r\nOpen\r\n\r\n-- Definition --\r\nStatus of anomaly after recording it in the information system."@en ;
        skos:inScheme    cap-iacs-basecode:StatusOfAnomalyValue .

cap-iacs-basecode:RecurenceValue
        a                skos:ConceptScheme ;
        rdfs:label       "List of recurence values"@en ;
        dct:isFormatOf   cap-iacs-base:RecurenceValue ;
        skos:definition  "-- Definition --\r\nNotification recurrence value list.\r\n-- Description --\r\nList of possible notification recurrence values."@en .

<http://lpis.ec.europa.eu/registry/applicationschema/cap-iacs-base/code#SpecieCodeValue/festucaOvinaLSheepsFescue>
        a                cap-iacs-base:SpecieCodeValue ;
        rdfs:label       "Festuca ovina L. Sheep's fescue"@en ;
        skos:definition  "-- Definition --\r\nFestuca ovina L. Sheep's fescue.\r\n-- Description --\r\nList of agricultural species -A\r\nII. Fodder plants\r\nNOTE. Initial value: A - 15."@en ;
        skos:inScheme    cap-iacs-basecode:SpecieCodeValue .

<http://lpis.ec.europa.eu/registry/applicationschema/cap-iacs-base/code#SupportSchemeTypeValue/paymentForAgriculturalPracticesBeneficialForTheClimateAndTheEnvironment>
        a                cap-iacs-base:SupportSchemeTypeValue ;
        rdfs:label       "Payment for agricultural practices beneficial for the climate and the environment"@en ;
        skos:definition  "Payment for agricultural practices beneficial for the climate and the environment \r\n\r\nFarmers entitled to a payment under the basic payment scheme or the single area payment scheme shall observe, on all their eligible hectares within the meaning of Article 32(2) to (5), the agricultural practices beneficial for the climate and the environment referred to in paragraph 2 of this Article or the equivalent practices referred to in paragraph 3 of this Article.\r\n\r\nAccording to Title III, Chapter 3 of 1307/2013 Regulation  it is a decoupled payment. Also known as the Green Payment."@en ;
        skos:inScheme    cap-iacs-basecode:SupportSchemeTypeValue .

<http://lpis.ec.europa.eu/registry/applicationschema/cap-iacs-base/code#FarmStructureSurveyNumberValue/barley>
        a                cap-iacs-base:FarmStructureSurveyNumberValue ;
        rdfs:label       "Barley"@en ;
        skos:definition  "-- Definition --\r\nBarley.\r\n-- Description --\r\nHordeum vulgare L.\r\nNOTE. Initial value:2.01.01.04"@en ;
        skos:inScheme    cap-iacs-basecode:FarmStructureSurveyNumberValue .

<http://lpis.ec.europa.eu/registry/applicationschema/cap-iacs-base/code#RecurenceValue/weekly>
        a                cap-iacs-base:RecurenceValue ;
        rdfs:label       "Weekly recurrence"@en ;
        skos:definition  "-- Definition --\r\nWeekly recurrence.\r\n-- Description --\r\nItem description."@en ;
        skos:inScheme    cap-iacs-basecode:RecurenceValue .

<http://lpis.ec.europa.eu/registry/applicationschema/cap-iacs-base/code#CropItemCodeValue/cucumbers>
        a                cap-iacs-base:CropItemCodeValue ;
        rdfs:label       "Cucumbers"@en ;
        skos:definition  "-- Definition --\r\n|||Cucumbers.\r\n-- Description --\r\nCereals and main crops - C\r\nNOTE. Initial value:C1761"@en ;
        skos:inScheme    cap-iacs-basecode:CropItemCodeValue .

<http://lpis.ec.europa.eu/registry/applicationschema/cap-iacs-base/code#CauseOfAnomalyValue/appearanceOfPermanentConstruction>
        a                cap-iacs-base:CauseOfAnomalyValue ;
        rdfs:label       "Cause flaged as Type II. The appearance of permanent construction"@en ;
        skos:definition  "--Name--\r\nAppearance of permanent construction\r\n\r\n-- Description --\r\nThe appearance of buildings, roads, and other sealed surfaces that are likely to stay in the place of former agricultural land more than three years."@en ;
        skos:inScheme    cap-iacs-basecode:CauseOfAnomalyValue .

<http://lpis.ec.europa.eu/registry/applicationschema/cap-iacs-base/code#ConformanceRequirementClassValue/mandatory>
        a                cap-iacs-base:ConformanceRequirementClassValue ;
        rdfs:label       "Mandatory requirement"@en ;
        skos:definition  "--Name--\r\nMandatory\r\n\r\n--Definition--\r\nRequirement that shall be observed in all cases. \r\n\r\n--Description--\r\nThis has to be fulfilled for conformance."@en ;
        skos:inScheme    cap-iacs-basecode:ConformanceRequirementClassValue .

<http://lpis.ec.europa.eu/registry/applicationschema/cap-iacs-base/code#CropItemCodeValue/pulses>
        a                cap-iacs-base:CropItemCodeValue ;
        rdfs:label       "Pulses"@en ;
        skos:definition  "-- Definition --\r\n||Pulses.\r\n-- Description --\r\nCereals and main crops - C\r\nNOTE. Initial value:C1885"@en ;
        skos:inScheme    cap-iacs-basecode:CropItemCodeValue .

<http://lpis.ec.europa.eu/registry/applicationschema/cap-iacs-base/code#StatusValue/rejected>
        a                cap-iacs-base:StatusValue ;
        rdfs:label       "Rejected, not valid, archival"@en ;
        skos:definition  "-- Name--\r\nRejected\r\n\r\n--Definition--\r\nStatus of an object according to the state machine diagram.\r\n\r\n-- Description --\r\nStatus of the change request after the negative outcome of the preliminary evaluation or the cross-check. It also means that no modification to the existing information can be executed.\r\n\r\nNOTE: For transparency, the rejected change requests shall be archived."@en ;
        skos:inScheme    cap-iacs-basecode:StatusValue .

<http://lpis.ec.europa.eu/registry/applicationschema/cap-iacs-base/code#FarmStructureSurveyNumberValue/fruitAndBerryPlantations>
        a                cap-iacs-base:FarmStructureSurveyNumberValue ;
        rdfs:label       "Fruit and berry plantations"@en ;
        skos:definition  "-- Definition --\r\nFruit and berry plantations.\r\n-- Description --\r\nAreas containing trees, bushes and perennial berry plants other than strawberries for the production of fruit. Orchards may be of the continuous type with minimum spacing between trees or of the non-continuous type with wide spacing.\r\nNOTE. Initial value:2.04.01"@en ;
        skos:inScheme    cap-iacs-basecode:FarmStructureSurveyNumberValue .

<http://lpis.ec.europa.eu/registry/applicationschema/cap-iacs-base/code#CropItemCodeValue/vineyards>
        a                cap-iacs-base:CropItemCodeValue ;
        rdfs:label       "Vineyards"@en ;
        skos:definition  "-- Definition --\r\n|||Vineyards.\r\n-- Description --\r\nLand use of Agriculture Area in Use -L\r\nNOTE. Initial value:L2410"@en ;
        skos:inScheme    cap-iacs-basecode:CropItemCodeValue .

<http://lpis.ec.europa.eu/registry/applicationschema/cap-iacs-base/code#CrossComplianceRuleValue/publicHealthAnimalHealthAndPlantHealthFoodSafetySmr5>
        a                cap-iacs-base:CrossComplianceRuleValue ;
        rdfs:label       "Public health, animal health and plant health  - Food safety SMR5"@en ;
        skos:definition  "-- Definition --\r\nPublic health, animal health and plant health  - Food safety SMR5.\r\n-- Description --\r\nCouncil Directive 96/22/EC of 29 April 1996 concerning the prohibition on the use in stockfarming of certain substances having a hormonal or thyrostatic action and beta-agonists, and repealing Directives 81/602/EEC, 88/146/EEC and 88/299/EEC (OJ L 125, 23.5.1996, p. 3). Article 3(a), (b), (d) and (e) and Articles 4, 5 and 7.\r\nNOTE. Initial value:SMR5"@en ;
        skos:inScheme    cap-iacs-basecode:CrossComplianceRuleValue .

<http://lpis.ec.europa.eu/registry/applicationschema/cap-iacs-base/code#SpecieCodeValue/brassicaOleraceaLBrusselsSprouts>
        a                cap-iacs-base:SpecieCodeValue ;
        rdfs:label       "Brassica oleracea L. Brussels sprouts"@en ;
        skos:definition  "-- Definition --\r\nBrassica oleracea L. Brussels sprouts.\r\n-- Description --\r\nList of vegetable specie -H\r\nNOTE. Initial value: H - 10.4"@en ;
        skos:inScheme    cap-iacs-basecode:SpecieCodeValue .

<http://lpis.ec.europa.eu/registry/applicationschema/cap-iacs-base/code#SpecieCodeValue/brassicaOleraceaLWhiteCabbage>
        a                cap-iacs-base:SpecieCodeValue ;
        rdfs:label       "Brassica oleracea L. White cabbage"@en ;
        skos:definition  "-- Definition --\r\nBrassica oleracea L. White cabbage.\r\n-- Description --\r\nList of vegetable specie -H\r\nNOTE. Initial value: H - 10.6"@en ;
        skos:inScheme    cap-iacs-basecode:SpecieCodeValue .

cap-iacs-basecode:TestVerdictValue
        a                skos:ConceptScheme ;
        rdfs:label       "Test verdict value list"@en ;
        dct:isFormatOf   cap-iacs-base:TestVerdictValue ;
        skos:definition  "--Name--\r\nTest verdict value\r\n\r\n-- Definition --\r\nList of values describing test verdicts.\r\n\r\n-- Description --\r\nList of possible test verdict values according to ISO 19105:2000."@en .

<http://lpis.ec.europa.eu/registry/applicationschema/cap-iacs-base/code#FarmStructureSurveyNumberValue/mushroomsIrrigatedAreaEnergyCropsAndGeneticallyModifiedCrops>
        a                cap-iacs-base:FarmStructureSurveyNumberValue ;
        rdfs:label       "Mushrooms, irrigated area, energy crops and genetically modified crops"@en ;
        skos:definition  "-- Definition --\r\nMushrooms, irrigated area, energy crops and genetically modified crops.\r\n-- Description --\r\nMushrooms, irrigated area, energy crops and genetically modified crops.\r\nNOTE. Initial value:2.06"@en ;
        skos:inScheme    cap-iacs-basecode:FarmStructureSurveyNumberValue .

<http://lpis.ec.europa.eu/registry/applicationschema/cap-iacs-base/code#SpecieCodeValue/gossypiumSppCotton>
        a                cap-iacs-base:SpecieCodeValue ;
        rdfs:label       "Gossypium spp. Cotton "@en ;
        skos:definition  "-- Definition --\r\nGossypium spp. Cotton.\r\n-- Description --\r\nList of agricultural species -A\r\nIII. Oil and fibre plants\r\nNOTE. Initial value: A - 66."@en ;
        skos:inScheme    cap-iacs-basecode:SpecieCodeValue .

<http://lpis.ec.europa.eu/registry/applicationschema/cap-iacs-base/code#CropItemCodeValue/commonWheatAndSpelt>
        a                cap-iacs-base:CropItemCodeValue ;
        rdfs:label       "Common wheat and spelt"@en ;
        skos:definition  "-- Definition --\r\n||||Common wheat and spelt.\r\n-- Description --\r\nCereals and main crops - C\r\nNOTE. Initial value:C1120"@en ;
        skos:inScheme    cap-iacs-basecode:CropItemCodeValue .

<http://lpis.ec.europa.eu/registry/applicationschema/cap-iacs-base/code#NotificationGroupValue/notificationOnTheResultsOfOtsc>
        a                cap-iacs-base:NotificationGroupValue ;
        rdfs:label       "Notifications concerning complementary national direct payments (BG and RO only)"@en ;
        skos:definition  "Notification on the results of OTSC\r\n\r\nEach year, by 15 July, for all direct payment schemes, rural development measures and technical assistance and support schemes in the wine sector Member States shall notify the Commission of the control data and control statistics covering results of administrative, on-the-spot checks and ex post checks [Art. 9(1)(a) of R 809/2014]."@en ;
        skos:inScheme    cap-iacs-basecode:NotificationGroupValue .

<http://lpis.ec.europa.eu/registry/applicationschema/cap-iacs-base/code#CropItemCodeValue/permanentCropsL0003>
        a                cap-iacs-base:CropItemCodeValue ;
        rdfs:label       "Permanent crops L0003"@en ;
        skos:definition  "-- Definition --\r\n||Permanent crops L0003.\r\n-- Description --\r\nLand use of Agriculture Area in Use -L\r\nNOTE. Initial value:L0003"@en ;
        skos:inScheme    cap-iacs-basecode:CropItemCodeValue .

<http://lpis.ec.europa.eu/registry/applicationschema/cap-iacs-base/code#CrossComplianceRuleValue/environmentClimateChangeGoodAgriculturalConditionOfLandSoilAndCarbonStockGaec5>
        a                cap-iacs-base:CrossComplianceRuleValue ;
        rdfs:label       "Environment, climate change, good agricultural condition of land  - Soil and carbon stock  GAEC5"@en ;
        skos:definition  "-- Definition --\r\nEnvironment, climate change, good agricultural condition of land  - Soil and carbon stock  GAEC5.\r\n-- Description --\r\nMinimum land management reflecting site specific conditions to limit erosion. \r\nNOTE. Initial value:GAEC5"@en ;
        skos:inScheme    cap-iacs-basecode:CrossComplianceRuleValue .

<http://lpis.ec.europa.eu/registry/applicationschema/cap-iacs-base/code#FarmStructureSurveyNumberValue/leguminousPlants>
        a                cap-iacs-base:FarmStructureSurveyNumberValue ;
        rdfs:label       "Leguminous plants"@en ;
        skos:definition  "-- Definition --\r\nLeguminous plants.\r\n-- Description --\r\nLeguminous plants grown and harvested green as the whole plant mainly for forage.\r\nMixtures of predominantly leguminous (normally > 80 %) forage crops and grass plants, harvested green or as dried hay are included here.\r\nNOTE. Initial value:2.01.09.02.02"@en ;
        skos:inScheme    cap-iacs-basecode:FarmStructureSurveyNumberValue .

<http://lpis.ec.europa.eu/registry/applicationschema/cap-iacs-base/code#CropItemCodeValue/broadAndFieldBeansC1335>
        a                cap-iacs-base:CropItemCodeValue ;
        rdfs:label       "Broad and field beans C1335"@en ;
        skos:definition  "-- Definition --\r\n||Broad and field beans C1335.\r\n-- Description --\r\nCereals and main crops - C\r\nNOTE. Initial value:C1335"@en ;
        skos:inScheme    cap-iacs-basecode:CropItemCodeValue .

<http://lpis.ec.europa.eu/registry/applicationschema/cap-iacs-base/code#SpecieCodeValue/brassicaOleraceaLKohlrabi>
        a                cap-iacs-base:SpecieCodeValue ;
        rdfs:label       "Brassica oleracea L. Kohlrabi "@en ;
        skos:definition  "-- Definition --\r\nBrassica oleracea L. Kohlrabi.\r\n-- Description --\r\nList of vegetable specie -H\r\nNOTE. Initial value: H - 10.8"@en ;
        skos:inScheme    cap-iacs-basecode:SpecieCodeValue .

<http://lpis.ec.europa.eu/registry/applicationschema/cap-iacs-base/code#NotificationGroupValue/notificationsRelatingDecisionsToReviewOfPreviousNotifications>
        a                cap-iacs-base:NotificationGroupValue ;
        rdfs:label       "Notifications relating decisions to review of previous notifications"@en ;
        skos:definition  "-- Definition --\r\nNotifications relating decisions to review of previous notifications.\r\n-- Description --\r\nNOTE.75"@en ;
        skos:inScheme    cap-iacs-basecode:NotificationGroupValue .

<http://lpis.ec.europa.eu/registry/applicationschema/cap-iacs-base/code#SpecieCodeValue/hordeumVulgareLBarley6RowBarley>
        a                cap-iacs-base:SpecieCodeValue ;
        rdfs:label       "Hordeum vulgare L. Barley 6-row barley "@en ;
        skos:definition  "-- Definition --\r\nHordeum vulgare L. Barley 6-row barley.\r\n-- Description --\r\nList of agricultural species -A   \r\nIV. Cereals\r\nNOTE. Initial value: A - 75.2"@en ;
        skos:inScheme    cap-iacs-basecode:SpecieCodeValue .

<http://lpis.ec.europa.eu/registry/applicationschema/cap-iacs-base/code#SpecieCodeValue/medicago×VariaLSandLucerne>
        a                cap-iacs-base:SpecieCodeValue ;
        rdfs:label       "Medicago × varia L. Sand lucerne"@en ;
        skos:definition  "-- Definition --\r\nMedicago × varia L. Sand lucerne.\r\n-- Description --\r\nList of agricultural species -A\r\nII. Fodder plants\r\nNOTE. Initial value:A - 40."@en ;
        skos:inScheme    cap-iacs-basecode:SpecieCodeValue .

<http://lpis.ec.europa.eu/registry/applicationschema/cap-iacs-base/code#CrossComplianceRuleValue/publicHealthAnimalHealthAndPlantHealthIdentificationAndRegistrationOfAnimalsSmr8>
        a                cap-iacs-base:CrossComplianceRuleValue ;
        rdfs:label       "Public health, animal health and plant health  - Identification and registration of animals SMR8"@en ;
        skos:definition  "-- Definition --\r\nPublic health, animal health and plant health  - Identification and registration of animals SMR8.\r\n-- Description --\r\nCouncil Regulation (EC) No 21/2004 of 17 December 2003 establishing a system for the identification and registration of ovine and caprine animals and amending Regulation (EC) No 1782/2003 and Directives 92/102/EEC and 64/432/EEC (OJ L 5, 9.1.2004, p. 8). Articles 3, 4 and 5.\r\nNOTE. Initial value:SMR8"@en ;
        skos:inScheme    cap-iacs-basecode:CrossComplianceRuleValue .

<http://lpis.ec.europa.eu/registry/applicationschema/cap-iacs-base/code#CauseOfAnomalyValue/irreversibleConversionsOfAgriculturalLandCovers>
        a                cap-iacs-base:CauseOfAnomalyValue ;
        rdfs:label       "Cause flaged as Type I. Irreversible conversions of agricultural land covers"@en ;
        skos:definition  "--Name--\r\nIrreversible conversion of agricultural land covers\r\n\r\n-- Description --\r\nAppearance of forests, deserted areas, rock outcrops, inundated areas, etc. in the place of former agricultural land."@en ;
        skos:inScheme    cap-iacs-basecode:CauseOfAnomalyValue .

<http://lpis.ec.europa.eu/registry/applicationschema/cap-iacs-base/code#TestTypeValue/capability>
        a                cap-iacs-base:TestTypeValue ;
        rdfs:label       "Capability test"@en ;
        skos:definition  "--Name--\r\nCapability\r\n\r\n-- Definition --\r\nCapability test.\r\n\r\n-- Description --\r\nCapability tests (CT), should investigate an implementation as thoroughly as it is practical over the full range of conformance requirements specified in a standard/legal act. Capability tests should be provided to check the mandatory capabilities and those optional capabilities that are identified in the ICS as being supported by the IUT.\r\n\r\nNOTE 1. CT shall be used to check that the capabilities of the IUT are consistent with the conformance requirements, that is, to determine whether or not an implementation conforms.\r\n\r\nNOTE 2. CT shall be used to investigate causes of failure."@en ;
        skos:inScheme    cap-iacs-basecode:TestTypeValue .

<http://lpis.ec.europa.eu/registry/applicationschema/cap-iacs-base/code#FarmStructureSurveyNumberValue/otherWines>
        a                cap-iacs-base:FarmStructureSurveyNumberValue ;
        rdfs:label       "Other wines"@en ;
        skos:definition  "-- Definition --\r\nOther wines.\r\n-- Description --\r\nGrape varieties normally grown for the production of wines other than PDO and PGI wines.\r\nNOTE. Initial value:2.04.04.02"@en ;
        skos:inScheme    cap-iacs-basecode:FarmStructureSurveyNumberValue .

<http://lpis.ec.europa.eu/registry/applicationschema/cap-iacs-base/code#WeekdayValue/saturday>
        a                cap-iacs-base:WeekdayValue ;
        rdfs:label       "Saturday"@en ;
        skos:definition  "-- Definition --\r\nSaturday.\r\n-- Description --\r\nItem description."@en ;
        skos:inScheme    cap-iacs-basecode:WeekdayValue .

<http://lpis.ec.europa.eu/registry/applicationschema/cap-iacs-base/code#FarmStructureSurveyNumberValue/otherFibreCrops>
        a                cap-iacs-base:FarmStructureSurveyNumberValue ;
        rdfs:label       "Other fibre crops"@en ;
        skos:definition  "-- Definition --\r\nOther fibre crops.\r\n-- Description --\r\nOther plants grown mainly for their fibre content, not mentioned elsewhere.\r\nNOTE. Initial value:2.01.06.11"@en ;
        skos:inScheme    cap-iacs-basecode:FarmStructureSurveyNumberValue .

<http://lpis.ec.europa.eu/registry/applicationschema/cap-iacs-base/code#SpecieCodeValue/lolium×BoucheanumKunthHybridRyegrass>
        a                cap-iacs-base:SpecieCodeValue ;
        rdfs:label       "Lolium × boucheanum Kunth Hybrid ryegrass "@en ;
        skos:definition  "-- Definition --\r\nLolium × boucheanum Kunth Hybrid ryegrass.\r\n-- Description --\r\nList of agricultural species -A\r\nII. Fodder plants\r\nNOTE. Initial value: A - 22."@en ;
        skos:inScheme    cap-iacs-basecode:SpecieCodeValue .

<http://lpis.ec.europa.eu/registry/applicationschema/cap-iacs-base/code#ConformanceClassValue/classA>
        a                cap-iacs-base:ConformanceClassValue ;
        rdfs:label       "Class A"@en ;
        skos:definition  "--Name--\r\nClass A\r\n\r\n--Definition--\r\nSpecified conformance class.\r\n\r\n--Description--\r\nSeparate ATS must be provided if a class is defined within ConformanceClause."@en ;
        skos:inScheme    cap-iacs-basecode:ConformanceClassValue .

<http://lpis.ec.europa.eu/registry/applicationschema/cap-iacs-base/code#FarmStructureSurveyNumberValue/mushrooms>
        a                cap-iacs-base:FarmStructureSurveyNumberValue ;
        rdfs:label       "Mushrooms"@en ;
        skos:definition  "-- Definition --\r\nMushrooms.\r\n-- Description --\r\nCultivated mushrooms grown in buildings which have been specially erected or adapted for growing mushrooms, as well as in underground premises, caves and cellars.\r\nNOTE. Initial value:2.06.01"@en ;
        skos:inScheme    cap-iacs-basecode:FarmStructureSurveyNumberValue .

<http://lpis.ec.europa.eu/registry/applicationschema/cap-iacs-base/code#FarmStructureSurveyNumberValue/sugarBeetExcludingSeed>
        a                cap-iacs-base:FarmStructureSurveyNumberValue ;
        rdfs:label       "Sugar beet (excluding seed)"@en ;
        skos:definition  "-- Definition --\r\nSugar beet (excluding seed).\r\n-- Description --\r\nBeta vulgaris L. intended for the sugar industry and alcohol production (including energy production).\r\nNOTE. Initial value:2.01.04"@en ;
        skos:inScheme    cap-iacs-basecode:FarmStructureSurveyNumberValue .

<http://lpis.ec.europa.eu/registry/applicationschema/cap-iacs-base/code#SpecieCodeValue/betaVulgarisLFodderBeet>
        a                cap-iacs-base:SpecieCodeValue ;
        rdfs:label       "Beta vulgaris L. Fodder beet "@en ;
        skos:definition  "-- Definition --\r\nBeta vulgaris L. Fodder beet.\r\n-- Description --\r\nList of agricultural species -A\r\nI. Beet\r\nNOTE. Initial value: A - 2."@en ;
        skos:inScheme    cap-iacs-basecode:SpecieCodeValue .

<http://lpis.ec.europa.eu/registry/applicationschema/cap-iacs-base/code#CropItemCodeValue/otherFreshVegetablesNec>
        a                cap-iacs-base:CropItemCodeValue ;
        rdfs:label       "Other fresh vegetables n.e.c."@en ;
        skos:definition  "-- Definition --\r\n||Other fresh vegetables n.e.c.\r\n-- Description --\r\nCereals and main crops - C\r\nNOTE. Initial value:C1920"@en ;
        skos:inScheme    cap-iacs-basecode:CropItemCodeValue .

<http://lpis.ec.europa.eu/registry/applicationschema/cap-iacs-base/code#SpecieCodeValue/cynaraCardunculusLCardoon>
        a                cap-iacs-base:SpecieCodeValue ;
        rdfs:label       "Cynara cardunculus L. Cardoon"@en ;
        skos:definition  "-- Definition --\r\nCynara cardunculus L. Cardoon.\r\n-- Description --\r\nList of vegetable specie -H\r\nNOTE. Initial value: H - 20.2"@en ;
        skos:inScheme    cap-iacs-basecode:SpecieCodeValue .

<http://lpis.ec.europa.eu/registry/applicationschema/cap-iacs-base/code#SupportSchemeTypeValue/redistributivePayment>
        a                cap-iacs-base:SupportSchemeTypeValue ;
        rdfs:label       "Redistributive payment "@en ;
        skos:definition  "Redistributive payment\r\n\r\nConditional payment scheme decided by MS to grant an annual payment to farmers who are entitled to a payment under the basic payment scheme or under the single area payment scheme.\r\n\r\nArt. 4 of Title III, Chapter 2 of R 1307/2013 sets the calculation method:\r\nIt shall be calculated \r\n\t- each year by Member States\r\n\t- by multiplying a figure to be set by the Member State, which shall not be higher than 65 % of the national or regional average payment per hectare, by the number of payment entitlements or by the number of eligible hectares. \r\nThe number of such payment entitlements or hectares shall not exceed a maximum to be set by Member States which shall not be higher than 30 hectares or the average size of agricultural holdings set out in Annex VIII if that average size exceeds 30 hectares in the Member State concerned.\r\n\r\nNOTE\r\nMS may establish a graduation in the number of hectares that is equally applied to every farmer.\r\n-- Description --\r\nRegulation / Decoupled payment."@en ;
        skos:inScheme    cap-iacs-basecode:SupportSchemeTypeValue .

<http://lpis.ec.europa.eu/registry/applicationschema/cap-iacs-base/code#CropItemCodeValue/utilisedAgriculturalAreaUAA>
        a                cap-iacs-base:CropItemCodeValue ;
        rdfs:label       "Utilised agricultural area (UAA)"@en ;
        skos:definition  "-- Definition --\r\n|Utilised agricultural area (UAA).\r\n-- Description --\r\nLand use of Agriculture Area in Use -L\r\nNOTE. Initial value:L0005"@en ;
        skos:inScheme    cap-iacs-basecode:CropItemCodeValue .

<http://lpis.ec.europa.eu/registry/applicationschema/cap-iacs-base/code#CropItemCodeValue/cottonFibre>
        a                cap-iacs-base:CropItemCodeValue ;
        rdfs:label       "Cotton fibre "@en ;
        skos:definition  "-- Definition --\r\n|||Cotton fibre.\r\n-- Description --\r\nCereals and main crops - C\r\nNOTE. Initial value:C1540"@en ;
        skos:inScheme    cap-iacs-basecode:CropItemCodeValue .

<http://lpis.ec.europa.eu/registry/applicationschema/cap-iacs-base/code#SpecieCodeValue/medicagoSativaLLucerne>
        a                cap-iacs-base:SpecieCodeValue ;
        rdfs:label       "Medicago sativa L. Lucerne "@en ;
        skos:definition  "-- Definition --\r\nMedicago sativa L. Lucerne.\r\n-- Description --\r\nList of agricultural species -A\r\nII. Fodder plants\r\nNOTE. Initial value: A - 39."@en ;
        skos:inScheme    cap-iacs-basecode:SpecieCodeValue .

<http://lpis.ec.europa.eu/registry/applicationschema/cap-iacs-base/code#MonthValue/may>
        a                cap-iacs-base:MonthValue ;
        rdfs:label       "May"@en ;
        skos:definition  "-- Definition --\r\nMay.\r\n-- Description --\r\nItem description."@en ;
        skos:inScheme    cap-iacs-basecode:MonthValue .

<http://lpis.ec.europa.eu/registry/applicationschema/cap-iacs-base/code#StatusValue/inProgress>
        a                cap-iacs-base:StatusValue ;
        rdfs:label       "Under construction"@en ;
        skos:definition  "-- Name--\r\nIn progress\r\n\r\n--Definition--\r\nStatus of an object according to the state machine diagram.\r\n\r\n-- Description --\r\nThe value shall be assigned when processing of the issue/anomaly has been started. The value is applicable to\r\n- the issue/anomaly that reported the change request\r\n- the object (schema element or data) that is subject of the change request.\r\n\r\nEXAMPLE 1. Schema element objects are:\r\n- the entire application schema,\r\n- feature and data types\r\n- attributes, association roles,\r\n- constraints\r\n- value types (etc).\r\n\r\nEXAMPLE 2. Data objects are specific instances of a feature or data types (e.g. RP, farmer, anomaly, payment. The change may be applied to \r\n- the instance as a whole (depreciation of an obsolete instance or introduction of a new instance),\r\n- a specific value (attribute) of an instance.\r\n\r\nNOTE: Rules for depreciation are defined by internal business rules of the MS/Region"@en ;
        skos:inScheme    cap-iacs-basecode:StatusValue .

<http://lpis.ec.europa.eu/registry/applicationschema/cap-iacs-base/code#CropItemCodeValue/sugarBeetExcludingSeedL1370>
        a                cap-iacs-base:CropItemCodeValue ;
        rdfs:label       "Sugar beet (excluding seed) L1370"@en ;
        skos:definition  "-- Definition --\r\n||||Sugar beet (excluding seed) L1370.\r\n-- Description --\r\nLand use of Agriculture Area in Use -L\r\nNOTE. Initial value:L1370"@en ;
        skos:inScheme    cap-iacs-basecode:CropItemCodeValue .

<http://lpis.ec.europa.eu/registry/applicationschema/cap-iacs-base/code#CropItemCodeValue/citrusFruitsC2300>
        a                cap-iacs-base:CropItemCodeValue ;
        rdfs:label       "Citrus fruits C2300"@en ;
        skos:definition  "-- Definition --\r\n||Citrus fruits C2300.\r\n-- Description --\r\nCereals and main crops - C\r\nNOTE. Initial value:C2300"@en ;
        skos:inScheme    cap-iacs-basecode:CropItemCodeValue .

<http://lpis.ec.europa.eu/registry/applicationschema/cap-iacs-base/code#FarmStructureSurveyNumberValue/cotton>
        a                cap-iacs-base:FarmStructureSurveyNumberValue ;
        rdfs:label       "Cotton"@en ;
        skos:definition  "-- Definition --\r\nCotton.\r\n-- Description --\r\nGossypium spp., harvested for fibre as well as for oil-seeds.\r\nNOTE. Initial value:2.01.06.03"@en ;
        skos:inScheme    cap-iacs-basecode:FarmStructureSurveyNumberValue .

<http://lpis.ec.europa.eu/registry/applicationschema/cap-iacs-base/code#AffectedElementTypeValue/codeList>
        a                cap-iacs-base:AffectedElementTypeValue ;
        rdfs:label       "Code list"@en ;
        skos:definition  "--Name--\r\nCode list\r\n\r\n-- Definition --\r\nSet of pre-defined values that an attribute may take."@en ;
        skos:inScheme    cap-iacs-basecode:AffectedElementTypeValue .

<http://lpis.ec.europa.eu/registry/applicationschema/cap-iacs-base/code#CropItemCodeValue/springBarley>
        a                cap-iacs-base:CropItemCodeValue ;
        rdfs:label       "Spring barley"@en ;
        skos:definition  "-- Definition --\r\n||||Spring barley.\r\n-- Description --\r\nCereals and main crops - C\r\nNOTE. Initial value:C1164"@en ;
        skos:inScheme    cap-iacs-basecode:CropItemCodeValue .

<http://lpis.ec.europa.eu/registry/applicationschema/cap-iacs-base/code#SpecieCodeValue/brassicaOleraceaLCauliflower>
        a                cap-iacs-base:SpecieCodeValue ;
        rdfs:label       "Brassica oleracea L. Cauliflower"@en ;
        skos:definition  "-- Definition --\r\nBrassica oleracea L. Cauliflower.\r\n-- Description --\r\nList of vegetable specie -H\r\nNOTE. Initial value: H - 10.2"@en ;
        skos:inScheme    cap-iacs-basecode:SpecieCodeValue .

<http://lpis.ec.europa.eu/registry/applicationschema/cap-iacs-base/code#FarmStructureSurveyNumberValue/sunflower>
        a                cap-iacs-base:FarmStructureSurveyNumberValue ;
        rdfs:label       "Sunflower"@en ;
        skos:definition  "-- Definition --\r\nSunflower.\r\n-- Description --\r\nHelianthus annuus L., harvested as dry grains.\r\nNOTE. Initial value:2.01.06.05"@en ;
        skos:inScheme    cap-iacs-basecode:FarmStructureSurveyNumberValue .

<http://lpis.ec.europa.eu/registry/applicationschema/cap-iacs-base/code#SpecieCodeValue/loliumPerenneLPerennialRyegrass>
        a                cap-iacs-base:SpecieCodeValue ;
        rdfs:label       "Lolium perenne L. Perennial ryegrass"@en ;
        skos:definition  "-- Definition --\r\nLolium perenne L. Perennial ryegrass.\r\n-- Description --\r\nList of agricultural species -A\r\nII. Fodder plants\r\nNOTE. Initial value: A - 21."@en ;
        skos:inScheme    cap-iacs-basecode:SpecieCodeValue .

<http://lpis.ec.europa.eu/registry/applicationschema/cap-iacs-base/code#StatusOfAnomalyValue/archived>
        a                cap-iacs-base:StatusOfAnomalyValue ;
        rdfs:label       "Closed"@en ;
        skos:definition  "--Name--\r\nArchived\r\n\r\n-- Definition --\r\nStatus of anomaly as soon as it has been resolved.\r\n\r\n--Description--\r\nAnomalies are archived for historic reference."@en ;
        skos:inScheme    cap-iacs-basecode:StatusOfAnomalyValue .

<http://lpis.ec.europa.eu/registry/applicationschema/cap-iacs-base/code>
        a       owl:Ontology ;
        rdfs:label       "Base types code lists"@en ;
        owl:versionIRI   <http://lpis.ec.europa.eu/registry/applicationschema/cap-iacs-base/code/3.0> ;
        owl:versionInfo  "3.0" ;
        dct:creator [ schema:affiliation [ foaf:name "PSNC" ] ;
                      rdfs:seeAlso <http://orcid.org/0000-0003-4289-4922> ;
                      foaf:name "Raul Palma"
                    ] ;
        dct:title "JRC IACS - Base Types Code Lists"@en ;
        dct:description "Ontology of the base types code lists used in IACS, generated from the transformation of the corresponding JRC application schema"@en ;
        dct:source "JRC IACS application schema. https://doi.org/10.1016/j.landusepol.2016.05.023"@en ;
        dct:rights "This ontology is distributed under Creative Commons Attribution 4.0 License - http://creativecommons.org/licenses/by/4.0"@en .

<http://lpis.ec.europa.eu/registry/applicationschema/cap-iacs-base/code#SpecieCodeValue/sorghumSudanenseLSudanGrass>
        a                cap-iacs-base:SpecieCodeValue ;
        rdfs:label       "Sorghum sudanense L. Sudan grass "@en ;
        skos:definition  "-- Definition --\r\nSorghum sudanense L. Sudan grass.\r\n-- Description --\r\nList of agricultural species -A   \r\nIV. Cereals\r\nNOTE. Initial value: A - 80."@en ;
        skos:inScheme    cap-iacs-basecode:SpecieCodeValue .

<http://lpis.ec.europa.eu/registry/applicationschema/cap-iacs-base/code#ConformanceRequirementStatementValue/negative>
        a                cap-iacs-base:ConformanceRequirementStatementValue ;
        rdfs:label       "Negative statement"@en ;
        skos:definition  "--Name--\r\nNegative\r\n\r\n--Definition--\r\nNegative statement.\r\n\r\n--Description--\r\nNegative statement state what is required not to be observed."@en ;
        skos:inScheme    cap-iacs-basecode:ConformanceRequirementStatementValue .

<http://lpis.ec.europa.eu/registry/applicationschema/cap-iacs-base/code#FarmStructureSurveyNumberValue/rapeAndTurnipRape>
        a                cap-iacs-base:FarmStructureSurveyNumberValue ;
        rdfs:label       "Rape and turnip rape"@en ;
        skos:definition  "-- Definition --\r\nRape and turnip rape.\r\n-- Description --\r\nBrassica napus L. (partim) and Brassica rapa L. var. sylvestris (Lam.) Briggs, grown for the production of oil, harvested as dry grains.\r\nNOTE. Initial value:2.01.06.04"@en ;
        skos:inScheme    cap-iacs-basecode:FarmStructureSurveyNumberValue .

<http://lpis.ec.europa.eu/registry/applicationschema/cap-iacs-base/code#CropItemCodeValue/industrialCropsL1400>
        a                cap-iacs-base:CropItemCodeValue ;
        rdfs:label       "Industrial crops L1400"@en ;
        skos:definition  "-- Definition --\r\n|||Industrial crops L1400.\r\n-- Description --\r\nLand use of Agriculture Area in Use -L\r\nNOTE. Initial value:L1400"@en ;
        skos:inScheme    cap-iacs-basecode:CropItemCodeValue .

<http://lpis.ec.europa.eu/registry/applicationschema/cap-iacs-base/code#FarmStructureSurveyNumberValue/fruitSpeciesOfWhichFruitOfTemperateClimateZones>
        a                cap-iacs-base:FarmStructureSurveyNumberValue ;
        rdfs:label       "Fruit species, of which: Fruit of temperate climate zones"@en ;
        skos:definition  "-- Definition --\r\nFruit species, of which: Fruit of temperate climate zones.\r\n-- Description --\r\nFruit tree plantations which are traditionally cropped in temperate climates for producing fruits.\r\nNOTE. Initial value:2.04.01.01.01"@en ;
        skos:inScheme    cap-iacs-basecode:FarmStructureSurveyNumberValue .

<http://lpis.ec.europa.eu/registry/applicationschema/cap-iacs-base/code#SpecieCodeValue/cucurbitaPepoLMarrowOrCourgette>
        a                cap-iacs-base:SpecieCodeValue ;
        rdfs:label       "Cucurbita pepo L. Marrow or Courgette"@en ;
        skos:definition  "-- Definition --\r\nCucurbita pepo L. Marrow or Courgette.\r\n-- Description --\r\nList of vegetable specie -H\r\nNOTE. Initial value: H - 19."@en ;
        skos:inScheme    cap-iacs-basecode:SpecieCodeValue .

<http://lpis.ec.europa.eu/registry/applicationschema/cap-iacs-base/code#CropItemCodeValue/almonds>
        a                cap-iacs-base:CropItemCodeValue ;
        rdfs:label       "Almonds"@en ;
        skos:definition  "-- Definition --\r\n|||Almonds.\r\n-- Description --\r\nCereals and main crops - C\r\nNOTE. Initial value:C2233"@en ;
        skos:inScheme    cap-iacs-basecode:CropItemCodeValue .

<http://lpis.ec.europa.eu/registry/applicationschema/cap-iacs-base/code#OrdinalNumberValue/third>
        a                cap-iacs-base:OrdinalNumberValue ;
        rdfs:label       "Third"@en ;
        skos:definition  "-- Definition --\r\nThird.\r\n-- Description --\r\nItem description."@en ;
        skos:inScheme    cap-iacs-basecode:OrdinalNumberValue .

<http://lpis.ec.europa.eu/registry/applicationschema/cap-iacs-base/code#CropItemCodeValue/rootCrops>
        a                cap-iacs-base:CropItemCodeValue ;
        rdfs:label       "Root crops"@en ;
        skos:definition  "-- Definition --\r\n|Root crops.\r\n-- Description --\r\nCereals and main crops - C\r\nNOTE. Initial value:C1350"@en ;
        skos:inScheme    cap-iacs-basecode:CropItemCodeValue .

<http://lpis.ec.europa.eu/registry/applicationschema/cap-iacs-base/code#CropItemCodeValue/maslin>
        a                cap-iacs-base:CropItemCodeValue ;
        rdfs:label       "Maslin"@en ;
        skos:definition  "-- Definition --\r\n||||Maslin.\r\n-- Description --\r\nCereals and main crops - C\r\nNOTE. Initial value:C1155"@en ;
        skos:inScheme    cap-iacs-basecode:CropItemCodeValue .

cap-iacs-basecode:OrdinalNumberValue
        a                skos:ConceptScheme ;
        rdfs:label       "Ordinal number value list"@en ;
        dct:isFormatOf   cap-iacs-base:OrdinalNumberValue ;
        skos:definition  "-- Definition --\r\nOrdinal number value list.\r\n\r\n-- Description --\r\nList of possible ordinal number values used for date identification."@en .

<http://lpis.ec.europa.eu/registry/applicationschema/cap-iacs-base/code#CropItemCodeValue/vineyardsForOtherWines>
        a                cap-iacs-base:CropItemCodeValue ;
        rdfs:label       "Vineyards for other wines"@en ;
        skos:definition  "-- Definition --\r\n||||Vineyards for other wines.\r\n-- Description --\r\nCereals and main crops - C\r\nNOTE. Initial value:C2443"@en ;
        skos:inScheme    cap-iacs-basecode:CropItemCodeValue .

<http://lpis.ec.europa.eu/registry/applicationschema/cap-iacs-base/code#SpecieCodeValue/raphanusSativusLVarOleiformisPersFodderRadish>
        a                cap-iacs-base:SpecieCodeValue ;
        rdfs:label       "Raphanus sativus L. var. oleiformis Pers. Fodder radish"@en ;
        skos:definition  "-- Definition --\r\nRaphanus sativus L. var. oleiformis Pers. Fodder radish.\r\n-- Description --\r\nList of agricultural species -A\r\nII. Fodder plants\r\nNOTE. Initial value: A - 57."@en ;
        skos:inScheme    cap-iacs-basecode:SpecieCodeValue .

<http://lpis.ec.europa.eu/registry/applicationschema/cap-iacs-base/code#MonthValue/december>
        a                cap-iacs-base:MonthValue ;
        rdfs:label       "December"@en ;
        skos:definition  "-- Definition --\r\nDecember.\r\n-- Description --\r\nItem description."@en ;
        skos:inScheme    cap-iacs-basecode:MonthValue .

<http://lpis.ec.europa.eu/registry/applicationschema/cap-iacs-base/code#SpecieCodeValue/lycopersiconEsculentumLxSHabrochaite>
        a                cap-iacs-base:SpecieCodeValue ;
        rdfs:label       "Lycopersicon esculentum L. x S. habrochaites"@en ;
        skos:definition  "-- Definition --\r\nLycopersicon esculentum L. x S. habrochaites.\r\n-- Description --\r\nList of vegetable specie -H\r\nNOTE. Initial value: H - 37.4"@en ;
        skos:inScheme    cap-iacs-basecode:SpecieCodeValue .

<http://lpis.ec.europa.eu/registry/applicationschema/cap-iacs-base/code#CropItemCodeValue/barley>
        a                cap-iacs-base:CropItemCodeValue ;
        rdfs:label       "Barley"@en ;
        skos:definition  "-- Definition --\r\n|||Barley.\r\n-- Description --\r\nCereals and main crops - C\r\nNOTE. Initial value:C1160"@en ;
        skos:inScheme    cap-iacs-basecode:CropItemCodeValue .

<http://lpis.ec.europa.eu/registry/applicationschema/cap-iacs-base/code#WeekdayValue/tuesday>
        a                cap-iacs-base:WeekdayValue ;
        rdfs:label       "Tuesday"@en ;
        skos:definition  "-- Definition --\r\nTuesday.\r\n-- Description --\r\nItem description."@en ;
        skos:inScheme    cap-iacs-basecode:WeekdayValue .

<http://lpis.ec.europa.eu/registry/applicationschema/cap-iacs-base/code#AffectedElementTypeValue/dataType>
        a                cap-iacs-base:AffectedElementTypeValue ;
        rdfs:label       "Data type"@en ;
        skos:definition  "--Name--\r\nData type\r\n\r\n-- Definition --\r\nSpecification of a value domain with operations allowed on values in this domain [ISO 19103:2005].\r\n\r\n-- Description --\r\nFor purposes of LCM, this term is used for proprietary (user-defined) and imported (from third parties) data types."@en ;
        skos:inScheme    cap-iacs-basecode:AffectedElementTypeValue .

<http://lpis.ec.europa.eu/registry/applicationschema/cap-iacs-base/code#SpecieCodeValue/secaleCerealeLRye>
        a                cap-iacs-base:SpecieCodeValue ;
        rdfs:label       "Secale cereale L. Rye   "@en ;
        skos:definition  "-- Definition --\r\nSecale cereale L. Rye.\r\n-- Description --\r\nList of agricultural species -A   \r\nIV. Cereals\r\nNOTE. Initial value: A - 78."@en ;
        skos:inScheme    cap-iacs-basecode:SpecieCodeValue .

<http://lpis.ec.europa.eu/registry/applicationschema/cap-iacs-base/code#StatusValue/archived>
        a                cap-iacs-base:StatusValue ;
        skos:definition  "--Name--\r\nArchived\r\n\r\n--Definition--\r\nStatus of an object according to the state machine diagram.\r\n\r\n-- Description--\r\nFinal state of an object after its depreciation (retirement).\r\nSuch object is no more in use; its life cycle has been completed.\r\n\r\nNOTE 1. FeatureLevelMetadata.endLifespanVersion<>Null\r\n\r\nNOTE 2. NOTE 2: If applied, FeatureLevelMetadata.validTo<>Null"@en ;
        skos:inScheme    cap-iacs-basecode:StatusValue .

<http://lpis.ec.europa.eu/registry/applicationschema/cap-iacs-base/code#NotificationGroupValue/notificationsConcerningAdjustmentRateForAGroupAtTheLevelOfItsMembers>
        a                cap-iacs-base:NotificationGroupValue ;
        rdfs:label       "Notifications concerning adjustment rate for a group at the level of its members"@en ;
        skos:definition  "-- Definition --\r\nNotifications concerning adjustment rate for a group at the level of its members\r\n-- Description --\r\nNOTE.71"@en ;
        skos:inScheme    cap-iacs-basecode:NotificationGroupValue .

<http://lpis.ec.europa.eu/registry/applicationschema/cap-iacs-base/code#CropItemCodeValue/buckwheatMilletCanarySeedOtherCereals>
        a                cap-iacs-base:CropItemCodeValue ;
        rdfs:label       "Buckwheat, millet, canary seed (other cereals)"@en ;
        skos:definition  "-- Definition --\r\n|||Buckwheat, millet, canary seed (other cereals).\r\n-- Description --\r\nCereals and main crops - C\r\nNOTE. Initial value:C1219"@en ;
        skos:inScheme    cap-iacs-basecode:CropItemCodeValue .

<http://lpis.ec.europa.eu/registry/applicationschema/cap-iacs-base/code#CropItemCodeValue/otherVegetablesCultivatedForFruitNec>
        a                cap-iacs-base:CropItemCodeValue ;
        rdfs:label       "Other vegetables cultivated for fruit n.e.c."@en ;
        skos:definition  "-- Definition --\r\n|||Other vegetables cultivated for fruit n.e.c.\r\n-- Description --\r\nCereals and main crops - C\r\nNOTE. Initial value:C1799"@en ;
        skos:inScheme    cap-iacs-basecode:CropItemCodeValue .

<http://lpis.ec.europa.eu/registry/applicationschema/cap-iacs-base/code#CropItemCodeValue/energyCrops>
        a                cap-iacs-base:CropItemCodeValue ;
        rdfs:label       "Energy crops"@en ;
        skos:definition  "-- Definition --\r\n|Energy crops.\r\n-- Description --\r\nCereals and main crops - C\r\nNOTE. Initial value:C1590"@en ;
        skos:inScheme    cap-iacs-basecode:CropItemCodeValue .

<http://lpis.ec.europa.eu/registry/applicationschema/cap-iacs-base/code#SpecieCodeValue/trifotiumHybridumLAlsikeClover>
        a                cap-iacs-base:SpecieCodeValue ;
        rdfs:label       "Trifolium hybridum L. Alsike clover"@en ;
        skos:definition  "-- Definition --\r\nTrifolium hybridum L. Alsike clover.\r\n-- Description --\r\nList of agricultural species -A\r\nII. Fodder plants\r\nNOTE. Initial value: A - 44."@en ;
        skos:inScheme    cap-iacs-basecode:SpecieCodeValue .

<http://lpis.ec.europa.eu/registry/applicationschema/cap-iacs-base/code#SpecieCodeValue/daucusCarotaLFodderCarrot>
        a                cap-iacs-base:SpecieCodeValue ;
        rdfs:label       "Daucus carota L. Fodder carrot"@en ;
        skos:definition  "-- Definition --\r\nDaucus carota L. Fodder carrot.\r\n-- Description --\r\nList of vegetable specie -H\r\nNOTE. Initial value: H - 21.2"@en ;
        skos:inScheme    cap-iacs-basecode:SpecieCodeValue .

<http://lpis.ec.europa.eu/registry/applicationschema/cap-iacs-base/code#CropItemCodeValue/onions>
        a                cap-iacs-base:CropItemCodeValue ;
        rdfs:label       "Onions"@en ;
        skos:definition  "-- Definition --\r\n|||Onions.\r\n-- Description --\r\nCereals and main crops - C\r\nNOTE. Initial value:C1851"@en ;
        skos:inScheme    cap-iacs-basecode:CropItemCodeValue .

<http://lpis.ec.europa.eu/registry/applicationschema/cap-iacs-base/code#CropItemCodeValue/otherDriedPulsesNecC1345>
        a                cap-iacs-base:CropItemCodeValue ;
        rdfs:label       "Other dried pulses n.e.c. C1345"@en ;
        skos:definition  "-- Definition --\r\n||Other dried pulses n.e.c. C1345.\r\n-- Description --\r\nCereals and main crops - C\r\nNOTE. Initial value:C1345"@en ;
        skos:inScheme    cap-iacs-basecode:CropItemCodeValue .

<http://lpis.ec.europa.eu/registry/applicationschema/cap-iacs-base/code#CropItemCodeValue/cucumbersUnderGlassOrHighAccessibleCoverC1762>
        a                cap-iacs-base:CropItemCodeValue ;
        rdfs:label       "Cucumbers under glass or high accessible cover C1762 "@en ;
        skos:definition  "-- Definition --\r\n||||Cucumbers under glass or high accessible cover C1762.\r\n-- Description --\r\nCereals and main crops - C\r\nNOTE. Initial value:C1762"@en ;
        skos:inScheme    cap-iacs-basecode:CropItemCodeValue .

<http://lpis.ec.europa.eu/registry/applicationschema/cap-iacs-base/code#CropItemCodeValue/gherkins>
        a                cap-iacs-base:CropItemCodeValue ;
        rdfs:label       "Gherkins"@en ;
        skos:definition  "-- Definition --\r\n|||Gherkins.\r\n-- Description --\r\nCereals and main crops - C\r\nNOTE. Initial value:C1766"@en ;
        skos:inScheme    cap-iacs-basecode:CropItemCodeValue .

<http://lpis.ec.europa.eu/registry/applicationschema/cap-iacs-base/code#NotificationGroupValue/notificationsConcerningTheSmallFarmersScheme>
        a                cap-iacs-base:NotificationGroupValue ;
        rdfs:label       "Notifications concerning the small farmers scheme"@en ;
        skos:definition  "-- Definition --\r\nNotifications concerning the small farmers scheme.\r\n-- Description --\r\nNOTE.70"@en ;
        skos:inScheme    cap-iacs-basecode:NotificationGroupValue .

<http://lpis.ec.europa.eu/registry/applicationschema/cap-iacs-base/code#MonthValue/april>
        a                cap-iacs-base:MonthValue ;
        rdfs:label       "April"@en ;
        skos:definition  "-- Definition --\r\nApril.\r\n-- Description --\r\nItem description."@en ;
        skos:inScheme    cap-iacs-basecode:MonthValue .

<http://lpis.ec.europa.eu/registry/applicationschema/cap-iacs-base/code#SpecieCodeValue/viciaPannonicaLHungarianVetch>
        a                cap-iacs-base:SpecieCodeValue ;
        rdfs:label       "Vicia pannonica L. Hungarian vetch "@en ;
        skos:definition  "-- Definition --\r\nVicia pannonica L. Hungarian vetch.\r\n-- Description --\r\nList of agricultural species -A\r\nII. Fodder plants\r\nNOTE. Initial value: A - 51."@en ;
        skos:inScheme    cap-iacs-basecode:SpecieCodeValue .

<http://lpis.ec.europa.eu/registry/applicationschema/cap-iacs-base/code#SpecieCodeValue/lupinusAlbusLWhiteLupin>
        a                cap-iacs-base:SpecieCodeValue ;
        rdfs:label       "Lupinus albus L. White lupin"@en ;
        skos:definition  "-- Definition --\r\nLupinus albus L. White lupin.\r\n-- Description --\r\nList of agricultural species -A\r\nII. Fodder plants\r\nNOTE. Initial value: A - 35."@en ;
        skos:inScheme    cap-iacs-basecode:SpecieCodeValue .

<http://lpis.ec.europa.eu/registry/applicationschema/cap-iacs-base/code#SpecieCodeValue/solanumMelongenaLAubergineEggPlant>
        a                cap-iacs-base:SpecieCodeValue ;
        rdfs:label       "Solanum melongena L. Aubergine / Egg plant"@en ;
        skos:definition  "-- Definition --\r\nSolanum melongena L. Aubergine / Egg plant.\r\n-- Description --\r\nList of vegetable specie -H\r\nNOTE. Initial value: H - 32."@en ;
        skos:inScheme    cap-iacs-basecode:SpecieCodeValue .

<http://lpis.ec.europa.eu/registry/applicationschema/cap-iacs-base/code#FarmStructureSurveyNumberValue/citrusPlantations>
        a                cap-iacs-base:FarmStructureSurveyNumberValue ;
        rdfs:label       "Citrus plantations"@en ;
        skos:definition  "-- Definition --\r\nCitrus plantations.\r\n-- Description --\r\nPlantations of Citrus spp.\r\nNOTE. Initial value:2.04.02"@en ;
        skos:inScheme    cap-iacs-basecode:FarmStructureSurveyNumberValue .

<http://lpis.ec.europa.eu/registry/applicationschema/cap-iacs-base/code#CauseOfAnomalyValue/misclassifiedProrataClass>
        a              cap-iacs-base:CauseOfAnomalyValue ;
        skos:inScheme  cap-iacs-basecode:CauseOfAnomalyValue .

<http://lpis.ec.europa.eu/registry/applicationschema/cap-iacs-base/code#SpecieCodeValue/avenaNudaLSmallNakedOatHullessOat>
        a                cap-iacs-base:SpecieCodeValue ;
        rdfs:label       "Avena nuda L. Small naked oat / Hulless oat "@en ;
        skos:definition  "-- Definition --\r\nAvena nuda L. Small naked oat / Hulless oat.\r\n-- Description --\r\nList of agricultural species -A   \r\nIV. Cereals\r\nNOTE. Initial value: A - 72."@en ;
        skos:inScheme    cap-iacs-basecode:SpecieCodeValue .

<http://lpis.ec.europa.eu/registry/applicationschema/cap-iacs-base/code#AffectedElementTypeValue/attribute>
        a                cap-iacs-base:AffectedElementTypeValue ;
        rdfs:label       "Property"@en ;
        skos:definition  "--Name--\r\nAttribute\r\n\r\n-- Definition --\r\nUML feature  within a classifier that describes a range of values (B.515) that instances of the classifier may hold. [ISO/TS 19103:2005 – adapted from ISO/IEC 19501]"@en ;
        skos:inScheme    cap-iacs-basecode:AffectedElementTypeValue .

<http://lpis.ec.europa.eu/registry/applicationschema/cap-iacs-base/code#FarmStructureSurveyNumberValue/durumWheat>
        a                cap-iacs-base:FarmStructureSurveyNumberValue ;
        rdfs:label       "Durum wheat"@en ;
        skos:definition  "-- Definition --\r\nDurum wheat.\r\n-- Description --\r\nTriticum durum Desf.\r\nNOTE. Initial value:2.01.01.02"@en ;
        skos:inScheme    cap-iacs-basecode:FarmStructureSurveyNumberValue .

<http://lpis.ec.europa.eu/registry/applicationschema/cap-iacs-base/code#ConformanceStatementValue/nonConforming>
        a                cap-iacs-base:ConformanceStatementValue ;
        rdfs:label       "Non-conforming"@en ;
        skos:definition  "-- Name--\r\nNon-conforming\r\n\r\n-- Description --\r\nThe tested object does not comply with rules, standards, or laws."@en ;
        skos:inScheme    cap-iacs-basecode:ConformanceStatementValue .

cap-iacs-basecode:TestTypeValue
        a                skos:ConceptScheme ;
        rdfs:label       "Test type value list"@en ;
        dct:isFormatOf   cap-iacs-base:TestTypeValue ;
        skos:definition  "--Name--\r\nTest type value\r\n\r\n-- Definition --\r\nIndication whether a test belong to the basic or the capability test type.\r\n\r\n-- Description --\r\nA basic test is an initial test intended to identify clear cases of non-conformance. If the ATS identifies tests to be used as basic tests, they shall be used at the start of the conformance assessment process.\r\n\r\nCapability test is designed to determine whether an IUT conforms to a particular characteristic specified as requirements."@en .

<http://lpis.ec.europa.eu/registry/applicationschema/cap-iacs-base/code#SpecieCodeValue/daucusCarotaLCarrot>
        a                cap-iacs-base:SpecieCodeValue ;
        rdfs:label       "Daucus carota L. Carrot"@en ;
        skos:definition  "-- Definition --\r\nDaucus carota L. Carrot.\r\n-- Description --\r\nList of vegetable specie -H\r\nNOTE. Initial value: H - 21.1"@en ;
        skos:inScheme    cap-iacs-basecode:SpecieCodeValue .

<http://lpis.ec.europa.eu/registry/applicationschema/cap-iacs-base/code#MonthValue/july>
        a                cap-iacs-base:MonthValue ;
        rdfs:label       "July"@en ;
        skos:definition  "-- Definition --\r\nJuly.\r\n-- Description --\r\nItem description."@en ;
        skos:inScheme    cap-iacs-basecode:MonthValue .

<http://lpis.ec.europa.eu/registry/applicationschema/cap-iacs-base/code#SupportSchemeTypeValue/voluntaryCoupledSupport>
        a                cap-iacs-base:SupportSchemeTypeValue ;
        rdfs:label       "Voluntary coupled support"@en ;
        skos:definition  "Voluntary coupled support\r\n\r\nMember States may grant coupled support to farmers  for\r\n\t- cereals, \r\n\t- oilseeds, \r\n\t- protein crops, \r\n\t- grain legumes, \r\n\t- flax, \r\n\t- hemp, \r\n\t- rice, \r\n\t- nuts, \r\n\t- starch potato, \r\n\t- milk and milk products, \r\n\t- seeds, \r\n\t- sheepmeat and goatmeat, \r\n\t- beef and veal, \r\n\t- olive oil, \r\n\t- silkworms, \r\n\t- dried fodder, \r\n\t- hops, \r\n\t- sugar beet, \r\n\t- cane and chicory, \r\n\t- fruit and vegetables and \r\n\t- short rotation coppice.\r\n\r\nNOTE\r\nDetails in Title IV, Chapter 1 of R 1307/2013."@en ;
        skos:inScheme    cap-iacs-basecode:SupportSchemeTypeValue .

<http://lpis.ec.europa.eu/registry/applicationschema/cap-iacs-base/code#CropItemCodeValue/fruitAndBerryPlantations>
        a                cap-iacs-base:CropItemCodeValue ;
        rdfs:label       "Fruit and berry plantations"@en ;
        skos:definition  "-- Definition --\r\n|||Fruit and berry plantations.\r\n-- Description --\r\nLand use of Agriculture Area in Use -L\r\nNOTE. Initial value:L0011"@en ;
        skos:inScheme    cap-iacs-basecode:CropItemCodeValue .

<http://lpis.ec.europa.eu/registry/applicationschema/cap-iacs-base/code#CropItemCodeValue/annualPlantsHarvestedGreenC2611>
        a                cap-iacs-base:CropItemCodeValue ;
        rdfs:label       "Annual plants harvested green C2611"@en ;
        skos:definition  "-- Definition --\r\n||Annual plants harvested green C2611.\r\n-- Description --\r\nCereals and main crops - C\r\nNOTE. Initial value:C2611"@en ;
        skos:inScheme    cap-iacs-basecode:CropItemCodeValue .

<http://lpis.ec.europa.eu/registry/applicationschema/cap-iacs-base/code#CropItemCodeValue/chicoryForInulin>
        a                cap-iacs-base:CropItemCodeValue ;
        rdfs:label       "Chicory for inulin"@en ;
        skos:definition  "-- Definition --\r\n||||Chicory for inulin.\r\n-- Description --\r\nCereals and main crops - C\r\nNOTE. Initial value:C1572"@en ;
        skos:inScheme    cap-iacs-basecode:CropItemCodeValue .

<http://lpis.ec.europa.eu/registry/applicationschema/cap-iacs-base/code#CropItemCodeValue/lucerne>
        a                cap-iacs-base:CropItemCodeValue ;
        rdfs:label       "Lucerne"@en ;
        skos:definition  "-- Definition --\r\n|||Lucerne.\r\n-- Description --\r\nCereals and main crops - C\r\nNOTE. Initial value:C2672"@en ;
        skos:inScheme    cap-iacs-basecode:CropItemCodeValue .

<http://lpis.ec.europa.eu/registry/applicationschema/cap-iacs-base/code#SpecieCodeValue/brassicaOleraceaLFodderKale>
        a                cap-iacs-base:SpecieCodeValue ;
        rdfs:label       "Brassica oleracea L. Fodder kale "@en ;
        skos:definition  "-- Definition --\r\nBrassica oleracea L. Fodder kale.\r\n-- Description --\r\nList of agricultural species -A\r\nII. Fodder plants\r\nNOTE. Initial value: A - 55."@en ;
        skos:inScheme    cap-iacs-basecode:SpecieCodeValue .

<http://lpis.ec.europa.eu/registry/applicationschema/cap-iacs-base/code#FarmStructureSurveyNumberValue/tableGrapes>
        a                cap-iacs-base:FarmStructureSurveyNumberValue ;
        rdfs:label       "Table grapes"@en ;
        skos:definition  "-- Definition --\r\nTable grapes.\r\n-- Description --\r\nGrape varieties normally grown for the production of fresh grapes.\r\nNOTE. Initial value:2.04.04.03"@en ;
        skos:inScheme    cap-iacs-basecode:FarmStructureSurveyNumberValue .

<http://lpis.ec.europa.eu/registry/applicationschema/cap-iacs-base/code#WeekdayValue/friday>
        a                cap-iacs-base:WeekdayValue ;
        rdfs:label       "Friday"@en ;
        skos:definition  "-- Definition --\r\nFriday.\r\n-- Description --\r\nItem description."@en ;
        skos:inScheme    cap-iacs-basecode:WeekdayValue .

<http://lpis.ec.europa.eu/registry/applicationschema/cap-iacs-base/code#CropItemCodeValue/grainMaizeAndCornCobMix>
        a                cap-iacs-base:CropItemCodeValue ;
        rdfs:label       "Grain maize and corn cob mix"@en ;
        skos:definition  "-- Definition --\r\n|||Grain maize and corn cob mix.\r\n-- Description --\r\nCereals and main crops - C\r\nNOTE. Initial value:C1201"@en ;
        skos:inScheme    cap-iacs-basecode:CropItemCodeValue .

<http://lpis.ec.europa.eu/registry/applicationschema/cap-iacs-base/code#CropItemCodeValue/celeriac>
        a                cap-iacs-base:CropItemCodeValue ;
        rdfs:label       "Celeriac"@en ;
        skos:definition  "-- Definition --\r\n|||Celeriac.\r\n-- Description --\r\nCereals and main crops - C\r\nNOTE. Initial value:C1872"@en ;
        skos:inScheme    cap-iacs-basecode:CropItemCodeValue .

<http://lpis.ec.europa.eu/registry/applicationschema/cap-iacs-base/code#SpecieCodeValue/poaAnnuaLAnnualMeadowgrass>
        a                cap-iacs-base:SpecieCodeValue ;
        rdfs:label       "Poa annua L. Annual meadowgrass"@en ;
        skos:definition  "-- Definition --\r\nPoa annua L. Annual meadowgrass.\r\n-- Description --\r\nList of agricultural species -A\r\nII. Fodder plants\r\nNOTE. Initial value: A - 26."@en ;
        skos:inScheme    cap-iacs-basecode:SpecieCodeValue .

<http://lpis.ec.europa.eu/registry/applicationschema/cap-iacs-base/code#FarmStructureSurveyNumberValue/lallowLandWithoutAnySubsidies>
        a                cap-iacs-base:FarmStructureSurveyNumberValue ;
        rdfs:label       "Fallow land without any subsidies"@en ;
        skos:definition  "-- Definition --\r\nFallow land without any subsidies.\r\n-- Description --\r\nFallow land for which no financial aid or subsidy is paid.\r\nNOTE. Initial value:2.01.12.01"@en ;
        skos:inScheme    cap-iacs-basecode:FarmStructureSurveyNumberValue .

<http://lpis.ec.europa.eu/registry/applicationschema/cap-iacs-base/code#SpecieCodeValue/hordeumVulgareLBarley2RowBarley>
        a                cap-iacs-base:SpecieCodeValue ;
        rdfs:label       "Hordeum vulgare L. Barley 2-row barley "@en ;
        skos:definition  "-- Definition --\r\nHordeum vulgare L. Barley 2-row barley \r\n-- Description --\r\nList of agricultural species -A   \r\nIV. Cereals\r\nNOTE. Initial value: A - 75.1"@en ;
        skos:inScheme    cap-iacs-basecode:SpecieCodeValue .

<http://lpis.ec.europa.eu/registry/applicationschema/cap-iacs-base/code#CropItemCodeValue/mainOilSeedCrops>
        a                cap-iacs-base:CropItemCodeValue ;
        rdfs:label       "Main oil seed crops"@en ;
        skos:definition  "-- Definition --\r\n|||Main oil seed crops.\r\n-- Description --\r\nCereals and main crops - C\r\nNOTE. Initial value:C1415"@en ;
        skos:inScheme    cap-iacs-basecode:CropItemCodeValue .

<http://lpis.ec.europa.eu/registry/applicationschema/cap-iacs-base/code#CropItemCodeValue/watermelons>
        a                cap-iacs-base:CropItemCodeValue ;
        rdfs:label       "Watermelons"@en ;
        skos:definition  "-- Definition --\r\n||Watermelons.\r\n-- Description --\r\nCereals and main crops - C\r\nNOTE. Initial value:C1777"@en ;
        skos:inScheme    cap-iacs-basecode:CropItemCodeValue .

cap-iacs-basecode:ConformanceClassValue
        a                skos:ConceptScheme ;
        rdfs:label       "List of conformance class values"@en ;
        dct:isFormatOf   cap-iacs-base:ConformanceClassValue ;
        skos:definition  "--Name--\r\nConformance class value\r\n\r\n--Definition--\r\nList of conformance class values.\r\n\r\n--Description--\r\nAny product claiming conformance with one of these classes shall pass all requirements described in the corresponding abstract test suite.\r\n\r\nNOTE. Requirements of conformance classes may overlap in which case subparts of the abstract test suite may be shared between different conformance classes."@en .

<http://lpis.ec.europa.eu/registry/applicationschema/cap-iacs-base/code#WeekdayValue/wednesday>
        a                cap-iacs-base:WeekdayValue ;
        rdfs:label       "Wednesday"@en ;
        skos:definition  "-- Definition --\r\nWednesday.\r\n-- Description --\r\nItem description."@en ;
        skos:inScheme    cap-iacs-basecode:WeekdayValue .

<http://lpis.ec.europa.eu/registry/applicationschema/cap-iacs-base/code#TestingTypeValue/automated>
        a                cap-iacs-base:TestingTypeValue ;
        rdfs:label       "Automated testing"@en ;
        skos:definition  "--Name--\r\nAutomated\r\n\r\n-- Definition --\r\nAutomated test.\r\n\r\n-- Description --\r\nAutomated testing may implement the required tests as a software system using either verification testing or falsification testing."@en ;
        skos:inScheme    cap-iacs-basecode:TestingTypeValue .

<http://lpis.ec.europa.eu/registry/applicationschema/cap-iacs-base/code#CropItemCodeValue/otherRootCropsNecL1380>
        a                cap-iacs-base:CropItemCodeValue ;
        rdfs:label       "Other root crops n.e.c. L1380"@en ;
        skos:definition  "-- Definition --\r\n||||Other root crops n.e.c. L1380.\r\n-- Description --\r\nLand use of Agriculture Area in Use -L\r\nNOTE. Initial value:L1380"@en ;
        skos:inScheme    cap-iacs-basecode:CropItemCodeValue .

<http://lpis.ec.europa.eu/registry/applicationschema/cap-iacs-base/code#SpecieCodeValue/phleumNodosumLSmallTimothy>
        a                cap-iacs-base:SpecieCodeValue ;
        rdfs:label       "Phleum nodosum L. Small timothy"@en ;
        skos:definition  "-- Definition --\r\nPhleum nodosum L. Small timothy.\r\n-- Description --\r\nList of agricultural species -A\r\nII. Fodder plants\r\nNOTE. Initial value: A - 24."@en ;
        skos:inScheme    cap-iacs-basecode:SpecieCodeValue .

<http://lpis.ec.europa.eu/registry/applicationschema/cap-iacs-base/code#CropItemCodeValue/otherPermanentCrops>
        a                cap-iacs-base:CropItemCodeValue ;
        rdfs:label       "Other permanent crops"@en ;
        skos:definition  "-- Definition --\r\n|||Other permanent crops.\r\n-- Description --\r\nLand use of Agriculture Area in Use -L\r\nNOTE. Initial value:L2980"@en ;
        skos:inScheme    cap-iacs-basecode:CropItemCodeValue .

<http://lpis.ec.europa.eu/registry/applicationschema/cap-iacs-base/code#CropItemCodeValue/eggplantsGourdsMarrowsCourgettesPumpkins>
        a                cap-iacs-base:CropItemCodeValue ;
        rdfs:label       "Eggplants, gourds, marrows, courgettes, pumpkins"@en ;
        skos:definition  "-- Definition --\r\n|||Eggplants, gourds, marrows, courgettes, pumpkins.\r\n-- Description --\r\nCereals and main crops - C\r\nNOTE. Initial value:C1780"@en ;
        skos:inScheme    cap-iacs-basecode:CropItemCodeValue .

<http://lpis.ec.europa.eu/registry/applicationschema/cap-iacs-base/code#CropItemCodeValue/flowersAndOrnamentalPlantsUnderGlassHighAccessibleCover>
        a                cap-iacs-base:CropItemCodeValue ;
        rdfs:label       "Flowers and ornamental plants under glass high accessible cover"@en ;
        skos:definition  "-- Definition --\r\nFlowers and ornamental plants under glass high accessible cover.\r\n-- Description --\r\nLand use of Agriculture Area in Use -L. Special aggregates\r\nNOTE. Initial value:L1113"@en ;
        skos:inScheme    cap-iacs-basecode:CropItemCodeValue .

<http://lpis.ec.europa.eu/registry/applicationschema/cap-iacs-base/code#FarmStructureSurveyNumberValue/otherArableLandCrops>
        a                cap-iacs-base:FarmStructureSurveyNumberValue ;
        rdfs:label       "Other arable land crops"@en ;
        skos:definition  "-- Definition --\r\nOther arable land crops.\r\n-- Description --\r\nArable crops not included elsewhere.\r\nNOTE. Initial value:2.01.11"@en ;
        skos:inScheme    cap-iacs-basecode:FarmStructureSurveyNumberValue .

<http://lpis.ec.europa.eu/registry/applicationschema/cap-iacs-base/code#NotificationGroupValue/notificationsConcerningThePaymentForAreasWithNaturalConstraints>
        a                cap-iacs-base:NotificationGroupValue ;
        rdfs:label       "Notifications concerning the payment for areas with natural constraints"@en ;
        skos:definition  "-- Definition --\r\nNotifications concerning the payment for areas with natural constraints.\r\n-- Description --\r\nNOTE.69"@en ;
        skos:inScheme    cap-iacs-basecode:NotificationGroupValue .

<http://lpis.ec.europa.eu/registry/applicationschema/cap-iacs-base/code#CropItemCodeValue/aromaticPlantsMedicinalAndCulinaryPlants>
        a                cap-iacs-base:CropItemCodeValue ;
        rdfs:label       "Aromatic plants, medicinal and culinary plants"@en ;
        skos:definition  "-- Definition --\r\n|||Aromatic plants, medicinal and culinary plants.\r\n-- Description --\r\nCereals and main crops - C\r\nNOTE. Initial value:C1580"@en ;
        skos:inScheme    cap-iacs-basecode:CropItemCodeValue .

<http://lpis.ec.europa.eu/registry/applicationschema/cap-iacs-base/code#CropItemCodeValue/redPepperCapsicumUnderGlassOrHighAccessibleCoverC1791>
        a                cap-iacs-base:CropItemCodeValue ;
        rdfs:label       "Red pepper, capsicum under glass or high accessible cover C1791"@en ;
        skos:definition  "-- Definition --\r\n||||Red pepper, capsicum under glass or high accessible cover C1791.\r\n-- Description --\r\nCereals and main crops - C\r\nNOTE. Initial value:C1791"@en ;
        skos:inScheme    cap-iacs-basecode:CropItemCodeValue .

<http://lpis.ec.europa.eu/registry/applicationschema/cap-iacs-base/code#SpecieCodeValue/asparagusOfficinalisLAsparagus>
        a                cap-iacs-base:SpecieCodeValue ;
        rdfs:label       "Asparagus officinalis L. Asparagus"@en ;
        skos:definition  "-- Definition --\r\nAsparagus officinalis L. Asparagus.\r\n-- Description --\r\nList of vegetable specie -H\r\nNOTE. Initial value: H - 8."@en ;
        skos:inScheme    cap-iacs-basecode:SpecieCodeValue .

<http://lpis.ec.europa.eu/registry/applicationschema/cap-iacs-base/code#SupportSchemeTypeValue/smallFarmersScheme>
        a                cap-iacs-base:SupportSchemeTypeValue ;
        rdfs:label       "Small farmers scheme"@en ;
        skos:definition  "Small farmers scheme\r\n\r\nMember States may establish a scheme for small farmers in accordance with the conditions laid down in this Title.\r\n\r\nAccording to Title V of 1307/2013 Regulation it is a decoupled payment."@en ;
        skos:inScheme    cap-iacs-basecode:SupportSchemeTypeValue .

<http://lpis.ec.europa.eu/registry/applicationschema/cap-iacs-base/code#FarmStructureSurveyNumberValue/raisins>
        a                cap-iacs-base:FarmStructureSurveyNumberValue ;
        rdfs:label       "Raisins"@en ;
        skos:definition  "-- Definition --\r\nRaisins.\r\n-- Description --\r\nGrape varieties normally grown for the production of raisins.\r\nNOTE. Initial value:2.04.04.04"@en ;
        skos:inScheme    cap-iacs-basecode:FarmStructureSurveyNumberValue .

<http://lpis.ec.europa.eu/registry/applicationschema/cap-iacs-base/code#SupportSchemeTypeValue/aegeanIslands>
        a                cap-iacs-base:SupportSchemeTypeValue ;
        rdfs:label       "Aegean islands"@en ;
        skos:definition  "Aegean islands\r\n\r\nChapter IV of Regulation (EU) No 229/2013 / Direct payments under measures established in the programmes: Specific measures in favour of the smaller Aegean islands."@en ;
        skos:inScheme    cap-iacs-basecode:SupportSchemeTypeValue .

<http://lpis.ec.europa.eu/registry/applicationschema/cap-iacs-base/code#NotificationGroupValue/notificationsRelatingToTheImplementationOfGaecAndFas>
        a                cap-iacs-base:NotificationGroupValue ;
        rdfs:label       "Notifications relating to the implementation of GAEC and FAS"@en ;
        skos:definition  "-- Definition --\r\nNotifications relating to the implementation of GAEC and FAS.\r\n-- Description --\r\nMember States shall inform the Commission in detail of the measures taken to implement the good agricultural and environmental condition referred to in Article 94 and the details of the farm advisory system referred to in Title \r\nIII.\r\nNOTE.1012"@en ;
        skos:inScheme    cap-iacs-basecode:NotificationGroupValue .

<http://lpis.ec.europa.eu/registry/applicationschema/cap-iacs-base/code#ConformanceLevelValue/level1>
        a                cap-iacs-base:ConformanceLevelValue ;
        rdfs:label       "Level 1 low"@en ;
        skos:definition  "--Name--\r\nLevel 1\r\n\r\n--Definition--\r\nLowest level conformance.\r\n\r\n--Description--\r\nA separate abstract test suite must be provided if a level is defined within ConformanceClause."@en ;
        skos:inScheme    cap-iacs-basecode:ConformanceLevelValue .

<http://lpis.ec.europa.eu/registry/applicationschema/cap-iacs-base/code#FarmStructureSurveyNumberValue/marketGardening>
        a                cap-iacs-base:FarmStructureSurveyNumberValue ;
        rdfs:label       "Market gardening"@en ;
        skos:definition  "-- Definition --\r\nMarket gardening.\r\n-- Description --\r\nFresh vegetables, melons and strawberries grown on arable land in rotation with other horticultural crops.\r\nNOTE. Initial value:2.01.07.01.02"@en ;
        skos:inScheme    cap-iacs-basecode:FarmStructureSurveyNumberValue .

<http://lpis.ec.europa.eu/registry/applicationschema/cap-iacs-base/code#SupportSchemeTypeValue/paymentForYoungFarmers>
        a                cap-iacs-base:SupportSchemeTypeValue ;
        rdfs:label       "Payment for young farmers"@en ;
        skos:definition  "Payment for young farmers\r\n\r\nMember States shall grant an annual payment to young farmers who are entitled to a payment under the basic payment scheme or the single area payment scheme referred to in Chapter 1.\r\n\r\nAccording to Title III, Chapter 5 of 1307/2013 Regulation it is a decoupled payment."@en ;
        skos:inScheme    cap-iacs-basecode:SupportSchemeTypeValue .

<http://lpis.ec.europa.eu/registry/applicationschema/cap-iacs-base/code#CropItemCodeValue/cultivatedMushrooms>
        a                cap-iacs-base:CropItemCodeValue ;
        rdfs:label       "Cultivated mushrooms"@en ;
        skos:definition  "-- Definition --\r\n|Cultivated mushrooms.\r\n-- Description --\r\nCereals and main crops - C\r\nNOTE. Initial value:C1910"@en ;
        skos:inScheme    cap-iacs-basecode:CropItemCodeValue .

<http://lpis.ec.europa.eu/registry/applicationschema/cap-iacs-base/code#SpecieCodeValue/lupinusAngustifoliusLNarrowLeavedLupin>
        a                cap-iacs-base:SpecieCodeValue ;
        rdfs:label       "Lupinus angustifolius L. Narrow leaved lupin"@en ;
        skos:definition  "-- Definition --\r\nLupinus angustifolius L. Narrow leaved lupin.\r\n-- Description --\r\nList of agricultural species -A\r\nII. Fodder plants\r\nNOTE. Initial value: A - 36."@en ;
        skos:inScheme    cap-iacs-basecode:SpecieCodeValue .

<http://lpis.ec.europa.eu/registry/applicationschema/cap-iacs-base/code#CropItemCodeValue/lettuces>
        a                cap-iacs-base:CropItemCodeValue ;
        rdfs:label       "Lettuces"@en ;
        skos:definition  "-- Definition --\r\n|||Lettuces.\r\n-- Description --\r\nCereals and main crops - C\r\nNOTE. Initial value:C1680"@en ;
        skos:inScheme    cap-iacs-basecode:CropItemCodeValue .

<http://lpis.ec.europa.eu/registry/applicationschema/cap-iacs-base/code#CropItemCodeValue/pears>
        a                cap-iacs-base:CropItemCodeValue ;
        rdfs:label       "Pears"@en ;
        skos:definition  "-- Definition --\r\n||Pears.\r\n-- Description --\r\nCereals and main crops - C\r\nNOTE. Initial value:C2095"@en ;
        skos:inScheme    cap-iacs-basecode:CropItemCodeValue .

<http://lpis.ec.europa.eu/registry/applicationschema/cap-iacs-base/code#CropItemCodeValue/beans>
        a                cap-iacs-base:CropItemCodeValue ;
        rdfs:label       "Beans"@en ;
        skos:definition  "-- Definition --\r\n|||Beans.\r\n-- Description --\r\nCereals and main crops - C\r\nNOTE. Initial value:C1901"@en ;
        skos:inScheme    cap-iacs-basecode:CropItemCodeValue .

<http://lpis.ec.europa.eu/registry/applicationschema/cap-iacs-base/code#ConformanceClassValue/classC>
        a                cap-iacs-base:ConformanceClassValue ;
        rdfs:label       "Class C"@en ;
        skos:definition  "--Name--\r\nClass C\r\n\r\n--Definition--\r\nSpecified conformance class.\r\n\r\n--Description--\r\nSeparate ATS must be provided if a class is defined within ConformanceClause."@en ;
        skos:inScheme    cap-iacs-basecode:ConformanceClassValue .

<http://lpis.ec.europa.eu/registry/applicationschema/cap-iacs-base/code#SpecieCodeValue/cichoriumIntybusLIndustrialChicory>
        a                cap-iacs-base:SpecieCodeValue ;
        rdfs:label       "Cichorium intybus L. Industrial chicory"@en ;
        skos:definition  "-- Definition --\r\nCichorium intybus L. Industrial chicory.\r\n-- Description --\r\nList of vegetable specie -H\r\nNOTE. Initial value: H - 14.3"@en ;
        skos:inScheme    cap-iacs-basecode:SpecieCodeValue .

<http://lpis.ec.europa.eu/registry/applicationschema/cap-iacs-base/code#AffectedElementTypeValue/multiplicity>
        a                cap-iacs-base:AffectedElementTypeValue ;
        rdfs:label       "Enumeration"@en ;
        skos:definition  "--Name--\r\nMultiplicity\r\n\r\n-- Definition --\r\nSpecification of the range of allowable cardinalities that a set may assume."@en ;
        skos:inScheme    cap-iacs-basecode:AffectedElementTypeValue .

<http://lpis.ec.europa.eu/registry/applicationschema/cap-iacs-base/code#FarmStructureSurveyNumberValue/freshVegetablesMelonsAndStrawberriesOfWhich>
        a                cap-iacs-base:FarmStructureSurveyNumberValue ;
        rdfs:label       "Fresh vegetables, melons and strawberries of which:"@en ;
        skos:definition  "-- Definition --\r\nFresh vegetables, melons and strawberries of which:\r\n-- Description --\r\nFresh vegetables, melons and strawberries of which:\r\nNOTE. Initial value:2.01.07"@en ;
        skos:inScheme    cap-iacs-basecode:FarmStructureSurveyNumberValue .

<http://lpis.ec.europa.eu/registry/applicationschema/cap-iacs-base/code#NotificationGroupValue/notificationsRelatingToTheApplicationOfTheIntegratedSystem>
        a                cap-iacs-base:NotificationGroupValue ;
        rdfs:label       "Notifications relating to the application of the integrated system"@en ;
        skos:definition  "-- Definition --\r\nNotifications relating to the the application of the integrated system.\r\n-- Description --\r\nMember State shall inform the Commission regularly of the application of the integrated system referred to in Chapter II of Title V. The Commission shall organize exchanges of views on this subject with the Member States.\r\nNOTE.1023"@en ;
        skos:inScheme    cap-iacs-basecode:NotificationGroupValue .

<http://lpis.ec.europa.eu/registry/applicationschema/cap-iacs-base/code#FarmStructureSurveyNumberValue/fallowLand>
        a                cap-iacs-base:FarmStructureSurveyNumberValue ;
        rdfs:label       "Fallow land"@en ;
        skos:definition  "-- Definition --\r\nFallow land.\r\n-- Description --\r\nAll arable land included in the crop rotation system, whether worked or not, but with no intention to produce a harvest for the duration of a crop year.\r\nThe essential characteristic of fallow land is that it is left to recover, normally for the whole of a crop year.\r\nFallow land may be:\r\n1. bare land bearing no crops at all;\r\n2. land with spontaneous natural growth, which may be used as feed or ploughed in;\r\n3. land sown exclusively for the production of green manure (green fallow).\r\nAll areas of arable land maintained in good agricultural and environmental conditions as set out in Article 5 of the Council Regulation (EC) No 1782/2003(1)\r\nOJ L 270, 21.10.2003, p. 1. (1) or, where applicable, in the most recent legislation, regardless of whether they are part of the crop rotation or not, are included.\r\nNOTE. Initial value:2.01.12"@en ;
        skos:inScheme    cap-iacs-basecode:FarmStructureSurveyNumberValue .

<http://lpis.ec.europa.eu/registry/applicationschema/cap-iacs-base/code#FarmStructureSurveyNumberValue/outdoorOrUnderLowNotAccessibleProtectiveCover>
        a                cap-iacs-base:FarmStructureSurveyNumberValue ;
        rdfs:label       "Outdoor or under low (not accessible) protective cover"@en ;
        skos:definition  "-- Definition --\r\nOutdoor or under low (not accessible) protective cover.\r\n-- Description --\r\nFresh vegetables, melons and strawberries, outdoor or under low (non-accessible) cover.\r\nNOTE. Initial value:2.01.07.01"@en ;
        skos:inScheme    cap-iacs-basecode:FarmStructureSurveyNumberValue .

<http://lpis.ec.europa.eu/registry/applicationschema/cap-iacs-base/code#NotificationGroupValue/notificationsRelatingToTheCertificationBodies>
        a                cap-iacs-base:NotificationGroupValue ;
        rdfs:label       "Notifications relating to the certification bodies"@en ;
        skos:definition  "-- Definition --\r\nNotifications relating to the certification bodies.\r\n-- Description --\r\nIn addition to the provisions laid down in the sectoral Regulations, Member States shall send to the Commission the information, declarations and documents:  for certification bodies:\r\n(b)(i) their name;\r\n(b)(ii) their address,\r\nNOTE.1011b"@en ;
        skos:inScheme    cap-iacs-basecode:NotificationGroupValue .

<http://lpis.ec.europa.eu/registry/applicationschema/cap-iacs-base/code#SpecieCodeValue/trifoliumRepensLWhiteClover>
        a                cap-iacs-base:SpecieCodeValue ;
        rdfs:label       "Trifolium repens L. White clover"@en ;
        skos:definition  "-- Definition --\r\nTrifolium repens L. White clover.\r\n-- Description --\r\nList of agricultural species -A\r\nII. Fodder plants\r\nNOTE. Initial value: A - 47."@en ;
        skos:inScheme    cap-iacs-basecode:SpecieCodeValue .

<http://lpis.ec.europa.eu/registry/applicationschema/cap-iacs-base/code#SpecieCodeValue/trifoliumResupinatumLPersianClover>
        a                cap-iacs-base:SpecieCodeValue ;
        rdfs:label       "Trifolium resupinatum L. Persian clover"@en ;
        skos:definition  "-- Definition --\r\nTrifolium resupinatum L. Persian clover.\r\n-- Description --\r\nList of agricultural species -A\r\nII. Fodder plants\r\nNOTE. Initial value: A - 48."@en ;
        skos:inScheme    cap-iacs-basecode:SpecieCodeValue .

<http://lpis.ec.europa.eu/registry/applicationschema/cap-iacs-base/code#FarmStructureSurveyNumberValue/flowersAndOrnamentalPlantsExcludingNurseries>
        a                cap-iacs-base:FarmStructureSurveyNumberValue ;
        rdfs:label       "Flowers and ornamental plants (excluding nurseries)"@en ;
        skos:definition  "-- Definition --\r\nFlowers and ornamental plants (excluding nurseries).\r\n-- Description --\r\nFlowers and ornamental plants (excluding nurseries).\r\nNOTE. Initial value:2.01.08"@en ;
        skos:inScheme    cap-iacs-basecode:FarmStructureSurveyNumberValue .

<http://lpis.ec.europa.eu/registry/applicationschema/cap-iacs-base/code#CropItemCodeValue/soya>
        a                cap-iacs-base:CropItemCodeValue ;
        rdfs:label       "Soya "@en ;
        skos:definition  "-- Definition --\r\n||||Soya.\r\n-- Description --\r\nCereals and main crops - C\r\nNOTE. Initial value:C1470"@en ;
        skos:inScheme    cap-iacs-basecode:CropItemCodeValue .

<http://lpis.ec.europa.eu/registry/applicationschema/cap-iacs-base/code#FarmStructureSurveyNumberValue/rye>
        a                cap-iacs-base:FarmStructureSurveyNumberValue ;
        rdfs:label       "Rye"@en ;
        skos:definition  "-- Definition --\r\nRye.\r\n-- Description --\r\nSecale cereale L., including mixtures of rye and other cereals sown in the autumn (maslin).\r\nNOTE. Initial value:2.01.01.03"@en ;
        skos:inScheme    cap-iacs-basecode:FarmStructureSurveyNumberValue .

<http://lpis.ec.europa.eu/registry/applicationschema/cap-iacs-base/code#FarmStructureSurveyNumberValue/otherPlantsHarvestedGreen>
        a                cap-iacs-base:FarmStructureSurveyNumberValue ;
        rdfs:label       "Other plants harvested green"@en ;
        skos:definition  "-- Definition --\r\nOther plants harvested green.\r\n-- Description --\r\nOther annual or multiannual (less than five years) fodder crops.\r\nNOTE. Initial value:2.01.09.02"@en ;
        skos:inScheme    cap-iacs-basecode:FarmStructureSurveyNumberValue .

<http://lpis.ec.europa.eu/registry/applicationschema/cap-iacs-base/code#SpecieCodeValue/trifoliumIncarnatumLCrimsonClover>
        a                cap-iacs-base:SpecieCodeValue ;
        rdfs:label       "Trifolium incarnatum L. Crimson clover"@en ;
        skos:definition  "-- Definition --\r\nTrifolium incarnatum L. Crimson clover.\r\n-- Description --\r\nList of agricultural species -A\r\nII. Fodder plants\r\nNOTE. Initial value: A - 45."@en ;
        skos:inScheme    cap-iacs-basecode:SpecieCodeValue .

<http://lpis.ec.europa.eu/registry/applicationschema/cap-iacs-base/code#RecurenceValue/monthly>
        a                cap-iacs-base:RecurenceValue ;
        rdfs:label       "Monthly recurrence"@en ;
        skos:definition  "-- Definition --\r\nMonthly recurrence.\r\n-- Description --\r\nItem description."@en ;
        skos:inScheme    cap-iacs-basecode:RecurenceValue .

<http://lpis.ec.europa.eu/registry/applicationschema/cap-iacs-base/code#CropItemCodeValue/linseedOilFlax>
        a                cap-iacs-base:CropItemCodeValue ;
        rdfs:label       "Linseed (oil flax)"@en ;
        skos:definition  "-- Definition --\r\n||||Linseed (oil flax).\r\n-- Description --\r\nCereals and main crops - C\r\nNOTE. Initial value:C1460"@en ;
        skos:inScheme    cap-iacs-basecode:CropItemCodeValue .

<http://lpis.ec.europa.eu/registry/applicationschema/cap-iacs-base/code#SpecieCodeValue/brassicaOleraceaLSproutingBroccoliCalabrese>
        a                cap-iacs-base:SpecieCodeValue ;
        rdfs:label       "Brassica oleracea L. Sprouting broccoli / Calabrese"@en ;
        skos:definition  "-- Definition --\r\nBrassica oleracea L. Sprouting broccoli / Calabrese.\r\n-- Description --\r\nList of vegetable specie -H\r\nNOTE. Initial value: H - 10.3"@en ;
        skos:inScheme    cap-iacs-basecode:SpecieCodeValue .

<http://lpis.ec.europa.eu/registry/applicationschema/cap-iacs-base/code#CropItemCodeValue/springDurumWheat>
        a                cap-iacs-base:CropItemCodeValue ;
        rdfs:label       "Spring durum wheat"@en ;
        skos:definition  "-- Definition --\r\n|||||Spring durum wheat.\r\n-- Description --\r\nCereals and main crops - C\r\nNOTE. Initial value:C1134"@en ;
        skos:inScheme    cap-iacs-basecode:CropItemCodeValue .

<http://lpis.ec.europa.eu/registry/applicationschema/cap-iacs-base/code#SpecieCodeValue/foeniculumVulgareMillFennel>
        a                cap-iacs-base:SpecieCodeValue ;
        rdfs:label       "Foeniculum vulgare Mill. Fennel"@en ;
        skos:definition  "-- Definition --\r\nFoeniculum vulgare Mill. Fennel.\r\n-- Description --\r\nList of vegetable specie -H\r\nNOTE. Initial value: H - 22."@en ;
        skos:inScheme    cap-iacs-basecode:SpecieCodeValue .

<http://lpis.ec.europa.eu/registry/applicationschema/cap-iacs-base/code#CropItemCodeValue/vineyardsForTableGrapes>
        a                cap-iacs-base:CropItemCodeValue ;
        rdfs:label       "Vineyards for table grapes"@en ;
        skos:definition  "-- Definition --\r\n|||Vineyards for table grapes.\r\n-- Description --\r\nCereals and main crops - C\r\nNOTE. Initial value:C2420"@en ;
        skos:inScheme    cap-iacs-basecode:CropItemCodeValue .

<http://lpis.ec.europa.eu/registry/applicationschema/cap-iacs-base/code#SpecieCodeValue/sspAlternativum>
        a                cap-iacs-base:SpecieCodeValue ;
        rdfs:label       "Ssp. alternativum"@en ;
        skos:definition  "-- Definition --\r\nLolium multiflorum Lam. Italian ryegrass (including Westerwold ryegrass) Ssp. alternativum. \r\n-- Description --\r\nList of agricultural species -A\r\nII. Fodder plants\r\nNOTE. Initial value: A - 20.1"@en ;
        skos:inScheme    cap-iacs-basecode:SpecieCodeValue .

<http://lpis.ec.europa.eu/registry/applicationschema/cap-iacs-base/code#SpecieCodeValue/viciaFabaLPartimBroadBean>
        a                cap-iacs-base:SpecieCodeValue ;
        rdfs:label       "Vicia faba L. (partim) Broad bean"@en ;
        skos:definition  "-- Definition --\r\nVicia faba L. (partim) Broad bean.\r\n-- Description --\r\nList of vegetable specie -H\r\nNOTE. Initial value: H - 35."@en ;
        skos:inScheme    cap-iacs-basecode:SpecieCodeValue .

<http://lpis.ec.europa.eu/registry/applicationschema/cap-iacs-base/code#FarmStructureSurveyNumberValue/underGlassOrOtherAccessibleProtectiveCover>
        a                cap-iacs-base:FarmStructureSurveyNumberValue ;
        rdfs:label       "Under glass or other (accessible) protective cover"@en ;
        skos:definition  "-- Definition --\r\nUnder glass or other (accessible) protective cover.\r\n-- Description --\r\nCrops, which for the whole of their period of growth or for the predominant part of it are covered by greenhouses or fixed or mobile high cover (glass or rigid or flexible plastic).\r\nNOTE. Initial value:2.01.07.02"@en ;
        skos:inScheme    cap-iacs-basecode:FarmStructureSurveyNumberValue .

<http://lpis.ec.europa.eu/registry/applicationschema/cap-iacs-base/code#FarmStructureSurveyNumberValue/otherOilSeedCrops>
        a                cap-iacs-base:FarmStructureSurveyNumberValue ;
        rdfs:label       "Other oil seed crops"@en ;
        skos:definition  "-- Definition --\r\nOther oil seed crops.\r\n-- Description --\r\nOther crops grown mainly for their oil content, harvested as dry grains, which are not mentioned elsewhere.\r\nNOTE. Initial value:2.01.06.08"@en ;
        skos:inScheme    cap-iacs-basecode:FarmStructureSurveyNumberValue .

<http://lpis.ec.europa.eu/registry/applicationschema/cap-iacs-base/code#FarmStructureSurveyNumberValue/vineyardsOfWhichNormallyProducing>
        a                cap-iacs-base:FarmStructureSurveyNumberValue ;
        rdfs:label       "Vineyards, of which normally producing:"@en ;
        skos:definition  "-- Definition --\r\nVineyards, of which normally producing:\r\n-- Description --\r\nPlantations of Vitis vinifera L.\r\nNOTE. Initial value:2.04.04"@en ;
        skos:inScheme    cap-iacs-basecode:FarmStructureSurveyNumberValue .

<http://lpis.ec.europa.eu/registry/applicationschema/cap-iacs-base/code#CropItemCodeValue/tobacco>
        a                cap-iacs-base:CropItemCodeValue ;
        rdfs:label       "Tobacco"@en ;
        skos:definition  "-- Definition --\r\n||Tobacco.\r\n-- Description --\r\nCereals and main crops - C\r\nNOTE. Initial value:C1550"@en ;
        skos:inScheme    cap-iacs-basecode:CropItemCodeValue .

<http://lpis.ec.europa.eu/registry/applicationschema/cap-iacs-base/code#SpecieCodeValue/onobrychisViciifoliaScopSainfoin>
        a                cap-iacs-base:SpecieCodeValue ;
        rdfs:label       "Onobrychis viciifolia Scop. Sainfoin"@en ;
        skos:definition  "-- Definition --\r\nOnobrychis viciifolia Scop. Sainfoin.\r\n-- Description --\r\nList of agricultural species -A\r\nII. Fodder plants\r\nNOTE. Initial value: A - 41."@en ;
        skos:inScheme    cap-iacs-basecode:SpecieCodeValue .

<http://lpis.ec.europa.eu/registry/applicationschema/cap-iacs-base/code#NotificationGroupValue/notificationsConcerningThePriorApprovaSystemForHempCultivation>
        a                cap-iacs-base:NotificationGroupValue ;
        rdfs:label       "Notifications concerning the small farmers scheme"@en ;
        skos:definition  "Notifications concerning the prior approval system for hemp cultivation"@en ;
        skos:inScheme    cap-iacs-basecode:NotificationGroupValue .

<http://lpis.ec.europa.eu/registry/applicationschema/cap-iacs-base/code#SpecieCodeValue/cucurbitaMaximaDuchesneGourd>
        a                cap-iacs-base:SpecieCodeValue ;
        rdfs:label       "Cucurbita Maxima Duchesne Gourd"@en ;
        skos:definition  "-- Definition --\r\nCucurbita Maxima Duchesne Gourd.\r\n-- Description --\r\nList of vegetable specie -H\r\nNOTE. Initial value: H - 18."@en ;
        skos:inScheme    cap-iacs-basecode:SpecieCodeValue .

<http://lpis.ec.europa.eu/registry/applicationschema/cap-iacs-base/code#VarietalNameValue/armador>
        a                cap-iacs-base:VarietalNameValue ;
        rdfs:label       "H - 1.1  Armador"@en ;
        skos:definition  "-- Definition --\r\nH - 1.1  Armador\r\n-- Description --\r\nH - 1.1 Allium cepa L. Aggregatum group - Shallot /  Armador.\r\nNOTE. Initial value: Armador\r\nNOTE. MS - NL (Netherlands)."@en ;
        skos:inScheme    cap-iacs-basecode:VarietalNameValue .

<http://lpis.ec.europa.eu/registry/applicationschema/cap-iacs-base/code#CropItemCodeValue/springRye>
        a                cap-iacs-base:CropItemCodeValue ;
        rdfs:label       "Spring rye"@en ;
        skos:definition  "-- Definition --\r\n|||||Spring rye.\r\n-- Description --\r\nCereals and main crops - C\r\nNOTE. Initial value:C1152"@en ;
        skos:inScheme    cap-iacs-basecode:CropItemCodeValue .

<http://lpis.ec.europa.eu/registry/applicationschema/cap-iacs-base/code#CropItemCodeValue/wheatIncludingSpelt>
        a                cap-iacs-base:CropItemCodeValue ;
        rdfs:label       "Wheat (including spelt)"@en ;
        skos:definition  "-- Definition --\r\n|||Wheat (including spelt).\r\n-- Description --\r\nCereals and main crops - C\r\nNOTE. Initial value:C1100"@en ;
        skos:inScheme    cap-iacs-basecode:CropItemCodeValue .

<http://lpis.ec.europa.eu/registry/applicationschema/cap-iacs-base/code#FarmStructureSurveyNumberValue/totalIrrigableArea>
        a                cap-iacs-base:FarmStructureSurveyNumberValue ;
        rdfs:label       "Total irrigable area"@en ;
        skos:definition  "-- Definition --\r\nTotal irrigable area.\r\n-- Description --\r\nTotal maximum utilised agricultural area which could be irrigated in the reference year using the equipment and the quantity of water normally available on the holding.\r\nNOTE. Initial value:2.06.02.01"@en ;
        skos:inScheme    cap-iacs-basecode:FarmStructureSurveyNumberValue .

<http://lpis.ec.europa.eu/registry/applicationschema/cap-iacs-base/code#FarmStructureSurveyNumberValue/energyCropsForTheProductionOfBiofuelsOrOtherRenewableEnergy>
        a                cap-iacs-base:FarmStructureSurveyNumberValue ;
        rdfs:label       "Energy crops (for the production of biofuels or other renewable energy)"@en ;
        skos:definition  "-- Definition --\r\nEnergy crops (for the production of biofuels or other renewable energy).\r\n-- Description --\r\nThe production area of energy crops benefiting from the following support schemes under Regulation (EC) No 1782/2003: the specific aid for energy crops (Article 88), the payment linked to set-aside entitlement when production takes place on set-aside area (Article 55 or 56).\r\nOther areas used for the production of energy crops (notably benefiting of the payment linked to‘normal’ entitlement under the Single Payment Scheme or the Simplified Area Payment Scheme) are not covered.\r\nNOTE. Initial value:2.06.03"@en ;
        skos:inScheme    cap-iacs-basecode:FarmStructureSurveyNumberValue .

<http://lpis.ec.europa.eu/registry/applicationschema/cap-iacs-base/code#OrdinalNumberValue/second>
        a                cap-iacs-base:OrdinalNumberValue ;
        rdfs:label       "Second"@en ;
        skos:definition  "-- Definition --\r\nSecond.\r\n-- Description --\r\nItem description."@en ;
        skos:inScheme    cap-iacs-basecode:OrdinalNumberValue .

<http://lpis.ec.europa.eu/registry/applicationschema/cap-iacs-base/code#MonthValue/august>
        a                cap-iacs-base:MonthValue ;
        rdfs:label       "August"@en ;
        skos:definition  "-- Definition --\r\nAugust.\r\n-- Description --\r\nItem description."@en ;
        skos:inScheme    cap-iacs-basecode:MonthValue .

<http://lpis.ec.europa.eu/registry/applicationschema/cap-iacs-base/code#CrossComplianceRuleValue/environmentClimateChangeGoodAgriculturalConditionOfLandWaterGaec1>
        a                cap-iacs-base:CrossComplianceRuleValue ;
        rdfs:label       "Environment, climate change, good agricultural condition of land  - Water GAEC1"@en ;
        skos:definition  "-- Definition --\r\nEnvironment, climate change, good agricultural condition of land  - Water GAEC1.\r\n-- Description --\r\nEstablishment of buffer strips along water courses. The GAEC buffer strips must respect, both within and outside vulnerable zones designated pursuant to Article 3(2) of Directive 91/676/EEC, at least the requirements relating to the conditions for land application of fertiliser near water courses, referred to in point A.4 of Annex II to Directive 91/676/EEC to be applied in accordance with the action programmes of Member States established under Article 5(4) of Directive 91/676/EEC.\r\nNOTE. Initial value:GAEC1"@en ;
        skos:inScheme    cap-iacs-basecode:CrossComplianceRuleValue .

<http://lpis.ec.europa.eu/registry/applicationschema/cap-iacs-base/code#CropItemCodeValue/industrialCrops>
        a                cap-iacs-base:CropItemCodeValue ;
        rdfs:label       "Industrial crops "@en ;
        skos:definition  "-- Definition --\r\n|Industrial crops .\r\n-- Description --\r\nCereals and main crops - C\r\nNOTE. Initial value:C1400"@en ;
        skos:inScheme    cap-iacs-basecode:CropItemCodeValue .

<http://lpis.ec.europa.eu/registry/applicationschema/cap-iacs-base/code#FarmStructureSurveyNumberValue/permanentCropsUnderGlass>
        a                cap-iacs-base:FarmStructureSurveyNumberValue ;
        rdfs:label       "Permanent crops under glass"@en ;
        skos:definition  "-- Definition --\r\nPermanent crops under glass.\r\n-- Description --\r\nPermanent crops under glass.\r\nNOTE. Initial value:2.04.07"@en ;
        skos:inScheme    cap-iacs-basecode:FarmStructureSurveyNumberValue .

<http://lpis.ec.europa.eu/registry/applicationschema/cap-iacs-base/code#FarmStructureSurveyNumberValue/temporaryGrass>
        a                cap-iacs-base:FarmStructureSurveyNumberValue ;
        rdfs:label       "Temporary grass"@en ;
        skos:definition  "-- Definition --\r\nTemporary grass.\r\n-- Description --\r\nGrass plants for grazing, hay or silage included as a part of a normal crop rotation, lasting at least one crop year and less than five years, sown with grass or grass mixtures. The areas are broken up by ploughing or other tilling or the plants are destroyed by other means such as by herbicides before they are sown again.\r\nMixtures of predominantly grass plants and other forage crops (usually leguminous), grazed, harvested green or as dried hay are included here.\r\nNOTE. Initial value:2.01.09.01"@en ;
        skos:inScheme    cap-iacs-basecode:FarmStructureSurveyNumberValue .

cap-iacs-basecode:VarietalNameValue
        a                skos:ConceptScheme ;
        rdfs:label       "List of varietal names"@en ;
        dct:isFormatOf   cap-iacs-base:VarietalNameValue ;
        skos:definition  "-- Definition --\r\nList of varietal names within vegetable and agricultural plant species. \r\n-- Desription --\r\nCommon catalogue of varieties of agricultural plant species. Fifth supplement to the 29th complete edition (2011/C 168 A/01).\r\nCommon catalogue of varieties of vegetable species. 32nd complete edition (2013/C 312 A/01).\r\nThis codeList decided and maintained by MS.  Varietal names are MS specific.\r\nDictionary: http://ec.europa.eu/food/plant/propagation/catalogues/database/public/index.cfm?event=homepage\r\nNOTE. CODE LIST IS NOT FINISHED. ONLY SOME EXAMPLES ARE PROVIDED."@en .

<http://lpis.ec.europa.eu/registry/applicationschema/cap-iacs-base/code#WeekdayValue/thursday>
        a                cap-iacs-base:WeekdayValue ;
        rdfs:label       "Thursday"@en ;
        skos:definition  "-- Definition --\r\nThursday.\r\n-- Description --\r\nItem description."@en ;
        skos:inScheme    cap-iacs-basecode:WeekdayValue .

<http://lpis.ec.europa.eu/registry/applicationschema/cap-iacs-base/code#SpecieCodeValue/alliumSchoenoprasumLChives>
        a                cap-iacs-base:SpecieCodeValue ;
        rdfs:label       "Allium schoenoprasum L. Chives"@en ;
        skos:definition  "-- Definition --\r\nAllium schoenoprasum L. Chives.\r\n-- Description --\r\nList of vegetable specie -H\r\nNOTE. Initial value: H - 5."@en ;
        skos:inScheme    cap-iacs-basecode:SpecieCodeValue .

<http://lpis.ec.europa.eu/registry/applicationschema/cap-iacs-base/code#CropItemCodeValue/fibreCrops>
        a                cap-iacs-base:CropItemCodeValue ;
        rdfs:label       "Fibre crops"@en ;
        skos:definition  "-- Definition --\r\n||Fibre crops.\r\n-- Description --\r\nCereals and main crops - C\r\nNOTE. Initial value:C1500"@en ;
        skos:inScheme    cap-iacs-basecode:CropItemCodeValue .

<http://lpis.ec.europa.eu/registry/applicationschema/cap-iacs-base/code#CropItemCodeValue/oilseeds>
        a                cap-iacs-base:CropItemCodeValue ;
        rdfs:label       "Oilseeds"@en ;
        skos:definition  "-- Definition --\r\n||Oilseeds.\r\n-- Description --\r\nCereals and main crops - C\r\nNOTE. Initial value:C1410"@en ;
        skos:inScheme    cap-iacs-basecode:CropItemCodeValue .

<http://lpis.ec.europa.eu/registry/applicationschema/cap-iacs-base/code#CropItemCodeValue/otherStoneFruitsNec>
        a                cap-iacs-base:CropItemCodeValue ;
        rdfs:label       "Other stone fruits n.e.c."@en ;
        skos:definition  "-- Definition --\r\n|||Other stone fruits n.e.c.\r\n-- Description --\r\nCereals and main crops - C\r\nNOTE. Initial value:C2229"@en ;
        skos:inScheme    cap-iacs-basecode:CropItemCodeValue .

cap-iacs-basecode:TestingTypeValue
        a                skos:ConceptScheme ;
        rdfs:label       "Testing type value list"@en ;
        dct:isFormatOf   cap-iacs-base:TestingTypeValue ;
        skos:definition  "--Name--\r\nTesting type value\r\n\r\n-- Definition --\r\nTesting type value list.\r\n\r\n-- Description --\r\nIn manual testing, the specified requirements are verified by a trained operator who follows the steps described in the test method.\r\nIn automated testing, specific software is used that operates on the computer readable schema of the eligibility profile."@en .

<http://lpis.ec.europa.eu/registry/applicationschema/cap-iacs-base/code#FarmStructureSurveyNumberValue/arableLandSeedAndSeedlings>
        a                cap-iacs-base:FarmStructureSurveyNumberValue ;
        rdfs:label       "Arable land seed and seedlings"@en ;
        skos:definition  "-- Definition --\r\nArable land seed and seedlings.\r\n-- Description --\r\nAreas producing seeds and seedlings for sale, excluding cereals, rice, pulses, potatoes and oil seeds.\r\nNOTE. Initial value:2.01.10"@en ;
        skos:inScheme    cap-iacs-basecode:FarmStructureSurveyNumberValue .

<http://lpis.ec.europa.eu/registry/applicationschema/cap-iacs-base/code#SpecieCodeValue/brassicaJunceaLBrownMustard>
        a                cap-iacs-base:SpecieCodeValue ;
        rdfs:label       "Brassica juncea L. Brown mustard "@en ;
        skos:definition  "-- Definition --\r\nBrassica juncea L. Brown mustard.\r\n-- Description --\r\nList of agricultural species -A\r\nIII. Oil and fibre plants\r\nNOTE. Initial value: A - 60."@en ;
        skos:inScheme    cap-iacs-basecode:SpecieCodeValue .

<http://lpis.ec.europa.eu/registry/applicationschema/cap-iacs-base/code#CropItemCodeValue/grainMaize>
        a                cap-iacs-base:CropItemCodeValue ;
        rdfs:label       "Grain maize"@en ;
        skos:definition  "-- Definition --\r\n||||Grain maize.\r\n-- Description --\r\nCereals and main crops - C\r\nNOTE. Initial value:C1200"@en ;
        skos:inScheme    cap-iacs-basecode:CropItemCodeValue .

<http://lpis.ec.europa.eu/registry/applicationschema/cap-iacs-base/code#CrossComplianceRuleValue/animalWelfareAnimalWelfareSmr11>
        a                cap-iacs-base:CrossComplianceRuleValue ;
        rdfs:label       "Animal welfare - Animal welfare SMR11"@en ;
        skos:definition  "-- Definition --\r\nAnimal welfare - Animal welfare SMR11.\r\n-- Description --\r\nCouncil Directive 2008/119/EC of 18 December 2008 laying down minimum standards for the protection of calves (OJ L 10, 15.1.2009, p. 7) . Articles 3 and 4.\r\nNOTE. Initial value:SMR11"@en ;
        skos:inScheme    cap-iacs-basecode:CrossComplianceRuleValue .

<http://lpis.ec.europa.eu/registry/applicationschema/cap-iacs-base/code#CropItemCodeValue/avocados>
        a                cap-iacs-base:CropItemCodeValue ;
        rdfs:label       "Avocados"@en ;
        skos:definition  "-- Definition --\r\n|||Avocados.\r\n-- Description --\r\nCereals and main crops - C\r\nNOTE. Initial value:C2253"@en ;
        skos:inScheme    cap-iacs-basecode:CropItemCodeValue .

<http://lpis.ec.europa.eu/registry/applicationschema/cap-iacs-base/code#CropItemCodeValue/riceIndica>
        a                cap-iacs-base:CropItemCodeValue ;
        rdfs:label       "Rice Indica "@en ;
        skos:definition  "-- Definition --\r\n|||Rice Indica.\r\n-- Description --\r\nCereals and main crops - C\r\nNOTE. Initial value:C1251"@en ;
        skos:inScheme    cap-iacs-basecode:CropItemCodeValue .

<http://lpis.ec.europa.eu/registry/applicationschema/cap-iacs-base/code#CropItemCodeValue/seedsAndSeedlings>
        a                cap-iacs-base:CropItemCodeValue ;
        rdfs:label       "Seeds and seedlings"@en ;
        skos:definition  "-- Definition --\r\n|||Seeds and seedlings.\r\n-- Description --\r\nLand use of Agriculture Area in Use -L\r\nNOTE. Initial value:L3310"@en ;
        skos:inScheme    cap-iacs-basecode:CropItemCodeValue .

<http://lpis.ec.europa.eu/registry/applicationschema/cap-iacs-base/code#FarmStructureSurveyNumberValue/ofWhichChristmasTrees>
        a                cap-iacs-base:FarmStructureSurveyNumberValue ;
        rdfs:label       "of which Christmas trees(1)"@en ;
        skos:definition  "-- Definition --\r\nof which Christmas trees(1).\r\n-- Description --\r\nNot to be provided in 2010. (1)\r\nTrees planted for commercial purposes as Christmas trees on the utilised agricultural area.\r\nNOTE. Initial value:2.04.06.01"@en ;
        skos:inScheme    cap-iacs-basecode:FarmStructureSurveyNumberValue .

<http://lpis.ec.europa.eu/registry/applicationschema/cap-iacs-base/code#NotificationGroupValue/notificationsRelatingToThePaymentForYoungFarmers>
        a                cap-iacs-base:NotificationGroupValue ;
        rdfs:label       "Notifications relating to the payment for young farmers"@en ;
        skos:definition  "-- Definition --\r\nNotifications relating to the payment for young farmers.\r\n-- Description --\r\nNOTE.65"@en ;
        skos:inScheme    cap-iacs-basecode:NotificationGroupValue .

<http://lpis.ec.europa.eu/registry/applicationschema/cap-iacs-base/code#CropItemCodeValue/oliveTreesC2450>
        a                cap-iacs-base:CropItemCodeValue ;
        rdfs:label       "Olive trees C2450"@en ;
        skos:definition  "-- Definition --\r\n||Olive trees C2450.\r\n-- Description --\r\nCereals and main crops - C\r\nNOTE. Initial value:C2450"@en ;
        skos:inScheme    cap-iacs-basecode:CropItemCodeValue .

<http://lpis.ec.europa.eu/registry/applicationschema/cap-iacs-base/code#FarmStructureSurveyNumberValue/flax>
        a                cap-iacs-base:FarmStructureSurveyNumberValue ;
        rdfs:label       "Flax"@en ;
        skos:definition  "-- Definition --\r\nFlax.\r\n-- Description --\r\nLinum usitatissimum L., varieties grown mainly for producing fibre.\r\nNOTE. Initial value:2.01.06.09"@en ;
        skos:inScheme    cap-iacs-basecode:FarmStructureSurveyNumberValue .

<http://lpis.ec.europa.eu/registry/applicationschema/cap-iacs-base/code#SpecieCodeValue/cichoriumIntybusLWitloofChicory>
        a                cap-iacs-base:SpecieCodeValue ;
        rdfs:label       "Cichorium intybus L. Witloof chicory"@en ;
        skos:definition  "-- Definition --\r\nCichorium intybus L. Witloof chicory.\r\n-- Description --\r\nList of vegetable specie -H\r\nNOTE. Initial value: H - 14.1"@en ;
        skos:inScheme    cap-iacs-basecode:SpecieCodeValue .

<http://lpis.ec.europa.eu/registry/applicationschema/cap-iacs-base/code#SpecieCodeValue/phaseolusVulgarisLDwarfFrenchBean>
        a                cap-iacs-base:SpecieCodeValue ;
        rdfs:label       "Phaseolus vulgaris L. Dwarf French bean"@en ;
        skos:definition  "-- Definition --\r\nPhaseolus vulgaris L. Dwarf French bean.\r\n-- Description --\r\nList of vegetable specie -H\r\nNOTE. Initial value: H - 27.1"@en ;
        skos:inScheme    cap-iacs-basecode:SpecieCodeValue .

<http://lpis.ec.europa.eu/registry/applicationschema/cap-iacs-base/code#VarietalNameValue/adonis>
        a                cap-iacs-base:VarietalNameValue ;
        rdfs:label       "H - 1.2  Adonis"@en ;
        skos:definition  "-- Definition --\r\nH - 1.2  Adonis\r\n-- Description --\r\nH - 1.2 Allium cepa L. Cepa group - Onion, Echalion /  Adonis.\r\nNOTE. Initial value: Adonis\r\nNOTE. MS - NL (Netherlands)."@en ;
        skos:inScheme    cap-iacs-basecode:VarietalNameValue .

<http://lpis.ec.europa.eu/registry/applicationschema/cap-iacs-base/code#SpecieCodeValue/helianthusAnnuusLSunflower>
        a                cap-iacs-base:SpecieCodeValue ;
        rdfs:label       "Helianthus annuus L. Sunflower "@en ;
        skos:definition  "-- Definition --\r\nHelianthus annuus L. Sunflower.\r\n-- Description --\r\nList of agricultural species -A\r\nIII. Oil and fibre plants\r\nNOTE. Initial value: A - 67."@en ;
        skos:inScheme    cap-iacs-basecode:SpecieCodeValue .

<http://lpis.ec.europa.eu/registry/applicationschema/cap-iacs-base/code#CropItemCodeValue/permanentCrops>
        a                cap-iacs-base:CropItemCodeValue ;
        rdfs:label       "Permanent crops"@en ;
        skos:definition  "-- Definition --\r\n|Permanent crops.\r\n-- Description --\r\nCereals and main crops - C\r\nNOTE. Initial value:C2007"@en ;
        skos:inScheme    cap-iacs-basecode:CropItemCodeValue .

<http://lpis.ec.europa.eu/registry/applicationschema/cap-iacs-base/code#CropItemCodeValue/plantsHarvestedGreenC2610>
        a                cap-iacs-base:CropItemCodeValue ;
        rdfs:label       "Plants harvested green C2610 "@en ;
        skos:definition  "-- Definition --\r\n|Plants harvested green C2610.\r\n-- Description --\r\nCereals and main crops - C\r\nNOTE. Initial value:C2610"@en ;
        skos:inScheme    cap-iacs-basecode:CropItemCodeValue .

<http://lpis.ec.europa.eu/registry/applicationschema/cap-iacs-base/code#SpecieCodeValue/cichoriumIntybusLLargeLeavedChicoryItalianChicory>
        a                cap-iacs-base:SpecieCodeValue ;
        rdfs:label       "Cichorium intybus L. Large-leaved chicory / Italian chicory"@en ;
        skos:definition  "-- Definition --\r\nCichorium intybus L. Large-leaved chicory / Italian chicory.\r\n-- Description --\r\nList of vegetable specie -H\r\nNOTE. Initial value: H - 14.2"@en ;
        skos:inScheme    cap-iacs-basecode:SpecieCodeValue .

<http://lpis.ec.europa.eu/registry/applicationschema/cap-iacs-base/code#WeekdayValue/monday>
        a                cap-iacs-base:WeekdayValue ;
        rdfs:label       "Monday"@en ;
        skos:definition  "-- Definition --\r\nMonday.\r\n-- Description --\r\nItem description."@en ;
        skos:inScheme    cap-iacs-basecode:WeekdayValue .

<http://lpis.ec.europa.eu/registry/applicationschema/cap-iacs-base/code#FarmStructureSurveyNumberValue/openField>
        a                cap-iacs-base:FarmStructureSurveyNumberValue ;
        rdfs:label       "Open field"@en ;
        skos:definition  "-- Definition --\r\nOpen field.\r\n-- Description --\r\nFresh vegetables, melons and strawberries grown on arable land in rotation with other agricultural crops.\r\nNOTE. Initial value:2.01.07.01.01"@en ;
        skos:inScheme    cap-iacs-basecode:FarmStructureSurveyNumberValue .

<http://lpis.ec.europa.eu/registry/applicationschema/cap-iacs-base/code#SpecieCodeValue/brassicaOleraceaLSavoyCabbage>
        a                cap-iacs-base:SpecieCodeValue ;
        rdfs:label       "Brassica oleracea L. Savoy cabbage"@en ;
        skos:definition  "-- Definition --\r\nBrassica oleracea L. Savoy cabbage.\r\n-- Description --\r\nList of vegetable specie -H\r\nNOTE. Initial value: H - 10.5"@en ;
        skos:inScheme    cap-iacs-basecode:SpecieCodeValue .

<http://lpis.ec.europa.eu/registry/applicationschema/cap-iacs-base/code#CropItemCodeValue/rapeAndTurnipRape>
        a                cap-iacs-base:CropItemCodeValue ;
        rdfs:label       "Rape and turnip rape"@en ;
        skos:definition  "-- Definition --\r\n||||Rape and turnip rape.\r\n-- Description --\r\nCereals and main crops - C\r\nNOTE. Initial value:C1420"@en ;
        skos:inScheme    cap-iacs-basecode:CropItemCodeValue .

<http://lpis.ec.europa.eu/registry/applicationschema/cap-iacs-base/code#OrdinalNumberValue/fourth>
        a                cap-iacs-base:OrdinalNumberValue ;
        rdfs:label       "Fourth"@en ;
        skos:definition  "-- Definition --\r\nFourth.\r\n-- Description --\r\nItem description."@en ;
        skos:inScheme    cap-iacs-basecode:OrdinalNumberValue .

<http://lpis.ec.europa.eu/registry/applicationschema/cap-iacs-base/code#SpecieCodeValue/brassicaNapusLPartimSwedeRape>
        a                cap-iacs-base:SpecieCodeValue ;
        rdfs:label       "Brassica napus L. (partim) Swede rape "@en ;
        skos:definition  "-- Definition --\r\nBrassica napus L. (partim) Swede rape.\r\n-- Description --\r\nList of agricultural species -A\r\nIII. Oil and fibre plants\r\nNOTE. Initial value: A - 61."@en ;
        skos:inScheme    cap-iacs-basecode:SpecieCodeValue .

<http://lpis.ec.europa.eu/registry/applicationschema/cap-iacs-base/code#SpecieCodeValue/triticumAestivumLWheat>
        a                cap-iacs-base:SpecieCodeValue ;
        rdfs:label       "Triticum aestivum L. Wheat"@en ;
        skos:definition  "-- Definition --\r\nTriticum aestivum L. Wheat.\r\n-- Description --\r\nList of agricultural species -A   \r\nIV. Cereals\r\nNOTE. Initial value: A - 83."@en ;
        skos:inScheme    cap-iacs-basecode:SpecieCodeValue .

<http://lpis.ec.europa.eu/registry/applicationschema/cap-iacs-base/code#AffectedElementTypeValue/associationRole>
        a                cap-iacs-base:AffectedElementTypeValue ;
        rdfs:label       "Relationship"@en ;
        skos:definition  "--Name--\r\nAssociation role\r\n\r\n-- Definition --\r\nSemantic relationship that can occur between type instances [ISO 19103:2005]"@en ;
        skos:inScheme    cap-iacs-basecode:AffectedElementTypeValue .

<http://lpis.ec.europa.eu/registry/applicationschema/cap-iacs-base/code#FarmStructureSurveyNumberValue/fruitSpeciesOfWhich>
        a                cap-iacs-base:FarmStructureSurveyNumberValue ;
        rdfs:label       "Fruit species, of which:"@en ;
        skos:definition  "-- Definition --\r\nFruit species, of which:\r\n-- Description --\r\nFruit species, of which:\r\nNOTE. Initial value:2.04.01.01"@en ;
        skos:inScheme    cap-iacs-basecode:FarmStructureSurveyNumberValue .

<http://lpis.ec.europa.eu/registry/applicationschema/cap-iacs-base/code#FarmStructureSurveyNumberValue/arableLand>
        a                cap-iacs-base:FarmStructureSurveyNumberValue ;
        rdfs:label       "Arable land"@en ;
        skos:definition  "-- Definition --\r\nArable land.\r\n-- Description --\r\nLand worked (ploughed or tilled) regularly, generally under a system of crop rotation.\r\nCrop rotation is the practice of alternating annual crops grown on a specific field in a planned pattern or sequence in successive crop years so that crops of the same species are not grown without interruption on the same field. Normally the crops are changed annually, but they can also be multiannual. To distinguish arable land from permanent crops or permanent grassland, a threshold of five years is used. This means that if a plot is used for the same crop for five years or more, without in the meantime removing the preceding crop and establishing a new one, it is not considered arable land.\r\nNOTE. Initial value:2.01"@en ;
        skos:inScheme    cap-iacs-basecode:FarmStructureSurveyNumberValue .

<http://lpis.ec.europa.eu/registry/applicationschema/cap-iacs-base/code#CropItemCodeValue/otherIndustrialCropsNec>
        a                cap-iacs-base:CropItemCodeValue ;
        rdfs:label       "Other industrial crops n.e.c."@en ;
        skos:definition  "-- Definition --\r\n|||Other industrial crops n.e.c.\r\n-- Description --\r\nCereals and main crops - C\r\nNOTE. Initial value:C1589"@en ;
        skos:inScheme    cap-iacs-basecode:CropItemCodeValue .

<http://lpis.ec.europa.eu/registry/applicationschema/cap-iacs-base/code#SpecieCodeValue/pisumSativumLPartimRoundPea>
        a                cap-iacs-base:SpecieCodeValue ;
        rdfs:label       "Pisum sativum L. (partim) Round pea"@en ;
        skos:definition  "-- Definition --\r\nPisum sativum L. (partim) Round pea.\r\n-- Description --\r\nList of vegetable specie -H\r\nNOTE. Initial value: H - 28.2"@en ;
        skos:inScheme    cap-iacs-basecode:SpecieCodeValue .

<http://lpis.ec.europa.eu/registry/applicationschema/cap-iacs-base/code#CropItemCodeValue/winterRape>
        a                cap-iacs-base:CropItemCodeValue ;
        rdfs:label       "Winter rape"@en ;
        skos:definition  "-- Definition --\r\n||||||Winter rape.\r\n-- Description --\r\nCereals and main crops - C\r\nNOTE. Initial value:C1431"@en ;
        skos:inScheme    cap-iacs-basecode:CropItemCodeValue .

<http://lpis.ec.europa.eu/registry/applicationschema/cap-iacs-base/code#CropItemCodeValue/otherArableLandCrops>
        a                cap-iacs-base:CropItemCodeValue ;
        rdfs:label       "Other arable-land crops"@en ;
        skos:definition  "-- Definition --\r\n|||Other arable-land crops.\r\n-- Description --\r\nLand use of Agriculture Area in Use -L\r\nNOTE. Initial value:L2690"@en ;
        skos:inScheme    cap-iacs-basecode:CropItemCodeValue .

<http://lpis.ec.europa.eu/registry/applicationschema/cap-iacs-base/code#CropItemCodeValue/stoneFruits>
        a                cap-iacs-base:CropItemCodeValue ;
        rdfs:label       "Stone fruits"@en ;
        skos:definition  "-- Definition --\r\n||Stone fruits.\r\n-- Description --\r\nCereals and main crops - C\r\nNOTE. Initial value:C2170"@en ;
        skos:inScheme    cap-iacs-basecode:CropItemCodeValue .

<http://lpis.ec.europa.eu/registry/applicationschema/cap-iacs-base/code#CropItemCodeValue/otherBrassicasNec>
        a                cap-iacs-base:CropItemCodeValue ;
        rdfs:label       "Other brassicas n.e.c."@en ;
        skos:definition  "-- Definition --\r\n|||Other brassicas n.e.c.\r\n-- Description --\r\nCereals and main crops - C\r\nNOTE. Initial value:C1655"@en ;
        skos:inScheme    cap-iacs-basecode:CropItemCodeValue .

<http://lpis.ec.europa.eu/registry/applicationschema/cap-iacs-base/code#FarmStructureSurveyNumberValue/driedPulsesAndProteinCropsForTheProductionOfGrain>
        a                cap-iacs-base:FarmStructureSurveyNumberValue ;
        rdfs:label       "Dried pulses and protein crops for the production of grain"@en ;
        skos:definition  "-- Definition --\r\nDried pulses and protein crops for the production of grain.\r\n-- Description --\r\nDried pulses and protein crops for the production of grain (including seed and mixtures of cereals and pulses)\r\nCrops sown and harvested mainly for their protein content.\r\nAll areas of dried pulses and protein crops harvested dry for grain, regardless of use, shall be recorded here (including crops used for renewable energy production).\r\nNOTE. Initial value:2.01.02"@en ;
        skos:inScheme    cap-iacs-basecode:FarmStructureSurveyNumberValue .

<http://lpis.ec.europa.eu/registry/applicationschema/cap-iacs-base/code#CropItemCodeValue/blackCurrants>
        a                cap-iacs-base:CropItemCodeValue ;
        rdfs:label       "Black currants"@en ;
        skos:definition  "-- Definition --\r\n||||Black currants.\r\n-- Description --\r\nCereals and main crops - C\r\nNOTE. Initial value:C2272"@en ;
        skos:inScheme    cap-iacs-basecode:CropItemCodeValue .

<http://lpis.ec.europa.eu/registry/applicationschema/cap-iacs-base/code#CropItemCodeValue/nutsC2230>
        a                cap-iacs-base:CropItemCodeValue ;
        rdfs:label       "Nuts C2230"@en ;
        skos:definition  "-- Definition --\r\n||Nuts C2230.\r\n-- Description --\r\nCereals and main crops - C\r\nNOTE. Initial value:C2230"@en ;
        skos:inScheme    cap-iacs-basecode:CropItemCodeValue .

<http://lpis.ec.europa.eu/registry/applicationschema/cap-iacs-base/code#SpecieCodeValue/zeaMaysLMaize>
        a                cap-iacs-base:SpecieCodeValue ;
        rdfs:label       "Zea mays L. Maize  "@en ;
        skos:definition  "-- Definition --\r\nZea mays L. Maize.\r\n-- Description --\r\nList of agricultural species -A   \r\nIV. Cereals\r\nNOTE. Initial value: A - 86."@en ;
        skos:inScheme    cap-iacs-basecode:SpecieCodeValue .

<http://lpis.ec.europa.eu/registry/applicationschema/cap-iacs-base/code#StatusValue/underApproval>
        a                cap-iacs-base:StatusValue ;
        rdfs:label       "Under aprooval"@en ;
        skos:definition  "-- Name--\r\nUnder approval\r\n\r\n--Definition--\r\nStatus of an object according to the state machine diagram.\r\n\r\n-- Description --\r\nBased on the outcome of cross checks the change request is approved. The object is waiting for finalisation."@en ;
        skos:inScheme    cap-iacs-basecode:StatusValue .

<http://lpis.ec.europa.eu/registry/applicationschema/cap-iacs-base/code#SpecieCodeValue/brassicaRapaLTurnip>
        a                cap-iacs-base:SpecieCodeValue ;
        rdfs:label       "Brassica rapa L. Turnip"@en ;
        skos:definition  "-- Definition --\r\nBrassica rapa L. Turnip.\r\n-- Description --\r\nList of vegetable specie -H\r\nNOTE. Initial value: H - 11.2"@en ;
        skos:inScheme    cap-iacs-basecode:SpecieCodeValue .

<http://lpis.ec.europa.eu/registry/applicationschema/cap-iacs-base/code#CropItemCodeValue/chestnuts>
        a                cap-iacs-base:CropItemCodeValue ;
        rdfs:label       "Chestnuts"@en ;
        skos:definition  "-- Definition --\r\n|||Chestnuts.\r\n-- Description --\r\nCereals and main crops - C\r\nNOTE. Initial value:C2236"@en ;
        skos:inScheme    cap-iacs-basecode:CropItemCodeValue .

<http://lpis.ec.europa.eu/registry/applicationschema/cap-iacs-base/code#NotificationGroupValue/notificationsConcerningComplementaryNationalDirectPaymentsBgRo>
        a                cap-iacs-base:NotificationGroupValue ;
        rdfs:label       "Notifications concerning complementary national direct payments (BG and RO only)"@en ;
        skos:definition  "-- Definition --\r\nNotifications concerning complementary national direct payments (BG and RO only).\r\n-- Description --\r\nNOTE.73"@en ;
        skos:inScheme    cap-iacs-basecode:NotificationGroupValue .

<http://lpis.ec.europa.eu/registry/applicationschema/cap-iacs-base/code#SpecieCodeValue/cucurbitaFicifoliaBouche>
        a                cap-iacs-base:SpecieCodeValue ;
        rdfs:label       "Cucurbita ficifolia Bouché"@en ;
        skos:definition  "-- Definition --\r\nCucurbita ficifolia Bouché.\r\n-- Description --\r\nList of vegetable specie -H\r\nNOTE. Initial value: H - 37.1"@en ;
        skos:inScheme    cap-iacs-basecode:SpecieCodeValue .

<http://lpis.ec.europa.eu/registry/applicationschema/cap-iacs-base/code#CropItemCodeValue/smallCitrusFruits>
        a                cap-iacs-base:CropItemCodeValue ;
        rdfs:label       "Small citrus fruits"@en ;
        skos:definition  "-- Definition --\r\n|||Small citrus fruits.\r\n-- Description --\r\nCereals and main crops - C\r\nNOTE. Initial value:C2340"@en ;
        skos:inScheme    cap-iacs-basecode:CropItemCodeValue .

<http://lpis.ec.europa.eu/registry/applicationschema/cap-iacs-base/code#CropItemCodeValue/otherIndustrialCrops>
        a                cap-iacs-base:CropItemCodeValue ;
        rdfs:label       "Other industrial crops"@en ;
        skos:definition  "-- Definition --\r\n||Other industrial crops.\r\n-- Description --\r\nCereals and main crops - C\r\nNOTE. Initial value:C1570"@en ;
        skos:inScheme    cap-iacs-basecode:CropItemCodeValue .

<http://lpis.ec.europa.eu/registry/applicationschema/cap-iacs-base/code#CropItemCodeValue/otherLeafyOrStalkedVegetablesNec>
        a                cap-iacs-base:CropItemCodeValue ;
        rdfs:label       "Other leafy or stalked vegetables n.e.c."@en ;
        skos:definition  "-- Definition --\r\n|||Other leafy or stalked vegetables n.e.c.\r\n-- Description --\r\nCereals and main crops - C\r\nNOTE. Initial value:C1725"@en ;
        skos:inScheme    cap-iacs-basecode:CropItemCodeValue .

<http://lpis.ec.europa.eu/registry/applicationschema/cap-iacs-base/code#FarmStructureSurveyNumberValue/fallowLandSubjectToThePaymentOfSubsidiesWithNoEconomicUse>
        a                cap-iacs-base:FarmStructureSurveyNumberValue ;
        rdfs:label       "Fallow land subject to the payment of subsidies, with no economic use"@en ;
        skos:definition  "-- Definition --\r\nFallow land subject to the payment of subsidies, with no economic use.\r\n-- Description --\r\nFallow land for which the holding is entitled to financial aid.\r\nNOTE. Initial value:2.01.12.02"@en ;
        skos:inScheme    cap-iacs-basecode:FarmStructureSurveyNumberValue .

cap-iacs-basecode:AffectedElementTypeValue
        a                skos:ConceptScheme ;
        rdfs:label       "Affected element type value list"@en ;
        dct:isFormatOf   cap-iacs-base:AffectedElementTypeValue ;
        skos:definition  "--Name--\r\nAffected element type value.\r\n\r\n-- Definition --\r\nApplication schema or its element that might be a subject of an issue.\r\n\r\n-- Description --\r\nList of possible affected elements that might be changed within the model."@en .

<http://lpis.ec.europa.eu/registry/applicationschema/cap-iacs-base/code#CrossComplianceRuleValue/environmentClimateChangeGoodAgriculturalConditionOfLandBiodiversitySmr3>
        a                cap-iacs-base:CrossComplianceRuleValue ;
        rdfs:label       "Environment, climate change, good agricultural condition of land  - Biodiversity SMR3"@en ;
        skos:definition  "-- Definition --\r\nEnvironment, climate change, good agricultural condition of land  - Biodiversity SMR3.\r\n-- Description --\r\nCouncil Directive 92/43/EEC of 21 May 1992 on the conservation of natural habitats and of wild flora and fauna (OJ L 206, 22.7.1992, p. 7) . Article 6(1) and (2).\r\nNOTE. Initial value:SMR3"@en ;
        skos:inScheme    cap-iacs-basecode:CrossComplianceRuleValue .

<http://lpis.ec.europa.eu/registry/applicationschema/cap-iacs-base/code#AffectedElementTypeValue/union>
        a                cap-iacs-base:AffectedElementTypeValue ;
        rdfs:label       "Union"@en ;
        skos:definition  "--Name--\r\nUnion\r\n\r\n-- Definition --\r\nA class, which defines a collection of Simple Types defined in ISO 19103:2005."@en ;
        skos:inScheme    cap-iacs-basecode:AffectedElementTypeValue .

<http://lpis.ec.europa.eu/registry/applicationschema/cap-iacs-base/code#WeekdayValue/sunday>
        a                cap-iacs-base:WeekdayValue ;
        rdfs:label       "Sunday"@en ;
        skos:definition  "-- Definition --\r\nSunday.\r\n-- Description --\r\nItem description."@en ;
        skos:inScheme    cap-iacs-basecode:WeekdayValue .

<http://lpis.ec.europa.eu/registry/applicationschema/cap-iacs-base/code#ConformanceLevelValue/level3>
        a                cap-iacs-base:ConformanceLevelValue ;
        rdfs:label       "Level 3 high"@en ;
        skos:definition  "--Name--\r\nLevel 3\r\n\r\n--Definition--\r\nHighest level conformance.\r\n\r\n--Description--\r\nA separate abstract test suite must be provided if a level is defined within ConformanceClause."@en ;
        skos:inScheme    cap-iacs-basecode:ConformanceLevelValue .

<http://lpis.ec.europa.eu/registry/applicationschema/cap-iacs-base/code#SpecieCodeValue/raphanusSativusLRadish>
        a                cap-iacs-base:SpecieCodeValue ;
        rdfs:label       "Raphanus sativus L. Radish"@en ;
        skos:definition  "-- Definition --\r\nRaphanus sativus L. Radish.\r\n-- Description --\r\nList of vegetable specie -H\r\nNOTE. Initial value: H - 29.1"@en ;
        skos:inScheme    cap-iacs-basecode:SpecieCodeValue .

<http://lpis.ec.europa.eu/registry/applicationschema/cap-iacs-base/code#CropItemCodeValue/citrusPlantations>
        a                cap-iacs-base:CropItemCodeValue ;
        rdfs:label       "Citrus plantations"@en ;
        skos:definition  "-- Definition --\r\n||||Citrus plantations.\r\n-- Description --\r\nLand use of Agriculture Area in Use -L\r\nNOTE. Initial value:L2300"@en ;
        skos:inScheme    cap-iacs-basecode:CropItemCodeValue .

<http://lpis.ec.europa.eu/registry/applicationschema/cap-iacs-base/code#FarmStructureSurveyNumberValue/commonWheatAndSpelt>
        a                cap-iacs-base:FarmStructureSurveyNumberValue ;
        rdfs:label       "Common wheat and spelt"@en ;
        skos:definition  "-- Definition --\r\nCommon wheat and spelt.\r\n-- Description --\r\nTriticum aestivum L. emend. Fiori et Paol., Triticum spelta L. and Triticum monococcum L.\r\nNOTE. Initial value:2.01.01.01"@en ;
        skos:inScheme    cap-iacs-basecode:FarmStructureSurveyNumberValue .

<http://lpis.ec.europa.eu/registry/applicationschema/cap-iacs-base/code#SpecieCodeValue/brassicaOleraceaLCurlyKale>
        a                cap-iacs-base:SpecieCodeValue ;
        rdfs:label       "Brassica oleracea L. Curly kale"@en ;
        skos:definition  "-- Definition --\r\nBrassica oleracea L. Curly kale.\r\n-- Description --\r\nList of vegetable specie -H\r\nNOTE. Initial value: H - 10.1"@en ;
        skos:inScheme    cap-iacs-basecode:SpecieCodeValue .

<http://lpis.ec.europa.eu/registry/applicationschema/cap-iacs-base/code#CropItemCodeValue/endives>
        a                cap-iacs-base:CropItemCodeValue ;
        rdfs:label       "Endives"@en ;
        skos:definition  "-- Definition --\r\n|||Endives.\r\n-- Description --\r\nCereals and main crops - C\r\nNOTE. Initial value:C1685"@en ;
        skos:inScheme    cap-iacs-basecode:CropItemCodeValue .

<http://lpis.ec.europa.eu/registry/applicationschema/cap-iacs-base/code#CropItemCodeValue/clementines>
        a                cap-iacs-base:CropItemCodeValue ;
        rdfs:label       "Clementines"@en ;
        skos:definition  "-- Definition --\r\n||||Clementines.\r\n-- Description --\r\nCereals and main crops - C\r\nNOTE. Initial value:C2360"@en ;
        skos:inScheme    cap-iacs-basecode:CropItemCodeValue .

<http://lpis.ec.europa.eu/registry/applicationschema/cap-iacs-base/code#CropItemCodeValue/berriesExcludingStrawberries>
        a                cap-iacs-base:CropItemCodeValue ;
        rdfs:label       "Berries (excluding strawberries)"@en ;
        skos:definition  "-- Definition --\r\n||Berries (excluding strawberries).\r\n-- Description --\r\nCereals and main crops - C\r\nNOTE. Initial value:C2270"@en ;
        skos:inScheme    cap-iacs-basecode:CropItemCodeValue .

<http://lpis.ec.europa.eu/registry/applicationschema/cap-iacs-base/code#CropItemCodeValue/winterBarley>
        a                cap-iacs-base:CropItemCodeValue ;
        rdfs:label       "Winter barley"@en ;
        skos:definition  "-- Definition --\r\n||||Winter barley.\r\n-- Description --\r\nCereals and main crops - C\r\nNOTE. Initial value:C1163"@en ;
        skos:inScheme    cap-iacs-basecode:CropItemCodeValue .

<http://lpis.ec.europa.eu/registry/applicationschema/cap-iacs-base/code#SpecieCodeValue/avenaSativaLIncludingAByzantinaKKochOatAndRedOat>
        a                cap-iacs-base:SpecieCodeValue ;
        rdfs:label       "Avena sativa L. (including A. byzantina K. Koch) Oat and Red oat"@en ;
        skos:definition  "-- Definition --\r\nAvena sativa L. (including A. byzantina K. Koch) Oat and Red oat.\r\n-- Description --\r\nList of agricultural species -A   \r\nIV. Cereals\r\nNOTE. Initial value: A - 73."@en ;
        skos:inScheme    cap-iacs-basecode:SpecieCodeValue .

<http://lpis.ec.europa.eu/registry/applicationschema/cap-iacs-base/code#CrossComplianceRuleValue/environmentClimateChangeGoodAgriculturalConditionOfLandWaterSmr1>
        a                cap-iacs-base:CrossComplianceRuleValue ;
        rdfs:label       "Environment, climate change, good agricultural condition of land  - Water SMR1"@en ;
        skos:definition  "-- Definition --\r\nEnvironment, climate change, good agricultural condition of land  - Water SMR1.\r\n-- Description --\r\nCouncil Directive 91/676/EEC of 12 December 1991 concerning the protection of waters against pollution caused by nitrates from agricultural sources (OJ L 375, 31.12.1991, p. 1) . Articles 4 and 5.\r\nNOTE. Initial value:SMR1"@en ;
        skos:inScheme    cap-iacs-basecode:CrossComplianceRuleValue .

<http://lpis.ec.europa.eu/registry/applicationschema/cap-iacs-base/code#FarmStructureSurveyNumberValue/soya>
        a                cap-iacs-base:FarmStructureSurveyNumberValue ;
        rdfs:label       "Soya"@en ;
        skos:definition  "-- Definition --\r\nSoya.\r\n-- Description --\r\nGlycine max L. Merril, harvested as dry grains.\r\nNOTE. Initial value:2.01.06.06"@en ;
        skos:inScheme    cap-iacs-basecode:FarmStructureSurveyNumberValue .

<http://lpis.ec.europa.eu/registry/applicationschema/cap-iacs-base/code#CropItemCodeValue/artichokes>
        a                cap-iacs-base:CropItemCodeValue ;
        rdfs:label       "Artichokes"@en ;
        skos:definition  "-- Definition --\r\n|||Artichokes.\r\n-- Description --\r\nCereals and main crops - C\r\nNOTE. Initial value:C1720"@en ;
        skos:inScheme    cap-iacs-basecode:CropItemCodeValue .

<http://lpis.ec.europa.eu/registry/applicationschema/cap-iacs-base/code#MonthValue/october>
        a                cap-iacs-base:MonthValue ;
        rdfs:label       "October"@en ;
        skos:definition  "-- Definition --\r\nOctober.\r\n-- Description --\r\nItem description."@en ;
        skos:inScheme    cap-iacs-basecode:MonthValue .

<http://lpis.ec.europa.eu/registry/applicationschema/cap-iacs-base/code#CrossComplianceRuleValue/publicHealthAnimalHealthAndPlantHealthAnimalDiseasesSmr9>
        a                cap-iacs-base:CrossComplianceRuleValue ;
        rdfs:label       "Public health, animal health and plant health  - Animal diseases SMR9"@en ;
        skos:definition  "-- Definition --\r\nPublic health, animal health and plant health  - Animal diseases SMR9.\r\n-- Description --\r\nRegulation (EC) No 999/2001 of the European Parliament and of the Council of 22 May 2001 laying down rules for the prevention, control and eradication of certain transmissible spongiform encephalopathies (OJ L 147, 31.5.2001, p. 1). Articles 7, 11, 12, 13 and 15.\r\nNOTE. Initial value:SMR9"@en ;
        skos:inScheme    cap-iacs-basecode:CrossComplianceRuleValue .

<http://lpis.ec.europa.eu/registry/applicationschema/cap-iacs-base/code#VarietalNameValue/biztro>
        a                cap-iacs-base:VarietalNameValue ;
        rdfs:label       "H - 1.1  Biztro"@en ;
        skos:definition  "-- Definition --\r\nH - 1.1  Biztro\r\n-- Description --\r\nH - 1.1 Allium cepa L. Aggregatum group - Shallot /  Biztro.\r\nNOTE. Initial value: Biztro\r\nNOTE. MS - NL (Netherlands)."@en ;
        skos:inScheme    cap-iacs-basecode:VarietalNameValue .

<http://lpis.ec.europa.eu/registry/applicationschema/cap-iacs-base/code#MonthValue/november>
        a                cap-iacs-base:MonthValue ;
        rdfs:label       "November"@en ;
        skos:definition  "-- Definition --\r\nNovember.\r\n-- Description --\r\nItem description."@en ;
        skos:inScheme    cap-iacs-basecode:MonthValue .

<http://lpis.ec.europa.eu/registry/applicationschema/cap-iacs-base/code#SpecieCodeValue/phalarisAquaticaLHardingGrassPhalaris>
        a                cap-iacs-base:SpecieCodeValue ;
        rdfs:label       "Phalaris aquatica L. Harding grass/Phalaris"@en ;
        skos:definition  "-- Definition --\r\nPhalaris aquatica L. Harding grass/Phalaris.\r\n-- Description --\r\nList of agricultural species -A\r\nII. Fodder plants\r\nNOTE. Initial value: A - 23."@en ;
        skos:inScheme    cap-iacs-basecode:SpecieCodeValue .

<http://lpis.ec.europa.eu/registry/applicationschema/cap-iacs-base/code#SpecieCodeValue/viciaVillosaRothHairyVetch>
        a                cap-iacs-base:SpecieCodeValue ;
        rdfs:label       "Vicia villosa Roth. Hairy vetch"@en ;
        skos:definition  "-- Definition --\r\nVicia villosa Roth. Hairy vetch.\r\n-- Description --\r\nList of agricultural species -A\r\nII. Fodder plants\r\nNOTE. Initial value: A - 53."@en ;
        skos:inScheme    cap-iacs-basecode:SpecieCodeValue .

<http://lpis.ec.europa.eu/registry/applicationschema/cap-iacs-base/code#CropItemCodeValue/peaches>
        a                cap-iacs-base:CropItemCodeValue ;
        rdfs:label       "Peaches"@en ;
        skos:definition  "-- Definition --\r\n|||Peaches.\r\n-- Description --\r\nCereals and main crops - C\r\nNOTE. Initial value:C2180"@en ;
        skos:inScheme    cap-iacs-basecode:CropItemCodeValue .

<http://lpis.ec.europa.eu/registry/applicationschema/cap-iacs-base/code#CropItemCodeValue/temporaryGrassesAndGrazing>
        a                cap-iacs-base:CropItemCodeValue ;
        rdfs:label       "Temporary grasses and grazing "@en ;
        skos:definition  "-- Definition --\r\n||Temporary grasses and grazing.\r\n-- Description --\r\nCereals and main crops - C\r\nNOTE. Initial value:C2680"@en ;
        skos:inScheme    cap-iacs-basecode:CropItemCodeValue .

<http://lpis.ec.europa.eu/registry/applicationschema/cap-iacs-base/code#CropItemCodeValue/oranges>
        a                cap-iacs-base:CropItemCodeValue ;
        rdfs:label       "Oranges"@en ;
        skos:definition  "-- Definition --\r\n|||Oranges.\r\n-- Description --\r\nCereals and main crops - C\r\nNOTE. Initial value:C2320"@en ;
        skos:inScheme    cap-iacs-basecode:CropItemCodeValue .

<http://lpis.ec.europa.eu/registry/applicationschema/cap-iacs-base/code#ConformanceStatementValue/conforming>
        a                cap-iacs-base:ConformanceStatementValue ;
        rdfs:label       "Confroming"@en ;
        skos:definition  "-- Name--\r\nConforming\r\n\r\n-- Description --\r\nThe tested object complies with rules, standards, or laws."@en ;
        skos:inScheme    cap-iacs-basecode:ConformanceStatementValue .

<http://lpis.ec.europa.eu/registry/applicationschema/cap-iacs-base/code#CropItemCodeValue/spinach>
        a                cap-iacs-base:CropItemCodeValue ;
        rdfs:label       "Spinach"@en ;
        skos:definition  "-- Definition --\r\n|||Spinach.\r\n-- Description --\r\nCereals and main crops - C\r\nNOTE. Initial value:C1690"@en ;
        skos:inScheme    cap-iacs-basecode:CropItemCodeValue .

<http://lpis.ec.europa.eu/registry/applicationschema/cap-iacs-base/code#SpecieCodeValue/papaverSomniferumLPoppy>
        a                cap-iacs-base:SpecieCodeValue ;
        rdfs:label       "Papaver somniferum L. Poppy"@en ;
        skos:definition  "-- Definition --\r\nPapaver somniferum L. Poppy.\r\n-- Description --\r\nList of agricultural species -A\r\nIII. Oil and fibre plants\r\nNOTE. Initial value: A - 69."@en ;
        skos:inScheme    cap-iacs-basecode:SpecieCodeValue .

<http://lpis.ec.europa.eu/registry/applicationschema/cap-iacs-base/code#StatusValue/valid>
        a                cap-iacs-base:StatusValue ;
        skos:definition  "-- Name--\r\nValid\r\n\r\n--Definition--\r\nStatus of an object according to the state machine diagram.\r\n\r\n-- Description --\r\nThe most current state of the object that shall be used by the users. \r\n\r\nNOTE 1: It is a current object whose life-cycle has not ended.\r\nFeatureLevelMetadata.endLifespanVersion=Null\r\n\r\nNOTE 2: If applied, FeatureLevelMetadata.validTo=Null"@en ;
        skos:inScheme    cap-iacs-basecode:StatusValue .

<http://lpis.ec.europa.eu/registry/applicationschema/cap-iacs-base/code#SpecieCodeValue/capsicumAnnuumLChiliPepper>
        a                cap-iacs-base:SpecieCodeValue ;
        rdfs:label       "Capsicum annuum L. Chili, Pepper "@en ;
        skos:definition  "-- Definition --\r\nCapsicum annuum L. Chili, Pepper.\r\n-- Description --\r\nList of vegetable specie -H\r\nNOTE. Initial value: H - 12."@en ;
        skos:inScheme    cap-iacs-basecode:SpecieCodeValue .

<http://lpis.ec.europa.eu/registry/applicationschema/cap-iacs-base/code#CrossComplianceRuleValue/publicHealthAnimalHealthAndPlantHealthFoodSafetySmr4>
        a                cap-iacs-base:CrossComplianceRuleValue ;
        rdfs:label       "Public health, animal health and plant health  - Food safety SMR4"@en ;
        skos:definition  "-- Definition --\r\nPublic health, animal health and plant health  - Food safety SMR4.\r\n-- Description --\r\nRegulation (EC) No 178/2002 of the European Parliament and of the Council of 28 January 2002 laying down the general principles and requirements of food law, establishing the European Food Safety Authority and laying down procedures in matters of food safety (OJ L 31, 1.2.2002, p. 1). Articles 14 and 15, Article 17(1) [3] and Articles 18, 19 and 20 [3] As implemented in particular by:- Article 14 of Regulation (EC) No 470/2009 and the Annex of Regulation (EC) No 37/2010,- Regulation (EC) No 852/2004: Article 4(1) and Annex I part A (II 4 (g, h, j), 5 (f, h), 6; III 8 (a, b, d, e), 9 (a, c)),- Regulation (EC) No 853/2004: Article 3(1) and Annex III Section IX Chapter 1 (I-1 b, c, d, e; I-2 a (i, ii, iii), b (i, ii), c; I-3; I-4; I-5; II-A 1, 2, 3, 4; II-B 1(a, d), 2, 4 (a, b)), Annex III Section X Chapter 1(1),- Regulation (EC) No 183/2005: Article 5(1) and Annex I, part A (I-4 e, g; II-2 a, b, e), Article 5(5) and Annex III (1, 2), Article 5(6), and- Regulation (EC) No 396/2005: Article 18.\r\nNOTE. Initial value:SMR4"@en ;
        skos:inScheme    cap-iacs-basecode:CrossComplianceRuleValue .

<http://lpis.ec.europa.eu/registry/applicationschema/cap-iacs-base/code#NotificationGroupValue/notificationsConcerningApplicationOfLinearReductions>
        a                cap-iacs-base:NotificationGroupValue ;
        rdfs:label       "Notifications concerning application of linear reductions"@en ;
        skos:definition  "-- Definition --\r\nNotifications concerning application of linear reductions.\r\n-- Description --\r\nNOTE.72"@en ;
        skos:inScheme    cap-iacs-basecode:NotificationGroupValue .

<http://lpis.ec.europa.eu/registry/applicationschema/cap-iacs-base/code#FarmStructureSurveyNumberValue/tobacco>
        a                cap-iacs-base:FarmStructureSurveyNumberValue ;
        rdfs:label       "Tobacco"@en ;
        skos:definition  "-- Definition --\r\nTobacco\r\n-- Description --\r\nNicotiana tabacum L.\r\nNOTE. Initial value:2.01.06.01"@en ;
        skos:inScheme    cap-iacs-basecode:FarmStructureSurveyNumberValue .

<http://lpis.ec.europa.eu/registry/applicationschema/cap-iacs-base/code#SpecieCodeValue/cucurbitaMaximaDuchxCMoschataDuch>
        a                cap-iacs-base:SpecieCodeValue ;
        rdfs:label       "Cucurbita maxima Duch. x C. moschata Duch."@en ;
        skos:definition  "-- Definition --\r\nCucurbita maxima Duch. x C. moschata Duch.\r\n-- Description --\r\nList of vegetable specie -H\r\nNOTE. Initial value: H - 37.2"@en ;
        skos:inScheme    cap-iacs-basecode:SpecieCodeValue .

<http://lpis.ec.europa.eu/registry/applicationschema/cap-iacs-base/code#CropItemCodeValue/brassicas>
        a                cap-iacs-base:CropItemCodeValue ;
        rdfs:label       "Brassicas"@en ;
        skos:definition  "-- Definition --\r\n||Brassicas.\r\n-- Description --\r\nCereals and main crops - C\r\nNOTE. Initial value:C1610"@en ;
        skos:inScheme    cap-iacs-basecode:CropItemCodeValue .

<http://lpis.ec.europa.eu/registry/applicationschema/cap-iacs-base/code#CropItemCodeValue/plums>
        a                cap-iacs-base:CropItemCodeValue ;
        rdfs:label       "Plums"@en ;
        skos:definition  "-- Definition --\r\n|||Plums.\r\n-- Description --\r\nCereals and main crops - C\r\nNOTE. Initial value:C2210"@en ;
        skos:inScheme    cap-iacs-basecode:CropItemCodeValue .

<http://lpis.ec.europa.eu/registry/applicationschema/cap-iacs-base/code#ConformanceRequirementClassValue/optional>
        a                cap-iacs-base:ConformanceRequirementClassValue ;
        rdfs:label       "Optional requirement"@en ;
        skos:definition  "--Name--\r\nOptional\r\n\r\n--Definition--\r\nRequirement that may be selected to suit the implementation, provided that any condition applicable to the option are observed."@en ;
        skos:inScheme    cap-iacs-basecode:ConformanceRequirementClassValue .

<http://lpis.ec.europa.eu/registry/applicationschema/cap-iacs-base/code#CropItemCodeValue/redPepperCapsicum>
        a                cap-iacs-base:CropItemCodeValue ;
        rdfs:label       "Red pepper, capsicum"@en ;
        skos:definition  "-- Definition --\r\n|||Red pepper, capsicum.\r\n-- Description --\r\nCereals and main crops - C\r\nNOTE. Initial value:C1790"@en ;
        skos:inScheme    cap-iacs-basecode:CropItemCodeValue .

<http://lpis.ec.europa.eu/registry/applicationschema/cap-iacs-base/code#FarmStructureSurveyNumberValue/permanentGrasslandNoLongerUsedForProductionPurposesAndEligibleForThePaymentOfSubsidies>
        a                cap-iacs-base:FarmStructureSurveyNumberValue ;
        rdfs:label       "Permanent grassland no longer used for production purposes and eligible for the payment of subsidies"@en ;
        skos:definition  "-- Definition --\r\nPermanent grassland no longer used for production purposes and eligible for the payment of subsidies.\r\n-- Description --\r\nAreas of permanent grassland and meadows no longer used for production purposes which, in line with Regulation (EC) No 1782/2003 or, where applicable, the most recent legislation, are maintained in good agricultural and environmental condition and are eligible for financial support.\r\nNOTE. Initial value:2.03.03"@en ;
        skos:inScheme    cap-iacs-basecode:FarmStructureSurveyNumberValue .

<http://lpis.ec.europa.eu/registry/applicationschema/cap-iacs-base/code#CropItemCodeValue/winterTriticale>
        a                cap-iacs-base:CropItemCodeValue ;
        rdfs:label       "Winter triticale"@en ;
        skos:definition  "-- Definition --\r\n||||Winter triticale.\r\n-- Description --\r\nCereals and main crops - C\r\nNOTE. Initial value:C1213"@en ;
        skos:inScheme    cap-iacs-basecode:CropItemCodeValue .

<http://lpis.ec.europa.eu/registry/applicationschema/cap-iacs-base/code#CropItemCodeValue/oats>
        a                cap-iacs-base:CropItemCodeValue ;
        rdfs:label       "Oats"@en ;
        skos:definition  "-- Definition --\r\n||||Oats.\r\n-- Description --\r\nCereals and main crops - C\r\nNOTE. Initial value:C1180"@en ;
        skos:inScheme    cap-iacs-basecode:CropItemCodeValue .

<http://lpis.ec.europa.eu/registry/applicationschema/cap-iacs-base/code#CropItemCodeValue/goldenDelicious>
        a                cap-iacs-base:CropItemCodeValue ;
        rdfs:label       "Golden Delicious"@en ;
        skos:definition  "-- Definition --\r\n||||Golden Delicious.\r\n-- Description --\r\nCereals and main crops - C\r\nNOTE. Initial value:C2112"@en ;
        skos:inScheme    cap-iacs-basecode:CropItemCodeValue .

<http://lpis.ec.europa.eu/registry/applicationschema/cap-iacs-base/code#FarmStructureSurveyNumberValue/otherLand>
        a                cap-iacs-base:FarmStructureSurveyNumberValue ;
        rdfs:label       "Other land"@en ;
        skos:definition  "-- Definition --\r\nOther land.\r\n-- Description --\r\n‘Other land’ includes unutilised agricultural land (agricultural land which is no longer farmed, for economic, social or other reasons, and which is not used in the crop rotation system), wooded area and other land occupied by buildings, farmyards, tracks, ponds, quarries, infertile land, rock, etc.\r\nNOTE. Initial value:2.05"@en ;
        skos:inScheme    cap-iacs-basecode:FarmStructureSurveyNumberValue .

<http://lpis.ec.europa.eu/registry/applicationschema/cap-iacs-base/code#SpecieCodeValue/cucurbitaMoschata>
        a                cap-iacs-base:SpecieCodeValue ;
        rdfs:label       "Cucurbita moschata"@en ;
        skos:definition  "-- Definition --\r\nCucurbita moschata.\r\n-- Description --\r\nList of vegetable specie -H\r\nNOTE. Initial value: H - 37.7"@en ;
        skos:inScheme    cap-iacs-basecode:SpecieCodeValue .

<http://lpis.ec.europa.eu/registry/applicationschema/cap-iacs-base/code#CrossComplianceRuleValue/environmentClimateChangeGoodAgriculturalConditionOfLandSoilAndCarbonStockGaec4>
        a                cap-iacs-base:CrossComplianceRuleValue ;
        rdfs:label       "Environment, climate change, good agricultural condition of land  - Soil and carbon stock  GAEC4"@en ;
        skos:definition  "-- Definition --\r\nEnvironment, climate change, good agricultural condition of land  - Soil and carbon stock  GAEC4.\r\n-- Description --\r\nMinimum soil cover. \r\nNOTE. Initial value:GAEC4"@en ;
        skos:inScheme    cap-iacs-basecode:CrossComplianceRuleValue .

<http://lpis.ec.europa.eu/registry/applicationschema/cap-iacs-base/code#SpecieCodeValue/brassicaNapusLSwede>
        a                cap-iacs-base:SpecieCodeValue ;
        rdfs:label       "Brassica napus L. Swede "@en ;
        skos:definition  "-- Definition --\r\nBrassica napus L. Swede.\r\n-- Description --\r\nList of agricultural species -A\r\nII. Fodder plants\r\nNOTE. Initial value: A - 54."@en ;
        skos:inScheme    cap-iacs-basecode:SpecieCodeValue .

cap-iacs-basecode:ConformanceRequirementStatementValue
        a                skos:ConceptScheme ;
        rdfs:label       "List of conformance requirement statement values"@en ;
        dct:isFormatOf   cap-iacs-base:ConformanceRequirementStatementValue ;
        skos:definition  "--Name--\r\nConformance requirement statement value\r\n\r\n--Definition--\r\nList of conformance requirement statement values."@en .

<http://lpis.ec.europa.eu/registry/applicationschema/cap-iacs-base/code#CropItemCodeValue/vineyardsForWinesWithProtectedGeographicalIndicationPGI>
        a                cap-iacs-base:CropItemCodeValue ;
        rdfs:label       "Vineyards for wines with protected geographical indication (PGI)"@en ;
        skos:definition  "-- Definition --\r\n||||Vineyards for wines with protected geographical indication (PGI).\r\n-- Description --\r\nCereals and main crops - C\r\nNOTE. Initial value:C2442"@en ;
        skos:inScheme    cap-iacs-basecode:CropItemCodeValue .

<http://lpis.ec.europa.eu/registry/applicationschema/cap-iacs-base/code#CropItemCodeValue/plantsHarvestedGreenGrownOnArableLand>
        a                cap-iacs-base:CropItemCodeValue ;
        rdfs:label       "Plants harvested green (grown on arable land)"@en ;
        skos:definition  "-- Definition --\r\n|||Plants harvested green (grown on arable land).\r\n-- Description --\r\nLand use of Agriculture Area in Use -L\r\nNOTE. Initial value:L2610"@en ;
        skos:inScheme    cap-iacs-basecode:CropItemCodeValue .

<http://lpis.ec.europa.eu/registry/applicationschema/cap-iacs-base/code#CropItemCodeValue/riceJaponica>
        a                cap-iacs-base:CropItemCodeValue ;
        rdfs:label       "Rice Japonica"@en ;
        skos:definition  "-- Definition --\r\n|||Rice Japonica.\r\n-- Description --\r\nCereals and main crops - C\r\nNOTE. Initial value:C1252"@en ;
        skos:inScheme    cap-iacs-basecode:CropItemCodeValue .

<http://lpis.ec.europa.eu/registry/applicationschema/cap-iacs-base/code#CropItemCodeValue/beetroot>
        a                cap-iacs-base:CropItemCodeValue ;
        rdfs:label       "Beetroot"@en ;
        skos:definition  "-- Definition --\r\n|||Beetroot.\r\n-- Description --\r\nCereals and main crops - C\r\nNOTE. Initial value:C1860"@en ;
        skos:inScheme    cap-iacs-basecode:CropItemCodeValue .

<http://lpis.ec.europa.eu/registry/applicationschema/cap-iacs-base/code#TestingTypeValue/manual>
        a                cap-iacs-base:TestingTypeValue ;
        rdfs:label       "Manual testing"@en ;
        skos:definition  "--Name--\r\nManual\r\n\r\n-- Definition --\r\nManual testing.\r\n\r\n-- Description --\r\nManual testing may be required when automated testing is too complex and/or human judgement is required. Manual testing should be used only for those standards where automatic testing is not viable."@en ;
        skos:inScheme    cap-iacs-basecode:TestingTypeValue .

<http://lpis.ec.europa.eu/registry/applicationschema/cap-iacs-base/code#CrossComplianceRuleValue/publicHealthAnimalHealthAndPlantHealthIdentificationAndRegistrationOfAnimalsSmr7>
        a                cap-iacs-base:CrossComplianceRuleValue ;
        rdfs:label       "Public health, animal health and plant health  - Identification and registration of animals SMR7"@en ;
        skos:definition  "-- Definition --\r\nPublic health, animal health and plant health  - Identification and registration of animals SMR7.\r\n-- Description --\r\nRegulation (EC) No 1760/2000 of the European Parliament and of the Council of 17 July 2000 establishing a system for the identification and registration of bovine animals and regarding the labelling of beef and beef products and repealing Council Regulation (EC) No 820/97(OJ L 204, 11.8.2000, p. 1) . Articles 4 and 7.\r\nNOTE. Initial value:SMR7"@en ;
        skos:inScheme    cap-iacs-basecode:CrossComplianceRuleValue .

<http://lpis.ec.europa.eu/registry/applicationschema/cap-iacs-base/code#CropItemCodeValue/otherOilSeedCropsNec>
        a                cap-iacs-base:CropItemCodeValue ;
        rdfs:label       "Other oil seed crops n.e.c. "@en ;
        skos:definition  "-- Definition --\r\n|||Other oil seed crops n.e.c. \r\n-- Description --\r\nCereals and main crops - C\r\nNOTE. Initial value:C1480"@en ;
        skos:inScheme    cap-iacs-basecode:CropItemCodeValue .

<http://lpis.ec.europa.eu/registry/applicationschema/cap-iacs-base/code#FarmStructureSurveyNumberValue/unutilisedAgriculturalLand>
        a                cap-iacs-base:FarmStructureSurveyNumberValue ;
        rdfs:label       "Unutilised agricultural land"@en ;
        skos:definition  "-- Definition --\r\nUnutilised agricultural land.\r\n-- Description --\r\nArea previously used as an agricultural area and, during the reference year of the survey, no longer worked for economic, social or other reasons and which is not used in the crop rotation system, i.e. land where no agricultural use is intended.\r\nThis land could be brought back into cultivation using the resources normally available on an agricultural holding.\r\nNOTE. Initial value:2.05.01"@en ;
        skos:inScheme    cap-iacs-basecode:FarmStructureSurveyNumberValue .

<http://lpis.ec.europa.eu/registry/applicationschema/cap-iacs-base/code#CrossComplianceRuleValue/environmentClimateChangeGoodAgriculturalConditionOfLandWaterGaec3>
        a                cap-iacs-base:CrossComplianceRuleValue ;
        rdfs:label       "Environment, climate change, good agricultural condition of land  - Water GAEC3"@en ;
        skos:definition  "-- Definition --\r\nEnvironment, climate change, good agricultural condition of land  - Water GAEC3.\r\n-- Description --\r\nProtection of ground water against pollution: prohibition of direct discharge into groundwater and measures to prevent indirect pollution of groundwater through discharge on the ground and percolation through the soil of dangerous substances, as listed in the Annex to Directive 80/68/EEC in its version in force on the last day of its validity, as far as it relates to agricultural activity. \r\nNOTE. Initial value:GAEC3"@en ;
        skos:inScheme    cap-iacs-basecode:CrossComplianceRuleValue .

<http://lpis.ec.europa.eu/registry/applicationschema/cap-iacs-base/code#CropItemCodeValue/rye>
        a                cap-iacs-base:CropItemCodeValue ;
        rdfs:label       "Rye"@en ;
        skos:definition  "-- Definition --\r\n||||Rye.\r\n-- Description --\r\nCereals and main crops - C\r\nNOTE. Initial value:C1150"@en ;
        skos:inScheme    cap-iacs-basecode:CropItemCodeValue .

<http://lpis.ec.europa.eu/registry/applicationschema/cap-iacs-base/code#FarmStructureSurveyNumberValue/ofWhichPeasFieldBeansAndSweetLupins>
        a                cap-iacs-base:FarmStructureSurveyNumberValue ;
        rdfs:label       "of which peas, field beans and sweet lupins"@en ;
        skos:definition  "-- Definition --\r\nof which peas, field beans and sweet lupins.\r\n-- Description --\r\nPisum sativum L., Vicia faba L., Lupinus spp., sown in pure crops, harvested dry for grain.\r\nNOTE. Initial value:2.01.02.01"@en ;
        skos:inScheme    cap-iacs-basecode:FarmStructureSurveyNumberValue .

<http://lpis.ec.europa.eu/registry/applicationschema/cap-iacs-base/code#NotificationGroupValue/notificationsRelatingToTheBasicPayment>
        a                cap-iacs-base:NotificationGroupValue ;
        rdfs:label       "Notifications relating to the basic payment"@en ;
        skos:definition  "-- Definition --\r\nNotifications relating to the basic payment.\r\n-- Description --\r\nNOTE.63"@en ;
        skos:inScheme    cap-iacs-basecode:NotificationGroupValue .

<http://lpis.ec.europa.eu/registry/applicationschema/cap-iacs-base/code#SpecieCodeValue/festucaRubraLRedFescue>
        a                cap-iacs-base:SpecieCodeValue ;
        rdfs:label       "Festuca rubra L. Red fescue"@en ;
        skos:definition  "-- Definition --\r\nFestuca rubra L. Red fescue.\r\n-- Description --\r\nList of agricultural species -A\r\nII. Fodder plants\r\nNOTE. Initial value: A - 17."@en ;
        skos:inScheme    cap-iacs-basecode:SpecieCodeValue .

<http://lpis.ec.europa.eu/registry/applicationschema/cap-iacs-base/code#CropItemCodeValue/salsifyAndScorzonera>
        a                cap-iacs-base:CropItemCodeValue ;
        rdfs:label       "Salsify and scorzonera"@en ;
        skos:definition  "-- Definition --\r\n|||Salsify and scorzonera.\r\n-- Description --\r\nCereals and main crops - C\r\nNOTE. Initial value:C1870"@en ;
        skos:inScheme    cap-iacs-basecode:CropItemCodeValue .

<http://lpis.ec.europa.eu/registry/applicationschema/cap-iacs-base/code#SpecieCodeValue/lycopersiconEsculentumLxLPimpinellifolium>
        a                cap-iacs-base:SpecieCodeValue ;
        rdfs:label       "Lycopersicon esculentum L. x L. pimpinellifolium"@en ;
        skos:definition  "-- Definition --\r\nLycopersicon esculentum L. x L. pimpinellifolium.\r\n-- Description --\r\nList of vegetable specie -H\r\nNOTE. Initial value: H - 37.5"@en ;
        skos:inScheme    cap-iacs-basecode:SpecieCodeValue .

<http://lpis.ec.europa.eu/registry/applicationschema/cap-iacs-base/code#CropItemCodeValue/raspberries>
        a                cap-iacs-base:CropItemCodeValue ;
        rdfs:label       "Raspberries"@en ;
        skos:definition  "-- Definition --\r\n|||Raspberries.\r\n-- Description --\r\nCereals and main crops - C\r\nNOTE. Initial value:C2278"@en ;
        skos:inScheme    cap-iacs-basecode:CropItemCodeValue .

<http://lpis.ec.europa.eu/registry/applicationschema/cap-iacs-base/code#StatusOfIssueValue/archived>
        a                cap-iacs-base:StatusOfIssueValue ;
        rdfs:label       "Closed"@en ;
        skos:definition  "--Name--\r\nArchived\r\n\r\n-- Definition --\r\nStatus of issue as soon as it has been resolved.\r\n\r\n--Description--\r\nIssues are archived for historic reference."@en ;
        skos:inScheme    cap-iacs-basecode:StatusOfIssueValue .

<http://lpis.ec.europa.eu/registry/applicationschema/cap-iacs-base/code#CrossComplianceRuleValue/animalWelfareAnimalWelfareSmr13>
        a                cap-iacs-base:CrossComplianceRuleValue ;
        rdfs:label       "Animal welfare - Animal welfare SMR13"@en ;
        skos:definition  "-- Definition --\r\nAnimal welfare - Animal welfare SMR13.\r\n-- Description --\r\nCouncil Directive 98/58/EC of 20 July 1998 concerning the protection of animals kept for farming purposes (OJ L 221, 8.8.1998, p. 23) . Article 4 .\r\nNOTE. Initial value:SMR13"@en ;
        skos:inScheme    cap-iacs-basecode:CrossComplianceRuleValue .

<http://lpis.ec.europa.eu/registry/applicationschema/cap-iacs-base/code#AffectedElementTypeValue/applicationSchemaLeaf>
        a                cap-iacs-base:AffectedElementTypeValue ;
        rdfs:label       "Leaf of application schema"@en ;
        skos:definition  "--Name--\r\nApplication schema leaf\r\n\r\n-- Definition --\r\nSpecific package within the application schema that cannot include further (sub)packages."@en ;
        skos:inScheme    cap-iacs-basecode:AffectedElementTypeValue .

<http://lpis.ec.europa.eu/registry/applicationschema/cap-iacs-base/code#FarmStructureSurveyNumberValue/roughGrazings>
        a                cap-iacs-base:FarmStructureSurveyNumberValue ;
        rdfs:label       "Rough grazings"@en ;
        skos:definition  "-- Definition --\r\nRough grazings.\r\n-- Description --\r\nLow yielding permanent grassland, usually on low quality soil, for example on hilly land and at high altitudes, usually unimproved by fertiliser, cultivation, reseeding or drainage.\r\nThese areas can normally be used only for extensive grazing and are not normally mown or are mown in an extensive manner; they cannot support a large density of animals.\r\nNOTE. Initial value:2.03.02"@en ;
        skos:inScheme    cap-iacs-basecode:FarmStructureSurveyNumberValue .

<http://lpis.ec.europa.eu/registry/applicationschema/cap-iacs-base/code#SpecieCodeValue/alliumCepaLCepaGroupOnionEchalion>
        a                cap-iacs-base:SpecieCodeValue ;
        rdfs:label       "Allium cepa L. Cepa group - Onion, Echalion"@en ;
        skos:definition  "-- Definition --\r\nAllium cepa L. Cepa group - Onion, Echalion.\r\n-- Description --\r\nList of vegetable specie -H\r\nNOTE. Initial value: H - 1.2"@en ;
        skos:inScheme    cap-iacs-basecode:SpecieCodeValue .

<http://lpis.ec.europa.eu/registry/applicationschema/cap-iacs-base/code#FarmStructureSurveyNumberValue/underGlassOrOtherAccessibleProtectiveCoverFlowers>
        a                cap-iacs-base:FarmStructureSurveyNumberValue ;
        rdfs:label       "Under glass or other (accessible)  protective cover"@en ;
        skos:definition  "-- Definition --\r\nUnder glass or other (accessible)  protective cover.\r\n-- Description --\r\nFlowers and ornamental plants (excluding nurseries), which for the whole of their period of growth or for the predominant part of it are covered by greenhouses or fixed or mobile high cover (glass or rigid or flexible plastic).\r\nNOTE. Initial value:2.01.08.02"@en ;
        skos:inScheme    cap-iacs-basecode:FarmStructureSurveyNumberValue .

<http://lpis.ec.europa.eu/registry/applicationschema/cap-iacs-base/code#SpecieCodeValue/triticumDurumDesfDurumWheat>
        a                cap-iacs-base:SpecieCodeValue ;
        rdfs:label       "Triticum durum Desf. Durum wheat "@en ;
        skos:definition  "-- Definition --\r\nTriticum durum Desf. Durum wheat.\r\n-- Description --\r\nList of agricultural species -A   \r\nIV. Cereals\r\nNOTE. Initial value: A - 84."@en ;
        skos:inScheme    cap-iacs-basecode:SpecieCodeValue .

<http://lpis.ec.europa.eu/registry/applicationschema/cap-iacs-base/code#CropItemCodeValue/brusselsSprouts>
        a                cap-iacs-base:CropItemCodeValue ;
        rdfs:label       "Brussels sprouts"@en ;
        skos:definition  "-- Definition --\r\n|||Brussels sprouts.\r\n-- Description --\r\nCereals and main crops - C\r\nNOTE. Initial value:C1631"@en ;
        skos:inScheme    cap-iacs-basecode:CropItemCodeValue .

<http://lpis.ec.europa.eu/registry/applicationschema/cap-iacs-base/code#CropItemCodeValue/kitchenGardens>
        a                cap-iacs-base:CropItemCodeValue ;
        rdfs:label       "Kitchen gardens"@en ;
        skos:definition  "-- Definition --\r\n||Kitchen gardens.\r\n-- Description --\r\nLand use of Agriculture Area in Use -L\r\nNOTE. Initial value:L0004"@en ;
        skos:inScheme    cap-iacs-basecode:CropItemCodeValue .

<http://lpis.ec.europa.eu/registry/applicationschema/cap-iacs-base/code#NotificationGroupValue/notificationsRelatingToGreening>
        a                cap-iacs-base:NotificationGroupValue ;
        rdfs:label       "Notifications relating to greening"@en ;
        skos:definition  "-- Definition --\r\nNotifications relating to greening.\r\n-- Description --\r\nNOTE.64"@en ;
        skos:inScheme    cap-iacs-basecode:NotificationGroupValue .

<http://lpis.ec.europa.eu/registry/applicationschema/cap-iacs-base/code#CropItemCodeValue/cornCobMixC1200>
        a                cap-iacs-base:CropItemCodeValue ;
        rdfs:label       "Corn cob mix C1200"@en ;
        skos:definition  "-- Definition --\r\n||||Corn cob mix C1200.\r\n-- Description --\r\nCereals and main crops - C\r\nNOTE. Initial value:C1202"@en ;
        skos:inScheme    cap-iacs-basecode:CropItemCodeValue .

<http://lpis.ec.europa.eu/registry/applicationschema/cap-iacs-base/code#CropItemCodeValue/peas>
        a                cap-iacs-base:CropItemCodeValue ;
        rdfs:label       "Peas"@en ;
        skos:definition  "-- Definition --\r\n|||Peas.\r\n-- Description --\r\nCereals and main crops - C\r\nNOTE. Initial value:C1890"@en ;
        skos:inScheme    cap-iacs-basecode:CropItemCodeValue .

<http://lpis.ec.europa.eu/registry/applicationschema/cap-iacs-base/code#SpecieCodeValue/pisumSativumLPartimWrinkledPea>
        a                cap-iacs-base:SpecieCodeValue ;
        rdfs:label       "Pisum sativum L. (partim) Wrinkled pea"@en ;
        skos:definition  "-- Definition --\r\nPisum sativum L. (partim) Wrinkled pea.\r\n-- Description --\r\nList of vegetable specie -H\r\nNOTE. Initial value: H - 28.1"@en ;
        skos:inScheme    cap-iacs-basecode:SpecieCodeValue .

<http://lpis.ec.europa.eu/registry/applicationschema/cap-iacs-base/code#SpecieCodeValue/sicyosAngulatus>
        a                cap-iacs-base:SpecieCodeValue ;
        rdfs:label       "Sicyos angulatus"@en ;
        skos:definition  "-- Definition --\r\nSicyos angulatus.\r\n-- Description --\r\nList of vegetable specie -H\r\nNOTE. Initial value: H - 37.6"@en ;
        skos:inScheme    cap-iacs-basecode:SpecieCodeValue .

<http://lpis.ec.europa.eu/registry/applicationschema/cap-iacs-base/code#CropItemCodeValue/cherries>
        a                cap-iacs-base:CropItemCodeValue ;
        rdfs:label       "Cherries"@en ;
        skos:definition  "-- Definition --\r\n|||Cherries.\r\n-- Description --\r\nCereals and main crops - C\r\nNOTE. Initial value:C2200"@en ;
        skos:inScheme    cap-iacs-basecode:CropItemCodeValue .

<http://lpis.ec.europa.eu/registry/applicationschema/cap-iacs-base/code#FarmStructureSurveyNumberValue/otherIndustrialCropsNotMentionedElsewhere>
        a                cap-iacs-base:FarmStructureSurveyNumberValue ;
        rdfs:label       "Other industrial crops not mentioned elsewhere"@en ;
        skos:definition  "-- Definition --\r\nOther industrial crops not mentioned elsewhere.\r\n-- Description --\r\nOther industrial crops that have not been mentioned elsewhere.\r\nAreas of crops used exclusively for renewable energy production are included.\r\nNOTE. Initial value:2.01.06.99"@en ;
        skos:inScheme    cap-iacs-basecode:FarmStructureSurveyNumberValue .

<http://lpis.ec.europa.eu/registry/applicationschema/cap-iacs-base/code#NotificationGroupValue/notificationsRelatingToTheFinancialAdjustmentsMadeByMemberStatesInConnectionWithRuralDevelopment>
        a                cap-iacs-base:NotificationGroupValue ;
        rdfs:label       "Notifications relating to the financial adjustments made by Member States in connection with rural development"@en ;
        skos:definition  "-- Definition --\r\nNotifications relating to the financial adjustments made by Member States in connection with rural development.\r\n-- Description --\r\nNOTE.104"@en ;
        skos:inScheme    cap-iacs-basecode:NotificationGroupValue .

<http://lpis.ec.europa.eu/registry/applicationschema/cap-iacs-base/code#SpecieCodeValue/agrostisCaninaLVelvetBent>
        a                cap-iacs-base:SpecieCodeValue ;
        rdfs:label       "Agrostis canina L. Velvet bent"@en ;
        skos:definition  "-- Definition --\r\nAgrostis canina L. Velvet bent.\r\n-- Description --\r\nList of agricultural species -A\r\nII. Fodder plants\r\nNOTE. Initial value: A - 3."@en ;
        skos:inScheme    cap-iacs-basecode:SpecieCodeValue .

cap-iacs-basecode:StatusOfIssueValue
        a                skos:ConceptScheme ;
        rdfs:label       "Issue status value list"@en ;
        dct:isFormatOf   cap-iacs-base:StatusOfIssueValue ;
        skos:definition  "--Name--\r\nStatus of issue value\r\n\r\n-- Definition --\r\nCode list of possible issue status values.\r\n\r\n-- Description --\r\nList of possible issue status values used for documentation of anomaly in the LPIS."@en .

<http://lpis.ec.europa.eu/registry/applicationschema/cap-iacs-base/code#CropItemCodeValue/rice>
        a                cap-iacs-base:CropItemCodeValue ;
        rdfs:label       "Rice "@en ;
        skos:definition  "-- Definition --\r\n||Rice.\r\n-- Description --\r\nCereals and main crops - C\r\nNOTE. Initial value:C1250"@en ;
        skos:inScheme    cap-iacs-basecode:CropItemCodeValue .

<http://lpis.ec.europa.eu/registry/applicationschema/cap-iacs-base/code#NotificationGroupValue/notificationsConcerningTheRedistributivePayment>
        a                cap-iacs-base:NotificationGroupValue ;
        rdfs:label       "Notifications concerning the redistributive payment"@en ;
        skos:definition  "-- Definition --\r\nNotifications concerning the redistributive payment.\r\n-- Description --\r\nNOTE.68"@en ;
        skos:inScheme    cap-iacs-basecode:NotificationGroupValue .

<http://lpis.ec.europa.eu/registry/applicationschema/cap-iacs-base/code#CropItemCodeValue/oatsAndMixedGrainOtherThanMaslin>
        a                cap-iacs-base:CropItemCodeValue ;
        rdfs:label       "Oats and mixed grain other than maslin"@en ;
        skos:definition  "-- Definition --\r\n|||Oats and mixed grain other than maslin.\r\n-- Description --\r\nCereals and main crops - C\r\nNOTE. Initial value:C1170"@en ;
        skos:inScheme    cap-iacs-basecode:CropItemCodeValue .

cap-iacs-basecode:MonthValue
        a                skos:ConceptScheme ;
        rdfs:label       "List of month values"@en ;
        dct:isFormatOf   cap-iacs-base:MonthValue ;
        skos:definition  "-- Definition --\r\nList of months.\r\n-- Description --\r\nList of months."@en .

<http://lpis.ec.europa.eu/registry/applicationschema/cap-iacs-base/code#SpecieCodeValue/betaVulgarisLSugarBeet>
        a                cap-iacs-base:SpecieCodeValue ;
        rdfs:label       "Beta vulgaris L. Sugar beet"@en ;
        skos:definition  "-- Definition --\r\nBeta vulgaris L. Sugar beet.\r\n-- Description --\r\nList of agricultural species -A\r\nI. Beet\r\nNOTE. Initial value: A - 1."@en ;
        skos:inScheme    cap-iacs-basecode:SpecieCodeValue .

<http://lpis.ec.europa.eu/registry/applicationschema/cap-iacs-base/code#SpecieCodeValue/zeaMaysLPopcorn>
        a                cap-iacs-base:SpecieCodeValue ;
        rdfs:label       "Zea mays L. Popcorn"@en ;
        skos:definition  "-- Definition --\r\nZea mays L. Popcorn.\r\n-- Description --\r\nList of vegetable specie -H\r\nNOTE. Initial value: H - 36.2"@en ;
        skos:inScheme    cap-iacs-basecode:SpecieCodeValue .

<http://lpis.ec.europa.eu/registry/applicationschema/cap-iacs-base/code#CropItemCodeValue/otherFibreCropsNec>
        a                cap-iacs-base:CropItemCodeValue ;
        rdfs:label       "Other fibre crops n.e.c."@en ;
        skos:definition  "-- Definition --\r\n|||Other fibre crops n.e.c.\r\n-- Description --\r\nCereals and main crops - C\r\nNOTE. Initial value:C1510"@en ;
        skos:inScheme    cap-iacs-basecode:CropItemCodeValue .

<http://lpis.ec.europa.eu/registry/applicationschema/cap-iacs-base/code#SpecieCodeValue/cichoriumEndiviaLCurledLeavedEndive>
        a                cap-iacs-base:SpecieCodeValue ;
        rdfs:label       "Cichorium endivia L. Curled-leaved endive"@en ;
        skos:definition  "-- Definition --\r\nCichorium endivia L. Curled-leaved endive.\r\n-- Description --\r\nList of vegetable specie -H\r\nNOTE. Initial value: H - 13.1"@en ;
        skos:inScheme    cap-iacs-basecode:SpecieCodeValue .

<http://lpis.ec.europa.eu/registry/applicationschema/cap-iacs-base/code#CropItemCodeValue/greenMaize>
        a                cap-iacs-base:CropItemCodeValue ;
        rdfs:label       "Green maize"@en ;
        skos:definition  "-- Definition --\r\n|||Green maize.\r\n-- Description --\r\nCereals and main crops - C\r\nNOTE. Initial value:C2625"@en ;
        skos:inScheme    cap-iacs-basecode:CropItemCodeValue .

<http://lpis.ec.europa.eu/registry/applicationschema/cap-iacs-base/code#CauseOfAnomalyValue/changeInThePerimeterAdditionOfAgriculturalLand>
        a                cap-iacs-base:CauseOfAnomalyValue ;
        rdfs:label       "Cause flaged as Type III. Change in the perimeter (addition of agricultural land)"@en ;
        skos:definition  "--Name--\r\nChange in the perimeter due to addition of agricultural land\r\n\r\n-- Description --\r\nNew agricultural area has been appended to an existing reference parcel.\r\n\r\nNOTE. Previously known as Type III anomaly."@en ;
        skos:inScheme    cap-iacs-basecode:CauseOfAnomalyValue .

<http://lpis.ec.europa.eu/registry/applicationschema/cap-iacs-base/code#CropItemCodeValue/carrots>
        a                cap-iacs-base:CropItemCodeValue ;
        rdfs:label       "Carrots"@en ;
        skos:definition  "-- Definition --\r\n|||Carrots.\r\n-- Description --\r\nCereals and main crops - C\r\nNOTE. Initial value:C1830"@en ;
        skos:inScheme    cap-iacs-basecode:CropItemCodeValue .

<http://lpis.ec.europa.eu/registry/applicationschema/cap-iacs-base/code#SupportSchemeTypeValue/cropSpecificPaymentForCotton>
        a                cap-iacs-base:SupportSchemeTypeValue ;
        rdfs:label       "Crop-specific payment for cotton"@en ;
        skos:definition  "Crop-specific payment for cotton\r\n\r\nAid shall be granted to farmers producing cotton falling within CN code 5201 00 under the conditions laid down in this Chapter.\r\n\r\nTitle IV, Chapter 2 of 1307/2013 Regulation / Area payment."@en ;
        skos:inScheme    cap-iacs-basecode:SupportSchemeTypeValue .

<http://lpis.ec.europa.eu/registry/applicationschema/cap-iacs-base/code#SpecieCodeValue/carthamusTinctoriusLSafflower>
        a                cap-iacs-base:SpecieCodeValue ;
        rdfs:label       "Carthamus tinctorius L. Safflower"@en ;
        skos:definition  "-- Definition --\r\nCarthamus tinctorius L. Safflower.\r\n-- Description --\r\nList of agricultural species -A\r\nIII. Oil and fibre plants\r\nNOTE. Initial value: A - 64."@en ;
        skos:inScheme    cap-iacs-basecode:SpecieCodeValue .

<http://lpis.ec.europa.eu/registry/applicationschema/cap-iacs-base/code#SpecieCodeValue/festucaFiliformisLFineLeavedSheeps>
        a                cap-iacs-base:SpecieCodeValue ;
        rdfs:label       "Festuca filiformis L. Fine leaved sheep's"@en ;
        skos:definition  "-- Definition --\r\nFestuca filiformis L. Fine leaved sheep's.\r\n-- Description --\r\nList of agricultural species -A\r\nII. Fodder plants\r\nNOTE. Initial value: A - 14."@en ;
        skos:inScheme    cap-iacs-basecode:SpecieCodeValue .

<http://lpis.ec.europa.eu/registry/applicationschema/cap-iacs-base/code#CropItemCodeValue/figs>
        a                cap-iacs-base:CropItemCodeValue ;
        rdfs:label       "Figs"@en ;
        skos:definition  "-- Definition --\r\n|||Figs.\r\n-- Description --\r\nCereals and main crops - C\r\nNOTE. Initial value:C2251"@en ;
        skos:inScheme    cap-iacs-basecode:CropItemCodeValue .

<http://lpis.ec.europa.eu/registry/applicationschema/cap-iacs-base/code#NotificationGroupValue/notificationsRelatingToTheMeasuresRelatedToOperationsFinancedByTheFunds>
        a                cap-iacs-base:NotificationGroupValue ;
        rdfs:label       "Notifications relating to the  measures related to operations financed by the Funds"@en ;
        skos:definition  "-- Definition --\r\nNotifications relating to the  measures related to operations financed by the Funds.\r\n-- Description --\r\nIn addition to the provisions laid down in the sectoral Regulations, Member States shall send to the Commission the information, declarations and documents:  for measures relating to operations financed by the Funds:\r\n(c)(i) declarations of expenditure, which also act as payment requests, signed by the accredited paying agency or the accredited coordinating body and accompanied by the requisite information;\r\n(c)(ii) estimates of their financial requirements, with regard to the EAGF and, with regard to the EAFRD, an update of estimated declarations of expenditure which will be submitted during the year and estimated declarations of \r\nexpenditure in respect of the following financial year;\r\n(c)(iii) the management declaration and the annual accounts of the accredited paying agencies;\r\n(c)(iv) an annual summary of the results of all available audits and checks carried out in accordance with the schedule and detailed provisions laid down in the sector specific rules.\r\nThe annual accounts of accredited paying agencies relating to EAFRD expenditure shall be submitted at the level of each programme.\r\nNOTE.1011c"@en ;
        skos:inScheme    cap-iacs-basecode:NotificationGroupValue .

<http://lpis.ec.europa.eu/registry/applicationschema/cap-iacs-base/code#SpecieCodeValue/citrullusLanatusThunbMatsumEtNakaiWatermelon>
        a                cap-iacs-base:SpecieCodeValue ;
        rdfs:label       "Citrullus lanatus (Thunb.) Matsum. et Nakai Watermelon"@en ;
        skos:definition  "-- Definition --\r\nCitrullus lanatus (Thunb.) Matsum. et Nakai Watermelon.\r\n-- Description --\r\nList of vegetable specie -H\r\nNOTE. Initial value: H - 15."@en ;
        skos:inScheme    cap-iacs-basecode:SpecieCodeValue .

<http://lpis.ec.europa.eu/registry/applicationschema/cap-iacs-base/code#CropItemCodeValue/apples>
        a                cap-iacs-base:CropItemCodeValue ;
        rdfs:label       "Apples"@en ;
        skos:definition  "-- Definition --\r\n||Apples.\r\n-- Description --\r\nCereals and main crops - C\r\nNOTE. Initial value:C2090"@en ;
        skos:inScheme    cap-iacs-basecode:CropItemCodeValue .

<http://lpis.ec.europa.eu/registry/applicationschema/cap-iacs-base/code#SpecieCodeValue/brassicaOleraceaLRedCabbage>
        a                cap-iacs-base:SpecieCodeValue ;
        rdfs:label       "Brassica oleracea L. Red cabbage"@en ;
        skos:definition  "-- Definition --\r\nBrassica oleracea L. Red cabbage.\r\n-- Description --\r\nList of vegetable specie -H\r\nNOTE. Initial value: H - 10.7"@en ;
        skos:inScheme    cap-iacs-basecode:SpecieCodeValue .

<http://lpis.ec.europa.eu/registry/applicationschema/cap-iacs-base/code#ConformanceRequirementStatementValue/positive>
        a                cap-iacs-base:ConformanceRequirementStatementValue ;
        rdfs:label       "Positive statement"@en ;
        skos:definition  "--Name--\r\nPositive\r\n\r\n--Definition--\r\nAffirmative statement.\r\n\r\n--Description--\r\nPositive statement state what is required to be done."@en ;
        skos:inScheme    cap-iacs-basecode:ConformanceRequirementStatementValue .

<http://lpis.ec.europa.eu/registry/applicationschema/cap-iacs-base/code#SpecieCodeValue/viciaFabaLPartimFieldBean>
        a                cap-iacs-base:SpecieCodeValue ;
        rdfs:label       "Vicia faba L. (Partim) Field bean"@en ;
        skos:definition  "-- Definition --\r\nVicia faba L. (Partim) Field bean.\r\n-- Description --\r\nList of agricultural species -A\r\nII. Fodder plants\r\nNOTE. Initial value: A - 50."@en ;
        skos:inScheme    cap-iacs-basecode:SpecieCodeValue .

<http://lpis.ec.europa.eu/registry/applicationschema/cap-iacs-base/code#SpecieCodeValue/lupinusLuteusLYellowLupin>
        a                cap-iacs-base:SpecieCodeValue ;
        rdfs:label       "Lupinus luteus L. Yellow lupin"@en ;
        skos:definition  "-- Definition --\r\nLupinus luteus L. Yellow lupin.\r\n-- Description --\r\nList of agricultural species -A\r\nII. Fodder plants\r\nNOTE. Initial value: A - 37."@en ;
        skos:inScheme    cap-iacs-basecode:SpecieCodeValue .

<http://lpis.ec.europa.eu/registry/applicationschema/cap-iacs-base/code#FarmStructureSurveyNumberValue/aromaticPlantsMedicinalAndCulinaryPlants>
        a                cap-iacs-base:FarmStructureSurveyNumberValue ;
        rdfs:label       "Aromatic plants, medicinal and culinary plants"@en ;
        skos:definition  "-- Definition --\r\nAromatic plants, medicinal and culinary plants.\r\n-- Description --\r\nPlants or parts of plants for pharmaceutical purposes, perfume manufacture or human consumption.\r\nCulinary plants are distinguished from vegetables in that they are used in small amounts and provide flavour rather than substance to food.\r\nNOTE. Initial value:2.01.06.12"@en ;
        skos:inScheme    cap-iacs-basecode:FarmStructureSurveyNumberValue .

<http://lpis.ec.europa.eu/registry/applicationschema/cap-iacs-base/code#SpecieCodeValue/cynaraCardunculusLGlobeArtichoke>
        a                cap-iacs-base:SpecieCodeValue ;
        rdfs:label       "Cynara cardunculus L. Globe artichoke"@en ;
        skos:definition  "-- Definition --\r\nCynara cardunculus L. Globe artichoke.\r\n-- Description --\r\nList of vegetable specie -H\r\nNOTE. Initial value: H - 20.1"@en ;
        skos:inScheme    cap-iacs-basecode:SpecieCodeValue .

<http://lpis.ec.europa.eu/registry/applicationschema/cap-iacs-base/code#CrossComplianceRuleValue/publicHealthAnimalHealthAndPlantHealthPlantProtectionProductsSmr10>
        a                cap-iacs-base:CrossComplianceRuleValue ;
        rdfs:label       "Public health, animal health and plant health  - Plant protection products SMR10"@en ;
        skos:definition  "-- Definition --\r\nPublic health, animal health and plant health  - Plant protection products SMR10\r\n-- Description --\r\nRegulation (EC) No 1107/2009 of the European Parliament and of the Council of 21 October 2009 concerning the placing of plant protection products on the market and repealing Council Directives 79/117/EEC and 91/414/EEC (OJ L 309, 24.11.2009, p. 1). Article 55, first and second sentence.\r\nNOTE. Initial value:SMR10"@en ;
        skos:inScheme    cap-iacs-basecode:CrossComplianceRuleValue .

<http://lpis.ec.europa.eu/registry/applicationschema/cap-iacs-base/code#NotificationGroupValue/notificationsConcerningAnyAdditionalDetailsToBeProvidedOnRequest>
        a                cap-iacs-base:NotificationGroupValue ;
        rdfs:label       "Notifications concerning any additional details to be provided on request"@en ;
        skos:definition  "-- Definition --\r\nNotifications concerning any additional details to be provided on request.\r\n-- Description --\r\nNOTE.721"@en ;
        skos:inScheme    cap-iacs-basecode:NotificationGroupValue .

<http://lpis.ec.europa.eu/registry/applicationschema/cap-iacs-base/code#FarmStructureSurveyNumberValue/grainMaize>
        a                cap-iacs-base:FarmStructureSurveyNumberValue ;
        rdfs:label       "Grain maize"@en ;
        skos:definition  "-- Definition --\r\nGrain maize.\r\n-- Description --\r\nMaize (Zea mays L.) harvested for grain.\r\nNOTE. Initial value:2.01.01.06"@en ;
        skos:inScheme    cap-iacs-basecode:FarmStructureSurveyNumberValue .

<http://lpis.ec.europa.eu/registry/applicationschema/cap-iacs-base/code#SpecieCodeValue/trigonellaFoenumGraecumLFenugreek>
        a                cap-iacs-base:SpecieCodeValue ;
        rdfs:label       "Trigonella foenum-graecum L. Fenugreek   "@en ;
        skos:definition  "-- Definition --\r\nTrigonella foenum-graecum L. Fenugreek.\r\n-- Description --\r\nList of agricultural species -A\r\nII. Fodder plants\r\nNOTE. Initial value: A - 49."@en ;
        skos:inScheme    cap-iacs-basecode:SpecieCodeValue .

<http://lpis.ec.europa.eu/registry/applicationschema/cap-iacs-base/code#TestVerdictValue/pass>
        a                cap-iacs-base:TestVerdictValue ;
        rdfs:label       "Pas verdict"@en ;
        skos:definition  "--Name--\r\nPass\r\n\r\n-- Definition --\r\nPass verdict to indicate that the tested requirements are fulfilled.\r\n\r\n-- Description --\r\nTest verdict of conformance."@en ;
        skos:inScheme    cap-iacs-basecode:TestVerdictValue .

<http://lpis.ec.europa.eu/registry/applicationschema/cap-iacs-base/code#SpecieCodeValue/dactylisGlomerataLCocksfoot>
        a                cap-iacs-base:SpecieCodeValue ;
        rdfs:label       "Dactylis glomerata L. Cocksfoot "@en ;
        skos:definition  "-- Definition --\r\nDactylis glomerata L. Cocksfoot.\r\n-- Description --\r\nList of agricultural species -A\r\nII. Fodder plants\r\nNOTE. Initial value: A - 12."@en ;
        skos:inScheme    cap-iacs-basecode:SpecieCodeValue .

cap-iacs-basecode:FarmStructureSurveyNumberValue
        a                skos:ConceptScheme ;
        rdfs:label       "List of farm structure survey numbers"@en ;
        dct:isFormatOf   cap-iacs-base:FarmStructureSurveyNumberValue ;
        skos:definition  "-- Definition --\r\nList of farm structure survey numbers (aggregate of crop items).\r\n-- Desription --\r\nScope - LAND part only. Commision regulations (EC) No 1200/2009 of 30 November 2009 Implementing Regulation (EC) No 1166/2008 of the European Parliament and of the Council on farm structure surveys and the survey on agricultural production methods, as regards livestock unit coefficients and definitions of the characteristics (Text with EEA relevance)."@en .

<http://lpis.ec.europa.eu/registry/applicationschema/cap-iacs-base/code#CropItemCodeValue/sunflowerSeed>
        a                cap-iacs-base:CropItemCodeValue ;
        rdfs:label       "Sunflower seed "@en ;
        skos:definition  "-- Definition --\r\n||||Sunflower seed.\r\n-- Description --\r\nCereals and main crops - C\r\nNOTE. Initial value:C1450"@en ;
        skos:inScheme    cap-iacs-basecode:CropItemCodeValue .

<http://lpis.ec.europa.eu/registry/applicationschema/cap-iacs-base/code#SpecieCodeValue/phalarisCanariensisLCanaryGrass>
        a                cap-iacs-base:SpecieCodeValue ;
        rdfs:label       "Phalaris canariensis L. Canary grass"@en ;
        skos:definition  "-- Definition --\r\nPhalaris canariensis L. Canary grass.\r\n-- Description --\r\nList of agricultural species -A   \r\nIV. Cereals\r\nNOTE. Initial value: A - 77."@en ;
        skos:inScheme    cap-iacs-basecode:SpecieCodeValue .

<http://lpis.ec.europa.eu/registry/applicationschema/cap-iacs-base/code#SpecieCodeValue/sinapisAlbaLWhiteMustard>
        a                cap-iacs-base:SpecieCodeValue ;
        rdfs:label       "Sinapis alba L. White mustard"@en ;
        skos:definition  "-- Definition --\r\nSinapis alba L. White mustard.\r\n-- Description --\r\nList of agricultural species -A\r\nIII. Oil and fibre plants\r\nNOTE. Initial value: A - 70."@en ;
        skos:inScheme    cap-iacs-basecode:SpecieCodeValue .

<http://lpis.ec.europa.eu/registry/applicationschema/cap-iacs-base/code#AffectedElementTypeValue/type>
        a                cap-iacs-base:AffectedElementTypeValue ;
        rdfs:label       "Type"@en ;
        skos:definition  "--Name--\r\nType\r\n\r\n-- Definition --\r\nSpecification of a value domain [ISO 19103:2005].\r\n\r\n-- Description --\r\nTypes include data types, enumerated types, code list values, etc.\r\n\r\nEXAMPLE 1. Primitive types defined in international standards: integer, boolean, GM_Object, etc.\r\n\r\nEXAMPLE 2. Own types defined in the model and re-used for different purposes. LPIS QA uses the TechnicalReasonValue type to describe critical defects and contaminations with the same technical terms.\r\n\r\nEXAMPLE 3. Types defined in other model and imported for re-use. LCM uses  DocumentCitation type defined in INSPIRE."@en ;
        skos:inScheme    cap-iacs-basecode:AffectedElementTypeValue .

<http://lpis.ec.europa.eu/registry/applicationschema/cap-iacs-base/code#CropItemCodeValue/celery>
        a                cap-iacs-base:CropItemCodeValue ;
        rdfs:label       "Celery"@en ;
        skos:definition  "-- Definition --\r\n|||Celery.\r\n-- Description --\r\nCereals and main crops - C\r\nNOTE. Initial value:C1672"@en ;
        skos:inScheme    cap-iacs-basecode:CropItemCodeValue .

<http://lpis.ec.europa.eu/registry/applicationschema/cap-iacs-base/code#StatusValue/underEvaluation>
        a                cap-iacs-base:StatusValue ;
        rdfs:label       "Under evaluation"@en ;
        skos:definition  "-- Name--\r\nUnder evaluation\r\n\r\n--Definition--\r\nStatus of an object according to the state machine diagram.\r\n\r\n-- Description --\r\nPreliminary assessment about the impact of the Upgrade issue or the anomaly. This value should be assigned in the phase when\r\n- supporting evidences are collected  and/or\r\n- checks for issue/anomaly duplicates are performed.  \r\nThe assessment may conclude that no modification to the existing data is needed, or that the reported change request has to be further processed."@en ;
        skos:inScheme    cap-iacs-basecode:StatusValue .

<http://lpis.ec.europa.eu/registry/applicationschema/cap-iacs-base/code#CropItemCodeValue/earlyPotatoes>
        a                cap-iacs-base:CropItemCodeValue ;
        rdfs:label       "Early potatoes"@en ;
        skos:definition  "-- Definition --\r\n|||Early potatoes.\r\n-- Description --\r\nCereals and main crops - C\r\nNOTE. Initial value:C1362"@en ;
        skos:inScheme    cap-iacs-basecode:CropItemCodeValue .

<http://lpis.ec.europa.eu/registry/applicationschema/cap-iacs-base/code#AffectedElementTypeValue/ocl>
        a                cap-iacs-base:AffectedElementTypeValue ;
        rdfs:label       "OCL"@en ;
        skos:definition  "--Name--\r\nOCL\r\n\r\n-- Definition --\r\nThe Object Constraint Language (OCL) is a declarative language for describing rules that apply to Unified Modelling Language (UML) models."@en ;
        skos:inScheme    cap-iacs-basecode:AffectedElementTypeValue .

<http://lpis.ec.europa.eu/registry/applicationschema/cap-iacs-base/code#CropItemCodeValue/fallowLand>
        a                cap-iacs-base:CropItemCodeValue ;
        rdfs:label       "Fallow land"@en ;
        skos:definition  "-- Definition --\r\n|||Fallow land.\r\n-- Description --\r\nLand use of Agriculture Area in Use -L\r\nNOTE. Initial value:L2696"@en ;
        skos:inScheme    cap-iacs-basecode:CropItemCodeValue .

<http://lpis.ec.europa.eu/registry/applicationschema/cap-iacs-base/code#CropItemCodeValue/rape>
        a                cap-iacs-base:CropItemCodeValue ;
        rdfs:label       "Rape"@en ;
        skos:definition  "-- Definition --\r\n|||||Rape.\r\n-- Description --\r\nCereals and main crops - C\r\nNOTE. Initial value:C1430"@en ;
        skos:inScheme    cap-iacs-basecode:CropItemCodeValue .

<http://lpis.ec.europa.eu/registry/applicationschema/cap-iacs-base/code#FarmStructureSurveyNumberValue/permanentGrassland>
        a                cap-iacs-base:FarmStructureSurveyNumberValue ;
        rdfs:label       "Permanent grassland"@en ;
        skos:definition  "-- Definition --\r\nPermanent grassland.\r\n-- Description --\r\nLand used permanently (for five years or more) to grow herbaceous forage crops, through cultivation (sown) or naturally (self-seeded), and that is not included in the crop rotation on the holding.\r\nThe land can be used for grazing or mown for silage, hay or used for renewable energy production.\r\nNOTE. Initial value:2.03"@en ;
        skos:inScheme    cap-iacs-basecode:FarmStructureSurveyNumberValue .

<http://lpis.ec.europa.eu/registry/applicationschema/cap-iacs-base/code#FarmStructureSurveyNumberValue/otherPermanentCrops>
        a                cap-iacs-base:FarmStructureSurveyNumberValue ;
        rdfs:label       "Other permanent crops"@en ;
        skos:definition  "-- Definition --\r\nOther permanent crops.\r\n-- Description --\r\nOpen-air permanent crops other than those under the previous heading and in particular those used for plaiting or weaving, harvested generally every year.\r\nNOTE. Initial value:2.04.06"@en ;
        skos:inScheme    cap-iacs-basecode:FarmStructureSurveyNumberValue .

<http://lpis.ec.europa.eu/registry/applicationschema/cap-iacs-base/code#CropItemCodeValue/potatoesIncludingEarlyPotatoesAndSeedPotatoesL1360>
        a                cap-iacs-base:CropItemCodeValue ;
        rdfs:label       "Potatoes (including early potatoes and seed potatoes) L1360"@en ;
        skos:definition  "-- Definition --\r\n||||Potatoes (including early potatoes and seed potatoes) L1360.\r\n-- Description --\r\nLand use of Agriculture Area in Use -L\r\nNOTE. Initial value:L1360"@en ;
        skos:inScheme    cap-iacs-basecode:CropItemCodeValue .

<http://lpis.ec.europa.eu/registry/applicationschema/cap-iacs-base/code#CropItemCodeValue/shallots>
        a                cap-iacs-base:CropItemCodeValue ;
        rdfs:label       "Shallots"@en ;
        skos:definition  "-- Definition --\r\n|||Shallots.\r\n-- Description --\r\nCereals and main crops - C\r\nNOTE. Initial value:C1855"@en ;
        skos:inScheme    cap-iacs-basecode:CropItemCodeValue .

<http://lpis.ec.europa.eu/registry/applicationschema/cap-iacs-base/code#CropItemCodeValue/tomatoesForFreshConsumptionUnderGlassOrHighAccessibleCover>
        a                cap-iacs-base:CropItemCodeValue ;
        rdfs:label       "Tomatoes for fresh consumption under glass or high accessible cover"@en ;
        skos:definition  "-- Definition --\r\n|||||Tomatoes for fresh consumption under glass or high accessible cover.\r\n-- Description --\r\nCereals and main crops - C\r\nNOTE. Initial value:C1752"@en ;
        skos:inScheme    cap-iacs-basecode:CropItemCodeValue .

<http://lpis.ec.europa.eu/registry/applicationschema/cap-iacs-base/code#NotificationGroupValue/notificationsRelatingToTheReductionCoefficient>
        a                cap-iacs-base:NotificationGroupValue ;
        rdfs:label       "Notifications relating to the reduction coefficient"@en ;
        skos:definition  "-- Definition --\r\nNotifications relating to the reduction coefficient.\r\n-- Description --\r\nNOTE.62"@en ;
        skos:inScheme    cap-iacs-basecode:NotificationGroupValue .

cap-iacs-basecode:CropItemCodeValue
        a                skos:ConceptScheme ;
        rdfs:label       "List of crop items"@en ;
        dct:isFormatOf   cap-iacs-base:CropItemCodeValue ;
        skos:definition  "-- Definition --\r\nList of crop items (aggregate of a species)\r\nEurostat Handbook for Annual Crop Statistics (Regulation 543/2009) (Revision 2013 – Presented in the WPM of the 12).\r\n-- Description --\r\nLand use of Agriculture Area in Use -L\r\nCereals and main crops - C"@en .

<http://lpis.ec.europa.eu/registry/applicationschema/cap-iacs-base/code#FarmStructureSurveyNumberValue/nurseries>
        a                cap-iacs-base:FarmStructureSurveyNumberValue ;
        rdfs:label       "Nurseries"@en ;
        skos:definition  "-- Definition --\r\nNurseries.\r\n-- Description --\r\nAreas of young ligneous (woody) plants grown in the open air for subsequent transplantation:\r\n(a) vine and root-stock nurseries;\r\n(b) fruit tree and berries nurseries;\r\n(c) ornamental nurseries;\r\n(d) commercial nurseries of forest trees (excluding those for the holding’s own requirements grown within woodland);\r\n(e) trees and bushes for planting in gardens, parks, at the roadside and on embankments (e.g. hedgerow plants, rose trees and other ornamental bushes, ornamental conifers), including in all cases their stocks and young seedlings.\r\nNOTE. Initial value:2.04.05"@en ;
        skos:inScheme    cap-iacs-basecode:FarmStructureSurveyNumberValue .

<http://lpis.ec.europa.eu/registry/applicationschema/cap-iacs-base/code#CropItemCodeValue/hops>
        a                cap-iacs-base:CropItemCodeValue ;
        rdfs:label       "Hops"@en ;
        skos:definition  "-- Definition --\r\n||Hops.\r\n-- Description --\r\nCereals and main crops - C\r\nNOTE. Initial value:C1560"@en ;
        skos:inScheme    cap-iacs-basecode:CropItemCodeValue .

<http://lpis.ec.europa.eu/registry/applicationschema/cap-iacs-base/code#RecurenceValue/yearly>
        a                cap-iacs-base:RecurenceValue ;
        rdfs:label       "Yearly recurrence"@en ;
        skos:definition  "-- Definition --\r\nYearly recurrence.\r\n-- Description --\r\nItem description."@en ;
        skos:inScheme    cap-iacs-basecode:RecurenceValue .

<http://lpis.ec.europa.eu/registry/applicationschema/cap-iacs-base/code#NotificationGroupValue/notificationsConcerningTheValueOfPaymentEntitlementsSpsAndConvergence>
        a                cap-iacs-base:NotificationGroupValue ;
        rdfs:label       "Notifications concerning the value of payment entitlements (SPS) and convergence"@en ;
        skos:definition  "-- Definition --\r\nNotifications concerning the value of payment entitlements (SPS) and convergence.\r\n-- Description --\r\nNOTE.76"@en ;
        skos:inScheme    cap-iacs-basecode:NotificationGroupValue .

<http://lpis.ec.europa.eu/registry/applicationschema/cap-iacs-base/code#CropItemCodeValue/flowersAndOrnamentalPlantsExcludingNurseries>
        a                cap-iacs-base:CropItemCodeValue ;
        rdfs:label       "Flowers and ornamental plants (excluding nurseries)"@en ;
        skos:definition  "-- Definition --\r\n|||Flowers and ornamental plants (excluding nurseries).\r\n-- Description --\r\nLand use of Agriculture Area in Use -L\r\nNOTE. Initial value:L3001"@en ;
        skos:inScheme    cap-iacs-basecode:CropItemCodeValue .

<http://lpis.ec.europa.eu/registry/applicationschema/cap-iacs-base/code#SpecieCodeValue/cucumisSativusLCucumber>
        a                cap-iacs-base:SpecieCodeValue ;
        rdfs:label       "Cucumis sativus L. Cucumber"@en ;
        skos:definition  "-- Definition --\r\nCucumis sativus L. Cucumber.\r\n-- Description --\r\nList of vegetable specie -H\r\nNOTE. Initial value: H - 17.1"@en ;
        skos:inScheme    cap-iacs-basecode:SpecieCodeValue .

<http://lpis.ec.europa.eu/registry/applicationschema/cap-iacs-base/code#CropItemCodeValue/cropProductionUnderGlassOrHighAccessibleCover>
        a                cap-iacs-base:CropItemCodeValue ;
        rdfs:label       "Crop production under glass or high accessible cover"@en ;
        skos:definition  "-- Definition --\r\nCrop production under glass or high accessible cover.\r\n-- Description --\r\nLand use of Agriculture Area in Use -L. Special aggregates\r\nNOTE. Initial value:L0900"@en ;
        skos:inScheme    cap-iacs-basecode:CropItemCodeValue .

<http://lpis.ec.europa.eu/registry/applicationschema/cap-iacs-base/code#SpecieCodeValue/sorghumBicolorLMoench×SorghumSudanensePiperStapfHybrids>
        a                cap-iacs-base:SpecieCodeValue ;
        rdfs:label       "Sorghum bicolor (L.) Moench × Sorghum sudanense (Piper) Stapf. Hybrids"@en ;
        skos:definition  "-- Definition --\r\nSorghum bicolor (L.) Moench × Sorghum sudanense (Piper) Stapf. Hybrids resulting from the crossing of Sorghum bicolor and Sorghum sudanense.\r\n-- Description --\r\nList of agricultural species -A   \r\nIV. Cereals\r\nNOTE. Initial value: A - 81."@en ;
        skos:inScheme    cap-iacs-basecode:SpecieCodeValue .

<http://lpis.ec.europa.eu/registry/applicationschema/cap-iacs-base/code#SpecieCodeValue/spinaciaOleraceaLSpinach>
        a                cap-iacs-base:SpecieCodeValue ;
        rdfs:label       "Spinacia oleracea L. Spinach"@en ;
        skos:definition  "-- Definition --\r\nSpinacia oleracea L. Spinach.\r\n-- Description --\r\nList of vegetable specie -H\r\nNOTE. Initial value: H - 33."@en ;
        skos:inScheme    cap-iacs-basecode:SpecieCodeValue .

cap-iacs-basecode:ConformanceRequirementClassValue
        a                skos:ConceptScheme ;
        rdfs:label       "List of conformance requirement class values"@en ;
        dct:isFormatOf   cap-iacs-base:ConformanceRequirementClassValue ;
        skos:definition  "--Name--\r\nConformance requirement class value\r\n\r\n--Definition--\r\nList of conformance requirement class values."@en .

<http://lpis.ec.europa.eu/registry/applicationschema/cap-iacs-base/code#CropItemCodeValue/satsumas>
        a                cap-iacs-base:CropItemCodeValue ;
        rdfs:label       "Satsumas"@en ;
        skos:definition  "-- Definition --\r\n||||Satsumas.\r\n-- Description --\r\nCereals and main crops - C\r\nNOTE. Initial value:C2352"@en ;
        skos:inScheme    cap-iacs-basecode:CropItemCodeValue .

<http://lpis.ec.europa.eu/registry/applicationschema/cap-iacs-base/code#FarmStructureSurveyNumberValue/oats>
        a                cap-iacs-base:FarmStructureSurveyNumberValue ;
        rdfs:label       "Oats"@en ;
        skos:definition  "-- Definition --\r\nOats.\r\n-- Description --\r\nAvena sativa L., including mixtures of oats and other cereals sown in the spring.\r\nNOTE. Initial value:2.01.01.05"@en ;
        skos:inScheme    cap-iacs-basecode:FarmStructureSurveyNumberValue .

<http://lpis.ec.europa.eu/registry/applicationschema/cap-iacs-base/code#CauseOfAnomalyValue/causeUnknown>
        a                cap-iacs-base:CauseOfAnomalyValue ;
        rdfs:label       "The cause is flagged as unknown"@en ;
        skos:definition  "--Name--\r\nCause unknown\r\n\r\n-- Description --\r\nNo case can be detected and/or no third party information is available about the possible cause of anomaly."@en ;
        skos:inScheme    cap-iacs-basecode:CauseOfAnomalyValue .

<http://lpis.ec.europa.eu/registry/applicationschema/cap-iacs-base/code#CropItemCodeValue/caraway>
        a                cap-iacs-base:CropItemCodeValue ;
        rdfs:label       "Caraway"@en ;
        skos:definition  "-- Definition --\r\n||||Caraway.\r\n-- Description --\r\nCereals and main crops - C\r\nNOTE. Initial value:C1582"@en ;
        skos:inScheme    cap-iacs-basecode:CropItemCodeValue .

cap-iacs-basecode:CauseOfAnomalyValue
        a                skos:ConceptScheme ;
        rdfs:label       "Anomaly cause value list"@en ;
        dct:isFormatOf   cap-iacs-base:CauseOfAnomalyValue ;
        skos:definition  "--Name--\r\nCause of anomaly value\r\n\r\n-- Definition --\r\nCode list defining the values of the case of anomaly attribute.\r\n\r\n-- Description --\r\nList of possible anomaly causes used for documentation of an anomaly."@en .

<http://lpis.ec.europa.eu/registry/applicationschema/cap-iacs-base/code#CropItemCodeValue/permanentCropsUnderGlassOrHighAccessibleCover>
        a                cap-iacs-base:CropItemCodeValue ;
        rdfs:label       "Permanent crops under glass or high accessible cover"@en ;
        skos:definition  "-- Definition --\r\nPermanent crops under glass or high accessible cover.\r\n-- Description --\r\nLand use of Agriculture Area in Use -L. Special aggregates\r\nNOTE. Initial value:L1114"@en ;
        skos:inScheme    cap-iacs-basecode:CropItemCodeValue .

<http://lpis.ec.europa.eu/registry/applicationschema/cap-iacs-base/code#SpecieCodeValue/brassicaNigraLBlackMustard>
        a                cap-iacs-base:SpecieCodeValue ;
        rdfs:label       "Brassica nigra L. Black mustard "@en ;
        skos:definition  "-- Definition --\r\nBrassica nigra L. Black mustard.\r\n-- Description --\r\nList of agricultural species -A\r\nIII. Oil and fibre plants\r\nNOTE. Initial value: A - 62."@en ;
        skos:inScheme    cap-iacs-basecode:SpecieCodeValue .

<http://lpis.ec.europa.eu/registry/applicationschema/cap-iacs-base/code#CropItemCodeValue/turnipRape>
        a                cap-iacs-base:CropItemCodeValue ;
        rdfs:label       "Turnip rape"@en ;
        skos:definition  "-- Definition --\r\n|||||Turnip rape.\r\n-- Description --\r\nCereals and main crops - C\r\nNOTE. Initial value:C1440"@en ;
        skos:inScheme    cap-iacs-basecode:CropItemCodeValue .

<http://lpis.ec.europa.eu/registry/applicationschema/cap-iacs-base/code#CropItemCodeValue/leeks>
        a                cap-iacs-base:CropItemCodeValue ;
        rdfs:label       "Leeks"@en ;
        skos:definition  "-- Definition --\r\n|||Leeks.\r\n-- Description --\r\nCereals and main crops - C\r\nNOTE. Initial value:C1675"@en ;
        skos:inScheme    cap-iacs-basecode:CropItemCodeValue .

<http://lpis.ec.europa.eu/registry/applicationschema/cap-iacs-base/code#CropItemCodeValue/vineyardsForRaisins>
        a                cap-iacs-base:CropItemCodeValue ;
        rdfs:label       "Vineyards for raisins"@en ;
        skos:definition  "-- Definition --\r\n|||Vineyards for raisins.\r\n-- Description --\r\nCereals and main crops - C\r\nNOTE. Initial value:C2416"@en ;
        skos:inScheme    cap-iacs-basecode:CropItemCodeValue .

<http://lpis.ec.europa.eu/registry/applicationschema/cap-iacs-base/code#CropItemCodeValue/potatoesIncludingEarlyPotatoesAndSeedPotatoes>
        a                cap-iacs-base:CropItemCodeValue ;
        rdfs:label       "Potatoes (including early potatoes and seed potatoes)"@en ;
        skos:definition  "-- Definition --\r\n||Potatoes (including early potatoes and seed potatoes).\r\n-- Description --\r\nCereals and main crops - C\r\nNOTE. Initial value:C1360"@en ;
        skos:inScheme    cap-iacs-basecode:CropItemCodeValue .

<http://lpis.ec.europa.eu/registry/applicationschema/cap-iacs-base/code#CrossComplianceRuleValue/environmentClimateChangeGoodAgriculturalConditionOfLandSoilAndCarbonStockGaec6>
        a                cap-iacs-base:CrossComplianceRuleValue ;
        rdfs:label       "Environment, climate change, good agricultural condition of land  - Soil and carbon stock  GAEC6"@en ;
        skos:definition  "-- Definition --\r\nEnvironment, climate change, good agricultural condition of land  - Soil and carbon stock  GAEC6.\r\n-- Description --\r\nMaintenance of soil organic matter level through appropriate practices including ban on burning arable stubble, except for plant health reasons.. The requirement can be limited to a general ban on burning arable stubble, but a Member State may decide to prescribe further requirements.\r\nNOTE. Initial value:GAEC6"@en ;
        skos:inScheme    cap-iacs-basecode:CrossComplianceRuleValue .

<http://lpis.ec.europa.eu/registry/applicationschema/cap-iacs-base/code#CropItemCodeValue/vegetablesMelonsAndStrawberriesExcludingKitchenGardens>
        a                cap-iacs-base:CropItemCodeValue ;
        rdfs:label       "Vegetables, melons and strawberries (excluding kitchen gardens)"@en ;
        skos:definition  "-- Definition --\r\n|Vegetables, melons and strawberries (excluding kitchen gardens).\r\n-- Description --\r\nCereals and main crops - C\r\nNOTE. Initial value:C1600"@en ;
        skos:inScheme    cap-iacs-basecode:CropItemCodeValue .

<http://lpis.ec.europa.eu/registry/applicationschema/cap-iacs-base/code#CropItemCodeValue/riceOp>
        a                cap-iacs-base:CropItemCodeValue ;
        rdfs:label       "Rice Op"@en ;
        skos:definition  "-- Definition --\r\n|||Rice Op.\r\n-- Description --\r\nLand use of Agriculture Area in Use -L\r\nNOTE. Initial value:L1250"@en ;
        skos:inScheme    cap-iacs-basecode:CropItemCodeValue .

<http://lpis.ec.europa.eu/registry/applicationschema/cap-iacs-base/code#CropItemCodeValue/quinces>
        a                cap-iacs-base:CropItemCodeValue ;
        rdfs:label       "Quinces"@en ;
        skos:definition  "-- Definition --\r\n|||Quinces.\r\n-- Description --\r\nCereals and main crops - C\r\nNOTE. Initial value:C2252"@en ;
        skos:inScheme    cap-iacs-basecode:CropItemCodeValue .

<http://lpis.ec.europa.eu/registry/applicationschema/cap-iacs-base/code#FarmStructureSurveyNumberValue/berrySpecies>
        a                cap-iacs-base:FarmStructureSurveyNumberValue ;
        rdfs:label       "Berry species"@en ;
        skos:definition  "-- Definition --\r\nBerry species.\r\n-- Description --\r\nBerry plantations which are traditionally cropped both in temperate and subtropical climates for producing berries.\r\nNOTE. Initial value:2.04.01.02"@en ;
        skos:inScheme    cap-iacs-basecode:FarmStructureSurveyNumberValue .

<http://lpis.ec.europa.eu/registry/applicationschema/cap-iacs-base/code#CropItemCodeValue/otherRootAndTuberVegetablesNec>
        a                cap-iacs-base:CropItemCodeValue ;
        rdfs:label       "Other root and tuber vegetables n.e.c."@en ;
        skos:definition  "-- Definition --\r\n|||Other root and tuber vegetables n.e.c.\r\n-- Description --\r\nCereals and main crops - C\r\nNOTE. Initial value:C1884"@en ;
        skos:inScheme    cap-iacs-basecode:CropItemCodeValue .

<http://lpis.ec.europa.eu/registry/applicationschema/cap-iacs-base/code#SpecieCodeValue/alliumFistulosumLJapaneseBunchingOnionWelshOnion>
        a                cap-iacs-base:SpecieCodeValue ;
        rdfs:label       "Allium fistulosum L. Japanese bunching onion / Welsh onion"@en ;
        skos:definition  "-- Definition --\r\nAllium fistulosum L. Japanese bunching onion / Welsh onion.\r\n-- Description --\r\nList of vegetable specie -H\r\nNOTE. Initial value: H - 2."@en ;
        skos:inScheme    cap-iacs-basecode:SpecieCodeValue .

<http://lpis.ec.europa.eu/registry/applicationschema/cap-iacs-base/code#CropItemCodeValue/mixedGrainOtherThanMaslinC1185>
        a                cap-iacs-base:CropItemCodeValue ;
        rdfs:label       "Mixed grain other than maslin C1185"@en ;
        skos:definition  "-- Definition --\r\n||||Mixed grain other than maslin C1185.\r\n-- Description --\r\nCereals and main crops - C\r\nNOTE. Initial value:C1185"@en ;
        skos:inScheme    cap-iacs-basecode:CropItemCodeValue .

<http://lpis.ec.europa.eu/registry/applicationschema/cap-iacs-base/code#ConformanceClassValue/classB>
        a                cap-iacs-base:ConformanceClassValue ;
        rdfs:label       "Class B"@en ;
        skos:definition  "--Name--\r\nClass B\r\n\r\n--Definition--\r\nSpecified conformance class.\r\n\r\n--Description--\r\nSeparate ATS must be provided if a class is defined within ConformanceClause"@en ;
        skos:inScheme    cap-iacs-basecode:ConformanceClassValue .

<http://lpis.ec.europa.eu/registry/applicationschema/cap-iacs-base/code#CropItemCodeValue/lettucesUnderGlassOrHighAccessibleCoverC1681>
        a                cap-iacs-base:CropItemCodeValue ;
        rdfs:label       "Lettuces under glass or high accessible cover C1681 "@en ;
        skos:definition  "-- Definition --\r\n||||Lettuces under glass or high accessible cover C1681.\r\n-- Description --\r\nCereals and main crops - C\r\nNOTE. Initial value:C1681"@en ;
        skos:inScheme    cap-iacs-basecode:CropItemCodeValue .

<http://lpis.ec.europa.eu/registry/applicationschema/cap-iacs-base/code#SpecieCodeValue/festucaTrachyphyllaHackKrajinaHardFescue>
        a                cap-iacs-base:SpecieCodeValue ;
        rdfs:label       "Festuca trachyphylla (Hack.) Krajina Hard fescue "@en ;
        skos:definition  "-- Definition --\r\nFestuca trachyphylla (Hack.) Krajina Hard fescue.\r\n-- Description --\r\nList of agricultural species -A\r\nII. Fodder plants\r\nNOTE. Initial value: A - 18."@en ;
        skos:inScheme    cap-iacs-basecode:SpecieCodeValue .

<http://lpis.ec.europa.eu/registry/applicationschema/cap-iacs-base/code#SpecieCodeValue/petroselinumCrispumMillNymanExAWHillParsley>
        a                cap-iacs-base:SpecieCodeValue ;
        rdfs:label       "Petroselinum crispum (Mill.) Nyman ex A. W. Hill Parsley"@en ;
        skos:definition  "-- Definition --\r\nPetroselinum crispum (Mill.) Nyman ex A. W. Hill Parsley.\r\n-- Description --\r\nList of vegetable specie -H\r\nNOTE. Initial value: H - 25."@en ;
        skos:inScheme    cap-iacs-basecode:SpecieCodeValue .

<http://lpis.ec.europa.eu/registry/applicationschema/cap-iacs-base/code#CropItemCodeValue/hemp>
        a                cap-iacs-base:CropItemCodeValue ;
        rdfs:label       "Hemp"@en ;
        skos:definition  "-- Definition --\r\n|||Hemp.\r\n-- Description --\r\nCereals and main crops - C\r\nNOTE. Initial value:C1530"@en ;
        skos:inScheme    cap-iacs-basecode:CropItemCodeValue .

cap-iacs-basecode:ConformanceLevelValue
        a                skos:ConceptScheme ;
        rdfs:label       "List of conformance level values"@en ;
        dct:isFormatOf   cap-iacs-base:ConformanceLevelValue ;
        skos:definition  "--Name--\r\nConformance level value\r\n\r\n-- Definition --\r\nList of conformance level values.\r\n\r\n-- Description --\r\nList of conformance level values. Any product claiming conformance with one of these levels shall pass all requirements described in the corresponding abstract test suite.\r\n\r\nNOTE. Requirements of a higher level contain all requirements of a lower level."@en .

<http://lpis.ec.europa.eu/registry/applicationschema/cap-iacs-base/code#CropItemCodeValue/winterDurumWheat>
        a                cap-iacs-base:CropItemCodeValue ;
        rdfs:label       "Winter durum wheat"@en ;
        skos:definition  "-- Definition --\r\n|||||Winter durum wheat.\r\n-- Description --\r\nCereals and main crops - C\r\nNOTE. Initial value:C1133"@en ;
        skos:inScheme    cap-iacs-basecode:CropItemCodeValue .

<http://lpis.ec.europa.eu/registry/applicationschema/cap-iacs-base/code#FarmStructureSurveyNumberValue/otherPlantsHarvestedGreenNotMentionedElsewhere>
        a                cap-iacs-base:FarmStructureSurveyNumberValue ;
        rdfs:label       "Other plants harvested green not mentioned elsewhere"@en ;
        skos:definition  "-- Definition --\r\nOther plants harvested green not mentioned elsewhere.\r\n-- Description --\r\nOther arable crops intended mainly for animal fodder, harvested green, not mentioned elsewhere.\r\nNOTE. Initial value:2.01.09.02.99"@en ;
        skos:inScheme    cap-iacs-basecode:FarmStructureSurveyNumberValue .

<http://lpis.ec.europa.eu/registry/applicationschema/cap-iacs-base/code#FarmStructureSurveyNumberValue/cerealsForTheProductionOfGrainIncludingSeed>
        a                cap-iacs-base:FarmStructureSurveyNumberValue ;
        rdfs:label       "Cereals for the production of grain (including seed)"@en ;
        skos:definition  "-- Definition --\r\nCereals for the production of grain (including seed).\r\n-- Description --\r\nAll areas of cereals harvested dry for grain, regardless of use, shall be recorded here (including cereals used for renewable energy production).\r\nNOTE. Initial value:2.01.01"@en ;
        skos:inScheme    cap-iacs-basecode:FarmStructureSurveyNumberValue .

<http://lpis.ec.europa.eu/registry/applicationschema/cap-iacs-base/code#CropItemCodeValue/nurseries>
        a                cap-iacs-base:CropItemCodeValue ;
        rdfs:label       "Nurseries"@en ;
        skos:definition  "-- Definition --\r\n|||Nurseries.\r\n-- Description --\r\nLand use of Agriculture Area in Use -L\r\nNOTE. Initial value:L2810"@en ;
        skos:inScheme    cap-iacs-basecode:CropItemCodeValue .

<http://lpis.ec.europa.eu/registry/applicationschema/cap-iacs-base/code#CropItemCodeValue/cerealsExcludingRice>
        a                cap-iacs-base:CropItemCodeValue ;
        rdfs:label       "Cereals (excluding rice) "@en ;
        skos:definition  "-- Definition --\r\n||Cereals (excluding rice) .\r\n-- Description --\r\nCereals and main crops - C\r\nNOTE. Initial value: C1050"@en ;
        skos:inScheme    cap-iacs-basecode:CropItemCodeValue .

<http://lpis.ec.europa.eu/registry/applicationschema/cap-iacs-base/code#SpecieCodeValue/alliumCepaLAggregatumGroupShallot>
        a                cap-iacs-base:SpecieCodeValue ;
        rdfs:label       "Allium cepa L. Aggregatum group - Shallot"@en ;
        skos:definition  "-- Definition --\r\nAllium cepa L. Aggregatum group - Shallot.\r\n-- Description --\r\nList of vegetable specie -H\r\nNOTE. Initial value: H - 1.1"@en ;
        skos:inScheme    cap-iacs-basecode:SpecieCodeValue .

<http://lpis.ec.europa.eu/registry/applicationschema/cap-iacs-base/code#FarmStructureSurveyNumberValue/irrigatedArea>
        a                cap-iacs-base:FarmStructureSurveyNumberValue ;
        rdfs:label       "Irrigated area"@en ;
        skos:definition  "-- Definition --\r\nIrrigated area.\r\n-- Description --\r\nIrrigated area.\r\nNOTE. Initial value:2.06.02"@en ;
        skos:inScheme    cap-iacs-basecode:FarmStructureSurveyNumberValue .

<http://lpis.ec.europa.eu/registry/applicationschema/cap-iacs-base/code#CauseOfAnomalyValue/notConfirmed>
        a                cap-iacs-base:CauseOfAnomalyValue ;
        rdfs:label       "Cause flagged as no change in the data"@en ;
        skos:definition  "--Name--\r\nNot confirmed\r\n\r\n-- Description--\r\nThe preliminary classification of the anomaly cause cannot be confirmed."@en ;
        skos:inScheme    cap-iacs-basecode:CauseOfAnomalyValue .

<http://lpis.ec.europa.eu/registry/applicationschema/cap-iacs-base/code#SpecieCodeValue/hedysarumCoronariumLSulla>
        a                cap-iacs-base:SpecieCodeValue ;
        rdfs:label       "Hedysarum coronarium L. Sulla "@en ;
        skos:definition  "-- Definition --\r\nHedysarum coronarium L. Sulla\r\n-- Description --\r\nList of agricultural species -A\r\nII. Fodder plants\r\nNOTE. Initial value: A - 33."@en ;
        skos:inScheme    cap-iacs-basecode:SpecieCodeValue .

<http://lpis.ec.europa.eu/registry/applicationschema/cap-iacs-base/code#SpecieCodeValue/poaTrivialisLRoughStalkedMeadowgrass>
        a                cap-iacs-base:SpecieCodeValue ;
        rdfs:label       "Poa trivialis L. Rough-stalked meadowgrass"@en ;
        skos:definition  "-- Definition --\r\nPoa trivialis L. Rough-stalked meadowgrass.\r\n-- Description --\r\nList of agricultural species -A\r\nII. Fodder plants\r\nNOTE. Initial value: A - 30."@en ;
        skos:inScheme    cap-iacs-basecode:SpecieCodeValue .

<http://lpis.ec.europa.eu/registry/applicationschema/cap-iacs-base/code#SpecieCodeValue/brassicaRapaLVarSilvestrisLamBriggsTurnipRape>
        a                cap-iacs-base:SpecieCodeValue ;
        rdfs:label       "Brassica rapa L. var. silvestris (Lam.) Briggs Turnip rape "@en ;
        skos:definition  "-- Definition --\r\nBrassica rapa L. var. silvestris (Lam.) Briggs Turnip rape.\r\n-- Description --\r\nList of agricultural species -A\r\nIII. Oil and fibre plants\r\nNOTE. Initial value: A - 59."@en ;
        skos:inScheme    cap-iacs-basecode:SpecieCodeValue .

<http://lpis.ec.europa.eu/registry/applicationschema/cap-iacs-base/code#CropItemCodeValue/vegetablesFromKitchenGardensC2992>
        a                cap-iacs-base:CropItemCodeValue ;
        rdfs:label       "Vegetables from kitchen gardens C2992"@en ;
        skos:definition  "-- Definition --\r\nVegetables from kitchen gardens C2992.\r\n-- Description --\r\nCereals and main crops - C\r\nNOTE. Initial value:C2992"@en ;
        skos:inScheme    cap-iacs-basecode:CropItemCodeValue .

<http://lpis.ec.europa.eu/registry/applicationschema/cap-iacs-base/code#SpecieCodeValue/phaseolusCoccineusLRunnerBean>
        a                cap-iacs-base:SpecieCodeValue ;
        rdfs:label       "Phaseolus coccineus L. Runner bean"@en ;
        skos:definition  "-- Definition --\r\nPhaseolus coccineus L. Runner bean.\r\n-- Description --\r\nList of vegetable specie -H\r\nNOTE. Initial value: H - 26."@en ;
        skos:inScheme    cap-iacs-basecode:SpecieCodeValue .

<http://lpis.ec.europa.eu/registry/applicationschema/cap-iacs-base/code#CropItemCodeValue/garlic>
        a                cap-iacs-base:CropItemCodeValue ;
        rdfs:label       "Garlic"@en ;
        skos:definition  "-- Definition --\r\n|||Garlic.\r\n-- Description --\r\nCereals and main crops - C\r\nNOTE. Initial value:C1840"@en ;
        skos:inScheme    cap-iacs-basecode:CropItemCodeValue .

<http://lpis.ec.europa.eu/registry/applicationschema/cap-iacs-base/code#CropItemCodeValue/turnips>
        a                cap-iacs-base:CropItemCodeValue ;
        rdfs:label       "Turnips"@en ;
        skos:definition  "-- Definition --\r\n|||Turnips.\r\n-- Description --\r\nCereals and main crops - C\r\nNOTE. Initial value:C1820"@en ;
        skos:inScheme    cap-iacs-basecode:CropItemCodeValue .

<http://lpis.ec.europa.eu/registry/applicationschema/cap-iacs-base/code#SpecieCodeValue/linumUsitatissimumLFlaxLinseed>
        a                cap-iacs-base:SpecieCodeValue ;
        rdfs:label       "Linum usitatissimum L. Flax, Linseed "@en ;
        skos:definition  "-- Definition --\r\nLinum usitatissimum L. Flax, Linseed.\r\n-- Description --\r\nList of agricultural species -A\r\nIII. Oil and fibre plants\r\nNOTE. Initial value: A - 68."@en ;
        skos:inScheme    cap-iacs-basecode:SpecieCodeValue .

<http://lpis.ec.europa.eu/registry/applicationschema/cap-iacs-base/code#FarmStructureSurveyNumberValue/qualityWine>
        a                cap-iacs-base:FarmStructureSurveyNumberValue ;
        rdfs:label       "Quality wine"@en ;
        skos:definition  "-- Definition --\r\nQuality wine.\r\n-- Description --\r\nGrape varieties normally grown for the production of wines with a protected designation of origin (PDO) which comply with the requirements (i) of Council Regulation (EC) No 479/2008(1)\r\nOJ L 148, 6.6.2008, p. 1. (1) or, where applicable, the most recent legislation; and (ii) the corresponding national rules.\r\nGrape varieties normally grown for the production of wines with a protected geographical indication (PGI) which comply with the requirements (i) of Regulation (EC) No 479/2008 or, where applicable, the most recent legislation; and (ii) the corresponding national rules.\r\nNOTE. Initial value:2.04.04.01"@en ;
        skos:inScheme    cap-iacs-basecode:FarmStructureSurveyNumberValue .

<http://lpis.ec.europa.eu/registry/applicationschema/cap-iacs-base/code#SpecieCodeValue/poaNemoralisLWoodMeadowgrass>
        a                cap-iacs-base:SpecieCodeValue ;
        rdfs:label       "Poa nemoralis L.Wood meadowgrass"@en ;
        skos:definition  "-- Definition --\r\nPoa nemoralis L.Wood meadowgrass\r\n-- Description --\r\nList of agricultural species -A\r\nII. Fodder plants\r\nNOTE. Initial value: A - 27."@en ;
        skos:inScheme    cap-iacs-basecode:SpecieCodeValue .

<http://lpis.ec.europa.eu/registry/applicationschema/cap-iacs-base/code#CropItemCodeValue/arableLand>
        a                cap-iacs-base:CropItemCodeValue ;
        rdfs:label       "Arable land"@en ;
        skos:definition  "-- Definition --\r\n||Arable land.\r\n-- Description --\r\nLand use of Agriculture Area in Use -L\r\nNOTE. Initial value:L0001"@en ;
        skos:inScheme    cap-iacs-basecode:CropItemCodeValue .

<http://lpis.ec.europa.eu/registry/applicationschema/cap-iacs-base/code#FarmStructureSurveyNumberValue/ofWhichShortRotationCoppices>
        a                cap-iacs-base:FarmStructureSurveyNumberValue ;
        rdfs:label       "of which short rotation coppices"@en ;
        skos:definition  "-- Definition --\r\nof which short rotation coppices.\r\n-- Description --\r\nWooded areas managed for growing wooded plants, where the rotation period is 20 years or less.\r\nThe rotation period is the time between the first sowing/planting of the trees and the harvest of the final product, where harvesting does not include normal management actions like thinning.\r\nNOTE. Initial value:2.05.02.01"@en ;
        skos:inScheme    cap-iacs-basecode:FarmStructureSurveyNumberValue .

<http://lpis.ec.europa.eu/registry/applicationschema/cap-iacs-base/code#SpecieCodeValue/solanumTorvumSw>
        a                cap-iacs-base:SpecieCodeValue ;
        rdfs:label       "Solanum torvum Sw."@en ;
        skos:definition  "-- Definition --\r\nSolanum torvum Sw.\r\n-- Description --\r\nList of vegetable specie -H\r\nNOTE. Initial value: H - 37.8"@en ;
        skos:inScheme    cap-iacs-basecode:SpecieCodeValue .

<http://lpis.ec.europa.eu/registry/applicationschema/cap-iacs-base/code#CropItemCodeValue/pearsForFreshConsumption>
        a                cap-iacs-base:CropItemCodeValue ;
        rdfs:label       "Pears for fresh consumption"@en ;
        skos:definition  "-- Definition --\r\n|||Pears for fresh consumption.\r\n-- Description --\r\nCereals and main crops - C\r\nNOTE. Initial value:C2130"@en ;
        skos:inScheme    cap-iacs-basecode:CropItemCodeValue .

<http://lpis.ec.europa.eu/registry/applicationschema/cap-iacs-base/code#FarmStructureSurveyNumberValue/rice>
        a                cap-iacs-base:FarmStructureSurveyNumberValue ;
        rdfs:label       "Rice"@en ;
        skos:definition  "-- Definition --\r\nRice.\r\n-- Description --\r\nOryza sativa L.\r\nNOTE. Initial value:2.01.01.07"@en ;
        skos:inScheme    cap-iacs-basecode:FarmStructureSurveyNumberValue .

<http://lpis.ec.europa.eu/registry/applicationschema/cap-iacs-base/code#SpecieCodeValue/lycopersiconEsculentumMillTomato>
        a                cap-iacs-base:SpecieCodeValue ;
        rdfs:label       "Lycopersicon esculentum Mill. Tomato"@en ;
        skos:definition  "-- Definition --\r\nLycopersicon esculentum Mill. Tomato.\r\n-- Description --\r\nList of vegetable specie -H\r\nNOTE. Initial value: H - 24."@en ;
        skos:inScheme    cap-iacs-basecode:SpecieCodeValue .

<http://lpis.ec.europa.eu/registry/applicationschema/cap-iacs-base/code#CropItemCodeValue/otherNutsNec>
        a                cap-iacs-base:CropItemCodeValue ;
        rdfs:label       "Other nuts n.e.c."@en ;
        skos:definition  "-- Definition --\r\n|||Other nuts n.e.c.\r\n-- Description --\r\nCereals and main crops - C\r\nNOTE. Initial value:C2240"@en ;
        skos:inScheme    cap-iacs-basecode:CropItemCodeValue .

<http://lpis.ec.europa.eu/registry/applicationschema/cap-iacs-base/code#CropItemCodeValue/vineyardsC2410>
        a                cap-iacs-base:CropItemCodeValue ;
        rdfs:label       "Vineyards C2410"@en ;
        skos:definition  "-- Definition --\r\n||Vineyards C2410.\r\n-- Description --\r\nCereals and main crops - C\r\nNOTE. Initial value:C2410"@en ;
        skos:inScheme    cap-iacs-basecode:CropItemCodeValue .

cap-iacs-basecode:NotificationGroupValue
        a                skos:ConceptScheme ;
        rdfs:label       "List of notification groups."@en ;
        dct:isFormatOf   cap-iacs-base:NotificationGroupValue ;
        skos:definition  "-- Definition --\r\nList of notification groups.\r\n-- Description --\r\nList of notification groups prescribed in legal documents.\r\nNOTE. Not finite number of notification groups. List may be extended by MS."@en .

<http://lpis.ec.europa.eu/registry/applicationschema/cap-iacs-base/code#SpecieCodeValue/agrostisStoloniferaLCreepingBent>
        a                cap-iacs-base:SpecieCodeValue ;
        rdfs:label       "Agrostis stolonifera L. Creeping bent"@en ;
        skos:definition  "-- Definition --\r\nAgrostis stolonifera L. Creeping bent.\r\n-- Description --\r\nList of agricultural species -A\r\nII. Fodder plants\r\nNOTE. Initial value: A - 5."@en ;
        skos:inScheme    cap-iacs-basecode:SpecieCodeValue .

<http://lpis.ec.europa.eu/registry/applicationschema/cap-iacs-base/code#SpecieCodeValue/galegaOrientalisLFodderGalega>
        a                cap-iacs-base:SpecieCodeValue ;
        rdfs:label       "Galega orientalis L. Fodder galega"@en ;
        skos:definition  "-- Definition --\r\nGalega orientalis L. Fodder galega\r\n-- Description --\r\nList of agricultural species -A\r\nII. Fodder plants\r\nNOTE. Initial value: A - 32."@en ;
        skos:inScheme    cap-iacs-basecode:SpecieCodeValue .

<http://lpis.ec.europa.eu/registry/applicationschema/cap-iacs-base/code#SpecieCodeValue/bromusCatharticusLRescueGrass>
        a                cap-iacs-base:SpecieCodeValue ;
        rdfs:label       "Bromus catharticus L. Rescue grass"@en ;
        skos:definition  "-- Definition --\r\nBromus catharticus L. Rescue grass.\r\n-- Description --\r\nList of agricultural species -A\r\nII. Fodder plants\r\nNOTE. Initial value: A - 9."@en ;
        skos:inScheme    cap-iacs-basecode:SpecieCodeValue .

<http://lpis.ec.europa.eu/registry/applicationschema/cap-iacs-base/code#CropItemCodeValue/otherLeguminousPlantsNec>
        a                cap-iacs-base:CropItemCodeValue ;
        rdfs:label       "Other leguminous plants n.e.c."@en ;
        skos:definition  "-- Definition --\r\n|||Other leguminous plants n.e.c.\r\n-- Description --\r\nCereals and main crops - C\r\nNOTE. Initial value:C2673"@en ;
        skos:inScheme    cap-iacs-basecode:CropItemCodeValue .

<http://lpis.ec.europa.eu/registry/applicationschema/cap-iacs-base/code#CrossComplianceRuleValue/environmentClimateChangeGoodAgriculturalConditionOfLandLandscapeMinimumLevelOfMaintenanceGaec7>
        a                cap-iacs-base:CrossComplianceRuleValue ;
        rdfs:label       "Environment, climate change, good agricultural condition of land  - Landscape, minimum level of maintenance GAEC7"@en ;
        skos:definition  "-- Definition --\r\nEnvironment, climate change, good agricultural condition of land  - Landscape, minimum level of maintenance GAEC7.\r\n-- Description --\r\nRetention of landscape features, including where appropriate, hedges, ponds, ditches, trees in line, in group or isolated, field margins and terraces, and including a ban on cutting hedges and trees during the bird breeding and rearing season and, as an option, measures for avoiding invasive plant species. \r\nNOTE. Initial value:GAEC7."@en ;
        skos:inScheme    cap-iacs-basecode:CrossComplianceRuleValue .

<http://lpis.ec.europa.eu/registry/applicationschema/cap-iacs-base/code#SpecieCodeValue/valerianellaLocustaLLaterrCornSaladLambsLettuce>
        a                cap-iacs-base:SpecieCodeValue ;
        rdfs:label       "Valerianella locusta (L.) Laterr. Corn salad / Lamb's lettuce"@en ;
        skos:definition  "-- Definition --\r\nValerianella locusta (L.) Laterr. Corn salad / Lamb's lettuce.\r\n-- Description --\r\nList of vegetable specie -H\r\nNOTE. Initial value: H - 34."@en ;
        skos:inScheme    cap-iacs-basecode:SpecieCodeValue .

<http://lpis.ec.europa.eu/registry/applicationschema/cap-iacs-base/code#SpecieCodeValue/medicagoLupulinaLTrefoil>
        a                cap-iacs-base:SpecieCodeValue ;
        rdfs:label       "Medicago lupulina L. Trefoil"@en ;
        skos:definition  "-- Definition --\r\nMedicago lupulina L. Trefoil.\r\n-- Description --\r\nList of agricultural species -A\r\nII. Fodder plants\r\nNOTE. Initial value: A - 38."@en ;
        skos:inScheme    cap-iacs-basecode:SpecieCodeValue .

<http://lpis.ec.europa.eu/registry/applicationschema/cap-iacs-base/code#CropItemCodeValue/vineyardsForWinesWithProtectedDesignationOfOriginPDO>
        a                cap-iacs-base:CropItemCodeValue ;
        rdfs:label       "Vineyards for wines with protected designation of origin (PDO)"@en ;
        skos:definition  "-- Definition --\r\n||||Vineyards for wines with protected designation of origin (PDO).\r\n-- Description --\r\nCereals and main crops - C\r\nNOTE. Initial value:C2441"@en ;
        skos:inScheme    cap-iacs-basecode:CropItemCodeValue .

<http://lpis.ec.europa.eu/registry/applicationschema/cap-iacs-base/code#CropItemCodeValue/chicoryC1710>
        a                cap-iacs-base:CropItemCodeValue ;
        rdfs:label       "Chicory C1710"@en ;
        skos:definition  "-- Definition --\r\n|||Chicory C1710.\r\n-- Description --\r\nCereals and main crops - C\r\nNOTE. Initial value:C1710"@en ;
        skos:inScheme    cap-iacs-basecode:CropItemCodeValue .

<http://lpis.ec.europa.eu/registry/applicationschema/cap-iacs-base/code#MonthValue/september>
        a                cap-iacs-base:MonthValue ;
        rdfs:label       "September"@en ;
        skos:definition  "-- Definition --\r\nSeptember.\r\n-- Description --\r\nItem description."@en ;
        skos:inScheme    cap-iacs-basecode:MonthValue .

<http://lpis.ec.europa.eu/registry/applicationschema/cap-iacs-base/code#CropItemCodeValue/vineyardsForOtherGrapeProductionNec>
        a                cap-iacs-base:CropItemCodeValue ;
        rdfs:label       "Vineyards for other grape production n.e.c."@en ;
        skos:definition  "-- Definition --\r\n|||Vineyards for other grape production n.e.c.\r\n-- Description --\r\nCereals and main crops - C\r\nNOTE. Initial value:C2445"@en ;
        skos:inScheme    cap-iacs-basecode:CropItemCodeValue .

<http://lpis.ec.europa.eu/registry/applicationschema/cap-iacs-base/code#SupportSchemeTypeValue/basicPaymentScheme>
        a                cap-iacs-base:SupportSchemeTypeValue ;
        rdfs:label       "Basic payment scheme"@en ;
        skos:definition  "Basic payment scheme\r\n\r\nBasic payment scheme - BPS as described in Title III, Chapter 1, Sections 1, 2, 3 and 5 of Regulation (EU) 1307/2013.\r\n\r\nDecoupled payment that is based on entitlements."@en ;
        skos:inScheme    cap-iacs-basecode:SupportSchemeTypeValue .

<http://lpis.ec.europa.eu/registry/applicationschema/cap-iacs-base/code#StatusValue/underCrossCheck>
        a                cap-iacs-base:StatusValue ;
        rdfs:label       "Under construction"@en ;
        skos:definition  "-- Name--\r\nUnder cross-check\r\n\r\n--Definition--\r\nStatus of an object according to the state machine diagram.\r\n\r\n-- Description --\r\nWhenever a transaction in the information system is performed, the system shall be checked for integrity of the schema and the consistency of data. \r\n\r\nNOTE 1. Cross checks are also the tools to find further issues/anomalies. When a new upgrade issue/anomaly is found, the \"open\" value shall be assigned and the full life cycle assessment of the object has to be performed."@en ;
        skos:inScheme    cap-iacs-basecode:StatusValue .

<http://lpis.ec.europa.eu/registry/applicationschema/cap-iacs-base/code#CropItemCodeValue/tomatoesForFreshConsumption>
        a                cap-iacs-base:CropItemCodeValue ;
        rdfs:label       "Tomatoes for fresh consumption"@en ;
        skos:definition  "-- Definition --\r\n||||Tomatoes for fresh consumption.\r\n-- Description --\r\nCereals and main crops - C\r\nNOTE. Initial value:C1751"@en ;
        skos:inScheme    cap-iacs-basecode:CropItemCodeValue .

<http://lpis.ec.europa.eu/registry/applicationschema/cap-iacs-base/code#OrdinalNumberValue/last>
        a                cap-iacs-base:OrdinalNumberValue ;
        rdfs:label       "Last"@en ;
        skos:definition  "-- Definition --\r\nLast.\r\n-- Description --\r\nItem description."@en ;
        skos:inScheme    cap-iacs-basecode:OrdinalNumberValue .

<http://lpis.ec.europa.eu/registry/applicationschema/cap-iacs-base/code#CropItemCodeValue/ryeAndMaslin>
        a                cap-iacs-base:CropItemCodeValue ;
        rdfs:label       "Rye and maslin"@en ;
        skos:definition  "-- Definition --\r\n|||Rye and maslin.\r\n-- Description --\r\nCereals and main crops - C\r\nNOTE. Initial value:C1140"@en ;
        skos:inScheme    cap-iacs-basecode:CropItemCodeValue .

<http://lpis.ec.europa.eu/registry/applicationschema/cap-iacs-base/code#SpecieCodeValue/arachisHypogeaLGroundnutPeanut>
        a                cap-iacs-base:SpecieCodeValue ;
        rdfs:label       "Arachis hypogea L. Groundnut/Peanut"@en ;
        skos:definition  "-- Definition --\r\nArachis hypogea L. Groundnut/Peanut.\r\n-- Description --\r\nList of agricultural species -A\r\nIII. Oil and fibre plants\r\nNOTE. Initial value: A - 58."@en ;
        skos:inScheme    cap-iacs-basecode:SpecieCodeValue .

<http://lpis.ec.europa.eu/registry/applicationschema/cap-iacs-base/code#RecurenceValue/noRecurrence>
        a                cap-iacs-base:RecurenceValue ;
        rdfs:label       "No recurrence"@en ;
        skos:definition  "-- Definition --\r\nNo recurrence.\r\n-- Description --\r\nItem description."@en ;
        skos:inScheme    cap-iacs-basecode:RecurenceValue .

<http://lpis.ec.europa.eu/registry/applicationschema/cap-iacs-base/code#VarietalNameValue/ambition>
        a                cap-iacs-base:VarietalNameValue ;
        rdfs:label       "H - 1.1  Ambition"@en ;
        skos:definition  "-- Definition --\r\nH - 1.1  Ambition\r\n-- Description --\r\nH - 1.1 Allium cepa L. Aggregatum group - Shallot /  Ambition.\r\nNOTE. Initial value: Ambition\r\nNOTE. MS - NL (Netherlands)."@en ;
        skos:inScheme    cap-iacs-basecode:VarietalNameValue .

<http://lpis.ec.europa.eu/registry/applicationschema/cap-iacs-base/code#SpecieCodeValue/scorzoneraHispanicaLScorzoneraBlackSalsify>
        a                cap-iacs-base:SpecieCodeValue ;
        rdfs:label       "Scorzonera hispanica L. Scorzonera / Black salsify"@en ;
        skos:definition  "-- Definition --\r\nScorzonera hispanica L. Scorzonera / Black salsify.\r\n-- Description --\r\nList of vegetable specie -H\r\nNOTE. Initial value: H - 31."@en ;
        skos:inScheme    cap-iacs-basecode:SpecieCodeValue .

<http://lpis.ec.europa.eu/registry/applicationschema/cap-iacs-base/code#SpecieCodeValue/anthriscusCerefoliumLHoffmChervil>
        a                cap-iacs-base:SpecieCodeValue ;
        rdfs:label       "Anthriscus cerefolium (L.) Hoffm. Chervil"@en ;
        skos:definition  "-- Definition --\r\nAnthriscus cerefolium (L.) Hoffm. Chervil.\r\n-- Description --\r\nList of vegetable specie -H\r\nNOTE. Initial value: H - 6."@en ;
        skos:inScheme    cap-iacs-basecode:SpecieCodeValue .

<http://lpis.ec.europa.eu/registry/applicationschema/cap-iacs-base/code#CropItemCodeValue/driedPulsesAndProteinCropsForTheProductionOfGrainIncludingSeedAndMixturesOfCerealsAndPulsesC1300>
        a                cap-iacs-base:CropItemCodeValue ;
        rdfs:label       "Dried pulses and protein crops for the production of grain (including seed and mixtures of cereals and pulses) C1300"@en ;
        skos:definition  "-- Definition --\r\n|Dried pulses and protein crops for the production of grain (including seed and mixtures of cereals and pulses) C1300.\r\n-- Description --\r\nCereals and main crops - C\r\nNOTE. Initial value:C1300"@en ;
        skos:inScheme    cap-iacs-basecode:CropItemCodeValue .

<http://lpis.ec.europa.eu/registry/applicationschema/cap-iacs-base/code#SpecieCodeValue/alopecurusPratensisLMeadowFoxtail>
        a                cap-iacs-base:SpecieCodeValue ;
        rdfs:label       "Alopecurus pratensis L. Meadow foxtail "@en ;
        skos:definition  "-- Definition --\r\nAlopecurus pratensis L. Meadow foxtail.\r\n-- Description --\r\nList of agricultural species -A\r\nII. Fodder plants\r\nNOTE. Initial value: A - 7."@en ;
        skos:inScheme    cap-iacs-basecode:SpecieCodeValue .

cap-iacs-basecode:StatusValue
        a                skos:ConceptScheme ;
        rdfs:label       "List of status values"@en ;
        dct:isFormatOf   cap-iacs-base:StatusValue ;
        skos:definition  "-- Name--\r\nStatus value\r\n\r\n--Definition --\r\nCode list of possible status values.\r\n\r\n-- Description --\r\nList of status types based on state machine diagrams (Dynamic CAP model) for new and existing object features or schema. The values included in this code list are applicable both to introduction of a new object/feature or to processing a change request.\r\n\r\nNOTE. These are generic values applicable in IACS. These concepts have been reused in LPIS upgrade and LPIS update processes."@en .

<http://lpis.ec.europa.eu/registry/applicationschema/cap-iacs-base/code#TestTypeValue/basic>
        a                cap-iacs-base:TestTypeValue ;
        rdfs:label       "Basic test"@en ;
        skos:definition  "--Name--\r\nBasic\r\n\r\n-- Definition --\r\nBasic test .\r\n\r\n-- Description --\r\nBasic tests (BT) provide limited testing of IUT in order to establish whether or not it is appropriate to perform more thorough testing. They may be used to determine the degree of conformance prior to deciding whether or not to proceed with thorough capability testing. Basic tests are simple capability tests. Conformance clauses should identify those test cases that may be used as a basic test.\r\n\r\nNOTE1. BT shall be used to for detecting obvious cases of non-conformity.\r\n\r\nNOTE2. BT shall be used as a preliminary step in order to decide whether or not to run capability tests."@en ;
        skos:inScheme    cap-iacs-basecode:TestTypeValue .

<http://lpis.ec.europa.eu/registry/applicationschema/cap-iacs-base/code#FarmStructureSurveyNumberValue/fodderRootsAndBrassicasExcludingSeed>
        a                cap-iacs-base:FarmStructureSurveyNumberValue ;
        rdfs:label       "Fodder roots and brassicas (excluding seed)"@en ;
        skos:definition  "-- Definition --\r\nFodder roots and brassicas (excluding seed)\r\n-- Description --\r\nFodder beet (Beta vulgaris L.) and plants of the Brassicae family harvested mainly for animal feed, regardless whether it is the root or the stem, and other plants cultivated mainly for their roots for fodder, not mentioned elsewhere.\r\nNOTE. Initial value:2.01.05"@en ;
        skos:inScheme    cap-iacs-basecode:FarmStructureSurveyNumberValue .

<http://lpis.ec.europa.eu/registry/applicationschema/cap-iacs-base/code#SpecieCodeValue/pisumSativumLPartimSugarPea>
        a                cap-iacs-base:SpecieCodeValue ;
        rdfs:label       "Pisum sativum L. (partim) Sugar pea"@en ;
        skos:definition  "-- Definition --\r\nPisum sativum L. (partim) Sugar pea.\r\n-- Description --\r\nList of vegetable specie -H\r\nNOTE. Initial value:H - 28.3"@en ;
        skos:inScheme    cap-iacs-basecode:SpecieCodeValue .

<http://lpis.ec.europa.eu/registry/applicationschema/cap-iacs-base/code#CropItemCodeValue/otherApplesForFreshConsumption>
        a                cap-iacs-base:CropItemCodeValue ;
        rdfs:label       "Other apples for fresh consumption"@en ;
        skos:definition  "-- Definition --\r\n||||Other apples for fresh consumption.\r\n-- Description --\r\nCereals and main crops - C\r\nNOTE. Initial value:C2113"@en ;
        skos:inScheme    cap-iacs-basecode:CropItemCodeValue .

<http://lpis.ec.europa.eu/registry/applicationschema/cap-iacs-base/code#CropItemCodeValue/melons>
        a                cap-iacs-base:CropItemCodeValue ;
        rdfs:label       "Melons"@en ;
        skos:definition  "-- Definition --\r\n||Melons.\r\n-- Description --\r\nCereals and main crops - C\r\nNOTE. Initial value:C1771"@en ;
        skos:inScheme    cap-iacs-basecode:CropItemCodeValue .

<http://lpis.ec.europa.eu/registry/applicationschema/cap-iacs-base/code#FarmStructureSurveyNumberValue/kitchenGardens>
        a                cap-iacs-base:FarmStructureSurveyNumberValue ;
        rdfs:label       "Kitchen gardens"@en ;
        skos:definition  "-- Definition --\r\nKitchen gardens.\r\n-- Description --\r\nAreas devoted to the cultivation of agricultural products intended for self-consumption by the holder and his household, normally separated off from the rest of the agricultural land, and recognisable as kitchen gardens.\r\nOnly occasional surplus products coming from this area are sold off from the holding. All areas from which products are consistently sold on the market belong under other items, even if part of the production is consumed by the holder and his household.\r\nNOTE. Initial value:2.02"@en ;
        skos:inScheme    cap-iacs-basecode:FarmStructureSurveyNumberValue .

<http://lpis.ec.europa.eu/registry/applicationschema/cap-iacs-base/code#SpecieCodeValue/betaVulgarisLBeetrootIncludingCheltenhamBeet>
        a                cap-iacs-base:SpecieCodeValue ;
        rdfs:label       "Beta vulgaris L. Beetroot, including Cheltenham beet"@en ;
        skos:definition  "-- Definition --\r\nBeta vulgaris L. Beetroot, including Cheltenham beet.\r\n-- Description --\r\nList of vegetable specie -H\r\nNOTE. Initial value: H - 9.1"@en ;
        skos:inScheme    cap-iacs-basecode:SpecieCodeValue .

<http://lpis.ec.europa.eu/registry/applicationschema/cap-iacs-base/code#CropItemCodeValue/driedPulsesAndProteinCropsForTheProductionOfGrainIncludingSeedAndMixturesOfCerealsAndPulses>
        a                cap-iacs-base:CropItemCodeValue ;
        rdfs:label       "Dried pulses and protein crops for the production of grain (including seed and mixtures of cereals and pulses)"@en ;
        skos:definition  "-- Definition --\r\n|||Dried pulses and protein crops for the production of grain (including seed and mixtures of cereals and pulses).\r\n-- Description --\r\nLand use of Agriculture Area in Use -L\r\nNOTE. Initial value:L1300"@en ;
        skos:inScheme    cap-iacs-basecode:CropItemCodeValue .

<http://lpis.ec.europa.eu/registry/applicationschema/cap-iacs-base/code#SpecieCodeValue/trisetumFlavescensLGoldenOatgrass>
        a                cap-iacs-base:SpecieCodeValue ;
        rdfs:label       "Trisetum flavescens L. Golden oatgrass"@en ;
        skos:definition  "-- Definition --\r\nTrisetum flavescens L. Golden oatgrass\r\n-- Description --\r\nList of agricultural species -A\r\nII. Fodder plants\r\nNOTE. Initial value: A - 31."@en ;
        skos:inScheme    cap-iacs-basecode:SpecieCodeValue .

<http://lpis.ec.europa.eu/registry/applicationschema/cap-iacs-base/code#SpecieCodeValue/bromusSitchensisLAlaskaBromeGrass>
        a                cap-iacs-base:SpecieCodeValue ;
        rdfs:label       "Bromus sitchensis L. Alaska brome-grass"@en ;
        skos:definition  "-- Definition --\r\nBromus sitchensis L. Alaska brome-grass.\r\n-- Description --\r\nList of agricultural species -A\r\nII. Fodder plants\r\nNOTE. Initial value: A - 10."@en ;
        skos:inScheme    cap-iacs-basecode:SpecieCodeValue .

<http://lpis.ec.europa.eu/registry/applicationschema/cap-iacs-base/code#CropItemCodeValue/applesForFreshConsumption>
        a                cap-iacs-base:CropItemCodeValue ;
        rdfs:label       "Apples for fresh consumption"@en ;
        skos:definition  "-- Definition --\r\n|||Apples for fresh consumption.\r\n-- Description --\r\nCereals and main crops - C\r\nNOTE. Initial value:C2110"@en ;
        skos:inScheme    cap-iacs-basecode:CropItemCodeValue .

<http://lpis.ec.europa.eu/registry/applicationschema/cap-iacs-base/code#CropItemCodeValue/otherCitrusFruitsNec>
        a                cap-iacs-base:CropItemCodeValue ;
        rdfs:label       "Other citrus fruits n.e.c."@en ;
        skos:definition  "-- Definition --\r\n|||Other citrus fruits n.e.c.\r\n-- Description --\r\nCereals and main crops - C\r\nNOTE. Initial value:C2390"@en ;
        skos:inScheme    cap-iacs-basecode:CropItemCodeValue .

<http://lpis.ec.europa.eu/registry/applicationschema/cap-iacs-base/code#SpecieCodeValue/phaseolusVulgarisLClimbingFrenchBean>
        a                cap-iacs-base:SpecieCodeValue ;
        rdfs:label       "Phaseolus vulgaris L. Climbing French bean"@en ;
        skos:definition  "-- Definition --\r\nPhaseolus vulgaris L. Climbing French bean.\r\n-- Description --\r\nList of vegetable specie -H\r\nNOTE. Initial value: H - 27.2"@en ;
        skos:inScheme    cap-iacs-basecode:SpecieCodeValue .

<http://lpis.ec.europa.eu/registry/applicationschema/cap-iacs-base/code#CropItemCodeValue/cabbageWhite>
        a                cap-iacs-base:CropItemCodeValue ;
        rdfs:label       "Cabbage (white)"@en ;
        skos:definition  "-- Definition --\r\n|||Cabbage (white).\r\n-- Description --\r\nCereals and main crops - C\r\nNOTE. Initial value:C1635"@en ;
        skos:inScheme    cap-iacs-basecode:CropItemCodeValue .

<http://lpis.ec.europa.eu/registry/applicationschema/cap-iacs-base/code#SpecieCodeValue/lagenariaSicerariaMolStandl>
        a                cap-iacs-base:SpecieCodeValue ;
        rdfs:label       "Lagenaria siceraria (Mol.) Standl."@en ;
        skos:definition  "-- Definition --\r\nLagenaria siceraria (Mol.) Standl.\r\n-- Description --\r\nList of vegetable specie -H\r\nNOTE. Initial value: H - 37.3"@en ;
        skos:inScheme    cap-iacs-basecode:SpecieCodeValue .

<http://lpis.ec.europa.eu/registry/applicationschema/cap-iacs-base/code#FarmStructureSurveyNumberValue/hops>
        a                cap-iacs-base:FarmStructureSurveyNumberValue ;
        rdfs:label       "Hops"@en ;
        skos:definition  "-- Definition --\r\nHops.\r\n-- Description --\r\nHumulus lupulus L.\r\nNOTE. Initial value:2.01.06.02"@en ;
        skos:inScheme    cap-iacs-basecode:FarmStructureSurveyNumberValue .

<http://lpis.ec.europa.eu/registry/applicationschema/cap-iacs-base/code#SpecieCodeValue/cichoriumEndiviaLPlainLeavedEndive>
        a                cap-iacs-base:SpecieCodeValue ;
        rdfs:label       "Cichorium endivia L. Plain-leaved endive"@en ;
        skos:definition  "-- Definition --\r\nCichorium endivia L. Plain-leaved endive.\r\n-- Description --\r\nList of vegetable specie -H\r\nNOTE. Initial value: H - 13.2"@en ;
        skos:inScheme    cap-iacs-basecode:SpecieCodeValue .

<http://lpis.ec.europa.eu/registry/applicationschema/cap-iacs-base/code#FarmStructureSurveyNumberValue/woodedArea>
        a                cap-iacs-base:FarmStructureSurveyNumberValue ;
        rdfs:label       "Wooded area"@en ;
        skos:definition  "-- Definition --\r\nWooded area.\r\n-- Description --\r\nAreas covered with trees or forest shrubs, including poplar plantations inside or outside woods and forest-tree nurseries grown in woodland for the holding’s own requirements, as well as forest facilities (forest roads, storage depots for timber, etc.).\r\nNOTE. Initial value:2.05.02"@en ;
        skos:inScheme    cap-iacs-basecode:FarmStructureSurveyNumberValue .

<http://lpis.ec.europa.eu/registry/applicationschema/cap-iacs-base/code#CropItemCodeValue/tomatoes>
        a                cap-iacs-base:CropItemCodeValue ;
        rdfs:label       "Tomatoes"@en ;
        skos:definition  "-- Definition --\r\n|||Tomatoes.\r\n-- Description --\r\nCereals and main crops - C\r\nNOTE. Initial value:C1750"@en ;
        skos:inScheme    cap-iacs-basecode:CropItemCodeValue .

<http://lpis.ec.europa.eu/registry/applicationschema/cap-iacs-base/code#CropItemCodeValue/cauliflowerAndBroccoli>
        a                cap-iacs-base:CropItemCodeValue ;
        rdfs:label       "Cauliflower and broccoli"@en ;
        skos:definition  "-- Definition --\r\n|||Cauliflower and broccoli.\r\n-- Description --\r\nCereals and main crops - C\r\nNOTE. Initial value:C1620"@en ;
        skos:inScheme    cap-iacs-basecode:CropItemCodeValue .

<http://lpis.ec.europa.eu/registry/applicationschema/cap-iacs-base/code#NotificationGroupValue/notificationsConcerningTheMinimumRequirementsForReceivingDirectPayments>
        a                cap-iacs-base:NotificationGroupValue ;
        rdfs:label       "Notifications concerning the minimum requirements for receiving direct payments"@en ;
        skos:definition  "-- Definition --\r\nNotifications concerning the minimum requirements for receiving direct payments.\r\n-- Description --\r\nNOTE.67"@en ;
        skos:inScheme    cap-iacs-basecode:NotificationGroupValue .

<http://lpis.ec.europa.eu/registry/applicationschema/cap-iacs-base/code#SpecieCodeValue/poaPalustrisLSwampMeadowgras>
        a                cap-iacs-base:SpecieCodeValue ;
        rdfs:label       "Poa palustris L. Swamp meadowgras"@en ;
        skos:definition  "-- Definition --\r\nPoa palustris L. Swamp meadowgras.\r\n-- Description --\r\nList of agricultural species -A\r\nII. Fodder plants\r\nNOTE. Initial value: A - 28."@en ;
        skos:inScheme    cap-iacs-basecode:SpecieCodeValue .

<http://lpis.ec.europa.eu/registry/applicationschema/cap-iacs-base/code#SpecieCodeValue/×TriticosecaleWittmExACamusHybrids>
        a                cap-iacs-base:SpecieCodeValue ;
        rdfs:label       "×Triticosecale Wittm. ex A. Camus Hybrids"@en ;
        skos:definition  "-- Definition --\r\n×Triticosecale Wittm. ex A. Camus Hybrids resulting from the crossing of a species of the genus Triticum and a species of the genus Secale.\r\n-- Description --\r\nList of agricultural species -A   \r\nIV. Cereals\r\nNOTE. Initial value: A - 82."@en ;
        skos:inScheme    cap-iacs-basecode:SpecieCodeValue .

<http://lpis.ec.europa.eu/registry/applicationschema/cap-iacs-base/code#FarmStructureSurveyNumberValue/pastureAndMeadowExcludingRoughGrazings>
        a                cap-iacs-base:FarmStructureSurveyNumberValue ;
        rdfs:label       "Pasture and meadow, excluding rough grazings"@en ;
        skos:definition  "-- Definition --\r\nPasture and meadow, excluding rough grazings.\r\n-- Description --\r\nPermanent pasture on good or medium quality soils. These areas can normally be used for intensive grazing.\r\nNOTE. Initial value:2.03.01"@en ;
        skos:inScheme    cap-iacs-basecode:FarmStructureSurveyNumberValue .

<http://lpis.ec.europa.eu/registry/applicationschema/cap-iacs-base/code#CropItemCodeValue/otherRootCropsNec>
        a                cap-iacs-base:CropItemCodeValue ;
        rdfs:label       "Other root crops n.e.c. "@en ;
        skos:definition  "-- Definition --\r\n||Other root crops n.e.c. \r\n-- Description --\r\nCereals and main crops - C\r\nNOTE. Initial value:C1380"@en ;
        skos:inScheme    cap-iacs-basecode:CropItemCodeValue .

<http://lpis.ec.europa.eu/registry/applicationschema/cap-iacs-base/code#MonthValue/january>
        a                cap-iacs-base:MonthValue ;
        rdfs:label       "January"@en ;
        skos:definition  "-- Definition --\r\nJanuary.\r\n-- Description --\r\nItem description."@en ;
        skos:inScheme    cap-iacs-basecode:MonthValue .

<http://lpis.ec.europa.eu/registry/applicationschema/cap-iacs-base/code#SpecieCodeValue/festucaPratensisHudsMeadowFescue>
        a                cap-iacs-base:SpecieCodeValue ;
        rdfs:label       "Festuca pratensis Huds. Meadow fescue   "@en ;
        skos:definition  "-- Definition --\r\nFestuca pratensis Huds. Meadow fescue.\r\n-- Description --\r\nList of agricultural species -A\r\nII. Fodder plants\r\nNOTE. Initial value: A - 16."@en ;
        skos:inScheme    cap-iacs-basecode:SpecieCodeValue .

<http://lpis.ec.europa.eu/registry/applicationschema/cap-iacs-base/code#CropItemCodeValue/yellowLemons>
        a                cap-iacs-base:CropItemCodeValue ;
        rdfs:label       "Yellow lemons"@en ;
        skos:definition  "-- Definition --\r\n||||Yellow lemons.\r\n-- Description --\r\nCereals and main crops - C\r\nNOTE. Initial value:C2371"@en ;
        skos:inScheme    cap-iacs-basecode:CropItemCodeValue .

<http://lpis.ec.europa.eu/registry/applicationschema/cap-iacs-base/code#FarmStructureSurveyNumberValue/fruitSpeciesOfWhichFruitOfSubtropicalClimateZones>
        a                cap-iacs-base:FarmStructureSurveyNumberValue ;
        rdfs:label       "Fruit species, of which: Fruit of subtropical climate zones"@en ;
        skos:definition  "-- Definition --\r\nFruit species, of which: Fruit of subtropical climate zones.\r\n-- Description --\r\nFruit tree plantations which are traditionally cropped in subtropical climates for producing fruits.\r\nNOTE. Initial value:2.04.01.01.02"@en ;
        skos:inScheme    cap-iacs-basecode:FarmStructureSurveyNumberValue .

<http://lpis.ec.europa.eu/registry/applicationschema/cap-iacs-base/code#StatusOfIssueValue/inProgress>
        a                cap-iacs-base:StatusOfIssueValue ;
        rdfs:label       "In progress"@en ;
        skos:definition  "--Name--\r\nIn progress\r\n\r\n-- Definition --\r\nStatus of the issue as soon as its processing has started or has been flagged for later resolution."@en ;
        skos:inScheme    cap-iacs-basecode:StatusOfIssueValue .

<http://lpis.ec.europa.eu/registry/applicationschema/cap-iacs-base/code#CauseOfAnomalyValue/changeInThePerimeterExchangeOfAgriculturalLand>
        a                cap-iacs-base:CauseOfAnomalyValue ;
        rdfs:label       "Cause flaged as Type IV. Change in the perimeter (exchange of agricultural land)"@en ;
        skos:definition  "--Name--\r\nChange in the perimeter due to exchange of agricultural land\r\n\r\n-- Description --\r\nThe minimum number of involved parcels is two. The anomaly is manifested by a change of their shape and area.\r\n\r\nNOTE. Previously this cause was flagged as Type IV anomaly."@en ;
        skos:inScheme    cap-iacs-basecode:CauseOfAnomalyValue .

<http://lpis.ec.europa.eu/registry/applicationschema/cap-iacs-base/code#SpecieCodeValue/viciaSativaLCommonVetch>
        a                cap-iacs-base:SpecieCodeValue ;
        rdfs:label       "Vicia sativa L. Common vetch "@en ;
        skos:definition  "-- Definition --\r\nVicia sativa L. Common vetch.\r\n-- Description --\r\nList of agricultural species -A\r\nII. Fodder plants\r\nNOTE. Initial value: A - 52."@en ;
        skos:inScheme    cap-iacs-basecode:SpecieCodeValue .

<http://lpis.ec.europa.eu/registry/applicationschema/cap-iacs-base/code#SupportSchemeTypeValue/posei>
        a                cap-iacs-base:SupportSchemeTypeValue ;
        rdfs:label       "Posei"@en ;
        skos:definition  "POSEI\r\n\r\nChapter IV of Regulation (EU) No 228/2013 / Direct payments under measures established in the programmes.\r\n\r\nNOTE\r\nIn full: \"Programme d'Options Spécifiques à l'Éloignement et l'Insularité\"."@en ;
        skos:inScheme    cap-iacs-basecode:SupportSchemeTypeValue .

<http://lpis.ec.europa.eu/registry/applicationschema/cap-iacs-base/code#CropItemCodeValue/lemonsAndAcidLimesC2370>
        a                cap-iacs-base:CropItemCodeValue ;
        rdfs:label       "Lemons and acid limes C2370"@en ;
        skos:definition  "-- Definition --\r\n|||Lemons and acid limes C2370.\r\n-- Description --\r\nCereals and main crops - C\r\nNOTE. Initial value:C2370"@en ;
        skos:inScheme    cap-iacs-basecode:CropItemCodeValue .

<http://lpis.ec.europa.eu/registry/applicationschema/cap-iacs-base/code#FarmStructureSurveyNumberValue/greenMaize>
        a                cap-iacs-base:FarmStructureSurveyNumberValue ;
        rdfs:label       "Green maize"@en ;
        skos:definition  "-- Definition --\r\nGreen maize.\r\n-- Description --\r\nAll forms of maize (Zea mays L.) grown mainly for silage, which is not harvested for grain (whole cob, parts of or whole plant).\r\nThis includes green maize directly consumed by animals (without silage) and whole cobs (grain, rachis, husk) harvested for feedstuff or silage as well as for renewable energy production.\r\nNOTE. Initial value:2.01.09.02.01"@en ;
        skos:inScheme    cap-iacs-basecode:FarmStructureSurveyNumberValue .

<http://lpis.ec.europa.eu/registry/applicationschema/cap-iacs-base/code#StatusValue/open>
        a                cap-iacs-base:StatusValue ;
        rdfs:label       "Registered"@en ;
        skos:definition  "--Name--\r\nOpen\r\n\r\n--Definition--\r\nStatus of an object according to the state machine diagram.\r\n\r\n--Description --\r\nThis status is applicable to UpgradeIssue and Anomaly feature types only. The value is assigned in the moment when an instance of these feature types is introduced in the information system."@en ;
        skos:inScheme    cap-iacs-basecode:StatusValue .

<http://lpis.ec.europa.eu/registry/applicationschema/cap-iacs-base/code#CropItemCodeValue/cottonSeed>
        a                cap-iacs-base:CropItemCodeValue ;
        rdfs:label       "Cotton seed"@en ;
        skos:definition  "-- Definition --\r\n||||Cotton seed.\r\n-- Description --\r\nCereals and main crops - C\r\nNOTE. Initial value:C1490"@en ;
        skos:inScheme    cap-iacs-basecode:CropItemCodeValue .

<http://lpis.ec.europa.eu/registry/applicationschema/cap-iacs-base/code#SupportSchemeTypeValue/paymentForAreasWithNaturalConstraints>
        a                cap-iacs-base:SupportSchemeTypeValue ;
        rdfs:label       "Payment for areas with natural constraints"@en ;
        skos:definition  "Payment for areas with natural constraints\r\n\r\nPayment to farmers who are entitled to BPS/SAPS and whose holdings are fully or partly situated in areas with natural constraints designated by Member States in accordance with Article 32(1) of Regulation (EU) No 1305/2013. \r\n\r\nNOTE\r\nRules in Title III, Chapter 4 of R 1307/2013"@en ;
        skos:inScheme    cap-iacs-basecode:SupportSchemeTypeValue .

<http://lpis.ec.europa.eu/registry/applicationschema/cap-iacs-base/code#SpecieCodeValue/agrostisGiganteaLRedTop>
        a                cap-iacs-base:SpecieCodeValue ;
        rdfs:label       "Agrostis gigantea L. Red top"@en ;
        skos:definition  "-- Definition --\r\nAgrostis gigantea L. Red top.\r\n-- Description --\r\nList of agricultural species -A\r\nII. Fodder plants\r\nNOTE. Initial value: A - 4."@en ;
        skos:inScheme    cap-iacs-basecode:SpecieCodeValue .

<http://lpis.ec.europa.eu/registry/applicationschema/cap-iacs-base/code#CropItemCodeValue/vegetablesCultivatedForFruit>
        a                cap-iacs-base:CropItemCodeValue ;
        rdfs:label       "Vegetables cultivated for fruit"@en ;
        skos:definition  "-- Definition --\r\n||Vegetables cultivated for fruit.\r\n-- Description --\r\nCereals and main crops - C\r\nNOTE. Initial value:C1740"@en ;
        skos:inScheme    cap-iacs-basecode:CropItemCodeValue .

<http://lpis.ec.europa.eu/registry/applicationschema/cap-iacs-base/code#SpecieCodeValue/betaVulgarisLSpinachBeetOrChard>
        a                cap-iacs-base:SpecieCodeValue ;
        rdfs:label       "Beta vulgaris L. Spinach beet or Chard"@en ;
        skos:definition  "-- Definition --\r\nBeta vulgaris L. Spinach beet or Chard.\r\n-- Description --\r\nList of vegetable specie -H\r\nNOTE. Initial value: H - 9.2"@en ;
        skos:inScheme    cap-iacs-basecode:SpecieCodeValue .

<http://lpis.ec.europa.eu/registry/applicationschema/cap-iacs-base/code#CropItemCodeValue/sugarBeetExcludingSeed>
        a                cap-iacs-base:CropItemCodeValue ;
        rdfs:label       "Sugar beet (excluding seed)"@en ;
        skos:definition  "-- Definition --\r\n||Sugar beet (excluding seed).\r\n-- Description --\r\nCereals and main crops - C\r\nNOTE. Initial value:C1370"@en ;
        skos:inScheme    cap-iacs-basecode:CropItemCodeValue .

<http://lpis.ec.europa.eu/registry/applicationschema/cap-iacs-base/code#VarietalNameValue/abelia>
        a                cap-iacs-base:VarietalNameValue ;
        rdfs:label       "H - 1.2  Abelia"@en ;
        skos:definition  "-- Definition --\r\nH - 1.2  Abelia\r\n-- Description --\r\nH - 1.2 Allium cepa L. Cepa group - Onion, Echalion /  Abelia.\r\nNOTE. Initial value: Abelia\r\nNOTE. MS - NL (Netherlands)."@en ;
        skos:inScheme    cap-iacs-basecode:VarietalNameValue .

<http://lpis.ec.europa.eu/registry/applicationschema/cap-iacs-base/code#StatusValue/approved>
        a                cap-iacs-base:StatusValue ;
        rdfs:label       "Approved, valid, archival"@en ;
        skos:definition  "-- Definition --\r\nApproved,\r\n\r\n--Definition--\r\nStatus of an object according to the state machine diagram.\r\n\r\n-- Description --\r\nStatus of the targeted schema / data object after final controls (consistency with IACS  and local rules)."@en ;
        skos:inScheme    cap-iacs-basecode:StatusValue .

<http://lpis.ec.europa.eu/registry/applicationschema/cap-iacs-base/code#TestVerdictValue/fail>
        a                cap-iacs-base:TestVerdictValue ;
        rdfs:label       "Fail verdict"@en ;
        skos:definition  "--Name--\r\nFail\r\n\r\n-- Definition --\r\nFail verdict to indicate that SUT does not fulfil the requirements.\r\n\r\n-- Description --\r\nTest verdict of non-conformance . Failure to fulfil one or more requirements specified."@en ;
        skos:inScheme    cap-iacs-basecode:TestVerdictValue .

<http://lpis.ec.europa.eu/registry/applicationschema/cap-iacs-base/code#SpecieCodeValue/zeaMaysLSweetCorn>
        a                cap-iacs-base:SpecieCodeValue ;
        rdfs:label       "Zea mays L. Sweet corn"@en ;
        skos:definition  "-- Definition --\r\nZea mays L. Sweet corn.\r\n-- Description --\r\nList of vegetable specie -H\r\nNOTE. Initial value: H - 36.1"@en ;
        skos:inScheme    cap-iacs-basecode:SpecieCodeValue .

<http://lpis.ec.europa.eu/registry/applicationschema/cap-iacs-base/code#CrossComplianceRuleValue/environmentClimateChangeGoodAgriculturalConditionOfLandBiodiversitySmr2>
        a                cap-iacs-base:CrossComplianceRuleValue ;
        rdfs:label       "Environment, climate change, good agricultural condition of land  - Biodiversity SMR2"@en ;
        skos:definition  "-- Definition --\r\nEnvironment, climate change, good agricultural condition of land  - Biodiversity SMR2.\r\n-- Description --\r\nDirective 2009/147/EC of the European Parliament and of the Council of 30 November 2009 on the conservation of wild birds (OJ L 20, 26.1.2010, p. 7). Article 3(1), Article 3(2)(b), Article 4(1), (2) and (4).\r\nNOTE. Initial value:SMR2"@en ;
        skos:inScheme    cap-iacs-basecode:CrossComplianceRuleValue .

<http://lpis.ec.europa.eu/registry/applicationschema/cap-iacs-base/code#CropItemCodeValue/kiwis>
        a                cap-iacs-base:CropItemCodeValue ;
        rdfs:label       "Kiwis"@en ;
        skos:definition  "-- Definition --\r\n|||Kiwis.\r\n-- Description --\r\nCereals and main crops - C\r\nNOTE. Initial value:C2285"@en ;
        skos:inScheme    cap-iacs-basecode:CropItemCodeValue .

<http://lpis.ec.europa.eu/registry/applicationschema/cap-iacs-base/code#SpecieCodeValue/triticumSpeltaLSpeltWheat>
        a                cap-iacs-base:SpecieCodeValue ;
        rdfs:label       "Triticum spelta L. Spelt wheat  "@en ;
        skos:definition  "-- Definition --\r\nTriticum spelta L. Spelt wheat.\r\n-- Description --\r\nList of agricultural species -A   \r\nIV. Cereals\r\nNOTE. Initial value: A - 85."@en ;
        skos:inScheme    cap-iacs-basecode:SpecieCodeValue .

<http://lpis.ec.europa.eu/registry/applicationschema/cap-iacs-base/code#SpecieCodeValue/×FestuloliumAschEtGraebnHybrids>
        a                cap-iacs-base:SpecieCodeValue ;
        rdfs:label       "×Festulolium Asch. et Graebn. Hybrids"@en ;
        skos:definition  "-- Definition --\r\n×Festulolium Asch. et Graebn. Hybrids resulting from the crossing of a species of the genus Festuca with a species of the genus Lolium.\r\n-- Description --\r\nList of agricultural species -A\r\nII. Fodder plants\r\nNOTE. Initial value: A - 19."@en ;
        skos:inScheme    cap-iacs-basecode:SpecieCodeValue .

<http://lpis.ec.europa.eu/registry/applicationschema/cap-iacs-base/code#NotificationGroupValue/notificationsRelatingToTheVoluntaryCoupledSupport>
        a                cap-iacs-base:NotificationGroupValue ;
        rdfs:label       "Notifications relating to the voluntary coupled support"@en ;
        skos:definition  "-- Definition --\r\nNotifications relating to the voluntary coupled support.\r\n-- Description --\r\nNOTE.66"@en ;
        skos:inScheme    cap-iacs-basecode:NotificationGroupValue .

<http://lpis.ec.europa.eu/registry/applicationschema/cap-iacs-base/code#ConformanceLevelValue/level2>
        a                cap-iacs-base:ConformanceLevelValue ;
        rdfs:label       "Level 2 medium"@en ;
        skos:definition  "--Name--\r\nLevel 2\r\n\r\n--Definition--\r\nLowest level conformance.\r\n\r\n--Description--\r\nA separate abstract test suite must be provided if a level is defined within ConformanceClause."@en ;
        skos:inScheme    cap-iacs-basecode:ConformanceLevelValue .

<http://lpis.ec.europa.eu/registry/applicationschema/cap-iacs-base/code#CropItemCodeValue/weavingPlants>
        a                cap-iacs-base:CropItemCodeValue ;
        rdfs:label       "Weaving plants"@en ;
        skos:definition  "-- Definition --\r\n|||Weaving plants.\r\n-- Description --\r\nLand use of Agriculture Area in Use -L\r\nNOTE. Initial value:L2960"@en ;
        skos:inScheme    cap-iacs-basecode:CropItemCodeValue .

<http://lpis.ec.europa.eu/registry/applicationschema/cap-iacs-base/code#CropItemCodeValue/rootCropsL1350>
        a                cap-iacs-base:CropItemCodeValue ;
        rdfs:label       "Root crops L1350"@en ;
        skos:definition  "-- Definition --\r\n|||Root crops L1350.\r\n-- Description --\r\nLand use of Agriculture Area in Use -L\r\nNOTE. Initial value:L1350"@en ;
        skos:inScheme    cap-iacs-basecode:CropItemCodeValue .

<http://lpis.ec.europa.eu/registry/applicationschema/cap-iacs-base/code#MonthValue/february>
        a                cap-iacs-base:MonthValue ;
        rdfs:label       "February"@en ;
        skos:definition  "-- Definition --\r\nFebruary.\r\n-- Description --\r\nItem description."@en ;
        skos:inScheme    cap-iacs-basecode:MonthValue .

<http://lpis.ec.europa.eu/registry/applicationschema/cap-iacs-base/code#SpecieCodeValue/oryzaSativaLRice>
        a                cap-iacs-base:SpecieCodeValue ;
        rdfs:label       "Oryza sativa L. Rice "@en ;
        skos:definition  "-- Definition --\r\nOryza sativa L. Rice.\r\n-- Description --\r\nList of agricultural species -A   \r\nIV. Cereals\r\nNOTE. Initial value: A - 76."@en ;
        skos:inScheme    cap-iacs-basecode:SpecieCodeValue .

<http://lpis.ec.europa.eu/registry/applicationschema/cap-iacs-base/code#CropItemCodeValue/strawberries>
        a                cap-iacs-base:CropItemCodeValue ;
        rdfs:label       "Strawberries"@en ;
        skos:definition  "-- Definition --\r\n||Strawberries.\r\n-- Description --\r\nCereals and main crops - C\r\nNOTE. Initial value:C2260"@en ;
        skos:inScheme    cap-iacs-basecode:CropItemCodeValue .

<http://lpis.ec.europa.eu/registry/applicationschema/cap-iacs-base/code#CropItemCodeValue/sorghum>
        a                cap-iacs-base:CropItemCodeValue ;
        rdfs:label       "Sorghum "@en ;
        skos:definition  "-- Definition --\r\n|||Sorghum.\r\n-- Description --\r\nCereals and main crops - C\r\nNOTE. Initial value:C1211"@en ;
        skos:inScheme    cap-iacs-basecode:CropItemCodeValue .

<http://lpis.ec.europa.eu/registry/applicationschema/cap-iacs-base/code#NotificationGroupValue/notificationsRelatingToTheAccreditedPayingAgenciesAndCoordinatingBodies>
        a                cap-iacs-base:NotificationGroupValue ;
        rdfs:label       "Notifications relating to the accredited paying agencies and coordinating bodies"@en ;
        skos:definition  "-- Definition --\r\nNotifications relating to the accredited paying agencies and coordinating bodies.\r\n-- Description --\r\nIn addition to the provisions laid down in the sectoral Regulations, Member States shall send to the Commission the information, declarations and documents: for accredited paying agencies and accredited coordinating bodies\r\n(a)(i) their accreditation document;\r\n(a)(ii) their function (accredited paying agency or accredited coordinating body);\r\n(a)(iii) where relevant, the withdrawal of their accreditation.\r\nNOTE.1011a"@en ;
        skos:inScheme    cap-iacs-basecode:NotificationGroupValue .

<http://lpis.ec.europa.eu/registry/applicationschema/cap-iacs-base/code#FarmStructureSurveyNumberValue/hemp>
        a                cap-iacs-base:FarmStructureSurveyNumberValue ;
        rdfs:label       "Hemp"@en ;
        skos:definition  "-- Definition --\r\nHemp.\r\n-- Description --\r\nCannabis sativa L.\r\nNOTE. Initial value:2.01.06.10"@en ;
        skos:inScheme    cap-iacs-basecode:FarmStructureSurveyNumberValue .

<http://lpis.ec.europa.eu/registry/applicationschema/cap-iacs-base/code#CropItemCodeValue/eggplants>
        a                cap-iacs-base:CropItemCodeValue ;
        rdfs:label       "Eggplants"@en ;
        skos:definition  "-- Definition --\r\n||||Eggplants.\r\n-- Description --\r\nCereals and main crops - C\r\nNOTE. Initial value:C1781"@en ;
        skos:inScheme    cap-iacs-basecode:CropItemCodeValue .

<http://lpis.ec.europa.eu/registry/applicationschema/cap-iacs-base/code#FarmStructureSurveyNumberValue/nuts>
        a                cap-iacs-base:FarmStructureSurveyNumberValue ;
        rdfs:label       "Nuts"@en ;
        skos:definition  "-- Definition --\r\nNuts.\r\n-- Description --\r\nNut tree plantations which are traditionally cropped in temperate and subtropical climates.\r\nNOTE. Initial value:2.04.01.03"@en ;
        skos:inScheme    cap-iacs-basecode:FarmStructureSurveyNumberValue .

<http://lpis.ec.europa.eu/registry/applicationschema/cap-iacs-base/code#SpecieCodeValue/poaPratensisLSmoothStalkedMeadowgrass>
        a                cap-iacs-base:SpecieCodeValue ;
        rdfs:label       "Poa pratensis L. Smooth-stalked meadowgrass"@en ;
        skos:definition  "-- Definition --\r\nPoa pratensis L. Smooth-stalked meadowgrass.\r\n-- Description --\r\nList of agricultural species -A\r\nII. Fodder plants\r\nNOTE. Initial value: A - 29."@en ;
        skos:inScheme    cap-iacs-basecode:SpecieCodeValue .

<http://lpis.ec.europa.eu/registry/applicationschema/cap-iacs-base/code#FarmStructureSurveyNumberValue/potatoesIncludingEarlyPotatoesAndSeedPotatoes>
        a                cap-iacs-base:FarmStructureSurveyNumberValue ;
        rdfs:label       "Potatoes (including early potatoes and seed potatoes)"@en ;
        skos:definition  "-- Definition --\r\nPotatoes (including early potatoes and seed potatoes).\r\n-- Description --\r\nSolanum tuberosum L.\r\nNOTE. Initial value:2.01.03"@en ;
        skos:inScheme    cap-iacs-basecode:FarmStructureSurveyNumberValue .

<http://lpis.ec.europa.eu/registry/applicationschema/cap-iacs-base/code#CropItemCodeValue/winterRye>
        a                cap-iacs-base:CropItemCodeValue ;
        rdfs:label       "Winter rye"@en ;
        skos:definition  "-- Definition --\r\n|||||Winter rye.\r\n-- Description --\r\nCereals and main crops - C\r\nNOTE. Initial value:C1151"@en ;
        skos:inScheme    cap-iacs-basecode:CropItemCodeValue .

<http://lpis.ec.europa.eu/registry/applicationschema/cap-iacs-base/code#CropItemCodeValue/cerealsForTheProductionOfGrainIncludingSeedButExcludingRice>
        a                cap-iacs-base:CropItemCodeValue ;
        rdfs:label       "Cereals for the production of grain (including seed but excluding rice)"@en ;
        skos:definition  "-- Definition --\r\n|||Cereals for the production of grain (including seed but excluding rice).\r\n-- Description --\r\nLand use of Agriculture Area in Use -L\r\nNOTE. Initial value:L1050"@en ;
        skos:inScheme    cap-iacs-basecode:CropItemCodeValue .

<http://lpis.ec.europa.eu/registry/applicationschema/cap-iacs-base/code#CropItemCodeValue/fieldPeas>
        a                cap-iacs-base:CropItemCodeValue ;
        rdfs:label       "Field peas"@en ;
        skos:definition  "-- Definition --\r\n||Field peas.\r\n-- Description --\r\nCereals and main crops - C\r\nNOTE. Initial value:C1320"@en ;
        skos:inScheme    cap-iacs-basecode:CropItemCodeValue .

<http://lpis.ec.europa.eu/registry/applicationschema/cap-iacs-base/code#StatusOfAnomalyValue/inProgress>
        a                cap-iacs-base:StatusOfAnomalyValue ;
        rdfs:label       "In progress"@en ;
        skos:definition  "--Name--\r\nIn progress\r\n\r\n-- Definition --\r\nStatus of the anomaly as soon as its processing has started or has been flagged for later resolution."@en ;
        skos:inScheme    cap-iacs-basecode:StatusOfAnomalyValue .

<http://lpis.ec.europa.eu/registry/applicationschema/cap-iacs-base/code#CropItemCodeValue/courgettes>
        a                cap-iacs-base:CropItemCodeValue ;
        rdfs:label       "Courgettes"@en ;
        skos:definition  "-- Definition --\r\n||||Courgettes.\r\n-- Description --\r\nCereals and main crops - C\r\nNOTE. Initial value:C1787"@en ;
        skos:inScheme    cap-iacs-basecode:CropItemCodeValue .

cap-iacs-basecode:SpecieCodeValue
        a                skos:ConceptScheme ;
        rdfs:label       "List of vegetable and agricultural plant species"@en ;
        dct:isFormatOf   cap-iacs-base:SpecieCodeValue ;
        skos:definition  "-- Definition --\r\nList of vegetable and agricultural plant species (aggregate of a varieties). \r\n-- Description --\r\nA culture of any of the different genera defined in the botanical classification of crops. In this case code list consist of binomial names of species from the taxonomy of Linnaeus (classification for plants).\r\nNOTE. Common catalogue of varieties of agricultural plant species. Fifth supplement to the 29th complete edition (2011/C 168 A/01)\r\nList of agricultural species -A\r\nI. Beet\r\nII. Fodder plants\r\nIII. Oil and fibre plants    \r\nIV. Cereals\r\nV. Potatoes \r\nNOTE. Common catalogue of varieties of vegetable species. 32nd complete edition (2013/C 312 A/01)\r\nList of vegetable species - H"@en .

<http://lpis.ec.europa.eu/registry/applicationschema/cap-iacs-base/code#SpecieCodeValue/phaceliaTanacetifoliaLCaliforniaBluebell>
        a                cap-iacs-base:SpecieCodeValue ;
        rdfs:label       "Phacelia tanacetifolia L. California bluebell "@en ;
        skos:definition  "-- Definition --\r\nPhacelia tanacetifolia L. California bluebell.\r\n-- Description --\r\nList of agricultural species -A\r\nII. Fodder plants\r\nNOTE. Initial value: A - 56."@en ;
        skos:inScheme    cap-iacs-basecode:SpecieCodeValue .

<http://lpis.ec.europa.eu/registry/applicationschema/cap-iacs-base/code#SpecieCodeValue/apiumGraveolensLCeleriac>
        a                cap-iacs-base:SpecieCodeValue ;
        rdfs:label       "Apium graveolens L. Celeriac"@en ;
        skos:definition  "-- Definition --\r\nApium graveolens L. Celeriac.\r\n-- Description --\r\nList of vegetable specie -H\r\nNOTE. Initial value: H - 7.2"@en ;
        skos:inScheme    cap-iacs-basecode:SpecieCodeValue .

<http://lpis.ec.europa.eu/registry/applicationschema/cap-iacs-base/code#SpecieCodeValue/phleumPratenseLTimothy>
        a                cap-iacs-base:SpecieCodeValue ;
        rdfs:label       "Phleum pratense L. Timothy "@en ;
        skos:definition  "-- Definition --\r\nPhleum pratense L. Timothy.\r\n-- Description --\r\nList of agricultural species -A\r\nII. Fodder plants\r\nNOTE. Initial value: A - 25."@en ;
        skos:inScheme    cap-iacs-basecode:SpecieCodeValue .

<http://lpis.ec.europa.eu/registry/applicationschema/cap-iacs-base/code#CropItemCodeValue/otherFruitsFromFruitTreesNec>
        a                cap-iacs-base:CropItemCodeValue ;
        rdfs:label       "Other fruits from fruit trees n.e.c."@en ;
        skos:definition  "-- Definition --\r\n|||Other fruits from fruit trees n.e.c.\r\n-- Description --\r\nCereals and main crops - C\r\nNOTE. Initial value:C2259"@en ;
        skos:inScheme    cap-iacs-basecode:CropItemCodeValue .

<http://lpis.ec.europa.eu/registry/applicationschema/cap-iacs-base/code#FarmStructureSurveyNumberValue/otherLandLandOccupiedByBuildingsFarmyardsTracksPondsQuarriesInfertileLandRockEtc>
        a                cap-iacs-base:FarmStructureSurveyNumberValue ;
        rdfs:label       "Other land (land occupied by buildings, farmyards, tracks, ponds, quarries, infertile land, rock, etc.)"@en ;
        skos:definition  "-- Definition --\r\nOther land (land occupied by buildings, farmyards, tracks, ponds, quarries, infertile land, rock, etc.)\r\n-- Description --\r\nAll those parts of the total area belonging to the agricultural holding which constitute neither utilised agricultural area, unutilised agricultural area nor wooded area.\r\nNOTE. Initial value:2.05.03"@en ;
        skos:inScheme    cap-iacs-basecode:FarmStructureSurveyNumberValue .

<http://lpis.ec.europa.eu/registry/applicationschema/cap-iacs-base/code#CropItemCodeValue/springRape>
        a                cap-iacs-base:CropItemCodeValue ;
        rdfs:label       "Spring rape"@en ;
        skos:definition  "-- Definition --\r\n||||||Spring rape.\r\n-- Description --\r\nCereals and main crops - C\r\nNOTE. Initial value:C1432"@en ;
        skos:inScheme    cap-iacs-basecode:CropItemCodeValue .

<http://lpis.ec.europa.eu/registry/applicationschema/cap-iacs-base/code#TestVerdictValue/inconclusive>
        a                cap-iacs-base:TestVerdictValue ;
        rdfs:label       "Inconclusive verdict"@en ;
        skos:definition  "--Name--\r\nInconclusive\r\n\r\n-- Definition --\r\nA value “inconclusive” indicates that the testing process has not yet yield a verdict.\r\n\r\n\r\n-- Description --\r\nNeither fail nor pass verdict can be assigned based on the test."@en ;
        skos:inScheme    cap-iacs-basecode:TestVerdictValue .

<http://lpis.ec.europa.eu/registry/applicationschema/cap-iacs-base/code#CropItemCodeValue/otherBerriesNec>
        a                cap-iacs-base:CropItemCodeValue ;
        rdfs:label       "Other berries n.e.c."@en ;
        skos:definition  "-- Definition --\r\n|||Other berries n.e.c.\r\n-- Description --\r\nCereals and main crops - C\r\nNOTE. Initial value:C2290"@en ;
        skos:inScheme    cap-iacs-basecode:CropItemCodeValue .

<http://lpis.ec.europa.eu/registry/applicationschema/cap-iacs-base/code#CropItemCodeValue/vegetablesMelonsAndStrawberries>
        a                cap-iacs-base:CropItemCodeValue ;
        rdfs:label       "Vegetables, melons and strawberries"@en ;
        skos:definition  "-- Definition --\r\n|||Vegetables, melons and strawberries.\r\n-- Description --\r\nLand use of Agriculture Area in Use -L\r\nNOTE. Initial value:L1600"@en ;
        skos:inScheme    cap-iacs-basecode:CropItemCodeValue .

<http://lpis.ec.europa.eu/registry/applicationschema/cap-iacs-base/code#CropItemCodeValue/chicory>
        a                cap-iacs-base:CropItemCodeValue ;
        rdfs:label       "Chicory"@en ;
        skos:definition  "-- Definition --\r\n|||Chicory.\r\n-- Description --\r\nCereals and main crops - C\r\nNOTE. Initial value:C1571"@en ;
        skos:inScheme    cap-iacs-basecode:CropItemCodeValue .

<http://lpis.ec.europa.eu/registry/applicationschema/cap-iacs-base/code#SpecieCodeValue/trifoliumPratenseLRedClover>
        a                cap-iacs-base:SpecieCodeValue ;
        rdfs:label       "Trifolium pratense L. Red clover"@en ;
        skos:definition  "-- Definition --\r\nTrifolium pratense L. Red clover.\r\n-- Description --\r\nList of agricultural species -A\r\nII. Fodder plants\r\nNOTE. Initial value: A - 46."@en ;
        skos:inScheme    cap-iacs-basecode:SpecieCodeValue .

<http://lpis.ec.europa.eu/registry/applicationschema/cap-iacs-base/code#CropItemCodeValue/otherPulsesNec>
        a                cap-iacs-base:CropItemCodeValue ;
        rdfs:label       "Other pulses n.e.c."@en ;
        skos:definition  "-- Definition --\r\n|||Other pulses n.e.c.\r\n-- Description --\r\nCereals and main crops - C\r\nNOTE. Initial value:C1905"@en ;
        skos:inScheme    cap-iacs-basecode:CropItemCodeValue .

<http://lpis.ec.europa.eu/registry/applicationschema/cap-iacs-base/code#CropItemCodeValue/commonWinterWheat>
        a                cap-iacs-base:CropItemCodeValue ;
        rdfs:label       "Common winter wheat"@en ;
        skos:definition  "-- Definition --\r\n|||||Common winter wheat.\r\n-- Description --\r\nCereals and main crops - C\r\nNOTE. Initial value:C1123"@en ;
        skos:inScheme    cap-iacs-basecode:CropItemCodeValue .

<http://lpis.ec.europa.eu/registry/applicationschema/cap-iacs-base/code#CropItemCodeValue/permanentGrassland>
        a                cap-iacs-base:CropItemCodeValue ;
        rdfs:label       "Permanent grassland"@en ;
        skos:definition  "-- Definition --\r\n||Permanent grassland.\r\n-- Description --\r\nLand use of Agriculture Area in Use -L\r\nNOTE. Initial value:L0002"@en ;
        skos:inScheme    cap-iacs-basecode:CropItemCodeValue .

<http://lpis.ec.europa.eu/registry/applicationschema/cap-iacs-base/code#SpecieCodeValue/cannabisSativaLHemp>
        a                cap-iacs-base:SpecieCodeValue ;
        rdfs:label       "Cannabis sativa L. Hemp "@en ;
        skos:definition  "-- Definition --\r\nCannabis sativa L. Hemp.\r\n-- Description --\r\nList of agricultural species -A\r\nIII. Oil and fibre plants\r\nNOTE. Initial value: A - 63."@en ;
        skos:inScheme    cap-iacs-basecode:SpecieCodeValue .

<http://lpis.ec.europa.eu/registry/applicationschema/cap-iacs-base/code#FarmStructureSurveyNumberValue/industrialCrops>
        a                cap-iacs-base:FarmStructureSurveyNumberValue ;
        rdfs:label       "Industrial crops"@en ;
        skos:definition  "-- Definition --\r\nIndustrial crops.\r\n-- Description --\r\nCrops that are normally not sold directly for consumption because they need to be industrially processed prior to final use.\r\nAll harvested areas of industrial crops, regardless of use, shall be recorded here (including crops used for renewable energy production).\r\nNOTE. Initial value:2.01.06"@en ;
        skos:inScheme    cap-iacs-basecode:FarmStructureSurveyNumberValue .

<http://lpis.ec.europa.eu/registry/applicationschema/cap-iacs-base/code#SpecieCodeValue/slycineMaxLMerrillSoyaBean>
        a                cap-iacs-base:SpecieCodeValue ;
        rdfs:label       "Glycine max (L.) Merrill Soya bean  "@en ;
        skos:definition  "-- Definition --\r\nGlycine max (L.) Merrill Soya bean.\r\n-- Description --\r\nList of agricultural species -A\r\nIII. Oil and fibre plants\r\nNOTE. Initial value: A - 71."@en ;
        skos:inScheme    cap-iacs-basecode:SpecieCodeValue .

<http://lpis.ec.europa.eu/registry/applicationschema/cap-iacs-base/code#CropItemCodeValue/olivePlantations>
        a                cap-iacs-base:CropItemCodeValue ;
        rdfs:label       "Olive plantations"@en ;
        skos:definition  "-- Definition --\r\n|||Olive plantations.\r\n-- Description --\r\nLand use of Agriculture Area in Use -L\r\nNOTE. Initial value:L2450"@en ;
        skos:inScheme    cap-iacs-basecode:CropItemCodeValue .

<http://lpis.ec.europa.eu/registry/applicationschema/cap-iacs-base/code#FarmStructureSurveyNumberValue/normallyProducingTableOlives>
        a                cap-iacs-base:FarmStructureSurveyNumberValue ;
        rdfs:label       "Normally producing table olives"@en ;
        skos:definition  "-- Definition --\r\nNormally producing table olives.\r\n-- Description --\r\nPlantations of varieties normally grown for producing table olives.\r\nNOTE. Initial value:2.04.03.01"@en ;
        skos:inScheme    cap-iacs-basecode:FarmStructureSurveyNumberValue .

<http://lpis.ec.europa.eu/registry/applicationschema/cap-iacs-base/code#AffectedElementTypeValue/featureType>
        a                cap-iacs-base:AffectedElementTypeValue ;
        rdfs:label       "Feature type"@en ;
        skos:definition  "--Name--\r\nFeature type\r\n\r\n-- Definition --\r\nA class that specifies set of spatial objects sharing common properties and operations applicable to the objects."@en ;
        skos:inScheme    cap-iacs-basecode:AffectedElementTypeValue .

cap-iacs-basecode:SupportSchemeTypeValue
        a                skos:ConceptScheme ;
        rdfs:label       "List of support schemas"@en ;
        dct:isFormatOf   cap-iacs-base:SupportSchemeTypeValue ;
        skos:definition  "Support scheme type value\r\n\r\nList of support schemes as defined in Regulation (EU) 1307/2013.\r\n\r\nNOTE\r\nPayment schema type list may be extended or shortened by MS."@en .

<http://lpis.ec.europa.eu/registry/applicationschema/cap-iacs-base/code#CropItemCodeValue/gourdsMarrowsAndPumpkins>
        a                cap-iacs-base:CropItemCodeValue ;
        rdfs:label       "Gourds, marrows and pumpkins"@en ;
        skos:definition  "-- Definition --\r\n||||Gourds, marrows and pumpkins.\r\n-- Description --\r\nCereals and main crops - C\r\nNOTE. Initial value:C1786"@en ;
        skos:inScheme    cap-iacs-basecode:CropItemCodeValue .

<http://lpis.ec.europa.eu/registry/applicationschema/cap-iacs-base/code#SupportSchemeTypeValue/singleAreaPaymentScheme>
        a                cap-iacs-base:SupportSchemeTypeValue ;
        rdfs:label       "Single area payment scheme"@en ;
        skos:definition  "Single area payment scheme \r\n\r\nPayment scheme based on the single area payment granted on an annual basis for each eligible hectare declared by the farmer in accordance with point (a) of the first subparagraph of Article 72(1) of Regulation (EU) No 1306/2013.\r\n\r\nAs described in Article 36 of 1307/2013 Regulation  it is a decoupled payment based on utilised land."@en ;
        skos:inScheme    cap-iacs-basecode:SupportSchemeTypeValue .

<http://lpis.ec.europa.eu/registry/applicationschema/cap-iacs-base/code#SpecieCodeValue/raphanusSativusLBlackRadish>
        a                cap-iacs-base:SpecieCodeValue ;
        rdfs:label       "Raphanus sativus L. Black radish"@en ;
        skos:definition  "-- Definition --\r\nRaphanus sativus L. Black radish.\r\n-- Description --\r\nList of vegetable specie -H\r\nNOTE. Initial value: H - 29.2"@en ;
        skos:inScheme    cap-iacs-basecode:SpecieCodeValue .

<http://lpis.ec.europa.eu/registry/applicationschema/cap-iacs-base/code#CropItemCodeValue/sourCherries>
        a                cap-iacs-base:CropItemCodeValue ;
        rdfs:label       "Sour cherries"@en ;
        skos:definition  "-- Definition --\r\n||||Sour cherries.\r\n-- Description --\r\nCereals and main crops - C\r\nNOTE. Initial value:C2201"@en ;
        skos:inScheme    cap-iacs-basecode:CropItemCodeValue .

cap-iacs-basecode:CrossComplianceRuleValue
        a                skos:ConceptScheme ;
        rdfs:label       "List of rules for cross-compliance"@en ;
        dct:isFormatOf   cap-iacs-base:CrossComplianceRuleValue ;
        skos:definition  "-- Definition --\r\nList of rules for cross-compliance\r\n-- Description --\r\nList of rules for cross-compliance. Rules for SMR and GAEC."@en .

<http://lpis.ec.europa.eu/registry/applicationschema/cap-iacs-base/code#SpecieCodeValue/brassicaRapaLChineseCabbage>
        a                cap-iacs-base:SpecieCodeValue ;
        rdfs:label       "Brassica rapa L. Chinese cabbage"@en ;
        skos:definition  "-- Definition --\r\nBrassica rapa L. Chinese cabbage.\r\n-- Description --\r\nList of vegetable specie -H\r\nNOTE. Initial value: H - 11.1"@en ;
        skos:inScheme    cap-iacs-basecode:SpecieCodeValue .

<http://lpis.ec.europa.eu/registry/applicationschema/cap-iacs-base/code#CrossComplianceRuleValue/publicHealthAnimalHealthAndPlantHealthIdentificationAndRegistrationOfAnimalsSmr6>
        a                cap-iacs-base:CrossComplianceRuleValue ;
        rdfs:label       "Public health, animal health and plant health  - Identification and registration of animals SMR6"@en ;
        skos:definition  "-- Definition --\r\nPublic health, animal health and plant health  - Identification and registration of animals SMR6.\r\n-- Description --\r\nCouncil Directive 2008/71/EC of 15 July 2008 on identification and registration of pigs (OJ L 213, 8.8.2005, p. 31). Articles 3, 4 and 5.\r\nNOTE. Initial value:SMR6"@en ;
        skos:inScheme    cap-iacs-basecode:CrossComplianceRuleValue .

<http://lpis.ec.europa.eu/registry/applicationschema/cap-iacs-base/code#FarmStructureSurveyNumberValue/geneticallyModifiedCrops>
        a                cap-iacs-base:FarmStructureSurveyNumberValue ;
        rdfs:label       "Genetically modified crops"@en ;
        skos:definition  "-- Definition --\r\nGenetically modified crops.\r\n-- Description --\r\n‘Genetically modified crops (GMC)’ mean any organism as defined in Article 2 of Council Directive 2001/18/EC(1) OJ L 106, 17.4.2001, p. 1. (1) or, where applicable, the most recent legislation.\r\nNOTE. Initial value:2.06.04"@en ;
        skos:inScheme    cap-iacs-basecode:FarmStructureSurveyNumberValue .

<http://lpis.ec.europa.eu/registry/applicationschema/cap-iacs-base/code#SpecieCodeValue/cucumisMeloLMelon>
        a                cap-iacs-base:SpecieCodeValue ;
        rdfs:label       "Cucumis melo L. Melon"@en ;
        skos:definition  "-- Definition --\r\nCucumis melo L. Melon.\r\n-- Description --\r\nList of vegetable specie -H\r\nNOTE. Initial value: H - 16."@en ;
        skos:inScheme    cap-iacs-basecode:SpecieCodeValue .

<http://lpis.ec.europa.eu/registry/applicationschema/cap-iacs-base/code#CropItemCodeValue/vegetablesMelonsAndStrawberriesUnderGlassHighAccessibleCover>
        a                cap-iacs-base:CropItemCodeValue ;
        rdfs:label       "Vegetables, melons and strawberries under glass high accessible cover"@en ;
        skos:definition  "-- Definition --\r\nVegetables, melons and strawberries under glass high accessible cover.\r\n-- Description --\r\nLand use of Agriculture Area in Use -L. Special aggregates\r\nNOTE. Initial value:L1112"@en ;
        skos:inScheme    cap-iacs-basecode:CropItemCodeValue .

<http://lpis.ec.europa.eu/registry/applicationschema/cap-iacs-base/code#SpecieCodeValue/cynodonDactylonLBermudaGrass>
        a                cap-iacs-base:SpecieCodeValue ;
        rdfs:label       "Cynodon dactylon L. Bermuda grass"@en ;
        skos:definition  "-- Definition --\r\nCynodon dactylon L. Bermuda grass.\r\n-- Description --\r\nList of agricultural species -A\r\nII. Fodder plants\r\nNOTE. Initial value: A - 11."@en ;
        skos:inScheme    cap-iacs-basecode:SpecieCodeValue .

<http://lpis.ec.europa.eu/registry/applicationschema/cap-iacs-base/code#CrossComplianceRuleValue/environmentClimateChangeGoodAgriculturalConditionOfLandWaterGaec2>
        a                cap-iacs-base:CrossComplianceRuleValue ;
        rdfs:label       "Environment, climate change, good agricultural condition of land  - Water GAEC2"@en ;
        skos:definition  "-- Definition --\r\nEnvironment, climate change, good agricultural condition of land  - Water GAEC2.\r\n-- Description --\r\nWhere use of water for irrigation is subject to authorisation, compliance with authorisation procedures. \r\nNOTE. Initial value:GAEC2"@en ;
        skos:inScheme    cap-iacs-basecode:CrossComplianceRuleValue .

<http://lpis.ec.europa.eu/registry/applicationschema/cap-iacs-base/code#CropItemCodeValue/permanentGrasslandPasturesAndMeadows>
        a                cap-iacs-base:CropItemCodeValue ;
        rdfs:label       "Permanent grassland (pastures and meadows)"@en ;
        skos:definition  "-- Definition --\r\n|Permanent grassland (pastures and meadows).\r\n-- Description --\r\nCereals and main crops - C\r\nNOTE. Initial value:C0002"@en ;
        skos:inScheme    cap-iacs-basecode:CropItemCodeValue .

<http://lpis.ec.europa.eu/registry/applicationschema/cap-iacs-base/code#AffectedElementTypeValue/applicationSchema>
        a                cap-iacs-base:AffectedElementTypeValue ;
        rdfs:label       "Application schema"@en ;
        skos:definition  "--Name--\r\nApplication schema\r\n\r\n-- Definition --\r\nConceptual schema for data required for one or more applications [ISO 19101:2002]."@en ;
        skos:inScheme    cap-iacs-basecode:AffectedElementTypeValue .

<http://lpis.ec.europa.eu/registry/applicationschema/cap-iacs-base/code#CropItemCodeValue/apricots>
        a                cap-iacs-base:CropItemCodeValue ;
        rdfs:label       "Apricots"@en ;
        skos:definition  "-- Definition --\r\n|||Apricots.\r\n-- Description --\r\nCereals and main crops - C\r\nNOTE. Initial value:C2190"@en ;
        skos:inScheme    cap-iacs-basecode:CropItemCodeValue .

<http://lpis.ec.europa.eu/registry/applicationschema/cap-iacs-base/code#OrdinalNumberValue/first>
        a                cap-iacs-base:OrdinalNumberValue ;
        rdfs:label       "First"@en ;
        skos:definition  "-- Definition --\r\nFirst.\r\n-- Description --\r\nItem description."@en ;
        skos:inScheme    cap-iacs-basecode:OrdinalNumberValue .

<http://lpis.ec.europa.eu/registry/applicationschema/cap-iacs-base/code#FarmStructureSurveyNumberValue/olivePlantations>
        a                cap-iacs-base:FarmStructureSurveyNumberValue ;
        rdfs:label       "Olive plantations"@en ;
        skos:definition  "-- Definition --\r\nOlive plantations.\r\n-- Description --\r\nPlantations of Olea europea L.\r\nNOTE. Initial value:2.04.03"@en ;
        skos:inScheme    cap-iacs-basecode:FarmStructureSurveyNumberValue .

<http://lpis.ec.europa.eu/registry/applicationschema/cap-iacs-base/code#CropItemCodeValue/kohlRabiC1650>
        a                cap-iacs-base:CropItemCodeValue ;
        rdfs:label       "Kohl-Rabi C1650"@en ;
        skos:definition  "-- Definition --\r\n|||Kohl-Rabi C1650.\r\n-- Description --\r\nCereals and main crops - C\r\nNOTE. Initial value:C1650"@en ;
        skos:inScheme    cap-iacs-basecode:CropItemCodeValue .

<http://lpis.ec.europa.eu/registry/applicationschema/cap-iacs-base/code#CropItemCodeValue/rootAndTuberVegetables>
        a                cap-iacs-base:CropItemCodeValue ;
        rdfs:label       "Root and tuber vegetables"@en ;
        skos:definition  "-- Definition --\r\n||Root and tuber vegetables.\r\n-- Description --\r\nCereals and main crops - C\r\nNOTE. Initial value:C1800"@en ;
        skos:inScheme    cap-iacs-basecode:CropItemCodeValue .

<http://lpis.ec.europa.eu/registry/applicationschema/cap-iacs-base/code#CrossComplianceRuleValue/animalWelfareAnimalWelfareSmr12>
        a                cap-iacs-base:CrossComplianceRuleValue ;
        rdfs:label       "Animal welfare - Animal welfare SMR12"@en ;
        skos:definition  "-- Definition --\r\nAnimal welfare - Animal welfare SMR12.\r\n-- Description --\r\nCouncil Directive 2008/120/EC of 18 December 2008 laying down minimum standards for the protection of pigs (OJ L 47, 18.2.2009, p. 5). Article 3 and Article 4.\r\nNOTE. Initial value:SMR12"@en ;
        skos:inScheme    cap-iacs-basecode:CrossComplianceRuleValue .

<http://lpis.ec.europa.eu/registry/applicationschema/cap-iacs-base/code#SpecieCodeValue/avenaStrigosaSchrebLBlackOatBristle>
        a                cap-iacs-base:SpecieCodeValue ;
        rdfs:label       "Avena strigosa Schreb. L. Black oat / Bristle"@en ;
        skos:definition  "-- Definition --\r\nAvena strigosa Schreb. L. Black oat / Bristle.\r\n-- Description --\r\nList of agricultural species -A   \r\nIV. Cereals\r\nNOTE. Initial value: A - 74."@en ;
        skos:inScheme    cap-iacs-basecode:SpecieCodeValue .

<http://lpis.ec.europa.eu/registry/applicationschema/cap-iacs-base/code#CropItemCodeValue/otherUtilisedAgriculturalArea>
        a                cap-iacs-base:CropItemCodeValue ;
        rdfs:label       "Other utilised agricultural area"@en ;
        skos:definition  "-- Definition --\r\n||Other utilised agricultural area.\r\n-- Description --\r\nLand use of Agriculture Area in Use -L\r\nNOTE. Initial value:L2990"@en ;
        skos:inScheme    cap-iacs-basecode:CropItemCodeValue .

<http://lpis.ec.europa.eu/registry/applicationschema/cap-iacs-base/code#CropItemCodeValue/otherPotatoes>
        a                cap-iacs-base:CropItemCodeValue ;
        rdfs:label       "Other potatoes"@en ;
        skos:definition  "-- Definition --\r\n|||Other potatoes.\r\n-- Description --\r\nCereals and main crops - C\r\nNOTE. Initial value:C1363"@en ;
        skos:inScheme    cap-iacs-basecode:CropItemCodeValue .

<http://lpis.ec.europa.eu/registry/applicationschema/cap-iacs-base/code#CropItemCodeValue/otherFruitsFromFruitTrees>
        a                cap-iacs-base:CropItemCodeValue ;
        rdfs:label       "Other fruits from fruit trees"@en ;
        skos:definition  "-- Definition --\r\n||Other fruits from fruit trees.\r\n-- Description --\r\nCereals and main crops - C\r\nNOTE. Initial value:C2250"@en ;
        skos:inScheme    cap-iacs-basecode:CropItemCodeValue .

<http://lpis.ec.europa.eu/registry/applicationschema/cap-iacs-base/code#CropItemCodeValue/durumWheat>
        a                cap-iacs-base:CropItemCodeValue ;
        rdfs:label       "Durum wheat"@en ;
        skos:definition  "-- Definition --\r\n||||Durum wheat.\r\n-- Description --\r\nCereals and main crops - C\r\nNOTE. Initial value:C1130"@en ;
        skos:inScheme    cap-iacs-basecode:CropItemCodeValue .

<http://lpis.ec.europa.eu/registry/applicationschema/cap-iacs-base/code#CropItemCodeValue/currants>
        a                cap-iacs-base:CropItemCodeValue ;
        rdfs:label       "Currants"@en ;
        skos:definition  "-- Definition --\r\n|||Currants.\r\n-- Description --\r\nCereals and main crops - C\r\nNOTE. Initial value:C2271"@en ;
        skos:inScheme    cap-iacs-basecode:CropItemCodeValue .

<http://lpis.ec.europa.eu/registry/applicationschema/cap-iacs-base/code#CropItemCodeValue/leafyOrStalkedVegetablesExcludingBrassicas>
        a                cap-iacs-base:CropItemCodeValue ;
        rdfs:label       "Leafy or stalked vegetables (excluding brassicas)"@en ;
        skos:definition  "-- Definition --\r\n||Leafy or stalked vegetables (excluding brassicas).\r\n-- Description --\r\nCereals and main crops - C\r\nNOTE. Initial value:C1660"@en ;
        skos:inScheme    cap-iacs-basecode:CropItemCodeValue .

<http://lpis.ec.europa.eu/registry/applicationschema/cap-iacs-base/code#FarmStructureSurveyNumberValue/linseedOilFlax>
        a                cap-iacs-base:FarmStructureSurveyNumberValue ;
        rdfs:label       "Linseed (oil flax)"@en ;
        skos:definition  "-- Definition --\r\nLinseed (oil flax).\r\n-- Description --\r\nLinum usitatissimum L., varieties grown mainly for producing oil, harvested as dry grains.\r\nNOTE. Initial value:2.01.06.07"@en ;
        skos:inScheme    cap-iacs-basecode:FarmStructureSurveyNumberValue .

<http://lpis.ec.europa.eu/registry/applicationschema/cap-iacs-base/code#CropItemCodeValue/cerealsForTheProductionOfGrainIncludingRiceAndSeed>
        a                cap-iacs-base:CropItemCodeValue ;
        rdfs:label       "Cereals for the production of grain (including rice and seed)"@en ;
        skos:definition  "-- Definition --\r\n|Cereals for the production of grain (including rice and seed).\r\n-- Description --\r\nCereals and main crops - C\r\nNOTE. Initial value:C1040"@en ;
        skos:inScheme    cap-iacs-basecode:CropItemCodeValue .

<http://lpis.ec.europa.eu/registry/applicationschema/cap-iacs-base/code#CropItemCodeValue/sweetLupinsC1343>
        a                cap-iacs-base:CropItemCodeValue ;
        rdfs:label       "Sweet lupins C1343"@en ;
        skos:definition  "-- Definition --\r\n||Sweet lupins C1343.\r\n-- Description --\r\nCereals and main crops - C\r\nNOTE. Initial value:C1343"@en ;
        skos:inScheme    cap-iacs-basecode:CropItemCodeValue .

<http://lpis.ec.europa.eu/registry/applicationschema/cap-iacs-base/code#FarmStructureSurveyNumberValue/ofWhichOnSetAsideArea>
        a                cap-iacs-base:FarmStructureSurveyNumberValue ;
        rdfs:label       "of which on set-aside area"@en ;
        skos:definition  "-- Definition --\r\nof which on set-aside area.\r\n-- Description --\r\nThe production area of energy crops benefiting of the payment linked to set-aside entitlement when production takes place on set-aside area (Council Regulation (EC) No 1782/2003, Article 55 or 56).\r\nNOTE. Initial value:2.06.03.01"@en ;
        skos:inScheme    cap-iacs-basecode:FarmStructureSurveyNumberValue .

<http://lpis.ec.europa.eu/registry/applicationschema/cap-iacs-base/code#CropItemCodeValue/vineyardsForWine>
        a                cap-iacs-base:CropItemCodeValue ;
        rdfs:label       "Vineyards for wine"@en ;
        skos:definition  "-- Definition --\r\n|||Vineyards for wine.\r\n-- Description --\r\nCereals and main crops - C\r\nNOTE. Initial value:C2440"@en ;
        skos:inScheme    cap-iacs-basecode:CropItemCodeValue .

<http://lpis.ec.europa.eu/registry/applicationschema/cap-iacs-base/code#FarmStructureSurveyNumberValue/totalCultivatedAreaIrrigatedAtLeastOnceDuringThePrevious12Months>
        a                cap-iacs-base:FarmStructureSurveyNumberValue ;
        rdfs:label       "Total cultivated area irrigated at least once during the previous 12 months"@en ;
        skos:definition  "-- Definition --\r\nTotal cultivated area irrigated at least once during the previous 12 months.\r\n-- Description --\r\nArea of crops which have actually been irrigated at least once during the 12 months prior to the reference day of the survey.\r\nNOTE. Initial value:2.06.02.02"@en ;
        skos:inScheme    cap-iacs-basecode:FarmStructureSurveyNumberValue .

<http://lpis.ec.europa.eu/registry/applicationschema/cap-iacs-base/code#CropItemCodeValue/cloverAndMixtures>
        a                cap-iacs-base:CropItemCodeValue ;
        rdfs:label       "Clover and mixtures"@en ;
        skos:definition  "-- Definition --\r\n|||Clover and mixtures.\r\n-- Description --\r\nCereals and main crops - C\r\nNOTE. Initial value:C2671"@en ;
        skos:inScheme    cap-iacs-basecode:CropItemCodeValue .

<http://lpis.ec.europa.eu/registry/applicationschema/cap-iacs-base/code#MonthValue/june>
        a                cap-iacs-base:MonthValue ;
        rdfs:label       "June"@en ;
        skos:definition  "-- Definition --\r\nJune.\r\n-- Description --\r\nItem description."@en ;
        skos:inScheme    cap-iacs-basecode:MonthValue .

<http://lpis.ec.europa.eu/registry/applicationschema/cap-iacs-base/code#CropItemCodeValue/gooseberries>
        a                cap-iacs-base:CropItemCodeValue ;
        rdfs:label       "Gooseberries"@en ;
        skos:definition  "-- Definition --\r\n|||Gooseberries.\r\n-- Description --\r\nCereals and main crops - C\r\nNOTE. Initial value:C2281"@en ;
        skos:inScheme    cap-iacs-basecode:CropItemCodeValue .

<http://lpis.ec.europa.eu/registry/applicationschema/cap-iacs-base/code#SpecieCodeValue/lotusCorniculatusLBirdsfootTrefoil>
        a                cap-iacs-base:SpecieCodeValue ;
        rdfs:label       "Lotus corniculatus L. Birdsfoot trefoil"@en ;
        skos:definition  "-- Definition --\r\nLotus corniculatus L. Birdsfoot trefoil\r\n-- Description --\r\nList of agricultural species -A\r\nII. Fodder plants\r\nNOTE. Initial value: A - 34."@en ;
        skos:inScheme    cap-iacs-basecode:SpecieCodeValue .

<http://lpis.ec.europa.eu/registry/applicationschema/cap-iacs-base/code#SpecieCodeValue/sspNonAlternativum>
        a                cap-iacs-base:SpecieCodeValue ;
        rdfs:label       "Ssp. non alternativum"@en ;
        skos:definition  "-- Definition --\r\nLolium multiflorum Lam. Italian ryegrass (including Westerwold ryegrass) Ssp. non alternativum.\r\n-- Description --\r\nNOTE. Initial value: A - 20.2"@en ;
        skos:inScheme    cap-iacs-basecode:SpecieCodeValue .

<http://lpis.ec.europa.eu/registry/applicationschema/cap-iacs-base/code#SpecieCodeValue/agrostisCapillarisLBrownTop>
        a                cap-iacs-base:SpecieCodeValue ;
        rdfs:label       "Agrostis capillaris L. Brown top"@en ;
        skos:definition  "-- Definition --\r\nAgrostis capillaris L. Brown top.\r\n-- Description --\r\nList of agricultural species -A\r\nII. Fodder plants\r\nNOTE. Initial value: A - 6."@en ;
        skos:inScheme    cap-iacs-basecode:SpecieCodeValue .

<http://lpis.ec.europa.eu/registry/applicationschema/cap-iacs-base/code#CropItemCodeValue/bananas>
        a                cap-iacs-base:CropItemCodeValue ;
        rdfs:label       "Bananas"@en ;
        skos:definition  "-- Definition --\r\n|||Bananas.\r\n-- Description --\r\nCereals and main crops - C\r\nNOTE. Initial value:C2254"@en ;
        skos:inScheme    cap-iacs-basecode:CropItemCodeValue .

<http://lpis.ec.europa.eu/registry/applicationschema/cap-iacs-base/code#SpecieCodeValue/sorghumBicolorLMoenchSorghum>
        a                cap-iacs-base:SpecieCodeValue ;
        rdfs:label       "Sorghum bicolor (L.) Moench Sorghum "@en ;
        skos:definition  "-- Definition --\r\nSorghum bicolor (L.) Moench Sorghum.\r\n-- Description --\r\nList of agricultural species -A   \r\nIV. Cereals\r\nNOTE. Initial value: A - 79."@en ;
        skos:inScheme    cap-iacs-basecode:SpecieCodeValue .

<http://lpis.ec.europa.eu/registry/applicationschema/cap-iacs-base/code#CropItemCodeValue/radishes>
        a                cap-iacs-base:CropItemCodeValue ;
        rdfs:label       "Radishes"@en ;
        skos:definition  "-- Definition --\r\n|||Radishes.\r\n-- Description --\r\nCereals and main crops - C\r\nNOTE. Initial value:C1877"@en ;
        skos:inScheme    cap-iacs-basecode:CropItemCodeValue .

<http://lpis.ec.europa.eu/registry/applicationschema/cap-iacs-base/code#RecurenceValue/daily>
        a                cap-iacs-base:RecurenceValue ;
        rdfs:label       "Daily recurrence"@en ;
        skos:definition  "-- Definition --\r\nDaily recurrence.\r\n-- Description --\r\nItem description."@en ;
        skos:inScheme    cap-iacs-basecode:RecurenceValue .

<http://lpis.ec.europa.eu/registry/applicationschema/cap-iacs-base/code#SpecieCodeValue/pisumSativumLPartimFieldPea>
        a                cap-iacs-base:SpecieCodeValue ;
        rdfs:label       "Pisum sativum L. (Partim) Field pea"@en ;
        skos:definition  "-- Definition --\r\nPisum sativum L. (Partim) Field pea.\r\n-- Description --\r\nList of agricultural species -A\r\nII. Fodder plants\r\nNOTE. Initial value: A - 42."@en ;
        skos:inScheme    cap-iacs-basecode:SpecieCodeValue .
