@prefix owl:   <http://www.w3.org/2002/07/owl#> .
@prefix gsp:   <http://www.opengis.net/ont/geosparql#> .
@prefix rdf:   <http://www.w3.org/1999/02/22-rdf-syntax-ns#> .
@prefix xsd:   <http://www.w3.org/2001/XMLSchema#> .
@prefix skos:  <http://www.w3.org/2004/02/skos/core#> .
@prefix rdfs:  <http://www.w3.org/2000/01/rdf-schema#> .
@prefix foaf:  <http://xmlns.com/foaf/0.1/> .
@prefix dct:   <http://purl.org/dc/terms/> .
@prefix schema: <http://schema.org/> .
@prefix om:    <http://www.ontology-of-units-of-measure.org/resource/om-2/> .
@prefix qudt: <http://qudt.org/schema/qudt/> .
@prefix cap-iacs-base: <http://lpis.ec.europa.eu/registry/applicationschema/cap-iacs-base#> .
@prefix cap-iacs-basecode: <http://lpis.ec.europa.eu/registry/applicationschema/cap-iacs-base/code#> .
@prefix cap-iacs-parcel: <http://lpis.ec.europa.eu/registry/applicationschema/cap-iacs-parcel#> .
@prefix cap-iacs-parcelcode: <http://lpis.ec.europa.eu/registry/applicationschema/cap-iacs-parcel/code#> .
@prefix cap-iacs-beneficiery: <http://lpis.ec.europa.eu/registry/applicationschema/cap-iacs-beneficiery#> .
@prefix cap-iacs-beneficierycode: <http://lpis.ec.europa.eu/registry/applicationschema/cap-iacs-beneficiery/code#> .
@prefix cap-iacs-control: <http://lpis.ec.europa.eu/registry/applicationschema/cap-iacs-control#> .
@prefix cap-iacs-controlcode: <http://lpis.ec.europa.eu/registry/applicationschema/cap-iacs-control/code#> .
@prefix cap-iacs-aid: <http://lpis.ec.europa.eu/registry/applicationschema/cap-iacs-aid#> .
@prefix cap-iacs-aidcode: <http://lpis.ec.europa.eu/registry/applicationschema/cap-iacs-aid/code#> .
@prefix cap-fas: <http://lpis.ec.europa.eu/registry/applicationschema/cap-fas#> .
@prefix cap-iacs-animal: <http://lpis.ec.europa.eu/registry/applicationschema/cap-iacs-animal#> .
@prefix cap-iacs-entitlement: <http://lpis.ec.europa.eu/registry/applicationschema/cap-iacs-entitlement#> .
@prefix cap-iacs-entitlementcode: <http://lpis.ec.europa.eu/registry/applicationschema/cap-iacs-entitlement/code#> .
@prefix cap-iacs-parcel-ext: <http://lpis.ec.europa.eu/registry/applicationschema/cap-iacs-parcel#> .


<http://lpis.ec.europa.eu/registry/applicationschema/cap-parcel-ext>
        a                owl:Ontology ;
        owl:versionIRI   <http://lpis.ec.europa.eu/registry/applicationschema/cap-parcel-ext/1.0> ;
        owl:versionInfo  "1.0" ;
        dct:creator [ schema:affiliation [ foaf:name "PSNC" ] ;
                      rdfs:seeAlso <http://orcid.org/0000-0003-4289-4922> ;
                      foaf:name "Raul Palma"
                    ] ,
                    [ schema:affiliation [ foaf:name "PSNC" ] ;
                      foaf:name "Bogusz Janiak"
                    ] ;
        owl:imports <https://raw.githubusercontent.com/rapw3k/cap-iacs/main/cap-iacs-parcel.ttl> ;
        dct:title "JRC IACS Extension - Extension of the identification System for Agricultural Parcels Ontology"@en ;
        dct:description "Extension of the identification system for agricultural parcels Ontology used in IACS that includes former Reference Parcel subtypes : CadParcel, AgrParcel, FarBlock, PhyBlock, TopoBlock and MixedParcelType"@en ;
        dct:source "JRC IACS application schema. https://doi.org/10.1016/j.landusepol.2016.05.023"@en ;
        dct:rights "This ontology is distributed under Creative Commons Attribution 4.0 License - http://creativecommons.org/licenses/by/4.0"@en .
        
cap-iacs-parcel:CadParcel
        a                owl:Class ;
        rdfs:label       "Cadastral parcel"@en ;
        rdfs:subClassOf  cap-iacs-parcel:ReferenceParcel ;        
        skos:definition  "Reference Parcel subtype that is not anymore a core element of current IACS model. Main Features: i) one or more farmers; ii) based on ownership; iii) one or more crop groups"@en .
        
cap-iacs-parcel:FarBlock
        a                owl:Class ;
        rdfs:label       "Farmer's block"@en ;
        rdfs:subClassOf  cap-iacs-parcel:ReferenceParcel ;        
        skos:definition  "Reference Parcel subtype that is not anymore a core element of current IACS model. Main Features: i) single farmer; ii) one or more crop groups; iii) no natural boundaries"@en .
        
cap-iacs-parcel:PhyBlock
        a                owl:Class ;
        rdfs:label       "Physical block"@en ;
        owl:equivalentClass cap-iacs-parcel:TopoBlock ;
        rdfs:subClassOf  cap-iacs-parcel:ReferenceParcel ;        
        skos:definition  "Reference Parcel subtype that is not anymore a core element of current IACS model. Main Features: i) one or more farmers; ii) area bordered by certain features; iii) one or more crop groups"@en .        
        
cap-iacs-parcel:TopoBlock
        a                owl:Class ;
        rdfs:label       "Topographical block"@en ;
        owl:equivalentClass cap-iacs-parcel:PhyBlock ;
        rdfs:subClassOf  cap-iacs-parcel:ReferenceParcel ;        
        skos:definition  "Reference Parcel subtype that is not anymore a core element of current IACS model. Main Features: i) one or more farmers; ii) area bordered by certain features; iii) one or more crop groups"@en .  
        
cap-iacs-parcel:MixedParcel
        a                owl:Class ;
        rdfs:label       "Mixed parcel"@en ;
        rdfs:subClassOf  cap-iacs-parcel:ReferenceParcel ;        
        skos:definition  "Reference Parcel subtype that is not anymore a core element of current IACS model. Mixed parcel type"@en .                        