@prefix cap-iacs-controlcode: <http://lpis.ec.europa.eu/registry/applicationschema/cap-iacs-control/code#> .
@prefix cap-iacs-control: <http://lpis.ec.europa.eu/registry/applicationschema/cap-iacs-control#> .
@prefix dct:   <http://purl.org/dc/terms/> .
@prefix owl:   <http://www.w3.org/2002/07/owl#> .
@prefix rdf:   <http://www.w3.org/1999/02/22-rdf-syntax-ns#> .
@prefix xsd:   <http://www.w3.org/2001/XMLSchema#> .
@prefix skos:  <http://www.w3.org/2004/02/skos/core#> .
@prefix rdfs:  <http://www.w3.org/2000/01/rdf-schema#> .

<http://lpis.ec.europa.eu/registry/applicationschema/cap-iacs-control/code#SamplingStrategyTypeValue/riskBasedMultiCriteriaSelection>
        a                cap-iacs-control:SamplingStrategyTypeValue ;
        rdfs:label       "Risk based sampling strategy"@en ;
        skos:definition  "Risk based multi-criteria selection\r\n\r\nRisk based selection based on multi-criteria analysis.\r\nExamples of aspects of analysis:\r\n\t- areas of recent land cover / land use change (from third party data)\r\n\t- Landscape\r\n\t- Agronomic conditions\r\n\t- Non-participation in FAS or certification schemes of farmers\r\n\r\nNOTE \r\nThe method is especially applicable for selecting risk based CwRS zones."@en ;
        skos:inScheme    cap-iacs-controlcode:SamplingStrategyTypeValue .

<http://lpis.ec.europa.eu/registry/applicationschema/cap-iacs-control/code#SampleTypeValue/observingGreening>
        a                cap-iacs-control:SampleTypeValue ;
        skos:definition  "Observing greening\r\n\r\nItems selected for controlling beneficiaries observing greening. The composition of the population\r\n\t- 1,0-1,25% selected randomly \r\n\t- 3,75-4,0% selected on risk base\r\nThe related sample includes items selected for the sensitive grassland sample."@en ;
        skos:inScheme    cap-iacs-controlcode:SampleTypeValue .

<http://lpis.ec.europa.eu/registry/applicationschema/cap-iacs-control/code#OnTheSpotCheckTypeValue/crossCompliance>
        a                cap-iacs-control:OnTheSpotCheckTypeValue ;
        rdfs:label       "Cross compliance"@en ;
        skos:definition  "Cross compliance\r\n\r\nOTSC in sense of Art. 96(3) of R 1306/2013."@en ;
        skos:inScheme    cap-iacs-controlcode:OnTheSpotCheckTypeValue .

<http://lpis.ec.europa.eu/registry/applicationschema/cap-iacs-control/code#ControlRateTypeValue/100%OfMandarotyReconversionIntoSensitivePermanentGrassland>
        a                cap-iacs-control:ControlRateTypeValue ;
        rdfs:label       "100 % of all beneficiaries with an obligation to re-convert land into land under permanent grassland, redistributive"@en ;
        skos:definition  "100% of mandatory reconversion into sensitive permanent grassland\r\n\r\nIn accordance with Art.31(1)(g) of R (EU) 809/2014 100 % of beneficiaries with an obligation to re-convert land into land under permanent grassland shall be controlled."@en ;
        skos:inScheme    cap-iacs-controlcode:ControlRateTypeValue .

<http://lpis.ec.europa.eu/registry/applicationschema/cap-iacs-control/code#OnTheSpotCheckTypeValue/crossComplianceStandards>
        a                cap-iacs-control:OnTheSpotCheckTypeValue ;
        rdfs:label       "Cross compliance"@en ;
        skos:definition  "Cross compliance standards\r\n\r\nAs required by Art. 24(1)(c) of R 809/2014."@en ;
        skos:inScheme    cap-iacs-controlcode:OnTheSpotCheckTypeValue .

<http://lpis.ec.europa.eu/registry/applicationschema/cap-iacs-control/code#CrossCheckTypeValue/betweenInterBranchOrganisationsAndTheListOfTheirMembers>
        a                cap-iacs-control:CrossCheckTypeValue ;
        rdfs:label       "Between inter-branch organisations and the list of their members"@en ;
        skos:definition  "-- Definition --\r\nBetween inter-branch organisations and the list of their members.\r\n-- Description --\r\nWhere appropriate, the administrative checks shall include cross-checks: the compliance with  the  criteria for the approval of inter-branch organisations and the list of their members shall be verified at least once every 5 years."@en ;
        skos:inScheme    cap-iacs-controlcode:CrossCheckTypeValue .

<http://lpis.ec.europa.eu/registry/applicationschema/cap-iacs-control/code#SampleTypeValue/topUpForBps/Saps>
        a                cap-iacs-control:SampleTypeValue ;
        skos:definition  "Top-up for BPS/SAPS\r\n\r\nRandomly selected items to complete the BPS/SAPS population after integrating the items out of the following samples: \r\n\t- Initial 1,0-2,15% sample for BPS SAPS\r\n\t- Greening samples\r\n\t- Redistributive payment\r\n\t- Areas with natural constraints\r\n\t- Young farmers\r\n\t- Voluntary couples support\r\n\t- Hemp\r\n\t- Cotton"@en ;
        skos:inScheme    cap-iacs-controlcode:SampleTypeValue .

<http://lpis.ec.europa.eu/registry/applicationschema/cap-iacs-control/code#OnTheSpotCheckTypeValue/commitmentsAndObligations>
        a                cap-iacs-control:OnTheSpotCheckTypeValue ;
        rdfs:label       "Cross compliance"@en ;
        skos:definition  "Cross compliance\r\n\r\nOTSC in sense of Art. 96(3) of R 1306/2013 and Art. 26(3) of R 809/2014."@en ;
        skos:inScheme    cap-iacs-controlcode:OnTheSpotCheckTypeValue .

cap-iacs-controlcode:SampleTypeValue
        a                skos:ConceptScheme ;
        dct:isFormatOf   cap-iacs-control:SampleTypeValue ;
        skos:definition  "Sample Type value\r\n\r\nThe sample type property shall be attributed to each sampled item (application). One item can be sampled to one or more payment/support schemes. \r\n\r\nNOTE\r\nThe categories of sample type values have to support the traceability of the sampling cascade. This is the reason for distinguishing the initial and the top-up samples for BPS/SAPS."@en .

<http://lpis.ec.europa.eu/registry/applicationschema/cap-iacs-control/code#RiskTypeValue/nonParticipationInCertificationScheme>
        a                cap-iacs-control:RiskTypeValue ;
        skos:definition  "Non-participation in certification scheme\r\n\r\nAt risk based sampling MS may consider beneficiary’s participation in a certification system if the scheme in question is relevant for the requirements and standards concerned [Art. 69(1)(b) of R 809/2014]."@en ;
        skos:inScheme    cap-iacs-controlcode:RiskTypeValue .

cap-iacs-controlcode:SamplingStrategyTypeValue
        a                skos:ConceptScheme ;
        rdfs:label       "List of sampling strategy types"@en ;
        dct:isFormatOf   cap-iacs-control:SamplingStrategyTypeValue ;
        skos:definition  "Sampling Strategy Type Value\r\n\r\nList of sampling strategy types.\r\n\r\nIn accordance with Preamble (34) of R 809/2014 sampling should comprise a random part in order to obtain a representative error rate and a risk based part for the following Payment/support schemes:\r\n\t- greening payment\r\n\t- animal aid schemes\r\n\t- rural development measure\r\n\r\nNOTE 1\r\nTo ensure a relevant and efficient risk analysis, the effectiveness of the risk analysis should be assessed and updated on an annual basis taking into account the relevance of each risk factor, comparing the results of randomly and risk-based selected samples and the specific situation [Preamble (68) and Art. 34(5) of R 809/2014].\r\n\r\nNOTE 2\r\nThe sampling method should be selected and documented by the competent authority of the MS/Region. The values of the code list can be extended.\r\n\r\nNOTE 3\r\nThe exemplary values of the code list in this application schema are taken from DSCG/2014/32 guideline and best statistical practices."@en .

<http://lpis.ec.europa.eu/registry/applicationschema/cap-iacs-control/code#SampleTypeValue/areasWithNaturalConstraints>
        a                cap-iacs-control:SampleTypeValue ;
        skos:definition  "Areas with natural constraints\r\n\r\nItem selected for controlling the correctness of payments for areas with natural constraints."@en ;
        skos:inScheme    cap-iacs-controlcode:SampleTypeValue .

cap-iacs-controlcode:InspectorsSurveyObjectTypeValue
        a                skos:ConceptScheme ;
        rdfs:label       "List of feature types"@en ;
        dct:isFormatOf   cap-iacs-control:InspectorsSurveyObjectTypeValue ;
        skos:definition  "Inspectors survey type value\r\n\r\nList of possible real objects measured by an inspector.\r\n\r\nNOTE\r\nList may be extended or subtracted depending on how MS organizing on-the-spot check process."@en .

<http://lpis.ec.europa.eu/registry/applicationschema/cap-iacs-control/code#ControlRateTypeValue/atLeast5%ForBps/Saps>
        a                cap-iacs-control:ControlRateTypeValue ;
        rdfs:label       "At least 5% of all beneficiaries required to observe the agricultural practices having areas covered with permanent grasslands"@en ;
        skos:definition  "At least 5% for BPS or SAPS\r\n\r\nIn sense of Art. 30(a) of Regulation (EU) 809/2014 5% of beneficiaries applying for the basic payment or single area payment scheme shall be controlled.\r\n\r\nThis control sample shall contain at least 5 % of all beneficiaries declaring mainly agricultural areas which are areas naturally kept in a state suitable for grazing in accordance with Article 10(1) of Delegated Regulation (EU) No 639/2014."@en ;
        skos:inScheme    cap-iacs-controlcode:ControlRateTypeValue .

<http://lpis.ec.europa.eu/registry/applicationschema/cap-iacs-control/code#SampleTypeValue/regional/NationalCertificationScheme>
        a                cap-iacs-control:SampleTypeValue ;
        skos:definition  "Regional/national certification scheme\r\n\r\nItems selected for controlling greening according to Art.43 (3)(b) of R 1307/2013. The equivalent practices are listed in Annex IX of this regulation and the AgriculturalEquivalentPracticeTypeValue code list of the Aid applications and payment claims application schema."@en ;
        skos:inScheme    cap-iacs-controlcode:SampleTypeValue .

<http://lpis.ec.europa.eu/registry/applicationschema/cap-iacs-control/code#InspectorsSurveyObjectTypeValue/ecologicalFocusArea>
        a                cap-iacs-control:InspectorsSurveyObjectTypeValue ;
        rdfs:label       "Ecological focus area"@en ;
        skos:definition  "Ecological focus area\r\n\r\nEcological focus areas as referred to in Article 46 of R (EU) No1307/2013 and its Delegated Regulation (EU) No 639/2014."@en ;
        skos:inScheme    cap-iacs-controlcode:InspectorsSurveyObjectTypeValue .

<http://lpis.ec.europa.eu/registry/applicationschema/cap-iacs-control/code#CrossCheckTypeValue/betweenThePaymentEntitlementsAndTheAreaDetermined>
        a                cap-iacs-control:CrossCheckTypeValue ;
        rdfs:label       "Between the payment entitlements and the area determined"@en ;
        skos:definition  "-- Definition --\r\nBetween the payment entitlements and the area determined.\r\n-- Description --\r\nWhere appropriate, the administrative checks shall include cross-checks:between the payment entitlements and the area determined in order to verify that the entitlements are accompanied by at least an equal number of eligible hectares \r\r\nas defined in Article 32(2) to (6) of Regulation (EC) No 1307/2013."@en ;
        skos:inScheme    cap-iacs-controlcode:CrossCheckTypeValue .

<http://lpis.ec.europa.eu/registry/applicationschema/cap-iacs-control/code#ControlRateTypeValue/atLeast5%OfCollectiveImplementation>
        a                cap-iacs-control:ControlRateTypeValue ;
        rdfs:label       "At least 5 % of  the  collective implementation"@en ;
        skos:definition  "At least 5 % of the collective implementation\r\n\r\nIn sensed of Art. 31(1)(e) od R EU) 809/2014 5 % of  the  collective implementation in accordance with Article 46(6) of Regulation (EU) No 1307/2013 shall be controlled."@en ;
        skos:inScheme    cap-iacs-controlcode:ControlRateTypeValue .

<http://lpis.ec.europa.eu/registry/applicationschema/cap-iacs-control/code#SamplingStrategyTypeValue/systematicRandomBasedSelection>
        a                cap-iacs-control:SamplingStrategyTypeValue ;
        skos:definition  "Systematic random selection\r\n\r\nRandom selection of the first initial item (i.e. application) and taking the rest based on the sequential number (e.g. every 100 application) [Section 1.3.2 of DSCG/2014/32].\r\n\r\nNOTE 1\r\nThis method allows to start OTSC before the end of the application period.\r\n\r\nNOTE 2\r\nThe sequential number has to be automatically assigned to the applications, or the key (i.e. property or properties) that serve for the basis of selection has to be specified and documented before starting the sampling process.\r\n\r\nNOTE 3\r\nThe population has to be homogenous."@en ;
        skos:inScheme    cap-iacs-controlcode:SamplingStrategyTypeValue .

<http://lpis.ec.europa.eu/registry/applicationschema/cap-iacs-control/code>
        a       owl:Ontology ;
        rdfs:label       "Integrated control system code lists"@en ;
        owl:versionIRI   "http://lpis.ec.europa.eu/registry/applicationschema/cap-iacs-base/code/3.0" ;
        owl:versionInfo  "3.0" ;
        dct:creator [ schema:affiliation [ foaf:name "PSNC" ] ;
                      rdfs:seeAlso <http://orcid.org/0000-0003-4289-4922> ;
                      foaf:name "Raul Palma"
                    ] ;
        dct:title "JRC IACS - Integrated Control System Code Lists"@en ;
        dct:description "Ontology of the integrated control system code lists used in IACS, generated from the transformation of the corresponding JRC application schema"@en ;
        dct:source "JRC IACS application schema. https://doi.org/10.1016/j.landusepol.2016.05.023"@en ;
        dct:rights "This ontology is distributed under Creative Commons Attribution 4.0 License - http://creativecommons.org/licenses/by/4.0"@en .

<http://lpis.ec.europa.eu/registry/applicationschema/cap-iacs-control/code#OnTheSpotCheckTypeValue/controlArea>
        a                cap-iacs-control:OnTheSpotCheckTypeValue ;
        rdfs:label       "Control area"@en ;
        skos:definition  "Control area\r\n\r\nVerification of the declared area values by means of measurements."@en ;
        skos:inScheme    cap-iacs-controlcode:OnTheSpotCheckTypeValue .

<http://lpis.ec.europa.eu/registry/applicationschema/cap-iacs-control/code#ControlRateTypeValue/atLeast5%ForRedistributivePayment>
        a                cap-iacs-control:ControlRateTypeValue ;
        rdfs:label       "At least 5% of all beneficiaries required to observe the agricultural practices having areas covered with permanent grasslands"@en ;
        skos:definition  "At least 5% for the redistributive payment\r\n\r\nIn sense of Art. 30(b) of Regulation (EU) 809/2014 5% of beneficiaries applying for the redistributive payment shall be controlled."@en ;
        skos:inScheme    cap-iacs-controlcode:ControlRateTypeValue .

<http://lpis.ec.europa.eu/registry/applicationschema/cap-iacs-control/code#ControlRateTypeValue/atLeast5%ForVoluntaryCoupledSupport>
        a                cap-iacs-control:ControlRateTypeValue ;
        rdfs:label       "At least 5% of all beneficiaries required to observe the agricultural practices having areas covered with permanent grasslands"@en ;
        skos:definition  "At least 5% for the voluntary coupled support\r\n\r\nIn sense of Art. 30(e) of Regulation (EU) 809/2014 5% of beneficiaries applying for the voluntary coupled shall be controlled."@en ;
        skos:inScheme    cap-iacs-controlcode:ControlRateTypeValue .

<http://lpis.ec.europa.eu/registry/applicationschema/cap-iacs-control/code#ControlRateTypeValue/100%OfTheContiguousStructuresOfAdjacentEfa>
        a                cap-iacs-control:ControlRateTypeValue ;
        rdfs:label       "100 % of the contiguous structures of adjacent ecological focus areas"@en ;
        skos:definition  "100 % of the contiguous structures of adjacent EFA\r\n\r\nIn sense of Art. 31(1)(f) of R (EU) 809/2014  100 % of the contiguous structures of adjacent ecological focus areas as referred to in Article 46(5) of Regulation (EU) 1307/2013 shall be controlled."@en ;
        skos:inScheme    cap-iacs-controlcode:ControlRateTypeValue .

<http://lpis.ec.europa.eu/registry/applicationschema/cap-iacs-control/code#SampleTypeValue/voluntaryCoupledSupport>
        a                cap-iacs-control:SampleTypeValue ;
        skos:definition  "Voluntary coupled support\r\n\r\nItem selected for controlling beneficiaries applying for voluntary coupled support."@en ;
        skos:inScheme    cap-iacs-controlcode:SampleTypeValue .

<http://lpis.ec.europa.eu/registry/applicationschema/cap-iacs-control/code#SampleTypeValue/collectiveImplementation>
        a                cap-iacs-control:SampleTypeValue ;
        skos:definition  "Collective implementation\r\n\r\nItems selected for controlling beneficiaries participating in collective implementation of EFA. The composition of the population\r\n\t- 1,0-1,25% selected randomly \r\n\t- 3,75-4,0% selected on risk base\r\n\r\nIssue:\r\nThe purpose of collective implementation (See Art. 46(a) of 1307/2013) and regional implementation (see Art. 46(3) of R 639/2014) is to form contiguous areas of EFA. If so, what is the reason to have separate samples for collective implementation, regional implementation and contiguous EFA?"@en ;
        skos:inScheme    cap-iacs-controlcode:SampleTypeValue .

<http://lpis.ec.europa.eu/registry/applicationschema/cap-iacs-control/code#RiskTypeValue/nonParticipationInFas>
        a                cap-iacs-control:RiskTypeValue ;
        skos:definition  "Non participation in FAS\r\n\r\nSampling of OTSC for cross-compliance can be improved by taking into account the risk analysis concerning the beneficiary’s participation in the farm advisory system [Preamble (69) and Art. 69(1)(a) of R 809/2014]."@en ;
        skos:inScheme    cap-iacs-controlcode:RiskTypeValue .

<http://lpis.ec.europa.eu/registry/applicationschema/cap-iacs-control/code#ControlRateTypeValue/atLeast3%ForRedistributivePayment>
        a                cap-iacs-control:ControlRateTypeValue ;
        rdfs:label       "At least 5% of all beneficiaries required to observe the agricultural practices having areas covered with permanent grasslands"@en ;
        skos:definition  "At least 3% or redistributive payment \r\n\r\nArt. 36(2) of Regulation (EU) 809/2014 allows the reduction of the control rate for redistributive payment from 5% to 3% when the cross checks based on geospatial applications are carried out."@en ;
        skos:inScheme    cap-iacs-controlcode:ControlRateTypeValue .

<http://lpis.ec.europa.eu/registry/applicationschema/cap-iacs-control/code#SamplingStrategyTypeValue/riskBasedCartSelection>
        a                cap-iacs-control:SamplingStrategyTypeValue ;
        rdfs:label       "Risk based sampling strategy"@en ;
        skos:definition  "Risk based CART selection\r\n\r\nA probability proportional risk based method for selecting and grouping items (applications) in risk groups based on a specific criterion (e.g. area not found) [DSCG/2014/32]."@en ;
        skos:inScheme    cap-iacs-controlcode:SamplingStrategyTypeValue .

<http://lpis.ec.europa.eu/registry/applicationschema/cap-iacs-control/code#ControlRateTypeValue/atLeast20%ForProductionOfHemp>
        a                cap-iacs-control:ControlRateTypeValue ;
        rdfs:label       "At least 5% of all beneficiaries required to observe the agricultural practices having areas covered with permanent grasslands"@en ;
        skos:definition  "At least 20% for production of hemp\r\n\r\nArt. 36(6) of Regulation (EU) 809/2014 allows the reduction of the control rate for production of hemp from 30% to 20% when a MS introduces a prior approval for the cultivation of hemp.\r\n\r\nNOTE\r\nMS shall notify the EC about the rules (or changes in the rules) of the approval system."@en ;
        skos:inScheme    cap-iacs-controlcode:ControlRateTypeValue .

<http://lpis.ec.europa.eu/registry/applicationschema/cap-iacs-control/code#CrossCheckTypeValue/toVerifyEligibilityForTheAnimalAid>
        a                cap-iacs-control:CrossCheckTypeValue ;
        rdfs:label       "Verify eligibility for the animal aid"@en ;
        skos:definition  "-- Definition --\r\nVerify eligibility for the animal aid.\r\n-- Description --\r\nWhere appropriate, the administrative checks shall include cross-checks: by means of the system for the identification and registration of animals, to verify eligibility for the aid and/or support and to avoid undue multiple granting of \r\r\nthe same aid and/or support in respect of the same calendar or claim year."@en ;
        skos:inScheme    cap-iacs-controlcode:CrossCheckTypeValue .

<http://lpis.ec.europa.eu/registry/applicationschema/cap-iacs-control/code#SamplingStrategyTypeValue/clusteredRandomSelection>
        a                cap-iacs-control:SamplingStrategyTypeValue ;
        skos:definition  "Clustered random selection\r\n\r\nCluster sampling is a selection of items that are clustered (e.g. spatially or temporally) within the population.\r\n\r\nEXAMPLE\r\nGeographic cluster of a CwRS zone.\r\n\r\nNOTE 1\r\nThe criteria for each cluster has to be registered.\r\n\r\nNOTE 2\r\nThe clusters regarded as primary samples by geographic or temporal distribution can be further sampled by a second level of sampling. In that case the method is called multistage sampling."@en ;
        skos:inScheme    cap-iacs-controlcode:SamplingStrategyTypeValue .

<http://lpis.ec.europa.eu/registry/applicationschema/cap-iacs-control/code#InspectorsSurveyObjectTypeValue/agriculturalParcel>
        a                cap-iacs-control:InspectorsSurveyObjectTypeValue ;
        rdfs:label       "Agricultural parcel"@en ;
        skos:definition  "Agricultural parcel\r\n\r\nAgricultural parcel as defined by R (EU) 1307/2013."@en ;
        skos:inScheme    cap-iacs-controlcode:InspectorsSurveyObjectTypeValue .

<http://lpis.ec.europa.eu/registry/applicationschema/cap-iacs-control/code#SampleTypeValue/reconversionOfPg>
        a                cap-iacs-control:SampleTypeValue ;
        skos:definition  "Reconversion of permanent grassland\r\n\r\nItems corresponding to beneficiaries obliged to re-convert agricultural areas in permanent grassland."@en ;
        skos:inScheme    cap-iacs-controlcode:SampleTypeValue .

cap-iacs-controlcode:ControlRateGroupAnimalAidSchemaValue
        a                skos:ConceptScheme ;
        rdfs:label       "List of control rate groups for animal aid schemas"@en ;
        dct:isFormatOf   cap-iacs-control:ControlRateGroupAnimalAidSchemaValue ;
        skos:definition  "Control Rate Group Animal Aid Scheme Value\r\n\r\nList of control rate groups for animal aid schemas.\r\n\r\nNOTE\r\nCurrently placeholder only."@en .

<http://lpis.ec.europa.eu/registry/applicationschema/cap-iacs-control/code#SampleTypeValue/smallFarmers>
        a                cap-iacs-control:SampleTypeValue ;
        skos:definition  "Small farmers\r\n\r\nItem selected for controlling beneficiaries participating in the small farmers scheme."@en ;
        skos:inScheme    cap-iacs-controlcode:SampleTypeValue .

cap-iacs-controlcode:OnTheSpotCheckTypeValue
        a                skos:ConceptScheme ;
        rdfs:label       "List of on the spot check types"@en ;
        dct:isFormatOf   cap-iacs-control:OnTheSpotCheckTypeValue ;
        skos:definition  "On-the-spot check type value\r\n\r\nList of on the spot check types. that describe the purpose of the control."@en .

<http://lpis.ec.europa.eu/registry/applicationschema/cap-iacs-control/code#SamplingStrategyTypeValue/multistageSampling>
        a                cap-iacs-control:SamplingStrategyTypeValue ;
        skos:definition  "Multistage sampling\r\n\r\nFurther, secondary sampling of clusters that have been  selected on geographic, or temporal criteria."@en ;
        skos:inScheme    cap-iacs-controlcode:SamplingStrategyTypeValue .

<http://lpis.ec.europa.eu/registry/applicationschema/cap-iacs-control/code#SampleTypeValue/cotton>
        a                cap-iacs-control:SampleTypeValue ;
        skos:definition  "Cotton\r\n\r\nItem selected for controlling beneficiaries applying for the specific payment for cotton."@en ;
        skos:inScheme    cap-iacs-controlcode:SampleTypeValue .

<http://lpis.ec.europa.eu/registry/applicationschema/cap-iacs-control/code#OnTheSpotCheckTypeValue/complianceToEuLaw>
        a                cap-iacs-control:OnTheSpotCheckTypeValue ;
        rdfs:label       "Cross compliance"@en ;
        skos:definition  "Compliance to EU law\r\n\r\nAs required by Art. 24(2) of R 809/2014."@en ;
        skos:inScheme    cap-iacs-controlcode:OnTheSpotCheckTypeValue .

<http://lpis.ec.europa.eu/registry/applicationschema/cap-iacs-control/code#ControlRateTypeValue/atLeast5%ForYoungFarmers>
        a                cap-iacs-control:ControlRateTypeValue ;
        rdfs:label       "At least 5% of all beneficiaries required to observe the agricultural practices having areas covered with permanent grasslands"@en ;
        skos:definition  "At least 5% for the young farmers\r\n\r\nIn sense of Art. 30(d) of Regulation (EU) 809/2014 5% of beneficiaries applying for the young farmer payment shall be controlled."@en ;
        skos:inScheme    cap-iacs-controlcode:ControlRateTypeValue .

<http://lpis.ec.europa.eu/registry/applicationschema/cap-iacs-control/code#CrossCheckTypeValue/toVerifyEligibilityForTheIncreaseOfTheAid>
        a                cap-iacs-control:CrossCheckTypeValue ;
        rdfs:label       "Verify eligibility for the increase of the aid"@en ;
        skos:definition  "-- Definition --\r\nVerify eligibility for the increase of the aid.\r\n-- Description --\r\nWhere appropriate, the administrative checks shall include cross-checks:between the declarations of the beneficiary in the single application to be a member of an approved inter-branch organisation, the information under Article 16(8) \r\r\nof this Regulation and the information transmitted by the approved inter-branch organisations concerned, to verify eligibility for the increase of the aid provided for in Article 60(2) of Regulation (EU) No 1307/2013."@en ;
        skos:inScheme    cap-iacs-controlcode:CrossCheckTypeValue .

<http://lpis.ec.europa.eu/registry/applicationschema/cap-iacs-control/code#SamplingStrategyTypeValue/simpleRandomBasedSelection>
        a                cap-iacs-control:SamplingStrategyTypeValue ;
        rdfs:label       "Random based sampling strategy"@en ;
        skos:definition  "Simple random based selection\r\n\r\nSelection from the full population of the dossiers through generation of a random key [Section 1.3.2 of DSCG/2014/32].\r\n\r\nNOTE 1\r\nThe population has to be homogenous for this method.\r\n\r\nNOTE 2\r\nThis method requires waiting until the full population is known."@en ;
        skos:inScheme    cap-iacs-controlcode:SamplingStrategyTypeValue .

<http://lpis.ec.europa.eu/registry/applicationschema/cap-iacs-control/code#SampleTypeValue/redistributivePayment>
        a                cap-iacs-control:SampleTypeValue ;
        skos:definition  "Redistributive payment\r\n\r\nItem selected for controlling beneficiaries applying for redistributive payment."@en ;
        skos:inScheme    cap-iacs-controlcode:SampleTypeValue .

<http://lpis.ec.europa.eu/registry/applicationschema/cap-iacs-control/code#ControlRateTypeValue/atLeast10%OfCollectiveImplementation>
        a                cap-iacs-control:ControlRateTypeValue ;
        rdfs:label       "At least 5 % of  the  collective implementation"@en ;
        skos:definition  "At least 10% of the collective implementation\r\n\r\nIncreased control rate (5% normal+5% supplementary) in sense of Art. 31(3) for beneficiaries required to follow greening practices."@en ;
        skos:inScheme    cap-iacs-controlcode:ControlRateTypeValue .

<http://lpis.ec.europa.eu/registry/applicationschema/cap-iacs-control/code#OnTheSpotCheckTypeValue/correctnessAndCompletenessOfInformation>
        a                cap-iacs-control:OnTheSpotCheckTypeValue ;
        rdfs:label       "Cross compliance"@en ;
        skos:definition  "Correctness and completeness of the information\r\n\r\nAs required by Art. 24(1)(a) of R 809/2014."@en ;
        skos:inScheme    cap-iacs-controlcode:OnTheSpotCheckTypeValue .

<http://lpis.ec.europa.eu/registry/applicationschema/cap-iacs-control/code#SampleTypeValue/exemptedFromGreening>
        a                cap-iacs-control:SampleTypeValue ;
        skos:definition  "Exempted from greening\r\n\r\nItems selected to control beneficiaries exempted from greening obligations by not meeting the specified thresholds.  They include:\r\n\t- Beneficiaries exempted from crop diversification (Art. 44(3) of R 1307/2013)\r\n\t- Beneficiaries exempted from EFA (Art. 46 (1) of R 307/2013)"@en ;
        skos:inScheme    cap-iacs-controlcode:SampleTypeValue .

<http://lpis.ec.europa.eu/registry/applicationschema/cap-iacs-control/code#CrossCheckTypeValue/toVerifyDeclaredEntitlementsOnDeclaredAgriculturalParcels>
        a                cap-iacs-control:CrossCheckTypeValue ;
        rdfs:label       "Verify declared payment entitlements on declared agricultural parcels"@en ;
        skos:definition  "-- Definition --\r\nVerify declared payment entitlements on declared agricultural parcels.\r\n-- Description --\r\nWhere appropriate, the administrative checks shall include cross-checks:o n declared payment entitlements and on declared agricultural parcels, respectively, in order to avoid multiple granting of the same aid or support in respect of \r\r\nthe same calendar or claim year and to prevent any undue accumulation of aid granted under area-related aid schemes listed in Annex I to Regulation (EU) No 1307/2013 and Annex VI to Council Regulation (EC) No 73/2009[17], and area-\r\r\nrelated support measures as defined in point (21) of the second subparagraph of Article 2 of Delegated Regulation (EU) No […] [DA IACS]."@en ;
        skos:inScheme    cap-iacs-controlcode:CrossCheckTypeValue .

<http://lpis.ec.europa.eu/registry/applicationschema/cap-iacs-control/code#ControlRateTypeValue/atLeast10%OfFollowingGreeningByUsingEnvironmentalCertificationSchemes>
        a                cap-iacs-control:ControlRateTypeValue ;
        rdfs:label       "At least 5 % of all beneficiaries required to observe the greening practices and using national or regional environmental certification schemes"@en ;
        skos:definition  "At least 10 % following greening practices by using environmental certification schemes\r\n\r\nIncreased control rate (5% normal+5% supplementary) in sense of Art. 31(3) for beneficiaries required to follow greening practices."@en ;
        skos:inScheme    cap-iacs-controlcode:ControlRateTypeValue .

<http://lpis.ec.europa.eu/registry/applicationschema/cap-iacs-control/code#InspectorsSurveyObjectTypeValue/referenceParcel>
        a                cap-iacs-control:InspectorsSurveyObjectTypeValue ;
        rdfs:label       "Reference parcel"@en ;
        skos:definition  "Reference parcel\r\n\r\nReference parcel as defined in R (EU) 1307/2013."@en ;
        skos:inScheme    cap-iacs-controlcode:InspectorsSurveyObjectTypeValue .

cap-iacs-controlcode:ControlRateTypeValue
        a                skos:ConceptScheme ;
        rdfs:label       "List of control rate groups for greening"@en ;
        dct:isFormatOf   cap-iacs-control:ControlRateTypeValue ;
        skos:definition  "Control rate type value\r\n\r\nList of applicable control rate values as prescribed by Art. 30, 31, 36(2) and 36(6) of R 809/2014.\r\n\r\nNOTE\r\nThis code list currently does not contain values for rural development measures (Art. 32) and animal aid schemes (Art. 33 of R 809/2014)."@en .

<http://lpis.ec.europa.eu/registry/applicationschema/cap-iacs-control/code#OnTheSpotCheckTypeValue/supportingDocuments>
        a                cap-iacs-control:OnTheSpotCheckTypeValue ;
        rdfs:label       "Control cross-compliance"@en ;
        skos:definition  "Supporting Documents\r\n\r\nVerification of the existence of the requisite supporting documents [Art. 47(1)(b) of  R 1306/2013]"@en ;
        skos:inScheme    cap-iacs-controlcode:OnTheSpotCheckTypeValue .

<http://lpis.ec.europa.eu/registry/applicationschema/cap-iacs-control/code#ControlRateTypeValue/atLeast10%OfFollowingGreeningPractices>
        a                cap-iacs-control:ControlRateTypeValue ;
        rdfs:label       "At least 5% of all beneficiaries required to observe the agricultural practices having areas covered with permanent grasslands"@en ;
        skos:definition  "At least 10% of following greening practices\r\n\r\nIncreased control rate (5% normal+5% supplementary) in sense of Art. 31(3) of R 809/2014 for beneficiaries required to follow greening practices. \r\n\r\nWhere the ecological focus areas are not identified in the identification system for agricultural parcels as referred to in Article 70 of Regulation (EU) No 1306/2013, the control rate laid down in points (a) and (c) to (e) of paragraph 1 shall be supplemented by 5% of all beneficiaries of the respective control sample who are required to have ecological focus area on the agricultural area in accordance with Articles 43 and 46 of Regulation (EU) No 1307/2013."@en ;
        skos:inScheme    cap-iacs-controlcode:ControlRateTypeValue .

<http://lpis.ec.europa.eu/registry/applicationschema/cap-iacs-control/code#ControlRateTypeValue/atLeast5%ForAreasWithNaturalConstraints>
        a                cap-iacs-control:ControlRateTypeValue ;
        rdfs:label       "At least 5% of all beneficiaries required to observe the agricultural practices having areas covered with permanent grasslands"@en ;
        skos:definition  "At least 5% for areas with natural constraints \r\n\r\nIn sense of Art. 30(c) of Regulation (EU) 809/2014 5% of beneficiaries applying for the payment for areas with natural constraints shall be controlled."@en ;
        skos:inScheme    cap-iacs-controlcode:ControlRateTypeValue .

<http://lpis.ec.europa.eu/registry/applicationschema/cap-iacs-control/code#SampleTypeValue/youngFarmers>
        a                cap-iacs-control:SampleTypeValue ;
        skos:definition  "Young farmers\r\n\r\nItem selected for controlling beneficiaries applying for young farmer payment."@en ;
        skos:inScheme    cap-iacs-controlcode:SampleTypeValue .

<http://lpis.ec.europa.eu/registry/applicationschema/cap-iacs-control/code#InspectorsSurveyObjectTypeValue/holdingSite>
        a                cap-iacs-control:InspectorsSurveyObjectTypeValue ;
        rdfs:label       "Holding site"@en ;
        skos:definition  "Holding site\r\n\r\nMeasurement of the whole holding."@en ;
        skos:inScheme    cap-iacs-controlcode:InspectorsSurveyObjectTypeValue .

<http://lpis.ec.europa.eu/registry/applicationschema/cap-iacs-control/code#CrossCheckTypeValue/toVerifyPaymentEntitlements>
        a                cap-iacs-control:CrossCheckTypeValue ;
        rdfs:label       "Verify payment entitlements"@en ;
        skos:definition  "-- Definition --\r\nVerify payment entitlements.\r\n-- Description --\r\nWhere appropriate, the administrative checks shall include cross-checks: on the payment entitlements to verify their existence and the eligibility."@en ;
        skos:inScheme    cap-iacs-controlcode:CrossCheckTypeValue .

<http://lpis.ec.europa.eu/registry/applicationschema/cap-iacs-control/code#ControlRateTypeValue/atLeast5%OfFollowingGreeningPractices>
        a                cap-iacs-control:ControlRateTypeValue ;
        rdfs:label       "At least 5% of all beneficiaries required to observe the agricultural practices having areas covered with permanent grasslands"@en ;
        skos:definition  "At least 5% of following greening practices\r\n\r\nIn sense of Art. 31(1) 5% of beneficiaries required to follow greening practices shall be controlled."@en ;
        skos:inScheme    cap-iacs-controlcode:ControlRateTypeValue .

<http://lpis.ec.europa.eu/registry/applicationschema/cap-iacs-control/code#ControlRateTypeValue/atLeast5%OfFollowingGreeningByUsingEnvironmentalCertificationSchemes>
        a                cap-iacs-control:ControlRateTypeValue ;
        rdfs:label       "At least 5 % of all beneficiaries required to observe the greening practices and using national or regional environmental certification schemes"@en ;
        skos:definition  "At least 5 % following greening practices by using environmental certification schemes\r\n\r\nIn sense of Art. 31(1)(c) 5 % of beneficiaries observing greening practices and using national or regional environmental certification schemes as referred to in Article 43(3)(b) of Regulation (EU) No 1307/2013 shall be controlled."@en ;
        skos:inScheme    cap-iacs-controlcode:ControlRateTypeValue .

<http://lpis.ec.europa.eu/registry/applicationschema/cap-iacs-control/code#SampleTypeValue/regionalImplementation>
        a                cap-iacs-control:SampleTypeValue ;
        skos:definition  "Regional implementation\r\n\r\nItems selected for controlling beneficiaries participating in regional implementation of EFA. The composition of the population\r\n\t- 1,0-1,25% selected randomly \r\n\t- 3,75-4,0% selected on risk base\r\n\r\nIssue:\r\nThe purpose of collective implementation (See Art. 46(a) of 1307/2013) and regional implementation (see Art. 46(3) of R 639/2014) is to form contiguous areas of EFA. If so, what is the reason to have separate samples for collective implementation, regional implementation and contiguous EFA?"@en ;
        skos:inScheme    cap-iacs-controlcode:SampleTypeValue .

<http://lpis.ec.europa.eu/registry/applicationschema/cap-iacs-control/code#SurveyMethodValue/rapidFieldVisit>
        a                cap-iacs-control:SurveyMethodValue ;
        rdfs:label       "Combined field measurement and CwRS"@en ;
        skos:definition  "Rapid field visit\r\n\r\nCombined measurement using field (e.g. GNSS)and  Remote Sensing methods.\r\n\r\nNOTE 1\r\nIn the event that photo-interpretation of orthoimages (satellite or aerial) do not provide results that would permit definitive conclusions to be drawn to the satisfaction of the competent authority concerning the eligibility or the correct size of the area that is the subject of administrative or on-the-spot checks [Art. 24(4) of R 809/2014].\r\n\r\nNOTE 2\r\nIt follows an inconclusive CAPI."@en ;
        skos:inScheme    cap-iacs-controlcode:SurveyMethodValue .

<http://lpis.ec.europa.eu/registry/applicationschema/cap-iacs-control/code#ControlRateTypeValue/atLeast5%ForCropSpecificCottonPayment>
        a                cap-iacs-control:ControlRateTypeValue ;
        rdfs:label       "At least 5% of all beneficiaries required to observe the agricultural practices having areas covered with permanent grasslands"@en ;
        skos:definition  "At least 5% for crop specific cotton payment\r\n\r\nIn sense of Art. 30(h) of Regulation (EU) 809/2014 5% of beneficiaries applying for the crop specific payment for cotton shall be controlled."@en ;
        skos:inScheme    cap-iacs-controlcode:ControlRateTypeValue .

<http://lpis.ec.europa.eu/registry/applicationschema/cap-iacs-control/code#ControlRateGroupRuralDevelopmentMeasureValue/placeholder>
        a              cap-iacs-control:ControlRateGroupRuralDevelopmentMeasureValue ;
        rdfs:label     "Currently out of scope"@en ;
        skos:inScheme  cap-iacs-controlcode:ControlRateGroupRuralDevelopmentMeasureValue .

<http://lpis.ec.europa.eu/registry/applicationschema/cap-iacs-control/code#InspectorsSurveyObjectTypeValue/agriculturalArea>
        a                cap-iacs-control:InspectorsSurveyObjectTypeValue ;
        rdfs:label       "Agricultural area"@en ;
        skos:definition  "Agricultural area\r\n\r\nAgricultural area as defined by R (EU) 1307/2013."@en ;
        skos:inScheme    cap-iacs-controlcode:InspectorsSurveyObjectTypeValue .

<http://lpis.ec.europa.eu/registry/applicationschema/cap-iacs-control/code#ControlRateTypeValue/atLeast3%OfExemptedFromGreeningPractices>
        a                cap-iacs-control:ControlRateTypeValue ;
        rdfs:label       "At least 3 % of all beneficiaries qualifying for the greening payment who are exempted from both the crop diversification and the EFA obligations"@en ;
        skos:definition  "At least 3% of exempted from greening practices\r\n\r\nIn sense of Art. 31 (1)(b) at least 3 % of all beneficiaries qualifying for the greening payment who are exempted from both the crop diversification and the EFA obligations shall be controlled.\r\n\r\nThe exemption is granted when the thresholds referred to in Articles 44 and 46 of Regulation (EU) No 1307/2013 are not met and the obligations referred to in Article 45 of that Regulation are not concerned."@en ;
        skos:inScheme    cap-iacs-controlcode:ControlRateTypeValue .

<http://lpis.ec.europa.eu/registry/applicationschema/cap-iacs-control/code#SampleTypeValue/reconversionOfSensitivePg>
        a                cap-iacs-control:SampleTypeValue ;
        skos:definition  "Reconversion of sensitive permanent grassland\r\n\r\nItems corresponding to beneficiaries obliged to re-convert agricultural areas in sensitive permanent grassland."@en ;
        skos:inScheme    cap-iacs-controlcode:SampleTypeValue .

<http://lpis.ec.europa.eu/registry/applicationschema/cap-iacs-control/code#RiskTypeValue/eligibilityCriteria>
        a                cap-iacs-control:RiskTypeValue ;
        skos:definition  "Eligibility Criteria\r\n\r\nMember States are also authorised to draw the control sample on the basis of the samples of beneficiaries that are selected for an on-the-spot check as regards eligibility criteria. [Preamble (71) of R 809/2014]."@en ;
        skos:inScheme    cap-iacs-controlcode:RiskTypeValue .

<http://lpis.ec.europa.eu/registry/applicationschema/cap-iacs-control/code#OnTheSpotCheckTypeValue/complianceToNationalLaw>
        a                cap-iacs-control:OnTheSpotCheckTypeValue ;
        rdfs:label       "Cross compliance"@en ;
        skos:definition  "Compliance to national law\r\n\r\nAs required by Art. 24(2) of R 809/2014."@en ;
        skos:inScheme    cap-iacs-controlcode:OnTheSpotCheckTypeValue .

cap-iacs-controlcode:ControlRateGroupRuralDevelopmentMeasureValue
        a                skos:ConceptScheme ;
        rdfs:label       "List of control rate groups for rural development measures"@en ;
        dct:isFormatOf   cap-iacs-control:ControlRateGroupRuralDevelopmentMeasureValue ;
        skos:definition  "Control Rate Group Rural Development Measure Value\r\n\r\nList of control rate groups for rural development measures.\r\n\r\nNOTE. Currently placeholder only."@en .

<http://lpis.ec.europa.eu/registry/applicationschema/cap-iacs-control/code#ControlRateTypeValue/atLeast5%OfRegionalImplementation>
        a                cap-iacs-control:ControlRateTypeValue ;
        rdfs:label       "At least  5 % of all beneficiaries participating in a regional implementation"@en ;
        skos:definition  "At least 5 % of all beneficiaries participating in a regional implementation\r\n\r\nIn sense of Art.31(1)(d)  of R (EU) 809/2014 5 % of all beneficiaries participating in a regional implementation in accordance with Article 46(5) of Regulation (EU) No 1307/2013 shall be controlled."@en ;
        skos:inScheme    cap-iacs-controlcode:ControlRateTypeValue .

<http://lpis.ec.europa.eu/registry/applicationschema/cap-iacs-control/code#ControlRateTypeValue/atLeast10%OfRegionalImplementation>
        a                cap-iacs-control:ControlRateTypeValue ;
        rdfs:label       "At least  5 % of all beneficiaries participating in a regional implementation"@en ;
        skos:definition  "At least 10 % of all beneficiaries participating in a regional implementation\r\n\r\nIncreased control rate (5% normal+5% supplementary) in sense of Art. 31(3) for beneficiaries required to follow greening practices."@en ;
        skos:inScheme    cap-iacs-controlcode:ControlRateTypeValue .

cap-iacs-controlcode:SurveyMethodValue
        a                skos:ConceptScheme ;
        rdfs:label       "List of survey types"@en ;
        dct:isFormatOf   cap-iacs-control:SurveyMethodValue ;
        skos:definition  "Survey method value\r\n\r\nList of survey method types in sense of Art. 74(3) of R 1306/2013."@en .

<http://lpis.ec.europa.eu/registry/applicationschema/cap-iacs-control/code#SampleTypeValue/initial1%And1,25%ForBps/Saps>
        a                cap-iacs-control:SampleTypeValue ;
        skos:definition  "Initial 1% and 1,25% for BPS/SAPS\r\n\r\nIt is the initial random sample drawn in sense of Art. 24(2)(a). This sample constitutes the basis of the following further samples:\r\n\t- Random part of the greening samples\r\n\t- Redistributive payment\r\n\t- Areas with natural constraints\r\n\t- Young farmers\r\n\t- Voluntary couples support\r\n\t- Hemp\r\n\t- Cotton"@en ;
        skos:inScheme    cap-iacs-controlcode:SampleTypeValue .

<http://lpis.ec.europa.eu/registry/applicationschema/cap-iacs-control/code#ControlRateGroupAnimalAidSchemaValue/placeholder>
        a              cap-iacs-control:ControlRateGroupAnimalAidSchemaValue ;
        rdfs:label     "Currently out of scope"@en ;
        skos:inScheme  cap-iacs-controlcode:ControlRateGroupAnimalAidSchemaValue .

<http://lpis.ec.europa.eu/registry/applicationschema/cap-iacs-control/code#ControlRateTypeValue/atLeast3%ForSmallFarmersScheme>
        a                cap-iacs-control:ControlRateTypeValue ;
        rdfs:label       "At least 5% of all beneficiaries required to observe the agricultural practices having areas covered with permanent grasslands"@en ;
        skos:definition  "At least 3% for small farmer scheme\r\n\r\nArt. 36(2) of Regulation (EU) 809/2014 allows the reduction of the control rate for the small farmer scheme  from 5% to 3% when the cross checks based on geospatial applications are carried out."@en ;
        skos:inScheme    cap-iacs-controlcode:ControlRateTypeValue .

<http://lpis.ec.europa.eu/registry/applicationschema/cap-iacs-control/code#SamplingStrategyTypeValue/stratifiedRandomSelection>
        a                cap-iacs-control:SamplingStrategyTypeValue ;
        skos:definition  "Stratified random selection\r\n\r\nMethod applicable when the population to be sampled is not homogenous. In order to achieve homogeneity, the population has to be sub-divided into strata based on objective criteria.\r\n\r\nNOTE\r\nThe criteria for each stratum has to be registered."@en ;
        skos:inScheme    cap-iacs-controlcode:SamplingStrategyTypeValue .

<http://lpis.ec.europa.eu/registry/applicationschema/cap-iacs-control/code#ControlRateTypeValue/atLeast20%OfMandarotyReconversionIntoPermanentGrassland>
        a                cap-iacs-control:ControlRateTypeValue ;
        rdfs:label       "100 % of all beneficiaries with an obligation to re-convert land into land under permanent grassland, redistributive"@en ;
        skos:definition  "At least 20% of mandatory reconversion into permanent grassland\r\n\r\nIn sense of Art. 31(1)(h) of R (EU) 809/2014 20 % of all beneficiaries with an obligation to re-convert land into permanent grassland shall be controlled."@en ;
        skos:inScheme    cap-iacs-controlcode:ControlRateTypeValue .

<http://lpis.ec.europa.eu/registry/applicationschema/cap-iacs-control/code#ControlRateTypeValue/atLeast5%ForSmallFarmersScheme>
        a                cap-iacs-control:ControlRateTypeValue ;
        rdfs:label       "At least 5% of all beneficiaries required to observe the agricultural practices having areas covered with permanent grasslands"@en ;
        skos:definition  "At least 5% for the small farmer scheme\r\n\r\nIn sense of Art. 30(f) of Regulation (EU) 809/2014 5% of beneficiaries applying for the small farmer scheme shall be controlled."@en ;
        skos:inScheme    cap-iacs-controlcode:ControlRateTypeValue .

<http://lpis.ec.europa.eu/registry/applicationschema/cap-iacs-control/code#SampleTypeValue/sensitiveGrassland>
        a                cap-iacs-control:SampleTypeValue ;
        skos:definition  "Sensitive grassland\r\n\r\nItems selected for controlling sensitive grassland. The composition of the population\r\n\t- 1,0-1,25% selected randomly \r\n\t- 3,75-4,0% selected on risk base\r\n\r\nNOTE\r\nThis sample is included in the generic sample of beneficiaries that are mandated to observe greening."@en ;
        skos:inScheme    cap-iacs-controlcode:SampleTypeValue .

<http://lpis.ec.europa.eu/registry/applicationschema/cap-iacs-control/code#SamplingStrategyTypeValue/simpleRiskBasedSelection>
        a                cap-iacs-control:SamplingStrategyTypeValue ;
        rdfs:label       "Risk based sampling strategy"@en ;
        skos:definition  "Simple risk based selection\r\n\r\nSampling process based on a single criterion retained to be effective in course of risk analysis. Input data for risk analysis can be taken from OTSC report of the previous year, other subsystems of IACS, third party data, etc.\r\n\r\nNOTE 1\r\nThe effectiveness of the criterion has to be proved by comparing the performance results from a random sample and a sample based on the criterion. \r\n\r\nNOTE 2\r\nThe performance criterion has to be documented before  starting the sampling process."@en ;
        skos:inScheme    cap-iacs-controlcode:SamplingStrategyTypeValue .

<http://lpis.ec.europa.eu/registry/applicationschema/cap-iacs-control/code#SampleTypeValue/hemp>
        a                cap-iacs-control:SampleTypeValue ;
        skos:definition  "Hemp\r\n\r\nItems selected for controlling beneficiaries growing hemp."@en ;
        skos:inScheme    cap-iacs-controlcode:SampleTypeValue .

<http://lpis.ec.europa.eu/registry/applicationschema/cap-iacs-control/code#SurveyMethodValue/cwrs>
        a                cap-iacs-control:SurveyMethodValue ;
        rdfs:label       "CwRS"@en ;
        skos:definition  "CwRS\r\n\r\nControl with Remote Sensing (VHR, or HR). [Art. 74(3) of R 1306/2013].\r\n\r\nNOTE.\r\nIt includes CAPI."@en ;
        skos:inScheme    cap-iacs-controlcode:SurveyMethodValue .

<http://lpis.ec.europa.eu/registry/applicationschema/cap-iacs-control/code#SurveyMethodValue/fieldMeasurement>
        a                cap-iacs-control:SurveyMethodValue ;
        rdfs:label       "Field measurement"@en ;
        skos:definition  "Field measurement\r\n\r\nAny field measurement including GNSS [Art. 74(3) of R 1306/2013]."@en ;
        skos:inScheme    cap-iacs-controlcode:SurveyMethodValue .

cap-iacs-controlcode:CrossCheckTypeValue
        a                skos:ConceptScheme ;
        rdfs:label       "List of on the cross-check types"@en ;
        dct:isFormatOf   cap-iacs-control:CrossCheckTypeValue ;
        skos:definition  "-- Definition --\r\nList of cross-check types.\r\n-- Description --\r\nList of cross-check types."@en .

<http://lpis.ec.europa.eu/registry/applicationschema/cap-iacs-control/code#OnTheSpotCheckTypeValue/eligibilityCriteria>
        a                cap-iacs-control:OnTheSpotCheckTypeValue ;
        rdfs:label       "Cross compliance"@en ;
        skos:definition  "Cross compliance\r\n\r\nOTSC in sense of Art. 96(3) of R 1306/2013, Art. 24(1)(b) and 26(3) of R 809/2014."@en ;
        skos:inScheme    cap-iacs-controlcode:OnTheSpotCheckTypeValue .

<http://lpis.ec.europa.eu/registry/applicationschema/cap-iacs-control/code#ControlRateTypeValue/atLeast30%ForProductionOfHemp>
        a                cap-iacs-control:ControlRateTypeValue ;
        rdfs:label       "At least 5% of all beneficiaries required to observe the agricultural practices having areas covered with permanent grasslands"@en ;
        skos:definition  "At least 30% for production of hemp\r\n\r\nIn sense of Art. 30(g) of Regulation (EU) 809/2014 30% of beneficiaries declaring hemp shall be controlled.\r\n\r\nNOTE\r\nIn accordance with art. 32(6) of R (EU) 1307/2013 only those varieties of hemp are eligible that have tetrahydrocannabinol content not exceeding 0,2 %."@en ;
        skos:inScheme    cap-iacs-controlcode:ControlRateTypeValue .

<http://lpis.ec.europa.eu/registry/applicationschema/cap-iacs-control/code#ControlRateTypeValue/atLeast10%OfAreasCoveredBySensitiveGrassland>
        a                cap-iacs-control:ControlRateTypeValue ;
        rdfs:label       "At least 5% of all beneficiaries required to observe the agricultural practices having areas covered with permanent grasslands"@en ;
        skos:definition  "At least 10% of areas covered by sensitive grassland\r\n\r\nIncreased control rate (5% normal+5% supplementary) in sense of Art. 31(3) for beneficiaries required to follow greening practices."@en ;
        skos:inScheme    cap-iacs-controlcode:ControlRateTypeValue .

<http://lpis.ec.europa.eu/registry/applicationschema/cap-iacs-control/code#ControlRateTypeValue/atLeast5%OfAreasCoveredBySensitiveGrassland>
        a                cap-iacs-control:ControlRateTypeValue ;
        rdfs:label       "At least 5% of all beneficiaries required to observe the agricultural practices having areas covered with permanent grasslands"@en ;
        skos:definition  "At least 5% of areas covered by sensitive grassland\r\n\r\nThe greenling sample in sense of Art. 31(1) of R (EU) 809/2014 shall cover at least 5 % of all beneficiaries having areas covered with permanent grasslands which are environmentally sensitive in areas covered by Council Directive 92/43/EEC[18] or Directive 2009/147/EC of the European Parliament and of the Council[19] and further sensitive areas referred to in Article 45(1) of Regulation (EU) No 1307/2013."@en ;
        skos:inScheme    cap-iacs-controlcode:ControlRateTypeValue .

cap-iacs-controlcode:RiskTypeValue
        a                skos:ConceptScheme ;
        dct:isFormatOf   cap-iacs-control:RiskTypeValue ;
        skos:definition  "Risk type value\r\n\r\nPreamble (33) of R (EU) 809/2014 requires that the competent authority should establish the risk factors targeting the areas where the risk of errors is the highest.\r\n\r\nNOTE\r\nRisk criteria should be assessed and updated on an annual basis taking into account the relevance of each risk criterion, comparing the results of randomly and risk-based selected samples, the specific situation in the Member States and the nature of the non-compliance."@en .

<http://lpis.ec.europa.eu/registry/applicationschema/cap-iacs-control/code#SampleTypeValue/contiguousEfa>
        a                cap-iacs-control:SampleTypeValue ;
        skos:definition  "Contiguous EFA\r\n\r\nItems selected for controlling contiguous EFA\r\n\r\nIssue:\r\nThe purpose of collective implementation (See Art. 46(a) of 1307/2013) and regional implementation (see Art. 46(3) of R 639/2014) is to form contiguous areas of EFA. If so, what is the reason to have separate samples for collective implementation, regional implementation and contiguous EFA?"@en ;
        skos:inScheme    cap-iacs-controlcode:SampleTypeValue .

<http://lpis.ec.europa.eu/registry/applicationschema/cap-iacs-control/code#CrossCheckTypeValue/betweenAgriculturalParcelsAndReferenceParcels>
        a                cap-iacs-control:CrossCheckTypeValue ;
        rdfs:label       "Between agricultural parcels and reference parcels"@en ;
        skos:definition  "-- Definition --\r\nBetween agricultural parcels and reference parcels.\r\n-- Description --\r\nWhere appropriate, the administrative checks shall include cross-checks: between the agricultural parcels as declared in the single application and/or payment claim and the information as contained in the identification system for \r\r\nagricultural parcels per reference parcel in accordance with Article 5(2) of Regulation (EU) No […] [DA IACS] to verify the eligibility for direct aid scheme and/or rural development support measure of the areas as such.\r\nNOTE. Where the integrated system provides for geo-spatial aid application forms, the cross-checks shall be carried out as spatial intersection of the digitised area declared with the identification system of agricultural parcels. In \r\r\naddition, cross-checks shall be carried out to prevent double claiming of the same area."@en ;
        skos:inScheme    cap-iacs-controlcode:CrossCheckTypeValue .

<http://lpis.ec.europa.eu/registry/applicationschema/cap-iacs-control/code#RiskTypeValue/areaOfIntensiveLcOrLuChange>
        a                cap-iacs-control:RiskTypeValue ;
        skos:definition  "Areas of Intensive LC or LU change\r\n\r\nAreas of intensive land cover and land use change may be detected in third party data e.g.\r\n\t- orthoimagery\r\n\t- cadastral maps\r\n\t- road maps\r\n\t- topographic maps\r\n\t- development plans"@en ;
        skos:inScheme    cap-iacs-controlcode:RiskTypeValue .

<http://lpis.ec.europa.eu/registry/applicationschema/cap-iacs-control/code#ControlRateTypeValue/atLeast3%ForBps/Saps>
        a                cap-iacs-control:ControlRateTypeValue ;
        rdfs:label       "At least 5% of all beneficiaries required to observe the agricultural practices having areas covered with permanent grasslands"@en ;
        skos:definition  "At least 3% for BPS or SAPS\r\n\r\nArt. 36(2) of Regulation (EU) 809/2014 allows the reduction of the control rate for BPS/SAPS from 5% to 3% when the cross checks based on geospatial applications are carried out."@en ;
        skos:inScheme    cap-iacs-controlcode:ControlRateTypeValue .
