@prefix owl:   <http://www.w3.org/2002/07/owl#> .
@prefix rdf:   <http://www.w3.org/1999/02/22-rdf-syntax-ns#> .
@prefix gsp:   <http://www.opengis.net/ont/geosparql#> .
@prefix cap-iacs-aid: <http://lpis.ec.europa.eu/registry/applicationschema/cap-iacs-aid#> .
@prefix xsd:   <http://www.w3.org/2001/XMLSchema#> .
@prefix skos:  <http://www.w3.org/2004/02/skos/core#> .
@prefix rdfs:  <http://www.w3.org/2000/01/rdf-schema#> .
@prefix cap-iacs-entitlement: <http://lpis.ec.europa.eu/registry/applicationschema/cap-iacs-entitlement#> .
@prefix om:    <http://www.ontology-of-units-of-measure.org/resource/om-2/> .
@prefix foaf:  <http://xmlns.com/foaf/0.1/> .
@prefix dct:   <http://purl.org/dc/terms/> .
@prefix schema: <http://schema.org/> .


cap-iacs-entitlement:OriginEntitlementObtainValue
        a                owl:Class ;
        rdfs:label       "Obtain origin values"@en ;
        rdfs:subClassOf  skos:Concept ;
        skos:definition  "-- Definition --\r\nEntitlement obtain origin values.\r\n-- Description --\r\nList of possible entitlement obtain sources."@en .

<http://lpis.ec.europa.eu/registry/applicationschema/cap-iacs-entitlement>
        a                owl:Ontology ;
        rdfs:label       "System for the identification and registration of payment entitlements"@en ;
        owl:imports      #<https://github.com/HajoRijgersberg/OM/raw/master/om-2.0.rdf> , 
        								 <https://raw.githubusercontent.com/rapw3k/cap-iacs/main/cap-iacs-aid.ttl> , 
        								 <http://www.opengis.net/ont/geosparql> ;
        owl:versionIRI   <http://lpis.ec.europa.eu/registry/applicationschema/cap-iacs-entitlement/3.0> ;
        owl:versionInfo  "3.0" ;
        skos:definition  "-- Name --\r\nSystem for the identification and registration of payment entitlements\r\n\r\n-- Definition --\r\nThis package is a placeholder for the Application schema for System for the identification and registration of payment entitlements.\r\n\r\n-- Description --\r\nThe contents of an «ApplicationSchema» package exported as a GML Application Schema file. The system for the identification and registration of payment entitlements shall allow for verification of the entitlements and for cross-checks with the aid applications and the identification system for agricultural parcels. Also shall allow direct and immediate consultation, through the competent authority of the Member State, of the data relating to at least the previous four consecutive calendar years."@en ;
        dct:creator [ schema:affiliation [ foaf:name "PSNC" ] ;
                      rdfs:seeAlso <http://orcid.org/0000-0003-4289-4922> ;
                      foaf:name "Raul Palma"
                    ] ;
        dct:title "JRC IACS - System for the Identification and Registration of Payment Entitlements Ontology"@en ;
        dct:description "Ontology of the system for the identification and registration of payment entitlements used in IACS, generated from the transformation of the corresponding JRC application schema"@en ;
        dct:source "JRC IACS application schema. https://doi.org/10.1016/j.landusepol.2016.05.023"@en ;
        dct:rights "This ontology is distributed under Creative Commons Attribution 4.0 License - http://creativecommons.org/licenses/by/4.0"@en .

cap-iacs-entitlement:regionalRestrictions
        a                owl:DatatypeProperty ;
        rdfs:label       "Regional restrictions"@en ;
        rdfs:range       xsd:string ;
        skos:definition  "-- Definition --\r\nRegional restrictions.\r\n-- Description --\r\nItem description.\r\nNOTE 1. Item note.\r\nEXAMPLE 1. Item example."@en .

cap-iacs-entitlement:OriginEntitlementReserveValue
        a                owl:Class ;
        rdfs:label       "Reserve origin values"@en ;
        rdfs:subClassOf  skos:Concept ;
        skos:definition  "-- Definition --\r\nEntitlement reserve origin values.\r\n-- Description --\r\nList of possible entitlement reserve sources."@en .

cap-iacs-entitlement:dateLastActivation
        a                owl:DatatypeProperty ;
        rdfs:label       "Date of last activation of entitlement"@en ;
        rdfs:range       xsd:date ;
        skos:definition  "-- Definition --\r\nDate of last activation of entitlement.\r\n-- Description --\r\nItem description.\r\nNOTE 1. Item note.\r\nEXAMPLE 1. Item example."@en .

cap-iacs-entitlement:entitlementConfirmationDetails
        a           owl:ObjectProperty ;
        rdfs:range  cap-iacs-aid:Application .

cap-iacs-entitlement:obtainOrigin
        a                owl:ObjectProperty ;
        rdfs:label       "Entitlement obtain source"@en ;
        rdfs:range       cap-iacs-entitlement:OriginEntitlementObtainValue ;
        skos:definition  "-- Definition --\r\nEntitlement obtain source.\r\n-- Description --\r\nItem description.\r\nNOTE 1. Item note.\r\nEXAMPLE 1. Item example."@en .

cap-iacs-entitlement:Entitlement
        a                owl:Class ;
        rdfs:label       "Entitlement"@en ;
        rdfs:subClassOf  gsp:Feature ;
        rdfs:subClassOf  [ a                owl:Restriction ;
                           owl:cardinality  "1"^^xsd:nonNegativeInteger ;
                           owl:onProperty   cap-iacs-entitlement:areaValue
                         ] ;
        rdfs:subClassOf  [ a                owl:Restriction ;
                           owl:cardinality  "1"^^xsd:nonNegativeInteger ;
                           owl:onProperty   cap-iacs-entitlement:obtainOrigin
                         ] ;
        rdfs:subClassOf  [ a                owl:Restriction ;
                           owl:cardinality  "1"^^xsd:nonNegativeInteger ;
                           owl:onProperty   cap-iacs-entitlement:reserveOrigin
                         ] ;
        rdfs:subClassOf  [ a                   owl:Restriction ;
                           owl:maxCardinality  "1"^^xsd:nonNegativeInteger ;
                           owl:onProperty      cap-iacs-entitlement:preReformStatus
                         ] ;
        rdfs:subClassOf  [ a                owl:Restriction ;
                           owl:cardinality  "1"^^xsd:nonNegativeInteger ;
                           owl:onProperty   cap-iacs-entitlement:entitlementId
                         ] ;
        rdfs:subClassOf  [ a                   owl:Restriction ;
                           owl:maxCardinality  "1"^^xsd:nonNegativeInteger ;
                           owl:onProperty      cap-iacs-entitlement:dateLastActivation
                         ] ;
        rdfs:subClassOf  [ a                owl:Restriction ;
                           owl:cardinality  "1"^^xsd:nonNegativeInteger ;
                           owl:onProperty   cap-iacs-entitlement:dateEstablishment
                         ] ;
        rdfs:subClassOf  [ a                   owl:Restriction ;
                           owl:maxCardinality  "1"^^xsd:nonNegativeInteger ;
                           owl:onProperty      cap-iacs-entitlement:entitlementConfirmationDetails
                         ] ;
        rdfs:subClassOf  [ a                   owl:Restriction ;
                           owl:maxCardinality  "1"^^xsd:nonNegativeInteger ;
                           owl:onProperty      cap-iacs-entitlement:regionalRestrictions
                         ] ;
        skos:definition  "-- Definition --\r\nPayment entitlements SPS only.\r\n-- Description --\r\nPlaceholder of payment entitlements for MS who use SPS systems only.\r\nNOTE. The system for the identification and registration of payment entitlements provided for in Article 71 of Regulation (EU) 1306/2013 shall be an electronic register at Member State level and shall, in particular with regard to the cross-checks provided for in paragraph 1 of that Article, ensure effective traceability."@en .

cap-iacs-entitlement:preReformStatus
        a                owl:DatatypeProperty ;
        rdfs:label       "Pre-reform status"@en ;
        rdfs:range       xsd:string ;
        skos:definition  "-- Definition --\r\nPre-reform status.\r\n-- Description --\r\nItem description.\r\nNOTE 1. Item note.\r\nEXAMPLE 1. Item example."@en .

cap-iacs-entitlement:areaValue
        a                owl:DatatypeProperty ;
        rdfs:label       "Annual area value"@en ;
        rdfs:range       om:Measure ;
        skos:definition  "-- Definition --\r\nAnnual area value.\r\n-- Description --\r\nItem description.\r\nNOTE 1. Item note.\r\nEXAMPLE 1. Item example."@en .

cap-iacs-entitlement:reserveOrigin
        a                owl:ObjectProperty ;
        rdfs:label       "Entitlement reserve source"@en ;
        rdfs:range       cap-iacs-entitlement:OriginEntitlementReserveValue ;
        skos:definition  "-- Definition --\r\nEntitlement reserve source.\r\n-- Description --\r\nItem description.\r\nNOTE 1. Item note.\r\nEXAMPLE 1. Item example."@en .

cap-iacs-entitlement:dateEstablishment
        a                owl:DatatypeProperty ;
        rdfs:label       "Date of entitlement establishment"@en ;
        rdfs:range       xsd:date ;
        skos:definition  "-- Definition --\r\nDate of entitlement establishment.\r\n-- Description --\r\nDate when entitlement was legally established."@en .

cap-iacs-entitlement:entitlementId
        a                owl:DatatypeProperty ;
        rdfs:label       "Unique thematic ID of a payment entitlement"@en ;
        rdfs:range       xsd:string ;
        skos:definition  "-- Definition --\r\nUnique thematic ID of a payment entitlement.\r\n-- Description --\r\nThematic identifier at national level, generally the full national code of the payment entitlement."@en .
