<?xml version="1.0"?>
<rdf:RDF xmlns="http://lpis.ec.europa.eu/registry/applicationschema/cap-iacs-control/code#"
     xml:base="http://lpis.ec.europa.eu/registry/applicationschema/cap-iacs-control/code"
     xmlns:owl="http://www.w3.org/2002/07/owl#"
     xmlns:rdf="http://www.w3.org/1999/02/22-rdf-syntax-ns#"
     xmlns:xml="http://www.w3.org/XML/1998/namespace"
     xmlns:xsd="http://www.w3.org/2001/XMLSchema#"
     xmlns:foaf="http://xmlns.com/foaf/0.1/"
     xmlns:rdfs="http://www.w3.org/2000/01/rdf-schema#"
     xmlns:skos="http://www.w3.org/2004/02/skos/core#"
     xmlns:terms="http://purl.org/dc/terms/"
     xmlns:schema="http://schema.org/">
    <owl:Ontology rdf:about="http://lpis.ec.europa.eu/registry/applicationschema/cap-iacs-control/code">
        <owl:versionIRI rdf:resource="http://lpis.ec.europa.eu/registry/applicationschema/cap-iacs-base/code/3.0"/>
        <terms:creator rdf:nodeID="genid1"/>
        <terms:description xml:lang="en">Ontology of the integrated control system code lists used in IACS, generated from the transformation of the corresponding JRC application schema</terms:description>
        <terms:rights xml:lang="en">This ontology is distributed under Creative Commons Attribution 4.0 License - http://creativecommons.org/licenses/by/4.0</terms:rights>
        <terms:source xml:lang="en">JRC IACS application schema. https://doi.org/10.1016/j.landusepol.2016.05.023</terms:source>
        <terms:title xml:lang="en">JRC IACS - Integrated Control System Code Lists</terms:title>
        <rdfs:label xml:lang="en">Integrated control system code lists</rdfs:label>
        <owl:versionInfo>3.0</owl:versionInfo>
    </owl:Ontology>
    <rdf:Description rdf:nodeID="genid1">
        <schema:affiliation>
            <rdf:Description>
                <foaf:name>PSNC</foaf:name>
            </rdf:Description>
        </schema:affiliation>
        <rdfs:seeAlso rdf:resource="http://orcid.org/0000-0003-4289-4922"/>
        <foaf:name>Raul Palma</foaf:name>
    </rdf:Description>
    


    <!-- 
    ///////////////////////////////////////////////////////////////////////////////////////
    //
    // Annotation properties
    //
    ///////////////////////////////////////////////////////////////////////////////////////
     -->


    


    <!-- http://purl.org/dc/terms/creator -->


    <owl:AnnotationProperty rdf:about="http://purl.org/dc/terms/creator"/>
    


    <!-- http://purl.org/dc/terms/description -->


    <owl:AnnotationProperty rdf:about="http://purl.org/dc/terms/description"/>
    


    <!-- http://purl.org/dc/terms/isFormatOf -->


    <owl:AnnotationProperty rdf:about="http://purl.org/dc/terms/isFormatOf"/>
    


    <!-- http://purl.org/dc/terms/rights -->


    <owl:AnnotationProperty rdf:about="http://purl.org/dc/terms/rights"/>
    


    <!-- http://purl.org/dc/terms/source -->


    <owl:AnnotationProperty rdf:about="http://purl.org/dc/terms/source"/>
    


    <!-- http://purl.org/dc/terms/title -->


    <owl:AnnotationProperty rdf:about="http://purl.org/dc/terms/title"/>
    


    <!-- http://schema.org/affiliation -->


    <owl:AnnotationProperty rdf:about="http://schema.org/affiliation"/>
    


    <!-- http://www.w3.org/2004/02/skos/core#definition -->


    <owl:AnnotationProperty rdf:about="http://www.w3.org/2004/02/skos/core#definition"/>
    


    <!-- http://www.w3.org/2004/02/skos/core#inScheme -->


    <owl:AnnotationProperty rdf:about="http://www.w3.org/2004/02/skos/core#inScheme"/>
    


    <!-- http://xmlns.com/foaf/0.1/name -->


    <owl:AnnotationProperty rdf:about="http://xmlns.com/foaf/0.1/name"/>
    


    <!-- 
    ///////////////////////////////////////////////////////////////////////////////////////
    //
    // Classes
    //
    ///////////////////////////////////////////////////////////////////////////////////////
     -->


    


    <!-- http://lpis.ec.europa.eu/registry/applicationschema/cap-iacs-control#ControlRateGroupAnimalAidSchemaValue -->


    <owl:Class rdf:about="http://lpis.ec.europa.eu/registry/applicationschema/cap-iacs-control#ControlRateGroupAnimalAidSchemaValue"/>
    


    <!-- http://lpis.ec.europa.eu/registry/applicationschema/cap-iacs-control#ControlRateGroupRuralDevelopmentMeasureValue -->


    <owl:Class rdf:about="http://lpis.ec.europa.eu/registry/applicationschema/cap-iacs-control#ControlRateGroupRuralDevelopmentMeasureValue"/>
    


    <!-- http://lpis.ec.europa.eu/registry/applicationschema/cap-iacs-control#ControlRateTypeValue -->


    <owl:Class rdf:about="http://lpis.ec.europa.eu/registry/applicationschema/cap-iacs-control#ControlRateTypeValue"/>
    


    <!-- http://lpis.ec.europa.eu/registry/applicationschema/cap-iacs-control#CrossCheckTypeValue -->


    <owl:Class rdf:about="http://lpis.ec.europa.eu/registry/applicationschema/cap-iacs-control#CrossCheckTypeValue"/>
    


    <!-- http://lpis.ec.europa.eu/registry/applicationschema/cap-iacs-control#InspectorsSurveyObjectTypeValue -->


    <owl:Class rdf:about="http://lpis.ec.europa.eu/registry/applicationschema/cap-iacs-control#InspectorsSurveyObjectTypeValue"/>
    


    <!-- http://lpis.ec.europa.eu/registry/applicationschema/cap-iacs-control#OnTheSpotCheckTypeValue -->


    <owl:Class rdf:about="http://lpis.ec.europa.eu/registry/applicationschema/cap-iacs-control#OnTheSpotCheckTypeValue"/>
    


    <!-- http://lpis.ec.europa.eu/registry/applicationschema/cap-iacs-control#RiskTypeValue -->


    <owl:Class rdf:about="http://lpis.ec.europa.eu/registry/applicationschema/cap-iacs-control#RiskTypeValue"/>
    


    <!-- http://lpis.ec.europa.eu/registry/applicationschema/cap-iacs-control#SampleTypeValue -->


    <owl:Class rdf:about="http://lpis.ec.europa.eu/registry/applicationschema/cap-iacs-control#SampleTypeValue"/>
    


    <!-- http://lpis.ec.europa.eu/registry/applicationschema/cap-iacs-control#SamplingStrategyTypeValue -->


    <owl:Class rdf:about="http://lpis.ec.europa.eu/registry/applicationschema/cap-iacs-control#SamplingStrategyTypeValue"/>
    


    <!-- http://lpis.ec.europa.eu/registry/applicationschema/cap-iacs-control#SurveyMethodValue -->


    <owl:Class rdf:about="http://lpis.ec.europa.eu/registry/applicationschema/cap-iacs-control#SurveyMethodValue"/>
    


    <!-- http://www.w3.org/2004/02/skos/core#ConceptScheme -->


    <owl:Class rdf:about="http://www.w3.org/2004/02/skos/core#ConceptScheme"/>
    


    <!-- 
    ///////////////////////////////////////////////////////////////////////////////////////
    //
    // Individuals
    //
    ///////////////////////////////////////////////////////////////////////////////////////
     -->


    


    <!-- http://lpis.ec.europa.eu/registry/applicationschema/cap-iacs-control/code#ControlRateGroupAnimalAidSchemaValue -->


    <owl:NamedIndividual rdf:about="http://lpis.ec.europa.eu/registry/applicationschema/cap-iacs-control/code#ControlRateGroupAnimalAidSchemaValue">
        <rdf:type rdf:resource="http://www.w3.org/2004/02/skos/core#ConceptScheme"/>
        <terms:isFormatOf rdf:resource="http://lpis.ec.europa.eu/registry/applicationschema/cap-iacs-control#ControlRateGroupAnimalAidSchemaValue"/>
        <rdfs:label xml:lang="en">List of control rate groups for animal aid schemas</rdfs:label>
        <skos:definition xml:lang="en">Control Rate Group Animal Aid Scheme Value

List of control rate groups for animal aid schemas.

NOTE
Currently placeholder only.</skos:definition>
    </owl:NamedIndividual>
    


    <!-- http://lpis.ec.europa.eu/registry/applicationschema/cap-iacs-control/code#ControlRateGroupRuralDevelopmentMeasureValue -->


    <owl:NamedIndividual rdf:about="http://lpis.ec.europa.eu/registry/applicationschema/cap-iacs-control/code#ControlRateGroupRuralDevelopmentMeasureValue">
        <rdf:type rdf:resource="http://www.w3.org/2004/02/skos/core#ConceptScheme"/>
        <terms:isFormatOf rdf:resource="http://lpis.ec.europa.eu/registry/applicationschema/cap-iacs-control#ControlRateGroupRuralDevelopmentMeasureValue"/>
        <rdfs:label xml:lang="en">List of control rate groups for rural development measures</rdfs:label>
        <skos:definition xml:lang="en">Control Rate Group Rural Development Measure Value

List of control rate groups for rural development measures.

NOTE. Currently placeholder only.</skos:definition>
    </owl:NamedIndividual>
    


    <!-- http://lpis.ec.europa.eu/registry/applicationschema/cap-iacs-control/code#ControlRateTypeValue -->


    <owl:NamedIndividual rdf:about="http://lpis.ec.europa.eu/registry/applicationschema/cap-iacs-control/code#ControlRateTypeValue">
        <rdf:type rdf:resource="http://www.w3.org/2004/02/skos/core#ConceptScheme"/>
        <terms:isFormatOf rdf:resource="http://lpis.ec.europa.eu/registry/applicationschema/cap-iacs-control#ControlRateTypeValue"/>
        <rdfs:label xml:lang="en">List of control rate groups for greening</rdfs:label>
        <skos:definition xml:lang="en">Control rate type value

List of applicable control rate values as prescribed by Art. 30, 31, 36(2) and 36(6) of R 809/2014.

NOTE
This code list currently does not contain values for rural development measures (Art. 32) and animal aid schemes (Art. 33 of R 809/2014).</skos:definition>
    </owl:NamedIndividual>
    


    <!-- http://lpis.ec.europa.eu/registry/applicationschema/cap-iacs-control/code#CrossCheckTypeValue -->


    <owl:NamedIndividual rdf:about="http://lpis.ec.europa.eu/registry/applicationschema/cap-iacs-control/code#CrossCheckTypeValue">
        <rdf:type rdf:resource="http://www.w3.org/2004/02/skos/core#ConceptScheme"/>
        <terms:isFormatOf rdf:resource="http://lpis.ec.europa.eu/registry/applicationschema/cap-iacs-control#CrossCheckTypeValue"/>
        <rdfs:label xml:lang="en">List of on the cross-check types</rdfs:label>
        <skos:definition xml:lang="en">-- Definition --
List of cross-check types.
-- Description --
List of cross-check types.</skos:definition>
    </owl:NamedIndividual>
    


    <!-- http://lpis.ec.europa.eu/registry/applicationschema/cap-iacs-control/code#InspectorsSurveyObjectTypeValue -->


    <owl:NamedIndividual rdf:about="http://lpis.ec.europa.eu/registry/applicationschema/cap-iacs-control/code#InspectorsSurveyObjectTypeValue">
        <rdf:type rdf:resource="http://www.w3.org/2004/02/skos/core#ConceptScheme"/>
        <terms:isFormatOf rdf:resource="http://lpis.ec.europa.eu/registry/applicationschema/cap-iacs-control#InspectorsSurveyObjectTypeValue"/>
        <rdfs:label xml:lang="en">List of feature types</rdfs:label>
        <skos:definition xml:lang="en">Inspectors survey type value

List of possible real objects measured by an inspector.

NOTE
List may be extended or subtracted depending on how MS organizing on-the-spot check process.</skos:definition>
    </owl:NamedIndividual>
    


    <!-- http://lpis.ec.europa.eu/registry/applicationschema/cap-iacs-control/code#OnTheSpotCheckTypeValue -->


    <owl:NamedIndividual rdf:about="http://lpis.ec.europa.eu/registry/applicationschema/cap-iacs-control/code#OnTheSpotCheckTypeValue">
        <rdf:type rdf:resource="http://www.w3.org/2004/02/skos/core#ConceptScheme"/>
        <terms:isFormatOf rdf:resource="http://lpis.ec.europa.eu/registry/applicationschema/cap-iacs-control#OnTheSpotCheckTypeValue"/>
        <rdfs:label xml:lang="en">List of on the spot check types</rdfs:label>
        <skos:definition xml:lang="en">On-the-spot check type value

List of on the spot check types. that describe the purpose of the control.</skos:definition>
    </owl:NamedIndividual>
    


    <!-- http://lpis.ec.europa.eu/registry/applicationschema/cap-iacs-control/code#RiskTypeValue -->


    <owl:NamedIndividual rdf:about="http://lpis.ec.europa.eu/registry/applicationschema/cap-iacs-control/code#RiskTypeValue">
        <rdf:type rdf:resource="http://www.w3.org/2004/02/skos/core#ConceptScheme"/>
        <terms:isFormatOf rdf:resource="http://lpis.ec.europa.eu/registry/applicationschema/cap-iacs-control#RiskTypeValue"/>
        <skos:definition xml:lang="en">Risk type value

Preamble (33) of R (EU) 809/2014 requires that the competent authority should establish the risk factors targeting the areas where the risk of errors is the highest.

NOTE
Risk criteria should be assessed and updated on an annual basis taking into account the relevance of each risk criterion, comparing the results of randomly and risk-based selected samples, the specific situation in the Member States and the nature of the non-compliance.</skos:definition>
    </owl:NamedIndividual>
    


    <!-- http://lpis.ec.europa.eu/registry/applicationschema/cap-iacs-control/code#SampleTypeValue -->


    <owl:NamedIndividual rdf:about="http://lpis.ec.europa.eu/registry/applicationschema/cap-iacs-control/code#SampleTypeValue">
        <rdf:type rdf:resource="http://www.w3.org/2004/02/skos/core#ConceptScheme"/>
        <terms:isFormatOf rdf:resource="http://lpis.ec.europa.eu/registry/applicationschema/cap-iacs-control#SampleTypeValue"/>
        <skos:definition xml:lang="en">Sample Type value

The sample type property shall be attributed to each sampled item (application). One item can be sampled to one or more payment/support schemes. 

NOTE
The categories of sample type values have to support the traceability of the sampling cascade. This is the reason for distinguishing the initial and the top-up samples for BPS/SAPS.</skos:definition>
    </owl:NamedIndividual>
    


    <!-- http://lpis.ec.europa.eu/registry/applicationschema/cap-iacs-control/code#SamplingStrategyTypeValue -->


    <owl:NamedIndividual rdf:about="http://lpis.ec.europa.eu/registry/applicationschema/cap-iacs-control/code#SamplingStrategyTypeValue">
        <rdf:type rdf:resource="http://www.w3.org/2004/02/skos/core#ConceptScheme"/>
        <terms:isFormatOf rdf:resource="http://lpis.ec.europa.eu/registry/applicationschema/cap-iacs-control#SamplingStrategyTypeValue"/>
        <rdfs:label xml:lang="en">List of sampling strategy types</rdfs:label>
        <skos:definition xml:lang="en">Sampling Strategy Type Value

List of sampling strategy types.

In accordance with Preamble (34) of R 809/2014 sampling should comprise a random part in order to obtain a representative error rate and a risk based part for the following Payment/support schemes:
	- greening payment
	- animal aid schemes
	- rural development measure

NOTE 1
To ensure a relevant and efficient risk analysis, the effectiveness of the risk analysis should be assessed and updated on an annual basis taking into account the relevance of each risk factor, comparing the results of randomly and risk-based selected samples and the specific situation [Preamble (68) and Art. 34(5) of R 809/2014].

NOTE 2
The sampling method should be selected and documented by the competent authority of the MS/Region. The values of the code list can be extended.

NOTE 3
The exemplary values of the code list in this application schema are taken from DSCG/2014/32 guideline and best statistical practices.</skos:definition>
    </owl:NamedIndividual>
    


    <!-- http://lpis.ec.europa.eu/registry/applicationschema/cap-iacs-control/code#SurveyMethodValue -->


    <owl:NamedIndividual rdf:about="http://lpis.ec.europa.eu/registry/applicationschema/cap-iacs-control/code#SurveyMethodValue">
        <rdf:type rdf:resource="http://www.w3.org/2004/02/skos/core#ConceptScheme"/>
        <terms:isFormatOf rdf:resource="http://lpis.ec.europa.eu/registry/applicationschema/cap-iacs-control#SurveyMethodValue"/>
        <rdfs:label xml:lang="en">List of survey types</rdfs:label>
        <skos:definition xml:lang="en">Survey method value

List of survey method types in sense of Art. 74(3) of R 1306/2013.</skos:definition>
    </owl:NamedIndividual>
    


    <!-- http://lpis.ec.europa.eu/registry/applicationschema/cap-iacs-control/code#ControlRateGroupAnimalAidSchemaValue/placeholder -->


    <owl:NamedIndividual rdf:about="http://lpis.ec.europa.eu/registry/applicationschema/cap-iacs-control/code#ControlRateGroupAnimalAidSchemaValue/placeholder">
        <rdf:type rdf:resource="http://lpis.ec.europa.eu/registry/applicationschema/cap-iacs-control#ControlRateGroupAnimalAidSchemaValue"/>
        <rdfs:label xml:lang="en">Currently out of scope</rdfs:label>
        <skos:inScheme rdf:resource="http://lpis.ec.europa.eu/registry/applicationschema/cap-iacs-control/code#ControlRateGroupAnimalAidSchemaValue"/>
    </owl:NamedIndividual>
    


    <!-- http://lpis.ec.europa.eu/registry/applicationschema/cap-iacs-control/code#ControlRateGroupRuralDevelopmentMeasureValue/placeholder -->


    <owl:NamedIndividual rdf:about="http://lpis.ec.europa.eu/registry/applicationschema/cap-iacs-control/code#ControlRateGroupRuralDevelopmentMeasureValue/placeholder">
        <rdf:type rdf:resource="http://lpis.ec.europa.eu/registry/applicationschema/cap-iacs-control#ControlRateGroupRuralDevelopmentMeasureValue"/>
        <rdfs:label xml:lang="en">Currently out of scope</rdfs:label>
        <skos:inScheme rdf:resource="http://lpis.ec.europa.eu/registry/applicationschema/cap-iacs-control/code#ControlRateGroupRuralDevelopmentMeasureValue"/>
    </owl:NamedIndividual>
    


    <!-- http://lpis.ec.europa.eu/registry/applicationschema/cap-iacs-control/code#ControlRateTypeValue/100%OfMandarotyReconversionIntoSensitivePermanentGrassland -->


    <owl:NamedIndividual rdf:about="http://lpis.ec.europa.eu/registry/applicationschema/cap-iacs-control/code#ControlRateTypeValue/100%OfMandarotyReconversionIntoSensitivePermanentGrassland">
        <rdf:type rdf:resource="http://lpis.ec.europa.eu/registry/applicationschema/cap-iacs-control#ControlRateTypeValue"/>
        <rdfs:label xml:lang="en">100 % of all beneficiaries with an obligation to re-convert land into land under permanent grassland, redistributive</rdfs:label>
        <skos:definition xml:lang="en">100% of mandatory reconversion into sensitive permanent grassland

In accordance with Art.31(1)(g) of R (EU) 809/2014 100 % of beneficiaries with an obligation to re-convert land into land under permanent grassland shall be controlled.</skos:definition>
        <skos:inScheme rdf:resource="http://lpis.ec.europa.eu/registry/applicationschema/cap-iacs-control/code#ControlRateTypeValue"/>
    </owl:NamedIndividual>
    


    <!-- http://lpis.ec.europa.eu/registry/applicationschema/cap-iacs-control/code#ControlRateTypeValue/100%OfTheContiguousStructuresOfAdjacentEfa -->


    <owl:NamedIndividual rdf:about="http://lpis.ec.europa.eu/registry/applicationschema/cap-iacs-control/code#ControlRateTypeValue/100%OfTheContiguousStructuresOfAdjacentEfa">
        <rdf:type rdf:resource="http://lpis.ec.europa.eu/registry/applicationschema/cap-iacs-control#ControlRateTypeValue"/>
        <rdfs:label xml:lang="en">100 % of the contiguous structures of adjacent ecological focus areas</rdfs:label>
        <skos:definition xml:lang="en">100 % of the contiguous structures of adjacent EFA

In sense of Art. 31(1)(f) of R (EU) 809/2014  100 % of the contiguous structures of adjacent ecological focus areas as referred to in Article 46(5) of Regulation (EU) 1307/2013 shall be controlled.</skos:definition>
        <skos:inScheme rdf:resource="http://lpis.ec.europa.eu/registry/applicationschema/cap-iacs-control/code#ControlRateTypeValue"/>
    </owl:NamedIndividual>
    


    <!-- http://lpis.ec.europa.eu/registry/applicationschema/cap-iacs-control/code#ControlRateTypeValue/atLeast10%OfAreasCoveredBySensitiveGrassland -->


    <owl:NamedIndividual rdf:about="http://lpis.ec.europa.eu/registry/applicationschema/cap-iacs-control/code#ControlRateTypeValue/atLeast10%OfAreasCoveredBySensitiveGrassland">
        <rdf:type rdf:resource="http://lpis.ec.europa.eu/registry/applicationschema/cap-iacs-control#ControlRateTypeValue"/>
        <rdfs:label xml:lang="en">At least 5% of all beneficiaries required to observe the agricultural practices having areas covered with permanent grasslands</rdfs:label>
        <skos:definition xml:lang="en">At least 10% of areas covered by sensitive grassland

Increased control rate (5% normal+5% supplementary) in sense of Art. 31(3) for beneficiaries required to follow greening practices.</skos:definition>
        <skos:inScheme rdf:resource="http://lpis.ec.europa.eu/registry/applicationschema/cap-iacs-control/code#ControlRateTypeValue"/>
    </owl:NamedIndividual>
    


    <!-- http://lpis.ec.europa.eu/registry/applicationschema/cap-iacs-control/code#ControlRateTypeValue/atLeast10%OfCollectiveImplementation -->


    <owl:NamedIndividual rdf:about="http://lpis.ec.europa.eu/registry/applicationschema/cap-iacs-control/code#ControlRateTypeValue/atLeast10%OfCollectiveImplementation">
        <rdf:type rdf:resource="http://lpis.ec.europa.eu/registry/applicationschema/cap-iacs-control#ControlRateTypeValue"/>
        <rdfs:label xml:lang="en">At least 5 % of  the  collective implementation</rdfs:label>
        <skos:definition xml:lang="en">At least 10% of the collective implementation

Increased control rate (5% normal+5% supplementary) in sense of Art. 31(3) for beneficiaries required to follow greening practices.</skos:definition>
        <skos:inScheme rdf:resource="http://lpis.ec.europa.eu/registry/applicationschema/cap-iacs-control/code#ControlRateTypeValue"/>
    </owl:NamedIndividual>
    


    <!-- http://lpis.ec.europa.eu/registry/applicationschema/cap-iacs-control/code#ControlRateTypeValue/atLeast10%OfFollowingGreeningByUsingEnvironmentalCertificationSchemes -->


    <owl:NamedIndividual rdf:about="http://lpis.ec.europa.eu/registry/applicationschema/cap-iacs-control/code#ControlRateTypeValue/atLeast10%OfFollowingGreeningByUsingEnvironmentalCertificationSchemes">
        <rdf:type rdf:resource="http://lpis.ec.europa.eu/registry/applicationschema/cap-iacs-control#ControlRateTypeValue"/>
        <rdfs:label xml:lang="en">At least 5 % of all beneficiaries required to observe the greening practices and using national or regional environmental certification schemes</rdfs:label>
        <skos:definition xml:lang="en">At least 10 % following greening practices by using environmental certification schemes

Increased control rate (5% normal+5% supplementary) in sense of Art. 31(3) for beneficiaries required to follow greening practices.</skos:definition>
        <skos:inScheme rdf:resource="http://lpis.ec.europa.eu/registry/applicationschema/cap-iacs-control/code#ControlRateTypeValue"/>
    </owl:NamedIndividual>
    


    <!-- http://lpis.ec.europa.eu/registry/applicationschema/cap-iacs-control/code#ControlRateTypeValue/atLeast10%OfFollowingGreeningPractices -->


    <owl:NamedIndividual rdf:about="http://lpis.ec.europa.eu/registry/applicationschema/cap-iacs-control/code#ControlRateTypeValue/atLeast10%OfFollowingGreeningPractices">
        <rdf:type rdf:resource="http://lpis.ec.europa.eu/registry/applicationschema/cap-iacs-control#ControlRateTypeValue"/>
        <rdfs:label xml:lang="en">At least 5% of all beneficiaries required to observe the agricultural practices having areas covered with permanent grasslands</rdfs:label>
        <skos:definition xml:lang="en">At least 10% of following greening practices

Increased control rate (5% normal+5% supplementary) in sense of Art. 31(3) of R 809/2014 for beneficiaries required to follow greening practices. 

Where the ecological focus areas are not identified in the identification system for agricultural parcels as referred to in Article 70 of Regulation (EU) No 1306/2013, the control rate laid down in points (a) and (c) to (e) of paragraph 1 shall be supplemented by 5% of all beneficiaries of the respective control sample who are required to have ecological focus area on the agricultural area in accordance with Articles 43 and 46 of Regulation (EU) No 1307/2013.</skos:definition>
        <skos:inScheme rdf:resource="http://lpis.ec.europa.eu/registry/applicationschema/cap-iacs-control/code#ControlRateTypeValue"/>
    </owl:NamedIndividual>
    


    <!-- http://lpis.ec.europa.eu/registry/applicationschema/cap-iacs-control/code#ControlRateTypeValue/atLeast10%OfRegionalImplementation -->


    <owl:NamedIndividual rdf:about="http://lpis.ec.europa.eu/registry/applicationschema/cap-iacs-control/code#ControlRateTypeValue/atLeast10%OfRegionalImplementation">
        <rdf:type rdf:resource="http://lpis.ec.europa.eu/registry/applicationschema/cap-iacs-control#ControlRateTypeValue"/>
        <rdfs:label xml:lang="en">At least  5 % of all beneficiaries participating in a regional implementation</rdfs:label>
        <skos:definition xml:lang="en">At least 10 % of all beneficiaries participating in a regional implementation

Increased control rate (5% normal+5% supplementary) in sense of Art. 31(3) for beneficiaries required to follow greening practices.</skos:definition>
        <skos:inScheme rdf:resource="http://lpis.ec.europa.eu/registry/applicationschema/cap-iacs-control/code#ControlRateTypeValue"/>
    </owl:NamedIndividual>
    


    <!-- http://lpis.ec.europa.eu/registry/applicationschema/cap-iacs-control/code#ControlRateTypeValue/atLeast20%ForProductionOfHemp -->


    <owl:NamedIndividual rdf:about="http://lpis.ec.europa.eu/registry/applicationschema/cap-iacs-control/code#ControlRateTypeValue/atLeast20%ForProductionOfHemp">
        <rdf:type rdf:resource="http://lpis.ec.europa.eu/registry/applicationschema/cap-iacs-control#ControlRateTypeValue"/>
        <rdfs:label xml:lang="en">At least 5% of all beneficiaries required to observe the agricultural practices having areas covered with permanent grasslands</rdfs:label>
        <skos:definition xml:lang="en">At least 20% for production of hemp

Art. 36(6) of Regulation (EU) 809/2014 allows the reduction of the control rate for production of hemp from 30% to 20% when a MS introduces a prior approval for the cultivation of hemp.

NOTE
MS shall notify the EC about the rules (or changes in the rules) of the approval system.</skos:definition>
        <skos:inScheme rdf:resource="http://lpis.ec.europa.eu/registry/applicationschema/cap-iacs-control/code#ControlRateTypeValue"/>
    </owl:NamedIndividual>
    


    <!-- http://lpis.ec.europa.eu/registry/applicationschema/cap-iacs-control/code#ControlRateTypeValue/atLeast20%OfMandarotyReconversionIntoPermanentGrassland -->


    <owl:NamedIndividual rdf:about="http://lpis.ec.europa.eu/registry/applicationschema/cap-iacs-control/code#ControlRateTypeValue/atLeast20%OfMandarotyReconversionIntoPermanentGrassland">
        <rdf:type rdf:resource="http://lpis.ec.europa.eu/registry/applicationschema/cap-iacs-control#ControlRateTypeValue"/>
        <rdfs:label xml:lang="en">100 % of all beneficiaries with an obligation to re-convert land into land under permanent grassland, redistributive</rdfs:label>
        <skos:definition xml:lang="en">At least 20% of mandatory reconversion into permanent grassland

In sense of Art. 31(1)(h) of R (EU) 809/2014 20 % of all beneficiaries with an obligation to re-convert land into permanent grassland shall be controlled.</skos:definition>
        <skos:inScheme rdf:resource="http://lpis.ec.europa.eu/registry/applicationschema/cap-iacs-control/code#ControlRateTypeValue"/>
    </owl:NamedIndividual>
    


    <!-- http://lpis.ec.europa.eu/registry/applicationschema/cap-iacs-control/code#ControlRateTypeValue/atLeast3%ForRedistributivePayment -->


    <owl:NamedIndividual rdf:about="http://lpis.ec.europa.eu/registry/applicationschema/cap-iacs-control/code#ControlRateTypeValue/atLeast3%ForRedistributivePayment">
        <rdf:type rdf:resource="http://lpis.ec.europa.eu/registry/applicationschema/cap-iacs-control#ControlRateTypeValue"/>
        <rdfs:label xml:lang="en">At least 5% of all beneficiaries required to observe the agricultural practices having areas covered with permanent grasslands</rdfs:label>
        <skos:definition xml:lang="en">At least 3% or redistributive payment 

Art. 36(2) of Regulation (EU) 809/2014 allows the reduction of the control rate for redistributive payment from 5% to 3% when the cross checks based on geospatial applications are carried out.</skos:definition>
        <skos:inScheme rdf:resource="http://lpis.ec.europa.eu/registry/applicationschema/cap-iacs-control/code#ControlRateTypeValue"/>
    </owl:NamedIndividual>
    


    <!-- http://lpis.ec.europa.eu/registry/applicationschema/cap-iacs-control/code#ControlRateTypeValue/atLeast3%ForSmallFarmersScheme -->


    <owl:NamedIndividual rdf:about="http://lpis.ec.europa.eu/registry/applicationschema/cap-iacs-control/code#ControlRateTypeValue/atLeast3%ForSmallFarmersScheme">
        <rdf:type rdf:resource="http://lpis.ec.europa.eu/registry/applicationschema/cap-iacs-control#ControlRateTypeValue"/>
        <rdfs:label xml:lang="en">At least 5% of all beneficiaries required to observe the agricultural practices having areas covered with permanent grasslands</rdfs:label>
        <skos:definition xml:lang="en">At least 3% for small farmer scheme

Art. 36(2) of Regulation (EU) 809/2014 allows the reduction of the control rate for the small farmer scheme  from 5% to 3% when the cross checks based on geospatial applications are carried out.</skos:definition>
        <skos:inScheme rdf:resource="http://lpis.ec.europa.eu/registry/applicationschema/cap-iacs-control/code#ControlRateTypeValue"/>
    </owl:NamedIndividual>
    


    <!-- http://lpis.ec.europa.eu/registry/applicationschema/cap-iacs-control/code#ControlRateTypeValue/atLeast3%OfExemptedFromGreeningPractices -->


    <owl:NamedIndividual rdf:about="http://lpis.ec.europa.eu/registry/applicationschema/cap-iacs-control/code#ControlRateTypeValue/atLeast3%OfExemptedFromGreeningPractices">
        <rdf:type rdf:resource="http://lpis.ec.europa.eu/registry/applicationschema/cap-iacs-control#ControlRateTypeValue"/>
        <rdfs:label xml:lang="en">At least 3 % of all beneficiaries qualifying for the greening payment who are exempted from both the crop diversification and the EFA obligations</rdfs:label>
        <skos:definition xml:lang="en">At least 3% of exempted from greening practices

In sense of Art. 31 (1)(b) at least 3 % of all beneficiaries qualifying for the greening payment who are exempted from both the crop diversification and the EFA obligations shall be controlled.

The exemption is granted when the thresholds referred to in Articles 44 and 46 of Regulation (EU) No 1307/2013 are not met and the obligations referred to in Article 45 of that Regulation are not concerned.</skos:definition>
        <skos:inScheme rdf:resource="http://lpis.ec.europa.eu/registry/applicationschema/cap-iacs-control/code#ControlRateTypeValue"/>
    </owl:NamedIndividual>
    


    <!-- http://lpis.ec.europa.eu/registry/applicationschema/cap-iacs-control/code#ControlRateTypeValue/atLeast3%ForBps/Saps -->


    <owl:NamedIndividual rdf:about="http://lpis.ec.europa.eu/registry/applicationschema/cap-iacs-control/code#ControlRateTypeValue/atLeast3%ForBps/Saps">
        <rdf:type rdf:resource="http://lpis.ec.europa.eu/registry/applicationschema/cap-iacs-control#ControlRateTypeValue"/>
        <rdfs:label xml:lang="en">At least 5% of all beneficiaries required to observe the agricultural practices having areas covered with permanent grasslands</rdfs:label>
        <skos:definition xml:lang="en">At least 3% for BPS or SAPS

Art. 36(2) of Regulation (EU) 809/2014 allows the reduction of the control rate for BPS/SAPS from 5% to 3% when the cross checks based on geospatial applications are carried out.</skos:definition>
        <skos:inScheme rdf:resource="http://lpis.ec.europa.eu/registry/applicationschema/cap-iacs-control/code#ControlRateTypeValue"/>
    </owl:NamedIndividual>
    


    <!-- http://lpis.ec.europa.eu/registry/applicationschema/cap-iacs-control/code#ControlRateTypeValue/atLeast30%ForProductionOfHemp -->


    <owl:NamedIndividual rdf:about="http://lpis.ec.europa.eu/registry/applicationschema/cap-iacs-control/code#ControlRateTypeValue/atLeast30%ForProductionOfHemp">
        <rdf:type rdf:resource="http://lpis.ec.europa.eu/registry/applicationschema/cap-iacs-control#ControlRateTypeValue"/>
        <rdfs:label xml:lang="en">At least 5% of all beneficiaries required to observe the agricultural practices having areas covered with permanent grasslands</rdfs:label>
        <skos:definition xml:lang="en">At least 30% for production of hemp

In sense of Art. 30(g) of Regulation (EU) 809/2014 30% of beneficiaries declaring hemp shall be controlled.

NOTE
In accordance with art. 32(6) of R (EU) 1307/2013 only those varieties of hemp are eligible that have tetrahydrocannabinol content not exceeding 0,2 %.</skos:definition>
        <skos:inScheme rdf:resource="http://lpis.ec.europa.eu/registry/applicationschema/cap-iacs-control/code#ControlRateTypeValue"/>
    </owl:NamedIndividual>
    


    <!-- http://lpis.ec.europa.eu/registry/applicationschema/cap-iacs-control/code#ControlRateTypeValue/atLeast5%ForAreasWithNaturalConstraints -->


    <owl:NamedIndividual rdf:about="http://lpis.ec.europa.eu/registry/applicationschema/cap-iacs-control/code#ControlRateTypeValue/atLeast5%ForAreasWithNaturalConstraints">
        <rdf:type rdf:resource="http://lpis.ec.europa.eu/registry/applicationschema/cap-iacs-control#ControlRateTypeValue"/>
        <rdfs:label xml:lang="en">At least 5% of all beneficiaries required to observe the agricultural practices having areas covered with permanent grasslands</rdfs:label>
        <skos:definition xml:lang="en">At least 5% for areas with natural constraints 

In sense of Art. 30(c) of Regulation (EU) 809/2014 5% of beneficiaries applying for the payment for areas with natural constraints shall be controlled.</skos:definition>
        <skos:inScheme rdf:resource="http://lpis.ec.europa.eu/registry/applicationschema/cap-iacs-control/code#ControlRateTypeValue"/>
    </owl:NamedIndividual>
    


    <!-- http://lpis.ec.europa.eu/registry/applicationschema/cap-iacs-control/code#ControlRateTypeValue/atLeast5%ForCropSpecificCottonPayment -->


    <owl:NamedIndividual rdf:about="http://lpis.ec.europa.eu/registry/applicationschema/cap-iacs-control/code#ControlRateTypeValue/atLeast5%ForCropSpecificCottonPayment">
        <rdf:type rdf:resource="http://lpis.ec.europa.eu/registry/applicationschema/cap-iacs-control#ControlRateTypeValue"/>
        <rdfs:label xml:lang="en">At least 5% of all beneficiaries required to observe the agricultural practices having areas covered with permanent grasslands</rdfs:label>
        <skos:definition xml:lang="en">At least 5% for crop specific cotton payment

In sense of Art. 30(h) of Regulation (EU) 809/2014 5% of beneficiaries applying for the crop specific payment for cotton shall be controlled.</skos:definition>
        <skos:inScheme rdf:resource="http://lpis.ec.europa.eu/registry/applicationschema/cap-iacs-control/code#ControlRateTypeValue"/>
    </owl:NamedIndividual>
    


    <!-- http://lpis.ec.europa.eu/registry/applicationschema/cap-iacs-control/code#ControlRateTypeValue/atLeast5%ForRedistributivePayment -->


    <owl:NamedIndividual rdf:about="http://lpis.ec.europa.eu/registry/applicationschema/cap-iacs-control/code#ControlRateTypeValue/atLeast5%ForRedistributivePayment">
        <rdf:type rdf:resource="http://lpis.ec.europa.eu/registry/applicationschema/cap-iacs-control#ControlRateTypeValue"/>
        <rdfs:label xml:lang="en">At least 5% of all beneficiaries required to observe the agricultural practices having areas covered with permanent grasslands</rdfs:label>
        <skos:definition xml:lang="en">At least 5% for the redistributive payment

In sense of Art. 30(b) of Regulation (EU) 809/2014 5% of beneficiaries applying for the redistributive payment shall be controlled.</skos:definition>
        <skos:inScheme rdf:resource="http://lpis.ec.europa.eu/registry/applicationschema/cap-iacs-control/code#ControlRateTypeValue"/>
    </owl:NamedIndividual>
    


    <!-- http://lpis.ec.europa.eu/registry/applicationschema/cap-iacs-control/code#ControlRateTypeValue/atLeast5%ForSmallFarmersScheme -->


    <owl:NamedIndividual rdf:about="http://lpis.ec.europa.eu/registry/applicationschema/cap-iacs-control/code#ControlRateTypeValue/atLeast5%ForSmallFarmersScheme">
        <rdf:type rdf:resource="http://lpis.ec.europa.eu/registry/applicationschema/cap-iacs-control#ControlRateTypeValue"/>
        <rdfs:label xml:lang="en">At least 5% of all beneficiaries required to observe the agricultural practices having areas covered with permanent grasslands</rdfs:label>
        <skos:definition xml:lang="en">At least 5% for the small farmer scheme

In sense of Art. 30(f) of Regulation (EU) 809/2014 5% of beneficiaries applying for the small farmer scheme shall be controlled.</skos:definition>
        <skos:inScheme rdf:resource="http://lpis.ec.europa.eu/registry/applicationschema/cap-iacs-control/code#ControlRateTypeValue"/>
    </owl:NamedIndividual>
    


    <!-- http://lpis.ec.europa.eu/registry/applicationschema/cap-iacs-control/code#ControlRateTypeValue/atLeast5%ForVoluntaryCoupledSupport -->


    <owl:NamedIndividual rdf:about="http://lpis.ec.europa.eu/registry/applicationschema/cap-iacs-control/code#ControlRateTypeValue/atLeast5%ForVoluntaryCoupledSupport">
        <rdf:type rdf:resource="http://lpis.ec.europa.eu/registry/applicationschema/cap-iacs-control#ControlRateTypeValue"/>
        <rdfs:label xml:lang="en">At least 5% of all beneficiaries required to observe the agricultural practices having areas covered with permanent grasslands</rdfs:label>
        <skos:definition xml:lang="en">At least 5% for the voluntary coupled support

In sense of Art. 30(e) of Regulation (EU) 809/2014 5% of beneficiaries applying for the voluntary coupled shall be controlled.</skos:definition>
        <skos:inScheme rdf:resource="http://lpis.ec.europa.eu/registry/applicationschema/cap-iacs-control/code#ControlRateTypeValue"/>
    </owl:NamedIndividual>
    


    <!-- http://lpis.ec.europa.eu/registry/applicationschema/cap-iacs-control/code#ControlRateTypeValue/atLeast5%ForYoungFarmers -->


    <owl:NamedIndividual rdf:about="http://lpis.ec.europa.eu/registry/applicationschema/cap-iacs-control/code#ControlRateTypeValue/atLeast5%ForYoungFarmers">
        <rdf:type rdf:resource="http://lpis.ec.europa.eu/registry/applicationschema/cap-iacs-control#ControlRateTypeValue"/>
        <rdfs:label xml:lang="en">At least 5% of all beneficiaries required to observe the agricultural practices having areas covered with permanent grasslands</rdfs:label>
        <skos:definition xml:lang="en">At least 5% for the young farmers

In sense of Art. 30(d) of Regulation (EU) 809/2014 5% of beneficiaries applying for the young farmer payment shall be controlled.</skos:definition>
        <skos:inScheme rdf:resource="http://lpis.ec.europa.eu/registry/applicationschema/cap-iacs-control/code#ControlRateTypeValue"/>
    </owl:NamedIndividual>
    


    <!-- http://lpis.ec.europa.eu/registry/applicationschema/cap-iacs-control/code#ControlRateTypeValue/atLeast5%OfAreasCoveredBySensitiveGrassland -->


    <owl:NamedIndividual rdf:about="http://lpis.ec.europa.eu/registry/applicationschema/cap-iacs-control/code#ControlRateTypeValue/atLeast5%OfAreasCoveredBySensitiveGrassland">
        <rdf:type rdf:resource="http://lpis.ec.europa.eu/registry/applicationschema/cap-iacs-control#ControlRateTypeValue"/>
        <rdfs:label xml:lang="en">At least 5% of all beneficiaries required to observe the agricultural practices having areas covered with permanent grasslands</rdfs:label>
        <skos:definition xml:lang="en">At least 5% of areas covered by sensitive grassland

The greenling sample in sense of Art. 31(1) of R (EU) 809/2014 shall cover at least 5 % of all beneficiaries having areas covered with permanent grasslands which are environmentally sensitive in areas covered by Council Directive 92/43/EEC[18] or Directive 2009/147/EC of the European Parliament and of the Council[19] and further sensitive areas referred to in Article 45(1) of Regulation (EU) No 1307/2013.</skos:definition>
        <skos:inScheme rdf:resource="http://lpis.ec.europa.eu/registry/applicationschema/cap-iacs-control/code#ControlRateTypeValue"/>
    </owl:NamedIndividual>
    


    <!-- http://lpis.ec.europa.eu/registry/applicationschema/cap-iacs-control/code#ControlRateTypeValue/atLeast5%OfCollectiveImplementation -->


    <owl:NamedIndividual rdf:about="http://lpis.ec.europa.eu/registry/applicationschema/cap-iacs-control/code#ControlRateTypeValue/atLeast5%OfCollectiveImplementation">
        <rdf:type rdf:resource="http://lpis.ec.europa.eu/registry/applicationschema/cap-iacs-control#ControlRateTypeValue"/>
        <rdfs:label xml:lang="en">At least 5 % of  the  collective implementation</rdfs:label>
        <skos:definition xml:lang="en">At least 5 % of the collective implementation

In sensed of Art. 31(1)(e) od R EU) 809/2014 5 % of  the  collective implementation in accordance with Article 46(6) of Regulation (EU) No 1307/2013 shall be controlled.</skos:definition>
        <skos:inScheme rdf:resource="http://lpis.ec.europa.eu/registry/applicationschema/cap-iacs-control/code#ControlRateTypeValue"/>
    </owl:NamedIndividual>
    


    <!-- http://lpis.ec.europa.eu/registry/applicationschema/cap-iacs-control/code#ControlRateTypeValue/atLeast5%OfFollowingGreeningByUsingEnvironmentalCertificationSchemes -->


    <owl:NamedIndividual rdf:about="http://lpis.ec.europa.eu/registry/applicationschema/cap-iacs-control/code#ControlRateTypeValue/atLeast5%OfFollowingGreeningByUsingEnvironmentalCertificationSchemes">
        <rdf:type rdf:resource="http://lpis.ec.europa.eu/registry/applicationschema/cap-iacs-control#ControlRateTypeValue"/>
        <rdfs:label xml:lang="en">At least 5 % of all beneficiaries required to observe the greening practices and using national or regional environmental certification schemes</rdfs:label>
        <skos:definition xml:lang="en">At least 5 % following greening practices by using environmental certification schemes

In sense of Art. 31(1)(c) 5 % of beneficiaries observing greening practices and using national or regional environmental certification schemes as referred to in Article 43(3)(b) of Regulation (EU) No 1307/2013 shall be controlled.</skos:definition>
        <skos:inScheme rdf:resource="http://lpis.ec.europa.eu/registry/applicationschema/cap-iacs-control/code#ControlRateTypeValue"/>
    </owl:NamedIndividual>
    


    <!-- http://lpis.ec.europa.eu/registry/applicationschema/cap-iacs-control/code#ControlRateTypeValue/atLeast5%OfFollowingGreeningPractices -->


    <owl:NamedIndividual rdf:about="http://lpis.ec.europa.eu/registry/applicationschema/cap-iacs-control/code#ControlRateTypeValue/atLeast5%OfFollowingGreeningPractices">
        <rdf:type rdf:resource="http://lpis.ec.europa.eu/registry/applicationschema/cap-iacs-control#ControlRateTypeValue"/>
        <rdfs:label xml:lang="en">At least 5% of all beneficiaries required to observe the agricultural practices having areas covered with permanent grasslands</rdfs:label>
        <skos:definition xml:lang="en">At least 5% of following greening practices

In sense of Art. 31(1) 5% of beneficiaries required to follow greening practices shall be controlled.</skos:definition>
        <skos:inScheme rdf:resource="http://lpis.ec.europa.eu/registry/applicationschema/cap-iacs-control/code#ControlRateTypeValue"/>
    </owl:NamedIndividual>
    


    <!-- http://lpis.ec.europa.eu/registry/applicationschema/cap-iacs-control/code#ControlRateTypeValue/atLeast5%OfRegionalImplementation -->


    <owl:NamedIndividual rdf:about="http://lpis.ec.europa.eu/registry/applicationschema/cap-iacs-control/code#ControlRateTypeValue/atLeast5%OfRegionalImplementation">
        <rdf:type rdf:resource="http://lpis.ec.europa.eu/registry/applicationschema/cap-iacs-control#ControlRateTypeValue"/>
        <rdfs:label xml:lang="en">At least  5 % of all beneficiaries participating in a regional implementation</rdfs:label>
        <skos:definition xml:lang="en">At least 5 % of all beneficiaries participating in a regional implementation

In sense of Art.31(1)(d)  of R (EU) 809/2014 5 % of all beneficiaries participating in a regional implementation in accordance with Article 46(5) of Regulation (EU) No 1307/2013 shall be controlled.</skos:definition>
        <skos:inScheme rdf:resource="http://lpis.ec.europa.eu/registry/applicationschema/cap-iacs-control/code#ControlRateTypeValue"/>
    </owl:NamedIndividual>
    


    <!-- http://lpis.ec.europa.eu/registry/applicationschema/cap-iacs-control/code#ControlRateTypeValue/atLeast5%ForBps/Saps -->


    <owl:NamedIndividual rdf:about="http://lpis.ec.europa.eu/registry/applicationschema/cap-iacs-control/code#ControlRateTypeValue/atLeast5%ForBps/Saps">
        <rdf:type rdf:resource="http://lpis.ec.europa.eu/registry/applicationschema/cap-iacs-control#ControlRateTypeValue"/>
        <rdfs:label xml:lang="en">At least 5% of all beneficiaries required to observe the agricultural practices having areas covered with permanent grasslands</rdfs:label>
        <skos:definition xml:lang="en">At least 5% for BPS or SAPS

In sense of Art. 30(a) of Regulation (EU) 809/2014 5% of beneficiaries applying for the basic payment or single area payment scheme shall be controlled.

This control sample shall contain at least 5 % of all beneficiaries declaring mainly agricultural areas which are areas naturally kept in a state suitable for grazing in accordance with Article 10(1) of Delegated Regulation (EU) No 639/2014.</skos:definition>
        <skos:inScheme rdf:resource="http://lpis.ec.europa.eu/registry/applicationschema/cap-iacs-control/code#ControlRateTypeValue"/>
    </owl:NamedIndividual>
    


    <!-- http://lpis.ec.europa.eu/registry/applicationschema/cap-iacs-control/code#CrossCheckTypeValue/betweenAgriculturalParcelsAndReferenceParcels -->


    <owl:NamedIndividual rdf:about="http://lpis.ec.europa.eu/registry/applicationschema/cap-iacs-control/code#CrossCheckTypeValue/betweenAgriculturalParcelsAndReferenceParcels">
        <rdf:type rdf:resource="http://lpis.ec.europa.eu/registry/applicationschema/cap-iacs-control#CrossCheckTypeValue"/>
        <rdfs:label xml:lang="en">Between agricultural parcels and reference parcels</rdfs:label>
        <skos:definition xml:lang="en">-- Definition --
Between agricultural parcels and reference parcels.
-- Description --
Where appropriate, the administrative checks shall include cross-checks: between the agricultural parcels as declared in the single application and/or payment claim and the information as contained in the identification system for 
agricultural parcels per reference parcel in accordance with Article 5(2) of Regulation (EU) No […] [DA IACS] to verify the eligibility for direct aid scheme and/or rural development support measure of the areas as such.
NOTE. Where the integrated system provides for geo-spatial aid application forms, the cross-checks shall be carried out as spatial intersection of the digitised area declared with the identification system of agricultural parcels. In 
addition, cross-checks shall be carried out to prevent double claiming of the same area.</skos:definition>
        <skos:inScheme rdf:resource="http://lpis.ec.europa.eu/registry/applicationschema/cap-iacs-control/code#CrossCheckTypeValue"/>
    </owl:NamedIndividual>
    


    <!-- http://lpis.ec.europa.eu/registry/applicationschema/cap-iacs-control/code#CrossCheckTypeValue/betweenInterBranchOrganisationsAndTheListOfTheirMembers -->


    <owl:NamedIndividual rdf:about="http://lpis.ec.europa.eu/registry/applicationschema/cap-iacs-control/code#CrossCheckTypeValue/betweenInterBranchOrganisationsAndTheListOfTheirMembers">
        <rdf:type rdf:resource="http://lpis.ec.europa.eu/registry/applicationschema/cap-iacs-control#CrossCheckTypeValue"/>
        <rdfs:label xml:lang="en">Between inter-branch organisations and the list of their members</rdfs:label>
        <skos:definition xml:lang="en">-- Definition --
Between inter-branch organisations and the list of their members.
-- Description --
Where appropriate, the administrative checks shall include cross-checks: the compliance with  the  criteria for the approval of inter-branch organisations and the list of their members shall be verified at least once every 5 years.</skos:definition>
        <skos:inScheme rdf:resource="http://lpis.ec.europa.eu/registry/applicationschema/cap-iacs-control/code#CrossCheckTypeValue"/>
    </owl:NamedIndividual>
    


    <!-- http://lpis.ec.europa.eu/registry/applicationschema/cap-iacs-control/code#CrossCheckTypeValue/betweenThePaymentEntitlementsAndTheAreaDetermined -->


    <owl:NamedIndividual rdf:about="http://lpis.ec.europa.eu/registry/applicationschema/cap-iacs-control/code#CrossCheckTypeValue/betweenThePaymentEntitlementsAndTheAreaDetermined">
        <rdf:type rdf:resource="http://lpis.ec.europa.eu/registry/applicationschema/cap-iacs-control#CrossCheckTypeValue"/>
        <rdfs:label xml:lang="en">Between the payment entitlements and the area determined</rdfs:label>
        <skos:definition xml:lang="en">-- Definition --
Between the payment entitlements and the area determined.
-- Description --
Where appropriate, the administrative checks shall include cross-checks:between the payment entitlements and the area determined in order to verify that the entitlements are accompanied by at least an equal number of eligible hectares 
as defined in Article 32(2) to (6) of Regulation (EC) No 1307/2013.</skos:definition>
        <skos:inScheme rdf:resource="http://lpis.ec.europa.eu/registry/applicationschema/cap-iacs-control/code#CrossCheckTypeValue"/>
    </owl:NamedIndividual>
    


    <!-- http://lpis.ec.europa.eu/registry/applicationschema/cap-iacs-control/code#CrossCheckTypeValue/toVerifyDeclaredEntitlementsOnDeclaredAgriculturalParcels -->


    <owl:NamedIndividual rdf:about="http://lpis.ec.europa.eu/registry/applicationschema/cap-iacs-control/code#CrossCheckTypeValue/toVerifyDeclaredEntitlementsOnDeclaredAgriculturalParcels">
        <rdf:type rdf:resource="http://lpis.ec.europa.eu/registry/applicationschema/cap-iacs-control#CrossCheckTypeValue"/>
        <rdfs:label xml:lang="en">Verify declared payment entitlements on declared agricultural parcels</rdfs:label>
        <skos:definition xml:lang="en">-- Definition --
Verify declared payment entitlements on declared agricultural parcels.
-- Description --
Where appropriate, the administrative checks shall include cross-checks:o n declared payment entitlements and on declared agricultural parcels, respectively, in order to avoid multiple granting of the same aid or support in respect of 
the same calendar or claim year and to prevent any undue accumulation of aid granted under area-related aid schemes listed in Annex I to Regulation (EU) No 1307/2013 and Annex VI to Council Regulation (EC) No 73/2009[17], and area-
related support measures as defined in point (21) of the second subparagraph of Article 2 of Delegated Regulation (EU) No […] [DA IACS].</skos:definition>
        <skos:inScheme rdf:resource="http://lpis.ec.europa.eu/registry/applicationschema/cap-iacs-control/code#CrossCheckTypeValue"/>
    </owl:NamedIndividual>
    


    <!-- http://lpis.ec.europa.eu/registry/applicationschema/cap-iacs-control/code#CrossCheckTypeValue/toVerifyEligibilityForTheAnimalAid -->


    <owl:NamedIndividual rdf:about="http://lpis.ec.europa.eu/registry/applicationschema/cap-iacs-control/code#CrossCheckTypeValue/toVerifyEligibilityForTheAnimalAid">
        <rdf:type rdf:resource="http://lpis.ec.europa.eu/registry/applicationschema/cap-iacs-control#CrossCheckTypeValue"/>
        <rdfs:label xml:lang="en">Verify eligibility for the animal aid</rdfs:label>
        <skos:definition xml:lang="en">-- Definition --
Verify eligibility for the animal aid.
-- Description --
Where appropriate, the administrative checks shall include cross-checks: by means of the system for the identification and registration of animals, to verify eligibility for the aid and/or support and to avoid undue multiple granting of 
the same aid and/or support in respect of the same calendar or claim year.</skos:definition>
        <skos:inScheme rdf:resource="http://lpis.ec.europa.eu/registry/applicationschema/cap-iacs-control/code#CrossCheckTypeValue"/>
    </owl:NamedIndividual>
    


    <!-- http://lpis.ec.europa.eu/registry/applicationschema/cap-iacs-control/code#CrossCheckTypeValue/toVerifyEligibilityForTheIncreaseOfTheAid -->


    <owl:NamedIndividual rdf:about="http://lpis.ec.europa.eu/registry/applicationschema/cap-iacs-control/code#CrossCheckTypeValue/toVerifyEligibilityForTheIncreaseOfTheAid">
        <rdf:type rdf:resource="http://lpis.ec.europa.eu/registry/applicationschema/cap-iacs-control#CrossCheckTypeValue"/>
        <rdfs:label xml:lang="en">Verify eligibility for the increase of the aid</rdfs:label>
        <skos:definition xml:lang="en">-- Definition --
Verify eligibility for the increase of the aid.
-- Description --
Where appropriate, the administrative checks shall include cross-checks:between the declarations of the beneficiary in the single application to be a member of an approved inter-branch organisation, the information under Article 16(8) 
of this Regulation and the information transmitted by the approved inter-branch organisations concerned, to verify eligibility for the increase of the aid provided for in Article 60(2) of Regulation (EU) No 1307/2013.</skos:definition>
        <skos:inScheme rdf:resource="http://lpis.ec.europa.eu/registry/applicationschema/cap-iacs-control/code#CrossCheckTypeValue"/>
    </owl:NamedIndividual>
    


    <!-- http://lpis.ec.europa.eu/registry/applicationschema/cap-iacs-control/code#CrossCheckTypeValue/toVerifyPaymentEntitlements -->


    <owl:NamedIndividual rdf:about="http://lpis.ec.europa.eu/registry/applicationschema/cap-iacs-control/code#CrossCheckTypeValue/toVerifyPaymentEntitlements">
        <rdf:type rdf:resource="http://lpis.ec.europa.eu/registry/applicationschema/cap-iacs-control#CrossCheckTypeValue"/>
        <rdfs:label xml:lang="en">Verify payment entitlements</rdfs:label>
        <skos:definition xml:lang="en">-- Definition --
Verify payment entitlements.
-- Description --
Where appropriate, the administrative checks shall include cross-checks: on the payment entitlements to verify their existence and the eligibility.</skos:definition>
        <skos:inScheme rdf:resource="http://lpis.ec.europa.eu/registry/applicationschema/cap-iacs-control/code#CrossCheckTypeValue"/>
    </owl:NamedIndividual>
    


    <!-- http://lpis.ec.europa.eu/registry/applicationschema/cap-iacs-control/code#InspectorsSurveyObjectTypeValue/agriculturalArea -->


    <owl:NamedIndividual rdf:about="http://lpis.ec.europa.eu/registry/applicationschema/cap-iacs-control/code#InspectorsSurveyObjectTypeValue/agriculturalArea">
        <rdf:type rdf:resource="http://lpis.ec.europa.eu/registry/applicationschema/cap-iacs-control#InspectorsSurveyObjectTypeValue"/>
        <rdfs:label xml:lang="en">Agricultural area</rdfs:label>
        <skos:definition xml:lang="en">Agricultural area

Agricultural area as defined by R (EU) 1307/2013.</skos:definition>
        <skos:inScheme rdf:resource="http://lpis.ec.europa.eu/registry/applicationschema/cap-iacs-control/code#InspectorsSurveyObjectTypeValue"/>
    </owl:NamedIndividual>
    


    <!-- http://lpis.ec.europa.eu/registry/applicationschema/cap-iacs-control/code#InspectorsSurveyObjectTypeValue/agriculturalParcel -->


    <owl:NamedIndividual rdf:about="http://lpis.ec.europa.eu/registry/applicationschema/cap-iacs-control/code#InspectorsSurveyObjectTypeValue/agriculturalParcel">
        <rdf:type rdf:resource="http://lpis.ec.europa.eu/registry/applicationschema/cap-iacs-control#InspectorsSurveyObjectTypeValue"/>
        <rdfs:label xml:lang="en">Agricultural parcel</rdfs:label>
        <skos:definition xml:lang="en">Agricultural parcel

Agricultural parcel as defined by R (EU) 1307/2013.</skos:definition>
        <skos:inScheme rdf:resource="http://lpis.ec.europa.eu/registry/applicationschema/cap-iacs-control/code#InspectorsSurveyObjectTypeValue"/>
    </owl:NamedIndividual>
    


    <!-- http://lpis.ec.europa.eu/registry/applicationschema/cap-iacs-control/code#InspectorsSurveyObjectTypeValue/ecologicalFocusArea -->


    <owl:NamedIndividual rdf:about="http://lpis.ec.europa.eu/registry/applicationschema/cap-iacs-control/code#InspectorsSurveyObjectTypeValue/ecologicalFocusArea">
        <rdf:type rdf:resource="http://lpis.ec.europa.eu/registry/applicationschema/cap-iacs-control#InspectorsSurveyObjectTypeValue"/>
        <rdfs:label xml:lang="en">Ecological focus area</rdfs:label>
        <skos:definition xml:lang="en">Ecological focus area

Ecological focus areas as referred to in Article 46 of R (EU) No1307/2013 and its Delegated Regulation (EU) No 639/2014.</skos:definition>
        <skos:inScheme rdf:resource="http://lpis.ec.europa.eu/registry/applicationschema/cap-iacs-control/code#InspectorsSurveyObjectTypeValue"/>
    </owl:NamedIndividual>
    


    <!-- http://lpis.ec.europa.eu/registry/applicationschema/cap-iacs-control/code#InspectorsSurveyObjectTypeValue/holdingSite -->


    <owl:NamedIndividual rdf:about="http://lpis.ec.europa.eu/registry/applicationschema/cap-iacs-control/code#InspectorsSurveyObjectTypeValue/holdingSite">
        <rdf:type rdf:resource="http://lpis.ec.europa.eu/registry/applicationschema/cap-iacs-control#InspectorsSurveyObjectTypeValue"/>
        <rdfs:label xml:lang="en">Holding site</rdfs:label>
        <skos:definition xml:lang="en">Holding site

Measurement of the whole holding.</skos:definition>
        <skos:inScheme rdf:resource="http://lpis.ec.europa.eu/registry/applicationschema/cap-iacs-control/code#InspectorsSurveyObjectTypeValue"/>
    </owl:NamedIndividual>
    


    <!-- http://lpis.ec.europa.eu/registry/applicationschema/cap-iacs-control/code#InspectorsSurveyObjectTypeValue/referenceParcel -->


    <owl:NamedIndividual rdf:about="http://lpis.ec.europa.eu/registry/applicationschema/cap-iacs-control/code#InspectorsSurveyObjectTypeValue/referenceParcel">
        <rdf:type rdf:resource="http://lpis.ec.europa.eu/registry/applicationschema/cap-iacs-control#InspectorsSurveyObjectTypeValue"/>
        <rdfs:label xml:lang="en">Reference parcel</rdfs:label>
        <skos:definition xml:lang="en">Reference parcel

Reference parcel as defined in R (EU) 1307/2013.</skos:definition>
        <skos:inScheme rdf:resource="http://lpis.ec.europa.eu/registry/applicationschema/cap-iacs-control/code#InspectorsSurveyObjectTypeValue"/>
    </owl:NamedIndividual>
    


    <!-- http://lpis.ec.europa.eu/registry/applicationschema/cap-iacs-control/code#OnTheSpotCheckTypeValue/commitmentsAndObligations -->


    <owl:NamedIndividual rdf:about="http://lpis.ec.europa.eu/registry/applicationschema/cap-iacs-control/code#OnTheSpotCheckTypeValue/commitmentsAndObligations">
        <rdf:type rdf:resource="http://lpis.ec.europa.eu/registry/applicationschema/cap-iacs-control#OnTheSpotCheckTypeValue"/>
        <rdfs:label xml:lang="en">Cross compliance</rdfs:label>
        <skos:definition xml:lang="en">Cross compliance

OTSC in sense of Art. 96(3) of R 1306/2013 and Art. 26(3) of R 809/2014.</skos:definition>
        <skos:inScheme rdf:resource="http://lpis.ec.europa.eu/registry/applicationschema/cap-iacs-control/code#OnTheSpotCheckTypeValue"/>
    </owl:NamedIndividual>
    


    <!-- http://lpis.ec.europa.eu/registry/applicationschema/cap-iacs-control/code#OnTheSpotCheckTypeValue/complianceToEuLaw -->


    <owl:NamedIndividual rdf:about="http://lpis.ec.europa.eu/registry/applicationschema/cap-iacs-control/code#OnTheSpotCheckTypeValue/complianceToEuLaw">
        <rdf:type rdf:resource="http://lpis.ec.europa.eu/registry/applicationschema/cap-iacs-control#OnTheSpotCheckTypeValue"/>
        <rdfs:label xml:lang="en">Cross compliance</rdfs:label>
        <skos:definition xml:lang="en">Compliance to EU law

As required by Art. 24(2) of R 809/2014.</skos:definition>
        <skos:inScheme rdf:resource="http://lpis.ec.europa.eu/registry/applicationschema/cap-iacs-control/code#OnTheSpotCheckTypeValue"/>
    </owl:NamedIndividual>
    


    <!-- http://lpis.ec.europa.eu/registry/applicationschema/cap-iacs-control/code#OnTheSpotCheckTypeValue/complianceToNationalLaw -->


    <owl:NamedIndividual rdf:about="http://lpis.ec.europa.eu/registry/applicationschema/cap-iacs-control/code#OnTheSpotCheckTypeValue/complianceToNationalLaw">
        <rdf:type rdf:resource="http://lpis.ec.europa.eu/registry/applicationschema/cap-iacs-control#OnTheSpotCheckTypeValue"/>
        <rdfs:label xml:lang="en">Cross compliance</rdfs:label>
        <skos:definition xml:lang="en">Compliance to national law

As required by Art. 24(2) of R 809/2014.</skos:definition>
        <skos:inScheme rdf:resource="http://lpis.ec.europa.eu/registry/applicationschema/cap-iacs-control/code#OnTheSpotCheckTypeValue"/>
    </owl:NamedIndividual>
    


    <!-- http://lpis.ec.europa.eu/registry/applicationschema/cap-iacs-control/code#OnTheSpotCheckTypeValue/controlArea -->


    <owl:NamedIndividual rdf:about="http://lpis.ec.europa.eu/registry/applicationschema/cap-iacs-control/code#OnTheSpotCheckTypeValue/controlArea">
        <rdf:type rdf:resource="http://lpis.ec.europa.eu/registry/applicationschema/cap-iacs-control#OnTheSpotCheckTypeValue"/>
        <rdfs:label xml:lang="en">Control area</rdfs:label>
        <skos:definition xml:lang="en">Control area

Verification of the declared area values by means of measurements.</skos:definition>
        <skos:inScheme rdf:resource="http://lpis.ec.europa.eu/registry/applicationschema/cap-iacs-control/code#OnTheSpotCheckTypeValue"/>
    </owl:NamedIndividual>
    


    <!-- http://lpis.ec.europa.eu/registry/applicationschema/cap-iacs-control/code#OnTheSpotCheckTypeValue/correctnessAndCompletenessOfInformation -->


    <owl:NamedIndividual rdf:about="http://lpis.ec.europa.eu/registry/applicationschema/cap-iacs-control/code#OnTheSpotCheckTypeValue/correctnessAndCompletenessOfInformation">
        <rdf:type rdf:resource="http://lpis.ec.europa.eu/registry/applicationschema/cap-iacs-control#OnTheSpotCheckTypeValue"/>
        <rdfs:label xml:lang="en">Cross compliance</rdfs:label>
        <skos:definition xml:lang="en">Correctness and completeness of the information

As required by Art. 24(1)(a) of R 809/2014.</skos:definition>
        <skos:inScheme rdf:resource="http://lpis.ec.europa.eu/registry/applicationschema/cap-iacs-control/code#OnTheSpotCheckTypeValue"/>
    </owl:NamedIndividual>
    


    <!-- http://lpis.ec.europa.eu/registry/applicationschema/cap-iacs-control/code#OnTheSpotCheckTypeValue/crossCompliance -->


    <owl:NamedIndividual rdf:about="http://lpis.ec.europa.eu/registry/applicationschema/cap-iacs-control/code#OnTheSpotCheckTypeValue/crossCompliance">
        <rdf:type rdf:resource="http://lpis.ec.europa.eu/registry/applicationschema/cap-iacs-control#OnTheSpotCheckTypeValue"/>
        <rdfs:label xml:lang="en">Cross compliance</rdfs:label>
        <skos:definition xml:lang="en">Cross compliance

OTSC in sense of Art. 96(3) of R 1306/2013.</skos:definition>
        <skos:inScheme rdf:resource="http://lpis.ec.europa.eu/registry/applicationschema/cap-iacs-control/code#OnTheSpotCheckTypeValue"/>
    </owl:NamedIndividual>
    


    <!-- http://lpis.ec.europa.eu/registry/applicationschema/cap-iacs-control/code#OnTheSpotCheckTypeValue/crossComplianceStandards -->


    <owl:NamedIndividual rdf:about="http://lpis.ec.europa.eu/registry/applicationschema/cap-iacs-control/code#OnTheSpotCheckTypeValue/crossComplianceStandards">
        <rdf:type rdf:resource="http://lpis.ec.europa.eu/registry/applicationschema/cap-iacs-control#OnTheSpotCheckTypeValue"/>
        <rdfs:label xml:lang="en">Cross compliance</rdfs:label>
        <skos:definition xml:lang="en">Cross compliance standards

As required by Art. 24(1)(c) of R 809/2014.</skos:definition>
        <skos:inScheme rdf:resource="http://lpis.ec.europa.eu/registry/applicationschema/cap-iacs-control/code#OnTheSpotCheckTypeValue"/>
    </owl:NamedIndividual>
    


    <!-- http://lpis.ec.europa.eu/registry/applicationschema/cap-iacs-control/code#OnTheSpotCheckTypeValue/eligibilityCriteria -->


    <owl:NamedIndividual rdf:about="http://lpis.ec.europa.eu/registry/applicationschema/cap-iacs-control/code#OnTheSpotCheckTypeValue/eligibilityCriteria">
        <rdf:type rdf:resource="http://lpis.ec.europa.eu/registry/applicationschema/cap-iacs-control#OnTheSpotCheckTypeValue"/>
        <rdfs:label xml:lang="en">Cross compliance</rdfs:label>
        <skos:definition xml:lang="en">Cross compliance

OTSC in sense of Art. 96(3) of R 1306/2013, Art. 24(1)(b) and 26(3) of R 809/2014.</skos:definition>
        <skos:inScheme rdf:resource="http://lpis.ec.europa.eu/registry/applicationschema/cap-iacs-control/code#OnTheSpotCheckTypeValue"/>
    </owl:NamedIndividual>
    


    <!-- http://lpis.ec.europa.eu/registry/applicationschema/cap-iacs-control/code#OnTheSpotCheckTypeValue/supportingDocuments -->


    <owl:NamedIndividual rdf:about="http://lpis.ec.europa.eu/registry/applicationschema/cap-iacs-control/code#OnTheSpotCheckTypeValue/supportingDocuments">
        <rdf:type rdf:resource="http://lpis.ec.europa.eu/registry/applicationschema/cap-iacs-control#OnTheSpotCheckTypeValue"/>
        <rdfs:label xml:lang="en">Control cross-compliance</rdfs:label>
        <skos:definition xml:lang="en">Supporting Documents

Verification of the existence of the requisite supporting documents [Art. 47(1)(b) of  R 1306/2013]</skos:definition>
        <skos:inScheme rdf:resource="http://lpis.ec.europa.eu/registry/applicationschema/cap-iacs-control/code#OnTheSpotCheckTypeValue"/>
    </owl:NamedIndividual>
    


    <!-- http://lpis.ec.europa.eu/registry/applicationschema/cap-iacs-control/code#RiskTypeValue/areaOfIntensiveLcOrLuChange -->


    <owl:NamedIndividual rdf:about="http://lpis.ec.europa.eu/registry/applicationschema/cap-iacs-control/code#RiskTypeValue/areaOfIntensiveLcOrLuChange">
        <rdf:type rdf:resource="http://lpis.ec.europa.eu/registry/applicationschema/cap-iacs-control#RiskTypeValue"/>
        <skos:definition xml:lang="en">Areas of Intensive LC or LU change

Areas of intensive land cover and land use change may be detected in third party data e.g.
	- orthoimagery
	- cadastral maps
	- road maps
	- topographic maps
	- development plans</skos:definition>
        <skos:inScheme rdf:resource="http://lpis.ec.europa.eu/registry/applicationschema/cap-iacs-control/code#RiskTypeValue"/>
    </owl:NamedIndividual>
    


    <!-- http://lpis.ec.europa.eu/registry/applicationschema/cap-iacs-control/code#RiskTypeValue/eligibilityCriteria -->


    <owl:NamedIndividual rdf:about="http://lpis.ec.europa.eu/registry/applicationschema/cap-iacs-control/code#RiskTypeValue/eligibilityCriteria">
        <rdf:type rdf:resource="http://lpis.ec.europa.eu/registry/applicationschema/cap-iacs-control#RiskTypeValue"/>
        <skos:definition xml:lang="en">Eligibility Criteria

Member States are also authorised to draw the control sample on the basis of the samples of beneficiaries that are selected for an on-the-spot check as regards eligibility criteria. [Preamble (71) of R 809/2014].</skos:definition>
        <skos:inScheme rdf:resource="http://lpis.ec.europa.eu/registry/applicationschema/cap-iacs-control/code#RiskTypeValue"/>
    </owl:NamedIndividual>
    


    <!-- http://lpis.ec.europa.eu/registry/applicationschema/cap-iacs-control/code#RiskTypeValue/nonParticipationInCertificationScheme -->


    <owl:NamedIndividual rdf:about="http://lpis.ec.europa.eu/registry/applicationschema/cap-iacs-control/code#RiskTypeValue/nonParticipationInCertificationScheme">
        <rdf:type rdf:resource="http://lpis.ec.europa.eu/registry/applicationschema/cap-iacs-control#RiskTypeValue"/>
        <skos:definition xml:lang="en">Non-participation in certification scheme

At risk based sampling MS may consider beneficiary’s participation in a certification system if the scheme in question is relevant for the requirements and standards concerned [Art. 69(1)(b) of R 809/2014].</skos:definition>
        <skos:inScheme rdf:resource="http://lpis.ec.europa.eu/registry/applicationschema/cap-iacs-control/code#RiskTypeValue"/>
    </owl:NamedIndividual>
    


    <!-- http://lpis.ec.europa.eu/registry/applicationschema/cap-iacs-control/code#RiskTypeValue/nonParticipationInFas -->


    <owl:NamedIndividual rdf:about="http://lpis.ec.europa.eu/registry/applicationschema/cap-iacs-control/code#RiskTypeValue/nonParticipationInFas">
        <rdf:type rdf:resource="http://lpis.ec.europa.eu/registry/applicationschema/cap-iacs-control#RiskTypeValue"/>
        <skos:definition xml:lang="en">Non participation in FAS

Sampling of OTSC for cross-compliance can be improved by taking into account the risk analysis concerning the beneficiary’s participation in the farm advisory system [Preamble (69) and Art. 69(1)(a) of R 809/2014].</skos:definition>
        <skos:inScheme rdf:resource="http://lpis.ec.europa.eu/registry/applicationschema/cap-iacs-control/code#RiskTypeValue"/>
    </owl:NamedIndividual>
    


    <!-- http://lpis.ec.europa.eu/registry/applicationschema/cap-iacs-control/code#SampleTypeValue/areasWithNaturalConstraints -->


    <owl:NamedIndividual rdf:about="http://lpis.ec.europa.eu/registry/applicationschema/cap-iacs-control/code#SampleTypeValue/areasWithNaturalConstraints">
        <rdf:type rdf:resource="http://lpis.ec.europa.eu/registry/applicationschema/cap-iacs-control#SampleTypeValue"/>
        <skos:definition xml:lang="en">Areas with natural constraints

Item selected for controlling the correctness of payments for areas with natural constraints.</skos:definition>
        <skos:inScheme rdf:resource="http://lpis.ec.europa.eu/registry/applicationschema/cap-iacs-control/code#SampleTypeValue"/>
    </owl:NamedIndividual>
    


    <!-- http://lpis.ec.europa.eu/registry/applicationschema/cap-iacs-control/code#SampleTypeValue/collectiveImplementation -->


    <owl:NamedIndividual rdf:about="http://lpis.ec.europa.eu/registry/applicationschema/cap-iacs-control/code#SampleTypeValue/collectiveImplementation">
        <rdf:type rdf:resource="http://lpis.ec.europa.eu/registry/applicationschema/cap-iacs-control#SampleTypeValue"/>
        <skos:definition xml:lang="en">Collective implementation

Items selected for controlling beneficiaries participating in collective implementation of EFA. The composition of the population
	- 1,0-1,25% selected randomly 
	- 3,75-4,0% selected on risk base

Issue:
The purpose of collective implementation (See Art. 46(a) of 1307/2013) and regional implementation (see Art. 46(3) of R 639/2014) is to form contiguous areas of EFA. If so, what is the reason to have separate samples for collective implementation, regional implementation and contiguous EFA?</skos:definition>
        <skos:inScheme rdf:resource="http://lpis.ec.europa.eu/registry/applicationschema/cap-iacs-control/code#SampleTypeValue"/>
    </owl:NamedIndividual>
    


    <!-- http://lpis.ec.europa.eu/registry/applicationschema/cap-iacs-control/code#SampleTypeValue/contiguousEfa -->


    <owl:NamedIndividual rdf:about="http://lpis.ec.europa.eu/registry/applicationschema/cap-iacs-control/code#SampleTypeValue/contiguousEfa">
        <rdf:type rdf:resource="http://lpis.ec.europa.eu/registry/applicationschema/cap-iacs-control#SampleTypeValue"/>
        <skos:definition xml:lang="en">Contiguous EFA

Items selected for controlling contiguous EFA

Issue:
The purpose of collective implementation (See Art. 46(a) of 1307/2013) and regional implementation (see Art. 46(3) of R 639/2014) is to form contiguous areas of EFA. If so, what is the reason to have separate samples for collective implementation, regional implementation and contiguous EFA?</skos:definition>
        <skos:inScheme rdf:resource="http://lpis.ec.europa.eu/registry/applicationschema/cap-iacs-control/code#SampleTypeValue"/>
    </owl:NamedIndividual>
    


    <!-- http://lpis.ec.europa.eu/registry/applicationschema/cap-iacs-control/code#SampleTypeValue/cotton -->


    <owl:NamedIndividual rdf:about="http://lpis.ec.europa.eu/registry/applicationschema/cap-iacs-control/code#SampleTypeValue/cotton">
        <rdf:type rdf:resource="http://lpis.ec.europa.eu/registry/applicationschema/cap-iacs-control#SampleTypeValue"/>
        <skos:definition xml:lang="en">Cotton

Item selected for controlling beneficiaries applying for the specific payment for cotton.</skos:definition>
        <skos:inScheme rdf:resource="http://lpis.ec.europa.eu/registry/applicationschema/cap-iacs-control/code#SampleTypeValue"/>
    </owl:NamedIndividual>
    


    <!-- http://lpis.ec.europa.eu/registry/applicationschema/cap-iacs-control/code#SampleTypeValue/exemptedFromGreening -->


    <owl:NamedIndividual rdf:about="http://lpis.ec.europa.eu/registry/applicationschema/cap-iacs-control/code#SampleTypeValue/exemptedFromGreening">
        <rdf:type rdf:resource="http://lpis.ec.europa.eu/registry/applicationschema/cap-iacs-control#SampleTypeValue"/>
        <skos:definition xml:lang="en">Exempted from greening

Items selected to control beneficiaries exempted from greening obligations by not meeting the specified thresholds.  They include:
	- Beneficiaries exempted from crop diversification (Art. 44(3) of R 1307/2013)
	- Beneficiaries exempted from EFA (Art. 46 (1) of R 307/2013)</skos:definition>
        <skos:inScheme rdf:resource="http://lpis.ec.europa.eu/registry/applicationschema/cap-iacs-control/code#SampleTypeValue"/>
    </owl:NamedIndividual>
    


    <!-- http://lpis.ec.europa.eu/registry/applicationschema/cap-iacs-control/code#SampleTypeValue/hemp -->


    <owl:NamedIndividual rdf:about="http://lpis.ec.europa.eu/registry/applicationschema/cap-iacs-control/code#SampleTypeValue/hemp">
        <rdf:type rdf:resource="http://lpis.ec.europa.eu/registry/applicationschema/cap-iacs-control#SampleTypeValue"/>
        <skos:definition xml:lang="en">Hemp

Items selected for controlling beneficiaries growing hemp.</skos:definition>
        <skos:inScheme rdf:resource="http://lpis.ec.europa.eu/registry/applicationschema/cap-iacs-control/code#SampleTypeValue"/>
    </owl:NamedIndividual>
    


    <!-- http://lpis.ec.europa.eu/registry/applicationschema/cap-iacs-control/code#SampleTypeValue/observingGreening -->


    <owl:NamedIndividual rdf:about="http://lpis.ec.europa.eu/registry/applicationschema/cap-iacs-control/code#SampleTypeValue/observingGreening">
        <rdf:type rdf:resource="http://lpis.ec.europa.eu/registry/applicationschema/cap-iacs-control#SampleTypeValue"/>
        <skos:definition xml:lang="en">Observing greening

Items selected for controlling beneficiaries observing greening. The composition of the population
	- 1,0-1,25% selected randomly 
	- 3,75-4,0% selected on risk base
The related sample includes items selected for the sensitive grassland sample.</skos:definition>
        <skos:inScheme rdf:resource="http://lpis.ec.europa.eu/registry/applicationschema/cap-iacs-control/code#SampleTypeValue"/>
    </owl:NamedIndividual>
    


    <!-- http://lpis.ec.europa.eu/registry/applicationschema/cap-iacs-control/code#SampleTypeValue/reconversionOfPg -->


    <owl:NamedIndividual rdf:about="http://lpis.ec.europa.eu/registry/applicationschema/cap-iacs-control/code#SampleTypeValue/reconversionOfPg">
        <rdf:type rdf:resource="http://lpis.ec.europa.eu/registry/applicationschema/cap-iacs-control#SampleTypeValue"/>
        <skos:definition xml:lang="en">Reconversion of permanent grassland

Items corresponding to beneficiaries obliged to re-convert agricultural areas in permanent grassland.</skos:definition>
        <skos:inScheme rdf:resource="http://lpis.ec.europa.eu/registry/applicationschema/cap-iacs-control/code#SampleTypeValue"/>
    </owl:NamedIndividual>
    


    <!-- http://lpis.ec.europa.eu/registry/applicationschema/cap-iacs-control/code#SampleTypeValue/reconversionOfSensitivePg -->


    <owl:NamedIndividual rdf:about="http://lpis.ec.europa.eu/registry/applicationschema/cap-iacs-control/code#SampleTypeValue/reconversionOfSensitivePg">
        <rdf:type rdf:resource="http://lpis.ec.europa.eu/registry/applicationschema/cap-iacs-control#SampleTypeValue"/>
        <skos:definition xml:lang="en">Reconversion of sensitive permanent grassland

Items corresponding to beneficiaries obliged to re-convert agricultural areas in sensitive permanent grassland.</skos:definition>
        <skos:inScheme rdf:resource="http://lpis.ec.europa.eu/registry/applicationschema/cap-iacs-control/code#SampleTypeValue"/>
    </owl:NamedIndividual>
    


    <!-- http://lpis.ec.europa.eu/registry/applicationschema/cap-iacs-control/code#SampleTypeValue/redistributivePayment -->


    <owl:NamedIndividual rdf:about="http://lpis.ec.europa.eu/registry/applicationschema/cap-iacs-control/code#SampleTypeValue/redistributivePayment">
        <rdf:type rdf:resource="http://lpis.ec.europa.eu/registry/applicationschema/cap-iacs-control#SampleTypeValue"/>
        <skos:definition xml:lang="en">Redistributive payment

Item selected for controlling beneficiaries applying for redistributive payment.</skos:definition>
        <skos:inScheme rdf:resource="http://lpis.ec.europa.eu/registry/applicationschema/cap-iacs-control/code#SampleTypeValue"/>
    </owl:NamedIndividual>
    


    <!-- http://lpis.ec.europa.eu/registry/applicationschema/cap-iacs-control/code#SampleTypeValue/regionalImplementation -->


    <owl:NamedIndividual rdf:about="http://lpis.ec.europa.eu/registry/applicationschema/cap-iacs-control/code#SampleTypeValue/regionalImplementation">
        <rdf:type rdf:resource="http://lpis.ec.europa.eu/registry/applicationschema/cap-iacs-control#SampleTypeValue"/>
        <skos:definition xml:lang="en">Regional implementation

Items selected for controlling beneficiaries participating in regional implementation of EFA. The composition of the population
	- 1,0-1,25% selected randomly 
	- 3,75-4,0% selected on risk base

Issue:
The purpose of collective implementation (See Art. 46(a) of 1307/2013) and regional implementation (see Art. 46(3) of R 639/2014) is to form contiguous areas of EFA. If so, what is the reason to have separate samples for collective implementation, regional implementation and contiguous EFA?</skos:definition>
        <skos:inScheme rdf:resource="http://lpis.ec.europa.eu/registry/applicationschema/cap-iacs-control/code#SampleTypeValue"/>
    </owl:NamedIndividual>
    


    <!-- http://lpis.ec.europa.eu/registry/applicationschema/cap-iacs-control/code#SampleTypeValue/sensitiveGrassland -->


    <owl:NamedIndividual rdf:about="http://lpis.ec.europa.eu/registry/applicationschema/cap-iacs-control/code#SampleTypeValue/sensitiveGrassland">
        <rdf:type rdf:resource="http://lpis.ec.europa.eu/registry/applicationschema/cap-iacs-control#SampleTypeValue"/>
        <skos:definition xml:lang="en">Sensitive grassland

Items selected for controlling sensitive grassland. The composition of the population
	- 1,0-1,25% selected randomly 
	- 3,75-4,0% selected on risk base

NOTE
This sample is included in the generic sample of beneficiaries that are mandated to observe greening.</skos:definition>
        <skos:inScheme rdf:resource="http://lpis.ec.europa.eu/registry/applicationschema/cap-iacs-control/code#SampleTypeValue"/>
    </owl:NamedIndividual>
    


    <!-- http://lpis.ec.europa.eu/registry/applicationschema/cap-iacs-control/code#SampleTypeValue/smallFarmers -->


    <owl:NamedIndividual rdf:about="http://lpis.ec.europa.eu/registry/applicationschema/cap-iacs-control/code#SampleTypeValue/smallFarmers">
        <rdf:type rdf:resource="http://lpis.ec.europa.eu/registry/applicationschema/cap-iacs-control#SampleTypeValue"/>
        <skos:definition xml:lang="en">Small farmers

Item selected for controlling beneficiaries participating in the small farmers scheme.</skos:definition>
        <skos:inScheme rdf:resource="http://lpis.ec.europa.eu/registry/applicationschema/cap-iacs-control/code#SampleTypeValue"/>
    </owl:NamedIndividual>
    


    <!-- http://lpis.ec.europa.eu/registry/applicationschema/cap-iacs-control/code#SampleTypeValue/voluntaryCoupledSupport -->


    <owl:NamedIndividual rdf:about="http://lpis.ec.europa.eu/registry/applicationschema/cap-iacs-control/code#SampleTypeValue/voluntaryCoupledSupport">
        <rdf:type rdf:resource="http://lpis.ec.europa.eu/registry/applicationschema/cap-iacs-control#SampleTypeValue"/>
        <skos:definition xml:lang="en">Voluntary coupled support

Item selected for controlling beneficiaries applying for voluntary coupled support.</skos:definition>
        <skos:inScheme rdf:resource="http://lpis.ec.europa.eu/registry/applicationschema/cap-iacs-control/code#SampleTypeValue"/>
    </owl:NamedIndividual>
    


    <!-- http://lpis.ec.europa.eu/registry/applicationschema/cap-iacs-control/code#SampleTypeValue/youngFarmers -->


    <owl:NamedIndividual rdf:about="http://lpis.ec.europa.eu/registry/applicationschema/cap-iacs-control/code#SampleTypeValue/youngFarmers">
        <rdf:type rdf:resource="http://lpis.ec.europa.eu/registry/applicationschema/cap-iacs-control#SampleTypeValue"/>
        <skos:definition xml:lang="en">Young farmers

Item selected for controlling beneficiaries applying for young farmer payment.</skos:definition>
        <skos:inScheme rdf:resource="http://lpis.ec.europa.eu/registry/applicationschema/cap-iacs-control/code#SampleTypeValue"/>
    </owl:NamedIndividual>
    


    <!-- http://lpis.ec.europa.eu/registry/applicationschema/cap-iacs-control/code#SampleTypeValue/initial1%And1,25%ForBps/Saps -->


    <owl:NamedIndividual rdf:about="http://lpis.ec.europa.eu/registry/applicationschema/cap-iacs-control/code#SampleTypeValue/initial1%And1,25%ForBps/Saps">
        <rdf:type rdf:resource="http://lpis.ec.europa.eu/registry/applicationschema/cap-iacs-control#SampleTypeValue"/>
        <skos:definition xml:lang="en">Initial 1% and 1,25% for BPS/SAPS

It is the initial random sample drawn in sense of Art. 24(2)(a). This sample constitutes the basis of the following further samples:
	- Random part of the greening samples
	- Redistributive payment
	- Areas with natural constraints
	- Young farmers
	- Voluntary couples support
	- Hemp
	- Cotton</skos:definition>
        <skos:inScheme rdf:resource="http://lpis.ec.europa.eu/registry/applicationschema/cap-iacs-control/code#SampleTypeValue"/>
    </owl:NamedIndividual>
    


    <!-- http://lpis.ec.europa.eu/registry/applicationschema/cap-iacs-control/code#SampleTypeValue/regional/NationalCertificationScheme -->


    <owl:NamedIndividual rdf:about="http://lpis.ec.europa.eu/registry/applicationschema/cap-iacs-control/code#SampleTypeValue/regional/NationalCertificationScheme">
        <rdf:type rdf:resource="http://lpis.ec.europa.eu/registry/applicationschema/cap-iacs-control#SampleTypeValue"/>
        <skos:definition xml:lang="en">Regional/national certification scheme

Items selected for controlling greening according to Art.43 (3)(b) of R 1307/2013. The equivalent practices are listed in Annex IX of this regulation and the AgriculturalEquivalentPracticeTypeValue code list of the Aid applications and payment claims application schema.</skos:definition>
        <skos:inScheme rdf:resource="http://lpis.ec.europa.eu/registry/applicationschema/cap-iacs-control/code#SampleTypeValue"/>
    </owl:NamedIndividual>
    


    <!-- http://lpis.ec.europa.eu/registry/applicationschema/cap-iacs-control/code#SampleTypeValue/topUpForBps/Saps -->


    <owl:NamedIndividual rdf:about="http://lpis.ec.europa.eu/registry/applicationschema/cap-iacs-control/code#SampleTypeValue/topUpForBps/Saps">
        <rdf:type rdf:resource="http://lpis.ec.europa.eu/registry/applicationschema/cap-iacs-control#SampleTypeValue"/>
        <skos:definition xml:lang="en">Top-up for BPS/SAPS

Randomly selected items to complete the BPS/SAPS population after integrating the items out of the following samples: 
	- Initial 1,0-2,15% sample for BPS SAPS
	- Greening samples
	- Redistributive payment
	- Areas with natural constraints
	- Young farmers
	- Voluntary couples support
	- Hemp
	- Cotton</skos:definition>
        <skos:inScheme rdf:resource="http://lpis.ec.europa.eu/registry/applicationschema/cap-iacs-control/code#SampleTypeValue"/>
    </owl:NamedIndividual>
    


    <!-- http://lpis.ec.europa.eu/registry/applicationschema/cap-iacs-control/code#SamplingStrategyTypeValue/clusteredRandomSelection -->


    <owl:NamedIndividual rdf:about="http://lpis.ec.europa.eu/registry/applicationschema/cap-iacs-control/code#SamplingStrategyTypeValue/clusteredRandomSelection">
        <rdf:type rdf:resource="http://lpis.ec.europa.eu/registry/applicationschema/cap-iacs-control#SamplingStrategyTypeValue"/>
        <skos:definition xml:lang="en">Clustered random selection

Cluster sampling is a selection of items that are clustered (e.g. spatially or temporally) within the population.

EXAMPLE
Geographic cluster of a CwRS zone.

NOTE 1
The criteria for each cluster has to be registered.

NOTE 2
The clusters regarded as primary samples by geographic or temporal distribution can be further sampled by a second level of sampling. In that case the method is called multistage sampling.</skos:definition>
        <skos:inScheme rdf:resource="http://lpis.ec.europa.eu/registry/applicationschema/cap-iacs-control/code#SamplingStrategyTypeValue"/>
    </owl:NamedIndividual>
    


    <!-- http://lpis.ec.europa.eu/registry/applicationschema/cap-iacs-control/code#SamplingStrategyTypeValue/multistageSampling -->


    <owl:NamedIndividual rdf:about="http://lpis.ec.europa.eu/registry/applicationschema/cap-iacs-control/code#SamplingStrategyTypeValue/multistageSampling">
        <rdf:type rdf:resource="http://lpis.ec.europa.eu/registry/applicationschema/cap-iacs-control#SamplingStrategyTypeValue"/>
        <skos:definition xml:lang="en">Multistage sampling

Further, secondary sampling of clusters that have been  selected on geographic, or temporal criteria.</skos:definition>
        <skos:inScheme rdf:resource="http://lpis.ec.europa.eu/registry/applicationschema/cap-iacs-control/code#SamplingStrategyTypeValue"/>
    </owl:NamedIndividual>
    


    <!-- http://lpis.ec.europa.eu/registry/applicationschema/cap-iacs-control/code#SamplingStrategyTypeValue/riskBasedCartSelection -->


    <owl:NamedIndividual rdf:about="http://lpis.ec.europa.eu/registry/applicationschema/cap-iacs-control/code#SamplingStrategyTypeValue/riskBasedCartSelection">
        <rdf:type rdf:resource="http://lpis.ec.europa.eu/registry/applicationschema/cap-iacs-control#SamplingStrategyTypeValue"/>
        <rdfs:label xml:lang="en">Risk based sampling strategy</rdfs:label>
        <skos:definition xml:lang="en">Risk based CART selection

A probability proportional risk based method for selecting and grouping items (applications) in risk groups based on a specific criterion (e.g. area not found) [DSCG/2014/32].</skos:definition>
        <skos:inScheme rdf:resource="http://lpis.ec.europa.eu/registry/applicationschema/cap-iacs-control/code#SamplingStrategyTypeValue"/>
    </owl:NamedIndividual>
    


    <!-- http://lpis.ec.europa.eu/registry/applicationschema/cap-iacs-control/code#SamplingStrategyTypeValue/riskBasedMultiCriteriaSelection -->


    <owl:NamedIndividual rdf:about="http://lpis.ec.europa.eu/registry/applicationschema/cap-iacs-control/code#SamplingStrategyTypeValue/riskBasedMultiCriteriaSelection">
        <rdf:type rdf:resource="http://lpis.ec.europa.eu/registry/applicationschema/cap-iacs-control#SamplingStrategyTypeValue"/>
        <rdfs:label xml:lang="en">Risk based sampling strategy</rdfs:label>
        <skos:definition xml:lang="en">Risk based multi-criteria selection

Risk based selection based on multi-criteria analysis.
Examples of aspects of analysis:
	- areas of recent land cover / land use change (from third party data)
	- Landscape
	- Agronomic conditions
	- Non-participation in FAS or certification schemes of farmers

NOTE 
The method is especially applicable for selecting risk based CwRS zones.</skos:definition>
        <skos:inScheme rdf:resource="http://lpis.ec.europa.eu/registry/applicationschema/cap-iacs-control/code#SamplingStrategyTypeValue"/>
    </owl:NamedIndividual>
    


    <!-- http://lpis.ec.europa.eu/registry/applicationschema/cap-iacs-control/code#SamplingStrategyTypeValue/simpleRandomBasedSelection -->


    <owl:NamedIndividual rdf:about="http://lpis.ec.europa.eu/registry/applicationschema/cap-iacs-control/code#SamplingStrategyTypeValue/simpleRandomBasedSelection">
        <rdf:type rdf:resource="http://lpis.ec.europa.eu/registry/applicationschema/cap-iacs-control#SamplingStrategyTypeValue"/>
        <rdfs:label xml:lang="en">Random based sampling strategy</rdfs:label>
        <skos:definition xml:lang="en">Simple random based selection

Selection from the full population of the dossiers through generation of a random key [Section 1.3.2 of DSCG/2014/32].

NOTE 1
The population has to be homogenous for this method.

NOTE 2
This method requires waiting until the full population is known.</skos:definition>
        <skos:inScheme rdf:resource="http://lpis.ec.europa.eu/registry/applicationschema/cap-iacs-control/code#SamplingStrategyTypeValue"/>
    </owl:NamedIndividual>
    


    <!-- http://lpis.ec.europa.eu/registry/applicationschema/cap-iacs-control/code#SamplingStrategyTypeValue/simpleRiskBasedSelection -->


    <owl:NamedIndividual rdf:about="http://lpis.ec.europa.eu/registry/applicationschema/cap-iacs-control/code#SamplingStrategyTypeValue/simpleRiskBasedSelection">
        <rdf:type rdf:resource="http://lpis.ec.europa.eu/registry/applicationschema/cap-iacs-control#SamplingStrategyTypeValue"/>
        <rdfs:label xml:lang="en">Risk based sampling strategy</rdfs:label>
        <skos:definition xml:lang="en">Simple risk based selection

Sampling process based on a single criterion retained to be effective in course of risk analysis. Input data for risk analysis can be taken from OTSC report of the previous year, other subsystems of IACS, third party data, etc.

NOTE 1
The effectiveness of the criterion has to be proved by comparing the performance results from a random sample and a sample based on the criterion. 

NOTE 2
The performance criterion has to be documented before  starting the sampling process.</skos:definition>
        <skos:inScheme rdf:resource="http://lpis.ec.europa.eu/registry/applicationschema/cap-iacs-control/code#SamplingStrategyTypeValue"/>
    </owl:NamedIndividual>
    


    <!-- http://lpis.ec.europa.eu/registry/applicationschema/cap-iacs-control/code#SamplingStrategyTypeValue/stratifiedRandomSelection -->


    <owl:NamedIndividual rdf:about="http://lpis.ec.europa.eu/registry/applicationschema/cap-iacs-control/code#SamplingStrategyTypeValue/stratifiedRandomSelection">
        <rdf:type rdf:resource="http://lpis.ec.europa.eu/registry/applicationschema/cap-iacs-control#SamplingStrategyTypeValue"/>
        <skos:definition xml:lang="en">Stratified random selection

Method applicable when the population to be sampled is not homogenous. In order to achieve homogeneity, the population has to be sub-divided into strata based on objective criteria.

NOTE
The criteria for each stratum has to be registered.</skos:definition>
        <skos:inScheme rdf:resource="http://lpis.ec.europa.eu/registry/applicationschema/cap-iacs-control/code#SamplingStrategyTypeValue"/>
    </owl:NamedIndividual>
    


    <!-- http://lpis.ec.europa.eu/registry/applicationschema/cap-iacs-control/code#SamplingStrategyTypeValue/systematicRandomBasedSelection -->


    <owl:NamedIndividual rdf:about="http://lpis.ec.europa.eu/registry/applicationschema/cap-iacs-control/code#SamplingStrategyTypeValue/systematicRandomBasedSelection">
        <rdf:type rdf:resource="http://lpis.ec.europa.eu/registry/applicationschema/cap-iacs-control#SamplingStrategyTypeValue"/>
        <skos:definition xml:lang="en">Systematic random selection

Random selection of the first initial item (i.e. application) and taking the rest based on the sequential number (e.g. every 100 application) [Section 1.3.2 of DSCG/2014/32].

NOTE 1
This method allows to start OTSC before the end of the application period.

NOTE 2
The sequential number has to be automatically assigned to the applications, or the key (i.e. property or properties) that serve for the basis of selection has to be specified and documented before starting the sampling process.

NOTE 3
The population has to be homogenous.</skos:definition>
        <skos:inScheme rdf:resource="http://lpis.ec.europa.eu/registry/applicationschema/cap-iacs-control/code#SamplingStrategyTypeValue"/>
    </owl:NamedIndividual>
    


    <!-- http://lpis.ec.europa.eu/registry/applicationschema/cap-iacs-control/code#SurveyMethodValue/cwrs -->


    <owl:NamedIndividual rdf:about="http://lpis.ec.europa.eu/registry/applicationschema/cap-iacs-control/code#SurveyMethodValue/cwrs">
        <rdf:type rdf:resource="http://lpis.ec.europa.eu/registry/applicationschema/cap-iacs-control#SurveyMethodValue"/>
        <rdfs:label xml:lang="en">CwRS</rdfs:label>
        <skos:definition xml:lang="en">CwRS

Control with Remote Sensing (VHR, or HR). [Art. 74(3) of R 1306/2013].

NOTE.
It includes CAPI.</skos:definition>
        <skos:inScheme rdf:resource="http://lpis.ec.europa.eu/registry/applicationschema/cap-iacs-control/code#SurveyMethodValue"/>
    </owl:NamedIndividual>
    


    <!-- http://lpis.ec.europa.eu/registry/applicationschema/cap-iacs-control/code#SurveyMethodValue/fieldMeasurement -->


    <owl:NamedIndividual rdf:about="http://lpis.ec.europa.eu/registry/applicationschema/cap-iacs-control/code#SurveyMethodValue/fieldMeasurement">
        <rdf:type rdf:resource="http://lpis.ec.europa.eu/registry/applicationschema/cap-iacs-control#SurveyMethodValue"/>
        <rdfs:label xml:lang="en">Field measurement</rdfs:label>
        <skos:definition xml:lang="en">Field measurement

Any field measurement including GNSS [Art. 74(3) of R 1306/2013].</skos:definition>
        <skos:inScheme rdf:resource="http://lpis.ec.europa.eu/registry/applicationschema/cap-iacs-control/code#SurveyMethodValue"/>
    </owl:NamedIndividual>
    


    <!-- http://lpis.ec.europa.eu/registry/applicationschema/cap-iacs-control/code#SurveyMethodValue/rapidFieldVisit -->


    <owl:NamedIndividual rdf:about="http://lpis.ec.europa.eu/registry/applicationschema/cap-iacs-control/code#SurveyMethodValue/rapidFieldVisit">
        <rdf:type rdf:resource="http://lpis.ec.europa.eu/registry/applicationschema/cap-iacs-control#SurveyMethodValue"/>
        <rdfs:label xml:lang="en">Combined field measurement and CwRS</rdfs:label>
        <skos:definition xml:lang="en">Rapid field visit

Combined measurement using field (e.g. GNSS)and  Remote Sensing methods.

NOTE 1
In the event that photo-interpretation of orthoimages (satellite or aerial) do not provide results that would permit definitive conclusions to be drawn to the satisfaction of the competent authority concerning the eligibility or the correct size of the area that is the subject of administrative or on-the-spot checks [Art. 24(4) of R 809/2014].

NOTE 2
It follows an inconclusive CAPI.</skos:definition>
        <skos:inScheme rdf:resource="http://lpis.ec.europa.eu/registry/applicationschema/cap-iacs-control/code#SurveyMethodValue"/>
    </owl:NamedIndividual>
</rdf:RDF>



<!-- Generated by the OWL API (version 5.1.18) https://github.com/owlcs/owlapi/ -->


