<?xml version="1.0"?>
<rdf:RDF xmlns="http://lpis.ec.europa.eu/registry/applicationschema/cap-iacs-parcel#"
     xml:base="http://lpis.ec.europa.eu/registry/applicationschema/cap-iacs-parcel"
     xmlns:dc="http://purl.org/dc/elements/1.1/"
     xmlns:owl="http://www.w3.org/2002/07/owl#"
     xmlns:rdf="http://www.w3.org/1999/02/22-rdf-syntax-ns#"
     xmlns:xml="http://www.w3.org/XML/1998/namespace"
     xmlns:xsd="http://www.w3.org/2001/XMLSchema#"
     xmlns:foaf="http://xmlns.com/foaf/0.1/"
     xmlns:rdfs="http://www.w3.org/2000/01/rdf-schema#"
     xmlns:skos="http://www.w3.org/2004/02/skos/core#"
     xmlns:terms="http://purl.org/dc/terms/"
     xmlns:schema="http://schema.org/">
    <owl:Ontology rdf:about="http://lpis.ec.europa.eu/registry/applicationschema/cap-iacs-parcel">
        <owl:versionIRI rdf:resource="http://lpis.ec.europa.eu/registry/applicationschema/cap-iacs-parcel/3.0"/>
        <owl:imports rdf:resource="http://www.opengis.net/ont/geosparql"/>
        <owl:imports rdf:resource="https://raw.githubusercontent.com/rapw3k/cap-iacs/main/cap-iacs-base.ttl"/>
        <terms:creator rdf:nodeID="genid1"/>
        <terms:description xml:lang="en">Ontology of the identification system for agricultural parcels used in IACS, generated from the transformation of the corresponding JRC application schema</terms:description>
        <terms:rights xml:lang="en">This ontology is distributed under Creative Commons Attribution 4.0 License - http://creativecommons.org/licenses/by/4.0</terms:rights>
        <terms:source xml:lang="en">JRC IACS application schema. https://doi.org/10.1016/j.landusepol.2016.05.023</terms:source>
        <terms:title xml:lang="en">JRC IACS - Identification System for Agricultural Parcels Ontology</terms:title>
        <rdfs:label xml:lang="en">Identification system for agricultural parcels</rdfs:label>
        <owl:versionInfo>3.0</owl:versionInfo>
        <skos:definition xml:lang="en">-- Name --
Identification system for agricultural parcels

-- Definition --
Application schema of Identification system for agricultural parcels.

-- Description --
The contents of an «ApplicationSchema» package exported as a GML Application Schema file.

NOTE. This subsystem of IACS is commonly named as Land PArcel Identification System. (LPIS).</skos:definition>
    </owl:Ontology>
    <rdf:Description rdf:nodeID="genid1">
        <schema:affiliation>
            <rdf:Description>
                <foaf:name>PSNC</foaf:name>
            </rdf:Description>
        </schema:affiliation>
        <rdfs:seeAlso rdf:resource="http://orcid.org/0000-0003-4289-4922"/>
        <foaf:name>Raul Palma</foaf:name>
    </rdf:Description>
    


    <!-- 
    ///////////////////////////////////////////////////////////////////////////////////////
    //
    // Object Properties
    //
    ///////////////////////////////////////////////////////////////////////////////////////
     -->


    


    <!-- http://lpis.ec.europa.eu/registry/applicationschema/cap-iacs-parcel#abstractTestType -->


    <owl:ObjectProperty rdf:about="http://lpis.ec.europa.eu/registry/applicationschema/cap-iacs-parcel#abstractTestType">
        <rdfs:range rdf:resource="http://lpis.ec.europa.eu/registry/applicationschema/cap-iacs-parcel#TestTypeMtsValue"/>
        <rdfs:label xml:lang="en">Type of test</rdfs:label>
        <skos:definition xml:lang="en">--Name--
Abstract test type

-- Definition --
Reference to the abstract test case for which the executable test case(s) is (are) performed.

-- Description --
The values of this attribute shall come from the TestTypeMtsValue code list. To one abstract test case at least one executable test case shall correspond.</skos:definition>
    </owl:ObjectProperty>
    


    <!-- http://lpis.ec.europa.eu/registry/applicationschema/cap-iacs-parcel#acceptanceNumber -->


    <owl:ObjectProperty rdf:about="http://lpis.ec.europa.eu/registry/applicationschema/cap-iacs-parcel#acceptanceNumber">
        <rdfs:range rdf:resource="http://lpis.ec.europa.eu/registry/applicationschema/cap-iacs-parcel#AcceptanceNumberValue"/>
        <rdfs:label xml:lang="en">Acceptance value</rdfs:label>
        <skos:definition xml:lang="en">--Name--
Acceptance number

-- Definition --
Indicator that is used to determine the acceptability of the lot based on inspection by sampling.

-- Description --
If the number of nonconforming items, or the total number of non-conformities, found in the sample is equal to or less than the acceptance number (Ac) specified in the plan, the lot shall be accepted [ISO 2859-2:1985].</skos:definition>
    </owl:ObjectProperty>
    


    <!-- http://lpis.ec.europa.eu/registry/applicationschema/cap-iacs-parcel#agriculturalArea -->


    <owl:ObjectProperty rdf:about="http://lpis.ec.europa.eu/registry/applicationschema/cap-iacs-parcel#agriculturalArea">
        <rdfs:range rdf:resource="http://qudt.org/schema/qudt/QuantityValue"/>
    </owl:ObjectProperty>
    


    <!-- http://lpis.ec.europa.eu/registry/applicationschema/cap-iacs-parcel#agriculturalAreaDetailsForEcologicalFocusArea -->


    <owl:ObjectProperty rdf:about="http://lpis.ec.europa.eu/registry/applicationschema/cap-iacs-parcel#agriculturalAreaDetailsForEcologicalFocusArea">
        <rdfs:range rdf:resource="http://lpis.ec.europa.eu/registry/applicationschema/cap-iacs-parcel#EcologicalFocusArea"/>
    </owl:ObjectProperty>
    


    <!-- http://lpis.ec.europa.eu/registry/applicationschema/cap-iacs-parcel#agriculturalAreaType -->


    <owl:ObjectProperty rdf:about="http://lpis.ec.europa.eu/registry/applicationschema/cap-iacs-parcel#agriculturalAreaType">
        <rdfs:range rdf:resource="http://lpis.ec.europa.eu/registry/applicationschema/cap-iacs-parcel#AgriculturalAreaTypeValue"/>
        <rdfs:label xml:lang="en">Agricultural area type</rdfs:label>
        <skos:definition xml:lang="en">--Name--
Agricultural area type

-- Definition --
Agricultural area type.

-- Description --
Any area taken up by arable land, permanent grassland and permanent pasture, or permanent crops. 1307/2013 4(1)(e).</skos:definition>
    </owl:ObjectProperty>
    


    <!-- http://lpis.ec.europa.eu/registry/applicationschema/cap-iacs-parcel#agriculturalAreaWithinReferenceParcel -->


    <owl:ObjectProperty rdf:about="http://lpis.ec.europa.eu/registry/applicationschema/cap-iacs-parcel#agriculturalAreaWithinReferenceParcel">
        <rdfs:range rdf:resource="http://lpis.ec.europa.eu/registry/applicationschema/cap-iacs-parcel#ReferenceParcel"/>
    </owl:ObjectProperty>
    


    <!-- http://lpis.ec.europa.eu/registry/applicationschema/cap-iacs-parcel#areaNonConformanceCause -->


    <owl:ObjectProperty rdf:about="http://lpis.ec.europa.eu/registry/applicationschema/cap-iacs-parcel#areaNonConformanceCause">
        <rdfs:range rdf:resource="http://lpis.ec.europa.eu/registry/applicationschema/cap-iacs-parcel#TechnicalReasonValue"/>
        <rdfs:label xml:lang="en">Technical reasons for non-conformance</rdfs:label>
        <skos:definition xml:lang="en">--Name--
Area non-conformance cause

-- Definition --
Statement of the technical cause(s) leading to non-conformance in terms of the observed area of the item under inspection.

-- Description --
The technical reason shall be assigned from the following list:
- missed  update
- missed upgrade
- incomplete processing
- processing error
- incompatible design

NOTE: One or more technical reason value selected from the TechnicalReasonValue enumeration.</skos:definition>
    </owl:ObjectProperty>
    


    <!-- http://lpis.ec.europa.eu/registry/applicationschema/cap-iacs-parcel#collectiveImplementationCitation -->


    <owl:ObjectProperty rdf:about="http://lpis.ec.europa.eu/registry/applicationschema/cap-iacs-parcel#collectiveImplementationCitation">
        <rdfs:range rdf:resource="http://lpis.ec.europa.eu/registry/applicationschema/cap-iacs-base#SupplementaryDocument"/>
        <rdfs:label xml:lang="en">Non-structured evidence - citation</rdfs:label>
        <skos:definition xml:lang="en">--Name--
Collective implementation citation

-- Definition --
Citation proving that EFA is subject to collective implementation as referred to in Art. 46(6) of (EU) R 1307/2013.

-- Description --
If subjectToCollectiveImplementation=TRUE then a document or a citation proving that EFA is subject to collective implementation must be provided.

EXAMPLE: citation of the legal basis.</skos:definition>
    </owl:ObjectProperty>
    


    <!-- http://lpis.ec.europa.eu/registry/applicationschema/cap-iacs-parcel#collectiveImplementationDocument -->


    <owl:ObjectProperty rdf:about="http://lpis.ec.europa.eu/registry/applicationschema/cap-iacs-parcel#collectiveImplementationDocument">
        <rdfs:range rdf:resource="http://lpis.ec.europa.eu/registry/applicationschema/cap-iacs-base#SupplementaryDocument"/>
        <rdfs:label xml:lang="en">Non-structured evidence - document</rdfs:label>
        <skos:definition xml:lang="en">--Name--
Collective implementation document

-- Definition --
Any record proving that EFA is subject to collective implementation as referred to in Art. 46(6) of (EU) R 1307/2013.

-- Description --
If subjectToCollectiveImplementation=TRUE then a document or a citation proving that EFA is subject to collective implementation must be provided.

EXAMPLE:  Supporting document might be:
- designation of authorities addressed to the farmer;
- contract of participants, etc.

NOTE: Farmers participating in the collective implementation shall conclude a written agreement that includes details on the internal arrangements of financial compensation and as regards the administrative penalties in case of non-compliance on the common ecological focus area. [Art. 47(4) of (EU) R No 639/2014].</skos:definition>
    </owl:ObjectProperty>
    


    <!-- http://lpis.ec.europa.eu/registry/applicationschema/cap-iacs-parcel#conformingItemsArea -->


    <owl:ObjectProperty rdf:about="http://lpis.ec.europa.eu/registry/applicationschema/cap-iacs-parcel#conformingItemsArea">
        <rdfs:range rdf:resource="http://qudt.org/schema/qudt/QuantityValue"/>
    </owl:ObjectProperty>
    


    <!-- http://lpis.ec.europa.eu/registry/applicationschema/cap-iacs-parcel#contaminationCause -->


    <owl:ObjectProperty rdf:about="http://lpis.ec.europa.eu/registry/applicationschema/cap-iacs-parcel#contaminationCause">
        <rdfs:range rdf:resource="http://lpis.ec.europa.eu/registry/applicationschema/cap-iacs-parcel#TechnicalReasonValue"/>
        <rdfs:label xml:lang="en">Cause of contamination</rdfs:label>
        <skos:definition xml:lang="en">--Name--
Contamination cause

-- Definition --
Technical reason that has presumably caused  the contamination.

-- Description --
Technical reason shall be selected from the TechnicalReasonValue code list.

NOTE. Contamination cause shall be given when value of waivered is FALSE.</skos:definition>
    </owl:ObjectProperty>
    


    <!-- http://lpis.ec.europa.eu/registry/applicationschema/cap-iacs-parcel#contaminationType -->


    <owl:ObjectProperty rdf:about="http://lpis.ec.europa.eu/registry/applicationschema/cap-iacs-parcel#contaminationType">
        <rdfs:range rdf:resource="http://lpis.ec.europa.eu/registry/applicationschema/cap-iacs-parcel#ContaminationTypeValue"/>
        <rdfs:label xml:lang="en">Type of contamination</rdfs:label>
        <skos:definition xml:lang="en">--Name--
Contamination type

-- Definition --
Classification of contamination types.

-- Description --
Contamination types are defined according to the ContaminationTypeValues code list.</skos:definition>
    </owl:ObjectProperty>
    


    <!-- http://lpis.ec.europa.eu/registry/applicationschema/cap-iacs-parcel#conversionDetailsForEfa -->


    <owl:ObjectProperty rdf:about="http://lpis.ec.europa.eu/registry/applicationschema/cap-iacs-parcel#conversionDetailsForEfa">
        <rdfs:range rdf:resource="http://lpis.ec.europa.eu/registry/applicationschema/cap-iacs-parcel#EcologicalFocusArea"/>
    </owl:ObjectProperty>
    


    <!-- http://lpis.ec.europa.eu/registry/applicationschema/cap-iacs-parcel#conversionParameterForDeterminationOfEcologicalFocusArea -->


    <owl:ObjectProperty rdf:about="http://lpis.ec.europa.eu/registry/applicationschema/cap-iacs-parcel#conversionParameterForDeterminationOfEcologicalFocusArea">
        <rdfs:range rdf:resource="http://lpis.ec.europa.eu/registry/applicationschema/cap-iacs-aid#EcologicalFocusAreaConverted"/>
    </owl:ObjectProperty>
    


    <!-- http://lpis.ec.europa.eu/registry/applicationschema/cap-iacs-parcel#convertedArea -->


    <owl:ObjectProperty rdf:about="http://lpis.ec.europa.eu/registry/applicationschema/cap-iacs-parcel#convertedArea">
        <rdfs:range rdf:resource="http://qudt.org/schema/qudt/QuantityValue"/>
    </owl:ObjectProperty>
    


    <!-- http://lpis.ec.europa.eu/registry/applicationschema/cap-iacs-parcel#criticalDefectAcceptanceNumber -->


    <owl:ObjectProperty rdf:about="http://lpis.ec.europa.eu/registry/applicationschema/cap-iacs-parcel#criticalDefectAcceptanceNumber">
        <rdfs:range rdf:resource="http://lpis.ec.europa.eu/registry/applicationschema/cap-iacs-parcel#AcceptanceNumberValue"/>
        <rdfs:label xml:lang="en">Critical defect acceptance number</rdfs:label>
        <skos:definition xml:lang="en">--Name--
Acceptance number for critical defects

-- Definition --
Acceptance number applicable for critical defect.

-- Description --
If the number of nonconforming items for critical defects is equal or less than specified acceptance number, the total lot shall be accepted. 
NOTE. Acceptance number of items with critical defect shall correspond to limiting quality 2,00 specified in ISO 2859-2:1985</skos:definition>
    </owl:ObjectProperty>
    


    <!-- http://lpis.ec.europa.eu/registry/applicationschema/cap-iacs-parcel#criticalDefectCause -->


    <owl:ObjectProperty rdf:about="http://lpis.ec.europa.eu/registry/applicationschema/cap-iacs-parcel#criticalDefectCause">
        <rdfs:range rdf:resource="http://lpis.ec.europa.eu/registry/applicationschema/cap-iacs-parcel#TechnicalReasonValue"/>
        <rdfs:label xml:lang="en">Cause of critical defect</rdfs:label>
        <skos:definition xml:lang="en">--Name--
Critical defect cause

-- Definition --
Technical reason that has presumably caused the critical defect.

-- Description --
Technical reason shall be selected from theTechnicalReasonValue code list.</skos:definition>
    </owl:ObjectProperty>
    


    <!-- http://lpis.ec.europa.eu/registry/applicationschema/cap-iacs-parcel#criticalDefectEfaCompositionDetails -->


    <owl:ObjectProperty rdf:about="http://lpis.ec.europa.eu/registry/applicationschema/cap-iacs-parcel#criticalDefectEfaCompositionDetails">
        <rdfs:range rdf:resource="http://lpis.ec.europa.eu/registry/applicationschema/cap-iacs-parcel#CriticalDefectEfa"/>
    </owl:ObjectProperty>
    


    <!-- http://lpis.ec.europa.eu/registry/applicationschema/cap-iacs-parcel#criticalDefectType -->


    <owl:ObjectProperty rdf:about="http://lpis.ec.europa.eu/registry/applicationschema/cap-iacs-parcel#criticalDefectType">
        <rdfs:range rdf:resource="http://lpis.ec.europa.eu/registry/applicationschema/cap-iacs-parcel#CriticalDefectTypeValue"/>
        <rdfs:label xml:lang="en">Type of critical defect</rdfs:label>
        <skos:definition xml:lang="en">--Name--
Critical defect type

-- Definition --
Classification of critical defect.

-- Description --
Critical defects are classified according to the categories defined in CriticalDefectTypeValue code list.</skos:definition>
    </owl:ObjectProperty>
    


    <!-- http://lpis.ec.europa.eu/registry/applicationschema/cap-iacs-parcel#dataQualityMeasureDescription -->


    <owl:ObjectProperty rdf:about="http://lpis.ec.europa.eu/registry/applicationschema/cap-iacs-parcel#dataQualityMeasureDescription">
        <rdfs:range rdf:resource="http://lpis.ec.europa.eu/registry/applicationschema/cap-iacs-parcel#DataQualityMeasure"/>
        <rdfs:label xml:lang="en">Description of data quality measure</rdfs:label>
        <skos:definition xml:lang="en">--Name--
Data quality measure description

-- Definition --
This is a placeholder only; currently not to be implemented.

Description of particular data quality measure.

-- Description --
Extended description of data quality measure.
NOTE. Depends on selected dataQualityMeasureType.</skos:definition>
    </owl:ObjectProperty>
    


    <!-- http://lpis.ec.europa.eu/registry/applicationschema/cap-iacs-parcel#dataQualityMeasureDocumentation -->


    <owl:ObjectProperty rdf:about="http://lpis.ec.europa.eu/registry/applicationschema/cap-iacs-parcel#dataQualityMeasureDocumentation">
        <rdfs:range rdf:resource="http://lpis.ec.europa.eu/registry/applicationschema/cap-iacs-parcel#DataQualityMeasure"/>
        <rdfs:label xml:lang="en">Description of data quality measure</rdfs:label>
        <skos:definition xml:lang="en">--Name--
Data quality measure documentation

-- Definition --
Description of a particular data quality measure in terms of ISO 19157:2013. 

-- Description --
Detailed description of data quality measure according to the profile of DQM_Measure data type derived from ISO 19157:2013.</skos:definition>
    </owl:ObjectProperty>
    


    <!-- http://lpis.ec.europa.eu/registry/applicationschema/cap-iacs-parcel#dataQualityMeasureType -->


    <owl:ObjectProperty rdf:about="http://lpis.ec.europa.eu/registry/applicationschema/cap-iacs-parcel#dataQualityMeasureType">
        <rdfs:range rdf:resource="http://lpis.ec.europa.eu/registry/applicationschema/cap-iacs-parcel#DataQualityMeasureTypeIuiValue"/>
        <rdfs:label xml:lang="en">Type of data quality measure</rdfs:label>
        <skos:definition xml:lang="en">--Name--
Data quality measure type

-- Definition --
List of data quality measures applied in LPISQA.

-- Description --
Data Quality measures shall be selected from DataQualityMeasureTypeIuiValue.</skos:definition>
    </owl:ObjectProperty>
    


    <!-- http://lpis.ec.europa.eu/registry/applicationschema/cap-iacs-parcel#declaredArea -->


    <owl:ObjectProperty rdf:about="http://lpis.ec.europa.eu/registry/applicationschema/cap-iacs-parcel#declaredArea">
        <rdfs:range rdf:resource="http://qudt.org/schema/qudt/QuantityValue"/>
    </owl:ObjectProperty>
    


    <!-- http://lpis.ec.europa.eu/registry/applicationschema/cap-iacs-parcel#description -->


    <owl:ObjectProperty rdf:about="http://lpis.ec.europa.eu/registry/applicationschema/cap-iacs-parcel#description">
        <rdfs:range rdf:resource="http://lpis.ec.europa.eu/registry/applicationschema/cap-iacs-parcel#DataQualityMeasureDescription"/>
        <rdfs:label xml:lang="en">Description</rdfs:label>
        <skos:definition xml:lang="en">--Name--
Description

--Definition--
Description of the data quality measure, including all formulae and/or illustrations needed to establish the result of applying the measure.

--Description--
When it serves understanding, description may include historic reference to the older versions of LCM or LPISQA.</skos:definition>
    </owl:ObjectProperty>
    


    <!-- http://lpis.ec.europa.eu/registry/applicationschema/cap-iacs-parcel#detailsOfPreselectedParcelForInspection -->


    <owl:ObjectProperty rdf:about="http://lpis.ec.europa.eu/registry/applicationschema/cap-iacs-parcel#detailsOfPreselectedParcelForInspection">
        <rdfs:range rdf:resource="http://lpis.ec.europa.eu/registry/applicationschema/cap-iacs-parcel#EtsItemUnderInspection"/>
    </owl:ObjectProperty>
    


    <!-- http://lpis.ec.europa.eu/registry/applicationschema/cap-iacs-parcel#detailsOfselectedEfaForInspection -->


    <owl:ObjectProperty rdf:about="http://lpis.ec.europa.eu/registry/applicationschema/cap-iacs-parcel#detailsOfselectedEfaForInspection">
        <rdfs:range rdf:resource="http://lpis.ec.europa.eu/registry/applicationschema/cap-iacs-parcel#EfaItemUnderInspection"/>
    </owl:ObjectProperty>
    


    <!-- http://lpis.ec.europa.eu/registry/applicationschema/cap-iacs-parcel#determinedArea -->


    <owl:ObjectProperty rdf:about="http://lpis.ec.europa.eu/registry/applicationschema/cap-iacs-parcel#determinedArea">
        <rdfs:range rdf:resource="http://qudt.org/schema/qudt/QuantityValue"/>
    </owl:ObjectProperty>
    


    <!-- http://lpis.ec.europa.eu/registry/applicationschema/cap-iacs-parcel#ecologicalFocusArea -->


    <owl:ObjectProperty rdf:about="http://lpis.ec.europa.eu/registry/applicationschema/cap-iacs-parcel#ecologicalFocusArea">
        <rdfs:range rdf:resource="http://qudt.org/schema/qudt/QuantityValue"/>
    </owl:ObjectProperty>
    


    <!-- http://lpis.ec.europa.eu/registry/applicationschema/cap-iacs-parcel#ecologicalFocusAreaRegionDetailsForMandatedArea -->


    <owl:ObjectProperty rdf:about="http://lpis.ec.europa.eu/registry/applicationschema/cap-iacs-parcel#ecologicalFocusAreaRegionDetailsForMandatedArea">
        <rdfs:range rdf:resource="http://lpis.ec.europa.eu/registry/applicationschema/cap-iacs-parcel#EcologicalFocusAreaRegionMandatedArea"/>
    </owl:ObjectProperty>
    


    <!-- http://lpis.ec.europa.eu/registry/applicationschema/cap-iacs-parcel#ecologicalFocusAreaType -->


    <owl:ObjectProperty rdf:about="http://lpis.ec.europa.eu/registry/applicationschema/cap-iacs-parcel#ecologicalFocusAreaType">
        <rdfs:range rdf:resource="http://lpis.ec.europa.eu/registry/applicationschema/cap-iacs-parcel#EcologicalFocusAreaTypeValue"/>
        <rdfs:label xml:lang="en">Ecological focus area type</rdfs:label>
        <skos:definition xml:lang="en">--Name--
Ecological focus area type

-- Definition --
Ecological focus area type as listed in Art. 46(2) of (EU) R 1307/2013.

-- Description --
The value of this attribute shall be taken from the EcologicalFocusAreaTypeValue code list.</skos:definition>
    </owl:ObjectProperty>
    


    <!-- http://lpis.ec.europa.eu/registry/applicationschema/cap-iacs-parcel#ecologicalFocusAreaWithinCropGroupGreening -->


    <owl:ObjectProperty rdf:about="http://lpis.ec.europa.eu/registry/applicationschema/cap-iacs-parcel#ecologicalFocusAreaWithinCropGroupGreening">
        <rdfs:range rdf:resource="http://lpis.ec.europa.eu/registry/applicationschema/cap-iacs-aid#CropGroupGreening"/>
    </owl:ObjectProperty>
    


    <!-- http://lpis.ec.europa.eu/registry/applicationschema/cap-iacs-parcel#ecologicalFocusAreasAggregationDetails -->


    <owl:ObjectProperty rdf:about="http://lpis.ec.europa.eu/registry/applicationschema/cap-iacs-parcel#ecologicalFocusAreasAggregationDetails">
        <rdfs:range rdf:resource="http://lpis.ec.europa.eu/registry/applicationschema/cap-iacs-parcel#EcologicalFocusArea"/>
    </owl:ObjectProperty>
    


    <!-- http://lpis.ec.europa.eu/registry/applicationschema/cap-iacs-parcel#efaItemUnderInspectionCompositionDetails -->


    <owl:ObjectProperty rdf:about="http://lpis.ec.europa.eu/registry/applicationschema/cap-iacs-parcel#efaItemUnderInspectionCompositionDetails">
        <rdfs:range rdf:resource="http://lpis.ec.europa.eu/registry/applicationschema/cap-iacs-parcel#EfaItemUnderInspection"/>
    </owl:ObjectProperty>
    


    <!-- http://lpis.ec.europa.eu/registry/applicationschema/cap-iacs-parcel#efaItemUnderInspectionWithinEfaSampleDetails -->


    <owl:ObjectProperty rdf:about="http://lpis.ec.europa.eu/registry/applicationschema/cap-iacs-parcel#efaItemUnderInspectionWithinEfaSampleDetails">
        <rdfs:range rdf:resource="http://lpis.ec.europa.eu/registry/applicationschema/cap-iacs-parcel#EfaSample"/>
    </owl:ObjectProperty>
    


    <!-- http://lpis.ec.europa.eu/registry/applicationschema/cap-iacs-parcel#efaMissclassificationCause -->


    <owl:ObjectProperty rdf:about="http://lpis.ec.europa.eu/registry/applicationschema/cap-iacs-parcel#efaMissclassificationCause">
        <rdfs:range rdf:resource="http://lpis.ec.europa.eu/registry/applicationschema/cap-iacs-parcel#TechnicalReasonValue"/>
        <rdfs:label xml:lang="en">Technical reasons for non-conformance</rdfs:label>
        <skos:definition xml:lang="en">--Name--
Area non-conformance cause.

-- Definition --
This is a placeholder only; currently not to be implemented.

-- Description --
Technical reasons for non-conformance.</skos:definition>
    </owl:ObjectProperty>
    


    <!-- http://lpis.ec.europa.eu/registry/applicationschema/cap-iacs-parcel#efaRemedialActionPlan -->


    <owl:ObjectProperty rdf:about="http://lpis.ec.europa.eu/registry/applicationschema/cap-iacs-parcel#efaRemedialActionPlan">
        <rdfs:range rdf:resource="http://lpis.ec.europa.eu/registry/applicationschema/cap-iacs-base#SupplementaryDocument"/>
        <rdfs:label xml:lang="en">Remedial action plan</rdfs:label>
        <skos:definition xml:lang="en">--Name--
EFA remedial action plan

--Definition--
This is a placeholder only; currently not to be implemented.

Report describing measures and timescale of actions to be taken by the authority responsible for the maintenance of EFA.

-- Description --
This additional to the EFA report shall be delivered when the EFA sample results to be non conforming for quality elements.   It shall also provide analysis of quality measures not evaluated by conformance results.</skos:definition>
    </owl:ObjectProperty>
    


    <!-- http://lpis.ec.europa.eu/registry/applicationschema/cap-iacs-parcel#efaReport -->


    <owl:ObjectProperty rdf:about="http://lpis.ec.europa.eu/registry/applicationschema/cap-iacs-parcel#efaReport">
        <rdfs:range rdf:resource="http://lpis.ec.europa.eu/registry/applicationschema/cap-iacs-base#SupplementaryDocument"/>
        <rdfs:label xml:lang="en">EFA report</rdfs:label>
        <skos:definition xml:lang="en">--Name--
EFA quality assessment report

-- Definition --
This is a placeholder only; currently not to be implemented.

-- Description --
Report summarising the results of the EFA inspection, the quality elements and their evaluation.</skos:definition>
    </owl:ObjectProperty>
    


    <!-- http://lpis.ec.europa.eu/registry/applicationschema/cap-iacs-parcel#efaSampleDetailsForItemsUnderInspectionEfa -->


    <owl:ObjectProperty rdf:about="http://lpis.ec.europa.eu/registry/applicationschema/cap-iacs-parcel#efaSampleDetailsForItemsUnderInspectionEfa">
        <rdfs:range rdf:resource="http://lpis.ec.europa.eu/registry/applicationschema/cap-iacs-parcel#EfaItemUnderInspection"/>
    </owl:ObjectProperty>
    


    <!-- http://lpis.ec.europa.eu/registry/applicationschema/cap-iacs-parcel#efaSampleDetailsForLpisLot -->


    <owl:ObjectProperty rdf:about="http://lpis.ec.europa.eu/registry/applicationschema/cap-iacs-parcel#efaSampleDetailsForLpisLot">
        <rdfs:range rdf:resource="http://lpis.ec.europa.eu/registry/applicationschema/cap-iacs-parcel#LpisLot"/>
    </owl:ObjectProperty>
    


    <!-- http://lpis.ec.europa.eu/registry/applicationschema/cap-iacs-parcel#equivalentAecm -->


    <owl:ObjectProperty rdf:about="http://lpis.ec.europa.eu/registry/applicationschema/cap-iacs-parcel#equivalentAecm">
        <rdfs:range rdf:resource="http://lpis.ec.europa.eu/registry/applicationschema/cap-iacs-parcel#EcologicalFocusAreaEquivalentPracticeTypeValue"/>
        <rdfs:label xml:lang="en">Equivalinet practices</rdfs:label>
        <skos:definition xml:lang="en">--Name--
Equivalent EFA practice

-- Definition --
Equivalent practices with EFAs which are listed  in section III of Annex IX of Regulation (EU) No 1307/2013.

-- Description --
EFA equivalent practices include:
-ecological set-aside;
-buffer zones for high nature value areas ( Natura 2000 or similar);
-uncultivated buffer strips and field margins;
-patches managed for wildlife or specific fauna;
-management of LF;
-keeping arable peaty or wet soils under grass;
-production on arable land without fertilizers or plant protection products (for 2 years with different crops);
-conversion of arable land into permanent grassland extensively used.

NOTE: The specific AECM reason has to be linked to the EFA type.</skos:definition>
    </owl:ObjectProperty>
    


    <!-- http://lpis.ec.europa.eu/registry/applicationschema/cap-iacs-parcel#etsItemUnderInspectionWithinEtsSampleDetails -->


    <owl:ObjectProperty rdf:about="http://lpis.ec.europa.eu/registry/applicationschema/cap-iacs-parcel#etsItemUnderInspectionWithinEtsSampleDetails">
        <rdfs:range rdf:resource="http://lpis.ec.europa.eu/registry/applicationschema/cap-iacs-parcel#EtsSample"/>
    </owl:ObjectProperty>
    


    <!-- http://lpis.ec.europa.eu/registry/applicationschema/cap-iacs-parcel#etsReport -->


    <owl:ObjectProperty rdf:about="http://lpis.ec.europa.eu/registry/applicationschema/cap-iacs-parcel#etsReport">
        <rdfs:range rdf:resource="http://lpis.ec.europa.eu/registry/applicationschema/cap-iacs-base#SupplementaryDocument"/>
        <rdfs:label xml:lang="en">ETS report</rdfs:label>
        <skos:definition xml:lang="en">--Name--
ETS report

-- Definition --
Presentation of the results of ETS .

-- Description --
Report summarizing the results of the ETS inspection, the quality elements and their evaluation.</skos:definition>
    </owl:ObjectProperty>
    


    <!-- http://lpis.ec.europa.eu/registry/applicationschema/cap-iacs-parcel#etsSampleDetailsForEtsItemsUnderInspection -->


    <owl:ObjectProperty rdf:about="http://lpis.ec.europa.eu/registry/applicationschema/cap-iacs-parcel#etsSampleDetailsForEtsItemsUnderInspection">
        <rdfs:range rdf:resource="http://lpis.ec.europa.eu/registry/applicationschema/cap-iacs-parcel#EtsItemUnderInspection"/>
    </owl:ObjectProperty>
    


    <!-- http://lpis.ec.europa.eu/registry/applicationschema/cap-iacs-parcel#etsSampleDetailsForLpisLot -->


    <owl:ObjectProperty rdf:about="http://lpis.ec.europa.eu/registry/applicationschema/cap-iacs-parcel#etsSampleDetailsForLpisLot">
        <rdfs:range rdf:resource="http://lpis.ec.europa.eu/registry/applicationschema/cap-iacs-parcel#LpisLot"/>
    </owl:ObjectProperty>
    


    <!-- http://lpis.ec.europa.eu/registry/applicationschema/cap-iacs-parcel#example -->


    <owl:ObjectProperty rdf:about="http://lpis.ec.europa.eu/registry/applicationschema/cap-iacs-parcel#example">
        <rdfs:range rdf:resource="http://lpis.ec.europa.eu/registry/applicationschema/cap-iacs-parcel#DataQualityMeasureDescription"/>
        <rdfs:label xml:lang="en">Example</rdfs:label>
        <skos:definition xml:lang="en">--Name--
Example

--Definition--
Illustration of the use of a data quality measure.

--Description--
The Commission Services provides illustrations of the use for the DQM proposed for LPISQA.  When and MS/region opts for other than these DQM, examples shall be given (otherwise can be omitted).</skos:definition>
    </owl:ObjectProperty>
    


    <!-- http://lpis.ec.europa.eu/registry/applicationschema/cap-iacs-parcel#executableTestResult -->


    <owl:ObjectProperty rdf:about="http://lpis.ec.europa.eu/registry/applicationschema/cap-iacs-parcel#executableTestResult">
        <rdfs:range rdf:resource="http://lpis.ec.europa.eu/registry/applicationschema/cap-iacs-base#TestVerdictValue"/>
        <rdfs:label xml:lang="en">Result of test</rdfs:label>
        <skos:definition xml:lang="en">--Name--
Executable test result

-- Definition --
Verdict on the outcome on the specific executable test case.

-- Description --
Conformance result on the outcome of a specific ETS test case.</skos:definition>
    </owl:ObjectProperty>
    


    <!-- http://lpis.ec.europa.eu/registry/applicationschema/cap-iacs-parcel#extendedDescription -->


    <owl:ObjectProperty rdf:about="http://lpis.ec.europa.eu/registry/applicationschema/cap-iacs-parcel#extendedDescription">
        <rdfs:range rdf:resource="http://www.w3.org/2002/07/owl#Class"/>
        <rdfs:label xml:lang="en">Cross-compliance rule description</rdfs:label>
        <skos:definition xml:lang="en">--Name--
Extended description

--Definition--
Illustration that explains the use of the data quality measure.

--Description--
For LPISQA, when applicable, illustrations are given by the Commission Services. In case when an MS/Region opts for using other quality assessment framework, when necessary illustrations may be provided.</skos:definition>
    </owl:ObjectProperty>
    


    <!-- http://lpis.ec.europa.eu/registry/applicationschema/cap-iacs-parcel#geometry -->


    <owl:ObjectProperty rdf:about="http://lpis.ec.europa.eu/registry/applicationschema/cap-iacs-parcel#geometry">
        <rdfs:range rdf:resource="http://www.opengis.net/ont/geosparql#Geometry"/>
        <rdfs:label xml:lang="en">Geometry of ecological focus area</rdfs:label>
        <skos:definition xml:lang="en">--Name--
Geometry

-- Definition --
Geometry of landscape feature.

-- Description --
Representation of the geographical dimension/position of the landscape feature. LF may be represented as , point, curve, or surface depending on the options allowed by Art 46(3) of (EU) R No 1307/2013 and the choice of the MS/region.</skos:definition>
    </owl:ObjectProperty>
    


    <!-- http://lpis.ec.europa.eu/registry/applicationschema/cap-iacs-parcel#homogeneityType -->


    <owl:ObjectProperty rdf:about="http://lpis.ec.europa.eu/registry/applicationschema/cap-iacs-parcel#homogeneityType">
        <rdfs:range rdf:resource="http://lpis.ec.europa.eu/registry/applicationschema/cap-iacs-parcel#HomogeneityTypeValue"/>
        <rdfs:label xml:lang="en">Homogeneity type</rdfs:label>
        <skos:definition xml:lang="en">--Name--
Homogeneity type

-- Definition --
Homogeneity type for single and homogenous geographical areas with similar agricultural and environmental conditions as referred to Art. 46(1) of (EU) R 639/2014.

-- Description --
The values of homogeneity type shall be taken from the centrally managed code list provided in LCM.</skos:definition>
    </owl:ObjectProperty>
    


    <!-- http://lpis.ec.europa.eu/registry/applicationschema/cap-iacs-parcel#homogeneityTypeCitation -->


    <owl:ObjectProperty rdf:about="http://lpis.ec.europa.eu/registry/applicationschema/cap-iacs-parcel#homogeneityTypeCitation">
        <rdfs:range rdf:resource="http://lpis.ec.europa.eu/registry/applicationschema/cap-iacs-base#SupplementaryDocumentCitation"/>
        <skos:definition xml:lang="en">--Name--
Homogeneity document citation

-- Definition --
Citation of the document defining the homogeneity type.

-- Description --
Citation of the document describing criteria for the homogeneity type applied for defining EFA regions.

NOTE 1: SDI solutions (links to registry items) are preferred.

NOTE 2: When EFA regions are applied the homogeneity criterion shall be clarified either using a citation or by a supplementary document.</skos:definition>
    </owl:ObjectProperty>
    


    <!-- http://lpis.ec.europa.eu/registry/applicationschema/cap-iacs-parcel#homogeneityTypeDocument -->


    <owl:ObjectProperty rdf:about="http://lpis.ec.europa.eu/registry/applicationschema/cap-iacs-parcel#homogeneityTypeDocument">
        <rdfs:range rdf:resource="http://lpis.ec.europa.eu/registry/applicationschema/cap-iacs-base#SupplementaryDocument"/>
        <rdfs:label xml:lang="en">Homogeinity type documenation</rdfs:label>
        <skos:definition xml:lang="en">--Name--
Homogeneity document

-- Definition --
Document defining the homogeneity type.

-- Description --
Document describing criteria for the homogeneity type applied for defining EFA regions.

NOTE: When EFA regions are applied the homogeneity criterion shall be clarified either using a citation or by a supplementary document.</skos:definition>
    </owl:ObjectProperty>
    


    <!-- http://lpis.ec.europa.eu/registry/applicationschema/cap-iacs-parcel#inspectionMethod -->


    <owl:ObjectProperty rdf:about="http://lpis.ec.europa.eu/registry/applicationschema/cap-iacs-parcel#inspectionMethod">
        <rdfs:range rdf:resource="http://lpis.ec.europa.eu/registry/applicationschema/cap-iacs-parcel#InspectionMethodValue"/>
        <rdfs:label xml:lang="en">Inspection method</rdfs:label>
        <skos:definition xml:lang="en">--Name--
Inspection method

-- Definition --
Method applied for the quality assessment process.

-- Description --
The value shall be selected from the InspecionMethodValue code list before the inspection starts. The selected method shall be applied to all inspected items. Changing the inspection method from item to item is forbidden.

NOTE: MS/Region have the opportunity to change the inspection method from year to year. The selected method shall be reported together with the PointZeroState file.</skos:definition>
    </owl:ObjectProperty>
    


    <!-- http://lpis.ec.europa.eu/registry/applicationschema/cap-iacs-parcel#itemAgriculturalLandDetails -->


    <owl:ObjectProperty rdf:about="http://lpis.ec.europa.eu/registry/applicationschema/cap-iacs-parcel#itemAgriculturalLandDetails">
        <rdfs:range rdf:resource="http://lpis.ec.europa.eu/registry/applicationschema/cap-iacs-parcel#EtsItemUnderInspection"/>
    </owl:ObjectProperty>
    


    <!-- http://lpis.ec.europa.eu/registry/applicationschema/cap-iacs-parcel#itemContaminationDetails -->


    <owl:ObjectProperty rdf:about="http://lpis.ec.europa.eu/registry/applicationschema/cap-iacs-parcel#itemContaminationDetails">
        <rdfs:range rdf:resource="http://lpis.ec.europa.eu/registry/applicationschema/cap-iacs-parcel#EtsItemUnderInspection"/>
    </owl:ObjectProperty>
    


    <!-- http://lpis.ec.europa.eu/registry/applicationschema/cap-iacs-parcel#itemCriticalDefectDetails -->


    <owl:ObjectProperty rdf:about="http://lpis.ec.europa.eu/registry/applicationschema/cap-iacs-parcel#itemCriticalDefectDetails">
        <rdfs:range rdf:resource="http://lpis.ec.europa.eu/registry/applicationschema/cap-iacs-parcel#EtsItemUnderInspection"/>
    </owl:ObjectProperty>
    


    <!-- http://lpis.ec.europa.eu/registry/applicationschema/cap-iacs-parcel#itemUnderInspectionEfaCriticalDefectDetails -->


    <owl:ObjectProperty rdf:about="http://lpis.ec.europa.eu/registry/applicationschema/cap-iacs-parcel#itemUnderInspectionEfaCriticalDefectDetails">
        <rdfs:range rdf:resource="http://lpis.ec.europa.eu/registry/applicationschema/cap-iacs-parcel#EfaItemUnderInspection"/>
    </owl:ObjectProperty>
    


    <!-- http://lpis.ec.europa.eu/registry/applicationschema/cap-iacs-parcel#landCover -->


    <owl:ObjectProperty rdf:about="http://lpis.ec.europa.eu/registry/applicationschema/cap-iacs-parcel#landCover">
        <rdfs:range rdf:resource="http://lpis.ec.europa.eu/registry/applicationschema/cap-iacs-parcel#AgriculturalAreaTypeValue"/>
        <rdfs:label xml:lang="en">Land cover</rdfs:label>
        <skos:definition xml:lang="en">--Name--
Land cover

--Definition--
Classification of the LC according to the types defined in the eligibility profile.

-- Description --
Identifiable instances of a land cover type listed in the eligibility profile located within the item under inspection. The value of this attribute has to be taken from the AgriculturalAreaValueType code list.

NOTE. Land cover classes with different pro-rata coefficients constitute separate land cover classes.</skos:definition>
    </owl:ObjectProperty>
    


    <!-- http://lpis.ec.europa.eu/registry/applicationschema/cap-iacs-parcel#landscapeFeatureArea -->


    <owl:ObjectProperty rdf:about="http://lpis.ec.europa.eu/registry/applicationschema/cap-iacs-parcel#landscapeFeatureArea">
        <rdfs:range rdf:resource="http://qudt.org/schema/qudt/QuantityValue"/>
    </owl:ObjectProperty>
    


    <!-- http://lpis.ec.europa.eu/registry/applicationschema/cap-iacs-parcel#landscapeFeatureAsEfaItemUnderInspectionDetails -->


    <owl:ObjectProperty rdf:about="http://lpis.ec.europa.eu/registry/applicationschema/cap-iacs-parcel#landscapeFeatureAsEfaItemUnderInspectionDetails">
        <rdfs:range rdf:resource="http://lpis.ec.europa.eu/registry/applicationschema/cap-iacs-parcel#EfaItemUnderInspection"/>
    </owl:ObjectProperty>
    


    <!-- http://lpis.ec.europa.eu/registry/applicationschema/cap-iacs-parcel#landscapeFeatureDetailsForCrossCompliance -->


    <owl:ObjectProperty rdf:about="http://lpis.ec.europa.eu/registry/applicationschema/cap-iacs-parcel#landscapeFeatureDetailsForCrossCompliance">
        <rdfs:range rdf:resource="http://lpis.ec.europa.eu/registry/applicationschema/cap-iacs-aid#CrossCompliance"/>
    </owl:ObjectProperty>
    


    <!-- http://lpis.ec.europa.eu/registry/applicationschema/cap-iacs-parcel#landscapeFeatureForEcologicalFocusArea -->


    <owl:ObjectProperty rdf:about="http://lpis.ec.europa.eu/registry/applicationschema/cap-iacs-parcel#landscapeFeatureForEcologicalFocusArea">
        <rdfs:range rdf:resource="http://lpis.ec.europa.eu/registry/applicationschema/cap-iacs-parcel#EcologicalFocusArea"/>
    </owl:ObjectProperty>
    


    <!-- http://lpis.ec.europa.eu/registry/applicationschema/cap-iacs-parcel#landscapeFeatureSelectionDetails -->


    <owl:ObjectProperty rdf:about="http://lpis.ec.europa.eu/registry/applicationschema/cap-iacs-parcel#landscapeFeatureSelectionDetails">
        <rdfs:range rdf:resource="http://lpis.ec.europa.eu/registry/applicationschema/cap-iacs-parcel#LandscapeFeature"/>
    </owl:ObjectProperty>
    


    <!-- http://lpis.ec.europa.eu/registry/applicationschema/cap-iacs-parcel#landscapeFeatureType -->


    <owl:ObjectProperty rdf:about="http://lpis.ec.europa.eu/registry/applicationschema/cap-iacs-parcel#landscapeFeatureType">
        <rdfs:range rdf:resource="http://lpis.ec.europa.eu/registry/applicationschema/cap-iacs-parcel#LandscapeFeatureValueType"/>
        <rdfs:label xml:lang="en">Landscape feature type</rdfs:label>
        <skos:definition xml:lang="en">--Name--
Landscape feature type

-- Definition --
Landscape feature type as listed in Art. 46(2) of (EU) R 1307/2013.

-- Description --
The value of this attribute are taken from the LandcapeFeatureValueType code list of the eligibility profile.</skos:definition>
    </owl:ObjectProperty>
    


    <!-- http://lpis.ec.europa.eu/registry/applicationschema/cap-iacs-parcel#limitingQuality -->


    <owl:ObjectProperty rdf:about="http://lpis.ec.europa.eu/registry/applicationschema/cap-iacs-parcel#limitingQuality">
        <rdfs:range rdf:resource="http://lpis.ec.europa.eu/registry/applicationschema/cap-iacs-parcel#LimitingQualityValue"/>
        <rdfs:label xml:lang="en">Default value of limiting quality parameter</rdfs:label>
        <skos:definition xml:lang="en">--Name--
Limiting quality 

-- Definition --
Sampling parameter (index) necessary for the definition of the acceptance values as function of a given sample size. 

-- Description --
Limiting quality value shall be taken from the  corresponding enumeration. LQ applied for critical defects shall be 2,00. For any other conformance result LQ shall be 12,50.</skos:definition>
    </owl:ObjectProperty>
    


    <!-- http://lpis.ec.europa.eu/registry/applicationschema/cap-iacs-parcel#lotSize -->


    <owl:ObjectProperty rdf:about="http://lpis.ec.europa.eu/registry/applicationschema/cap-iacs-parcel#lotSize">
        <rdfs:range rdf:resource="http://lpis.ec.europa.eu/registry/applicationschema/cap-iacs-parcel#LotSizeValue"/>
        <rdfs:label xml:lang="en">Lot size value</rdfs:label>
        <skos:definition xml:lang="en">--Name--
Lot size

-- Definition --
Number of items in a lot [ISO 2859-1:1999].

-- Description --
It is the number of reference parcels within the LPIS lot.</skos:definition>
    </owl:ObjectProperty>
    


    <!-- http://lpis.ec.europa.eu/registry/applicationschema/cap-iacs-parcel#lpisLotDetailsForEfaSample -->


    <owl:ObjectProperty rdf:about="http://lpis.ec.europa.eu/registry/applicationschema/cap-iacs-parcel#lpisLotDetailsForEfaSample">
        <rdfs:range rdf:resource="http://lpis.ec.europa.eu/registry/applicationschema/cap-iacs-parcel#EfaSample"/>
    </owl:ObjectProperty>
    


    <!-- http://lpis.ec.europa.eu/registry/applicationschema/cap-iacs-parcel#lpisRemedialActionPlan -->


    <owl:ObjectProperty rdf:about="http://lpis.ec.europa.eu/registry/applicationschema/cap-iacs-parcel#lpisRemedialActionPlan">
        <rdfs:range rdf:resource="http://lpis.ec.europa.eu/registry/applicationschema/cap-iacs-base#SupplementaryDocument"/>
        <rdfs:label xml:lang="en">Remedial action plan</rdfs:label>
        <skos:definition xml:lang="en">--Name--
LPIS remedial action plan

--Definition--
Report describing measures and timescale of actions to be taken by the authority responsible for the maintenance of LPIS.

-- Description --
This additional to the ETS report shall be delivered when the ETS sample results to be non-conforming for quality elements QE1, QE2, QE3, and QE6. It shall also provide analysis of quality measures not evaluated by conformance results.</skos:definition>
    </owl:ObjectProperty>
    


    <!-- http://lpis.ec.europa.eu/registry/applicationschema/cap-iacs-parcel#mandatedAreaWithinRegion -->


    <owl:ObjectProperty rdf:about="http://lpis.ec.europa.eu/registry/applicationschema/cap-iacs-parcel#mandatedAreaWithinRegion">
        <rdfs:range rdf:resource="http://lpis.ec.europa.eu/registry/applicationschema/cap-iacs-parcel#EcologicalFocusAreaRegion"/>
    </owl:ObjectProperty>
    


    <!-- http://lpis.ec.europa.eu/registry/applicationschema/cap-iacs-parcel#measureIdentifier -->


    <owl:ObjectProperty rdf:about="http://lpis.ec.europa.eu/registry/applicationschema/cap-iacs-parcel#measureIdentifier">
        <rdfs:range rdf:resource="http://lpis.ec.europa.eu/registry/applicationschema/cap-iacs-parcel#DataQualityMeasureNameValue"/>
        <rdfs:label xml:lang="en">Measure identifier</rdfs:label>
        <skos:definition xml:lang="en">--Name--
Measure identifier

--Definition --
Identifier uniquely identifying a DQM within a namespace.

--Description--
Identifiers for data quality measures for LPISQA are listed in the description of the specific DQM.</skos:definition>
    </owl:ObjectProperty>
    


    <!-- http://lpis.ec.europa.eu/registry/applicationschema/cap-iacs-parcel#metadata -->


    <owl:ObjectProperty rdf:about="http://lpis.ec.europa.eu/registry/applicationschema/cap-iacs-parcel#metadata">
        <rdfs:range rdf:resource="http://lpis.ec.europa.eu/registry/applicationschema/cap-iacs-base#FeatureLevelMetadata"/>
        <rdfs:label xml:lang="en">Feature-level metadata</rdfs:label>
        <skos:definition xml:lang="en">--Name--
Metadata

-- Definition --
Feature-level metadata are attributes of a feature type that is used to store auxiliary information about the data record belonging to that type

-- Description --
Feature level metadata can include information about the life-cycle, status, data quality, usability, responsible entity, etc.</skos:definition>
    </owl:ObjectProperty>
    


    <!-- http://lpis.ec.europa.eu/registry/applicationschema/cap-iacs-parcel#misclasificationCause -->


    <owl:ObjectProperty rdf:about="http://lpis.ec.europa.eu/registry/applicationschema/cap-iacs-parcel#misclasificationCause">
        <rdfs:range rdf:resource="http://lpis.ec.europa.eu/registry/applicationschema/cap-iacs-parcel#TechnicalReasonValue"/>
        <rdfs:label xml:lang="en">Technical reasons for misclassification</rdfs:label>
        <skos:definition xml:lang="en">--Name--
Misclassification cause.

-- Definition --
Technical reasons for misclassification.

-- Description --
Reason for misclassification shall be taken from the TechnicalReasonValue code list.
  
NOTE. MisclassificationCause shall be given when value of LandscapeFeature.dataQualityMeasureResult is FALSE (in present release only if: LandscapeFeature.dataQualityMeasyreType=classificationCorrectness).</skos:definition>
    </owl:ObjectProperty>
    


    <!-- http://lpis.ec.europa.eu/registry/applicationschema/cap-iacs-parcel#misclassificationCause -->


    <owl:ObjectProperty rdf:about="http://lpis.ec.europa.eu/registry/applicationschema/cap-iacs-parcel#misclassificationCause">
        <rdfs:range rdf:resource="http://lpis.ec.europa.eu/registry/applicationschema/cap-iacs-parcel#TechnicalReasonValue"/>
        <rdfs:label xml:lang="en">Technical reasons for misclassification</rdfs:label>
        <skos:definition xml:lang="en">--Name--
Misclassification cause

-- Definition --
Technical reasons for misclassification.

-- Description --
Reason for misclassification shall be taken from the TechnicalReasonValue code list.
  
NOTE. MisclassificationCause shall be given when value of AgriculturalLand.dataQualityMeasureResult is FALSE (where AgriculturalLand.dataQualityMeasyreType=classificationCorrectness).</skos:definition>
    </owl:ObjectProperty>
    


    <!-- http://lpis.ec.europa.eu/registry/applicationschema/cap-iacs-parcel#mtsItemUnderInspectionDetailsForExecutableTestCase -->


    <owl:ObjectProperty rdf:about="http://lpis.ec.europa.eu/registry/applicationschema/cap-iacs-parcel#mtsItemUnderInspectionDetailsForExecutableTestCase">
        <rdfs:range rdf:resource="http://lpis.ec.europa.eu/registry/applicationschema/cap-iacs-base#ExecutableTestCase"/>
    </owl:ObjectProperty>
    


    <!-- http://lpis.ec.europa.eu/registry/applicationschema/cap-iacs-parcel#mtsReport -->


    <owl:ObjectProperty rdf:about="http://lpis.ec.europa.eu/registry/applicationschema/cap-iacs-parcel#mtsReport">
        <rdfs:range rdf:resource="http://lpis.ec.europa.eu/registry/applicationschema/cap-iacs-base#SupplementaryDocument"/>
        <rdfs:label xml:lang="en">MTS report</rdfs:label>
        <skos:definition xml:lang="en">--Name--
MTS report

-- Definition --
Documentation of the inspection process in form of standard report.

-- Description --
The report shall contain the results of testing (according to the xml schemas), their analysis and an action plan to deal with non-conformities.</skos:definition>
    </owl:ObjectProperty>
    


    <!-- http://lpis.ec.europa.eu/registry/applicationschema/cap-iacs-parcel#nonConformingItemAcceptanceNumber -->


    <owl:ObjectProperty rdf:about="http://lpis.ec.europa.eu/registry/applicationschema/cap-iacs-parcel#nonConformingItemAcceptanceNumber">
        <rdfs:range rdf:resource="http://lpis.ec.europa.eu/registry/applicationschema/cap-iacs-parcel#AcceptanceNumberValue"/>
        <rdfs:label xml:lang="en">Non-conforming item acceptance number</rdfs:label>
        <skos:definition xml:lang="en">--Name--
Acceptance number for non-conforming items

-- Definition --
Acceptance number applicable for non-conforming items.

-- Description --
If the number of non-conforming items is equal or less than specified acceptance number, the total  lot shall be accepted.
NOTE. Acceptance number of non-conforming items shall correspond to limiting quality value 12.5 specified in ISO 2859-2:1985.</skos:definition>
    </owl:ObjectProperty>
    


    <!-- http://lpis.ec.europa.eu/registry/applicationschema/cap-iacs-parcel#nonStructuredEvidenceCitation -->


    <owl:ObjectProperty rdf:about="http://lpis.ec.europa.eu/registry/applicationschema/cap-iacs-parcel#nonStructuredEvidenceCitation">
        <rdfs:range rdf:resource="http://lpis.ec.europa.eu/registry/applicationschema/cap-iacs-base#SupplementaryDocumentCitation"/>
        <rdfs:label xml:lang="en">Non-structured evidence - citation</rdfs:label>
        <skos:definition xml:lang="en">--Name--
Non-structured evidence citation

-- Definition --
Any citation that supports the decisions made during the inspection process.

-- Description --
URI of services where the supporting document (ground photographs, documents, measurement results, etc.) are accessible.</skos:definition>
    </owl:ObjectProperty>
    


    <!-- http://lpis.ec.europa.eu/registry/applicationschema/cap-iacs-parcel#nonStructuredEvidenceDocument -->


    <owl:ObjectProperty rdf:about="http://lpis.ec.europa.eu/registry/applicationschema/cap-iacs-parcel#nonStructuredEvidenceDocument">
        <rdfs:range rdf:resource="http://lpis.ec.europa.eu/registry/applicationschema/cap-iacs-base#SupplementaryDocument"/>
        <rdfs:label xml:lang="en">Non-structured evidence - document</rdfs:label>
        <skos:definition xml:lang="en">--Name--
Non-structured evidence document

-- Definition --
Any record that supports  or documents the decisions made during the inspection process.

-- Description --
EXAMPLES: description, sketch, photo, document, additional measurement data, etc.</skos:definition>
    </owl:ObjectProperty>
    


    <!-- http://lpis.ec.europa.eu/registry/applicationschema/cap-iacs-parcel#observedArea -->


    <owl:ObjectProperty rdf:about="http://lpis.ec.europa.eu/registry/applicationschema/cap-iacs-parcel#observedArea">
        <rdfs:range rdf:resource="http://qudt.org/schema/qudt/QuantityValue"/>
    </owl:ObjectProperty>
    


    <!-- http://lpis.ec.europa.eu/registry/applicationschema/cap-iacs-parcel#observedEfaType -->


    <owl:ObjectProperty rdf:about="http://lpis.ec.europa.eu/registry/applicationschema/cap-iacs-parcel#observedEfaType">
        <rdfs:range rdf:resource="http://lpis.ec.europa.eu/registry/applicationschema/cap-iacs-parcel#EcologicalFocusAreaTypeValue"/>
        <rdfs:label xml:lang="en">EFA type observed</rdfs:label>
        <skos:definition xml:lang="en">-- Name--
Observed EFA type 

-- Definition --
This is a placeholder only; currently not to be implemented.</skos:definition>
    </owl:ObjectProperty>
    


    <!-- http://lpis.ec.europa.eu/registry/applicationschema/cap-iacs-parcel#parameterDescription -->


    <owl:ObjectProperty rdf:about="http://lpis.ec.europa.eu/registry/applicationschema/cap-iacs-parcel#parameterDescription">
        <rdfs:range rdf:resource="http://lpis.ec.europa.eu/registry/applicationschema/cap-iacs-parcel#LimitingQualityParameter"/>
        <rdfs:label xml:lang="en">Limiting quality parameter decription</rdfs:label>
        <skos:definition xml:lang="en">--Name--
Parameter desciption

-- Definition --
Description of limiting quality parameter applicable to the LPIS lot.

-- Description --
Sampling schema parameter used. ISO2859-2: Sampling procedures for inspection by attributes, Part 2: Sampling plans indexed by limiting quality (LQ) for isolated lot inspection. 

NOTE: Record set must be maintained by MS.</skos:definition>
    </owl:ObjectProperty>
    


    <!-- http://lpis.ec.europa.eu/registry/applicationschema/cap-iacs-parcel#permanentGrasslandProRata -->


    <owl:ObjectProperty rdf:about="http://lpis.ec.europa.eu/registry/applicationschema/cap-iacs-parcel#permanentGrasslandProRata">
        <rdfs:range rdf:resource="http://lpis.ec.europa.eu/registry/applicationschema/cap-iacs-parcel#ProRataCategoryValue"/>
        <rdfs:label xml:lang="en">Prorata applicable for permanent grassland only</rdfs:label>
        <skos:definition xml:lang="en">--Name--
Permanent grassland pro-rata

-- Definition --
Homogeneous land cover type for which a fixed reduction coefficient based on the percentage of ineligible area is applied (Art. 10 of EU 640/2014).

-- Description --
Pro-rata applicable for permanent grassland only.</skos:definition>
    </owl:ObjectProperty>
    


    <!-- http://lpis.ec.europa.eu/registry/applicationschema/cap-iacs-parcel#preselectedReferenceParcelWithinTheLotDetails -->


    <owl:ObjectProperty rdf:about="http://lpis.ec.europa.eu/registry/applicationschema/cap-iacs-parcel#preselectedReferenceParcelWithinTheLotDetails">
        <rdfs:range rdf:resource="http://lpis.ec.europa.eu/registry/applicationschema/cap-iacs-parcel#LpisLot"/>
    </owl:ObjectProperty>
    


    <!-- http://lpis.ec.europa.eu/registry/applicationschema/cap-iacs-parcel#recordedArea -->


    <owl:ObjectProperty rdf:about="http://lpis.ec.europa.eu/registry/applicationschema/cap-iacs-parcel#recordedArea">
        <rdfs:range rdf:resource="http://qudt.org/schema/qudt/QuantityValue"/>
    </owl:ObjectProperty>
    


    <!-- http://lpis.ec.europa.eu/registry/applicationschema/cap-iacs-parcel#recordedEfaType -->


    <owl:ObjectProperty rdf:about="http://lpis.ec.europa.eu/registry/applicationschema/cap-iacs-parcel#recordedEfaType">
        <rdfs:range rdf:resource="http://lpis.ec.europa.eu/registry/applicationschema/cap-iacs-parcel#EcologicalFocusAreaTypeValue"/>
        <rdfs:label xml:lang="en">EFA type recorded</rdfs:label>
        <skos:definition xml:lang="en">-- Name--
Recorded EFA type 

-- Definition --
This is a placeholder only; currently not to be implemented.

-- Description --
EFA type recorded.</skos:definition>
    </owl:ObjectProperty>
    


    <!-- http://lpis.ec.europa.eu/registry/applicationschema/cap-iacs-parcel#referenceArea -->


    <owl:ObjectProperty rdf:about="http://lpis.ec.europa.eu/registry/applicationschema/cap-iacs-parcel#referenceArea">
        <rdfs:range rdf:resource="http://qudt.org/schema/qudt/QuantityValue"/>
    </owl:ObjectProperty>
    


    <!-- http://lpis.ec.europa.eu/registry/applicationschema/cap-iacs-parcel#referenceParcelDetailsForAggregation -->


    <owl:ObjectProperty rdf:about="http://lpis.ec.europa.eu/registry/applicationschema/cap-iacs-parcel#referenceParcelDetailsForAggregation">
        <rdfs:range rdf:resource="http://lpis.ec.europa.eu/registry/applicationschema/cap-iacs-parcel#EtsItemUnderInspection"/>
    </owl:ObjectProperty>
    


    <!-- http://lpis.ec.europa.eu/registry/applicationschema/cap-iacs-parcel#referenceParcelWithinTheLotDetails -->


    <owl:ObjectProperty rdf:about="http://lpis.ec.europa.eu/registry/applicationschema/cap-iacs-parcel#referenceParcelWithinTheLotDetails">
        <rdfs:range rdf:resource="http://lpis.ec.europa.eu/registry/applicationschema/cap-iacs-parcel#ReferenceParcel"/>
    </owl:ObjectProperty>
    


    <!-- http://lpis.ec.europa.eu/registry/applicationschema/cap-iacs-parcel#referenceParcelsLotDetails -->


    <owl:ObjectProperty rdf:about="http://lpis.ec.europa.eu/registry/applicationschema/cap-iacs-parcel#referenceParcelsLotDetails">
        <rdfs:range rdf:resource="http://lpis.ec.europa.eu/registry/applicationschema/cap-iacs-parcel#LpisLot"/>
    </owl:ObjectProperty>
    


    <!-- http://lpis.ec.europa.eu/registry/applicationschema/cap-iacs-parcel#sampleSize -->


    <owl:ObjectProperty rdf:about="http://lpis.ec.europa.eu/registry/applicationschema/cap-iacs-parcel#sampleSize">
        <rdfs:range rdf:resource="http://lpis.ec.europa.eu/registry/applicationschema/cap-iacs-parcel#SampleSizeValue"/>
        <rdfs:label xml:lang="en">Sample size value</rdfs:label>
        <skos:definition xml:lang="en">--Name--
Sample size

-- Definition --
Number of items in the sample [ISO 2859-1:1999].

-- Description --
Number of reference parcels sufficient for the purposes of LPISQA. Should be selected by the MS/Region as function of LQ and LPIS lot size.</skos:definition>
    </owl:ObjectProperty>
    


    <!-- http://lpis.ec.europa.eu/registry/applicationschema/cap-iacs-parcel#selectedReferenceParcelDetails -->


    <owl:ObjectProperty rdf:about="http://lpis.ec.europa.eu/registry/applicationschema/cap-iacs-parcel#selectedReferenceParcelDetails">
        <rdfs:range rdf:resource="http://lpis.ec.europa.eu/registry/applicationschema/cap-iacs-parcel#PreselectedParcel"/>
    </owl:ObjectProperty>
    


    <!-- http://lpis.ec.europa.eu/registry/applicationschema/cap-iacs-parcel#skippingReasonType -->


    <owl:ObjectProperty rdf:about="http://lpis.ec.europa.eu/registry/applicationschema/cap-iacs-parcel#skippingReasonType">
        <rdfs:range rdf:resource="http://lpis.ec.europa.eu/registry/applicationschema/cap-iacs-parcel#SkippingReasonTypeValue"/>
        <rdfs:label xml:lang="en">Skipping reason type</rdfs:label>
        <skos:definition xml:lang="en">--Name--
Skipping reason type

-- Definition --
Technical reasons that prevent the inspection of the given reference parcel.

-- Description --
Technical reasons that do not allow the inspection of the given reference parcel. Required if feasibilityForInspection value is TRUE. The values shall be taken from the SkippingReasonTypeValue code list.</skos:definition>
    </owl:ObjectProperty>
    


    <!-- http://lpis.ec.europa.eu/registry/applicationschema/cap-iacs-parcel#supportSchemaType -->


    <owl:ObjectProperty rdf:about="http://lpis.ec.europa.eu/registry/applicationschema/cap-iacs-parcel#supportSchemaType">
        <rdfs:range rdf:resource="http://lpis.ec.europa.eu/registry/applicationschema/cap-iacs-base#SupportSchemeTypeValue"/>
        <rdfs:label xml:lang="en">Support schema type</rdfs:label>
        <skos:definition xml:lang="en">--Name--
Support schema type

-- Definition --
Support schema type as defined in Annex I of Regulation  (EU) 1307/2013.

-- Description --
The maximum eligible area for a given reference parcel (i.e. the reference area value) used for the automatic crosscheck of the farmer‘s application depends on the support scheme. It is necessary therefore to indicate the support scheme, for which a specific area value is valid.

NOTE. Currently in this model version only maximum 11 schemas have placeholders.</skos:definition>
    </owl:ObjectProperty>
    


    <!-- http://lpis.ec.europa.eu/registry/applicationschema/cap-iacs-parcel#totalDeclaredArea -->


    <owl:ObjectProperty rdf:about="http://lpis.ec.europa.eu/registry/applicationschema/cap-iacs-parcel#totalDeclaredArea">
        <rdfs:range rdf:resource="http://qudt.org/schema/qudt/QuantityValue"/>
    </owl:ObjectProperty>
    


    <!-- http://lpis.ec.europa.eu/registry/applicationschema/cap-iacs-parcel#totalDeclaredAreaMeasuredItems -->


    <owl:ObjectProperty rdf:about="http://lpis.ec.europa.eu/registry/applicationschema/cap-iacs-parcel#totalDeclaredAreaMeasuredItems">
        <rdfs:range rdf:resource="http://qudt.org/schema/qudt/QuantityValue"/>
    </owl:ObjectProperty>
    


    <!-- http://lpis.ec.europa.eu/registry/applicationschema/cap-iacs-parcel#totalOverestimatedArea -->


    <owl:ObjectProperty rdf:about="http://lpis.ec.europa.eu/registry/applicationschema/cap-iacs-parcel#totalOverestimatedArea">
        <rdfs:range rdf:resource="http://qudt.org/schema/qudt/QuantityValue"/>
    </owl:ObjectProperty>
    


    <!-- http://lpis.ec.europa.eu/registry/applicationschema/cap-iacs-parcel#totalReferenceArea -->


    <owl:ObjectProperty rdf:about="http://lpis.ec.europa.eu/registry/applicationschema/cap-iacs-parcel#totalReferenceArea">
        <rdfs:range rdf:resource="http://qudt.org/schema/qudt/QuantityValue"/>
    </owl:ObjectProperty>
    


    <!-- http://lpis.ec.europa.eu/registry/applicationschema/cap-iacs-parcel#totalReferenceAreaMeasuredItems -->


    <owl:ObjectProperty rdf:about="http://lpis.ec.europa.eu/registry/applicationschema/cap-iacs-parcel#totalReferenceAreaMeasuredItems">
        <rdfs:range rdf:resource="http://qudt.org/schema/qudt/QuantityValue"/>
    </owl:ObjectProperty>
    


    <!-- http://lpis.ec.europa.eu/registry/applicationschema/cap-iacs-parcel#totalUnderestimatedArea -->


    <owl:ObjectProperty rdf:about="http://lpis.ec.europa.eu/registry/applicationschema/cap-iacs-parcel#totalUnderestimatedArea">
        <rdfs:range rdf:resource="http://qudt.org/schema/qudt/QuantityValue"/>
    </owl:ObjectProperty>
    


    <!-- http://lpis.ec.europa.eu/registry/applicationschema/cap-iacs-parcel#valueStructure -->


    <owl:ObjectProperty rdf:about="http://lpis.ec.europa.eu/registry/applicationschema/cap-iacs-parcel#valueStructure">
        <rdfs:range rdf:resource="http://lpis.ec.europa.eu/registry/applicationschema/cap-iacs-parcel#DataQualityMeasureValueStructureValue"/>
        <rdfs:label xml:lang="en">Value structure</rdfs:label>
        <skos:definition xml:lang="en">--Name--
Value structure

--Definition--
Structure for reporting a complex data quality result.

--Description--
The applicable in LPISQA value structures are defined in ISO 19157:2013 in the DQM_ValueStructure code list.</skos:definition>
    </owl:ObjectProperty>
    


    <!-- http://lpis.ec.europa.eu/registry/applicationschema/cap-iacs-parcel#weightedArea -->


    <owl:ObjectProperty rdf:about="http://lpis.ec.europa.eu/registry/applicationschema/cap-iacs-parcel#weightedArea">
        <rdfs:range rdf:resource="http://qudt.org/schema/qudt/QuantityValue"/>
    </owl:ObjectProperty>
    


    <!-- 
    ///////////////////////////////////////////////////////////////////////////////////////
    //
    // Data properties
    //
    ///////////////////////////////////////////////////////////////////////////////////////
     -->


    


    <!-- http://lpis.ec.europa.eu/registry/applicationschema/cap-iacs-parcel#agriculturalArea -->


    <owl:DatatypeProperty rdf:about="http://lpis.ec.europa.eu/registry/applicationschema/cap-iacs-parcel#agriculturalArea"/>
    


    <!-- http://lpis.ec.europa.eu/registry/applicationschema/cap-iacs-parcel#alias -->


    <owl:DatatypeProperty rdf:about="http://lpis.ec.europa.eu/registry/applicationschema/cap-iacs-parcel#alias">
        <rdfs:range rdf:resource="http://www.w3.org/2001/XMLSchema#string"/>
        <rdfs:label xml:lang="en">Alias</rdfs:label>
        <skos:definition xml:lang="en">--Name--
Alias

--Definition--
Other recognized name, an abbreviation or a short name for the same data quality measure

-- Description--
Mnemonic name and the corresponding alias (if any) of DQM are given in the documentation of the as attributes of the DtsItemUnderInspection and DtsSample code lists.</skos:definition>
    </owl:DatatypeProperty>
    


    <!-- http://lpis.ec.europa.eu/registry/applicationschema/cap-iacs-parcel#conformingItemsArea -->


    <owl:DatatypeProperty rdf:about="http://lpis.ec.europa.eu/registry/applicationschema/cap-iacs-parcel#conformingItemsArea"/>
    


    <!-- http://lpis.ec.europa.eu/registry/applicationschema/cap-iacs-parcel#conversionFactor -->


    <owl:DatatypeProperty rdf:about="http://lpis.ec.europa.eu/registry/applicationschema/cap-iacs-parcel#conversionFactor">
        <rdfs:range rdf:resource="http://www.w3.org/2001/XMLSchema#double"/>
        <rdfs:label xml:lang="en">Conversion factor</rdfs:label>
        <skos:definition xml:lang="en">--Name--
Conversion factor

-- Definition --
Parameter in sense of Art. 43(3) of R (EU) 1307/2013  used for calculating the total hectares represented by the ecological focus area.

--Description--
The conversion factor is used by simplified geometric representation of EFA (point or curve) in order to arrive area values.

NOTE
Conversion factor is not applicable when EFA are represented by surfaces (GM_Surface).</skos:definition>
    </owl:DatatypeProperty>
    


    <!-- http://lpis.ec.europa.eu/registry/applicationschema/cap-iacs-parcel#convertedArea -->


    <owl:DatatypeProperty rdf:about="http://lpis.ec.europa.eu/registry/applicationschema/cap-iacs-parcel#convertedArea"/>
    


    <!-- http://lpis.ec.europa.eu/registry/applicationschema/cap-iacs-parcel#dataQualityMeasureResult -->


    <owl:DatatypeProperty rdf:about="http://lpis.ec.europa.eu/registry/applicationschema/cap-iacs-parcel#dataQualityMeasureResult">
        <rdfs:range rdf:resource="http://www.w3.org/2001/XMLSchema#string"/>
        <rdfs:label xml:lang="en">Result of data quality measure</rdfs:label>
        <skos:definition xml:lang="en">--Name--
Data quality measure result

-- Definition --
Value or values that describes the result of the quality assessment process.

-- Description --
This value can be a quantitative result, a conformance result, or descriptive result.</skos:definition>
    </owl:DatatypeProperty>
    


    <!-- http://lpis.ec.europa.eu/registry/applicationschema/cap-iacs-parcel#declaredArea -->


    <owl:DatatypeProperty rdf:about="http://lpis.ec.europa.eu/registry/applicationschema/cap-iacs-parcel#declaredArea"/>
    


    <!-- http://lpis.ec.europa.eu/registry/applicationschema/cap-iacs-parcel#declaredToRecordedArea -->


    <owl:DatatypeProperty rdf:about="http://lpis.ec.europa.eu/registry/applicationschema/cap-iacs-parcel#declaredToRecordedArea">
        <rdfs:range rdf:resource="http://www.w3.org/2001/XMLSchema#double"/>
        <rdfs:label xml:lang="en">Ratio of total declared area to recorded in LPIS area</rdfs:label>
        <skos:definition xml:lang="en">--Name--
Declared to recorded area

-- Definition --
Ratio of the total declared hectares with respect to the total number of eligible hectares recorded in LPIS.

-- Description --
The scope of this data quality element are only items with areaConformance=TRUE value.

NOTE. Previously known as QE5 V2, 10206 LPIS_RP_DCA V2</skos:definition>
    </owl:DatatypeProperty>
    


    <!-- http://lpis.ec.europa.eu/registry/applicationschema/cap-iacs-parcel#declaredToRecordedAreaMeasuredItems -->


    <owl:DatatypeProperty rdf:about="http://lpis.ec.europa.eu/registry/applicationschema/cap-iacs-parcel#declaredToRecordedAreaMeasuredItems">
        <rdfs:range rdf:resource="http://www.w3.org/2001/XMLSchema#double"/>
        <rdfs:label xml:lang="en">Declared to IACS sample area</rdfs:label>
        <skos:definition xml:lang="en">--Name--
Declared to recorded area of measured items

-- Definition --
Ratio of the declared area of the conforming sample to the corresponding area of measured items recorded in LPIS.

-- Description --
The scope of this data quality element are only items with areaConformance=TRUE value.

NOTE. Previously known as QE5 V1, 10206 LPIS_RP_DCA V1</skos:definition>
    </owl:DatatypeProperty>
    


    <!-- http://lpis.ec.europa.eu/registry/applicationschema/cap-iacs-parcel#definition -->


    <owl:DatatypeProperty rdf:about="http://lpis.ec.europa.eu/registry/applicationschema/cap-iacs-parcel#definition">
        <rdfs:range rdf:resource="http://www.w3.org/2001/XMLSchema#string"/>
        <rdfs:label xml:lang="en">Definition</rdfs:label>
        <skos:definition xml:lang="en">--Name--
Definition

--Definition--
Definition of the fundamental concept for the data quality measure.

--Description--
Whenever possible, definitions are taken from the legal acts and the related guidelines of CAP and from standard technical vocabularies (ISO, INSPIRE, mainstream IT).</skos:definition>
    </owl:DatatypeProperty>
    


    <!-- http://lpis.ec.europa.eu/registry/applicationschema/cap-iacs-parcel#determinedArea -->


    <owl:DatatypeProperty rdf:about="http://lpis.ec.europa.eu/registry/applicationschema/cap-iacs-parcel#determinedArea"/>
    


    <!-- http://lpis.ec.europa.eu/registry/applicationschema/cap-iacs-parcel#ecologicalFocusArea -->


    <owl:DatatypeProperty rdf:about="http://lpis.ec.europa.eu/registry/applicationschema/cap-iacs-parcel#ecologicalFocusArea"/>
    


    <!-- http://lpis.ec.europa.eu/registry/applicationschema/cap-iacs-parcel#ecologicalFocusAreaRegionId -->


    <owl:DatatypeProperty rdf:about="http://lpis.ec.europa.eu/registry/applicationschema/cap-iacs-parcel#ecologicalFocusAreaRegionId">
        <rdfs:range rdf:resource="http://www.w3.org/2001/XMLSchema#string"/>
        <rdfs:label xml:lang="en">Unique thematic ID of ecological focus area ragion</rdfs:label>
        <skos:definition xml:lang="en">--Name--
EFA region ID

-- Definition --
Unique thematic ID of ecological focus area region.

-- Description --
Nation-wide unique alphanumerical identification code of ecological focus area region.</skos:definition>
    </owl:DatatypeProperty>
    


    <!-- http://lpis.ec.europa.eu/registry/applicationschema/cap-iacs-parcel#elementName -->


    <owl:DatatypeProperty rdf:about="http://lpis.ec.europa.eu/registry/applicationschema/cap-iacs-parcel#elementName">
        <rdfs:range rdf:resource="http://www.w3.org/2001/XMLSchema#NCName"/>
        <rdfs:label xml:lang="en">Element name</rdfs:label>
        <skos:definition xml:lang="en">--Name--
Element name

--Definition--
Name of the data quality element for which quality is reported.

--Description--

The data quality elements corresponding to the data quality measures are listed in the description of the specific DQM.</skos:definition>
    </owl:DatatypeProperty>
    


    <!-- http://lpis.ec.europa.eu/registry/applicationschema/cap-iacs-parcel#elementlId -->


    <owl:DatatypeProperty rdf:about="http://lpis.ec.europa.eu/registry/applicationschema/cap-iacs-parcel#elementlId">
        <rdfs:range rdf:resource="http://www.w3.org/2001/XMLSchema#string"/>
        <rdfs:label xml:lang="en">Unique thematic ID of SUT element</rdfs:label>
        <skos:definition xml:lang="en">--Name--
Element identifier

-- Definition --
Unique thematic ID of SUT.

-- Description --
Nation-wide unique alphanumerical thematic identification of SUT. It can be a unique name or a unique code of the eligibility profile.</skos:definition>
    </owl:DatatypeProperty>
    


    <!-- http://lpis.ec.europa.eu/registry/applicationschema/cap-iacs-parcel#feasibilityForInspection -->


    <owl:DatatypeProperty rdf:about="http://lpis.ec.europa.eu/registry/applicationschema/cap-iacs-parcel#feasibilityForInspection">
        <rdfs:range rdf:resource="http://www.w3.org/2001/XMLSchema#boolean"/>
        <rdfs:label xml:lang="en">Feasibility for inspection</rdfs:label>
        <skos:definition xml:lang="en">--Name--
Feasibility for inspection

-- Definition --
Correctness, completeness, and usability of input data  as well as physical conditions that allow observations necessary for quality assessment.

-- Description --
Regardless of the inspection methodology the input and source data should be correct and complete and no force major conditions should prevent the inspection process. In addition, for CAPI inspection feasibility for inspection  also depends on the usability and the  completeness of the orthoimagery coverage.  

NOTE: When inspection is not feasible, the preventing reason shall be documented using the values of the SkippingReasonTypeValue code list.</skos:definition>
    </owl:DatatypeProperty>
    


    <!-- http://lpis.ec.europa.eu/registry/applicationschema/cap-iacs-parcel#feasibilityForMeasurement -->


    <owl:DatatypeProperty rdf:about="http://lpis.ec.europa.eu/registry/applicationschema/cap-iacs-parcel#feasibilityForMeasurement">
        <rdfs:range rdf:resource="http://www.w3.org/2001/XMLSchema#boolean"/>
        <rdfs:label xml:lang="en">Feasibility for measurement</rdfs:label>
        <skos:definition xml:lang="en">--Name--
Feasibility for measurement

-- Definition --
Usability (fitness for purpose) of the input vector and imagery data to quantify the area of each eligible land cover type present in the inspected item.

-- Description --
Area measurement of the item under inspection is feasible on imagery when its whole territory is free of cloud, haze and any other phenomenon that prevents the observation of its boundaries and interior.  The input vector data (LPIS) is fit for the purpose when it unambiguously defines the geometric extent of the item under inspection. In case of field measurements it comprises the necessary conditions for field measurement (unobscured visibility along the perimeter, absence of force major reason (e.g. land slide at a boundary section).

NOTE 1. If measurement is not feasible (feasibilityForMeasurement=false) then only values for itemCriticalDefectConformance and ItemConformance DQM should be defined in dataQualityMeasureType.

NOTE 2: In ETS 5.3 this measure was named 10101 RP_FSM.</skos:definition>
    </owl:DatatypeProperty>
    


    <!-- http://lpis.ec.europa.eu/registry/applicationschema/cap-iacs-parcel#landscapeFeatureArea -->


    <owl:DatatypeProperty rdf:about="http://lpis.ec.europa.eu/registry/applicationschema/cap-iacs-parcel#landscapeFeatureArea"/>
    


    <!-- http://lpis.ec.europa.eu/registry/applicationschema/cap-iacs-parcel#lpisLotName -->


    <owl:DatatypeProperty rdf:about="http://lpis.ec.europa.eu/registry/applicationschema/cap-iacs-parcel#lpisLotName">
        <rdfs:range rdf:resource="http://www.w3.org/2001/XMLSchema#string"/>
        <rdfs:label xml:lang="en">Unique name of LPIS lot</rdfs:label>
        <skos:definition xml:lang="en">--Name--
LPIS lot name

-- Definition --
Unique name of LPIS lot.

-- Description --
The name is defined by MS/Region.</skos:definition>
    </owl:DatatypeProperty>
    


    <!-- http://lpis.ec.europa.eu/registry/applicationschema/cap-iacs-parcel#lpisLotSize -->


    <owl:DatatypeProperty rdf:about="http://lpis.ec.europa.eu/registry/applicationschema/cap-iacs-parcel#lpisLotSize">
        <rdfs:range rdf:resource="http://www.w3.org/2001/XMLSchema#integer"/>
        <rdfs:label xml:lang="en">The size of LPIS lot</rdfs:label>
        <skos:definition xml:lang="en">--Name--
LPIS lot size

-- Definition --
Number of items in a lot [ISO 2859-1:1999].

-- Description --
It is the number of reference parcels within the LPIS lot.</skos:definition>
    </owl:DatatypeProperty>
    


    <!-- http://lpis.ec.europa.eu/registry/applicationschema/cap-iacs-parcel#mandatedAreaId -->


    <owl:DatatypeProperty rdf:about="http://lpis.ec.europa.eu/registry/applicationschema/cap-iacs-parcel#mandatedAreaId">
        <rdfs:range rdf:resource="http://www.w3.org/2001/XMLSchema#string"/>
        <rdfs:label xml:lang="en">Unique thematic ID of mandated area within region of ecological focus area</rdfs:label>
        <skos:definition xml:lang="en">--Name--
Mandated area ID

-- Definition --
Unique thematic ID of mandated area within region of ecological focus area.

-- Description --
Nation-wide unique alphanumerical identification code of mandated area within region of ecological focus area.</skos:definition>
    </owl:DatatypeProperty>
    


    <!-- http://lpis.ec.europa.eu/registry/applicationschema/cap-iacs-parcel#name -->


    <owl:DatatypeProperty rdf:about="http://lpis.ec.europa.eu/registry/applicationschema/cap-iacs-parcel#name">
        <rdfs:range rdf:resource="http://www.w3.org/2001/XMLSchema#string"/>
        <rdfs:label xml:lang="en">Name</rdfs:label>
        <skos:definition xml:lang="en">--Name--
Name

--Definition--
Name of the data quality measure applied in LPISQA.

-- Description--
Mnemonic names and the documentation of corresponding names of DQM are defined as attributes of the DtsItemUnderInspection and DtsSample code lists.</skos:definition>
    </owl:DatatypeProperty>
    


    <!-- http://lpis.ec.europa.eu/registry/applicationschema/cap-iacs-parcel#numberOfIncompatibleDesign -->


    <owl:DatatypeProperty rdf:about="http://lpis.ec.europa.eu/registry/applicationschema/cap-iacs-parcel#numberOfIncompatibleDesign">
        <rdfs:range rdf:resource="http://www.w3.org/2001/XMLSchema#integer"/>
        <rdfs:label xml:lang="en">Number of incompatible design</rdfs:label>
        <skos:definition xml:lang="en">--Name--
Number of incompatible design

-- Definition --
Abundance of incompatible design instances within the sample as technical cause for critical defects and non-conformances.

--Description --
Occurrences of incompatibelDesign value assigned to the items under inspection within the sample. It comprises values of misclassificationCause, criticalDefectCasue, contaminationCause, and areaNonConformityCause.
The scope of this data quality element are the above listed properties. 

NOTE. Previously known as part of Abundance for the causes for occurrence of non-conforming reference parcels, or 10204 LPIS_RP_CEA.</skos:definition>
    </owl:DatatypeProperty>
    


    <!-- http://lpis.ec.europa.eu/registry/applicationschema/cap-iacs-parcel#numberOfIncompleteProcessing -->


    <owl:DatatypeProperty rdf:about="http://lpis.ec.europa.eu/registry/applicationschema/cap-iacs-parcel#numberOfIncompleteProcessing">
        <rdfs:range rdf:resource="http://www.w3.org/2001/XMLSchema#integer"/>
        <rdfs:label xml:lang="en">Number of incomplete processing</rdfs:label>
        <skos:definition xml:lang="en">--Name--
Number of incomplete processing

-- Definition --
Abundance of incomplete processing instances within the sample as technical cause for critical defects and non-conformances.

--Description --
Occurrences of incompleteProcessing value assigned to the items under inspection within the sample. It comprises values of misclassificationCause, criticalDefectCasue, contaminationCause, and areaNonConformityCause. 
The scope of this data quality element are the above listed properties. 

NOTE. Previously known as part of Abundance for the causes for occurrence of non-conforming reference parcels, or 10204 LPIS_RP_CEA.</skos:definition>
    </owl:DatatypeProperty>
    


    <!-- http://lpis.ec.europa.eu/registry/applicationschema/cap-iacs-parcel#numberOfInspectedEfa -->


    <owl:DatatypeProperty rdf:about="http://lpis.ec.europa.eu/registry/applicationschema/cap-iacs-parcel#numberOfInspectedEfa">
        <rdfs:range rdf:resource="http://www.w3.org/2001/XMLSchema#integer"/>
        <rdfs:label xml:lang="en">Number of inspected EFA</rdfs:label>
        <skos:definition xml:lang="en">--Name--
Number of inspected EFA eleemnts

-- Definition --
This is a placeholder only; currently not to be implemented.

-- Description --
Number of EFA, for which inspection was feasible.</skos:definition>
    </owl:DatatypeProperty>
    


    <!-- http://lpis.ec.europa.eu/registry/applicationschema/cap-iacs-parcel#numberOfInspectedItems -->


    <owl:DatatypeProperty rdf:about="http://lpis.ec.europa.eu/registry/applicationschema/cap-iacs-parcel#numberOfInspectedItems">
        <rdfs:range rdf:resource="http://www.w3.org/2001/XMLSchema#integer"/>
        <rdfs:label xml:lang="en">Number of inspected items</rdfs:label>
        <skos:definition xml:lang="en">--Name--
Number of inspected items

-- Definition --
Number of items, for which inspection was feasible.

-- Description --
The items can correspond to single or aggregated parcels. A set of aggregated parcels counts as 1. The need for aggregation is defined as function of feasibility for measurement. Once an aggregated item is being measured, that item shall be inspected in full.

NOTE. Number of inspected parcels shall not be less than the SampleSizeValue corresponding to limiting quality LQ=2.</skos:definition>
    </owl:DatatypeProperty>
    


    <!-- http://lpis.ec.europa.eu/registry/applicationschema/cap-iacs-parcel#numberOfLargeMeasuredItems -->


    <owl:DatatypeProperty rdf:about="http://lpis.ec.europa.eu/registry/applicationschema/cap-iacs-parcel#numberOfLargeMeasuredItems">
        <rdfs:range rdf:resource="http://www.w3.org/2001/XMLSchema#integer"/>
        <rdfs:label xml:lang="en">Number of large measured items</rdfs:label>
        <skos:definition xml:lang="en">--Name--
Number of large measured items

--Definition --
Number of items under inspection  with surfaceArea&gt;1000 m2, for which delineation of land cover was feasible.

-- Description --
The items  under inspection can correspond to single or aggregated parcels. A set of aggregated parcels counts as 1.</skos:definition>
    </owl:DatatypeProperty>
    


    <!-- http://lpis.ec.europa.eu/registry/applicationschema/cap-iacs-parcel#numberOfMeasuredItems -->


    <owl:DatatypeProperty rdf:about="http://lpis.ec.europa.eu/registry/applicationschema/cap-iacs-parcel#numberOfMeasuredItems">
        <rdfs:range rdf:resource="http://www.w3.org/2001/XMLSchema#integer"/>
        <rdfs:label xml:lang="en">Number of measured items</rdfs:label>
        <skos:definition xml:lang="en">--Name--
Number of measured items

--Definition --
Number of items under inspection for which the delineation of land cover was feasible.

-- Description --
The items under inspection can correspond to single or aggregated parcels. A set of aggregated parcels counts as 1 item.

NOTE. Number of Measured parcels shall not be less than 200.</skos:definition>
    </owl:DatatypeProperty>
    


    <!-- http://lpis.ec.europa.eu/registry/applicationschema/cap-iacs-parcel#numberOfMissedUpdates -->


    <owl:DatatypeProperty rdf:about="http://lpis.ec.europa.eu/registry/applicationschema/cap-iacs-parcel#numberOfMissedUpdates">
        <rdfs:range rdf:resource="http://www.w3.org/2001/XMLSchema#integer"/>
        <rdfs:label xml:lang="en">Number of missed updates</rdfs:label>
        <skos:definition xml:lang="en">--Name--
Number of missed updates

-- Definition --
Abundance of missed updates within the sample as technical cause for critical defects and non-conformances.

--Description --
Occurrences of missedUpdate value assigned to the items under inspection within the sample. It comprises values of misclassificationCause, criticalDefectCasue, contaminationCause, and areaNonConformityCause.
The scope of this data quality element are the above listed properties. 

NOTE. Previously known as part of Abundance for the causes for occurrence of non-conforming reference parcels, or 10204 LPIS_RP_CEA.</skos:definition>
    </owl:DatatypeProperty>
    


    <!-- http://lpis.ec.europa.eu/registry/applicationschema/cap-iacs-parcel#numberOfMissedUpgrades -->


    <owl:DatatypeProperty rdf:about="http://lpis.ec.europa.eu/registry/applicationschema/cap-iacs-parcel#numberOfMissedUpgrades">
        <rdfs:range rdf:resource="http://www.w3.org/2001/XMLSchema#integer"/>
        <rdfs:label xml:lang="en">Number of missed upgrades</rdfs:label>
        <skos:definition xml:lang="en">--Name--
Number of missed upgrades

-- Definition --
Abundance of missed upgrades within the sample as technical cause for critical defects and non-conformances.

--Description --
Occurrences of missedUpgrade value assigned to the items under inspection within the sample. It comprises values of misclassificationCause, criticalDefectCasue, contaminationCause, and areaNonConformityCause. 
The scope of this data quality element are the above listed properties. 

NOTE. Previously known as part of Abundance for the causes for occurrence of non-conforming reference parcels, or 10204 LPIS_RP_CEA.</skos:definition>
    </owl:DatatypeProperty>
    


    <!-- http://lpis.ec.europa.eu/registry/applicationschema/cap-iacs-parcel#numberOfProcessingErrors -->


    <owl:DatatypeProperty rdf:about="http://lpis.ec.europa.eu/registry/applicationschema/cap-iacs-parcel#numberOfProcessingErrors">
        <rdfs:range rdf:resource="http://www.w3.org/2001/XMLSchema#integer"/>
        <rdfs:label xml:lang="en">Number of processing errors</rdfs:label>
        <skos:definition xml:lang="en">--Name--
Number of processing errors

-- Definition --
Abundance of processing errors within the sample as technical cause for critical defects and non-conformances.

--Description --
Occurrences of processingErrors value assigned to the items under inspection within the sample. It comprises values of misclassificationCause, criticalDefectCasue, contaminationCause, and areaNonConformityCause.
The scope of this data quality element are the above listed properties.  

NOTE. Previously known as part of Abundance for the causes for occurrence of non-conforming reference parcels, or 10204 LPIS_RP_CEA.</skos:definition>
    </owl:DatatypeProperty>
    


    <!-- http://lpis.ec.europa.eu/registry/applicationschema/cap-iacs-parcel#observedArea -->


    <owl:DatatypeProperty rdf:about="http://lpis.ec.europa.eu/registry/applicationschema/cap-iacs-parcel#observedArea"/>
    


    <!-- http://lpis.ec.europa.eu/registry/applicationschema/cap-iacs-parcel#ordinalNumber -->


    <owl:DatatypeProperty rdf:about="http://lpis.ec.europa.eu/registry/applicationschema/cap-iacs-parcel#ordinalNumber">
        <rdfs:range rdf:resource="http://www.w3.org/2001/XMLSchema#integer"/>
        <rdfs:label xml:lang="en">Sequential number of preselected reference parcel</rdfs:label>
        <skos:definition xml:lang="en">--Name--
Ordinal number

-- Definition --
Sequential number of pre-selected reference parcel defining the order of inspection.

-- Description --
The range of ordinal number is larger than the range of numbers of reference parcels to be inspected.</skos:definition>
    </owl:DatatypeProperty>
    


    <!-- http://lpis.ec.europa.eu/registry/applicationschema/cap-iacs-parcel#oversamplingParameter -->


    <owl:DatatypeProperty rdf:about="http://lpis.ec.europa.eu/registry/applicationschema/cap-iacs-parcel#oversamplingParameter">
        <rdfs:range rdf:resource="http://www.w3.org/2001/XMLSchema#double"/>
        <rdfs:label xml:lang="en">Oversampling parameter</rdfs:label>
        <skos:definition xml:lang="en">--Name--
Oversampling parameter.

-- Definition --
Extent of oversampling due to the difference between acceptance numbers prescribed by the indexes LQ=2.00 and LQ=12.50.

--Description --
For decisions based on LQ=12.50 the prescribed sample size is 200. However a number of items prescribed by LQ=2.00 is inspected and measured (oversampling). This parameter shows how the actual and sufficient population relate to one another.  

EXAMPLE. The sample size for LQ=2.00 is 1250 items. They have been inspected. Out of these items 1115 have been measured. The oversampling parameter will be defined proportionally (1115/200=5,575). It means that out of the measured items 100 (5,575x18=100,35 truncated) can be non-conforming.

NOTE: the prescribed sample size and acceptance number for LQ=2.00 test are NOT subject to proportional adaptation. I.e. only the first 500, 800 or 1250 inspected items are evaluated against an invariant acceptance number of 18.</skos:definition>
    </owl:DatatypeProperty>
    


    <!-- http://lpis.ec.europa.eu/registry/applicationschema/cap-iacs-parcel#parcelAggregation -->


    <owl:DatatypeProperty rdf:about="http://lpis.ec.europa.eu/registry/applicationschema/cap-iacs-parcel#parcelAggregation">
        <rdfs:range rdf:resource="http://www.w3.org/2001/XMLSchema#boolean"/>
        <rdfs:label xml:lang="en">Parcel aggregation</rdfs:label>
        <skos:definition xml:lang="en">--Name--
Parcel aggregation

-- Definition --
Substitution of the single parcel targeted for inspection by an inspection item formed by the aggregation of reference parcels that represent the extension of agricultural land covering this single parcel.

-- Description --
This method is mostly relevant to the LPIS based on cadastral and agricultural parcels. When a boundary section of the RP  cannot be measures because it is invisible, the item under inspection shall be extended till the visible  boundaries of each LC types present in the parcel. All observations and measurement shall be performed for this extended parcel, which is, in fact, and aggregate of parcels. The IDs of parcels that enter in aggregation shall be noted in the ETS observation report.

NOTE: Parcel aggregation is frequently applicable for LPIS based on cadastral or agricultural parcels, but must be considered by all designs.</skos:definition>
    </owl:DatatypeProperty>
    


    <!-- http://lpis.ec.europa.eu/registry/applicationschema/cap-iacs-parcel#percentage -->


    <owl:DatatypeProperty rdf:about="http://lpis.ec.europa.eu/registry/applicationschema/cap-iacs-parcel#percentage">
        <rdfs:range rdf:resource="http://www.w3.org/2001/XMLSchema#double"/>
        <rdfs:label xml:lang="en">Percentage value</rdfs:label>
        <skos:definition xml:lang="en">--Name--
Percentage

-- Definition --
Within the defined regions, Member States shall designate the areas where up to half of the percentage points of the ecological focus area requirement has to be implemented.</skos:definition>
    </owl:DatatypeProperty>
    


    <!-- http://lpis.ec.europa.eu/registry/applicationschema/cap-iacs-parcel#recordedArea -->


    <owl:DatatypeProperty rdf:about="http://lpis.ec.europa.eu/registry/applicationschema/cap-iacs-parcel#recordedArea"/>
    


    <!-- http://lpis.ec.europa.eu/registry/applicationschema/cap-iacs-parcel#referenceArea -->


    <owl:DatatypeProperty rdf:about="http://lpis.ec.europa.eu/registry/applicationschema/cap-iacs-parcel#referenceArea"/>
    


    <!-- http://lpis.ec.europa.eu/registry/applicationschema/cap-iacs-parcel#subjectToCollectiveImplementation -->


    <owl:DatatypeProperty rdf:about="http://lpis.ec.europa.eu/registry/applicationschema/cap-iacs-parcel#subjectToCollectiveImplementation">
        <rdfs:range rdf:resource="http://www.w3.org/2001/XMLSchema#boolean"/>
        <rdfs:label xml:lang="en">Subject to collective implementation</rdfs:label>
        <skos:definition xml:lang="en">--Name--
Subject for collective implementation

-- Definition --
Indication whether the EFA instance is subject for collective implementation as referred to in Art. 46(6) of (EU) R 1307/2013.

-- Description --
Collective implementation is allowed when:
- the holdings of farmers concerned are in close proximity;
- the ecological focus areas concerned are contiguous.
In order to underpin the implementation of Union policies on the environment, climate and biodiversity, Member States may designate the areas on which collective implementation is possible and may impose further obligations upon farmers or groups of farmers participating in such collective implementation.

NOTE: Aspect of collective implementation:
- If EFA is fully situated within or adjacent to arable land within one application then EFA is not subject to collective implementation.
- If EFA situated on or adjacent to arable land and covered by several applications - is subject to collective implementation.
- If subjectToCollectiveImplementation = TRUE then EFA must be contiguous.</skos:definition>
    </owl:DatatypeProperty>
    


    <!-- http://lpis.ec.europa.eu/registry/applicationschema/cap-iacs-parcel#textDescription -->


    <owl:DatatypeProperty rdf:about="http://lpis.ec.europa.eu/registry/applicationschema/cap-iacs-parcel#textDescription">
        <rdfs:range rdf:resource="http://www.w3.org/2001/XMLSchema#string"/>
        <rdfs:label xml:lang="en">Cross-compliance rule description</rdfs:label>
        <skos:definition xml:lang="en">--Name--
Text description

--Definition--
Text description of the data quality measure.

--Description--
In case and MS/Region opts for using other than LPISQA for assessing quality, the descriptions of DQM shall be given also in English.</skos:definition>
    </owl:DatatypeProperty>
    


    <!-- http://lpis.ec.europa.eu/registry/applicationschema/cap-iacs-parcel#totalDeclaredArea -->


    <owl:DatatypeProperty rdf:about="http://lpis.ec.europa.eu/registry/applicationschema/cap-iacs-parcel#totalDeclaredArea"/>
    


    <!-- http://lpis.ec.europa.eu/registry/applicationschema/cap-iacs-parcel#totalDeclaredAreaMeasuredItems -->


    <owl:DatatypeProperty rdf:about="http://lpis.ec.europa.eu/registry/applicationschema/cap-iacs-parcel#totalDeclaredAreaMeasuredItems"/>
    


    <!-- http://lpis.ec.europa.eu/registry/applicationschema/cap-iacs-parcel#totalOverestimatedArea -->


    <owl:DatatypeProperty rdf:about="http://lpis.ec.europa.eu/registry/applicationschema/cap-iacs-parcel#totalOverestimatedArea"/>
    


    <!-- http://lpis.ec.europa.eu/registry/applicationschema/cap-iacs-parcel#totalReferenceArea -->


    <owl:DatatypeProperty rdf:about="http://lpis.ec.europa.eu/registry/applicationschema/cap-iacs-parcel#totalReferenceArea"/>
    


    <!-- http://lpis.ec.europa.eu/registry/applicationschema/cap-iacs-parcel#totalReferenceAreaMeasuredItems -->


    <owl:DatatypeProperty rdf:about="http://lpis.ec.europa.eu/registry/applicationschema/cap-iacs-parcel#totalReferenceAreaMeasuredItems"/>
    


    <!-- http://lpis.ec.europa.eu/registry/applicationschema/cap-iacs-parcel#totalUnderestimatedArea -->


    <owl:DatatypeProperty rdf:about="http://lpis.ec.europa.eu/registry/applicationschema/cap-iacs-parcel#totalUnderestimatedArea"/>
    


    <!-- http://lpis.ec.europa.eu/registry/applicationschema/cap-iacs-parcel#unit -->


    <owl:DatatypeProperty rdf:about="http://lpis.ec.europa.eu/registry/applicationschema/cap-iacs-parcel#unit">
        <rdfs:range rdf:resource="http://www.w3.org/2001/XMLSchema#string"/>
        <rdfs:label xml:lang="en">Measurement unit</rdfs:label>
        <skos:definition xml:lang="en">--Name--
Unit of measure

-- Definition --
Units of measures applicable for conversion parameters

-- Description --
The unit of measures of conversion parameters shall be define in such way that the product of the unit of measure used for EFA geometry and the conversion factor result in square meters.

NOTE 1. For linear elements the unit of measure of conversion factor shall be meter.

NOTE 2. For point element the unit of measure of conversion factor shall be square meter.</skos:definition>
    </owl:DatatypeProperty>
    


    <!-- http://lpis.ec.europa.eu/registry/applicationschema/cap-iacs-parcel#valueType -->


    <owl:DatatypeProperty rdf:about="http://lpis.ec.europa.eu/registry/applicationschema/cap-iacs-parcel#valueType">
        <rdfs:range rdf:resource="http://www.w3.org/2001/XMLSchema#NCName"/>
        <rdfs:label xml:lang="en">Value type</rdfs:label>
        <skos:definition xml:lang="en">--Name--
Value type

--Definition--
Value type is the data type used for reporting the result of the measure. The data types defined in ISO/TS 19103:2005 shall be used. 

--Description--
For purposes of LPISQA the following data types are used:
- Primitive types: CharacterString, Integer, Real, Boolean
- Collections: Sequence, matrix

NOTE: Section 7 of ISO/TS 19103:2005 provides and overview of the applicable core data types.</skos:definition>
    </owl:DatatypeProperty>
    


    <!-- http://lpis.ec.europa.eu/registry/applicationschema/cap-iacs-parcel#waivered -->


    <owl:DatatypeProperty rdf:about="http://lpis.ec.europa.eu/registry/applicationschema/cap-iacs-parcel#waivered">
        <rdfs:range rdf:resource="http://www.w3.org/2001/XMLSchema#boolean"/>
        <rdfs:label xml:lang="en">Waivered</rdfs:label>
        <skos:definition xml:lang="en">--Name--
Waivered

-- Definition --
Immunity that vindicates a physical contamination to cause non-conformance of the item under inspection.

-- Description --
A waiver can be applied when the following conditions are met:
- the usability of the parcel remains intact;
- the deviation from the generic rule stems from the semantic definition of the LPIS;
- the waiver has been created and approved before the inspection starts.

EXAMPLE: A road crosscutting an RP in an LPIS based on topographic blocks or cadastral parcels can be waivered. NB: the area the road shall always be deducted from the reference area.</skos:definition>
    </owl:DatatypeProperty>
    


    <!-- http://lpis.ec.europa.eu/registry/applicationschema/cap-iacs-parcel#weightedArea -->


    <owl:DatatypeProperty rdf:about="http://lpis.ec.europa.eu/registry/applicationschema/cap-iacs-parcel#weightedArea"/>
    


    <!-- http://lpis.ec.europa.eu/registry/applicationschema/cap-iacs-parcel#weightingFactor -->


    <owl:DatatypeProperty rdf:about="http://lpis.ec.europa.eu/registry/applicationschema/cap-iacs-parcel#weightingFactor">
        <rdfs:range rdf:resource="http://www.w3.org/2001/XMLSchema#double"/>
        <rdfs:label xml:lang="en">Weighting factor</rdfs:label>
        <skos:definition xml:lang="en">--Name--
Weighting factor

-- Definition --
Parameter in sense of Art. 43(3) of R (EU) 1307/2013  used for calculating the total hectares represented by the ecological focus area.

-- Description --
Values indicated in the weighting factor column of the table presented in Annex X of R (EU) 639/2014.

NOTE 1
When the weighting of less than 1 is applied, the use of the weighting factors set out in Annex X of Regulation (EU) 639/2014 shall be mandatory.

NOTE 2
Regulation (EU) No 1001/2014 has change the weighting factor for nitrogen fixing crops from 0,3 to 0,7.</skos:definition>
    </owl:DatatypeProperty>
    


    <!-- 
    ///////////////////////////////////////////////////////////////////////////////////////
    //
    // Classes
    //
    ///////////////////////////////////////////////////////////////////////////////////////
     -->


    


    <!-- http://lpis.ec.europa.eu/registry/applicationschema/cap-iacs-aid#CropGroupGreening -->


    <owl:Class rdf:about="http://lpis.ec.europa.eu/registry/applicationschema/cap-iacs-aid#CropGroupGreening"/>
    


    <!-- http://lpis.ec.europa.eu/registry/applicationschema/cap-iacs-aid#EcologicalFocusAreaConverted -->


    <owl:Class rdf:about="http://lpis.ec.europa.eu/registry/applicationschema/cap-iacs-aid#EcologicalFocusAreaConverted"/>
    


    <!-- http://lpis.ec.europa.eu/registry/applicationschema/cap-iacs-parcel#AcceptanceNumberValue -->


    <owl:Class rdf:about="http://lpis.ec.europa.eu/registry/applicationschema/cap-iacs-parcel#AcceptanceNumberValue">
        <owl:equivalentClass>
            <owl:Class>
                <owl:oneOf rdf:parseType="Collection">
                    <rdf:Description rdf:about="http://lpis.ec.europa.eu/registry/applicationschema/cap-iacs-parcel/code#AcceptanceNumberValue/10"/>
                    <rdf:Description rdf:about="http://lpis.ec.europa.eu/registry/applicationschema/cap-iacs-parcel/code#AcceptanceNumberValue/18"/>
                    <rdf:Description rdf:about="http://lpis.ec.europa.eu/registry/applicationschema/cap-iacs-parcel/code#AcceptanceNumberValue/5"/>
                </owl:oneOf>
            </owl:Class>
        </owl:equivalentClass>
        <rdfs:subClassOf rdf:resource="http://www.w3.org/2004/02/skos/core#Concept"/>
        <rdfs:label xml:lang="en">List of possible acceptance values</rdfs:label>
        <skos:definition xml:lang="en">--Name--
Acceptance number value

-- Definition --
List of possible acceptance values.

-- Description --
Acceptance values are selected based on the sample size and the limiting quality values defined in ISO 2859-2:1985 Sampling procedures for inspection by attributes, Part 2: Sampling plans indexed by limiting quality (LQ) for isolated lot inspection.</skos:definition>
    </owl:Class>
    


    <!-- http://lpis.ec.europa.eu/registry/applicationschema/cap-iacs-parcel#AgriculturalArea -->


    <owl:Class rdf:about="http://lpis.ec.europa.eu/registry/applicationschema/cap-iacs-parcel#AgriculturalArea">
        <rdfs:subClassOf rdf:resource="http://www.opengis.net/ont/geosparql#Feature"/>
        <rdfs:subClassOf>
            <owl:Restriction>
                <owl:onProperty rdf:resource="http://lpis.ec.europa.eu/registry/applicationschema/cap-iacs-parcel#agriculturalArea"/>
                <owl:cardinality rdf:datatype="http://www.w3.org/2001/XMLSchema#nonNegativeInteger">1</owl:cardinality>
            </owl:Restriction>
        </rdfs:subClassOf>
        <rdfs:subClassOf>
            <owl:Restriction>
                <owl:onProperty rdf:resource="http://lpis.ec.europa.eu/registry/applicationschema/cap-iacs-parcel#agriculturalAreaType"/>
                <owl:cardinality rdf:datatype="http://www.w3.org/2001/XMLSchema#nonNegativeInteger">1</owl:cardinality>
            </owl:Restriction>
        </rdfs:subClassOf>
        <rdfs:subClassOf>
            <owl:Restriction>
                <owl:onProperty rdf:resource="http://lpis.ec.europa.eu/registry/applicationschema/cap-iacs-parcel#agriculturalAreaWithinReferenceParcel"/>
                <owl:cardinality rdf:datatype="http://www.w3.org/2001/XMLSchema#nonNegativeInteger">1</owl:cardinality>
            </owl:Restriction>
        </rdfs:subClassOf>
        <rdfs:subClassOf>
            <owl:Restriction>
                <owl:onProperty rdf:resource="http://lpis.ec.europa.eu/registry/applicationschema/cap-iacs-parcel#permanentGrasslandProRata"/>
                <owl:maxCardinality rdf:datatype="http://www.w3.org/2001/XMLSchema#nonNegativeInteger">1</owl:maxCardinality>
            </owl:Restriction>
        </rdfs:subClassOf>
        <rdfs:label xml:lang="en">Agricultural area</rdfs:label>
        <skos:definition xml:lang="en">--Name--
Agricultural area

-- Definition --
&quot;Agricultural area&quot; means any area taken up by arable land, permanent grassland and permanent pasture, or permanent crops. Art. 4(1)(e) of R 1307/2013.

-- Description --
Areas taken by these land cover types, or their subtypes (narrower categories) comprising designated landscape features and/or trees included in these areas [DSCG/2014/33].

NOTE 1: The distinction between the different types of agricultural area should be done in two ways depending on the situation:
- By alphanumerical recording of the types and the corresponding area values as attributes of the reference parcel (RP),
- By delineation (assigning geometries to each type within the RP).

NOTE 2: For calculating greening obligations the area of LF shall be accounted as part of the &quot;parent&quot;  land cover type (i.e. LC type where they are embedded in or are adjacent to). In case a designated landscape feature lays at the boundary of two LC types its area shall be subdivided.

NOTE 3: The maximum width of eligible LF  is 2 m, unless the LF has been designated under Art. 9(2) of R (EU) No 640/2014 as subject of cross compliance, or unless the MS notified about eligibility to the Commission before 09/12/2009.  

NOTE 4:  The provisions of Art. 9(1) of Regulation (EU) No 640/2014 cannot apply to permanent grassland with landscape features and trees where the MS has decided to apply Art. 10 of the same Regulation (pro-rata system). 

NOTE 5:  Non agricultural areas (not taken up with the allowed LC types) above 100 sq.m. shall be excluded by delineation.

NOTE 6: It is not necessary to deduct the area of a non agricultural area LC type when it is smaller than 100 sq.m. However, in course of OTSC and LPIS QA,  when the cumulative area (per type) of such smaller features is more than 100 sq.m., the deduction shall be applied.

NOTE 7: Woods (in parcels not declared as short rotation coppice) should be interpreted as areas within an agricultural parcel with tree-cover (including bushes, etc.) preventing growth of vegetative under-storey suitable for grazing and should thus be excluded from the eligible area of the RP [DSCG/2014/33]. 

NOTE 8: MS shall define the maximum tree density to be applied when assessing eligibility together with the characteristics of the trees. Grazable trees on permanent grasslands should not be counted. Groups of threes shall not be spread over the whole area, but shall be excluded if bigger than 100 sq.m..

NOTE 9: Each pro-rata category shall correspond to separate LC type.</skos:definition>
    </owl:Class>
    


    <!-- http://lpis.ec.europa.eu/registry/applicationschema/cap-iacs-parcel#AgriculturalAreaTypeValue -->


    <owl:Class rdf:about="http://lpis.ec.europa.eu/registry/applicationschema/cap-iacs-parcel#AgriculturalAreaTypeValue">
        <rdfs:subClassOf rdf:resource="http://www.w3.org/2004/02/skos/core#Concept"/>
        <rdfs:label xml:lang="en">List of agricultural area type values</rdfs:label>
        <skos:definition xml:lang="en">--Name--
Agricultural area type value

-- Definition --
Types of agricultural area.

-- Description --
List of agricultural area type values.  QAF: Eligibility profile value.

NOTE 1:  According to DSCG/2014/33  arableLand, permanentCrop and permanetGrassland are the minimum level of details of land cover types needed for distinction of agricultural area.

NOTE 2:  sensitivePermanetGrassland type to be protected under greening  is required by Art.5(2)(d) of Regulation (EU) No 640/2014.

NOTE 3: This code list can be extended with narrower categories replacing the listed broader code list values. 

 

NOTE 4: For the purposes of ETS MS/Region may use the same code list applied in IACS, or a generalised one. For the purposes of ETS the generalised code list is sufficient.
When detailed  (crop level) agricultural area types are used, in course of MTS the mapping to the general categories listed in the LCM has to be given.

EXAMPLE: Sensitive permanent grassland may be replaced by any sub-category (narrower value) referred to in Art. 41 of (EU) R 639/2014.</skos:definition>
    </owl:Class>
    


    <!-- http://lpis.ec.europa.eu/registry/applicationschema/cap-iacs-parcel#AgriculturalLand -->


    <owl:Class rdf:about="http://lpis.ec.europa.eu/registry/applicationschema/cap-iacs-parcel#AgriculturalLand">
        <rdfs:subClassOf rdf:resource="http://www.opengis.net/ont/geosparql#Feature"/>
        <rdfs:subClassOf>
            <owl:Restriction>
                <owl:onProperty rdf:resource="http://lpis.ec.europa.eu/registry/applicationschema/cap-iacs-parcel#dataQualityMeasureDocumentation"/>
                <owl:cardinality rdf:datatype="http://www.w3.org/2001/XMLSchema#nonNegativeInteger">1</owl:cardinality>
            </owl:Restriction>
        </rdfs:subClassOf>
        <rdfs:subClassOf>
            <owl:Restriction>
                <owl:onProperty rdf:resource="http://lpis.ec.europa.eu/registry/applicationschema/cap-iacs-parcel#dataQualityMeasureType"/>
                <owl:cardinality rdf:datatype="http://www.w3.org/2001/XMLSchema#nonNegativeInteger">1</owl:cardinality>
            </owl:Restriction>
        </rdfs:subClassOf>
        <rdfs:subClassOf>
            <owl:Restriction>
                <owl:onProperty rdf:resource="http://lpis.ec.europa.eu/registry/applicationschema/cap-iacs-parcel#determinedArea"/>
                <owl:cardinality rdf:datatype="http://www.w3.org/2001/XMLSchema#nonNegativeInteger">1</owl:cardinality>
            </owl:Restriction>
        </rdfs:subClassOf>
        <rdfs:subClassOf>
            <owl:Restriction>
                <owl:onProperty rdf:resource="http://lpis.ec.europa.eu/registry/applicationschema/cap-iacs-parcel#itemAgriculturalLandDetails"/>
                <owl:cardinality rdf:datatype="http://www.w3.org/2001/XMLSchema#nonNegativeInteger">1</owl:cardinality>
            </owl:Restriction>
        </rdfs:subClassOf>
        <rdfs:subClassOf>
            <owl:Restriction>
                <owl:onProperty rdf:resource="http://lpis.ec.europa.eu/registry/applicationschema/cap-iacs-parcel#landCover"/>
                <owl:cardinality rdf:datatype="http://www.w3.org/2001/XMLSchema#nonNegativeInteger">1</owl:cardinality>
            </owl:Restriction>
        </rdfs:subClassOf>
        <rdfs:subClassOf>
            <owl:Restriction>
                <owl:onProperty rdf:resource="http://lpis.ec.europa.eu/registry/applicationschema/cap-iacs-parcel#misclassificationCause"/>
                <owl:cardinality rdf:datatype="http://www.w3.org/2001/XMLSchema#nonNegativeInteger">1</owl:cardinality>
            </owl:Restriction>
        </rdfs:subClassOf>
        <rdfs:subClassOf>
            <owl:Restriction>
                <owl:onProperty rdf:resource="http://lpis.ec.europa.eu/registry/applicationschema/cap-iacs-parcel#geometry"/>
                <owl:maxCardinality rdf:datatype="http://www.w3.org/2001/XMLSchema#nonNegativeInteger">1</owl:maxCardinality>
            </owl:Restriction>
        </rdfs:subClassOf>
        <rdfs:subClassOf>
            <owl:Restriction>
                <owl:onProperty rdf:resource="http://lpis.ec.europa.eu/registry/applicationschema/cap-iacs-parcel#dataQualityMeasureResult"/>
                <owl:cardinality rdf:datatype="http://www.w3.org/2001/XMLSchema#nonNegativeInteger">1</owl:cardinality>
            </owl:Restriction>
        </rdfs:subClassOf>
        <rdfs:label xml:lang="en">Agricultural land</rdfs:label>
        <skos:definition xml:lang="en">--Name--
Agricultural land

-- Definition--
Inventory of agricultural area types within the item of inspection according to the eligibility profile of the MS /region.  

-- Description--
The eligibility profile is based on land cover types defined by the MS / region.</skos:definition>
    </owl:Class>
    


    <!-- http://lpis.ec.europa.eu/registry/applicationschema/cap-iacs-parcel#Contamination -->


    <owl:Class rdf:about="http://lpis.ec.europa.eu/registry/applicationschema/cap-iacs-parcel#Contamination">
        <rdfs:subClassOf rdf:resource="http://www.opengis.net/ont/geosparql#Feature"/>
        <rdfs:subClassOf>
            <owl:Restriction>
                <owl:onProperty rdf:resource="http://lpis.ec.europa.eu/registry/applicationschema/cap-iacs-parcel#contaminationCause"/>
                <owl:cardinality rdf:datatype="http://www.w3.org/2001/XMLSchema#nonNegativeInteger">1</owl:cardinality>
            </owl:Restriction>
        </rdfs:subClassOf>
        <rdfs:subClassOf>
            <owl:Restriction>
                <owl:onProperty rdf:resource="http://lpis.ec.europa.eu/registry/applicationschema/cap-iacs-parcel#contaminationType"/>
                <owl:cardinality rdf:datatype="http://www.w3.org/2001/XMLSchema#nonNegativeInteger">1</owl:cardinality>
            </owl:Restriction>
        </rdfs:subClassOf>
        <rdfs:subClassOf>
            <owl:Restriction>
                <owl:onProperty rdf:resource="http://lpis.ec.europa.eu/registry/applicationschema/cap-iacs-parcel#geometry"/>
                <owl:cardinality rdf:datatype="http://www.w3.org/2001/XMLSchema#nonNegativeInteger">1</owl:cardinality>
            </owl:Restriction>
        </rdfs:subClassOf>
        <rdfs:subClassOf>
            <owl:Restriction>
                <owl:onProperty rdf:resource="http://lpis.ec.europa.eu/registry/applicationschema/cap-iacs-parcel#itemContaminationDetails"/>
                <owl:cardinality rdf:datatype="http://www.w3.org/2001/XMLSchema#nonNegativeInteger">1</owl:cardinality>
            </owl:Restriction>
        </rdfs:subClassOf>
        <rdfs:subClassOf>
            <owl:Restriction>
                <owl:onProperty rdf:resource="http://lpis.ec.europa.eu/registry/applicationschema/cap-iacs-parcel#waivered"/>
                <owl:cardinality rdf:datatype="http://www.w3.org/2001/XMLSchema#nonNegativeInteger">1</owl:cardinality>
            </owl:Restriction>
        </rdfs:subClassOf>
        <rdfs:label xml:lang="en">Contamination</rdfs:label>
        <skos:definition xml:lang="en">--Name--
Contamination

-- Definition --
Unaccounted non-agricultural land cover features partly or totally located inside the item under inspection (Wikicap).

-- Description --
Instances of LC types that are not included in the eligibility profile. The contaminations shall be classified according to the ContaminationTypeValue code list. A contamination indicates that there is an issue with the parcel that should be further assesses (triggers an anomaly and a potential update of the parcel).

NOTE 1. Each contamination shall open an anomaly instance.

NOTE2. Each detected contamination is instantiated as a separate non-conformity from ETS v6.0.

NOTE 3. The concept of contamination is applicable only for those item under inspection that have &quot;true&quot; value of area conformity.</skos:definition>
    </owl:Class>
    


    <!-- http://lpis.ec.europa.eu/registry/applicationschema/cap-iacs-parcel#ContaminationTypeValue -->


    <owl:Class rdf:about="http://lpis.ec.europa.eu/registry/applicationschema/cap-iacs-parcel#ContaminationTypeValue">
        <rdfs:subClassOf rdf:resource="http://www.w3.org/2004/02/skos/core#Concept"/>
        <rdfs:label xml:lang="en">Contamination type value list</rdfs:label>
        <skos:definition xml:lang="en">--Name--
Contamination type value

-- Definition --
List of contamination type values.

-- Description --
NOTE: the code list is centrally managed by the Commission services and cannot be extended by MS/Regions.</skos:definition>
    </owl:Class>
    


    <!-- http://lpis.ec.europa.eu/registry/applicationschema/cap-iacs-parcel#ConversionParameter -->


    <owl:Class rdf:about="http://lpis.ec.europa.eu/registry/applicationschema/cap-iacs-parcel#ConversionParameter">
        <rdfs:subClassOf rdf:resource="http://www.opengis.net/ont/geosparql#Feature"/>
        <rdfs:subClassOf>
            <owl:Restriction>
                <owl:onProperty rdf:resource="http://lpis.ec.europa.eu/registry/applicationschema/cap-iacs-parcel#conversionParameterForDeterminationOfEcologicalFocusArea"/>
                <owl:maxCardinality rdf:datatype="http://www.w3.org/2001/XMLSchema#nonNegativeInteger">1</owl:maxCardinality>
            </owl:Restriction>
        </rdfs:subClassOf>
        <rdfs:subClassOf>
            <owl:Restriction>
                <owl:onProperty rdf:resource="http://lpis.ec.europa.eu/registry/applicationschema/cap-iacs-parcel#unit"/>
                <owl:cardinality rdf:datatype="http://www.w3.org/2001/XMLSchema#nonNegativeInteger">1</owl:cardinality>
            </owl:Restriction>
        </rdfs:subClassOf>
        <rdfs:subClassOf>
            <owl:Restriction>
                <owl:onProperty rdf:resource="http://lpis.ec.europa.eu/registry/applicationschema/cap-iacs-parcel#weightingFactor"/>
                <owl:cardinality rdf:datatype="http://www.w3.org/2001/XMLSchema#nonNegativeInteger">1</owl:cardinality>
            </owl:Restriction>
        </rdfs:subClassOf>
        <rdfs:subClassOf>
            <owl:Restriction>
                <owl:onProperty rdf:resource="http://lpis.ec.europa.eu/registry/applicationschema/cap-iacs-parcel#conversionFactor"/>
                <owl:maxCardinality rdf:datatype="http://www.w3.org/2001/XMLSchema#nonNegativeInteger">1</owl:maxCardinality>
            </owl:Restriction>
        </rdfs:subClassOf>
        <rdfs:label xml:lang="en">Conversion parameters for ecological focus area</rdfs:label>
        <skos:definition xml:lang="en">--Name--
Conversion parameter

-- Definition --
Conversion and weighting factors  for calculating EFA  area referred to in Art 46(3) of (EU) R No 1307/2013.

-- Description --
Conversion factors needed for calculating the converted area of EFA based on spatial representation with reduced dimensions (point, curve) and the weighting factor expressing the ecological weight of EFA.</skos:definition>
    </owl:Class>
    


    <!-- http://lpis.ec.europa.eu/registry/applicationschema/cap-iacs-parcel#CriticalDefect -->


    <owl:Class rdf:about="http://lpis.ec.europa.eu/registry/applicationschema/cap-iacs-parcel#CriticalDefect">
        <rdfs:subClassOf rdf:resource="http://www.opengis.net/ont/geosparql#Feature"/>
        <rdfs:subClassOf>
            <owl:Restriction>
                <owl:onProperty rdf:resource="http://lpis.ec.europa.eu/registry/applicationschema/cap-iacs-parcel#criticalDefectCause"/>
                <owl:cardinality rdf:datatype="http://www.w3.org/2001/XMLSchema#nonNegativeInteger">1</owl:cardinality>
            </owl:Restriction>
        </rdfs:subClassOf>
        <rdfs:subClassOf>
            <owl:Restriction>
                <owl:onProperty rdf:resource="http://lpis.ec.europa.eu/registry/applicationschema/cap-iacs-parcel#criticalDefectType"/>
                <owl:cardinality rdf:datatype="http://www.w3.org/2001/XMLSchema#nonNegativeInteger">1</owl:cardinality>
            </owl:Restriction>
        </rdfs:subClassOf>
        <rdfs:subClassOf>
            <owl:Restriction>
                <owl:onProperty rdf:resource="http://lpis.ec.europa.eu/registry/applicationschema/cap-iacs-parcel#itemCriticalDefectDetails"/>
                <owl:cardinality rdf:datatype="http://www.w3.org/2001/XMLSchema#nonNegativeInteger">1</owl:cardinality>
            </owl:Restriction>
        </rdfs:subClassOf>
        <rdfs:subClassOf>
            <owl:Restriction>
                <owl:onProperty rdf:resource="http://lpis.ec.europa.eu/registry/applicationschema/cap-iacs-parcel#geometry"/>
                <owl:maxCardinality rdf:datatype="http://www.w3.org/2001/XMLSchema#nonNegativeInteger">1</owl:maxCardinality>
            </owl:Restriction>
        </rdfs:subClassOf>
        <rdfs:label xml:lang="en">Critical defect</rdfs:label>
        <skos:definition xml:lang="en">--Name--
Critical defect

-- Definition --
Critical defect is a non-conformance  that obstructs the use of the item under inspection regarding the unambiguous localization of agricultural parcels, or the unique identification for cross-checks (Wikicap).

-- Description --
The usability of the RP can be obstructed by misclassification of the LC (no agricultural land present in the RP), by violating the design (semantic definition) if the LPIS or by processing errors within LPIS.</skos:definition>
    </owl:Class>
    


    <!-- http://lpis.ec.europa.eu/registry/applicationschema/cap-iacs-parcel#CriticalDefectEfa -->


    <owl:Class rdf:about="http://lpis.ec.europa.eu/registry/applicationschema/cap-iacs-parcel#CriticalDefectEfa">
        <rdfs:subClassOf rdf:resource="http://www.opengis.net/ont/geosparql#Feature"/>
        <rdfs:subClassOf>
            <owl:Restriction>
                <owl:onProperty rdf:resource="http://lpis.ec.europa.eu/registry/applicationschema/cap-iacs-parcel#criticalDefectType"/>
                <owl:cardinality rdf:datatype="http://www.w3.org/2001/XMLSchema#nonNegativeInteger">1</owl:cardinality>
            </owl:Restriction>
        </rdfs:subClassOf>
        <rdfs:subClassOf>
            <owl:Restriction>
                <owl:onProperty rdf:resource="http://lpis.ec.europa.eu/registry/applicationschema/cap-iacs-parcel#itemUnderInspectionEfaCriticalDefectDetails"/>
                <owl:cardinality rdf:datatype="http://www.w3.org/2001/XMLSchema#nonNegativeInteger">1</owl:cardinality>
            </owl:Restriction>
        </rdfs:subClassOf>
        <rdfs:subClassOf>
            <owl:Restriction>
                <owl:onProperty rdf:resource="http://lpis.ec.europa.eu/registry/applicationschema/cap-iacs-parcel#criticalDefectCause"/>
                <owl:maxCardinality rdf:datatype="http://www.w3.org/2001/XMLSchema#nonNegativeInteger">1</owl:maxCardinality>
            </owl:Restriction>
        </rdfs:subClassOf>
        <rdfs:subClassOf>
            <owl:Restriction>
                <owl:onProperty rdf:resource="http://lpis.ec.europa.eu/registry/applicationschema/cap-iacs-parcel#geometry"/>
                <owl:maxCardinality rdf:datatype="http://www.w3.org/2001/XMLSchema#nonNegativeInteger">1</owl:maxCardinality>
            </owl:Restriction>
        </rdfs:subClassOf>
        <rdfs:label xml:lang="en">Critical defect</rdfs:label>
        <skos:definition xml:lang="en">--Name--
Critical defect of EFA

-- Definition --
This is a placeholder only; currently not to be implemented.

-- Description --
EFA critical defect.</skos:definition>
    </owl:Class>
    


    <!-- http://lpis.ec.europa.eu/registry/applicationschema/cap-iacs-parcel#CriticalDefectTypeEfaValue -->


    <owl:Class rdf:about="http://lpis.ec.europa.eu/registry/applicationschema/cap-iacs-parcel#CriticalDefectTypeEfaValue">
        <rdfs:subClassOf rdf:resource="http://www.w3.org/2004/02/skos/core#Concept"/>
        <rdfs:label xml:lang="en">Critical defect type value</rdfs:label>
        <skos:definition xml:lang="en">--Name--
EFA critical defect type

-- Definition --
This is a placeholder only; currently not to be implemented.

-- Description --
List of error types leading to obstruction of usability of the item under inspection (critical defect).</skos:definition>
    </owl:Class>
    


    <!-- http://lpis.ec.europa.eu/registry/applicationschema/cap-iacs-parcel#CriticalDefectTypeValue -->


    <owl:Class rdf:about="http://lpis.ec.europa.eu/registry/applicationschema/cap-iacs-parcel#CriticalDefectTypeValue">
        <rdfs:subClassOf rdf:resource="http://www.w3.org/2004/02/skos/core#Concept"/>
        <rdfs:label xml:lang="en">Critical defect type value</rdfs:label>
        <skos:definition xml:lang="en">--Name--
Critical defect type value

-- Definition --
List of critical defect type values.

-- Description --
List of error types leading to obstruction of usability of the item under inspection (critical defect).</skos:definition>
    </owl:Class>
    


    <!-- http://lpis.ec.europa.eu/registry/applicationschema/cap-iacs-parcel#DataQualityMeasure -->


    <owl:Class rdf:about="http://lpis.ec.europa.eu/registry/applicationschema/cap-iacs-parcel#DataQualityMeasure">
        <rdfs:subClassOf>
            <owl:Restriction>
                <owl:onProperty rdf:resource="http://lpis.ec.europa.eu/registry/applicationschema/cap-iacs-parcel#measureIdentifier"/>
                <owl:cardinality rdf:datatype="http://www.w3.org/2001/XMLSchema#nonNegativeInteger">1</owl:cardinality>
            </owl:Restriction>
        </rdfs:subClassOf>
        <rdfs:subClassOf>
            <owl:Restriction>
                <owl:onProperty rdf:resource="http://lpis.ec.europa.eu/registry/applicationschema/cap-iacs-parcel#description"/>
                <owl:maxCardinality rdf:datatype="http://www.w3.org/2001/XMLSchema#nonNegativeInteger">1</owl:maxCardinality>
            </owl:Restriction>
        </rdfs:subClassOf>
        <rdfs:subClassOf>
            <owl:Restriction>
                <owl:onProperty rdf:resource="http://lpis.ec.europa.eu/registry/applicationschema/cap-iacs-parcel#valueStructure"/>
                <owl:maxCardinality rdf:datatype="http://www.w3.org/2001/XMLSchema#nonNegativeInteger">1</owl:maxCardinality>
            </owl:Restriction>
        </rdfs:subClassOf>
        <rdfs:subClassOf>
            <owl:Restriction>
                <owl:onProperty rdf:resource="http://lpis.ec.europa.eu/registry/applicationschema/cap-iacs-parcel#elementName"/>
                <owl:minCardinality rdf:datatype="http://www.w3.org/2001/XMLSchema#nonNegativeInteger">1</owl:minCardinality>
            </owl:Restriction>
        </rdfs:subClassOf>
        <rdfs:subClassOf>
            <owl:Restriction>
                <owl:onProperty rdf:resource="http://lpis.ec.europa.eu/registry/applicationschema/cap-iacs-parcel#definition"/>
                <owl:cardinality rdf:datatype="http://www.w3.org/2001/XMLSchema#nonNegativeInteger">1</owl:cardinality>
            </owl:Restriction>
        </rdfs:subClassOf>
        <rdfs:subClassOf>
            <owl:Restriction>
                <owl:onProperty rdf:resource="http://lpis.ec.europa.eu/registry/applicationschema/cap-iacs-parcel#name"/>
                <owl:cardinality rdf:datatype="http://www.w3.org/2001/XMLSchema#nonNegativeInteger">1</owl:cardinality>
            </owl:Restriction>
        </rdfs:subClassOf>
        <rdfs:subClassOf>
            <owl:Restriction>
                <owl:onProperty rdf:resource="http://lpis.ec.europa.eu/registry/applicationschema/cap-iacs-parcel#valueType"/>
                <owl:cardinality rdf:datatype="http://www.w3.org/2001/XMLSchema#nonNegativeInteger">1</owl:cardinality>
            </owl:Restriction>
        </rdfs:subClassOf>
        <rdfs:label xml:lang="en">LPIS QAF DQM measure</rdfs:label>
        <skos:definition xml:lang="en">--Name--
Data quality measure

--Definition --
Data quality measure is a descriptor of a data quality element used for evaluating data quality.

--Description --
In LPISQA specific data quality measures are used that are defined on the basis of data quality elements of ISO 19157:2013. The data quality measures are listed in the following code lists:
- DataQualityMeasureTypeIuiValue (for items under inspection)
- DataQualityMeasureTypeDTSValue (for LPIS as a whole)</skos:definition>
    </owl:Class>
    


    <!-- http://lpis.ec.europa.eu/registry/applicationschema/cap-iacs-parcel#DataQualityMeasureDescription -->


    <owl:Class rdf:about="http://lpis.ec.europa.eu/registry/applicationschema/cap-iacs-parcel#DataQualityMeasureDescription">
        <rdfs:subClassOf>
            <owl:Restriction>
                <owl:onProperty rdf:resource="http://lpis.ec.europa.eu/registry/applicationschema/cap-iacs-parcel#extendedDescription"/>
                <owl:maxCardinality rdf:datatype="http://www.w3.org/2001/XMLSchema#nonNegativeInteger">1</owl:maxCardinality>
            </owl:Restriction>
        </rdfs:subClassOf>
        <rdfs:subClassOf>
            <owl:Restriction>
                <owl:onProperty rdf:resource="http://lpis.ec.europa.eu/registry/applicationschema/cap-iacs-parcel#textDescription"/>
                <owl:cardinality rdf:datatype="http://www.w3.org/2001/XMLSchema#nonNegativeInteger">1</owl:cardinality>
            </owl:Restriction>
        </rdfs:subClassOf>
        <rdfs:label xml:lang="en">LPIS QAF DQM description</rdfs:label>
        <skos:definition xml:lang="en">--Name--
Data quality measure description

--Definition--
Narrative description of the data quality measure.

--Description--
This element is part of the LPISQA conceptual model provided by the Commission Services. In case a MS/Region opts for using other quality assessment system, the description of DQM shall be given in the eligibility profile. Otherwise it can be omitted.</skos:definition>
    </owl:Class>
    


    <!-- http://lpis.ec.europa.eu/registry/applicationschema/cap-iacs-parcel#DataQualityMeasureNameValue -->


    <owl:Class rdf:about="http://lpis.ec.europa.eu/registry/applicationschema/cap-iacs-parcel#DataQualityMeasureNameValue">
        <rdfs:subClassOf rdf:resource="http://www.w3.org/2004/02/skos/core#Concept"/>
        <rdfs:label xml:lang="en">ETS data quality measure name list</rdfs:label>
        <skos:definition xml:lang="en">--Name--
Data quality measure name value

-- Definition --
Data quality measures applicable for LPIS quality assessment process.

-- Description --
This is the unified code list of all DQM applied at item and sample level.</skos:definition>
    </owl:Class>
    


    <!-- http://lpis.ec.europa.eu/registry/applicationschema/cap-iacs-parcel#DataQualityMeasureTypeEfaValue -->


    <owl:Class rdf:about="http://lpis.ec.europa.eu/registry/applicationschema/cap-iacs-parcel#DataQualityMeasureTypeEfaValue">
        <rdfs:subClassOf rdf:resource="http://www.w3.org/2004/02/skos/core#Concept"/>
        <rdfs:label xml:lang="en">EFA data quality measure type list</rdfs:label>
        <skos:definition xml:lang="en">--Name--
Data quality measure types applicable to the EFA inspection sample

-- Definition --
This is a placeholder only; currently not to be implemented.

-- Description --
Data quality measure type list for EFA sample. 
NOTE. Full description of each value must be provided in DQM_Measure.</skos:definition>
    </owl:Class>
    


    <!-- http://lpis.ec.europa.eu/registry/applicationschema/cap-iacs-parcel#DataQualityMeasureTypeEtsValue -->


    <owl:Class rdf:about="http://lpis.ec.europa.eu/registry/applicationschema/cap-iacs-parcel#DataQualityMeasureTypeEtsValue">
        <rdfs:subClassOf rdf:resource="http://www.w3.org/2004/02/skos/core#Concept"/>
        <rdfs:label xml:lang="en">DTS data quality measure type list</rdfs:label>
        <skos:definition xml:lang="en">--Name--
Data quality measure types applicable for ETS sample

-- Definition --
Data quality measures applicable for LPIS quality assessment process at sample level.

--Description--
By exclusion of misclassification  matrix the elements of the code list are user defined data quality measures to assess quality of the ETS sample. Misclassification matrix comes directly from ISO 19157:2013.</skos:definition>
    </owl:Class>
    


    <!-- http://lpis.ec.europa.eu/registry/applicationschema/cap-iacs-parcel#DataQualityMeasureTypeIuiCcValue -->


    <owl:Class rdf:about="http://lpis.ec.europa.eu/registry/applicationschema/cap-iacs-parcel#DataQualityMeasureTypeIuiCcValue">
        <rdfs:subClassOf rdf:resource="http://www.w3.org/2004/02/skos/core#Concept"/>
        <rdfs:label xml:lang="en">IUI CC data quality measure type list</rdfs:label>
        <skos:definition xml:lang="en">--Name--
Classification Correctness DQM value

-- Definition --
Data quality measure describing the correctness of classification of the feature type.

-- Description --
The classification shall be performed according to the types defined in the eligibility profile. This DQM is applicable for evaluating the classification correctness of agricultural land(s) and the landscape feature(s) present in the item under inspection.  

NOTE: This is a new quality measure from ETS v 6.0 on.</skos:definition>
    </owl:Class>
    


    <!-- http://lpis.ec.europa.eu/registry/applicationschema/cap-iacs-parcel#DataQualityMeasureTypeIuiEfaValue -->


    <owl:Class rdf:about="http://lpis.ec.europa.eu/registry/applicationschema/cap-iacs-parcel#DataQualityMeasureTypeIuiEfaValue">
        <rdfs:subClassOf rdf:resource="http://www.w3.org/2004/02/skos/core#Concept"/>
        <rdfs:label xml:lang="en">IUI EFA data quality measure type list</rdfs:label>
        <skos:definition xml:lang="en">--Name--
Data quality measure types applicable to EFA items

-- Definition --
This is a placeholder only; currently not to be implemented.

-- Description --
Data quality measure type list for items under inspection.
NOTE. Full description of each value must be provided in DQM_Measure.</skos:definition>
    </owl:Class>
    


    <!-- http://lpis.ec.europa.eu/registry/applicationschema/cap-iacs-parcel#DataQualityMeasureTypeIuiValue -->


    <owl:Class rdf:about="http://lpis.ec.europa.eu/registry/applicationschema/cap-iacs-parcel#DataQualityMeasureTypeIuiValue">
        <rdfs:subClassOf rdf:resource="http://www.w3.org/2004/02/skos/core#Concept"/>
        <rdfs:label xml:lang="en">IUI data quality measure type list</rdfs:label>
        <skos:definition xml:lang="en">--Name--
Data quality measure types applicable to items under inspection

-- Definition --
List of data quality measure types applicable for inspecting items of reference parcels.

-- Description --
These user defined data quality measures are used to assess the quality of reference parcels in terms of area measurement accuracy and thematic classification correctness.</skos:definition>
    </owl:Class>
    


    <!-- http://lpis.ec.europa.eu/registry/applicationschema/cap-iacs-parcel#DataQualityMeasureValueStructureValue -->


    <owl:Class rdf:about="http://lpis.ec.europa.eu/registry/applicationschema/cap-iacs-parcel#DataQualityMeasureValueStructureValue">
        <rdfs:subClassOf rdf:resource="http://www.w3.org/2004/02/skos/core#Concept"/>
        <rdfs:label xml:lang="en">Data quality measure value structure value list</rdfs:label>
        <skos:definition xml:lang="en">--Name--
Data quality Measure value structure

--Definition--
Structure used for presenting multiple values of DQ results.

--Description--
A result may consist of multiple values. In such cases, the result shall be structured using the value structure as given in C.3.3 of ISO 19157:2013. 

EXAMPLE: The results for misclassification shall be given as a matrix.</skos:definition>
    </owl:Class>
    


    <!-- http://lpis.ec.europa.eu/registry/applicationschema/cap-iacs-parcel#EcologicalFocusArea -->


    <owl:Class rdf:about="http://lpis.ec.europa.eu/registry/applicationschema/cap-iacs-parcel#EcologicalFocusArea">
        <rdfs:subClassOf rdf:resource="http://www.opengis.net/ont/geosparql#Feature"/>
        <rdfs:subClassOf>
            <owl:Restriction>
                <owl:onProperty rdf:resource="http://lpis.ec.europa.eu/registry/applicationschema/cap-iacs-parcel#ecologicalFocusArea"/>
                <owl:cardinality rdf:datatype="http://www.w3.org/2001/XMLSchema#nonNegativeInteger">1</owl:cardinality>
            </owl:Restriction>
        </rdfs:subClassOf>
        <rdfs:subClassOf>
            <owl:Restriction>
                <owl:onProperty rdf:resource="http://lpis.ec.europa.eu/registry/applicationschema/cap-iacs-parcel#ecologicalFocusAreaType"/>
                <owl:cardinality rdf:datatype="http://www.w3.org/2001/XMLSchema#nonNegativeInteger">1</owl:cardinality>
            </owl:Restriction>
        </rdfs:subClassOf>
        <rdfs:subClassOf>
            <owl:Restriction>
                <owl:onProperty rdf:resource="http://lpis.ec.europa.eu/registry/applicationschema/cap-iacs-parcel#geometry"/>
                <owl:cardinality rdf:datatype="http://www.w3.org/2001/XMLSchema#nonNegativeInteger">1</owl:cardinality>
            </owl:Restriction>
        </rdfs:subClassOf>
        <rdfs:subClassOf>
            <owl:Restriction>
                <owl:onProperty rdf:resource="http://lpis.ec.europa.eu/registry/applicationschema/cap-iacs-parcel#detailsOfselectedEfaForInspection"/>
                <owl:maxCardinality rdf:datatype="http://www.w3.org/2001/XMLSchema#nonNegativeInteger">1</owl:maxCardinality>
            </owl:Restriction>
        </rdfs:subClassOf>
        <rdfs:subClassOf>
            <owl:Restriction>
                <owl:onProperty rdf:resource="http://lpis.ec.europa.eu/registry/applicationschema/cap-iacs-parcel#ecologicalFocusAreaWithinCropGroupGreening"/>
                <owl:maxCardinality rdf:datatype="http://www.w3.org/2001/XMLSchema#nonNegativeInteger">1</owl:maxCardinality>
            </owl:Restriction>
        </rdfs:subClassOf>
        <rdfs:subClassOf>
            <owl:Restriction>
                <owl:onProperty rdf:resource="http://lpis.ec.europa.eu/registry/applicationschema/cap-iacs-parcel#subjectToCollectiveImplementation"/>
                <owl:cardinality rdf:datatype="http://www.w3.org/2001/XMLSchema#nonNegativeInteger">1</owl:cardinality>
            </owl:Restriction>
        </rdfs:subClassOf>
        <rdfs:label xml:lang="en">Ecological focus area</rdfs:label>
        <skos:definition xml:lang="en">--Name--
Ecological Focus Area

-- Definition --
Ecological focus areas as referred to in Article 46 of R (EU) No1307/2013 and its Delegated Regulation (EU) No 639/2014.

-- Description --
Areas contributing to practices beneficial for the climate and the environment as referred to in Art. 43(2)(c) of (EU) R No 1307/2013.

NOTE 1: This is the feature type that allows the creation of the EFA layer in sense of Art. 70(2) of (EU) R 1306/2013. 

NOTE 2: All instances of potential EFA that remain in place at least for 3 years shall be included [DSCG/2014/31]..

NOTE 3: „Potentiality“ means implies that any EFA situated on holdings of farmers who are exempted (small farmers, organic farming) are is also subject of data collection (mapping) [DSCG/2014/31].

NOTE 4: When an EFA instance (without altering the geometry ) that has been declared for three consecutive year with geospatial application, it should be regarded as permanent, thus within the scope of LPIS.

NOTE 5: EFA instances established under equivalent agri-environmental-climate measures (AECM) are expected to last at least 5 years, therefore they should be regarded to be in scope of LPIS [DSCG/2014/31].</skos:definition>
    </owl:Class>
    


    <!-- http://lpis.ec.europa.eu/registry/applicationschema/cap-iacs-parcel#EcologicalFocusAreaEquivalentPracticeTypeValue -->


    <owl:Class rdf:about="http://lpis.ec.europa.eu/registry/applicationschema/cap-iacs-parcel#EcologicalFocusAreaEquivalentPracticeTypeValue">
        <rdfs:subClassOf rdf:resource="http://www.w3.org/2004/02/skos/core#Concept"/>
        <rdfs:label xml:lang="en">List of EFA equivalent practices</rdfs:label>
        <skos:definition xml:lang="en">--Name--
EFA equivalent practice type

-- Definition --
Equivalent practices with EFAs which are listed  in print III of Annex IX of Regulation (EU) No 1307/2013.

-- Description --
The specific AECM reason has to be linked to the EFA type.</skos:definition>
    </owl:Class>
    


    <!-- http://lpis.ec.europa.eu/registry/applicationschema/cap-iacs-parcel#EcologicalFocusAreaRegion -->


    <owl:Class rdf:about="http://lpis.ec.europa.eu/registry/applicationschema/cap-iacs-parcel#EcologicalFocusAreaRegion">
        <rdfs:subClassOf rdf:resource="http://www.opengis.net/ont/geosparql#Feature"/>
        <rdfs:subClassOf>
            <owl:Restriction>
                <owl:onProperty rdf:resource="http://lpis.ec.europa.eu/registry/applicationschema/cap-iacs-parcel#ecologicalFocusAreaRegionDetailsForMandatedArea"/>
                <owl:minCardinality rdf:datatype="http://www.w3.org/2001/XMLSchema#nonNegativeInteger">1</owl:minCardinality>
            </owl:Restriction>
        </rdfs:subClassOf>
        <rdfs:subClassOf>
            <owl:Restriction>
                <owl:onProperty rdf:resource="http://lpis.ec.europa.eu/registry/applicationschema/cap-iacs-parcel#ecologicalFocusAreasAggregationDetails"/>
                <owl:minCardinality rdf:datatype="http://www.w3.org/2001/XMLSchema#nonNegativeInteger">1</owl:minCardinality>
            </owl:Restriction>
        </rdfs:subClassOf>
        <rdfs:subClassOf>
            <owl:Restriction>
                <owl:onProperty rdf:resource="http://lpis.ec.europa.eu/registry/applicationschema/cap-iacs-parcel#homogeneityType"/>
                <owl:cardinality rdf:datatype="http://www.w3.org/2001/XMLSchema#nonNegativeInteger">1</owl:cardinality>
            </owl:Restriction>
        </rdfs:subClassOf>
        <rdfs:subClassOf>
            <owl:Restriction>
                <owl:onProperty rdf:resource="http://lpis.ec.europa.eu/registry/applicationschema/cap-iacs-parcel#metadata"/>
                <owl:cardinality rdf:datatype="http://www.w3.org/2001/XMLSchema#nonNegativeInteger">1</owl:cardinality>
            </owl:Restriction>
        </rdfs:subClassOf>
        <rdfs:subClassOf>
            <owl:Restriction>
                <owl:onProperty rdf:resource="http://lpis.ec.europa.eu/registry/applicationschema/cap-iacs-parcel#geometry"/>
                <owl:maxCardinality rdf:datatype="http://www.w3.org/2001/XMLSchema#nonNegativeInteger">1</owl:maxCardinality>
            </owl:Restriction>
        </rdfs:subClassOf>
        <rdfs:subClassOf>
            <owl:Restriction>
                <owl:onProperty rdf:resource="http://lpis.ec.europa.eu/registry/applicationschema/cap-iacs-parcel#homogeneityTypeCitation"/>
                <owl:maxCardinality rdf:datatype="http://www.w3.org/2001/XMLSchema#nonNegativeInteger">1</owl:maxCardinality>
            </owl:Restriction>
        </rdfs:subClassOf>
        <rdfs:subClassOf>
            <owl:Restriction>
                <owl:onProperty rdf:resource="http://lpis.ec.europa.eu/registry/applicationschema/cap-iacs-parcel#homogeneityTypeDocument"/>
                <owl:maxCardinality rdf:datatype="http://www.w3.org/2001/XMLSchema#nonNegativeInteger">1</owl:maxCardinality>
            </owl:Restriction>
        </rdfs:subClassOf>
        <rdfs:subClassOf>
            <owl:Restriction>
                <owl:onProperty rdf:resource="http://lpis.ec.europa.eu/registry/applicationschema/cap-iacs-parcel#ecologicalFocusAreaRegionId"/>
                <owl:cardinality rdf:datatype="http://www.w3.org/2001/XMLSchema#nonNegativeInteger">1</owl:cardinality>
            </owl:Restriction>
        </rdfs:subClassOf>
        <rdfs:label xml:lang="en">Region of ecological focus area</rdfs:label>
        <skos:definition xml:lang="en">--Name--
EFA region

-- Definition --
Regions for regional EFA implementation as referred to in Art. 46(5) of (EU) R No 1307/2013.

-- Description --
Member States may decide to implement up to half of the percentage points of EFA at regional level in order to obtain adjacent ecological focus areas. The regions to be defined shall consist of single and homogenous geographical areas with similar agricultural and environmental conditions. Ecological focus areas must be contiguous for regional implementation (and must be subject to collective implementation).

NOTE
Member States may decide to implement up to half of the percentage points of the ecological focus area referred to in paragraph 1 at regional level in order to obtain adjacent ecological focus areas.</skos:definition>
    </owl:Class>
    


    <!-- http://lpis.ec.europa.eu/registry/applicationschema/cap-iacs-parcel#EcologicalFocusAreaRegionMandatedArea -->


    <owl:Class rdf:about="http://lpis.ec.europa.eu/registry/applicationschema/cap-iacs-parcel#EcologicalFocusAreaRegionMandatedArea">
        <rdfs:subClassOf rdf:resource="http://www.opengis.net/ont/geosparql#Feature"/>
        <rdfs:subClassOf>
            <owl:Restriction>
                <owl:onProperty rdf:resource="http://lpis.ec.europa.eu/registry/applicationschema/cap-iacs-parcel#mandatedAreaWithinRegion"/>
                <owl:cardinality rdf:datatype="http://www.w3.org/2001/XMLSchema#nonNegativeInteger">1</owl:cardinality>
            </owl:Restriction>
        </rdfs:subClassOf>
        <rdfs:subClassOf>
            <owl:Restriction>
                <owl:onProperty rdf:resource="http://lpis.ec.europa.eu/registry/applicationschema/cap-iacs-parcel#geometry"/>
                <owl:maxCardinality rdf:datatype="http://www.w3.org/2001/XMLSchema#nonNegativeInteger">1</owl:maxCardinality>
            </owl:Restriction>
        </rdfs:subClassOf>
        <rdfs:subClassOf>
            <owl:Restriction>
                <owl:onProperty rdf:resource="http://lpis.ec.europa.eu/registry/applicationschema/cap-iacs-parcel#mandatedAreaId"/>
                <owl:cardinality rdf:datatype="http://www.w3.org/2001/XMLSchema#nonNegativeInteger">1</owl:cardinality>
            </owl:Restriction>
        </rdfs:subClassOf>
        <rdfs:subClassOf>
            <owl:Restriction>
                <owl:onProperty rdf:resource="http://lpis.ec.europa.eu/registry/applicationschema/cap-iacs-parcel#percentage"/>
                <owl:cardinality rdf:datatype="http://www.w3.org/2001/XMLSchema#nonNegativeInteger">1</owl:cardinality>
            </owl:Restriction>
        </rdfs:subClassOf>
        <rdfs:label xml:lang="en">Mandated areas within region of ecological focus area</rdfs:label>
        <skos:definition xml:lang="en">--Name--
EFA region mandated area

-- Definition --
Mandated areas within regions of ecological focus area as referred to in Art. 46(5) and 46(6) of (EU) R 1307/2013.

-- Description --
MS shall designate the areas and the obligations of participating farmers or groups of farmers.

NOTE:  The aim of the designation of areas and obligations shall be to underpin the implementation of Union policies on the environment, climate biodiversity, river basin management, and Natura 2000 network [Art. 47(2) of (EU) R No 639/2014] .</skos:definition>
    </owl:Class>
    


    <!-- http://lpis.ec.europa.eu/registry/applicationschema/cap-iacs-parcel#EcologicalFocusAreaTypeValue -->


    <owl:Class rdf:about="http://lpis.ec.europa.eu/registry/applicationschema/cap-iacs-parcel#EcologicalFocusAreaTypeValue">
        <rdfs:subClassOf rdf:resource="http://www.w3.org/2004/02/skos/core#Concept"/>
        <rdfs:label xml:lang="en">List of ecological focuse areas</rdfs:label>
        <skos:definition xml:lang="en">--Name--
Ecological focus area type value

-- Definition --
Types of EFA as listed in Art. 46(2) of (EU) R 1307/2013.

-- Description --
MS shall decide that one or more values of this code list  are considered to be ecological focus area.

NOTE 1: Member States may decide to limit the selection of landscape features to those under GAEC 7, SMR 2 or SMR 3  as referred to in Annex II to Regulation (EU) No 640/2013 and/or to one or more of those listed in point (a) to (h) of the first subparagraph, where duly justified. Should it be the case, the code list of EFA types have to be modifie accordingly.

NOTE 2: The extension of this code list shall be documented in the eligibility profile of the MS/region. It is recommended to use  a register / registry service to publish the extended values and their definitions.

NOTE 3: Landscape features shall be:
-at the disposal of the farmer;
-shall be those that are protected under GAEC 7, SMR 2 or SMR 3 as referred to in Annex II to Regulation (EU) No 640/2014.</skos:definition>
    </owl:Class>
    


    <!-- http://lpis.ec.europa.eu/registry/applicationschema/cap-iacs-parcel#EfaItemUnderInspection -->


    <owl:Class rdf:about="http://lpis.ec.europa.eu/registry/applicationschema/cap-iacs-parcel#EfaItemUnderInspection">
        <rdfs:subClassOf rdf:resource="http://www.opengis.net/ont/geosparql#Feature"/>
        <rdfs:subClassOf>
            <owl:Restriction>
                <owl:onProperty rdf:resource="http://lpis.ec.europa.eu/registry/applicationschema/cap-iacs-parcel#dataQualityMeasureDocumentation"/>
                <owl:minCardinality rdf:datatype="http://www.w3.org/2001/XMLSchema#nonNegativeInteger">1</owl:minCardinality>
            </owl:Restriction>
        </rdfs:subClassOf>
        <rdfs:subClassOf>
            <owl:Restriction>
                <owl:onProperty rdf:resource="http://lpis.ec.europa.eu/registry/applicationschema/cap-iacs-parcel#dataQualityMeasureType"/>
                <owl:minCardinality rdf:datatype="http://www.w3.org/2001/XMLSchema#nonNegativeInteger">1</owl:minCardinality>
            </owl:Restriction>
        </rdfs:subClassOf>
        <rdfs:subClassOf>
            <owl:Restriction>
                <owl:onProperty rdf:resource="http://lpis.ec.europa.eu/registry/applicationschema/cap-iacs-parcel#determinedArea"/>
                <owl:cardinality rdf:datatype="http://www.w3.org/2001/XMLSchema#nonNegativeInteger">1</owl:cardinality>
            </owl:Restriction>
        </rdfs:subClassOf>
        <rdfs:subClassOf>
            <owl:Restriction>
                <owl:onProperty rdf:resource="http://lpis.ec.europa.eu/registry/applicationschema/cap-iacs-parcel#efaItemUnderInspectionWithinEfaSampleDetails"/>
                <owl:cardinality rdf:datatype="http://www.w3.org/2001/XMLSchema#nonNegativeInteger">1</owl:cardinality>
            </owl:Restriction>
        </rdfs:subClassOf>
        <rdfs:subClassOf>
            <owl:Restriction>
                <owl:onProperty rdf:resource="http://lpis.ec.europa.eu/registry/applicationschema/cap-iacs-parcel#observedEfaType"/>
                <owl:cardinality rdf:datatype="http://www.w3.org/2001/XMLSchema#nonNegativeInteger">1</owl:cardinality>
            </owl:Restriction>
        </rdfs:subClassOf>
        <rdfs:subClassOf>
            <owl:Restriction>
                <owl:onProperty rdf:resource="http://lpis.ec.europa.eu/registry/applicationschema/cap-iacs-parcel#recordedArea"/>
                <owl:cardinality rdf:datatype="http://www.w3.org/2001/XMLSchema#nonNegativeInteger">1</owl:cardinality>
            </owl:Restriction>
        </rdfs:subClassOf>
        <rdfs:subClassOf>
            <owl:Restriction>
                <owl:onProperty rdf:resource="http://lpis.ec.europa.eu/registry/applicationschema/cap-iacs-parcel#recordedEfaType"/>
                <owl:cardinality rdf:datatype="http://www.w3.org/2001/XMLSchema#nonNegativeInteger">1</owl:cardinality>
            </owl:Restriction>
        </rdfs:subClassOf>
        <rdfs:subClassOf>
            <owl:Restriction>
                <owl:onProperty rdf:resource="http://lpis.ec.europa.eu/registry/applicationschema/cap-iacs-parcel#convertedArea"/>
                <owl:maxCardinality rdf:datatype="http://www.w3.org/2001/XMLSchema#nonNegativeInteger">1</owl:maxCardinality>
            </owl:Restriction>
        </rdfs:subClassOf>
        <rdfs:subClassOf>
            <owl:Restriction>
                <owl:onProperty rdf:resource="http://lpis.ec.europa.eu/registry/applicationschema/cap-iacs-parcel#efaMissclassificationCause"/>
                <owl:maxCardinality rdf:datatype="http://www.w3.org/2001/XMLSchema#nonNegativeInteger">1</owl:maxCardinality>
            </owl:Restriction>
        </rdfs:subClassOf>
        <rdfs:subClassOf>
            <owl:Restriction>
                <owl:onProperty rdf:resource="http://lpis.ec.europa.eu/registry/applicationschema/cap-iacs-parcel#weightedArea"/>
                <owl:maxCardinality rdf:datatype="http://www.w3.org/2001/XMLSchema#nonNegativeInteger">1</owl:maxCardinality>
            </owl:Restriction>
        </rdfs:subClassOf>
        <rdfs:subClassOf>
            <owl:Restriction>
                <owl:onProperty rdf:resource="http://lpis.ec.europa.eu/registry/applicationschema/cap-iacs-parcel#dataQualityMeasureResult"/>
                <owl:minCardinality rdf:datatype="http://www.w3.org/2001/XMLSchema#nonNegativeInteger">1</owl:minCardinality>
            </owl:Restriction>
        </rdfs:subClassOf>
        <rdfs:label xml:lang="en">Preselected EFA</rdfs:label>
        <skos:definition xml:lang="en">--Name--
EFA item under inspection

-- Definition --
This is a placeholder only; currently not to be implemented.

-- Description --
Visible land  in the imagery or in the field that is supposed to represent the sampled EFA.</skos:definition>
    </owl:Class>
    


    <!-- http://lpis.ec.europa.eu/registry/applicationschema/cap-iacs-parcel#EfaSample -->


    <owl:Class rdf:about="http://lpis.ec.europa.eu/registry/applicationschema/cap-iacs-parcel#EfaSample">
        <rdfs:subClassOf rdf:resource="http://www.opengis.net/ont/geosparql#Feature"/>
        <rdfs:subClassOf>
            <owl:Restriction>
                <owl:onProperty rdf:resource="http://lpis.ec.europa.eu/registry/applicationschema/cap-iacs-parcel#dataQualityMeasureDescription"/>
                <owl:minCardinality rdf:datatype="http://www.w3.org/2001/XMLSchema#nonNegativeInteger">1</owl:minCardinality>
            </owl:Restriction>
        </rdfs:subClassOf>
        <rdfs:subClassOf>
            <owl:Restriction>
                <owl:onProperty rdf:resource="http://lpis.ec.europa.eu/registry/applicationschema/cap-iacs-parcel#dataQualityMeasureType"/>
                <owl:minCardinality rdf:datatype="http://www.w3.org/2001/XMLSchema#nonNegativeInteger">1</owl:minCardinality>
            </owl:Restriction>
        </rdfs:subClassOf>
        <rdfs:subClassOf>
            <owl:Restriction>
                <owl:onProperty rdf:resource="http://lpis.ec.europa.eu/registry/applicationschema/cap-iacs-parcel#efaSampleDetailsForItemsUnderInspectionEfa"/>
                <owl:minCardinality rdf:datatype="http://www.w3.org/2001/XMLSchema#nonNegativeInteger">1</owl:minCardinality>
            </owl:Restriction>
        </rdfs:subClassOf>
        <rdfs:subClassOf>
            <owl:Restriction>
                <owl:onProperty rdf:resource="http://lpis.ec.europa.eu/registry/applicationschema/cap-iacs-parcel#efaReport"/>
                <owl:cardinality rdf:datatype="http://www.w3.org/2001/XMLSchema#nonNegativeInteger">1</owl:cardinality>
            </owl:Restriction>
        </rdfs:subClassOf>
        <rdfs:subClassOf>
            <owl:Restriction>
                <owl:onProperty rdf:resource="http://lpis.ec.europa.eu/registry/applicationschema/cap-iacs-parcel#efaSampleDetailsForLpisLot"/>
                <owl:cardinality rdf:datatype="http://www.w3.org/2001/XMLSchema#nonNegativeInteger">1</owl:cardinality>
            </owl:Restriction>
        </rdfs:subClassOf>
        <rdfs:subClassOf>
            <owl:Restriction>
                <owl:onProperty rdf:resource="http://lpis.ec.europa.eu/registry/applicationschema/cap-iacs-parcel#efaRemedialActionPlan"/>
                <owl:maxCardinality rdf:datatype="http://www.w3.org/2001/XMLSchema#nonNegativeInteger">1</owl:maxCardinality>
            </owl:Restriction>
        </rdfs:subClassOf>
        <rdfs:subClassOf>
            <owl:Restriction>
                <owl:onProperty rdf:resource="http://lpis.ec.europa.eu/registry/applicationschema/cap-iacs-parcel#dataQualityMeasureResult"/>
                <owl:minCardinality rdf:datatype="http://www.w3.org/2001/XMLSchema#nonNegativeInteger">1</owl:minCardinality>
            </owl:Restriction>
        </rdfs:subClassOf>
        <rdfs:subClassOf>
            <owl:Restriction>
                <owl:onProperty rdf:resource="http://lpis.ec.europa.eu/registry/applicationschema/cap-iacs-parcel#numberOfInspectedEfa"/>
                <owl:cardinality rdf:datatype="http://www.w3.org/2001/XMLSchema#nonNegativeInteger">1</owl:cardinality>
            </owl:Restriction>
        </rdfs:subClassOf>
        <rdfs:label xml:lang="en">EFA sample</rdfs:label>
        <skos:definition xml:lang="en">--Name--
EFA sample

-- Definition --
This is a placeholder only; currently not to be implemented.

Set of randomly selected EFA with ordered sequence.</skos:definition>
    </owl:Class>
    


    <!-- http://lpis.ec.europa.eu/registry/applicationschema/cap-iacs-parcel#EtsItemUnderInspection -->


    <owl:Class rdf:about="http://lpis.ec.europa.eu/registry/applicationschema/cap-iacs-parcel#EtsItemUnderInspection">
        <rdfs:subClassOf rdf:resource="http://www.opengis.net/ont/geosparql#Feature"/>
        <rdfs:subClassOf>
            <owl:Restriction>
                <owl:onProperty rdf:resource="http://lpis.ec.europa.eu/registry/applicationschema/cap-iacs-parcel#dataQualityMeasureDocumentation"/>
                <owl:minCardinality rdf:datatype="http://www.w3.org/2001/XMLSchema#nonNegativeInteger">1</owl:minCardinality>
            </owl:Restriction>
        </rdfs:subClassOf>
        <rdfs:subClassOf>
            <owl:Restriction>
                <owl:onProperty rdf:resource="http://lpis.ec.europa.eu/registry/applicationschema/cap-iacs-parcel#dataQualityMeasureType"/>
                <owl:minCardinality rdf:datatype="http://www.w3.org/2001/XMLSchema#nonNegativeInteger">1</owl:minCardinality>
            </owl:Restriction>
        </rdfs:subClassOf>
        <rdfs:subClassOf>
            <owl:Restriction>
                <owl:onProperty rdf:resource="http://lpis.ec.europa.eu/registry/applicationschema/cap-iacs-parcel#declaredArea"/>
                <owl:cardinality rdf:datatype="http://www.w3.org/2001/XMLSchema#nonNegativeInteger">1</owl:cardinality>
            </owl:Restriction>
        </rdfs:subClassOf>
        <rdfs:subClassOf>
            <owl:Restriction>
                <owl:onProperty rdf:resource="http://lpis.ec.europa.eu/registry/applicationschema/cap-iacs-parcel#etsItemUnderInspectionWithinEtsSampleDetails"/>
                <owl:cardinality rdf:datatype="http://www.w3.org/2001/XMLSchema#nonNegativeInteger">1</owl:cardinality>
            </owl:Restriction>
        </rdfs:subClassOf>
        <rdfs:subClassOf>
            <owl:Restriction>
                <owl:onProperty rdf:resource="http://lpis.ec.europa.eu/registry/applicationschema/cap-iacs-parcel#observedArea"/>
                <owl:cardinality rdf:datatype="http://www.w3.org/2001/XMLSchema#nonNegativeInteger">1</owl:cardinality>
            </owl:Restriction>
        </rdfs:subClassOf>
        <rdfs:subClassOf>
            <owl:Restriction>
                <owl:onProperty rdf:resource="http://lpis.ec.europa.eu/registry/applicationschema/cap-iacs-parcel#referenceArea"/>
                <owl:cardinality rdf:datatype="http://www.w3.org/2001/XMLSchema#nonNegativeInteger">1</owl:cardinality>
            </owl:Restriction>
        </rdfs:subClassOf>
        <rdfs:subClassOf>
            <owl:Restriction>
                <owl:onProperty rdf:resource="http://lpis.ec.europa.eu/registry/applicationschema/cap-iacs-parcel#areaNonConformanceCause"/>
                <owl:maxCardinality rdf:datatype="http://www.w3.org/2001/XMLSchema#nonNegativeInteger">1</owl:maxCardinality>
            </owl:Restriction>
        </rdfs:subClassOf>
        <rdfs:subClassOf>
            <owl:Restriction>
                <owl:onProperty rdf:resource="http://lpis.ec.europa.eu/registry/applicationschema/cap-iacs-parcel#dataQualityMeasureResult"/>
                <owl:minCardinality rdf:datatype="http://www.w3.org/2001/XMLSchema#nonNegativeInteger">1</owl:minCardinality>
            </owl:Restriction>
        </rdfs:subClassOf>
        <rdfs:subClassOf>
            <owl:Restriction>
                <owl:onProperty rdf:resource="http://lpis.ec.europa.eu/registry/applicationschema/cap-iacs-parcel#feasibilityForMeasurement"/>
                <owl:cardinality rdf:datatype="http://www.w3.org/2001/XMLSchema#nonNegativeInteger">1</owl:cardinality>
            </owl:Restriction>
        </rdfs:subClassOf>
        <rdfs:label xml:lang="en">Item under inspection</rdfs:label>
        <skos:definition xml:lang="en">--Name--
ETS item under inspection

-- Definition--
Reference parcel or, where applicable, aggregation of reference parcels sampled for LPIS quality assessment process.

-- Description --
The attributes of the instances of this feature type (except the reference parcel ID and the declared area) are defined in course of direct observations and measurements carried out according to the specifications of the given LPIS. The procedures to be followed are described in the Perform ETS use case of the LPIS dynamic model. The inspection methodology is based on observing the land cover types present in the RP.

NOTE: Previously this  concept was called as land under inspection (LUI).  According to ISO 2859-2 &quot;item&quot; is the standard  term used for subjects of inspection. This approach also allows to extend the QA methodology for other objects (e.g. EFA elements).</skos:definition>
    </owl:Class>
    


    <!-- http://lpis.ec.europa.eu/registry/applicationschema/cap-iacs-parcel#EtsSample -->


    <owl:Class rdf:about="http://lpis.ec.europa.eu/registry/applicationschema/cap-iacs-parcel#EtsSample">
        <rdfs:subClassOf rdf:resource="http://www.opengis.net/ont/geosparql#Feature"/>
        <rdfs:subClassOf>
            <owl:Restriction>
                <owl:onProperty rdf:resource="http://lpis.ec.europa.eu/registry/applicationschema/cap-iacs-parcel#dataQualityMeasureDocumentation"/>
                <owl:minCardinality rdf:datatype="http://www.w3.org/2001/XMLSchema#nonNegativeInteger">1</owl:minCardinality>
            </owl:Restriction>
        </rdfs:subClassOf>
        <rdfs:subClassOf>
            <owl:Restriction>
                <owl:onProperty rdf:resource="http://lpis.ec.europa.eu/registry/applicationschema/cap-iacs-parcel#dataQualityMeasureType"/>
                <owl:minCardinality rdf:datatype="http://www.w3.org/2001/XMLSchema#nonNegativeInteger">1</owl:minCardinality>
            </owl:Restriction>
        </rdfs:subClassOf>
        <rdfs:subClassOf>
            <owl:Restriction>
                <owl:onProperty rdf:resource="http://lpis.ec.europa.eu/registry/applicationschema/cap-iacs-parcel#etsSampleDetailsForEtsItemsUnderInspection"/>
                <owl:minCardinality rdf:datatype="http://www.w3.org/2001/XMLSchema#nonNegativeInteger">1</owl:minCardinality>
            </owl:Restriction>
        </rdfs:subClassOf>
        <rdfs:subClassOf>
            <owl:Restriction>
                <owl:onProperty rdf:resource="http://lpis.ec.europa.eu/registry/applicationschema/cap-iacs-parcel#conformingItemsArea"/>
                <owl:cardinality rdf:datatype="http://www.w3.org/2001/XMLSchema#nonNegativeInteger">1</owl:cardinality>
            </owl:Restriction>
        </rdfs:subClassOf>
        <rdfs:subClassOf>
            <owl:Restriction>
                <owl:onProperty rdf:resource="http://lpis.ec.europa.eu/registry/applicationschema/cap-iacs-parcel#etsReport"/>
                <owl:cardinality rdf:datatype="http://www.w3.org/2001/XMLSchema#nonNegativeInteger">1</owl:cardinality>
            </owl:Restriction>
        </rdfs:subClassOf>
        <rdfs:subClassOf>
            <owl:Restriction>
                <owl:onProperty rdf:resource="http://lpis.ec.europa.eu/registry/applicationschema/cap-iacs-parcel#etsSampleDetailsForLpisLot"/>
                <owl:cardinality rdf:datatype="http://www.w3.org/2001/XMLSchema#nonNegativeInteger">1</owl:cardinality>
            </owl:Restriction>
        </rdfs:subClassOf>
        <rdfs:subClassOf>
            <owl:Restriction>
                <owl:onProperty rdf:resource="http://lpis.ec.europa.eu/registry/applicationschema/cap-iacs-parcel#totalDeclaredArea"/>
                <owl:cardinality rdf:datatype="http://www.w3.org/2001/XMLSchema#nonNegativeInteger">1</owl:cardinality>
            </owl:Restriction>
        </rdfs:subClassOf>
        <rdfs:subClassOf>
            <owl:Restriction>
                <owl:onProperty rdf:resource="http://lpis.ec.europa.eu/registry/applicationschema/cap-iacs-parcel#totalDeclaredAreaMeasuredItems"/>
                <owl:cardinality rdf:datatype="http://www.w3.org/2001/XMLSchema#nonNegativeInteger">1</owl:cardinality>
            </owl:Restriction>
        </rdfs:subClassOf>
        <rdfs:subClassOf>
            <owl:Restriction>
                <owl:onProperty rdf:resource="http://lpis.ec.europa.eu/registry/applicationschema/cap-iacs-parcel#totalOverestimatedArea"/>
                <owl:cardinality rdf:datatype="http://www.w3.org/2001/XMLSchema#nonNegativeInteger">1</owl:cardinality>
            </owl:Restriction>
        </rdfs:subClassOf>
        <rdfs:subClassOf>
            <owl:Restriction>
                <owl:onProperty rdf:resource="http://lpis.ec.europa.eu/registry/applicationschema/cap-iacs-parcel#totalReferenceArea"/>
                <owl:cardinality rdf:datatype="http://www.w3.org/2001/XMLSchema#nonNegativeInteger">1</owl:cardinality>
            </owl:Restriction>
        </rdfs:subClassOf>
        <rdfs:subClassOf>
            <owl:Restriction>
                <owl:onProperty rdf:resource="http://lpis.ec.europa.eu/registry/applicationschema/cap-iacs-parcel#totalReferenceAreaMeasuredItems"/>
                <owl:cardinality rdf:datatype="http://www.w3.org/2001/XMLSchema#nonNegativeInteger">1</owl:cardinality>
            </owl:Restriction>
        </rdfs:subClassOf>
        <rdfs:subClassOf>
            <owl:Restriction>
                <owl:onProperty rdf:resource="http://lpis.ec.europa.eu/registry/applicationschema/cap-iacs-parcel#totalUnderestimatedArea"/>
                <owl:cardinality rdf:datatype="http://www.w3.org/2001/XMLSchema#nonNegativeInteger">1</owl:cardinality>
            </owl:Restriction>
        </rdfs:subClassOf>
        <rdfs:subClassOf>
            <owl:Restriction>
                <owl:onProperty rdf:resource="http://lpis.ec.europa.eu/registry/applicationschema/cap-iacs-parcel#lpisRemedialActionPlan"/>
                <owl:maxCardinality rdf:datatype="http://www.w3.org/2001/XMLSchema#nonNegativeInteger">1</owl:maxCardinality>
            </owl:Restriction>
        </rdfs:subClassOf>
        <rdfs:subClassOf>
            <owl:Restriction>
                <owl:onProperty rdf:resource="http://lpis.ec.europa.eu/registry/applicationschema/cap-iacs-parcel#dataQualityMeasureResult"/>
                <owl:minCardinality rdf:datatype="http://www.w3.org/2001/XMLSchema#nonNegativeInteger">1</owl:minCardinality>
            </owl:Restriction>
        </rdfs:subClassOf>
        <rdfs:subClassOf>
            <owl:Restriction>
                <owl:onProperty rdf:resource="http://lpis.ec.europa.eu/registry/applicationschema/cap-iacs-parcel#declaredToRecordedArea"/>
                <owl:cardinality rdf:datatype="http://www.w3.org/2001/XMLSchema#nonNegativeInteger">1</owl:cardinality>
            </owl:Restriction>
        </rdfs:subClassOf>
        <rdfs:subClassOf>
            <owl:Restriction>
                <owl:onProperty rdf:resource="http://lpis.ec.europa.eu/registry/applicationschema/cap-iacs-parcel#declaredToRecordedAreaMeasuredItems"/>
                <owl:cardinality rdf:datatype="http://www.w3.org/2001/XMLSchema#nonNegativeInteger">1</owl:cardinality>
            </owl:Restriction>
        </rdfs:subClassOf>
        <rdfs:subClassOf>
            <owl:Restriction>
                <owl:onProperty rdf:resource="http://lpis.ec.europa.eu/registry/applicationschema/cap-iacs-parcel#numberOfIncompatibleDesign"/>
                <owl:cardinality rdf:datatype="http://www.w3.org/2001/XMLSchema#nonNegativeInteger">1</owl:cardinality>
            </owl:Restriction>
        </rdfs:subClassOf>
        <rdfs:subClassOf>
            <owl:Restriction>
                <owl:onProperty rdf:resource="http://lpis.ec.europa.eu/registry/applicationschema/cap-iacs-parcel#numberOfIncompleteProcessing"/>
                <owl:cardinality rdf:datatype="http://www.w3.org/2001/XMLSchema#nonNegativeInteger">1</owl:cardinality>
            </owl:Restriction>
        </rdfs:subClassOf>
        <rdfs:subClassOf>
            <owl:Restriction>
                <owl:onProperty rdf:resource="http://lpis.ec.europa.eu/registry/applicationschema/cap-iacs-parcel#numberOfInspectedItems"/>
                <owl:cardinality rdf:datatype="http://www.w3.org/2001/XMLSchema#nonNegativeInteger">1</owl:cardinality>
            </owl:Restriction>
        </rdfs:subClassOf>
        <rdfs:subClassOf>
            <owl:Restriction>
                <owl:onProperty rdf:resource="http://lpis.ec.europa.eu/registry/applicationschema/cap-iacs-parcel#numberOfLargeMeasuredItems"/>
                <owl:cardinality rdf:datatype="http://www.w3.org/2001/XMLSchema#nonNegativeInteger">1</owl:cardinality>
            </owl:Restriction>
        </rdfs:subClassOf>
        <rdfs:subClassOf>
            <owl:Restriction>
                <owl:onProperty rdf:resource="http://lpis.ec.europa.eu/registry/applicationschema/cap-iacs-parcel#numberOfMeasuredItems"/>
                <owl:cardinality rdf:datatype="http://www.w3.org/2001/XMLSchema#nonNegativeInteger">1</owl:cardinality>
            </owl:Restriction>
        </rdfs:subClassOf>
        <rdfs:subClassOf>
            <owl:Restriction>
                <owl:onProperty rdf:resource="http://lpis.ec.europa.eu/registry/applicationschema/cap-iacs-parcel#numberOfMissedUpdates"/>
                <owl:cardinality rdf:datatype="http://www.w3.org/2001/XMLSchema#nonNegativeInteger">1</owl:cardinality>
            </owl:Restriction>
        </rdfs:subClassOf>
        <rdfs:subClassOf>
            <owl:Restriction>
                <owl:onProperty rdf:resource="http://lpis.ec.europa.eu/registry/applicationschema/cap-iacs-parcel#numberOfMissedUpgrades"/>
                <owl:cardinality rdf:datatype="http://www.w3.org/2001/XMLSchema#nonNegativeInteger">1</owl:cardinality>
            </owl:Restriction>
        </rdfs:subClassOf>
        <rdfs:subClassOf>
            <owl:Restriction>
                <owl:onProperty rdf:resource="http://lpis.ec.europa.eu/registry/applicationschema/cap-iacs-parcel#numberOfProcessingErrors"/>
                <owl:cardinality rdf:datatype="http://www.w3.org/2001/XMLSchema#nonNegativeInteger">1</owl:cardinality>
            </owl:Restriction>
        </rdfs:subClassOf>
        <rdfs:subClassOf>
            <owl:Restriction>
                <owl:onProperty rdf:resource="http://lpis.ec.europa.eu/registry/applicationschema/cap-iacs-parcel#oversamplingParameter"/>
                <owl:cardinality rdf:datatype="http://www.w3.org/2001/XMLSchema#nonNegativeInteger">2</owl:cardinality>
            </owl:Restriction>
        </rdfs:subClassOf>
        <rdfs:label xml:lang="en">ETS sample</rdfs:label>
        <skos:definition xml:lang="en">--Name--
ETS sample

-- Definition --
Set of randomly selected parcel with ordered sequence.

-- Description --
The inspection process follows the sequential order prescribed by DG JRC.</skos:definition>
    </owl:Class>
    


    <!-- http://lpis.ec.europa.eu/registry/applicationschema/cap-iacs-parcel#HomogeneityTypeValue -->


    <owl:Class rdf:about="http://lpis.ec.europa.eu/registry/applicationschema/cap-iacs-parcel#HomogeneityTypeValue">
        <rdfs:subClassOf rdf:resource="http://www.w3.org/2004/02/skos/core#Concept"/>
        <rdfs:label xml:lang="en">List of homogeneity type</rdfs:label>
        <skos:definition xml:lang="en">--Name--
Homogeneity type value

-- Definition --
Code list of homogeneity types for single and homogenous geographical areas with similar agricultural and environmental conditions as referred to Art. 46(1) of (EU) R 639/2014.

-- Description --
It is a code list managed by the Commission Services, therefore is not extensible by the MS/regions.</skos:definition>
    </owl:Class>
    


    <!-- http://lpis.ec.europa.eu/registry/applicationschema/cap-iacs-parcel#InspectionMethodValue -->


    <owl:Class rdf:about="http://lpis.ec.europa.eu/registry/applicationschema/cap-iacs-parcel#InspectionMethodValue">
        <rdfs:subClassOf rdf:resource="http://www.w3.org/2004/02/skos/core#Concept"/>
        <rdfs:label xml:lang="en">List of inspection methods</rdfs:label>
        <skos:definition xml:lang="en">--Name--
Inspection method  value

-- Definition --
Data collection methods applicable for LPISQA.

-- Description --
MS/Regions shall chose on of the following methods:
- field survey,
- computer assisted photo interpretation (CAPI)
- combined CAPI and field measurements.</skos:definition>
    </owl:Class>
    


    <!-- http://lpis.ec.europa.eu/registry/applicationschema/cap-iacs-parcel#LandscapeFeature -->


    <owl:Class rdf:about="http://lpis.ec.europa.eu/registry/applicationschema/cap-iacs-parcel#LandscapeFeature">
        <rdfs:subClassOf rdf:resource="http://www.opengis.net/ont/geosparql#Feature"/>
        <rdfs:subClassOf>
            <owl:Restriction>
                <owl:onProperty rdf:resource="http://lpis.ec.europa.eu/registry/applicationschema/cap-iacs-parcel#landscapeFeatureDetailsForCrossCompliance"/>
                <owl:cardinality rdf:datatype="http://www.w3.org/2001/XMLSchema#nonNegativeInteger">1</owl:cardinality>
            </owl:Restriction>
        </rdfs:subClassOf>
        <rdfs:subClassOf>
            <owl:Restriction>
                <owl:onProperty rdf:resource="http://lpis.ec.europa.eu/registry/applicationschema/cap-iacs-parcel#landscapeFeatureType"/>
                <owl:cardinality rdf:datatype="http://www.w3.org/2001/XMLSchema#nonNegativeInteger">1</owl:cardinality>
            </owl:Restriction>
        </rdfs:subClassOf>
        <rdfs:subClassOf>
            <owl:Restriction>
                <owl:onProperty rdf:resource="http://lpis.ec.europa.eu/registry/applicationschema/cap-iacs-parcel#geometry"/>
                <owl:maxCardinality rdf:datatype="http://www.w3.org/2001/XMLSchema#nonNegativeInteger">1</owl:maxCardinality>
            </owl:Restriction>
        </rdfs:subClassOf>
        <rdfs:subClassOf>
            <owl:Restriction>
                <owl:onProperty rdf:resource="http://lpis.ec.europa.eu/registry/applicationschema/cap-iacs-parcel#landscapeFeatureArea"/>
                <owl:maxCardinality rdf:datatype="http://www.w3.org/2001/XMLSchema#nonNegativeInteger">1</owl:maxCardinality>
            </owl:Restriction>
        </rdfs:subClassOf>
        <rdfs:subClassOf>
            <owl:Restriction>
                <owl:onProperty rdf:resource="http://lpis.ec.europa.eu/registry/applicationschema/cap-iacs-parcel#landscapeFeatureForEcologicalFocusArea"/>
                <owl:maxCardinality rdf:datatype="http://www.w3.org/2001/XMLSchema#nonNegativeInteger">1</owl:maxCardinality>
            </owl:Restriction>
        </rdfs:subClassOf>
        <rdfs:label xml:lang="en">Landscape feature</rdfs:label>
        <skos:definition xml:lang="en">--Name--
Landscape feature

-- Definition--
Elements of the agricultural area that are traditionally part of good agriculture cropping or utilization practices [Regulation (EU) 640/2014 Art. 9(1)].

-- Description --
Any landscape feature subject to the requirements and standards listed in Annex II to Regulation (EU) No 1306/2013 which forms part of the total area of an agricultural parcel shall be considered part of the eligible area.</skos:definition>
    </owl:Class>
    


    <!-- http://lpis.ec.europa.eu/registry/applicationschema/cap-iacs-parcel#LandscapeFeatureUnderInspection -->


    <owl:Class rdf:about="http://lpis.ec.europa.eu/registry/applicationschema/cap-iacs-parcel#LandscapeFeatureUnderInspection">
        <rdfs:subClassOf rdf:resource="http://www.opengis.net/ont/geosparql#Feature"/>
        <rdfs:subClassOf>
            <owl:Restriction>
                <owl:onProperty rdf:resource="http://lpis.ec.europa.eu/registry/applicationschema/cap-iacs-parcel#dataQualityMeasureDocumentation"/>
                <owl:cardinality rdf:datatype="http://www.w3.org/2001/XMLSchema#nonNegativeInteger">1</owl:cardinality>
            </owl:Restriction>
        </rdfs:subClassOf>
        <rdfs:subClassOf>
            <owl:Restriction>
                <owl:onProperty rdf:resource="http://lpis.ec.europa.eu/registry/applicationschema/cap-iacs-parcel#dataQualityMeasureType"/>
                <owl:cardinality rdf:datatype="http://www.w3.org/2001/XMLSchema#nonNegativeInteger">1</owl:cardinality>
            </owl:Restriction>
        </rdfs:subClassOf>
        <rdfs:subClassOf>
            <owl:Restriction>
                <owl:onProperty rdf:resource="http://lpis.ec.europa.eu/registry/applicationschema/cap-iacs-parcel#landscapeFeatureSelectionDetails"/>
                <owl:cardinality rdf:datatype="http://www.w3.org/2001/XMLSchema#nonNegativeInteger">1</owl:cardinality>
            </owl:Restriction>
        </rdfs:subClassOf>
        <rdfs:subClassOf>
            <owl:Restriction>
                <owl:onProperty rdf:resource="http://lpis.ec.europa.eu/registry/applicationschema/cap-iacs-parcel#landscapeFeatureType"/>
                <owl:cardinality rdf:datatype="http://www.w3.org/2001/XMLSchema#nonNegativeInteger">1</owl:cardinality>
            </owl:Restriction>
        </rdfs:subClassOf>
        <rdfs:subClassOf>
            <owl:Restriction>
                <owl:onProperty rdf:resource="http://lpis.ec.europa.eu/registry/applicationschema/cap-iacs-parcel#misclasificationCause"/>
                <owl:cardinality rdf:datatype="http://www.w3.org/2001/XMLSchema#nonNegativeInteger">1</owl:cardinality>
            </owl:Restriction>
        </rdfs:subClassOf>
        <rdfs:subClassOf>
            <owl:Restriction>
                <owl:onProperty rdf:resource="http://lpis.ec.europa.eu/registry/applicationschema/cap-iacs-parcel#landscapeFeatureAsEfaItemUnderInspectionDetails"/>
                <owl:maxCardinality rdf:datatype="http://www.w3.org/2001/XMLSchema#nonNegativeInteger">1</owl:maxCardinality>
            </owl:Restriction>
        </rdfs:subClassOf>
        <rdfs:subClassOf>
            <owl:Restriction>
                <owl:onProperty rdf:resource="http://lpis.ec.europa.eu/registry/applicationschema/cap-iacs-parcel#dataQualityMeasureResult"/>
                <owl:cardinality rdf:datatype="http://www.w3.org/2001/XMLSchema#nonNegativeInteger">1</owl:cardinality>
            </owl:Restriction>
        </rdfs:subClassOf>
        <rdfs:label xml:lang="en">Landscape feature under inspection</rdfs:label>
        <skos:definition xml:lang="en">--Name--
Landscape feature under inspection

-- Description --
Elements of the agricultural area that are traditionally part of good agriculture cropping or utilization practices (EU 640/2014 Art. 9(1)).

-- Description --
The applicable LF types (if any) shall be taken from the eligibility profile of the MS/Region.</skos:definition>
    </owl:Class>
    


    <!-- http://lpis.ec.europa.eu/registry/applicationschema/cap-iacs-parcel#LandscapeFeatureValueType -->


    <owl:Class rdf:about="http://lpis.ec.europa.eu/registry/applicationschema/cap-iacs-parcel#LandscapeFeatureValueType">
        <rdfs:subClassOf rdf:resource="http://www.w3.org/2004/02/skos/core#Concept"/>
        <rdfs:label xml:lang="en">List of landscape features</rdfs:label>
        <skos:definition xml:lang="en">--Name--
Landscape feature value type

-- Definition --
Types of landscape features.

-- Description --
MS shall decide that one or more values of this code list  are considered to be landscape feature. The code list can be extended.</skos:definition>
    </owl:Class>
    


    <!-- http://lpis.ec.europa.eu/registry/applicationschema/cap-iacs-parcel#LimitingQualityParameter -->


    <owl:Class rdf:about="http://lpis.ec.europa.eu/registry/applicationschema/cap-iacs-parcel#LimitingQualityParameter">
        <rdfs:subClassOf>
            <owl:Restriction>
                <owl:onProperty rdf:resource="http://lpis.ec.europa.eu/registry/applicationschema/cap-iacs-parcel#acceptanceNumber"/>
                <owl:cardinality rdf:datatype="http://www.w3.org/2001/XMLSchema#nonNegativeInteger">1</owl:cardinality>
            </owl:Restriction>
        </rdfs:subClassOf>
        <rdfs:subClassOf>
            <owl:Restriction>
                <owl:onProperty rdf:resource="http://lpis.ec.europa.eu/registry/applicationschema/cap-iacs-parcel#limitingQuality"/>
                <owl:cardinality rdf:datatype="http://www.w3.org/2001/XMLSchema#nonNegativeInteger">1</owl:cardinality>
            </owl:Restriction>
        </rdfs:subClassOf>
        <rdfs:subClassOf>
            <owl:Restriction>
                <owl:onProperty rdf:resource="http://lpis.ec.europa.eu/registry/applicationschema/cap-iacs-parcel#lotSize"/>
                <owl:cardinality rdf:datatype="http://www.w3.org/2001/XMLSchema#nonNegativeInteger">1</owl:cardinality>
            </owl:Restriction>
        </rdfs:subClassOf>
        <rdfs:subClassOf>
            <owl:Restriction>
                <owl:onProperty rdf:resource="http://lpis.ec.europa.eu/registry/applicationschema/cap-iacs-parcel#sampleSize"/>
                <owl:cardinality rdf:datatype="http://www.w3.org/2001/XMLSchema#nonNegativeInteger">1</owl:cardinality>
            </owl:Restriction>
        </rdfs:subClassOf>
        <rdfs:label xml:lang="en">Sampling schema parameter table</rdfs:label>
        <skos:definition xml:lang="en">--Name--
Limiting quality parameter

-- Definition --
Limiting quality parameter as defined in the sampling schema parameter table of ISO 2859-2.

-- Description --
Applicable set  of values must be selected  by MS/Region based on the population size of their LPIS from ISO 2859-2:1985 (Sampling procedures for inspection by attributes, Part 2: Sampling plans indexed by limiting quality (LQ) for isolated lot inspection).</skos:definition>
    </owl:Class>
    


    <!-- http://lpis.ec.europa.eu/registry/applicationschema/cap-iacs-parcel#LimitingQualityValue -->


    <owl:Class rdf:about="http://lpis.ec.europa.eu/registry/applicationschema/cap-iacs-parcel#LimitingQualityValue">
        <owl:equivalentClass>
            <owl:Class>
                <owl:oneOf rdf:parseType="Collection">
                    <rdf:Description rdf:about="http://lpis.ec.europa.eu/registry/applicationschema/cap-iacs-parcel/code#LimitingQualityValue/12.50"/>
                    <rdf:Description rdf:about="http://lpis.ec.europa.eu/registry/applicationschema/cap-iacs-parcel/code#LimitingQualityValue/2.00"/>
                </owl:oneOf>
            </owl:Class>
        </owl:equivalentClass>
        <rdfs:subClassOf rdf:resource="http://www.w3.org/2004/02/skos/core#Concept"/>
        <rdfs:label xml:lang="en">List of possible limiting quality values</rdfs:label>
        <skos:definition xml:lang="en">--Name--
Limiting quality value

-- Definition --
List of limiting quality values applicable in LPISQA.

-- Description --
Limiting quality values are defined by ISO 2859-2:1985.</skos:definition>
    </owl:Class>
    


    <!-- http://lpis.ec.europa.eu/registry/applicationschema/cap-iacs-parcel#LotSizeValue -->


    <owl:Class rdf:about="http://lpis.ec.europa.eu/registry/applicationschema/cap-iacs-parcel#LotSizeValue">
        <owl:equivalentClass>
            <owl:Class>
                <owl:oneOf rdf:parseType="Collection">
                    <rdf:Description rdf:about="http://lpis.ec.europa.eu/registry/applicationschema/cap-iacs-parcel/code#LotSizeValue/150001to500000"/>
                    <rdf:Description rdf:about="http://lpis.ec.europa.eu/registry/applicationschema/cap-iacs-parcel/code#LotSizeValue/35001to150000"/>
                    <rdf:Description rdf:about="http://lpis.ec.europa.eu/registry/applicationschema/cap-iacs-parcel/code#LotSizeValue/500000+"/>
                </owl:oneOf>
            </owl:Class>
        </owl:equivalentClass>
        <rdfs:subClassOf rdf:resource="http://www.w3.org/2004/02/skos/core#Concept"/>
        <rdfs:label xml:lang="en">List of possible lot size range values</rdfs:label>
        <skos:definition xml:lang="en">--Name--
Lot size value

-- Definition --
List of possible lot size range values. according to ISO 2859-2:1985.

-- Description --
The ranges are defined in ISO 2859-2:1985 Sampling procedures for inspection by attributes, Part 2: Sampling plans indexed by limiting quality (LQ) for isolated lot inspection.</skos:definition>
    </owl:Class>
    


    <!-- http://lpis.ec.europa.eu/registry/applicationschema/cap-iacs-parcel#LpisLot -->


    <owl:Class rdf:about="http://lpis.ec.europa.eu/registry/applicationschema/cap-iacs-parcel#LpisLot">
        <rdfs:subClassOf rdf:resource="http://www.opengis.net/ont/geosparql#Feature"/>
        <rdfs:subClassOf>
            <owl:Restriction>
                <owl:onProperty rdf:resource="http://lpis.ec.europa.eu/registry/applicationschema/cap-iacs-parcel#referenceParcelWithinTheLotDetails"/>
                <owl:minCardinality rdf:datatype="http://www.w3.org/2001/XMLSchema#nonNegativeInteger">1</owl:minCardinality>
            </owl:Restriction>
        </rdfs:subClassOf>
        <rdfs:subClassOf>
            <owl:Restriction>
                <owl:onProperty rdf:resource="http://lpis.ec.europa.eu/registry/applicationschema/cap-iacs-parcel#criticalDefectAcceptanceNumber"/>
                <owl:cardinality rdf:datatype="http://www.w3.org/2001/XMLSchema#nonNegativeInteger">1</owl:cardinality>
            </owl:Restriction>
        </rdfs:subClassOf>
        <rdfs:subClassOf>
            <owl:Restriction>
                <owl:onProperty rdf:resource="http://lpis.ec.europa.eu/registry/applicationschema/cap-iacs-parcel#inspectionMethod"/>
                <owl:cardinality rdf:datatype="http://www.w3.org/2001/XMLSchema#nonNegativeInteger">1</owl:cardinality>
            </owl:Restriction>
        </rdfs:subClassOf>
        <rdfs:subClassOf>
            <owl:Restriction>
                <owl:onProperty rdf:resource="http://lpis.ec.europa.eu/registry/applicationschema/cap-iacs-parcel#lpisLotDetailsForEfaSample"/>
                <owl:cardinality rdf:datatype="http://www.w3.org/2001/XMLSchema#nonNegativeInteger">1</owl:cardinality>
            </owl:Restriction>
        </rdfs:subClassOf>
        <rdfs:subClassOf>
            <owl:Restriction>
                <owl:onProperty rdf:resource="http://lpis.ec.europa.eu/registry/applicationschema/cap-iacs-parcel#metadata"/>
                <owl:cardinality rdf:datatype="http://www.w3.org/2001/XMLSchema#nonNegativeInteger">1</owl:cardinality>
            </owl:Restriction>
        </rdfs:subClassOf>
        <rdfs:subClassOf>
            <owl:Restriction>
                <owl:onProperty rdf:resource="http://lpis.ec.europa.eu/registry/applicationschema/cap-iacs-parcel#nonConformingItemAcceptanceNumber"/>
                <owl:cardinality rdf:datatype="http://www.w3.org/2001/XMLSchema#nonNegativeInteger">1</owl:cardinality>
            </owl:Restriction>
        </rdfs:subClassOf>
        <rdfs:subClassOf>
            <owl:Restriction>
                <owl:onProperty rdf:resource="http://lpis.ec.europa.eu/registry/applicationschema/cap-iacs-parcel#parameterDescription"/>
                <owl:cardinality rdf:datatype="http://www.w3.org/2001/XMLSchema#nonNegativeInteger">1</owl:cardinality>
            </owl:Restriction>
        </rdfs:subClassOf>
        <rdfs:subClassOf>
            <owl:Restriction>
                <owl:onProperty rdf:resource="http://lpis.ec.europa.eu/registry/applicationschema/cap-iacs-parcel#lpisLotName"/>
                <owl:cardinality rdf:datatype="http://www.w3.org/2001/XMLSchema#nonNegativeInteger">1</owl:cardinality>
            </owl:Restriction>
        </rdfs:subClassOf>
        <rdfs:subClassOf>
            <owl:Restriction>
                <owl:onProperty rdf:resource="http://lpis.ec.europa.eu/registry/applicationschema/cap-iacs-parcel#lpisLotSize"/>
                <owl:cardinality rdf:datatype="http://www.w3.org/2001/XMLSchema#nonNegativeInteger">1</owl:cardinality>
            </owl:Restriction>
        </rdfs:subClassOf>
        <rdfs:subClassOf>
            <owl:Restriction>
                <owl:onProperty rdf:resource="http://lpis.ec.europa.eu/registry/applicationschema/cap-iacs-parcel#parcelAggregation"/>
                <owl:cardinality rdf:datatype="http://www.w3.org/2001/XMLSchema#nonNegativeInteger">1</owl:cardinality>
            </owl:Restriction>
        </rdfs:subClassOf>
        <rdfs:label xml:lang="en">LPIS lot</rdfs:label>
        <skos:definition xml:lang="en">--Name--
LPIS lot

-- Definition --
Definite number of reference parcels present in LPIS [adopted from ISO 2859-1:1999].

-- Description --
Total population of reference parcels within the LPIS subject of LPISQA. It comprises all the RPs  that 
 - were declared in the previous year and
 - which reference area does not equal to zero.</skos:definition>
    </owl:Class>
    


    <!-- http://lpis.ec.europa.eu/registry/applicationschema/cap-iacs-parcel#MtsItemUnderInspection -->


    <owl:Class rdf:about="http://lpis.ec.europa.eu/registry/applicationschema/cap-iacs-parcel#MtsItemUnderInspection">
        <rdfs:subClassOf rdf:resource="http://www.opengis.net/ont/geosparql#Feature"/>
        <rdfs:subClassOf>
            <owl:Restriction>
                <owl:onProperty rdf:resource="http://lpis.ec.europa.eu/registry/applicationschema/cap-iacs-parcel#abstractTestType"/>
                <owl:minCardinality rdf:datatype="http://www.w3.org/2001/XMLSchema#nonNegativeInteger">1</owl:minCardinality>
            </owl:Restriction>
        </rdfs:subClassOf>
        <rdfs:subClassOf>
            <owl:Restriction>
                <owl:onProperty rdf:resource="http://lpis.ec.europa.eu/registry/applicationschema/cap-iacs-parcel#mtsItemUnderInspectionDetailsForExecutableTestCase"/>
                <owl:minCardinality rdf:datatype="http://www.w3.org/2001/XMLSchema#nonNegativeInteger">1</owl:minCardinality>
            </owl:Restriction>
        </rdfs:subClassOf>
        <rdfs:subClassOf>
            <owl:Restriction>
                <owl:onProperty rdf:resource="http://lpis.ec.europa.eu/registry/applicationschema/cap-iacs-parcel#executableTestResult"/>
                <owl:cardinality rdf:datatype="http://www.w3.org/2001/XMLSchema#nonNegativeInteger">1</owl:cardinality>
            </owl:Restriction>
        </rdfs:subClassOf>
        <rdfs:subClassOf>
            <owl:Restriction>
                <owl:onProperty rdf:resource="http://lpis.ec.europa.eu/registry/applicationschema/cap-iacs-parcel#mtsReport"/>
                <owl:cardinality rdf:datatype="http://www.w3.org/2001/XMLSchema#nonNegativeInteger">1</owl:cardinality>
            </owl:Restriction>
        </rdfs:subClassOf>
        <rdfs:subClassOf>
            <owl:Restriction>
                <owl:onProperty rdf:resource="http://lpis.ec.europa.eu/registry/applicationschema/cap-iacs-parcel#elementlId"/>
                <owl:cardinality rdf:datatype="http://www.w3.org/2001/XMLSchema#nonNegativeInteger">1</owl:cardinality>
            </owl:Restriction>
        </rdfs:subClassOf>
        <rdfs:label xml:lang="en">Item under inspection</rdfs:label>
        <skos:definition xml:lang="en">--Name--
MTS item under inspection

-- Definition--
Eligibility profile or their elements presented as System under Test (SUT) for conformance testing. [Adapted from ISO 19105:2000].

-- Description --
As first step of LPISQA, the Model Test Suit (MTS ) of the eligibility profile has to be performed to assess conformance with the LCM. The initial MTS shall be run on the whole eligibility profile. When a specific element of the eligibility profile is upgraded, partial MTS can be performed following the ETS test cases that are relevant to that element.</skos:definition>
    </owl:Class>
    


    <!-- http://lpis.ec.europa.eu/registry/applicationschema/cap-iacs-parcel#PreselectedParcel -->


    <owl:Class rdf:about="http://lpis.ec.europa.eu/registry/applicationschema/cap-iacs-parcel#PreselectedParcel">
        <rdfs:subClassOf rdf:resource="http://www.opengis.net/ont/geosparql#Feature"/>
        <rdfs:subClassOf>
            <owl:Restriction>
                <owl:onProperty rdf:resource="http://lpis.ec.europa.eu/registry/applicationschema/cap-iacs-parcel#preselectedReferenceParcelWithinTheLotDetails"/>
                <owl:cardinality rdf:datatype="http://www.w3.org/2001/XMLSchema#nonNegativeInteger">1</owl:cardinality>
            </owl:Restriction>
        </rdfs:subClassOf>
        <rdfs:subClassOf>
            <owl:Restriction>
                <owl:onProperty rdf:resource="http://lpis.ec.europa.eu/registry/applicationschema/cap-iacs-parcel#detailsOfPreselectedParcelForInspection"/>
                <owl:maxCardinality rdf:datatype="http://www.w3.org/2001/XMLSchema#nonNegativeInteger">1</owl:maxCardinality>
            </owl:Restriction>
        </rdfs:subClassOf>
        <rdfs:subClassOf>
            <owl:Restriction>
                <owl:onProperty rdf:resource="http://lpis.ec.europa.eu/registry/applicationschema/cap-iacs-parcel#skippingReasonType"/>
                <owl:maxCardinality rdf:datatype="http://www.w3.org/2001/XMLSchema#nonNegativeInteger">1</owl:maxCardinality>
            </owl:Restriction>
        </rdfs:subClassOf>
        <rdfs:subClassOf>
            <owl:Restriction>
                <owl:onProperty rdf:resource="http://lpis.ec.europa.eu/registry/applicationschema/cap-iacs-parcel#feasibilityForInspection"/>
                <owl:cardinality rdf:datatype="http://www.w3.org/2001/XMLSchema#nonNegativeInteger">1</owl:cardinality>
            </owl:Restriction>
        </rdfs:subClassOf>
        <rdfs:subClassOf>
            <owl:Restriction>
                <owl:onProperty rdf:resource="http://lpis.ec.europa.eu/registry/applicationschema/cap-iacs-parcel#ordinalNumber"/>
                <owl:cardinality rdf:datatype="http://www.w3.org/2001/XMLSchema#nonNegativeInteger">1</owl:cardinality>
            </owl:Restriction>
        </rdfs:subClassOf>
        <rdfs:label xml:lang="en">Preselected parcel</rdfs:label>
        <skos:definition xml:lang="en">--Name--
Pre-selected parcel

-- Definition --
List of parcels produced in the sample pre-selection process performed by DG JRC in order to provide a preliminary sample of parcels for the executable test suit (ETS).

-- Description --
The population of the pre-selected parcels is three times more than the sample size defined as function the total LPIS population and the limiting quality value LQ=2 in ISO 2859-2. The identifiers of randomly pre-selected parcels are provided to the MS in a strict order, which prescribes the sequence of the inspection process. As soon as the prescribed sample size is reached the inspection process is considered to be complete.</skos:definition>
    </owl:Class>
    


    <!-- http://lpis.ec.europa.eu/registry/applicationschema/cap-iacs-parcel#ProRataCategoryValue -->


    <owl:Class rdf:about="http://lpis.ec.europa.eu/registry/applicationschema/cap-iacs-parcel#ProRataCategoryValue">
        <rdfs:subClassOf rdf:resource="http://www.w3.org/2004/02/skos/core#Concept"/>
        <rdfs:label xml:lang="en">List of pro rata category values</rdfs:label>
        <skos:definition xml:lang="en">--Name--
Pro-rata category value

-- Definition --
Pro rata categories represent groups of land cover classes that share an eligibility rate.

-- Description --
Categories are predefined by MS/Regions. The code list can be extended.</skos:definition>
    </owl:Class>
    


    <!-- http://lpis.ec.europa.eu/registry/applicationschema/cap-iacs-parcel#ReferenceParcel -->


    <owl:Class rdf:about="http://lpis.ec.europa.eu/registry/applicationschema/cap-iacs-parcel#ReferenceParcel">
        <rdfs:subClassOf rdf:resource="http://www.opengis.net/ont/geosparql#Feature"/>
        <rdfs:subClassOf>
            <owl:Restriction>
                <owl:onProperty rdf:resource="http://lpis.ec.europa.eu/registry/applicationschema/cap-iacs-parcel#referenceArea"/>
                <owl:minCardinality rdf:datatype="http://www.w3.org/2001/XMLSchema#nonNegativeInteger">1</owl:minCardinality>
            </owl:Restriction>
        </rdfs:subClassOf>
        <rdfs:subClassOf>
            <owl:Restriction>
                <owl:onProperty rdf:resource="http://lpis.ec.europa.eu/registry/applicationschema/cap-iacs-parcel#supportSchemaType"/>
                <owl:minCardinality rdf:datatype="http://www.w3.org/2001/XMLSchema#nonNegativeInteger">1</owl:minCardinality>
            </owl:Restriction>
        </rdfs:subClassOf>
        <rdfs:subClassOf>
            <owl:Restriction>
                <owl:onProperty rdf:resource="http://lpis.ec.europa.eu/registry/applicationschema/cap-iacs-parcel#geometry"/>
                <owl:cardinality rdf:datatype="http://www.w3.org/2001/XMLSchema#nonNegativeInteger">1</owl:cardinality>
            </owl:Restriction>
        </rdfs:subClassOf>
        <rdfs:subClassOf>
            <owl:Restriction>
                <owl:onProperty rdf:resource="http://lpis.ec.europa.eu/registry/applicationschema/cap-iacs-parcel#referenceParcelsLotDetails"/>
                <owl:cardinality rdf:datatype="http://www.w3.org/2001/XMLSchema#nonNegativeInteger">1</owl:cardinality>
            </owl:Restriction>
        </rdfs:subClassOf>
        <rdfs:subClassOf>
            <owl:Restriction>
                <owl:onProperty rdf:resource="http://lpis.ec.europa.eu/registry/applicationschema/cap-iacs-parcel#referenceParcelDetailsForAggregation"/>
                <owl:maxCardinality rdf:datatype="http://www.w3.org/2001/XMLSchema#nonNegativeInteger">1</owl:maxCardinality>
            </owl:Restriction>
        </rdfs:subClassOf>
        <rdfs:subClassOf>
            <owl:Restriction>
                <owl:onProperty rdf:resource="http://lpis.ec.europa.eu/registry/applicationschema/cap-iacs-parcel#selectedReferenceParcelDetails"/>
                <owl:maxCardinality rdf:datatype="http://www.w3.org/2001/XMLSchema#nonNegativeInteger">1</owl:maxCardinality>
            </owl:Restriction>
        </rdfs:subClassOf>
        <rdfs:label xml:lang="en">Reference parcel</rdfs:label>
        <skos:definition xml:lang="en">--Name--
Reference parcel

-- Definition --
Means a geographically delimited area retaining a unique identification as registered in the LPIS. a.k.a. identification system for agricultural parcels referred to in Article 70 of Regulation (EU) No 1306/2013. 

-- Description --
Basic spatial unit for the administration and geographical localization of agricultural parcels. May contain one or more declared agricultural parcels in IACS and may be cultivated by one or more farmers (or producers association). Does not necessarily cover a territory nationwide, but overlaps are not allowed. 

NOTE.  Definition in the past. Reference parcel - a continuous area of agricultural land (production block) grouping together a number of neighboring agricultural parcels (production units) cultivated by one or more farmer(s) and delineated by most stable boundaries. Subtypes (used in the past): CadParcel, AgrParcel, FarBlock, PhyBlock, TopoBlock and MixedParcelType. It current model it is not implemented, since these concepts are not core elements of current IACS model.</skos:definition>
    </owl:Class>
    


    <!-- http://lpis.ec.europa.eu/registry/applicationschema/cap-iacs-parcel#SampleSizeValue -->


    <owl:Class rdf:about="http://lpis.ec.europa.eu/registry/applicationschema/cap-iacs-parcel#SampleSizeValue">
        <owl:equivalentClass>
            <owl:Class>
                <owl:oneOf rdf:parseType="Collection">
                    <rdf:Description rdf:about="http://lpis.ec.europa.eu/registry/applicationschema/cap-iacs-parcel/code#SampleSizeValue/1250"/>
                    <rdf:Description rdf:about="http://lpis.ec.europa.eu/registry/applicationschema/cap-iacs-parcel/code#SampleSizeValue/200"/>
                    <rdf:Description rdf:about="http://lpis.ec.europa.eu/registry/applicationschema/cap-iacs-parcel/code#SampleSizeValue/500"/>
                    <rdf:Description rdf:about="http://lpis.ec.europa.eu/registry/applicationschema/cap-iacs-parcel/code#SampleSizeValue/800"/>
                </owl:oneOf>
            </owl:Class>
        </owl:equivalentClass>
        <rdfs:subClassOf rdf:resource="http://www.w3.org/2004/02/skos/core#Concept"/>
        <rdfs:label xml:lang="en">List of possible sample size values</rdfs:label>
        <skos:definition xml:lang="en">--Name--
Sample size value

-- Definition --
List of sample size values applicable for LPISQA.

-- Description --
The sample size is selected as function of the lot size and the limiting quality defined in  ISO 2859-2:1985 (Sampling procedures for inspection by attributes, Part 2: Sampling plans indexed by limiting quality (LQ) for isolated lot inspection).</skos:definition>
    </owl:Class>
    


    <!-- http://lpis.ec.europa.eu/registry/applicationschema/cap-iacs-parcel#SkippingReasonTypeValue -->


    <owl:Class rdf:about="http://lpis.ec.europa.eu/registry/applicationschema/cap-iacs-parcel#SkippingReasonTypeValue">
        <rdfs:subClassOf rdf:resource="http://www.w3.org/2004/02/skos/core#Concept"/>
        <rdfs:label xml:lang="en">Skipping reason type value</rdfs:label>
        <skos:definition xml:lang="en">--Name--
Skipping reason value type

-- Definition --
List  of reasons that do not allow the inspection of a given item under inspection.

-- Description --
Objective reasons for skipping  an item under inspection.

NOTE: This code list is managed by DG JRC. MS/Regions are not allowed to extend it.</skos:definition>
    </owl:Class>
    


    <!-- http://lpis.ec.europa.eu/registry/applicationschema/cap-iacs-parcel#TechnicalReasonValue -->


    <owl:Class rdf:about="http://lpis.ec.europa.eu/registry/applicationschema/cap-iacs-parcel#TechnicalReasonValue">
        <rdfs:subClassOf rdf:resource="http://www.w3.org/2004/02/skos/core#Concept"/>
        <rdfs:label xml:lang="en">List of possible technical reason values</rdfs:label>
        <skos:definition xml:lang="en">--Name--
Technical reason value

--Definition --
List of the technical reasons.

--Description--
List of the causes leading to non-conformance of items under inspection.</skos:definition>
    </owl:Class>
    


    <!-- http://lpis.ec.europa.eu/registry/applicationschema/cap-iacs-parcel#TestTypeMtsValue -->


    <owl:Class rdf:about="http://lpis.ec.europa.eu/registry/applicationschema/cap-iacs-parcel#TestTypeMtsValue">
        <rdfs:subClassOf rdf:resource="http://www.w3.org/2004/02/skos/core#Concept"/>
        <rdfs:label xml:lang="en">MTS test type value list</rdfs:label>
        <skos:definition xml:lang="en">--Name--
MTS  test type values

--Definition--
Abstract test cases applicable in model based testing for LPISQA.

--Description--
These abstract test cases are applicable for conformance testing of the eligibility profile in general. They should  be further specified  in the executable test cases according to the implementation choices of the MS/Regions.</skos:definition>
    </owl:Class>
    


    <!-- 
    ///////////////////////////////////////////////////////////////////////////////////////
    //
    // Individuals
    //
    ///////////////////////////////////////////////////////////////////////////////////////
     -->


    


    <!-- http://lpis.ec.europa.eu/registry/applicationschema/cap-iacs-parcel/code#AcceptanceNumberValue/10 -->


    <owl:NamedIndividual rdf:about="http://lpis.ec.europa.eu/registry/applicationschema/cap-iacs-parcel/code#AcceptanceNumberValue/10"/>
    


    <!-- http://lpis.ec.europa.eu/registry/applicationschema/cap-iacs-parcel/code#AcceptanceNumberValue/18 -->


    <owl:NamedIndividual rdf:about="http://lpis.ec.europa.eu/registry/applicationschema/cap-iacs-parcel/code#AcceptanceNumberValue/18"/>
    


    <!-- http://lpis.ec.europa.eu/registry/applicationschema/cap-iacs-parcel/code#AcceptanceNumberValue/5 -->


    <owl:NamedIndividual rdf:about="http://lpis.ec.europa.eu/registry/applicationschema/cap-iacs-parcel/code#AcceptanceNumberValue/5"/>
    


    <!-- http://lpis.ec.europa.eu/registry/applicationschema/cap-iacs-parcel/code#LimitingQualityValue/12.50 -->


    <owl:NamedIndividual rdf:about="http://lpis.ec.europa.eu/registry/applicationschema/cap-iacs-parcel/code#LimitingQualityValue/12.50"/>
    


    <!-- http://lpis.ec.europa.eu/registry/applicationschema/cap-iacs-parcel/code#LimitingQualityValue/2.00 -->


    <owl:NamedIndividual rdf:about="http://lpis.ec.europa.eu/registry/applicationschema/cap-iacs-parcel/code#LimitingQualityValue/2.00"/>
    


    <!-- http://lpis.ec.europa.eu/registry/applicationschema/cap-iacs-parcel/code#LotSizeValue/150001to500000 -->


    <owl:NamedIndividual rdf:about="http://lpis.ec.europa.eu/registry/applicationschema/cap-iacs-parcel/code#LotSizeValue/150001to500000"/>
    


    <!-- http://lpis.ec.europa.eu/registry/applicationschema/cap-iacs-parcel/code#LotSizeValue/35001to150000 -->


    <owl:NamedIndividual rdf:about="http://lpis.ec.europa.eu/registry/applicationschema/cap-iacs-parcel/code#LotSizeValue/35001to150000"/>
    


    <!-- http://lpis.ec.europa.eu/registry/applicationschema/cap-iacs-parcel/code#LotSizeValue/500000+ -->


    <owl:NamedIndividual rdf:about="http://lpis.ec.europa.eu/registry/applicationschema/cap-iacs-parcel/code#LotSizeValue/500000+"/>
    


    <!-- http://lpis.ec.europa.eu/registry/applicationschema/cap-iacs-parcel/code#SampleSizeValue/1250 -->


    <owl:NamedIndividual rdf:about="http://lpis.ec.europa.eu/registry/applicationschema/cap-iacs-parcel/code#SampleSizeValue/1250"/>
    


    <!-- http://lpis.ec.europa.eu/registry/applicationschema/cap-iacs-parcel/code#SampleSizeValue/200 -->


    <owl:NamedIndividual rdf:about="http://lpis.ec.europa.eu/registry/applicationschema/cap-iacs-parcel/code#SampleSizeValue/200"/>
    


    <!-- http://lpis.ec.europa.eu/registry/applicationschema/cap-iacs-parcel/code#SampleSizeValue/500 -->


    <owl:NamedIndividual rdf:about="http://lpis.ec.europa.eu/registry/applicationschema/cap-iacs-parcel/code#SampleSizeValue/500"/>
    


    <!-- http://lpis.ec.europa.eu/registry/applicationschema/cap-iacs-parcel/code#SampleSizeValue/800 -->


    <owl:NamedIndividual rdf:about="http://lpis.ec.europa.eu/registry/applicationschema/cap-iacs-parcel/code#SampleSizeValue/800"/>
    


    <!-- 
    ///////////////////////////////////////////////////////////////////////////////////////
    //
    // Annotations
    //
    ///////////////////////////////////////////////////////////////////////////////////////
     -->


    <rdf:Description rdf:about="http://lpis.ec.europa.eu/registry/applicationschema/cap-iacs-parcel#agriculturalArea">
        <rdfs:label xml:lang="en">Agricultural area</rdfs:label>
        <skos:definition xml:lang="en">--Name--
Agricultural area

-- Definition --
Quantification of agricultural area.

-- Description --
Registered area value giving quantification of the area.

NOTE: The are can be derived from geometric representation of the feature (if exists) or can be other alphanumerical recording [DSCG/2014/33].</skos:definition>
    </rdf:Description>
    <rdf:Description rdf:about="http://lpis.ec.europa.eu/registry/applicationschema/cap-iacs-parcel#conformingItemsArea">
        <rdfs:label xml:lang="en">Conforming sample area</rdfs:label>
        <skos:definition xml:lang="en">--Name--
Area of conforming items

-- Definition --
Total area of items under inspection found conforming in terms of area values. 

--Description--
Sum of the observed area for all conforming items (single and aggregated).</skos:definition>
    </rdf:Description>
    <rdf:Description rdf:about="http://lpis.ec.europa.eu/registry/applicationschema/cap-iacs-parcel#convertedArea">
        <rdfs:label xml:lang="en">Area converted</rdfs:label>
        <skos:definition xml:lang="en">-- Name--
Converted area 

-- Definition --
This is a placeholder only; currently not to be implemented.</skos:definition>
    </rdf:Description>
    <rdf:Description rdf:about="http://lpis.ec.europa.eu/registry/applicationschema/cap-iacs-parcel#declaredArea">
        <rdfs:label xml:lang="en">Area declared</rdfs:label>
        <skos:definition xml:lang="en">--Name--
Declared area

-- Definition --
Area declared by the farmer for the given reference parcel for the assessment year.

--Description--
The value of declared area is taken from the aid application register of IACS IACS for the assessment year.

NOTE 1. In our conceptual model this is the value of areaDeclared attribute. 

NOTE 2. The area value shall be given in hectares.</skos:definition>
    </rdf:Description>
    <rdf:Description rdf:about="http://lpis.ec.europa.eu/registry/applicationschema/cap-iacs-parcel#determinedArea">
        <rdfs:label xml:lang="en">Area determined</rdfs:label>
        <skos:definition xml:lang="en">--Name--
Determined area

-- Description --
Area for which all eligibility criteria have been met.

-- Description --
Area calculated as product of the surface area and the eventual pro-rata coefficient. When pro-rata is not applied it equals to the surface area  directly taken from the representation geometry (from GM_Surface).

NOTE: the area value shall be given in square meters.
/* Value of determinedArea shall be given in square meters. */
inv: self.determinedArea.uom.uomSymbol=&apos;m2&apos;</skos:definition>
    </rdf:Description>
    <rdf:Description rdf:about="http://lpis.ec.europa.eu/registry/applicationschema/cap-iacs-parcel#ecologicalFocusArea">
        <rdfs:label xml:lang="en">Area of ecological focus area</rdfs:label>
        <skos:definition xml:lang="en">--Name--
Ecological focus area

-- Definition --
Official area of EFA that can be accounted for fulfilling the obligation detailed in Art. 46(1) of (EU) R No 1307/2013.

-- Description --
This is the area value after applying the eventual conversion and weighting factors (DSCG/2014/31).

NOTE 1: According to DSCG/2014/31 
- Established area: Area resulting from direct field measurement or from delineation using ortho imagery
- Converted area: Virtual area of EFAs obtained when using the conversion factors of Annex II of Regulation (EU) No 639/2014.
- Weighted area: Virtual area of EFAs obtained after multiplying the established area or the converted area by the weighting factor of Annex II of Regulation (EU) No 639/2014.

NOTE 2: EFA area shall be given in ha.</skos:definition>
    </rdf:Description>
    <rdf:Description rdf:about="http://lpis.ec.europa.eu/registry/applicationschema/cap-iacs-parcel#landscapeFeatureArea">
        <rdfs:label xml:lang="en">Area of landscape feature</rdfs:label>
        <skos:definition xml:lang="en">--Name--
Landscape feature area

-- Definition --
Official area of LF recorded in LPIS.

--Description--
This are can be defined by measurement (delineation) or by numeric estimation.

NOTE: Geometric representation and area  are mandatory when a LF becomes an EFA element.</skos:definition>
    </rdf:Description>
    <rdf:Description rdf:about="http://lpis.ec.europa.eu/registry/applicationschema/cap-iacs-parcel#observedArea">
        <rdfs:label xml:lang="en">Area observed BPS/SPS area</rdfs:label>
        <skos:definition xml:lang="en">--Name--
Observed area

-- Definition --
Totality of  the areas of all eligible land cover types within the parcel.

-- Description --
This area value comprises the sum of areas of eligible agricultural land  and landscape features contained within the item under inspection. The minimum condition for assigning a value for this attribute is the existence of one eligible agricultural land cover type within the item under inspection.

NOTE 1: By definition, a stand-alone LF (i.e. LF without agricultural land) does not constitute agricultural land. If a RP does not contain agricultural land, it is a critical defect.

NOTE 2: The unit of meaurement shall be m2.
/* Value of observedArea shall be given in square meters. */
inv: self.observedArea.uom.uomSymbol=&apos;m2&apos;</skos:definition>
    </rdf:Description>
    <rdf:Description rdf:about="http://lpis.ec.europa.eu/registry/applicationschema/cap-iacs-parcel#recordedArea">
        <rdfs:label xml:lang="en">Area recorded</rdfs:label>
        <skos:definition xml:lang="en">-- Name--
Area recorded.

-- Definition --
This is a placeholder only; currently not to be implemented.

--Description--
Area recorded.</skos:definition>
    </rdf:Description>
    <rdf:Description rdf:about="http://lpis.ec.europa.eu/registry/applicationschema/cap-iacs-parcel#referenceArea">
        <rdfs:label xml:lang="en">Maximum eligable area</rdfs:label>
        <skos:definition xml:lang="en">--Name--
Reference area

-- Definition --
Value for the quantification of area as referred to in Art. 5(3) of (EU) R 640/2014.

-- Description --
Officially known area of reference  parcel in hectare, which corresponds to the maximum area, for which an application can be made.

NOTE 1:  Reference area value shall be expressed in hectares.
/* Value of referenceArea shall be given in hectars. */
inv: self.referenceArea.uom.uomSymbol=&apos;ha&apos;

NOTE 2: Reference area equals to MEA under BPS/SAPS [DSCG/2014/33]. For other payments schemes (e.g. voluntary coupled support) other MEA values may apply. Currently Annex I of regulation 1307/2013 define 11 support schema types.

NOTE 3: When no pro-rata applies , the reference area corresponds to the geometric area within the 2% stability margin.

NOTE 4:  Area reductions are subject of applying pro-rata system, or applying the  100 sq.m  limit for cumulative area of ineligible features of the same type.

NOTE 5: It is not necessary to deduct the area of a non agricultural area LC type when it is smaller than 100 sq.m.. However, in course of LPISQA or OTSC, when the cumulative area (per type) of such smaller features is more, the deduction shall be applied.

NOTE 6: Pro-rata shall be applied to &quot;clean&quot;, homogenous LC  (E.g. after all ineligible features are excluded).</skos:definition>
    </rdf:Description>
    <rdf:Description rdf:about="http://lpis.ec.europa.eu/registry/applicationschema/cap-iacs-parcel#totalDeclaredArea">
        <rdfs:label xml:lang="en">Total declared LPIS area</rdfs:label>
        <skos:definition xml:lang="en">--Name--
Total declared area

--Definition --
Total declared area in LPIS.

--Description --
Sum of the declared areas recorded in LPIS.</skos:definition>
    </rdf:Description>
    <rdf:Description rdf:about="http://lpis.ec.europa.eu/registry/applicationschema/cap-iacs-parcel#totalDeclaredAreaMeasuredItems">
        <rdfs:label xml:lang="en">Total declared area of measured items</rdfs:label>
        <skos:definition xml:lang="en">--Name--
Total declared area of measured items

--Definition --
Total declared area of measured items within LPIS sample.

--Description --
Sum of the declared areas recorded in LPIS for measured items.</skos:definition>
    </rdf:Description>
    <rdf:Description rdf:about="http://lpis.ec.europa.eu/registry/applicationschema/cap-iacs-parcel#totalOverestimatedArea">
        <rdfs:label xml:lang="en">Total overestimated area</rdfs:label>
        <skos:definition xml:lang="en">--Name--
Total overestimated area

--Definition --
Total area of the items under inspection that have discrepancy equal or more than -3%.

-- Description
NOTE. Previously it was: parameter of 10102_2 LPIS_RP_MEA_B</skos:definition>
    </rdf:Description>
    <rdf:Description rdf:about="http://lpis.ec.europa.eu/registry/applicationschema/cap-iacs-parcel#totalReferenceArea">
        <rdfs:label xml:lang="en">Total reference / recorded area</rdfs:label>
        <skos:definition xml:lang="en">--Name--
Total reference area

--Definition --
Total reference area recorded in LPIS.

--Description --
Sum of the reference areas of all RPs in LPIS.</skos:definition>
    </rdf:Description>
    <rdf:Description rdf:about="http://lpis.ec.europa.eu/registry/applicationschema/cap-iacs-parcel#totalReferenceAreaMeasuredItems">
        <rdfs:label xml:lang="en">Total reference / recorded area</rdfs:label>
        <skos:definition xml:lang="en">--Name--
Total reference area of measured items

--Definition --
Total reference  area of measured items as is recorded in LPIS.

--Description --
Sum of the reference areas recorded in LPIS for each measured item under inspection.</skos:definition>
    </rdf:Description>
    <rdf:Description rdf:about="http://lpis.ec.europa.eu/registry/applicationschema/cap-iacs-parcel#totalUnderestimatedArea">
        <rdfs:label xml:lang="en">Total underestimated area</rdfs:label>
        <skos:definition xml:lang="en">--Name--
Total underestimated area

--Definition --
Total area of the items under inspection that have a discrepancy equal or less than 3%.

-- Description--
NOTE. Previously it was: parameter of 10102_2 LPIS_RP_MEA_B.</skos:definition>
    </rdf:Description>
    <rdf:Description rdf:about="http://lpis.ec.europa.eu/registry/applicationschema/cap-iacs-parcel#weightedArea">
        <rdfs:label xml:lang="en">Area weighted</rdfs:label>
        <skos:definition xml:lang="en">-- Name--
Weighted area 

-- Definition --
This is a placeholder only; currently not to be implemented.</skos:definition>
    </rdf:Description>
</rdf:RDF>



<!-- Generated by the OWL API (version 5.1.18) https://github.com/owlcs/owlapi/ -->


