@prefix : <http://lpis.ec.europa.eu/registry/applicationschema/cap-iacs-beneficiery#> .
@prefix owl: <http://www.w3.org/2002/07/owl#> .
@prefix rdf: <http://www.w3.org/1999/02/22-rdf-syntax-ns#> .
@prefix xml: <http://www.w3.org/XML/1998/namespace> .
@prefix xsd: <http://www.w3.org/2001/XMLSchema#> .
@prefix rdfs: <http://www.w3.org/2000/01/rdf-schema#> .
@base <http://lpis.ec.europa.eu/registry/applicationschema/cap-iacs-beneficiery#> .

<http://lpis.ec.europa.eu/registry/applicationschema/cap-iacs-beneficiery> rdf:type owl:Ontology ;
                                                                            owl:versionIRI <http://lpis.ec.europa.eu/registry/applicationschema/cap-iacs-beneficiery/3.0> ;
                                                                            owl:imports <http://www.opengis.net/ont/geosparql> ,
                                                                                        <https://raw.githubusercontent.com/rapw3k/cap-iacs/main/cap-iacs-base.ttl> ;
                                                                            <http://purl.org/dc/terms/creator> _:genid1 ;
                                                                            <http://purl.org/dc/terms/description> "Ontology of the system to record the identity of each beneficiary used in IACS, generated from the transformation of the corresponding JRC application schema"@en ;
                                                                            <http://purl.org/dc/terms/rights> "This ontology is distributed under Creative Commons Attribution 4.0 License - http://creativecommons.org/licenses/by/4.0"@en ;
                                                                            <http://purl.org/dc/terms/source> "JRC IACS application schema. https://doi.org/10.1016/j.landusepol.2016.05.023"@en ;
                                                                            <http://purl.org/dc/terms/title> "JRC IACS - System to Record the Identity of Each Beneficiary Ontology"@en ;
                                                                            rdfs:label "System to record the identity of each beneficiary"@en ;
                                                                            owl:versionInfo "3.0" ;
                                                                            <http://www.w3.org/2004/02/skos/core#definition> """-- Name --
System to record the identity of each beneficiary

-- Definition --
Placeholder package for the Application schema for System to record the identity of each beneficiary.

-- Description --
The contents of an «ApplicationSchema» package exported as a GML Application Schema file."""@en .

_:genid1 <http://schema.org/affiliation> [ <http://xmlns.com/foaf/0.1/name> "PSNC"
                                          ] ;
          rdfs:seeAlso <http://orcid.org/0000-0003-4289-4922> ;
          <http://xmlns.com/foaf/0.1/name> "Raul Palma" .

#################################################################
#    Object Properties
#################################################################

###  http://lpis.ec.europa.eu/registry/applicationschema/cap-iacs-beneficiery#farmerDescription
:farmerDescription rdf:type owl:ObjectProperty ;
                   rdfs:range <http://xmlns.com/foaf/0.1/Agent> ;
                   rdfs:label "Farmer address"@en ;
                   <http://www.w3.org/2004/02/skos/core#definition> """-- Definition --
Farmer description.
-- Description --
Description of responsible individual or organization (farmer).
NOTE. role = pointOfContact."""@en .


###  http://lpis.ec.europa.eu/registry/applicationschema/cap-iacs-beneficiery#farmerDetailsForCollectiveImplementation
:farmerDetailsForCollectiveImplementation rdf:type owl:ObjectProperty ;
                                          rdfs:range <http://lpis.ec.europa.eu/registry/applicationschema/cap-iacs-aid#CollectiveImplementation> .


###  http://lpis.ec.europa.eu/registry/applicationschema/cap-iacs-beneficiery#farmerDetailsForOnTheSpotChecks
:farmerDetailsForOnTheSpotChecks rdf:type owl:ObjectProperty ;
                                 rdfs:range <http://lpis.ec.europa.eu/registry/applicationschema/cap-iacs-control#OnTheSpotCheck> .


###  http://lpis.ec.europa.eu/registry/applicationschema/cap-iacs-beneficiery#farmerQualification
:farmerQualification rdf:type owl:ObjectProperty ;
                     rdfs:range <http://lpis.ec.europa.eu/registry/applicationschema/cap-iacs-base#ConformanceStatementValue> ;
                     rdfs:label "Farmer occupational skills and competence"@en ;
                     <http://www.w3.org/2004/02/skos/core#definition> """-- Definition --
Farmer occupational skills and competence.
-- Description --
Farmer types created based on actor model.The occupational skills and competence  of a farmer. Required for young farmer scheme. Meet / do not meet requirements for competence of a farmer."""@en .


###  http://lpis.ec.europa.eu/registry/applicationschema/cap-iacs-beneficiery#farmerType
:farmerType rdf:type owl:ObjectProperty ;
            rdfs:range :FarmerTypeValue ;
            rdfs:label "Farmer type"@en ;
            <http://www.w3.org/2004/02/skos/core#definition> """-- Definition --
Farmer type.
-- Description --
Farmer types created based on actor model."""@en .


#################################################################
#    Data properties
#################################################################

###  http://lpis.ec.europa.eu/registry/applicationschema/cap-iacs-beneficiery#farmerBirthDate
:farmerBirthDate rdf:type owl:DatatypeProperty ;
                 rdfs:range xsd:date ;
                 rdfs:label "Birth date of farmer"@en ;
                 <http://www.w3.org/2004/02/skos/core#definition> """-- Definition --
Birth date of farmer.
-- Description --
The birth date of a farmer. Required for young farmer scheme."""@en .


#################################################################
#    Classes
#################################################################

###  http://lpis.ec.europa.eu/registry/applicationschema/cap-iacs-beneficiery#Farmer
:Farmer rdf:type owl:Class ;
        rdfs:subClassOf <http://www.opengis.net/ont/geosparql#Feature> ,
                        [ rdf:type owl:Restriction ;
                          owl:onProperty :farmerDetailsForCollectiveImplementation ;
                          owl:minCardinality "2"^^xsd:nonNegativeInteger
                        ] ,
                        [ rdf:type owl:Restriction ;
                          owl:onProperty :farmerQualification ;
                          owl:cardinality "1"^^xsd:nonNegativeInteger
                        ] ,
                        [ rdf:type owl:Restriction ;
                          owl:onProperty :farmerType ;
                          owl:cardinality "1"^^xsd:nonNegativeInteger
                        ] ,
                        [ rdf:type owl:Restriction ;
                          owl:onProperty :farmerDescription ;
                          owl:maxCardinality "1"^^xsd:nonNegativeInteger
                        ] ,
                        [ rdf:type owl:Restriction ;
                          owl:onProperty :farmerDetailsForCollectiveImplementation ;
                          owl:maxCardinality "10"^^xsd:nonNegativeInteger
                        ] ,
                        [ rdf:type owl:Restriction ;
                          owl:onProperty :farmerBirthDate ;
                          owl:maxCardinality "1"^^xsd:nonNegativeInteger
                        ] ;
        rdfs:label "Farmer"@en ;
        <http://www.w3.org/2004/02/skos/core#definition> """-- Definition --
Farmer.
-- Description --
Farmer is natural or legal person, or a group of natural or legal persons, regardless of the legal status granted to such group and its members by national law, whose holding is situated within the territorial scope of the Treaties, as defined in Article 52 TEU in conjunction with Articles 349 and 355 TFEU, and who exercises an agricultural activity. 1307/2013 4 (1)(a).
NOTE. Main class of a single system to record the identity of each beneficiary of the support referred to in Article 67(2) who submits an aid application or a payment claim."""@en .


###  http://lpis.ec.europa.eu/registry/applicationschema/cap-iacs-beneficiery#FarmerTypeValue
:FarmerTypeValue rdf:type owl:Class ;
                 owl:equivalentClass [ rdf:type owl:Class ;
                                       owl:oneOf ( <http://lpis.ec.europa.eu/registry/applicationschema/cap-iacs-beneficiery/code#FarmerTypeValue/farmer>
                                                   <http://lpis.ec.europa.eu/registry/applicationschema/cap-iacs-beneficiery/code#FarmerTypeValue/farmerActive>
                                                   <http://lpis.ec.europa.eu/registry/applicationschema/cap-iacs-beneficiery/code#FarmerTypeValue/farmerActiveApplicant>
                                                   <http://lpis.ec.europa.eu/registry/applicationschema/cap-iacs-beneficiery/code#FarmerTypeValue/farmerActiveApplicantBeneficiery>
                                                 )
                                     ] ;
                 rdfs:subClassOf <http://www.w3.org/2004/02/skos/core#Concept> ;
                 rdfs:label "List of farmer type values"@en ;
                 <http://www.w3.org/2004/02/skos/core#definition> """-- Definition --
List of farmer type values.
-- Description --
List of possible farmer type values based on Actor model (Dynamic Model)."""@en .


###  http://lpis.ec.europa.eu/registry/applicationschema/cap-iacs-control#OnTheSpotCheck
<http://lpis.ec.europa.eu/registry/applicationschema/cap-iacs-control#OnTheSpotCheck> rdf:type owl:Class .


#################################################################
#    Individuals
#################################################################

###  http://lpis.ec.europa.eu/registry/applicationschema/cap-iacs-beneficiery/code#FarmerTypeValue/farmer
<http://lpis.ec.europa.eu/registry/applicationschema/cap-iacs-beneficiery/code#FarmerTypeValue/farmer> rdf:type owl:NamedIndividual .


###  http://lpis.ec.europa.eu/registry/applicationschema/cap-iacs-beneficiery/code#FarmerTypeValue/farmerActive
<http://lpis.ec.europa.eu/registry/applicationschema/cap-iacs-beneficiery/code#FarmerTypeValue/farmerActive> rdf:type owl:NamedIndividual .


###  http://lpis.ec.europa.eu/registry/applicationschema/cap-iacs-beneficiery/code#FarmerTypeValue/farmerActiveApplicant
<http://lpis.ec.europa.eu/registry/applicationschema/cap-iacs-beneficiery/code#FarmerTypeValue/farmerActiveApplicant> rdf:type owl:NamedIndividual .


###  http://lpis.ec.europa.eu/registry/applicationschema/cap-iacs-beneficiery/code#FarmerTypeValue/farmerActiveApplicantBeneficiery
<http://lpis.ec.europa.eu/registry/applicationschema/cap-iacs-beneficiery/code#FarmerTypeValue/farmerActiveApplicantBeneficiery> rdf:type owl:NamedIndividual .


###  Generated by the OWL API (version 5.1.18) https://github.com/owlcs/owlapi/
