<?xml version="1.0"?>
<rdf:RDF xmlns="http://lpis.ec.europa.eu/registry/applicationschema/cap-iacs-base/code#"
     xml:base="http://lpis.ec.europa.eu/registry/applicationschema/cap-iacs-base/code"
     xmlns:owl="http://www.w3.org/2002/07/owl#"
     xmlns:rdf="http://www.w3.org/1999/02/22-rdf-syntax-ns#"
     xmlns:xml="http://www.w3.org/XML/1998/namespace"
     xmlns:xsd="http://www.w3.org/2001/XMLSchema#"
     xmlns:foaf="http://xmlns.com/foaf/0.1/"
     xmlns:rdfs="http://www.w3.org/2000/01/rdf-schema#"
     xmlns:skos="http://www.w3.org/2004/02/skos/core#"
     xmlns:terms="http://purl.org/dc/terms/"
     xmlns:schema="http://schema.org/">
    <owl:Ontology rdf:about="http://lpis.ec.europa.eu/registry/applicationschema/cap-iacs-base/code">
        <owl:versionIRI rdf:resource="http://lpis.ec.europa.eu/registry/applicationschema/cap-iacs-base/code/3.0"/>
        <terms:creator rdf:nodeID="genid1"/>
        <terms:description xml:lang="en">Ontology of the base types code lists used in IACS, generated from the transformation of the corresponding JRC application schema</terms:description>
        <terms:rights xml:lang="en">This ontology is distributed under Creative Commons Attribution 4.0 License - http://creativecommons.org/licenses/by/4.0</terms:rights>
        <terms:source xml:lang="en">JRC IACS application schema. https://doi.org/10.1016/j.landusepol.2016.05.023</terms:source>
        <terms:title xml:lang="en">JRC IACS - Base Types Code Lists</terms:title>
        <rdfs:label xml:lang="en">Base types code lists</rdfs:label>
        <owl:versionInfo>3.0</owl:versionInfo>
    </owl:Ontology>
    <rdf:Description rdf:nodeID="genid1">
        <schema:affiliation>
            <rdf:Description>
                <foaf:name>PSNC</foaf:name>
            </rdf:Description>
        </schema:affiliation>
        <rdfs:seeAlso rdf:resource="http://orcid.org/0000-0003-4289-4922"/>
        <foaf:name>Raul Palma</foaf:name>
    </rdf:Description>
    


    <!-- 
    ///////////////////////////////////////////////////////////////////////////////////////
    //
    // Annotation properties
    //
    ///////////////////////////////////////////////////////////////////////////////////////
     -->


    


    <!-- http://purl.org/dc/terms/creator -->


    <owl:AnnotationProperty rdf:about="http://purl.org/dc/terms/creator"/>
    


    <!-- http://purl.org/dc/terms/description -->


    <owl:AnnotationProperty rdf:about="http://purl.org/dc/terms/description"/>
    


    <!-- http://purl.org/dc/terms/isFormatOf -->


    <owl:AnnotationProperty rdf:about="http://purl.org/dc/terms/isFormatOf"/>
    


    <!-- http://purl.org/dc/terms/rights -->


    <owl:AnnotationProperty rdf:about="http://purl.org/dc/terms/rights"/>
    


    <!-- http://purl.org/dc/terms/source -->


    <owl:AnnotationProperty rdf:about="http://purl.org/dc/terms/source"/>
    


    <!-- http://purl.org/dc/terms/title -->


    <owl:AnnotationProperty rdf:about="http://purl.org/dc/terms/title"/>
    


    <!-- http://schema.org/affiliation -->


    <owl:AnnotationProperty rdf:about="http://schema.org/affiliation"/>
    


    <!-- http://www.w3.org/2004/02/skos/core#definition -->


    <owl:AnnotationProperty rdf:about="http://www.w3.org/2004/02/skos/core#definition"/>
    


    <!-- http://www.w3.org/2004/02/skos/core#inScheme -->


    <owl:AnnotationProperty rdf:about="http://www.w3.org/2004/02/skos/core#inScheme"/>
    


    <!-- http://xmlns.com/foaf/0.1/name -->


    <owl:AnnotationProperty rdf:about="http://xmlns.com/foaf/0.1/name"/>
    


    <!-- 
    ///////////////////////////////////////////////////////////////////////////////////////
    //
    // Classes
    //
    ///////////////////////////////////////////////////////////////////////////////////////
     -->


    


    <!-- http://lpis.ec.europa.eu/registry/applicationschema/cap-iacs-base#AffectedElementTypeValue -->


    <owl:Class rdf:about="http://lpis.ec.europa.eu/registry/applicationschema/cap-iacs-base#AffectedElementTypeValue"/>
    


    <!-- http://lpis.ec.europa.eu/registry/applicationschema/cap-iacs-base#CauseOfAnomalyValue -->


    <owl:Class rdf:about="http://lpis.ec.europa.eu/registry/applicationschema/cap-iacs-base#CauseOfAnomalyValue"/>
    


    <!-- http://lpis.ec.europa.eu/registry/applicationschema/cap-iacs-base#ConformanceClassValue -->


    <owl:Class rdf:about="http://lpis.ec.europa.eu/registry/applicationschema/cap-iacs-base#ConformanceClassValue"/>
    


    <!-- http://lpis.ec.europa.eu/registry/applicationschema/cap-iacs-base#ConformanceLevelValue -->


    <owl:Class rdf:about="http://lpis.ec.europa.eu/registry/applicationschema/cap-iacs-base#ConformanceLevelValue"/>
    


    <!-- http://lpis.ec.europa.eu/registry/applicationschema/cap-iacs-base#ConformanceRequirementClassValue -->


    <owl:Class rdf:about="http://lpis.ec.europa.eu/registry/applicationschema/cap-iacs-base#ConformanceRequirementClassValue"/>
    


    <!-- http://lpis.ec.europa.eu/registry/applicationschema/cap-iacs-base#ConformanceRequirementStatementValue -->


    <owl:Class rdf:about="http://lpis.ec.europa.eu/registry/applicationschema/cap-iacs-base#ConformanceRequirementStatementValue"/>
    


    <!-- http://lpis.ec.europa.eu/registry/applicationschema/cap-iacs-base#ConformanceStatementValue -->


    <owl:Class rdf:about="http://lpis.ec.europa.eu/registry/applicationschema/cap-iacs-base#ConformanceStatementValue"/>
    


    <!-- http://lpis.ec.europa.eu/registry/applicationschema/cap-iacs-base#CropItemCodeValue -->


    <owl:Class rdf:about="http://lpis.ec.europa.eu/registry/applicationschema/cap-iacs-base#CropItemCodeValue"/>
    


    <!-- http://lpis.ec.europa.eu/registry/applicationschema/cap-iacs-base#CrossComplianceRuleValue -->


    <owl:Class rdf:about="http://lpis.ec.europa.eu/registry/applicationschema/cap-iacs-base#CrossComplianceRuleValue"/>
    


    <!-- http://lpis.ec.europa.eu/registry/applicationschema/cap-iacs-base#FarmStructureSurveyNumberValue -->


    <owl:Class rdf:about="http://lpis.ec.europa.eu/registry/applicationschema/cap-iacs-base#FarmStructureSurveyNumberValue"/>
    


    <!-- http://lpis.ec.europa.eu/registry/applicationschema/cap-iacs-base#MonthValue -->


    <owl:Class rdf:about="http://lpis.ec.europa.eu/registry/applicationschema/cap-iacs-base#MonthValue"/>
    


    <!-- http://lpis.ec.europa.eu/registry/applicationschema/cap-iacs-base#NotificationGroupValue -->


    <owl:Class rdf:about="http://lpis.ec.europa.eu/registry/applicationschema/cap-iacs-base#NotificationGroupValue"/>
    


    <!-- http://lpis.ec.europa.eu/registry/applicationschema/cap-iacs-base#OrdinalNumberValue -->


    <owl:Class rdf:about="http://lpis.ec.europa.eu/registry/applicationschema/cap-iacs-base#OrdinalNumberValue"/>
    


    <!-- http://lpis.ec.europa.eu/registry/applicationschema/cap-iacs-base#RecurenceValue -->


    <owl:Class rdf:about="http://lpis.ec.europa.eu/registry/applicationschema/cap-iacs-base#RecurenceValue"/>
    


    <!-- http://lpis.ec.europa.eu/registry/applicationschema/cap-iacs-base#SpecieCodeValue -->


    <owl:Class rdf:about="http://lpis.ec.europa.eu/registry/applicationschema/cap-iacs-base#SpecieCodeValue"/>
    


    <!-- http://lpis.ec.europa.eu/registry/applicationschema/cap-iacs-base#StatusOfAnomalyValue -->


    <owl:Class rdf:about="http://lpis.ec.europa.eu/registry/applicationschema/cap-iacs-base#StatusOfAnomalyValue"/>
    


    <!-- http://lpis.ec.europa.eu/registry/applicationschema/cap-iacs-base#StatusOfIssueValue -->


    <owl:Class rdf:about="http://lpis.ec.europa.eu/registry/applicationschema/cap-iacs-base#StatusOfIssueValue"/>
    


    <!-- http://lpis.ec.europa.eu/registry/applicationschema/cap-iacs-base#StatusValue -->


    <owl:Class rdf:about="http://lpis.ec.europa.eu/registry/applicationschema/cap-iacs-base#StatusValue"/>
    


    <!-- http://lpis.ec.europa.eu/registry/applicationschema/cap-iacs-base#SupportSchemeTypeValue -->


    <owl:Class rdf:about="http://lpis.ec.europa.eu/registry/applicationschema/cap-iacs-base#SupportSchemeTypeValue"/>
    


    <!-- http://lpis.ec.europa.eu/registry/applicationschema/cap-iacs-base#TestTypeValue -->


    <owl:Class rdf:about="http://lpis.ec.europa.eu/registry/applicationschema/cap-iacs-base#TestTypeValue"/>
    


    <!-- http://lpis.ec.europa.eu/registry/applicationschema/cap-iacs-base#TestVerdictValue -->


    <owl:Class rdf:about="http://lpis.ec.europa.eu/registry/applicationschema/cap-iacs-base#TestVerdictValue"/>
    


    <!-- http://lpis.ec.europa.eu/registry/applicationschema/cap-iacs-base#TestingTypeValue -->


    <owl:Class rdf:about="http://lpis.ec.europa.eu/registry/applicationschema/cap-iacs-base#TestingTypeValue"/>
    


    <!-- http://lpis.ec.europa.eu/registry/applicationschema/cap-iacs-base#VarietalNameValue -->


    <owl:Class rdf:about="http://lpis.ec.europa.eu/registry/applicationschema/cap-iacs-base#VarietalNameValue"/>
    


    <!-- http://lpis.ec.europa.eu/registry/applicationschema/cap-iacs-base#WeekdayValue -->


    <owl:Class rdf:about="http://lpis.ec.europa.eu/registry/applicationschema/cap-iacs-base#WeekdayValue"/>
    


    <!-- http://www.w3.org/2004/02/skos/core#ConceptScheme -->


    <owl:Class rdf:about="http://www.w3.org/2004/02/skos/core#ConceptScheme"/>
    


    <!-- 
    ///////////////////////////////////////////////////////////////////////////////////////
    //
    // Individuals
    //
    ///////////////////////////////////////////////////////////////////////////////////////
     -->


    


    <!-- http://lpis.ec.europa.eu/registry/applicationschema/cap-iacs-base/code#AffectedElementTypeValue -->


    <owl:NamedIndividual rdf:about="http://lpis.ec.europa.eu/registry/applicationschema/cap-iacs-base/code#AffectedElementTypeValue">
        <rdf:type rdf:resource="http://www.w3.org/2004/02/skos/core#ConceptScheme"/>
        <terms:isFormatOf rdf:resource="http://lpis.ec.europa.eu/registry/applicationschema/cap-iacs-base#AffectedElementTypeValue"/>
        <rdfs:label xml:lang="en">Affected element type value list</rdfs:label>
        <skos:definition xml:lang="en">--Name--
Affected element type value.

-- Definition --
Application schema or its element that might be a subject of an issue.

-- Description --
List of possible affected elements that might be changed within the model.</skos:definition>
    </owl:NamedIndividual>
    


    <!-- http://lpis.ec.europa.eu/registry/applicationschema/cap-iacs-base/code#CauseOfAnomalyValue -->


    <owl:NamedIndividual rdf:about="http://lpis.ec.europa.eu/registry/applicationschema/cap-iacs-base/code#CauseOfAnomalyValue">
        <rdf:type rdf:resource="http://www.w3.org/2004/02/skos/core#ConceptScheme"/>
        <terms:isFormatOf rdf:resource="http://lpis.ec.europa.eu/registry/applicationschema/cap-iacs-base#CauseOfAnomalyValue"/>
        <rdfs:label xml:lang="en">Anomaly cause value list</rdfs:label>
        <skos:definition xml:lang="en">--Name--
Cause of anomaly value

-- Definition --
Code list defining the values of the case of anomaly attribute.

-- Description --
List of possible anomaly causes used for documentation of an anomaly.</skos:definition>
    </owl:NamedIndividual>
    


    <!-- http://lpis.ec.europa.eu/registry/applicationschema/cap-iacs-base/code#ConformanceClassValue -->


    <owl:NamedIndividual rdf:about="http://lpis.ec.europa.eu/registry/applicationschema/cap-iacs-base/code#ConformanceClassValue">
        <rdf:type rdf:resource="http://www.w3.org/2004/02/skos/core#ConceptScheme"/>
        <terms:isFormatOf rdf:resource="http://lpis.ec.europa.eu/registry/applicationschema/cap-iacs-base#ConformanceClassValue"/>
        <rdfs:label xml:lang="en">List of conformance class values</rdfs:label>
        <skos:definition xml:lang="en">--Name--
Conformance class value

--Definition--
List of conformance class values.

--Description--
Any product claiming conformance with one of these classes shall pass all requirements described in the corresponding abstract test suite.

NOTE. Requirements of conformance classes may overlap in which case subparts of the abstract test suite may be shared between different conformance classes.</skos:definition>
    </owl:NamedIndividual>
    


    <!-- http://lpis.ec.europa.eu/registry/applicationschema/cap-iacs-base/code#ConformanceLevelValue -->


    <owl:NamedIndividual rdf:about="http://lpis.ec.europa.eu/registry/applicationschema/cap-iacs-base/code#ConformanceLevelValue">
        <rdf:type rdf:resource="http://www.w3.org/2004/02/skos/core#ConceptScheme"/>
        <terms:isFormatOf rdf:resource="http://lpis.ec.europa.eu/registry/applicationschema/cap-iacs-base#ConformanceLevelValue"/>
        <rdfs:label xml:lang="en">List of conformance level values</rdfs:label>
        <skos:definition xml:lang="en">--Name--
Conformance level value

-- Definition --
List of conformance level values.

-- Description --
List of conformance level values. Any product claiming conformance with one of these levels shall pass all requirements described in the corresponding abstract test suite.

NOTE. Requirements of a higher level contain all requirements of a lower level.</skos:definition>
    </owl:NamedIndividual>
    


    <!-- http://lpis.ec.europa.eu/registry/applicationschema/cap-iacs-base/code#ConformanceRequirementClassValue -->


    <owl:NamedIndividual rdf:about="http://lpis.ec.europa.eu/registry/applicationschema/cap-iacs-base/code#ConformanceRequirementClassValue">
        <rdf:type rdf:resource="http://www.w3.org/2004/02/skos/core#ConceptScheme"/>
        <terms:isFormatOf rdf:resource="http://lpis.ec.europa.eu/registry/applicationschema/cap-iacs-base#ConformanceRequirementClassValue"/>
        <rdfs:label xml:lang="en">List of conformance requirement class values</rdfs:label>
        <skos:definition xml:lang="en">--Name--
Conformance requirement class value

--Definition--
List of conformance requirement class values.</skos:definition>
    </owl:NamedIndividual>
    


    <!-- http://lpis.ec.europa.eu/registry/applicationschema/cap-iacs-base/code#ConformanceRequirementStatementValue -->


    <owl:NamedIndividual rdf:about="http://lpis.ec.europa.eu/registry/applicationschema/cap-iacs-base/code#ConformanceRequirementStatementValue">
        <rdf:type rdf:resource="http://www.w3.org/2004/02/skos/core#ConceptScheme"/>
        <terms:isFormatOf rdf:resource="http://lpis.ec.europa.eu/registry/applicationschema/cap-iacs-base#ConformanceRequirementStatementValue"/>
        <rdfs:label xml:lang="en">List of conformance requirement statement values</rdfs:label>
        <skos:definition xml:lang="en">--Name--
Conformance requirement statement value

--Definition--
List of conformance requirement statement values.</skos:definition>
    </owl:NamedIndividual>
    


    <!-- http://lpis.ec.europa.eu/registry/applicationschema/cap-iacs-base/code#ConformanceStatementValue -->


    <owl:NamedIndividual rdf:about="http://lpis.ec.europa.eu/registry/applicationschema/cap-iacs-base/code#ConformanceStatementValue">
        <rdf:type rdf:resource="http://www.w3.org/2004/02/skos/core#ConceptScheme"/>
        <terms:isFormatOf rdf:resource="http://lpis.ec.europa.eu/registry/applicationschema/cap-iacs-base#ConformanceStatementValue"/>
        <rdfs:label xml:lang="en">List of conformance statement values</rdfs:label>
        <skos:definition xml:lang="en">--Name--
Conformance Statement Value

-- Definition --
Enumeration of conformance statement values.

-- Description --
List of possible conformance verdicts whether the subject of testing (e.g. SUT, schema element, source data, etc.) conforms to the specified rules.</skos:definition>
    </owl:NamedIndividual>
    


    <!-- http://lpis.ec.europa.eu/registry/applicationschema/cap-iacs-base/code#CropItemCodeValue -->


    <owl:NamedIndividual rdf:about="http://lpis.ec.europa.eu/registry/applicationschema/cap-iacs-base/code#CropItemCodeValue">
        <rdf:type rdf:resource="http://www.w3.org/2004/02/skos/core#ConceptScheme"/>
        <terms:isFormatOf rdf:resource="http://lpis.ec.europa.eu/registry/applicationschema/cap-iacs-base#CropItemCodeValue"/>
        <rdfs:label xml:lang="en">List of crop items</rdfs:label>
        <skos:definition xml:lang="en">-- Definition --
List of crop items (aggregate of a species)
Eurostat Handbook for Annual Crop Statistics (Regulation 543/2009) (Revision 2013 – Presented in the WPM of the 12).
-- Description --
Land use of Agriculture Area in Use -L
Cereals and main crops - C</skos:definition>
    </owl:NamedIndividual>
    


    <!-- http://lpis.ec.europa.eu/registry/applicationschema/cap-iacs-base/code#CrossComplianceRuleValue -->


    <owl:NamedIndividual rdf:about="http://lpis.ec.europa.eu/registry/applicationschema/cap-iacs-base/code#CrossComplianceRuleValue">
        <rdf:type rdf:resource="http://www.w3.org/2004/02/skos/core#ConceptScheme"/>
        <terms:isFormatOf rdf:resource="http://lpis.ec.europa.eu/registry/applicationschema/cap-iacs-base#CrossComplianceRuleValue"/>
        <rdfs:label xml:lang="en">List of rules for cross-compliance</rdfs:label>
        <skos:definition xml:lang="en">-- Definition --
List of rules for cross-compliance
-- Description --
List of rules for cross-compliance. Rules for SMR and GAEC.</skos:definition>
    </owl:NamedIndividual>
    


    <!-- http://lpis.ec.europa.eu/registry/applicationschema/cap-iacs-base/code#FarmStructureSurveyNumberValue -->


    <owl:NamedIndividual rdf:about="http://lpis.ec.europa.eu/registry/applicationschema/cap-iacs-base/code#FarmStructureSurveyNumberValue">
        <rdf:type rdf:resource="http://www.w3.org/2004/02/skos/core#ConceptScheme"/>
        <terms:isFormatOf rdf:resource="http://lpis.ec.europa.eu/registry/applicationschema/cap-iacs-base#FarmStructureSurveyNumberValue"/>
        <rdfs:label xml:lang="en">List of farm structure survey numbers</rdfs:label>
        <skos:definition xml:lang="en">-- Definition --
List of farm structure survey numbers (aggregate of crop items).
-- Desription --
Scope - LAND part only. Commision regulations (EC) No 1200/2009 of 30 November 2009 Implementing Regulation (EC) No 1166/2008 of the European Parliament and of the Council on farm structure surveys and the survey on agricultural production methods, as regards livestock unit coefficients and definitions of the characteristics (Text with EEA relevance).</skos:definition>
    </owl:NamedIndividual>
    


    <!-- http://lpis.ec.europa.eu/registry/applicationschema/cap-iacs-base/code#MonthValue -->


    <owl:NamedIndividual rdf:about="http://lpis.ec.europa.eu/registry/applicationschema/cap-iacs-base/code#MonthValue">
        <rdf:type rdf:resource="http://www.w3.org/2004/02/skos/core#ConceptScheme"/>
        <terms:isFormatOf rdf:resource="http://lpis.ec.europa.eu/registry/applicationschema/cap-iacs-base#MonthValue"/>
        <rdfs:label xml:lang="en">List of month values</rdfs:label>
        <skos:definition xml:lang="en">-- Definition --
List of months.
-- Description --
List of months.</skos:definition>
    </owl:NamedIndividual>
    


    <!-- http://lpis.ec.europa.eu/registry/applicationschema/cap-iacs-base/code#NotificationGroupValue -->


    <owl:NamedIndividual rdf:about="http://lpis.ec.europa.eu/registry/applicationschema/cap-iacs-base/code#NotificationGroupValue">
        <rdf:type rdf:resource="http://www.w3.org/2004/02/skos/core#ConceptScheme"/>
        <terms:isFormatOf rdf:resource="http://lpis.ec.europa.eu/registry/applicationschema/cap-iacs-base#NotificationGroupValue"/>
        <rdfs:label xml:lang="en">List of notification groups.</rdfs:label>
        <skos:definition xml:lang="en">-- Definition --
List of notification groups.
-- Description --
List of notification groups prescribed in legal documents.
NOTE. Not finite number of notification groups. List may be extended by MS.</skos:definition>
    </owl:NamedIndividual>
    


    <!-- http://lpis.ec.europa.eu/registry/applicationschema/cap-iacs-base/code#OrdinalNumberValue -->


    <owl:NamedIndividual rdf:about="http://lpis.ec.europa.eu/registry/applicationschema/cap-iacs-base/code#OrdinalNumberValue">
        <rdf:type rdf:resource="http://www.w3.org/2004/02/skos/core#ConceptScheme"/>
        <terms:isFormatOf rdf:resource="http://lpis.ec.europa.eu/registry/applicationschema/cap-iacs-base#OrdinalNumberValue"/>
        <rdfs:label xml:lang="en">Ordinal number value list</rdfs:label>
        <skos:definition xml:lang="en">-- Definition --
Ordinal number value list.

-- Description --
List of possible ordinal number values used for date identification.</skos:definition>
    </owl:NamedIndividual>
    


    <!-- http://lpis.ec.europa.eu/registry/applicationschema/cap-iacs-base/code#RecurenceValue -->


    <owl:NamedIndividual rdf:about="http://lpis.ec.europa.eu/registry/applicationschema/cap-iacs-base/code#RecurenceValue">
        <rdf:type rdf:resource="http://www.w3.org/2004/02/skos/core#ConceptScheme"/>
        <terms:isFormatOf rdf:resource="http://lpis.ec.europa.eu/registry/applicationschema/cap-iacs-base#RecurenceValue"/>
        <rdfs:label xml:lang="en">List of recurence values</rdfs:label>
        <skos:definition xml:lang="en">-- Definition --
Notification recurrence value list.
-- Description --
List of possible notification recurrence values.</skos:definition>
    </owl:NamedIndividual>
    


    <!-- http://lpis.ec.europa.eu/registry/applicationschema/cap-iacs-base/code#SpecieCodeValue -->


    <owl:NamedIndividual rdf:about="http://lpis.ec.europa.eu/registry/applicationschema/cap-iacs-base/code#SpecieCodeValue">
        <rdf:type rdf:resource="http://www.w3.org/2004/02/skos/core#ConceptScheme"/>
        <terms:isFormatOf rdf:resource="http://lpis.ec.europa.eu/registry/applicationschema/cap-iacs-base#SpecieCodeValue"/>
        <rdfs:label xml:lang="en">List of vegetable and agricultural plant species</rdfs:label>
        <skos:definition xml:lang="en">-- Definition --
List of vegetable and agricultural plant species (aggregate of a varieties). 
-- Description --
A culture of any of the different genera defined in the botanical classification of crops. In this case code list consist of binomial names of species from the taxonomy of Linnaeus (classification for plants).
NOTE. Common catalogue of varieties of agricultural plant species. Fifth supplement to the 29th complete edition (2011/C 168 A/01)
List of agricultural species -A
I. Beet
II. Fodder plants
III. Oil and fibre plants    
IV. Cereals
V. Potatoes 
NOTE. Common catalogue of varieties of vegetable species. 32nd complete edition (2013/C 312 A/01)
List of vegetable species - H</skos:definition>
    </owl:NamedIndividual>
    


    <!-- http://lpis.ec.europa.eu/registry/applicationschema/cap-iacs-base/code#StatusOfAnomalyValue -->


    <owl:NamedIndividual rdf:about="http://lpis.ec.europa.eu/registry/applicationschema/cap-iacs-base/code#StatusOfAnomalyValue">
        <rdf:type rdf:resource="http://www.w3.org/2004/02/skos/core#ConceptScheme"/>
        <terms:isFormatOf rdf:resource="http://lpis.ec.europa.eu/registry/applicationschema/cap-iacs-base#StatusOfAnomalyValue"/>
        <rdfs:label xml:lang="en">Anomaly status value list</rdfs:label>
        <skos:definition xml:lang="en">--Name--
Status of anomaly value

-- Definition --
Code list of possible anomaly status values.

-- Description --
List of possible anomaly status values used for documentation of anomaly in the information system.

NOTE. Under information system IACS is understood. Most probably anomalies are registered in the Integrated control systems or in the quality assessment leaf of LPIS QA.</skos:definition>
    </owl:NamedIndividual>
    


    <!-- http://lpis.ec.europa.eu/registry/applicationschema/cap-iacs-base/code#StatusOfIssueValue -->


    <owl:NamedIndividual rdf:about="http://lpis.ec.europa.eu/registry/applicationschema/cap-iacs-base/code#StatusOfIssueValue">
        <rdf:type rdf:resource="http://www.w3.org/2004/02/skos/core#ConceptScheme"/>
        <terms:isFormatOf rdf:resource="http://lpis.ec.europa.eu/registry/applicationschema/cap-iacs-base#StatusOfIssueValue"/>
        <rdfs:label xml:lang="en">Issue status value list</rdfs:label>
        <skos:definition xml:lang="en">--Name--
Status of issue value

-- Definition --
Code list of possible issue status values.

-- Description --
List of possible issue status values used for documentation of anomaly in the LPIS.</skos:definition>
    </owl:NamedIndividual>
    


    <!-- http://lpis.ec.europa.eu/registry/applicationschema/cap-iacs-base/code#StatusValue -->


    <owl:NamedIndividual rdf:about="http://lpis.ec.europa.eu/registry/applicationschema/cap-iacs-base/code#StatusValue">
        <rdf:type rdf:resource="http://www.w3.org/2004/02/skos/core#ConceptScheme"/>
        <terms:isFormatOf rdf:resource="http://lpis.ec.europa.eu/registry/applicationschema/cap-iacs-base#StatusValue"/>
        <rdfs:label xml:lang="en">List of status values</rdfs:label>
        <skos:definition xml:lang="en">-- Name--
Status value

--Definition --
Code list of possible status values.

-- Description --
List of status types based on state machine diagrams (Dynamic CAP model) for new and existing object features or schema. The values included in this code list are applicable both to introduction of a new object/feature or to processing a change request.

NOTE. These are generic values applicable in IACS. These concepts have been reused in LPIS upgrade and LPIS update processes.</skos:definition>
    </owl:NamedIndividual>
    


    <!-- http://lpis.ec.europa.eu/registry/applicationschema/cap-iacs-base/code#SupportSchemeTypeValue -->


    <owl:NamedIndividual rdf:about="http://lpis.ec.europa.eu/registry/applicationschema/cap-iacs-base/code#SupportSchemeTypeValue">
        <rdf:type rdf:resource="http://www.w3.org/2004/02/skos/core#ConceptScheme"/>
        <terms:isFormatOf rdf:resource="http://lpis.ec.europa.eu/registry/applicationschema/cap-iacs-base#SupportSchemeTypeValue"/>
        <rdfs:label xml:lang="en">List of support schemas</rdfs:label>
        <skos:definition xml:lang="en">Support scheme type value

List of support schemes as defined in Regulation (EU) 1307/2013.

NOTE
Payment schema type list may be extended or shortened by MS.</skos:definition>
    </owl:NamedIndividual>
    


    <!-- http://lpis.ec.europa.eu/registry/applicationschema/cap-iacs-base/code#TestTypeValue -->


    <owl:NamedIndividual rdf:about="http://lpis.ec.europa.eu/registry/applicationschema/cap-iacs-base/code#TestTypeValue">
        <rdf:type rdf:resource="http://www.w3.org/2004/02/skos/core#ConceptScheme"/>
        <terms:isFormatOf rdf:resource="http://lpis.ec.europa.eu/registry/applicationschema/cap-iacs-base#TestTypeValue"/>
        <rdfs:label xml:lang="en">Test type value list</rdfs:label>
        <skos:definition xml:lang="en">--Name--
Test type value

-- Definition --
Indication whether a test belong to the basic or the capability test type.

-- Description --
A basic test is an initial test intended to identify clear cases of non-conformance. If the ATS identifies tests to be used as basic tests, they shall be used at the start of the conformance assessment process.

Capability test is designed to determine whether an IUT conforms to a particular characteristic specified as requirements.</skos:definition>
    </owl:NamedIndividual>
    


    <!-- http://lpis.ec.europa.eu/registry/applicationschema/cap-iacs-base/code#TestVerdictValue -->


    <owl:NamedIndividual rdf:about="http://lpis.ec.europa.eu/registry/applicationschema/cap-iacs-base/code#TestVerdictValue">
        <rdf:type rdf:resource="http://www.w3.org/2004/02/skos/core#ConceptScheme"/>
        <terms:isFormatOf rdf:resource="http://lpis.ec.europa.eu/registry/applicationschema/cap-iacs-base#TestVerdictValue"/>
        <rdfs:label xml:lang="en">Test verdict value list</rdfs:label>
        <skos:definition xml:lang="en">--Name--
Test verdict value

-- Definition --
List of values describing test verdicts.

-- Description --
List of possible test verdict values according to ISO 19105:2000.</skos:definition>
    </owl:NamedIndividual>
    


    <!-- http://lpis.ec.europa.eu/registry/applicationschema/cap-iacs-base/code#TestingTypeValue -->


    <owl:NamedIndividual rdf:about="http://lpis.ec.europa.eu/registry/applicationschema/cap-iacs-base/code#TestingTypeValue">
        <rdf:type rdf:resource="http://www.w3.org/2004/02/skos/core#ConceptScheme"/>
        <terms:isFormatOf rdf:resource="http://lpis.ec.europa.eu/registry/applicationschema/cap-iacs-base#TestingTypeValue"/>
        <rdfs:label xml:lang="en">Testing type value list</rdfs:label>
        <skos:definition xml:lang="en">--Name--
Testing type value

-- Definition --
Testing type value list.

-- Description --
In manual testing, the specified requirements are verified by a trained operator who follows the steps described in the test method.
In automated testing, specific software is used that operates on the computer readable schema of the eligibility profile.</skos:definition>
    </owl:NamedIndividual>
    


    <!-- http://lpis.ec.europa.eu/registry/applicationschema/cap-iacs-base/code#VarietalNameValue -->


    <owl:NamedIndividual rdf:about="http://lpis.ec.europa.eu/registry/applicationschema/cap-iacs-base/code#VarietalNameValue">
        <rdf:type rdf:resource="http://www.w3.org/2004/02/skos/core#ConceptScheme"/>
        <terms:isFormatOf rdf:resource="http://lpis.ec.europa.eu/registry/applicationschema/cap-iacs-base#VarietalNameValue"/>
        <rdfs:label xml:lang="en">List of varietal names</rdfs:label>
        <skos:definition xml:lang="en">-- Definition --
List of varietal names within vegetable and agricultural plant species. 
-- Desription --
Common catalogue of varieties of agricultural plant species. Fifth supplement to the 29th complete edition (2011/C 168 A/01).
Common catalogue of varieties of vegetable species. 32nd complete edition (2013/C 312 A/01).
This codeList decided and maintained by MS.  Varietal names are MS specific.
Dictionary: http://ec.europa.eu/food/plant/propagation/catalogues/database/public/index.cfm?event=homepage
NOTE. CODE LIST IS NOT FINISHED. ONLY SOME EXAMPLES ARE PROVIDED.</skos:definition>
    </owl:NamedIndividual>
    


    <!-- http://lpis.ec.europa.eu/registry/applicationschema/cap-iacs-base/code#WeekdayValue -->


    <owl:NamedIndividual rdf:about="http://lpis.ec.europa.eu/registry/applicationschema/cap-iacs-base/code#WeekdayValue">
        <rdf:type rdf:resource="http://www.w3.org/2004/02/skos/core#ConceptScheme"/>
        <terms:isFormatOf rdf:resource="http://lpis.ec.europa.eu/registry/applicationschema/cap-iacs-base#WeekdayValue"/>
        <rdfs:label xml:lang="en">List of weekday values</rdfs:label>
        <skos:definition xml:lang="en">-- Definition --
List of possible weekdays.
-- Description --
List of possible weekdays.</skos:definition>
    </owl:NamedIndividual>
    


    <!-- http://lpis.ec.europa.eu/registry/applicationschema/cap-iacs-base/code#AffectedElementTypeValue/applicationSchema -->


    <owl:NamedIndividual rdf:about="http://lpis.ec.europa.eu/registry/applicationschema/cap-iacs-base/code#AffectedElementTypeValue/applicationSchema">
        <rdf:type rdf:resource="http://lpis.ec.europa.eu/registry/applicationschema/cap-iacs-base#AffectedElementTypeValue"/>
        <rdfs:label xml:lang="en">Application schema</rdfs:label>
        <skos:definition xml:lang="en">--Name--
Application schema

-- Definition --
Conceptual schema for data required for one or more applications [ISO 19101:2002].</skos:definition>
        <skos:inScheme rdf:resource="http://lpis.ec.europa.eu/registry/applicationschema/cap-iacs-base/code#AffectedElementTypeValue"/>
    </owl:NamedIndividual>
    


    <!-- http://lpis.ec.europa.eu/registry/applicationschema/cap-iacs-base/code#AffectedElementTypeValue/applicationSchemaLeaf -->


    <owl:NamedIndividual rdf:about="http://lpis.ec.europa.eu/registry/applicationschema/cap-iacs-base/code#AffectedElementTypeValue/applicationSchemaLeaf">
        <rdf:type rdf:resource="http://lpis.ec.europa.eu/registry/applicationschema/cap-iacs-base#AffectedElementTypeValue"/>
        <rdfs:label xml:lang="en">Leaf of application schema</rdfs:label>
        <skos:definition xml:lang="en">--Name--
Application schema leaf

-- Definition --
Specific package within the application schema that cannot include further (sub)packages.</skos:definition>
        <skos:inScheme rdf:resource="http://lpis.ec.europa.eu/registry/applicationschema/cap-iacs-base/code#AffectedElementTypeValue"/>
    </owl:NamedIndividual>
    


    <!-- http://lpis.ec.europa.eu/registry/applicationschema/cap-iacs-base/code#AffectedElementTypeValue/associationRole -->


    <owl:NamedIndividual rdf:about="http://lpis.ec.europa.eu/registry/applicationschema/cap-iacs-base/code#AffectedElementTypeValue/associationRole">
        <rdf:type rdf:resource="http://lpis.ec.europa.eu/registry/applicationschema/cap-iacs-base#AffectedElementTypeValue"/>
        <rdfs:label xml:lang="en">Relationship</rdfs:label>
        <skos:definition xml:lang="en">--Name--
Association role

-- Definition --
Semantic relationship that can occur between type instances [ISO 19103:2005]</skos:definition>
        <skos:inScheme rdf:resource="http://lpis.ec.europa.eu/registry/applicationschema/cap-iacs-base/code#AffectedElementTypeValue"/>
    </owl:NamedIndividual>
    


    <!-- http://lpis.ec.europa.eu/registry/applicationschema/cap-iacs-base/code#AffectedElementTypeValue/attribute -->


    <owl:NamedIndividual rdf:about="http://lpis.ec.europa.eu/registry/applicationschema/cap-iacs-base/code#AffectedElementTypeValue/attribute">
        <rdf:type rdf:resource="http://lpis.ec.europa.eu/registry/applicationschema/cap-iacs-base#AffectedElementTypeValue"/>
        <rdfs:label xml:lang="en">Property</rdfs:label>
        <skos:definition xml:lang="en">--Name--
Attribute

-- Definition --
UML feature  within a classifier that describes a range of values (B.515) that instances of the classifier may hold. [ISO/TS 19103:2005 – adapted from ISO/IEC 19501]</skos:definition>
        <skos:inScheme rdf:resource="http://lpis.ec.europa.eu/registry/applicationschema/cap-iacs-base/code#AffectedElementTypeValue"/>
    </owl:NamedIndividual>
    


    <!-- http://lpis.ec.europa.eu/registry/applicationschema/cap-iacs-base/code#AffectedElementTypeValue/codeList -->


    <owl:NamedIndividual rdf:about="http://lpis.ec.europa.eu/registry/applicationschema/cap-iacs-base/code#AffectedElementTypeValue/codeList">
        <rdf:type rdf:resource="http://lpis.ec.europa.eu/registry/applicationschema/cap-iacs-base#AffectedElementTypeValue"/>
        <rdfs:label xml:lang="en">Code list</rdfs:label>
        <skos:definition xml:lang="en">--Name--
Code list

-- Definition --
Set of pre-defined values that an attribute may take.</skos:definition>
        <skos:inScheme rdf:resource="http://lpis.ec.europa.eu/registry/applicationschema/cap-iacs-base/code#AffectedElementTypeValue"/>
    </owl:NamedIndividual>
    


    <!-- http://lpis.ec.europa.eu/registry/applicationschema/cap-iacs-base/code#AffectedElementTypeValue/dataType -->


    <owl:NamedIndividual rdf:about="http://lpis.ec.europa.eu/registry/applicationschema/cap-iacs-base/code#AffectedElementTypeValue/dataType">
        <rdf:type rdf:resource="http://lpis.ec.europa.eu/registry/applicationschema/cap-iacs-base#AffectedElementTypeValue"/>
        <rdfs:label xml:lang="en">Data type</rdfs:label>
        <skos:definition xml:lang="en">--Name--
Data type

-- Definition --
Specification of a value domain with operations allowed on values in this domain [ISO 19103:2005].

-- Description --
For purposes of LCM, this term is used for proprietary (user-defined) and imported (from third parties) data types.</skos:definition>
        <skos:inScheme rdf:resource="http://lpis.ec.europa.eu/registry/applicationschema/cap-iacs-base/code#AffectedElementTypeValue"/>
    </owl:NamedIndividual>
    


    <!-- http://lpis.ec.europa.eu/registry/applicationschema/cap-iacs-base/code#AffectedElementTypeValue/featureType -->


    <owl:NamedIndividual rdf:about="http://lpis.ec.europa.eu/registry/applicationschema/cap-iacs-base/code#AffectedElementTypeValue/featureType">
        <rdf:type rdf:resource="http://lpis.ec.europa.eu/registry/applicationschema/cap-iacs-base#AffectedElementTypeValue"/>
        <rdfs:label xml:lang="en">Feature type</rdfs:label>
        <skos:definition xml:lang="en">--Name--
Feature type

-- Definition --
A class that specifies set of spatial objects sharing common properties and operations applicable to the objects.</skos:definition>
        <skos:inScheme rdf:resource="http://lpis.ec.europa.eu/registry/applicationschema/cap-iacs-base/code#AffectedElementTypeValue"/>
    </owl:NamedIndividual>
    


    <!-- http://lpis.ec.europa.eu/registry/applicationschema/cap-iacs-base/code#AffectedElementTypeValue/multiplicity -->


    <owl:NamedIndividual rdf:about="http://lpis.ec.europa.eu/registry/applicationschema/cap-iacs-base/code#AffectedElementTypeValue/multiplicity">
        <rdf:type rdf:resource="http://lpis.ec.europa.eu/registry/applicationschema/cap-iacs-base#AffectedElementTypeValue"/>
        <rdfs:label xml:lang="en">Enumeration</rdfs:label>
        <skos:definition xml:lang="en">--Name--
Multiplicity

-- Definition --
Specification of the range of allowable cardinalities that a set may assume.</skos:definition>
        <skos:inScheme rdf:resource="http://lpis.ec.europa.eu/registry/applicationschema/cap-iacs-base/code#AffectedElementTypeValue"/>
    </owl:NamedIndividual>
    


    <!-- http://lpis.ec.europa.eu/registry/applicationschema/cap-iacs-base/code#AffectedElementTypeValue/ocl -->


    <owl:NamedIndividual rdf:about="http://lpis.ec.europa.eu/registry/applicationschema/cap-iacs-base/code#AffectedElementTypeValue/ocl">
        <rdf:type rdf:resource="http://lpis.ec.europa.eu/registry/applicationschema/cap-iacs-base#AffectedElementTypeValue"/>
        <rdfs:label xml:lang="en">OCL</rdfs:label>
        <skos:definition xml:lang="en">--Name--
OCL

-- Definition --
The Object Constraint Language (OCL) is a declarative language for describing rules that apply to Unified Modelling Language (UML) models.</skos:definition>
        <skos:inScheme rdf:resource="http://lpis.ec.europa.eu/registry/applicationschema/cap-iacs-base/code#AffectedElementTypeValue"/>
    </owl:NamedIndividual>
    


    <!-- http://lpis.ec.europa.eu/registry/applicationschema/cap-iacs-base/code#AffectedElementTypeValue/type -->


    <owl:NamedIndividual rdf:about="http://lpis.ec.europa.eu/registry/applicationschema/cap-iacs-base/code#AffectedElementTypeValue/type">
        <rdf:type rdf:resource="http://lpis.ec.europa.eu/registry/applicationschema/cap-iacs-base#AffectedElementTypeValue"/>
        <rdfs:label xml:lang="en">Type</rdfs:label>
        <skos:definition xml:lang="en">--Name--
Type

-- Definition --
Specification of a value domain [ISO 19103:2005].

-- Description --
Types include data types, enumerated types, code list values, etc.

EXAMPLE 1. Primitive types defined in international standards: integer, boolean, GM_Object, etc.

EXAMPLE 2. Own types defined in the model and re-used for different purposes. LPIS QA uses the TechnicalReasonValue type to describe critical defects and contaminations with the same technical terms.

EXAMPLE 3. Types defined in other model and imported for re-use. LCM uses  DocumentCitation type defined in INSPIRE.</skos:definition>
        <skos:inScheme rdf:resource="http://lpis.ec.europa.eu/registry/applicationschema/cap-iacs-base/code#AffectedElementTypeValue"/>
    </owl:NamedIndividual>
    


    <!-- http://lpis.ec.europa.eu/registry/applicationschema/cap-iacs-base/code#AffectedElementTypeValue/union -->


    <owl:NamedIndividual rdf:about="http://lpis.ec.europa.eu/registry/applicationschema/cap-iacs-base/code#AffectedElementTypeValue/union">
        <rdf:type rdf:resource="http://lpis.ec.europa.eu/registry/applicationschema/cap-iacs-base#AffectedElementTypeValue"/>
        <rdfs:label xml:lang="en">Union</rdfs:label>
        <skos:definition xml:lang="en">--Name--
Union

-- Definition --
A class, which defines a collection of Simple Types defined in ISO 19103:2005.</skos:definition>
        <skos:inScheme rdf:resource="http://lpis.ec.europa.eu/registry/applicationschema/cap-iacs-base/code#AffectedElementTypeValue"/>
    </owl:NamedIndividual>
    


    <!-- http://lpis.ec.europa.eu/registry/applicationschema/cap-iacs-base/code#CauseOfAnomalyValue/appearanceOfPermanentConstruction -->


    <owl:NamedIndividual rdf:about="http://lpis.ec.europa.eu/registry/applicationschema/cap-iacs-base/code#CauseOfAnomalyValue/appearanceOfPermanentConstruction">
        <rdf:type rdf:resource="http://lpis.ec.europa.eu/registry/applicationschema/cap-iacs-base#CauseOfAnomalyValue"/>
        <rdfs:label xml:lang="en">Cause flaged as Type II. The appearance of permanent construction</rdfs:label>
        <skos:definition xml:lang="en">--Name--
Appearance of permanent construction

-- Description --
The appearance of buildings, roads, and other sealed surfaces that are likely to stay in the place of former agricultural land more than three years.</skos:definition>
        <skos:inScheme rdf:resource="http://lpis.ec.europa.eu/registry/applicationschema/cap-iacs-base/code#CauseOfAnomalyValue"/>
    </owl:NamedIndividual>
    


    <!-- http://lpis.ec.europa.eu/registry/applicationschema/cap-iacs-base/code#CauseOfAnomalyValue/causeUnknown -->


    <owl:NamedIndividual rdf:about="http://lpis.ec.europa.eu/registry/applicationschema/cap-iacs-base/code#CauseOfAnomalyValue/causeUnknown">
        <rdf:type rdf:resource="http://lpis.ec.europa.eu/registry/applicationschema/cap-iacs-base#CauseOfAnomalyValue"/>
        <rdfs:label xml:lang="en">The cause is flagged as unknown</rdfs:label>
        <skos:definition xml:lang="en">--Name--
Cause unknown

-- Description --
No case can be detected and/or no third party information is available about the possible cause of anomaly.</skos:definition>
        <skos:inScheme rdf:resource="http://lpis.ec.europa.eu/registry/applicationschema/cap-iacs-base/code#CauseOfAnomalyValue"/>
    </owl:NamedIndividual>
    


    <!-- http://lpis.ec.europa.eu/registry/applicationschema/cap-iacs-base/code#CauseOfAnomalyValue/changeInThePerimeterAdditionOfAgriculturalLand -->


    <owl:NamedIndividual rdf:about="http://lpis.ec.europa.eu/registry/applicationschema/cap-iacs-base/code#CauseOfAnomalyValue/changeInThePerimeterAdditionOfAgriculturalLand">
        <rdf:type rdf:resource="http://lpis.ec.europa.eu/registry/applicationschema/cap-iacs-base#CauseOfAnomalyValue"/>
        <rdfs:label xml:lang="en">Cause flaged as Type III. Change in the perimeter (addition of agricultural land)</rdfs:label>
        <skos:definition xml:lang="en">--Name--
Change in the perimeter due to addition of agricultural land

-- Description --
New agricultural area has been appended to an existing reference parcel.

NOTE. Previously known as Type III anomaly.</skos:definition>
        <skos:inScheme rdf:resource="http://lpis.ec.europa.eu/registry/applicationschema/cap-iacs-base/code#CauseOfAnomalyValue"/>
    </owl:NamedIndividual>
    


    <!-- http://lpis.ec.europa.eu/registry/applicationschema/cap-iacs-base/code#CauseOfAnomalyValue/changeInThePerimeterExchangeOfAgriculturalLand -->


    <owl:NamedIndividual rdf:about="http://lpis.ec.europa.eu/registry/applicationschema/cap-iacs-base/code#CauseOfAnomalyValue/changeInThePerimeterExchangeOfAgriculturalLand">
        <rdf:type rdf:resource="http://lpis.ec.europa.eu/registry/applicationschema/cap-iacs-base#CauseOfAnomalyValue"/>
        <rdfs:label xml:lang="en">Cause flaged as Type IV. Change in the perimeter (exchange of agricultural land)</rdfs:label>
        <skos:definition xml:lang="en">--Name--
Change in the perimeter due to exchange of agricultural land

-- Description --
The minimum number of involved parcels is two. The anomaly is manifested by a change of their shape and area.

NOTE. Previously this cause was flagged as Type IV anomaly.</skos:definition>
        <skos:inScheme rdf:resource="http://lpis.ec.europa.eu/registry/applicationschema/cap-iacs-base/code#CauseOfAnomalyValue"/>
    </owl:NamedIndividual>
    


    <!-- http://lpis.ec.europa.eu/registry/applicationschema/cap-iacs-base/code#CauseOfAnomalyValue/irreversibleConversionsOfAgriculturalLandCovers -->


    <owl:NamedIndividual rdf:about="http://lpis.ec.europa.eu/registry/applicationschema/cap-iacs-base/code#CauseOfAnomalyValue/irreversibleConversionsOfAgriculturalLandCovers">
        <rdf:type rdf:resource="http://lpis.ec.europa.eu/registry/applicationschema/cap-iacs-base#CauseOfAnomalyValue"/>
        <rdfs:label xml:lang="en">Cause flaged as Type I. Irreversible conversions of agricultural land covers</rdfs:label>
        <skos:definition xml:lang="en">--Name--
Irreversible conversion of agricultural land covers

-- Description --
Appearance of forests, deserted areas, rock outcrops, inundated areas, etc. in the place of former agricultural land.</skos:definition>
        <skos:inScheme rdf:resource="http://lpis.ec.europa.eu/registry/applicationschema/cap-iacs-base/code#CauseOfAnomalyValue"/>
    </owl:NamedIndividual>
    


    <!-- http://lpis.ec.europa.eu/registry/applicationschema/cap-iacs-base/code#CauseOfAnomalyValue/misclassifiedProrataClass -->


    <owl:NamedIndividual rdf:about="http://lpis.ec.europa.eu/registry/applicationschema/cap-iacs-base/code#CauseOfAnomalyValue/misclassifiedProrataClass">
        <rdf:type rdf:resource="http://lpis.ec.europa.eu/registry/applicationschema/cap-iacs-base#CauseOfAnomalyValue"/>
        <skos:inScheme rdf:resource="http://lpis.ec.europa.eu/registry/applicationschema/cap-iacs-base/code#CauseOfAnomalyValue"/>
    </owl:NamedIndividual>
    


    <!-- http://lpis.ec.europa.eu/registry/applicationschema/cap-iacs-base/code#CauseOfAnomalyValue/notConfirmed -->


    <owl:NamedIndividual rdf:about="http://lpis.ec.europa.eu/registry/applicationschema/cap-iacs-base/code#CauseOfAnomalyValue/notConfirmed">
        <rdf:type rdf:resource="http://lpis.ec.europa.eu/registry/applicationschema/cap-iacs-base#CauseOfAnomalyValue"/>
        <rdfs:label xml:lang="en">Cause flagged as no change in the data</rdfs:label>
        <skos:definition xml:lang="en">--Name--
Not confirmed

-- Description--
The preliminary classification of the anomaly cause cannot be confirmed.</skos:definition>
        <skos:inScheme rdf:resource="http://lpis.ec.europa.eu/registry/applicationschema/cap-iacs-base/code#CauseOfAnomalyValue"/>
    </owl:NamedIndividual>
    


    <!-- http://lpis.ec.europa.eu/registry/applicationschema/cap-iacs-base/code#ConformanceClassValue/classA -->


    <owl:NamedIndividual rdf:about="http://lpis.ec.europa.eu/registry/applicationschema/cap-iacs-base/code#ConformanceClassValue/classA">
        <rdf:type rdf:resource="http://lpis.ec.europa.eu/registry/applicationschema/cap-iacs-base#ConformanceClassValue"/>
        <rdfs:label xml:lang="en">Class A</rdfs:label>
        <skos:definition xml:lang="en">--Name--
Class A

--Definition--
Specified conformance class.

--Description--
Separate ATS must be provided if a class is defined within ConformanceClause.</skos:definition>
        <skos:inScheme rdf:resource="http://lpis.ec.europa.eu/registry/applicationschema/cap-iacs-base/code#ConformanceClassValue"/>
    </owl:NamedIndividual>
    


    <!-- http://lpis.ec.europa.eu/registry/applicationschema/cap-iacs-base/code#ConformanceClassValue/classB -->


    <owl:NamedIndividual rdf:about="http://lpis.ec.europa.eu/registry/applicationschema/cap-iacs-base/code#ConformanceClassValue/classB">
        <rdf:type rdf:resource="http://lpis.ec.europa.eu/registry/applicationschema/cap-iacs-base#ConformanceClassValue"/>
        <rdfs:label xml:lang="en">Class B</rdfs:label>
        <skos:definition xml:lang="en">--Name--
Class B

--Definition--
Specified conformance class.

--Description--
Separate ATS must be provided if a class is defined within ConformanceClause</skos:definition>
        <skos:inScheme rdf:resource="http://lpis.ec.europa.eu/registry/applicationschema/cap-iacs-base/code#ConformanceClassValue"/>
    </owl:NamedIndividual>
    


    <!-- http://lpis.ec.europa.eu/registry/applicationschema/cap-iacs-base/code#ConformanceClassValue/classC -->


    <owl:NamedIndividual rdf:about="http://lpis.ec.europa.eu/registry/applicationschema/cap-iacs-base/code#ConformanceClassValue/classC">
        <rdf:type rdf:resource="http://lpis.ec.europa.eu/registry/applicationschema/cap-iacs-base#ConformanceClassValue"/>
        <rdfs:label xml:lang="en">Class C</rdfs:label>
        <skos:definition xml:lang="en">--Name--
Class C

--Definition--
Specified conformance class.

--Description--
Separate ATS must be provided if a class is defined within ConformanceClause.</skos:definition>
        <skos:inScheme rdf:resource="http://lpis.ec.europa.eu/registry/applicationschema/cap-iacs-base/code#ConformanceClassValue"/>
    </owl:NamedIndividual>
    


    <!-- http://lpis.ec.europa.eu/registry/applicationschema/cap-iacs-base/code#ConformanceLevelValue/level1 -->


    <owl:NamedIndividual rdf:about="http://lpis.ec.europa.eu/registry/applicationschema/cap-iacs-base/code#ConformanceLevelValue/level1">
        <rdf:type rdf:resource="http://lpis.ec.europa.eu/registry/applicationschema/cap-iacs-base#ConformanceLevelValue"/>
        <rdfs:label xml:lang="en">Level 1 low</rdfs:label>
        <skos:definition xml:lang="en">--Name--
Level 1

--Definition--
Lowest level conformance.

--Description--
A separate abstract test suite must be provided if a level is defined within ConformanceClause.</skos:definition>
        <skos:inScheme rdf:resource="http://lpis.ec.europa.eu/registry/applicationschema/cap-iacs-base/code#ConformanceLevelValue"/>
    </owl:NamedIndividual>
    


    <!-- http://lpis.ec.europa.eu/registry/applicationschema/cap-iacs-base/code#ConformanceLevelValue/level2 -->


    <owl:NamedIndividual rdf:about="http://lpis.ec.europa.eu/registry/applicationschema/cap-iacs-base/code#ConformanceLevelValue/level2">
        <rdf:type rdf:resource="http://lpis.ec.europa.eu/registry/applicationschema/cap-iacs-base#ConformanceLevelValue"/>
        <rdfs:label xml:lang="en">Level 2 medium</rdfs:label>
        <skos:definition xml:lang="en">--Name--
Level 2

--Definition--
Lowest level conformance.

--Description--
A separate abstract test suite must be provided if a level is defined within ConformanceClause.</skos:definition>
        <skos:inScheme rdf:resource="http://lpis.ec.europa.eu/registry/applicationschema/cap-iacs-base/code#ConformanceLevelValue"/>
    </owl:NamedIndividual>
    


    <!-- http://lpis.ec.europa.eu/registry/applicationschema/cap-iacs-base/code#ConformanceLevelValue/level3 -->


    <owl:NamedIndividual rdf:about="http://lpis.ec.europa.eu/registry/applicationschema/cap-iacs-base/code#ConformanceLevelValue/level3">
        <rdf:type rdf:resource="http://lpis.ec.europa.eu/registry/applicationschema/cap-iacs-base#ConformanceLevelValue"/>
        <rdfs:label xml:lang="en">Level 3 high</rdfs:label>
        <skos:definition xml:lang="en">--Name--
Level 3

--Definition--
Highest level conformance.

--Description--
A separate abstract test suite must be provided if a level is defined within ConformanceClause.</skos:definition>
        <skos:inScheme rdf:resource="http://lpis.ec.europa.eu/registry/applicationschema/cap-iacs-base/code#ConformanceLevelValue"/>
    </owl:NamedIndividual>
    


    <!-- http://lpis.ec.europa.eu/registry/applicationschema/cap-iacs-base/code#ConformanceRequirementClassValue/conditional -->


    <owl:NamedIndividual rdf:about="http://lpis.ec.europa.eu/registry/applicationschema/cap-iacs-base/code#ConformanceRequirementClassValue/conditional">
        <rdf:type rdf:resource="http://lpis.ec.europa.eu/registry/applicationschema/cap-iacs-base#ConformanceRequirementClassValue"/>
        <rdfs:label xml:lang="en">Conditional requirement</rdfs:label>
        <skos:definition xml:lang="en">--Name--
Conditional

--Definition--
Requirement that shall be observed if the conditions set out in the specification apply.</skos:definition>
        <skos:inScheme rdf:resource="http://lpis.ec.europa.eu/registry/applicationschema/cap-iacs-base/code#ConformanceRequirementClassValue"/>
    </owl:NamedIndividual>
    


    <!-- http://lpis.ec.europa.eu/registry/applicationschema/cap-iacs-base/code#ConformanceRequirementClassValue/mandatory -->


    <owl:NamedIndividual rdf:about="http://lpis.ec.europa.eu/registry/applicationschema/cap-iacs-base/code#ConformanceRequirementClassValue/mandatory">
        <rdf:type rdf:resource="http://lpis.ec.europa.eu/registry/applicationschema/cap-iacs-base#ConformanceRequirementClassValue"/>
        <rdfs:label xml:lang="en">Mandatory requirement</rdfs:label>
        <skos:definition xml:lang="en">--Name--
Mandatory

--Definition--
Requirement that shall be observed in all cases. 

--Description--
This has to be fulfilled for conformance.</skos:definition>
        <skos:inScheme rdf:resource="http://lpis.ec.europa.eu/registry/applicationschema/cap-iacs-base/code#ConformanceRequirementClassValue"/>
    </owl:NamedIndividual>
    


    <!-- http://lpis.ec.europa.eu/registry/applicationschema/cap-iacs-base/code#ConformanceRequirementClassValue/optional -->


    <owl:NamedIndividual rdf:about="http://lpis.ec.europa.eu/registry/applicationschema/cap-iacs-base/code#ConformanceRequirementClassValue/optional">
        <rdf:type rdf:resource="http://lpis.ec.europa.eu/registry/applicationschema/cap-iacs-base#ConformanceRequirementClassValue"/>
        <rdfs:label xml:lang="en">Optional requirement</rdfs:label>
        <skos:definition xml:lang="en">--Name--
Optional

--Definition--
Requirement that may be selected to suit the implementation, provided that any condition applicable to the option are observed.</skos:definition>
        <skos:inScheme rdf:resource="http://lpis.ec.europa.eu/registry/applicationschema/cap-iacs-base/code#ConformanceRequirementClassValue"/>
    </owl:NamedIndividual>
    


    <!-- http://lpis.ec.europa.eu/registry/applicationschema/cap-iacs-base/code#ConformanceRequirementStatementValue/negative -->


    <owl:NamedIndividual rdf:about="http://lpis.ec.europa.eu/registry/applicationschema/cap-iacs-base/code#ConformanceRequirementStatementValue/negative">
        <rdf:type rdf:resource="http://lpis.ec.europa.eu/registry/applicationschema/cap-iacs-base#ConformanceRequirementStatementValue"/>
        <rdfs:label xml:lang="en">Negative statement</rdfs:label>
        <skos:definition xml:lang="en">--Name--
Negative

--Definition--
Negative statement.

--Description--
Negative statement state what is required not to be observed.</skos:definition>
        <skos:inScheme rdf:resource="http://lpis.ec.europa.eu/registry/applicationschema/cap-iacs-base/code#ConformanceRequirementStatementValue"/>
    </owl:NamedIndividual>
    


    <!-- http://lpis.ec.europa.eu/registry/applicationschema/cap-iacs-base/code#ConformanceRequirementStatementValue/positive -->


    <owl:NamedIndividual rdf:about="http://lpis.ec.europa.eu/registry/applicationschema/cap-iacs-base/code#ConformanceRequirementStatementValue/positive">
        <rdf:type rdf:resource="http://lpis.ec.europa.eu/registry/applicationschema/cap-iacs-base#ConformanceRequirementStatementValue"/>
        <rdfs:label xml:lang="en">Positive statement</rdfs:label>
        <skos:definition xml:lang="en">--Name--
Positive

--Definition--
Affirmative statement.

--Description--
Positive statement state what is required to be done.</skos:definition>
        <skos:inScheme rdf:resource="http://lpis.ec.europa.eu/registry/applicationschema/cap-iacs-base/code#ConformanceRequirementStatementValue"/>
    </owl:NamedIndividual>
    


    <!-- http://lpis.ec.europa.eu/registry/applicationschema/cap-iacs-base/code#ConformanceStatementValue/conforming -->


    <owl:NamedIndividual rdf:about="http://lpis.ec.europa.eu/registry/applicationschema/cap-iacs-base/code#ConformanceStatementValue/conforming">
        <rdf:type rdf:resource="http://lpis.ec.europa.eu/registry/applicationschema/cap-iacs-base#ConformanceStatementValue"/>
        <rdfs:label xml:lang="en">Confroming</rdfs:label>
        <skos:definition xml:lang="en">-- Name--
Conforming

-- Description --
The tested object complies with rules, standards, or laws.</skos:definition>
        <skos:inScheme rdf:resource="http://lpis.ec.europa.eu/registry/applicationschema/cap-iacs-base/code#ConformanceStatementValue"/>
    </owl:NamedIndividual>
    


    <!-- http://lpis.ec.europa.eu/registry/applicationschema/cap-iacs-base/code#ConformanceStatementValue/nonConforming -->


    <owl:NamedIndividual rdf:about="http://lpis.ec.europa.eu/registry/applicationschema/cap-iacs-base/code#ConformanceStatementValue/nonConforming">
        <rdf:type rdf:resource="http://lpis.ec.europa.eu/registry/applicationschema/cap-iacs-base#ConformanceStatementValue"/>
        <rdfs:label xml:lang="en">Non-conforming</rdfs:label>
        <skos:definition xml:lang="en">-- Name--
Non-conforming

-- Description --
The tested object does not comply with rules, standards, or laws.</skos:definition>
        <skos:inScheme rdf:resource="http://lpis.ec.europa.eu/registry/applicationschema/cap-iacs-base/code#ConformanceStatementValue"/>
    </owl:NamedIndividual>
    


    <!-- http://lpis.ec.europa.eu/registry/applicationschema/cap-iacs-base/code#CropItemCodeValue/almonds -->


    <owl:NamedIndividual rdf:about="http://lpis.ec.europa.eu/registry/applicationschema/cap-iacs-base/code#CropItemCodeValue/almonds">
        <rdf:type rdf:resource="http://lpis.ec.europa.eu/registry/applicationschema/cap-iacs-base#CropItemCodeValue"/>
        <rdfs:label xml:lang="en">Almonds</rdfs:label>
        <skos:definition xml:lang="en">-- Definition --
|||Almonds.
-- Description --
Cereals and main crops - C
NOTE. Initial value:C2233</skos:definition>
        <skos:inScheme rdf:resource="http://lpis.ec.europa.eu/registry/applicationschema/cap-iacs-base/code#CropItemCodeValue"/>
    </owl:NamedIndividual>
    


    <!-- http://lpis.ec.europa.eu/registry/applicationschema/cap-iacs-base/code#CropItemCodeValue/annualPlantsHarvestedGreenC2611 -->


    <owl:NamedIndividual rdf:about="http://lpis.ec.europa.eu/registry/applicationschema/cap-iacs-base/code#CropItemCodeValue/annualPlantsHarvestedGreenC2611">
        <rdf:type rdf:resource="http://lpis.ec.europa.eu/registry/applicationschema/cap-iacs-base#CropItemCodeValue"/>
        <rdfs:label xml:lang="en">Annual plants harvested green C2611</rdfs:label>
        <skos:definition xml:lang="en">-- Definition --
||Annual plants harvested green C2611.
-- Description --
Cereals and main crops - C
NOTE. Initial value:C2611</skos:definition>
        <skos:inScheme rdf:resource="http://lpis.ec.europa.eu/registry/applicationschema/cap-iacs-base/code#CropItemCodeValue"/>
    </owl:NamedIndividual>
    


    <!-- http://lpis.ec.europa.eu/registry/applicationschema/cap-iacs-base/code#CropItemCodeValue/apples -->


    <owl:NamedIndividual rdf:about="http://lpis.ec.europa.eu/registry/applicationschema/cap-iacs-base/code#CropItemCodeValue/apples">
        <rdf:type rdf:resource="http://lpis.ec.europa.eu/registry/applicationschema/cap-iacs-base#CropItemCodeValue"/>
        <rdfs:label xml:lang="en">Apples</rdfs:label>
        <skos:definition xml:lang="en">-- Definition --
||Apples.
-- Description --
Cereals and main crops - C
NOTE. Initial value:C2090</skos:definition>
        <skos:inScheme rdf:resource="http://lpis.ec.europa.eu/registry/applicationschema/cap-iacs-base/code#CropItemCodeValue"/>
    </owl:NamedIndividual>
    


    <!-- http://lpis.ec.europa.eu/registry/applicationschema/cap-iacs-base/code#CropItemCodeValue/applesForFreshConsumption -->


    <owl:NamedIndividual rdf:about="http://lpis.ec.europa.eu/registry/applicationschema/cap-iacs-base/code#CropItemCodeValue/applesForFreshConsumption">
        <rdf:type rdf:resource="http://lpis.ec.europa.eu/registry/applicationschema/cap-iacs-base#CropItemCodeValue"/>
        <rdfs:label xml:lang="en">Apples for fresh consumption</rdfs:label>
        <skos:definition xml:lang="en">-- Definition --
|||Apples for fresh consumption.
-- Description --
Cereals and main crops - C
NOTE. Initial value:C2110</skos:definition>
        <skos:inScheme rdf:resource="http://lpis.ec.europa.eu/registry/applicationschema/cap-iacs-base/code#CropItemCodeValue"/>
    </owl:NamedIndividual>
    


    <!-- http://lpis.ec.europa.eu/registry/applicationschema/cap-iacs-base/code#CropItemCodeValue/apricots -->


    <owl:NamedIndividual rdf:about="http://lpis.ec.europa.eu/registry/applicationschema/cap-iacs-base/code#CropItemCodeValue/apricots">
        <rdf:type rdf:resource="http://lpis.ec.europa.eu/registry/applicationschema/cap-iacs-base#CropItemCodeValue"/>
        <rdfs:label xml:lang="en">Apricots</rdfs:label>
        <skos:definition xml:lang="en">-- Definition --
|||Apricots.
-- Description --
Cereals and main crops - C
NOTE. Initial value:C2190</skos:definition>
        <skos:inScheme rdf:resource="http://lpis.ec.europa.eu/registry/applicationschema/cap-iacs-base/code#CropItemCodeValue"/>
    </owl:NamedIndividual>
    


    <!-- http://lpis.ec.europa.eu/registry/applicationschema/cap-iacs-base/code#CropItemCodeValue/arableLand -->


    <owl:NamedIndividual rdf:about="http://lpis.ec.europa.eu/registry/applicationschema/cap-iacs-base/code#CropItemCodeValue/arableLand">
        <rdf:type rdf:resource="http://lpis.ec.europa.eu/registry/applicationschema/cap-iacs-base#CropItemCodeValue"/>
        <rdfs:label xml:lang="en">Arable land</rdfs:label>
        <skos:definition xml:lang="en">-- Definition --
||Arable land.
-- Description --
Land use of Agriculture Area in Use -L
NOTE. Initial value:L0001</skos:definition>
        <skos:inScheme rdf:resource="http://lpis.ec.europa.eu/registry/applicationschema/cap-iacs-base/code#CropItemCodeValue"/>
    </owl:NamedIndividual>
    


    <!-- http://lpis.ec.europa.eu/registry/applicationschema/cap-iacs-base/code#CropItemCodeValue/aromaticPlantsMedicinalAndCulinaryPlants -->


    <owl:NamedIndividual rdf:about="http://lpis.ec.europa.eu/registry/applicationschema/cap-iacs-base/code#CropItemCodeValue/aromaticPlantsMedicinalAndCulinaryPlants">
        <rdf:type rdf:resource="http://lpis.ec.europa.eu/registry/applicationschema/cap-iacs-base#CropItemCodeValue"/>
        <rdfs:label xml:lang="en">Aromatic plants, medicinal and culinary plants</rdfs:label>
        <skos:definition xml:lang="en">-- Definition --
|||Aromatic plants, medicinal and culinary plants.
-- Description --
Cereals and main crops - C
NOTE. Initial value:C1580</skos:definition>
        <skos:inScheme rdf:resource="http://lpis.ec.europa.eu/registry/applicationschema/cap-iacs-base/code#CropItemCodeValue"/>
    </owl:NamedIndividual>
    


    <!-- http://lpis.ec.europa.eu/registry/applicationschema/cap-iacs-base/code#CropItemCodeValue/artichokes -->


    <owl:NamedIndividual rdf:about="http://lpis.ec.europa.eu/registry/applicationschema/cap-iacs-base/code#CropItemCodeValue/artichokes">
        <rdf:type rdf:resource="http://lpis.ec.europa.eu/registry/applicationschema/cap-iacs-base#CropItemCodeValue"/>
        <rdfs:label xml:lang="en">Artichokes</rdfs:label>
        <skos:definition xml:lang="en">-- Definition --
|||Artichokes.
-- Description --
Cereals and main crops - C
NOTE. Initial value:C1720</skos:definition>
        <skos:inScheme rdf:resource="http://lpis.ec.europa.eu/registry/applicationschema/cap-iacs-base/code#CropItemCodeValue"/>
    </owl:NamedIndividual>
    


    <!-- http://lpis.ec.europa.eu/registry/applicationschema/cap-iacs-base/code#CropItemCodeValue/asparagus -->


    <owl:NamedIndividual rdf:about="http://lpis.ec.europa.eu/registry/applicationschema/cap-iacs-base/code#CropItemCodeValue/asparagus">
        <rdf:type rdf:resource="http://lpis.ec.europa.eu/registry/applicationschema/cap-iacs-base#CropItemCodeValue"/>
        <rdfs:label xml:lang="en">Asparagus</rdfs:label>
        <skos:definition xml:lang="en">-- Definition --
|||Asparagus.
-- Description --
Cereals and main crops - C
NOTE. Initial value:C1700</skos:definition>
        <skos:inScheme rdf:resource="http://lpis.ec.europa.eu/registry/applicationschema/cap-iacs-base/code#CropItemCodeValue"/>
    </owl:NamedIndividual>
    


    <!-- http://lpis.ec.europa.eu/registry/applicationschema/cap-iacs-base/code#CropItemCodeValue/avocados -->


    <owl:NamedIndividual rdf:about="http://lpis.ec.europa.eu/registry/applicationschema/cap-iacs-base/code#CropItemCodeValue/avocados">
        <rdf:type rdf:resource="http://lpis.ec.europa.eu/registry/applicationschema/cap-iacs-base#CropItemCodeValue"/>
        <rdfs:label xml:lang="en">Avocados</rdfs:label>
        <skos:definition xml:lang="en">-- Definition --
|||Avocados.
-- Description --
Cereals and main crops - C
NOTE. Initial value:C2253</skos:definition>
        <skos:inScheme rdf:resource="http://lpis.ec.europa.eu/registry/applicationschema/cap-iacs-base/code#CropItemCodeValue"/>
    </owl:NamedIndividual>
    


    <!-- http://lpis.ec.europa.eu/registry/applicationschema/cap-iacs-base/code#CropItemCodeValue/bananas -->


    <owl:NamedIndividual rdf:about="http://lpis.ec.europa.eu/registry/applicationschema/cap-iacs-base/code#CropItemCodeValue/bananas">
        <rdf:type rdf:resource="http://lpis.ec.europa.eu/registry/applicationschema/cap-iacs-base#CropItemCodeValue"/>
        <rdfs:label xml:lang="en">Bananas</rdfs:label>
        <skos:definition xml:lang="en">-- Definition --
|||Bananas.
-- Description --
Cereals and main crops - C
NOTE. Initial value:C2254</skos:definition>
        <skos:inScheme rdf:resource="http://lpis.ec.europa.eu/registry/applicationschema/cap-iacs-base/code#CropItemCodeValue"/>
    </owl:NamedIndividual>
    


    <!-- http://lpis.ec.europa.eu/registry/applicationschema/cap-iacs-base/code#CropItemCodeValue/barley -->


    <owl:NamedIndividual rdf:about="http://lpis.ec.europa.eu/registry/applicationschema/cap-iacs-base/code#CropItemCodeValue/barley">
        <rdf:type rdf:resource="http://lpis.ec.europa.eu/registry/applicationschema/cap-iacs-base#CropItemCodeValue"/>
        <rdfs:label xml:lang="en">Barley</rdfs:label>
        <skos:definition xml:lang="en">-- Definition --
|||Barley.
-- Description --
Cereals and main crops - C
NOTE. Initial value:C1160</skos:definition>
        <skos:inScheme rdf:resource="http://lpis.ec.europa.eu/registry/applicationschema/cap-iacs-base/code#CropItemCodeValue"/>
    </owl:NamedIndividual>
    


    <!-- http://lpis.ec.europa.eu/registry/applicationschema/cap-iacs-base/code#CropItemCodeValue/beans -->


    <owl:NamedIndividual rdf:about="http://lpis.ec.europa.eu/registry/applicationschema/cap-iacs-base/code#CropItemCodeValue/beans">
        <rdf:type rdf:resource="http://lpis.ec.europa.eu/registry/applicationschema/cap-iacs-base#CropItemCodeValue"/>
        <rdfs:label xml:lang="en">Beans</rdfs:label>
        <skos:definition xml:lang="en">-- Definition --
|||Beans.
-- Description --
Cereals and main crops - C
NOTE. Initial value:C1901</skos:definition>
        <skos:inScheme rdf:resource="http://lpis.ec.europa.eu/registry/applicationschema/cap-iacs-base/code#CropItemCodeValue"/>
    </owl:NamedIndividual>
    


    <!-- http://lpis.ec.europa.eu/registry/applicationschema/cap-iacs-base/code#CropItemCodeValue/beetroot -->


    <owl:NamedIndividual rdf:about="http://lpis.ec.europa.eu/registry/applicationschema/cap-iacs-base/code#CropItemCodeValue/beetroot">
        <rdf:type rdf:resource="http://lpis.ec.europa.eu/registry/applicationschema/cap-iacs-base#CropItemCodeValue"/>
        <rdfs:label xml:lang="en">Beetroot</rdfs:label>
        <skos:definition xml:lang="en">-- Definition --
|||Beetroot.
-- Description --
Cereals and main crops - C
NOTE. Initial value:C1860</skos:definition>
        <skos:inScheme rdf:resource="http://lpis.ec.europa.eu/registry/applicationschema/cap-iacs-base/code#CropItemCodeValue"/>
    </owl:NamedIndividual>
    


    <!-- http://lpis.ec.europa.eu/registry/applicationschema/cap-iacs-base/code#CropItemCodeValue/berriesExcludingStrawberries -->


    <owl:NamedIndividual rdf:about="http://lpis.ec.europa.eu/registry/applicationschema/cap-iacs-base/code#CropItemCodeValue/berriesExcludingStrawberries">
        <rdf:type rdf:resource="http://lpis.ec.europa.eu/registry/applicationschema/cap-iacs-base#CropItemCodeValue"/>
        <rdfs:label xml:lang="en">Berries (excluding strawberries)</rdfs:label>
        <skos:definition xml:lang="en">-- Definition --
||Berries (excluding strawberries).
-- Description --
Cereals and main crops - C
NOTE. Initial value:C2270</skos:definition>
        <skos:inScheme rdf:resource="http://lpis.ec.europa.eu/registry/applicationschema/cap-iacs-base/code#CropItemCodeValue"/>
    </owl:NamedIndividual>
    


    <!-- http://lpis.ec.europa.eu/registry/applicationschema/cap-iacs-base/code#CropItemCodeValue/blackCurrants -->


    <owl:NamedIndividual rdf:about="http://lpis.ec.europa.eu/registry/applicationschema/cap-iacs-base/code#CropItemCodeValue/blackCurrants">
        <rdf:type rdf:resource="http://lpis.ec.europa.eu/registry/applicationschema/cap-iacs-base#CropItemCodeValue"/>
        <rdfs:label xml:lang="en">Black currants</rdfs:label>
        <skos:definition xml:lang="en">-- Definition --
||||Black currants.
-- Description --
Cereals and main crops - C
NOTE. Initial value:C2272</skos:definition>
        <skos:inScheme rdf:resource="http://lpis.ec.europa.eu/registry/applicationschema/cap-iacs-base/code#CropItemCodeValue"/>
    </owl:NamedIndividual>
    


    <!-- http://lpis.ec.europa.eu/registry/applicationschema/cap-iacs-base/code#CropItemCodeValue/brassicas -->


    <owl:NamedIndividual rdf:about="http://lpis.ec.europa.eu/registry/applicationschema/cap-iacs-base/code#CropItemCodeValue/brassicas">
        <rdf:type rdf:resource="http://lpis.ec.europa.eu/registry/applicationschema/cap-iacs-base#CropItemCodeValue"/>
        <rdfs:label xml:lang="en">Brassicas</rdfs:label>
        <skos:definition xml:lang="en">-- Definition --
||Brassicas.
-- Description --
Cereals and main crops - C
NOTE. Initial value:C1610</skos:definition>
        <skos:inScheme rdf:resource="http://lpis.ec.europa.eu/registry/applicationschema/cap-iacs-base/code#CropItemCodeValue"/>
    </owl:NamedIndividual>
    


    <!-- http://lpis.ec.europa.eu/registry/applicationschema/cap-iacs-base/code#CropItemCodeValue/broadAndFieldBeansC1335 -->


    <owl:NamedIndividual rdf:about="http://lpis.ec.europa.eu/registry/applicationschema/cap-iacs-base/code#CropItemCodeValue/broadAndFieldBeansC1335">
        <rdf:type rdf:resource="http://lpis.ec.europa.eu/registry/applicationschema/cap-iacs-base#CropItemCodeValue"/>
        <rdfs:label xml:lang="en">Broad and field beans C1335</rdfs:label>
        <skos:definition xml:lang="en">-- Definition --
||Broad and field beans C1335.
-- Description --
Cereals and main crops - C
NOTE. Initial value:C1335</skos:definition>
        <skos:inScheme rdf:resource="http://lpis.ec.europa.eu/registry/applicationschema/cap-iacs-base/code#CropItemCodeValue"/>
    </owl:NamedIndividual>
    


    <!-- http://lpis.ec.europa.eu/registry/applicationschema/cap-iacs-base/code#CropItemCodeValue/brusselsSprouts -->


    <owl:NamedIndividual rdf:about="http://lpis.ec.europa.eu/registry/applicationschema/cap-iacs-base/code#CropItemCodeValue/brusselsSprouts">
        <rdf:type rdf:resource="http://lpis.ec.europa.eu/registry/applicationschema/cap-iacs-base#CropItemCodeValue"/>
        <rdfs:label xml:lang="en">Brussels sprouts</rdfs:label>
        <skos:definition xml:lang="en">-- Definition --
|||Brussels sprouts.
-- Description --
Cereals and main crops - C
NOTE. Initial value:C1631</skos:definition>
        <skos:inScheme rdf:resource="http://lpis.ec.europa.eu/registry/applicationschema/cap-iacs-base/code#CropItemCodeValue"/>
    </owl:NamedIndividual>
    


    <!-- http://lpis.ec.europa.eu/registry/applicationschema/cap-iacs-base/code#CropItemCodeValue/buckwheatMilletCanarySeedOtherCereals -->


    <owl:NamedIndividual rdf:about="http://lpis.ec.europa.eu/registry/applicationschema/cap-iacs-base/code#CropItemCodeValue/buckwheatMilletCanarySeedOtherCereals">
        <rdf:type rdf:resource="http://lpis.ec.europa.eu/registry/applicationschema/cap-iacs-base#CropItemCodeValue"/>
        <rdfs:label xml:lang="en">Buckwheat, millet, canary seed (other cereals)</rdfs:label>
        <skos:definition xml:lang="en">-- Definition --
|||Buckwheat, millet, canary seed (other cereals).
-- Description --
Cereals and main crops - C
NOTE. Initial value:C1219</skos:definition>
        <skos:inScheme rdf:resource="http://lpis.ec.europa.eu/registry/applicationschema/cap-iacs-base/code#CropItemCodeValue"/>
    </owl:NamedIndividual>
    


    <!-- http://lpis.ec.europa.eu/registry/applicationschema/cap-iacs-base/code#CropItemCodeValue/cabbageWhite -->


    <owl:NamedIndividual rdf:about="http://lpis.ec.europa.eu/registry/applicationschema/cap-iacs-base/code#CropItemCodeValue/cabbageWhite">
        <rdf:type rdf:resource="http://lpis.ec.europa.eu/registry/applicationschema/cap-iacs-base#CropItemCodeValue"/>
        <rdfs:label xml:lang="en">Cabbage (white)</rdfs:label>
        <skos:definition xml:lang="en">-- Definition --
|||Cabbage (white).
-- Description --
Cereals and main crops - C
NOTE. Initial value:C1635</skos:definition>
        <skos:inScheme rdf:resource="http://lpis.ec.europa.eu/registry/applicationschema/cap-iacs-base/code#CropItemCodeValue"/>
    </owl:NamedIndividual>
    


    <!-- http://lpis.ec.europa.eu/registry/applicationschema/cap-iacs-base/code#CropItemCodeValue/caraway -->


    <owl:NamedIndividual rdf:about="http://lpis.ec.europa.eu/registry/applicationschema/cap-iacs-base/code#CropItemCodeValue/caraway">
        <rdf:type rdf:resource="http://lpis.ec.europa.eu/registry/applicationschema/cap-iacs-base#CropItemCodeValue"/>
        <rdfs:label xml:lang="en">Caraway</rdfs:label>
        <skos:definition xml:lang="en">-- Definition --
||||Caraway.
-- Description --
Cereals and main crops - C
NOTE. Initial value:C1582</skos:definition>
        <skos:inScheme rdf:resource="http://lpis.ec.europa.eu/registry/applicationschema/cap-iacs-base/code#CropItemCodeValue"/>
    </owl:NamedIndividual>
    


    <!-- http://lpis.ec.europa.eu/registry/applicationschema/cap-iacs-base/code#CropItemCodeValue/carrots -->


    <owl:NamedIndividual rdf:about="http://lpis.ec.europa.eu/registry/applicationschema/cap-iacs-base/code#CropItemCodeValue/carrots">
        <rdf:type rdf:resource="http://lpis.ec.europa.eu/registry/applicationschema/cap-iacs-base#CropItemCodeValue"/>
        <rdfs:label xml:lang="en">Carrots</rdfs:label>
        <skos:definition xml:lang="en">-- Definition --
|||Carrots.
-- Description --
Cereals and main crops - C
NOTE. Initial value:C1830</skos:definition>
        <skos:inScheme rdf:resource="http://lpis.ec.europa.eu/registry/applicationschema/cap-iacs-base/code#CropItemCodeValue"/>
    </owl:NamedIndividual>
    


    <!-- http://lpis.ec.europa.eu/registry/applicationschema/cap-iacs-base/code#CropItemCodeValue/cauliflowerAndBroccoli -->


    <owl:NamedIndividual rdf:about="http://lpis.ec.europa.eu/registry/applicationschema/cap-iacs-base/code#CropItemCodeValue/cauliflowerAndBroccoli">
        <rdf:type rdf:resource="http://lpis.ec.europa.eu/registry/applicationschema/cap-iacs-base#CropItemCodeValue"/>
        <rdfs:label xml:lang="en">Cauliflower and broccoli</rdfs:label>
        <skos:definition xml:lang="en">-- Definition --
|||Cauliflower and broccoli.
-- Description --
Cereals and main crops - C
NOTE. Initial value:C1620</skos:definition>
        <skos:inScheme rdf:resource="http://lpis.ec.europa.eu/registry/applicationschema/cap-iacs-base/code#CropItemCodeValue"/>
    </owl:NamedIndividual>
    


    <!-- http://lpis.ec.europa.eu/registry/applicationschema/cap-iacs-base/code#CropItemCodeValue/celeriac -->


    <owl:NamedIndividual rdf:about="http://lpis.ec.europa.eu/registry/applicationschema/cap-iacs-base/code#CropItemCodeValue/celeriac">
        <rdf:type rdf:resource="http://lpis.ec.europa.eu/registry/applicationschema/cap-iacs-base#CropItemCodeValue"/>
        <rdfs:label xml:lang="en">Celeriac</rdfs:label>
        <skos:definition xml:lang="en">-- Definition --
|||Celeriac.
-- Description --
Cereals and main crops - C
NOTE. Initial value:C1872</skos:definition>
        <skos:inScheme rdf:resource="http://lpis.ec.europa.eu/registry/applicationschema/cap-iacs-base/code#CropItemCodeValue"/>
    </owl:NamedIndividual>
    


    <!-- http://lpis.ec.europa.eu/registry/applicationschema/cap-iacs-base/code#CropItemCodeValue/celery -->


    <owl:NamedIndividual rdf:about="http://lpis.ec.europa.eu/registry/applicationschema/cap-iacs-base/code#CropItemCodeValue/celery">
        <rdf:type rdf:resource="http://lpis.ec.europa.eu/registry/applicationschema/cap-iacs-base#CropItemCodeValue"/>
        <rdfs:label xml:lang="en">Celery</rdfs:label>
        <skos:definition xml:lang="en">-- Definition --
|||Celery.
-- Description --
Cereals and main crops - C
NOTE. Initial value:C1672</skos:definition>
        <skos:inScheme rdf:resource="http://lpis.ec.europa.eu/registry/applicationschema/cap-iacs-base/code#CropItemCodeValue"/>
    </owl:NamedIndividual>
    


    <!-- http://lpis.ec.europa.eu/registry/applicationschema/cap-iacs-base/code#CropItemCodeValue/cerealsExcludingRice -->


    <owl:NamedIndividual rdf:about="http://lpis.ec.europa.eu/registry/applicationschema/cap-iacs-base/code#CropItemCodeValue/cerealsExcludingRice">
        <rdf:type rdf:resource="http://lpis.ec.europa.eu/registry/applicationschema/cap-iacs-base#CropItemCodeValue"/>
        <rdfs:label xml:lang="en">Cereals (excluding rice) </rdfs:label>
        <skos:definition xml:lang="en">-- Definition --
||Cereals (excluding rice) .
-- Description --
Cereals and main crops - C
NOTE. Initial value: C1050</skos:definition>
        <skos:inScheme rdf:resource="http://lpis.ec.europa.eu/registry/applicationschema/cap-iacs-base/code#CropItemCodeValue"/>
    </owl:NamedIndividual>
    


    <!-- http://lpis.ec.europa.eu/registry/applicationschema/cap-iacs-base/code#CropItemCodeValue/cerealsForTheProductionOfGrainIncludingRiceAndSeed -->


    <owl:NamedIndividual rdf:about="http://lpis.ec.europa.eu/registry/applicationschema/cap-iacs-base/code#CropItemCodeValue/cerealsForTheProductionOfGrainIncludingRiceAndSeed">
        <rdf:type rdf:resource="http://lpis.ec.europa.eu/registry/applicationschema/cap-iacs-base#CropItemCodeValue"/>
        <rdfs:label xml:lang="en">Cereals for the production of grain (including rice and seed)</rdfs:label>
        <skos:definition xml:lang="en">-- Definition --
|Cereals for the production of grain (including rice and seed).
-- Description --
Cereals and main crops - C
NOTE. Initial value:C1040</skos:definition>
        <skos:inScheme rdf:resource="http://lpis.ec.europa.eu/registry/applicationschema/cap-iacs-base/code#CropItemCodeValue"/>
    </owl:NamedIndividual>
    


    <!-- http://lpis.ec.europa.eu/registry/applicationschema/cap-iacs-base/code#CropItemCodeValue/cerealsForTheProductionOfGrainIncludingSeedButExcludingRice -->


    <owl:NamedIndividual rdf:about="http://lpis.ec.europa.eu/registry/applicationschema/cap-iacs-base/code#CropItemCodeValue/cerealsForTheProductionOfGrainIncludingSeedButExcludingRice">
        <rdf:type rdf:resource="http://lpis.ec.europa.eu/registry/applicationschema/cap-iacs-base#CropItemCodeValue"/>
        <rdfs:label xml:lang="en">Cereals for the production of grain (including seed but excluding rice)</rdfs:label>
        <skos:definition xml:lang="en">-- Definition --
|||Cereals for the production of grain (including seed but excluding rice).
-- Description --
Land use of Agriculture Area in Use -L
NOTE. Initial value:L1050</skos:definition>
        <skos:inScheme rdf:resource="http://lpis.ec.europa.eu/registry/applicationschema/cap-iacs-base/code#CropItemCodeValue"/>
    </owl:NamedIndividual>
    


    <!-- http://lpis.ec.europa.eu/registry/applicationschema/cap-iacs-base/code#CropItemCodeValue/cerealsHarvestedGreen -->


    <owl:NamedIndividual rdf:about="http://lpis.ec.europa.eu/registry/applicationschema/cap-iacs-base/code#CropItemCodeValue/cerealsHarvestedGreen">
        <rdf:type rdf:resource="http://lpis.ec.europa.eu/registry/applicationschema/cap-iacs-base#CropItemCodeValue"/>
        <rdfs:label xml:lang="en">Cereals harvested green</rdfs:label>
        <skos:definition xml:lang="en">-- Definition --
|||Cereals harvested green.
-- Description --
Cereals and main crops - C
NOTE. Initial value:C2626</skos:definition>
        <skos:inScheme rdf:resource="http://lpis.ec.europa.eu/registry/applicationschema/cap-iacs-base/code#CropItemCodeValue"/>
    </owl:NamedIndividual>
    


    <!-- http://lpis.ec.europa.eu/registry/applicationschema/cap-iacs-base/code#CropItemCodeValue/cherries -->


    <owl:NamedIndividual rdf:about="http://lpis.ec.europa.eu/registry/applicationschema/cap-iacs-base/code#CropItemCodeValue/cherries">
        <rdf:type rdf:resource="http://lpis.ec.europa.eu/registry/applicationschema/cap-iacs-base#CropItemCodeValue"/>
        <rdfs:label xml:lang="en">Cherries</rdfs:label>
        <skos:definition xml:lang="en">-- Definition --
|||Cherries.
-- Description --
Cereals and main crops - C
NOTE. Initial value:C2200</skos:definition>
        <skos:inScheme rdf:resource="http://lpis.ec.europa.eu/registry/applicationschema/cap-iacs-base/code#CropItemCodeValue"/>
    </owl:NamedIndividual>
    


    <!-- http://lpis.ec.europa.eu/registry/applicationschema/cap-iacs-base/code#CropItemCodeValue/chestnuts -->


    <owl:NamedIndividual rdf:about="http://lpis.ec.europa.eu/registry/applicationschema/cap-iacs-base/code#CropItemCodeValue/chestnuts">
        <rdf:type rdf:resource="http://lpis.ec.europa.eu/registry/applicationschema/cap-iacs-base#CropItemCodeValue"/>
        <rdfs:label xml:lang="en">Chestnuts</rdfs:label>
        <skos:definition xml:lang="en">-- Definition --
|||Chestnuts.
-- Description --
Cereals and main crops - C
NOTE. Initial value:C2236</skos:definition>
        <skos:inScheme rdf:resource="http://lpis.ec.europa.eu/registry/applicationschema/cap-iacs-base/code#CropItemCodeValue"/>
    </owl:NamedIndividual>
    


    <!-- http://lpis.ec.europa.eu/registry/applicationschema/cap-iacs-base/code#CropItemCodeValue/chicory -->


    <owl:NamedIndividual rdf:about="http://lpis.ec.europa.eu/registry/applicationschema/cap-iacs-base/code#CropItemCodeValue/chicory">
        <rdf:type rdf:resource="http://lpis.ec.europa.eu/registry/applicationschema/cap-iacs-base#CropItemCodeValue"/>
        <rdfs:label xml:lang="en">Chicory</rdfs:label>
        <skos:definition xml:lang="en">-- Definition --
|||Chicory.
-- Description --
Cereals and main crops - C
NOTE. Initial value:C1571</skos:definition>
        <skos:inScheme rdf:resource="http://lpis.ec.europa.eu/registry/applicationschema/cap-iacs-base/code#CropItemCodeValue"/>
    </owl:NamedIndividual>
    


    <!-- http://lpis.ec.europa.eu/registry/applicationschema/cap-iacs-base/code#CropItemCodeValue/chicoryC1710 -->


    <owl:NamedIndividual rdf:about="http://lpis.ec.europa.eu/registry/applicationschema/cap-iacs-base/code#CropItemCodeValue/chicoryC1710">
        <rdf:type rdf:resource="http://lpis.ec.europa.eu/registry/applicationschema/cap-iacs-base#CropItemCodeValue"/>
        <rdfs:label xml:lang="en">Chicory C1710</rdfs:label>
        <skos:definition xml:lang="en">-- Definition --
|||Chicory C1710.
-- Description --
Cereals and main crops - C
NOTE. Initial value:C1710</skos:definition>
        <skos:inScheme rdf:resource="http://lpis.ec.europa.eu/registry/applicationschema/cap-iacs-base/code#CropItemCodeValue"/>
    </owl:NamedIndividual>
    


    <!-- http://lpis.ec.europa.eu/registry/applicationschema/cap-iacs-base/code#CropItemCodeValue/chicoryForInulin -->


    <owl:NamedIndividual rdf:about="http://lpis.ec.europa.eu/registry/applicationschema/cap-iacs-base/code#CropItemCodeValue/chicoryForInulin">
        <rdf:type rdf:resource="http://lpis.ec.europa.eu/registry/applicationschema/cap-iacs-base#CropItemCodeValue"/>
        <rdfs:label xml:lang="en">Chicory for inulin</rdfs:label>
        <skos:definition xml:lang="en">-- Definition --
||||Chicory for inulin.
-- Description --
Cereals and main crops - C
NOTE. Initial value:C1572</skos:definition>
        <skos:inScheme rdf:resource="http://lpis.ec.europa.eu/registry/applicationschema/cap-iacs-base/code#CropItemCodeValue"/>
    </owl:NamedIndividual>
    


    <!-- http://lpis.ec.europa.eu/registry/applicationschema/cap-iacs-base/code#CropItemCodeValue/citrusFruitsC2300 -->


    <owl:NamedIndividual rdf:about="http://lpis.ec.europa.eu/registry/applicationschema/cap-iacs-base/code#CropItemCodeValue/citrusFruitsC2300">
        <rdf:type rdf:resource="http://lpis.ec.europa.eu/registry/applicationschema/cap-iacs-base#CropItemCodeValue"/>
        <rdfs:label xml:lang="en">Citrus fruits C2300</rdfs:label>
        <skos:definition xml:lang="en">-- Definition --
||Citrus fruits C2300.
-- Description --
Cereals and main crops - C
NOTE. Initial value:C2300</skos:definition>
        <skos:inScheme rdf:resource="http://lpis.ec.europa.eu/registry/applicationschema/cap-iacs-base/code#CropItemCodeValue"/>
    </owl:NamedIndividual>
    


    <!-- http://lpis.ec.europa.eu/registry/applicationschema/cap-iacs-base/code#CropItemCodeValue/citrusPlantations -->


    <owl:NamedIndividual rdf:about="http://lpis.ec.europa.eu/registry/applicationschema/cap-iacs-base/code#CropItemCodeValue/citrusPlantations">
        <rdf:type rdf:resource="http://lpis.ec.europa.eu/registry/applicationschema/cap-iacs-base#CropItemCodeValue"/>
        <rdfs:label xml:lang="en">Citrus plantations</rdfs:label>
        <skos:definition xml:lang="en">-- Definition --
||||Citrus plantations.
-- Description --
Land use of Agriculture Area in Use -L
NOTE. Initial value:L2300</skos:definition>
        <skos:inScheme rdf:resource="http://lpis.ec.europa.eu/registry/applicationschema/cap-iacs-base/code#CropItemCodeValue"/>
    </owl:NamedIndividual>
    


    <!-- http://lpis.ec.europa.eu/registry/applicationschema/cap-iacs-base/code#CropItemCodeValue/clementines -->


    <owl:NamedIndividual rdf:about="http://lpis.ec.europa.eu/registry/applicationschema/cap-iacs-base/code#CropItemCodeValue/clementines">
        <rdf:type rdf:resource="http://lpis.ec.europa.eu/registry/applicationschema/cap-iacs-base#CropItemCodeValue"/>
        <rdfs:label xml:lang="en">Clementines</rdfs:label>
        <skos:definition xml:lang="en">-- Definition --
||||Clementines.
-- Description --
Cereals and main crops - C
NOTE. Initial value:C2360</skos:definition>
        <skos:inScheme rdf:resource="http://lpis.ec.europa.eu/registry/applicationschema/cap-iacs-base/code#CropItemCodeValue"/>
    </owl:NamedIndividual>
    


    <!-- http://lpis.ec.europa.eu/registry/applicationschema/cap-iacs-base/code#CropItemCodeValue/cloverAndMixtures -->


    <owl:NamedIndividual rdf:about="http://lpis.ec.europa.eu/registry/applicationschema/cap-iacs-base/code#CropItemCodeValue/cloverAndMixtures">
        <rdf:type rdf:resource="http://lpis.ec.europa.eu/registry/applicationschema/cap-iacs-base#CropItemCodeValue"/>
        <rdfs:label xml:lang="en">Clover and mixtures</rdfs:label>
        <skos:definition xml:lang="en">-- Definition --
|||Clover and mixtures.
-- Description --
Cereals and main crops - C
NOTE. Initial value:C2671</skos:definition>
        <skos:inScheme rdf:resource="http://lpis.ec.europa.eu/registry/applicationschema/cap-iacs-base/code#CropItemCodeValue"/>
    </owl:NamedIndividual>
    


    <!-- http://lpis.ec.europa.eu/registry/applicationschema/cap-iacs-base/code#CropItemCodeValue/commonSpringWheat -->


    <owl:NamedIndividual rdf:about="http://lpis.ec.europa.eu/registry/applicationschema/cap-iacs-base/code#CropItemCodeValue/commonSpringWheat">
        <rdf:type rdf:resource="http://lpis.ec.europa.eu/registry/applicationschema/cap-iacs-base#CropItemCodeValue"/>
        <rdfs:label xml:lang="en">Common spring wheat</rdfs:label>
        <skos:definition xml:lang="en">-- Definition --
|||||Common spring wheat.
-- Description --
Cereals and main crops - C
NOTE. Initial value:C1124</skos:definition>
        <skos:inScheme rdf:resource="http://lpis.ec.europa.eu/registry/applicationschema/cap-iacs-base/code#CropItemCodeValue"/>
    </owl:NamedIndividual>
    


    <!-- http://lpis.ec.europa.eu/registry/applicationschema/cap-iacs-base/code#CropItemCodeValue/commonWheatAndSpelt -->


    <owl:NamedIndividual rdf:about="http://lpis.ec.europa.eu/registry/applicationschema/cap-iacs-base/code#CropItemCodeValue/commonWheatAndSpelt">
        <rdf:type rdf:resource="http://lpis.ec.europa.eu/registry/applicationschema/cap-iacs-base#CropItemCodeValue"/>
        <rdfs:label xml:lang="en">Common wheat and spelt</rdfs:label>
        <skos:definition xml:lang="en">-- Definition --
||||Common wheat and spelt.
-- Description --
Cereals and main crops - C
NOTE. Initial value:C1120</skos:definition>
        <skos:inScheme rdf:resource="http://lpis.ec.europa.eu/registry/applicationschema/cap-iacs-base/code#CropItemCodeValue"/>
    </owl:NamedIndividual>
    


    <!-- http://lpis.ec.europa.eu/registry/applicationschema/cap-iacs-base/code#CropItemCodeValue/commonWinterWheat -->


    <owl:NamedIndividual rdf:about="http://lpis.ec.europa.eu/registry/applicationschema/cap-iacs-base/code#CropItemCodeValue/commonWinterWheat">
        <rdf:type rdf:resource="http://lpis.ec.europa.eu/registry/applicationschema/cap-iacs-base#CropItemCodeValue"/>
        <rdfs:label xml:lang="en">Common winter wheat</rdfs:label>
        <skos:definition xml:lang="en">-- Definition --
|||||Common winter wheat.
-- Description --
Cereals and main crops - C
NOTE. Initial value:C1123</skos:definition>
        <skos:inScheme rdf:resource="http://lpis.ec.europa.eu/registry/applicationschema/cap-iacs-base/code#CropItemCodeValue"/>
    </owl:NamedIndividual>
    


    <!-- http://lpis.ec.europa.eu/registry/applicationschema/cap-iacs-base/code#CropItemCodeValue/cornCobMixC1200 -->


    <owl:NamedIndividual rdf:about="http://lpis.ec.europa.eu/registry/applicationschema/cap-iacs-base/code#CropItemCodeValue/cornCobMixC1200">
        <rdf:type rdf:resource="http://lpis.ec.europa.eu/registry/applicationschema/cap-iacs-base#CropItemCodeValue"/>
        <rdfs:label xml:lang="en">Corn cob mix C1200</rdfs:label>
        <skos:definition xml:lang="en">-- Definition --
||||Corn cob mix C1200.
-- Description --
Cereals and main crops - C
NOTE. Initial value:C1202</skos:definition>
        <skos:inScheme rdf:resource="http://lpis.ec.europa.eu/registry/applicationschema/cap-iacs-base/code#CropItemCodeValue"/>
    </owl:NamedIndividual>
    


    <!-- http://lpis.ec.europa.eu/registry/applicationschema/cap-iacs-base/code#CropItemCodeValue/cottonFibre -->


    <owl:NamedIndividual rdf:about="http://lpis.ec.europa.eu/registry/applicationschema/cap-iacs-base/code#CropItemCodeValue/cottonFibre">
        <rdf:type rdf:resource="http://lpis.ec.europa.eu/registry/applicationschema/cap-iacs-base#CropItemCodeValue"/>
        <rdfs:label xml:lang="en">Cotton fibre </rdfs:label>
        <skos:definition xml:lang="en">-- Definition --
|||Cotton fibre.
-- Description --
Cereals and main crops - C
NOTE. Initial value:C1540</skos:definition>
        <skos:inScheme rdf:resource="http://lpis.ec.europa.eu/registry/applicationschema/cap-iacs-base/code#CropItemCodeValue"/>
    </owl:NamedIndividual>
    


    <!-- http://lpis.ec.europa.eu/registry/applicationschema/cap-iacs-base/code#CropItemCodeValue/cottonSeed -->


    <owl:NamedIndividual rdf:about="http://lpis.ec.europa.eu/registry/applicationschema/cap-iacs-base/code#CropItemCodeValue/cottonSeed">
        <rdf:type rdf:resource="http://lpis.ec.europa.eu/registry/applicationschema/cap-iacs-base#CropItemCodeValue"/>
        <rdfs:label xml:lang="en">Cotton seed</rdfs:label>
        <skos:definition xml:lang="en">-- Definition --
||||Cotton seed.
-- Description --
Cereals and main crops - C
NOTE. Initial value:C1490</skos:definition>
        <skos:inScheme rdf:resource="http://lpis.ec.europa.eu/registry/applicationschema/cap-iacs-base/code#CropItemCodeValue"/>
    </owl:NamedIndividual>
    


    <!-- http://lpis.ec.europa.eu/registry/applicationschema/cap-iacs-base/code#CropItemCodeValue/courgettes -->


    <owl:NamedIndividual rdf:about="http://lpis.ec.europa.eu/registry/applicationschema/cap-iacs-base/code#CropItemCodeValue/courgettes">
        <rdf:type rdf:resource="http://lpis.ec.europa.eu/registry/applicationschema/cap-iacs-base#CropItemCodeValue"/>
        <rdfs:label xml:lang="en">Courgettes</rdfs:label>
        <skos:definition xml:lang="en">-- Definition --
||||Courgettes.
-- Description --
Cereals and main crops - C
NOTE. Initial value:C1787</skos:definition>
        <skos:inScheme rdf:resource="http://lpis.ec.europa.eu/registry/applicationschema/cap-iacs-base/code#CropItemCodeValue"/>
    </owl:NamedIndividual>
    


    <!-- http://lpis.ec.europa.eu/registry/applicationschema/cap-iacs-base/code#CropItemCodeValue/cropProductionUnderGlassOrHighAccessibleCover -->


    <owl:NamedIndividual rdf:about="http://lpis.ec.europa.eu/registry/applicationschema/cap-iacs-base/code#CropItemCodeValue/cropProductionUnderGlassOrHighAccessibleCover">
        <rdf:type rdf:resource="http://lpis.ec.europa.eu/registry/applicationschema/cap-iacs-base#CropItemCodeValue"/>
        <rdfs:label xml:lang="en">Crop production under glass or high accessible cover</rdfs:label>
        <skos:definition xml:lang="en">-- Definition --
Crop production under glass or high accessible cover.
-- Description --
Land use of Agriculture Area in Use -L. Special aggregates
NOTE. Initial value:L0900</skos:definition>
        <skos:inScheme rdf:resource="http://lpis.ec.europa.eu/registry/applicationschema/cap-iacs-base/code#CropItemCodeValue"/>
    </owl:NamedIndividual>
    


    <!-- http://lpis.ec.europa.eu/registry/applicationschema/cap-iacs-base/code#CropItemCodeValue/cucumbers -->


    <owl:NamedIndividual rdf:about="http://lpis.ec.europa.eu/registry/applicationschema/cap-iacs-base/code#CropItemCodeValue/cucumbers">
        <rdf:type rdf:resource="http://lpis.ec.europa.eu/registry/applicationschema/cap-iacs-base#CropItemCodeValue"/>
        <rdfs:label xml:lang="en">Cucumbers</rdfs:label>
        <skos:definition xml:lang="en">-- Definition --
|||Cucumbers.
-- Description --
Cereals and main crops - C
NOTE. Initial value:C1761</skos:definition>
        <skos:inScheme rdf:resource="http://lpis.ec.europa.eu/registry/applicationschema/cap-iacs-base/code#CropItemCodeValue"/>
    </owl:NamedIndividual>
    


    <!-- http://lpis.ec.europa.eu/registry/applicationschema/cap-iacs-base/code#CropItemCodeValue/cucumbersUnderGlassOrHighAccessibleCoverC1762 -->


    <owl:NamedIndividual rdf:about="http://lpis.ec.europa.eu/registry/applicationschema/cap-iacs-base/code#CropItemCodeValue/cucumbersUnderGlassOrHighAccessibleCoverC1762">
        <rdf:type rdf:resource="http://lpis.ec.europa.eu/registry/applicationschema/cap-iacs-base#CropItemCodeValue"/>
        <rdfs:label xml:lang="en">Cucumbers under glass or high accessible cover C1762 </rdfs:label>
        <skos:definition xml:lang="en">-- Definition --
||||Cucumbers under glass or high accessible cover C1762.
-- Description --
Cereals and main crops - C
NOTE. Initial value:C1762</skos:definition>
        <skos:inScheme rdf:resource="http://lpis.ec.europa.eu/registry/applicationschema/cap-iacs-base/code#CropItemCodeValue"/>
    </owl:NamedIndividual>
    


    <!-- http://lpis.ec.europa.eu/registry/applicationschema/cap-iacs-base/code#CropItemCodeValue/cultivatedMushrooms -->


    <owl:NamedIndividual rdf:about="http://lpis.ec.europa.eu/registry/applicationschema/cap-iacs-base/code#CropItemCodeValue/cultivatedMushrooms">
        <rdf:type rdf:resource="http://lpis.ec.europa.eu/registry/applicationschema/cap-iacs-base#CropItemCodeValue"/>
        <rdfs:label xml:lang="en">Cultivated mushrooms</rdfs:label>
        <skos:definition xml:lang="en">-- Definition --
|Cultivated mushrooms.
-- Description --
Cereals and main crops - C
NOTE. Initial value:C1910</skos:definition>
        <skos:inScheme rdf:resource="http://lpis.ec.europa.eu/registry/applicationschema/cap-iacs-base/code#CropItemCodeValue"/>
    </owl:NamedIndividual>
    


    <!-- http://lpis.ec.europa.eu/registry/applicationschema/cap-iacs-base/code#CropItemCodeValue/currants -->


    <owl:NamedIndividual rdf:about="http://lpis.ec.europa.eu/registry/applicationschema/cap-iacs-base/code#CropItemCodeValue/currants">
        <rdf:type rdf:resource="http://lpis.ec.europa.eu/registry/applicationschema/cap-iacs-base#CropItemCodeValue"/>
        <rdfs:label xml:lang="en">Currants</rdfs:label>
        <skos:definition xml:lang="en">-- Definition --
|||Currants.
-- Description --
Cereals and main crops - C
NOTE. Initial value:C2271</skos:definition>
        <skos:inScheme rdf:resource="http://lpis.ec.europa.eu/registry/applicationschema/cap-iacs-base/code#CropItemCodeValue"/>
    </owl:NamedIndividual>
    


    <!-- http://lpis.ec.europa.eu/registry/applicationschema/cap-iacs-base/code#CropItemCodeValue/driedPulsesAndProteinCropsForTheProductionOfGrainIncludingSeedAndMixturesOfCerealsAndPulses -->


    <owl:NamedIndividual rdf:about="http://lpis.ec.europa.eu/registry/applicationschema/cap-iacs-base/code#CropItemCodeValue/driedPulsesAndProteinCropsForTheProductionOfGrainIncludingSeedAndMixturesOfCerealsAndPulses">
        <rdf:type rdf:resource="http://lpis.ec.europa.eu/registry/applicationschema/cap-iacs-base#CropItemCodeValue"/>
        <rdfs:label xml:lang="en">Dried pulses and protein crops for the production of grain (including seed and mixtures of cereals and pulses)</rdfs:label>
        <skos:definition xml:lang="en">-- Definition --
|||Dried pulses and protein crops for the production of grain (including seed and mixtures of cereals and pulses).
-- Description --
Land use of Agriculture Area in Use -L
NOTE. Initial value:L1300</skos:definition>
        <skos:inScheme rdf:resource="http://lpis.ec.europa.eu/registry/applicationschema/cap-iacs-base/code#CropItemCodeValue"/>
    </owl:NamedIndividual>
    


    <!-- http://lpis.ec.europa.eu/registry/applicationschema/cap-iacs-base/code#CropItemCodeValue/driedPulsesAndProteinCropsForTheProductionOfGrainIncludingSeedAndMixturesOfCerealsAndPulsesC1300 -->


    <owl:NamedIndividual rdf:about="http://lpis.ec.europa.eu/registry/applicationschema/cap-iacs-base/code#CropItemCodeValue/driedPulsesAndProteinCropsForTheProductionOfGrainIncludingSeedAndMixturesOfCerealsAndPulsesC1300">
        <rdf:type rdf:resource="http://lpis.ec.europa.eu/registry/applicationschema/cap-iacs-base#CropItemCodeValue"/>
        <rdfs:label xml:lang="en">Dried pulses and protein crops for the production of grain (including seed and mixtures of cereals and pulses) C1300</rdfs:label>
        <skos:definition xml:lang="en">-- Definition --
|Dried pulses and protein crops for the production of grain (including seed and mixtures of cereals and pulses) C1300.
-- Description --
Cereals and main crops - C
NOTE. Initial value:C1300</skos:definition>
        <skos:inScheme rdf:resource="http://lpis.ec.europa.eu/registry/applicationschema/cap-iacs-base/code#CropItemCodeValue"/>
    </owl:NamedIndividual>
    


    <!-- http://lpis.ec.europa.eu/registry/applicationschema/cap-iacs-base/code#CropItemCodeValue/durumWheat -->


    <owl:NamedIndividual rdf:about="http://lpis.ec.europa.eu/registry/applicationschema/cap-iacs-base/code#CropItemCodeValue/durumWheat">
        <rdf:type rdf:resource="http://lpis.ec.europa.eu/registry/applicationschema/cap-iacs-base#CropItemCodeValue"/>
        <rdfs:label xml:lang="en">Durum wheat</rdfs:label>
        <skos:definition xml:lang="en">-- Definition --
||||Durum wheat.
-- Description --
Cereals and main crops - C
NOTE. Initial value:C1130</skos:definition>
        <skos:inScheme rdf:resource="http://lpis.ec.europa.eu/registry/applicationschema/cap-iacs-base/code#CropItemCodeValue"/>
    </owl:NamedIndividual>
    


    <!-- http://lpis.ec.europa.eu/registry/applicationschema/cap-iacs-base/code#CropItemCodeValue/earlyPotatoes -->


    <owl:NamedIndividual rdf:about="http://lpis.ec.europa.eu/registry/applicationschema/cap-iacs-base/code#CropItemCodeValue/earlyPotatoes">
        <rdf:type rdf:resource="http://lpis.ec.europa.eu/registry/applicationschema/cap-iacs-base#CropItemCodeValue"/>
        <rdfs:label xml:lang="en">Early potatoes</rdfs:label>
        <skos:definition xml:lang="en">-- Definition --
|||Early potatoes.
-- Description --
Cereals and main crops - C
NOTE. Initial value:C1362</skos:definition>
        <skos:inScheme rdf:resource="http://lpis.ec.europa.eu/registry/applicationschema/cap-iacs-base/code#CropItemCodeValue"/>
    </owl:NamedIndividual>
    


    <!-- http://lpis.ec.europa.eu/registry/applicationschema/cap-iacs-base/code#CropItemCodeValue/eggplants -->


    <owl:NamedIndividual rdf:about="http://lpis.ec.europa.eu/registry/applicationschema/cap-iacs-base/code#CropItemCodeValue/eggplants">
        <rdf:type rdf:resource="http://lpis.ec.europa.eu/registry/applicationschema/cap-iacs-base#CropItemCodeValue"/>
        <rdfs:label xml:lang="en">Eggplants</rdfs:label>
        <skos:definition xml:lang="en">-- Definition --
||||Eggplants.
-- Description --
Cereals and main crops - C
NOTE. Initial value:C1781</skos:definition>
        <skos:inScheme rdf:resource="http://lpis.ec.europa.eu/registry/applicationschema/cap-iacs-base/code#CropItemCodeValue"/>
    </owl:NamedIndividual>
    


    <!-- http://lpis.ec.europa.eu/registry/applicationschema/cap-iacs-base/code#CropItemCodeValue/eggplantsGourdsMarrowsCourgettesPumpkins -->


    <owl:NamedIndividual rdf:about="http://lpis.ec.europa.eu/registry/applicationschema/cap-iacs-base/code#CropItemCodeValue/eggplantsGourdsMarrowsCourgettesPumpkins">
        <rdf:type rdf:resource="http://lpis.ec.europa.eu/registry/applicationschema/cap-iacs-base#CropItemCodeValue"/>
        <rdfs:label xml:lang="en">Eggplants, gourds, marrows, courgettes, pumpkins</rdfs:label>
        <skos:definition xml:lang="en">-- Definition --
|||Eggplants, gourds, marrows, courgettes, pumpkins.
-- Description --
Cereals and main crops - C
NOTE. Initial value:C1780</skos:definition>
        <skos:inScheme rdf:resource="http://lpis.ec.europa.eu/registry/applicationschema/cap-iacs-base/code#CropItemCodeValue"/>
    </owl:NamedIndividual>
    


    <!-- http://lpis.ec.europa.eu/registry/applicationschema/cap-iacs-base/code#CropItemCodeValue/endives -->


    <owl:NamedIndividual rdf:about="http://lpis.ec.europa.eu/registry/applicationschema/cap-iacs-base/code#CropItemCodeValue/endives">
        <rdf:type rdf:resource="http://lpis.ec.europa.eu/registry/applicationschema/cap-iacs-base#CropItemCodeValue"/>
        <rdfs:label xml:lang="en">Endives</rdfs:label>
        <skos:definition xml:lang="en">-- Definition --
|||Endives.
-- Description --
Cereals and main crops - C
NOTE. Initial value:C1685</skos:definition>
        <skos:inScheme rdf:resource="http://lpis.ec.europa.eu/registry/applicationschema/cap-iacs-base/code#CropItemCodeValue"/>
    </owl:NamedIndividual>
    


    <!-- http://lpis.ec.europa.eu/registry/applicationschema/cap-iacs-base/code#CropItemCodeValue/energyCrops -->


    <owl:NamedIndividual rdf:about="http://lpis.ec.europa.eu/registry/applicationschema/cap-iacs-base/code#CropItemCodeValue/energyCrops">
        <rdf:type rdf:resource="http://lpis.ec.europa.eu/registry/applicationschema/cap-iacs-base#CropItemCodeValue"/>
        <rdfs:label xml:lang="en">Energy crops</rdfs:label>
        <skos:definition xml:lang="en">-- Definition --
|Energy crops.
-- Description --
Cereals and main crops - C
NOTE. Initial value:C1590</skos:definition>
        <skos:inScheme rdf:resource="http://lpis.ec.europa.eu/registry/applicationschema/cap-iacs-base/code#CropItemCodeValue"/>
    </owl:NamedIndividual>
    


    <!-- http://lpis.ec.europa.eu/registry/applicationschema/cap-iacs-base/code#CropItemCodeValue/fallowLand -->


    <owl:NamedIndividual rdf:about="http://lpis.ec.europa.eu/registry/applicationschema/cap-iacs-base/code#CropItemCodeValue/fallowLand">
        <rdf:type rdf:resource="http://lpis.ec.europa.eu/registry/applicationschema/cap-iacs-base#CropItemCodeValue"/>
        <rdfs:label xml:lang="en">Fallow land</rdfs:label>
        <skos:definition xml:lang="en">-- Definition --
|||Fallow land.
-- Description --
Land use of Agriculture Area in Use -L
NOTE. Initial value:L2696</skos:definition>
        <skos:inScheme rdf:resource="http://lpis.ec.europa.eu/registry/applicationschema/cap-iacs-base/code#CropItemCodeValue"/>
    </owl:NamedIndividual>
    


    <!-- http://lpis.ec.europa.eu/registry/applicationschema/cap-iacs-base/code#CropItemCodeValue/fibreCrops -->


    <owl:NamedIndividual rdf:about="http://lpis.ec.europa.eu/registry/applicationschema/cap-iacs-base/code#CropItemCodeValue/fibreCrops">
        <rdf:type rdf:resource="http://lpis.ec.europa.eu/registry/applicationschema/cap-iacs-base#CropItemCodeValue"/>
        <rdfs:label xml:lang="en">Fibre crops</rdfs:label>
        <skos:definition xml:lang="en">-- Definition --
||Fibre crops.
-- Description --
Cereals and main crops - C
NOTE. Initial value:C1500</skos:definition>
        <skos:inScheme rdf:resource="http://lpis.ec.europa.eu/registry/applicationschema/cap-iacs-base/code#CropItemCodeValue"/>
    </owl:NamedIndividual>
    


    <!-- http://lpis.ec.europa.eu/registry/applicationschema/cap-iacs-base/code#CropItemCodeValue/fibreFlax -->


    <owl:NamedIndividual rdf:about="http://lpis.ec.europa.eu/registry/applicationschema/cap-iacs-base/code#CropItemCodeValue/fibreFlax">
        <rdf:type rdf:resource="http://lpis.ec.europa.eu/registry/applicationschema/cap-iacs-base#CropItemCodeValue"/>
        <rdfs:label xml:lang="en">Fibre flax</rdfs:label>
        <skos:definition xml:lang="en">-- Definition --
|||Fibre flax.
-- Description --
Cereals and main crops - C
NOTE. Initial value:C1520</skos:definition>
        <skos:inScheme rdf:resource="http://lpis.ec.europa.eu/registry/applicationschema/cap-iacs-base/code#CropItemCodeValue"/>
    </owl:NamedIndividual>
    


    <!-- http://lpis.ec.europa.eu/registry/applicationschema/cap-iacs-base/code#CropItemCodeValue/fieldPeas -->


    <owl:NamedIndividual rdf:about="http://lpis.ec.europa.eu/registry/applicationschema/cap-iacs-base/code#CropItemCodeValue/fieldPeas">
        <rdf:type rdf:resource="http://lpis.ec.europa.eu/registry/applicationschema/cap-iacs-base#CropItemCodeValue"/>
        <rdfs:label xml:lang="en">Field peas</rdfs:label>
        <skos:definition xml:lang="en">-- Definition --
||Field peas.
-- Description --
Cereals and main crops - C
NOTE. Initial value:C1320</skos:definition>
        <skos:inScheme rdf:resource="http://lpis.ec.europa.eu/registry/applicationschema/cap-iacs-base/code#CropItemCodeValue"/>
    </owl:NamedIndividual>
    


    <!-- http://lpis.ec.europa.eu/registry/applicationschema/cap-iacs-base/code#CropItemCodeValue/figs -->


    <owl:NamedIndividual rdf:about="http://lpis.ec.europa.eu/registry/applicationschema/cap-iacs-base/code#CropItemCodeValue/figs">
        <rdf:type rdf:resource="http://lpis.ec.europa.eu/registry/applicationschema/cap-iacs-base#CropItemCodeValue"/>
        <rdfs:label xml:lang="en">Figs</rdfs:label>
        <skos:definition xml:lang="en">-- Definition --
|||Figs.
-- Description --
Cereals and main crops - C
NOTE. Initial value:C2251</skos:definition>
        <skos:inScheme rdf:resource="http://lpis.ec.europa.eu/registry/applicationschema/cap-iacs-base/code#CropItemCodeValue"/>
    </owl:NamedIndividual>
    


    <!-- http://lpis.ec.europa.eu/registry/applicationschema/cap-iacs-base/code#CropItemCodeValue/flowersAndOrnamentalPlantsExcludingNurseries -->


    <owl:NamedIndividual rdf:about="http://lpis.ec.europa.eu/registry/applicationschema/cap-iacs-base/code#CropItemCodeValue/flowersAndOrnamentalPlantsExcludingNurseries">
        <rdf:type rdf:resource="http://lpis.ec.europa.eu/registry/applicationschema/cap-iacs-base#CropItemCodeValue"/>
        <rdfs:label xml:lang="en">Flowers and ornamental plants (excluding nurseries)</rdfs:label>
        <skos:definition xml:lang="en">-- Definition --
|||Flowers and ornamental plants (excluding nurseries).
-- Description --
Land use of Agriculture Area in Use -L
NOTE. Initial value:L3001</skos:definition>
        <skos:inScheme rdf:resource="http://lpis.ec.europa.eu/registry/applicationschema/cap-iacs-base/code#CropItemCodeValue"/>
    </owl:NamedIndividual>
    


    <!-- http://lpis.ec.europa.eu/registry/applicationschema/cap-iacs-base/code#CropItemCodeValue/flowersAndOrnamentalPlantsUnderGlassHighAccessibleCover -->


    <owl:NamedIndividual rdf:about="http://lpis.ec.europa.eu/registry/applicationschema/cap-iacs-base/code#CropItemCodeValue/flowersAndOrnamentalPlantsUnderGlassHighAccessibleCover">
        <rdf:type rdf:resource="http://lpis.ec.europa.eu/registry/applicationschema/cap-iacs-base#CropItemCodeValue"/>
        <rdfs:label xml:lang="en">Flowers and ornamental plants under glass high accessible cover</rdfs:label>
        <skos:definition xml:lang="en">-- Definition --
Flowers and ornamental plants under glass high accessible cover.
-- Description --
Land use of Agriculture Area in Use -L. Special aggregates
NOTE. Initial value:L1113</skos:definition>
        <skos:inScheme rdf:resource="http://lpis.ec.europa.eu/registry/applicationschema/cap-iacs-base/code#CropItemCodeValue"/>
    </owl:NamedIndividual>
    


    <!-- http://lpis.ec.europa.eu/registry/applicationschema/cap-iacs-base/code#CropItemCodeValue/fruitAndBerryPlantations -->


    <owl:NamedIndividual rdf:about="http://lpis.ec.europa.eu/registry/applicationschema/cap-iacs-base/code#CropItemCodeValue/fruitAndBerryPlantations">
        <rdf:type rdf:resource="http://lpis.ec.europa.eu/registry/applicationschema/cap-iacs-base#CropItemCodeValue"/>
        <rdfs:label xml:lang="en">Fruit and berry plantations</rdfs:label>
        <skos:definition xml:lang="en">-- Definition --
|||Fruit and berry plantations.
-- Description --
Land use of Agriculture Area in Use -L
NOTE. Initial value:L0011</skos:definition>
        <skos:inScheme rdf:resource="http://lpis.ec.europa.eu/registry/applicationschema/cap-iacs-base/code#CropItemCodeValue"/>
    </owl:NamedIndividual>
    


    <!-- http://lpis.ec.europa.eu/registry/applicationschema/cap-iacs-base/code#CropItemCodeValue/garlic -->


    <owl:NamedIndividual rdf:about="http://lpis.ec.europa.eu/registry/applicationschema/cap-iacs-base/code#CropItemCodeValue/garlic">
        <rdf:type rdf:resource="http://lpis.ec.europa.eu/registry/applicationschema/cap-iacs-base#CropItemCodeValue"/>
        <rdfs:label xml:lang="en">Garlic</rdfs:label>
        <skos:definition xml:lang="en">-- Definition --
|||Garlic.
-- Description --
Cereals and main crops - C
NOTE. Initial value:C1840</skos:definition>
        <skos:inScheme rdf:resource="http://lpis.ec.europa.eu/registry/applicationschema/cap-iacs-base/code#CropItemCodeValue"/>
    </owl:NamedIndividual>
    


    <!-- http://lpis.ec.europa.eu/registry/applicationschema/cap-iacs-base/code#CropItemCodeValue/gherkins -->


    <owl:NamedIndividual rdf:about="http://lpis.ec.europa.eu/registry/applicationschema/cap-iacs-base/code#CropItemCodeValue/gherkins">
        <rdf:type rdf:resource="http://lpis.ec.europa.eu/registry/applicationschema/cap-iacs-base#CropItemCodeValue"/>
        <rdfs:label xml:lang="en">Gherkins</rdfs:label>
        <skos:definition xml:lang="en">-- Definition --
|||Gherkins.
-- Description --
Cereals and main crops - C
NOTE. Initial value:C1766</skos:definition>
        <skos:inScheme rdf:resource="http://lpis.ec.europa.eu/registry/applicationschema/cap-iacs-base/code#CropItemCodeValue"/>
    </owl:NamedIndividual>
    


    <!-- http://lpis.ec.europa.eu/registry/applicationschema/cap-iacs-base/code#CropItemCodeValue/goldenDelicious -->


    <owl:NamedIndividual rdf:about="http://lpis.ec.europa.eu/registry/applicationschema/cap-iacs-base/code#CropItemCodeValue/goldenDelicious">
        <rdf:type rdf:resource="http://lpis.ec.europa.eu/registry/applicationschema/cap-iacs-base#CropItemCodeValue"/>
        <rdfs:label xml:lang="en">Golden Delicious</rdfs:label>
        <skos:definition xml:lang="en">-- Definition --
||||Golden Delicious.
-- Description --
Cereals and main crops - C
NOTE. Initial value:C2112</skos:definition>
        <skos:inScheme rdf:resource="http://lpis.ec.europa.eu/registry/applicationschema/cap-iacs-base/code#CropItemCodeValue"/>
    </owl:NamedIndividual>
    


    <!-- http://lpis.ec.europa.eu/registry/applicationschema/cap-iacs-base/code#CropItemCodeValue/gooseberries -->


    <owl:NamedIndividual rdf:about="http://lpis.ec.europa.eu/registry/applicationschema/cap-iacs-base/code#CropItemCodeValue/gooseberries">
        <rdf:type rdf:resource="http://lpis.ec.europa.eu/registry/applicationschema/cap-iacs-base#CropItemCodeValue"/>
        <rdfs:label xml:lang="en">Gooseberries</rdfs:label>
        <skos:definition xml:lang="en">-- Definition --
|||Gooseberries.
-- Description --
Cereals and main crops - C
NOTE. Initial value:C2281</skos:definition>
        <skos:inScheme rdf:resource="http://lpis.ec.europa.eu/registry/applicationschema/cap-iacs-base/code#CropItemCodeValue"/>
    </owl:NamedIndividual>
    


    <!-- http://lpis.ec.europa.eu/registry/applicationschema/cap-iacs-base/code#CropItemCodeValue/gourdsMarrowsAndPumpkins -->


    <owl:NamedIndividual rdf:about="http://lpis.ec.europa.eu/registry/applicationschema/cap-iacs-base/code#CropItemCodeValue/gourdsMarrowsAndPumpkins">
        <rdf:type rdf:resource="http://lpis.ec.europa.eu/registry/applicationschema/cap-iacs-base#CropItemCodeValue"/>
        <rdfs:label xml:lang="en">Gourds, marrows and pumpkins</rdfs:label>
        <skos:definition xml:lang="en">-- Definition --
||||Gourds, marrows and pumpkins.
-- Description --
Cereals and main crops - C
NOTE. Initial value:C1786</skos:definition>
        <skos:inScheme rdf:resource="http://lpis.ec.europa.eu/registry/applicationschema/cap-iacs-base/code#CropItemCodeValue"/>
    </owl:NamedIndividual>
    


    <!-- http://lpis.ec.europa.eu/registry/applicationschema/cap-iacs-base/code#CropItemCodeValue/grainMaize -->


    <owl:NamedIndividual rdf:about="http://lpis.ec.europa.eu/registry/applicationschema/cap-iacs-base/code#CropItemCodeValue/grainMaize">
        <rdf:type rdf:resource="http://lpis.ec.europa.eu/registry/applicationschema/cap-iacs-base#CropItemCodeValue"/>
        <rdfs:label xml:lang="en">Grain maize</rdfs:label>
        <skos:definition xml:lang="en">-- Definition --
||||Grain maize.
-- Description --
Cereals and main crops - C
NOTE. Initial value:C1200</skos:definition>
        <skos:inScheme rdf:resource="http://lpis.ec.europa.eu/registry/applicationschema/cap-iacs-base/code#CropItemCodeValue"/>
    </owl:NamedIndividual>
    


    <!-- http://lpis.ec.europa.eu/registry/applicationschema/cap-iacs-base/code#CropItemCodeValue/grainMaizeAndCornCobMix -->


    <owl:NamedIndividual rdf:about="http://lpis.ec.europa.eu/registry/applicationschema/cap-iacs-base/code#CropItemCodeValue/grainMaizeAndCornCobMix">
        <rdf:type rdf:resource="http://lpis.ec.europa.eu/registry/applicationschema/cap-iacs-base#CropItemCodeValue"/>
        <rdfs:label xml:lang="en">Grain maize and corn cob mix</rdfs:label>
        <skos:definition xml:lang="en">-- Definition --
|||Grain maize and corn cob mix.
-- Description --
Cereals and main crops - C
NOTE. Initial value:C1201</skos:definition>
        <skos:inScheme rdf:resource="http://lpis.ec.europa.eu/registry/applicationschema/cap-iacs-base/code#CropItemCodeValue"/>
    </owl:NamedIndividual>
    


    <!-- http://lpis.ec.europa.eu/registry/applicationschema/cap-iacs-base/code#CropItemCodeValue/greenMaize -->


    <owl:NamedIndividual rdf:about="http://lpis.ec.europa.eu/registry/applicationschema/cap-iacs-base/code#CropItemCodeValue/greenMaize">
        <rdf:type rdf:resource="http://lpis.ec.europa.eu/registry/applicationschema/cap-iacs-base#CropItemCodeValue"/>
        <rdfs:label xml:lang="en">Green maize</rdfs:label>
        <skos:definition xml:lang="en">-- Definition --
|||Green maize.
-- Description --
Cereals and main crops - C
NOTE. Initial value:C2625</skos:definition>
        <skos:inScheme rdf:resource="http://lpis.ec.europa.eu/registry/applicationschema/cap-iacs-base/code#CropItemCodeValue"/>
    </owl:NamedIndividual>
    


    <!-- http://lpis.ec.europa.eu/registry/applicationschema/cap-iacs-base/code#CropItemCodeValue/hazelnuts -->


    <owl:NamedIndividual rdf:about="http://lpis.ec.europa.eu/registry/applicationschema/cap-iacs-base/code#CropItemCodeValue/hazelnuts">
        <rdf:type rdf:resource="http://lpis.ec.europa.eu/registry/applicationschema/cap-iacs-base#CropItemCodeValue"/>
        <rdfs:label xml:lang="en">Hazelnuts</rdfs:label>
        <skos:definition xml:lang="en">-- Definition --
|||Hazelnuts.
-- Description --
Cereals and main crops - C
NOTE. Initial value:C2232</skos:definition>
        <skos:inScheme rdf:resource="http://lpis.ec.europa.eu/registry/applicationschema/cap-iacs-base/code#CropItemCodeValue"/>
    </owl:NamedIndividual>
    


    <!-- http://lpis.ec.europa.eu/registry/applicationschema/cap-iacs-base/code#CropItemCodeValue/hemp -->


    <owl:NamedIndividual rdf:about="http://lpis.ec.europa.eu/registry/applicationschema/cap-iacs-base/code#CropItemCodeValue/hemp">
        <rdf:type rdf:resource="http://lpis.ec.europa.eu/registry/applicationschema/cap-iacs-base#CropItemCodeValue"/>
        <rdfs:label xml:lang="en">Hemp</rdfs:label>
        <skos:definition xml:lang="en">-- Definition --
|||Hemp.
-- Description --
Cereals and main crops - C
NOTE. Initial value:C1530</skos:definition>
        <skos:inScheme rdf:resource="http://lpis.ec.europa.eu/registry/applicationschema/cap-iacs-base/code#CropItemCodeValue"/>
    </owl:NamedIndividual>
    


    <!-- http://lpis.ec.europa.eu/registry/applicationschema/cap-iacs-base/code#CropItemCodeValue/hops -->


    <owl:NamedIndividual rdf:about="http://lpis.ec.europa.eu/registry/applicationschema/cap-iacs-base/code#CropItemCodeValue/hops">
        <rdf:type rdf:resource="http://lpis.ec.europa.eu/registry/applicationschema/cap-iacs-base#CropItemCodeValue"/>
        <rdfs:label xml:lang="en">Hops</rdfs:label>
        <skos:definition xml:lang="en">-- Definition --
||Hops.
-- Description --
Cereals and main crops - C
NOTE. Initial value:C1560</skos:definition>
        <skos:inScheme rdf:resource="http://lpis.ec.europa.eu/registry/applicationschema/cap-iacs-base/code#CropItemCodeValue"/>
    </owl:NamedIndividual>
    


    <!-- http://lpis.ec.europa.eu/registry/applicationschema/cap-iacs-base/code#CropItemCodeValue/industrialCrops -->


    <owl:NamedIndividual rdf:about="http://lpis.ec.europa.eu/registry/applicationschema/cap-iacs-base/code#CropItemCodeValue/industrialCrops">
        <rdf:type rdf:resource="http://lpis.ec.europa.eu/registry/applicationschema/cap-iacs-base#CropItemCodeValue"/>
        <rdfs:label xml:lang="en">Industrial crops </rdfs:label>
        <skos:definition xml:lang="en">-- Definition --
|Industrial crops .
-- Description --
Cereals and main crops - C
NOTE. Initial value:C1400</skos:definition>
        <skos:inScheme rdf:resource="http://lpis.ec.europa.eu/registry/applicationschema/cap-iacs-base/code#CropItemCodeValue"/>
    </owl:NamedIndividual>
    


    <!-- http://lpis.ec.europa.eu/registry/applicationschema/cap-iacs-base/code#CropItemCodeValue/industrialCropsL1400 -->


    <owl:NamedIndividual rdf:about="http://lpis.ec.europa.eu/registry/applicationschema/cap-iacs-base/code#CropItemCodeValue/industrialCropsL1400">
        <rdf:type rdf:resource="http://lpis.ec.europa.eu/registry/applicationschema/cap-iacs-base#CropItemCodeValue"/>
        <rdfs:label xml:lang="en">Industrial crops L1400</rdfs:label>
        <skos:definition xml:lang="en">-- Definition --
|||Industrial crops L1400.
-- Description --
Land use of Agriculture Area in Use -L
NOTE. Initial value:L1400</skos:definition>
        <skos:inScheme rdf:resource="http://lpis.ec.europa.eu/registry/applicationschema/cap-iacs-base/code#CropItemCodeValue"/>
    </owl:NamedIndividual>
    


    <!-- http://lpis.ec.europa.eu/registry/applicationschema/cap-iacs-base/code#CropItemCodeValue/kitchenGardens -->


    <owl:NamedIndividual rdf:about="http://lpis.ec.europa.eu/registry/applicationschema/cap-iacs-base/code#CropItemCodeValue/kitchenGardens">
        <rdf:type rdf:resource="http://lpis.ec.europa.eu/registry/applicationschema/cap-iacs-base#CropItemCodeValue"/>
        <rdfs:label xml:lang="en">Kitchen gardens</rdfs:label>
        <skos:definition xml:lang="en">-- Definition --
||Kitchen gardens.
-- Description --
Land use of Agriculture Area in Use -L
NOTE. Initial value:L0004</skos:definition>
        <skos:inScheme rdf:resource="http://lpis.ec.europa.eu/registry/applicationschema/cap-iacs-base/code#CropItemCodeValue"/>
    </owl:NamedIndividual>
    


    <!-- http://lpis.ec.europa.eu/registry/applicationschema/cap-iacs-base/code#CropItemCodeValue/kiwis -->


    <owl:NamedIndividual rdf:about="http://lpis.ec.europa.eu/registry/applicationschema/cap-iacs-base/code#CropItemCodeValue/kiwis">
        <rdf:type rdf:resource="http://lpis.ec.europa.eu/registry/applicationschema/cap-iacs-base#CropItemCodeValue"/>
        <rdfs:label xml:lang="en">Kiwis</rdfs:label>
        <skos:definition xml:lang="en">-- Definition --
|||Kiwis.
-- Description --
Cereals and main crops - C
NOTE. Initial value:C2285</skos:definition>
        <skos:inScheme rdf:resource="http://lpis.ec.europa.eu/registry/applicationschema/cap-iacs-base/code#CropItemCodeValue"/>
    </owl:NamedIndividual>
    


    <!-- http://lpis.ec.europa.eu/registry/applicationschema/cap-iacs-base/code#CropItemCodeValue/kohlRabiC1650 -->


    <owl:NamedIndividual rdf:about="http://lpis.ec.europa.eu/registry/applicationschema/cap-iacs-base/code#CropItemCodeValue/kohlRabiC1650">
        <rdf:type rdf:resource="http://lpis.ec.europa.eu/registry/applicationschema/cap-iacs-base#CropItemCodeValue"/>
        <rdfs:label xml:lang="en">Kohl-Rabi C1650</rdfs:label>
        <skos:definition xml:lang="en">-- Definition --
|||Kohl-Rabi C1650.
-- Description --
Cereals and main crops - C
NOTE. Initial value:C1650</skos:definition>
        <skos:inScheme rdf:resource="http://lpis.ec.europa.eu/registry/applicationschema/cap-iacs-base/code#CropItemCodeValue"/>
    </owl:NamedIndividual>
    


    <!-- http://lpis.ec.europa.eu/registry/applicationschema/cap-iacs-base/code#CropItemCodeValue/leafyOrStalkedVegetablesExcludingBrassicas -->


    <owl:NamedIndividual rdf:about="http://lpis.ec.europa.eu/registry/applicationschema/cap-iacs-base/code#CropItemCodeValue/leafyOrStalkedVegetablesExcludingBrassicas">
        <rdf:type rdf:resource="http://lpis.ec.europa.eu/registry/applicationschema/cap-iacs-base#CropItemCodeValue"/>
        <rdfs:label xml:lang="en">Leafy or stalked vegetables (excluding brassicas)</rdfs:label>
        <skos:definition xml:lang="en">-- Definition --
||Leafy or stalked vegetables (excluding brassicas).
-- Description --
Cereals and main crops - C
NOTE. Initial value:C1660</skos:definition>
        <skos:inScheme rdf:resource="http://lpis.ec.europa.eu/registry/applicationschema/cap-iacs-base/code#CropItemCodeValue"/>
    </owl:NamedIndividual>
    


    <!-- http://lpis.ec.europa.eu/registry/applicationschema/cap-iacs-base/code#CropItemCodeValue/leeks -->


    <owl:NamedIndividual rdf:about="http://lpis.ec.europa.eu/registry/applicationschema/cap-iacs-base/code#CropItemCodeValue/leeks">
        <rdf:type rdf:resource="http://lpis.ec.europa.eu/registry/applicationschema/cap-iacs-base#CropItemCodeValue"/>
        <rdfs:label xml:lang="en">Leeks</rdfs:label>
        <skos:definition xml:lang="en">-- Definition --
|||Leeks.
-- Description --
Cereals and main crops - C
NOTE. Initial value:C1675</skos:definition>
        <skos:inScheme rdf:resource="http://lpis.ec.europa.eu/registry/applicationschema/cap-iacs-base/code#CropItemCodeValue"/>
    </owl:NamedIndividual>
    


    <!-- http://lpis.ec.europa.eu/registry/applicationschema/cap-iacs-base/code#CropItemCodeValue/leguminousPlants -->


    <owl:NamedIndividual rdf:about="http://lpis.ec.europa.eu/registry/applicationschema/cap-iacs-base/code#CropItemCodeValue/leguminousPlants">
        <rdf:type rdf:resource="http://lpis.ec.europa.eu/registry/applicationschema/cap-iacs-base#CropItemCodeValue"/>
        <rdfs:label xml:lang="en">Leguminous plants</rdfs:label>
        <skos:definition xml:lang="en">-- Definition --
||Leguminous plants.
-- Description --
Cereals and main crops - C
NOTE. Initial value:C2670</skos:definition>
        <skos:inScheme rdf:resource="http://lpis.ec.europa.eu/registry/applicationschema/cap-iacs-base/code#CropItemCodeValue"/>
    </owl:NamedIndividual>
    


    <!-- http://lpis.ec.europa.eu/registry/applicationschema/cap-iacs-base/code#CropItemCodeValue/lemonsAndAcidLimesC2370 -->


    <owl:NamedIndividual rdf:about="http://lpis.ec.europa.eu/registry/applicationschema/cap-iacs-base/code#CropItemCodeValue/lemonsAndAcidLimesC2370">
        <rdf:type rdf:resource="http://lpis.ec.europa.eu/registry/applicationschema/cap-iacs-base#CropItemCodeValue"/>
        <rdfs:label xml:lang="en">Lemons and acid limes C2370</rdfs:label>
        <skos:definition xml:lang="en">-- Definition --
|||Lemons and acid limes C2370.
-- Description --
Cereals and main crops - C
NOTE. Initial value:C2370</skos:definition>
        <skos:inScheme rdf:resource="http://lpis.ec.europa.eu/registry/applicationschema/cap-iacs-base/code#CropItemCodeValue"/>
    </owl:NamedIndividual>
    


    <!-- http://lpis.ec.europa.eu/registry/applicationschema/cap-iacs-base/code#CropItemCodeValue/lettuces -->


    <owl:NamedIndividual rdf:about="http://lpis.ec.europa.eu/registry/applicationschema/cap-iacs-base/code#CropItemCodeValue/lettuces">
        <rdf:type rdf:resource="http://lpis.ec.europa.eu/registry/applicationschema/cap-iacs-base#CropItemCodeValue"/>
        <rdfs:label xml:lang="en">Lettuces</rdfs:label>
        <skos:definition xml:lang="en">-- Definition --
|||Lettuces.
-- Description --
Cereals and main crops - C
NOTE. Initial value:C1680</skos:definition>
        <skos:inScheme rdf:resource="http://lpis.ec.europa.eu/registry/applicationschema/cap-iacs-base/code#CropItemCodeValue"/>
    </owl:NamedIndividual>
    


    <!-- http://lpis.ec.europa.eu/registry/applicationschema/cap-iacs-base/code#CropItemCodeValue/lettucesUnderGlassOrHighAccessibleCoverC1681 -->


    <owl:NamedIndividual rdf:about="http://lpis.ec.europa.eu/registry/applicationschema/cap-iacs-base/code#CropItemCodeValue/lettucesUnderGlassOrHighAccessibleCoverC1681">
        <rdf:type rdf:resource="http://lpis.ec.europa.eu/registry/applicationschema/cap-iacs-base#CropItemCodeValue"/>
        <rdfs:label xml:lang="en">Lettuces under glass or high accessible cover C1681 </rdfs:label>
        <skos:definition xml:lang="en">-- Definition --
||||Lettuces under glass or high accessible cover C1681.
-- Description --
Cereals and main crops - C
NOTE. Initial value:C1681</skos:definition>
        <skos:inScheme rdf:resource="http://lpis.ec.europa.eu/registry/applicationschema/cap-iacs-base/code#CropItemCodeValue"/>
    </owl:NamedIndividual>
    


    <!-- http://lpis.ec.europa.eu/registry/applicationschema/cap-iacs-base/code#CropItemCodeValue/linseedOilFlax -->


    <owl:NamedIndividual rdf:about="http://lpis.ec.europa.eu/registry/applicationschema/cap-iacs-base/code#CropItemCodeValue/linseedOilFlax">
        <rdf:type rdf:resource="http://lpis.ec.europa.eu/registry/applicationschema/cap-iacs-base#CropItemCodeValue"/>
        <rdfs:label xml:lang="en">Linseed (oil flax)</rdfs:label>
        <skos:definition xml:lang="en">-- Definition --
||||Linseed (oil flax).
-- Description --
Cereals and main crops - C
NOTE. Initial value:C1460</skos:definition>
        <skos:inScheme rdf:resource="http://lpis.ec.europa.eu/registry/applicationschema/cap-iacs-base/code#CropItemCodeValue"/>
    </owl:NamedIndividual>
    


    <!-- http://lpis.ec.europa.eu/registry/applicationschema/cap-iacs-base/code#CropItemCodeValue/lucerne -->


    <owl:NamedIndividual rdf:about="http://lpis.ec.europa.eu/registry/applicationschema/cap-iacs-base/code#CropItemCodeValue/lucerne">
        <rdf:type rdf:resource="http://lpis.ec.europa.eu/registry/applicationschema/cap-iacs-base#CropItemCodeValue"/>
        <rdfs:label xml:lang="en">Lucerne</rdfs:label>
        <skos:definition xml:lang="en">-- Definition --
|||Lucerne.
-- Description --
Cereals and main crops - C
NOTE. Initial value:C2672</skos:definition>
        <skos:inScheme rdf:resource="http://lpis.ec.europa.eu/registry/applicationschema/cap-iacs-base/code#CropItemCodeValue"/>
    </owl:NamedIndividual>
    


    <!-- http://lpis.ec.europa.eu/registry/applicationschema/cap-iacs-base/code#CropItemCodeValue/mainOilSeedCrops -->


    <owl:NamedIndividual rdf:about="http://lpis.ec.europa.eu/registry/applicationschema/cap-iacs-base/code#CropItemCodeValue/mainOilSeedCrops">
        <rdf:type rdf:resource="http://lpis.ec.europa.eu/registry/applicationschema/cap-iacs-base#CropItemCodeValue"/>
        <rdfs:label xml:lang="en">Main oil seed crops</rdfs:label>
        <skos:definition xml:lang="en">-- Definition --
|||Main oil seed crops.
-- Description --
Cereals and main crops - C
NOTE. Initial value:C1415</skos:definition>
        <skos:inScheme rdf:resource="http://lpis.ec.europa.eu/registry/applicationschema/cap-iacs-base/code#CropItemCodeValue"/>
    </owl:NamedIndividual>
    


    <!-- http://lpis.ec.europa.eu/registry/applicationschema/cap-iacs-base/code#CropItemCodeValue/maslin -->


    <owl:NamedIndividual rdf:about="http://lpis.ec.europa.eu/registry/applicationschema/cap-iacs-base/code#CropItemCodeValue/maslin">
        <rdf:type rdf:resource="http://lpis.ec.europa.eu/registry/applicationschema/cap-iacs-base#CropItemCodeValue"/>
        <rdfs:label xml:lang="en">Maslin</rdfs:label>
        <skos:definition xml:lang="en">-- Definition --
||||Maslin.
-- Description --
Cereals and main crops - C
NOTE. Initial value:C1155</skos:definition>
        <skos:inScheme rdf:resource="http://lpis.ec.europa.eu/registry/applicationschema/cap-iacs-base/code#CropItemCodeValue"/>
    </owl:NamedIndividual>
    


    <!-- http://lpis.ec.europa.eu/registry/applicationschema/cap-iacs-base/code#CropItemCodeValue/melons -->


    <owl:NamedIndividual rdf:about="http://lpis.ec.europa.eu/registry/applicationschema/cap-iacs-base/code#CropItemCodeValue/melons">
        <rdf:type rdf:resource="http://lpis.ec.europa.eu/registry/applicationschema/cap-iacs-base#CropItemCodeValue"/>
        <rdfs:label xml:lang="en">Melons</rdfs:label>
        <skos:definition xml:lang="en">-- Definition --
||Melons.
-- Description --
Cereals and main crops - C
NOTE. Initial value:C1771</skos:definition>
        <skos:inScheme rdf:resource="http://lpis.ec.europa.eu/registry/applicationschema/cap-iacs-base/code#CropItemCodeValue"/>
    </owl:NamedIndividual>
    


    <!-- http://lpis.ec.europa.eu/registry/applicationschema/cap-iacs-base/code#CropItemCodeValue/mixedGrainOtherThanMaslinC1185 -->


    <owl:NamedIndividual rdf:about="http://lpis.ec.europa.eu/registry/applicationschema/cap-iacs-base/code#CropItemCodeValue/mixedGrainOtherThanMaslinC1185">
        <rdf:type rdf:resource="http://lpis.ec.europa.eu/registry/applicationschema/cap-iacs-base#CropItemCodeValue"/>
        <rdfs:label xml:lang="en">Mixed grain other than maslin C1185</rdfs:label>
        <skos:definition xml:lang="en">-- Definition --
||||Mixed grain other than maslin C1185.
-- Description --
Cereals and main crops - C
NOTE. Initial value:C1185</skos:definition>
        <skos:inScheme rdf:resource="http://lpis.ec.europa.eu/registry/applicationschema/cap-iacs-base/code#CropItemCodeValue"/>
    </owl:NamedIndividual>
    


    <!-- http://lpis.ec.europa.eu/registry/applicationschema/cap-iacs-base/code#CropItemCodeValue/nectarines -->


    <owl:NamedIndividual rdf:about="http://lpis.ec.europa.eu/registry/applicationschema/cap-iacs-base/code#CropItemCodeValue/nectarines">
        <rdf:type rdf:resource="http://lpis.ec.europa.eu/registry/applicationschema/cap-iacs-base#CropItemCodeValue"/>
        <rdfs:label xml:lang="en">Nectarines</rdfs:label>
        <skos:definition xml:lang="en">-- Definition --
|||Nectarines.
-- Description --
Cereals and main crops - C
NOTE. Initial value:C2221</skos:definition>
        <skos:inScheme rdf:resource="http://lpis.ec.europa.eu/registry/applicationschema/cap-iacs-base/code#CropItemCodeValue"/>
    </owl:NamedIndividual>
    


    <!-- http://lpis.ec.europa.eu/registry/applicationschema/cap-iacs-base/code#CropItemCodeValue/nurseries -->


    <owl:NamedIndividual rdf:about="http://lpis.ec.europa.eu/registry/applicationschema/cap-iacs-base/code#CropItemCodeValue/nurseries">
        <rdf:type rdf:resource="http://lpis.ec.europa.eu/registry/applicationschema/cap-iacs-base#CropItemCodeValue"/>
        <rdfs:label xml:lang="en">Nurseries</rdfs:label>
        <skos:definition xml:lang="en">-- Definition --
|||Nurseries.
-- Description --
Land use of Agriculture Area in Use -L
NOTE. Initial value:L2810</skos:definition>
        <skos:inScheme rdf:resource="http://lpis.ec.europa.eu/registry/applicationschema/cap-iacs-base/code#CropItemCodeValue"/>
    </owl:NamedIndividual>
    


    <!-- http://lpis.ec.europa.eu/registry/applicationschema/cap-iacs-base/code#CropItemCodeValue/nutsC2230 -->


    <owl:NamedIndividual rdf:about="http://lpis.ec.europa.eu/registry/applicationschema/cap-iacs-base/code#CropItemCodeValue/nutsC2230">
        <rdf:type rdf:resource="http://lpis.ec.europa.eu/registry/applicationschema/cap-iacs-base#CropItemCodeValue"/>
        <rdfs:label xml:lang="en">Nuts C2230</rdfs:label>
        <skos:definition xml:lang="en">-- Definition --
||Nuts C2230.
-- Description --
Cereals and main crops - C
NOTE. Initial value:C2230</skos:definition>
        <skos:inScheme rdf:resource="http://lpis.ec.europa.eu/registry/applicationschema/cap-iacs-base/code#CropItemCodeValue"/>
    </owl:NamedIndividual>
    


    <!-- http://lpis.ec.europa.eu/registry/applicationschema/cap-iacs-base/code#CropItemCodeValue/oats -->


    <owl:NamedIndividual rdf:about="http://lpis.ec.europa.eu/registry/applicationschema/cap-iacs-base/code#CropItemCodeValue/oats">
        <rdf:type rdf:resource="http://lpis.ec.europa.eu/registry/applicationschema/cap-iacs-base#CropItemCodeValue"/>
        <rdfs:label xml:lang="en">Oats</rdfs:label>
        <skos:definition xml:lang="en">-- Definition --
||||Oats.
-- Description --
Cereals and main crops - C
NOTE. Initial value:C1180</skos:definition>
        <skos:inScheme rdf:resource="http://lpis.ec.europa.eu/registry/applicationschema/cap-iacs-base/code#CropItemCodeValue"/>
    </owl:NamedIndividual>
    


    <!-- http://lpis.ec.europa.eu/registry/applicationschema/cap-iacs-base/code#CropItemCodeValue/oatsAndMixedGrainOtherThanMaslin -->


    <owl:NamedIndividual rdf:about="http://lpis.ec.europa.eu/registry/applicationschema/cap-iacs-base/code#CropItemCodeValue/oatsAndMixedGrainOtherThanMaslin">
        <rdf:type rdf:resource="http://lpis.ec.europa.eu/registry/applicationschema/cap-iacs-base#CropItemCodeValue"/>
        <rdfs:label xml:lang="en">Oats and mixed grain other than maslin</rdfs:label>
        <skos:definition xml:lang="en">-- Definition --
|||Oats and mixed grain other than maslin.
-- Description --
Cereals and main crops - C
NOTE. Initial value:C1170</skos:definition>
        <skos:inScheme rdf:resource="http://lpis.ec.europa.eu/registry/applicationschema/cap-iacs-base/code#CropItemCodeValue"/>
    </owl:NamedIndividual>
    


    <!-- http://lpis.ec.europa.eu/registry/applicationschema/cap-iacs-base/code#CropItemCodeValue/oilseeds -->


    <owl:NamedIndividual rdf:about="http://lpis.ec.europa.eu/registry/applicationschema/cap-iacs-base/code#CropItemCodeValue/oilseeds">
        <rdf:type rdf:resource="http://lpis.ec.europa.eu/registry/applicationschema/cap-iacs-base#CropItemCodeValue"/>
        <rdfs:label xml:lang="en">Oilseeds</rdfs:label>
        <skos:definition xml:lang="en">-- Definition --
||Oilseeds.
-- Description --
Cereals and main crops - C
NOTE. Initial value:C1410</skos:definition>
        <skos:inScheme rdf:resource="http://lpis.ec.europa.eu/registry/applicationschema/cap-iacs-base/code#CropItemCodeValue"/>
    </owl:NamedIndividual>
    


    <!-- http://lpis.ec.europa.eu/registry/applicationschema/cap-iacs-base/code#CropItemCodeValue/olivePlantations -->


    <owl:NamedIndividual rdf:about="http://lpis.ec.europa.eu/registry/applicationschema/cap-iacs-base/code#CropItemCodeValue/olivePlantations">
        <rdf:type rdf:resource="http://lpis.ec.europa.eu/registry/applicationschema/cap-iacs-base#CropItemCodeValue"/>
        <rdfs:label xml:lang="en">Olive plantations</rdfs:label>
        <skos:definition xml:lang="en">-- Definition --
|||Olive plantations.
-- Description --
Land use of Agriculture Area in Use -L
NOTE. Initial value:L2450</skos:definition>
        <skos:inScheme rdf:resource="http://lpis.ec.europa.eu/registry/applicationschema/cap-iacs-base/code#CropItemCodeValue"/>
    </owl:NamedIndividual>
    


    <!-- http://lpis.ec.europa.eu/registry/applicationschema/cap-iacs-base/code#CropItemCodeValue/oliveTreesC2450 -->


    <owl:NamedIndividual rdf:about="http://lpis.ec.europa.eu/registry/applicationschema/cap-iacs-base/code#CropItemCodeValue/oliveTreesC2450">
        <rdf:type rdf:resource="http://lpis.ec.europa.eu/registry/applicationschema/cap-iacs-base#CropItemCodeValue"/>
        <rdfs:label xml:lang="en">Olive trees C2450</rdfs:label>
        <skos:definition xml:lang="en">-- Definition --
||Olive trees C2450.
-- Description --
Cereals and main crops - C
NOTE. Initial value:C2450</skos:definition>
        <skos:inScheme rdf:resource="http://lpis.ec.europa.eu/registry/applicationschema/cap-iacs-base/code#CropItemCodeValue"/>
    </owl:NamedIndividual>
    


    <!-- http://lpis.ec.europa.eu/registry/applicationschema/cap-iacs-base/code#CropItemCodeValue/onions -->


    <owl:NamedIndividual rdf:about="http://lpis.ec.europa.eu/registry/applicationschema/cap-iacs-base/code#CropItemCodeValue/onions">
        <rdf:type rdf:resource="http://lpis.ec.europa.eu/registry/applicationschema/cap-iacs-base#CropItemCodeValue"/>
        <rdfs:label xml:lang="en">Onions</rdfs:label>
        <skos:definition xml:lang="en">-- Definition --
|||Onions.
-- Description --
Cereals and main crops - C
NOTE. Initial value:C1851</skos:definition>
        <skos:inScheme rdf:resource="http://lpis.ec.europa.eu/registry/applicationschema/cap-iacs-base/code#CropItemCodeValue"/>
    </owl:NamedIndividual>
    


    <!-- http://lpis.ec.europa.eu/registry/applicationschema/cap-iacs-base/code#CropItemCodeValue/oranges -->


    <owl:NamedIndividual rdf:about="http://lpis.ec.europa.eu/registry/applicationschema/cap-iacs-base/code#CropItemCodeValue/oranges">
        <rdf:type rdf:resource="http://lpis.ec.europa.eu/registry/applicationschema/cap-iacs-base#CropItemCodeValue"/>
        <rdfs:label xml:lang="en">Oranges</rdfs:label>
        <skos:definition xml:lang="en">-- Definition --
|||Oranges.
-- Description --
Cereals and main crops - C
NOTE. Initial value:C2320</skos:definition>
        <skos:inScheme rdf:resource="http://lpis.ec.europa.eu/registry/applicationschema/cap-iacs-base/code#CropItemCodeValue"/>
    </owl:NamedIndividual>
    


    <!-- http://lpis.ec.europa.eu/registry/applicationschema/cap-iacs-base/code#CropItemCodeValue/otherAnnualPlantsHarvestedGreenNecC2612 -->


    <owl:NamedIndividual rdf:about="http://lpis.ec.europa.eu/registry/applicationschema/cap-iacs-base/code#CropItemCodeValue/otherAnnualPlantsHarvestedGreenNecC2612">
        <rdf:type rdf:resource="http://lpis.ec.europa.eu/registry/applicationschema/cap-iacs-base#CropItemCodeValue"/>
        <rdfs:label xml:lang="en">Other annual plants harvested green n.e.c. C2612</rdfs:label>
        <skos:definition xml:lang="en">-- Definition --
|||Other annual plants harvested green n.e.c. C2612.
-- Description --
Cereals and main crops - C
NOTE. Initial value:C2612</skos:definition>
        <skos:inScheme rdf:resource="http://lpis.ec.europa.eu/registry/applicationschema/cap-iacs-base/code#CropItemCodeValue"/>
    </owl:NamedIndividual>
    


    <!-- http://lpis.ec.europa.eu/registry/applicationschema/cap-iacs-base/code#CropItemCodeValue/otherApplesForFreshConsumption -->


    <owl:NamedIndividual rdf:about="http://lpis.ec.europa.eu/registry/applicationschema/cap-iacs-base/code#CropItemCodeValue/otherApplesForFreshConsumption">
        <rdf:type rdf:resource="http://lpis.ec.europa.eu/registry/applicationschema/cap-iacs-base#CropItemCodeValue"/>
        <rdfs:label xml:lang="en">Other apples for fresh consumption</rdfs:label>
        <skos:definition xml:lang="en">-- Definition --
||||Other apples for fresh consumption.
-- Description --
Cereals and main crops - C
NOTE. Initial value:C2113</skos:definition>
        <skos:inScheme rdf:resource="http://lpis.ec.europa.eu/registry/applicationschema/cap-iacs-base/code#CropItemCodeValue"/>
    </owl:NamedIndividual>
    


    <!-- http://lpis.ec.europa.eu/registry/applicationschema/cap-iacs-base/code#CropItemCodeValue/otherArableLandCrops -->


    <owl:NamedIndividual rdf:about="http://lpis.ec.europa.eu/registry/applicationschema/cap-iacs-base/code#CropItemCodeValue/otherArableLandCrops">
        <rdf:type rdf:resource="http://lpis.ec.europa.eu/registry/applicationschema/cap-iacs-base#CropItemCodeValue"/>
        <rdfs:label xml:lang="en">Other arable-land crops</rdfs:label>
        <skos:definition xml:lang="en">-- Definition --
|||Other arable-land crops.
-- Description --
Land use of Agriculture Area in Use -L
NOTE. Initial value:L2690</skos:definition>
        <skos:inScheme rdf:resource="http://lpis.ec.europa.eu/registry/applicationschema/cap-iacs-base/code#CropItemCodeValue"/>
    </owl:NamedIndividual>
    


    <!-- http://lpis.ec.europa.eu/registry/applicationschema/cap-iacs-base/code#CropItemCodeValue/otherBerriesNec -->


    <owl:NamedIndividual rdf:about="http://lpis.ec.europa.eu/registry/applicationschema/cap-iacs-base/code#CropItemCodeValue/otherBerriesNec">
        <rdf:type rdf:resource="http://lpis.ec.europa.eu/registry/applicationschema/cap-iacs-base#CropItemCodeValue"/>
        <rdfs:label xml:lang="en">Other berries n.e.c.</rdfs:label>
        <skos:definition xml:lang="en">-- Definition --
|||Other berries n.e.c.
-- Description --
Cereals and main crops - C
NOTE. Initial value:C2290</skos:definition>
        <skos:inScheme rdf:resource="http://lpis.ec.europa.eu/registry/applicationschema/cap-iacs-base/code#CropItemCodeValue"/>
    </owl:NamedIndividual>
    


    <!-- http://lpis.ec.europa.eu/registry/applicationschema/cap-iacs-base/code#CropItemCodeValue/otherBrassicasNec -->


    <owl:NamedIndividual rdf:about="http://lpis.ec.europa.eu/registry/applicationschema/cap-iacs-base/code#CropItemCodeValue/otherBrassicasNec">
        <rdf:type rdf:resource="http://lpis.ec.europa.eu/registry/applicationschema/cap-iacs-base#CropItemCodeValue"/>
        <rdfs:label xml:lang="en">Other brassicas n.e.c.</rdfs:label>
        <skos:definition xml:lang="en">-- Definition --
|||Other brassicas n.e.c.
-- Description --
Cereals and main crops - C
NOTE. Initial value:C1655</skos:definition>
        <skos:inScheme rdf:resource="http://lpis.ec.europa.eu/registry/applicationschema/cap-iacs-base/code#CropItemCodeValue"/>
    </owl:NamedIndividual>
    


    <!-- http://lpis.ec.europa.eu/registry/applicationschema/cap-iacs-base/code#CropItemCodeValue/otherCitrusFruitsNec -->


    <owl:NamedIndividual rdf:about="http://lpis.ec.europa.eu/registry/applicationschema/cap-iacs-base/code#CropItemCodeValue/otherCitrusFruitsNec">
        <rdf:type rdf:resource="http://lpis.ec.europa.eu/registry/applicationschema/cap-iacs-base#CropItemCodeValue"/>
        <rdfs:label xml:lang="en">Other citrus fruits n.e.c.</rdfs:label>
        <skos:definition xml:lang="en">-- Definition --
|||Other citrus fruits n.e.c.
-- Description --
Cereals and main crops - C
NOTE. Initial value:C2390</skos:definition>
        <skos:inScheme rdf:resource="http://lpis.ec.europa.eu/registry/applicationschema/cap-iacs-base/code#CropItemCodeValue"/>
    </owl:NamedIndividual>
    


    <!-- http://lpis.ec.europa.eu/registry/applicationschema/cap-iacs-base/code#CropItemCodeValue/otherDriedPulsesNecC1345 -->


    <owl:NamedIndividual rdf:about="http://lpis.ec.europa.eu/registry/applicationschema/cap-iacs-base/code#CropItemCodeValue/otherDriedPulsesNecC1345">
        <rdf:type rdf:resource="http://lpis.ec.europa.eu/registry/applicationschema/cap-iacs-base#CropItemCodeValue"/>
        <rdfs:label xml:lang="en">Other dried pulses n.e.c. C1345</rdfs:label>
        <skos:definition xml:lang="en">-- Definition --
||Other dried pulses n.e.c. C1345.
-- Description --
Cereals and main crops - C
NOTE. Initial value:C1345</skos:definition>
        <skos:inScheme rdf:resource="http://lpis.ec.europa.eu/registry/applicationschema/cap-iacs-base/code#CropItemCodeValue"/>
    </owl:NamedIndividual>
    


    <!-- http://lpis.ec.europa.eu/registry/applicationschema/cap-iacs-base/code#CropItemCodeValue/otherFibreCropsNec -->


    <owl:NamedIndividual rdf:about="http://lpis.ec.europa.eu/registry/applicationschema/cap-iacs-base/code#CropItemCodeValue/otherFibreCropsNec">
        <rdf:type rdf:resource="http://lpis.ec.europa.eu/registry/applicationschema/cap-iacs-base#CropItemCodeValue"/>
        <rdfs:label xml:lang="en">Other fibre crops n.e.c.</rdfs:label>
        <skos:definition xml:lang="en">-- Definition --
|||Other fibre crops n.e.c.
-- Description --
Cereals and main crops - C
NOTE. Initial value:C1510</skos:definition>
        <skos:inScheme rdf:resource="http://lpis.ec.europa.eu/registry/applicationschema/cap-iacs-base/code#CropItemCodeValue"/>
    </owl:NamedIndividual>
    


    <!-- http://lpis.ec.europa.eu/registry/applicationschema/cap-iacs-base/code#CropItemCodeValue/otherFreshVegetablesNec -->


    <owl:NamedIndividual rdf:about="http://lpis.ec.europa.eu/registry/applicationschema/cap-iacs-base/code#CropItemCodeValue/otherFreshVegetablesNec">
        <rdf:type rdf:resource="http://lpis.ec.europa.eu/registry/applicationschema/cap-iacs-base#CropItemCodeValue"/>
        <rdfs:label xml:lang="en">Other fresh vegetables n.e.c.</rdfs:label>
        <skos:definition xml:lang="en">-- Definition --
||Other fresh vegetables n.e.c.
-- Description --
Cereals and main crops - C
NOTE. Initial value:C1920</skos:definition>
        <skos:inScheme rdf:resource="http://lpis.ec.europa.eu/registry/applicationschema/cap-iacs-base/code#CropItemCodeValue"/>
    </owl:NamedIndividual>
    


    <!-- http://lpis.ec.europa.eu/registry/applicationschema/cap-iacs-base/code#CropItemCodeValue/otherFruitsFromFruitTrees -->


    <owl:NamedIndividual rdf:about="http://lpis.ec.europa.eu/registry/applicationschema/cap-iacs-base/code#CropItemCodeValue/otherFruitsFromFruitTrees">
        <rdf:type rdf:resource="http://lpis.ec.europa.eu/registry/applicationschema/cap-iacs-base#CropItemCodeValue"/>
        <rdfs:label xml:lang="en">Other fruits from fruit trees</rdfs:label>
        <skos:definition xml:lang="en">-- Definition --
||Other fruits from fruit trees.
-- Description --
Cereals and main crops - C
NOTE. Initial value:C2250</skos:definition>
        <skos:inScheme rdf:resource="http://lpis.ec.europa.eu/registry/applicationschema/cap-iacs-base/code#CropItemCodeValue"/>
    </owl:NamedIndividual>
    


    <!-- http://lpis.ec.europa.eu/registry/applicationschema/cap-iacs-base/code#CropItemCodeValue/otherFruitsFromFruitTreesNec -->


    <owl:NamedIndividual rdf:about="http://lpis.ec.europa.eu/registry/applicationschema/cap-iacs-base/code#CropItemCodeValue/otherFruitsFromFruitTreesNec">
        <rdf:type rdf:resource="http://lpis.ec.europa.eu/registry/applicationschema/cap-iacs-base#CropItemCodeValue"/>
        <rdfs:label xml:lang="en">Other fruits from fruit trees n.e.c.</rdfs:label>
        <skos:definition xml:lang="en">-- Definition --
|||Other fruits from fruit trees n.e.c.
-- Description --
Cereals and main crops - C
NOTE. Initial value:C2259</skos:definition>
        <skos:inScheme rdf:resource="http://lpis.ec.europa.eu/registry/applicationschema/cap-iacs-base/code#CropItemCodeValue"/>
    </owl:NamedIndividual>
    


    <!-- http://lpis.ec.europa.eu/registry/applicationschema/cap-iacs-base/code#CropItemCodeValue/otherIndustrialCrops -->


    <owl:NamedIndividual rdf:about="http://lpis.ec.europa.eu/registry/applicationschema/cap-iacs-base/code#CropItemCodeValue/otherIndustrialCrops">
        <rdf:type rdf:resource="http://lpis.ec.europa.eu/registry/applicationschema/cap-iacs-base#CropItemCodeValue"/>
        <rdfs:label xml:lang="en">Other industrial crops</rdfs:label>
        <skos:definition xml:lang="en">-- Definition --
||Other industrial crops.
-- Description --
Cereals and main crops - C
NOTE. Initial value:C1570</skos:definition>
        <skos:inScheme rdf:resource="http://lpis.ec.europa.eu/registry/applicationschema/cap-iacs-base/code#CropItemCodeValue"/>
    </owl:NamedIndividual>
    


    <!-- http://lpis.ec.europa.eu/registry/applicationschema/cap-iacs-base/code#CropItemCodeValue/otherIndustrialCropsNec -->


    <owl:NamedIndividual rdf:about="http://lpis.ec.europa.eu/registry/applicationschema/cap-iacs-base/code#CropItemCodeValue/otherIndustrialCropsNec">
        <rdf:type rdf:resource="http://lpis.ec.europa.eu/registry/applicationschema/cap-iacs-base#CropItemCodeValue"/>
        <rdfs:label xml:lang="en">Other industrial crops n.e.c.</rdfs:label>
        <skos:definition xml:lang="en">-- Definition --
|||Other industrial crops n.e.c.
-- Description --
Cereals and main crops - C
NOTE. Initial value:C1589</skos:definition>
        <skos:inScheme rdf:resource="http://lpis.ec.europa.eu/registry/applicationschema/cap-iacs-base/code#CropItemCodeValue"/>
    </owl:NamedIndividual>
    


    <!-- http://lpis.ec.europa.eu/registry/applicationschema/cap-iacs-base/code#CropItemCodeValue/otherLeafyOrStalkedVegetablesNec -->


    <owl:NamedIndividual rdf:about="http://lpis.ec.europa.eu/registry/applicationschema/cap-iacs-base/code#CropItemCodeValue/otherLeafyOrStalkedVegetablesNec">
        <rdf:type rdf:resource="http://lpis.ec.europa.eu/registry/applicationschema/cap-iacs-base#CropItemCodeValue"/>
        <rdfs:label xml:lang="en">Other leafy or stalked vegetables n.e.c.</rdfs:label>
        <skos:definition xml:lang="en">-- Definition --
|||Other leafy or stalked vegetables n.e.c.
-- Description --
Cereals and main crops - C
NOTE. Initial value:C1725</skos:definition>
        <skos:inScheme rdf:resource="http://lpis.ec.europa.eu/registry/applicationschema/cap-iacs-base/code#CropItemCodeValue"/>
    </owl:NamedIndividual>
    


    <!-- http://lpis.ec.europa.eu/registry/applicationschema/cap-iacs-base/code#CropItemCodeValue/otherLeguminousPlantsNec -->


    <owl:NamedIndividual rdf:about="http://lpis.ec.europa.eu/registry/applicationschema/cap-iacs-base/code#CropItemCodeValue/otherLeguminousPlantsNec">
        <rdf:type rdf:resource="http://lpis.ec.europa.eu/registry/applicationschema/cap-iacs-base#CropItemCodeValue"/>
        <rdfs:label xml:lang="en">Other leguminous plants n.e.c.</rdfs:label>
        <skos:definition xml:lang="en">-- Definition --
|||Other leguminous plants n.e.c.
-- Description --
Cereals and main crops - C
NOTE. Initial value:C2673</skos:definition>
        <skos:inScheme rdf:resource="http://lpis.ec.europa.eu/registry/applicationschema/cap-iacs-base/code#CropItemCodeValue"/>
    </owl:NamedIndividual>
    


    <!-- http://lpis.ec.europa.eu/registry/applicationschema/cap-iacs-base/code#CropItemCodeValue/otherNutsNec -->


    <owl:NamedIndividual rdf:about="http://lpis.ec.europa.eu/registry/applicationschema/cap-iacs-base/code#CropItemCodeValue/otherNutsNec">
        <rdf:type rdf:resource="http://lpis.ec.europa.eu/registry/applicationschema/cap-iacs-base#CropItemCodeValue"/>
        <rdfs:label xml:lang="en">Other nuts n.e.c.</rdfs:label>
        <skos:definition xml:lang="en">-- Definition --
|||Other nuts n.e.c.
-- Description --
Cereals and main crops - C
NOTE. Initial value:C2240</skos:definition>
        <skos:inScheme rdf:resource="http://lpis.ec.europa.eu/registry/applicationschema/cap-iacs-base/code#CropItemCodeValue"/>
    </owl:NamedIndividual>
    


    <!-- http://lpis.ec.europa.eu/registry/applicationschema/cap-iacs-base/code#CropItemCodeValue/otherOilSeedCropsNec -->


    <owl:NamedIndividual rdf:about="http://lpis.ec.europa.eu/registry/applicationschema/cap-iacs-base/code#CropItemCodeValue/otherOilSeedCropsNec">
        <rdf:type rdf:resource="http://lpis.ec.europa.eu/registry/applicationschema/cap-iacs-base#CropItemCodeValue"/>
        <rdfs:label xml:lang="en">Other oil seed crops n.e.c. </rdfs:label>
        <skos:definition xml:lang="en">-- Definition --
|||Other oil seed crops n.e.c. 
-- Description --
Cereals and main crops - C
NOTE. Initial value:C1480</skos:definition>
        <skos:inScheme rdf:resource="http://lpis.ec.europa.eu/registry/applicationschema/cap-iacs-base/code#CropItemCodeValue"/>
    </owl:NamedIndividual>
    


    <!-- http://lpis.ec.europa.eu/registry/applicationschema/cap-iacs-base/code#CropItemCodeValue/otherPermanentCrops -->


    <owl:NamedIndividual rdf:about="http://lpis.ec.europa.eu/registry/applicationschema/cap-iacs-base/code#CropItemCodeValue/otherPermanentCrops">
        <rdf:type rdf:resource="http://lpis.ec.europa.eu/registry/applicationschema/cap-iacs-base#CropItemCodeValue"/>
        <rdfs:label xml:lang="en">Other permanent crops</rdfs:label>
        <skos:definition xml:lang="en">-- Definition --
|||Other permanent crops.
-- Description --
Land use of Agriculture Area in Use -L
NOTE. Initial value:L2980</skos:definition>
        <skos:inScheme rdf:resource="http://lpis.ec.europa.eu/registry/applicationschema/cap-iacs-base/code#CropItemCodeValue"/>
    </owl:NamedIndividual>
    


    <!-- http://lpis.ec.europa.eu/registry/applicationschema/cap-iacs-base/code#CropItemCodeValue/otherPotatoes -->


    <owl:NamedIndividual rdf:about="http://lpis.ec.europa.eu/registry/applicationschema/cap-iacs-base/code#CropItemCodeValue/otherPotatoes">
        <rdf:type rdf:resource="http://lpis.ec.europa.eu/registry/applicationschema/cap-iacs-base#CropItemCodeValue"/>
        <rdfs:label xml:lang="en">Other potatoes</rdfs:label>
        <skos:definition xml:lang="en">-- Definition --
|||Other potatoes.
-- Description --
Cereals and main crops - C
NOTE. Initial value:C1363</skos:definition>
        <skos:inScheme rdf:resource="http://lpis.ec.europa.eu/registry/applicationschema/cap-iacs-base/code#CropItemCodeValue"/>
    </owl:NamedIndividual>
    


    <!-- http://lpis.ec.europa.eu/registry/applicationschema/cap-iacs-base/code#CropItemCodeValue/otherPulsesNec -->


    <owl:NamedIndividual rdf:about="http://lpis.ec.europa.eu/registry/applicationschema/cap-iacs-base/code#CropItemCodeValue/otherPulsesNec">
        <rdf:type rdf:resource="http://lpis.ec.europa.eu/registry/applicationschema/cap-iacs-base#CropItemCodeValue"/>
        <rdfs:label xml:lang="en">Other pulses n.e.c.</rdfs:label>
        <skos:definition xml:lang="en">-- Definition --
|||Other pulses n.e.c.
-- Description --
Cereals and main crops - C
NOTE. Initial value:C1905</skos:definition>
        <skos:inScheme rdf:resource="http://lpis.ec.europa.eu/registry/applicationschema/cap-iacs-base/code#CropItemCodeValue"/>
    </owl:NamedIndividual>
    


    <!-- http://lpis.ec.europa.eu/registry/applicationschema/cap-iacs-base/code#CropItemCodeValue/otherRootAndTuberVegetablesNec -->


    <owl:NamedIndividual rdf:about="http://lpis.ec.europa.eu/registry/applicationschema/cap-iacs-base/code#CropItemCodeValue/otherRootAndTuberVegetablesNec">
        <rdf:type rdf:resource="http://lpis.ec.europa.eu/registry/applicationschema/cap-iacs-base#CropItemCodeValue"/>
        <rdfs:label xml:lang="en">Other root and tuber vegetables n.e.c.</rdfs:label>
        <skos:definition xml:lang="en">-- Definition --
|||Other root and tuber vegetables n.e.c.
-- Description --
Cereals and main crops - C
NOTE. Initial value:C1884</skos:definition>
        <skos:inScheme rdf:resource="http://lpis.ec.europa.eu/registry/applicationschema/cap-iacs-base/code#CropItemCodeValue"/>
    </owl:NamedIndividual>
    


    <!-- http://lpis.ec.europa.eu/registry/applicationschema/cap-iacs-base/code#CropItemCodeValue/otherRootCropsNec -->


    <owl:NamedIndividual rdf:about="http://lpis.ec.europa.eu/registry/applicationschema/cap-iacs-base/code#CropItemCodeValue/otherRootCropsNec">
        <rdf:type rdf:resource="http://lpis.ec.europa.eu/registry/applicationschema/cap-iacs-base#CropItemCodeValue"/>
        <rdfs:label xml:lang="en">Other root crops n.e.c. </rdfs:label>
        <skos:definition xml:lang="en">-- Definition --
||Other root crops n.e.c. 
-- Description --
Cereals and main crops - C
NOTE. Initial value:C1380</skos:definition>
        <skos:inScheme rdf:resource="http://lpis.ec.europa.eu/registry/applicationschema/cap-iacs-base/code#CropItemCodeValue"/>
    </owl:NamedIndividual>
    


    <!-- http://lpis.ec.europa.eu/registry/applicationschema/cap-iacs-base/code#CropItemCodeValue/otherRootCropsNecL1380 -->


    <owl:NamedIndividual rdf:about="http://lpis.ec.europa.eu/registry/applicationschema/cap-iacs-base/code#CropItemCodeValue/otherRootCropsNecL1380">
        <rdf:type rdf:resource="http://lpis.ec.europa.eu/registry/applicationschema/cap-iacs-base#CropItemCodeValue"/>
        <rdfs:label xml:lang="en">Other root crops n.e.c. L1380</rdfs:label>
        <skos:definition xml:lang="en">-- Definition --
||||Other root crops n.e.c. L1380.
-- Description --
Land use of Agriculture Area in Use -L
NOTE. Initial value:L1380</skos:definition>
        <skos:inScheme rdf:resource="http://lpis.ec.europa.eu/registry/applicationschema/cap-iacs-base/code#CropItemCodeValue"/>
    </owl:NamedIndividual>
    


    <!-- http://lpis.ec.europa.eu/registry/applicationschema/cap-iacs-base/code#CropItemCodeValue/otherStoneFruitsNec -->


    <owl:NamedIndividual rdf:about="http://lpis.ec.europa.eu/registry/applicationschema/cap-iacs-base/code#CropItemCodeValue/otherStoneFruitsNec">
        <rdf:type rdf:resource="http://lpis.ec.europa.eu/registry/applicationschema/cap-iacs-base#CropItemCodeValue"/>
        <rdfs:label xml:lang="en">Other stone fruits n.e.c.</rdfs:label>
        <skos:definition xml:lang="en">-- Definition --
|||Other stone fruits n.e.c.
-- Description --
Cereals and main crops - C
NOTE. Initial value:C2229</skos:definition>
        <skos:inScheme rdf:resource="http://lpis.ec.europa.eu/registry/applicationschema/cap-iacs-base/code#CropItemCodeValue"/>
    </owl:NamedIndividual>
    


    <!-- http://lpis.ec.europa.eu/registry/applicationschema/cap-iacs-base/code#CropItemCodeValue/otherUtilisedAgriculturalArea -->


    <owl:NamedIndividual rdf:about="http://lpis.ec.europa.eu/registry/applicationschema/cap-iacs-base/code#CropItemCodeValue/otherUtilisedAgriculturalArea">
        <rdf:type rdf:resource="http://lpis.ec.europa.eu/registry/applicationschema/cap-iacs-base#CropItemCodeValue"/>
        <rdfs:label xml:lang="en">Other utilised agricultural area</rdfs:label>
        <skos:definition xml:lang="en">-- Definition --
||Other utilised agricultural area.
-- Description --
Land use of Agriculture Area in Use -L
NOTE. Initial value:L2990</skos:definition>
        <skos:inScheme rdf:resource="http://lpis.ec.europa.eu/registry/applicationschema/cap-iacs-base/code#CropItemCodeValue"/>
    </owl:NamedIndividual>
    


    <!-- http://lpis.ec.europa.eu/registry/applicationschema/cap-iacs-base/code#CropItemCodeValue/otherVegetablesCultivatedForFruitNec -->


    <owl:NamedIndividual rdf:about="http://lpis.ec.europa.eu/registry/applicationschema/cap-iacs-base/code#CropItemCodeValue/otherVegetablesCultivatedForFruitNec">
        <rdf:type rdf:resource="http://lpis.ec.europa.eu/registry/applicationschema/cap-iacs-base#CropItemCodeValue"/>
        <rdfs:label xml:lang="en">Other vegetables cultivated for fruit n.e.c.</rdfs:label>
        <skos:definition xml:lang="en">-- Definition --
|||Other vegetables cultivated for fruit n.e.c.
-- Description --
Cereals and main crops - C
NOTE. Initial value:C1799</skos:definition>
        <skos:inScheme rdf:resource="http://lpis.ec.europa.eu/registry/applicationschema/cap-iacs-base/code#CropItemCodeValue"/>
    </owl:NamedIndividual>
    


    <!-- http://lpis.ec.europa.eu/registry/applicationschema/cap-iacs-base/code#CropItemCodeValue/peaches -->


    <owl:NamedIndividual rdf:about="http://lpis.ec.europa.eu/registry/applicationschema/cap-iacs-base/code#CropItemCodeValue/peaches">
        <rdf:type rdf:resource="http://lpis.ec.europa.eu/registry/applicationschema/cap-iacs-base#CropItemCodeValue"/>
        <rdfs:label xml:lang="en">Peaches</rdfs:label>
        <skos:definition xml:lang="en">-- Definition --
|||Peaches.
-- Description --
Cereals and main crops - C
NOTE. Initial value:C2180</skos:definition>
        <skos:inScheme rdf:resource="http://lpis.ec.europa.eu/registry/applicationschema/cap-iacs-base/code#CropItemCodeValue"/>
    </owl:NamedIndividual>
    


    <!-- http://lpis.ec.europa.eu/registry/applicationschema/cap-iacs-base/code#CropItemCodeValue/pears -->


    <owl:NamedIndividual rdf:about="http://lpis.ec.europa.eu/registry/applicationschema/cap-iacs-base/code#CropItemCodeValue/pears">
        <rdf:type rdf:resource="http://lpis.ec.europa.eu/registry/applicationschema/cap-iacs-base#CropItemCodeValue"/>
        <rdfs:label xml:lang="en">Pears</rdfs:label>
        <skos:definition xml:lang="en">-- Definition --
||Pears.
-- Description --
Cereals and main crops - C
NOTE. Initial value:C2095</skos:definition>
        <skos:inScheme rdf:resource="http://lpis.ec.europa.eu/registry/applicationschema/cap-iacs-base/code#CropItemCodeValue"/>
    </owl:NamedIndividual>
    


    <!-- http://lpis.ec.europa.eu/registry/applicationschema/cap-iacs-base/code#CropItemCodeValue/pearsForFreshConsumption -->


    <owl:NamedIndividual rdf:about="http://lpis.ec.europa.eu/registry/applicationschema/cap-iacs-base/code#CropItemCodeValue/pearsForFreshConsumption">
        <rdf:type rdf:resource="http://lpis.ec.europa.eu/registry/applicationschema/cap-iacs-base#CropItemCodeValue"/>
        <rdfs:label xml:lang="en">Pears for fresh consumption</rdfs:label>
        <skos:definition xml:lang="en">-- Definition --
|||Pears for fresh consumption.
-- Description --
Cereals and main crops - C
NOTE. Initial value:C2130</skos:definition>
        <skos:inScheme rdf:resource="http://lpis.ec.europa.eu/registry/applicationschema/cap-iacs-base/code#CropItemCodeValue"/>
    </owl:NamedIndividual>
    


    <!-- http://lpis.ec.europa.eu/registry/applicationschema/cap-iacs-base/code#CropItemCodeValue/peas -->


    <owl:NamedIndividual rdf:about="http://lpis.ec.europa.eu/registry/applicationschema/cap-iacs-base/code#CropItemCodeValue/peas">
        <rdf:type rdf:resource="http://lpis.ec.europa.eu/registry/applicationschema/cap-iacs-base#CropItemCodeValue"/>
        <rdfs:label xml:lang="en">Peas</rdfs:label>
        <skos:definition xml:lang="en">-- Definition --
|||Peas.
-- Description --
Cereals and main crops - C
NOTE. Initial value:C1890</skos:definition>
        <skos:inScheme rdf:resource="http://lpis.ec.europa.eu/registry/applicationschema/cap-iacs-base/code#CropItemCodeValue"/>
    </owl:NamedIndividual>
    


    <!-- http://lpis.ec.europa.eu/registry/applicationschema/cap-iacs-base/code#CropItemCodeValue/permanentCrops -->


    <owl:NamedIndividual rdf:about="http://lpis.ec.europa.eu/registry/applicationschema/cap-iacs-base/code#CropItemCodeValue/permanentCrops">
        <rdf:type rdf:resource="http://lpis.ec.europa.eu/registry/applicationschema/cap-iacs-base#CropItemCodeValue"/>
        <rdfs:label xml:lang="en">Permanent crops</rdfs:label>
        <skos:definition xml:lang="en">-- Definition --
|Permanent crops.
-- Description --
Cereals and main crops - C
NOTE. Initial value:C2007</skos:definition>
        <skos:inScheme rdf:resource="http://lpis.ec.europa.eu/registry/applicationschema/cap-iacs-base/code#CropItemCodeValue"/>
    </owl:NamedIndividual>
    


    <!-- http://lpis.ec.europa.eu/registry/applicationschema/cap-iacs-base/code#CropItemCodeValue/permanentCropsL0003 -->


    <owl:NamedIndividual rdf:about="http://lpis.ec.europa.eu/registry/applicationschema/cap-iacs-base/code#CropItemCodeValue/permanentCropsL0003">
        <rdf:type rdf:resource="http://lpis.ec.europa.eu/registry/applicationschema/cap-iacs-base#CropItemCodeValue"/>
        <rdfs:label xml:lang="en">Permanent crops L0003</rdfs:label>
        <skos:definition xml:lang="en">-- Definition --
||Permanent crops L0003.
-- Description --
Land use of Agriculture Area in Use -L
NOTE. Initial value:L0003</skos:definition>
        <skos:inScheme rdf:resource="http://lpis.ec.europa.eu/registry/applicationschema/cap-iacs-base/code#CropItemCodeValue"/>
    </owl:NamedIndividual>
    


    <!-- http://lpis.ec.europa.eu/registry/applicationschema/cap-iacs-base/code#CropItemCodeValue/permanentCropsUnderGlassOrHighAccessibleCover -->


    <owl:NamedIndividual rdf:about="http://lpis.ec.europa.eu/registry/applicationschema/cap-iacs-base/code#CropItemCodeValue/permanentCropsUnderGlassOrHighAccessibleCover">
        <rdf:type rdf:resource="http://lpis.ec.europa.eu/registry/applicationschema/cap-iacs-base#CropItemCodeValue"/>
        <rdfs:label xml:lang="en">Permanent crops under glass or high accessible cover</rdfs:label>
        <skos:definition xml:lang="en">-- Definition --
Permanent crops under glass or high accessible cover.
-- Description --
Land use of Agriculture Area in Use -L. Special aggregates
NOTE. Initial value:L1114</skos:definition>
        <skos:inScheme rdf:resource="http://lpis.ec.europa.eu/registry/applicationschema/cap-iacs-base/code#CropItemCodeValue"/>
    </owl:NamedIndividual>
    


    <!-- http://lpis.ec.europa.eu/registry/applicationschema/cap-iacs-base/code#CropItemCodeValue/permanentGrassland -->


    <owl:NamedIndividual rdf:about="http://lpis.ec.europa.eu/registry/applicationschema/cap-iacs-base/code#CropItemCodeValue/permanentGrassland">
        <rdf:type rdf:resource="http://lpis.ec.europa.eu/registry/applicationschema/cap-iacs-base#CropItemCodeValue"/>
        <rdfs:label xml:lang="en">Permanent grassland</rdfs:label>
        <skos:definition xml:lang="en">-- Definition --
||Permanent grassland.
-- Description --
Land use of Agriculture Area in Use -L
NOTE. Initial value:L0002</skos:definition>
        <skos:inScheme rdf:resource="http://lpis.ec.europa.eu/registry/applicationschema/cap-iacs-base/code#CropItemCodeValue"/>
    </owl:NamedIndividual>
    


    <!-- http://lpis.ec.europa.eu/registry/applicationschema/cap-iacs-base/code#CropItemCodeValue/permanentGrasslandPasturesAndMeadows -->


    <owl:NamedIndividual rdf:about="http://lpis.ec.europa.eu/registry/applicationschema/cap-iacs-base/code#CropItemCodeValue/permanentGrasslandPasturesAndMeadows">
        <rdf:type rdf:resource="http://lpis.ec.europa.eu/registry/applicationschema/cap-iacs-base#CropItemCodeValue"/>
        <rdfs:label xml:lang="en">Permanent grassland (pastures and meadows)</rdfs:label>
        <skos:definition xml:lang="en">-- Definition --
|Permanent grassland (pastures and meadows).
-- Description --
Cereals and main crops - C
NOTE. Initial value:C0002</skos:definition>
        <skos:inScheme rdf:resource="http://lpis.ec.europa.eu/registry/applicationschema/cap-iacs-base/code#CropItemCodeValue"/>
    </owl:NamedIndividual>
    


    <!-- http://lpis.ec.europa.eu/registry/applicationschema/cap-iacs-base/code#CropItemCodeValue/plantsHarvestedGreenC2610 -->


    <owl:NamedIndividual rdf:about="http://lpis.ec.europa.eu/registry/applicationschema/cap-iacs-base/code#CropItemCodeValue/plantsHarvestedGreenC2610">
        <rdf:type rdf:resource="http://lpis.ec.europa.eu/registry/applicationschema/cap-iacs-base#CropItemCodeValue"/>
        <rdfs:label xml:lang="en">Plants harvested green C2610 </rdfs:label>
        <skos:definition xml:lang="en">-- Definition --
|Plants harvested green C2610.
-- Description --
Cereals and main crops - C
NOTE. Initial value:C2610</skos:definition>
        <skos:inScheme rdf:resource="http://lpis.ec.europa.eu/registry/applicationschema/cap-iacs-base/code#CropItemCodeValue"/>
    </owl:NamedIndividual>
    


    <!-- http://lpis.ec.europa.eu/registry/applicationschema/cap-iacs-base/code#CropItemCodeValue/plantsHarvestedGreenGrownOnArableLand -->


    <owl:NamedIndividual rdf:about="http://lpis.ec.europa.eu/registry/applicationschema/cap-iacs-base/code#CropItemCodeValue/plantsHarvestedGreenGrownOnArableLand">
        <rdf:type rdf:resource="http://lpis.ec.europa.eu/registry/applicationschema/cap-iacs-base#CropItemCodeValue"/>
        <rdfs:label xml:lang="en">Plants harvested green (grown on arable land)</rdfs:label>
        <skos:definition xml:lang="en">-- Definition --
|||Plants harvested green (grown on arable land).
-- Description --
Land use of Agriculture Area in Use -L
NOTE. Initial value:L2610</skos:definition>
        <skos:inScheme rdf:resource="http://lpis.ec.europa.eu/registry/applicationschema/cap-iacs-base/code#CropItemCodeValue"/>
    </owl:NamedIndividual>
    


    <!-- http://lpis.ec.europa.eu/registry/applicationschema/cap-iacs-base/code#CropItemCodeValue/plums -->


    <owl:NamedIndividual rdf:about="http://lpis.ec.europa.eu/registry/applicationschema/cap-iacs-base/code#CropItemCodeValue/plums">
        <rdf:type rdf:resource="http://lpis.ec.europa.eu/registry/applicationschema/cap-iacs-base#CropItemCodeValue"/>
        <rdfs:label xml:lang="en">Plums</rdfs:label>
        <skos:definition xml:lang="en">-- Definition --
|||Plums.
-- Description --
Cereals and main crops - C
NOTE. Initial value:C2210</skos:definition>
        <skos:inScheme rdf:resource="http://lpis.ec.europa.eu/registry/applicationschema/cap-iacs-base/code#CropItemCodeValue"/>
    </owl:NamedIndividual>
    


    <!-- http://lpis.ec.europa.eu/registry/applicationschema/cap-iacs-base/code#CropItemCodeValue/pomelosAndGrapefruitC2380 -->


    <owl:NamedIndividual rdf:about="http://lpis.ec.europa.eu/registry/applicationschema/cap-iacs-base/code#CropItemCodeValue/pomelosAndGrapefruitC2380">
        <rdf:type rdf:resource="http://lpis.ec.europa.eu/registry/applicationschema/cap-iacs-base#CropItemCodeValue"/>
        <rdfs:label xml:lang="en">Pomelos and grapefruit C2380</rdfs:label>
        <skos:definition xml:lang="en">-- Definition --
|||Pomelos and grapefruit C2380.
-- Description --
Cereals and main crops - C
NOTE. Initial value:C2380</skos:definition>
        <skos:inScheme rdf:resource="http://lpis.ec.europa.eu/registry/applicationschema/cap-iacs-base/code#CropItemCodeValue"/>
    </owl:NamedIndividual>
    


    <!-- http://lpis.ec.europa.eu/registry/applicationschema/cap-iacs-base/code#CropItemCodeValue/potatoesIncludingEarlyPotatoesAndSeedPotatoes -->


    <owl:NamedIndividual rdf:about="http://lpis.ec.europa.eu/registry/applicationschema/cap-iacs-base/code#CropItemCodeValue/potatoesIncludingEarlyPotatoesAndSeedPotatoes">
        <rdf:type rdf:resource="http://lpis.ec.europa.eu/registry/applicationschema/cap-iacs-base#CropItemCodeValue"/>
        <rdfs:label xml:lang="en">Potatoes (including early potatoes and seed potatoes)</rdfs:label>
        <skos:definition xml:lang="en">-- Definition --
||Potatoes (including early potatoes and seed potatoes).
-- Description --
Cereals and main crops - C
NOTE. Initial value:C1360</skos:definition>
        <skos:inScheme rdf:resource="http://lpis.ec.europa.eu/registry/applicationschema/cap-iacs-base/code#CropItemCodeValue"/>
    </owl:NamedIndividual>
    


    <!-- http://lpis.ec.europa.eu/registry/applicationschema/cap-iacs-base/code#CropItemCodeValue/potatoesIncludingEarlyPotatoesAndSeedPotatoesL1360 -->


    <owl:NamedIndividual rdf:about="http://lpis.ec.europa.eu/registry/applicationschema/cap-iacs-base/code#CropItemCodeValue/potatoesIncludingEarlyPotatoesAndSeedPotatoesL1360">
        <rdf:type rdf:resource="http://lpis.ec.europa.eu/registry/applicationschema/cap-iacs-base#CropItemCodeValue"/>
        <rdfs:label xml:lang="en">Potatoes (including early potatoes and seed potatoes) L1360</rdfs:label>
        <skos:definition xml:lang="en">-- Definition --
||||Potatoes (including early potatoes and seed potatoes) L1360.
-- Description --
Land use of Agriculture Area in Use -L
NOTE. Initial value:L1360</skos:definition>
        <skos:inScheme rdf:resource="http://lpis.ec.europa.eu/registry/applicationschema/cap-iacs-base/code#CropItemCodeValue"/>
    </owl:NamedIndividual>
    


    <!-- http://lpis.ec.europa.eu/registry/applicationschema/cap-iacs-base/code#CropItemCodeValue/pulses -->


    <owl:NamedIndividual rdf:about="http://lpis.ec.europa.eu/registry/applicationschema/cap-iacs-base/code#CropItemCodeValue/pulses">
        <rdf:type rdf:resource="http://lpis.ec.europa.eu/registry/applicationschema/cap-iacs-base#CropItemCodeValue"/>
        <rdfs:label xml:lang="en">Pulses</rdfs:label>
        <skos:definition xml:lang="en">-- Definition --
||Pulses.
-- Description --
Cereals and main crops - C
NOTE. Initial value:C1885</skos:definition>
        <skos:inScheme rdf:resource="http://lpis.ec.europa.eu/registry/applicationschema/cap-iacs-base/code#CropItemCodeValue"/>
    </owl:NamedIndividual>
    


    <!-- http://lpis.ec.europa.eu/registry/applicationschema/cap-iacs-base/code#CropItemCodeValue/quinces -->


    <owl:NamedIndividual rdf:about="http://lpis.ec.europa.eu/registry/applicationschema/cap-iacs-base/code#CropItemCodeValue/quinces">
        <rdf:type rdf:resource="http://lpis.ec.europa.eu/registry/applicationschema/cap-iacs-base#CropItemCodeValue"/>
        <rdfs:label xml:lang="en">Quinces</rdfs:label>
        <skos:definition xml:lang="en">-- Definition --
|||Quinces.
-- Description --
Cereals and main crops - C
NOTE. Initial value:C2252</skos:definition>
        <skos:inScheme rdf:resource="http://lpis.ec.europa.eu/registry/applicationschema/cap-iacs-base/code#CropItemCodeValue"/>
    </owl:NamedIndividual>
    


    <!-- http://lpis.ec.europa.eu/registry/applicationschema/cap-iacs-base/code#CropItemCodeValue/radishes -->


    <owl:NamedIndividual rdf:about="http://lpis.ec.europa.eu/registry/applicationschema/cap-iacs-base/code#CropItemCodeValue/radishes">
        <rdf:type rdf:resource="http://lpis.ec.europa.eu/registry/applicationschema/cap-iacs-base#CropItemCodeValue"/>
        <rdfs:label xml:lang="en">Radishes</rdfs:label>
        <skos:definition xml:lang="en">-- Definition --
|||Radishes.
-- Description --
Cereals and main crops - C
NOTE. Initial value:C1877</skos:definition>
        <skos:inScheme rdf:resource="http://lpis.ec.europa.eu/registry/applicationschema/cap-iacs-base/code#CropItemCodeValue"/>
    </owl:NamedIndividual>
    


    <!-- http://lpis.ec.europa.eu/registry/applicationschema/cap-iacs-base/code#CropItemCodeValue/rape -->


    <owl:NamedIndividual rdf:about="http://lpis.ec.europa.eu/registry/applicationschema/cap-iacs-base/code#CropItemCodeValue/rape">
        <rdf:type rdf:resource="http://lpis.ec.europa.eu/registry/applicationschema/cap-iacs-base#CropItemCodeValue"/>
        <rdfs:label xml:lang="en">Rape</rdfs:label>
        <skos:definition xml:lang="en">-- Definition --
|||||Rape.
-- Description --
Cereals and main crops - C
NOTE. Initial value:C1430</skos:definition>
        <skos:inScheme rdf:resource="http://lpis.ec.europa.eu/registry/applicationschema/cap-iacs-base/code#CropItemCodeValue"/>
    </owl:NamedIndividual>
    


    <!-- http://lpis.ec.europa.eu/registry/applicationschema/cap-iacs-base/code#CropItemCodeValue/rapeAndTurnipRape -->


    <owl:NamedIndividual rdf:about="http://lpis.ec.europa.eu/registry/applicationschema/cap-iacs-base/code#CropItemCodeValue/rapeAndTurnipRape">
        <rdf:type rdf:resource="http://lpis.ec.europa.eu/registry/applicationschema/cap-iacs-base#CropItemCodeValue"/>
        <rdfs:label xml:lang="en">Rape and turnip rape</rdfs:label>
        <skos:definition xml:lang="en">-- Definition --
||||Rape and turnip rape.
-- Description --
Cereals and main crops - C
NOTE. Initial value:C1420</skos:definition>
        <skos:inScheme rdf:resource="http://lpis.ec.europa.eu/registry/applicationschema/cap-iacs-base/code#CropItemCodeValue"/>
    </owl:NamedIndividual>
    


    <!-- http://lpis.ec.europa.eu/registry/applicationschema/cap-iacs-base/code#CropItemCodeValue/raspberries -->


    <owl:NamedIndividual rdf:about="http://lpis.ec.europa.eu/registry/applicationschema/cap-iacs-base/code#CropItemCodeValue/raspberries">
        <rdf:type rdf:resource="http://lpis.ec.europa.eu/registry/applicationschema/cap-iacs-base#CropItemCodeValue"/>
        <rdfs:label xml:lang="en">Raspberries</rdfs:label>
        <skos:definition xml:lang="en">-- Definition --
|||Raspberries.
-- Description --
Cereals and main crops - C
NOTE. Initial value:C2278</skos:definition>
        <skos:inScheme rdf:resource="http://lpis.ec.europa.eu/registry/applicationschema/cap-iacs-base/code#CropItemCodeValue"/>
    </owl:NamedIndividual>
    


    <!-- http://lpis.ec.europa.eu/registry/applicationschema/cap-iacs-base/code#CropItemCodeValue/redCurrants -->


    <owl:NamedIndividual rdf:about="http://lpis.ec.europa.eu/registry/applicationschema/cap-iacs-base/code#CropItemCodeValue/redCurrants">
        <rdf:type rdf:resource="http://lpis.ec.europa.eu/registry/applicationschema/cap-iacs-base#CropItemCodeValue"/>
        <rdfs:label xml:lang="en">Red currants</rdfs:label>
        <skos:definition xml:lang="en">-- Definition --
||||Red currants.
-- Description --
Cereals and main crops - C
NOTE. Initial value:C2275</skos:definition>
        <skos:inScheme rdf:resource="http://lpis.ec.europa.eu/registry/applicationschema/cap-iacs-base/code#CropItemCodeValue"/>
    </owl:NamedIndividual>
    


    <!-- http://lpis.ec.europa.eu/registry/applicationschema/cap-iacs-base/code#CropItemCodeValue/redPepperCapsicum -->


    <owl:NamedIndividual rdf:about="http://lpis.ec.europa.eu/registry/applicationschema/cap-iacs-base/code#CropItemCodeValue/redPepperCapsicum">
        <rdf:type rdf:resource="http://lpis.ec.europa.eu/registry/applicationschema/cap-iacs-base#CropItemCodeValue"/>
        <rdfs:label xml:lang="en">Red pepper, capsicum</rdfs:label>
        <skos:definition xml:lang="en">-- Definition --
|||Red pepper, capsicum.
-- Description --
Cereals and main crops - C
NOTE. Initial value:C1790</skos:definition>
        <skos:inScheme rdf:resource="http://lpis.ec.europa.eu/registry/applicationschema/cap-iacs-base/code#CropItemCodeValue"/>
    </owl:NamedIndividual>
    


    <!-- http://lpis.ec.europa.eu/registry/applicationschema/cap-iacs-base/code#CropItemCodeValue/redPepperCapsicumUnderGlassOrHighAccessibleCoverC1791 -->


    <owl:NamedIndividual rdf:about="http://lpis.ec.europa.eu/registry/applicationschema/cap-iacs-base/code#CropItemCodeValue/redPepperCapsicumUnderGlassOrHighAccessibleCoverC1791">
        <rdf:type rdf:resource="http://lpis.ec.europa.eu/registry/applicationschema/cap-iacs-base#CropItemCodeValue"/>
        <rdfs:label xml:lang="en">Red pepper, capsicum under glass or high accessible cover C1791</rdfs:label>
        <skos:definition xml:lang="en">-- Definition --
||||Red pepper, capsicum under glass or high accessible cover C1791.
-- Description --
Cereals and main crops - C
NOTE. Initial value:C1791</skos:definition>
        <skos:inScheme rdf:resource="http://lpis.ec.europa.eu/registry/applicationschema/cap-iacs-base/code#CropItemCodeValue"/>
    </owl:NamedIndividual>
    


    <!-- http://lpis.ec.europa.eu/registry/applicationschema/cap-iacs-base/code#CropItemCodeValue/rice -->


    <owl:NamedIndividual rdf:about="http://lpis.ec.europa.eu/registry/applicationschema/cap-iacs-base/code#CropItemCodeValue/rice">
        <rdf:type rdf:resource="http://lpis.ec.europa.eu/registry/applicationschema/cap-iacs-base#CropItemCodeValue"/>
        <rdfs:label xml:lang="en">Rice </rdfs:label>
        <skos:definition xml:lang="en">-- Definition --
||Rice.
-- Description --
Cereals and main crops - C
NOTE. Initial value:C1250</skos:definition>
        <skos:inScheme rdf:resource="http://lpis.ec.europa.eu/registry/applicationschema/cap-iacs-base/code#CropItemCodeValue"/>
    </owl:NamedIndividual>
    


    <!-- http://lpis.ec.europa.eu/registry/applicationschema/cap-iacs-base/code#CropItemCodeValue/riceIndica -->


    <owl:NamedIndividual rdf:about="http://lpis.ec.europa.eu/registry/applicationschema/cap-iacs-base/code#CropItemCodeValue/riceIndica">
        <rdf:type rdf:resource="http://lpis.ec.europa.eu/registry/applicationschema/cap-iacs-base#CropItemCodeValue"/>
        <rdfs:label xml:lang="en">Rice Indica </rdfs:label>
        <skos:definition xml:lang="en">-- Definition --
|||Rice Indica.
-- Description --
Cereals and main crops - C
NOTE. Initial value:C1251</skos:definition>
        <skos:inScheme rdf:resource="http://lpis.ec.europa.eu/registry/applicationschema/cap-iacs-base/code#CropItemCodeValue"/>
    </owl:NamedIndividual>
    


    <!-- http://lpis.ec.europa.eu/registry/applicationschema/cap-iacs-base/code#CropItemCodeValue/riceJaponica -->


    <owl:NamedIndividual rdf:about="http://lpis.ec.europa.eu/registry/applicationschema/cap-iacs-base/code#CropItemCodeValue/riceJaponica">
        <rdf:type rdf:resource="http://lpis.ec.europa.eu/registry/applicationschema/cap-iacs-base#CropItemCodeValue"/>
        <rdfs:label xml:lang="en">Rice Japonica</rdfs:label>
        <skos:definition xml:lang="en">-- Definition --
|||Rice Japonica.
-- Description --
Cereals and main crops - C
NOTE. Initial value:C1252</skos:definition>
        <skos:inScheme rdf:resource="http://lpis.ec.europa.eu/registry/applicationschema/cap-iacs-base/code#CropItemCodeValue"/>
    </owl:NamedIndividual>
    


    <!-- http://lpis.ec.europa.eu/registry/applicationschema/cap-iacs-base/code#CropItemCodeValue/riceOp -->


    <owl:NamedIndividual rdf:about="http://lpis.ec.europa.eu/registry/applicationschema/cap-iacs-base/code#CropItemCodeValue/riceOp">
        <rdf:type rdf:resource="http://lpis.ec.europa.eu/registry/applicationschema/cap-iacs-base#CropItemCodeValue"/>
        <rdfs:label xml:lang="en">Rice Op</rdfs:label>
        <skos:definition xml:lang="en">-- Definition --
|||Rice Op.
-- Description --
Land use of Agriculture Area in Use -L
NOTE. Initial value:L1250</skos:definition>
        <skos:inScheme rdf:resource="http://lpis.ec.europa.eu/registry/applicationschema/cap-iacs-base/code#CropItemCodeValue"/>
    </owl:NamedIndividual>
    


    <!-- http://lpis.ec.europa.eu/registry/applicationschema/cap-iacs-base/code#CropItemCodeValue/rootAndTuberVegetables -->


    <owl:NamedIndividual rdf:about="http://lpis.ec.europa.eu/registry/applicationschema/cap-iacs-base/code#CropItemCodeValue/rootAndTuberVegetables">
        <rdf:type rdf:resource="http://lpis.ec.europa.eu/registry/applicationschema/cap-iacs-base#CropItemCodeValue"/>
        <rdfs:label xml:lang="en">Root and tuber vegetables</rdfs:label>
        <skos:definition xml:lang="en">-- Definition --
||Root and tuber vegetables.
-- Description --
Cereals and main crops - C
NOTE. Initial value:C1800</skos:definition>
        <skos:inScheme rdf:resource="http://lpis.ec.europa.eu/registry/applicationschema/cap-iacs-base/code#CropItemCodeValue"/>
    </owl:NamedIndividual>
    


    <!-- http://lpis.ec.europa.eu/registry/applicationschema/cap-iacs-base/code#CropItemCodeValue/rootCrops -->


    <owl:NamedIndividual rdf:about="http://lpis.ec.europa.eu/registry/applicationschema/cap-iacs-base/code#CropItemCodeValue/rootCrops">
        <rdf:type rdf:resource="http://lpis.ec.europa.eu/registry/applicationschema/cap-iacs-base#CropItemCodeValue"/>
        <rdfs:label xml:lang="en">Root crops</rdfs:label>
        <skos:definition xml:lang="en">-- Definition --
|Root crops.
-- Description --
Cereals and main crops - C
NOTE. Initial value:C1350</skos:definition>
        <skos:inScheme rdf:resource="http://lpis.ec.europa.eu/registry/applicationschema/cap-iacs-base/code#CropItemCodeValue"/>
    </owl:NamedIndividual>
    


    <!-- http://lpis.ec.europa.eu/registry/applicationschema/cap-iacs-base/code#CropItemCodeValue/rootCropsL1350 -->


    <owl:NamedIndividual rdf:about="http://lpis.ec.europa.eu/registry/applicationschema/cap-iacs-base/code#CropItemCodeValue/rootCropsL1350">
        <rdf:type rdf:resource="http://lpis.ec.europa.eu/registry/applicationschema/cap-iacs-base#CropItemCodeValue"/>
        <rdfs:label xml:lang="en">Root crops L1350</rdfs:label>
        <skos:definition xml:lang="en">-- Definition --
|||Root crops L1350.
-- Description --
Land use of Agriculture Area in Use -L
NOTE. Initial value:L1350</skos:definition>
        <skos:inScheme rdf:resource="http://lpis.ec.europa.eu/registry/applicationschema/cap-iacs-base/code#CropItemCodeValue"/>
    </owl:NamedIndividual>
    


    <!-- http://lpis.ec.europa.eu/registry/applicationschema/cap-iacs-base/code#CropItemCodeValue/rye -->


    <owl:NamedIndividual rdf:about="http://lpis.ec.europa.eu/registry/applicationschema/cap-iacs-base/code#CropItemCodeValue/rye">
        <rdf:type rdf:resource="http://lpis.ec.europa.eu/registry/applicationschema/cap-iacs-base#CropItemCodeValue"/>
        <rdfs:label xml:lang="en">Rye</rdfs:label>
        <skos:definition xml:lang="en">-- Definition --
||||Rye.
-- Description --
Cereals and main crops - C
NOTE. Initial value:C1150</skos:definition>
        <skos:inScheme rdf:resource="http://lpis.ec.europa.eu/registry/applicationschema/cap-iacs-base/code#CropItemCodeValue"/>
    </owl:NamedIndividual>
    


    <!-- http://lpis.ec.europa.eu/registry/applicationschema/cap-iacs-base/code#CropItemCodeValue/ryeAndMaslin -->


    <owl:NamedIndividual rdf:about="http://lpis.ec.europa.eu/registry/applicationschema/cap-iacs-base/code#CropItemCodeValue/ryeAndMaslin">
        <rdf:type rdf:resource="http://lpis.ec.europa.eu/registry/applicationschema/cap-iacs-base#CropItemCodeValue"/>
        <rdfs:label xml:lang="en">Rye and maslin</rdfs:label>
        <skos:definition xml:lang="en">-- Definition --
|||Rye and maslin.
-- Description --
Cereals and main crops - C
NOTE. Initial value:C1140</skos:definition>
        <skos:inScheme rdf:resource="http://lpis.ec.europa.eu/registry/applicationschema/cap-iacs-base/code#CropItemCodeValue"/>
    </owl:NamedIndividual>
    


    <!-- http://lpis.ec.europa.eu/registry/applicationschema/cap-iacs-base/code#CropItemCodeValue/salsifyAndScorzonera -->


    <owl:NamedIndividual rdf:about="http://lpis.ec.europa.eu/registry/applicationschema/cap-iacs-base/code#CropItemCodeValue/salsifyAndScorzonera">
        <rdf:type rdf:resource="http://lpis.ec.europa.eu/registry/applicationschema/cap-iacs-base#CropItemCodeValue"/>
        <rdfs:label xml:lang="en">Salsify and scorzonera</rdfs:label>
        <skos:definition xml:lang="en">-- Definition --
|||Salsify and scorzonera.
-- Description --
Cereals and main crops - C
NOTE. Initial value:C1870</skos:definition>
        <skos:inScheme rdf:resource="http://lpis.ec.europa.eu/registry/applicationschema/cap-iacs-base/code#CropItemCodeValue"/>
    </owl:NamedIndividual>
    


    <!-- http://lpis.ec.europa.eu/registry/applicationschema/cap-iacs-base/code#CropItemCodeValue/satsumas -->


    <owl:NamedIndividual rdf:about="http://lpis.ec.europa.eu/registry/applicationschema/cap-iacs-base/code#CropItemCodeValue/satsumas">
        <rdf:type rdf:resource="http://lpis.ec.europa.eu/registry/applicationschema/cap-iacs-base#CropItemCodeValue"/>
        <rdfs:label xml:lang="en">Satsumas</rdfs:label>
        <skos:definition xml:lang="en">-- Definition --
||||Satsumas.
-- Description --
Cereals and main crops - C
NOTE. Initial value:C2352</skos:definition>
        <skos:inScheme rdf:resource="http://lpis.ec.europa.eu/registry/applicationschema/cap-iacs-base/code#CropItemCodeValue"/>
    </owl:NamedIndividual>
    


    <!-- http://lpis.ec.europa.eu/registry/applicationschema/cap-iacs-base/code#CropItemCodeValue/seedsAndSeedlings -->


    <owl:NamedIndividual rdf:about="http://lpis.ec.europa.eu/registry/applicationschema/cap-iacs-base/code#CropItemCodeValue/seedsAndSeedlings">
        <rdf:type rdf:resource="http://lpis.ec.europa.eu/registry/applicationschema/cap-iacs-base#CropItemCodeValue"/>
        <rdfs:label xml:lang="en">Seeds and seedlings</rdfs:label>
        <skos:definition xml:lang="en">-- Definition --
|||Seeds and seedlings.
-- Description --
Land use of Agriculture Area in Use -L
NOTE. Initial value:L3310</skos:definition>
        <skos:inScheme rdf:resource="http://lpis.ec.europa.eu/registry/applicationschema/cap-iacs-base/code#CropItemCodeValue"/>
    </owl:NamedIndividual>
    


    <!-- http://lpis.ec.europa.eu/registry/applicationschema/cap-iacs-base/code#CropItemCodeValue/shallots -->


    <owl:NamedIndividual rdf:about="http://lpis.ec.europa.eu/registry/applicationschema/cap-iacs-base/code#CropItemCodeValue/shallots">
        <rdf:type rdf:resource="http://lpis.ec.europa.eu/registry/applicationschema/cap-iacs-base#CropItemCodeValue"/>
        <rdfs:label xml:lang="en">Shallots</rdfs:label>
        <skos:definition xml:lang="en">-- Definition --
|||Shallots.
-- Description --
Cereals and main crops - C
NOTE. Initial value:C1855</skos:definition>
        <skos:inScheme rdf:resource="http://lpis.ec.europa.eu/registry/applicationschema/cap-iacs-base/code#CropItemCodeValue"/>
    </owl:NamedIndividual>
    


    <!-- http://lpis.ec.europa.eu/registry/applicationschema/cap-iacs-base/code#CropItemCodeValue/smallCitrusFruits -->


    <owl:NamedIndividual rdf:about="http://lpis.ec.europa.eu/registry/applicationschema/cap-iacs-base/code#CropItemCodeValue/smallCitrusFruits">
        <rdf:type rdf:resource="http://lpis.ec.europa.eu/registry/applicationschema/cap-iacs-base#CropItemCodeValue"/>
        <rdfs:label xml:lang="en">Small citrus fruits</rdfs:label>
        <skos:definition xml:lang="en">-- Definition --
|||Small citrus fruits.
-- Description --
Cereals and main crops - C
NOTE. Initial value:C2340</skos:definition>
        <skos:inScheme rdf:resource="http://lpis.ec.europa.eu/registry/applicationschema/cap-iacs-base/code#CropItemCodeValue"/>
    </owl:NamedIndividual>
    


    <!-- http://lpis.ec.europa.eu/registry/applicationschema/cap-iacs-base/code#CropItemCodeValue/sorghum -->


    <owl:NamedIndividual rdf:about="http://lpis.ec.europa.eu/registry/applicationschema/cap-iacs-base/code#CropItemCodeValue/sorghum">
        <rdf:type rdf:resource="http://lpis.ec.europa.eu/registry/applicationschema/cap-iacs-base#CropItemCodeValue"/>
        <rdfs:label xml:lang="en">Sorghum </rdfs:label>
        <skos:definition xml:lang="en">-- Definition --
|||Sorghum.
-- Description --
Cereals and main crops - C
NOTE. Initial value:C1211</skos:definition>
        <skos:inScheme rdf:resource="http://lpis.ec.europa.eu/registry/applicationschema/cap-iacs-base/code#CropItemCodeValue"/>
    </owl:NamedIndividual>
    


    <!-- http://lpis.ec.europa.eu/registry/applicationschema/cap-iacs-base/code#CropItemCodeValue/sourCherries -->


    <owl:NamedIndividual rdf:about="http://lpis.ec.europa.eu/registry/applicationschema/cap-iacs-base/code#CropItemCodeValue/sourCherries">
        <rdf:type rdf:resource="http://lpis.ec.europa.eu/registry/applicationschema/cap-iacs-base#CropItemCodeValue"/>
        <rdfs:label xml:lang="en">Sour cherries</rdfs:label>
        <skos:definition xml:lang="en">-- Definition --
||||Sour cherries.
-- Description --
Cereals and main crops - C
NOTE. Initial value:C2201</skos:definition>
        <skos:inScheme rdf:resource="http://lpis.ec.europa.eu/registry/applicationschema/cap-iacs-base/code#CropItemCodeValue"/>
    </owl:NamedIndividual>
    


    <!-- http://lpis.ec.europa.eu/registry/applicationschema/cap-iacs-base/code#CropItemCodeValue/soya -->


    <owl:NamedIndividual rdf:about="http://lpis.ec.europa.eu/registry/applicationschema/cap-iacs-base/code#CropItemCodeValue/soya">
        <rdf:type rdf:resource="http://lpis.ec.europa.eu/registry/applicationschema/cap-iacs-base#CropItemCodeValue"/>
        <rdfs:label xml:lang="en">Soya </rdfs:label>
        <skos:definition xml:lang="en">-- Definition --
||||Soya.
-- Description --
Cereals and main crops - C
NOTE. Initial value:C1470</skos:definition>
        <skos:inScheme rdf:resource="http://lpis.ec.europa.eu/registry/applicationschema/cap-iacs-base/code#CropItemCodeValue"/>
    </owl:NamedIndividual>
    


    <!-- http://lpis.ec.europa.eu/registry/applicationschema/cap-iacs-base/code#CropItemCodeValue/spinach -->


    <owl:NamedIndividual rdf:about="http://lpis.ec.europa.eu/registry/applicationschema/cap-iacs-base/code#CropItemCodeValue/spinach">
        <rdf:type rdf:resource="http://lpis.ec.europa.eu/registry/applicationschema/cap-iacs-base#CropItemCodeValue"/>
        <rdfs:label xml:lang="en">Spinach</rdfs:label>
        <skos:definition xml:lang="en">-- Definition --
|||Spinach.
-- Description --
Cereals and main crops - C
NOTE. Initial value:C1690</skos:definition>
        <skos:inScheme rdf:resource="http://lpis.ec.europa.eu/registry/applicationschema/cap-iacs-base/code#CropItemCodeValue"/>
    </owl:NamedIndividual>
    


    <!-- http://lpis.ec.europa.eu/registry/applicationschema/cap-iacs-base/code#CropItemCodeValue/springBarley -->


    <owl:NamedIndividual rdf:about="http://lpis.ec.europa.eu/registry/applicationschema/cap-iacs-base/code#CropItemCodeValue/springBarley">
        <rdf:type rdf:resource="http://lpis.ec.europa.eu/registry/applicationschema/cap-iacs-base#CropItemCodeValue"/>
        <rdfs:label xml:lang="en">Spring barley</rdfs:label>
        <skos:definition xml:lang="en">-- Definition --
||||Spring barley.
-- Description --
Cereals and main crops - C
NOTE. Initial value:C1164</skos:definition>
        <skos:inScheme rdf:resource="http://lpis.ec.europa.eu/registry/applicationschema/cap-iacs-base/code#CropItemCodeValue"/>
    </owl:NamedIndividual>
    


    <!-- http://lpis.ec.europa.eu/registry/applicationschema/cap-iacs-base/code#CropItemCodeValue/springDurumWheat -->


    <owl:NamedIndividual rdf:about="http://lpis.ec.europa.eu/registry/applicationschema/cap-iacs-base/code#CropItemCodeValue/springDurumWheat">
        <rdf:type rdf:resource="http://lpis.ec.europa.eu/registry/applicationschema/cap-iacs-base#CropItemCodeValue"/>
        <rdfs:label xml:lang="en">Spring durum wheat</rdfs:label>
        <skos:definition xml:lang="en">-- Definition --
|||||Spring durum wheat.
-- Description --
Cereals and main crops - C
NOTE. Initial value:C1134</skos:definition>
        <skos:inScheme rdf:resource="http://lpis.ec.europa.eu/registry/applicationschema/cap-iacs-base/code#CropItemCodeValue"/>
    </owl:NamedIndividual>
    


    <!-- http://lpis.ec.europa.eu/registry/applicationschema/cap-iacs-base/code#CropItemCodeValue/springRape -->


    <owl:NamedIndividual rdf:about="http://lpis.ec.europa.eu/registry/applicationschema/cap-iacs-base/code#CropItemCodeValue/springRape">
        <rdf:type rdf:resource="http://lpis.ec.europa.eu/registry/applicationschema/cap-iacs-base#CropItemCodeValue"/>
        <rdfs:label xml:lang="en">Spring rape</rdfs:label>
        <skos:definition xml:lang="en">-- Definition --
||||||Spring rape.
-- Description --
Cereals and main crops - C
NOTE. Initial value:C1432</skos:definition>
        <skos:inScheme rdf:resource="http://lpis.ec.europa.eu/registry/applicationschema/cap-iacs-base/code#CropItemCodeValue"/>
    </owl:NamedIndividual>
    


    <!-- http://lpis.ec.europa.eu/registry/applicationschema/cap-iacs-base/code#CropItemCodeValue/springRye -->


    <owl:NamedIndividual rdf:about="http://lpis.ec.europa.eu/registry/applicationschema/cap-iacs-base/code#CropItemCodeValue/springRye">
        <rdf:type rdf:resource="http://lpis.ec.europa.eu/registry/applicationschema/cap-iacs-base#CropItemCodeValue"/>
        <rdfs:label xml:lang="en">Spring rye</rdfs:label>
        <skos:definition xml:lang="en">-- Definition --
|||||Spring rye.
-- Description --
Cereals and main crops - C
NOTE. Initial value:C1152</skos:definition>
        <skos:inScheme rdf:resource="http://lpis.ec.europa.eu/registry/applicationschema/cap-iacs-base/code#CropItemCodeValue"/>
    </owl:NamedIndividual>
    


    <!-- http://lpis.ec.europa.eu/registry/applicationschema/cap-iacs-base/code#CropItemCodeValue/stoneFruits -->


    <owl:NamedIndividual rdf:about="http://lpis.ec.europa.eu/registry/applicationschema/cap-iacs-base/code#CropItemCodeValue/stoneFruits">
        <rdf:type rdf:resource="http://lpis.ec.europa.eu/registry/applicationschema/cap-iacs-base#CropItemCodeValue"/>
        <rdfs:label xml:lang="en">Stone fruits</rdfs:label>
        <skos:definition xml:lang="en">-- Definition --
||Stone fruits.
-- Description --
Cereals and main crops - C
NOTE. Initial value:C2170</skos:definition>
        <skos:inScheme rdf:resource="http://lpis.ec.europa.eu/registry/applicationschema/cap-iacs-base/code#CropItemCodeValue"/>
    </owl:NamedIndividual>
    


    <!-- http://lpis.ec.europa.eu/registry/applicationschema/cap-iacs-base/code#CropItemCodeValue/strawberries -->


    <owl:NamedIndividual rdf:about="http://lpis.ec.europa.eu/registry/applicationschema/cap-iacs-base/code#CropItemCodeValue/strawberries">
        <rdf:type rdf:resource="http://lpis.ec.europa.eu/registry/applicationschema/cap-iacs-base#CropItemCodeValue"/>
        <rdfs:label xml:lang="en">Strawberries</rdfs:label>
        <skos:definition xml:lang="en">-- Definition --
||Strawberries.
-- Description --
Cereals and main crops - C
NOTE. Initial value:C2260</skos:definition>
        <skos:inScheme rdf:resource="http://lpis.ec.europa.eu/registry/applicationschema/cap-iacs-base/code#CropItemCodeValue"/>
    </owl:NamedIndividual>
    


    <!-- http://lpis.ec.europa.eu/registry/applicationschema/cap-iacs-base/code#CropItemCodeValue/strawberriesUnderGlassOrHighAccessibleCoverC2261 -->


    <owl:NamedIndividual rdf:about="http://lpis.ec.europa.eu/registry/applicationschema/cap-iacs-base/code#CropItemCodeValue/strawberriesUnderGlassOrHighAccessibleCoverC2261">
        <rdf:type rdf:resource="http://lpis.ec.europa.eu/registry/applicationschema/cap-iacs-base#CropItemCodeValue"/>
        <rdfs:label xml:lang="en">Strawberries under glass or high accessible cover C2261 </rdfs:label>
        <skos:definition xml:lang="en">-- Definition --
|||Strawberries under glass or high accessible cover C2261.
-- Description --
Cereals and main crops - C
NOTE. Initial value:C2261</skos:definition>
        <skos:inScheme rdf:resource="http://lpis.ec.europa.eu/registry/applicationschema/cap-iacs-base/code#CropItemCodeValue"/>
    </owl:NamedIndividual>
    


    <!-- http://lpis.ec.europa.eu/registry/applicationschema/cap-iacs-base/code#CropItemCodeValue/sugarBeetExcludingSeed -->


    <owl:NamedIndividual rdf:about="http://lpis.ec.europa.eu/registry/applicationschema/cap-iacs-base/code#CropItemCodeValue/sugarBeetExcludingSeed">
        <rdf:type rdf:resource="http://lpis.ec.europa.eu/registry/applicationschema/cap-iacs-base#CropItemCodeValue"/>
        <rdfs:label xml:lang="en">Sugar beet (excluding seed)</rdfs:label>
        <skos:definition xml:lang="en">-- Definition --
||Sugar beet (excluding seed).
-- Description --
Cereals and main crops - C
NOTE. Initial value:C1370</skos:definition>
        <skos:inScheme rdf:resource="http://lpis.ec.europa.eu/registry/applicationschema/cap-iacs-base/code#CropItemCodeValue"/>
    </owl:NamedIndividual>
    


    <!-- http://lpis.ec.europa.eu/registry/applicationschema/cap-iacs-base/code#CropItemCodeValue/sugarBeetExcludingSeedL1370 -->


    <owl:NamedIndividual rdf:about="http://lpis.ec.europa.eu/registry/applicationschema/cap-iacs-base/code#CropItemCodeValue/sugarBeetExcludingSeedL1370">
        <rdf:type rdf:resource="http://lpis.ec.europa.eu/registry/applicationschema/cap-iacs-base#CropItemCodeValue"/>
        <rdfs:label xml:lang="en">Sugar beet (excluding seed) L1370</rdfs:label>
        <skos:definition xml:lang="en">-- Definition --
||||Sugar beet (excluding seed) L1370.
-- Description --
Land use of Agriculture Area in Use -L
NOTE. Initial value:L1370</skos:definition>
        <skos:inScheme rdf:resource="http://lpis.ec.europa.eu/registry/applicationschema/cap-iacs-base/code#CropItemCodeValue"/>
    </owl:NamedIndividual>
    


    <!-- http://lpis.ec.europa.eu/registry/applicationschema/cap-iacs-base/code#CropItemCodeValue/sunflowerSeed -->


    <owl:NamedIndividual rdf:about="http://lpis.ec.europa.eu/registry/applicationschema/cap-iacs-base/code#CropItemCodeValue/sunflowerSeed">
        <rdf:type rdf:resource="http://lpis.ec.europa.eu/registry/applicationschema/cap-iacs-base#CropItemCodeValue"/>
        <rdfs:label xml:lang="en">Sunflower seed </rdfs:label>
        <skos:definition xml:lang="en">-- Definition --
||||Sunflower seed.
-- Description --
Cereals and main crops - C
NOTE. Initial value:C1450</skos:definition>
        <skos:inScheme rdf:resource="http://lpis.ec.europa.eu/registry/applicationschema/cap-iacs-base/code#CropItemCodeValue"/>
    </owl:NamedIndividual>
    


    <!-- http://lpis.ec.europa.eu/registry/applicationschema/cap-iacs-base/code#CropItemCodeValue/sweetLupinsC1343 -->


    <owl:NamedIndividual rdf:about="http://lpis.ec.europa.eu/registry/applicationschema/cap-iacs-base/code#CropItemCodeValue/sweetLupinsC1343">
        <rdf:type rdf:resource="http://lpis.ec.europa.eu/registry/applicationschema/cap-iacs-base#CropItemCodeValue"/>
        <rdfs:label xml:lang="en">Sweet lupins C1343</rdfs:label>
        <skos:definition xml:lang="en">-- Definition --
||Sweet lupins C1343.
-- Description --
Cereals and main crops - C
NOTE. Initial value:C1343</skos:definition>
        <skos:inScheme rdf:resource="http://lpis.ec.europa.eu/registry/applicationschema/cap-iacs-base/code#CropItemCodeValue"/>
    </owl:NamedIndividual>
    


    <!-- http://lpis.ec.europa.eu/registry/applicationschema/cap-iacs-base/code#CropItemCodeValue/temporaryGrassesAndGrazing -->


    <owl:NamedIndividual rdf:about="http://lpis.ec.europa.eu/registry/applicationschema/cap-iacs-base/code#CropItemCodeValue/temporaryGrassesAndGrazing">
        <rdf:type rdf:resource="http://lpis.ec.europa.eu/registry/applicationschema/cap-iacs-base#CropItemCodeValue"/>
        <rdfs:label xml:lang="en">Temporary grasses and grazing </rdfs:label>
        <skos:definition xml:lang="en">-- Definition --
||Temporary grasses and grazing.
-- Description --
Cereals and main crops - C
NOTE. Initial value:C2680</skos:definition>
        <skos:inScheme rdf:resource="http://lpis.ec.europa.eu/registry/applicationschema/cap-iacs-base/code#CropItemCodeValue"/>
    </owl:NamedIndividual>
    


    <!-- http://lpis.ec.europa.eu/registry/applicationschema/cap-iacs-base/code#CropItemCodeValue/tobacco -->


    <owl:NamedIndividual rdf:about="http://lpis.ec.europa.eu/registry/applicationschema/cap-iacs-base/code#CropItemCodeValue/tobacco">
        <rdf:type rdf:resource="http://lpis.ec.europa.eu/registry/applicationschema/cap-iacs-base#CropItemCodeValue"/>
        <rdfs:label xml:lang="en">Tobacco</rdfs:label>
        <skos:definition xml:lang="en">-- Definition --
||Tobacco.
-- Description --
Cereals and main crops - C
NOTE. Initial value:C1550</skos:definition>
        <skos:inScheme rdf:resource="http://lpis.ec.europa.eu/registry/applicationschema/cap-iacs-base/code#CropItemCodeValue"/>
    </owl:NamedIndividual>
    


    <!-- http://lpis.ec.europa.eu/registry/applicationschema/cap-iacs-base/code#CropItemCodeValue/tomatoes -->


    <owl:NamedIndividual rdf:about="http://lpis.ec.europa.eu/registry/applicationschema/cap-iacs-base/code#CropItemCodeValue/tomatoes">
        <rdf:type rdf:resource="http://lpis.ec.europa.eu/registry/applicationschema/cap-iacs-base#CropItemCodeValue"/>
        <rdfs:label xml:lang="en">Tomatoes</rdfs:label>
        <skos:definition xml:lang="en">-- Definition --
|||Tomatoes.
-- Description --
Cereals and main crops - C
NOTE. Initial value:C1750</skos:definition>
        <skos:inScheme rdf:resource="http://lpis.ec.europa.eu/registry/applicationschema/cap-iacs-base/code#CropItemCodeValue"/>
    </owl:NamedIndividual>
    


    <!-- http://lpis.ec.europa.eu/registry/applicationschema/cap-iacs-base/code#CropItemCodeValue/tomatoesForFreshConsumption -->


    <owl:NamedIndividual rdf:about="http://lpis.ec.europa.eu/registry/applicationschema/cap-iacs-base/code#CropItemCodeValue/tomatoesForFreshConsumption">
        <rdf:type rdf:resource="http://lpis.ec.europa.eu/registry/applicationschema/cap-iacs-base#CropItemCodeValue"/>
        <rdfs:label xml:lang="en">Tomatoes for fresh consumption</rdfs:label>
        <skos:definition xml:lang="en">-- Definition --
||||Tomatoes for fresh consumption.
-- Description --
Cereals and main crops - C
NOTE. Initial value:C1751</skos:definition>
        <skos:inScheme rdf:resource="http://lpis.ec.europa.eu/registry/applicationschema/cap-iacs-base/code#CropItemCodeValue"/>
    </owl:NamedIndividual>
    


    <!-- http://lpis.ec.europa.eu/registry/applicationschema/cap-iacs-base/code#CropItemCodeValue/tomatoesForFreshConsumptionUnderGlassOrHighAccessibleCover -->


    <owl:NamedIndividual rdf:about="http://lpis.ec.europa.eu/registry/applicationschema/cap-iacs-base/code#CropItemCodeValue/tomatoesForFreshConsumptionUnderGlassOrHighAccessibleCover">
        <rdf:type rdf:resource="http://lpis.ec.europa.eu/registry/applicationschema/cap-iacs-base#CropItemCodeValue"/>
        <rdfs:label xml:lang="en">Tomatoes for fresh consumption under glass or high accessible cover</rdfs:label>
        <skos:definition xml:lang="en">-- Definition --
|||||Tomatoes for fresh consumption under glass or high accessible cover.
-- Description --
Cereals and main crops - C
NOTE. Initial value:C1752</skos:definition>
        <skos:inScheme rdf:resource="http://lpis.ec.europa.eu/registry/applicationschema/cap-iacs-base/code#CropItemCodeValue"/>
    </owl:NamedIndividual>
    


    <!-- http://lpis.ec.europa.eu/registry/applicationschema/cap-iacs-base/code#CropItemCodeValue/triticale -->


    <owl:NamedIndividual rdf:about="http://lpis.ec.europa.eu/registry/applicationschema/cap-iacs-base/code#CropItemCodeValue/triticale">
        <rdf:type rdf:resource="http://lpis.ec.europa.eu/registry/applicationschema/cap-iacs-base#CropItemCodeValue"/>
        <rdfs:label xml:lang="en">Triticale</rdfs:label>
        <skos:definition xml:lang="en">-- Definition --
|||Triticale.
-- Description --
Cereals and main crops - C
NOTE. Initial value:C1212</skos:definition>
        <skos:inScheme rdf:resource="http://lpis.ec.europa.eu/registry/applicationschema/cap-iacs-base/code#CropItemCodeValue"/>
    </owl:NamedIndividual>
    


    <!-- http://lpis.ec.europa.eu/registry/applicationschema/cap-iacs-base/code#CropItemCodeValue/turnipRape -->


    <owl:NamedIndividual rdf:about="http://lpis.ec.europa.eu/registry/applicationschema/cap-iacs-base/code#CropItemCodeValue/turnipRape">
        <rdf:type rdf:resource="http://lpis.ec.europa.eu/registry/applicationschema/cap-iacs-base#CropItemCodeValue"/>
        <rdfs:label xml:lang="en">Turnip rape</rdfs:label>
        <skos:definition xml:lang="en">-- Definition --
|||||Turnip rape.
-- Description --
Cereals and main crops - C
NOTE. Initial value:C1440</skos:definition>
        <skos:inScheme rdf:resource="http://lpis.ec.europa.eu/registry/applicationschema/cap-iacs-base/code#CropItemCodeValue"/>
    </owl:NamedIndividual>
    


    <!-- http://lpis.ec.europa.eu/registry/applicationschema/cap-iacs-base/code#CropItemCodeValue/turnips -->


    <owl:NamedIndividual rdf:about="http://lpis.ec.europa.eu/registry/applicationschema/cap-iacs-base/code#CropItemCodeValue/turnips">
        <rdf:type rdf:resource="http://lpis.ec.europa.eu/registry/applicationschema/cap-iacs-base#CropItemCodeValue"/>
        <rdfs:label xml:lang="en">Turnips</rdfs:label>
        <skos:definition xml:lang="en">-- Definition --
|||Turnips.
-- Description --
Cereals and main crops - C
NOTE. Initial value:C1820</skos:definition>
        <skos:inScheme rdf:resource="http://lpis.ec.europa.eu/registry/applicationschema/cap-iacs-base/code#CropItemCodeValue"/>
    </owl:NamedIndividual>
    


    <!-- http://lpis.ec.europa.eu/registry/applicationschema/cap-iacs-base/code#CropItemCodeValue/utilisedAgriculturalAreaUAA -->


    <owl:NamedIndividual rdf:about="http://lpis.ec.europa.eu/registry/applicationschema/cap-iacs-base/code#CropItemCodeValue/utilisedAgriculturalAreaUAA">
        <rdf:type rdf:resource="http://lpis.ec.europa.eu/registry/applicationschema/cap-iacs-base#CropItemCodeValue"/>
        <rdfs:label xml:lang="en">Utilised agricultural area (UAA)</rdfs:label>
        <skos:definition xml:lang="en">-- Definition --
|Utilised agricultural area (UAA).
-- Description --
Land use of Agriculture Area in Use -L
NOTE. Initial value:L0005</skos:definition>
        <skos:inScheme rdf:resource="http://lpis.ec.europa.eu/registry/applicationschema/cap-iacs-base/code#CropItemCodeValue"/>
    </owl:NamedIndividual>
    


    <!-- http://lpis.ec.europa.eu/registry/applicationschema/cap-iacs-base/code#CropItemCodeValue/vegetablesCultivatedForFruit -->


    <owl:NamedIndividual rdf:about="http://lpis.ec.europa.eu/registry/applicationschema/cap-iacs-base/code#CropItemCodeValue/vegetablesCultivatedForFruit">
        <rdf:type rdf:resource="http://lpis.ec.europa.eu/registry/applicationschema/cap-iacs-base#CropItemCodeValue"/>
        <rdfs:label xml:lang="en">Vegetables cultivated for fruit</rdfs:label>
        <skos:definition xml:lang="en">-- Definition --
||Vegetables cultivated for fruit.
-- Description --
Cereals and main crops - C
NOTE. Initial value:C1740</skos:definition>
        <skos:inScheme rdf:resource="http://lpis.ec.europa.eu/registry/applicationschema/cap-iacs-base/code#CropItemCodeValue"/>
    </owl:NamedIndividual>
    


    <!-- http://lpis.ec.europa.eu/registry/applicationschema/cap-iacs-base/code#CropItemCodeValue/vegetablesFromKitchenGardensC2992 -->


    <owl:NamedIndividual rdf:about="http://lpis.ec.europa.eu/registry/applicationschema/cap-iacs-base/code#CropItemCodeValue/vegetablesFromKitchenGardensC2992">
        <rdf:type rdf:resource="http://lpis.ec.europa.eu/registry/applicationschema/cap-iacs-base#CropItemCodeValue"/>
        <rdfs:label xml:lang="en">Vegetables from kitchen gardens C2992</rdfs:label>
        <skos:definition xml:lang="en">-- Definition --
Vegetables from kitchen gardens C2992.
-- Description --
Cereals and main crops - C
NOTE. Initial value:C2992</skos:definition>
        <skos:inScheme rdf:resource="http://lpis.ec.europa.eu/registry/applicationschema/cap-iacs-base/code#CropItemCodeValue"/>
    </owl:NamedIndividual>
    


    <!-- http://lpis.ec.europa.eu/registry/applicationschema/cap-iacs-base/code#CropItemCodeValue/vegetablesMelonsAndStrawberries -->


    <owl:NamedIndividual rdf:about="http://lpis.ec.europa.eu/registry/applicationschema/cap-iacs-base/code#CropItemCodeValue/vegetablesMelonsAndStrawberries">
        <rdf:type rdf:resource="http://lpis.ec.europa.eu/registry/applicationschema/cap-iacs-base#CropItemCodeValue"/>
        <rdfs:label xml:lang="en">Vegetables, melons and strawberries</rdfs:label>
        <skos:definition xml:lang="en">-- Definition --
|||Vegetables, melons and strawberries.
-- Description --
Land use of Agriculture Area in Use -L
NOTE. Initial value:L1600</skos:definition>
        <skos:inScheme rdf:resource="http://lpis.ec.europa.eu/registry/applicationschema/cap-iacs-base/code#CropItemCodeValue"/>
    </owl:NamedIndividual>
    


    <!-- http://lpis.ec.europa.eu/registry/applicationschema/cap-iacs-base/code#CropItemCodeValue/vegetablesMelonsAndStrawberriesExcludingKitchenGardens -->


    <owl:NamedIndividual rdf:about="http://lpis.ec.europa.eu/registry/applicationschema/cap-iacs-base/code#CropItemCodeValue/vegetablesMelonsAndStrawberriesExcludingKitchenGardens">
        <rdf:type rdf:resource="http://lpis.ec.europa.eu/registry/applicationschema/cap-iacs-base#CropItemCodeValue"/>
        <rdfs:label xml:lang="en">Vegetables, melons and strawberries (excluding kitchen gardens)</rdfs:label>
        <skos:definition xml:lang="en">-- Definition --
|Vegetables, melons and strawberries (excluding kitchen gardens).
-- Description --
Cereals and main crops - C
NOTE. Initial value:C1600</skos:definition>
        <skos:inScheme rdf:resource="http://lpis.ec.europa.eu/registry/applicationschema/cap-iacs-base/code#CropItemCodeValue"/>
    </owl:NamedIndividual>
    


    <!-- http://lpis.ec.europa.eu/registry/applicationschema/cap-iacs-base/code#CropItemCodeValue/vegetablesMelonsAndStrawberriesUnderGlassHighAccessibleCover -->


    <owl:NamedIndividual rdf:about="http://lpis.ec.europa.eu/registry/applicationschema/cap-iacs-base/code#CropItemCodeValue/vegetablesMelonsAndStrawberriesUnderGlassHighAccessibleCover">
        <rdf:type rdf:resource="http://lpis.ec.europa.eu/registry/applicationschema/cap-iacs-base#CropItemCodeValue"/>
        <rdfs:label xml:lang="en">Vegetables, melons and strawberries under glass high accessible cover</rdfs:label>
        <skos:definition xml:lang="en">-- Definition --
Vegetables, melons and strawberries under glass high accessible cover.
-- Description --
Land use of Agriculture Area in Use -L. Special aggregates
NOTE. Initial value:L1112</skos:definition>
        <skos:inScheme rdf:resource="http://lpis.ec.europa.eu/registry/applicationschema/cap-iacs-base/code#CropItemCodeValue"/>
    </owl:NamedIndividual>
    


    <!-- http://lpis.ec.europa.eu/registry/applicationschema/cap-iacs-base/code#CropItemCodeValue/vineyards -->


    <owl:NamedIndividual rdf:about="http://lpis.ec.europa.eu/registry/applicationschema/cap-iacs-base/code#CropItemCodeValue/vineyards">
        <rdf:type rdf:resource="http://lpis.ec.europa.eu/registry/applicationschema/cap-iacs-base#CropItemCodeValue"/>
        <rdfs:label xml:lang="en">Vineyards</rdfs:label>
        <skos:definition xml:lang="en">-- Definition --
|||Vineyards.
-- Description --
Land use of Agriculture Area in Use -L
NOTE. Initial value:L2410</skos:definition>
        <skos:inScheme rdf:resource="http://lpis.ec.europa.eu/registry/applicationschema/cap-iacs-base/code#CropItemCodeValue"/>
    </owl:NamedIndividual>
    


    <!-- http://lpis.ec.europa.eu/registry/applicationschema/cap-iacs-base/code#CropItemCodeValue/vineyardsC2410 -->


    <owl:NamedIndividual rdf:about="http://lpis.ec.europa.eu/registry/applicationschema/cap-iacs-base/code#CropItemCodeValue/vineyardsC2410">
        <rdf:type rdf:resource="http://lpis.ec.europa.eu/registry/applicationschema/cap-iacs-base#CropItemCodeValue"/>
        <rdfs:label xml:lang="en">Vineyards C2410</rdfs:label>
        <skos:definition xml:lang="en">-- Definition --
||Vineyards C2410.
-- Description --
Cereals and main crops - C
NOTE. Initial value:C2410</skos:definition>
        <skos:inScheme rdf:resource="http://lpis.ec.europa.eu/registry/applicationschema/cap-iacs-base/code#CropItemCodeValue"/>
    </owl:NamedIndividual>
    


    <!-- http://lpis.ec.europa.eu/registry/applicationschema/cap-iacs-base/code#CropItemCodeValue/vineyardsForOtherGrapeProductionNec -->


    <owl:NamedIndividual rdf:about="http://lpis.ec.europa.eu/registry/applicationschema/cap-iacs-base/code#CropItemCodeValue/vineyardsForOtherGrapeProductionNec">
        <rdf:type rdf:resource="http://lpis.ec.europa.eu/registry/applicationschema/cap-iacs-base#CropItemCodeValue"/>
        <rdfs:label xml:lang="en">Vineyards for other grape production n.e.c.</rdfs:label>
        <skos:definition xml:lang="en">-- Definition --
|||Vineyards for other grape production n.e.c.
-- Description --
Cereals and main crops - C
NOTE. Initial value:C2445</skos:definition>
        <skos:inScheme rdf:resource="http://lpis.ec.europa.eu/registry/applicationschema/cap-iacs-base/code#CropItemCodeValue"/>
    </owl:NamedIndividual>
    


    <!-- http://lpis.ec.europa.eu/registry/applicationschema/cap-iacs-base/code#CropItemCodeValue/vineyardsForOtherWines -->


    <owl:NamedIndividual rdf:about="http://lpis.ec.europa.eu/registry/applicationschema/cap-iacs-base/code#CropItemCodeValue/vineyardsForOtherWines">
        <rdf:type rdf:resource="http://lpis.ec.europa.eu/registry/applicationschema/cap-iacs-base#CropItemCodeValue"/>
        <rdfs:label xml:lang="en">Vineyards for other wines</rdfs:label>
        <skos:definition xml:lang="en">-- Definition --
||||Vineyards for other wines.
-- Description --
Cereals and main crops - C
NOTE. Initial value:C2443</skos:definition>
        <skos:inScheme rdf:resource="http://lpis.ec.europa.eu/registry/applicationschema/cap-iacs-base/code#CropItemCodeValue"/>
    </owl:NamedIndividual>
    


    <!-- http://lpis.ec.europa.eu/registry/applicationschema/cap-iacs-base/code#CropItemCodeValue/vineyardsForRaisins -->


    <owl:NamedIndividual rdf:about="http://lpis.ec.europa.eu/registry/applicationschema/cap-iacs-base/code#CropItemCodeValue/vineyardsForRaisins">
        <rdf:type rdf:resource="http://lpis.ec.europa.eu/registry/applicationschema/cap-iacs-base#CropItemCodeValue"/>
        <rdfs:label xml:lang="en">Vineyards for raisins</rdfs:label>
        <skos:definition xml:lang="en">-- Definition --
|||Vineyards for raisins.
-- Description --
Cereals and main crops - C
NOTE. Initial value:C2416</skos:definition>
        <skos:inScheme rdf:resource="http://lpis.ec.europa.eu/registry/applicationschema/cap-iacs-base/code#CropItemCodeValue"/>
    </owl:NamedIndividual>
    


    <!-- http://lpis.ec.europa.eu/registry/applicationschema/cap-iacs-base/code#CropItemCodeValue/vineyardsForTableGrapes -->


    <owl:NamedIndividual rdf:about="http://lpis.ec.europa.eu/registry/applicationschema/cap-iacs-base/code#CropItemCodeValue/vineyardsForTableGrapes">
        <rdf:type rdf:resource="http://lpis.ec.europa.eu/registry/applicationschema/cap-iacs-base#CropItemCodeValue"/>
        <rdfs:label xml:lang="en">Vineyards for table grapes</rdfs:label>
        <skos:definition xml:lang="en">-- Definition --
|||Vineyards for table grapes.
-- Description --
Cereals and main crops - C
NOTE. Initial value:C2420</skos:definition>
        <skos:inScheme rdf:resource="http://lpis.ec.europa.eu/registry/applicationschema/cap-iacs-base/code#CropItemCodeValue"/>
    </owl:NamedIndividual>
    


    <!-- http://lpis.ec.europa.eu/registry/applicationschema/cap-iacs-base/code#CropItemCodeValue/vineyardsForWine -->


    <owl:NamedIndividual rdf:about="http://lpis.ec.europa.eu/registry/applicationschema/cap-iacs-base/code#CropItemCodeValue/vineyardsForWine">
        <rdf:type rdf:resource="http://lpis.ec.europa.eu/registry/applicationschema/cap-iacs-base#CropItemCodeValue"/>
        <rdfs:label xml:lang="en">Vineyards for wine</rdfs:label>
        <skos:definition xml:lang="en">-- Definition --
|||Vineyards for wine.
-- Description --
Cereals and main crops - C
NOTE. Initial value:C2440</skos:definition>
        <skos:inScheme rdf:resource="http://lpis.ec.europa.eu/registry/applicationschema/cap-iacs-base/code#CropItemCodeValue"/>
    </owl:NamedIndividual>
    


    <!-- http://lpis.ec.europa.eu/registry/applicationschema/cap-iacs-base/code#CropItemCodeValue/vineyardsForWinesWithProtectedDesignationOfOriginPDO -->


    <owl:NamedIndividual rdf:about="http://lpis.ec.europa.eu/registry/applicationschema/cap-iacs-base/code#CropItemCodeValue/vineyardsForWinesWithProtectedDesignationOfOriginPDO">
        <rdf:type rdf:resource="http://lpis.ec.europa.eu/registry/applicationschema/cap-iacs-base#CropItemCodeValue"/>
        <rdfs:label xml:lang="en">Vineyards for wines with protected designation of origin (PDO)</rdfs:label>
        <skos:definition xml:lang="en">-- Definition --
||||Vineyards for wines with protected designation of origin (PDO).
-- Description --
Cereals and main crops - C
NOTE. Initial value:C2441</skos:definition>
        <skos:inScheme rdf:resource="http://lpis.ec.europa.eu/registry/applicationschema/cap-iacs-base/code#CropItemCodeValue"/>
    </owl:NamedIndividual>
    


    <!-- http://lpis.ec.europa.eu/registry/applicationschema/cap-iacs-base/code#CropItemCodeValue/vineyardsForWinesWithProtectedGeographicalIndicationPGI -->


    <owl:NamedIndividual rdf:about="http://lpis.ec.europa.eu/registry/applicationschema/cap-iacs-base/code#CropItemCodeValue/vineyardsForWinesWithProtectedGeographicalIndicationPGI">
        <rdf:type rdf:resource="http://lpis.ec.europa.eu/registry/applicationschema/cap-iacs-base#CropItemCodeValue"/>
        <rdfs:label xml:lang="en">Vineyards for wines with protected geographical indication (PGI)</rdfs:label>
        <skos:definition xml:lang="en">-- Definition --
||||Vineyards for wines with protected geographical indication (PGI).
-- Description --
Cereals and main crops - C
NOTE. Initial value:C2442</skos:definition>
        <skos:inScheme rdf:resource="http://lpis.ec.europa.eu/registry/applicationschema/cap-iacs-base/code#CropItemCodeValue"/>
    </owl:NamedIndividual>
    


    <!-- http://lpis.ec.europa.eu/registry/applicationschema/cap-iacs-base/code#CropItemCodeValue/walnuts -->


    <owl:NamedIndividual rdf:about="http://lpis.ec.europa.eu/registry/applicationschema/cap-iacs-base/code#CropItemCodeValue/walnuts">
        <rdf:type rdf:resource="http://lpis.ec.europa.eu/registry/applicationschema/cap-iacs-base#CropItemCodeValue"/>
        <rdfs:label xml:lang="en">Walnuts</rdfs:label>
        <skos:definition xml:lang="en">-- Definition --
|||Walnuts.
-- Description --
Cereals and main crops - C
NOTE. Initial value:C2231</skos:definition>
        <skos:inScheme rdf:resource="http://lpis.ec.europa.eu/registry/applicationschema/cap-iacs-base/code#CropItemCodeValue"/>
    </owl:NamedIndividual>
    


    <!-- http://lpis.ec.europa.eu/registry/applicationschema/cap-iacs-base/code#CropItemCodeValue/watermelons -->


    <owl:NamedIndividual rdf:about="http://lpis.ec.europa.eu/registry/applicationschema/cap-iacs-base/code#CropItemCodeValue/watermelons">
        <rdf:type rdf:resource="http://lpis.ec.europa.eu/registry/applicationschema/cap-iacs-base#CropItemCodeValue"/>
        <rdfs:label xml:lang="en">Watermelons</rdfs:label>
        <skos:definition xml:lang="en">-- Definition --
||Watermelons.
-- Description --
Cereals and main crops - C
NOTE. Initial value:C1777</skos:definition>
        <skos:inScheme rdf:resource="http://lpis.ec.europa.eu/registry/applicationschema/cap-iacs-base/code#CropItemCodeValue"/>
    </owl:NamedIndividual>
    


    <!-- http://lpis.ec.europa.eu/registry/applicationschema/cap-iacs-base/code#CropItemCodeValue/weavingPlants -->


    <owl:NamedIndividual rdf:about="http://lpis.ec.europa.eu/registry/applicationschema/cap-iacs-base/code#CropItemCodeValue/weavingPlants">
        <rdf:type rdf:resource="http://lpis.ec.europa.eu/registry/applicationschema/cap-iacs-base#CropItemCodeValue"/>
        <rdfs:label xml:lang="en">Weaving plants</rdfs:label>
        <skos:definition xml:lang="en">-- Definition --
|||Weaving plants.
-- Description --
Land use of Agriculture Area in Use -L
NOTE. Initial value:L2960</skos:definition>
        <skos:inScheme rdf:resource="http://lpis.ec.europa.eu/registry/applicationschema/cap-iacs-base/code#CropItemCodeValue"/>
    </owl:NamedIndividual>
    


    <!-- http://lpis.ec.europa.eu/registry/applicationschema/cap-iacs-base/code#CropItemCodeValue/wheatIncludingSpelt -->


    <owl:NamedIndividual rdf:about="http://lpis.ec.europa.eu/registry/applicationschema/cap-iacs-base/code#CropItemCodeValue/wheatIncludingSpelt">
        <rdf:type rdf:resource="http://lpis.ec.europa.eu/registry/applicationschema/cap-iacs-base#CropItemCodeValue"/>
        <rdfs:label xml:lang="en">Wheat (including spelt)</rdfs:label>
        <skos:definition xml:lang="en">-- Definition --
|||Wheat (including spelt).
-- Description --
Cereals and main crops - C
NOTE. Initial value:C1100</skos:definition>
        <skos:inScheme rdf:resource="http://lpis.ec.europa.eu/registry/applicationschema/cap-iacs-base/code#CropItemCodeValue"/>
    </owl:NamedIndividual>
    


    <!-- http://lpis.ec.europa.eu/registry/applicationschema/cap-iacs-base/code#CropItemCodeValue/winterBarley -->


    <owl:NamedIndividual rdf:about="http://lpis.ec.europa.eu/registry/applicationschema/cap-iacs-base/code#CropItemCodeValue/winterBarley">
        <rdf:type rdf:resource="http://lpis.ec.europa.eu/registry/applicationschema/cap-iacs-base#CropItemCodeValue"/>
        <rdfs:label xml:lang="en">Winter barley</rdfs:label>
        <skos:definition xml:lang="en">-- Definition --
||||Winter barley.
-- Description --
Cereals and main crops - C
NOTE. Initial value:C1163</skos:definition>
        <skos:inScheme rdf:resource="http://lpis.ec.europa.eu/registry/applicationschema/cap-iacs-base/code#CropItemCodeValue"/>
    </owl:NamedIndividual>
    


    <!-- http://lpis.ec.europa.eu/registry/applicationschema/cap-iacs-base/code#CropItemCodeValue/winterDurumWheat -->


    <owl:NamedIndividual rdf:about="http://lpis.ec.europa.eu/registry/applicationschema/cap-iacs-base/code#CropItemCodeValue/winterDurumWheat">
        <rdf:type rdf:resource="http://lpis.ec.europa.eu/registry/applicationschema/cap-iacs-base#CropItemCodeValue"/>
        <rdfs:label xml:lang="en">Winter durum wheat</rdfs:label>
        <skos:definition xml:lang="en">-- Definition --
|||||Winter durum wheat.
-- Description --
Cereals and main crops - C
NOTE. Initial value:C1133</skos:definition>
        <skos:inScheme rdf:resource="http://lpis.ec.europa.eu/registry/applicationschema/cap-iacs-base/code#CropItemCodeValue"/>
    </owl:NamedIndividual>
    


    <!-- http://lpis.ec.europa.eu/registry/applicationschema/cap-iacs-base/code#CropItemCodeValue/winterRape -->


    <owl:NamedIndividual rdf:about="http://lpis.ec.europa.eu/registry/applicationschema/cap-iacs-base/code#CropItemCodeValue/winterRape">
        <rdf:type rdf:resource="http://lpis.ec.europa.eu/registry/applicationschema/cap-iacs-base#CropItemCodeValue"/>
        <rdfs:label xml:lang="en">Winter rape</rdfs:label>
        <skos:definition xml:lang="en">-- Definition --
||||||Winter rape.
-- Description --
Cereals and main crops - C
NOTE. Initial value:C1431</skos:definition>
        <skos:inScheme rdf:resource="http://lpis.ec.europa.eu/registry/applicationschema/cap-iacs-base/code#CropItemCodeValue"/>
    </owl:NamedIndividual>
    


    <!-- http://lpis.ec.europa.eu/registry/applicationschema/cap-iacs-base/code#CropItemCodeValue/winterRye -->


    <owl:NamedIndividual rdf:about="http://lpis.ec.europa.eu/registry/applicationschema/cap-iacs-base/code#CropItemCodeValue/winterRye">
        <rdf:type rdf:resource="http://lpis.ec.europa.eu/registry/applicationschema/cap-iacs-base#CropItemCodeValue"/>
        <rdfs:label xml:lang="en">Winter rye</rdfs:label>
        <skos:definition xml:lang="en">-- Definition --
|||||Winter rye.
-- Description --
Cereals and main crops - C
NOTE. Initial value:C1151</skos:definition>
        <skos:inScheme rdf:resource="http://lpis.ec.europa.eu/registry/applicationschema/cap-iacs-base/code#CropItemCodeValue"/>
    </owl:NamedIndividual>
    


    <!-- http://lpis.ec.europa.eu/registry/applicationschema/cap-iacs-base/code#CropItemCodeValue/winterTriticale -->


    <owl:NamedIndividual rdf:about="http://lpis.ec.europa.eu/registry/applicationschema/cap-iacs-base/code#CropItemCodeValue/winterTriticale">
        <rdf:type rdf:resource="http://lpis.ec.europa.eu/registry/applicationschema/cap-iacs-base#CropItemCodeValue"/>
        <rdfs:label xml:lang="en">Winter triticale</rdfs:label>
        <skos:definition xml:lang="en">-- Definition --
||||Winter triticale.
-- Description --
Cereals and main crops - C
NOTE. Initial value:C1213</skos:definition>
        <skos:inScheme rdf:resource="http://lpis.ec.europa.eu/registry/applicationschema/cap-iacs-base/code#CropItemCodeValue"/>
    </owl:NamedIndividual>
    


    <!-- http://lpis.ec.europa.eu/registry/applicationschema/cap-iacs-base/code#CropItemCodeValue/yellowLemons -->


    <owl:NamedIndividual rdf:about="http://lpis.ec.europa.eu/registry/applicationschema/cap-iacs-base/code#CropItemCodeValue/yellowLemons">
        <rdf:type rdf:resource="http://lpis.ec.europa.eu/registry/applicationschema/cap-iacs-base#CropItemCodeValue"/>
        <rdfs:label xml:lang="en">Yellow lemons</rdfs:label>
        <skos:definition xml:lang="en">-- Definition --
||||Yellow lemons.
-- Description --
Cereals and main crops - C
NOTE. Initial value:C2371</skos:definition>
        <skos:inScheme rdf:resource="http://lpis.ec.europa.eu/registry/applicationschema/cap-iacs-base/code#CropItemCodeValue"/>
    </owl:NamedIndividual>
    


    <!-- http://lpis.ec.europa.eu/registry/applicationschema/cap-iacs-base/code#CrossComplianceRuleValue/animalWelfareAnimalWelfareSmr11 -->


    <owl:NamedIndividual rdf:about="http://lpis.ec.europa.eu/registry/applicationschema/cap-iacs-base/code#CrossComplianceRuleValue/animalWelfareAnimalWelfareSmr11">
        <rdf:type rdf:resource="http://lpis.ec.europa.eu/registry/applicationschema/cap-iacs-base#CrossComplianceRuleValue"/>
        <rdfs:label xml:lang="en">Animal welfare - Animal welfare SMR11</rdfs:label>
        <skos:definition xml:lang="en">-- Definition --
Animal welfare - Animal welfare SMR11.
-- Description --
Council Directive 2008/119/EC of 18 December 2008 laying down minimum standards for the protection of calves (OJ L 10, 15.1.2009, p. 7) . Articles 3 and 4.
NOTE. Initial value:SMR11</skos:definition>
        <skos:inScheme rdf:resource="http://lpis.ec.europa.eu/registry/applicationschema/cap-iacs-base/code#CrossComplianceRuleValue"/>
    </owl:NamedIndividual>
    


    <!-- http://lpis.ec.europa.eu/registry/applicationschema/cap-iacs-base/code#CrossComplianceRuleValue/animalWelfareAnimalWelfareSmr12 -->


    <owl:NamedIndividual rdf:about="http://lpis.ec.europa.eu/registry/applicationschema/cap-iacs-base/code#CrossComplianceRuleValue/animalWelfareAnimalWelfareSmr12">
        <rdf:type rdf:resource="http://lpis.ec.europa.eu/registry/applicationschema/cap-iacs-base#CrossComplianceRuleValue"/>
        <rdfs:label xml:lang="en">Animal welfare - Animal welfare SMR12</rdfs:label>
        <skos:definition xml:lang="en">-- Definition --
Animal welfare - Animal welfare SMR12.
-- Description --
Council Directive 2008/120/EC of 18 December 2008 laying down minimum standards for the protection of pigs (OJ L 47, 18.2.2009, p. 5). Article 3 and Article 4.
NOTE. Initial value:SMR12</skos:definition>
        <skos:inScheme rdf:resource="http://lpis.ec.europa.eu/registry/applicationschema/cap-iacs-base/code#CrossComplianceRuleValue"/>
    </owl:NamedIndividual>
    


    <!-- http://lpis.ec.europa.eu/registry/applicationschema/cap-iacs-base/code#CrossComplianceRuleValue/animalWelfareAnimalWelfareSmr13 -->


    <owl:NamedIndividual rdf:about="http://lpis.ec.europa.eu/registry/applicationschema/cap-iacs-base/code#CrossComplianceRuleValue/animalWelfareAnimalWelfareSmr13">
        <rdf:type rdf:resource="http://lpis.ec.europa.eu/registry/applicationschema/cap-iacs-base#CrossComplianceRuleValue"/>
        <rdfs:label xml:lang="en">Animal welfare - Animal welfare SMR13</rdfs:label>
        <skos:definition xml:lang="en">-- Definition --
Animal welfare - Animal welfare SMR13.
-- Description --
Council Directive 98/58/EC of 20 July 1998 concerning the protection of animals kept for farming purposes (OJ L 221, 8.8.1998, p. 23) . Article 4 .
NOTE. Initial value:SMR13</skos:definition>
        <skos:inScheme rdf:resource="http://lpis.ec.europa.eu/registry/applicationschema/cap-iacs-base/code#CrossComplianceRuleValue"/>
    </owl:NamedIndividual>
    


    <!-- http://lpis.ec.europa.eu/registry/applicationschema/cap-iacs-base/code#CrossComplianceRuleValue/environmentClimateChangeGoodAgriculturalConditionOfLandBiodiversitySmr2 -->


    <owl:NamedIndividual rdf:about="http://lpis.ec.europa.eu/registry/applicationschema/cap-iacs-base/code#CrossComplianceRuleValue/environmentClimateChangeGoodAgriculturalConditionOfLandBiodiversitySmr2">
        <rdf:type rdf:resource="http://lpis.ec.europa.eu/registry/applicationschema/cap-iacs-base#CrossComplianceRuleValue"/>
        <rdfs:label xml:lang="en">Environment, climate change, good agricultural condition of land  - Biodiversity SMR2</rdfs:label>
        <skos:definition xml:lang="en">-- Definition --
Environment, climate change, good agricultural condition of land  - Biodiversity SMR2.
-- Description --
Directive 2009/147/EC of the European Parliament and of the Council of 30 November 2009 on the conservation of wild birds (OJ L 20, 26.1.2010, p. 7). Article 3(1), Article 3(2)(b), Article 4(1), (2) and (4).
NOTE. Initial value:SMR2</skos:definition>
        <skos:inScheme rdf:resource="http://lpis.ec.europa.eu/registry/applicationschema/cap-iacs-base/code#CrossComplianceRuleValue"/>
    </owl:NamedIndividual>
    


    <!-- http://lpis.ec.europa.eu/registry/applicationschema/cap-iacs-base/code#CrossComplianceRuleValue/environmentClimateChangeGoodAgriculturalConditionOfLandBiodiversitySmr3 -->


    <owl:NamedIndividual rdf:about="http://lpis.ec.europa.eu/registry/applicationschema/cap-iacs-base/code#CrossComplianceRuleValue/environmentClimateChangeGoodAgriculturalConditionOfLandBiodiversitySmr3">
        <rdf:type rdf:resource="http://lpis.ec.europa.eu/registry/applicationschema/cap-iacs-base#CrossComplianceRuleValue"/>
        <rdfs:label xml:lang="en">Environment, climate change, good agricultural condition of land  - Biodiversity SMR3</rdfs:label>
        <skos:definition xml:lang="en">-- Definition --
Environment, climate change, good agricultural condition of land  - Biodiversity SMR3.
-- Description --
Council Directive 92/43/EEC of 21 May 1992 on the conservation of natural habitats and of wild flora and fauna (OJ L 206, 22.7.1992, p. 7) . Article 6(1) and (2).
NOTE. Initial value:SMR3</skos:definition>
        <skos:inScheme rdf:resource="http://lpis.ec.europa.eu/registry/applicationschema/cap-iacs-base/code#CrossComplianceRuleValue"/>
    </owl:NamedIndividual>
    


    <!-- http://lpis.ec.europa.eu/registry/applicationschema/cap-iacs-base/code#CrossComplianceRuleValue/environmentClimateChangeGoodAgriculturalConditionOfLandLandscapeMinimumLevelOfMaintenanceGaec7 -->


    <owl:NamedIndividual rdf:about="http://lpis.ec.europa.eu/registry/applicationschema/cap-iacs-base/code#CrossComplianceRuleValue/environmentClimateChangeGoodAgriculturalConditionOfLandLandscapeMinimumLevelOfMaintenanceGaec7">
        <rdf:type rdf:resource="http://lpis.ec.europa.eu/registry/applicationschema/cap-iacs-base#CrossComplianceRuleValue"/>
        <rdfs:label xml:lang="en">Environment, climate change, good agricultural condition of land  - Landscape, minimum level of maintenance GAEC7</rdfs:label>
        <skos:definition xml:lang="en">-- Definition --
Environment, climate change, good agricultural condition of land  - Landscape, minimum level of maintenance GAEC7.
-- Description --
Retention of landscape features, including where appropriate, hedges, ponds, ditches, trees in line, in group or isolated, field margins and terraces, and including a ban on cutting hedges and trees during the bird breeding and rearing season and, as an option, measures for avoiding invasive plant species. 
NOTE. Initial value:GAEC7.</skos:definition>
        <skos:inScheme rdf:resource="http://lpis.ec.europa.eu/registry/applicationschema/cap-iacs-base/code#CrossComplianceRuleValue"/>
    </owl:NamedIndividual>
    


    <!-- http://lpis.ec.europa.eu/registry/applicationschema/cap-iacs-base/code#CrossComplianceRuleValue/environmentClimateChangeGoodAgriculturalConditionOfLandSoilAndCarbonStockGaec4 -->


    <owl:NamedIndividual rdf:about="http://lpis.ec.europa.eu/registry/applicationschema/cap-iacs-base/code#CrossComplianceRuleValue/environmentClimateChangeGoodAgriculturalConditionOfLandSoilAndCarbonStockGaec4">
        <rdf:type rdf:resource="http://lpis.ec.europa.eu/registry/applicationschema/cap-iacs-base#CrossComplianceRuleValue"/>
        <rdfs:label xml:lang="en">Environment, climate change, good agricultural condition of land  - Soil and carbon stock  GAEC4</rdfs:label>
        <skos:definition xml:lang="en">-- Definition --
Environment, climate change, good agricultural condition of land  - Soil and carbon stock  GAEC4.
-- Description --
Minimum soil cover. 
NOTE. Initial value:GAEC4</skos:definition>
        <skos:inScheme rdf:resource="http://lpis.ec.europa.eu/registry/applicationschema/cap-iacs-base/code#CrossComplianceRuleValue"/>
    </owl:NamedIndividual>
    


    <!-- http://lpis.ec.europa.eu/registry/applicationschema/cap-iacs-base/code#CrossComplianceRuleValue/environmentClimateChangeGoodAgriculturalConditionOfLandSoilAndCarbonStockGaec5 -->


    <owl:NamedIndividual rdf:about="http://lpis.ec.europa.eu/registry/applicationschema/cap-iacs-base/code#CrossComplianceRuleValue/environmentClimateChangeGoodAgriculturalConditionOfLandSoilAndCarbonStockGaec5">
        <rdf:type rdf:resource="http://lpis.ec.europa.eu/registry/applicationschema/cap-iacs-base#CrossComplianceRuleValue"/>
        <rdfs:label xml:lang="en">Environment, climate change, good agricultural condition of land  - Soil and carbon stock  GAEC5</rdfs:label>
        <skos:definition xml:lang="en">-- Definition --
Environment, climate change, good agricultural condition of land  - Soil and carbon stock  GAEC5.
-- Description --
Minimum land management reflecting site specific conditions to limit erosion. 
NOTE. Initial value:GAEC5</skos:definition>
        <skos:inScheme rdf:resource="http://lpis.ec.europa.eu/registry/applicationschema/cap-iacs-base/code#CrossComplianceRuleValue"/>
    </owl:NamedIndividual>
    


    <!-- http://lpis.ec.europa.eu/registry/applicationschema/cap-iacs-base/code#CrossComplianceRuleValue/environmentClimateChangeGoodAgriculturalConditionOfLandSoilAndCarbonStockGaec6 -->


    <owl:NamedIndividual rdf:about="http://lpis.ec.europa.eu/registry/applicationschema/cap-iacs-base/code#CrossComplianceRuleValue/environmentClimateChangeGoodAgriculturalConditionOfLandSoilAndCarbonStockGaec6">
        <rdf:type rdf:resource="http://lpis.ec.europa.eu/registry/applicationschema/cap-iacs-base#CrossComplianceRuleValue"/>
        <rdfs:label xml:lang="en">Environment, climate change, good agricultural condition of land  - Soil and carbon stock  GAEC6</rdfs:label>
        <skos:definition xml:lang="en">-- Definition --
Environment, climate change, good agricultural condition of land  - Soil and carbon stock  GAEC6.
-- Description --
Maintenance of soil organic matter level through appropriate practices including ban on burning arable stubble, except for plant health reasons.. The requirement can be limited to a general ban on burning arable stubble, but a Member State may decide to prescribe further requirements.
NOTE. Initial value:GAEC6</skos:definition>
        <skos:inScheme rdf:resource="http://lpis.ec.europa.eu/registry/applicationschema/cap-iacs-base/code#CrossComplianceRuleValue"/>
    </owl:NamedIndividual>
    


    <!-- http://lpis.ec.europa.eu/registry/applicationschema/cap-iacs-base/code#CrossComplianceRuleValue/environmentClimateChangeGoodAgriculturalConditionOfLandWaterGaec1 -->


    <owl:NamedIndividual rdf:about="http://lpis.ec.europa.eu/registry/applicationschema/cap-iacs-base/code#CrossComplianceRuleValue/environmentClimateChangeGoodAgriculturalConditionOfLandWaterGaec1">
        <rdf:type rdf:resource="http://lpis.ec.europa.eu/registry/applicationschema/cap-iacs-base#CrossComplianceRuleValue"/>
        <rdfs:label xml:lang="en">Environment, climate change, good agricultural condition of land  - Water GAEC1</rdfs:label>
        <skos:definition xml:lang="en">-- Definition --
Environment, climate change, good agricultural condition of land  - Water GAEC1.
-- Description --
Establishment of buffer strips along water courses. The GAEC buffer strips must respect, both within and outside vulnerable zones designated pursuant to Article 3(2) of Directive 91/676/EEC, at least the requirements relating to the conditions for land application of fertiliser near water courses, referred to in point A.4 of Annex II to Directive 91/676/EEC to be applied in accordance with the action programmes of Member States established under Article 5(4) of Directive 91/676/EEC.
NOTE. Initial value:GAEC1</skos:definition>
        <skos:inScheme rdf:resource="http://lpis.ec.europa.eu/registry/applicationschema/cap-iacs-base/code#CrossComplianceRuleValue"/>
    </owl:NamedIndividual>
    


    <!-- http://lpis.ec.europa.eu/registry/applicationschema/cap-iacs-base/code#CrossComplianceRuleValue/environmentClimateChangeGoodAgriculturalConditionOfLandWaterGaec2 -->


    <owl:NamedIndividual rdf:about="http://lpis.ec.europa.eu/registry/applicationschema/cap-iacs-base/code#CrossComplianceRuleValue/environmentClimateChangeGoodAgriculturalConditionOfLandWaterGaec2">
        <rdf:type rdf:resource="http://lpis.ec.europa.eu/registry/applicationschema/cap-iacs-base#CrossComplianceRuleValue"/>
        <rdfs:label xml:lang="en">Environment, climate change, good agricultural condition of land  - Water GAEC2</rdfs:label>
        <skos:definition xml:lang="en">-- Definition --
Environment, climate change, good agricultural condition of land  - Water GAEC2.
-- Description --
Where use of water for irrigation is subject to authorisation, compliance with authorisation procedures. 
NOTE. Initial value:GAEC2</skos:definition>
        <skos:inScheme rdf:resource="http://lpis.ec.europa.eu/registry/applicationschema/cap-iacs-base/code#CrossComplianceRuleValue"/>
    </owl:NamedIndividual>
    


    <!-- http://lpis.ec.europa.eu/registry/applicationschema/cap-iacs-base/code#CrossComplianceRuleValue/environmentClimateChangeGoodAgriculturalConditionOfLandWaterGaec3 -->


    <owl:NamedIndividual rdf:about="http://lpis.ec.europa.eu/registry/applicationschema/cap-iacs-base/code#CrossComplianceRuleValue/environmentClimateChangeGoodAgriculturalConditionOfLandWaterGaec3">
        <rdf:type rdf:resource="http://lpis.ec.europa.eu/registry/applicationschema/cap-iacs-base#CrossComplianceRuleValue"/>
        <rdfs:label xml:lang="en">Environment, climate change, good agricultural condition of land  - Water GAEC3</rdfs:label>
        <skos:definition xml:lang="en">-- Definition --
Environment, climate change, good agricultural condition of land  - Water GAEC3.
-- Description --
Protection of ground water against pollution: prohibition of direct discharge into groundwater and measures to prevent indirect pollution of groundwater through discharge on the ground and percolation through the soil of dangerous substances, as listed in the Annex to Directive 80/68/EEC in its version in force on the last day of its validity, as far as it relates to agricultural activity. 
NOTE. Initial value:GAEC3</skos:definition>
        <skos:inScheme rdf:resource="http://lpis.ec.europa.eu/registry/applicationschema/cap-iacs-base/code#CrossComplianceRuleValue"/>
    </owl:NamedIndividual>
    


    <!-- http://lpis.ec.europa.eu/registry/applicationschema/cap-iacs-base/code#CrossComplianceRuleValue/environmentClimateChangeGoodAgriculturalConditionOfLandWaterSmr1 -->


    <owl:NamedIndividual rdf:about="http://lpis.ec.europa.eu/registry/applicationschema/cap-iacs-base/code#CrossComplianceRuleValue/environmentClimateChangeGoodAgriculturalConditionOfLandWaterSmr1">
        <rdf:type rdf:resource="http://lpis.ec.europa.eu/registry/applicationschema/cap-iacs-base#CrossComplianceRuleValue"/>
        <rdfs:label xml:lang="en">Environment, climate change, good agricultural condition of land  - Water SMR1</rdfs:label>
        <skos:definition xml:lang="en">-- Definition --
Environment, climate change, good agricultural condition of land  - Water SMR1.
-- Description --
Council Directive 91/676/EEC of 12 December 1991 concerning the protection of waters against pollution caused by nitrates from agricultural sources (OJ L 375, 31.12.1991, p. 1) . Articles 4 and 5.
NOTE. Initial value:SMR1</skos:definition>
        <skos:inScheme rdf:resource="http://lpis.ec.europa.eu/registry/applicationschema/cap-iacs-base/code#CrossComplianceRuleValue"/>
    </owl:NamedIndividual>
    


    <!-- http://lpis.ec.europa.eu/registry/applicationschema/cap-iacs-base/code#CrossComplianceRuleValue/publicHealthAnimalHealthAndPlantHealthAnimalDiseasesSmr9 -->


    <owl:NamedIndividual rdf:about="http://lpis.ec.europa.eu/registry/applicationschema/cap-iacs-base/code#CrossComplianceRuleValue/publicHealthAnimalHealthAndPlantHealthAnimalDiseasesSmr9">
        <rdf:type rdf:resource="http://lpis.ec.europa.eu/registry/applicationschema/cap-iacs-base#CrossComplianceRuleValue"/>
        <rdfs:label xml:lang="en">Public health, animal health and plant health  - Animal diseases SMR9</rdfs:label>
        <skos:definition xml:lang="en">-- Definition --
Public health, animal health and plant health  - Animal diseases SMR9.
-- Description --
Regulation (EC) No 999/2001 of the European Parliament and of the Council of 22 May 2001 laying down rules for the prevention, control and eradication of certain transmissible spongiform encephalopathies (OJ L 147, 31.5.2001, p. 1). Articles 7, 11, 12, 13 and 15.
NOTE. Initial value:SMR9</skos:definition>
        <skos:inScheme rdf:resource="http://lpis.ec.europa.eu/registry/applicationschema/cap-iacs-base/code#CrossComplianceRuleValue"/>
    </owl:NamedIndividual>
    


    <!-- http://lpis.ec.europa.eu/registry/applicationschema/cap-iacs-base/code#CrossComplianceRuleValue/publicHealthAnimalHealthAndPlantHealthFoodSafetySmr4 -->


    <owl:NamedIndividual rdf:about="http://lpis.ec.europa.eu/registry/applicationschema/cap-iacs-base/code#CrossComplianceRuleValue/publicHealthAnimalHealthAndPlantHealthFoodSafetySmr4">
        <rdf:type rdf:resource="http://lpis.ec.europa.eu/registry/applicationschema/cap-iacs-base#CrossComplianceRuleValue"/>
        <rdfs:label xml:lang="en">Public health, animal health and plant health  - Food safety SMR4</rdfs:label>
        <skos:definition xml:lang="en">-- Definition --
Public health, animal health and plant health  - Food safety SMR4.
-- Description --
Regulation (EC) No 178/2002 of the European Parliament and of the Council of 28 January 2002 laying down the general principles and requirements of food law, establishing the European Food Safety Authority and laying down procedures in matters of food safety (OJ L 31, 1.2.2002, p. 1). Articles 14 and 15, Article 17(1) [3] and Articles 18, 19 and 20 [3] As implemented in particular by:- Article 14 of Regulation (EC) No 470/2009 and the Annex of Regulation (EC) No 37/2010,- Regulation (EC) No 852/2004: Article 4(1) and Annex I part A (II 4 (g, h, j), 5 (f, h), 6; III 8 (a, b, d, e), 9 (a, c)),- Regulation (EC) No 853/2004: Article 3(1) and Annex III Section IX Chapter 1 (I-1 b, c, d, e; I-2 a (i, ii, iii), b (i, ii), c; I-3; I-4; I-5; II-A 1, 2, 3, 4; II-B 1(a, d), 2, 4 (a, b)), Annex III Section X Chapter 1(1),- Regulation (EC) No 183/2005: Article 5(1) and Annex I, part A (I-4 e, g; II-2 a, b, e), Article 5(5) and Annex III (1, 2), Article 5(6), and- Regulation (EC) No 396/2005: Article 18.
NOTE. Initial value:SMR4</skos:definition>
        <skos:inScheme rdf:resource="http://lpis.ec.europa.eu/registry/applicationschema/cap-iacs-base/code#CrossComplianceRuleValue"/>
    </owl:NamedIndividual>
    


    <!-- http://lpis.ec.europa.eu/registry/applicationschema/cap-iacs-base/code#CrossComplianceRuleValue/publicHealthAnimalHealthAndPlantHealthFoodSafetySmr5 -->


    <owl:NamedIndividual rdf:about="http://lpis.ec.europa.eu/registry/applicationschema/cap-iacs-base/code#CrossComplianceRuleValue/publicHealthAnimalHealthAndPlantHealthFoodSafetySmr5">
        <rdf:type rdf:resource="http://lpis.ec.europa.eu/registry/applicationschema/cap-iacs-base#CrossComplianceRuleValue"/>
        <rdfs:label xml:lang="en">Public health, animal health and plant health  - Food safety SMR5</rdfs:label>
        <skos:definition xml:lang="en">-- Definition --
Public health, animal health and plant health  - Food safety SMR5.
-- Description --
Council Directive 96/22/EC of 29 April 1996 concerning the prohibition on the use in stockfarming of certain substances having a hormonal or thyrostatic action and beta-agonists, and repealing Directives 81/602/EEC, 88/146/EEC and 88/299/EEC (OJ L 125, 23.5.1996, p. 3). Article 3(a), (b), (d) and (e) and Articles 4, 5 and 7.
NOTE. Initial value:SMR5</skos:definition>
        <skos:inScheme rdf:resource="http://lpis.ec.europa.eu/registry/applicationschema/cap-iacs-base/code#CrossComplianceRuleValue"/>
    </owl:NamedIndividual>
    


    <!-- http://lpis.ec.europa.eu/registry/applicationschema/cap-iacs-base/code#CrossComplianceRuleValue/publicHealthAnimalHealthAndPlantHealthIdentificationAndRegistrationOfAnimalsSmr6 -->


    <owl:NamedIndividual rdf:about="http://lpis.ec.europa.eu/registry/applicationschema/cap-iacs-base/code#CrossComplianceRuleValue/publicHealthAnimalHealthAndPlantHealthIdentificationAndRegistrationOfAnimalsSmr6">
        <rdf:type rdf:resource="http://lpis.ec.europa.eu/registry/applicationschema/cap-iacs-base#CrossComplianceRuleValue"/>
        <rdfs:label xml:lang="en">Public health, animal health and plant health  - Identification and registration of animals SMR6</rdfs:label>
        <skos:definition xml:lang="en">-- Definition --
Public health, animal health and plant health  - Identification and registration of animals SMR6.
-- Description --
Council Directive 2008/71/EC of 15 July 2008 on identification and registration of pigs (OJ L 213, 8.8.2005, p. 31). Articles 3, 4 and 5.
NOTE. Initial value:SMR6</skos:definition>
        <skos:inScheme rdf:resource="http://lpis.ec.europa.eu/registry/applicationschema/cap-iacs-base/code#CrossComplianceRuleValue"/>
    </owl:NamedIndividual>
    


    <!-- http://lpis.ec.europa.eu/registry/applicationschema/cap-iacs-base/code#CrossComplianceRuleValue/publicHealthAnimalHealthAndPlantHealthIdentificationAndRegistrationOfAnimalsSmr7 -->


    <owl:NamedIndividual rdf:about="http://lpis.ec.europa.eu/registry/applicationschema/cap-iacs-base/code#CrossComplianceRuleValue/publicHealthAnimalHealthAndPlantHealthIdentificationAndRegistrationOfAnimalsSmr7">
        <rdf:type rdf:resource="http://lpis.ec.europa.eu/registry/applicationschema/cap-iacs-base#CrossComplianceRuleValue"/>
        <rdfs:label xml:lang="en">Public health, animal health and plant health  - Identification and registration of animals SMR7</rdfs:label>
        <skos:definition xml:lang="en">-- Definition --
Public health, animal health and plant health  - Identification and registration of animals SMR7.
-- Description --
Regulation (EC) No 1760/2000 of the European Parliament and of the Council of 17 July 2000 establishing a system for the identification and registration of bovine animals and regarding the labelling of beef and beef products and repealing Council Regulation (EC) No 820/97(OJ L 204, 11.8.2000, p. 1) . Articles 4 and 7.
NOTE. Initial value:SMR7</skos:definition>
        <skos:inScheme rdf:resource="http://lpis.ec.europa.eu/registry/applicationschema/cap-iacs-base/code#CrossComplianceRuleValue"/>
    </owl:NamedIndividual>
    


    <!-- http://lpis.ec.europa.eu/registry/applicationschema/cap-iacs-base/code#CrossComplianceRuleValue/publicHealthAnimalHealthAndPlantHealthIdentificationAndRegistrationOfAnimalsSmr8 -->


    <owl:NamedIndividual rdf:about="http://lpis.ec.europa.eu/registry/applicationschema/cap-iacs-base/code#CrossComplianceRuleValue/publicHealthAnimalHealthAndPlantHealthIdentificationAndRegistrationOfAnimalsSmr8">
        <rdf:type rdf:resource="http://lpis.ec.europa.eu/registry/applicationschema/cap-iacs-base#CrossComplianceRuleValue"/>
        <rdfs:label xml:lang="en">Public health, animal health and plant health  - Identification and registration of animals SMR8</rdfs:label>
        <skos:definition xml:lang="en">-- Definition --
Public health, animal health and plant health  - Identification and registration of animals SMR8.
-- Description --
Council Regulation (EC) No 21/2004 of 17 December 2003 establishing a system for the identification and registration of ovine and caprine animals and amending Regulation (EC) No 1782/2003 and Directives 92/102/EEC and 64/432/EEC (OJ L 5, 9.1.2004, p. 8). Articles 3, 4 and 5.
NOTE. Initial value:SMR8</skos:definition>
        <skos:inScheme rdf:resource="http://lpis.ec.europa.eu/registry/applicationschema/cap-iacs-base/code#CrossComplianceRuleValue"/>
    </owl:NamedIndividual>
    


    <!-- http://lpis.ec.europa.eu/registry/applicationschema/cap-iacs-base/code#CrossComplianceRuleValue/publicHealthAnimalHealthAndPlantHealthPlantProtectionProductsSmr10 -->


    <owl:NamedIndividual rdf:about="http://lpis.ec.europa.eu/registry/applicationschema/cap-iacs-base/code#CrossComplianceRuleValue/publicHealthAnimalHealthAndPlantHealthPlantProtectionProductsSmr10">
        <rdf:type rdf:resource="http://lpis.ec.europa.eu/registry/applicationschema/cap-iacs-base#CrossComplianceRuleValue"/>
        <rdfs:label xml:lang="en">Public health, animal health and plant health  - Plant protection products SMR10</rdfs:label>
        <skos:definition xml:lang="en">-- Definition --
Public health, animal health and plant health  - Plant protection products SMR10
-- Description --
Regulation (EC) No 1107/2009 of the European Parliament and of the Council of 21 October 2009 concerning the placing of plant protection products on the market and repealing Council Directives 79/117/EEC and 91/414/EEC (OJ L 309, 24.11.2009, p. 1). Article 55, first and second sentence.
NOTE. Initial value:SMR10</skos:definition>
        <skos:inScheme rdf:resource="http://lpis.ec.europa.eu/registry/applicationschema/cap-iacs-base/code#CrossComplianceRuleValue"/>
    </owl:NamedIndividual>
    


    <!-- http://lpis.ec.europa.eu/registry/applicationschema/cap-iacs-base/code#FarmStructureSurveyNumberValue/arableLand -->


    <owl:NamedIndividual rdf:about="http://lpis.ec.europa.eu/registry/applicationschema/cap-iacs-base/code#FarmStructureSurveyNumberValue/arableLand">
        <rdf:type rdf:resource="http://lpis.ec.europa.eu/registry/applicationschema/cap-iacs-base#FarmStructureSurveyNumberValue"/>
        <rdfs:label xml:lang="en">Arable land</rdfs:label>
        <skos:definition xml:lang="en">-- Definition --
Arable land.
-- Description --
Land worked (ploughed or tilled) regularly, generally under a system of crop rotation.
Crop rotation is the practice of alternating annual crops grown on a specific field in a planned pattern or sequence in successive crop years so that crops of the same species are not grown without interruption on the same field. Normally the crops are changed annually, but they can also be multiannual. To distinguish arable land from permanent crops or permanent grassland, a threshold of five years is used. This means that if a plot is used for the same crop for five years or more, without in the meantime removing the preceding crop and establishing a new one, it is not considered arable land.
NOTE. Initial value:2.01</skos:definition>
        <skos:inScheme rdf:resource="http://lpis.ec.europa.eu/registry/applicationschema/cap-iacs-base/code#FarmStructureSurveyNumberValue"/>
    </owl:NamedIndividual>
    


    <!-- http://lpis.ec.europa.eu/registry/applicationschema/cap-iacs-base/code#FarmStructureSurveyNumberValue/arableLandSeedAndSeedlings -->


    <owl:NamedIndividual rdf:about="http://lpis.ec.europa.eu/registry/applicationschema/cap-iacs-base/code#FarmStructureSurveyNumberValue/arableLandSeedAndSeedlings">
        <rdf:type rdf:resource="http://lpis.ec.europa.eu/registry/applicationschema/cap-iacs-base#FarmStructureSurveyNumberValue"/>
        <rdfs:label xml:lang="en">Arable land seed and seedlings</rdfs:label>
        <skos:definition xml:lang="en">-- Definition --
Arable land seed and seedlings.
-- Description --
Areas producing seeds and seedlings for sale, excluding cereals, rice, pulses, potatoes and oil seeds.
NOTE. Initial value:2.01.10</skos:definition>
        <skos:inScheme rdf:resource="http://lpis.ec.europa.eu/registry/applicationschema/cap-iacs-base/code#FarmStructureSurveyNumberValue"/>
    </owl:NamedIndividual>
    


    <!-- http://lpis.ec.europa.eu/registry/applicationschema/cap-iacs-base/code#FarmStructureSurveyNumberValue/aromaticPlantsMedicinalAndCulinaryPlants -->


    <owl:NamedIndividual rdf:about="http://lpis.ec.europa.eu/registry/applicationschema/cap-iacs-base/code#FarmStructureSurveyNumberValue/aromaticPlantsMedicinalAndCulinaryPlants">
        <rdf:type rdf:resource="http://lpis.ec.europa.eu/registry/applicationschema/cap-iacs-base#FarmStructureSurveyNumberValue"/>
        <rdfs:label xml:lang="en">Aromatic plants, medicinal and culinary plants</rdfs:label>
        <skos:definition xml:lang="en">-- Definition --
Aromatic plants, medicinal and culinary plants.
-- Description --
Plants or parts of plants for pharmaceutical purposes, perfume manufacture or human consumption.
Culinary plants are distinguished from vegetables in that they are used in small amounts and provide flavour rather than substance to food.
NOTE. Initial value:2.01.06.12</skos:definition>
        <skos:inScheme rdf:resource="http://lpis.ec.europa.eu/registry/applicationschema/cap-iacs-base/code#FarmStructureSurveyNumberValue"/>
    </owl:NamedIndividual>
    


    <!-- http://lpis.ec.europa.eu/registry/applicationschema/cap-iacs-base/code#FarmStructureSurveyNumberValue/barley -->


    <owl:NamedIndividual rdf:about="http://lpis.ec.europa.eu/registry/applicationschema/cap-iacs-base/code#FarmStructureSurveyNumberValue/barley">
        <rdf:type rdf:resource="http://lpis.ec.europa.eu/registry/applicationschema/cap-iacs-base#FarmStructureSurveyNumberValue"/>
        <rdfs:label xml:lang="en">Barley</rdfs:label>
        <skos:definition xml:lang="en">-- Definition --
Barley.
-- Description --
Hordeum vulgare L.
NOTE. Initial value:2.01.01.04</skos:definition>
        <skos:inScheme rdf:resource="http://lpis.ec.europa.eu/registry/applicationschema/cap-iacs-base/code#FarmStructureSurveyNumberValue"/>
    </owl:NamedIndividual>
    


    <!-- http://lpis.ec.europa.eu/registry/applicationschema/cap-iacs-base/code#FarmStructureSurveyNumberValue/berrySpecies -->


    <owl:NamedIndividual rdf:about="http://lpis.ec.europa.eu/registry/applicationschema/cap-iacs-base/code#FarmStructureSurveyNumberValue/berrySpecies">
        <rdf:type rdf:resource="http://lpis.ec.europa.eu/registry/applicationschema/cap-iacs-base#FarmStructureSurveyNumberValue"/>
        <rdfs:label xml:lang="en">Berry species</rdfs:label>
        <skos:definition xml:lang="en">-- Definition --
Berry species.
-- Description --
Berry plantations which are traditionally cropped both in temperate and subtropical climates for producing berries.
NOTE. Initial value:2.04.01.02</skos:definition>
        <skos:inScheme rdf:resource="http://lpis.ec.europa.eu/registry/applicationschema/cap-iacs-base/code#FarmStructureSurveyNumberValue"/>
    </owl:NamedIndividual>
    


    <!-- http://lpis.ec.europa.eu/registry/applicationschema/cap-iacs-base/code#FarmStructureSurveyNumberValue/cerealsForTheProductionOfGrainIncludingSeed -->


    <owl:NamedIndividual rdf:about="http://lpis.ec.europa.eu/registry/applicationschema/cap-iacs-base/code#FarmStructureSurveyNumberValue/cerealsForTheProductionOfGrainIncludingSeed">
        <rdf:type rdf:resource="http://lpis.ec.europa.eu/registry/applicationschema/cap-iacs-base#FarmStructureSurveyNumberValue"/>
        <rdfs:label xml:lang="en">Cereals for the production of grain (including seed)</rdfs:label>
        <skos:definition xml:lang="en">-- Definition --
Cereals for the production of grain (including seed).
-- Description --
All areas of cereals harvested dry for grain, regardless of use, shall be recorded here (including cereals used for renewable energy production).
NOTE. Initial value:2.01.01</skos:definition>
        <skos:inScheme rdf:resource="http://lpis.ec.europa.eu/registry/applicationschema/cap-iacs-base/code#FarmStructureSurveyNumberValue"/>
    </owl:NamedIndividual>
    


    <!-- http://lpis.ec.europa.eu/registry/applicationschema/cap-iacs-base/code#FarmStructureSurveyNumberValue/citrusPlantations -->


    <owl:NamedIndividual rdf:about="http://lpis.ec.europa.eu/registry/applicationschema/cap-iacs-base/code#FarmStructureSurveyNumberValue/citrusPlantations">
        <rdf:type rdf:resource="http://lpis.ec.europa.eu/registry/applicationschema/cap-iacs-base#FarmStructureSurveyNumberValue"/>
        <rdfs:label xml:lang="en">Citrus plantations</rdfs:label>
        <skos:definition xml:lang="en">-- Definition --
Citrus plantations.
-- Description --
Plantations of Citrus spp.
NOTE. Initial value:2.04.02</skos:definition>
        <skos:inScheme rdf:resource="http://lpis.ec.europa.eu/registry/applicationschema/cap-iacs-base/code#FarmStructureSurveyNumberValue"/>
    </owl:NamedIndividual>
    


    <!-- http://lpis.ec.europa.eu/registry/applicationschema/cap-iacs-base/code#FarmStructureSurveyNumberValue/commonWheatAndSpelt -->


    <owl:NamedIndividual rdf:about="http://lpis.ec.europa.eu/registry/applicationschema/cap-iacs-base/code#FarmStructureSurveyNumberValue/commonWheatAndSpelt">
        <rdf:type rdf:resource="http://lpis.ec.europa.eu/registry/applicationschema/cap-iacs-base#FarmStructureSurveyNumberValue"/>
        <rdfs:label xml:lang="en">Common wheat and spelt</rdfs:label>
        <skos:definition xml:lang="en">-- Definition --
Common wheat and spelt.
-- Description --
Triticum aestivum L. emend. Fiori et Paol., Triticum spelta L. and Triticum monococcum L.
NOTE. Initial value:2.01.01.01</skos:definition>
        <skos:inScheme rdf:resource="http://lpis.ec.europa.eu/registry/applicationschema/cap-iacs-base/code#FarmStructureSurveyNumberValue"/>
    </owl:NamedIndividual>
    


    <!-- http://lpis.ec.europa.eu/registry/applicationschema/cap-iacs-base/code#FarmStructureSurveyNumberValue/cotton -->


    <owl:NamedIndividual rdf:about="http://lpis.ec.europa.eu/registry/applicationschema/cap-iacs-base/code#FarmStructureSurveyNumberValue/cotton">
        <rdf:type rdf:resource="http://lpis.ec.europa.eu/registry/applicationschema/cap-iacs-base#FarmStructureSurveyNumberValue"/>
        <rdfs:label xml:lang="en">Cotton</rdfs:label>
        <skos:definition xml:lang="en">-- Definition --
Cotton.
-- Description --
Gossypium spp., harvested for fibre as well as for oil-seeds.
NOTE. Initial value:2.01.06.03</skos:definition>
        <skos:inScheme rdf:resource="http://lpis.ec.europa.eu/registry/applicationschema/cap-iacs-base/code#FarmStructureSurveyNumberValue"/>
    </owl:NamedIndividual>
    


    <!-- http://lpis.ec.europa.eu/registry/applicationschema/cap-iacs-base/code#FarmStructureSurveyNumberValue/driedPulsesAndProteinCropsForTheProductionOfGrain -->


    <owl:NamedIndividual rdf:about="http://lpis.ec.europa.eu/registry/applicationschema/cap-iacs-base/code#FarmStructureSurveyNumberValue/driedPulsesAndProteinCropsForTheProductionOfGrain">
        <rdf:type rdf:resource="http://lpis.ec.europa.eu/registry/applicationschema/cap-iacs-base#FarmStructureSurveyNumberValue"/>
        <rdfs:label xml:lang="en">Dried pulses and protein crops for the production of grain</rdfs:label>
        <skos:definition xml:lang="en">-- Definition --
Dried pulses and protein crops for the production of grain.
-- Description --
Dried pulses and protein crops for the production of grain (including seed and mixtures of cereals and pulses)
Crops sown and harvested mainly for their protein content.
All areas of dried pulses and protein crops harvested dry for grain, regardless of use, shall be recorded here (including crops used for renewable energy production).
NOTE. Initial value:2.01.02</skos:definition>
        <skos:inScheme rdf:resource="http://lpis.ec.europa.eu/registry/applicationschema/cap-iacs-base/code#FarmStructureSurveyNumberValue"/>
    </owl:NamedIndividual>
    


    <!-- http://lpis.ec.europa.eu/registry/applicationschema/cap-iacs-base/code#FarmStructureSurveyNumberValue/durumWheat -->


    <owl:NamedIndividual rdf:about="http://lpis.ec.europa.eu/registry/applicationschema/cap-iacs-base/code#FarmStructureSurveyNumberValue/durumWheat">
        <rdf:type rdf:resource="http://lpis.ec.europa.eu/registry/applicationschema/cap-iacs-base#FarmStructureSurveyNumberValue"/>
        <rdfs:label xml:lang="en">Durum wheat</rdfs:label>
        <skos:definition xml:lang="en">-- Definition --
Durum wheat.
-- Description --
Triticum durum Desf.
NOTE. Initial value:2.01.01.02</skos:definition>
        <skos:inScheme rdf:resource="http://lpis.ec.europa.eu/registry/applicationschema/cap-iacs-base/code#FarmStructureSurveyNumberValue"/>
    </owl:NamedIndividual>
    


    <!-- http://lpis.ec.europa.eu/registry/applicationschema/cap-iacs-base/code#FarmStructureSurveyNumberValue/energyCropsForTheProductionOfBiofuelsOrOtherRenewableEnergy -->


    <owl:NamedIndividual rdf:about="http://lpis.ec.europa.eu/registry/applicationschema/cap-iacs-base/code#FarmStructureSurveyNumberValue/energyCropsForTheProductionOfBiofuelsOrOtherRenewableEnergy">
        <rdf:type rdf:resource="http://lpis.ec.europa.eu/registry/applicationschema/cap-iacs-base#FarmStructureSurveyNumberValue"/>
        <rdfs:label xml:lang="en">Energy crops (for the production of biofuels or other renewable energy)</rdfs:label>
        <skos:definition xml:lang="en">-- Definition --
Energy crops (for the production of biofuels or other renewable energy).
-- Description --
The production area of energy crops benefiting from the following support schemes under Regulation (EC) No 1782/2003: the specific aid for energy crops (Article 88), the payment linked to set-aside entitlement when production takes place on set-aside area (Article 55 or 56).
Other areas used for the production of energy crops (notably benefiting of the payment linked to‘normal’ entitlement under the Single Payment Scheme or the Simplified Area Payment Scheme) are not covered.
NOTE. Initial value:2.06.03</skos:definition>
        <skos:inScheme rdf:resource="http://lpis.ec.europa.eu/registry/applicationschema/cap-iacs-base/code#FarmStructureSurveyNumberValue"/>
    </owl:NamedIndividual>
    


    <!-- http://lpis.ec.europa.eu/registry/applicationschema/cap-iacs-base/code#FarmStructureSurveyNumberValue/fallowLand -->


    <owl:NamedIndividual rdf:about="http://lpis.ec.europa.eu/registry/applicationschema/cap-iacs-base/code#FarmStructureSurveyNumberValue/fallowLand">
        <rdf:type rdf:resource="http://lpis.ec.europa.eu/registry/applicationschema/cap-iacs-base#FarmStructureSurveyNumberValue"/>
        <rdfs:label xml:lang="en">Fallow land</rdfs:label>
        <skos:definition xml:lang="en">-- Definition --
Fallow land.
-- Description --
All arable land included in the crop rotation system, whether worked or not, but with no intention to produce a harvest for the duration of a crop year.
The essential characteristic of fallow land is that it is left to recover, normally for the whole of a crop year.
Fallow land may be:
1. bare land bearing no crops at all;
2. land with spontaneous natural growth, which may be used as feed or ploughed in;
3. land sown exclusively for the production of green manure (green fallow).
All areas of arable land maintained in good agricultural and environmental conditions as set out in Article 5 of the Council Regulation (EC) No 1782/2003(1)
OJ L 270, 21.10.2003, p. 1. (1) or, where applicable, in the most recent legislation, regardless of whether they are part of the crop rotation or not, are included.
NOTE. Initial value:2.01.12</skos:definition>
        <skos:inScheme rdf:resource="http://lpis.ec.europa.eu/registry/applicationschema/cap-iacs-base/code#FarmStructureSurveyNumberValue"/>
    </owl:NamedIndividual>
    


    <!-- http://lpis.ec.europa.eu/registry/applicationschema/cap-iacs-base/code#FarmStructureSurveyNumberValue/fallowLandSubjectToThePaymentOfSubsidiesWithNoEconomicUse -->


    <owl:NamedIndividual rdf:about="http://lpis.ec.europa.eu/registry/applicationschema/cap-iacs-base/code#FarmStructureSurveyNumberValue/fallowLandSubjectToThePaymentOfSubsidiesWithNoEconomicUse">
        <rdf:type rdf:resource="http://lpis.ec.europa.eu/registry/applicationschema/cap-iacs-base#FarmStructureSurveyNumberValue"/>
        <rdfs:label xml:lang="en">Fallow land subject to the payment of subsidies, with no economic use</rdfs:label>
        <skos:definition xml:lang="en">-- Definition --
Fallow land subject to the payment of subsidies, with no economic use.
-- Description --
Fallow land for which the holding is entitled to financial aid.
NOTE. Initial value:2.01.12.02</skos:definition>
        <skos:inScheme rdf:resource="http://lpis.ec.europa.eu/registry/applicationschema/cap-iacs-base/code#FarmStructureSurveyNumberValue"/>
    </owl:NamedIndividual>
    


    <!-- http://lpis.ec.europa.eu/registry/applicationschema/cap-iacs-base/code#FarmStructureSurveyNumberValue/flax -->


    <owl:NamedIndividual rdf:about="http://lpis.ec.europa.eu/registry/applicationschema/cap-iacs-base/code#FarmStructureSurveyNumberValue/flax">
        <rdf:type rdf:resource="http://lpis.ec.europa.eu/registry/applicationschema/cap-iacs-base#FarmStructureSurveyNumberValue"/>
        <rdfs:label xml:lang="en">Flax</rdfs:label>
        <skos:definition xml:lang="en">-- Definition --
Flax.
-- Description --
Linum usitatissimum L., varieties grown mainly for producing fibre.
NOTE. Initial value:2.01.06.09</skos:definition>
        <skos:inScheme rdf:resource="http://lpis.ec.europa.eu/registry/applicationschema/cap-iacs-base/code#FarmStructureSurveyNumberValue"/>
    </owl:NamedIndividual>
    


    <!-- http://lpis.ec.europa.eu/registry/applicationschema/cap-iacs-base/code#FarmStructureSurveyNumberValue/flowersAndOrnamentalPlantsExcludingNurseries -->


    <owl:NamedIndividual rdf:about="http://lpis.ec.europa.eu/registry/applicationschema/cap-iacs-base/code#FarmStructureSurveyNumberValue/flowersAndOrnamentalPlantsExcludingNurseries">
        <rdf:type rdf:resource="http://lpis.ec.europa.eu/registry/applicationschema/cap-iacs-base#FarmStructureSurveyNumberValue"/>
        <rdfs:label xml:lang="en">Flowers and ornamental plants (excluding nurseries)</rdfs:label>
        <skos:definition xml:lang="en">-- Definition --
Flowers and ornamental plants (excluding nurseries).
-- Description --
Flowers and ornamental plants (excluding nurseries).
NOTE. Initial value:2.01.08</skos:definition>
        <skos:inScheme rdf:resource="http://lpis.ec.europa.eu/registry/applicationschema/cap-iacs-base/code#FarmStructureSurveyNumberValue"/>
    </owl:NamedIndividual>
    


    <!-- http://lpis.ec.europa.eu/registry/applicationschema/cap-iacs-base/code#FarmStructureSurveyNumberValue/fodderRootsAndBrassicasExcludingSeed -->


    <owl:NamedIndividual rdf:about="http://lpis.ec.europa.eu/registry/applicationschema/cap-iacs-base/code#FarmStructureSurveyNumberValue/fodderRootsAndBrassicasExcludingSeed">
        <rdf:type rdf:resource="http://lpis.ec.europa.eu/registry/applicationschema/cap-iacs-base#FarmStructureSurveyNumberValue"/>
        <rdfs:label xml:lang="en">Fodder roots and brassicas (excluding seed)</rdfs:label>
        <skos:definition xml:lang="en">-- Definition --
Fodder roots and brassicas (excluding seed)
-- Description --
Fodder beet (Beta vulgaris L.) and plants of the Brassicae family harvested mainly for animal feed, regardless whether it is the root or the stem, and other plants cultivated mainly for their roots for fodder, not mentioned elsewhere.
NOTE. Initial value:2.01.05</skos:definition>
        <skos:inScheme rdf:resource="http://lpis.ec.europa.eu/registry/applicationschema/cap-iacs-base/code#FarmStructureSurveyNumberValue"/>
    </owl:NamedIndividual>
    


    <!-- http://lpis.ec.europa.eu/registry/applicationschema/cap-iacs-base/code#FarmStructureSurveyNumberValue/freshVegetablesMelonsAndStrawberriesOfWhich -->


    <owl:NamedIndividual rdf:about="http://lpis.ec.europa.eu/registry/applicationschema/cap-iacs-base/code#FarmStructureSurveyNumberValue/freshVegetablesMelonsAndStrawberriesOfWhich">
        <rdf:type rdf:resource="http://lpis.ec.europa.eu/registry/applicationschema/cap-iacs-base#FarmStructureSurveyNumberValue"/>
        <rdfs:label xml:lang="en">Fresh vegetables, melons and strawberries of which:</rdfs:label>
        <skos:definition xml:lang="en">-- Definition --
Fresh vegetables, melons and strawberries of which:
-- Description --
Fresh vegetables, melons and strawberries of which:
NOTE. Initial value:2.01.07</skos:definition>
        <skos:inScheme rdf:resource="http://lpis.ec.europa.eu/registry/applicationschema/cap-iacs-base/code#FarmStructureSurveyNumberValue"/>
    </owl:NamedIndividual>
    


    <!-- http://lpis.ec.europa.eu/registry/applicationschema/cap-iacs-base/code#FarmStructureSurveyNumberValue/fruitAndBerryPlantations -->


    <owl:NamedIndividual rdf:about="http://lpis.ec.europa.eu/registry/applicationschema/cap-iacs-base/code#FarmStructureSurveyNumberValue/fruitAndBerryPlantations">
        <rdf:type rdf:resource="http://lpis.ec.europa.eu/registry/applicationschema/cap-iacs-base#FarmStructureSurveyNumberValue"/>
        <rdfs:label xml:lang="en">Fruit and berry plantations</rdfs:label>
        <skos:definition xml:lang="en">-- Definition --
Fruit and berry plantations.
-- Description --
Areas containing trees, bushes and perennial berry plants other than strawberries for the production of fruit. Orchards may be of the continuous type with minimum spacing between trees or of the non-continuous type with wide spacing.
NOTE. Initial value:2.04.01</skos:definition>
        <skos:inScheme rdf:resource="http://lpis.ec.europa.eu/registry/applicationschema/cap-iacs-base/code#FarmStructureSurveyNumberValue"/>
    </owl:NamedIndividual>
    


    <!-- http://lpis.ec.europa.eu/registry/applicationschema/cap-iacs-base/code#FarmStructureSurveyNumberValue/fruitSpeciesOfWhich -->


    <owl:NamedIndividual rdf:about="http://lpis.ec.europa.eu/registry/applicationschema/cap-iacs-base/code#FarmStructureSurveyNumberValue/fruitSpeciesOfWhich">
        <rdf:type rdf:resource="http://lpis.ec.europa.eu/registry/applicationschema/cap-iacs-base#FarmStructureSurveyNumberValue"/>
        <rdfs:label xml:lang="en">Fruit species, of which:</rdfs:label>
        <skos:definition xml:lang="en">-- Definition --
Fruit species, of which:
-- Description --
Fruit species, of which:
NOTE. Initial value:2.04.01.01</skos:definition>
        <skos:inScheme rdf:resource="http://lpis.ec.europa.eu/registry/applicationschema/cap-iacs-base/code#FarmStructureSurveyNumberValue"/>
    </owl:NamedIndividual>
    


    <!-- http://lpis.ec.europa.eu/registry/applicationschema/cap-iacs-base/code#FarmStructureSurveyNumberValue/fruitSpeciesOfWhichFruitOfSubtropicalClimateZones -->


    <owl:NamedIndividual rdf:about="http://lpis.ec.europa.eu/registry/applicationschema/cap-iacs-base/code#FarmStructureSurveyNumberValue/fruitSpeciesOfWhichFruitOfSubtropicalClimateZones">
        <rdf:type rdf:resource="http://lpis.ec.europa.eu/registry/applicationschema/cap-iacs-base#FarmStructureSurveyNumberValue"/>
        <rdfs:label xml:lang="en">Fruit species, of which: Fruit of subtropical climate zones</rdfs:label>
        <skos:definition xml:lang="en">-- Definition --
Fruit species, of which: Fruit of subtropical climate zones.
-- Description --
Fruit tree plantations which are traditionally cropped in subtropical climates for producing fruits.
NOTE. Initial value:2.04.01.01.02</skos:definition>
        <skos:inScheme rdf:resource="http://lpis.ec.europa.eu/registry/applicationschema/cap-iacs-base/code#FarmStructureSurveyNumberValue"/>
    </owl:NamedIndividual>
    


    <!-- http://lpis.ec.europa.eu/registry/applicationschema/cap-iacs-base/code#FarmStructureSurveyNumberValue/fruitSpeciesOfWhichFruitOfTemperateClimateZones -->


    <owl:NamedIndividual rdf:about="http://lpis.ec.europa.eu/registry/applicationschema/cap-iacs-base/code#FarmStructureSurveyNumberValue/fruitSpeciesOfWhichFruitOfTemperateClimateZones">
        <rdf:type rdf:resource="http://lpis.ec.europa.eu/registry/applicationschema/cap-iacs-base#FarmStructureSurveyNumberValue"/>
        <rdfs:label xml:lang="en">Fruit species, of which: Fruit of temperate climate zones</rdfs:label>
        <skos:definition xml:lang="en">-- Definition --
Fruit species, of which: Fruit of temperate climate zones.
-- Description --
Fruit tree plantations which are traditionally cropped in temperate climates for producing fruits.
NOTE. Initial value:2.04.01.01.01</skos:definition>
        <skos:inScheme rdf:resource="http://lpis.ec.europa.eu/registry/applicationschema/cap-iacs-base/code#FarmStructureSurveyNumberValue"/>
    </owl:NamedIndividual>
    


    <!-- http://lpis.ec.europa.eu/registry/applicationschema/cap-iacs-base/code#FarmStructureSurveyNumberValue/geneticallyModifiedCrops -->


    <owl:NamedIndividual rdf:about="http://lpis.ec.europa.eu/registry/applicationschema/cap-iacs-base/code#FarmStructureSurveyNumberValue/geneticallyModifiedCrops">
        <rdf:type rdf:resource="http://lpis.ec.europa.eu/registry/applicationschema/cap-iacs-base#FarmStructureSurveyNumberValue"/>
        <rdfs:label xml:lang="en">Genetically modified crops</rdfs:label>
        <skos:definition xml:lang="en">-- Definition --
Genetically modified crops.
-- Description --
‘Genetically modified crops (GMC)’ mean any organism as defined in Article 2 of Council Directive 2001/18/EC(1) OJ L 106, 17.4.2001, p. 1. (1) or, where applicable, the most recent legislation.
NOTE. Initial value:2.06.04</skos:definition>
        <skos:inScheme rdf:resource="http://lpis.ec.europa.eu/registry/applicationschema/cap-iacs-base/code#FarmStructureSurveyNumberValue"/>
    </owl:NamedIndividual>
    


    <!-- http://lpis.ec.europa.eu/registry/applicationschema/cap-iacs-base/code#FarmStructureSurveyNumberValue/grainMaize -->


    <owl:NamedIndividual rdf:about="http://lpis.ec.europa.eu/registry/applicationschema/cap-iacs-base/code#FarmStructureSurveyNumberValue/grainMaize">
        <rdf:type rdf:resource="http://lpis.ec.europa.eu/registry/applicationschema/cap-iacs-base#FarmStructureSurveyNumberValue"/>
        <rdfs:label xml:lang="en">Grain maize</rdfs:label>
        <skos:definition xml:lang="en">-- Definition --
Grain maize.
-- Description --
Maize (Zea mays L.) harvested for grain.
NOTE. Initial value:2.01.01.06</skos:definition>
        <skos:inScheme rdf:resource="http://lpis.ec.europa.eu/registry/applicationschema/cap-iacs-base/code#FarmStructureSurveyNumberValue"/>
    </owl:NamedIndividual>
    


    <!-- http://lpis.ec.europa.eu/registry/applicationschema/cap-iacs-base/code#FarmStructureSurveyNumberValue/greenMaize -->


    <owl:NamedIndividual rdf:about="http://lpis.ec.europa.eu/registry/applicationschema/cap-iacs-base/code#FarmStructureSurveyNumberValue/greenMaize">
        <rdf:type rdf:resource="http://lpis.ec.europa.eu/registry/applicationschema/cap-iacs-base#FarmStructureSurveyNumberValue"/>
        <rdfs:label xml:lang="en">Green maize</rdfs:label>
        <skos:definition xml:lang="en">-- Definition --
Green maize.
-- Description --
All forms of maize (Zea mays L.) grown mainly for silage, which is not harvested for grain (whole cob, parts of or whole plant).
This includes green maize directly consumed by animals (without silage) and whole cobs (grain, rachis, husk) harvested for feedstuff or silage as well as for renewable energy production.
NOTE. Initial value:2.01.09.02.01</skos:definition>
        <skos:inScheme rdf:resource="http://lpis.ec.europa.eu/registry/applicationschema/cap-iacs-base/code#FarmStructureSurveyNumberValue"/>
    </owl:NamedIndividual>
    


    <!-- http://lpis.ec.europa.eu/registry/applicationschema/cap-iacs-base/code#FarmStructureSurveyNumberValue/hemp -->


    <owl:NamedIndividual rdf:about="http://lpis.ec.europa.eu/registry/applicationschema/cap-iacs-base/code#FarmStructureSurveyNumberValue/hemp">
        <rdf:type rdf:resource="http://lpis.ec.europa.eu/registry/applicationschema/cap-iacs-base#FarmStructureSurveyNumberValue"/>
        <rdfs:label xml:lang="en">Hemp</rdfs:label>
        <skos:definition xml:lang="en">-- Definition --
Hemp.
-- Description --
Cannabis sativa L.
NOTE. Initial value:2.01.06.10</skos:definition>
        <skos:inScheme rdf:resource="http://lpis.ec.europa.eu/registry/applicationschema/cap-iacs-base/code#FarmStructureSurveyNumberValue"/>
    </owl:NamedIndividual>
    


    <!-- http://lpis.ec.europa.eu/registry/applicationschema/cap-iacs-base/code#FarmStructureSurveyNumberValue/hops -->


    <owl:NamedIndividual rdf:about="http://lpis.ec.europa.eu/registry/applicationschema/cap-iacs-base/code#FarmStructureSurveyNumberValue/hops">
        <rdf:type rdf:resource="http://lpis.ec.europa.eu/registry/applicationschema/cap-iacs-base#FarmStructureSurveyNumberValue"/>
        <rdfs:label xml:lang="en">Hops</rdfs:label>
        <skos:definition xml:lang="en">-- Definition --
Hops.
-- Description --
Humulus lupulus L.
NOTE. Initial value:2.01.06.02</skos:definition>
        <skos:inScheme rdf:resource="http://lpis.ec.europa.eu/registry/applicationschema/cap-iacs-base/code#FarmStructureSurveyNumberValue"/>
    </owl:NamedIndividual>
    


    <!-- http://lpis.ec.europa.eu/registry/applicationschema/cap-iacs-base/code#FarmStructureSurveyNumberValue/industrialCrops -->


    <owl:NamedIndividual rdf:about="http://lpis.ec.europa.eu/registry/applicationschema/cap-iacs-base/code#FarmStructureSurveyNumberValue/industrialCrops">
        <rdf:type rdf:resource="http://lpis.ec.europa.eu/registry/applicationschema/cap-iacs-base#FarmStructureSurveyNumberValue"/>
        <rdfs:label xml:lang="en">Industrial crops</rdfs:label>
        <skos:definition xml:lang="en">-- Definition --
Industrial crops.
-- Description --
Crops that are normally not sold directly for consumption because they need to be industrially processed prior to final use.
All harvested areas of industrial crops, regardless of use, shall be recorded here (including crops used for renewable energy production).
NOTE. Initial value:2.01.06</skos:definition>
        <skos:inScheme rdf:resource="http://lpis.ec.europa.eu/registry/applicationschema/cap-iacs-base/code#FarmStructureSurveyNumberValue"/>
    </owl:NamedIndividual>
    


    <!-- http://lpis.ec.europa.eu/registry/applicationschema/cap-iacs-base/code#FarmStructureSurveyNumberValue/irrigatedArea -->


    <owl:NamedIndividual rdf:about="http://lpis.ec.europa.eu/registry/applicationschema/cap-iacs-base/code#FarmStructureSurveyNumberValue/irrigatedArea">
        <rdf:type rdf:resource="http://lpis.ec.europa.eu/registry/applicationschema/cap-iacs-base#FarmStructureSurveyNumberValue"/>
        <rdfs:label xml:lang="en">Irrigated area</rdfs:label>
        <skos:definition xml:lang="en">-- Definition --
Irrigated area.
-- Description --
Irrigated area.
NOTE. Initial value:2.06.02</skos:definition>
        <skos:inScheme rdf:resource="http://lpis.ec.europa.eu/registry/applicationschema/cap-iacs-base/code#FarmStructureSurveyNumberValue"/>
    </owl:NamedIndividual>
    


    <!-- http://lpis.ec.europa.eu/registry/applicationschema/cap-iacs-base/code#FarmStructureSurveyNumberValue/kitchenGardens -->


    <owl:NamedIndividual rdf:about="http://lpis.ec.europa.eu/registry/applicationschema/cap-iacs-base/code#FarmStructureSurveyNumberValue/kitchenGardens">
        <rdf:type rdf:resource="http://lpis.ec.europa.eu/registry/applicationschema/cap-iacs-base#FarmStructureSurveyNumberValue"/>
        <rdfs:label xml:lang="en">Kitchen gardens</rdfs:label>
        <skos:definition xml:lang="en">-- Definition --
Kitchen gardens.
-- Description --
Areas devoted to the cultivation of agricultural products intended for self-consumption by the holder and his household, normally separated off from the rest of the agricultural land, and recognisable as kitchen gardens.
Only occasional surplus products coming from this area are sold off from the holding. All areas from which products are consistently sold on the market belong under other items, even if part of the production is consumed by the holder and his household.
NOTE. Initial value:2.02</skos:definition>
        <skos:inScheme rdf:resource="http://lpis.ec.europa.eu/registry/applicationschema/cap-iacs-base/code#FarmStructureSurveyNumberValue"/>
    </owl:NamedIndividual>
    


    <!-- http://lpis.ec.europa.eu/registry/applicationschema/cap-iacs-base/code#FarmStructureSurveyNumberValue/lallowLandWithoutAnySubsidies -->


    <owl:NamedIndividual rdf:about="http://lpis.ec.europa.eu/registry/applicationschema/cap-iacs-base/code#FarmStructureSurveyNumberValue/lallowLandWithoutAnySubsidies">
        <rdf:type rdf:resource="http://lpis.ec.europa.eu/registry/applicationschema/cap-iacs-base#FarmStructureSurveyNumberValue"/>
        <rdfs:label xml:lang="en">Fallow land without any subsidies</rdfs:label>
        <skos:definition xml:lang="en">-- Definition --
Fallow land without any subsidies.
-- Description --
Fallow land for which no financial aid or subsidy is paid.
NOTE. Initial value:2.01.12.01</skos:definition>
        <skos:inScheme rdf:resource="http://lpis.ec.europa.eu/registry/applicationschema/cap-iacs-base/code#FarmStructureSurveyNumberValue"/>
    </owl:NamedIndividual>
    


    <!-- http://lpis.ec.europa.eu/registry/applicationschema/cap-iacs-base/code#FarmStructureSurveyNumberValue/leguminousPlants -->


    <owl:NamedIndividual rdf:about="http://lpis.ec.europa.eu/registry/applicationschema/cap-iacs-base/code#FarmStructureSurveyNumberValue/leguminousPlants">
        <rdf:type rdf:resource="http://lpis.ec.europa.eu/registry/applicationschema/cap-iacs-base#FarmStructureSurveyNumberValue"/>
        <rdfs:label xml:lang="en">Leguminous plants</rdfs:label>
        <skos:definition xml:lang="en">-- Definition --
Leguminous plants.
-- Description --
Leguminous plants grown and harvested green as the whole plant mainly for forage.
Mixtures of predominantly leguminous (normally &gt; 80 %) forage crops and grass plants, harvested green or as dried hay are included here.
NOTE. Initial value:2.01.09.02.02</skos:definition>
        <skos:inScheme rdf:resource="http://lpis.ec.europa.eu/registry/applicationschema/cap-iacs-base/code#FarmStructureSurveyNumberValue"/>
    </owl:NamedIndividual>
    


    <!-- http://lpis.ec.europa.eu/registry/applicationschema/cap-iacs-base/code#FarmStructureSurveyNumberValue/linseedOilFlax -->


    <owl:NamedIndividual rdf:about="http://lpis.ec.europa.eu/registry/applicationschema/cap-iacs-base/code#FarmStructureSurveyNumberValue/linseedOilFlax">
        <rdf:type rdf:resource="http://lpis.ec.europa.eu/registry/applicationschema/cap-iacs-base#FarmStructureSurveyNumberValue"/>
        <rdfs:label xml:lang="en">Linseed (oil flax)</rdfs:label>
        <skos:definition xml:lang="en">-- Definition --
Linseed (oil flax).
-- Description --
Linum usitatissimum L., varieties grown mainly for producing oil, harvested as dry grains.
NOTE. Initial value:2.01.06.07</skos:definition>
        <skos:inScheme rdf:resource="http://lpis.ec.europa.eu/registry/applicationschema/cap-iacs-base/code#FarmStructureSurveyNumberValue"/>
    </owl:NamedIndividual>
    


    <!-- http://lpis.ec.europa.eu/registry/applicationschema/cap-iacs-base/code#FarmStructureSurveyNumberValue/marketGardening -->


    <owl:NamedIndividual rdf:about="http://lpis.ec.europa.eu/registry/applicationschema/cap-iacs-base/code#FarmStructureSurveyNumberValue/marketGardening">
        <rdf:type rdf:resource="http://lpis.ec.europa.eu/registry/applicationschema/cap-iacs-base#FarmStructureSurveyNumberValue"/>
        <rdfs:label xml:lang="en">Market gardening</rdfs:label>
        <skos:definition xml:lang="en">-- Definition --
Market gardening.
-- Description --
Fresh vegetables, melons and strawberries grown on arable land in rotation with other horticultural crops.
NOTE. Initial value:2.01.07.01.02</skos:definition>
        <skos:inScheme rdf:resource="http://lpis.ec.europa.eu/registry/applicationschema/cap-iacs-base/code#FarmStructureSurveyNumberValue"/>
    </owl:NamedIndividual>
    


    <!-- http://lpis.ec.europa.eu/registry/applicationschema/cap-iacs-base/code#FarmStructureSurveyNumberValue/mushrooms -->


    <owl:NamedIndividual rdf:about="http://lpis.ec.europa.eu/registry/applicationschema/cap-iacs-base/code#FarmStructureSurveyNumberValue/mushrooms">
        <rdf:type rdf:resource="http://lpis.ec.europa.eu/registry/applicationschema/cap-iacs-base#FarmStructureSurveyNumberValue"/>
        <rdfs:label xml:lang="en">Mushrooms</rdfs:label>
        <skos:definition xml:lang="en">-- Definition --
Mushrooms.
-- Description --
Cultivated mushrooms grown in buildings which have been specially erected or adapted for growing mushrooms, as well as in underground premises, caves and cellars.
NOTE. Initial value:2.06.01</skos:definition>
        <skos:inScheme rdf:resource="http://lpis.ec.europa.eu/registry/applicationschema/cap-iacs-base/code#FarmStructureSurveyNumberValue"/>
    </owl:NamedIndividual>
    


    <!-- http://lpis.ec.europa.eu/registry/applicationschema/cap-iacs-base/code#FarmStructureSurveyNumberValue/mushroomsIrrigatedAreaEnergyCropsAndGeneticallyModifiedCrops -->


    <owl:NamedIndividual rdf:about="http://lpis.ec.europa.eu/registry/applicationschema/cap-iacs-base/code#FarmStructureSurveyNumberValue/mushroomsIrrigatedAreaEnergyCropsAndGeneticallyModifiedCrops">
        <rdf:type rdf:resource="http://lpis.ec.europa.eu/registry/applicationschema/cap-iacs-base#FarmStructureSurveyNumberValue"/>
        <rdfs:label xml:lang="en">Mushrooms, irrigated area, energy crops and genetically modified crops</rdfs:label>
        <skos:definition xml:lang="en">-- Definition --
Mushrooms, irrigated area, energy crops and genetically modified crops.
-- Description --
Mushrooms, irrigated area, energy crops and genetically modified crops.
NOTE. Initial value:2.06</skos:definition>
        <skos:inScheme rdf:resource="http://lpis.ec.europa.eu/registry/applicationschema/cap-iacs-base/code#FarmStructureSurveyNumberValue"/>
    </owl:NamedIndividual>
    


    <!-- http://lpis.ec.europa.eu/registry/applicationschema/cap-iacs-base/code#FarmStructureSurveyNumberValue/normallyProducingOlivesForOilProduction -->


    <owl:NamedIndividual rdf:about="http://lpis.ec.europa.eu/registry/applicationschema/cap-iacs-base/code#FarmStructureSurveyNumberValue/normallyProducingOlivesForOilProduction">
        <rdf:type rdf:resource="http://lpis.ec.europa.eu/registry/applicationschema/cap-iacs-base#FarmStructureSurveyNumberValue"/>
        <rdfs:label xml:lang="en">Normally producing olives for oil production</rdfs:label>
        <skos:definition xml:lang="en">-- Definition --
Normally producing olives for oil production.
-- Description --
Plantations of varieties normally grown for producing olive oil.
NOTE. Initial value:2.04.03.02</skos:definition>
        <skos:inScheme rdf:resource="http://lpis.ec.europa.eu/registry/applicationschema/cap-iacs-base/code#FarmStructureSurveyNumberValue"/>
    </owl:NamedIndividual>
    


    <!-- http://lpis.ec.europa.eu/registry/applicationschema/cap-iacs-base/code#FarmStructureSurveyNumberValue/normallyProducingTableOlives -->


    <owl:NamedIndividual rdf:about="http://lpis.ec.europa.eu/registry/applicationschema/cap-iacs-base/code#FarmStructureSurveyNumberValue/normallyProducingTableOlives">
        <rdf:type rdf:resource="http://lpis.ec.europa.eu/registry/applicationschema/cap-iacs-base#FarmStructureSurveyNumberValue"/>
        <rdfs:label xml:lang="en">Normally producing table olives</rdfs:label>
        <skos:definition xml:lang="en">-- Definition --
Normally producing table olives.
-- Description --
Plantations of varieties normally grown for producing table olives.
NOTE. Initial value:2.04.03.01</skos:definition>
        <skos:inScheme rdf:resource="http://lpis.ec.europa.eu/registry/applicationschema/cap-iacs-base/code#FarmStructureSurveyNumberValue"/>
    </owl:NamedIndividual>
    


    <!-- http://lpis.ec.europa.eu/registry/applicationschema/cap-iacs-base/code#FarmStructureSurveyNumberValue/nurseries -->


    <owl:NamedIndividual rdf:about="http://lpis.ec.europa.eu/registry/applicationschema/cap-iacs-base/code#FarmStructureSurveyNumberValue/nurseries">
        <rdf:type rdf:resource="http://lpis.ec.europa.eu/registry/applicationschema/cap-iacs-base#FarmStructureSurveyNumberValue"/>
        <rdfs:label xml:lang="en">Nurseries</rdfs:label>
        <skos:definition xml:lang="en">-- Definition --
Nurseries.
-- Description --
Areas of young ligneous (woody) plants grown in the open air for subsequent transplantation:
(a) vine and root-stock nurseries;
(b) fruit tree and berries nurseries;
(c) ornamental nurseries;
(d) commercial nurseries of forest trees (excluding those for the holding’s own requirements grown within woodland);
(e) trees and bushes for planting in gardens, parks, at the roadside and on embankments (e.g. hedgerow plants, rose trees and other ornamental bushes, ornamental conifers), including in all cases their stocks and young seedlings.
NOTE. Initial value:2.04.05</skos:definition>
        <skos:inScheme rdf:resource="http://lpis.ec.europa.eu/registry/applicationschema/cap-iacs-base/code#FarmStructureSurveyNumberValue"/>
    </owl:NamedIndividual>
    


    <!-- http://lpis.ec.europa.eu/registry/applicationschema/cap-iacs-base/code#FarmStructureSurveyNumberValue/nuts -->


    <owl:NamedIndividual rdf:about="http://lpis.ec.europa.eu/registry/applicationschema/cap-iacs-base/code#FarmStructureSurveyNumberValue/nuts">
        <rdf:type rdf:resource="http://lpis.ec.europa.eu/registry/applicationschema/cap-iacs-base#FarmStructureSurveyNumberValue"/>
        <rdfs:label xml:lang="en">Nuts</rdfs:label>
        <skos:definition xml:lang="en">-- Definition --
Nuts.
-- Description --
Nut tree plantations which are traditionally cropped in temperate and subtropical climates.
NOTE. Initial value:2.04.01.03</skos:definition>
        <skos:inScheme rdf:resource="http://lpis.ec.europa.eu/registry/applicationschema/cap-iacs-base/code#FarmStructureSurveyNumberValue"/>
    </owl:NamedIndividual>
    


    <!-- http://lpis.ec.europa.eu/registry/applicationschema/cap-iacs-base/code#FarmStructureSurveyNumberValue/oats -->


    <owl:NamedIndividual rdf:about="http://lpis.ec.europa.eu/registry/applicationschema/cap-iacs-base/code#FarmStructureSurveyNumberValue/oats">
        <rdf:type rdf:resource="http://lpis.ec.europa.eu/registry/applicationschema/cap-iacs-base#FarmStructureSurveyNumberValue"/>
        <rdfs:label xml:lang="en">Oats</rdfs:label>
        <skos:definition xml:lang="en">-- Definition --
Oats.
-- Description --
Avena sativa L., including mixtures of oats and other cereals sown in the spring.
NOTE. Initial value:2.01.01.05</skos:definition>
        <skos:inScheme rdf:resource="http://lpis.ec.europa.eu/registry/applicationschema/cap-iacs-base/code#FarmStructureSurveyNumberValue"/>
    </owl:NamedIndividual>
    


    <!-- http://lpis.ec.europa.eu/registry/applicationschema/cap-iacs-base/code#FarmStructureSurveyNumberValue/ofWhichChristmasTrees -->


    <owl:NamedIndividual rdf:about="http://lpis.ec.europa.eu/registry/applicationschema/cap-iacs-base/code#FarmStructureSurveyNumberValue/ofWhichChristmasTrees">
        <rdf:type rdf:resource="http://lpis.ec.europa.eu/registry/applicationschema/cap-iacs-base#FarmStructureSurveyNumberValue"/>
        <rdfs:label xml:lang="en">of which Christmas trees(1)</rdfs:label>
        <skos:definition xml:lang="en">-- Definition --
of which Christmas trees(1).
-- Description --
Not to be provided in 2010. (1)
Trees planted for commercial purposes as Christmas trees on the utilised agricultural area.
NOTE. Initial value:2.04.06.01</skos:definition>
        <skos:inScheme rdf:resource="http://lpis.ec.europa.eu/registry/applicationschema/cap-iacs-base/code#FarmStructureSurveyNumberValue"/>
    </owl:NamedIndividual>
    


    <!-- http://lpis.ec.europa.eu/registry/applicationschema/cap-iacs-base/code#FarmStructureSurveyNumberValue/ofWhichOnSetAsideArea -->


    <owl:NamedIndividual rdf:about="http://lpis.ec.europa.eu/registry/applicationschema/cap-iacs-base/code#FarmStructureSurveyNumberValue/ofWhichOnSetAsideArea">
        <rdf:type rdf:resource="http://lpis.ec.europa.eu/registry/applicationschema/cap-iacs-base#FarmStructureSurveyNumberValue"/>
        <rdfs:label xml:lang="en">of which on set-aside area</rdfs:label>
        <skos:definition xml:lang="en">-- Definition --
of which on set-aside area.
-- Description --
The production area of energy crops benefiting of the payment linked to set-aside entitlement when production takes place on set-aside area (Council Regulation (EC) No 1782/2003, Article 55 or 56).
NOTE. Initial value:2.06.03.01</skos:definition>
        <skos:inScheme rdf:resource="http://lpis.ec.europa.eu/registry/applicationschema/cap-iacs-base/code#FarmStructureSurveyNumberValue"/>
    </owl:NamedIndividual>
    


    <!-- http://lpis.ec.europa.eu/registry/applicationschema/cap-iacs-base/code#FarmStructureSurveyNumberValue/ofWhichPeasFieldBeansAndSweetLupins -->


    <owl:NamedIndividual rdf:about="http://lpis.ec.europa.eu/registry/applicationschema/cap-iacs-base/code#FarmStructureSurveyNumberValue/ofWhichPeasFieldBeansAndSweetLupins">
        <rdf:type rdf:resource="http://lpis.ec.europa.eu/registry/applicationschema/cap-iacs-base#FarmStructureSurveyNumberValue"/>
        <rdfs:label xml:lang="en">of which peas, field beans and sweet lupins</rdfs:label>
        <skos:definition xml:lang="en">-- Definition --
of which peas, field beans and sweet lupins.
-- Description --
Pisum sativum L., Vicia faba L., Lupinus spp., sown in pure crops, harvested dry for grain.
NOTE. Initial value:2.01.02.01</skos:definition>
        <skos:inScheme rdf:resource="http://lpis.ec.europa.eu/registry/applicationschema/cap-iacs-base/code#FarmStructureSurveyNumberValue"/>
    </owl:NamedIndividual>
    


    <!-- http://lpis.ec.europa.eu/registry/applicationschema/cap-iacs-base/code#FarmStructureSurveyNumberValue/ofWhichShortRotationCoppices -->


    <owl:NamedIndividual rdf:about="http://lpis.ec.europa.eu/registry/applicationschema/cap-iacs-base/code#FarmStructureSurveyNumberValue/ofWhichShortRotationCoppices">
        <rdf:type rdf:resource="http://lpis.ec.europa.eu/registry/applicationschema/cap-iacs-base#FarmStructureSurveyNumberValue"/>
        <rdfs:label xml:lang="en">of which short rotation coppices</rdfs:label>
        <skos:definition xml:lang="en">-- Definition --
of which short rotation coppices.
-- Description --
Wooded areas managed for growing wooded plants, where the rotation period is 20 years or less.
The rotation period is the time between the first sowing/planting of the trees and the harvest of the final product, where harvesting does not include normal management actions like thinning.
NOTE. Initial value:2.05.02.01</skos:definition>
        <skos:inScheme rdf:resource="http://lpis.ec.europa.eu/registry/applicationschema/cap-iacs-base/code#FarmStructureSurveyNumberValue"/>
    </owl:NamedIndividual>
    


    <!-- http://lpis.ec.europa.eu/registry/applicationschema/cap-iacs-base/code#FarmStructureSurveyNumberValue/olivePlantations -->


    <owl:NamedIndividual rdf:about="http://lpis.ec.europa.eu/registry/applicationschema/cap-iacs-base/code#FarmStructureSurveyNumberValue/olivePlantations">
        <rdf:type rdf:resource="http://lpis.ec.europa.eu/registry/applicationschema/cap-iacs-base#FarmStructureSurveyNumberValue"/>
        <rdfs:label xml:lang="en">Olive plantations</rdfs:label>
        <skos:definition xml:lang="en">-- Definition --
Olive plantations.
-- Description --
Plantations of Olea europea L.
NOTE. Initial value:2.04.03</skos:definition>
        <skos:inScheme rdf:resource="http://lpis.ec.europa.eu/registry/applicationschema/cap-iacs-base/code#FarmStructureSurveyNumberValue"/>
    </owl:NamedIndividual>
    


    <!-- http://lpis.ec.europa.eu/registry/applicationschema/cap-iacs-base/code#FarmStructureSurveyNumberValue/openField -->


    <owl:NamedIndividual rdf:about="http://lpis.ec.europa.eu/registry/applicationschema/cap-iacs-base/code#FarmStructureSurveyNumberValue/openField">
        <rdf:type rdf:resource="http://lpis.ec.europa.eu/registry/applicationschema/cap-iacs-base#FarmStructureSurveyNumberValue"/>
        <rdfs:label xml:lang="en">Open field</rdfs:label>
        <skos:definition xml:lang="en">-- Definition --
Open field.
-- Description --
Fresh vegetables, melons and strawberries grown on arable land in rotation with other agricultural crops.
NOTE. Initial value:2.01.07.01.01</skos:definition>
        <skos:inScheme rdf:resource="http://lpis.ec.europa.eu/registry/applicationschema/cap-iacs-base/code#FarmStructureSurveyNumberValue"/>
    </owl:NamedIndividual>
    


    <!-- http://lpis.ec.europa.eu/registry/applicationschema/cap-iacs-base/code#FarmStructureSurveyNumberValue/otherArableLandCrops -->


    <owl:NamedIndividual rdf:about="http://lpis.ec.europa.eu/registry/applicationschema/cap-iacs-base/code#FarmStructureSurveyNumberValue/otherArableLandCrops">
        <rdf:type rdf:resource="http://lpis.ec.europa.eu/registry/applicationschema/cap-iacs-base#FarmStructureSurveyNumberValue"/>
        <rdfs:label xml:lang="en">Other arable land crops</rdfs:label>
        <skos:definition xml:lang="en">-- Definition --
Other arable land crops.
-- Description --
Arable crops not included elsewhere.
NOTE. Initial value:2.01.11</skos:definition>
        <skos:inScheme rdf:resource="http://lpis.ec.europa.eu/registry/applicationschema/cap-iacs-base/code#FarmStructureSurveyNumberValue"/>
    </owl:NamedIndividual>
    


    <!-- http://lpis.ec.europa.eu/registry/applicationschema/cap-iacs-base/code#FarmStructureSurveyNumberValue/otherCerealsForTheProductionOfGrain -->


    <owl:NamedIndividual rdf:about="http://lpis.ec.europa.eu/registry/applicationschema/cap-iacs-base/code#FarmStructureSurveyNumberValue/otherCerealsForTheProductionOfGrain">
        <rdf:type rdf:resource="http://lpis.ec.europa.eu/registry/applicationschema/cap-iacs-base#FarmStructureSurveyNumberValue"/>
        <rdfs:label xml:lang="en">Other cereals for the production of grain</rdfs:label>
        <skos:definition xml:lang="en">-- Definition --
Other cereals for the production of grain.
-- Description --
Cereals sown in pure crops, harvested dry for grain, and that are not recorded elsewhere under the previous items.
NOTE. Initial value:2.01.01.99</skos:definition>
        <skos:inScheme rdf:resource="http://lpis.ec.europa.eu/registry/applicationschema/cap-iacs-base/code#FarmStructureSurveyNumberValue"/>
    </owl:NamedIndividual>
    


    <!-- http://lpis.ec.europa.eu/registry/applicationschema/cap-iacs-base/code#FarmStructureSurveyNumberValue/otherFibreCrops -->


    <owl:NamedIndividual rdf:about="http://lpis.ec.europa.eu/registry/applicationschema/cap-iacs-base/code#FarmStructureSurveyNumberValue/otherFibreCrops">
        <rdf:type rdf:resource="http://lpis.ec.europa.eu/registry/applicationschema/cap-iacs-base#FarmStructureSurveyNumberValue"/>
        <rdfs:label xml:lang="en">Other fibre crops</rdfs:label>
        <skos:definition xml:lang="en">-- Definition --
Other fibre crops.
-- Description --
Other plants grown mainly for their fibre content, not mentioned elsewhere.
NOTE. Initial value:2.01.06.11</skos:definition>
        <skos:inScheme rdf:resource="http://lpis.ec.europa.eu/registry/applicationschema/cap-iacs-base/code#FarmStructureSurveyNumberValue"/>
    </owl:NamedIndividual>
    


    <!-- http://lpis.ec.europa.eu/registry/applicationschema/cap-iacs-base/code#FarmStructureSurveyNumberValue/otherIndustrialCropsNotMentionedElsewhere -->


    <owl:NamedIndividual rdf:about="http://lpis.ec.europa.eu/registry/applicationschema/cap-iacs-base/code#FarmStructureSurveyNumberValue/otherIndustrialCropsNotMentionedElsewhere">
        <rdf:type rdf:resource="http://lpis.ec.europa.eu/registry/applicationschema/cap-iacs-base#FarmStructureSurveyNumberValue"/>
        <rdfs:label xml:lang="en">Other industrial crops not mentioned elsewhere</rdfs:label>
        <skos:definition xml:lang="en">-- Definition --
Other industrial crops not mentioned elsewhere.
-- Description --
Other industrial crops that have not been mentioned elsewhere.
Areas of crops used exclusively for renewable energy production are included.
NOTE. Initial value:2.01.06.99</skos:definition>
        <skos:inScheme rdf:resource="http://lpis.ec.europa.eu/registry/applicationschema/cap-iacs-base/code#FarmStructureSurveyNumberValue"/>
    </owl:NamedIndividual>
    


    <!-- http://lpis.ec.europa.eu/registry/applicationschema/cap-iacs-base/code#FarmStructureSurveyNumberValue/otherLand -->


    <owl:NamedIndividual rdf:about="http://lpis.ec.europa.eu/registry/applicationschema/cap-iacs-base/code#FarmStructureSurveyNumberValue/otherLand">
        <rdf:type rdf:resource="http://lpis.ec.europa.eu/registry/applicationschema/cap-iacs-base#FarmStructureSurveyNumberValue"/>
        <rdfs:label xml:lang="en">Other land</rdfs:label>
        <skos:definition xml:lang="en">-- Definition --
Other land.
-- Description --
‘Other land’ includes unutilised agricultural land (agricultural land which is no longer farmed, for economic, social or other reasons, and which is not used in the crop rotation system), wooded area and other land occupied by buildings, farmyards, tracks, ponds, quarries, infertile land, rock, etc.
NOTE. Initial value:2.05</skos:definition>
        <skos:inScheme rdf:resource="http://lpis.ec.europa.eu/registry/applicationschema/cap-iacs-base/code#FarmStructureSurveyNumberValue"/>
    </owl:NamedIndividual>
    


    <!-- http://lpis.ec.europa.eu/registry/applicationschema/cap-iacs-base/code#FarmStructureSurveyNumberValue/otherLandLandOccupiedByBuildingsFarmyardsTracksPondsQuarriesInfertileLandRockEtc -->


    <owl:NamedIndividual rdf:about="http://lpis.ec.europa.eu/registry/applicationschema/cap-iacs-base/code#FarmStructureSurveyNumberValue/otherLandLandOccupiedByBuildingsFarmyardsTracksPondsQuarriesInfertileLandRockEtc">
        <rdf:type rdf:resource="http://lpis.ec.europa.eu/registry/applicationschema/cap-iacs-base#FarmStructureSurveyNumberValue"/>
        <rdfs:label xml:lang="en">Other land (land occupied by buildings, farmyards, tracks, ponds, quarries, infertile land, rock, etc.)</rdfs:label>
        <skos:definition xml:lang="en">-- Definition --
Other land (land occupied by buildings, farmyards, tracks, ponds, quarries, infertile land, rock, etc.)
-- Description --
All those parts of the total area belonging to the agricultural holding which constitute neither utilised agricultural area, unutilised agricultural area nor wooded area.
NOTE. Initial value:2.05.03</skos:definition>
        <skos:inScheme rdf:resource="http://lpis.ec.europa.eu/registry/applicationschema/cap-iacs-base/code#FarmStructureSurveyNumberValue"/>
    </owl:NamedIndividual>
    


    <!-- http://lpis.ec.europa.eu/registry/applicationschema/cap-iacs-base/code#FarmStructureSurveyNumberValue/otherOilSeedCrops -->


    <owl:NamedIndividual rdf:about="http://lpis.ec.europa.eu/registry/applicationschema/cap-iacs-base/code#FarmStructureSurveyNumberValue/otherOilSeedCrops">
        <rdf:type rdf:resource="http://lpis.ec.europa.eu/registry/applicationschema/cap-iacs-base#FarmStructureSurveyNumberValue"/>
        <rdfs:label xml:lang="en">Other oil seed crops</rdfs:label>
        <skos:definition xml:lang="en">-- Definition --
Other oil seed crops.
-- Description --
Other crops grown mainly for their oil content, harvested as dry grains, which are not mentioned elsewhere.
NOTE. Initial value:2.01.06.08</skos:definition>
        <skos:inScheme rdf:resource="http://lpis.ec.europa.eu/registry/applicationschema/cap-iacs-base/code#FarmStructureSurveyNumberValue"/>
    </owl:NamedIndividual>
    


    <!-- http://lpis.ec.europa.eu/registry/applicationschema/cap-iacs-base/code#FarmStructureSurveyNumberValue/otherPermanentCrops -->


    <owl:NamedIndividual rdf:about="http://lpis.ec.europa.eu/registry/applicationschema/cap-iacs-base/code#FarmStructureSurveyNumberValue/otherPermanentCrops">
        <rdf:type rdf:resource="http://lpis.ec.europa.eu/registry/applicationschema/cap-iacs-base#FarmStructureSurveyNumberValue"/>
        <rdfs:label xml:lang="en">Other permanent crops</rdfs:label>
        <skos:definition xml:lang="en">-- Definition --
Other permanent crops.
-- Description --
Open-air permanent crops other than those under the previous heading and in particular those used for plaiting or weaving, harvested generally every year.
NOTE. Initial value:2.04.06</skos:definition>
        <skos:inScheme rdf:resource="http://lpis.ec.europa.eu/registry/applicationschema/cap-iacs-base/code#FarmStructureSurveyNumberValue"/>
    </owl:NamedIndividual>
    


    <!-- http://lpis.ec.europa.eu/registry/applicationschema/cap-iacs-base/code#FarmStructureSurveyNumberValue/otherPlantsHarvestedGreen -->


    <owl:NamedIndividual rdf:about="http://lpis.ec.europa.eu/registry/applicationschema/cap-iacs-base/code#FarmStructureSurveyNumberValue/otherPlantsHarvestedGreen">
        <rdf:type rdf:resource="http://lpis.ec.europa.eu/registry/applicationschema/cap-iacs-base#FarmStructureSurveyNumberValue"/>
        <rdfs:label xml:lang="en">Other plants harvested green</rdfs:label>
        <skos:definition xml:lang="en">-- Definition --
Other plants harvested green.
-- Description --
Other annual or multiannual (less than five years) fodder crops.
NOTE. Initial value:2.01.09.02</skos:definition>
        <skos:inScheme rdf:resource="http://lpis.ec.europa.eu/registry/applicationschema/cap-iacs-base/code#FarmStructureSurveyNumberValue"/>
    </owl:NamedIndividual>
    


    <!-- http://lpis.ec.europa.eu/registry/applicationschema/cap-iacs-base/code#FarmStructureSurveyNumberValue/otherPlantsHarvestedGreenNotMentionedElsewhere -->


    <owl:NamedIndividual rdf:about="http://lpis.ec.europa.eu/registry/applicationschema/cap-iacs-base/code#FarmStructureSurveyNumberValue/otherPlantsHarvestedGreenNotMentionedElsewhere">
        <rdf:type rdf:resource="http://lpis.ec.europa.eu/registry/applicationschema/cap-iacs-base#FarmStructureSurveyNumberValue"/>
        <rdfs:label xml:lang="en">Other plants harvested green not mentioned elsewhere</rdfs:label>
        <skos:definition xml:lang="en">-- Definition --
Other plants harvested green not mentioned elsewhere.
-- Description --
Other arable crops intended mainly for animal fodder, harvested green, not mentioned elsewhere.
NOTE. Initial value:2.01.09.02.99</skos:definition>
        <skos:inScheme rdf:resource="http://lpis.ec.europa.eu/registry/applicationschema/cap-iacs-base/code#FarmStructureSurveyNumberValue"/>
    </owl:NamedIndividual>
    


    <!-- http://lpis.ec.europa.eu/registry/applicationschema/cap-iacs-base/code#FarmStructureSurveyNumberValue/otherWines -->


    <owl:NamedIndividual rdf:about="http://lpis.ec.europa.eu/registry/applicationschema/cap-iacs-base/code#FarmStructureSurveyNumberValue/otherWines">
        <rdf:type rdf:resource="http://lpis.ec.europa.eu/registry/applicationschema/cap-iacs-base#FarmStructureSurveyNumberValue"/>
        <rdfs:label xml:lang="en">Other wines</rdfs:label>
        <skos:definition xml:lang="en">-- Definition --
Other wines.
-- Description --
Grape varieties normally grown for the production of wines other than PDO and PGI wines.
NOTE. Initial value:2.04.04.02</skos:definition>
        <skos:inScheme rdf:resource="http://lpis.ec.europa.eu/registry/applicationschema/cap-iacs-base/code#FarmStructureSurveyNumberValue"/>
    </owl:NamedIndividual>
    


    <!-- http://lpis.ec.europa.eu/registry/applicationschema/cap-iacs-base/code#FarmStructureSurveyNumberValue/outdoorOrUnderLowNotAccessibleProtectiveCover -->


    <owl:NamedIndividual rdf:about="http://lpis.ec.europa.eu/registry/applicationschema/cap-iacs-base/code#FarmStructureSurveyNumberValue/outdoorOrUnderLowNotAccessibleProtectiveCover">
        <rdf:type rdf:resource="http://lpis.ec.europa.eu/registry/applicationschema/cap-iacs-base#FarmStructureSurveyNumberValue"/>
        <rdfs:label xml:lang="en">Outdoor or under low (not accessible) protective cover</rdfs:label>
        <skos:definition xml:lang="en">-- Definition --
Outdoor or under low (not accessible) protective cover.
-- Description --
Fresh vegetables, melons and strawberries, outdoor or under low (non-accessible) cover.
NOTE. Initial value:2.01.07.01</skos:definition>
        <skos:inScheme rdf:resource="http://lpis.ec.europa.eu/registry/applicationschema/cap-iacs-base/code#FarmStructureSurveyNumberValue"/>
    </owl:NamedIndividual>
    


    <!-- http://lpis.ec.europa.eu/registry/applicationschema/cap-iacs-base/code#FarmStructureSurveyNumberValue/pastureAndMeadowExcludingRoughGrazings -->


    <owl:NamedIndividual rdf:about="http://lpis.ec.europa.eu/registry/applicationschema/cap-iacs-base/code#FarmStructureSurveyNumberValue/pastureAndMeadowExcludingRoughGrazings">
        <rdf:type rdf:resource="http://lpis.ec.europa.eu/registry/applicationschema/cap-iacs-base#FarmStructureSurveyNumberValue"/>
        <rdfs:label xml:lang="en">Pasture and meadow, excluding rough grazings</rdfs:label>
        <skos:definition xml:lang="en">-- Definition --
Pasture and meadow, excluding rough grazings.
-- Description --
Permanent pasture on good or medium quality soils. These areas can normally be used for intensive grazing.
NOTE. Initial value:2.03.01</skos:definition>
        <skos:inScheme rdf:resource="http://lpis.ec.europa.eu/registry/applicationschema/cap-iacs-base/code#FarmStructureSurveyNumberValue"/>
    </owl:NamedIndividual>
    


    <!-- http://lpis.ec.europa.eu/registry/applicationschema/cap-iacs-base/code#FarmStructureSurveyNumberValue/permanentCrops -->


    <owl:NamedIndividual rdf:about="http://lpis.ec.europa.eu/registry/applicationschema/cap-iacs-base/code#FarmStructureSurveyNumberValue/permanentCrops">
        <rdf:type rdf:resource="http://lpis.ec.europa.eu/registry/applicationschema/cap-iacs-base#FarmStructureSurveyNumberValue"/>
        <rdfs:label xml:lang="en">Permanent crops</rdfs:label>
        <skos:definition xml:lang="en">-- Definition --
Permanent crops.
-- Description --
Crops not grown in rotation, other than permanent grassland, which occupy the soil for a long period and yield crops over several years.
NOTE. Initial value:2.04</skos:definition>
        <skos:inScheme rdf:resource="http://lpis.ec.europa.eu/registry/applicationschema/cap-iacs-base/code#FarmStructureSurveyNumberValue"/>
    </owl:NamedIndividual>
    


    <!-- http://lpis.ec.europa.eu/registry/applicationschema/cap-iacs-base/code#FarmStructureSurveyNumberValue/permanentCropsUnderGlass -->


    <owl:NamedIndividual rdf:about="http://lpis.ec.europa.eu/registry/applicationschema/cap-iacs-base/code#FarmStructureSurveyNumberValue/permanentCropsUnderGlass">
        <rdf:type rdf:resource="http://lpis.ec.europa.eu/registry/applicationschema/cap-iacs-base#FarmStructureSurveyNumberValue"/>
        <rdfs:label xml:lang="en">Permanent crops under glass</rdfs:label>
        <skos:definition xml:lang="en">-- Definition --
Permanent crops under glass.
-- Description --
Permanent crops under glass.
NOTE. Initial value:2.04.07</skos:definition>
        <skos:inScheme rdf:resource="http://lpis.ec.europa.eu/registry/applicationschema/cap-iacs-base/code#FarmStructureSurveyNumberValue"/>
    </owl:NamedIndividual>
    


    <!-- http://lpis.ec.europa.eu/registry/applicationschema/cap-iacs-base/code#FarmStructureSurveyNumberValue/permanentGrassland -->


    <owl:NamedIndividual rdf:about="http://lpis.ec.europa.eu/registry/applicationschema/cap-iacs-base/code#FarmStructureSurveyNumberValue/permanentGrassland">
        <rdf:type rdf:resource="http://lpis.ec.europa.eu/registry/applicationschema/cap-iacs-base#FarmStructureSurveyNumberValue"/>
        <rdfs:label xml:lang="en">Permanent grassland</rdfs:label>
        <skos:definition xml:lang="en">-- Definition --
Permanent grassland.
-- Description --
Land used permanently (for five years or more) to grow herbaceous forage crops, through cultivation (sown) or naturally (self-seeded), and that is not included in the crop rotation on the holding.
The land can be used for grazing or mown for silage, hay or used for renewable energy production.
NOTE. Initial value:2.03</skos:definition>
        <skos:inScheme rdf:resource="http://lpis.ec.europa.eu/registry/applicationschema/cap-iacs-base/code#FarmStructureSurveyNumberValue"/>
    </owl:NamedIndividual>
    


    <!-- http://lpis.ec.europa.eu/registry/applicationschema/cap-iacs-base/code#FarmStructureSurveyNumberValue/permanentGrasslandNoLongerUsedForProductionPurposesAndEligibleForThePaymentOfSubsidies -->


    <owl:NamedIndividual rdf:about="http://lpis.ec.europa.eu/registry/applicationschema/cap-iacs-base/code#FarmStructureSurveyNumberValue/permanentGrasslandNoLongerUsedForProductionPurposesAndEligibleForThePaymentOfSubsidies">
        <rdf:type rdf:resource="http://lpis.ec.europa.eu/registry/applicationschema/cap-iacs-base#FarmStructureSurveyNumberValue"/>
        <rdfs:label xml:lang="en">Permanent grassland no longer used for production purposes and eligible for the payment of subsidies</rdfs:label>
        <skos:definition xml:lang="en">-- Definition --
Permanent grassland no longer used for production purposes and eligible for the payment of subsidies.
-- Description --
Areas of permanent grassland and meadows no longer used for production purposes which, in line with Regulation (EC) No 1782/2003 or, where applicable, the most recent legislation, are maintained in good agricultural and environmental condition and are eligible for financial support.
NOTE. Initial value:2.03.03</skos:definition>
        <skos:inScheme rdf:resource="http://lpis.ec.europa.eu/registry/applicationschema/cap-iacs-base/code#FarmStructureSurveyNumberValue"/>
    </owl:NamedIndividual>
    


    <!-- http://lpis.ec.europa.eu/registry/applicationschema/cap-iacs-base/code#FarmStructureSurveyNumberValue/plantsHarvestedGreen -->


    <owl:NamedIndividual rdf:about="http://lpis.ec.europa.eu/registry/applicationschema/cap-iacs-base/code#FarmStructureSurveyNumberValue/plantsHarvestedGreen">
        <rdf:type rdf:resource="http://lpis.ec.europa.eu/registry/applicationschema/cap-iacs-base#FarmStructureSurveyNumberValue"/>
        <rdfs:label xml:lang="en">Plants harvested green</rdfs:label>
        <skos:definition xml:lang="en">-- Definition --
Plants harvested green.
-- Description --
All ‘green’ arable crops intended mainly for animal feed, grown in rotation with other crops and occupying the same parcel for less than five years (annual or multiannual fodder crops).
Green crops used for renewable energy production are included.
Crops not used on the holding but sold, either for direct use on other agricultural holdings or to industry, are included.
NOTE. Initial value:2.01.09</skos:definition>
        <skos:inScheme rdf:resource="http://lpis.ec.europa.eu/registry/applicationschema/cap-iacs-base/code#FarmStructureSurveyNumberValue"/>
    </owl:NamedIndividual>
    


    <!-- http://lpis.ec.europa.eu/registry/applicationschema/cap-iacs-base/code#FarmStructureSurveyNumberValue/potatoesIncludingEarlyPotatoesAndSeedPotatoes -->


    <owl:NamedIndividual rdf:about="http://lpis.ec.europa.eu/registry/applicationschema/cap-iacs-base/code#FarmStructureSurveyNumberValue/potatoesIncludingEarlyPotatoesAndSeedPotatoes">
        <rdf:type rdf:resource="http://lpis.ec.europa.eu/registry/applicationschema/cap-iacs-base#FarmStructureSurveyNumberValue"/>
        <rdfs:label xml:lang="en">Potatoes (including early potatoes and seed potatoes)</rdfs:label>
        <skos:definition xml:lang="en">-- Definition --
Potatoes (including early potatoes and seed potatoes).
-- Description --
Solanum tuberosum L.
NOTE. Initial value:2.01.03</skos:definition>
        <skos:inScheme rdf:resource="http://lpis.ec.europa.eu/registry/applicationschema/cap-iacs-base/code#FarmStructureSurveyNumberValue"/>
    </owl:NamedIndividual>
    


    <!-- http://lpis.ec.europa.eu/registry/applicationschema/cap-iacs-base/code#FarmStructureSurveyNumberValue/qualityWine -->


    <owl:NamedIndividual rdf:about="http://lpis.ec.europa.eu/registry/applicationschema/cap-iacs-base/code#FarmStructureSurveyNumberValue/qualityWine">
        <rdf:type rdf:resource="http://lpis.ec.europa.eu/registry/applicationschema/cap-iacs-base#FarmStructureSurveyNumberValue"/>
        <rdfs:label xml:lang="en">Quality wine</rdfs:label>
        <skos:definition xml:lang="en">-- Definition --
Quality wine.
-- Description --
Grape varieties normally grown for the production of wines with a protected designation of origin (PDO) which comply with the requirements (i) of Council Regulation (EC) No 479/2008(1)
OJ L 148, 6.6.2008, p. 1. (1) or, where applicable, the most recent legislation; and (ii) the corresponding national rules.
Grape varieties normally grown for the production of wines with a protected geographical indication (PGI) which comply with the requirements (i) of Regulation (EC) No 479/2008 or, where applicable, the most recent legislation; and (ii) the corresponding national rules.
NOTE. Initial value:2.04.04.01</skos:definition>
        <skos:inScheme rdf:resource="http://lpis.ec.europa.eu/registry/applicationschema/cap-iacs-base/code#FarmStructureSurveyNumberValue"/>
    </owl:NamedIndividual>
    


    <!-- http://lpis.ec.europa.eu/registry/applicationschema/cap-iacs-base/code#FarmStructureSurveyNumberValue/raisins -->


    <owl:NamedIndividual rdf:about="http://lpis.ec.europa.eu/registry/applicationschema/cap-iacs-base/code#FarmStructureSurveyNumberValue/raisins">
        <rdf:type rdf:resource="http://lpis.ec.europa.eu/registry/applicationschema/cap-iacs-base#FarmStructureSurveyNumberValue"/>
        <rdfs:label xml:lang="en">Raisins</rdfs:label>
        <skos:definition xml:lang="en">-- Definition --
Raisins.
-- Description --
Grape varieties normally grown for the production of raisins.
NOTE. Initial value:2.04.04.04</skos:definition>
        <skos:inScheme rdf:resource="http://lpis.ec.europa.eu/registry/applicationschema/cap-iacs-base/code#FarmStructureSurveyNumberValue"/>
    </owl:NamedIndividual>
    


    <!-- http://lpis.ec.europa.eu/registry/applicationschema/cap-iacs-base/code#FarmStructureSurveyNumberValue/rapeAndTurnipRape -->


    <owl:NamedIndividual rdf:about="http://lpis.ec.europa.eu/registry/applicationschema/cap-iacs-base/code#FarmStructureSurveyNumberValue/rapeAndTurnipRape">
        <rdf:type rdf:resource="http://lpis.ec.europa.eu/registry/applicationschema/cap-iacs-base#FarmStructureSurveyNumberValue"/>
        <rdfs:label xml:lang="en">Rape and turnip rape</rdfs:label>
        <skos:definition xml:lang="en">-- Definition --
Rape and turnip rape.
-- Description --
Brassica napus L. (partim) and Brassica rapa L. var. sylvestris (Lam.) Briggs, grown for the production of oil, harvested as dry grains.
NOTE. Initial value:2.01.06.04</skos:definition>
        <skos:inScheme rdf:resource="http://lpis.ec.europa.eu/registry/applicationschema/cap-iacs-base/code#FarmStructureSurveyNumberValue"/>
    </owl:NamedIndividual>
    


    <!-- http://lpis.ec.europa.eu/registry/applicationschema/cap-iacs-base/code#FarmStructureSurveyNumberValue/rice -->


    <owl:NamedIndividual rdf:about="http://lpis.ec.europa.eu/registry/applicationschema/cap-iacs-base/code#FarmStructureSurveyNumberValue/rice">
        <rdf:type rdf:resource="http://lpis.ec.europa.eu/registry/applicationschema/cap-iacs-base#FarmStructureSurveyNumberValue"/>
        <rdfs:label xml:lang="en">Rice</rdfs:label>
        <skos:definition xml:lang="en">-- Definition --
Rice.
-- Description --
Oryza sativa L.
NOTE. Initial value:2.01.01.07</skos:definition>
        <skos:inScheme rdf:resource="http://lpis.ec.europa.eu/registry/applicationschema/cap-iacs-base/code#FarmStructureSurveyNumberValue"/>
    </owl:NamedIndividual>
    


    <!-- http://lpis.ec.europa.eu/registry/applicationschema/cap-iacs-base/code#FarmStructureSurveyNumberValue/roughGrazings -->


    <owl:NamedIndividual rdf:about="http://lpis.ec.europa.eu/registry/applicationschema/cap-iacs-base/code#FarmStructureSurveyNumberValue/roughGrazings">
        <rdf:type rdf:resource="http://lpis.ec.europa.eu/registry/applicationschema/cap-iacs-base#FarmStructureSurveyNumberValue"/>
        <rdfs:label xml:lang="en">Rough grazings</rdfs:label>
        <skos:definition xml:lang="en">-- Definition --
Rough grazings.
-- Description --
Low yielding permanent grassland, usually on low quality soil, for example on hilly land and at high altitudes, usually unimproved by fertiliser, cultivation, reseeding or drainage.
These areas can normally be used only for extensive grazing and are not normally mown or are mown in an extensive manner; they cannot support a large density of animals.
NOTE. Initial value:2.03.02</skos:definition>
        <skos:inScheme rdf:resource="http://lpis.ec.europa.eu/registry/applicationschema/cap-iacs-base/code#FarmStructureSurveyNumberValue"/>
    </owl:NamedIndividual>
    


    <!-- http://lpis.ec.europa.eu/registry/applicationschema/cap-iacs-base/code#FarmStructureSurveyNumberValue/rye -->


    <owl:NamedIndividual rdf:about="http://lpis.ec.europa.eu/registry/applicationschema/cap-iacs-base/code#FarmStructureSurveyNumberValue/rye">
        <rdf:type rdf:resource="http://lpis.ec.europa.eu/registry/applicationschema/cap-iacs-base#FarmStructureSurveyNumberValue"/>
        <rdfs:label xml:lang="en">Rye</rdfs:label>
        <skos:definition xml:lang="en">-- Definition --
Rye.
-- Description --
Secale cereale L., including mixtures of rye and other cereals sown in the autumn (maslin).
NOTE. Initial value:2.01.01.03</skos:definition>
        <skos:inScheme rdf:resource="http://lpis.ec.europa.eu/registry/applicationschema/cap-iacs-base/code#FarmStructureSurveyNumberValue"/>
    </owl:NamedIndividual>
    


    <!-- http://lpis.ec.europa.eu/registry/applicationschema/cap-iacs-base/code#FarmStructureSurveyNumberValue/soya -->


    <owl:NamedIndividual rdf:about="http://lpis.ec.europa.eu/registry/applicationschema/cap-iacs-base/code#FarmStructureSurveyNumberValue/soya">
        <rdf:type rdf:resource="http://lpis.ec.europa.eu/registry/applicationschema/cap-iacs-base#FarmStructureSurveyNumberValue"/>
        <rdfs:label xml:lang="en">Soya</rdfs:label>
        <skos:definition xml:lang="en">-- Definition --
Soya.
-- Description --
Glycine max L. Merril, harvested as dry grains.
NOTE. Initial value:2.01.06.06</skos:definition>
        <skos:inScheme rdf:resource="http://lpis.ec.europa.eu/registry/applicationschema/cap-iacs-base/code#FarmStructureSurveyNumberValue"/>
    </owl:NamedIndividual>
    


    <!-- http://lpis.ec.europa.eu/registry/applicationschema/cap-iacs-base/code#FarmStructureSurveyNumberValue/sugarBeetExcludingSeed -->


    <owl:NamedIndividual rdf:about="http://lpis.ec.europa.eu/registry/applicationschema/cap-iacs-base/code#FarmStructureSurveyNumberValue/sugarBeetExcludingSeed">
        <rdf:type rdf:resource="http://lpis.ec.europa.eu/registry/applicationschema/cap-iacs-base#FarmStructureSurveyNumberValue"/>
        <rdfs:label xml:lang="en">Sugar beet (excluding seed)</rdfs:label>
        <skos:definition xml:lang="en">-- Definition --
Sugar beet (excluding seed).
-- Description --
Beta vulgaris L. intended for the sugar industry and alcohol production (including energy production).
NOTE. Initial value:2.01.04</skos:definition>
        <skos:inScheme rdf:resource="http://lpis.ec.europa.eu/registry/applicationschema/cap-iacs-base/code#FarmStructureSurveyNumberValue"/>
    </owl:NamedIndividual>
    


    <!-- http://lpis.ec.europa.eu/registry/applicationschema/cap-iacs-base/code#FarmStructureSurveyNumberValue/sunflower -->


    <owl:NamedIndividual rdf:about="http://lpis.ec.europa.eu/registry/applicationschema/cap-iacs-base/code#FarmStructureSurveyNumberValue/sunflower">
        <rdf:type rdf:resource="http://lpis.ec.europa.eu/registry/applicationschema/cap-iacs-base#FarmStructureSurveyNumberValue"/>
        <rdfs:label xml:lang="en">Sunflower</rdfs:label>
        <skos:definition xml:lang="en">-- Definition --
Sunflower.
-- Description --
Helianthus annuus L., harvested as dry grains.
NOTE. Initial value:2.01.06.05</skos:definition>
        <skos:inScheme rdf:resource="http://lpis.ec.europa.eu/registry/applicationschema/cap-iacs-base/code#FarmStructureSurveyNumberValue"/>
    </owl:NamedIndividual>
    


    <!-- http://lpis.ec.europa.eu/registry/applicationschema/cap-iacs-base/code#FarmStructureSurveyNumberValue/tableGrapes -->


    <owl:NamedIndividual rdf:about="http://lpis.ec.europa.eu/registry/applicationschema/cap-iacs-base/code#FarmStructureSurveyNumberValue/tableGrapes">
        <rdf:type rdf:resource="http://lpis.ec.europa.eu/registry/applicationschema/cap-iacs-base#FarmStructureSurveyNumberValue"/>
        <rdfs:label xml:lang="en">Table grapes</rdfs:label>
        <skos:definition xml:lang="en">-- Definition --
Table grapes.
-- Description --
Grape varieties normally grown for the production of fresh grapes.
NOTE. Initial value:2.04.04.03</skos:definition>
        <skos:inScheme rdf:resource="http://lpis.ec.europa.eu/registry/applicationschema/cap-iacs-base/code#FarmStructureSurveyNumberValue"/>
    </owl:NamedIndividual>
    


    <!-- http://lpis.ec.europa.eu/registry/applicationschema/cap-iacs-base/code#FarmStructureSurveyNumberValue/temporaryGrass -->


    <owl:NamedIndividual rdf:about="http://lpis.ec.europa.eu/registry/applicationschema/cap-iacs-base/code#FarmStructureSurveyNumberValue/temporaryGrass">
        <rdf:type rdf:resource="http://lpis.ec.europa.eu/registry/applicationschema/cap-iacs-base#FarmStructureSurveyNumberValue"/>
        <rdfs:label xml:lang="en">Temporary grass</rdfs:label>
        <skos:definition xml:lang="en">-- Definition --
Temporary grass.
-- Description --
Grass plants for grazing, hay or silage included as a part of a normal crop rotation, lasting at least one crop year and less than five years, sown with grass or grass mixtures. The areas are broken up by ploughing or other tilling or the plants are destroyed by other means such as by herbicides before they are sown again.
Mixtures of predominantly grass plants and other forage crops (usually leguminous), grazed, harvested green or as dried hay are included here.
NOTE. Initial value:2.01.09.01</skos:definition>
        <skos:inScheme rdf:resource="http://lpis.ec.europa.eu/registry/applicationschema/cap-iacs-base/code#FarmStructureSurveyNumberValue"/>
    </owl:NamedIndividual>
    


    <!-- http://lpis.ec.europa.eu/registry/applicationschema/cap-iacs-base/code#FarmStructureSurveyNumberValue/tobacco -->


    <owl:NamedIndividual rdf:about="http://lpis.ec.europa.eu/registry/applicationschema/cap-iacs-base/code#FarmStructureSurveyNumberValue/tobacco">
        <rdf:type rdf:resource="http://lpis.ec.europa.eu/registry/applicationschema/cap-iacs-base#FarmStructureSurveyNumberValue"/>
        <rdfs:label xml:lang="en">Tobacco</rdfs:label>
        <skos:definition xml:lang="en">-- Definition --
Tobacco
-- Description --
Nicotiana tabacum L.
NOTE. Initial value:2.01.06.01</skos:definition>
        <skos:inScheme rdf:resource="http://lpis.ec.europa.eu/registry/applicationschema/cap-iacs-base/code#FarmStructureSurveyNumberValue"/>
    </owl:NamedIndividual>
    


    <!-- http://lpis.ec.europa.eu/registry/applicationschema/cap-iacs-base/code#FarmStructureSurveyNumberValue/totalCultivatedAreaIrrigatedAtLeastOnceDuringThePrevious12Months -->


    <owl:NamedIndividual rdf:about="http://lpis.ec.europa.eu/registry/applicationschema/cap-iacs-base/code#FarmStructureSurveyNumberValue/totalCultivatedAreaIrrigatedAtLeastOnceDuringThePrevious12Months">
        <rdf:type rdf:resource="http://lpis.ec.europa.eu/registry/applicationschema/cap-iacs-base#FarmStructureSurveyNumberValue"/>
        <rdfs:label xml:lang="en">Total cultivated area irrigated at least once during the previous 12 months</rdfs:label>
        <skos:definition xml:lang="en">-- Definition --
Total cultivated area irrigated at least once during the previous 12 months.
-- Description --
Area of crops which have actually been irrigated at least once during the 12 months prior to the reference day of the survey.
NOTE. Initial value:2.06.02.02</skos:definition>
        <skos:inScheme rdf:resource="http://lpis.ec.europa.eu/registry/applicationschema/cap-iacs-base/code#FarmStructureSurveyNumberValue"/>
    </owl:NamedIndividual>
    


    <!-- http://lpis.ec.europa.eu/registry/applicationschema/cap-iacs-base/code#FarmStructureSurveyNumberValue/totalIrrigableArea -->


    <owl:NamedIndividual rdf:about="http://lpis.ec.europa.eu/registry/applicationschema/cap-iacs-base/code#FarmStructureSurveyNumberValue/totalIrrigableArea">
        <rdf:type rdf:resource="http://lpis.ec.europa.eu/registry/applicationschema/cap-iacs-base#FarmStructureSurveyNumberValue"/>
        <rdfs:label xml:lang="en">Total irrigable area</rdfs:label>
        <skos:definition xml:lang="en">-- Definition --
Total irrigable area.
-- Description --
Total maximum utilised agricultural area which could be irrigated in the reference year using the equipment and the quantity of water normally available on the holding.
NOTE. Initial value:2.06.02.01</skos:definition>
        <skos:inScheme rdf:resource="http://lpis.ec.europa.eu/registry/applicationschema/cap-iacs-base/code#FarmStructureSurveyNumberValue"/>
    </owl:NamedIndividual>
    


    <!-- http://lpis.ec.europa.eu/registry/applicationschema/cap-iacs-base/code#FarmStructureSurveyNumberValue/underGlassOrOtherAccessibleProtectiveCover -->


    <owl:NamedIndividual rdf:about="http://lpis.ec.europa.eu/registry/applicationschema/cap-iacs-base/code#FarmStructureSurveyNumberValue/underGlassOrOtherAccessibleProtectiveCover">
        <rdf:type rdf:resource="http://lpis.ec.europa.eu/registry/applicationschema/cap-iacs-base#FarmStructureSurveyNumberValue"/>
        <rdfs:label xml:lang="en">Under glass or other (accessible) protective cover</rdfs:label>
        <skos:definition xml:lang="en">-- Definition --
Under glass or other (accessible) protective cover.
-- Description --
Crops, which for the whole of their period of growth or for the predominant part of it are covered by greenhouses or fixed or mobile high cover (glass or rigid or flexible plastic).
NOTE. Initial value:2.01.07.02</skos:definition>
        <skos:inScheme rdf:resource="http://lpis.ec.europa.eu/registry/applicationschema/cap-iacs-base/code#FarmStructureSurveyNumberValue"/>
    </owl:NamedIndividual>
    


    <!-- http://lpis.ec.europa.eu/registry/applicationschema/cap-iacs-base/code#FarmStructureSurveyNumberValue/underGlassOrOtherAccessibleProtectiveCoverFlowers -->


    <owl:NamedIndividual rdf:about="http://lpis.ec.europa.eu/registry/applicationschema/cap-iacs-base/code#FarmStructureSurveyNumberValue/underGlassOrOtherAccessibleProtectiveCoverFlowers">
        <rdf:type rdf:resource="http://lpis.ec.europa.eu/registry/applicationschema/cap-iacs-base#FarmStructureSurveyNumberValue"/>
        <rdfs:label xml:lang="en">Under glass or other (accessible)  protective cover</rdfs:label>
        <skos:definition xml:lang="en">-- Definition --
Under glass or other (accessible)  protective cover.
-- Description --
Flowers and ornamental plants (excluding nurseries), which for the whole of their period of growth or for the predominant part of it are covered by greenhouses or fixed or mobile high cover (glass or rigid or flexible plastic).
NOTE. Initial value:2.01.08.02</skos:definition>
        <skos:inScheme rdf:resource="http://lpis.ec.europa.eu/registry/applicationschema/cap-iacs-base/code#FarmStructureSurveyNumberValue"/>
    </owl:NamedIndividual>
    


    <!-- http://lpis.ec.europa.eu/registry/applicationschema/cap-iacs-base/code#FarmStructureSurveyNumberValue/unutilisedAgriculturalLand -->


    <owl:NamedIndividual rdf:about="http://lpis.ec.europa.eu/registry/applicationschema/cap-iacs-base/code#FarmStructureSurveyNumberValue/unutilisedAgriculturalLand">
        <rdf:type rdf:resource="http://lpis.ec.europa.eu/registry/applicationschema/cap-iacs-base#FarmStructureSurveyNumberValue"/>
        <rdfs:label xml:lang="en">Unutilised agricultural land</rdfs:label>
        <skos:definition xml:lang="en">-- Definition --
Unutilised agricultural land.
-- Description --
Area previously used as an agricultural area and, during the reference year of the survey, no longer worked for economic, social or other reasons and which is not used in the crop rotation system, i.e. land where no agricultural use is intended.
This land could be brought back into cultivation using the resources normally available on an agricultural holding.
NOTE. Initial value:2.05.01</skos:definition>
        <skos:inScheme rdf:resource="http://lpis.ec.europa.eu/registry/applicationschema/cap-iacs-base/code#FarmStructureSurveyNumberValue"/>
    </owl:NamedIndividual>
    


    <!-- http://lpis.ec.europa.eu/registry/applicationschema/cap-iacs-base/code#FarmStructureSurveyNumberValue/vineyardsOfWhichNormallyProducing -->


    <owl:NamedIndividual rdf:about="http://lpis.ec.europa.eu/registry/applicationschema/cap-iacs-base/code#FarmStructureSurveyNumberValue/vineyardsOfWhichNormallyProducing">
        <rdf:type rdf:resource="http://lpis.ec.europa.eu/registry/applicationschema/cap-iacs-base#FarmStructureSurveyNumberValue"/>
        <rdfs:label xml:lang="en">Vineyards, of which normally producing:</rdfs:label>
        <skos:definition xml:lang="en">-- Definition --
Vineyards, of which normally producing:
-- Description --
Plantations of Vitis vinifera L.
NOTE. Initial value:2.04.04</skos:definition>
        <skos:inScheme rdf:resource="http://lpis.ec.europa.eu/registry/applicationschema/cap-iacs-base/code#FarmStructureSurveyNumberValue"/>
    </owl:NamedIndividual>
    


    <!-- http://lpis.ec.europa.eu/registry/applicationschema/cap-iacs-base/code#FarmStructureSurveyNumberValue/woodedArea -->


    <owl:NamedIndividual rdf:about="http://lpis.ec.europa.eu/registry/applicationschema/cap-iacs-base/code#FarmStructureSurveyNumberValue/woodedArea">
        <rdf:type rdf:resource="http://lpis.ec.europa.eu/registry/applicationschema/cap-iacs-base#FarmStructureSurveyNumberValue"/>
        <rdfs:label xml:lang="en">Wooded area</rdfs:label>
        <skos:definition xml:lang="en">-- Definition --
Wooded area.
-- Description --
Areas covered with trees or forest shrubs, including poplar plantations inside or outside woods and forest-tree nurseries grown in woodland for the holding’s own requirements, as well as forest facilities (forest roads, storage depots for timber, etc.).
NOTE. Initial value:2.05.02</skos:definition>
        <skos:inScheme rdf:resource="http://lpis.ec.europa.eu/registry/applicationschema/cap-iacs-base/code#FarmStructureSurveyNumberValue"/>
    </owl:NamedIndividual>
    


    <!-- http://lpis.ec.europa.eu/registry/applicationschema/cap-iacs-base/code#MonthValue/april -->


    <owl:NamedIndividual rdf:about="http://lpis.ec.europa.eu/registry/applicationschema/cap-iacs-base/code#MonthValue/april">
        <rdf:type rdf:resource="http://lpis.ec.europa.eu/registry/applicationschema/cap-iacs-base#MonthValue"/>
        <rdfs:label xml:lang="en">April</rdfs:label>
        <skos:definition xml:lang="en">-- Definition --
April.
-- Description --
Item description.</skos:definition>
        <skos:inScheme rdf:resource="http://lpis.ec.europa.eu/registry/applicationschema/cap-iacs-base/code#MonthValue"/>
    </owl:NamedIndividual>
    


    <!-- http://lpis.ec.europa.eu/registry/applicationschema/cap-iacs-base/code#MonthValue/august -->


    <owl:NamedIndividual rdf:about="http://lpis.ec.europa.eu/registry/applicationschema/cap-iacs-base/code#MonthValue/august">
        <rdf:type rdf:resource="http://lpis.ec.europa.eu/registry/applicationschema/cap-iacs-base#MonthValue"/>
        <rdfs:label xml:lang="en">August</rdfs:label>
        <skos:definition xml:lang="en">-- Definition --
August.
-- Description --
Item description.</skos:definition>
        <skos:inScheme rdf:resource="http://lpis.ec.europa.eu/registry/applicationschema/cap-iacs-base/code#MonthValue"/>
    </owl:NamedIndividual>
    


    <!-- http://lpis.ec.europa.eu/registry/applicationschema/cap-iacs-base/code#MonthValue/december -->


    <owl:NamedIndividual rdf:about="http://lpis.ec.europa.eu/registry/applicationschema/cap-iacs-base/code#MonthValue/december">
        <rdf:type rdf:resource="http://lpis.ec.europa.eu/registry/applicationschema/cap-iacs-base#MonthValue"/>
        <rdfs:label xml:lang="en">December</rdfs:label>
        <skos:definition xml:lang="en">-- Definition --
December.
-- Description --
Item description.</skos:definition>
        <skos:inScheme rdf:resource="http://lpis.ec.europa.eu/registry/applicationschema/cap-iacs-base/code#MonthValue"/>
    </owl:NamedIndividual>
    


    <!-- http://lpis.ec.europa.eu/registry/applicationschema/cap-iacs-base/code#MonthValue/february -->


    <owl:NamedIndividual rdf:about="http://lpis.ec.europa.eu/registry/applicationschema/cap-iacs-base/code#MonthValue/february">
        <rdf:type rdf:resource="http://lpis.ec.europa.eu/registry/applicationschema/cap-iacs-base#MonthValue"/>
        <rdfs:label xml:lang="en">February</rdfs:label>
        <skos:definition xml:lang="en">-- Definition --
February.
-- Description --
Item description.</skos:definition>
        <skos:inScheme rdf:resource="http://lpis.ec.europa.eu/registry/applicationschema/cap-iacs-base/code#MonthValue"/>
    </owl:NamedIndividual>
    


    <!-- http://lpis.ec.europa.eu/registry/applicationschema/cap-iacs-base/code#MonthValue/january -->


    <owl:NamedIndividual rdf:about="http://lpis.ec.europa.eu/registry/applicationschema/cap-iacs-base/code#MonthValue/january">
        <rdf:type rdf:resource="http://lpis.ec.europa.eu/registry/applicationschema/cap-iacs-base#MonthValue"/>
        <rdfs:label xml:lang="en">January</rdfs:label>
        <skos:definition xml:lang="en">-- Definition --
January.
-- Description --
Item description.</skos:definition>
        <skos:inScheme rdf:resource="http://lpis.ec.europa.eu/registry/applicationschema/cap-iacs-base/code#MonthValue"/>
    </owl:NamedIndividual>
    


    <!-- http://lpis.ec.europa.eu/registry/applicationschema/cap-iacs-base/code#MonthValue/july -->


    <owl:NamedIndividual rdf:about="http://lpis.ec.europa.eu/registry/applicationschema/cap-iacs-base/code#MonthValue/july">
        <rdf:type rdf:resource="http://lpis.ec.europa.eu/registry/applicationschema/cap-iacs-base#MonthValue"/>
        <rdfs:label xml:lang="en">July</rdfs:label>
        <skos:definition xml:lang="en">-- Definition --
July.
-- Description --
Item description.</skos:definition>
        <skos:inScheme rdf:resource="http://lpis.ec.europa.eu/registry/applicationschema/cap-iacs-base/code#MonthValue"/>
    </owl:NamedIndividual>
    


    <!-- http://lpis.ec.europa.eu/registry/applicationschema/cap-iacs-base/code#MonthValue/june -->


    <owl:NamedIndividual rdf:about="http://lpis.ec.europa.eu/registry/applicationschema/cap-iacs-base/code#MonthValue/june">
        <rdf:type rdf:resource="http://lpis.ec.europa.eu/registry/applicationschema/cap-iacs-base#MonthValue"/>
        <rdfs:label xml:lang="en">June</rdfs:label>
        <skos:definition xml:lang="en">-- Definition --
June.
-- Description --
Item description.</skos:definition>
        <skos:inScheme rdf:resource="http://lpis.ec.europa.eu/registry/applicationschema/cap-iacs-base/code#MonthValue"/>
    </owl:NamedIndividual>
    


    <!-- http://lpis.ec.europa.eu/registry/applicationschema/cap-iacs-base/code#MonthValue/march -->


    <owl:NamedIndividual rdf:about="http://lpis.ec.europa.eu/registry/applicationschema/cap-iacs-base/code#MonthValue/march">
        <rdf:type rdf:resource="http://lpis.ec.europa.eu/registry/applicationschema/cap-iacs-base#MonthValue"/>
        <rdfs:label xml:lang="en">March</rdfs:label>
        <skos:definition xml:lang="en">-- Definition --
March.
-- Description --
Item description.</skos:definition>
        <skos:inScheme rdf:resource="http://lpis.ec.europa.eu/registry/applicationschema/cap-iacs-base/code#MonthValue"/>
    </owl:NamedIndividual>
    


    <!-- http://lpis.ec.europa.eu/registry/applicationschema/cap-iacs-base/code#MonthValue/may -->


    <owl:NamedIndividual rdf:about="http://lpis.ec.europa.eu/registry/applicationschema/cap-iacs-base/code#MonthValue/may">
        <rdf:type rdf:resource="http://lpis.ec.europa.eu/registry/applicationschema/cap-iacs-base#MonthValue"/>
        <rdfs:label xml:lang="en">May</rdfs:label>
        <skos:definition xml:lang="en">-- Definition --
May.
-- Description --
Item description.</skos:definition>
        <skos:inScheme rdf:resource="http://lpis.ec.europa.eu/registry/applicationschema/cap-iacs-base/code#MonthValue"/>
    </owl:NamedIndividual>
    


    <!-- http://lpis.ec.europa.eu/registry/applicationschema/cap-iacs-base/code#MonthValue/november -->


    <owl:NamedIndividual rdf:about="http://lpis.ec.europa.eu/registry/applicationschema/cap-iacs-base/code#MonthValue/november">
        <rdf:type rdf:resource="http://lpis.ec.europa.eu/registry/applicationschema/cap-iacs-base#MonthValue"/>
        <rdfs:label xml:lang="en">November</rdfs:label>
        <skos:definition xml:lang="en">-- Definition --
November.
-- Description --
Item description.</skos:definition>
        <skos:inScheme rdf:resource="http://lpis.ec.europa.eu/registry/applicationschema/cap-iacs-base/code#MonthValue"/>
    </owl:NamedIndividual>
    


    <!-- http://lpis.ec.europa.eu/registry/applicationschema/cap-iacs-base/code#MonthValue/october -->


    <owl:NamedIndividual rdf:about="http://lpis.ec.europa.eu/registry/applicationschema/cap-iacs-base/code#MonthValue/october">
        <rdf:type rdf:resource="http://lpis.ec.europa.eu/registry/applicationschema/cap-iacs-base#MonthValue"/>
        <rdfs:label xml:lang="en">October</rdfs:label>
        <skos:definition xml:lang="en">-- Definition --
October.
-- Description --
Item description.</skos:definition>
        <skos:inScheme rdf:resource="http://lpis.ec.europa.eu/registry/applicationschema/cap-iacs-base/code#MonthValue"/>
    </owl:NamedIndividual>
    


    <!-- http://lpis.ec.europa.eu/registry/applicationschema/cap-iacs-base/code#MonthValue/september -->


    <owl:NamedIndividual rdf:about="http://lpis.ec.europa.eu/registry/applicationschema/cap-iacs-base/code#MonthValue/september">
        <rdf:type rdf:resource="http://lpis.ec.europa.eu/registry/applicationschema/cap-iacs-base#MonthValue"/>
        <rdfs:label xml:lang="en">September</rdfs:label>
        <skos:definition xml:lang="en">-- Definition --
September.
-- Description --
Item description.</skos:definition>
        <skos:inScheme rdf:resource="http://lpis.ec.europa.eu/registry/applicationschema/cap-iacs-base/code#MonthValue"/>
    </owl:NamedIndividual>
    


    <!-- http://lpis.ec.europa.eu/registry/applicationschema/cap-iacs-base/code#NotificationGroupValue/notificationOnTheResultsOfOtsc -->


    <owl:NamedIndividual rdf:about="http://lpis.ec.europa.eu/registry/applicationschema/cap-iacs-base/code#NotificationGroupValue/notificationOnTheResultsOfOtsc">
        <rdf:type rdf:resource="http://lpis.ec.europa.eu/registry/applicationschema/cap-iacs-base#NotificationGroupValue"/>
        <rdfs:label xml:lang="en">Notifications concerning complementary national direct payments (BG and RO only)</rdfs:label>
        <skos:definition xml:lang="en">Notification on the results of OTSC

Each year, by 15 July, for all direct payment schemes, rural development measures and technical assistance and support schemes in the wine sector Member States shall notify the Commission of the control data and control statistics covering results of administrative, on-the-spot checks and ex post checks [Art. 9(1)(a) of R 809/2014].</skos:definition>
        <skos:inScheme rdf:resource="http://lpis.ec.europa.eu/registry/applicationschema/cap-iacs-base/code#NotificationGroupValue"/>
    </owl:NamedIndividual>
    


    <!-- http://lpis.ec.europa.eu/registry/applicationschema/cap-iacs-base/code#NotificationGroupValue/notificationsConcerningAdjustmentRateForAGroupAtTheLevelOfItsMembers -->


    <owl:NamedIndividual rdf:about="http://lpis.ec.europa.eu/registry/applicationschema/cap-iacs-base/code#NotificationGroupValue/notificationsConcerningAdjustmentRateForAGroupAtTheLevelOfItsMembers">
        <rdf:type rdf:resource="http://lpis.ec.europa.eu/registry/applicationschema/cap-iacs-base#NotificationGroupValue"/>
        <rdfs:label xml:lang="en">Notifications concerning adjustment rate for a group at the level of its members</rdfs:label>
        <skos:definition xml:lang="en">-- Definition --
Notifications concerning adjustment rate for a group at the level of its members
-- Description --
NOTE.71</skos:definition>
        <skos:inScheme rdf:resource="http://lpis.ec.europa.eu/registry/applicationschema/cap-iacs-base/code#NotificationGroupValue"/>
    </owl:NamedIndividual>
    


    <!-- http://lpis.ec.europa.eu/registry/applicationschema/cap-iacs-base/code#NotificationGroupValue/notificationsConcerningAnyAdditionalDetailsToBeProvidedOnRequest -->


    <owl:NamedIndividual rdf:about="http://lpis.ec.europa.eu/registry/applicationschema/cap-iacs-base/code#NotificationGroupValue/notificationsConcerningAnyAdditionalDetailsToBeProvidedOnRequest">
        <rdf:type rdf:resource="http://lpis.ec.europa.eu/registry/applicationschema/cap-iacs-base#NotificationGroupValue"/>
        <rdfs:label xml:lang="en">Notifications concerning any additional details to be provided on request</rdfs:label>
        <skos:definition xml:lang="en">-- Definition --
Notifications concerning any additional details to be provided on request.
-- Description --
NOTE.721</skos:definition>
        <skos:inScheme rdf:resource="http://lpis.ec.europa.eu/registry/applicationschema/cap-iacs-base/code#NotificationGroupValue"/>
    </owl:NamedIndividual>
    


    <!-- http://lpis.ec.europa.eu/registry/applicationschema/cap-iacs-base/code#NotificationGroupValue/notificationsConcerningApplicationOfLinearReductions -->


    <owl:NamedIndividual rdf:about="http://lpis.ec.europa.eu/registry/applicationschema/cap-iacs-base/code#NotificationGroupValue/notificationsConcerningApplicationOfLinearReductions">
        <rdf:type rdf:resource="http://lpis.ec.europa.eu/registry/applicationschema/cap-iacs-base#NotificationGroupValue"/>
        <rdfs:label xml:lang="en">Notifications concerning application of linear reductions</rdfs:label>
        <skos:definition xml:lang="en">-- Definition --
Notifications concerning application of linear reductions.
-- Description --
NOTE.72</skos:definition>
        <skos:inScheme rdf:resource="http://lpis.ec.europa.eu/registry/applicationschema/cap-iacs-base/code#NotificationGroupValue"/>
    </owl:NamedIndividual>
    


    <!-- http://lpis.ec.europa.eu/registry/applicationschema/cap-iacs-base/code#NotificationGroupValue/notificationsConcerningComplementaryNationalDirectPaymentsBgRo -->


    <owl:NamedIndividual rdf:about="http://lpis.ec.europa.eu/registry/applicationschema/cap-iacs-base/code#NotificationGroupValue/notificationsConcerningComplementaryNationalDirectPaymentsBgRo">
        <rdf:type rdf:resource="http://lpis.ec.europa.eu/registry/applicationschema/cap-iacs-base#NotificationGroupValue"/>
        <rdfs:label xml:lang="en">Notifications concerning complementary national direct payments (BG and RO only)</rdfs:label>
        <skos:definition xml:lang="en">-- Definition --
Notifications concerning complementary national direct payments (BG and RO only).
-- Description --
NOTE.73</skos:definition>
        <skos:inScheme rdf:resource="http://lpis.ec.europa.eu/registry/applicationschema/cap-iacs-base/code#NotificationGroupValue"/>
    </owl:NamedIndividual>
    


    <!-- http://lpis.ec.europa.eu/registry/applicationschema/cap-iacs-base/code#NotificationGroupValue/notificationsConcerningTheMinimumRequirementsForReceivingDirectPayments -->


    <owl:NamedIndividual rdf:about="http://lpis.ec.europa.eu/registry/applicationschema/cap-iacs-base/code#NotificationGroupValue/notificationsConcerningTheMinimumRequirementsForReceivingDirectPayments">
        <rdf:type rdf:resource="http://lpis.ec.europa.eu/registry/applicationschema/cap-iacs-base#NotificationGroupValue"/>
        <rdfs:label xml:lang="en">Notifications concerning the minimum requirements for receiving direct payments</rdfs:label>
        <skos:definition xml:lang="en">-- Definition --
Notifications concerning the minimum requirements for receiving direct payments.
-- Description --
NOTE.67</skos:definition>
        <skos:inScheme rdf:resource="http://lpis.ec.europa.eu/registry/applicationschema/cap-iacs-base/code#NotificationGroupValue"/>
    </owl:NamedIndividual>
    


    <!-- http://lpis.ec.europa.eu/registry/applicationschema/cap-iacs-base/code#NotificationGroupValue/notificationsConcerningThePaymentForAreasWithNaturalConstraints -->


    <owl:NamedIndividual rdf:about="http://lpis.ec.europa.eu/registry/applicationschema/cap-iacs-base/code#NotificationGroupValue/notificationsConcerningThePaymentForAreasWithNaturalConstraints">
        <rdf:type rdf:resource="http://lpis.ec.europa.eu/registry/applicationschema/cap-iacs-base#NotificationGroupValue"/>
        <rdfs:label xml:lang="en">Notifications concerning the payment for areas with natural constraints</rdfs:label>
        <skos:definition xml:lang="en">-- Definition --
Notifications concerning the payment for areas with natural constraints.
-- Description --
NOTE.69</skos:definition>
        <skos:inScheme rdf:resource="http://lpis.ec.europa.eu/registry/applicationschema/cap-iacs-base/code#NotificationGroupValue"/>
    </owl:NamedIndividual>
    


    <!-- http://lpis.ec.europa.eu/registry/applicationschema/cap-iacs-base/code#NotificationGroupValue/notificationsConcerningThePriorApprovaSystemForHempCultivation -->


    <owl:NamedIndividual rdf:about="http://lpis.ec.europa.eu/registry/applicationschema/cap-iacs-base/code#NotificationGroupValue/notificationsConcerningThePriorApprovaSystemForHempCultivation">
        <rdf:type rdf:resource="http://lpis.ec.europa.eu/registry/applicationschema/cap-iacs-base#NotificationGroupValue"/>
        <rdfs:label xml:lang="en">Notifications concerning the small farmers scheme</rdfs:label>
        <skos:definition xml:lang="en">Notifications concerning the prior approval system for hemp cultivation</skos:definition>
        <skos:inScheme rdf:resource="http://lpis.ec.europa.eu/registry/applicationschema/cap-iacs-base/code#NotificationGroupValue"/>
    </owl:NamedIndividual>
    


    <!-- http://lpis.ec.europa.eu/registry/applicationschema/cap-iacs-base/code#NotificationGroupValue/notificationsConcerningTheRedistributivePayment -->


    <owl:NamedIndividual rdf:about="http://lpis.ec.europa.eu/registry/applicationschema/cap-iacs-base/code#NotificationGroupValue/notificationsConcerningTheRedistributivePayment">
        <rdf:type rdf:resource="http://lpis.ec.europa.eu/registry/applicationschema/cap-iacs-base#NotificationGroupValue"/>
        <rdfs:label xml:lang="en">Notifications concerning the redistributive payment</rdfs:label>
        <skos:definition xml:lang="en">-- Definition --
Notifications concerning the redistributive payment.
-- Description --
NOTE.68</skos:definition>
        <skos:inScheme rdf:resource="http://lpis.ec.europa.eu/registry/applicationschema/cap-iacs-base/code#NotificationGroupValue"/>
    </owl:NamedIndividual>
    


    <!-- http://lpis.ec.europa.eu/registry/applicationschema/cap-iacs-base/code#NotificationGroupValue/notificationsConcerningTheSmallFarmersScheme -->


    <owl:NamedIndividual rdf:about="http://lpis.ec.europa.eu/registry/applicationschema/cap-iacs-base/code#NotificationGroupValue/notificationsConcerningTheSmallFarmersScheme">
        <rdf:type rdf:resource="http://lpis.ec.europa.eu/registry/applicationschema/cap-iacs-base#NotificationGroupValue"/>
        <rdfs:label xml:lang="en">Notifications concerning the small farmers scheme</rdfs:label>
        <skos:definition xml:lang="en">-- Definition --
Notifications concerning the small farmers scheme.
-- Description --
NOTE.70</skos:definition>
        <skos:inScheme rdf:resource="http://lpis.ec.europa.eu/registry/applicationschema/cap-iacs-base/code#NotificationGroupValue"/>
    </owl:NamedIndividual>
    


    <!-- http://lpis.ec.europa.eu/registry/applicationschema/cap-iacs-base/code#NotificationGroupValue/notificationsConcerningTheValueOfPaymentEntitlementsSpsAndConvergence -->


    <owl:NamedIndividual rdf:about="http://lpis.ec.europa.eu/registry/applicationschema/cap-iacs-base/code#NotificationGroupValue/notificationsConcerningTheValueOfPaymentEntitlementsSpsAndConvergence">
        <rdf:type rdf:resource="http://lpis.ec.europa.eu/registry/applicationschema/cap-iacs-base#NotificationGroupValue"/>
        <rdfs:label xml:lang="en">Notifications concerning the value of payment entitlements (SPS) and convergence</rdfs:label>
        <skos:definition xml:lang="en">-- Definition --
Notifications concerning the value of payment entitlements (SPS) and convergence.
-- Description --
NOTE.76</skos:definition>
        <skos:inScheme rdf:resource="http://lpis.ec.europa.eu/registry/applicationschema/cap-iacs-base/code#NotificationGroupValue"/>
    </owl:NamedIndividual>
    


    <!-- http://lpis.ec.europa.eu/registry/applicationschema/cap-iacs-base/code#NotificationGroupValue/notificationsRelatingDecisionsToReviewOfPreviousNotifications -->


    <owl:NamedIndividual rdf:about="http://lpis.ec.europa.eu/registry/applicationschema/cap-iacs-base/code#NotificationGroupValue/notificationsRelatingDecisionsToReviewOfPreviousNotifications">
        <rdf:type rdf:resource="http://lpis.ec.europa.eu/registry/applicationschema/cap-iacs-base#NotificationGroupValue"/>
        <rdfs:label xml:lang="en">Notifications relating decisions to review of previous notifications</rdfs:label>
        <skos:definition xml:lang="en">-- Definition --
Notifications relating decisions to review of previous notifications.
-- Description --
NOTE.75</skos:definition>
        <skos:inScheme rdf:resource="http://lpis.ec.europa.eu/registry/applicationschema/cap-iacs-base/code#NotificationGroupValue"/>
    </owl:NamedIndividual>
    


    <!-- http://lpis.ec.europa.eu/registry/applicationschema/cap-iacs-base/code#NotificationGroupValue/notificationsRelatingToDefinitionsAndRelatedProvisions -->


    <owl:NamedIndividual rdf:about="http://lpis.ec.europa.eu/registry/applicationschema/cap-iacs-base/code#NotificationGroupValue/notificationsRelatingToDefinitionsAndRelatedProvisions">
        <rdf:type rdf:resource="http://lpis.ec.europa.eu/registry/applicationschema/cap-iacs-base#NotificationGroupValue"/>
        <rdfs:label xml:lang="en">Notifications relating to definitions and related provisions</rdfs:label>
        <skos:definition xml:lang="en">-- Definition --
Notifications relating to definitions and related provisions.
-- Description --
NOTE.61</skos:definition>
        <skos:inScheme rdf:resource="http://lpis.ec.europa.eu/registry/applicationschema/cap-iacs-base/code#NotificationGroupValue"/>
    </owl:NamedIndividual>
    


    <!-- http://lpis.ec.europa.eu/registry/applicationschema/cap-iacs-base/code#NotificationGroupValue/notificationsRelatingToGreening -->


    <owl:NamedIndividual rdf:about="http://lpis.ec.europa.eu/registry/applicationschema/cap-iacs-base/code#NotificationGroupValue/notificationsRelatingToGreening">
        <rdf:type rdf:resource="http://lpis.ec.europa.eu/registry/applicationschema/cap-iacs-base#NotificationGroupValue"/>
        <rdfs:label xml:lang="en">Notifications relating to greening</rdfs:label>
        <skos:definition xml:lang="en">-- Definition --
Notifications relating to greening.
-- Description --
NOTE.64</skos:definition>
        <skos:inScheme rdf:resource="http://lpis.ec.europa.eu/registry/applicationschema/cap-iacs-base/code#NotificationGroupValue"/>
    </owl:NamedIndividual>
    


    <!-- http://lpis.ec.europa.eu/registry/applicationschema/cap-iacs-base/code#NotificationGroupValue/notificationsRelatingToSapsDecisionsOnTransitionalNationalAid -->


    <owl:NamedIndividual rdf:about="http://lpis.ec.europa.eu/registry/applicationschema/cap-iacs-base/code#NotificationGroupValue/notificationsRelatingToSapsDecisionsOnTransitionalNationalAid">
        <rdf:type rdf:resource="http://lpis.ec.europa.eu/registry/applicationschema/cap-iacs-base#NotificationGroupValue"/>
        <rdfs:label xml:lang="en">Notifications relating to SAPS decisions on transitional national aid</rdfs:label>
        <skos:definition xml:lang="en">-- Definition --
Notifications relating to SAPS decisions on transitional national aid.
-- Description --
NOTE.74</skos:definition>
        <skos:inScheme rdf:resource="http://lpis.ec.europa.eu/registry/applicationschema/cap-iacs-base/code#NotificationGroupValue"/>
    </owl:NamedIndividual>
    


    <!-- http://lpis.ec.europa.eu/registry/applicationschema/cap-iacs-base/code#NotificationGroupValue/notificationsRelatingToTheAccreditedPayingAgenciesAndCoordinatingBodies -->


    <owl:NamedIndividual rdf:about="http://lpis.ec.europa.eu/registry/applicationschema/cap-iacs-base/code#NotificationGroupValue/notificationsRelatingToTheAccreditedPayingAgenciesAndCoordinatingBodies">
        <rdf:type rdf:resource="http://lpis.ec.europa.eu/registry/applicationschema/cap-iacs-base#NotificationGroupValue"/>
        <rdfs:label xml:lang="en">Notifications relating to the accredited paying agencies and coordinating bodies</rdfs:label>
        <skos:definition xml:lang="en">-- Definition --
Notifications relating to the accredited paying agencies and coordinating bodies.
-- Description --
In addition to the provisions laid down in the sectoral Regulations, Member States shall send to the Commission the information, declarations and documents: for accredited paying agencies and accredited coordinating bodies
(a)(i) their accreditation document;
(a)(ii) their function (accredited paying agency or accredited coordinating body);
(a)(iii) where relevant, the withdrawal of their accreditation.
NOTE.1011a</skos:definition>
        <skos:inScheme rdf:resource="http://lpis.ec.europa.eu/registry/applicationschema/cap-iacs-base/code#NotificationGroupValue"/>
    </owl:NamedIndividual>
    


    <!-- http://lpis.ec.europa.eu/registry/applicationschema/cap-iacs-base/code#NotificationGroupValue/notificationsRelatingToTheApplicationOfTheIntegratedSystem -->


    <owl:NamedIndividual rdf:about="http://lpis.ec.europa.eu/registry/applicationschema/cap-iacs-base/code#NotificationGroupValue/notificationsRelatingToTheApplicationOfTheIntegratedSystem">
        <rdf:type rdf:resource="http://lpis.ec.europa.eu/registry/applicationschema/cap-iacs-base#NotificationGroupValue"/>
        <rdfs:label xml:lang="en">Notifications relating to the application of the integrated system</rdfs:label>
        <skos:definition xml:lang="en">-- Definition --
Notifications relating to the the application of the integrated system.
-- Description --
Member State shall inform the Commission regularly of the application of the integrated system referred to in Chapter II of Title V. The Commission shall organize exchanges of views on this subject with the Member States.
NOTE.1023</skos:definition>
        <skos:inScheme rdf:resource="http://lpis.ec.europa.eu/registry/applicationschema/cap-iacs-base/code#NotificationGroupValue"/>
    </owl:NamedIndividual>
    


    <!-- http://lpis.ec.europa.eu/registry/applicationschema/cap-iacs-base/code#NotificationGroupValue/notificationsRelatingToTheBasicPayment -->


    <owl:NamedIndividual rdf:about="http://lpis.ec.europa.eu/registry/applicationschema/cap-iacs-base/code#NotificationGroupValue/notificationsRelatingToTheBasicPayment">
        <rdf:type rdf:resource="http://lpis.ec.europa.eu/registry/applicationschema/cap-iacs-base#NotificationGroupValue"/>
        <rdfs:label xml:lang="en">Notifications relating to the basic payment</rdfs:label>
        <skos:definition xml:lang="en">-- Definition --
Notifications relating to the basic payment.
-- Description --
NOTE.63</skos:definition>
        <skos:inScheme rdf:resource="http://lpis.ec.europa.eu/registry/applicationschema/cap-iacs-base/code#NotificationGroupValue"/>
    </owl:NamedIndividual>
    


    <!-- http://lpis.ec.europa.eu/registry/applicationschema/cap-iacs-base/code#NotificationGroupValue/notificationsRelatingToTheCertificationBodies -->


    <owl:NamedIndividual rdf:about="http://lpis.ec.europa.eu/registry/applicationschema/cap-iacs-base/code#NotificationGroupValue/notificationsRelatingToTheCertificationBodies">
        <rdf:type rdf:resource="http://lpis.ec.europa.eu/registry/applicationschema/cap-iacs-base#NotificationGroupValue"/>
        <rdfs:label xml:lang="en">Notifications relating to the certification bodies</rdfs:label>
        <skos:definition xml:lang="en">-- Definition --
Notifications relating to the certification bodies.
-- Description --
In addition to the provisions laid down in the sectoral Regulations, Member States shall send to the Commission the information, declarations and documents:  for certification bodies:
(b)(i) their name;
(b)(ii) their address,
NOTE.1011b</skos:definition>
        <skos:inScheme rdf:resource="http://lpis.ec.europa.eu/registry/applicationschema/cap-iacs-base/code#NotificationGroupValue"/>
    </owl:NamedIndividual>
    


    <!-- http://lpis.ec.europa.eu/registry/applicationschema/cap-iacs-base/code#NotificationGroupValue/notificationsRelatingToTheFinancialAdjustmentsMadeByMemberStatesInConnectionWithRuralDevelopment -->


    <owl:NamedIndividual rdf:about="http://lpis.ec.europa.eu/registry/applicationschema/cap-iacs-base/code#NotificationGroupValue/notificationsRelatingToTheFinancialAdjustmentsMadeByMemberStatesInConnectionWithRuralDevelopment">
        <rdf:type rdf:resource="http://lpis.ec.europa.eu/registry/applicationschema/cap-iacs-base#NotificationGroupValue"/>
        <rdfs:label xml:lang="en">Notifications relating to the financial adjustments made by Member States in connection with rural development</rdfs:label>
        <skos:definition xml:lang="en">-- Definition --
Notifications relating to the financial adjustments made by Member States in connection with rural development.
-- Description --
NOTE.104</skos:definition>
        <skos:inScheme rdf:resource="http://lpis.ec.europa.eu/registry/applicationschema/cap-iacs-base/code#NotificationGroupValue"/>
    </owl:NamedIndividual>
    


    <!-- http://lpis.ec.europa.eu/registry/applicationschema/cap-iacs-base/code#NotificationGroupValue/notificationsRelatingToTheImplementationOfGaecAndFas -->


    <owl:NamedIndividual rdf:about="http://lpis.ec.europa.eu/registry/applicationschema/cap-iacs-base/code#NotificationGroupValue/notificationsRelatingToTheImplementationOfGaecAndFas">
        <rdf:type rdf:resource="http://lpis.ec.europa.eu/registry/applicationschema/cap-iacs-base#NotificationGroupValue"/>
        <rdfs:label xml:lang="en">Notifications relating to the implementation of GAEC and FAS</rdfs:label>
        <skos:definition xml:lang="en">-- Definition --
Notifications relating to the implementation of GAEC and FAS.
-- Description --
Member States shall inform the Commission in detail of the measures taken to implement the good agricultural and environmental condition referred to in Article 94 and the details of the farm advisory system referred to in Title 
III.
NOTE.1012</skos:definition>
        <skos:inScheme rdf:resource="http://lpis.ec.europa.eu/registry/applicationschema/cap-iacs-base/code#NotificationGroupValue"/>
    </owl:NamedIndividual>
    


    <!-- http://lpis.ec.europa.eu/registry/applicationschema/cap-iacs-base/code#NotificationGroupValue/notificationsRelatingToTheMeasuresRelatedToOperationsFinancedByTheFunds -->


    <owl:NamedIndividual rdf:about="http://lpis.ec.europa.eu/registry/applicationschema/cap-iacs-base/code#NotificationGroupValue/notificationsRelatingToTheMeasuresRelatedToOperationsFinancedByTheFunds">
        <rdf:type rdf:resource="http://lpis.ec.europa.eu/registry/applicationschema/cap-iacs-base#NotificationGroupValue"/>
        <rdfs:label xml:lang="en">Notifications relating to the  measures related to operations financed by the Funds</rdfs:label>
        <skos:definition xml:lang="en">-- Definition --
Notifications relating to the  measures related to operations financed by the Funds.
-- Description --
In addition to the provisions laid down in the sectoral Regulations, Member States shall send to the Commission the information, declarations and documents:  for measures relating to operations financed by the Funds:
(c)(i) declarations of expenditure, which also act as payment requests, signed by the accredited paying agency or the accredited coordinating body and accompanied by the requisite information;
(c)(ii) estimates of their financial requirements, with regard to the EAGF and, with regard to the EAFRD, an update of estimated declarations of expenditure which will be submitted during the year and estimated declarations of 
expenditure in respect of the following financial year;
(c)(iii) the management declaration and the annual accounts of the accredited paying agencies;
(c)(iv) an annual summary of the results of all available audits and checks carried out in accordance with the schedule and detailed provisions laid down in the sector specific rules.
The annual accounts of accredited paying agencies relating to EAFRD expenditure shall be submitted at the level of each programme.
NOTE.1011c</skos:definition>
        <skos:inScheme rdf:resource="http://lpis.ec.europa.eu/registry/applicationschema/cap-iacs-base/code#NotificationGroupValue"/>
    </owl:NamedIndividual>
    


    <!-- http://lpis.ec.europa.eu/registry/applicationschema/cap-iacs-base/code#NotificationGroupValue/notificationsRelatingToThePaymentForYoungFarmers -->


    <owl:NamedIndividual rdf:about="http://lpis.ec.europa.eu/registry/applicationschema/cap-iacs-base/code#NotificationGroupValue/notificationsRelatingToThePaymentForYoungFarmers">
        <rdf:type rdf:resource="http://lpis.ec.europa.eu/registry/applicationschema/cap-iacs-base#NotificationGroupValue"/>
        <rdfs:label xml:lang="en">Notifications relating to the payment for young farmers</rdfs:label>
        <skos:definition xml:lang="en">-- Definition --
Notifications relating to the payment for young farmers.
-- Description --
NOTE.65</skos:definition>
        <skos:inScheme rdf:resource="http://lpis.ec.europa.eu/registry/applicationschema/cap-iacs-base/code#NotificationGroupValue"/>
    </owl:NamedIndividual>
    


    <!-- http://lpis.ec.europa.eu/registry/applicationschema/cap-iacs-base/code#NotificationGroupValue/notificationsRelatingToTheReductionCoefficient -->


    <owl:NamedIndividual rdf:about="http://lpis.ec.europa.eu/registry/applicationschema/cap-iacs-base/code#NotificationGroupValue/notificationsRelatingToTheReductionCoefficient">
        <rdf:type rdf:resource="http://lpis.ec.europa.eu/registry/applicationschema/cap-iacs-base#NotificationGroupValue"/>
        <rdfs:label xml:lang="en">Notifications relating to the reduction coefficient</rdfs:label>
        <skos:definition xml:lang="en">-- Definition --
Notifications relating to the reduction coefficient.
-- Description --
NOTE.62</skos:definition>
        <skos:inScheme rdf:resource="http://lpis.ec.europa.eu/registry/applicationschema/cap-iacs-base/code#NotificationGroupValue"/>
    </owl:NamedIndividual>
    


    <!-- http://lpis.ec.europa.eu/registry/applicationschema/cap-iacs-base/code#NotificationGroupValue/notificationsRelatingToTheVoluntaryCoupledSupport -->


    <owl:NamedIndividual rdf:about="http://lpis.ec.europa.eu/registry/applicationschema/cap-iacs-base/code#NotificationGroupValue/notificationsRelatingToTheVoluntaryCoupledSupport">
        <rdf:type rdf:resource="http://lpis.ec.europa.eu/registry/applicationschema/cap-iacs-base#NotificationGroupValue"/>
        <rdfs:label xml:lang="en">Notifications relating to the voluntary coupled support</rdfs:label>
        <skos:definition xml:lang="en">-- Definition --
Notifications relating to the voluntary coupled support.
-- Description --
NOTE.66</skos:definition>
        <skos:inScheme rdf:resource="http://lpis.ec.europa.eu/registry/applicationschema/cap-iacs-base/code#NotificationGroupValue"/>
    </owl:NamedIndividual>
    


    <!-- http://lpis.ec.europa.eu/registry/applicationschema/cap-iacs-base/code#OrdinalNumberValue/first -->


    <owl:NamedIndividual rdf:about="http://lpis.ec.europa.eu/registry/applicationschema/cap-iacs-base/code#OrdinalNumberValue/first">
        <rdf:type rdf:resource="http://lpis.ec.europa.eu/registry/applicationschema/cap-iacs-base#OrdinalNumberValue"/>
        <rdfs:label xml:lang="en">First</rdfs:label>
        <skos:definition xml:lang="en">-- Definition --
First.
-- Description --
Item description.</skos:definition>
        <skos:inScheme rdf:resource="http://lpis.ec.europa.eu/registry/applicationschema/cap-iacs-base/code#OrdinalNumberValue"/>
    </owl:NamedIndividual>
    


    <!-- http://lpis.ec.europa.eu/registry/applicationschema/cap-iacs-base/code#OrdinalNumberValue/fourth -->


    <owl:NamedIndividual rdf:about="http://lpis.ec.europa.eu/registry/applicationschema/cap-iacs-base/code#OrdinalNumberValue/fourth">
        <rdf:type rdf:resource="http://lpis.ec.europa.eu/registry/applicationschema/cap-iacs-base#OrdinalNumberValue"/>
        <rdfs:label xml:lang="en">Fourth</rdfs:label>
        <skos:definition xml:lang="en">-- Definition --
Fourth.
-- Description --
Item description.</skos:definition>
        <skos:inScheme rdf:resource="http://lpis.ec.europa.eu/registry/applicationschema/cap-iacs-base/code#OrdinalNumberValue"/>
    </owl:NamedIndividual>
    


    <!-- http://lpis.ec.europa.eu/registry/applicationschema/cap-iacs-base/code#OrdinalNumberValue/last -->


    <owl:NamedIndividual rdf:about="http://lpis.ec.europa.eu/registry/applicationschema/cap-iacs-base/code#OrdinalNumberValue/last">
        <rdf:type rdf:resource="http://lpis.ec.europa.eu/registry/applicationschema/cap-iacs-base#OrdinalNumberValue"/>
        <rdfs:label xml:lang="en">Last</rdfs:label>
        <skos:definition xml:lang="en">-- Definition --
Last.
-- Description --
Item description.</skos:definition>
        <skos:inScheme rdf:resource="http://lpis.ec.europa.eu/registry/applicationschema/cap-iacs-base/code#OrdinalNumberValue"/>
    </owl:NamedIndividual>
    


    <!-- http://lpis.ec.europa.eu/registry/applicationschema/cap-iacs-base/code#OrdinalNumberValue/second -->


    <owl:NamedIndividual rdf:about="http://lpis.ec.europa.eu/registry/applicationschema/cap-iacs-base/code#OrdinalNumberValue/second">
        <rdf:type rdf:resource="http://lpis.ec.europa.eu/registry/applicationschema/cap-iacs-base#OrdinalNumberValue"/>
        <rdfs:label xml:lang="en">Second</rdfs:label>
        <skos:definition xml:lang="en">-- Definition --
Second.
-- Description --
Item description.</skos:definition>
        <skos:inScheme rdf:resource="http://lpis.ec.europa.eu/registry/applicationschema/cap-iacs-base/code#OrdinalNumberValue"/>
    </owl:NamedIndividual>
    


    <!-- http://lpis.ec.europa.eu/registry/applicationschema/cap-iacs-base/code#OrdinalNumberValue/third -->


    <owl:NamedIndividual rdf:about="http://lpis.ec.europa.eu/registry/applicationschema/cap-iacs-base/code#OrdinalNumberValue/third">
        <rdf:type rdf:resource="http://lpis.ec.europa.eu/registry/applicationschema/cap-iacs-base#OrdinalNumberValue"/>
        <rdfs:label xml:lang="en">Third</rdfs:label>
        <skos:definition xml:lang="en">-- Definition --
Third.
-- Description --
Item description.</skos:definition>
        <skos:inScheme rdf:resource="http://lpis.ec.europa.eu/registry/applicationschema/cap-iacs-base/code#OrdinalNumberValue"/>
    </owl:NamedIndividual>
    


    <!-- http://lpis.ec.europa.eu/registry/applicationschema/cap-iacs-base/code#RecurenceValue/daily -->


    <owl:NamedIndividual rdf:about="http://lpis.ec.europa.eu/registry/applicationschema/cap-iacs-base/code#RecurenceValue/daily">
        <rdf:type rdf:resource="http://lpis.ec.europa.eu/registry/applicationschema/cap-iacs-base#RecurenceValue"/>
        <rdfs:label xml:lang="en">Daily recurrence</rdfs:label>
        <skos:definition xml:lang="en">-- Definition --
Daily recurrence.
-- Description --
Item description.</skos:definition>
        <skos:inScheme rdf:resource="http://lpis.ec.europa.eu/registry/applicationschema/cap-iacs-base/code#RecurenceValue"/>
    </owl:NamedIndividual>
    


    <!-- http://lpis.ec.europa.eu/registry/applicationschema/cap-iacs-base/code#RecurenceValue/monthly -->


    <owl:NamedIndividual rdf:about="http://lpis.ec.europa.eu/registry/applicationschema/cap-iacs-base/code#RecurenceValue/monthly">
        <rdf:type rdf:resource="http://lpis.ec.europa.eu/registry/applicationschema/cap-iacs-base#RecurenceValue"/>
        <rdfs:label xml:lang="en">Monthly recurrence</rdfs:label>
        <skos:definition xml:lang="en">-- Definition --
Monthly recurrence.
-- Description --
Item description.</skos:definition>
        <skos:inScheme rdf:resource="http://lpis.ec.europa.eu/registry/applicationschema/cap-iacs-base/code#RecurenceValue"/>
    </owl:NamedIndividual>
    


    <!-- http://lpis.ec.europa.eu/registry/applicationschema/cap-iacs-base/code#RecurenceValue/noRecurrence -->


    <owl:NamedIndividual rdf:about="http://lpis.ec.europa.eu/registry/applicationschema/cap-iacs-base/code#RecurenceValue/noRecurrence">
        <rdf:type rdf:resource="http://lpis.ec.europa.eu/registry/applicationschema/cap-iacs-base#RecurenceValue"/>
        <rdfs:label xml:lang="en">No recurrence</rdfs:label>
        <skos:definition xml:lang="en">-- Definition --
No recurrence.
-- Description --
Item description.</skos:definition>
        <skos:inScheme rdf:resource="http://lpis.ec.europa.eu/registry/applicationschema/cap-iacs-base/code#RecurenceValue"/>
    </owl:NamedIndividual>
    


    <!-- http://lpis.ec.europa.eu/registry/applicationschema/cap-iacs-base/code#RecurenceValue/weekly -->


    <owl:NamedIndividual rdf:about="http://lpis.ec.europa.eu/registry/applicationschema/cap-iacs-base/code#RecurenceValue/weekly">
        <rdf:type rdf:resource="http://lpis.ec.europa.eu/registry/applicationschema/cap-iacs-base#RecurenceValue"/>
        <rdfs:label xml:lang="en">Weekly recurrence</rdfs:label>
        <skos:definition xml:lang="en">-- Definition --
Weekly recurrence.
-- Description --
Item description.</skos:definition>
        <skos:inScheme rdf:resource="http://lpis.ec.europa.eu/registry/applicationschema/cap-iacs-base/code#RecurenceValue"/>
    </owl:NamedIndividual>
    


    <!-- http://lpis.ec.europa.eu/registry/applicationschema/cap-iacs-base/code#RecurenceValue/yearly -->


    <owl:NamedIndividual rdf:about="http://lpis.ec.europa.eu/registry/applicationschema/cap-iacs-base/code#RecurenceValue/yearly">
        <rdf:type rdf:resource="http://lpis.ec.europa.eu/registry/applicationschema/cap-iacs-base#RecurenceValue"/>
        <rdfs:label xml:lang="en">Yearly recurrence</rdfs:label>
        <skos:definition xml:lang="en">-- Definition --
Yearly recurrence.
-- Description --
Item description.</skos:definition>
        <skos:inScheme rdf:resource="http://lpis.ec.europa.eu/registry/applicationschema/cap-iacs-base/code#RecurenceValue"/>
    </owl:NamedIndividual>
    


    <!-- http://lpis.ec.europa.eu/registry/applicationschema/cap-iacs-base/code#SpecieCodeValue/agrostisCaninaLVelvetBent -->


    <owl:NamedIndividual rdf:about="http://lpis.ec.europa.eu/registry/applicationschema/cap-iacs-base/code#SpecieCodeValue/agrostisCaninaLVelvetBent">
        <rdf:type rdf:resource="http://lpis.ec.europa.eu/registry/applicationschema/cap-iacs-base#SpecieCodeValue"/>
        <rdfs:label xml:lang="en">Agrostis canina L. Velvet bent</rdfs:label>
        <skos:definition xml:lang="en">-- Definition --
Agrostis canina L. Velvet bent.
-- Description --
List of agricultural species -A
II. Fodder plants
NOTE. Initial value: A - 3.</skos:definition>
        <skos:inScheme rdf:resource="http://lpis.ec.europa.eu/registry/applicationschema/cap-iacs-base/code#SpecieCodeValue"/>
    </owl:NamedIndividual>
    


    <!-- http://lpis.ec.europa.eu/registry/applicationschema/cap-iacs-base/code#SpecieCodeValue/agrostisCapillarisLBrownTop -->


    <owl:NamedIndividual rdf:about="http://lpis.ec.europa.eu/registry/applicationschema/cap-iacs-base/code#SpecieCodeValue/agrostisCapillarisLBrownTop">
        <rdf:type rdf:resource="http://lpis.ec.europa.eu/registry/applicationschema/cap-iacs-base#SpecieCodeValue"/>
        <rdfs:label xml:lang="en">Agrostis capillaris L. Brown top</rdfs:label>
        <skos:definition xml:lang="en">-- Definition --
Agrostis capillaris L. Brown top.
-- Description --
List of agricultural species -A
II. Fodder plants
NOTE. Initial value: A - 6.</skos:definition>
        <skos:inScheme rdf:resource="http://lpis.ec.europa.eu/registry/applicationschema/cap-iacs-base/code#SpecieCodeValue"/>
    </owl:NamedIndividual>
    


    <!-- http://lpis.ec.europa.eu/registry/applicationschema/cap-iacs-base/code#SpecieCodeValue/agrostisGiganteaLRedTop -->


    <owl:NamedIndividual rdf:about="http://lpis.ec.europa.eu/registry/applicationschema/cap-iacs-base/code#SpecieCodeValue/agrostisGiganteaLRedTop">
        <rdf:type rdf:resource="http://lpis.ec.europa.eu/registry/applicationschema/cap-iacs-base#SpecieCodeValue"/>
        <rdfs:label xml:lang="en">Agrostis gigantea L. Red top</rdfs:label>
        <skos:definition xml:lang="en">-- Definition --
Agrostis gigantea L. Red top.
-- Description --
List of agricultural species -A
II. Fodder plants
NOTE. Initial value: A - 4.</skos:definition>
        <skos:inScheme rdf:resource="http://lpis.ec.europa.eu/registry/applicationschema/cap-iacs-base/code#SpecieCodeValue"/>
    </owl:NamedIndividual>
    


    <!-- http://lpis.ec.europa.eu/registry/applicationschema/cap-iacs-base/code#SpecieCodeValue/agrostisStoloniferaLCreepingBent -->


    <owl:NamedIndividual rdf:about="http://lpis.ec.europa.eu/registry/applicationschema/cap-iacs-base/code#SpecieCodeValue/agrostisStoloniferaLCreepingBent">
        <rdf:type rdf:resource="http://lpis.ec.europa.eu/registry/applicationschema/cap-iacs-base#SpecieCodeValue"/>
        <rdfs:label xml:lang="en">Agrostis stolonifera L. Creeping bent</rdfs:label>
        <skos:definition xml:lang="en">-- Definition --
Agrostis stolonifera L. Creeping bent.
-- Description --
List of agricultural species -A
II. Fodder plants
NOTE. Initial value: A - 5.</skos:definition>
        <skos:inScheme rdf:resource="http://lpis.ec.europa.eu/registry/applicationschema/cap-iacs-base/code#SpecieCodeValue"/>
    </owl:NamedIndividual>
    


    <!-- http://lpis.ec.europa.eu/registry/applicationschema/cap-iacs-base/code#SpecieCodeValue/alliumCepaLAggregatumGroupShallot -->


    <owl:NamedIndividual rdf:about="http://lpis.ec.europa.eu/registry/applicationschema/cap-iacs-base/code#SpecieCodeValue/alliumCepaLAggregatumGroupShallot">
        <rdf:type rdf:resource="http://lpis.ec.europa.eu/registry/applicationschema/cap-iacs-base#SpecieCodeValue"/>
        <rdfs:label xml:lang="en">Allium cepa L. Aggregatum group - Shallot</rdfs:label>
        <skos:definition xml:lang="en">-- Definition --
Allium cepa L. Aggregatum group - Shallot.
-- Description --
List of vegetable specie -H
NOTE. Initial value: H - 1.1</skos:definition>
        <skos:inScheme rdf:resource="http://lpis.ec.europa.eu/registry/applicationschema/cap-iacs-base/code#SpecieCodeValue"/>
    </owl:NamedIndividual>
    


    <!-- http://lpis.ec.europa.eu/registry/applicationschema/cap-iacs-base/code#SpecieCodeValue/alliumCepaLCepaGroupOnionEchalion -->


    <owl:NamedIndividual rdf:about="http://lpis.ec.europa.eu/registry/applicationschema/cap-iacs-base/code#SpecieCodeValue/alliumCepaLCepaGroupOnionEchalion">
        <rdf:type rdf:resource="http://lpis.ec.europa.eu/registry/applicationschema/cap-iacs-base#SpecieCodeValue"/>
        <rdfs:label xml:lang="en">Allium cepa L. Cepa group - Onion, Echalion</rdfs:label>
        <skos:definition xml:lang="en">-- Definition --
Allium cepa L. Cepa group - Onion, Echalion.
-- Description --
List of vegetable specie -H
NOTE. Initial value: H - 1.2</skos:definition>
        <skos:inScheme rdf:resource="http://lpis.ec.europa.eu/registry/applicationschema/cap-iacs-base/code#SpecieCodeValue"/>
    </owl:NamedIndividual>
    


    <!-- http://lpis.ec.europa.eu/registry/applicationschema/cap-iacs-base/code#SpecieCodeValue/alliumFistulosumLJapaneseBunchingOnionWelshOnion -->


    <owl:NamedIndividual rdf:about="http://lpis.ec.europa.eu/registry/applicationschema/cap-iacs-base/code#SpecieCodeValue/alliumFistulosumLJapaneseBunchingOnionWelshOnion">
        <rdf:type rdf:resource="http://lpis.ec.europa.eu/registry/applicationschema/cap-iacs-base#SpecieCodeValue"/>
        <rdfs:label xml:lang="en">Allium fistulosum L. Japanese bunching onion / Welsh onion</rdfs:label>
        <skos:definition xml:lang="en">-- Definition --
Allium fistulosum L. Japanese bunching onion / Welsh onion.
-- Description --
List of vegetable specie -H
NOTE. Initial value: H - 2.</skos:definition>
        <skos:inScheme rdf:resource="http://lpis.ec.europa.eu/registry/applicationschema/cap-iacs-base/code#SpecieCodeValue"/>
    </owl:NamedIndividual>
    


    <!-- http://lpis.ec.europa.eu/registry/applicationschema/cap-iacs-base/code#SpecieCodeValue/alliumPorrumLLeek -->


    <owl:NamedIndividual rdf:about="http://lpis.ec.europa.eu/registry/applicationschema/cap-iacs-base/code#SpecieCodeValue/alliumPorrumLLeek">
        <rdf:type rdf:resource="http://lpis.ec.europa.eu/registry/applicationschema/cap-iacs-base#SpecieCodeValue"/>
        <rdfs:label xml:lang="en">Allium porrum L. Leek</rdfs:label>
        <skos:definition xml:lang="en">-- Definition --
Allium porrum L. Leek.
-- Description --
List of vegetable specie -H
NOTE. Initial value: H - 3.</skos:definition>
        <skos:inScheme rdf:resource="http://lpis.ec.europa.eu/registry/applicationschema/cap-iacs-base/code#SpecieCodeValue"/>
    </owl:NamedIndividual>
    


    <!-- http://lpis.ec.europa.eu/registry/applicationschema/cap-iacs-base/code#SpecieCodeValue/alliumSativumLGarlic -->


    <owl:NamedIndividual rdf:about="http://lpis.ec.europa.eu/registry/applicationschema/cap-iacs-base/code#SpecieCodeValue/alliumSativumLGarlic">
        <rdf:type rdf:resource="http://lpis.ec.europa.eu/registry/applicationschema/cap-iacs-base#SpecieCodeValue"/>
        <rdfs:label xml:lang="en">Allium sativum L. Garlic</rdfs:label>
        <skos:definition xml:lang="en">-- Definition --
Allium sativum L. Garlic.
-- Description --
List of vegetable specie -H
NOTE. Initial value: H - 4.</skos:definition>
        <skos:inScheme rdf:resource="http://lpis.ec.europa.eu/registry/applicationschema/cap-iacs-base/code#SpecieCodeValue"/>
    </owl:NamedIndividual>
    


    <!-- http://lpis.ec.europa.eu/registry/applicationschema/cap-iacs-base/code#SpecieCodeValue/alliumSchoenoprasumLChives -->


    <owl:NamedIndividual rdf:about="http://lpis.ec.europa.eu/registry/applicationschema/cap-iacs-base/code#SpecieCodeValue/alliumSchoenoprasumLChives">
        <rdf:type rdf:resource="http://lpis.ec.europa.eu/registry/applicationschema/cap-iacs-base#SpecieCodeValue"/>
        <rdfs:label xml:lang="en">Allium schoenoprasum L. Chives</rdfs:label>
        <skos:definition xml:lang="en">-- Definition --
Allium schoenoprasum L. Chives.
-- Description --
List of vegetable specie -H
NOTE. Initial value: H - 5.</skos:definition>
        <skos:inScheme rdf:resource="http://lpis.ec.europa.eu/registry/applicationschema/cap-iacs-base/code#SpecieCodeValue"/>
    </owl:NamedIndividual>
    


    <!-- http://lpis.ec.europa.eu/registry/applicationschema/cap-iacs-base/code#SpecieCodeValue/alopecurusPratensisLMeadowFoxtail -->


    <owl:NamedIndividual rdf:about="http://lpis.ec.europa.eu/registry/applicationschema/cap-iacs-base/code#SpecieCodeValue/alopecurusPratensisLMeadowFoxtail">
        <rdf:type rdf:resource="http://lpis.ec.europa.eu/registry/applicationschema/cap-iacs-base#SpecieCodeValue"/>
        <rdfs:label xml:lang="en">Alopecurus pratensis L. Meadow foxtail </rdfs:label>
        <skos:definition xml:lang="en">-- Definition --
Alopecurus pratensis L. Meadow foxtail.
-- Description --
List of agricultural species -A
II. Fodder plants
NOTE. Initial value: A - 7.</skos:definition>
        <skos:inScheme rdf:resource="http://lpis.ec.europa.eu/registry/applicationschema/cap-iacs-base/code#SpecieCodeValue"/>
    </owl:NamedIndividual>
    


    <!-- http://lpis.ec.europa.eu/registry/applicationschema/cap-iacs-base/code#SpecieCodeValue/anthriscusCerefoliumLHoffmChervil -->


    <owl:NamedIndividual rdf:about="http://lpis.ec.europa.eu/registry/applicationschema/cap-iacs-base/code#SpecieCodeValue/anthriscusCerefoliumLHoffmChervil">
        <rdf:type rdf:resource="http://lpis.ec.europa.eu/registry/applicationschema/cap-iacs-base#SpecieCodeValue"/>
        <rdfs:label xml:lang="en">Anthriscus cerefolium (L.) Hoffm. Chervil</rdfs:label>
        <skos:definition xml:lang="en">-- Definition --
Anthriscus cerefolium (L.) Hoffm. Chervil.
-- Description --
List of vegetable specie -H
NOTE. Initial value: H - 6.</skos:definition>
        <skos:inScheme rdf:resource="http://lpis.ec.europa.eu/registry/applicationschema/cap-iacs-base/code#SpecieCodeValue"/>
    </owl:NamedIndividual>
    


    <!-- http://lpis.ec.europa.eu/registry/applicationschema/cap-iacs-base/code#SpecieCodeValue/apiumGraveolensLCeleriac -->


    <owl:NamedIndividual rdf:about="http://lpis.ec.europa.eu/registry/applicationschema/cap-iacs-base/code#SpecieCodeValue/apiumGraveolensLCeleriac">
        <rdf:type rdf:resource="http://lpis.ec.europa.eu/registry/applicationschema/cap-iacs-base#SpecieCodeValue"/>
        <rdfs:label xml:lang="en">Apium graveolens L. Celeriac</rdfs:label>
        <skos:definition xml:lang="en">-- Definition --
Apium graveolens L. Celeriac.
-- Description --
List of vegetable specie -H
NOTE. Initial value: H - 7.2</skos:definition>
        <skos:inScheme rdf:resource="http://lpis.ec.europa.eu/registry/applicationschema/cap-iacs-base/code#SpecieCodeValue"/>
    </owl:NamedIndividual>
    


    <!-- http://lpis.ec.europa.eu/registry/applicationschema/cap-iacs-base/code#SpecieCodeValue/apiumGraveolensLCelery -->


    <owl:NamedIndividual rdf:about="http://lpis.ec.europa.eu/registry/applicationschema/cap-iacs-base/code#SpecieCodeValue/apiumGraveolensLCelery">
        <rdf:type rdf:resource="http://lpis.ec.europa.eu/registry/applicationschema/cap-iacs-base#SpecieCodeValue"/>
        <rdfs:label xml:lang="en">Apium graveolens L. Celery</rdfs:label>
        <skos:definition xml:lang="en">-- Definition --
Apium graveolens L. Celery.
-- Description --
List of vegetable specie -H
NOTE. Initial value: H - 7.1</skos:definition>
        <skos:inScheme rdf:resource="http://lpis.ec.europa.eu/registry/applicationschema/cap-iacs-base/code#SpecieCodeValue"/>
    </owl:NamedIndividual>
    


    <!-- http://lpis.ec.europa.eu/registry/applicationschema/cap-iacs-base/code#SpecieCodeValue/arachisHypogeaLGroundnutPeanut -->


    <owl:NamedIndividual rdf:about="http://lpis.ec.europa.eu/registry/applicationschema/cap-iacs-base/code#SpecieCodeValue/arachisHypogeaLGroundnutPeanut">
        <rdf:type rdf:resource="http://lpis.ec.europa.eu/registry/applicationschema/cap-iacs-base#SpecieCodeValue"/>
        <rdfs:label xml:lang="en">Arachis hypogea L. Groundnut/Peanut</rdfs:label>
        <skos:definition xml:lang="en">-- Definition --
Arachis hypogea L. Groundnut/Peanut.
-- Description --
List of agricultural species -A
III. Oil and fibre plants
NOTE. Initial value: A - 58.</skos:definition>
        <skos:inScheme rdf:resource="http://lpis.ec.europa.eu/registry/applicationschema/cap-iacs-base/code#SpecieCodeValue"/>
    </owl:NamedIndividual>
    


    <!-- http://lpis.ec.europa.eu/registry/applicationschema/cap-iacs-base/code#SpecieCodeValue/arrhenatherumElatiusLTallOatgrass -->


    <owl:NamedIndividual rdf:about="http://lpis.ec.europa.eu/registry/applicationschema/cap-iacs-base/code#SpecieCodeValue/arrhenatherumElatiusLTallOatgrass">
        <rdf:type rdf:resource="http://lpis.ec.europa.eu/registry/applicationschema/cap-iacs-base#SpecieCodeValue"/>
        <rdfs:label xml:lang="en">Arrhenatherum elatius L. Tall oatgrass </rdfs:label>
        <skos:definition xml:lang="en">-- Definition --
Arrhenatherum elatius L. Tall oatgrass.
-- Description --
List of agricultural species -A
II. Fodder plants
NOTE. Initial value: A - 8.</skos:definition>
        <skos:inScheme rdf:resource="http://lpis.ec.europa.eu/registry/applicationschema/cap-iacs-base/code#SpecieCodeValue"/>
    </owl:NamedIndividual>
    


    <!-- http://lpis.ec.europa.eu/registry/applicationschema/cap-iacs-base/code#SpecieCodeValue/asparagusOfficinalisLAsparagus -->


    <owl:NamedIndividual rdf:about="http://lpis.ec.europa.eu/registry/applicationschema/cap-iacs-base/code#SpecieCodeValue/asparagusOfficinalisLAsparagus">
        <rdf:type rdf:resource="http://lpis.ec.europa.eu/registry/applicationschema/cap-iacs-base#SpecieCodeValue"/>
        <rdfs:label xml:lang="en">Asparagus officinalis L. Asparagus</rdfs:label>
        <skos:definition xml:lang="en">-- Definition --
Asparagus officinalis L. Asparagus.
-- Description --
List of vegetable specie -H
NOTE. Initial value: H - 8.</skos:definition>
        <skos:inScheme rdf:resource="http://lpis.ec.europa.eu/registry/applicationschema/cap-iacs-base/code#SpecieCodeValue"/>
    </owl:NamedIndividual>
    


    <!-- http://lpis.ec.europa.eu/registry/applicationschema/cap-iacs-base/code#SpecieCodeValue/avenaNudaLSmallNakedOatHullessOat -->


    <owl:NamedIndividual rdf:about="http://lpis.ec.europa.eu/registry/applicationschema/cap-iacs-base/code#SpecieCodeValue/avenaNudaLSmallNakedOatHullessOat">
        <rdf:type rdf:resource="http://lpis.ec.europa.eu/registry/applicationschema/cap-iacs-base#SpecieCodeValue"/>
        <rdfs:label xml:lang="en">Avena nuda L. Small naked oat / Hulless oat </rdfs:label>
        <skos:definition xml:lang="en">-- Definition --
Avena nuda L. Small naked oat / Hulless oat.
-- Description --
List of agricultural species -A   
IV. Cereals
NOTE. Initial value: A - 72.</skos:definition>
        <skos:inScheme rdf:resource="http://lpis.ec.europa.eu/registry/applicationschema/cap-iacs-base/code#SpecieCodeValue"/>
    </owl:NamedIndividual>
    


    <!-- http://lpis.ec.europa.eu/registry/applicationschema/cap-iacs-base/code#SpecieCodeValue/avenaSativaLIncludingAByzantinaKKochOatAndRedOat -->


    <owl:NamedIndividual rdf:about="http://lpis.ec.europa.eu/registry/applicationschema/cap-iacs-base/code#SpecieCodeValue/avenaSativaLIncludingAByzantinaKKochOatAndRedOat">
        <rdf:type rdf:resource="http://lpis.ec.europa.eu/registry/applicationschema/cap-iacs-base#SpecieCodeValue"/>
        <rdfs:label xml:lang="en">Avena sativa L. (including A. byzantina K. Koch) Oat and Red oat</rdfs:label>
        <skos:definition xml:lang="en">-- Definition --
Avena sativa L. (including A. byzantina K. Koch) Oat and Red oat.
-- Description --
List of agricultural species -A   
IV. Cereals
NOTE. Initial value: A - 73.</skos:definition>
        <skos:inScheme rdf:resource="http://lpis.ec.europa.eu/registry/applicationschema/cap-iacs-base/code#SpecieCodeValue"/>
    </owl:NamedIndividual>
    


    <!-- http://lpis.ec.europa.eu/registry/applicationschema/cap-iacs-base/code#SpecieCodeValue/avenaStrigosaSchrebLBlackOatBristle -->


    <owl:NamedIndividual rdf:about="http://lpis.ec.europa.eu/registry/applicationschema/cap-iacs-base/code#SpecieCodeValue/avenaStrigosaSchrebLBlackOatBristle">
        <rdf:type rdf:resource="http://lpis.ec.europa.eu/registry/applicationschema/cap-iacs-base#SpecieCodeValue"/>
        <rdfs:label xml:lang="en">Avena strigosa Schreb. L. Black oat / Bristle</rdfs:label>
        <skos:definition xml:lang="en">-- Definition --
Avena strigosa Schreb. L. Black oat / Bristle.
-- Description --
List of agricultural species -A   
IV. Cereals
NOTE. Initial value: A - 74.</skos:definition>
        <skos:inScheme rdf:resource="http://lpis.ec.europa.eu/registry/applicationschema/cap-iacs-base/code#SpecieCodeValue"/>
    </owl:NamedIndividual>
    


    <!-- http://lpis.ec.europa.eu/registry/applicationschema/cap-iacs-base/code#SpecieCodeValue/betaVulgarisLBeetrootIncludingCheltenhamBeet -->


    <owl:NamedIndividual rdf:about="http://lpis.ec.europa.eu/registry/applicationschema/cap-iacs-base/code#SpecieCodeValue/betaVulgarisLBeetrootIncludingCheltenhamBeet">
        <rdf:type rdf:resource="http://lpis.ec.europa.eu/registry/applicationschema/cap-iacs-base#SpecieCodeValue"/>
        <rdfs:label xml:lang="en">Beta vulgaris L. Beetroot, including Cheltenham beet</rdfs:label>
        <skos:definition xml:lang="en">-- Definition --
Beta vulgaris L. Beetroot, including Cheltenham beet.
-- Description --
List of vegetable specie -H
NOTE. Initial value: H - 9.1</skos:definition>
        <skos:inScheme rdf:resource="http://lpis.ec.europa.eu/registry/applicationschema/cap-iacs-base/code#SpecieCodeValue"/>
    </owl:NamedIndividual>
    


    <!-- http://lpis.ec.europa.eu/registry/applicationschema/cap-iacs-base/code#SpecieCodeValue/betaVulgarisLFodderBeet -->


    <owl:NamedIndividual rdf:about="http://lpis.ec.europa.eu/registry/applicationschema/cap-iacs-base/code#SpecieCodeValue/betaVulgarisLFodderBeet">
        <rdf:type rdf:resource="http://lpis.ec.europa.eu/registry/applicationschema/cap-iacs-base#SpecieCodeValue"/>
        <rdfs:label xml:lang="en">Beta vulgaris L. Fodder beet </rdfs:label>
        <skos:definition xml:lang="en">-- Definition --
Beta vulgaris L. Fodder beet.
-- Description --
List of agricultural species -A
I. Beet
NOTE. Initial value: A - 2.</skos:definition>
        <skos:inScheme rdf:resource="http://lpis.ec.europa.eu/registry/applicationschema/cap-iacs-base/code#SpecieCodeValue"/>
    </owl:NamedIndividual>
    


    <!-- http://lpis.ec.europa.eu/registry/applicationschema/cap-iacs-base/code#SpecieCodeValue/betaVulgarisLSpinachBeetOrChard -->


    <owl:NamedIndividual rdf:about="http://lpis.ec.europa.eu/registry/applicationschema/cap-iacs-base/code#SpecieCodeValue/betaVulgarisLSpinachBeetOrChard">
        <rdf:type rdf:resource="http://lpis.ec.europa.eu/registry/applicationschema/cap-iacs-base#SpecieCodeValue"/>
        <rdfs:label xml:lang="en">Beta vulgaris L. Spinach beet or Chard</rdfs:label>
        <skos:definition xml:lang="en">-- Definition --
Beta vulgaris L. Spinach beet or Chard.
-- Description --
List of vegetable specie -H
NOTE. Initial value: H - 9.2</skos:definition>
        <skos:inScheme rdf:resource="http://lpis.ec.europa.eu/registry/applicationschema/cap-iacs-base/code#SpecieCodeValue"/>
    </owl:NamedIndividual>
    


    <!-- http://lpis.ec.europa.eu/registry/applicationschema/cap-iacs-base/code#SpecieCodeValue/betaVulgarisLSugarBeet -->


    <owl:NamedIndividual rdf:about="http://lpis.ec.europa.eu/registry/applicationschema/cap-iacs-base/code#SpecieCodeValue/betaVulgarisLSugarBeet">
        <rdf:type rdf:resource="http://lpis.ec.europa.eu/registry/applicationschema/cap-iacs-base#SpecieCodeValue"/>
        <rdfs:label xml:lang="en">Beta vulgaris L. Sugar beet</rdfs:label>
        <skos:definition xml:lang="en">-- Definition --
Beta vulgaris L. Sugar beet.
-- Description --
List of agricultural species -A
I. Beet
NOTE. Initial value: A - 1.</skos:definition>
        <skos:inScheme rdf:resource="http://lpis.ec.europa.eu/registry/applicationschema/cap-iacs-base/code#SpecieCodeValue"/>
    </owl:NamedIndividual>
    


    <!-- http://lpis.ec.europa.eu/registry/applicationschema/cap-iacs-base/code#SpecieCodeValue/brassicaJunceaLBrownMustard -->


    <owl:NamedIndividual rdf:about="http://lpis.ec.europa.eu/registry/applicationschema/cap-iacs-base/code#SpecieCodeValue/brassicaJunceaLBrownMustard">
        <rdf:type rdf:resource="http://lpis.ec.europa.eu/registry/applicationschema/cap-iacs-base#SpecieCodeValue"/>
        <rdfs:label xml:lang="en">Brassica juncea L. Brown mustard </rdfs:label>
        <skos:definition xml:lang="en">-- Definition --
Brassica juncea L. Brown mustard.
-- Description --
List of agricultural species -A
III. Oil and fibre plants
NOTE. Initial value: A - 60.</skos:definition>
        <skos:inScheme rdf:resource="http://lpis.ec.europa.eu/registry/applicationschema/cap-iacs-base/code#SpecieCodeValue"/>
    </owl:NamedIndividual>
    


    <!-- http://lpis.ec.europa.eu/registry/applicationschema/cap-iacs-base/code#SpecieCodeValue/brassicaNapusLPartimSwedeRape -->


    <owl:NamedIndividual rdf:about="http://lpis.ec.europa.eu/registry/applicationschema/cap-iacs-base/code#SpecieCodeValue/brassicaNapusLPartimSwedeRape">
        <rdf:type rdf:resource="http://lpis.ec.europa.eu/registry/applicationschema/cap-iacs-base#SpecieCodeValue"/>
        <rdfs:label xml:lang="en">Brassica napus L. (partim) Swede rape </rdfs:label>
        <skos:definition xml:lang="en">-- Definition --
Brassica napus L. (partim) Swede rape.
-- Description --
List of agricultural species -A
III. Oil and fibre plants
NOTE. Initial value: A - 61.</skos:definition>
        <skos:inScheme rdf:resource="http://lpis.ec.europa.eu/registry/applicationschema/cap-iacs-base/code#SpecieCodeValue"/>
    </owl:NamedIndividual>
    


    <!-- http://lpis.ec.europa.eu/registry/applicationschema/cap-iacs-base/code#SpecieCodeValue/brassicaNapusLSwede -->


    <owl:NamedIndividual rdf:about="http://lpis.ec.europa.eu/registry/applicationschema/cap-iacs-base/code#SpecieCodeValue/brassicaNapusLSwede">
        <rdf:type rdf:resource="http://lpis.ec.europa.eu/registry/applicationschema/cap-iacs-base#SpecieCodeValue"/>
        <rdfs:label xml:lang="en">Brassica napus L. Swede </rdfs:label>
        <skos:definition xml:lang="en">-- Definition --
Brassica napus L. Swede.
-- Description --
List of agricultural species -A
II. Fodder plants
NOTE. Initial value: A - 54.</skos:definition>
        <skos:inScheme rdf:resource="http://lpis.ec.europa.eu/registry/applicationschema/cap-iacs-base/code#SpecieCodeValue"/>
    </owl:NamedIndividual>
    


    <!-- http://lpis.ec.europa.eu/registry/applicationschema/cap-iacs-base/code#SpecieCodeValue/brassicaNigraLBlackMustard -->


    <owl:NamedIndividual rdf:about="http://lpis.ec.europa.eu/registry/applicationschema/cap-iacs-base/code#SpecieCodeValue/brassicaNigraLBlackMustard">
        <rdf:type rdf:resource="http://lpis.ec.europa.eu/registry/applicationschema/cap-iacs-base#SpecieCodeValue"/>
        <rdfs:label xml:lang="en">Brassica nigra L. Black mustard </rdfs:label>
        <skos:definition xml:lang="en">-- Definition --
Brassica nigra L. Black mustard.
-- Description --
List of agricultural species -A
III. Oil and fibre plants
NOTE. Initial value: A - 62.</skos:definition>
        <skos:inScheme rdf:resource="http://lpis.ec.europa.eu/registry/applicationschema/cap-iacs-base/code#SpecieCodeValue"/>
    </owl:NamedIndividual>
    


    <!-- http://lpis.ec.europa.eu/registry/applicationschema/cap-iacs-base/code#SpecieCodeValue/brassicaOleraceaLBrusselsSprouts -->


    <owl:NamedIndividual rdf:about="http://lpis.ec.europa.eu/registry/applicationschema/cap-iacs-base/code#SpecieCodeValue/brassicaOleraceaLBrusselsSprouts">
        <rdf:type rdf:resource="http://lpis.ec.europa.eu/registry/applicationschema/cap-iacs-base#SpecieCodeValue"/>
        <rdfs:label xml:lang="en">Brassica oleracea L. Brussels sprouts</rdfs:label>
        <skos:definition xml:lang="en">-- Definition --
Brassica oleracea L. Brussels sprouts.
-- Description --
List of vegetable specie -H
NOTE. Initial value: H - 10.4</skos:definition>
        <skos:inScheme rdf:resource="http://lpis.ec.europa.eu/registry/applicationschema/cap-iacs-base/code#SpecieCodeValue"/>
    </owl:NamedIndividual>
    


    <!-- http://lpis.ec.europa.eu/registry/applicationschema/cap-iacs-base/code#SpecieCodeValue/brassicaOleraceaLCauliflower -->


    <owl:NamedIndividual rdf:about="http://lpis.ec.europa.eu/registry/applicationschema/cap-iacs-base/code#SpecieCodeValue/brassicaOleraceaLCauliflower">
        <rdf:type rdf:resource="http://lpis.ec.europa.eu/registry/applicationschema/cap-iacs-base#SpecieCodeValue"/>
        <rdfs:label xml:lang="en">Brassica oleracea L. Cauliflower</rdfs:label>
        <skos:definition xml:lang="en">-- Definition --
Brassica oleracea L. Cauliflower.
-- Description --
List of vegetable specie -H
NOTE. Initial value: H - 10.2</skos:definition>
        <skos:inScheme rdf:resource="http://lpis.ec.europa.eu/registry/applicationschema/cap-iacs-base/code#SpecieCodeValue"/>
    </owl:NamedIndividual>
    


    <!-- http://lpis.ec.europa.eu/registry/applicationschema/cap-iacs-base/code#SpecieCodeValue/brassicaOleraceaLCurlyKale -->


    <owl:NamedIndividual rdf:about="http://lpis.ec.europa.eu/registry/applicationschema/cap-iacs-base/code#SpecieCodeValue/brassicaOleraceaLCurlyKale">
        <rdf:type rdf:resource="http://lpis.ec.europa.eu/registry/applicationschema/cap-iacs-base#SpecieCodeValue"/>
        <rdfs:label xml:lang="en">Brassica oleracea L. Curly kale</rdfs:label>
        <skos:definition xml:lang="en">-- Definition --
Brassica oleracea L. Curly kale.
-- Description --
List of vegetable specie -H
NOTE. Initial value: H - 10.1</skos:definition>
        <skos:inScheme rdf:resource="http://lpis.ec.europa.eu/registry/applicationschema/cap-iacs-base/code#SpecieCodeValue"/>
    </owl:NamedIndividual>
    


    <!-- http://lpis.ec.europa.eu/registry/applicationschema/cap-iacs-base/code#SpecieCodeValue/brassicaOleraceaLFodderKale -->


    <owl:NamedIndividual rdf:about="http://lpis.ec.europa.eu/registry/applicationschema/cap-iacs-base/code#SpecieCodeValue/brassicaOleraceaLFodderKale">
        <rdf:type rdf:resource="http://lpis.ec.europa.eu/registry/applicationschema/cap-iacs-base#SpecieCodeValue"/>
        <rdfs:label xml:lang="en">Brassica oleracea L. Fodder kale </rdfs:label>
        <skos:definition xml:lang="en">-- Definition --
Brassica oleracea L. Fodder kale.
-- Description --
List of agricultural species -A
II. Fodder plants
NOTE. Initial value: A - 55.</skos:definition>
        <skos:inScheme rdf:resource="http://lpis.ec.europa.eu/registry/applicationschema/cap-iacs-base/code#SpecieCodeValue"/>
    </owl:NamedIndividual>
    


    <!-- http://lpis.ec.europa.eu/registry/applicationschema/cap-iacs-base/code#SpecieCodeValue/brassicaOleraceaLKohlrabi -->


    <owl:NamedIndividual rdf:about="http://lpis.ec.europa.eu/registry/applicationschema/cap-iacs-base/code#SpecieCodeValue/brassicaOleraceaLKohlrabi">
        <rdf:type rdf:resource="http://lpis.ec.europa.eu/registry/applicationschema/cap-iacs-base#SpecieCodeValue"/>
        <rdfs:label xml:lang="en">Brassica oleracea L. Kohlrabi </rdfs:label>
        <skos:definition xml:lang="en">-- Definition --
Brassica oleracea L. Kohlrabi.
-- Description --
List of vegetable specie -H
NOTE. Initial value: H - 10.8</skos:definition>
        <skos:inScheme rdf:resource="http://lpis.ec.europa.eu/registry/applicationschema/cap-iacs-base/code#SpecieCodeValue"/>
    </owl:NamedIndividual>
    


    <!-- http://lpis.ec.europa.eu/registry/applicationschema/cap-iacs-base/code#SpecieCodeValue/brassicaOleraceaLRedCabbage -->


    <owl:NamedIndividual rdf:about="http://lpis.ec.europa.eu/registry/applicationschema/cap-iacs-base/code#SpecieCodeValue/brassicaOleraceaLRedCabbage">
        <rdf:type rdf:resource="http://lpis.ec.europa.eu/registry/applicationschema/cap-iacs-base#SpecieCodeValue"/>
        <rdfs:label xml:lang="en">Brassica oleracea L. Red cabbage</rdfs:label>
        <skos:definition xml:lang="en">-- Definition --
Brassica oleracea L. Red cabbage.
-- Description --
List of vegetable specie -H
NOTE. Initial value: H - 10.7</skos:definition>
        <skos:inScheme rdf:resource="http://lpis.ec.europa.eu/registry/applicationschema/cap-iacs-base/code#SpecieCodeValue"/>
    </owl:NamedIndividual>
    


    <!-- http://lpis.ec.europa.eu/registry/applicationschema/cap-iacs-base/code#SpecieCodeValue/brassicaOleraceaLSavoyCabbage -->


    <owl:NamedIndividual rdf:about="http://lpis.ec.europa.eu/registry/applicationschema/cap-iacs-base/code#SpecieCodeValue/brassicaOleraceaLSavoyCabbage">
        <rdf:type rdf:resource="http://lpis.ec.europa.eu/registry/applicationschema/cap-iacs-base#SpecieCodeValue"/>
        <rdfs:label xml:lang="en">Brassica oleracea L. Savoy cabbage</rdfs:label>
        <skos:definition xml:lang="en">-- Definition --
Brassica oleracea L. Savoy cabbage.
-- Description --
List of vegetable specie -H
NOTE. Initial value: H - 10.5</skos:definition>
        <skos:inScheme rdf:resource="http://lpis.ec.europa.eu/registry/applicationschema/cap-iacs-base/code#SpecieCodeValue"/>
    </owl:NamedIndividual>
    


    <!-- http://lpis.ec.europa.eu/registry/applicationschema/cap-iacs-base/code#SpecieCodeValue/brassicaOleraceaLSproutingBroccoliCalabrese -->


    <owl:NamedIndividual rdf:about="http://lpis.ec.europa.eu/registry/applicationschema/cap-iacs-base/code#SpecieCodeValue/brassicaOleraceaLSproutingBroccoliCalabrese">
        <rdf:type rdf:resource="http://lpis.ec.europa.eu/registry/applicationschema/cap-iacs-base#SpecieCodeValue"/>
        <rdfs:label xml:lang="en">Brassica oleracea L. Sprouting broccoli / Calabrese</rdfs:label>
        <skos:definition xml:lang="en">-- Definition --
Brassica oleracea L. Sprouting broccoli / Calabrese.
-- Description --
List of vegetable specie -H
NOTE. Initial value: H - 10.3</skos:definition>
        <skos:inScheme rdf:resource="http://lpis.ec.europa.eu/registry/applicationschema/cap-iacs-base/code#SpecieCodeValue"/>
    </owl:NamedIndividual>
    


    <!-- http://lpis.ec.europa.eu/registry/applicationschema/cap-iacs-base/code#SpecieCodeValue/brassicaOleraceaLWhiteCabbage -->


    <owl:NamedIndividual rdf:about="http://lpis.ec.europa.eu/registry/applicationschema/cap-iacs-base/code#SpecieCodeValue/brassicaOleraceaLWhiteCabbage">
        <rdf:type rdf:resource="http://lpis.ec.europa.eu/registry/applicationschema/cap-iacs-base#SpecieCodeValue"/>
        <rdfs:label xml:lang="en">Brassica oleracea L. White cabbage</rdfs:label>
        <skos:definition xml:lang="en">-- Definition --
Brassica oleracea L. White cabbage.
-- Description --
List of vegetable specie -H
NOTE. Initial value: H - 10.6</skos:definition>
        <skos:inScheme rdf:resource="http://lpis.ec.europa.eu/registry/applicationschema/cap-iacs-base/code#SpecieCodeValue"/>
    </owl:NamedIndividual>
    


    <!-- http://lpis.ec.europa.eu/registry/applicationschema/cap-iacs-base/code#SpecieCodeValue/brassicaRapaLChineseCabbage -->


    <owl:NamedIndividual rdf:about="http://lpis.ec.europa.eu/registry/applicationschema/cap-iacs-base/code#SpecieCodeValue/brassicaRapaLChineseCabbage">
        <rdf:type rdf:resource="http://lpis.ec.europa.eu/registry/applicationschema/cap-iacs-base#SpecieCodeValue"/>
        <rdfs:label xml:lang="en">Brassica rapa L. Chinese cabbage</rdfs:label>
        <skos:definition xml:lang="en">-- Definition --
Brassica rapa L. Chinese cabbage.
-- Description --
List of vegetable specie -H
NOTE. Initial value: H - 11.1</skos:definition>
        <skos:inScheme rdf:resource="http://lpis.ec.europa.eu/registry/applicationschema/cap-iacs-base/code#SpecieCodeValue"/>
    </owl:NamedIndividual>
    


    <!-- http://lpis.ec.europa.eu/registry/applicationschema/cap-iacs-base/code#SpecieCodeValue/brassicaRapaLTurnip -->


    <owl:NamedIndividual rdf:about="http://lpis.ec.europa.eu/registry/applicationschema/cap-iacs-base/code#SpecieCodeValue/brassicaRapaLTurnip">
        <rdf:type rdf:resource="http://lpis.ec.europa.eu/registry/applicationschema/cap-iacs-base#SpecieCodeValue"/>
        <rdfs:label xml:lang="en">Brassica rapa L. Turnip</rdfs:label>
        <skos:definition xml:lang="en">-- Definition --
Brassica rapa L. Turnip.
-- Description --
List of vegetable specie -H
NOTE. Initial value: H - 11.2</skos:definition>
        <skos:inScheme rdf:resource="http://lpis.ec.europa.eu/registry/applicationschema/cap-iacs-base/code#SpecieCodeValue"/>
    </owl:NamedIndividual>
    


    <!-- http://lpis.ec.europa.eu/registry/applicationschema/cap-iacs-base/code#SpecieCodeValue/brassicaRapaLVarSilvestrisLamBriggsTurnipRape -->


    <owl:NamedIndividual rdf:about="http://lpis.ec.europa.eu/registry/applicationschema/cap-iacs-base/code#SpecieCodeValue/brassicaRapaLVarSilvestrisLamBriggsTurnipRape">
        <rdf:type rdf:resource="http://lpis.ec.europa.eu/registry/applicationschema/cap-iacs-base#SpecieCodeValue"/>
        <rdfs:label xml:lang="en">Brassica rapa L. var. silvestris (Lam.) Briggs Turnip rape </rdfs:label>
        <skos:definition xml:lang="en">-- Definition --
Brassica rapa L. var. silvestris (Lam.) Briggs Turnip rape.
-- Description --
List of agricultural species -A
III. Oil and fibre plants
NOTE. Initial value: A - 59.</skos:definition>
        <skos:inScheme rdf:resource="http://lpis.ec.europa.eu/registry/applicationschema/cap-iacs-base/code#SpecieCodeValue"/>
    </owl:NamedIndividual>
    


    <!-- http://lpis.ec.europa.eu/registry/applicationschema/cap-iacs-base/code#SpecieCodeValue/bromusCatharticusLRescueGrass -->


    <owl:NamedIndividual rdf:about="http://lpis.ec.europa.eu/registry/applicationschema/cap-iacs-base/code#SpecieCodeValue/bromusCatharticusLRescueGrass">
        <rdf:type rdf:resource="http://lpis.ec.europa.eu/registry/applicationschema/cap-iacs-base#SpecieCodeValue"/>
        <rdfs:label xml:lang="en">Bromus catharticus L. Rescue grass</rdfs:label>
        <skos:definition xml:lang="en">-- Definition --
Bromus catharticus L. Rescue grass.
-- Description --
List of agricultural species -A
II. Fodder plants
NOTE. Initial value: A - 9.</skos:definition>
        <skos:inScheme rdf:resource="http://lpis.ec.europa.eu/registry/applicationschema/cap-iacs-base/code#SpecieCodeValue"/>
    </owl:NamedIndividual>
    


    <!-- http://lpis.ec.europa.eu/registry/applicationschema/cap-iacs-base/code#SpecieCodeValue/bromusSitchensisLAlaskaBromeGrass -->


    <owl:NamedIndividual rdf:about="http://lpis.ec.europa.eu/registry/applicationschema/cap-iacs-base/code#SpecieCodeValue/bromusSitchensisLAlaskaBromeGrass">
        <rdf:type rdf:resource="http://lpis.ec.europa.eu/registry/applicationschema/cap-iacs-base#SpecieCodeValue"/>
        <rdfs:label xml:lang="en">Bromus sitchensis L. Alaska brome-grass</rdfs:label>
        <skos:definition xml:lang="en">-- Definition --
Bromus sitchensis L. Alaska brome-grass.
-- Description --
List of agricultural species -A
II. Fodder plants
NOTE. Initial value: A - 10.</skos:definition>
        <skos:inScheme rdf:resource="http://lpis.ec.europa.eu/registry/applicationschema/cap-iacs-base/code#SpecieCodeValue"/>
    </owl:NamedIndividual>
    


    <!-- http://lpis.ec.europa.eu/registry/applicationschema/cap-iacs-base/code#SpecieCodeValue/cannabisSativaLHemp -->


    <owl:NamedIndividual rdf:about="http://lpis.ec.europa.eu/registry/applicationschema/cap-iacs-base/code#SpecieCodeValue/cannabisSativaLHemp">
        <rdf:type rdf:resource="http://lpis.ec.europa.eu/registry/applicationschema/cap-iacs-base#SpecieCodeValue"/>
        <rdfs:label xml:lang="en">Cannabis sativa L. Hemp </rdfs:label>
        <skos:definition xml:lang="en">-- Definition --
Cannabis sativa L. Hemp.
-- Description --
List of agricultural species -A
III. Oil and fibre plants
NOTE. Initial value: A - 63.</skos:definition>
        <skos:inScheme rdf:resource="http://lpis.ec.europa.eu/registry/applicationschema/cap-iacs-base/code#SpecieCodeValue"/>
    </owl:NamedIndividual>
    


    <!-- http://lpis.ec.europa.eu/registry/applicationschema/cap-iacs-base/code#SpecieCodeValue/capsicumAnnuumLChiliPepper -->


    <owl:NamedIndividual rdf:about="http://lpis.ec.europa.eu/registry/applicationschema/cap-iacs-base/code#SpecieCodeValue/capsicumAnnuumLChiliPepper">
        <rdf:type rdf:resource="http://lpis.ec.europa.eu/registry/applicationschema/cap-iacs-base#SpecieCodeValue"/>
        <rdfs:label xml:lang="en">Capsicum annuum L. Chili, Pepper </rdfs:label>
        <skos:definition xml:lang="en">-- Definition --
Capsicum annuum L. Chili, Pepper.
-- Description --
List of vegetable specie -H
NOTE. Initial value: H - 12.</skos:definition>
        <skos:inScheme rdf:resource="http://lpis.ec.europa.eu/registry/applicationschema/cap-iacs-base/code#SpecieCodeValue"/>
    </owl:NamedIndividual>
    


    <!-- http://lpis.ec.europa.eu/registry/applicationschema/cap-iacs-base/code#SpecieCodeValue/carthamusTinctoriusLSafflower -->


    <owl:NamedIndividual rdf:about="http://lpis.ec.europa.eu/registry/applicationschema/cap-iacs-base/code#SpecieCodeValue/carthamusTinctoriusLSafflower">
        <rdf:type rdf:resource="http://lpis.ec.europa.eu/registry/applicationschema/cap-iacs-base#SpecieCodeValue"/>
        <rdfs:label xml:lang="en">Carthamus tinctorius L. Safflower</rdfs:label>
        <skos:definition xml:lang="en">-- Definition --
Carthamus tinctorius L. Safflower.
-- Description --
List of agricultural species -A
III. Oil and fibre plants
NOTE. Initial value: A - 64.</skos:definition>
        <skos:inScheme rdf:resource="http://lpis.ec.europa.eu/registry/applicationschema/cap-iacs-base/code#SpecieCodeValue"/>
    </owl:NamedIndividual>
    


    <!-- http://lpis.ec.europa.eu/registry/applicationschema/cap-iacs-base/code#SpecieCodeValue/carumCarviLCaraway -->


    <owl:NamedIndividual rdf:about="http://lpis.ec.europa.eu/registry/applicationschema/cap-iacs-base/code#SpecieCodeValue/carumCarviLCaraway">
        <rdf:type rdf:resource="http://lpis.ec.europa.eu/registry/applicationschema/cap-iacs-base#SpecieCodeValue"/>
        <rdfs:label xml:lang="en">Carum carvi L. Caraway</rdfs:label>
        <skos:definition xml:lang="en">-- Definition --
Carum carvi L. Caraway.
-- Description --
List of agricultural species -A
III. Oil and fibre plants
NOTE. Initial value: A - 65.</skos:definition>
        <skos:inScheme rdf:resource="http://lpis.ec.europa.eu/registry/applicationschema/cap-iacs-base/code#SpecieCodeValue"/>
    </owl:NamedIndividual>
    


    <!-- http://lpis.ec.europa.eu/registry/applicationschema/cap-iacs-base/code#SpecieCodeValue/cichoriumEndiviaLCurledLeavedEndive -->


    <owl:NamedIndividual rdf:about="http://lpis.ec.europa.eu/registry/applicationschema/cap-iacs-base/code#SpecieCodeValue/cichoriumEndiviaLCurledLeavedEndive">
        <rdf:type rdf:resource="http://lpis.ec.europa.eu/registry/applicationschema/cap-iacs-base#SpecieCodeValue"/>
        <rdfs:label xml:lang="en">Cichorium endivia L. Curled-leaved endive</rdfs:label>
        <skos:definition xml:lang="en">-- Definition --
Cichorium endivia L. Curled-leaved endive.
-- Description --
List of vegetable specie -H
NOTE. Initial value: H - 13.1</skos:definition>
        <skos:inScheme rdf:resource="http://lpis.ec.europa.eu/registry/applicationschema/cap-iacs-base/code#SpecieCodeValue"/>
    </owl:NamedIndividual>
    


    <!-- http://lpis.ec.europa.eu/registry/applicationschema/cap-iacs-base/code#SpecieCodeValue/cichoriumEndiviaLPlainLeavedEndive -->


    <owl:NamedIndividual rdf:about="http://lpis.ec.europa.eu/registry/applicationschema/cap-iacs-base/code#SpecieCodeValue/cichoriumEndiviaLPlainLeavedEndive">
        <rdf:type rdf:resource="http://lpis.ec.europa.eu/registry/applicationschema/cap-iacs-base#SpecieCodeValue"/>
        <rdfs:label xml:lang="en">Cichorium endivia L. Plain-leaved endive</rdfs:label>
        <skos:definition xml:lang="en">-- Definition --
Cichorium endivia L. Plain-leaved endive.
-- Description --
List of vegetable specie -H
NOTE. Initial value: H - 13.2</skos:definition>
        <skos:inScheme rdf:resource="http://lpis.ec.europa.eu/registry/applicationschema/cap-iacs-base/code#SpecieCodeValue"/>
    </owl:NamedIndividual>
    


    <!-- http://lpis.ec.europa.eu/registry/applicationschema/cap-iacs-base/code#SpecieCodeValue/cichoriumIntybusLIndustrialChicory -->


    <owl:NamedIndividual rdf:about="http://lpis.ec.europa.eu/registry/applicationschema/cap-iacs-base/code#SpecieCodeValue/cichoriumIntybusLIndustrialChicory">
        <rdf:type rdf:resource="http://lpis.ec.europa.eu/registry/applicationschema/cap-iacs-base#SpecieCodeValue"/>
        <rdfs:label xml:lang="en">Cichorium intybus L. Industrial chicory</rdfs:label>
        <skos:definition xml:lang="en">-- Definition --
Cichorium intybus L. Industrial chicory.
-- Description --
List of vegetable specie -H
NOTE. Initial value: H - 14.3</skos:definition>
        <skos:inScheme rdf:resource="http://lpis.ec.europa.eu/registry/applicationschema/cap-iacs-base/code#SpecieCodeValue"/>
    </owl:NamedIndividual>
    


    <!-- http://lpis.ec.europa.eu/registry/applicationschema/cap-iacs-base/code#SpecieCodeValue/cichoriumIntybusLLargeLeavedChicoryItalianChicory -->


    <owl:NamedIndividual rdf:about="http://lpis.ec.europa.eu/registry/applicationschema/cap-iacs-base/code#SpecieCodeValue/cichoriumIntybusLLargeLeavedChicoryItalianChicory">
        <rdf:type rdf:resource="http://lpis.ec.europa.eu/registry/applicationschema/cap-iacs-base#SpecieCodeValue"/>
        <rdfs:label xml:lang="en">Cichorium intybus L. Large-leaved chicory / Italian chicory</rdfs:label>
        <skos:definition xml:lang="en">-- Definition --
Cichorium intybus L. Large-leaved chicory / Italian chicory.
-- Description --
List of vegetable specie -H
NOTE. Initial value: H - 14.2</skos:definition>
        <skos:inScheme rdf:resource="http://lpis.ec.europa.eu/registry/applicationschema/cap-iacs-base/code#SpecieCodeValue"/>
    </owl:NamedIndividual>
    


    <!-- http://lpis.ec.europa.eu/registry/applicationschema/cap-iacs-base/code#SpecieCodeValue/cichoriumIntybusLWitloofChicory -->


    <owl:NamedIndividual rdf:about="http://lpis.ec.europa.eu/registry/applicationschema/cap-iacs-base/code#SpecieCodeValue/cichoriumIntybusLWitloofChicory">
        <rdf:type rdf:resource="http://lpis.ec.europa.eu/registry/applicationschema/cap-iacs-base#SpecieCodeValue"/>
        <rdfs:label xml:lang="en">Cichorium intybus L. Witloof chicory</rdfs:label>
        <skos:definition xml:lang="en">-- Definition --
Cichorium intybus L. Witloof chicory.
-- Description --
List of vegetable specie -H
NOTE. Initial value: H - 14.1</skos:definition>
        <skos:inScheme rdf:resource="http://lpis.ec.europa.eu/registry/applicationschema/cap-iacs-base/code#SpecieCodeValue"/>
    </owl:NamedIndividual>
    


    <!-- http://lpis.ec.europa.eu/registry/applicationschema/cap-iacs-base/code#SpecieCodeValue/citrullusLanatusThunbMatsumEtNakaiWatermelon -->


    <owl:NamedIndividual rdf:about="http://lpis.ec.europa.eu/registry/applicationschema/cap-iacs-base/code#SpecieCodeValue/citrullusLanatusThunbMatsumEtNakaiWatermelon">
        <rdf:type rdf:resource="http://lpis.ec.europa.eu/registry/applicationschema/cap-iacs-base#SpecieCodeValue"/>
        <rdfs:label xml:lang="en">Citrullus lanatus (Thunb.) Matsum. et Nakai Watermelon</rdfs:label>
        <skos:definition xml:lang="en">-- Definition --
Citrullus lanatus (Thunb.) Matsum. et Nakai Watermelon.
-- Description --
List of vegetable specie -H
NOTE. Initial value: H - 15.</skos:definition>
        <skos:inScheme rdf:resource="http://lpis.ec.europa.eu/registry/applicationschema/cap-iacs-base/code#SpecieCodeValue"/>
    </owl:NamedIndividual>
    


    <!-- http://lpis.ec.europa.eu/registry/applicationschema/cap-iacs-base/code#SpecieCodeValue/cucumisMeloLMelon -->


    <owl:NamedIndividual rdf:about="http://lpis.ec.europa.eu/registry/applicationschema/cap-iacs-base/code#SpecieCodeValue/cucumisMeloLMelon">
        <rdf:type rdf:resource="http://lpis.ec.europa.eu/registry/applicationschema/cap-iacs-base#SpecieCodeValue"/>
        <rdfs:label xml:lang="en">Cucumis melo L. Melon</rdfs:label>
        <skos:definition xml:lang="en">-- Definition --
Cucumis melo L. Melon.
-- Description --
List of vegetable specie -H
NOTE. Initial value: H - 16.</skos:definition>
        <skos:inScheme rdf:resource="http://lpis.ec.europa.eu/registry/applicationschema/cap-iacs-base/code#SpecieCodeValue"/>
    </owl:NamedIndividual>
    


    <!-- http://lpis.ec.europa.eu/registry/applicationschema/cap-iacs-base/code#SpecieCodeValue/cucumisSativusLCucumber -->


    <owl:NamedIndividual rdf:about="http://lpis.ec.europa.eu/registry/applicationschema/cap-iacs-base/code#SpecieCodeValue/cucumisSativusLCucumber">
        <rdf:type rdf:resource="http://lpis.ec.europa.eu/registry/applicationschema/cap-iacs-base#SpecieCodeValue"/>
        <rdfs:label xml:lang="en">Cucumis sativus L. Cucumber</rdfs:label>
        <skos:definition xml:lang="en">-- Definition --
Cucumis sativus L. Cucumber.
-- Description --
List of vegetable specie -H
NOTE. Initial value: H - 17.1</skos:definition>
        <skos:inScheme rdf:resource="http://lpis.ec.europa.eu/registry/applicationschema/cap-iacs-base/code#SpecieCodeValue"/>
    </owl:NamedIndividual>
    


    <!-- http://lpis.ec.europa.eu/registry/applicationschema/cap-iacs-base/code#SpecieCodeValue/cucumisSativusLGherkin -->


    <owl:NamedIndividual rdf:about="http://lpis.ec.europa.eu/registry/applicationschema/cap-iacs-base/code#SpecieCodeValue/cucumisSativusLGherkin">
        <rdf:type rdf:resource="http://lpis.ec.europa.eu/registry/applicationschema/cap-iacs-base#SpecieCodeValue"/>
        <rdfs:label xml:lang="en">Cucumis sativus L. Gherkin</rdfs:label>
        <skos:definition xml:lang="en">-- Definition --
Cucumis sativus L. Gherkin.
-- Description --
List of vegetable specie -H
NOTE. Initial value: H - 17.2</skos:definition>
        <skos:inScheme rdf:resource="http://lpis.ec.europa.eu/registry/applicationschema/cap-iacs-base/code#SpecieCodeValue"/>
    </owl:NamedIndividual>
    


    <!-- http://lpis.ec.europa.eu/registry/applicationschema/cap-iacs-base/code#SpecieCodeValue/cucurbitaFicifoliaBouche -->


    <owl:NamedIndividual rdf:about="http://lpis.ec.europa.eu/registry/applicationschema/cap-iacs-base/code#SpecieCodeValue/cucurbitaFicifoliaBouche">
        <rdf:type rdf:resource="http://lpis.ec.europa.eu/registry/applicationschema/cap-iacs-base#SpecieCodeValue"/>
        <rdfs:label xml:lang="en">Cucurbita ficifolia Bouché</rdfs:label>
        <skos:definition xml:lang="en">-- Definition --
Cucurbita ficifolia Bouché.
-- Description --
List of vegetable specie -H
NOTE. Initial value: H - 37.1</skos:definition>
        <skos:inScheme rdf:resource="http://lpis.ec.europa.eu/registry/applicationschema/cap-iacs-base/code#SpecieCodeValue"/>
    </owl:NamedIndividual>
    


    <!-- http://lpis.ec.europa.eu/registry/applicationschema/cap-iacs-base/code#SpecieCodeValue/cucurbitaMaximaDuchesneGourd -->


    <owl:NamedIndividual rdf:about="http://lpis.ec.europa.eu/registry/applicationschema/cap-iacs-base/code#SpecieCodeValue/cucurbitaMaximaDuchesneGourd">
        <rdf:type rdf:resource="http://lpis.ec.europa.eu/registry/applicationschema/cap-iacs-base#SpecieCodeValue"/>
        <rdfs:label xml:lang="en">Cucurbita Maxima Duchesne Gourd</rdfs:label>
        <skos:definition xml:lang="en">-- Definition --
Cucurbita Maxima Duchesne Gourd.
-- Description --
List of vegetable specie -H
NOTE. Initial value: H - 18.</skos:definition>
        <skos:inScheme rdf:resource="http://lpis.ec.europa.eu/registry/applicationschema/cap-iacs-base/code#SpecieCodeValue"/>
    </owl:NamedIndividual>
    


    <!-- http://lpis.ec.europa.eu/registry/applicationschema/cap-iacs-base/code#SpecieCodeValue/cucurbitaMaximaDuchxCMoschataDuch -->


    <owl:NamedIndividual rdf:about="http://lpis.ec.europa.eu/registry/applicationschema/cap-iacs-base/code#SpecieCodeValue/cucurbitaMaximaDuchxCMoschataDuch">
        <rdf:type rdf:resource="http://lpis.ec.europa.eu/registry/applicationschema/cap-iacs-base#SpecieCodeValue"/>
        <rdfs:label xml:lang="en">Cucurbita maxima Duch. x C. moschata Duch.</rdfs:label>
        <skos:definition xml:lang="en">-- Definition --
Cucurbita maxima Duch. x C. moschata Duch.
-- Description --
List of vegetable specie -H
NOTE. Initial value: H - 37.2</skos:definition>
        <skos:inScheme rdf:resource="http://lpis.ec.europa.eu/registry/applicationschema/cap-iacs-base/code#SpecieCodeValue"/>
    </owl:NamedIndividual>
    


    <!-- http://lpis.ec.europa.eu/registry/applicationschema/cap-iacs-base/code#SpecieCodeValue/cucurbitaMoschata -->


    <owl:NamedIndividual rdf:about="http://lpis.ec.europa.eu/registry/applicationschema/cap-iacs-base/code#SpecieCodeValue/cucurbitaMoschata">
        <rdf:type rdf:resource="http://lpis.ec.europa.eu/registry/applicationschema/cap-iacs-base#SpecieCodeValue"/>
        <rdfs:label xml:lang="en">Cucurbita moschata</rdfs:label>
        <skos:definition xml:lang="en">-- Definition --
Cucurbita moschata.
-- Description --
List of vegetable specie -H
NOTE. Initial value: H - 37.7</skos:definition>
        <skos:inScheme rdf:resource="http://lpis.ec.europa.eu/registry/applicationschema/cap-iacs-base/code#SpecieCodeValue"/>
    </owl:NamedIndividual>
    


    <!-- http://lpis.ec.europa.eu/registry/applicationschema/cap-iacs-base/code#SpecieCodeValue/cucurbitaPepoLMarrowOrCourgette -->


    <owl:NamedIndividual rdf:about="http://lpis.ec.europa.eu/registry/applicationschema/cap-iacs-base/code#SpecieCodeValue/cucurbitaPepoLMarrowOrCourgette">
        <rdf:type rdf:resource="http://lpis.ec.europa.eu/registry/applicationschema/cap-iacs-base#SpecieCodeValue"/>
        <rdfs:label xml:lang="en">Cucurbita pepo L. Marrow or Courgette</rdfs:label>
        <skos:definition xml:lang="en">-- Definition --
Cucurbita pepo L. Marrow or Courgette.
-- Description --
List of vegetable specie -H
NOTE. Initial value: H - 19.</skos:definition>
        <skos:inScheme rdf:resource="http://lpis.ec.europa.eu/registry/applicationschema/cap-iacs-base/code#SpecieCodeValue"/>
    </owl:NamedIndividual>
    


    <!-- http://lpis.ec.europa.eu/registry/applicationschema/cap-iacs-base/code#SpecieCodeValue/cynaraCardunculusLCardoon -->


    <owl:NamedIndividual rdf:about="http://lpis.ec.europa.eu/registry/applicationschema/cap-iacs-base/code#SpecieCodeValue/cynaraCardunculusLCardoon">
        <rdf:type rdf:resource="http://lpis.ec.europa.eu/registry/applicationschema/cap-iacs-base#SpecieCodeValue"/>
        <rdfs:label xml:lang="en">Cynara cardunculus L. Cardoon</rdfs:label>
        <skos:definition xml:lang="en">-- Definition --
Cynara cardunculus L. Cardoon.
-- Description --
List of vegetable specie -H
NOTE. Initial value: H - 20.2</skos:definition>
        <skos:inScheme rdf:resource="http://lpis.ec.europa.eu/registry/applicationschema/cap-iacs-base/code#SpecieCodeValue"/>
    </owl:NamedIndividual>
    


    <!-- http://lpis.ec.europa.eu/registry/applicationschema/cap-iacs-base/code#SpecieCodeValue/cynaraCardunculusLGlobeArtichoke -->


    <owl:NamedIndividual rdf:about="http://lpis.ec.europa.eu/registry/applicationschema/cap-iacs-base/code#SpecieCodeValue/cynaraCardunculusLGlobeArtichoke">
        <rdf:type rdf:resource="http://lpis.ec.europa.eu/registry/applicationschema/cap-iacs-base#SpecieCodeValue"/>
        <rdfs:label xml:lang="en">Cynara cardunculus L. Globe artichoke</rdfs:label>
        <skos:definition xml:lang="en">-- Definition --
Cynara cardunculus L. Globe artichoke.
-- Description --
List of vegetable specie -H
NOTE. Initial value: H - 20.1</skos:definition>
        <skos:inScheme rdf:resource="http://lpis.ec.europa.eu/registry/applicationschema/cap-iacs-base/code#SpecieCodeValue"/>
    </owl:NamedIndividual>
    


    <!-- http://lpis.ec.europa.eu/registry/applicationschema/cap-iacs-base/code#SpecieCodeValue/cynodonDactylonLBermudaGrass -->


    <owl:NamedIndividual rdf:about="http://lpis.ec.europa.eu/registry/applicationschema/cap-iacs-base/code#SpecieCodeValue/cynodonDactylonLBermudaGrass">
        <rdf:type rdf:resource="http://lpis.ec.europa.eu/registry/applicationschema/cap-iacs-base#SpecieCodeValue"/>
        <rdfs:label xml:lang="en">Cynodon dactylon L. Bermuda grass</rdfs:label>
        <skos:definition xml:lang="en">-- Definition --
Cynodon dactylon L. Bermuda grass.
-- Description --
List of agricultural species -A
II. Fodder plants
NOTE. Initial value: A - 11.</skos:definition>
        <skos:inScheme rdf:resource="http://lpis.ec.europa.eu/registry/applicationschema/cap-iacs-base/code#SpecieCodeValue"/>
    </owl:NamedIndividual>
    


    <!-- http://lpis.ec.europa.eu/registry/applicationschema/cap-iacs-base/code#SpecieCodeValue/dactylisGlomerataLCocksfoot -->


    <owl:NamedIndividual rdf:about="http://lpis.ec.europa.eu/registry/applicationschema/cap-iacs-base/code#SpecieCodeValue/dactylisGlomerataLCocksfoot">
        <rdf:type rdf:resource="http://lpis.ec.europa.eu/registry/applicationschema/cap-iacs-base#SpecieCodeValue"/>
        <rdfs:label xml:lang="en">Dactylis glomerata L. Cocksfoot </rdfs:label>
        <skos:definition xml:lang="en">-- Definition --
Dactylis glomerata L. Cocksfoot.
-- Description --
List of agricultural species -A
II. Fodder plants
NOTE. Initial value: A - 12.</skos:definition>
        <skos:inScheme rdf:resource="http://lpis.ec.europa.eu/registry/applicationschema/cap-iacs-base/code#SpecieCodeValue"/>
    </owl:NamedIndividual>
    


    <!-- http://lpis.ec.europa.eu/registry/applicationschema/cap-iacs-base/code#SpecieCodeValue/daucusCarotaLCarrot -->


    <owl:NamedIndividual rdf:about="http://lpis.ec.europa.eu/registry/applicationschema/cap-iacs-base/code#SpecieCodeValue/daucusCarotaLCarrot">
        <rdf:type rdf:resource="http://lpis.ec.europa.eu/registry/applicationschema/cap-iacs-base#SpecieCodeValue"/>
        <rdfs:label xml:lang="en">Daucus carota L. Carrot</rdfs:label>
        <skos:definition xml:lang="en">-- Definition --
Daucus carota L. Carrot.
-- Description --
List of vegetable specie -H
NOTE. Initial value: H - 21.1</skos:definition>
        <skos:inScheme rdf:resource="http://lpis.ec.europa.eu/registry/applicationschema/cap-iacs-base/code#SpecieCodeValue"/>
    </owl:NamedIndividual>
    


    <!-- http://lpis.ec.europa.eu/registry/applicationschema/cap-iacs-base/code#SpecieCodeValue/daucusCarotaLFodderCarrot -->


    <owl:NamedIndividual rdf:about="http://lpis.ec.europa.eu/registry/applicationschema/cap-iacs-base/code#SpecieCodeValue/daucusCarotaLFodderCarrot">
        <rdf:type rdf:resource="http://lpis.ec.europa.eu/registry/applicationschema/cap-iacs-base#SpecieCodeValue"/>
        <rdfs:label xml:lang="en">Daucus carota L. Fodder carrot</rdfs:label>
        <skos:definition xml:lang="en">-- Definition --
Daucus carota L. Fodder carrot.
-- Description --
List of vegetable specie -H
NOTE. Initial value: H - 21.2</skos:definition>
        <skos:inScheme rdf:resource="http://lpis.ec.europa.eu/registry/applicationschema/cap-iacs-base/code#SpecieCodeValue"/>
    </owl:NamedIndividual>
    


    <!-- http://lpis.ec.europa.eu/registry/applicationschema/cap-iacs-base/code#SpecieCodeValue/festucaArundinaceaSchreberTallFescue -->


    <owl:NamedIndividual rdf:about="http://lpis.ec.europa.eu/registry/applicationschema/cap-iacs-base/code#SpecieCodeValue/festucaArundinaceaSchreberTallFescue">
        <rdf:type rdf:resource="http://lpis.ec.europa.eu/registry/applicationschema/cap-iacs-base#SpecieCodeValue"/>
        <rdfs:label xml:lang="en">Festuca arundinacea Schreber Tall fescue</rdfs:label>
        <skos:definition xml:lang="en">-- Definition --
Festuca arundinacea Schreber Tall fescue.
-- Description --
List of agricultural species -A
II. Fodder plants
NOTE. Initial value: A - 13.</skos:definition>
        <skos:inScheme rdf:resource="http://lpis.ec.europa.eu/registry/applicationschema/cap-iacs-base/code#SpecieCodeValue"/>
    </owl:NamedIndividual>
    


    <!-- http://lpis.ec.europa.eu/registry/applicationschema/cap-iacs-base/code#SpecieCodeValue/festucaFiliformisLFineLeavedSheeps -->


    <owl:NamedIndividual rdf:about="http://lpis.ec.europa.eu/registry/applicationschema/cap-iacs-base/code#SpecieCodeValue/festucaFiliformisLFineLeavedSheeps">
        <rdf:type rdf:resource="http://lpis.ec.europa.eu/registry/applicationschema/cap-iacs-base#SpecieCodeValue"/>
        <rdfs:label xml:lang="en">Festuca filiformis L. Fine leaved sheep&apos;s</rdfs:label>
        <skos:definition xml:lang="en">-- Definition --
Festuca filiformis L. Fine leaved sheep&apos;s.
-- Description --
List of agricultural species -A
II. Fodder plants
NOTE. Initial value: A - 14.</skos:definition>
        <skos:inScheme rdf:resource="http://lpis.ec.europa.eu/registry/applicationschema/cap-iacs-base/code#SpecieCodeValue"/>
    </owl:NamedIndividual>
    


    <!-- http://lpis.ec.europa.eu/registry/applicationschema/cap-iacs-base/code#SpecieCodeValue/festucaOvinaLSheepsFescue -->


    <owl:NamedIndividual rdf:about="http://lpis.ec.europa.eu/registry/applicationschema/cap-iacs-base/code#SpecieCodeValue/festucaOvinaLSheepsFescue">
        <rdf:type rdf:resource="http://lpis.ec.europa.eu/registry/applicationschema/cap-iacs-base#SpecieCodeValue"/>
        <rdfs:label xml:lang="en">Festuca ovina L. Sheep&apos;s fescue</rdfs:label>
        <skos:definition xml:lang="en">-- Definition --
Festuca ovina L. Sheep&apos;s fescue.
-- Description --
List of agricultural species -A
II. Fodder plants
NOTE. Initial value: A - 15.</skos:definition>
        <skos:inScheme rdf:resource="http://lpis.ec.europa.eu/registry/applicationschema/cap-iacs-base/code#SpecieCodeValue"/>
    </owl:NamedIndividual>
    


    <!-- http://lpis.ec.europa.eu/registry/applicationschema/cap-iacs-base/code#SpecieCodeValue/festucaPratensisHudsMeadowFescue -->


    <owl:NamedIndividual rdf:about="http://lpis.ec.europa.eu/registry/applicationschema/cap-iacs-base/code#SpecieCodeValue/festucaPratensisHudsMeadowFescue">
        <rdf:type rdf:resource="http://lpis.ec.europa.eu/registry/applicationschema/cap-iacs-base#SpecieCodeValue"/>
        <rdfs:label xml:lang="en">Festuca pratensis Huds. Meadow fescue   </rdfs:label>
        <skos:definition xml:lang="en">-- Definition --
Festuca pratensis Huds. Meadow fescue.
-- Description --
List of agricultural species -A
II. Fodder plants
NOTE. Initial value: A - 16.</skos:definition>
        <skos:inScheme rdf:resource="http://lpis.ec.europa.eu/registry/applicationschema/cap-iacs-base/code#SpecieCodeValue"/>
    </owl:NamedIndividual>
    


    <!-- http://lpis.ec.europa.eu/registry/applicationschema/cap-iacs-base/code#SpecieCodeValue/festucaRubraLRedFescue -->


    <owl:NamedIndividual rdf:about="http://lpis.ec.europa.eu/registry/applicationschema/cap-iacs-base/code#SpecieCodeValue/festucaRubraLRedFescue">
        <rdf:type rdf:resource="http://lpis.ec.europa.eu/registry/applicationschema/cap-iacs-base#SpecieCodeValue"/>
        <rdfs:label xml:lang="en">Festuca rubra L. Red fescue</rdfs:label>
        <skos:definition xml:lang="en">-- Definition --
Festuca rubra L. Red fescue.
-- Description --
List of agricultural species -A
II. Fodder plants
NOTE. Initial value: A - 17.</skos:definition>
        <skos:inScheme rdf:resource="http://lpis.ec.europa.eu/registry/applicationschema/cap-iacs-base/code#SpecieCodeValue"/>
    </owl:NamedIndividual>
    


    <!-- http://lpis.ec.europa.eu/registry/applicationschema/cap-iacs-base/code#SpecieCodeValue/festucaTrachyphyllaHackKrajinaHardFescue -->


    <owl:NamedIndividual rdf:about="http://lpis.ec.europa.eu/registry/applicationschema/cap-iacs-base/code#SpecieCodeValue/festucaTrachyphyllaHackKrajinaHardFescue">
        <rdf:type rdf:resource="http://lpis.ec.europa.eu/registry/applicationschema/cap-iacs-base#SpecieCodeValue"/>
        <rdfs:label xml:lang="en">Festuca trachyphylla (Hack.) Krajina Hard fescue </rdfs:label>
        <skos:definition xml:lang="en">-- Definition --
Festuca trachyphylla (Hack.) Krajina Hard fescue.
-- Description --
List of agricultural species -A
II. Fodder plants
NOTE. Initial value: A - 18.</skos:definition>
        <skos:inScheme rdf:resource="http://lpis.ec.europa.eu/registry/applicationschema/cap-iacs-base/code#SpecieCodeValue"/>
    </owl:NamedIndividual>
    


    <!-- http://lpis.ec.europa.eu/registry/applicationschema/cap-iacs-base/code#SpecieCodeValue/foeniculumVulgareMillFennel -->


    <owl:NamedIndividual rdf:about="http://lpis.ec.europa.eu/registry/applicationschema/cap-iacs-base/code#SpecieCodeValue/foeniculumVulgareMillFennel">
        <rdf:type rdf:resource="http://lpis.ec.europa.eu/registry/applicationschema/cap-iacs-base#SpecieCodeValue"/>
        <rdfs:label xml:lang="en">Foeniculum vulgare Mill. Fennel</rdfs:label>
        <skos:definition xml:lang="en">-- Definition --
Foeniculum vulgare Mill. Fennel.
-- Description --
List of vegetable specie -H
NOTE. Initial value: H - 22.</skos:definition>
        <skos:inScheme rdf:resource="http://lpis.ec.europa.eu/registry/applicationschema/cap-iacs-base/code#SpecieCodeValue"/>
    </owl:NamedIndividual>
    


    <!-- http://lpis.ec.europa.eu/registry/applicationschema/cap-iacs-base/code#SpecieCodeValue/galegaOrientalisLFodderGalega -->


    <owl:NamedIndividual rdf:about="http://lpis.ec.europa.eu/registry/applicationschema/cap-iacs-base/code#SpecieCodeValue/galegaOrientalisLFodderGalega">
        <rdf:type rdf:resource="http://lpis.ec.europa.eu/registry/applicationschema/cap-iacs-base#SpecieCodeValue"/>
        <rdfs:label xml:lang="en">Galega orientalis L. Fodder galega</rdfs:label>
        <skos:definition xml:lang="en">-- Definition --
Galega orientalis L. Fodder galega
-- Description --
List of agricultural species -A
II. Fodder plants
NOTE. Initial value: A - 32.</skos:definition>
        <skos:inScheme rdf:resource="http://lpis.ec.europa.eu/registry/applicationschema/cap-iacs-base/code#SpecieCodeValue"/>
    </owl:NamedIndividual>
    


    <!-- http://lpis.ec.europa.eu/registry/applicationschema/cap-iacs-base/code#SpecieCodeValue/gossypiumSppCotton -->


    <owl:NamedIndividual rdf:about="http://lpis.ec.europa.eu/registry/applicationschema/cap-iacs-base/code#SpecieCodeValue/gossypiumSppCotton">
        <rdf:type rdf:resource="http://lpis.ec.europa.eu/registry/applicationschema/cap-iacs-base#SpecieCodeValue"/>
        <rdfs:label xml:lang="en">Gossypium spp. Cotton </rdfs:label>
        <skos:definition xml:lang="en">-- Definition --
Gossypium spp. Cotton.
-- Description --
List of agricultural species -A
III. Oil and fibre plants
NOTE. Initial value: A - 66.</skos:definition>
        <skos:inScheme rdf:resource="http://lpis.ec.europa.eu/registry/applicationschema/cap-iacs-base/code#SpecieCodeValue"/>
    </owl:NamedIndividual>
    


    <!-- http://lpis.ec.europa.eu/registry/applicationschema/cap-iacs-base/code#SpecieCodeValue/hedysarumCoronariumLSulla -->


    <owl:NamedIndividual rdf:about="http://lpis.ec.europa.eu/registry/applicationschema/cap-iacs-base/code#SpecieCodeValue/hedysarumCoronariumLSulla">
        <rdf:type rdf:resource="http://lpis.ec.europa.eu/registry/applicationschema/cap-iacs-base#SpecieCodeValue"/>
        <rdfs:label xml:lang="en">Hedysarum coronarium L. Sulla </rdfs:label>
        <skos:definition xml:lang="en">-- Definition --
Hedysarum coronarium L. Sulla
-- Description --
List of agricultural species -A
II. Fodder plants
NOTE. Initial value: A - 33.</skos:definition>
        <skos:inScheme rdf:resource="http://lpis.ec.europa.eu/registry/applicationschema/cap-iacs-base/code#SpecieCodeValue"/>
    </owl:NamedIndividual>
    


    <!-- http://lpis.ec.europa.eu/registry/applicationschema/cap-iacs-base/code#SpecieCodeValue/helianthusAnnuusLSunflower -->


    <owl:NamedIndividual rdf:about="http://lpis.ec.europa.eu/registry/applicationschema/cap-iacs-base/code#SpecieCodeValue/helianthusAnnuusLSunflower">
        <rdf:type rdf:resource="http://lpis.ec.europa.eu/registry/applicationschema/cap-iacs-base#SpecieCodeValue"/>
        <rdfs:label xml:lang="en">Helianthus annuus L. Sunflower </rdfs:label>
        <skos:definition xml:lang="en">-- Definition --
Helianthus annuus L. Sunflower.
-- Description --
List of agricultural species -A
III. Oil and fibre plants
NOTE. Initial value: A - 67.</skos:definition>
        <skos:inScheme rdf:resource="http://lpis.ec.europa.eu/registry/applicationschema/cap-iacs-base/code#SpecieCodeValue"/>
    </owl:NamedIndividual>
    


    <!-- http://lpis.ec.europa.eu/registry/applicationschema/cap-iacs-base/code#SpecieCodeValue/hordeumVulgareLBarley2RowBarley -->


    <owl:NamedIndividual rdf:about="http://lpis.ec.europa.eu/registry/applicationschema/cap-iacs-base/code#SpecieCodeValue/hordeumVulgareLBarley2RowBarley">
        <rdf:type rdf:resource="http://lpis.ec.europa.eu/registry/applicationschema/cap-iacs-base#SpecieCodeValue"/>
        <rdfs:label xml:lang="en">Hordeum vulgare L. Barley 2-row barley </rdfs:label>
        <skos:definition xml:lang="en">-- Definition --
Hordeum vulgare L. Barley 2-row barley 
-- Description --
List of agricultural species -A   
IV. Cereals
NOTE. Initial value: A - 75.1</skos:definition>
        <skos:inScheme rdf:resource="http://lpis.ec.europa.eu/registry/applicationschema/cap-iacs-base/code#SpecieCodeValue"/>
    </owl:NamedIndividual>
    


    <!-- http://lpis.ec.europa.eu/registry/applicationschema/cap-iacs-base/code#SpecieCodeValue/hordeumVulgareLBarley6RowBarley -->


    <owl:NamedIndividual rdf:about="http://lpis.ec.europa.eu/registry/applicationschema/cap-iacs-base/code#SpecieCodeValue/hordeumVulgareLBarley6RowBarley">
        <rdf:type rdf:resource="http://lpis.ec.europa.eu/registry/applicationschema/cap-iacs-base#SpecieCodeValue"/>
        <rdfs:label xml:lang="en">Hordeum vulgare L. Barley 6-row barley </rdfs:label>
        <skos:definition xml:lang="en">-- Definition --
Hordeum vulgare L. Barley 6-row barley.
-- Description --
List of agricultural species -A   
IV. Cereals
NOTE. Initial value: A - 75.2</skos:definition>
        <skos:inScheme rdf:resource="http://lpis.ec.europa.eu/registry/applicationschema/cap-iacs-base/code#SpecieCodeValue"/>
    </owl:NamedIndividual>
    


    <!-- http://lpis.ec.europa.eu/registry/applicationschema/cap-iacs-base/code#SpecieCodeValue/lactucaSativaLLettuce -->


    <owl:NamedIndividual rdf:about="http://lpis.ec.europa.eu/registry/applicationschema/cap-iacs-base/code#SpecieCodeValue/lactucaSativaLLettuce">
        <rdf:type rdf:resource="http://lpis.ec.europa.eu/registry/applicationschema/cap-iacs-base#SpecieCodeValue"/>
        <rdfs:label xml:lang="en">Lactuca sativa L. Lettuce</rdfs:label>
        <skos:definition xml:lang="en">-- Definition --
Lactuca sativa L. Lettuce.
-- Description --
List of vegetable specie -H
NOTE. Initial value: H - 23.</skos:definition>
        <skos:inScheme rdf:resource="http://lpis.ec.europa.eu/registry/applicationschema/cap-iacs-base/code#SpecieCodeValue"/>
    </owl:NamedIndividual>
    


    <!-- http://lpis.ec.europa.eu/registry/applicationschema/cap-iacs-base/code#SpecieCodeValue/lagenariaSicerariaMolStandl -->


    <owl:NamedIndividual rdf:about="http://lpis.ec.europa.eu/registry/applicationschema/cap-iacs-base/code#SpecieCodeValue/lagenariaSicerariaMolStandl">
        <rdf:type rdf:resource="http://lpis.ec.europa.eu/registry/applicationschema/cap-iacs-base#SpecieCodeValue"/>
        <rdfs:label xml:lang="en">Lagenaria siceraria (Mol.) Standl.</rdfs:label>
        <skos:definition xml:lang="en">-- Definition --
Lagenaria siceraria (Mol.) Standl.
-- Description --
List of vegetable specie -H
NOTE. Initial value: H - 37.3</skos:definition>
        <skos:inScheme rdf:resource="http://lpis.ec.europa.eu/registry/applicationschema/cap-iacs-base/code#SpecieCodeValue"/>
    </owl:NamedIndividual>
    


    <!-- http://lpis.ec.europa.eu/registry/applicationschema/cap-iacs-base/code#SpecieCodeValue/linumUsitatissimumLFlaxLinseed -->


    <owl:NamedIndividual rdf:about="http://lpis.ec.europa.eu/registry/applicationschema/cap-iacs-base/code#SpecieCodeValue/linumUsitatissimumLFlaxLinseed">
        <rdf:type rdf:resource="http://lpis.ec.europa.eu/registry/applicationschema/cap-iacs-base#SpecieCodeValue"/>
        <rdfs:label xml:lang="en">Linum usitatissimum L. Flax, Linseed </rdfs:label>
        <skos:definition xml:lang="en">-- Definition --
Linum usitatissimum L. Flax, Linseed.
-- Description --
List of agricultural species -A
III. Oil and fibre plants
NOTE. Initial value: A - 68.</skos:definition>
        <skos:inScheme rdf:resource="http://lpis.ec.europa.eu/registry/applicationschema/cap-iacs-base/code#SpecieCodeValue"/>
    </owl:NamedIndividual>
    


    <!-- http://lpis.ec.europa.eu/registry/applicationschema/cap-iacs-base/code#SpecieCodeValue/loliumPerenneLPerennialRyegrass -->


    <owl:NamedIndividual rdf:about="http://lpis.ec.europa.eu/registry/applicationschema/cap-iacs-base/code#SpecieCodeValue/loliumPerenneLPerennialRyegrass">
        <rdf:type rdf:resource="http://lpis.ec.europa.eu/registry/applicationschema/cap-iacs-base#SpecieCodeValue"/>
        <rdfs:label xml:lang="en">Lolium perenne L. Perennial ryegrass</rdfs:label>
        <skos:definition xml:lang="en">-- Definition --
Lolium perenne L. Perennial ryegrass.
-- Description --
List of agricultural species -A
II. Fodder plants
NOTE. Initial value: A - 21.</skos:definition>
        <skos:inScheme rdf:resource="http://lpis.ec.europa.eu/registry/applicationschema/cap-iacs-base/code#SpecieCodeValue"/>
    </owl:NamedIndividual>
    


    <!-- http://lpis.ec.europa.eu/registry/applicationschema/cap-iacs-base/code#SpecieCodeValue/lotusCorniculatusLBirdsfootTrefoil -->


    <owl:NamedIndividual rdf:about="http://lpis.ec.europa.eu/registry/applicationschema/cap-iacs-base/code#SpecieCodeValue/lotusCorniculatusLBirdsfootTrefoil">
        <rdf:type rdf:resource="http://lpis.ec.europa.eu/registry/applicationschema/cap-iacs-base#SpecieCodeValue"/>
        <rdfs:label xml:lang="en">Lotus corniculatus L. Birdsfoot trefoil</rdfs:label>
        <skos:definition xml:lang="en">-- Definition --
Lotus corniculatus L. Birdsfoot trefoil
-- Description --
List of agricultural species -A
II. Fodder plants
NOTE. Initial value: A - 34.</skos:definition>
        <skos:inScheme rdf:resource="http://lpis.ec.europa.eu/registry/applicationschema/cap-iacs-base/code#SpecieCodeValue"/>
    </owl:NamedIndividual>
    


    <!-- http://lpis.ec.europa.eu/registry/applicationschema/cap-iacs-base/code#SpecieCodeValue/lupinusAlbusLWhiteLupin -->


    <owl:NamedIndividual rdf:about="http://lpis.ec.europa.eu/registry/applicationschema/cap-iacs-base/code#SpecieCodeValue/lupinusAlbusLWhiteLupin">
        <rdf:type rdf:resource="http://lpis.ec.europa.eu/registry/applicationschema/cap-iacs-base#SpecieCodeValue"/>
        <rdfs:label xml:lang="en">Lupinus albus L. White lupin</rdfs:label>
        <skos:definition xml:lang="en">-- Definition --
Lupinus albus L. White lupin.
-- Description --
List of agricultural species -A
II. Fodder plants
NOTE. Initial value: A - 35.</skos:definition>
        <skos:inScheme rdf:resource="http://lpis.ec.europa.eu/registry/applicationschema/cap-iacs-base/code#SpecieCodeValue"/>
    </owl:NamedIndividual>
    


    <!-- http://lpis.ec.europa.eu/registry/applicationschema/cap-iacs-base/code#SpecieCodeValue/lupinusAngustifoliusLNarrowLeavedLupin -->


    <owl:NamedIndividual rdf:about="http://lpis.ec.europa.eu/registry/applicationschema/cap-iacs-base/code#SpecieCodeValue/lupinusAngustifoliusLNarrowLeavedLupin">
        <rdf:type rdf:resource="http://lpis.ec.europa.eu/registry/applicationschema/cap-iacs-base#SpecieCodeValue"/>
        <rdfs:label xml:lang="en">Lupinus angustifolius L. Narrow leaved lupin</rdfs:label>
        <skos:definition xml:lang="en">-- Definition --
Lupinus angustifolius L. Narrow leaved lupin.
-- Description --
List of agricultural species -A
II. Fodder plants
NOTE. Initial value: A - 36.</skos:definition>
        <skos:inScheme rdf:resource="http://lpis.ec.europa.eu/registry/applicationschema/cap-iacs-base/code#SpecieCodeValue"/>
    </owl:NamedIndividual>
    


    <!-- http://lpis.ec.europa.eu/registry/applicationschema/cap-iacs-base/code#SpecieCodeValue/lupinusLuteusLYellowLupin -->


    <owl:NamedIndividual rdf:about="http://lpis.ec.europa.eu/registry/applicationschema/cap-iacs-base/code#SpecieCodeValue/lupinusLuteusLYellowLupin">
        <rdf:type rdf:resource="http://lpis.ec.europa.eu/registry/applicationschema/cap-iacs-base#SpecieCodeValue"/>
        <rdfs:label xml:lang="en">Lupinus luteus L. Yellow lupin</rdfs:label>
        <skos:definition xml:lang="en">-- Definition --
Lupinus luteus L. Yellow lupin.
-- Description --
List of agricultural species -A
II. Fodder plants
NOTE. Initial value: A - 37.</skos:definition>
        <skos:inScheme rdf:resource="http://lpis.ec.europa.eu/registry/applicationschema/cap-iacs-base/code#SpecieCodeValue"/>
    </owl:NamedIndividual>
    


    <!-- http://lpis.ec.europa.eu/registry/applicationschema/cap-iacs-base/code#SpecieCodeValue/lycopersiconEsculentumLxLPimpinellifolium -->


    <owl:NamedIndividual rdf:about="http://lpis.ec.europa.eu/registry/applicationschema/cap-iacs-base/code#SpecieCodeValue/lycopersiconEsculentumLxLPimpinellifolium">
        <rdf:type rdf:resource="http://lpis.ec.europa.eu/registry/applicationschema/cap-iacs-base#SpecieCodeValue"/>
        <rdfs:label xml:lang="en">Lycopersicon esculentum L. x L. pimpinellifolium</rdfs:label>
        <skos:definition xml:lang="en">-- Definition --
Lycopersicon esculentum L. x L. pimpinellifolium.
-- Description --
List of vegetable specie -H
NOTE. Initial value: H - 37.5</skos:definition>
        <skos:inScheme rdf:resource="http://lpis.ec.europa.eu/registry/applicationschema/cap-iacs-base/code#SpecieCodeValue"/>
    </owl:NamedIndividual>
    


    <!-- http://lpis.ec.europa.eu/registry/applicationschema/cap-iacs-base/code#SpecieCodeValue/lycopersiconEsculentumLxSHabrochaite -->


    <owl:NamedIndividual rdf:about="http://lpis.ec.europa.eu/registry/applicationschema/cap-iacs-base/code#SpecieCodeValue/lycopersiconEsculentumLxSHabrochaite">
        <rdf:type rdf:resource="http://lpis.ec.europa.eu/registry/applicationschema/cap-iacs-base#SpecieCodeValue"/>
        <rdfs:label xml:lang="en">Lycopersicon esculentum L. x S. habrochaites</rdfs:label>
        <skos:definition xml:lang="en">-- Definition --
Lycopersicon esculentum L. x S. habrochaites.
-- Description --
List of vegetable specie -H
NOTE. Initial value: H - 37.4</skos:definition>
        <skos:inScheme rdf:resource="http://lpis.ec.europa.eu/registry/applicationschema/cap-iacs-base/code#SpecieCodeValue"/>
    </owl:NamedIndividual>
    


    <!-- http://lpis.ec.europa.eu/registry/applicationschema/cap-iacs-base/code#SpecieCodeValue/lycopersiconEsculentumMillTomato -->


    <owl:NamedIndividual rdf:about="http://lpis.ec.europa.eu/registry/applicationschema/cap-iacs-base/code#SpecieCodeValue/lycopersiconEsculentumMillTomato">
        <rdf:type rdf:resource="http://lpis.ec.europa.eu/registry/applicationschema/cap-iacs-base#SpecieCodeValue"/>
        <rdfs:label xml:lang="en">Lycopersicon esculentum Mill. Tomato</rdfs:label>
        <skos:definition xml:lang="en">-- Definition --
Lycopersicon esculentum Mill. Tomato.
-- Description --
List of vegetable specie -H
NOTE. Initial value: H - 24.</skos:definition>
        <skos:inScheme rdf:resource="http://lpis.ec.europa.eu/registry/applicationschema/cap-iacs-base/code#SpecieCodeValue"/>
    </owl:NamedIndividual>
    


    <!-- http://lpis.ec.europa.eu/registry/applicationschema/cap-iacs-base/code#SpecieCodeValue/medicagoLupulinaLTrefoil -->


    <owl:NamedIndividual rdf:about="http://lpis.ec.europa.eu/registry/applicationschema/cap-iacs-base/code#SpecieCodeValue/medicagoLupulinaLTrefoil">
        <rdf:type rdf:resource="http://lpis.ec.europa.eu/registry/applicationschema/cap-iacs-base#SpecieCodeValue"/>
        <rdfs:label xml:lang="en">Medicago lupulina L. Trefoil</rdfs:label>
        <skos:definition xml:lang="en">-- Definition --
Medicago lupulina L. Trefoil.
-- Description --
List of agricultural species -A
II. Fodder plants
NOTE. Initial value: A - 38.</skos:definition>
        <skos:inScheme rdf:resource="http://lpis.ec.europa.eu/registry/applicationschema/cap-iacs-base/code#SpecieCodeValue"/>
    </owl:NamedIndividual>
    


    <!-- http://lpis.ec.europa.eu/registry/applicationschema/cap-iacs-base/code#SpecieCodeValue/medicagoSativaLLucerne -->


    <owl:NamedIndividual rdf:about="http://lpis.ec.europa.eu/registry/applicationschema/cap-iacs-base/code#SpecieCodeValue/medicagoSativaLLucerne">
        <rdf:type rdf:resource="http://lpis.ec.europa.eu/registry/applicationschema/cap-iacs-base#SpecieCodeValue"/>
        <rdfs:label xml:lang="en">Medicago sativa L. Lucerne </rdfs:label>
        <skos:definition xml:lang="en">-- Definition --
Medicago sativa L. Lucerne.
-- Description --
List of agricultural species -A
II. Fodder plants
NOTE. Initial value: A - 39.</skos:definition>
        <skos:inScheme rdf:resource="http://lpis.ec.europa.eu/registry/applicationschema/cap-iacs-base/code#SpecieCodeValue"/>
    </owl:NamedIndividual>
    


    <!-- http://lpis.ec.europa.eu/registry/applicationschema/cap-iacs-base/code#SpecieCodeValue/onobrychisViciifoliaScopSainfoin -->


    <owl:NamedIndividual rdf:about="http://lpis.ec.europa.eu/registry/applicationschema/cap-iacs-base/code#SpecieCodeValue/onobrychisViciifoliaScopSainfoin">
        <rdf:type rdf:resource="http://lpis.ec.europa.eu/registry/applicationschema/cap-iacs-base#SpecieCodeValue"/>
        <rdfs:label xml:lang="en">Onobrychis viciifolia Scop. Sainfoin</rdfs:label>
        <skos:definition xml:lang="en">-- Definition --
Onobrychis viciifolia Scop. Sainfoin.
-- Description --
List of agricultural species -A
II. Fodder plants
NOTE. Initial value: A - 41.</skos:definition>
        <skos:inScheme rdf:resource="http://lpis.ec.europa.eu/registry/applicationschema/cap-iacs-base/code#SpecieCodeValue"/>
    </owl:NamedIndividual>
    


    <!-- http://lpis.ec.europa.eu/registry/applicationschema/cap-iacs-base/code#SpecieCodeValue/oryzaSativaLRice -->


    <owl:NamedIndividual rdf:about="http://lpis.ec.europa.eu/registry/applicationschema/cap-iacs-base/code#SpecieCodeValue/oryzaSativaLRice">
        <rdf:type rdf:resource="http://lpis.ec.europa.eu/registry/applicationschema/cap-iacs-base#SpecieCodeValue"/>
        <rdfs:label xml:lang="en">Oryza sativa L. Rice </rdfs:label>
        <skos:definition xml:lang="en">-- Definition --
Oryza sativa L. Rice.
-- Description --
List of agricultural species -A   
IV. Cereals
NOTE. Initial value: A - 76.</skos:definition>
        <skos:inScheme rdf:resource="http://lpis.ec.europa.eu/registry/applicationschema/cap-iacs-base/code#SpecieCodeValue"/>
    </owl:NamedIndividual>
    


    <!-- http://lpis.ec.europa.eu/registry/applicationschema/cap-iacs-base/code#SpecieCodeValue/papaverSomniferumLPoppy -->


    <owl:NamedIndividual rdf:about="http://lpis.ec.europa.eu/registry/applicationschema/cap-iacs-base/code#SpecieCodeValue/papaverSomniferumLPoppy">
        <rdf:type rdf:resource="http://lpis.ec.europa.eu/registry/applicationschema/cap-iacs-base#SpecieCodeValue"/>
        <rdfs:label xml:lang="en">Papaver somniferum L. Poppy</rdfs:label>
        <skos:definition xml:lang="en">-- Definition --
Papaver somniferum L. Poppy.
-- Description --
List of agricultural species -A
III. Oil and fibre plants
NOTE. Initial value: A - 69.</skos:definition>
        <skos:inScheme rdf:resource="http://lpis.ec.europa.eu/registry/applicationschema/cap-iacs-base/code#SpecieCodeValue"/>
    </owl:NamedIndividual>
    


    <!-- http://lpis.ec.europa.eu/registry/applicationschema/cap-iacs-base/code#SpecieCodeValue/petroselinumCrispumMillNymanExAWHillParsley -->


    <owl:NamedIndividual rdf:about="http://lpis.ec.europa.eu/registry/applicationschema/cap-iacs-base/code#SpecieCodeValue/petroselinumCrispumMillNymanExAWHillParsley">
        <rdf:type rdf:resource="http://lpis.ec.europa.eu/registry/applicationschema/cap-iacs-base#SpecieCodeValue"/>
        <rdfs:label xml:lang="en">Petroselinum crispum (Mill.) Nyman ex A. W. Hill Parsley</rdfs:label>
        <skos:definition xml:lang="en">-- Definition --
Petroselinum crispum (Mill.) Nyman ex A. W. Hill Parsley.
-- Description --
List of vegetable specie -H
NOTE. Initial value: H - 25.</skos:definition>
        <skos:inScheme rdf:resource="http://lpis.ec.europa.eu/registry/applicationschema/cap-iacs-base/code#SpecieCodeValue"/>
    </owl:NamedIndividual>
    


    <!-- http://lpis.ec.europa.eu/registry/applicationschema/cap-iacs-base/code#SpecieCodeValue/phaceliaTanacetifoliaLCaliforniaBluebell -->


    <owl:NamedIndividual rdf:about="http://lpis.ec.europa.eu/registry/applicationschema/cap-iacs-base/code#SpecieCodeValue/phaceliaTanacetifoliaLCaliforniaBluebell">
        <rdf:type rdf:resource="http://lpis.ec.europa.eu/registry/applicationschema/cap-iacs-base#SpecieCodeValue"/>
        <rdfs:label xml:lang="en">Phacelia tanacetifolia L. California bluebell </rdfs:label>
        <skos:definition xml:lang="en">-- Definition --
Phacelia tanacetifolia L. California bluebell.
-- Description --
List of agricultural species -A
II. Fodder plants
NOTE. Initial value: A - 56.</skos:definition>
        <skos:inScheme rdf:resource="http://lpis.ec.europa.eu/registry/applicationschema/cap-iacs-base/code#SpecieCodeValue"/>
    </owl:NamedIndividual>
    


    <!-- http://lpis.ec.europa.eu/registry/applicationschema/cap-iacs-base/code#SpecieCodeValue/phalarisAquaticaLHardingGrassPhalaris -->


    <owl:NamedIndividual rdf:about="http://lpis.ec.europa.eu/registry/applicationschema/cap-iacs-base/code#SpecieCodeValue/phalarisAquaticaLHardingGrassPhalaris">
        <rdf:type rdf:resource="http://lpis.ec.europa.eu/registry/applicationschema/cap-iacs-base#SpecieCodeValue"/>
        <rdfs:label xml:lang="en">Phalaris aquatica L. Harding grass/Phalaris</rdfs:label>
        <skos:definition xml:lang="en">-- Definition --
Phalaris aquatica L. Harding grass/Phalaris.
-- Description --
List of agricultural species -A
II. Fodder plants
NOTE. Initial value: A - 23.</skos:definition>
        <skos:inScheme rdf:resource="http://lpis.ec.europa.eu/registry/applicationschema/cap-iacs-base/code#SpecieCodeValue"/>
    </owl:NamedIndividual>
    


    <!-- http://lpis.ec.europa.eu/registry/applicationschema/cap-iacs-base/code#SpecieCodeValue/phalarisCanariensisLCanaryGrass -->


    <owl:NamedIndividual rdf:about="http://lpis.ec.europa.eu/registry/applicationschema/cap-iacs-base/code#SpecieCodeValue/phalarisCanariensisLCanaryGrass">
        <rdf:type rdf:resource="http://lpis.ec.europa.eu/registry/applicationschema/cap-iacs-base#SpecieCodeValue"/>
        <rdfs:label xml:lang="en">Phalaris canariensis L. Canary grass</rdfs:label>
        <skos:definition xml:lang="en">-- Definition --
Phalaris canariensis L. Canary grass.
-- Description --
List of agricultural species -A   
IV. Cereals
NOTE. Initial value: A - 77.</skos:definition>
        <skos:inScheme rdf:resource="http://lpis.ec.europa.eu/registry/applicationschema/cap-iacs-base/code#SpecieCodeValue"/>
    </owl:NamedIndividual>
    


    <!-- http://lpis.ec.europa.eu/registry/applicationschema/cap-iacs-base/code#SpecieCodeValue/phaseolusCoccineusLRunnerBean -->


    <owl:NamedIndividual rdf:about="http://lpis.ec.europa.eu/registry/applicationschema/cap-iacs-base/code#SpecieCodeValue/phaseolusCoccineusLRunnerBean">
        <rdf:type rdf:resource="http://lpis.ec.europa.eu/registry/applicationschema/cap-iacs-base#SpecieCodeValue"/>
        <rdfs:label xml:lang="en">Phaseolus coccineus L. Runner bean</rdfs:label>
        <skos:definition xml:lang="en">-- Definition --
Phaseolus coccineus L. Runner bean.
-- Description --
List of vegetable specie -H
NOTE. Initial value: H - 26.</skos:definition>
        <skos:inScheme rdf:resource="http://lpis.ec.europa.eu/registry/applicationschema/cap-iacs-base/code#SpecieCodeValue"/>
    </owl:NamedIndividual>
    


    <!-- http://lpis.ec.europa.eu/registry/applicationschema/cap-iacs-base/code#SpecieCodeValue/phaseolusVulgarisLClimbingFrenchBean -->


    <owl:NamedIndividual rdf:about="http://lpis.ec.europa.eu/registry/applicationschema/cap-iacs-base/code#SpecieCodeValue/phaseolusVulgarisLClimbingFrenchBean">
        <rdf:type rdf:resource="http://lpis.ec.europa.eu/registry/applicationschema/cap-iacs-base#SpecieCodeValue"/>
        <rdfs:label xml:lang="en">Phaseolus vulgaris L. Climbing French bean</rdfs:label>
        <skos:definition xml:lang="en">-- Definition --
Phaseolus vulgaris L. Climbing French bean.
-- Description --
List of vegetable specie -H
NOTE. Initial value: H - 27.2</skos:definition>
        <skos:inScheme rdf:resource="http://lpis.ec.europa.eu/registry/applicationschema/cap-iacs-base/code#SpecieCodeValue"/>
    </owl:NamedIndividual>
    


    <!-- http://lpis.ec.europa.eu/registry/applicationschema/cap-iacs-base/code#SpecieCodeValue/phaseolusVulgarisLDwarfFrenchBean -->


    <owl:NamedIndividual rdf:about="http://lpis.ec.europa.eu/registry/applicationschema/cap-iacs-base/code#SpecieCodeValue/phaseolusVulgarisLDwarfFrenchBean">
        <rdf:type rdf:resource="http://lpis.ec.europa.eu/registry/applicationschema/cap-iacs-base#SpecieCodeValue"/>
        <rdfs:label xml:lang="en">Phaseolus vulgaris L. Dwarf French bean</rdfs:label>
        <skos:definition xml:lang="en">-- Definition --
Phaseolus vulgaris L. Dwarf French bean.
-- Description --
List of vegetable specie -H
NOTE. Initial value: H - 27.1</skos:definition>
        <skos:inScheme rdf:resource="http://lpis.ec.europa.eu/registry/applicationschema/cap-iacs-base/code#SpecieCodeValue"/>
    </owl:NamedIndividual>
    


    <!-- http://lpis.ec.europa.eu/registry/applicationschema/cap-iacs-base/code#SpecieCodeValue/phleumNodosumLSmallTimothy -->


    <owl:NamedIndividual rdf:about="http://lpis.ec.europa.eu/registry/applicationschema/cap-iacs-base/code#SpecieCodeValue/phleumNodosumLSmallTimothy">
        <rdf:type rdf:resource="http://lpis.ec.europa.eu/registry/applicationschema/cap-iacs-base#SpecieCodeValue"/>
        <rdfs:label xml:lang="en">Phleum nodosum L. Small timothy</rdfs:label>
        <skos:definition xml:lang="en">-- Definition --
Phleum nodosum L. Small timothy.
-- Description --
List of agricultural species -A
II. Fodder plants
NOTE. Initial value: A - 24.</skos:definition>
        <skos:inScheme rdf:resource="http://lpis.ec.europa.eu/registry/applicationschema/cap-iacs-base/code#SpecieCodeValue"/>
    </owl:NamedIndividual>
    


    <!-- http://lpis.ec.europa.eu/registry/applicationschema/cap-iacs-base/code#SpecieCodeValue/phleumPratenseLTimothy -->


    <owl:NamedIndividual rdf:about="http://lpis.ec.europa.eu/registry/applicationschema/cap-iacs-base/code#SpecieCodeValue/phleumPratenseLTimothy">
        <rdf:type rdf:resource="http://lpis.ec.europa.eu/registry/applicationschema/cap-iacs-base#SpecieCodeValue"/>
        <rdfs:label xml:lang="en">Phleum pratense L. Timothy </rdfs:label>
        <skos:definition xml:lang="en">-- Definition --
Phleum pratense L. Timothy.
-- Description --
List of agricultural species -A
II. Fodder plants
NOTE. Initial value: A - 25.</skos:definition>
        <skos:inScheme rdf:resource="http://lpis.ec.europa.eu/registry/applicationschema/cap-iacs-base/code#SpecieCodeValue"/>
    </owl:NamedIndividual>
    


    <!-- http://lpis.ec.europa.eu/registry/applicationschema/cap-iacs-base/code#SpecieCodeValue/pisumSativumLPartimFieldPea -->


    <owl:NamedIndividual rdf:about="http://lpis.ec.europa.eu/registry/applicationschema/cap-iacs-base/code#SpecieCodeValue/pisumSativumLPartimFieldPea">
        <rdf:type rdf:resource="http://lpis.ec.europa.eu/registry/applicationschema/cap-iacs-base#SpecieCodeValue"/>
        <rdfs:label xml:lang="en">Pisum sativum L. (Partim) Field pea</rdfs:label>
        <skos:definition xml:lang="en">-- Definition --
Pisum sativum L. (Partim) Field pea.
-- Description --
List of agricultural species -A
II. Fodder plants
NOTE. Initial value: A - 42.</skos:definition>
        <skos:inScheme rdf:resource="http://lpis.ec.europa.eu/registry/applicationschema/cap-iacs-base/code#SpecieCodeValue"/>
    </owl:NamedIndividual>
    


    <!-- http://lpis.ec.europa.eu/registry/applicationschema/cap-iacs-base/code#SpecieCodeValue/pisumSativumLPartimRoundPea -->


    <owl:NamedIndividual rdf:about="http://lpis.ec.europa.eu/registry/applicationschema/cap-iacs-base/code#SpecieCodeValue/pisumSativumLPartimRoundPea">
        <rdf:type rdf:resource="http://lpis.ec.europa.eu/registry/applicationschema/cap-iacs-base#SpecieCodeValue"/>
        <rdfs:label xml:lang="en">Pisum sativum L. (partim) Round pea</rdfs:label>
        <skos:definition xml:lang="en">-- Definition --
Pisum sativum L. (partim) Round pea.
-- Description --
List of vegetable specie -H
NOTE. Initial value: H - 28.2</skos:definition>
        <skos:inScheme rdf:resource="http://lpis.ec.europa.eu/registry/applicationschema/cap-iacs-base/code#SpecieCodeValue"/>
    </owl:NamedIndividual>
    


    <!-- http://lpis.ec.europa.eu/registry/applicationschema/cap-iacs-base/code#SpecieCodeValue/pisumSativumLPartimSugarPea -->


    <owl:NamedIndividual rdf:about="http://lpis.ec.europa.eu/registry/applicationschema/cap-iacs-base/code#SpecieCodeValue/pisumSativumLPartimSugarPea">
        <rdf:type rdf:resource="http://lpis.ec.europa.eu/registry/applicationschema/cap-iacs-base#SpecieCodeValue"/>
        <rdfs:label xml:lang="en">Pisum sativum L. (partim) Sugar pea</rdfs:label>
        <skos:definition xml:lang="en">-- Definition --
Pisum sativum L. (partim) Sugar pea.
-- Description --
List of vegetable specie -H
NOTE. Initial value:H - 28.3</skos:definition>
        <skos:inScheme rdf:resource="http://lpis.ec.europa.eu/registry/applicationschema/cap-iacs-base/code#SpecieCodeValue"/>
    </owl:NamedIndividual>
    


    <!-- http://lpis.ec.europa.eu/registry/applicationschema/cap-iacs-base/code#SpecieCodeValue/pisumSativumLPartimWrinkledPea -->


    <owl:NamedIndividual rdf:about="http://lpis.ec.europa.eu/registry/applicationschema/cap-iacs-base/code#SpecieCodeValue/pisumSativumLPartimWrinkledPea">
        <rdf:type rdf:resource="http://lpis.ec.europa.eu/registry/applicationschema/cap-iacs-base#SpecieCodeValue"/>
        <rdfs:label xml:lang="en">Pisum sativum L. (partim) Wrinkled pea</rdfs:label>
        <skos:definition xml:lang="en">-- Definition --
Pisum sativum L. (partim) Wrinkled pea.
-- Description --
List of vegetable specie -H
NOTE. Initial value: H - 28.1</skos:definition>
        <skos:inScheme rdf:resource="http://lpis.ec.europa.eu/registry/applicationschema/cap-iacs-base/code#SpecieCodeValue"/>
    </owl:NamedIndividual>
    


    <!-- http://lpis.ec.europa.eu/registry/applicationschema/cap-iacs-base/code#SpecieCodeValue/poaAnnuaLAnnualMeadowgrass -->


    <owl:NamedIndividual rdf:about="http://lpis.ec.europa.eu/registry/applicationschema/cap-iacs-base/code#SpecieCodeValue/poaAnnuaLAnnualMeadowgrass">
        <rdf:type rdf:resource="http://lpis.ec.europa.eu/registry/applicationschema/cap-iacs-base#SpecieCodeValue"/>
        <rdfs:label xml:lang="en">Poa annua L. Annual meadowgrass</rdfs:label>
        <skos:definition xml:lang="en">-- Definition --
Poa annua L. Annual meadowgrass.
-- Description --
List of agricultural species -A
II. Fodder plants
NOTE. Initial value: A - 26.</skos:definition>
        <skos:inScheme rdf:resource="http://lpis.ec.europa.eu/registry/applicationschema/cap-iacs-base/code#SpecieCodeValue"/>
    </owl:NamedIndividual>
    


    <!-- http://lpis.ec.europa.eu/registry/applicationschema/cap-iacs-base/code#SpecieCodeValue/poaNemoralisLWoodMeadowgrass -->


    <owl:NamedIndividual rdf:about="http://lpis.ec.europa.eu/registry/applicationschema/cap-iacs-base/code#SpecieCodeValue/poaNemoralisLWoodMeadowgrass">
        <rdf:type rdf:resource="http://lpis.ec.europa.eu/registry/applicationschema/cap-iacs-base#SpecieCodeValue"/>
        <rdfs:label xml:lang="en">Poa nemoralis L.Wood meadowgrass</rdfs:label>
        <skos:definition xml:lang="en">-- Definition --
Poa nemoralis L.Wood meadowgrass
-- Description --
List of agricultural species -A
II. Fodder plants
NOTE. Initial value: A - 27.</skos:definition>
        <skos:inScheme rdf:resource="http://lpis.ec.europa.eu/registry/applicationschema/cap-iacs-base/code#SpecieCodeValue"/>
    </owl:NamedIndividual>
    


    <!-- http://lpis.ec.europa.eu/registry/applicationschema/cap-iacs-base/code#SpecieCodeValue/poaPalustrisLSwampMeadowgras -->


    <owl:NamedIndividual rdf:about="http://lpis.ec.europa.eu/registry/applicationschema/cap-iacs-base/code#SpecieCodeValue/poaPalustrisLSwampMeadowgras">
        <rdf:type rdf:resource="http://lpis.ec.europa.eu/registry/applicationschema/cap-iacs-base#SpecieCodeValue"/>
        <rdfs:label xml:lang="en">Poa palustris L. Swamp meadowgras</rdfs:label>
        <skos:definition xml:lang="en">-- Definition --
Poa palustris L. Swamp meadowgras.
-- Description --
List of agricultural species -A
II. Fodder plants
NOTE. Initial value: A - 28.</skos:definition>
        <skos:inScheme rdf:resource="http://lpis.ec.europa.eu/registry/applicationschema/cap-iacs-base/code#SpecieCodeValue"/>
    </owl:NamedIndividual>
    


    <!-- http://lpis.ec.europa.eu/registry/applicationschema/cap-iacs-base/code#SpecieCodeValue/poaPratensisLSmoothStalkedMeadowgrass -->


    <owl:NamedIndividual rdf:about="http://lpis.ec.europa.eu/registry/applicationschema/cap-iacs-base/code#SpecieCodeValue/poaPratensisLSmoothStalkedMeadowgrass">
        <rdf:type rdf:resource="http://lpis.ec.europa.eu/registry/applicationschema/cap-iacs-base#SpecieCodeValue"/>
        <rdfs:label xml:lang="en">Poa pratensis L. Smooth-stalked meadowgrass</rdfs:label>
        <skos:definition xml:lang="en">-- Definition --
Poa pratensis L. Smooth-stalked meadowgrass.
-- Description --
List of agricultural species -A
II. Fodder plants
NOTE. Initial value: A - 29.</skos:definition>
        <skos:inScheme rdf:resource="http://lpis.ec.europa.eu/registry/applicationschema/cap-iacs-base/code#SpecieCodeValue"/>
    </owl:NamedIndividual>
    


    <!-- http://lpis.ec.europa.eu/registry/applicationschema/cap-iacs-base/code#SpecieCodeValue/poaTrivialisLRoughStalkedMeadowgrass -->


    <owl:NamedIndividual rdf:about="http://lpis.ec.europa.eu/registry/applicationschema/cap-iacs-base/code#SpecieCodeValue/poaTrivialisLRoughStalkedMeadowgrass">
        <rdf:type rdf:resource="http://lpis.ec.europa.eu/registry/applicationschema/cap-iacs-base#SpecieCodeValue"/>
        <rdfs:label xml:lang="en">Poa trivialis L. Rough-stalked meadowgrass</rdfs:label>
        <skos:definition xml:lang="en">-- Definition --
Poa trivialis L. Rough-stalked meadowgrass.
-- Description --
List of agricultural species -A
II. Fodder plants
NOTE. Initial value: A - 30.</skos:definition>
        <skos:inScheme rdf:resource="http://lpis.ec.europa.eu/registry/applicationschema/cap-iacs-base/code#SpecieCodeValue"/>
    </owl:NamedIndividual>
    


    <!-- http://lpis.ec.europa.eu/registry/applicationschema/cap-iacs-base/code#SpecieCodeValue/raphanusSativusLBlackRadish -->


    <owl:NamedIndividual rdf:about="http://lpis.ec.europa.eu/registry/applicationschema/cap-iacs-base/code#SpecieCodeValue/raphanusSativusLBlackRadish">
        <rdf:type rdf:resource="http://lpis.ec.europa.eu/registry/applicationschema/cap-iacs-base#SpecieCodeValue"/>
        <rdfs:label xml:lang="en">Raphanus sativus L. Black radish</rdfs:label>
        <skos:definition xml:lang="en">-- Definition --
Raphanus sativus L. Black radish.
-- Description --
List of vegetable specie -H
NOTE. Initial value: H - 29.2</skos:definition>
        <skos:inScheme rdf:resource="http://lpis.ec.europa.eu/registry/applicationschema/cap-iacs-base/code#SpecieCodeValue"/>
    </owl:NamedIndividual>
    


    <!-- http://lpis.ec.europa.eu/registry/applicationschema/cap-iacs-base/code#SpecieCodeValue/raphanusSativusLRadish -->


    <owl:NamedIndividual rdf:about="http://lpis.ec.europa.eu/registry/applicationschema/cap-iacs-base/code#SpecieCodeValue/raphanusSativusLRadish">
        <rdf:type rdf:resource="http://lpis.ec.europa.eu/registry/applicationschema/cap-iacs-base#SpecieCodeValue"/>
        <rdfs:label xml:lang="en">Raphanus sativus L. Radish</rdfs:label>
        <skos:definition xml:lang="en">-- Definition --
Raphanus sativus L. Radish.
-- Description --
List of vegetable specie -H
NOTE. Initial value: H - 29.1</skos:definition>
        <skos:inScheme rdf:resource="http://lpis.ec.europa.eu/registry/applicationschema/cap-iacs-base/code#SpecieCodeValue"/>
    </owl:NamedIndividual>
    


    <!-- http://lpis.ec.europa.eu/registry/applicationschema/cap-iacs-base/code#SpecieCodeValue/raphanusSativusLVarOleiformisPersFodderRadish -->


    <owl:NamedIndividual rdf:about="http://lpis.ec.europa.eu/registry/applicationschema/cap-iacs-base/code#SpecieCodeValue/raphanusSativusLVarOleiformisPersFodderRadish">
        <rdf:type rdf:resource="http://lpis.ec.europa.eu/registry/applicationschema/cap-iacs-base#SpecieCodeValue"/>
        <rdfs:label xml:lang="en">Raphanus sativus L. var. oleiformis Pers. Fodder radish</rdfs:label>
        <skos:definition xml:lang="en">-- Definition --
Raphanus sativus L. var. oleiformis Pers. Fodder radish.
-- Description --
List of agricultural species -A
II. Fodder plants
NOTE. Initial value: A - 57.</skos:definition>
        <skos:inScheme rdf:resource="http://lpis.ec.europa.eu/registry/applicationschema/cap-iacs-base/code#SpecieCodeValue"/>
    </owl:NamedIndividual>
    


    <!-- http://lpis.ec.europa.eu/registry/applicationschema/cap-iacs-base/code#SpecieCodeValue/rheumRhabarbarumLRhubarb -->


    <owl:NamedIndividual rdf:about="http://lpis.ec.europa.eu/registry/applicationschema/cap-iacs-base/code#SpecieCodeValue/rheumRhabarbarumLRhubarb">
        <rdf:type rdf:resource="http://lpis.ec.europa.eu/registry/applicationschema/cap-iacs-base#SpecieCodeValue"/>
        <rdfs:label xml:lang="en">Rheum rhabarbarum L. Rhubarb</rdfs:label>
        <skos:definition xml:lang="en">-- Definition --
Rheum rhabarbarum L. Rhubarb.
-- Description --
List of vegetable specie -H
NOTE. Initial value: H - 30.</skos:definition>
        <skos:inScheme rdf:resource="http://lpis.ec.europa.eu/registry/applicationschema/cap-iacs-base/code#SpecieCodeValue"/>
    </owl:NamedIndividual>
    


    <!-- http://lpis.ec.europa.eu/registry/applicationschema/cap-iacs-base/code#SpecieCodeValue/scorzoneraHispanicaLScorzoneraBlackSalsify -->


    <owl:NamedIndividual rdf:about="http://lpis.ec.europa.eu/registry/applicationschema/cap-iacs-base/code#SpecieCodeValue/scorzoneraHispanicaLScorzoneraBlackSalsify">
        <rdf:type rdf:resource="http://lpis.ec.europa.eu/registry/applicationschema/cap-iacs-base#SpecieCodeValue"/>
        <rdfs:label xml:lang="en">Scorzonera hispanica L. Scorzonera / Black salsify</rdfs:label>
        <skos:definition xml:lang="en">-- Definition --
Scorzonera hispanica L. Scorzonera / Black salsify.
-- Description --
List of vegetable specie -H
NOTE. Initial value: H - 31.</skos:definition>
        <skos:inScheme rdf:resource="http://lpis.ec.europa.eu/registry/applicationschema/cap-iacs-base/code#SpecieCodeValue"/>
    </owl:NamedIndividual>
    


    <!-- http://lpis.ec.europa.eu/registry/applicationschema/cap-iacs-base/code#SpecieCodeValue/secaleCerealeLRye -->


    <owl:NamedIndividual rdf:about="http://lpis.ec.europa.eu/registry/applicationschema/cap-iacs-base/code#SpecieCodeValue/secaleCerealeLRye">
        <rdf:type rdf:resource="http://lpis.ec.europa.eu/registry/applicationschema/cap-iacs-base#SpecieCodeValue"/>
        <rdfs:label xml:lang="en">Secale cereale L. Rye   </rdfs:label>
        <skos:definition xml:lang="en">-- Definition --
Secale cereale L. Rye.
-- Description --
List of agricultural species -A   
IV. Cereals
NOTE. Initial value: A - 78.</skos:definition>
        <skos:inScheme rdf:resource="http://lpis.ec.europa.eu/registry/applicationschema/cap-iacs-base/code#SpecieCodeValue"/>
    </owl:NamedIndividual>
    


    <!-- http://lpis.ec.europa.eu/registry/applicationschema/cap-iacs-base/code#SpecieCodeValue/sicyosAngulatus -->


    <owl:NamedIndividual rdf:about="http://lpis.ec.europa.eu/registry/applicationschema/cap-iacs-base/code#SpecieCodeValue/sicyosAngulatus">
        <rdf:type rdf:resource="http://lpis.ec.europa.eu/registry/applicationschema/cap-iacs-base#SpecieCodeValue"/>
        <rdfs:label xml:lang="en">Sicyos angulatus</rdfs:label>
        <skos:definition xml:lang="en">-- Definition --
Sicyos angulatus.
-- Description --
List of vegetable specie -H
NOTE. Initial value: H - 37.6</skos:definition>
        <skos:inScheme rdf:resource="http://lpis.ec.europa.eu/registry/applicationschema/cap-iacs-base/code#SpecieCodeValue"/>
    </owl:NamedIndividual>
    


    <!-- http://lpis.ec.europa.eu/registry/applicationschema/cap-iacs-base/code#SpecieCodeValue/sinapisAlbaLWhiteMustard -->


    <owl:NamedIndividual rdf:about="http://lpis.ec.europa.eu/registry/applicationschema/cap-iacs-base/code#SpecieCodeValue/sinapisAlbaLWhiteMustard">
        <rdf:type rdf:resource="http://lpis.ec.europa.eu/registry/applicationschema/cap-iacs-base#SpecieCodeValue"/>
        <rdfs:label xml:lang="en">Sinapis alba L. White mustard</rdfs:label>
        <skos:definition xml:lang="en">-- Definition --
Sinapis alba L. White mustard.
-- Description --
List of agricultural species -A
III. Oil and fibre plants
NOTE. Initial value: A - 70.</skos:definition>
        <skos:inScheme rdf:resource="http://lpis.ec.europa.eu/registry/applicationschema/cap-iacs-base/code#SpecieCodeValue"/>
    </owl:NamedIndividual>
    


    <!-- http://lpis.ec.europa.eu/registry/applicationschema/cap-iacs-base/code#SpecieCodeValue/slycineMaxLMerrillSoyaBean -->


    <owl:NamedIndividual rdf:about="http://lpis.ec.europa.eu/registry/applicationschema/cap-iacs-base/code#SpecieCodeValue/slycineMaxLMerrillSoyaBean">
        <rdf:type rdf:resource="http://lpis.ec.europa.eu/registry/applicationschema/cap-iacs-base#SpecieCodeValue"/>
        <rdfs:label xml:lang="en">Glycine max (L.) Merrill Soya bean  </rdfs:label>
        <skos:definition xml:lang="en">-- Definition --
Glycine max (L.) Merrill Soya bean.
-- Description --
List of agricultural species -A
III. Oil and fibre plants
NOTE. Initial value: A - 71.</skos:definition>
        <skos:inScheme rdf:resource="http://lpis.ec.europa.eu/registry/applicationschema/cap-iacs-base/code#SpecieCodeValue"/>
    </owl:NamedIndividual>
    


    <!-- http://lpis.ec.europa.eu/registry/applicationschema/cap-iacs-base/code#SpecieCodeValue/solanumMelongenaLAubergineEggPlant -->


    <owl:NamedIndividual rdf:about="http://lpis.ec.europa.eu/registry/applicationschema/cap-iacs-base/code#SpecieCodeValue/solanumMelongenaLAubergineEggPlant">
        <rdf:type rdf:resource="http://lpis.ec.europa.eu/registry/applicationschema/cap-iacs-base#SpecieCodeValue"/>
        <rdfs:label xml:lang="en">Solanum melongena L. Aubergine / Egg plant</rdfs:label>
        <skos:definition xml:lang="en">-- Definition --
Solanum melongena L. Aubergine / Egg plant.
-- Description --
List of vegetable specie -H
NOTE. Initial value: H - 32.</skos:definition>
        <skos:inScheme rdf:resource="http://lpis.ec.europa.eu/registry/applicationschema/cap-iacs-base/code#SpecieCodeValue"/>
    </owl:NamedIndividual>
    


    <!-- http://lpis.ec.europa.eu/registry/applicationschema/cap-iacs-base/code#SpecieCodeValue/solanumTorvumSw -->


    <owl:NamedIndividual rdf:about="http://lpis.ec.europa.eu/registry/applicationschema/cap-iacs-base/code#SpecieCodeValue/solanumTorvumSw">
        <rdf:type rdf:resource="http://lpis.ec.europa.eu/registry/applicationschema/cap-iacs-base#SpecieCodeValue"/>
        <rdfs:label xml:lang="en">Solanum torvum Sw.</rdfs:label>
        <skos:definition xml:lang="en">-- Definition --
Solanum torvum Sw.
-- Description --
List of vegetable specie -H
NOTE. Initial value: H - 37.8</skos:definition>
        <skos:inScheme rdf:resource="http://lpis.ec.europa.eu/registry/applicationschema/cap-iacs-base/code#SpecieCodeValue"/>
    </owl:NamedIndividual>
    


    <!-- http://lpis.ec.europa.eu/registry/applicationschema/cap-iacs-base/code#SpecieCodeValue/solanumTuberosumLPotato -->


    <owl:NamedIndividual rdf:about="http://lpis.ec.europa.eu/registry/applicationschema/cap-iacs-base/code#SpecieCodeValue/solanumTuberosumLPotato">
        <rdf:type rdf:resource="http://lpis.ec.europa.eu/registry/applicationschema/cap-iacs-base#SpecieCodeValue"/>
        <rdfs:label xml:lang="en">Solanum tuberosum L. Potato</rdfs:label>
        <skos:definition xml:lang="en">-- Definition --
Solanum tuberosum L. Potato.
-- Description --
List of agricultural species -A   
V. Potatoes
NOTE. Initial value: A - 87.</skos:definition>
        <skos:inScheme rdf:resource="http://lpis.ec.europa.eu/registry/applicationschema/cap-iacs-base/code#SpecieCodeValue"/>
    </owl:NamedIndividual>
    


    <!-- http://lpis.ec.europa.eu/registry/applicationschema/cap-iacs-base/code#SpecieCodeValue/sorghumBicolorLMoenchSorghum -->


    <owl:NamedIndividual rdf:about="http://lpis.ec.europa.eu/registry/applicationschema/cap-iacs-base/code#SpecieCodeValue/sorghumBicolorLMoenchSorghum">
        <rdf:type rdf:resource="http://lpis.ec.europa.eu/registry/applicationschema/cap-iacs-base#SpecieCodeValue"/>
        <rdfs:label xml:lang="en">Sorghum bicolor (L.) Moench Sorghum </rdfs:label>
        <skos:definition xml:lang="en">-- Definition --
Sorghum bicolor (L.) Moench Sorghum.
-- Description --
List of agricultural species -A   
IV. Cereals
NOTE. Initial value: A - 79.</skos:definition>
        <skos:inScheme rdf:resource="http://lpis.ec.europa.eu/registry/applicationschema/cap-iacs-base/code#SpecieCodeValue"/>
    </owl:NamedIndividual>
    


    <!-- http://lpis.ec.europa.eu/registry/applicationschema/cap-iacs-base/code#SpecieCodeValue/sorghumSudanenseLSudanGrass -->


    <owl:NamedIndividual rdf:about="http://lpis.ec.europa.eu/registry/applicationschema/cap-iacs-base/code#SpecieCodeValue/sorghumSudanenseLSudanGrass">
        <rdf:type rdf:resource="http://lpis.ec.europa.eu/registry/applicationschema/cap-iacs-base#SpecieCodeValue"/>
        <rdfs:label xml:lang="en">Sorghum sudanense L. Sudan grass </rdfs:label>
        <skos:definition xml:lang="en">-- Definition --
Sorghum sudanense L. Sudan grass.
-- Description --
List of agricultural species -A   
IV. Cereals
NOTE. Initial value: A - 80.</skos:definition>
        <skos:inScheme rdf:resource="http://lpis.ec.europa.eu/registry/applicationschema/cap-iacs-base/code#SpecieCodeValue"/>
    </owl:NamedIndividual>
    


    <!-- http://lpis.ec.europa.eu/registry/applicationschema/cap-iacs-base/code#SpecieCodeValue/spinaciaOleraceaLSpinach -->


    <owl:NamedIndividual rdf:about="http://lpis.ec.europa.eu/registry/applicationschema/cap-iacs-base/code#SpecieCodeValue/spinaciaOleraceaLSpinach">
        <rdf:type rdf:resource="http://lpis.ec.europa.eu/registry/applicationschema/cap-iacs-base#SpecieCodeValue"/>
        <rdfs:label xml:lang="en">Spinacia oleracea L. Spinach</rdfs:label>
        <skos:definition xml:lang="en">-- Definition --
Spinacia oleracea L. Spinach.
-- Description --
List of vegetable specie -H
NOTE. Initial value: H - 33.</skos:definition>
        <skos:inScheme rdf:resource="http://lpis.ec.europa.eu/registry/applicationschema/cap-iacs-base/code#SpecieCodeValue"/>
    </owl:NamedIndividual>
    


    <!-- http://lpis.ec.europa.eu/registry/applicationschema/cap-iacs-base/code#SpecieCodeValue/sspAlternativum -->


    <owl:NamedIndividual rdf:about="http://lpis.ec.europa.eu/registry/applicationschema/cap-iacs-base/code#SpecieCodeValue/sspAlternativum">
        <rdf:type rdf:resource="http://lpis.ec.europa.eu/registry/applicationschema/cap-iacs-base#SpecieCodeValue"/>
        <rdfs:label xml:lang="en">Ssp. alternativum</rdfs:label>
        <skos:definition xml:lang="en">-- Definition --
Lolium multiflorum Lam. Italian ryegrass (including Westerwold ryegrass) Ssp. alternativum. 
-- Description --
List of agricultural species -A
II. Fodder plants
NOTE. Initial value: A - 20.1</skos:definition>
        <skos:inScheme rdf:resource="http://lpis.ec.europa.eu/registry/applicationschema/cap-iacs-base/code#SpecieCodeValue"/>
    </owl:NamedIndividual>
    


    <!-- http://lpis.ec.europa.eu/registry/applicationschema/cap-iacs-base/code#SpecieCodeValue/sspNonAlternativum -->


    <owl:NamedIndividual rdf:about="http://lpis.ec.europa.eu/registry/applicationschema/cap-iacs-base/code#SpecieCodeValue/sspNonAlternativum">
        <rdf:type rdf:resource="http://lpis.ec.europa.eu/registry/applicationschema/cap-iacs-base#SpecieCodeValue"/>
        <rdfs:label xml:lang="en">Ssp. non alternativum</rdfs:label>
        <skos:definition xml:lang="en">-- Definition --
Lolium multiflorum Lam. Italian ryegrass (including Westerwold ryegrass) Ssp. non alternativum.
-- Description --
NOTE. Initial value: A - 20.2</skos:definition>
        <skos:inScheme rdf:resource="http://lpis.ec.europa.eu/registry/applicationschema/cap-iacs-base/code#SpecieCodeValue"/>
    </owl:NamedIndividual>
    


    <!-- http://lpis.ec.europa.eu/registry/applicationschema/cap-iacs-base/code#SpecieCodeValue/trifoliumAlexandrinumLBerseemEgyptian -->


    <owl:NamedIndividual rdf:about="http://lpis.ec.europa.eu/registry/applicationschema/cap-iacs-base/code#SpecieCodeValue/trifoliumAlexandrinumLBerseemEgyptian">
        <rdf:type rdf:resource="http://lpis.ec.europa.eu/registry/applicationschema/cap-iacs-base#SpecieCodeValue"/>
        <rdfs:label xml:lang="en">Trifolium alexandrinum L. Berseem/Egyptian</rdfs:label>
        <skos:definition xml:lang="en">-- Definition --
Trifolium alexandrinum L. Berseem/Egyptian.
-- Description --
List of agricultural species -A
II. Fodder plants
NOTE. Initial value: A - 43.</skos:definition>
        <skos:inScheme rdf:resource="http://lpis.ec.europa.eu/registry/applicationschema/cap-iacs-base/code#SpecieCodeValue"/>
    </owl:NamedIndividual>
    


    <!-- http://lpis.ec.europa.eu/registry/applicationschema/cap-iacs-base/code#SpecieCodeValue/trifoliumIncarnatumLCrimsonClover -->


    <owl:NamedIndividual rdf:about="http://lpis.ec.europa.eu/registry/applicationschema/cap-iacs-base/code#SpecieCodeValue/trifoliumIncarnatumLCrimsonClover">
        <rdf:type rdf:resource="http://lpis.ec.europa.eu/registry/applicationschema/cap-iacs-base#SpecieCodeValue"/>
        <rdfs:label xml:lang="en">Trifolium incarnatum L. Crimson clover</rdfs:label>
        <skos:definition xml:lang="en">-- Definition --
Trifolium incarnatum L. Crimson clover.
-- Description --
List of agricultural species -A
II. Fodder plants
NOTE. Initial value: A - 45.</skos:definition>
        <skos:inScheme rdf:resource="http://lpis.ec.europa.eu/registry/applicationschema/cap-iacs-base/code#SpecieCodeValue"/>
    </owl:NamedIndividual>
    


    <!-- http://lpis.ec.europa.eu/registry/applicationschema/cap-iacs-base/code#SpecieCodeValue/trifoliumPratenseLRedClover -->


    <owl:NamedIndividual rdf:about="http://lpis.ec.europa.eu/registry/applicationschema/cap-iacs-base/code#SpecieCodeValue/trifoliumPratenseLRedClover">
        <rdf:type rdf:resource="http://lpis.ec.europa.eu/registry/applicationschema/cap-iacs-base#SpecieCodeValue"/>
        <rdfs:label xml:lang="en">Trifolium pratense L. Red clover</rdfs:label>
        <skos:definition xml:lang="en">-- Definition --
Trifolium pratense L. Red clover.
-- Description --
List of agricultural species -A
II. Fodder plants
NOTE. Initial value: A - 46.</skos:definition>
        <skos:inScheme rdf:resource="http://lpis.ec.europa.eu/registry/applicationschema/cap-iacs-base/code#SpecieCodeValue"/>
    </owl:NamedIndividual>
    


    <!-- http://lpis.ec.europa.eu/registry/applicationschema/cap-iacs-base/code#SpecieCodeValue/trifoliumRepensLWhiteClover -->


    <owl:NamedIndividual rdf:about="http://lpis.ec.europa.eu/registry/applicationschema/cap-iacs-base/code#SpecieCodeValue/trifoliumRepensLWhiteClover">
        <rdf:type rdf:resource="http://lpis.ec.europa.eu/registry/applicationschema/cap-iacs-base#SpecieCodeValue"/>
        <rdfs:label xml:lang="en">Trifolium repens L. White clover</rdfs:label>
        <skos:definition xml:lang="en">-- Definition --
Trifolium repens L. White clover.
-- Description --
List of agricultural species -A
II. Fodder plants
NOTE. Initial value: A - 47.</skos:definition>
        <skos:inScheme rdf:resource="http://lpis.ec.europa.eu/registry/applicationschema/cap-iacs-base/code#SpecieCodeValue"/>
    </owl:NamedIndividual>
    


    <!-- http://lpis.ec.europa.eu/registry/applicationschema/cap-iacs-base/code#SpecieCodeValue/trifoliumResupinatumLPersianClover -->


    <owl:NamedIndividual rdf:about="http://lpis.ec.europa.eu/registry/applicationschema/cap-iacs-base/code#SpecieCodeValue/trifoliumResupinatumLPersianClover">
        <rdf:type rdf:resource="http://lpis.ec.europa.eu/registry/applicationschema/cap-iacs-base#SpecieCodeValue"/>
        <rdfs:label xml:lang="en">Trifolium resupinatum L. Persian clover</rdfs:label>
        <skos:definition xml:lang="en">-- Definition --
Trifolium resupinatum L. Persian clover.
-- Description --
List of agricultural species -A
II. Fodder plants
NOTE. Initial value: A - 48.</skos:definition>
        <skos:inScheme rdf:resource="http://lpis.ec.europa.eu/registry/applicationschema/cap-iacs-base/code#SpecieCodeValue"/>
    </owl:NamedIndividual>
    


    <!-- http://lpis.ec.europa.eu/registry/applicationschema/cap-iacs-base/code#SpecieCodeValue/trifotiumHybridumLAlsikeClover -->


    <owl:NamedIndividual rdf:about="http://lpis.ec.europa.eu/registry/applicationschema/cap-iacs-base/code#SpecieCodeValue/trifotiumHybridumLAlsikeClover">
        <rdf:type rdf:resource="http://lpis.ec.europa.eu/registry/applicationschema/cap-iacs-base#SpecieCodeValue"/>
        <rdfs:label xml:lang="en">Trifolium hybridum L. Alsike clover</rdfs:label>
        <skos:definition xml:lang="en">-- Definition --
Trifolium hybridum L. Alsike clover.
-- Description --
List of agricultural species -A
II. Fodder plants
NOTE. Initial value: A - 44.</skos:definition>
        <skos:inScheme rdf:resource="http://lpis.ec.europa.eu/registry/applicationschema/cap-iacs-base/code#SpecieCodeValue"/>
    </owl:NamedIndividual>
    


    <!-- http://lpis.ec.europa.eu/registry/applicationschema/cap-iacs-base/code#SpecieCodeValue/trigonellaFoenumGraecumLFenugreek -->


    <owl:NamedIndividual rdf:about="http://lpis.ec.europa.eu/registry/applicationschema/cap-iacs-base/code#SpecieCodeValue/trigonellaFoenumGraecumLFenugreek">
        <rdf:type rdf:resource="http://lpis.ec.europa.eu/registry/applicationschema/cap-iacs-base#SpecieCodeValue"/>
        <rdfs:label xml:lang="en">Trigonella foenum-graecum L. Fenugreek   </rdfs:label>
        <skos:definition xml:lang="en">-- Definition --
Trigonella foenum-graecum L. Fenugreek.
-- Description --
List of agricultural species -A
II. Fodder plants
NOTE. Initial value: A - 49.</skos:definition>
        <skos:inScheme rdf:resource="http://lpis.ec.europa.eu/registry/applicationschema/cap-iacs-base/code#SpecieCodeValue"/>
    </owl:NamedIndividual>
    


    <!-- http://lpis.ec.europa.eu/registry/applicationschema/cap-iacs-base/code#SpecieCodeValue/trisetumFlavescensLGoldenOatgrass -->


    <owl:NamedIndividual rdf:about="http://lpis.ec.europa.eu/registry/applicationschema/cap-iacs-base/code#SpecieCodeValue/trisetumFlavescensLGoldenOatgrass">
        <rdf:type rdf:resource="http://lpis.ec.europa.eu/registry/applicationschema/cap-iacs-base#SpecieCodeValue"/>
        <rdfs:label xml:lang="en">Trisetum flavescens L. Golden oatgrass</rdfs:label>
        <skos:definition xml:lang="en">-- Definition --
Trisetum flavescens L. Golden oatgrass
-- Description --
List of agricultural species -A
II. Fodder plants
NOTE. Initial value: A - 31.</skos:definition>
        <skos:inScheme rdf:resource="http://lpis.ec.europa.eu/registry/applicationschema/cap-iacs-base/code#SpecieCodeValue"/>
    </owl:NamedIndividual>
    


    <!-- http://lpis.ec.europa.eu/registry/applicationschema/cap-iacs-base/code#SpecieCodeValue/triticumAestivumLWheat -->


    <owl:NamedIndividual rdf:about="http://lpis.ec.europa.eu/registry/applicationschema/cap-iacs-base/code#SpecieCodeValue/triticumAestivumLWheat">
        <rdf:type rdf:resource="http://lpis.ec.europa.eu/registry/applicationschema/cap-iacs-base#SpecieCodeValue"/>
        <rdfs:label xml:lang="en">Triticum aestivum L. Wheat</rdfs:label>
        <skos:definition xml:lang="en">-- Definition --
Triticum aestivum L. Wheat.
-- Description --
List of agricultural species -A   
IV. Cereals
NOTE. Initial value: A - 83.</skos:definition>
        <skos:inScheme rdf:resource="http://lpis.ec.europa.eu/registry/applicationschema/cap-iacs-base/code#SpecieCodeValue"/>
    </owl:NamedIndividual>
    


    <!-- http://lpis.ec.europa.eu/registry/applicationschema/cap-iacs-base/code#SpecieCodeValue/triticumDurumDesfDurumWheat -->


    <owl:NamedIndividual rdf:about="http://lpis.ec.europa.eu/registry/applicationschema/cap-iacs-base/code#SpecieCodeValue/triticumDurumDesfDurumWheat">
        <rdf:type rdf:resource="http://lpis.ec.europa.eu/registry/applicationschema/cap-iacs-base#SpecieCodeValue"/>
        <rdfs:label xml:lang="en">Triticum durum Desf. Durum wheat </rdfs:label>
        <skos:definition xml:lang="en">-- Definition --
Triticum durum Desf. Durum wheat.
-- Description --
List of agricultural species -A   
IV. Cereals
NOTE. Initial value: A - 84.</skos:definition>
        <skos:inScheme rdf:resource="http://lpis.ec.europa.eu/registry/applicationschema/cap-iacs-base/code#SpecieCodeValue"/>
    </owl:NamedIndividual>
    


    <!-- http://lpis.ec.europa.eu/registry/applicationschema/cap-iacs-base/code#SpecieCodeValue/triticumSpeltaLSpeltWheat -->


    <owl:NamedIndividual rdf:about="http://lpis.ec.europa.eu/registry/applicationschema/cap-iacs-base/code#SpecieCodeValue/triticumSpeltaLSpeltWheat">
        <rdf:type rdf:resource="http://lpis.ec.europa.eu/registry/applicationschema/cap-iacs-base#SpecieCodeValue"/>
        <rdfs:label xml:lang="en">Triticum spelta L. Spelt wheat  </rdfs:label>
        <skos:definition xml:lang="en">-- Definition --
Triticum spelta L. Spelt wheat.
-- Description --
List of agricultural species -A   
IV. Cereals
NOTE. Initial value: A - 85.</skos:definition>
        <skos:inScheme rdf:resource="http://lpis.ec.europa.eu/registry/applicationschema/cap-iacs-base/code#SpecieCodeValue"/>
    </owl:NamedIndividual>
    


    <!-- http://lpis.ec.europa.eu/registry/applicationschema/cap-iacs-base/code#SpecieCodeValue/valerianellaLocustaLLaterrCornSaladLambsLettuce -->


    <owl:NamedIndividual rdf:about="http://lpis.ec.europa.eu/registry/applicationschema/cap-iacs-base/code#SpecieCodeValue/valerianellaLocustaLLaterrCornSaladLambsLettuce">
        <rdf:type rdf:resource="http://lpis.ec.europa.eu/registry/applicationschema/cap-iacs-base#SpecieCodeValue"/>
        <rdfs:label xml:lang="en">Valerianella locusta (L.) Laterr. Corn salad / Lamb&apos;s lettuce</rdfs:label>
        <skos:definition xml:lang="en">-- Definition --
Valerianella locusta (L.) Laterr. Corn salad / Lamb&apos;s lettuce.
-- Description --
List of vegetable specie -H
NOTE. Initial value: H - 34.</skos:definition>
        <skos:inScheme rdf:resource="http://lpis.ec.europa.eu/registry/applicationschema/cap-iacs-base/code#SpecieCodeValue"/>
    </owl:NamedIndividual>
    


    <!-- http://lpis.ec.europa.eu/registry/applicationschema/cap-iacs-base/code#SpecieCodeValue/viciaFabaLPartimBroadBean -->


    <owl:NamedIndividual rdf:about="http://lpis.ec.europa.eu/registry/applicationschema/cap-iacs-base/code#SpecieCodeValue/viciaFabaLPartimBroadBean">
        <rdf:type rdf:resource="http://lpis.ec.europa.eu/registry/applicationschema/cap-iacs-base#SpecieCodeValue"/>
        <rdfs:label xml:lang="en">Vicia faba L. (partim) Broad bean</rdfs:label>
        <skos:definition xml:lang="en">-- Definition --
Vicia faba L. (partim) Broad bean.
-- Description --
List of vegetable specie -H
NOTE. Initial value: H - 35.</skos:definition>
        <skos:inScheme rdf:resource="http://lpis.ec.europa.eu/registry/applicationschema/cap-iacs-base/code#SpecieCodeValue"/>
    </owl:NamedIndividual>
    


    <!-- http://lpis.ec.europa.eu/registry/applicationschema/cap-iacs-base/code#SpecieCodeValue/viciaFabaLPartimFieldBean -->


    <owl:NamedIndividual rdf:about="http://lpis.ec.europa.eu/registry/applicationschema/cap-iacs-base/code#SpecieCodeValue/viciaFabaLPartimFieldBean">
        <rdf:type rdf:resource="http://lpis.ec.europa.eu/registry/applicationschema/cap-iacs-base#SpecieCodeValue"/>
        <rdfs:label xml:lang="en">Vicia faba L. (Partim) Field bean</rdfs:label>
        <skos:definition xml:lang="en">-- Definition --
Vicia faba L. (Partim) Field bean.
-- Description --
List of agricultural species -A
II. Fodder plants
NOTE. Initial value: A - 50.</skos:definition>
        <skos:inScheme rdf:resource="http://lpis.ec.europa.eu/registry/applicationschema/cap-iacs-base/code#SpecieCodeValue"/>
    </owl:NamedIndividual>
    


    <!-- http://lpis.ec.europa.eu/registry/applicationschema/cap-iacs-base/code#SpecieCodeValue/viciaPannonicaLHungarianVetch -->


    <owl:NamedIndividual rdf:about="http://lpis.ec.europa.eu/registry/applicationschema/cap-iacs-base/code#SpecieCodeValue/viciaPannonicaLHungarianVetch">
        <rdf:type rdf:resource="http://lpis.ec.europa.eu/registry/applicationschema/cap-iacs-base#SpecieCodeValue"/>
        <rdfs:label xml:lang="en">Vicia pannonica L. Hungarian vetch </rdfs:label>
        <skos:definition xml:lang="en">-- Definition --
Vicia pannonica L. Hungarian vetch.
-- Description --
List of agricultural species -A
II. Fodder plants
NOTE. Initial value: A - 51.</skos:definition>
        <skos:inScheme rdf:resource="http://lpis.ec.europa.eu/registry/applicationschema/cap-iacs-base/code#SpecieCodeValue"/>
    </owl:NamedIndividual>
    


    <!-- http://lpis.ec.europa.eu/registry/applicationschema/cap-iacs-base/code#SpecieCodeValue/viciaSativaLCommonVetch -->


    <owl:NamedIndividual rdf:about="http://lpis.ec.europa.eu/registry/applicationschema/cap-iacs-base/code#SpecieCodeValue/viciaSativaLCommonVetch">
        <rdf:type rdf:resource="http://lpis.ec.europa.eu/registry/applicationschema/cap-iacs-base#SpecieCodeValue"/>
        <rdfs:label xml:lang="en">Vicia sativa L. Common vetch </rdfs:label>
        <skos:definition xml:lang="en">-- Definition --
Vicia sativa L. Common vetch.
-- Description --
List of agricultural species -A
II. Fodder plants
NOTE. Initial value: A - 52.</skos:definition>
        <skos:inScheme rdf:resource="http://lpis.ec.europa.eu/registry/applicationschema/cap-iacs-base/code#SpecieCodeValue"/>
    </owl:NamedIndividual>
    


    <!-- http://lpis.ec.europa.eu/registry/applicationschema/cap-iacs-base/code#SpecieCodeValue/viciaVillosaRothHairyVetch -->


    <owl:NamedIndividual rdf:about="http://lpis.ec.europa.eu/registry/applicationschema/cap-iacs-base/code#SpecieCodeValue/viciaVillosaRothHairyVetch">
        <rdf:type rdf:resource="http://lpis.ec.europa.eu/registry/applicationschema/cap-iacs-base#SpecieCodeValue"/>
        <rdfs:label xml:lang="en">Vicia villosa Roth. Hairy vetch</rdfs:label>
        <skos:definition xml:lang="en">-- Definition --
Vicia villosa Roth. Hairy vetch.
-- Description --
List of agricultural species -A
II. Fodder plants
NOTE. Initial value: A - 53.</skos:definition>
        <skos:inScheme rdf:resource="http://lpis.ec.europa.eu/registry/applicationschema/cap-iacs-base/code#SpecieCodeValue"/>
    </owl:NamedIndividual>
    


    <!-- http://lpis.ec.europa.eu/registry/applicationschema/cap-iacs-base/code#SpecieCodeValue/zeaMaysLMaize -->


    <owl:NamedIndividual rdf:about="http://lpis.ec.europa.eu/registry/applicationschema/cap-iacs-base/code#SpecieCodeValue/zeaMaysLMaize">
        <rdf:type rdf:resource="http://lpis.ec.europa.eu/registry/applicationschema/cap-iacs-base#SpecieCodeValue"/>
        <rdfs:label xml:lang="en">Zea mays L. Maize  </rdfs:label>
        <skos:definition xml:lang="en">-- Definition --
Zea mays L. Maize.
-- Description --
List of agricultural species -A   
IV. Cereals
NOTE. Initial value: A - 86.</skos:definition>
        <skos:inScheme rdf:resource="http://lpis.ec.europa.eu/registry/applicationschema/cap-iacs-base/code#SpecieCodeValue"/>
    </owl:NamedIndividual>
    


    <!-- http://lpis.ec.europa.eu/registry/applicationschema/cap-iacs-base/code#SpecieCodeValue/zeaMaysLPopcorn -->


    <owl:NamedIndividual rdf:about="http://lpis.ec.europa.eu/registry/applicationschema/cap-iacs-base/code#SpecieCodeValue/zeaMaysLPopcorn">
        <rdf:type rdf:resource="http://lpis.ec.europa.eu/registry/applicationschema/cap-iacs-base#SpecieCodeValue"/>
        <rdfs:label xml:lang="en">Zea mays L. Popcorn</rdfs:label>
        <skos:definition xml:lang="en">-- Definition --
Zea mays L. Popcorn.
-- Description --
List of vegetable specie -H
NOTE. Initial value: H - 36.2</skos:definition>
        <skos:inScheme rdf:resource="http://lpis.ec.europa.eu/registry/applicationschema/cap-iacs-base/code#SpecieCodeValue"/>
    </owl:NamedIndividual>
    


    <!-- http://lpis.ec.europa.eu/registry/applicationschema/cap-iacs-base/code#SpecieCodeValue/zeaMaysLSweetCorn -->


    <owl:NamedIndividual rdf:about="http://lpis.ec.europa.eu/registry/applicationschema/cap-iacs-base/code#SpecieCodeValue/zeaMaysLSweetCorn">
        <rdf:type rdf:resource="http://lpis.ec.europa.eu/registry/applicationschema/cap-iacs-base#SpecieCodeValue"/>
        <rdfs:label xml:lang="en">Zea mays L. Sweet corn</rdfs:label>
        <skos:definition xml:lang="en">-- Definition --
Zea mays L. Sweet corn.
-- Description --
List of vegetable specie -H
NOTE. Initial value: H - 36.1</skos:definition>
        <skos:inScheme rdf:resource="http://lpis.ec.europa.eu/registry/applicationschema/cap-iacs-base/code#SpecieCodeValue"/>
    </owl:NamedIndividual>
    


    <!-- http://lpis.ec.europa.eu/registry/applicationschema/cap-iacs-base/code#SpecieCodeValue/lolium×BoucheanumKunthHybridRyegrass -->


    <owl:NamedIndividual rdf:about="http://lpis.ec.europa.eu/registry/applicationschema/cap-iacs-base/code#SpecieCodeValue/lolium×BoucheanumKunthHybridRyegrass">
        <rdf:type rdf:resource="http://lpis.ec.europa.eu/registry/applicationschema/cap-iacs-base#SpecieCodeValue"/>
        <rdfs:label xml:lang="en">Lolium × boucheanum Kunth Hybrid ryegrass </rdfs:label>
        <skos:definition xml:lang="en">-- Definition --
Lolium × boucheanum Kunth Hybrid ryegrass.
-- Description --
List of agricultural species -A
II. Fodder plants
NOTE. Initial value: A - 22.</skos:definition>
        <skos:inScheme rdf:resource="http://lpis.ec.europa.eu/registry/applicationschema/cap-iacs-base/code#SpecieCodeValue"/>
    </owl:NamedIndividual>
    


    <!-- http://lpis.ec.europa.eu/registry/applicationschema/cap-iacs-base/code#SpecieCodeValue/medicago×VariaLSandLucerne -->


    <owl:NamedIndividual rdf:about="http://lpis.ec.europa.eu/registry/applicationschema/cap-iacs-base/code#SpecieCodeValue/medicago×VariaLSandLucerne">
        <rdf:type rdf:resource="http://lpis.ec.europa.eu/registry/applicationschema/cap-iacs-base#SpecieCodeValue"/>
        <rdfs:label xml:lang="en">Medicago × varia L. Sand lucerne</rdfs:label>
        <skos:definition xml:lang="en">-- Definition --
Medicago × varia L. Sand lucerne.
-- Description --
List of agricultural species -A
II. Fodder plants
NOTE. Initial value:A - 40.</skos:definition>
        <skos:inScheme rdf:resource="http://lpis.ec.europa.eu/registry/applicationschema/cap-iacs-base/code#SpecieCodeValue"/>
    </owl:NamedIndividual>
    


    <!-- http://lpis.ec.europa.eu/registry/applicationschema/cap-iacs-base/code#SpecieCodeValue/sorghumBicolorLMoench×SorghumSudanensePiperStapfHybrids -->


    <owl:NamedIndividual rdf:about="http://lpis.ec.europa.eu/registry/applicationschema/cap-iacs-base/code#SpecieCodeValue/sorghumBicolorLMoench×SorghumSudanensePiperStapfHybrids">
        <rdf:type rdf:resource="http://lpis.ec.europa.eu/registry/applicationschema/cap-iacs-base#SpecieCodeValue"/>
        <rdfs:label xml:lang="en">Sorghum bicolor (L.) Moench × Sorghum sudanense (Piper) Stapf. Hybrids</rdfs:label>
        <skos:definition xml:lang="en">-- Definition --
Sorghum bicolor (L.) Moench × Sorghum sudanense (Piper) Stapf. Hybrids resulting from the crossing of Sorghum bicolor and Sorghum sudanense.
-- Description --
List of agricultural species -A   
IV. Cereals
NOTE. Initial value: A - 81.</skos:definition>
        <skos:inScheme rdf:resource="http://lpis.ec.europa.eu/registry/applicationschema/cap-iacs-base/code#SpecieCodeValue"/>
    </owl:NamedIndividual>
    


    <!-- http://lpis.ec.europa.eu/registry/applicationschema/cap-iacs-base/code#SpecieCodeValue/×FestuloliumAschEtGraebnHybrids -->


    <owl:NamedIndividual rdf:about="http://lpis.ec.europa.eu/registry/applicationschema/cap-iacs-base/code#SpecieCodeValue/×FestuloliumAschEtGraebnHybrids">
        <rdf:type rdf:resource="http://lpis.ec.europa.eu/registry/applicationschema/cap-iacs-base#SpecieCodeValue"/>
        <rdfs:label xml:lang="en">×Festulolium Asch. et Graebn. Hybrids</rdfs:label>
        <skos:definition xml:lang="en">-- Definition --
×Festulolium Asch. et Graebn. Hybrids resulting from the crossing of a species of the genus Festuca with a species of the genus Lolium.
-- Description --
List of agricultural species -A
II. Fodder plants
NOTE. Initial value: A - 19.</skos:definition>
        <skos:inScheme rdf:resource="http://lpis.ec.europa.eu/registry/applicationschema/cap-iacs-base/code#SpecieCodeValue"/>
    </owl:NamedIndividual>
    


    <!-- http://lpis.ec.europa.eu/registry/applicationschema/cap-iacs-base/code#SpecieCodeValue/×TriticosecaleWittmExACamusHybrids -->


    <owl:NamedIndividual rdf:about="http://lpis.ec.europa.eu/registry/applicationschema/cap-iacs-base/code#SpecieCodeValue/×TriticosecaleWittmExACamusHybrids">
        <rdf:type rdf:resource="http://lpis.ec.europa.eu/registry/applicationschema/cap-iacs-base#SpecieCodeValue"/>
        <rdfs:label xml:lang="en">×Triticosecale Wittm. ex A. Camus Hybrids</rdfs:label>
        <skos:definition xml:lang="en">-- Definition --
×Triticosecale Wittm. ex A. Camus Hybrids resulting from the crossing of a species of the genus Triticum and a species of the genus Secale.
-- Description --
List of agricultural species -A   
IV. Cereals
NOTE. Initial value: A - 82.</skos:definition>
        <skos:inScheme rdf:resource="http://lpis.ec.europa.eu/registry/applicationschema/cap-iacs-base/code#SpecieCodeValue"/>
    </owl:NamedIndividual>
    


    <!-- http://lpis.ec.europa.eu/registry/applicationschema/cap-iacs-base/code#StatusOfAnomalyValue/archived -->


    <owl:NamedIndividual rdf:about="http://lpis.ec.europa.eu/registry/applicationschema/cap-iacs-base/code#StatusOfAnomalyValue/archived">
        <rdf:type rdf:resource="http://lpis.ec.europa.eu/registry/applicationschema/cap-iacs-base#StatusOfAnomalyValue"/>
        <rdfs:label xml:lang="en">Closed</rdfs:label>
        <skos:definition xml:lang="en">--Name--
Archived

-- Definition --
Status of anomaly as soon as it has been resolved.

--Description--
Anomalies are archived for historic reference.</skos:definition>
        <skos:inScheme rdf:resource="http://lpis.ec.europa.eu/registry/applicationschema/cap-iacs-base/code#StatusOfAnomalyValue"/>
    </owl:NamedIndividual>
    


    <!-- http://lpis.ec.europa.eu/registry/applicationschema/cap-iacs-base/code#StatusOfAnomalyValue/inProgress -->


    <owl:NamedIndividual rdf:about="http://lpis.ec.europa.eu/registry/applicationschema/cap-iacs-base/code#StatusOfAnomalyValue/inProgress">
        <rdf:type rdf:resource="http://lpis.ec.europa.eu/registry/applicationschema/cap-iacs-base#StatusOfAnomalyValue"/>
        <rdfs:label xml:lang="en">In progress</rdfs:label>
        <skos:definition xml:lang="en">--Name--
In progress

-- Definition --
Status of the anomaly as soon as its processing has started or has been flagged for later resolution.</skos:definition>
        <skos:inScheme rdf:resource="http://lpis.ec.europa.eu/registry/applicationschema/cap-iacs-base/code#StatusOfAnomalyValue"/>
    </owl:NamedIndividual>
    


    <!-- http://lpis.ec.europa.eu/registry/applicationschema/cap-iacs-base/code#StatusOfAnomalyValue/open -->


    <owl:NamedIndividual rdf:about="http://lpis.ec.europa.eu/registry/applicationschema/cap-iacs-base/code#StatusOfAnomalyValue/open">
        <rdf:type rdf:resource="http://lpis.ec.europa.eu/registry/applicationschema/cap-iacs-base#StatusOfAnomalyValue"/>
        <rdfs:label xml:lang="en">Open</rdfs:label>
        <skos:definition xml:lang="en">--Name--
Open

-- Definition --
Status of anomaly after recording it in the information system.</skos:definition>
        <skos:inScheme rdf:resource="http://lpis.ec.europa.eu/registry/applicationschema/cap-iacs-base/code#StatusOfAnomalyValue"/>
    </owl:NamedIndividual>
    


    <!-- http://lpis.ec.europa.eu/registry/applicationschema/cap-iacs-base/code#StatusOfIssueValue/archived -->


    <owl:NamedIndividual rdf:about="http://lpis.ec.europa.eu/registry/applicationschema/cap-iacs-base/code#StatusOfIssueValue/archived">
        <rdf:type rdf:resource="http://lpis.ec.europa.eu/registry/applicationschema/cap-iacs-base#StatusOfIssueValue"/>
        <rdfs:label xml:lang="en">Closed</rdfs:label>
        <skos:definition xml:lang="en">--Name--
Archived

-- Definition --
Status of issue as soon as it has been resolved.

--Description--
Issues are archived for historic reference.</skos:definition>
        <skos:inScheme rdf:resource="http://lpis.ec.europa.eu/registry/applicationschema/cap-iacs-base/code#StatusOfIssueValue"/>
    </owl:NamedIndividual>
    


    <!-- http://lpis.ec.europa.eu/registry/applicationschema/cap-iacs-base/code#StatusOfIssueValue/inProgress -->


    <owl:NamedIndividual rdf:about="http://lpis.ec.europa.eu/registry/applicationschema/cap-iacs-base/code#StatusOfIssueValue/inProgress">
        <rdf:type rdf:resource="http://lpis.ec.europa.eu/registry/applicationschema/cap-iacs-base#StatusOfIssueValue"/>
        <rdfs:label xml:lang="en">In progress</rdfs:label>
        <skos:definition xml:lang="en">--Name--
In progress

-- Definition --
Status of the issue as soon as its processing has started or has been flagged for later resolution.</skos:definition>
        <skos:inScheme rdf:resource="http://lpis.ec.europa.eu/registry/applicationschema/cap-iacs-base/code#StatusOfIssueValue"/>
    </owl:NamedIndividual>
    


    <!-- http://lpis.ec.europa.eu/registry/applicationschema/cap-iacs-base/code#StatusOfIssueValue/open -->


    <owl:NamedIndividual rdf:about="http://lpis.ec.europa.eu/registry/applicationschema/cap-iacs-base/code#StatusOfIssueValue/open">
        <rdf:type rdf:resource="http://lpis.ec.europa.eu/registry/applicationschema/cap-iacs-base#StatusOfIssueValue"/>
        <rdfs:label xml:lang="en">Open</rdfs:label>
        <skos:definition xml:lang="en">--Name--
Open

-- Definition --
Status of issue after recording it in the information system.</skos:definition>
        <skos:inScheme rdf:resource="http://lpis.ec.europa.eu/registry/applicationschema/cap-iacs-base/code#StatusOfIssueValue"/>
    </owl:NamedIndividual>
    


    <!-- http://lpis.ec.europa.eu/registry/applicationschema/cap-iacs-base/code#StatusValue/approved -->


    <owl:NamedIndividual rdf:about="http://lpis.ec.europa.eu/registry/applicationschema/cap-iacs-base/code#StatusValue/approved">
        <rdf:type rdf:resource="http://lpis.ec.europa.eu/registry/applicationschema/cap-iacs-base#StatusValue"/>
        <rdfs:label xml:lang="en">Approved, valid, archival</rdfs:label>
        <skos:definition xml:lang="en">-- Definition --
Approved,

--Definition--
Status of an object according to the state machine diagram.

-- Description --
Status of the targeted schema / data object after final controls (consistency with IACS  and local rules).</skos:definition>
        <skos:inScheme rdf:resource="http://lpis.ec.europa.eu/registry/applicationschema/cap-iacs-base/code#StatusValue"/>
    </owl:NamedIndividual>
    


    <!-- http://lpis.ec.europa.eu/registry/applicationschema/cap-iacs-base/code#StatusValue/archived -->


    <owl:NamedIndividual rdf:about="http://lpis.ec.europa.eu/registry/applicationschema/cap-iacs-base/code#StatusValue/archived">
        <rdf:type rdf:resource="http://lpis.ec.europa.eu/registry/applicationschema/cap-iacs-base#StatusValue"/>
        <skos:definition xml:lang="en">--Name--
Archived

--Definition--
Status of an object according to the state machine diagram.

-- Description--
Final state of an object after its depreciation (retirement).
Such object is no more in use; its life cycle has been completed.

NOTE 1. FeatureLevelMetadata.endLifespanVersion&lt;&gt;Null

NOTE 2. NOTE 2: If applied, FeatureLevelMetadata.validTo&lt;&gt;Null</skos:definition>
        <skos:inScheme rdf:resource="http://lpis.ec.europa.eu/registry/applicationschema/cap-iacs-base/code#StatusValue"/>
    </owl:NamedIndividual>
    


    <!-- http://lpis.ec.europa.eu/registry/applicationschema/cap-iacs-base/code#StatusValue/inProgress -->


    <owl:NamedIndividual rdf:about="http://lpis.ec.europa.eu/registry/applicationschema/cap-iacs-base/code#StatusValue/inProgress">
        <rdf:type rdf:resource="http://lpis.ec.europa.eu/registry/applicationschema/cap-iacs-base#StatusValue"/>
        <rdfs:label xml:lang="en">Under construction</rdfs:label>
        <skos:definition xml:lang="en">-- Name--
In progress

--Definition--
Status of an object according to the state machine diagram.

-- Description --
The value shall be assigned when processing of the issue/anomaly has been started. The value is applicable to
- the issue/anomaly that reported the change request
- the object (schema element or data) that is subject of the change request.

EXAMPLE 1. Schema element objects are:
- the entire application schema,
- feature and data types
- attributes, association roles,
- constraints
- value types (etc).

EXAMPLE 2. Data objects are specific instances of a feature or data types (e.g. RP, farmer, anomaly, payment. The change may be applied to 
- the instance as a whole (depreciation of an obsolete instance or introduction of a new instance),
- a specific value (attribute) of an instance.

NOTE: Rules for depreciation are defined by internal business rules of the MS/Region</skos:definition>
        <skos:inScheme rdf:resource="http://lpis.ec.europa.eu/registry/applicationschema/cap-iacs-base/code#StatusValue"/>
    </owl:NamedIndividual>
    


    <!-- http://lpis.ec.europa.eu/registry/applicationschema/cap-iacs-base/code#StatusValue/open -->


    <owl:NamedIndividual rdf:about="http://lpis.ec.europa.eu/registry/applicationschema/cap-iacs-base/code#StatusValue/open">
        <rdf:type rdf:resource="http://lpis.ec.europa.eu/registry/applicationschema/cap-iacs-base#StatusValue"/>
        <rdfs:label xml:lang="en">Registered</rdfs:label>
        <skos:definition xml:lang="en">--Name--
Open

--Definition--
Status of an object according to the state machine diagram.

--Description --
This status is applicable to UpgradeIssue and Anomaly feature types only. The value is assigned in the moment when an instance of these feature types is introduced in the information system.</skos:definition>
        <skos:inScheme rdf:resource="http://lpis.ec.europa.eu/registry/applicationschema/cap-iacs-base/code#StatusValue"/>
    </owl:NamedIndividual>
    


    <!-- http://lpis.ec.europa.eu/registry/applicationschema/cap-iacs-base/code#StatusValue/rejected -->


    <owl:NamedIndividual rdf:about="http://lpis.ec.europa.eu/registry/applicationschema/cap-iacs-base/code#StatusValue/rejected">
        <rdf:type rdf:resource="http://lpis.ec.europa.eu/registry/applicationschema/cap-iacs-base#StatusValue"/>
        <rdfs:label xml:lang="en">Rejected, not valid, archival</rdfs:label>
        <skos:definition xml:lang="en">-- Name--
Rejected

--Definition--
Status of an object according to the state machine diagram.

-- Description --
Status of the change request after the negative outcome of the preliminary evaluation or the cross-check. It also means that no modification to the existing information can be executed.

NOTE: For transparency, the rejected change requests shall be archived.</skos:definition>
        <skos:inScheme rdf:resource="http://lpis.ec.europa.eu/registry/applicationschema/cap-iacs-base/code#StatusValue"/>
    </owl:NamedIndividual>
    


    <!-- http://lpis.ec.europa.eu/registry/applicationschema/cap-iacs-base/code#StatusValue/underApproval -->


    <owl:NamedIndividual rdf:about="http://lpis.ec.europa.eu/registry/applicationschema/cap-iacs-base/code#StatusValue/underApproval">
        <rdf:type rdf:resource="http://lpis.ec.europa.eu/registry/applicationschema/cap-iacs-base#StatusValue"/>
        <rdfs:label xml:lang="en">Under aprooval</rdfs:label>
        <skos:definition xml:lang="en">-- Name--
Under approval

--Definition--
Status of an object according to the state machine diagram.

-- Description --
Based on the outcome of cross checks the change request is approved. The object is waiting for finalisation.</skos:definition>
        <skos:inScheme rdf:resource="http://lpis.ec.europa.eu/registry/applicationschema/cap-iacs-base/code#StatusValue"/>
    </owl:NamedIndividual>
    


    <!-- http://lpis.ec.europa.eu/registry/applicationschema/cap-iacs-base/code#StatusValue/underCrossCheck -->


    <owl:NamedIndividual rdf:about="http://lpis.ec.europa.eu/registry/applicationschema/cap-iacs-base/code#StatusValue/underCrossCheck">
        <rdf:type rdf:resource="http://lpis.ec.europa.eu/registry/applicationschema/cap-iacs-base#StatusValue"/>
        <rdfs:label xml:lang="en">Under construction</rdfs:label>
        <skos:definition xml:lang="en">-- Name--
Under cross-check

--Definition--
Status of an object according to the state machine diagram.

-- Description --
Whenever a transaction in the information system is performed, the system shall be checked for integrity of the schema and the consistency of data. 

NOTE 1. Cross checks are also the tools to find further issues/anomalies. When a new upgrade issue/anomaly is found, the &quot;open&quot; value shall be assigned and the full life cycle assessment of the object has to be performed.</skos:definition>
        <skos:inScheme rdf:resource="http://lpis.ec.europa.eu/registry/applicationschema/cap-iacs-base/code#StatusValue"/>
    </owl:NamedIndividual>
    


    <!-- http://lpis.ec.europa.eu/registry/applicationschema/cap-iacs-base/code#StatusValue/underEvaluation -->


    <owl:NamedIndividual rdf:about="http://lpis.ec.europa.eu/registry/applicationschema/cap-iacs-base/code#StatusValue/underEvaluation">
        <rdf:type rdf:resource="http://lpis.ec.europa.eu/registry/applicationschema/cap-iacs-base#StatusValue"/>
        <rdfs:label xml:lang="en">Under evaluation</rdfs:label>
        <skos:definition xml:lang="en">-- Name--
Under evaluation

--Definition--
Status of an object according to the state machine diagram.

-- Description --
Preliminary assessment about the impact of the Upgrade issue or the anomaly. This value should be assigned in the phase when
- supporting evidences are collected  and/or
- checks for issue/anomaly duplicates are performed.  
The assessment may conclude that no modification to the existing data is needed, or that the reported change request has to be further processed.</skos:definition>
        <skos:inScheme rdf:resource="http://lpis.ec.europa.eu/registry/applicationschema/cap-iacs-base/code#StatusValue"/>
    </owl:NamedIndividual>
    


    <!-- http://lpis.ec.europa.eu/registry/applicationschema/cap-iacs-base/code#StatusValue/valid -->


    <owl:NamedIndividual rdf:about="http://lpis.ec.europa.eu/registry/applicationschema/cap-iacs-base/code#StatusValue/valid">
        <rdf:type rdf:resource="http://lpis.ec.europa.eu/registry/applicationschema/cap-iacs-base#StatusValue"/>
        <skos:definition xml:lang="en">-- Name--
Valid

--Definition--
Status of an object according to the state machine diagram.

-- Description --
The most current state of the object that shall be used by the users. 

NOTE 1: It is a current object whose life-cycle has not ended.
FeatureLevelMetadata.endLifespanVersion=Null

NOTE 2: If applied, FeatureLevelMetadata.validTo=Null</skos:definition>
        <skos:inScheme rdf:resource="http://lpis.ec.europa.eu/registry/applicationschema/cap-iacs-base/code#StatusValue"/>
    </owl:NamedIndividual>
    


    <!-- http://lpis.ec.europa.eu/registry/applicationschema/cap-iacs-base/code#SupportSchemeTypeValue/aegeanIslands -->


    <owl:NamedIndividual rdf:about="http://lpis.ec.europa.eu/registry/applicationschema/cap-iacs-base/code#SupportSchemeTypeValue/aegeanIslands">
        <rdf:type rdf:resource="http://lpis.ec.europa.eu/registry/applicationschema/cap-iacs-base#SupportSchemeTypeValue"/>
        <rdfs:label xml:lang="en">Aegean islands</rdfs:label>
        <skos:definition xml:lang="en">Aegean islands

Chapter IV of Regulation (EU) No 229/2013 / Direct payments under measures established in the programmes: Specific measures in favour of the smaller Aegean islands.</skos:definition>
        <skos:inScheme rdf:resource="http://lpis.ec.europa.eu/registry/applicationschema/cap-iacs-base/code#SupportSchemeTypeValue"/>
    </owl:NamedIndividual>
    


    <!-- http://lpis.ec.europa.eu/registry/applicationschema/cap-iacs-base/code#SupportSchemeTypeValue/basicPaymentScheme -->


    <owl:NamedIndividual rdf:about="http://lpis.ec.europa.eu/registry/applicationschema/cap-iacs-base/code#SupportSchemeTypeValue/basicPaymentScheme">
        <rdf:type rdf:resource="http://lpis.ec.europa.eu/registry/applicationschema/cap-iacs-base#SupportSchemeTypeValue"/>
        <rdfs:label xml:lang="en">Basic payment scheme</rdfs:label>
        <skos:definition xml:lang="en">Basic payment scheme

Basic payment scheme - BPS as described in Title III, Chapter 1, Sections 1, 2, 3 and 5 of Regulation (EU) 1307/2013.

Decoupled payment that is based on entitlements.</skos:definition>
        <skos:inScheme rdf:resource="http://lpis.ec.europa.eu/registry/applicationschema/cap-iacs-base/code#SupportSchemeTypeValue"/>
    </owl:NamedIndividual>
    


    <!-- http://lpis.ec.europa.eu/registry/applicationschema/cap-iacs-base/code#SupportSchemeTypeValue/cropSpecificPaymentForCotton -->


    <owl:NamedIndividual rdf:about="http://lpis.ec.europa.eu/registry/applicationschema/cap-iacs-base/code#SupportSchemeTypeValue/cropSpecificPaymentForCotton">
        <rdf:type rdf:resource="http://lpis.ec.europa.eu/registry/applicationschema/cap-iacs-base#SupportSchemeTypeValue"/>
        <rdfs:label xml:lang="en">Crop-specific payment for cotton</rdfs:label>
        <skos:definition xml:lang="en">Crop-specific payment for cotton

Aid shall be granted to farmers producing cotton falling within CN code 5201 00 under the conditions laid down in this Chapter.

Title IV, Chapter 2 of 1307/2013 Regulation / Area payment.</skos:definition>
        <skos:inScheme rdf:resource="http://lpis.ec.europa.eu/registry/applicationschema/cap-iacs-base/code#SupportSchemeTypeValue"/>
    </owl:NamedIndividual>
    


    <!-- http://lpis.ec.europa.eu/registry/applicationschema/cap-iacs-base/code#SupportSchemeTypeValue/paymentForAgriculturalPracticesBeneficialForTheClimateAndTheEnvironment -->


    <owl:NamedIndividual rdf:about="http://lpis.ec.europa.eu/registry/applicationschema/cap-iacs-base/code#SupportSchemeTypeValue/paymentForAgriculturalPracticesBeneficialForTheClimateAndTheEnvironment">
        <rdf:type rdf:resource="http://lpis.ec.europa.eu/registry/applicationschema/cap-iacs-base#SupportSchemeTypeValue"/>
        <rdfs:label xml:lang="en">Payment for agricultural practices beneficial for the climate and the environment</rdfs:label>
        <skos:definition xml:lang="en">Payment for agricultural practices beneficial for the climate and the environment 

Farmers entitled to a payment under the basic payment scheme or the single area payment scheme shall observe, on all their eligible hectares within the meaning of Article 32(2) to (5), the agricultural practices beneficial for the climate and the environment referred to in paragraph 2 of this Article or the equivalent practices referred to in paragraph 3 of this Article.

According to Title III, Chapter 3 of 1307/2013 Regulation  it is a decoupled payment. Also known as the Green Payment.</skos:definition>
        <skos:inScheme rdf:resource="http://lpis.ec.europa.eu/registry/applicationschema/cap-iacs-base/code#SupportSchemeTypeValue"/>
    </owl:NamedIndividual>
    


    <!-- http://lpis.ec.europa.eu/registry/applicationschema/cap-iacs-base/code#SupportSchemeTypeValue/paymentForAreasWithNaturalConstraints -->


    <owl:NamedIndividual rdf:about="http://lpis.ec.europa.eu/registry/applicationschema/cap-iacs-base/code#SupportSchemeTypeValue/paymentForAreasWithNaturalConstraints">
        <rdf:type rdf:resource="http://lpis.ec.europa.eu/registry/applicationschema/cap-iacs-base#SupportSchemeTypeValue"/>
        <rdfs:label xml:lang="en">Payment for areas with natural constraints</rdfs:label>
        <skos:definition xml:lang="en">Payment for areas with natural constraints

Payment to farmers who are entitled to BPS/SAPS and whose holdings are fully or partly situated in areas with natural constraints designated by Member States in accordance with Article 32(1) of Regulation (EU) No 1305/2013. 

NOTE
Rules in Title III, Chapter 4 of R 1307/2013</skos:definition>
        <skos:inScheme rdf:resource="http://lpis.ec.europa.eu/registry/applicationschema/cap-iacs-base/code#SupportSchemeTypeValue"/>
    </owl:NamedIndividual>
    


    <!-- http://lpis.ec.europa.eu/registry/applicationschema/cap-iacs-base/code#SupportSchemeTypeValue/paymentForYoungFarmers -->


    <owl:NamedIndividual rdf:about="http://lpis.ec.europa.eu/registry/applicationschema/cap-iacs-base/code#SupportSchemeTypeValue/paymentForYoungFarmers">
        <rdf:type rdf:resource="http://lpis.ec.europa.eu/registry/applicationschema/cap-iacs-base#SupportSchemeTypeValue"/>
        <rdfs:label xml:lang="en">Payment for young farmers</rdfs:label>
        <skos:definition xml:lang="en">Payment for young farmers

Member States shall grant an annual payment to young farmers who are entitled to a payment under the basic payment scheme or the single area payment scheme referred to in Chapter 1.

According to Title III, Chapter 5 of 1307/2013 Regulation it is a decoupled payment.</skos:definition>
        <skos:inScheme rdf:resource="http://lpis.ec.europa.eu/registry/applicationschema/cap-iacs-base/code#SupportSchemeTypeValue"/>
    </owl:NamedIndividual>
    


    <!-- http://lpis.ec.europa.eu/registry/applicationschema/cap-iacs-base/code#SupportSchemeTypeValue/posei -->


    <owl:NamedIndividual rdf:about="http://lpis.ec.europa.eu/registry/applicationschema/cap-iacs-base/code#SupportSchemeTypeValue/posei">
        <rdf:type rdf:resource="http://lpis.ec.europa.eu/registry/applicationschema/cap-iacs-base#SupportSchemeTypeValue"/>
        <rdfs:label xml:lang="en">Posei</rdfs:label>
        <skos:definition xml:lang="en">POSEI

Chapter IV of Regulation (EU) No 228/2013 / Direct payments under measures established in the programmes.

NOTE
In full: &quot;Programme d&apos;Options Spécifiques à l&apos;Éloignement et l&apos;Insularité&quot;.</skos:definition>
        <skos:inScheme rdf:resource="http://lpis.ec.europa.eu/registry/applicationschema/cap-iacs-base/code#SupportSchemeTypeValue"/>
    </owl:NamedIndividual>
    


    <!-- http://lpis.ec.europa.eu/registry/applicationschema/cap-iacs-base/code#SupportSchemeTypeValue/redistributivePayment -->


    <owl:NamedIndividual rdf:about="http://lpis.ec.europa.eu/registry/applicationschema/cap-iacs-base/code#SupportSchemeTypeValue/redistributivePayment">
        <rdf:type rdf:resource="http://lpis.ec.europa.eu/registry/applicationschema/cap-iacs-base#SupportSchemeTypeValue"/>
        <rdfs:label xml:lang="en">Redistributive payment </rdfs:label>
        <skos:definition xml:lang="en">Redistributive payment

Conditional payment scheme decided by MS to grant an annual payment to farmers who are entitled to a payment under the basic payment scheme or under the single area payment scheme.

Art. 4 of Title III, Chapter 2 of R 1307/2013 sets the calculation method:
It shall be calculated 
	- each year by Member States
	- by multiplying a figure to be set by the Member State, which shall not be higher than 65 % of the national or regional average payment per hectare, by the number of payment entitlements or by the number of eligible hectares. 
The number of such payment entitlements or hectares shall not exceed a maximum to be set by Member States which shall not be higher than 30 hectares or the average size of agricultural holdings set out in Annex VIII if that average size exceeds 30 hectares in the Member State concerned.

NOTE
MS may establish a graduation in the number of hectares that is equally applied to every farmer.
-- Description --
Regulation / Decoupled payment.</skos:definition>
        <skos:inScheme rdf:resource="http://lpis.ec.europa.eu/registry/applicationschema/cap-iacs-base/code#SupportSchemeTypeValue"/>
    </owl:NamedIndividual>
    


    <!-- http://lpis.ec.europa.eu/registry/applicationschema/cap-iacs-base/code#SupportSchemeTypeValue/singleAreaPaymentScheme -->


    <owl:NamedIndividual rdf:about="http://lpis.ec.europa.eu/registry/applicationschema/cap-iacs-base/code#SupportSchemeTypeValue/singleAreaPaymentScheme">
        <rdf:type rdf:resource="http://lpis.ec.europa.eu/registry/applicationschema/cap-iacs-base#SupportSchemeTypeValue"/>
        <rdfs:label xml:lang="en">Single area payment scheme</rdfs:label>
        <skos:definition xml:lang="en">Single area payment scheme 

Payment scheme based on the single area payment granted on an annual basis for each eligible hectare declared by the farmer in accordance with point (a) of the first subparagraph of Article 72(1) of Regulation (EU) No 1306/2013.

As described in Article 36 of 1307/2013 Regulation  it is a decoupled payment based on utilised land.</skos:definition>
        <skos:inScheme rdf:resource="http://lpis.ec.europa.eu/registry/applicationschema/cap-iacs-base/code#SupportSchemeTypeValue"/>
    </owl:NamedIndividual>
    


    <!-- http://lpis.ec.europa.eu/registry/applicationschema/cap-iacs-base/code#SupportSchemeTypeValue/smallFarmersScheme -->


    <owl:NamedIndividual rdf:about="http://lpis.ec.europa.eu/registry/applicationschema/cap-iacs-base/code#SupportSchemeTypeValue/smallFarmersScheme">
        <rdf:type rdf:resource="http://lpis.ec.europa.eu/registry/applicationschema/cap-iacs-base#SupportSchemeTypeValue"/>
        <rdfs:label xml:lang="en">Small farmers scheme</rdfs:label>
        <skos:definition xml:lang="en">Small farmers scheme

Member States may establish a scheme for small farmers in accordance with the conditions laid down in this Title.

According to Title V of 1307/2013 Regulation it is a decoupled payment.</skos:definition>
        <skos:inScheme rdf:resource="http://lpis.ec.europa.eu/registry/applicationschema/cap-iacs-base/code#SupportSchemeTypeValue"/>
    </owl:NamedIndividual>
    


    <!-- http://lpis.ec.europa.eu/registry/applicationschema/cap-iacs-base/code#SupportSchemeTypeValue/voluntaryCoupledSupport -->


    <owl:NamedIndividual rdf:about="http://lpis.ec.europa.eu/registry/applicationschema/cap-iacs-base/code#SupportSchemeTypeValue/voluntaryCoupledSupport">
        <rdf:type rdf:resource="http://lpis.ec.europa.eu/registry/applicationschema/cap-iacs-base#SupportSchemeTypeValue"/>
        <rdfs:label xml:lang="en">Voluntary coupled support</rdfs:label>
        <skos:definition xml:lang="en">Voluntary coupled support

Member States may grant coupled support to farmers  for
	- cereals, 
	- oilseeds, 
	- protein crops, 
	- grain legumes, 
	- flax, 
	- hemp, 
	- rice, 
	- nuts, 
	- starch potato, 
	- milk and milk products, 
	- seeds, 
	- sheepmeat and goatmeat, 
	- beef and veal, 
	- olive oil, 
	- silkworms, 
	- dried fodder, 
	- hops, 
	- sugar beet, 
	- cane and chicory, 
	- fruit and vegetables and 
	- short rotation coppice.

NOTE
Details in Title IV, Chapter 1 of R 1307/2013.</skos:definition>
        <skos:inScheme rdf:resource="http://lpis.ec.europa.eu/registry/applicationschema/cap-iacs-base/code#SupportSchemeTypeValue"/>
    </owl:NamedIndividual>
    


    <!-- http://lpis.ec.europa.eu/registry/applicationschema/cap-iacs-base/code#TestTypeValue/basic -->


    <owl:NamedIndividual rdf:about="http://lpis.ec.europa.eu/registry/applicationschema/cap-iacs-base/code#TestTypeValue/basic">
        <rdf:type rdf:resource="http://lpis.ec.europa.eu/registry/applicationschema/cap-iacs-base#TestTypeValue"/>
        <rdfs:label xml:lang="en">Basic test</rdfs:label>
        <skos:definition xml:lang="en">--Name--
Basic

-- Definition --
Basic test .

-- Description --
Basic tests (BT) provide limited testing of IUT in order to establish whether or not it is appropriate to perform more thorough testing. They may be used to determine the degree of conformance prior to deciding whether or not to proceed with thorough capability testing. Basic tests are simple capability tests. Conformance clauses should identify those test cases that may be used as a basic test.

NOTE1. BT shall be used to for detecting obvious cases of non-conformity.

NOTE2. BT shall be used as a preliminary step in order to decide whether or not to run capability tests.</skos:definition>
        <skos:inScheme rdf:resource="http://lpis.ec.europa.eu/registry/applicationschema/cap-iacs-base/code#TestTypeValue"/>
    </owl:NamedIndividual>
    


    <!-- http://lpis.ec.europa.eu/registry/applicationschema/cap-iacs-base/code#TestTypeValue/capability -->


    <owl:NamedIndividual rdf:about="http://lpis.ec.europa.eu/registry/applicationschema/cap-iacs-base/code#TestTypeValue/capability">
        <rdf:type rdf:resource="http://lpis.ec.europa.eu/registry/applicationschema/cap-iacs-base#TestTypeValue"/>
        <rdfs:label xml:lang="en">Capability test</rdfs:label>
        <skos:definition xml:lang="en">--Name--
Capability

-- Definition --
Capability test.

-- Description --
Capability tests (CT), should investigate an implementation as thoroughly as it is practical over the full range of conformance requirements specified in a standard/legal act. Capability tests should be provided to check the mandatory capabilities and those optional capabilities that are identified in the ICS as being supported by the IUT.

NOTE 1. CT shall be used to check that the capabilities of the IUT are consistent with the conformance requirements, that is, to determine whether or not an implementation conforms.

NOTE 2. CT shall be used to investigate causes of failure.</skos:definition>
        <skos:inScheme rdf:resource="http://lpis.ec.europa.eu/registry/applicationschema/cap-iacs-base/code#TestTypeValue"/>
    </owl:NamedIndividual>
    


    <!-- http://lpis.ec.europa.eu/registry/applicationschema/cap-iacs-base/code#TestVerdictValue/fail -->


    <owl:NamedIndividual rdf:about="http://lpis.ec.europa.eu/registry/applicationschema/cap-iacs-base/code#TestVerdictValue/fail">
        <rdf:type rdf:resource="http://lpis.ec.europa.eu/registry/applicationschema/cap-iacs-base#TestVerdictValue"/>
        <rdfs:label xml:lang="en">Fail verdict</rdfs:label>
        <skos:definition xml:lang="en">--Name--
Fail

-- Definition --
Fail verdict to indicate that SUT does not fulfil the requirements.

-- Description --
Test verdict of non-conformance . Failure to fulfil one or more requirements specified.</skos:definition>
        <skos:inScheme rdf:resource="http://lpis.ec.europa.eu/registry/applicationschema/cap-iacs-base/code#TestVerdictValue"/>
    </owl:NamedIndividual>
    


    <!-- http://lpis.ec.europa.eu/registry/applicationschema/cap-iacs-base/code#TestVerdictValue/inconclusive -->


    <owl:NamedIndividual rdf:about="http://lpis.ec.europa.eu/registry/applicationschema/cap-iacs-base/code#TestVerdictValue/inconclusive">
        <rdf:type rdf:resource="http://lpis.ec.europa.eu/registry/applicationschema/cap-iacs-base#TestVerdictValue"/>
        <rdfs:label xml:lang="en">Inconclusive verdict</rdfs:label>
        <skos:definition xml:lang="en">--Name--
Inconclusive

-- Definition --
A value “inconclusive” indicates that the testing process has not yet yield a verdict.


-- Description --
Neither fail nor pass verdict can be assigned based on the test.</skos:definition>
        <skos:inScheme rdf:resource="http://lpis.ec.europa.eu/registry/applicationschema/cap-iacs-base/code#TestVerdictValue"/>
    </owl:NamedIndividual>
    


    <!-- http://lpis.ec.europa.eu/registry/applicationschema/cap-iacs-base/code#TestVerdictValue/pass -->


    <owl:NamedIndividual rdf:about="http://lpis.ec.europa.eu/registry/applicationschema/cap-iacs-base/code#TestVerdictValue/pass">
        <rdf:type rdf:resource="http://lpis.ec.europa.eu/registry/applicationschema/cap-iacs-base#TestVerdictValue"/>
        <rdfs:label xml:lang="en">Pas verdict</rdfs:label>
        <skos:definition xml:lang="en">--Name--
Pass

-- Definition --
Pass verdict to indicate that the tested requirements are fulfilled.

-- Description --
Test verdict of conformance.</skos:definition>
        <skos:inScheme rdf:resource="http://lpis.ec.europa.eu/registry/applicationschema/cap-iacs-base/code#TestVerdictValue"/>
    </owl:NamedIndividual>
    


    <!-- http://lpis.ec.europa.eu/registry/applicationschema/cap-iacs-base/code#TestingTypeValue/automated -->


    <owl:NamedIndividual rdf:about="http://lpis.ec.europa.eu/registry/applicationschema/cap-iacs-base/code#TestingTypeValue/automated">
        <rdf:type rdf:resource="http://lpis.ec.europa.eu/registry/applicationschema/cap-iacs-base#TestingTypeValue"/>
        <rdfs:label xml:lang="en">Automated testing</rdfs:label>
        <skos:definition xml:lang="en">--Name--
Automated

-- Definition --
Automated test.

-- Description --
Automated testing may implement the required tests as a software system using either verification testing or falsification testing.</skos:definition>
        <skos:inScheme rdf:resource="http://lpis.ec.europa.eu/registry/applicationschema/cap-iacs-base/code#TestingTypeValue"/>
    </owl:NamedIndividual>
    


    <!-- http://lpis.ec.europa.eu/registry/applicationschema/cap-iacs-base/code#TestingTypeValue/manual -->


    <owl:NamedIndividual rdf:about="http://lpis.ec.europa.eu/registry/applicationschema/cap-iacs-base/code#TestingTypeValue/manual">
        <rdf:type rdf:resource="http://lpis.ec.europa.eu/registry/applicationschema/cap-iacs-base#TestingTypeValue"/>
        <rdfs:label xml:lang="en">Manual testing</rdfs:label>
        <skos:definition xml:lang="en">--Name--
Manual

-- Definition --
Manual testing.

-- Description --
Manual testing may be required when automated testing is too complex and/or human judgement is required. Manual testing should be used only for those standards where automatic testing is not viable.</skos:definition>
        <skos:inScheme rdf:resource="http://lpis.ec.europa.eu/registry/applicationschema/cap-iacs-base/code#TestingTypeValue"/>
    </owl:NamedIndividual>
    


    <!-- http://lpis.ec.europa.eu/registry/applicationschema/cap-iacs-base/code#VarietalNameValue/abelia -->


    <owl:NamedIndividual rdf:about="http://lpis.ec.europa.eu/registry/applicationschema/cap-iacs-base/code#VarietalNameValue/abelia">
        <rdf:type rdf:resource="http://lpis.ec.europa.eu/registry/applicationschema/cap-iacs-base#VarietalNameValue"/>
        <rdfs:label xml:lang="en">H - 1.2  Abelia</rdfs:label>
        <skos:definition xml:lang="en">-- Definition --
H - 1.2  Abelia
-- Description --
H - 1.2 Allium cepa L. Cepa group - Onion, Echalion /  Abelia.
NOTE. Initial value: Abelia
NOTE. MS - NL (Netherlands).</skos:definition>
        <skos:inScheme rdf:resource="http://lpis.ec.europa.eu/registry/applicationschema/cap-iacs-base/code#VarietalNameValue"/>
    </owl:NamedIndividual>
    


    <!-- http://lpis.ec.europa.eu/registry/applicationschema/cap-iacs-base/code#VarietalNameValue/accent -->


    <owl:NamedIndividual rdf:about="http://lpis.ec.europa.eu/registry/applicationschema/cap-iacs-base/code#VarietalNameValue/accent">
        <rdf:type rdf:resource="http://lpis.ec.europa.eu/registry/applicationschema/cap-iacs-base#VarietalNameValue"/>
        <rdfs:label xml:lang="en">H - 1.2  Accent</rdfs:label>
        <skos:definition xml:lang="en">-- Definition --
H - 1.2  Accent
-- Description --
H - 1.2 Allium cepa L. Cepa group - Onion, Echalion /  Accent.
NOTE. Initial value: Accent
NOTE. MS - NL (Netherlands).</skos:definition>
        <skos:inScheme rdf:resource="http://lpis.ec.europa.eu/registry/applicationschema/cap-iacs-base/code#VarietalNameValue"/>
    </owl:NamedIndividual>
    


    <!-- http://lpis.ec.europa.eu/registry/applicationschema/cap-iacs-base/code#VarietalNameValue/adonis -->


    <owl:NamedIndividual rdf:about="http://lpis.ec.europa.eu/registry/applicationschema/cap-iacs-base/code#VarietalNameValue/adonis">
        <rdf:type rdf:resource="http://lpis.ec.europa.eu/registry/applicationschema/cap-iacs-base#VarietalNameValue"/>
        <rdfs:label xml:lang="en">H - 1.2  Adonis</rdfs:label>
        <skos:definition xml:lang="en">-- Definition --
H - 1.2  Adonis
-- Description --
H - 1.2 Allium cepa L. Cepa group - Onion, Echalion /  Adonis.
NOTE. Initial value: Adonis
NOTE. MS - NL (Netherlands).</skos:definition>
        <skos:inScheme rdf:resource="http://lpis.ec.europa.eu/registry/applicationschema/cap-iacs-base/code#VarietalNameValue"/>
    </owl:NamedIndividual>
    


    <!-- http://lpis.ec.europa.eu/registry/applicationschema/cap-iacs-base/code#VarietalNameValue/ambition -->


    <owl:NamedIndividual rdf:about="http://lpis.ec.europa.eu/registry/applicationschema/cap-iacs-base/code#VarietalNameValue/ambition">
        <rdf:type rdf:resource="http://lpis.ec.europa.eu/registry/applicationschema/cap-iacs-base#VarietalNameValue"/>
        <rdfs:label xml:lang="en">H - 1.1  Ambition</rdfs:label>
        <skos:definition xml:lang="en">-- Definition --
H - 1.1  Ambition
-- Description --
H - 1.1 Allium cepa L. Aggregatum group - Shallot /  Ambition.
NOTE. Initial value: Ambition
NOTE. MS - NL (Netherlands).</skos:definition>
        <skos:inScheme rdf:resource="http://lpis.ec.europa.eu/registry/applicationschema/cap-iacs-base/code#VarietalNameValue"/>
    </owl:NamedIndividual>
    


    <!-- http://lpis.ec.europa.eu/registry/applicationschema/cap-iacs-base/code#VarietalNameValue/armador -->


    <owl:NamedIndividual rdf:about="http://lpis.ec.europa.eu/registry/applicationschema/cap-iacs-base/code#VarietalNameValue/armador">
        <rdf:type rdf:resource="http://lpis.ec.europa.eu/registry/applicationschema/cap-iacs-base#VarietalNameValue"/>
        <rdfs:label xml:lang="en">H - 1.1  Armador</rdfs:label>
        <skos:definition xml:lang="en">-- Definition --
H - 1.1  Armador
-- Description --
H - 1.1 Allium cepa L. Aggregatum group - Shallot /  Armador.
NOTE. Initial value: Armador
NOTE. MS - NL (Netherlands).</skos:definition>
        <skos:inScheme rdf:resource="http://lpis.ec.europa.eu/registry/applicationschema/cap-iacs-base/code#VarietalNameValue"/>
    </owl:NamedIndividual>
    


    <!-- http://lpis.ec.europa.eu/registry/applicationschema/cap-iacs-base/code#VarietalNameValue/biztro -->


    <owl:NamedIndividual rdf:about="http://lpis.ec.europa.eu/registry/applicationschema/cap-iacs-base/code#VarietalNameValue/biztro">
        <rdf:type rdf:resource="http://lpis.ec.europa.eu/registry/applicationschema/cap-iacs-base#VarietalNameValue"/>
        <rdfs:label xml:lang="en">H - 1.1  Biztro</rdfs:label>
        <skos:definition xml:lang="en">-- Definition --
H - 1.1  Biztro
-- Description --
H - 1.1 Allium cepa L. Aggregatum group - Shallot /  Biztro.
NOTE. Initial value: Biztro
NOTE. MS - NL (Netherlands).</skos:definition>
        <skos:inScheme rdf:resource="http://lpis.ec.europa.eu/registry/applicationschema/cap-iacs-base/code#VarietalNameValue"/>
    </owl:NamedIndividual>
    


    <!-- http://lpis.ec.europa.eu/registry/applicationschema/cap-iacs-base/code#WeekdayValue/friday -->


    <owl:NamedIndividual rdf:about="http://lpis.ec.europa.eu/registry/applicationschema/cap-iacs-base/code#WeekdayValue/friday">
        <rdf:type rdf:resource="http://lpis.ec.europa.eu/registry/applicationschema/cap-iacs-base#WeekdayValue"/>
        <rdfs:label xml:lang="en">Friday</rdfs:label>
        <skos:definition xml:lang="en">-- Definition --
Friday.
-- Description --
Item description.</skos:definition>
        <skos:inScheme rdf:resource="http://lpis.ec.europa.eu/registry/applicationschema/cap-iacs-base/code#WeekdayValue"/>
    </owl:NamedIndividual>
    


    <!-- http://lpis.ec.europa.eu/registry/applicationschema/cap-iacs-base/code#WeekdayValue/monday -->


    <owl:NamedIndividual rdf:about="http://lpis.ec.europa.eu/registry/applicationschema/cap-iacs-base/code#WeekdayValue/monday">
        <rdf:type rdf:resource="http://lpis.ec.europa.eu/registry/applicationschema/cap-iacs-base#WeekdayValue"/>
        <rdfs:label xml:lang="en">Monday</rdfs:label>
        <skos:definition xml:lang="en">-- Definition --
Monday.
-- Description --
Item description.</skos:definition>
        <skos:inScheme rdf:resource="http://lpis.ec.europa.eu/registry/applicationschema/cap-iacs-base/code#WeekdayValue"/>
    </owl:NamedIndividual>
    


    <!-- http://lpis.ec.europa.eu/registry/applicationschema/cap-iacs-base/code#WeekdayValue/saturday -->


    <owl:NamedIndividual rdf:about="http://lpis.ec.europa.eu/registry/applicationschema/cap-iacs-base/code#WeekdayValue/saturday">
        <rdf:type rdf:resource="http://lpis.ec.europa.eu/registry/applicationschema/cap-iacs-base#WeekdayValue"/>
        <rdfs:label xml:lang="en">Saturday</rdfs:label>
        <skos:definition xml:lang="en">-- Definition --
Saturday.
-- Description --
Item description.</skos:definition>
        <skos:inScheme rdf:resource="http://lpis.ec.europa.eu/registry/applicationschema/cap-iacs-base/code#WeekdayValue"/>
    </owl:NamedIndividual>
    


    <!-- http://lpis.ec.europa.eu/registry/applicationschema/cap-iacs-base/code#WeekdayValue/sunday -->


    <owl:NamedIndividual rdf:about="http://lpis.ec.europa.eu/registry/applicationschema/cap-iacs-base/code#WeekdayValue/sunday">
        <rdf:type rdf:resource="http://lpis.ec.europa.eu/registry/applicationschema/cap-iacs-base#WeekdayValue"/>
        <rdfs:label xml:lang="en">Sunday</rdfs:label>
        <skos:definition xml:lang="en">-- Definition --
Sunday.
-- Description --
Item description.</skos:definition>
        <skos:inScheme rdf:resource="http://lpis.ec.europa.eu/registry/applicationschema/cap-iacs-base/code#WeekdayValue"/>
    </owl:NamedIndividual>
    


    <!-- http://lpis.ec.europa.eu/registry/applicationschema/cap-iacs-base/code#WeekdayValue/thursday -->


    <owl:NamedIndividual rdf:about="http://lpis.ec.europa.eu/registry/applicationschema/cap-iacs-base/code#WeekdayValue/thursday">
        <rdf:type rdf:resource="http://lpis.ec.europa.eu/registry/applicationschema/cap-iacs-base#WeekdayValue"/>
        <rdfs:label xml:lang="en">Thursday</rdfs:label>
        <skos:definition xml:lang="en">-- Definition --
Thursday.
-- Description --
Item description.</skos:definition>
        <skos:inScheme rdf:resource="http://lpis.ec.europa.eu/registry/applicationschema/cap-iacs-base/code#WeekdayValue"/>
    </owl:NamedIndividual>
    


    <!-- http://lpis.ec.europa.eu/registry/applicationschema/cap-iacs-base/code#WeekdayValue/tuesday -->


    <owl:NamedIndividual rdf:about="http://lpis.ec.europa.eu/registry/applicationschema/cap-iacs-base/code#WeekdayValue/tuesday">
        <rdf:type rdf:resource="http://lpis.ec.europa.eu/registry/applicationschema/cap-iacs-base#WeekdayValue"/>
        <rdfs:label xml:lang="en">Tuesday</rdfs:label>
        <skos:definition xml:lang="en">-- Definition --
Tuesday.
-- Description --
Item description.</skos:definition>
        <skos:inScheme rdf:resource="http://lpis.ec.europa.eu/registry/applicationschema/cap-iacs-base/code#WeekdayValue"/>
    </owl:NamedIndividual>
    


    <!-- http://lpis.ec.europa.eu/registry/applicationschema/cap-iacs-base/code#WeekdayValue/wednesday -->


    <owl:NamedIndividual rdf:about="http://lpis.ec.europa.eu/registry/applicationschema/cap-iacs-base/code#WeekdayValue/wednesday">
        <rdf:type rdf:resource="http://lpis.ec.europa.eu/registry/applicationschema/cap-iacs-base#WeekdayValue"/>
        <rdfs:label xml:lang="en">Wednesday</rdfs:label>
        <skos:definition xml:lang="en">-- Definition --
Wednesday.
-- Description --
Item description.</skos:definition>
        <skos:inScheme rdf:resource="http://lpis.ec.europa.eu/registry/applicationschema/cap-iacs-base/code#WeekdayValue"/>
    </owl:NamedIndividual>
</rdf:RDF>



<!-- Generated by the OWL API (version 5.1.18) https://github.com/owlcs/owlapi/ -->


