@prefix : <http://lpis.ec.europa.eu/registry/applicationschema/cap-iacs-base/code#> .
@prefix owl: <http://www.w3.org/2002/07/owl#> .
@prefix rdf: <http://www.w3.org/1999/02/22-rdf-syntax-ns#> .
@prefix xml: <http://www.w3.org/XML/1998/namespace> .
@prefix xsd: <http://www.w3.org/2001/XMLSchema#> .
@prefix rdfs: <http://www.w3.org/2000/01/rdf-schema#> .
@base <http://lpis.ec.europa.eu/registry/applicationschema/cap-iacs-base/code#> .

<http://lpis.ec.europa.eu/registry/applicationschema/cap-iacs-base/code> rdf:type owl:Ontology ;
                                                                          owl:versionIRI <http://lpis.ec.europa.eu/registry/applicationschema/cap-iacs-base/code/3.0> ;
                                                                          <http://purl.org/dc/terms/creator> _:genid1 ;
                                                                          <http://purl.org/dc/terms/description> "Ontology of the base types code lists used in IACS, generated from the transformation of the corresponding JRC application schema"@en ;
                                                                          <http://purl.org/dc/terms/rights> "This ontology is distributed under Creative Commons Attribution 4.0 License - http://creativecommons.org/licenses/by/4.0"@en ;
                                                                          <http://purl.org/dc/terms/source> "JRC IACS application schema. https://doi.org/10.1016/j.landusepol.2016.05.023"@en ;
                                                                          <http://purl.org/dc/terms/title> "JRC IACS - Base Types Code Lists"@en ;
                                                                          rdfs:label "Base types code lists"@en ;
                                                                          owl:versionInfo "3.0" .

_:genid1 <http://schema.org/affiliation> [ <http://xmlns.com/foaf/0.1/name> "PSNC"
                                          ] ;
          rdfs:seeAlso <http://orcid.org/0000-0003-4289-4922> ;
          <http://xmlns.com/foaf/0.1/name> "Raul Palma" .

#################################################################
#    Annotation properties
#################################################################

###  http://purl.org/dc/terms/creator
<http://purl.org/dc/terms/creator> rdf:type owl:AnnotationProperty .


###  http://purl.org/dc/terms/description
<http://purl.org/dc/terms/description> rdf:type owl:AnnotationProperty .


###  http://purl.org/dc/terms/isFormatOf
<http://purl.org/dc/terms/isFormatOf> rdf:type owl:AnnotationProperty .


###  http://purl.org/dc/terms/rights
<http://purl.org/dc/terms/rights> rdf:type owl:AnnotationProperty .


###  http://purl.org/dc/terms/source
<http://purl.org/dc/terms/source> rdf:type owl:AnnotationProperty .


###  http://purl.org/dc/terms/title
<http://purl.org/dc/terms/title> rdf:type owl:AnnotationProperty .


###  http://schema.org/affiliation
<http://schema.org/affiliation> rdf:type owl:AnnotationProperty .


###  http://www.w3.org/2004/02/skos/core#definition
<http://www.w3.org/2004/02/skos/core#definition> rdf:type owl:AnnotationProperty .


###  http://www.w3.org/2004/02/skos/core#inScheme
<http://www.w3.org/2004/02/skos/core#inScheme> rdf:type owl:AnnotationProperty .


###  http://xmlns.com/foaf/0.1/name
<http://xmlns.com/foaf/0.1/name> rdf:type owl:AnnotationProperty .


#################################################################
#    Classes
#################################################################

###  http://lpis.ec.europa.eu/registry/applicationschema/cap-iacs-base#AffectedElementTypeValue
<http://lpis.ec.europa.eu/registry/applicationschema/cap-iacs-base#AffectedElementTypeValue> rdf:type owl:Class .


###  http://lpis.ec.europa.eu/registry/applicationschema/cap-iacs-base#CauseOfAnomalyValue
<http://lpis.ec.europa.eu/registry/applicationschema/cap-iacs-base#CauseOfAnomalyValue> rdf:type owl:Class .


###  http://lpis.ec.europa.eu/registry/applicationschema/cap-iacs-base#ConformanceClassValue
<http://lpis.ec.europa.eu/registry/applicationschema/cap-iacs-base#ConformanceClassValue> rdf:type owl:Class .


###  http://lpis.ec.europa.eu/registry/applicationschema/cap-iacs-base#ConformanceLevelValue
<http://lpis.ec.europa.eu/registry/applicationschema/cap-iacs-base#ConformanceLevelValue> rdf:type owl:Class .


###  http://lpis.ec.europa.eu/registry/applicationschema/cap-iacs-base#ConformanceRequirementClassValue
<http://lpis.ec.europa.eu/registry/applicationschema/cap-iacs-base#ConformanceRequirementClassValue> rdf:type owl:Class .


###  http://lpis.ec.europa.eu/registry/applicationschema/cap-iacs-base#ConformanceRequirementStatementValue
<http://lpis.ec.europa.eu/registry/applicationschema/cap-iacs-base#ConformanceRequirementStatementValue> rdf:type owl:Class .


###  http://lpis.ec.europa.eu/registry/applicationschema/cap-iacs-base#ConformanceStatementValue
<http://lpis.ec.europa.eu/registry/applicationschema/cap-iacs-base#ConformanceStatementValue> rdf:type owl:Class .


###  http://lpis.ec.europa.eu/registry/applicationschema/cap-iacs-base#CropItemCodeValue
<http://lpis.ec.europa.eu/registry/applicationschema/cap-iacs-base#CropItemCodeValue> rdf:type owl:Class .


###  http://lpis.ec.europa.eu/registry/applicationschema/cap-iacs-base#CrossComplianceRuleValue
<http://lpis.ec.europa.eu/registry/applicationschema/cap-iacs-base#CrossComplianceRuleValue> rdf:type owl:Class .


###  http://lpis.ec.europa.eu/registry/applicationschema/cap-iacs-base#FarmStructureSurveyNumberValue
<http://lpis.ec.europa.eu/registry/applicationschema/cap-iacs-base#FarmStructureSurveyNumberValue> rdf:type owl:Class .


###  http://lpis.ec.europa.eu/registry/applicationschema/cap-iacs-base#MonthValue
<http://lpis.ec.europa.eu/registry/applicationschema/cap-iacs-base#MonthValue> rdf:type owl:Class .


###  http://lpis.ec.europa.eu/registry/applicationschema/cap-iacs-base#NotificationGroupValue
<http://lpis.ec.europa.eu/registry/applicationschema/cap-iacs-base#NotificationGroupValue> rdf:type owl:Class .


###  http://lpis.ec.europa.eu/registry/applicationschema/cap-iacs-base#OrdinalNumberValue
<http://lpis.ec.europa.eu/registry/applicationschema/cap-iacs-base#OrdinalNumberValue> rdf:type owl:Class .


###  http://lpis.ec.europa.eu/registry/applicationschema/cap-iacs-base#RecurenceValue
<http://lpis.ec.europa.eu/registry/applicationschema/cap-iacs-base#RecurenceValue> rdf:type owl:Class .


###  http://lpis.ec.europa.eu/registry/applicationschema/cap-iacs-base#SpecieCodeValue
<http://lpis.ec.europa.eu/registry/applicationschema/cap-iacs-base#SpecieCodeValue> rdf:type owl:Class .


###  http://lpis.ec.europa.eu/registry/applicationschema/cap-iacs-base#StatusOfAnomalyValue
<http://lpis.ec.europa.eu/registry/applicationschema/cap-iacs-base#StatusOfAnomalyValue> rdf:type owl:Class .


###  http://lpis.ec.europa.eu/registry/applicationschema/cap-iacs-base#StatusOfIssueValue
<http://lpis.ec.europa.eu/registry/applicationschema/cap-iacs-base#StatusOfIssueValue> rdf:type owl:Class .


###  http://lpis.ec.europa.eu/registry/applicationschema/cap-iacs-base#StatusValue
<http://lpis.ec.europa.eu/registry/applicationschema/cap-iacs-base#StatusValue> rdf:type owl:Class .


###  http://lpis.ec.europa.eu/registry/applicationschema/cap-iacs-base#SupportSchemeTypeValue
<http://lpis.ec.europa.eu/registry/applicationschema/cap-iacs-base#SupportSchemeTypeValue> rdf:type owl:Class .


###  http://lpis.ec.europa.eu/registry/applicationschema/cap-iacs-base#TestTypeValue
<http://lpis.ec.europa.eu/registry/applicationschema/cap-iacs-base#TestTypeValue> rdf:type owl:Class .


###  http://lpis.ec.europa.eu/registry/applicationschema/cap-iacs-base#TestVerdictValue
<http://lpis.ec.europa.eu/registry/applicationschema/cap-iacs-base#TestVerdictValue> rdf:type owl:Class .


###  http://lpis.ec.europa.eu/registry/applicationschema/cap-iacs-base#TestingTypeValue
<http://lpis.ec.europa.eu/registry/applicationschema/cap-iacs-base#TestingTypeValue> rdf:type owl:Class .


###  http://lpis.ec.europa.eu/registry/applicationschema/cap-iacs-base#VarietalNameValue
<http://lpis.ec.europa.eu/registry/applicationschema/cap-iacs-base#VarietalNameValue> rdf:type owl:Class .


###  http://lpis.ec.europa.eu/registry/applicationschema/cap-iacs-base#WeekdayValue
<http://lpis.ec.europa.eu/registry/applicationschema/cap-iacs-base#WeekdayValue> rdf:type owl:Class .


###  http://www.w3.org/2004/02/skos/core#ConceptScheme
<http://www.w3.org/2004/02/skos/core#ConceptScheme> rdf:type owl:Class .


#################################################################
#    Individuals
#################################################################

###  http://lpis.ec.europa.eu/registry/applicationschema/cap-iacs-base/code#AffectedElementTypeValue
:AffectedElementTypeValue rdf:type owl:NamedIndividual ,
                                   <http://www.w3.org/2004/02/skos/core#ConceptScheme> ;
                          <http://purl.org/dc/terms/isFormatOf> <http://lpis.ec.europa.eu/registry/applicationschema/cap-iacs-base#AffectedElementTypeValue> ;
                          rdfs:label "Affected element type value list"@en ;
                          <http://www.w3.org/2004/02/skos/core#definition> """--Name--
Affected element type value.

-- Definition --
Application schema or its element that might be a subject of an issue.

-- Description --
List of possible affected elements that might be changed within the model."""@en .


###  http://lpis.ec.europa.eu/registry/applicationschema/cap-iacs-base/code#CauseOfAnomalyValue
:CauseOfAnomalyValue rdf:type owl:NamedIndividual ,
                              <http://www.w3.org/2004/02/skos/core#ConceptScheme> ;
                     <http://purl.org/dc/terms/isFormatOf> <http://lpis.ec.europa.eu/registry/applicationschema/cap-iacs-base#CauseOfAnomalyValue> ;
                     rdfs:label "Anomaly cause value list"@en ;
                     <http://www.w3.org/2004/02/skos/core#definition> """--Name--
Cause of anomaly value

-- Definition --
Code list defining the values of the case of anomaly attribute.

-- Description --
List of possible anomaly causes used for documentation of an anomaly."""@en .


###  http://lpis.ec.europa.eu/registry/applicationschema/cap-iacs-base/code#ConformanceClassValue
:ConformanceClassValue rdf:type owl:NamedIndividual ,
                                <http://www.w3.org/2004/02/skos/core#ConceptScheme> ;
                       <http://purl.org/dc/terms/isFormatOf> <http://lpis.ec.europa.eu/registry/applicationschema/cap-iacs-base#ConformanceClassValue> ;
                       rdfs:label "List of conformance class values"@en ;
                       <http://www.w3.org/2004/02/skos/core#definition> """--Name--
Conformance class value

--Definition--
List of conformance class values.

--Description--
Any product claiming conformance with one of these classes shall pass all requirements described in the corresponding abstract test suite.

NOTE. Requirements of conformance classes may overlap in which case subparts of the abstract test suite may be shared between different conformance classes."""@en .


###  http://lpis.ec.europa.eu/registry/applicationschema/cap-iacs-base/code#ConformanceLevelValue
:ConformanceLevelValue rdf:type owl:NamedIndividual ,
                                <http://www.w3.org/2004/02/skos/core#ConceptScheme> ;
                       <http://purl.org/dc/terms/isFormatOf> <http://lpis.ec.europa.eu/registry/applicationschema/cap-iacs-base#ConformanceLevelValue> ;
                       rdfs:label "List of conformance level values"@en ;
                       <http://www.w3.org/2004/02/skos/core#definition> """--Name--
Conformance level value

-- Definition --
List of conformance level values.

-- Description --
List of conformance level values. Any product claiming conformance with one of these levels shall pass all requirements described in the corresponding abstract test suite.

NOTE. Requirements of a higher level contain all requirements of a lower level."""@en .


###  http://lpis.ec.europa.eu/registry/applicationschema/cap-iacs-base/code#ConformanceRequirementClassValue
:ConformanceRequirementClassValue rdf:type owl:NamedIndividual ,
                                           <http://www.w3.org/2004/02/skos/core#ConceptScheme> ;
                                  <http://purl.org/dc/terms/isFormatOf> <http://lpis.ec.europa.eu/registry/applicationschema/cap-iacs-base#ConformanceRequirementClassValue> ;
                                  rdfs:label "List of conformance requirement class values"@en ;
                                  <http://www.w3.org/2004/02/skos/core#definition> """--Name--
Conformance requirement class value

--Definition--
List of conformance requirement class values."""@en .


###  http://lpis.ec.europa.eu/registry/applicationschema/cap-iacs-base/code#ConformanceRequirementStatementValue
:ConformanceRequirementStatementValue rdf:type owl:NamedIndividual ,
                                               <http://www.w3.org/2004/02/skos/core#ConceptScheme> ;
                                      <http://purl.org/dc/terms/isFormatOf> <http://lpis.ec.europa.eu/registry/applicationschema/cap-iacs-base#ConformanceRequirementStatementValue> ;
                                      rdfs:label "List of conformance requirement statement values"@en ;
                                      <http://www.w3.org/2004/02/skos/core#definition> """--Name--
Conformance requirement statement value

--Definition--
List of conformance requirement statement values."""@en .


###  http://lpis.ec.europa.eu/registry/applicationschema/cap-iacs-base/code#ConformanceStatementValue
:ConformanceStatementValue rdf:type owl:NamedIndividual ,
                                    <http://www.w3.org/2004/02/skos/core#ConceptScheme> ;
                           <http://purl.org/dc/terms/isFormatOf> <http://lpis.ec.europa.eu/registry/applicationschema/cap-iacs-base#ConformanceStatementValue> ;
                           rdfs:label "List of conformance statement values"@en ;
                           <http://www.w3.org/2004/02/skos/core#definition> """--Name--
Conformance Statement Value

-- Definition --
Enumeration of conformance statement values.

-- Description --
List of possible conformance verdicts whether the subject of testing (e.g. SUT, schema element, source data, etc.) conforms to the specified rules."""@en .


###  http://lpis.ec.europa.eu/registry/applicationschema/cap-iacs-base/code#CropItemCodeValue
:CropItemCodeValue rdf:type owl:NamedIndividual ,
                            <http://www.w3.org/2004/02/skos/core#ConceptScheme> ;
                   <http://purl.org/dc/terms/isFormatOf> <http://lpis.ec.europa.eu/registry/applicationschema/cap-iacs-base#CropItemCodeValue> ;
                   rdfs:label "List of crop items"@en ;
                   <http://www.w3.org/2004/02/skos/core#definition> """-- Definition --
List of crop items (aggregate of a species)
Eurostat Handbook for Annual Crop Statistics (Regulation 543/2009) (Revision 2013 – Presented in the WPM of the 12).
-- Description --
Land use of Agriculture Area in Use -L
Cereals and main crops - C"""@en .


###  http://lpis.ec.europa.eu/registry/applicationschema/cap-iacs-base/code#CrossComplianceRuleValue
:CrossComplianceRuleValue rdf:type owl:NamedIndividual ,
                                   <http://www.w3.org/2004/02/skos/core#ConceptScheme> ;
                          <http://purl.org/dc/terms/isFormatOf> <http://lpis.ec.europa.eu/registry/applicationschema/cap-iacs-base#CrossComplianceRuleValue> ;
                          rdfs:label "List of rules for cross-compliance"@en ;
                          <http://www.w3.org/2004/02/skos/core#definition> """-- Definition --
List of rules for cross-compliance
-- Description --
List of rules for cross-compliance. Rules for SMR and GAEC."""@en .


###  http://lpis.ec.europa.eu/registry/applicationschema/cap-iacs-base/code#FarmStructureSurveyNumberValue
:FarmStructureSurveyNumberValue rdf:type owl:NamedIndividual ,
                                         <http://www.w3.org/2004/02/skos/core#ConceptScheme> ;
                                <http://purl.org/dc/terms/isFormatOf> <http://lpis.ec.europa.eu/registry/applicationschema/cap-iacs-base#FarmStructureSurveyNumberValue> ;
                                rdfs:label "List of farm structure survey numbers"@en ;
                                <http://www.w3.org/2004/02/skos/core#definition> """-- Definition --
List of farm structure survey numbers (aggregate of crop items).
-- Desription --
Scope - LAND part only. Commision regulations (EC) No 1200/2009 of 30 November 2009 Implementing Regulation (EC) No 1166/2008 of the European Parliament and of the Council on farm structure surveys and the survey on agricultural production methods, as regards livestock unit coefficients and definitions of the characteristics (Text with EEA relevance)."""@en .


###  http://lpis.ec.europa.eu/registry/applicationschema/cap-iacs-base/code#MonthValue
:MonthValue rdf:type owl:NamedIndividual ,
                     <http://www.w3.org/2004/02/skos/core#ConceptScheme> ;
            <http://purl.org/dc/terms/isFormatOf> <http://lpis.ec.europa.eu/registry/applicationschema/cap-iacs-base#MonthValue> ;
            rdfs:label "List of month values"@en ;
            <http://www.w3.org/2004/02/skos/core#definition> """-- Definition --
List of months.
-- Description --
List of months."""@en .


###  http://lpis.ec.europa.eu/registry/applicationschema/cap-iacs-base/code#NotificationGroupValue
:NotificationGroupValue rdf:type owl:NamedIndividual ,
                                 <http://www.w3.org/2004/02/skos/core#ConceptScheme> ;
                        <http://purl.org/dc/terms/isFormatOf> <http://lpis.ec.europa.eu/registry/applicationschema/cap-iacs-base#NotificationGroupValue> ;
                        rdfs:label "List of notification groups."@en ;
                        <http://www.w3.org/2004/02/skos/core#definition> """-- Definition --
List of notification groups.
-- Description --
List of notification groups prescribed in legal documents.
NOTE. Not finite number of notification groups. List may be extended by MS."""@en .


###  http://lpis.ec.europa.eu/registry/applicationschema/cap-iacs-base/code#OrdinalNumberValue
:OrdinalNumberValue rdf:type owl:NamedIndividual ,
                             <http://www.w3.org/2004/02/skos/core#ConceptScheme> ;
                    <http://purl.org/dc/terms/isFormatOf> <http://lpis.ec.europa.eu/registry/applicationschema/cap-iacs-base#OrdinalNumberValue> ;
                    rdfs:label "Ordinal number value list"@en ;
                    <http://www.w3.org/2004/02/skos/core#definition> """-- Definition --
Ordinal number value list.

-- Description --
List of possible ordinal number values used for date identification."""@en .


###  http://lpis.ec.europa.eu/registry/applicationschema/cap-iacs-base/code#RecurenceValue
:RecurenceValue rdf:type owl:NamedIndividual ,
                         <http://www.w3.org/2004/02/skos/core#ConceptScheme> ;
                <http://purl.org/dc/terms/isFormatOf> <http://lpis.ec.europa.eu/registry/applicationschema/cap-iacs-base#RecurenceValue> ;
                rdfs:label "List of recurence values"@en ;
                <http://www.w3.org/2004/02/skos/core#definition> """-- Definition --
Notification recurrence value list.
-- Description --
List of possible notification recurrence values."""@en .


###  http://lpis.ec.europa.eu/registry/applicationschema/cap-iacs-base/code#SpecieCodeValue
:SpecieCodeValue rdf:type owl:NamedIndividual ,
                          <http://www.w3.org/2004/02/skos/core#ConceptScheme> ;
                 <http://purl.org/dc/terms/isFormatOf> <http://lpis.ec.europa.eu/registry/applicationschema/cap-iacs-base#SpecieCodeValue> ;
                 rdfs:label "List of vegetable and agricultural plant species"@en ;
                 <http://www.w3.org/2004/02/skos/core#definition> """-- Definition --
List of vegetable and agricultural plant species (aggregate of a varieties). 
-- Description --
A culture of any of the different genera defined in the botanical classification of crops. In this case code list consist of binomial names of species from the taxonomy of Linnaeus (classification for plants).
NOTE. Common catalogue of varieties of agricultural plant species. Fifth supplement to the 29th complete edition (2011/C 168 A/01)
List of agricultural species -A
I. Beet
II. Fodder plants
III. Oil and fibre plants    
IV. Cereals
V. Potatoes 
NOTE. Common catalogue of varieties of vegetable species. 32nd complete edition (2013/C 312 A/01)
List of vegetable species - H"""@en .


###  http://lpis.ec.europa.eu/registry/applicationschema/cap-iacs-base/code#StatusOfAnomalyValue
:StatusOfAnomalyValue rdf:type owl:NamedIndividual ,
                               <http://www.w3.org/2004/02/skos/core#ConceptScheme> ;
                      <http://purl.org/dc/terms/isFormatOf> <http://lpis.ec.europa.eu/registry/applicationschema/cap-iacs-base#StatusOfAnomalyValue> ;
                      rdfs:label "Anomaly status value list"@en ;
                      <http://www.w3.org/2004/02/skos/core#definition> """--Name--
Status of anomaly value

-- Definition --
Code list of possible anomaly status values.

-- Description --
List of possible anomaly status values used for documentation of anomaly in the information system.

NOTE. Under information system IACS is understood. Most probably anomalies are registered in the Integrated control systems or in the quality assessment leaf of LPIS QA."""@en .


###  http://lpis.ec.europa.eu/registry/applicationschema/cap-iacs-base/code#StatusOfIssueValue
:StatusOfIssueValue rdf:type owl:NamedIndividual ,
                             <http://www.w3.org/2004/02/skos/core#ConceptScheme> ;
                    <http://purl.org/dc/terms/isFormatOf> <http://lpis.ec.europa.eu/registry/applicationschema/cap-iacs-base#StatusOfIssueValue> ;
                    rdfs:label "Issue status value list"@en ;
                    <http://www.w3.org/2004/02/skos/core#definition> """--Name--
Status of issue value

-- Definition --
Code list of possible issue status values.

-- Description --
List of possible issue status values used for documentation of anomaly in the LPIS."""@en .


###  http://lpis.ec.europa.eu/registry/applicationschema/cap-iacs-base/code#StatusValue
:StatusValue rdf:type owl:NamedIndividual ,
                      <http://www.w3.org/2004/02/skos/core#ConceptScheme> ;
             <http://purl.org/dc/terms/isFormatOf> <http://lpis.ec.europa.eu/registry/applicationschema/cap-iacs-base#StatusValue> ;
             rdfs:label "List of status values"@en ;
             <http://www.w3.org/2004/02/skos/core#definition> """-- Name--
Status value

--Definition --
Code list of possible status values.

-- Description --
List of status types based on state machine diagrams (Dynamic CAP model) for new and existing object features or schema. The values included in this code list are applicable both to introduction of a new object/feature or to processing a change request.

NOTE. These are generic values applicable in IACS. These concepts have been reused in LPIS upgrade and LPIS update processes."""@en .


###  http://lpis.ec.europa.eu/registry/applicationschema/cap-iacs-base/code#SupportSchemeTypeValue
:SupportSchemeTypeValue rdf:type owl:NamedIndividual ,
                                 <http://www.w3.org/2004/02/skos/core#ConceptScheme> ;
                        <http://purl.org/dc/terms/isFormatOf> <http://lpis.ec.europa.eu/registry/applicationschema/cap-iacs-base#SupportSchemeTypeValue> ;
                        rdfs:label "List of support schemas"@en ;
                        <http://www.w3.org/2004/02/skos/core#definition> """Support scheme type value

List of support schemes as defined in Regulation (EU) 1307/2013.

NOTE
Payment schema type list may be extended or shortened by MS."""@en .


###  http://lpis.ec.europa.eu/registry/applicationschema/cap-iacs-base/code#TestTypeValue
:TestTypeValue rdf:type owl:NamedIndividual ,
                        <http://www.w3.org/2004/02/skos/core#ConceptScheme> ;
               <http://purl.org/dc/terms/isFormatOf> <http://lpis.ec.europa.eu/registry/applicationschema/cap-iacs-base#TestTypeValue> ;
               rdfs:label "Test type value list"@en ;
               <http://www.w3.org/2004/02/skos/core#definition> """--Name--
Test type value

-- Definition --
Indication whether a test belong to the basic or the capability test type.

-- Description --
A basic test is an initial test intended to identify clear cases of non-conformance. If the ATS identifies tests to be used as basic tests, they shall be used at the start of the conformance assessment process.

Capability test is designed to determine whether an IUT conforms to a particular characteristic specified as requirements."""@en .


###  http://lpis.ec.europa.eu/registry/applicationschema/cap-iacs-base/code#TestVerdictValue
:TestVerdictValue rdf:type owl:NamedIndividual ,
                           <http://www.w3.org/2004/02/skos/core#ConceptScheme> ;
                  <http://purl.org/dc/terms/isFormatOf> <http://lpis.ec.europa.eu/registry/applicationschema/cap-iacs-base#TestVerdictValue> ;
                  rdfs:label "Test verdict value list"@en ;
                  <http://www.w3.org/2004/02/skos/core#definition> """--Name--
Test verdict value

-- Definition --
List of values describing test verdicts.

-- Description --
List of possible test verdict values according to ISO 19105:2000."""@en .


###  http://lpis.ec.europa.eu/registry/applicationschema/cap-iacs-base/code#TestingTypeValue
:TestingTypeValue rdf:type owl:NamedIndividual ,
                           <http://www.w3.org/2004/02/skos/core#ConceptScheme> ;
                  <http://purl.org/dc/terms/isFormatOf> <http://lpis.ec.europa.eu/registry/applicationschema/cap-iacs-base#TestingTypeValue> ;
                  rdfs:label "Testing type value list"@en ;
                  <http://www.w3.org/2004/02/skos/core#definition> """--Name--
Testing type value

-- Definition --
Testing type value list.

-- Description --
In manual testing, the specified requirements are verified by a trained operator who follows the steps described in the test method.
In automated testing, specific software is used that operates on the computer readable schema of the eligibility profile."""@en .


###  http://lpis.ec.europa.eu/registry/applicationschema/cap-iacs-base/code#VarietalNameValue
:VarietalNameValue rdf:type owl:NamedIndividual ,
                            <http://www.w3.org/2004/02/skos/core#ConceptScheme> ;
                   <http://purl.org/dc/terms/isFormatOf> <http://lpis.ec.europa.eu/registry/applicationschema/cap-iacs-base#VarietalNameValue> ;
                   rdfs:label "List of varietal names"@en ;
                   <http://www.w3.org/2004/02/skos/core#definition> """-- Definition --
List of varietal names within vegetable and agricultural plant species. 
-- Desription --
Common catalogue of varieties of agricultural plant species. Fifth supplement to the 29th complete edition (2011/C 168 A/01).
Common catalogue of varieties of vegetable species. 32nd complete edition (2013/C 312 A/01).
This codeList decided and maintained by MS.  Varietal names are MS specific.
Dictionary: http://ec.europa.eu/food/plant/propagation/catalogues/database/public/index.cfm?event=homepage
NOTE. CODE LIST IS NOT FINISHED. ONLY SOME EXAMPLES ARE PROVIDED."""@en .


###  http://lpis.ec.europa.eu/registry/applicationschema/cap-iacs-base/code#WeekdayValue
:WeekdayValue rdf:type owl:NamedIndividual ,
                       <http://www.w3.org/2004/02/skos/core#ConceptScheme> ;
              <http://purl.org/dc/terms/isFormatOf> <http://lpis.ec.europa.eu/registry/applicationschema/cap-iacs-base#WeekdayValue> ;
              rdfs:label "List of weekday values"@en ;
              <http://www.w3.org/2004/02/skos/core#definition> """-- Definition --
List of possible weekdays.
-- Description --
List of possible weekdays."""@en .


###  http://lpis.ec.europa.eu/registry/applicationschema/cap-iacs-base/code#AffectedElementTypeValue/applicationSchema
<http://lpis.ec.europa.eu/registry/applicationschema/cap-iacs-base/code#AffectedElementTypeValue/applicationSchema> rdf:type owl:NamedIndividual ,
                                                                                                                             <http://lpis.ec.europa.eu/registry/applicationschema/cap-iacs-base#AffectedElementTypeValue> ;
                                                                                                                    rdfs:label "Application schema"@en ;
                                                                                                                    <http://www.w3.org/2004/02/skos/core#definition> """--Name--
Application schema

-- Definition --
Conceptual schema for data required for one or more applications [ISO 19101:2002]."""@en ;
                                                                                                                    <http://www.w3.org/2004/02/skos/core#inScheme> :AffectedElementTypeValue .


###  http://lpis.ec.europa.eu/registry/applicationschema/cap-iacs-base/code#AffectedElementTypeValue/applicationSchemaLeaf
<http://lpis.ec.europa.eu/registry/applicationschema/cap-iacs-base/code#AffectedElementTypeValue/applicationSchemaLeaf> rdf:type owl:NamedIndividual ,
                                                                                                                                 <http://lpis.ec.europa.eu/registry/applicationschema/cap-iacs-base#AffectedElementTypeValue> ;
                                                                                                                        rdfs:label "Leaf of application schema"@en ;
                                                                                                                        <http://www.w3.org/2004/02/skos/core#definition> """--Name--
Application schema leaf

-- Definition --
Specific package within the application schema that cannot include further (sub)packages."""@en ;
                                                                                                                        <http://www.w3.org/2004/02/skos/core#inScheme> :AffectedElementTypeValue .


###  http://lpis.ec.europa.eu/registry/applicationschema/cap-iacs-base/code#AffectedElementTypeValue/associationRole
<http://lpis.ec.europa.eu/registry/applicationschema/cap-iacs-base/code#AffectedElementTypeValue/associationRole> rdf:type owl:NamedIndividual ,
                                                                                                                           <http://lpis.ec.europa.eu/registry/applicationschema/cap-iacs-base#AffectedElementTypeValue> ;
                                                                                                                  rdfs:label "Relationship"@en ;
                                                                                                                  <http://www.w3.org/2004/02/skos/core#definition> """--Name--
Association role

-- Definition --
Semantic relationship that can occur between type instances [ISO 19103:2005]"""@en ;
                                                                                                                  <http://www.w3.org/2004/02/skos/core#inScheme> :AffectedElementTypeValue .


###  http://lpis.ec.europa.eu/registry/applicationschema/cap-iacs-base/code#AffectedElementTypeValue/attribute
<http://lpis.ec.europa.eu/registry/applicationschema/cap-iacs-base/code#AffectedElementTypeValue/attribute> rdf:type owl:NamedIndividual ,
                                                                                                                     <http://lpis.ec.europa.eu/registry/applicationschema/cap-iacs-base#AffectedElementTypeValue> ;
                                                                                                            rdfs:label "Property"@en ;
                                                                                                            <http://www.w3.org/2004/02/skos/core#definition> """--Name--
Attribute

-- Definition --
UML feature  within a classifier that describes a range of values (B.515) that instances of the classifier may hold. [ISO/TS 19103:2005 – adapted from ISO/IEC 19501]"""@en ;
                                                                                                            <http://www.w3.org/2004/02/skos/core#inScheme> :AffectedElementTypeValue .


###  http://lpis.ec.europa.eu/registry/applicationschema/cap-iacs-base/code#AffectedElementTypeValue/codeList
<http://lpis.ec.europa.eu/registry/applicationschema/cap-iacs-base/code#AffectedElementTypeValue/codeList> rdf:type owl:NamedIndividual ,
                                                                                                                    <http://lpis.ec.europa.eu/registry/applicationschema/cap-iacs-base#AffectedElementTypeValue> ;
                                                                                                           rdfs:label "Code list"@en ;
                                                                                                           <http://www.w3.org/2004/02/skos/core#definition> """--Name--
Code list

-- Definition --
Set of pre-defined values that an attribute may take."""@en ;
                                                                                                           <http://www.w3.org/2004/02/skos/core#inScheme> :AffectedElementTypeValue .


###  http://lpis.ec.europa.eu/registry/applicationschema/cap-iacs-base/code#AffectedElementTypeValue/dataType
<http://lpis.ec.europa.eu/registry/applicationschema/cap-iacs-base/code#AffectedElementTypeValue/dataType> rdf:type owl:NamedIndividual ,
                                                                                                                    <http://lpis.ec.europa.eu/registry/applicationschema/cap-iacs-base#AffectedElementTypeValue> ;
                                                                                                           rdfs:label "Data type"@en ;
                                                                                                           <http://www.w3.org/2004/02/skos/core#definition> """--Name--
Data type

-- Definition --
Specification of a value domain with operations allowed on values in this domain [ISO 19103:2005].

-- Description --
For purposes of LCM, this term is used for proprietary (user-defined) and imported (from third parties) data types."""@en ;
                                                                                                           <http://www.w3.org/2004/02/skos/core#inScheme> :AffectedElementTypeValue .


###  http://lpis.ec.europa.eu/registry/applicationschema/cap-iacs-base/code#AffectedElementTypeValue/featureType
<http://lpis.ec.europa.eu/registry/applicationschema/cap-iacs-base/code#AffectedElementTypeValue/featureType> rdf:type owl:NamedIndividual ,
                                                                                                                       <http://lpis.ec.europa.eu/registry/applicationschema/cap-iacs-base#AffectedElementTypeValue> ;
                                                                                                              rdfs:label "Feature type"@en ;
                                                                                                              <http://www.w3.org/2004/02/skos/core#definition> """--Name--
Feature type

-- Definition --
A class that specifies set of spatial objects sharing common properties and operations applicable to the objects."""@en ;
                                                                                                              <http://www.w3.org/2004/02/skos/core#inScheme> :AffectedElementTypeValue .


###  http://lpis.ec.europa.eu/registry/applicationschema/cap-iacs-base/code#AffectedElementTypeValue/multiplicity
<http://lpis.ec.europa.eu/registry/applicationschema/cap-iacs-base/code#AffectedElementTypeValue/multiplicity> rdf:type owl:NamedIndividual ,
                                                                                                                        <http://lpis.ec.europa.eu/registry/applicationschema/cap-iacs-base#AffectedElementTypeValue> ;
                                                                                                               rdfs:label "Enumeration"@en ;
                                                                                                               <http://www.w3.org/2004/02/skos/core#definition> """--Name--
Multiplicity

-- Definition --
Specification of the range of allowable cardinalities that a set may assume."""@en ;
                                                                                                               <http://www.w3.org/2004/02/skos/core#inScheme> :AffectedElementTypeValue .


###  http://lpis.ec.europa.eu/registry/applicationschema/cap-iacs-base/code#AffectedElementTypeValue/ocl
<http://lpis.ec.europa.eu/registry/applicationschema/cap-iacs-base/code#AffectedElementTypeValue/ocl> rdf:type owl:NamedIndividual ,
                                                                                                               <http://lpis.ec.europa.eu/registry/applicationschema/cap-iacs-base#AffectedElementTypeValue> ;
                                                                                                      rdfs:label "OCL"@en ;
                                                                                                      <http://www.w3.org/2004/02/skos/core#definition> """--Name--
OCL

-- Definition --
The Object Constraint Language (OCL) is a declarative language for describing rules that apply to Unified Modelling Language (UML) models."""@en ;
                                                                                                      <http://www.w3.org/2004/02/skos/core#inScheme> :AffectedElementTypeValue .


###  http://lpis.ec.europa.eu/registry/applicationschema/cap-iacs-base/code#AffectedElementTypeValue/type
<http://lpis.ec.europa.eu/registry/applicationschema/cap-iacs-base/code#AffectedElementTypeValue/type> rdf:type owl:NamedIndividual ,
                                                                                                                <http://lpis.ec.europa.eu/registry/applicationschema/cap-iacs-base#AffectedElementTypeValue> ;
                                                                                                       rdfs:label "Type"@en ;
                                                                                                       <http://www.w3.org/2004/02/skos/core#definition> """--Name--
Type

-- Definition --
Specification of a value domain [ISO 19103:2005].

-- Description --
Types include data types, enumerated types, code list values, etc.

EXAMPLE 1. Primitive types defined in international standards: integer, boolean, GM_Object, etc.

EXAMPLE 2. Own types defined in the model and re-used for different purposes. LPIS QA uses the TechnicalReasonValue type to describe critical defects and contaminations with the same technical terms.

EXAMPLE 3. Types defined in other model and imported for re-use. LCM uses  DocumentCitation type defined in INSPIRE."""@en ;
                                                                                                       <http://www.w3.org/2004/02/skos/core#inScheme> :AffectedElementTypeValue .


###  http://lpis.ec.europa.eu/registry/applicationschema/cap-iacs-base/code#AffectedElementTypeValue/union
<http://lpis.ec.europa.eu/registry/applicationschema/cap-iacs-base/code#AffectedElementTypeValue/union> rdf:type owl:NamedIndividual ,
                                                                                                                 <http://lpis.ec.europa.eu/registry/applicationschema/cap-iacs-base#AffectedElementTypeValue> ;
                                                                                                        rdfs:label "Union"@en ;
                                                                                                        <http://www.w3.org/2004/02/skos/core#definition> """--Name--
Union

-- Definition --
A class, which defines a collection of Simple Types defined in ISO 19103:2005."""@en ;
                                                                                                        <http://www.w3.org/2004/02/skos/core#inScheme> :AffectedElementTypeValue .


###  http://lpis.ec.europa.eu/registry/applicationschema/cap-iacs-base/code#CauseOfAnomalyValue/appearanceOfPermanentConstruction
<http://lpis.ec.europa.eu/registry/applicationschema/cap-iacs-base/code#CauseOfAnomalyValue/appearanceOfPermanentConstruction> rdf:type owl:NamedIndividual ,
                                                                                                                                        <http://lpis.ec.europa.eu/registry/applicationschema/cap-iacs-base#CauseOfAnomalyValue> ;
                                                                                                                               rdfs:label "Cause flaged as Type II. The appearance of permanent construction"@en ;
                                                                                                                               <http://www.w3.org/2004/02/skos/core#definition> """--Name--
Appearance of permanent construction

-- Description --
The appearance of buildings, roads, and other sealed surfaces that are likely to stay in the place of former agricultural land more than three years."""@en ;
                                                                                                                               <http://www.w3.org/2004/02/skos/core#inScheme> :CauseOfAnomalyValue .


###  http://lpis.ec.europa.eu/registry/applicationschema/cap-iacs-base/code#CauseOfAnomalyValue/causeUnknown
<http://lpis.ec.europa.eu/registry/applicationschema/cap-iacs-base/code#CauseOfAnomalyValue/causeUnknown> rdf:type owl:NamedIndividual ,
                                                                                                                   <http://lpis.ec.europa.eu/registry/applicationschema/cap-iacs-base#CauseOfAnomalyValue> ;
                                                                                                          rdfs:label "The cause is flagged as unknown"@en ;
                                                                                                          <http://www.w3.org/2004/02/skos/core#definition> """--Name--
Cause unknown

-- Description --
No case can be detected and/or no third party information is available about the possible cause of anomaly."""@en ;
                                                                                                          <http://www.w3.org/2004/02/skos/core#inScheme> :CauseOfAnomalyValue .


###  http://lpis.ec.europa.eu/registry/applicationschema/cap-iacs-base/code#CauseOfAnomalyValue/changeInThePerimeterAdditionOfAgriculturalLand
<http://lpis.ec.europa.eu/registry/applicationschema/cap-iacs-base/code#CauseOfAnomalyValue/changeInThePerimeterAdditionOfAgriculturalLand> rdf:type owl:NamedIndividual ,
                                                                                                                                                     <http://lpis.ec.europa.eu/registry/applicationschema/cap-iacs-base#CauseOfAnomalyValue> ;
                                                                                                                                            rdfs:label "Cause flaged as Type III. Change in the perimeter (addition of agricultural land)"@en ;
                                                                                                                                            <http://www.w3.org/2004/02/skos/core#definition> """--Name--
Change in the perimeter due to addition of agricultural land

-- Description --
New agricultural area has been appended to an existing reference parcel.

NOTE. Previously known as Type III anomaly."""@en ;
                                                                                                                                            <http://www.w3.org/2004/02/skos/core#inScheme> :CauseOfAnomalyValue .


###  http://lpis.ec.europa.eu/registry/applicationschema/cap-iacs-base/code#CauseOfAnomalyValue/changeInThePerimeterExchangeOfAgriculturalLand
<http://lpis.ec.europa.eu/registry/applicationschema/cap-iacs-base/code#CauseOfAnomalyValue/changeInThePerimeterExchangeOfAgriculturalLand> rdf:type owl:NamedIndividual ,
                                                                                                                                                     <http://lpis.ec.europa.eu/registry/applicationschema/cap-iacs-base#CauseOfAnomalyValue> ;
                                                                                                                                            rdfs:label "Cause flaged as Type IV. Change in the perimeter (exchange of agricultural land)"@en ;
                                                                                                                                            <http://www.w3.org/2004/02/skos/core#definition> """--Name--
Change in the perimeter due to exchange of agricultural land

-- Description --
The minimum number of involved parcels is two. The anomaly is manifested by a change of their shape and area.

NOTE. Previously this cause was flagged as Type IV anomaly."""@en ;
                                                                                                                                            <http://www.w3.org/2004/02/skos/core#inScheme> :CauseOfAnomalyValue .


###  http://lpis.ec.europa.eu/registry/applicationschema/cap-iacs-base/code#CauseOfAnomalyValue/irreversibleConversionsOfAgriculturalLandCovers
<http://lpis.ec.europa.eu/registry/applicationschema/cap-iacs-base/code#CauseOfAnomalyValue/irreversibleConversionsOfAgriculturalLandCovers> rdf:type owl:NamedIndividual ,
                                                                                                                                                      <http://lpis.ec.europa.eu/registry/applicationschema/cap-iacs-base#CauseOfAnomalyValue> ;
                                                                                                                                             rdfs:label "Cause flaged as Type I. Irreversible conversions of agricultural land covers"@en ;
                                                                                                                                             <http://www.w3.org/2004/02/skos/core#definition> """--Name--
Irreversible conversion of agricultural land covers

-- Description --
Appearance of forests, deserted areas, rock outcrops, inundated areas, etc. in the place of former agricultural land."""@en ;
                                                                                                                                             <http://www.w3.org/2004/02/skos/core#inScheme> :CauseOfAnomalyValue .


###  http://lpis.ec.europa.eu/registry/applicationschema/cap-iacs-base/code#CauseOfAnomalyValue/misclassifiedProrataClass
<http://lpis.ec.europa.eu/registry/applicationschema/cap-iacs-base/code#CauseOfAnomalyValue/misclassifiedProrataClass> rdf:type owl:NamedIndividual ,
                                                                                                                                <http://lpis.ec.europa.eu/registry/applicationschema/cap-iacs-base#CauseOfAnomalyValue> ;
                                                                                                                       <http://www.w3.org/2004/02/skos/core#inScheme> :CauseOfAnomalyValue .


###  http://lpis.ec.europa.eu/registry/applicationschema/cap-iacs-base/code#CauseOfAnomalyValue/notConfirmed
<http://lpis.ec.europa.eu/registry/applicationschema/cap-iacs-base/code#CauseOfAnomalyValue/notConfirmed> rdf:type owl:NamedIndividual ,
                                                                                                                   <http://lpis.ec.europa.eu/registry/applicationschema/cap-iacs-base#CauseOfAnomalyValue> ;
                                                                                                          rdfs:label "Cause flagged as no change in the data"@en ;
                                                                                                          <http://www.w3.org/2004/02/skos/core#definition> """--Name--
Not confirmed

-- Description--
The preliminary classification of the anomaly cause cannot be confirmed."""@en ;
                                                                                                          <http://www.w3.org/2004/02/skos/core#inScheme> :CauseOfAnomalyValue .


###  http://lpis.ec.europa.eu/registry/applicationschema/cap-iacs-base/code#ConformanceClassValue/classA
<http://lpis.ec.europa.eu/registry/applicationschema/cap-iacs-base/code#ConformanceClassValue/classA> rdf:type owl:NamedIndividual ,
                                                                                                               <http://lpis.ec.europa.eu/registry/applicationschema/cap-iacs-base#ConformanceClassValue> ;
                                                                                                      rdfs:label "Class A"@en ;
                                                                                                      <http://www.w3.org/2004/02/skos/core#definition> """--Name--
Class A

--Definition--
Specified conformance class.

--Description--
Separate ATS must be provided if a class is defined within ConformanceClause."""@en ;
                                                                                                      <http://www.w3.org/2004/02/skos/core#inScheme> :ConformanceClassValue .


###  http://lpis.ec.europa.eu/registry/applicationschema/cap-iacs-base/code#ConformanceClassValue/classB
<http://lpis.ec.europa.eu/registry/applicationschema/cap-iacs-base/code#ConformanceClassValue/classB> rdf:type owl:NamedIndividual ,
                                                                                                               <http://lpis.ec.europa.eu/registry/applicationschema/cap-iacs-base#ConformanceClassValue> ;
                                                                                                      rdfs:label "Class B"@en ;
                                                                                                      <http://www.w3.org/2004/02/skos/core#definition> """--Name--
Class B

--Definition--
Specified conformance class.

--Description--
Separate ATS must be provided if a class is defined within ConformanceClause"""@en ;
                                                                                                      <http://www.w3.org/2004/02/skos/core#inScheme> :ConformanceClassValue .


###  http://lpis.ec.europa.eu/registry/applicationschema/cap-iacs-base/code#ConformanceClassValue/classC
<http://lpis.ec.europa.eu/registry/applicationschema/cap-iacs-base/code#ConformanceClassValue/classC> rdf:type owl:NamedIndividual ,
                                                                                                               <http://lpis.ec.europa.eu/registry/applicationschema/cap-iacs-base#ConformanceClassValue> ;
                                                                                                      rdfs:label "Class C"@en ;
                                                                                                      <http://www.w3.org/2004/02/skos/core#definition> """--Name--
Class C

--Definition--
Specified conformance class.

--Description--
Separate ATS must be provided if a class is defined within ConformanceClause."""@en ;
                                                                                                      <http://www.w3.org/2004/02/skos/core#inScheme> :ConformanceClassValue .


###  http://lpis.ec.europa.eu/registry/applicationschema/cap-iacs-base/code#ConformanceLevelValue/level1
<http://lpis.ec.europa.eu/registry/applicationschema/cap-iacs-base/code#ConformanceLevelValue/level1> rdf:type owl:NamedIndividual ,
                                                                                                               <http://lpis.ec.europa.eu/registry/applicationschema/cap-iacs-base#ConformanceLevelValue> ;
                                                                                                      rdfs:label "Level 1 low"@en ;
                                                                                                      <http://www.w3.org/2004/02/skos/core#definition> """--Name--
Level 1

--Definition--
Lowest level conformance.

--Description--
A separate abstract test suite must be provided if a level is defined within ConformanceClause."""@en ;
                                                                                                      <http://www.w3.org/2004/02/skos/core#inScheme> :ConformanceLevelValue .


###  http://lpis.ec.europa.eu/registry/applicationschema/cap-iacs-base/code#ConformanceLevelValue/level2
<http://lpis.ec.europa.eu/registry/applicationschema/cap-iacs-base/code#ConformanceLevelValue/level2> rdf:type owl:NamedIndividual ,
                                                                                                               <http://lpis.ec.europa.eu/registry/applicationschema/cap-iacs-base#ConformanceLevelValue> ;
                                                                                                      rdfs:label "Level 2 medium"@en ;
                                                                                                      <http://www.w3.org/2004/02/skos/core#definition> """--Name--
Level 2

--Definition--
Lowest level conformance.

--Description--
A separate abstract test suite must be provided if a level is defined within ConformanceClause."""@en ;
                                                                                                      <http://www.w3.org/2004/02/skos/core#inScheme> :ConformanceLevelValue .


###  http://lpis.ec.europa.eu/registry/applicationschema/cap-iacs-base/code#ConformanceLevelValue/level3
<http://lpis.ec.europa.eu/registry/applicationschema/cap-iacs-base/code#ConformanceLevelValue/level3> rdf:type owl:NamedIndividual ,
                                                                                                               <http://lpis.ec.europa.eu/registry/applicationschema/cap-iacs-base#ConformanceLevelValue> ;
                                                                                                      rdfs:label "Level 3 high"@en ;
                                                                                                      <http://www.w3.org/2004/02/skos/core#definition> """--Name--
Level 3

--Definition--
Highest level conformance.

--Description--
A separate abstract test suite must be provided if a level is defined within ConformanceClause."""@en ;
                                                                                                      <http://www.w3.org/2004/02/skos/core#inScheme> :ConformanceLevelValue .


###  http://lpis.ec.europa.eu/registry/applicationschema/cap-iacs-base/code#ConformanceRequirementClassValue/conditional
<http://lpis.ec.europa.eu/registry/applicationschema/cap-iacs-base/code#ConformanceRequirementClassValue/conditional> rdf:type owl:NamedIndividual ,
                                                                                                                               <http://lpis.ec.europa.eu/registry/applicationschema/cap-iacs-base#ConformanceRequirementClassValue> ;
                                                                                                                      rdfs:label "Conditional requirement"@en ;
                                                                                                                      <http://www.w3.org/2004/02/skos/core#definition> """--Name--
Conditional

--Definition--
Requirement that shall be observed if the conditions set out in the specification apply."""@en ;
                                                                                                                      <http://www.w3.org/2004/02/skos/core#inScheme> :ConformanceRequirementClassValue .


###  http://lpis.ec.europa.eu/registry/applicationschema/cap-iacs-base/code#ConformanceRequirementClassValue/mandatory
<http://lpis.ec.europa.eu/registry/applicationschema/cap-iacs-base/code#ConformanceRequirementClassValue/mandatory> rdf:type owl:NamedIndividual ,
                                                                                                                             <http://lpis.ec.europa.eu/registry/applicationschema/cap-iacs-base#ConformanceRequirementClassValue> ;
                                                                                                                    rdfs:label "Mandatory requirement"@en ;
                                                                                                                    <http://www.w3.org/2004/02/skos/core#definition> """--Name--
Mandatory

--Definition--
Requirement that shall be observed in all cases. 

--Description--
This has to be fulfilled for conformance."""@en ;
                                                                                                                    <http://www.w3.org/2004/02/skos/core#inScheme> :ConformanceRequirementClassValue .


###  http://lpis.ec.europa.eu/registry/applicationschema/cap-iacs-base/code#ConformanceRequirementClassValue/optional
<http://lpis.ec.europa.eu/registry/applicationschema/cap-iacs-base/code#ConformanceRequirementClassValue/optional> rdf:type owl:NamedIndividual ,
                                                                                                                            <http://lpis.ec.europa.eu/registry/applicationschema/cap-iacs-base#ConformanceRequirementClassValue> ;
                                                                                                                   rdfs:label "Optional requirement"@en ;
                                                                                                                   <http://www.w3.org/2004/02/skos/core#definition> """--Name--
Optional

--Definition--
Requirement that may be selected to suit the implementation, provided that any condition applicable to the option are observed."""@en ;
                                                                                                                   <http://www.w3.org/2004/02/skos/core#inScheme> :ConformanceRequirementClassValue .


###  http://lpis.ec.europa.eu/registry/applicationschema/cap-iacs-base/code#ConformanceRequirementStatementValue/negative
<http://lpis.ec.europa.eu/registry/applicationschema/cap-iacs-base/code#ConformanceRequirementStatementValue/negative> rdf:type owl:NamedIndividual ,
                                                                                                                                <http://lpis.ec.europa.eu/registry/applicationschema/cap-iacs-base#ConformanceRequirementStatementValue> ;
                                                                                                                       rdfs:label "Negative statement"@en ;
                                                                                                                       <http://www.w3.org/2004/02/skos/core#definition> """--Name--
Negative

--Definition--
Negative statement.

--Description--
Negative statement state what is required not to be observed."""@en ;
                                                                                                                       <http://www.w3.org/2004/02/skos/core#inScheme> :ConformanceRequirementStatementValue .


###  http://lpis.ec.europa.eu/registry/applicationschema/cap-iacs-base/code#ConformanceRequirementStatementValue/positive
<http://lpis.ec.europa.eu/registry/applicationschema/cap-iacs-base/code#ConformanceRequirementStatementValue/positive> rdf:type owl:NamedIndividual ,
                                                                                                                                <http://lpis.ec.europa.eu/registry/applicationschema/cap-iacs-base#ConformanceRequirementStatementValue> ;
                                                                                                                       rdfs:label "Positive statement"@en ;
                                                                                                                       <http://www.w3.org/2004/02/skos/core#definition> """--Name--
Positive

--Definition--
Affirmative statement.

--Description--
Positive statement state what is required to be done."""@en ;
                                                                                                                       <http://www.w3.org/2004/02/skos/core#inScheme> :ConformanceRequirementStatementValue .


###  http://lpis.ec.europa.eu/registry/applicationschema/cap-iacs-base/code#ConformanceStatementValue/conforming
<http://lpis.ec.europa.eu/registry/applicationschema/cap-iacs-base/code#ConformanceStatementValue/conforming> rdf:type owl:NamedIndividual ,
                                                                                                                       <http://lpis.ec.europa.eu/registry/applicationschema/cap-iacs-base#ConformanceStatementValue> ;
                                                                                                              rdfs:label "Confroming"@en ;
                                                                                                              <http://www.w3.org/2004/02/skos/core#definition> """-- Name--
Conforming

-- Description --
The tested object complies with rules, standards, or laws."""@en ;
                                                                                                              <http://www.w3.org/2004/02/skos/core#inScheme> :ConformanceStatementValue .


###  http://lpis.ec.europa.eu/registry/applicationschema/cap-iacs-base/code#ConformanceStatementValue/nonConforming
<http://lpis.ec.europa.eu/registry/applicationschema/cap-iacs-base/code#ConformanceStatementValue/nonConforming> rdf:type owl:NamedIndividual ,
                                                                                                                          <http://lpis.ec.europa.eu/registry/applicationschema/cap-iacs-base#ConformanceStatementValue> ;
                                                                                                                 rdfs:label "Non-conforming"@en ;
                                                                                                                 <http://www.w3.org/2004/02/skos/core#definition> """-- Name--
Non-conforming

-- Description --
The tested object does not comply with rules, standards, or laws."""@en ;
                                                                                                                 <http://www.w3.org/2004/02/skos/core#inScheme> :ConformanceStatementValue .


###  http://lpis.ec.europa.eu/registry/applicationschema/cap-iacs-base/code#CropItemCodeValue/almonds
<http://lpis.ec.europa.eu/registry/applicationschema/cap-iacs-base/code#CropItemCodeValue/almonds> rdf:type owl:NamedIndividual ,
                                                                                                            <http://lpis.ec.europa.eu/registry/applicationschema/cap-iacs-base#CropItemCodeValue> ;
                                                                                                   rdfs:label "Almonds"@en ;
                                                                                                   <http://www.w3.org/2004/02/skos/core#definition> """-- Definition --
|||Almonds.
-- Description --
Cereals and main crops - C
NOTE. Initial value:C2233"""@en ;
                                                                                                   <http://www.w3.org/2004/02/skos/core#inScheme> :CropItemCodeValue .


###  http://lpis.ec.europa.eu/registry/applicationschema/cap-iacs-base/code#CropItemCodeValue/annualPlantsHarvestedGreenC2611
<http://lpis.ec.europa.eu/registry/applicationschema/cap-iacs-base/code#CropItemCodeValue/annualPlantsHarvestedGreenC2611> rdf:type owl:NamedIndividual ,
                                                                                                                                    <http://lpis.ec.europa.eu/registry/applicationschema/cap-iacs-base#CropItemCodeValue> ;
                                                                                                                           rdfs:label "Annual plants harvested green C2611"@en ;
                                                                                                                           <http://www.w3.org/2004/02/skos/core#definition> """-- Definition --
||Annual plants harvested green C2611.
-- Description --
Cereals and main crops - C
NOTE. Initial value:C2611"""@en ;
                                                                                                                           <http://www.w3.org/2004/02/skos/core#inScheme> :CropItemCodeValue .


###  http://lpis.ec.europa.eu/registry/applicationschema/cap-iacs-base/code#CropItemCodeValue/apples
<http://lpis.ec.europa.eu/registry/applicationschema/cap-iacs-base/code#CropItemCodeValue/apples> rdf:type owl:NamedIndividual ,
                                                                                                           <http://lpis.ec.europa.eu/registry/applicationschema/cap-iacs-base#CropItemCodeValue> ;
                                                                                                  rdfs:label "Apples"@en ;
                                                                                                  <http://www.w3.org/2004/02/skos/core#definition> """-- Definition --
||Apples.
-- Description --
Cereals and main crops - C
NOTE. Initial value:C2090"""@en ;
                                                                                                  <http://www.w3.org/2004/02/skos/core#inScheme> :CropItemCodeValue .


###  http://lpis.ec.europa.eu/registry/applicationschema/cap-iacs-base/code#CropItemCodeValue/applesForFreshConsumption
<http://lpis.ec.europa.eu/registry/applicationschema/cap-iacs-base/code#CropItemCodeValue/applesForFreshConsumption> rdf:type owl:NamedIndividual ,
                                                                                                                              <http://lpis.ec.europa.eu/registry/applicationschema/cap-iacs-base#CropItemCodeValue> ;
                                                                                                                     rdfs:label "Apples for fresh consumption"@en ;
                                                                                                                     <http://www.w3.org/2004/02/skos/core#definition> """-- Definition --
|||Apples for fresh consumption.
-- Description --
Cereals and main crops - C
NOTE. Initial value:C2110"""@en ;
                                                                                                                     <http://www.w3.org/2004/02/skos/core#inScheme> :CropItemCodeValue .


###  http://lpis.ec.europa.eu/registry/applicationschema/cap-iacs-base/code#CropItemCodeValue/apricots
<http://lpis.ec.europa.eu/registry/applicationschema/cap-iacs-base/code#CropItemCodeValue/apricots> rdf:type owl:NamedIndividual ,
                                                                                                             <http://lpis.ec.europa.eu/registry/applicationschema/cap-iacs-base#CropItemCodeValue> ;
                                                                                                    rdfs:label "Apricots"@en ;
                                                                                                    <http://www.w3.org/2004/02/skos/core#definition> """-- Definition --
|||Apricots.
-- Description --
Cereals and main crops - C
NOTE. Initial value:C2190"""@en ;
                                                                                                    <http://www.w3.org/2004/02/skos/core#inScheme> :CropItemCodeValue .


###  http://lpis.ec.europa.eu/registry/applicationschema/cap-iacs-base/code#CropItemCodeValue/arableLand
<http://lpis.ec.europa.eu/registry/applicationschema/cap-iacs-base/code#CropItemCodeValue/arableLand> rdf:type owl:NamedIndividual ,
                                                                                                               <http://lpis.ec.europa.eu/registry/applicationschema/cap-iacs-base#CropItemCodeValue> ;
                                                                                                      rdfs:label "Arable land"@en ;
                                                                                                      <http://www.w3.org/2004/02/skos/core#definition> """-- Definition --
||Arable land.
-- Description --
Land use of Agriculture Area in Use -L
NOTE. Initial value:L0001"""@en ;
                                                                                                      <http://www.w3.org/2004/02/skos/core#inScheme> :CropItemCodeValue .


###  http://lpis.ec.europa.eu/registry/applicationschema/cap-iacs-base/code#CropItemCodeValue/aromaticPlantsMedicinalAndCulinaryPlants
<http://lpis.ec.europa.eu/registry/applicationschema/cap-iacs-base/code#CropItemCodeValue/aromaticPlantsMedicinalAndCulinaryPlants> rdf:type owl:NamedIndividual ,
                                                                                                                                             <http://lpis.ec.europa.eu/registry/applicationschema/cap-iacs-base#CropItemCodeValue> ;
                                                                                                                                    rdfs:label "Aromatic plants, medicinal and culinary plants"@en ;
                                                                                                                                    <http://www.w3.org/2004/02/skos/core#definition> """-- Definition --
|||Aromatic plants, medicinal and culinary plants.
-- Description --
Cereals and main crops - C
NOTE. Initial value:C1580"""@en ;
                                                                                                                                    <http://www.w3.org/2004/02/skos/core#inScheme> :CropItemCodeValue .


###  http://lpis.ec.europa.eu/registry/applicationschema/cap-iacs-base/code#CropItemCodeValue/artichokes
<http://lpis.ec.europa.eu/registry/applicationschema/cap-iacs-base/code#CropItemCodeValue/artichokes> rdf:type owl:NamedIndividual ,
                                                                                                               <http://lpis.ec.europa.eu/registry/applicationschema/cap-iacs-base#CropItemCodeValue> ;
                                                                                                      rdfs:label "Artichokes"@en ;
                                                                                                      <http://www.w3.org/2004/02/skos/core#definition> """-- Definition --
|||Artichokes.
-- Description --
Cereals and main crops - C
NOTE. Initial value:C1720"""@en ;
                                                                                                      <http://www.w3.org/2004/02/skos/core#inScheme> :CropItemCodeValue .


###  http://lpis.ec.europa.eu/registry/applicationschema/cap-iacs-base/code#CropItemCodeValue/asparagus
<http://lpis.ec.europa.eu/registry/applicationschema/cap-iacs-base/code#CropItemCodeValue/asparagus> rdf:type owl:NamedIndividual ,
                                                                                                              <http://lpis.ec.europa.eu/registry/applicationschema/cap-iacs-base#CropItemCodeValue> ;
                                                                                                     rdfs:label "Asparagus"@en ;
                                                                                                     <http://www.w3.org/2004/02/skos/core#definition> """-- Definition --
|||Asparagus.
-- Description --
Cereals and main crops - C
NOTE. Initial value:C1700"""@en ;
                                                                                                     <http://www.w3.org/2004/02/skos/core#inScheme> :CropItemCodeValue .


###  http://lpis.ec.europa.eu/registry/applicationschema/cap-iacs-base/code#CropItemCodeValue/avocados
<http://lpis.ec.europa.eu/registry/applicationschema/cap-iacs-base/code#CropItemCodeValue/avocados> rdf:type owl:NamedIndividual ,
                                                                                                             <http://lpis.ec.europa.eu/registry/applicationschema/cap-iacs-base#CropItemCodeValue> ;
                                                                                                    rdfs:label "Avocados"@en ;
                                                                                                    <http://www.w3.org/2004/02/skos/core#definition> """-- Definition --
|||Avocados.
-- Description --
Cereals and main crops - C
NOTE. Initial value:C2253"""@en ;
                                                                                                    <http://www.w3.org/2004/02/skos/core#inScheme> :CropItemCodeValue .


###  http://lpis.ec.europa.eu/registry/applicationschema/cap-iacs-base/code#CropItemCodeValue/bananas
<http://lpis.ec.europa.eu/registry/applicationschema/cap-iacs-base/code#CropItemCodeValue/bananas> rdf:type owl:NamedIndividual ,
                                                                                                            <http://lpis.ec.europa.eu/registry/applicationschema/cap-iacs-base#CropItemCodeValue> ;
                                                                                                   rdfs:label "Bananas"@en ;
                                                                                                   <http://www.w3.org/2004/02/skos/core#definition> """-- Definition --
|||Bananas.
-- Description --
Cereals and main crops - C
NOTE. Initial value:C2254"""@en ;
                                                                                                   <http://www.w3.org/2004/02/skos/core#inScheme> :CropItemCodeValue .


###  http://lpis.ec.europa.eu/registry/applicationschema/cap-iacs-base/code#CropItemCodeValue/barley
<http://lpis.ec.europa.eu/registry/applicationschema/cap-iacs-base/code#CropItemCodeValue/barley> rdf:type owl:NamedIndividual ,
                                                                                                           <http://lpis.ec.europa.eu/registry/applicationschema/cap-iacs-base#CropItemCodeValue> ;
                                                                                                  rdfs:label "Barley"@en ;
                                                                                                  <http://www.w3.org/2004/02/skos/core#definition> """-- Definition --
|||Barley.
-- Description --
Cereals and main crops - C
NOTE. Initial value:C1160"""@en ;
                                                                                                  <http://www.w3.org/2004/02/skos/core#inScheme> :CropItemCodeValue .


###  http://lpis.ec.europa.eu/registry/applicationschema/cap-iacs-base/code#CropItemCodeValue/beans
<http://lpis.ec.europa.eu/registry/applicationschema/cap-iacs-base/code#CropItemCodeValue/beans> rdf:type owl:NamedIndividual ,
                                                                                                          <http://lpis.ec.europa.eu/registry/applicationschema/cap-iacs-base#CropItemCodeValue> ;
                                                                                                 rdfs:label "Beans"@en ;
                                                                                                 <http://www.w3.org/2004/02/skos/core#definition> """-- Definition --
|||Beans.
-- Description --
Cereals and main crops - C
NOTE. Initial value:C1901"""@en ;
                                                                                                 <http://www.w3.org/2004/02/skos/core#inScheme> :CropItemCodeValue .


###  http://lpis.ec.europa.eu/registry/applicationschema/cap-iacs-base/code#CropItemCodeValue/beetroot
<http://lpis.ec.europa.eu/registry/applicationschema/cap-iacs-base/code#CropItemCodeValue/beetroot> rdf:type owl:NamedIndividual ,
                                                                                                             <http://lpis.ec.europa.eu/registry/applicationschema/cap-iacs-base#CropItemCodeValue> ;
                                                                                                    rdfs:label "Beetroot"@en ;
                                                                                                    <http://www.w3.org/2004/02/skos/core#definition> """-- Definition --
|||Beetroot.
-- Description --
Cereals and main crops - C
NOTE. Initial value:C1860"""@en ;
                                                                                                    <http://www.w3.org/2004/02/skos/core#inScheme> :CropItemCodeValue .


###  http://lpis.ec.europa.eu/registry/applicationschema/cap-iacs-base/code#CropItemCodeValue/berriesExcludingStrawberries
<http://lpis.ec.europa.eu/registry/applicationschema/cap-iacs-base/code#CropItemCodeValue/berriesExcludingStrawberries> rdf:type owl:NamedIndividual ,
                                                                                                                                 <http://lpis.ec.europa.eu/registry/applicationschema/cap-iacs-base#CropItemCodeValue> ;
                                                                                                                        rdfs:label "Berries (excluding strawberries)"@en ;
                                                                                                                        <http://www.w3.org/2004/02/skos/core#definition> """-- Definition --
||Berries (excluding strawberries).
-- Description --
Cereals and main crops - C
NOTE. Initial value:C2270"""@en ;
                                                                                                                        <http://www.w3.org/2004/02/skos/core#inScheme> :CropItemCodeValue .


###  http://lpis.ec.europa.eu/registry/applicationschema/cap-iacs-base/code#CropItemCodeValue/blackCurrants
<http://lpis.ec.europa.eu/registry/applicationschema/cap-iacs-base/code#CropItemCodeValue/blackCurrants> rdf:type owl:NamedIndividual ,
                                                                                                                  <http://lpis.ec.europa.eu/registry/applicationschema/cap-iacs-base#CropItemCodeValue> ;
                                                                                                         rdfs:label "Black currants"@en ;
                                                                                                         <http://www.w3.org/2004/02/skos/core#definition> """-- Definition --
||||Black currants.
-- Description --
Cereals and main crops - C
NOTE. Initial value:C2272"""@en ;
                                                                                                         <http://www.w3.org/2004/02/skos/core#inScheme> :CropItemCodeValue .


###  http://lpis.ec.europa.eu/registry/applicationschema/cap-iacs-base/code#CropItemCodeValue/brassicas
<http://lpis.ec.europa.eu/registry/applicationschema/cap-iacs-base/code#CropItemCodeValue/brassicas> rdf:type owl:NamedIndividual ,
                                                                                                              <http://lpis.ec.europa.eu/registry/applicationschema/cap-iacs-base#CropItemCodeValue> ;
                                                                                                     rdfs:label "Brassicas"@en ;
                                                                                                     <http://www.w3.org/2004/02/skos/core#definition> """-- Definition --
||Brassicas.
-- Description --
Cereals and main crops - C
NOTE. Initial value:C1610"""@en ;
                                                                                                     <http://www.w3.org/2004/02/skos/core#inScheme> :CropItemCodeValue .


###  http://lpis.ec.europa.eu/registry/applicationschema/cap-iacs-base/code#CropItemCodeValue/broadAndFieldBeansC1335
<http://lpis.ec.europa.eu/registry/applicationschema/cap-iacs-base/code#CropItemCodeValue/broadAndFieldBeansC1335> rdf:type owl:NamedIndividual ,
                                                                                                                            <http://lpis.ec.europa.eu/registry/applicationschema/cap-iacs-base#CropItemCodeValue> ;
                                                                                                                   rdfs:label "Broad and field beans C1335"@en ;
                                                                                                                   <http://www.w3.org/2004/02/skos/core#definition> """-- Definition --
||Broad and field beans C1335.
-- Description --
Cereals and main crops - C
NOTE. Initial value:C1335"""@en ;
                                                                                                                   <http://www.w3.org/2004/02/skos/core#inScheme> :CropItemCodeValue .


###  http://lpis.ec.europa.eu/registry/applicationschema/cap-iacs-base/code#CropItemCodeValue/brusselsSprouts
<http://lpis.ec.europa.eu/registry/applicationschema/cap-iacs-base/code#CropItemCodeValue/brusselsSprouts> rdf:type owl:NamedIndividual ,
                                                                                                                    <http://lpis.ec.europa.eu/registry/applicationschema/cap-iacs-base#CropItemCodeValue> ;
                                                                                                           rdfs:label "Brussels sprouts"@en ;
                                                                                                           <http://www.w3.org/2004/02/skos/core#definition> """-- Definition --
|||Brussels sprouts.
-- Description --
Cereals and main crops - C
NOTE. Initial value:C1631"""@en ;
                                                                                                           <http://www.w3.org/2004/02/skos/core#inScheme> :CropItemCodeValue .


###  http://lpis.ec.europa.eu/registry/applicationschema/cap-iacs-base/code#CropItemCodeValue/buckwheatMilletCanarySeedOtherCereals
<http://lpis.ec.europa.eu/registry/applicationschema/cap-iacs-base/code#CropItemCodeValue/buckwheatMilletCanarySeedOtherCereals> rdf:type owl:NamedIndividual ,
                                                                                                                                          <http://lpis.ec.europa.eu/registry/applicationschema/cap-iacs-base#CropItemCodeValue> ;
                                                                                                                                 rdfs:label "Buckwheat, millet, canary seed (other cereals)"@en ;
                                                                                                                                 <http://www.w3.org/2004/02/skos/core#definition> """-- Definition --
|||Buckwheat, millet, canary seed (other cereals).
-- Description --
Cereals and main crops - C
NOTE. Initial value:C1219"""@en ;
                                                                                                                                 <http://www.w3.org/2004/02/skos/core#inScheme> :CropItemCodeValue .


###  http://lpis.ec.europa.eu/registry/applicationschema/cap-iacs-base/code#CropItemCodeValue/cabbageWhite
<http://lpis.ec.europa.eu/registry/applicationschema/cap-iacs-base/code#CropItemCodeValue/cabbageWhite> rdf:type owl:NamedIndividual ,
                                                                                                                 <http://lpis.ec.europa.eu/registry/applicationschema/cap-iacs-base#CropItemCodeValue> ;
                                                                                                        rdfs:label "Cabbage (white)"@en ;
                                                                                                        <http://www.w3.org/2004/02/skos/core#definition> """-- Definition --
|||Cabbage (white).
-- Description --
Cereals and main crops - C
NOTE. Initial value:C1635"""@en ;
                                                                                                        <http://www.w3.org/2004/02/skos/core#inScheme> :CropItemCodeValue .


###  http://lpis.ec.europa.eu/registry/applicationschema/cap-iacs-base/code#CropItemCodeValue/caraway
<http://lpis.ec.europa.eu/registry/applicationschema/cap-iacs-base/code#CropItemCodeValue/caraway> rdf:type owl:NamedIndividual ,
                                                                                                            <http://lpis.ec.europa.eu/registry/applicationschema/cap-iacs-base#CropItemCodeValue> ;
                                                                                                   rdfs:label "Caraway"@en ;
                                                                                                   <http://www.w3.org/2004/02/skos/core#definition> """-- Definition --
||||Caraway.
-- Description --
Cereals and main crops - C
NOTE. Initial value:C1582"""@en ;
                                                                                                   <http://www.w3.org/2004/02/skos/core#inScheme> :CropItemCodeValue .


###  http://lpis.ec.europa.eu/registry/applicationschema/cap-iacs-base/code#CropItemCodeValue/carrots
<http://lpis.ec.europa.eu/registry/applicationschema/cap-iacs-base/code#CropItemCodeValue/carrots> rdf:type owl:NamedIndividual ,
                                                                                                            <http://lpis.ec.europa.eu/registry/applicationschema/cap-iacs-base#CropItemCodeValue> ;
                                                                                                   rdfs:label "Carrots"@en ;
                                                                                                   <http://www.w3.org/2004/02/skos/core#definition> """-- Definition --
|||Carrots.
-- Description --
Cereals and main crops - C
NOTE. Initial value:C1830"""@en ;
                                                                                                   <http://www.w3.org/2004/02/skos/core#inScheme> :CropItemCodeValue .


###  http://lpis.ec.europa.eu/registry/applicationschema/cap-iacs-base/code#CropItemCodeValue/cauliflowerAndBroccoli
<http://lpis.ec.europa.eu/registry/applicationschema/cap-iacs-base/code#CropItemCodeValue/cauliflowerAndBroccoli> rdf:type owl:NamedIndividual ,
                                                                                                                           <http://lpis.ec.europa.eu/registry/applicationschema/cap-iacs-base#CropItemCodeValue> ;
                                                                                                                  rdfs:label "Cauliflower and broccoli"@en ;
                                                                                                                  <http://www.w3.org/2004/02/skos/core#definition> """-- Definition --
|||Cauliflower and broccoli.
-- Description --
Cereals and main crops - C
NOTE. Initial value:C1620"""@en ;
                                                                                                                  <http://www.w3.org/2004/02/skos/core#inScheme> :CropItemCodeValue .


###  http://lpis.ec.europa.eu/registry/applicationschema/cap-iacs-base/code#CropItemCodeValue/celeriac
<http://lpis.ec.europa.eu/registry/applicationschema/cap-iacs-base/code#CropItemCodeValue/celeriac> rdf:type owl:NamedIndividual ,
                                                                                                             <http://lpis.ec.europa.eu/registry/applicationschema/cap-iacs-base#CropItemCodeValue> ;
                                                                                                    rdfs:label "Celeriac"@en ;
                                                                                                    <http://www.w3.org/2004/02/skos/core#definition> """-- Definition --
|||Celeriac.
-- Description --
Cereals and main crops - C
NOTE. Initial value:C1872"""@en ;
                                                                                                    <http://www.w3.org/2004/02/skos/core#inScheme> :CropItemCodeValue .


###  http://lpis.ec.europa.eu/registry/applicationschema/cap-iacs-base/code#CropItemCodeValue/celery
<http://lpis.ec.europa.eu/registry/applicationschema/cap-iacs-base/code#CropItemCodeValue/celery> rdf:type owl:NamedIndividual ,
                                                                                                           <http://lpis.ec.europa.eu/registry/applicationschema/cap-iacs-base#CropItemCodeValue> ;
                                                                                                  rdfs:label "Celery"@en ;
                                                                                                  <http://www.w3.org/2004/02/skos/core#definition> """-- Definition --
|||Celery.
-- Description --
Cereals and main crops - C
NOTE. Initial value:C1672"""@en ;
                                                                                                  <http://www.w3.org/2004/02/skos/core#inScheme> :CropItemCodeValue .


###  http://lpis.ec.europa.eu/registry/applicationschema/cap-iacs-base/code#CropItemCodeValue/cerealsExcludingRice
<http://lpis.ec.europa.eu/registry/applicationschema/cap-iacs-base/code#CropItemCodeValue/cerealsExcludingRice> rdf:type owl:NamedIndividual ,
                                                                                                                         <http://lpis.ec.europa.eu/registry/applicationschema/cap-iacs-base#CropItemCodeValue> ;
                                                                                                                rdfs:label "Cereals (excluding rice) "@en ;
                                                                                                                <http://www.w3.org/2004/02/skos/core#definition> """-- Definition --
||Cereals (excluding rice) .
-- Description --
Cereals and main crops - C
NOTE. Initial value: C1050"""@en ;
                                                                                                                <http://www.w3.org/2004/02/skos/core#inScheme> :CropItemCodeValue .


###  http://lpis.ec.europa.eu/registry/applicationschema/cap-iacs-base/code#CropItemCodeValue/cerealsForTheProductionOfGrainIncludingRiceAndSeed
<http://lpis.ec.europa.eu/registry/applicationschema/cap-iacs-base/code#CropItemCodeValue/cerealsForTheProductionOfGrainIncludingRiceAndSeed> rdf:type owl:NamedIndividual ,
                                                                                                                                                       <http://lpis.ec.europa.eu/registry/applicationschema/cap-iacs-base#CropItemCodeValue> ;
                                                                                                                                              rdfs:label "Cereals for the production of grain (including rice and seed)"@en ;
                                                                                                                                              <http://www.w3.org/2004/02/skos/core#definition> """-- Definition --
|Cereals for the production of grain (including rice and seed).
-- Description --
Cereals and main crops - C
NOTE. Initial value:C1040"""@en ;
                                                                                                                                              <http://www.w3.org/2004/02/skos/core#inScheme> :CropItemCodeValue .


###  http://lpis.ec.europa.eu/registry/applicationschema/cap-iacs-base/code#CropItemCodeValue/cerealsForTheProductionOfGrainIncludingSeedButExcludingRice
<http://lpis.ec.europa.eu/registry/applicationschema/cap-iacs-base/code#CropItemCodeValue/cerealsForTheProductionOfGrainIncludingSeedButExcludingRice> rdf:type owl:NamedIndividual ,
                                                                                                                                                                <http://lpis.ec.europa.eu/registry/applicationschema/cap-iacs-base#CropItemCodeValue> ;
                                                                                                                                                       rdfs:label "Cereals for the production of grain (including seed but excluding rice)"@en ;
                                                                                                                                                       <http://www.w3.org/2004/02/skos/core#definition> """-- Definition --
|||Cereals for the production of grain (including seed but excluding rice).
-- Description --
Land use of Agriculture Area in Use -L
NOTE. Initial value:L1050"""@en ;
                                                                                                                                                       <http://www.w3.org/2004/02/skos/core#inScheme> :CropItemCodeValue .


###  http://lpis.ec.europa.eu/registry/applicationschema/cap-iacs-base/code#CropItemCodeValue/cerealsHarvestedGreen
<http://lpis.ec.europa.eu/registry/applicationschema/cap-iacs-base/code#CropItemCodeValue/cerealsHarvestedGreen> rdf:type owl:NamedIndividual ,
                                                                                                                          <http://lpis.ec.europa.eu/registry/applicationschema/cap-iacs-base#CropItemCodeValue> ;
                                                                                                                 rdfs:label "Cereals harvested green"@en ;
                                                                                                                 <http://www.w3.org/2004/02/skos/core#definition> """-- Definition --
|||Cereals harvested green.
-- Description --
Cereals and main crops - C
NOTE. Initial value:C2626"""@en ;
                                                                                                                 <http://www.w3.org/2004/02/skos/core#inScheme> :CropItemCodeValue .


###  http://lpis.ec.europa.eu/registry/applicationschema/cap-iacs-base/code#CropItemCodeValue/cherries
<http://lpis.ec.europa.eu/registry/applicationschema/cap-iacs-base/code#CropItemCodeValue/cherries> rdf:type owl:NamedIndividual ,
                                                                                                             <http://lpis.ec.europa.eu/registry/applicationschema/cap-iacs-base#CropItemCodeValue> ;
                                                                                                    rdfs:label "Cherries"@en ;
                                                                                                    <http://www.w3.org/2004/02/skos/core#definition> """-- Definition --
|||Cherries.
-- Description --
Cereals and main crops - C
NOTE. Initial value:C2200"""@en ;
                                                                                                    <http://www.w3.org/2004/02/skos/core#inScheme> :CropItemCodeValue .


###  http://lpis.ec.europa.eu/registry/applicationschema/cap-iacs-base/code#CropItemCodeValue/chestnuts
<http://lpis.ec.europa.eu/registry/applicationschema/cap-iacs-base/code#CropItemCodeValue/chestnuts> rdf:type owl:NamedIndividual ,
                                                                                                              <http://lpis.ec.europa.eu/registry/applicationschema/cap-iacs-base#CropItemCodeValue> ;
                                                                                                     rdfs:label "Chestnuts"@en ;
                                                                                                     <http://www.w3.org/2004/02/skos/core#definition> """-- Definition --
|||Chestnuts.
-- Description --
Cereals and main crops - C
NOTE. Initial value:C2236"""@en ;
                                                                                                     <http://www.w3.org/2004/02/skos/core#inScheme> :CropItemCodeValue .


###  http://lpis.ec.europa.eu/registry/applicationschema/cap-iacs-base/code#CropItemCodeValue/chicory
<http://lpis.ec.europa.eu/registry/applicationschema/cap-iacs-base/code#CropItemCodeValue/chicory> rdf:type owl:NamedIndividual ,
                                                                                                            <http://lpis.ec.europa.eu/registry/applicationschema/cap-iacs-base#CropItemCodeValue> ;
                                                                                                   rdfs:label "Chicory"@en ;
                                                                                                   <http://www.w3.org/2004/02/skos/core#definition> """-- Definition --
|||Chicory.
-- Description --
Cereals and main crops - C
NOTE. Initial value:C1571"""@en ;
                                                                                                   <http://www.w3.org/2004/02/skos/core#inScheme> :CropItemCodeValue .


###  http://lpis.ec.europa.eu/registry/applicationschema/cap-iacs-base/code#CropItemCodeValue/chicoryC1710
<http://lpis.ec.europa.eu/registry/applicationschema/cap-iacs-base/code#CropItemCodeValue/chicoryC1710> rdf:type owl:NamedIndividual ,
                                                                                                                 <http://lpis.ec.europa.eu/registry/applicationschema/cap-iacs-base#CropItemCodeValue> ;
                                                                                                        rdfs:label "Chicory C1710"@en ;
                                                                                                        <http://www.w3.org/2004/02/skos/core#definition> """-- Definition --
|||Chicory C1710.
-- Description --
Cereals and main crops - C
NOTE. Initial value:C1710"""@en ;
                                                                                                        <http://www.w3.org/2004/02/skos/core#inScheme> :CropItemCodeValue .


###  http://lpis.ec.europa.eu/registry/applicationschema/cap-iacs-base/code#CropItemCodeValue/chicoryForInulin
<http://lpis.ec.europa.eu/registry/applicationschema/cap-iacs-base/code#CropItemCodeValue/chicoryForInulin> rdf:type owl:NamedIndividual ,
                                                                                                                     <http://lpis.ec.europa.eu/registry/applicationschema/cap-iacs-base#CropItemCodeValue> ;
                                                                                                            rdfs:label "Chicory for inulin"@en ;
                                                                                                            <http://www.w3.org/2004/02/skos/core#definition> """-- Definition --
||||Chicory for inulin.
-- Description --
Cereals and main crops - C
NOTE. Initial value:C1572"""@en ;
                                                                                                            <http://www.w3.org/2004/02/skos/core#inScheme> :CropItemCodeValue .


###  http://lpis.ec.europa.eu/registry/applicationschema/cap-iacs-base/code#CropItemCodeValue/citrusFruitsC2300
<http://lpis.ec.europa.eu/registry/applicationschema/cap-iacs-base/code#CropItemCodeValue/citrusFruitsC2300> rdf:type owl:NamedIndividual ,
                                                                                                                      <http://lpis.ec.europa.eu/registry/applicationschema/cap-iacs-base#CropItemCodeValue> ;
                                                                                                             rdfs:label "Citrus fruits C2300"@en ;
                                                                                                             <http://www.w3.org/2004/02/skos/core#definition> """-- Definition --
||Citrus fruits C2300.
-- Description --
Cereals and main crops - C
NOTE. Initial value:C2300"""@en ;
                                                                                                             <http://www.w3.org/2004/02/skos/core#inScheme> :CropItemCodeValue .


###  http://lpis.ec.europa.eu/registry/applicationschema/cap-iacs-base/code#CropItemCodeValue/citrusPlantations
<http://lpis.ec.europa.eu/registry/applicationschema/cap-iacs-base/code#CropItemCodeValue/citrusPlantations> rdf:type owl:NamedIndividual ,
                                                                                                                      <http://lpis.ec.europa.eu/registry/applicationschema/cap-iacs-base#CropItemCodeValue> ;
                                                                                                             rdfs:label "Citrus plantations"@en ;
                                                                                                             <http://www.w3.org/2004/02/skos/core#definition> """-- Definition --
||||Citrus plantations.
-- Description --
Land use of Agriculture Area in Use -L
NOTE. Initial value:L2300"""@en ;
                                                                                                             <http://www.w3.org/2004/02/skos/core#inScheme> :CropItemCodeValue .


###  http://lpis.ec.europa.eu/registry/applicationschema/cap-iacs-base/code#CropItemCodeValue/clementines
<http://lpis.ec.europa.eu/registry/applicationschema/cap-iacs-base/code#CropItemCodeValue/clementines> rdf:type owl:NamedIndividual ,
                                                                                                                <http://lpis.ec.europa.eu/registry/applicationschema/cap-iacs-base#CropItemCodeValue> ;
                                                                                                       rdfs:label "Clementines"@en ;
                                                                                                       <http://www.w3.org/2004/02/skos/core#definition> """-- Definition --
||||Clementines.
-- Description --
Cereals and main crops - C
NOTE. Initial value:C2360"""@en ;
                                                                                                       <http://www.w3.org/2004/02/skos/core#inScheme> :CropItemCodeValue .


###  http://lpis.ec.europa.eu/registry/applicationschema/cap-iacs-base/code#CropItemCodeValue/cloverAndMixtures
<http://lpis.ec.europa.eu/registry/applicationschema/cap-iacs-base/code#CropItemCodeValue/cloverAndMixtures> rdf:type owl:NamedIndividual ,
                                                                                                                      <http://lpis.ec.europa.eu/registry/applicationschema/cap-iacs-base#CropItemCodeValue> ;
                                                                                                             rdfs:label "Clover and mixtures"@en ;
                                                                                                             <http://www.w3.org/2004/02/skos/core#definition> """-- Definition --
|||Clover and mixtures.
-- Description --
Cereals and main crops - C
NOTE. Initial value:C2671"""@en ;
                                                                                                             <http://www.w3.org/2004/02/skos/core#inScheme> :CropItemCodeValue .


###  http://lpis.ec.europa.eu/registry/applicationschema/cap-iacs-base/code#CropItemCodeValue/commonSpringWheat
<http://lpis.ec.europa.eu/registry/applicationschema/cap-iacs-base/code#CropItemCodeValue/commonSpringWheat> rdf:type owl:NamedIndividual ,
                                                                                                                      <http://lpis.ec.europa.eu/registry/applicationschema/cap-iacs-base#CropItemCodeValue> ;
                                                                                                             rdfs:label "Common spring wheat"@en ;
                                                                                                             <http://www.w3.org/2004/02/skos/core#definition> """-- Definition --
|||||Common spring wheat.
-- Description --
Cereals and main crops - C
NOTE. Initial value:C1124"""@en ;
                                                                                                             <http://www.w3.org/2004/02/skos/core#inScheme> :CropItemCodeValue .


###  http://lpis.ec.europa.eu/registry/applicationschema/cap-iacs-base/code#CropItemCodeValue/commonWheatAndSpelt
<http://lpis.ec.europa.eu/registry/applicationschema/cap-iacs-base/code#CropItemCodeValue/commonWheatAndSpelt> rdf:type owl:NamedIndividual ,
                                                                                                                        <http://lpis.ec.europa.eu/registry/applicationschema/cap-iacs-base#CropItemCodeValue> ;
                                                                                                               rdfs:label "Common wheat and spelt"@en ;
                                                                                                               <http://www.w3.org/2004/02/skos/core#definition> """-- Definition --
||||Common wheat and spelt.
-- Description --
Cereals and main crops - C
NOTE. Initial value:C1120"""@en ;
                                                                                                               <http://www.w3.org/2004/02/skos/core#inScheme> :CropItemCodeValue .


###  http://lpis.ec.europa.eu/registry/applicationschema/cap-iacs-base/code#CropItemCodeValue/commonWinterWheat
<http://lpis.ec.europa.eu/registry/applicationschema/cap-iacs-base/code#CropItemCodeValue/commonWinterWheat> rdf:type owl:NamedIndividual ,
                                                                                                                      <http://lpis.ec.europa.eu/registry/applicationschema/cap-iacs-base#CropItemCodeValue> ;
                                                                                                             rdfs:label "Common winter wheat"@en ;
                                                                                                             <http://www.w3.org/2004/02/skos/core#definition> """-- Definition --
|||||Common winter wheat.
-- Description --
Cereals and main crops - C
NOTE. Initial value:C1123"""@en ;
                                                                                                             <http://www.w3.org/2004/02/skos/core#inScheme> :CropItemCodeValue .


###  http://lpis.ec.europa.eu/registry/applicationschema/cap-iacs-base/code#CropItemCodeValue/cornCobMixC1200
<http://lpis.ec.europa.eu/registry/applicationschema/cap-iacs-base/code#CropItemCodeValue/cornCobMixC1200> rdf:type owl:NamedIndividual ,
                                                                                                                    <http://lpis.ec.europa.eu/registry/applicationschema/cap-iacs-base#CropItemCodeValue> ;
                                                                                                           rdfs:label "Corn cob mix C1200"@en ;
                                                                                                           <http://www.w3.org/2004/02/skos/core#definition> """-- Definition --
||||Corn cob mix C1200.
-- Description --
Cereals and main crops - C
NOTE. Initial value:C1202"""@en ;
                                                                                                           <http://www.w3.org/2004/02/skos/core#inScheme> :CropItemCodeValue .


###  http://lpis.ec.europa.eu/registry/applicationschema/cap-iacs-base/code#CropItemCodeValue/cottonFibre
<http://lpis.ec.europa.eu/registry/applicationschema/cap-iacs-base/code#CropItemCodeValue/cottonFibre> rdf:type owl:NamedIndividual ,
                                                                                                                <http://lpis.ec.europa.eu/registry/applicationschema/cap-iacs-base#CropItemCodeValue> ;
                                                                                                       rdfs:label "Cotton fibre "@en ;
                                                                                                       <http://www.w3.org/2004/02/skos/core#definition> """-- Definition --
|||Cotton fibre.
-- Description --
Cereals and main crops - C
NOTE. Initial value:C1540"""@en ;
                                                                                                       <http://www.w3.org/2004/02/skos/core#inScheme> :CropItemCodeValue .


###  http://lpis.ec.europa.eu/registry/applicationschema/cap-iacs-base/code#CropItemCodeValue/cottonSeed
<http://lpis.ec.europa.eu/registry/applicationschema/cap-iacs-base/code#CropItemCodeValue/cottonSeed> rdf:type owl:NamedIndividual ,
                                                                                                               <http://lpis.ec.europa.eu/registry/applicationschema/cap-iacs-base#CropItemCodeValue> ;
                                                                                                      rdfs:label "Cotton seed"@en ;
                                                                                                      <http://www.w3.org/2004/02/skos/core#definition> """-- Definition --
||||Cotton seed.
-- Description --
Cereals and main crops - C
NOTE. Initial value:C1490"""@en ;
                                                                                                      <http://www.w3.org/2004/02/skos/core#inScheme> :CropItemCodeValue .


###  http://lpis.ec.europa.eu/registry/applicationschema/cap-iacs-base/code#CropItemCodeValue/courgettes
<http://lpis.ec.europa.eu/registry/applicationschema/cap-iacs-base/code#CropItemCodeValue/courgettes> rdf:type owl:NamedIndividual ,
                                                                                                               <http://lpis.ec.europa.eu/registry/applicationschema/cap-iacs-base#CropItemCodeValue> ;
                                                                                                      rdfs:label "Courgettes"@en ;
                                                                                                      <http://www.w3.org/2004/02/skos/core#definition> """-- Definition --
||||Courgettes.
-- Description --
Cereals and main crops - C
NOTE. Initial value:C1787"""@en ;
                                                                                                      <http://www.w3.org/2004/02/skos/core#inScheme> :CropItemCodeValue .


###  http://lpis.ec.europa.eu/registry/applicationschema/cap-iacs-base/code#CropItemCodeValue/cropProductionUnderGlassOrHighAccessibleCover
<http://lpis.ec.europa.eu/registry/applicationschema/cap-iacs-base/code#CropItemCodeValue/cropProductionUnderGlassOrHighAccessibleCover> rdf:type owl:NamedIndividual ,
                                                                                                                                                  <http://lpis.ec.europa.eu/registry/applicationschema/cap-iacs-base#CropItemCodeValue> ;
                                                                                                                                         rdfs:label "Crop production under glass or high accessible cover"@en ;
                                                                                                                                         <http://www.w3.org/2004/02/skos/core#definition> """-- Definition --
Crop production under glass or high accessible cover.
-- Description --
Land use of Agriculture Area in Use -L. Special aggregates
NOTE. Initial value:L0900"""@en ;
                                                                                                                                         <http://www.w3.org/2004/02/skos/core#inScheme> :CropItemCodeValue .


###  http://lpis.ec.europa.eu/registry/applicationschema/cap-iacs-base/code#CropItemCodeValue/cucumbers
<http://lpis.ec.europa.eu/registry/applicationschema/cap-iacs-base/code#CropItemCodeValue/cucumbers> rdf:type owl:NamedIndividual ,
                                                                                                              <http://lpis.ec.europa.eu/registry/applicationschema/cap-iacs-base#CropItemCodeValue> ;
                                                                                                     rdfs:label "Cucumbers"@en ;
                                                                                                     <http://www.w3.org/2004/02/skos/core#definition> """-- Definition --
|||Cucumbers.
-- Description --
Cereals and main crops - C
NOTE. Initial value:C1761"""@en ;
                                                                                                     <http://www.w3.org/2004/02/skos/core#inScheme> :CropItemCodeValue .


###  http://lpis.ec.europa.eu/registry/applicationschema/cap-iacs-base/code#CropItemCodeValue/cucumbersUnderGlassOrHighAccessibleCoverC1762
<http://lpis.ec.europa.eu/registry/applicationschema/cap-iacs-base/code#CropItemCodeValue/cucumbersUnderGlassOrHighAccessibleCoverC1762> rdf:type owl:NamedIndividual ,
                                                                                                                                                  <http://lpis.ec.europa.eu/registry/applicationschema/cap-iacs-base#CropItemCodeValue> ;
                                                                                                                                         rdfs:label "Cucumbers under glass or high accessible cover C1762 "@en ;
                                                                                                                                         <http://www.w3.org/2004/02/skos/core#definition> """-- Definition --
||||Cucumbers under glass or high accessible cover C1762.
-- Description --
Cereals and main crops - C
NOTE. Initial value:C1762"""@en ;
                                                                                                                                         <http://www.w3.org/2004/02/skos/core#inScheme> :CropItemCodeValue .


###  http://lpis.ec.europa.eu/registry/applicationschema/cap-iacs-base/code#CropItemCodeValue/cultivatedMushrooms
<http://lpis.ec.europa.eu/registry/applicationschema/cap-iacs-base/code#CropItemCodeValue/cultivatedMushrooms> rdf:type owl:NamedIndividual ,
                                                                                                                        <http://lpis.ec.europa.eu/registry/applicationschema/cap-iacs-base#CropItemCodeValue> ;
                                                                                                               rdfs:label "Cultivated mushrooms"@en ;
                                                                                                               <http://www.w3.org/2004/02/skos/core#definition> """-- Definition --
|Cultivated mushrooms.
-- Description --
Cereals and main crops - C
NOTE. Initial value:C1910"""@en ;
                                                                                                               <http://www.w3.org/2004/02/skos/core#inScheme> :CropItemCodeValue .


###  http://lpis.ec.europa.eu/registry/applicationschema/cap-iacs-base/code#CropItemCodeValue/currants
<http://lpis.ec.europa.eu/registry/applicationschema/cap-iacs-base/code#CropItemCodeValue/currants> rdf:type owl:NamedIndividual ,
                                                                                                             <http://lpis.ec.europa.eu/registry/applicationschema/cap-iacs-base#CropItemCodeValue> ;
                                                                                                    rdfs:label "Currants"@en ;
                                                                                                    <http://www.w3.org/2004/02/skos/core#definition> """-- Definition --
|||Currants.
-- Description --
Cereals and main crops - C
NOTE. Initial value:C2271"""@en ;
                                                                                                    <http://www.w3.org/2004/02/skos/core#inScheme> :CropItemCodeValue .


###  http://lpis.ec.europa.eu/registry/applicationschema/cap-iacs-base/code#CropItemCodeValue/driedPulsesAndProteinCropsForTheProductionOfGrainIncludingSeedAndMixturesOfCerealsAndPulses
<http://lpis.ec.europa.eu/registry/applicationschema/cap-iacs-base/code#CropItemCodeValue/driedPulsesAndProteinCropsForTheProductionOfGrainIncludingSeedAndMixturesOfCerealsAndPulses> rdf:type owl:NamedIndividual ,
                                                                                                                                                                                                <http://lpis.ec.europa.eu/registry/applicationschema/cap-iacs-base#CropItemCodeValue> ;
                                                                                                                                                                                       rdfs:label "Dried pulses and protein crops for the production of grain (including seed and mixtures of cereals and pulses)"@en ;
                                                                                                                                                                                       <http://www.w3.org/2004/02/skos/core#definition> """-- Definition --
|||Dried pulses and protein crops for the production of grain (including seed and mixtures of cereals and pulses).
-- Description --
Land use of Agriculture Area in Use -L
NOTE. Initial value:L1300"""@en ;
                                                                                                                                                                                       <http://www.w3.org/2004/02/skos/core#inScheme> :CropItemCodeValue .


###  http://lpis.ec.europa.eu/registry/applicationschema/cap-iacs-base/code#CropItemCodeValue/driedPulsesAndProteinCropsForTheProductionOfGrainIncludingSeedAndMixturesOfCerealsAndPulsesC1300
<http://lpis.ec.europa.eu/registry/applicationschema/cap-iacs-base/code#CropItemCodeValue/driedPulsesAndProteinCropsForTheProductionOfGrainIncludingSeedAndMixturesOfCerealsAndPulsesC1300> rdf:type owl:NamedIndividual ,
                                                                                                                                                                                                     <http://lpis.ec.europa.eu/registry/applicationschema/cap-iacs-base#CropItemCodeValue> ;
                                                                                                                                                                                            rdfs:label "Dried pulses and protein crops for the production of grain (including seed and mixtures of cereals and pulses) C1300"@en ;
                                                                                                                                                                                            <http://www.w3.org/2004/02/skos/core#definition> """-- Definition --
|Dried pulses and protein crops for the production of grain (including seed and mixtures of cereals and pulses) C1300.
-- Description --
Cereals and main crops - C
NOTE. Initial value:C1300"""@en ;
                                                                                                                                                                                            <http://www.w3.org/2004/02/skos/core#inScheme> :CropItemCodeValue .


###  http://lpis.ec.europa.eu/registry/applicationschema/cap-iacs-base/code#CropItemCodeValue/durumWheat
<http://lpis.ec.europa.eu/registry/applicationschema/cap-iacs-base/code#CropItemCodeValue/durumWheat> rdf:type owl:NamedIndividual ,
                                                                                                               <http://lpis.ec.europa.eu/registry/applicationschema/cap-iacs-base#CropItemCodeValue> ;
                                                                                                      rdfs:label "Durum wheat"@en ;
                                                                                                      <http://www.w3.org/2004/02/skos/core#definition> """-- Definition --
||||Durum wheat.
-- Description --
Cereals and main crops - C
NOTE. Initial value:C1130"""@en ;
                                                                                                      <http://www.w3.org/2004/02/skos/core#inScheme> :CropItemCodeValue .


###  http://lpis.ec.europa.eu/registry/applicationschema/cap-iacs-base/code#CropItemCodeValue/earlyPotatoes
<http://lpis.ec.europa.eu/registry/applicationschema/cap-iacs-base/code#CropItemCodeValue/earlyPotatoes> rdf:type owl:NamedIndividual ,
                                                                                                                  <http://lpis.ec.europa.eu/registry/applicationschema/cap-iacs-base#CropItemCodeValue> ;
                                                                                                         rdfs:label "Early potatoes"@en ;
                                                                                                         <http://www.w3.org/2004/02/skos/core#definition> """-- Definition --
|||Early potatoes.
-- Description --
Cereals and main crops - C
NOTE. Initial value:C1362"""@en ;
                                                                                                         <http://www.w3.org/2004/02/skos/core#inScheme> :CropItemCodeValue .


###  http://lpis.ec.europa.eu/registry/applicationschema/cap-iacs-base/code#CropItemCodeValue/eggplants
<http://lpis.ec.europa.eu/registry/applicationschema/cap-iacs-base/code#CropItemCodeValue/eggplants> rdf:type owl:NamedIndividual ,
                                                                                                              <http://lpis.ec.europa.eu/registry/applicationschema/cap-iacs-base#CropItemCodeValue> ;
                                                                                                     rdfs:label "Eggplants"@en ;
                                                                                                     <http://www.w3.org/2004/02/skos/core#definition> """-- Definition --
||||Eggplants.
-- Description --
Cereals and main crops - C
NOTE. Initial value:C1781"""@en ;
                                                                                                     <http://www.w3.org/2004/02/skos/core#inScheme> :CropItemCodeValue .


###  http://lpis.ec.europa.eu/registry/applicationschema/cap-iacs-base/code#CropItemCodeValue/eggplantsGourdsMarrowsCourgettesPumpkins
<http://lpis.ec.europa.eu/registry/applicationschema/cap-iacs-base/code#CropItemCodeValue/eggplantsGourdsMarrowsCourgettesPumpkins> rdf:type owl:NamedIndividual ,
                                                                                                                                             <http://lpis.ec.europa.eu/registry/applicationschema/cap-iacs-base#CropItemCodeValue> ;
                                                                                                                                    rdfs:label "Eggplants, gourds, marrows, courgettes, pumpkins"@en ;
                                                                                                                                    <http://www.w3.org/2004/02/skos/core#definition> """-- Definition --
|||Eggplants, gourds, marrows, courgettes, pumpkins.
-- Description --
Cereals and main crops - C
NOTE. Initial value:C1780"""@en ;
                                                                                                                                    <http://www.w3.org/2004/02/skos/core#inScheme> :CropItemCodeValue .


###  http://lpis.ec.europa.eu/registry/applicationschema/cap-iacs-base/code#CropItemCodeValue/endives
<http://lpis.ec.europa.eu/registry/applicationschema/cap-iacs-base/code#CropItemCodeValue/endives> rdf:type owl:NamedIndividual ,
                                                                                                            <http://lpis.ec.europa.eu/registry/applicationschema/cap-iacs-base#CropItemCodeValue> ;
                                                                                                   rdfs:label "Endives"@en ;
                                                                                                   <http://www.w3.org/2004/02/skos/core#definition> """-- Definition --
|||Endives.
-- Description --
Cereals and main crops - C
NOTE. Initial value:C1685"""@en ;
                                                                                                   <http://www.w3.org/2004/02/skos/core#inScheme> :CropItemCodeValue .


###  http://lpis.ec.europa.eu/registry/applicationschema/cap-iacs-base/code#CropItemCodeValue/energyCrops
<http://lpis.ec.europa.eu/registry/applicationschema/cap-iacs-base/code#CropItemCodeValue/energyCrops> rdf:type owl:NamedIndividual ,
                                                                                                                <http://lpis.ec.europa.eu/registry/applicationschema/cap-iacs-base#CropItemCodeValue> ;
                                                                                                       rdfs:label "Energy crops"@en ;
                                                                                                       <http://www.w3.org/2004/02/skos/core#definition> """-- Definition --
|Energy crops.
-- Description --
Cereals and main crops - C
NOTE. Initial value:C1590"""@en ;
                                                                                                       <http://www.w3.org/2004/02/skos/core#inScheme> :CropItemCodeValue .


###  http://lpis.ec.europa.eu/registry/applicationschema/cap-iacs-base/code#CropItemCodeValue/fallowLand
<http://lpis.ec.europa.eu/registry/applicationschema/cap-iacs-base/code#CropItemCodeValue/fallowLand> rdf:type owl:NamedIndividual ,
                                                                                                               <http://lpis.ec.europa.eu/registry/applicationschema/cap-iacs-base#CropItemCodeValue> ;
                                                                                                      rdfs:label "Fallow land"@en ;
                                                                                                      <http://www.w3.org/2004/02/skos/core#definition> """-- Definition --
|||Fallow land.
-- Description --
Land use of Agriculture Area in Use -L
NOTE. Initial value:L2696"""@en ;
                                                                                                      <http://www.w3.org/2004/02/skos/core#inScheme> :CropItemCodeValue .


###  http://lpis.ec.europa.eu/registry/applicationschema/cap-iacs-base/code#CropItemCodeValue/fibreCrops
<http://lpis.ec.europa.eu/registry/applicationschema/cap-iacs-base/code#CropItemCodeValue/fibreCrops> rdf:type owl:NamedIndividual ,
                                                                                                               <http://lpis.ec.europa.eu/registry/applicationschema/cap-iacs-base#CropItemCodeValue> ;
                                                                                                      rdfs:label "Fibre crops"@en ;
                                                                                                      <http://www.w3.org/2004/02/skos/core#definition> """-- Definition --
||Fibre crops.
-- Description --
Cereals and main crops - C
NOTE. Initial value:C1500"""@en ;
                                                                                                      <http://www.w3.org/2004/02/skos/core#inScheme> :CropItemCodeValue .


###  http://lpis.ec.europa.eu/registry/applicationschema/cap-iacs-base/code#CropItemCodeValue/fibreFlax
<http://lpis.ec.europa.eu/registry/applicationschema/cap-iacs-base/code#CropItemCodeValue/fibreFlax> rdf:type owl:NamedIndividual ,
                                                                                                              <http://lpis.ec.europa.eu/registry/applicationschema/cap-iacs-base#CropItemCodeValue> ;
                                                                                                     rdfs:label "Fibre flax"@en ;
                                                                                                     <http://www.w3.org/2004/02/skos/core#definition> """-- Definition --
|||Fibre flax.
-- Description --
Cereals and main crops - C
NOTE. Initial value:C1520"""@en ;
                                                                                                     <http://www.w3.org/2004/02/skos/core#inScheme> :CropItemCodeValue .


###  http://lpis.ec.europa.eu/registry/applicationschema/cap-iacs-base/code#CropItemCodeValue/fieldPeas
<http://lpis.ec.europa.eu/registry/applicationschema/cap-iacs-base/code#CropItemCodeValue/fieldPeas> rdf:type owl:NamedIndividual ,
                                                                                                              <http://lpis.ec.europa.eu/registry/applicationschema/cap-iacs-base#CropItemCodeValue> ;
                                                                                                     rdfs:label "Field peas"@en ;
                                                                                                     <http://www.w3.org/2004/02/skos/core#definition> """-- Definition --
||Field peas.
-- Description --
Cereals and main crops - C
NOTE. Initial value:C1320"""@en ;
                                                                                                     <http://www.w3.org/2004/02/skos/core#inScheme> :CropItemCodeValue .


###  http://lpis.ec.europa.eu/registry/applicationschema/cap-iacs-base/code#CropItemCodeValue/figs
<http://lpis.ec.europa.eu/registry/applicationschema/cap-iacs-base/code#CropItemCodeValue/figs> rdf:type owl:NamedIndividual ,
                                                                                                         <http://lpis.ec.europa.eu/registry/applicationschema/cap-iacs-base#CropItemCodeValue> ;
                                                                                                rdfs:label "Figs"@en ;
                                                                                                <http://www.w3.org/2004/02/skos/core#definition> """-- Definition --
|||Figs.
-- Description --
Cereals and main crops - C
NOTE. Initial value:C2251"""@en ;
                                                                                                <http://www.w3.org/2004/02/skos/core#inScheme> :CropItemCodeValue .


###  http://lpis.ec.europa.eu/registry/applicationschema/cap-iacs-base/code#CropItemCodeValue/flowersAndOrnamentalPlantsExcludingNurseries
<http://lpis.ec.europa.eu/registry/applicationschema/cap-iacs-base/code#CropItemCodeValue/flowersAndOrnamentalPlantsExcludingNurseries> rdf:type owl:NamedIndividual ,
                                                                                                                                                 <http://lpis.ec.europa.eu/registry/applicationschema/cap-iacs-base#CropItemCodeValue> ;
                                                                                                                                        rdfs:label "Flowers and ornamental plants (excluding nurseries)"@en ;
                                                                                                                                        <http://www.w3.org/2004/02/skos/core#definition> """-- Definition --
|||Flowers and ornamental plants (excluding nurseries).
-- Description --
Land use of Agriculture Area in Use -L
NOTE. Initial value:L3001"""@en ;
                                                                                                                                        <http://www.w3.org/2004/02/skos/core#inScheme> :CropItemCodeValue .


###  http://lpis.ec.europa.eu/registry/applicationschema/cap-iacs-base/code#CropItemCodeValue/flowersAndOrnamentalPlantsUnderGlassHighAccessibleCover
<http://lpis.ec.europa.eu/registry/applicationschema/cap-iacs-base/code#CropItemCodeValue/flowersAndOrnamentalPlantsUnderGlassHighAccessibleCover> rdf:type owl:NamedIndividual ,
                                                                                                                                                            <http://lpis.ec.europa.eu/registry/applicationschema/cap-iacs-base#CropItemCodeValue> ;
                                                                                                                                                   rdfs:label "Flowers and ornamental plants under glass high accessible cover"@en ;
                                                                                                                                                   <http://www.w3.org/2004/02/skos/core#definition> """-- Definition --
Flowers and ornamental plants under glass high accessible cover.
-- Description --
Land use of Agriculture Area in Use -L. Special aggregates
NOTE. Initial value:L1113"""@en ;
                                                                                                                                                   <http://www.w3.org/2004/02/skos/core#inScheme> :CropItemCodeValue .


###  http://lpis.ec.europa.eu/registry/applicationschema/cap-iacs-base/code#CropItemCodeValue/fruitAndBerryPlantations
<http://lpis.ec.europa.eu/registry/applicationschema/cap-iacs-base/code#CropItemCodeValue/fruitAndBerryPlantations> rdf:type owl:NamedIndividual ,
                                                                                                                             <http://lpis.ec.europa.eu/registry/applicationschema/cap-iacs-base#CropItemCodeValue> ;
                                                                                                                    rdfs:label "Fruit and berry plantations"@en ;
                                                                                                                    <http://www.w3.org/2004/02/skos/core#definition> """-- Definition --
|||Fruit and berry plantations.
-- Description --
Land use of Agriculture Area in Use -L
NOTE. Initial value:L0011"""@en ;
                                                                                                                    <http://www.w3.org/2004/02/skos/core#inScheme> :CropItemCodeValue .


###  http://lpis.ec.europa.eu/registry/applicationschema/cap-iacs-base/code#CropItemCodeValue/garlic
<http://lpis.ec.europa.eu/registry/applicationschema/cap-iacs-base/code#CropItemCodeValue/garlic> rdf:type owl:NamedIndividual ,
                                                                                                           <http://lpis.ec.europa.eu/registry/applicationschema/cap-iacs-base#CropItemCodeValue> ;
                                                                                                  rdfs:label "Garlic"@en ;
                                                                                                  <http://www.w3.org/2004/02/skos/core#definition> """-- Definition --
|||Garlic.
-- Description --
Cereals and main crops - C
NOTE. Initial value:C1840"""@en ;
                                                                                                  <http://www.w3.org/2004/02/skos/core#inScheme> :CropItemCodeValue .


###  http://lpis.ec.europa.eu/registry/applicationschema/cap-iacs-base/code#CropItemCodeValue/gherkins
<http://lpis.ec.europa.eu/registry/applicationschema/cap-iacs-base/code#CropItemCodeValue/gherkins> rdf:type owl:NamedIndividual ,
                                                                                                             <http://lpis.ec.europa.eu/registry/applicationschema/cap-iacs-base#CropItemCodeValue> ;
                                                                                                    rdfs:label "Gherkins"@en ;
                                                                                                    <http://www.w3.org/2004/02/skos/core#definition> """-- Definition --
|||Gherkins.
-- Description --
Cereals and main crops - C
NOTE. Initial value:C1766"""@en ;
                                                                                                    <http://www.w3.org/2004/02/skos/core#inScheme> :CropItemCodeValue .


###  http://lpis.ec.europa.eu/registry/applicationschema/cap-iacs-base/code#CropItemCodeValue/goldenDelicious
<http://lpis.ec.europa.eu/registry/applicationschema/cap-iacs-base/code#CropItemCodeValue/goldenDelicious> rdf:type owl:NamedIndividual ,
                                                                                                                    <http://lpis.ec.europa.eu/registry/applicationschema/cap-iacs-base#CropItemCodeValue> ;
                                                                                                           rdfs:label "Golden Delicious"@en ;
                                                                                                           <http://www.w3.org/2004/02/skos/core#definition> """-- Definition --
||||Golden Delicious.
-- Description --
Cereals and main crops - C
NOTE. Initial value:C2112"""@en ;
                                                                                                           <http://www.w3.org/2004/02/skos/core#inScheme> :CropItemCodeValue .


###  http://lpis.ec.europa.eu/registry/applicationschema/cap-iacs-base/code#CropItemCodeValue/gooseberries
<http://lpis.ec.europa.eu/registry/applicationschema/cap-iacs-base/code#CropItemCodeValue/gooseberries> rdf:type owl:NamedIndividual ,
                                                                                                                 <http://lpis.ec.europa.eu/registry/applicationschema/cap-iacs-base#CropItemCodeValue> ;
                                                                                                        rdfs:label "Gooseberries"@en ;
                                                                                                        <http://www.w3.org/2004/02/skos/core#definition> """-- Definition --
|||Gooseberries.
-- Description --
Cereals and main crops - C
NOTE. Initial value:C2281"""@en ;
                                                                                                        <http://www.w3.org/2004/02/skos/core#inScheme> :CropItemCodeValue .


###  http://lpis.ec.europa.eu/registry/applicationschema/cap-iacs-base/code#CropItemCodeValue/gourdsMarrowsAndPumpkins
<http://lpis.ec.europa.eu/registry/applicationschema/cap-iacs-base/code#CropItemCodeValue/gourdsMarrowsAndPumpkins> rdf:type owl:NamedIndividual ,
                                                                                                                             <http://lpis.ec.europa.eu/registry/applicationschema/cap-iacs-base#CropItemCodeValue> ;
                                                                                                                    rdfs:label "Gourds, marrows and pumpkins"@en ;
                                                                                                                    <http://www.w3.org/2004/02/skos/core#definition> """-- Definition --
||||Gourds, marrows and pumpkins.
-- Description --
Cereals and main crops - C
NOTE. Initial value:C1786"""@en ;
                                                                                                                    <http://www.w3.org/2004/02/skos/core#inScheme> :CropItemCodeValue .


###  http://lpis.ec.europa.eu/registry/applicationschema/cap-iacs-base/code#CropItemCodeValue/grainMaize
<http://lpis.ec.europa.eu/registry/applicationschema/cap-iacs-base/code#CropItemCodeValue/grainMaize> rdf:type owl:NamedIndividual ,
                                                                                                               <http://lpis.ec.europa.eu/registry/applicationschema/cap-iacs-base#CropItemCodeValue> ;
                                                                                                      rdfs:label "Grain maize"@en ;
                                                                                                      <http://www.w3.org/2004/02/skos/core#definition> """-- Definition --
||||Grain maize.
-- Description --
Cereals and main crops - C
NOTE. Initial value:C1200"""@en ;
                                                                                                      <http://www.w3.org/2004/02/skos/core#inScheme> :CropItemCodeValue .


###  http://lpis.ec.europa.eu/registry/applicationschema/cap-iacs-base/code#CropItemCodeValue/grainMaizeAndCornCobMix
<http://lpis.ec.europa.eu/registry/applicationschema/cap-iacs-base/code#CropItemCodeValue/grainMaizeAndCornCobMix> rdf:type owl:NamedIndividual ,
                                                                                                                            <http://lpis.ec.europa.eu/registry/applicationschema/cap-iacs-base#CropItemCodeValue> ;
                                                                                                                   rdfs:label "Grain maize and corn cob mix"@en ;
                                                                                                                   <http://www.w3.org/2004/02/skos/core#definition> """-- Definition --
|||Grain maize and corn cob mix.
-- Description --
Cereals and main crops - C
NOTE. Initial value:C1201"""@en ;
                                                                                                                   <http://www.w3.org/2004/02/skos/core#inScheme> :CropItemCodeValue .


###  http://lpis.ec.europa.eu/registry/applicationschema/cap-iacs-base/code#CropItemCodeValue/greenMaize
<http://lpis.ec.europa.eu/registry/applicationschema/cap-iacs-base/code#CropItemCodeValue/greenMaize> rdf:type owl:NamedIndividual ,
                                                                                                               <http://lpis.ec.europa.eu/registry/applicationschema/cap-iacs-base#CropItemCodeValue> ;
                                                                                                      rdfs:label "Green maize"@en ;
                                                                                                      <http://www.w3.org/2004/02/skos/core#definition> """-- Definition --
|||Green maize.
-- Description --
Cereals and main crops - C
NOTE. Initial value:C2625"""@en ;
                                                                                                      <http://www.w3.org/2004/02/skos/core#inScheme> :CropItemCodeValue .


###  http://lpis.ec.europa.eu/registry/applicationschema/cap-iacs-base/code#CropItemCodeValue/hazelnuts
<http://lpis.ec.europa.eu/registry/applicationschema/cap-iacs-base/code#CropItemCodeValue/hazelnuts> rdf:type owl:NamedIndividual ,
                                                                                                              <http://lpis.ec.europa.eu/registry/applicationschema/cap-iacs-base#CropItemCodeValue> ;
                                                                                                     rdfs:label "Hazelnuts"@en ;
                                                                                                     <http://www.w3.org/2004/02/skos/core#definition> """-- Definition --
|||Hazelnuts.
-- Description --
Cereals and main crops - C
NOTE. Initial value:C2232"""@en ;
                                                                                                     <http://www.w3.org/2004/02/skos/core#inScheme> :CropItemCodeValue .


###  http://lpis.ec.europa.eu/registry/applicationschema/cap-iacs-base/code#CropItemCodeValue/hemp
<http://lpis.ec.europa.eu/registry/applicationschema/cap-iacs-base/code#CropItemCodeValue/hemp> rdf:type owl:NamedIndividual ,
                                                                                                         <http://lpis.ec.europa.eu/registry/applicationschema/cap-iacs-base#CropItemCodeValue> ;
                                                                                                rdfs:label "Hemp"@en ;
                                                                                                <http://www.w3.org/2004/02/skos/core#definition> """-- Definition --
|||Hemp.
-- Description --
Cereals and main crops - C
NOTE. Initial value:C1530"""@en ;
                                                                                                <http://www.w3.org/2004/02/skos/core#inScheme> :CropItemCodeValue .


###  http://lpis.ec.europa.eu/registry/applicationschema/cap-iacs-base/code#CropItemCodeValue/hops
<http://lpis.ec.europa.eu/registry/applicationschema/cap-iacs-base/code#CropItemCodeValue/hops> rdf:type owl:NamedIndividual ,
                                                                                                         <http://lpis.ec.europa.eu/registry/applicationschema/cap-iacs-base#CropItemCodeValue> ;
                                                                                                rdfs:label "Hops"@en ;
                                                                                                <http://www.w3.org/2004/02/skos/core#definition> """-- Definition --
||Hops.
-- Description --
Cereals and main crops - C
NOTE. Initial value:C1560"""@en ;
                                                                                                <http://www.w3.org/2004/02/skos/core#inScheme> :CropItemCodeValue .


###  http://lpis.ec.europa.eu/registry/applicationschema/cap-iacs-base/code#CropItemCodeValue/industrialCrops
<http://lpis.ec.europa.eu/registry/applicationschema/cap-iacs-base/code#CropItemCodeValue/industrialCrops> rdf:type owl:NamedIndividual ,
                                                                                                                    <http://lpis.ec.europa.eu/registry/applicationschema/cap-iacs-base#CropItemCodeValue> ;
                                                                                                           rdfs:label "Industrial crops "@en ;
                                                                                                           <http://www.w3.org/2004/02/skos/core#definition> """-- Definition --
|Industrial crops .
-- Description --
Cereals and main crops - C
NOTE. Initial value:C1400"""@en ;
                                                                                                           <http://www.w3.org/2004/02/skos/core#inScheme> :CropItemCodeValue .


###  http://lpis.ec.europa.eu/registry/applicationschema/cap-iacs-base/code#CropItemCodeValue/industrialCropsL1400
<http://lpis.ec.europa.eu/registry/applicationschema/cap-iacs-base/code#CropItemCodeValue/industrialCropsL1400> rdf:type owl:NamedIndividual ,
                                                                                                                         <http://lpis.ec.europa.eu/registry/applicationschema/cap-iacs-base#CropItemCodeValue> ;
                                                                                                                rdfs:label "Industrial crops L1400"@en ;
                                                                                                                <http://www.w3.org/2004/02/skos/core#definition> """-- Definition --
|||Industrial crops L1400.
-- Description --
Land use of Agriculture Area in Use -L
NOTE. Initial value:L1400"""@en ;
                                                                                                                <http://www.w3.org/2004/02/skos/core#inScheme> :CropItemCodeValue .


###  http://lpis.ec.europa.eu/registry/applicationschema/cap-iacs-base/code#CropItemCodeValue/kitchenGardens
<http://lpis.ec.europa.eu/registry/applicationschema/cap-iacs-base/code#CropItemCodeValue/kitchenGardens> rdf:type owl:NamedIndividual ,
                                                                                                                   <http://lpis.ec.europa.eu/registry/applicationschema/cap-iacs-base#CropItemCodeValue> ;
                                                                                                          rdfs:label "Kitchen gardens"@en ;
                                                                                                          <http://www.w3.org/2004/02/skos/core#definition> """-- Definition --
||Kitchen gardens.
-- Description --
Land use of Agriculture Area in Use -L
NOTE. Initial value:L0004"""@en ;
                                                                                                          <http://www.w3.org/2004/02/skos/core#inScheme> :CropItemCodeValue .


###  http://lpis.ec.europa.eu/registry/applicationschema/cap-iacs-base/code#CropItemCodeValue/kiwis
<http://lpis.ec.europa.eu/registry/applicationschema/cap-iacs-base/code#CropItemCodeValue/kiwis> rdf:type owl:NamedIndividual ,
                                                                                                          <http://lpis.ec.europa.eu/registry/applicationschema/cap-iacs-base#CropItemCodeValue> ;
                                                                                                 rdfs:label "Kiwis"@en ;
                                                                                                 <http://www.w3.org/2004/02/skos/core#definition> """-- Definition --
|||Kiwis.
-- Description --
Cereals and main crops - C
NOTE. Initial value:C2285"""@en ;
                                                                                                 <http://www.w3.org/2004/02/skos/core#inScheme> :CropItemCodeValue .


###  http://lpis.ec.europa.eu/registry/applicationschema/cap-iacs-base/code#CropItemCodeValue/kohlRabiC1650
<http://lpis.ec.europa.eu/registry/applicationschema/cap-iacs-base/code#CropItemCodeValue/kohlRabiC1650> rdf:type owl:NamedIndividual ,
                                                                                                                  <http://lpis.ec.europa.eu/registry/applicationschema/cap-iacs-base#CropItemCodeValue> ;
                                                                                                         rdfs:label "Kohl-Rabi C1650"@en ;
                                                                                                         <http://www.w3.org/2004/02/skos/core#definition> """-- Definition --
|||Kohl-Rabi C1650.
-- Description --
Cereals and main crops - C
NOTE. Initial value:C1650"""@en ;
                                                                                                         <http://www.w3.org/2004/02/skos/core#inScheme> :CropItemCodeValue .


###  http://lpis.ec.europa.eu/registry/applicationschema/cap-iacs-base/code#CropItemCodeValue/leafyOrStalkedVegetablesExcludingBrassicas
<http://lpis.ec.europa.eu/registry/applicationschema/cap-iacs-base/code#CropItemCodeValue/leafyOrStalkedVegetablesExcludingBrassicas> rdf:type owl:NamedIndividual ,
                                                                                                                                               <http://lpis.ec.europa.eu/registry/applicationschema/cap-iacs-base#CropItemCodeValue> ;
                                                                                                                                      rdfs:label "Leafy or stalked vegetables (excluding brassicas)"@en ;
                                                                                                                                      <http://www.w3.org/2004/02/skos/core#definition> """-- Definition --
||Leafy or stalked vegetables (excluding brassicas).
-- Description --
Cereals and main crops - C
NOTE. Initial value:C1660"""@en ;
                                                                                                                                      <http://www.w3.org/2004/02/skos/core#inScheme> :CropItemCodeValue .


###  http://lpis.ec.europa.eu/registry/applicationschema/cap-iacs-base/code#CropItemCodeValue/leeks
<http://lpis.ec.europa.eu/registry/applicationschema/cap-iacs-base/code#CropItemCodeValue/leeks> rdf:type owl:NamedIndividual ,
                                                                                                          <http://lpis.ec.europa.eu/registry/applicationschema/cap-iacs-base#CropItemCodeValue> ;
                                                                                                 rdfs:label "Leeks"@en ;
                                                                                                 <http://www.w3.org/2004/02/skos/core#definition> """-- Definition --
|||Leeks.
-- Description --
Cereals and main crops - C
NOTE. Initial value:C1675"""@en ;
                                                                                                 <http://www.w3.org/2004/02/skos/core#inScheme> :CropItemCodeValue .


###  http://lpis.ec.europa.eu/registry/applicationschema/cap-iacs-base/code#CropItemCodeValue/leguminousPlants
<http://lpis.ec.europa.eu/registry/applicationschema/cap-iacs-base/code#CropItemCodeValue/leguminousPlants> rdf:type owl:NamedIndividual ,
                                                                                                                     <http://lpis.ec.europa.eu/registry/applicationschema/cap-iacs-base#CropItemCodeValue> ;
                                                                                                            rdfs:label "Leguminous plants"@en ;
                                                                                                            <http://www.w3.org/2004/02/skos/core#definition> """-- Definition --
||Leguminous plants.
-- Description --
Cereals and main crops - C
NOTE. Initial value:C2670"""@en ;
                                                                                                            <http://www.w3.org/2004/02/skos/core#inScheme> :CropItemCodeValue .


###  http://lpis.ec.europa.eu/registry/applicationschema/cap-iacs-base/code#CropItemCodeValue/lemonsAndAcidLimesC2370
<http://lpis.ec.europa.eu/registry/applicationschema/cap-iacs-base/code#CropItemCodeValue/lemonsAndAcidLimesC2370> rdf:type owl:NamedIndividual ,
                                                                                                                            <http://lpis.ec.europa.eu/registry/applicationschema/cap-iacs-base#CropItemCodeValue> ;
                                                                                                                   rdfs:label "Lemons and acid limes C2370"@en ;
                                                                                                                   <http://www.w3.org/2004/02/skos/core#definition> """-- Definition --
|||Lemons and acid limes C2370.
-- Description --
Cereals and main crops - C
NOTE. Initial value:C2370"""@en ;
                                                                                                                   <http://www.w3.org/2004/02/skos/core#inScheme> :CropItemCodeValue .


###  http://lpis.ec.europa.eu/registry/applicationschema/cap-iacs-base/code#CropItemCodeValue/lettuces
<http://lpis.ec.europa.eu/registry/applicationschema/cap-iacs-base/code#CropItemCodeValue/lettuces> rdf:type owl:NamedIndividual ,
                                                                                                             <http://lpis.ec.europa.eu/registry/applicationschema/cap-iacs-base#CropItemCodeValue> ;
                                                                                                    rdfs:label "Lettuces"@en ;
                                                                                                    <http://www.w3.org/2004/02/skos/core#definition> """-- Definition --
|||Lettuces.
-- Description --
Cereals and main crops - C
NOTE. Initial value:C1680"""@en ;
                                                                                                    <http://www.w3.org/2004/02/skos/core#inScheme> :CropItemCodeValue .


###  http://lpis.ec.europa.eu/registry/applicationschema/cap-iacs-base/code#CropItemCodeValue/lettucesUnderGlassOrHighAccessibleCoverC1681
<http://lpis.ec.europa.eu/registry/applicationschema/cap-iacs-base/code#CropItemCodeValue/lettucesUnderGlassOrHighAccessibleCoverC1681> rdf:type owl:NamedIndividual ,
                                                                                                                                                 <http://lpis.ec.europa.eu/registry/applicationschema/cap-iacs-base#CropItemCodeValue> ;
                                                                                                                                        rdfs:label "Lettuces under glass or high accessible cover C1681 "@en ;
                                                                                                                                        <http://www.w3.org/2004/02/skos/core#definition> """-- Definition --
||||Lettuces under glass or high accessible cover C1681.
-- Description --
Cereals and main crops - C
NOTE. Initial value:C1681"""@en ;
                                                                                                                                        <http://www.w3.org/2004/02/skos/core#inScheme> :CropItemCodeValue .


###  http://lpis.ec.europa.eu/registry/applicationschema/cap-iacs-base/code#CropItemCodeValue/linseedOilFlax
<http://lpis.ec.europa.eu/registry/applicationschema/cap-iacs-base/code#CropItemCodeValue/linseedOilFlax> rdf:type owl:NamedIndividual ,
                                                                                                                   <http://lpis.ec.europa.eu/registry/applicationschema/cap-iacs-base#CropItemCodeValue> ;
                                                                                                          rdfs:label "Linseed (oil flax)"@en ;
                                                                                                          <http://www.w3.org/2004/02/skos/core#definition> """-- Definition --
||||Linseed (oil flax).
-- Description --
Cereals and main crops - C
NOTE. Initial value:C1460"""@en ;
                                                                                                          <http://www.w3.org/2004/02/skos/core#inScheme> :CropItemCodeValue .


###  http://lpis.ec.europa.eu/registry/applicationschema/cap-iacs-base/code#CropItemCodeValue/lucerne
<http://lpis.ec.europa.eu/registry/applicationschema/cap-iacs-base/code#CropItemCodeValue/lucerne> rdf:type owl:NamedIndividual ,
                                                                                                            <http://lpis.ec.europa.eu/registry/applicationschema/cap-iacs-base#CropItemCodeValue> ;
                                                                                                   rdfs:label "Lucerne"@en ;
                                                                                                   <http://www.w3.org/2004/02/skos/core#definition> """-- Definition --
|||Lucerne.
-- Description --
Cereals and main crops - C
NOTE. Initial value:C2672"""@en ;
                                                                                                   <http://www.w3.org/2004/02/skos/core#inScheme> :CropItemCodeValue .


###  http://lpis.ec.europa.eu/registry/applicationschema/cap-iacs-base/code#CropItemCodeValue/mainOilSeedCrops
<http://lpis.ec.europa.eu/registry/applicationschema/cap-iacs-base/code#CropItemCodeValue/mainOilSeedCrops> rdf:type owl:NamedIndividual ,
                                                                                                                     <http://lpis.ec.europa.eu/registry/applicationschema/cap-iacs-base#CropItemCodeValue> ;
                                                                                                            rdfs:label "Main oil seed crops"@en ;
                                                                                                            <http://www.w3.org/2004/02/skos/core#definition> """-- Definition --
|||Main oil seed crops.
-- Description --
Cereals and main crops - C
NOTE. Initial value:C1415"""@en ;
                                                                                                            <http://www.w3.org/2004/02/skos/core#inScheme> :CropItemCodeValue .


###  http://lpis.ec.europa.eu/registry/applicationschema/cap-iacs-base/code#CropItemCodeValue/maslin
<http://lpis.ec.europa.eu/registry/applicationschema/cap-iacs-base/code#CropItemCodeValue/maslin> rdf:type owl:NamedIndividual ,
                                                                                                           <http://lpis.ec.europa.eu/registry/applicationschema/cap-iacs-base#CropItemCodeValue> ;
                                                                                                  rdfs:label "Maslin"@en ;
                                                                                                  <http://www.w3.org/2004/02/skos/core#definition> """-- Definition --
||||Maslin.
-- Description --
Cereals and main crops - C
NOTE. Initial value:C1155"""@en ;
                                                                                                  <http://www.w3.org/2004/02/skos/core#inScheme> :CropItemCodeValue .


###  http://lpis.ec.europa.eu/registry/applicationschema/cap-iacs-base/code#CropItemCodeValue/melons
<http://lpis.ec.europa.eu/registry/applicationschema/cap-iacs-base/code#CropItemCodeValue/melons> rdf:type owl:NamedIndividual ,
                                                                                                           <http://lpis.ec.europa.eu/registry/applicationschema/cap-iacs-base#CropItemCodeValue> ;
                                                                                                  rdfs:label "Melons"@en ;
                                                                                                  <http://www.w3.org/2004/02/skos/core#definition> """-- Definition --
||Melons.
-- Description --
Cereals and main crops - C
NOTE. Initial value:C1771"""@en ;
                                                                                                  <http://www.w3.org/2004/02/skos/core#inScheme> :CropItemCodeValue .


###  http://lpis.ec.europa.eu/registry/applicationschema/cap-iacs-base/code#CropItemCodeValue/mixedGrainOtherThanMaslinC1185
<http://lpis.ec.europa.eu/registry/applicationschema/cap-iacs-base/code#CropItemCodeValue/mixedGrainOtherThanMaslinC1185> rdf:type owl:NamedIndividual ,
                                                                                                                                   <http://lpis.ec.europa.eu/registry/applicationschema/cap-iacs-base#CropItemCodeValue> ;
                                                                                                                          rdfs:label "Mixed grain other than maslin C1185"@en ;
                                                                                                                          <http://www.w3.org/2004/02/skos/core#definition> """-- Definition --
||||Mixed grain other than maslin C1185.
-- Description --
Cereals and main crops - C
NOTE. Initial value:C1185"""@en ;
                                                                                                                          <http://www.w3.org/2004/02/skos/core#inScheme> :CropItemCodeValue .


###  http://lpis.ec.europa.eu/registry/applicationschema/cap-iacs-base/code#CropItemCodeValue/nectarines
<http://lpis.ec.europa.eu/registry/applicationschema/cap-iacs-base/code#CropItemCodeValue/nectarines> rdf:type owl:NamedIndividual ,
                                                                                                               <http://lpis.ec.europa.eu/registry/applicationschema/cap-iacs-base#CropItemCodeValue> ;
                                                                                                      rdfs:label "Nectarines"@en ;
                                                                                                      <http://www.w3.org/2004/02/skos/core#definition> """-- Definition --
|||Nectarines.
-- Description --
Cereals and main crops - C
NOTE. Initial value:C2221"""@en ;
                                                                                                      <http://www.w3.org/2004/02/skos/core#inScheme> :CropItemCodeValue .


###  http://lpis.ec.europa.eu/registry/applicationschema/cap-iacs-base/code#CropItemCodeValue/nurseries
<http://lpis.ec.europa.eu/registry/applicationschema/cap-iacs-base/code#CropItemCodeValue/nurseries> rdf:type owl:NamedIndividual ,
                                                                                                              <http://lpis.ec.europa.eu/registry/applicationschema/cap-iacs-base#CropItemCodeValue> ;
                                                                                                     rdfs:label "Nurseries"@en ;
                                                                                                     <http://www.w3.org/2004/02/skos/core#definition> """-- Definition --
|||Nurseries.
-- Description --
Land use of Agriculture Area in Use -L
NOTE. Initial value:L2810"""@en ;
                                                                                                     <http://www.w3.org/2004/02/skos/core#inScheme> :CropItemCodeValue .


###  http://lpis.ec.europa.eu/registry/applicationschema/cap-iacs-base/code#CropItemCodeValue/nutsC2230
<http://lpis.ec.europa.eu/registry/applicationschema/cap-iacs-base/code#CropItemCodeValue/nutsC2230> rdf:type owl:NamedIndividual ,
                                                                                                              <http://lpis.ec.europa.eu/registry/applicationschema/cap-iacs-base#CropItemCodeValue> ;
                                                                                                     rdfs:label "Nuts C2230"@en ;
                                                                                                     <http://www.w3.org/2004/02/skos/core#definition> """-- Definition --
||Nuts C2230.
-- Description --
Cereals and main crops - C
NOTE. Initial value:C2230"""@en ;
                                                                                                     <http://www.w3.org/2004/02/skos/core#inScheme> :CropItemCodeValue .


###  http://lpis.ec.europa.eu/registry/applicationschema/cap-iacs-base/code#CropItemCodeValue/oats
<http://lpis.ec.europa.eu/registry/applicationschema/cap-iacs-base/code#CropItemCodeValue/oats> rdf:type owl:NamedIndividual ,
                                                                                                         <http://lpis.ec.europa.eu/registry/applicationschema/cap-iacs-base#CropItemCodeValue> ;
                                                                                                rdfs:label "Oats"@en ;
                                                                                                <http://www.w3.org/2004/02/skos/core#definition> """-- Definition --
||||Oats.
-- Description --
Cereals and main crops - C
NOTE. Initial value:C1180"""@en ;
                                                                                                <http://www.w3.org/2004/02/skos/core#inScheme> :CropItemCodeValue .


###  http://lpis.ec.europa.eu/registry/applicationschema/cap-iacs-base/code#CropItemCodeValue/oatsAndMixedGrainOtherThanMaslin
<http://lpis.ec.europa.eu/registry/applicationschema/cap-iacs-base/code#CropItemCodeValue/oatsAndMixedGrainOtherThanMaslin> rdf:type owl:NamedIndividual ,
                                                                                                                                     <http://lpis.ec.europa.eu/registry/applicationschema/cap-iacs-base#CropItemCodeValue> ;
                                                                                                                            rdfs:label "Oats and mixed grain other than maslin"@en ;
                                                                                                                            <http://www.w3.org/2004/02/skos/core#definition> """-- Definition --
|||Oats and mixed grain other than maslin.
-- Description --
Cereals and main crops - C
NOTE. Initial value:C1170"""@en ;
                                                                                                                            <http://www.w3.org/2004/02/skos/core#inScheme> :CropItemCodeValue .


###  http://lpis.ec.europa.eu/registry/applicationschema/cap-iacs-base/code#CropItemCodeValue/oilseeds
<http://lpis.ec.europa.eu/registry/applicationschema/cap-iacs-base/code#CropItemCodeValue/oilseeds> rdf:type owl:NamedIndividual ,
                                                                                                             <http://lpis.ec.europa.eu/registry/applicationschema/cap-iacs-base#CropItemCodeValue> ;
                                                                                                    rdfs:label "Oilseeds"@en ;
                                                                                                    <http://www.w3.org/2004/02/skos/core#definition> """-- Definition --
||Oilseeds.
-- Description --
Cereals and main crops - C
NOTE. Initial value:C1410"""@en ;
                                                                                                    <http://www.w3.org/2004/02/skos/core#inScheme> :CropItemCodeValue .


###  http://lpis.ec.europa.eu/registry/applicationschema/cap-iacs-base/code#CropItemCodeValue/olivePlantations
<http://lpis.ec.europa.eu/registry/applicationschema/cap-iacs-base/code#CropItemCodeValue/olivePlantations> rdf:type owl:NamedIndividual ,
                                                                                                                     <http://lpis.ec.europa.eu/registry/applicationschema/cap-iacs-base#CropItemCodeValue> ;
                                                                                                            rdfs:label "Olive plantations"@en ;
                                                                                                            <http://www.w3.org/2004/02/skos/core#definition> """-- Definition --
|||Olive plantations.
-- Description --
Land use of Agriculture Area in Use -L
NOTE. Initial value:L2450"""@en ;
                                                                                                            <http://www.w3.org/2004/02/skos/core#inScheme> :CropItemCodeValue .


###  http://lpis.ec.europa.eu/registry/applicationschema/cap-iacs-base/code#CropItemCodeValue/oliveTreesC2450
<http://lpis.ec.europa.eu/registry/applicationschema/cap-iacs-base/code#CropItemCodeValue/oliveTreesC2450> rdf:type owl:NamedIndividual ,
                                                                                                                    <http://lpis.ec.europa.eu/registry/applicationschema/cap-iacs-base#CropItemCodeValue> ;
                                                                                                           rdfs:label "Olive trees C2450"@en ;
                                                                                                           <http://www.w3.org/2004/02/skos/core#definition> """-- Definition --
||Olive trees C2450.
-- Description --
Cereals and main crops - C
NOTE. Initial value:C2450"""@en ;
                                                                                                           <http://www.w3.org/2004/02/skos/core#inScheme> :CropItemCodeValue .


###  http://lpis.ec.europa.eu/registry/applicationschema/cap-iacs-base/code#CropItemCodeValue/onions
<http://lpis.ec.europa.eu/registry/applicationschema/cap-iacs-base/code#CropItemCodeValue/onions> rdf:type owl:NamedIndividual ,
                                                                                                           <http://lpis.ec.europa.eu/registry/applicationschema/cap-iacs-base#CropItemCodeValue> ;
                                                                                                  rdfs:label "Onions"@en ;
                                                                                                  <http://www.w3.org/2004/02/skos/core#definition> """-- Definition --
|||Onions.
-- Description --
Cereals and main crops - C
NOTE. Initial value:C1851"""@en ;
                                                                                                  <http://www.w3.org/2004/02/skos/core#inScheme> :CropItemCodeValue .


###  http://lpis.ec.europa.eu/registry/applicationschema/cap-iacs-base/code#CropItemCodeValue/oranges
<http://lpis.ec.europa.eu/registry/applicationschema/cap-iacs-base/code#CropItemCodeValue/oranges> rdf:type owl:NamedIndividual ,
                                                                                                            <http://lpis.ec.europa.eu/registry/applicationschema/cap-iacs-base#CropItemCodeValue> ;
                                                                                                   rdfs:label "Oranges"@en ;
                                                                                                   <http://www.w3.org/2004/02/skos/core#definition> """-- Definition --
|||Oranges.
-- Description --
Cereals and main crops - C
NOTE. Initial value:C2320"""@en ;
                                                                                                   <http://www.w3.org/2004/02/skos/core#inScheme> :CropItemCodeValue .


###  http://lpis.ec.europa.eu/registry/applicationschema/cap-iacs-base/code#CropItemCodeValue/otherAnnualPlantsHarvestedGreenNecC2612
<http://lpis.ec.europa.eu/registry/applicationschema/cap-iacs-base/code#CropItemCodeValue/otherAnnualPlantsHarvestedGreenNecC2612> rdf:type owl:NamedIndividual ,
                                                                                                                                            <http://lpis.ec.europa.eu/registry/applicationschema/cap-iacs-base#CropItemCodeValue> ;
                                                                                                                                   rdfs:label "Other annual plants harvested green n.e.c. C2612"@en ;
                                                                                                                                   <http://www.w3.org/2004/02/skos/core#definition> """-- Definition --
|||Other annual plants harvested green n.e.c. C2612.
-- Description --
Cereals and main crops - C
NOTE. Initial value:C2612"""@en ;
                                                                                                                                   <http://www.w3.org/2004/02/skos/core#inScheme> :CropItemCodeValue .


###  http://lpis.ec.europa.eu/registry/applicationschema/cap-iacs-base/code#CropItemCodeValue/otherApplesForFreshConsumption
<http://lpis.ec.europa.eu/registry/applicationschema/cap-iacs-base/code#CropItemCodeValue/otherApplesForFreshConsumption> rdf:type owl:NamedIndividual ,
                                                                                                                                   <http://lpis.ec.europa.eu/registry/applicationschema/cap-iacs-base#CropItemCodeValue> ;
                                                                                                                          rdfs:label "Other apples for fresh consumption"@en ;
                                                                                                                          <http://www.w3.org/2004/02/skos/core#definition> """-- Definition --
||||Other apples for fresh consumption.
-- Description --
Cereals and main crops - C
NOTE. Initial value:C2113"""@en ;
                                                                                                                          <http://www.w3.org/2004/02/skos/core#inScheme> :CropItemCodeValue .


###  http://lpis.ec.europa.eu/registry/applicationschema/cap-iacs-base/code#CropItemCodeValue/otherArableLandCrops
<http://lpis.ec.europa.eu/registry/applicationschema/cap-iacs-base/code#CropItemCodeValue/otherArableLandCrops> rdf:type owl:NamedIndividual ,
                                                                                                                         <http://lpis.ec.europa.eu/registry/applicationschema/cap-iacs-base#CropItemCodeValue> ;
                                                                                                                rdfs:label "Other arable-land crops"@en ;
                                                                                                                <http://www.w3.org/2004/02/skos/core#definition> """-- Definition --
|||Other arable-land crops.
-- Description --
Land use of Agriculture Area in Use -L
NOTE. Initial value:L2690"""@en ;
                                                                                                                <http://www.w3.org/2004/02/skos/core#inScheme> :CropItemCodeValue .


###  http://lpis.ec.europa.eu/registry/applicationschema/cap-iacs-base/code#CropItemCodeValue/otherBerriesNec
<http://lpis.ec.europa.eu/registry/applicationschema/cap-iacs-base/code#CropItemCodeValue/otherBerriesNec> rdf:type owl:NamedIndividual ,
                                                                                                                    <http://lpis.ec.europa.eu/registry/applicationschema/cap-iacs-base#CropItemCodeValue> ;
                                                                                                           rdfs:label "Other berries n.e.c."@en ;
                                                                                                           <http://www.w3.org/2004/02/skos/core#definition> """-- Definition --
|||Other berries n.e.c.
-- Description --
Cereals and main crops - C
NOTE. Initial value:C2290"""@en ;
                                                                                                           <http://www.w3.org/2004/02/skos/core#inScheme> :CropItemCodeValue .


###  http://lpis.ec.europa.eu/registry/applicationschema/cap-iacs-base/code#CropItemCodeValue/otherBrassicasNec
<http://lpis.ec.europa.eu/registry/applicationschema/cap-iacs-base/code#CropItemCodeValue/otherBrassicasNec> rdf:type owl:NamedIndividual ,
                                                                                                                      <http://lpis.ec.europa.eu/registry/applicationschema/cap-iacs-base#CropItemCodeValue> ;
                                                                                                             rdfs:label "Other brassicas n.e.c."@en ;
                                                                                                             <http://www.w3.org/2004/02/skos/core#definition> """-- Definition --
|||Other brassicas n.e.c.
-- Description --
Cereals and main crops - C
NOTE. Initial value:C1655"""@en ;
                                                                                                             <http://www.w3.org/2004/02/skos/core#inScheme> :CropItemCodeValue .


###  http://lpis.ec.europa.eu/registry/applicationschema/cap-iacs-base/code#CropItemCodeValue/otherCitrusFruitsNec
<http://lpis.ec.europa.eu/registry/applicationschema/cap-iacs-base/code#CropItemCodeValue/otherCitrusFruitsNec> rdf:type owl:NamedIndividual ,
                                                                                                                         <http://lpis.ec.europa.eu/registry/applicationschema/cap-iacs-base#CropItemCodeValue> ;
                                                                                                                rdfs:label "Other citrus fruits n.e.c."@en ;
                                                                                                                <http://www.w3.org/2004/02/skos/core#definition> """-- Definition --
|||Other citrus fruits n.e.c.
-- Description --
Cereals and main crops - C
NOTE. Initial value:C2390"""@en ;
                                                                                                                <http://www.w3.org/2004/02/skos/core#inScheme> :CropItemCodeValue .


###  http://lpis.ec.europa.eu/registry/applicationschema/cap-iacs-base/code#CropItemCodeValue/otherDriedPulsesNecC1345
<http://lpis.ec.europa.eu/registry/applicationschema/cap-iacs-base/code#CropItemCodeValue/otherDriedPulsesNecC1345> rdf:type owl:NamedIndividual ,
                                                                                                                             <http://lpis.ec.europa.eu/registry/applicationschema/cap-iacs-base#CropItemCodeValue> ;
                                                                                                                    rdfs:label "Other dried pulses n.e.c. C1345"@en ;
                                                                                                                    <http://www.w3.org/2004/02/skos/core#definition> """-- Definition --
||Other dried pulses n.e.c. C1345.
-- Description --
Cereals and main crops - C
NOTE. Initial value:C1345"""@en ;
                                                                                                                    <http://www.w3.org/2004/02/skos/core#inScheme> :CropItemCodeValue .


###  http://lpis.ec.europa.eu/registry/applicationschema/cap-iacs-base/code#CropItemCodeValue/otherFibreCropsNec
<http://lpis.ec.europa.eu/registry/applicationschema/cap-iacs-base/code#CropItemCodeValue/otherFibreCropsNec> rdf:type owl:NamedIndividual ,
                                                                                                                       <http://lpis.ec.europa.eu/registry/applicationschema/cap-iacs-base#CropItemCodeValue> ;
                                                                                                              rdfs:label "Other fibre crops n.e.c."@en ;
                                                                                                              <http://www.w3.org/2004/02/skos/core#definition> """-- Definition --
|||Other fibre crops n.e.c.
-- Description --
Cereals and main crops - C
NOTE. Initial value:C1510"""@en ;
                                                                                                              <http://www.w3.org/2004/02/skos/core#inScheme> :CropItemCodeValue .


###  http://lpis.ec.europa.eu/registry/applicationschema/cap-iacs-base/code#CropItemCodeValue/otherFreshVegetablesNec
<http://lpis.ec.europa.eu/registry/applicationschema/cap-iacs-base/code#CropItemCodeValue/otherFreshVegetablesNec> rdf:type owl:NamedIndividual ,
                                                                                                                            <http://lpis.ec.europa.eu/registry/applicationschema/cap-iacs-base#CropItemCodeValue> ;
                                                                                                                   rdfs:label "Other fresh vegetables n.e.c."@en ;
                                                                                                                   <http://www.w3.org/2004/02/skos/core#definition> """-- Definition --
||Other fresh vegetables n.e.c.
-- Description --
Cereals and main crops - C
NOTE. Initial value:C1920"""@en ;
                                                                                                                   <http://www.w3.org/2004/02/skos/core#inScheme> :CropItemCodeValue .


###  http://lpis.ec.europa.eu/registry/applicationschema/cap-iacs-base/code#CropItemCodeValue/otherFruitsFromFruitTrees
<http://lpis.ec.europa.eu/registry/applicationschema/cap-iacs-base/code#CropItemCodeValue/otherFruitsFromFruitTrees> rdf:type owl:NamedIndividual ,
                                                                                                                              <http://lpis.ec.europa.eu/registry/applicationschema/cap-iacs-base#CropItemCodeValue> ;
                                                                                                                     rdfs:label "Other fruits from fruit trees"@en ;
                                                                                                                     <http://www.w3.org/2004/02/skos/core#definition> """-- Definition --
||Other fruits from fruit trees.
-- Description --
Cereals and main crops - C
NOTE. Initial value:C2250"""@en ;
                                                                                                                     <http://www.w3.org/2004/02/skos/core#inScheme> :CropItemCodeValue .


###  http://lpis.ec.europa.eu/registry/applicationschema/cap-iacs-base/code#CropItemCodeValue/otherFruitsFromFruitTreesNec
<http://lpis.ec.europa.eu/registry/applicationschema/cap-iacs-base/code#CropItemCodeValue/otherFruitsFromFruitTreesNec> rdf:type owl:NamedIndividual ,
                                                                                                                                 <http://lpis.ec.europa.eu/registry/applicationschema/cap-iacs-base#CropItemCodeValue> ;
                                                                                                                        rdfs:label "Other fruits from fruit trees n.e.c."@en ;
                                                                                                                        <http://www.w3.org/2004/02/skos/core#definition> """-- Definition --
|||Other fruits from fruit trees n.e.c.
-- Description --
Cereals and main crops - C
NOTE. Initial value:C2259"""@en ;
                                                                                                                        <http://www.w3.org/2004/02/skos/core#inScheme> :CropItemCodeValue .


###  http://lpis.ec.europa.eu/registry/applicationschema/cap-iacs-base/code#CropItemCodeValue/otherIndustrialCrops
<http://lpis.ec.europa.eu/registry/applicationschema/cap-iacs-base/code#CropItemCodeValue/otherIndustrialCrops> rdf:type owl:NamedIndividual ,
                                                                                                                         <http://lpis.ec.europa.eu/registry/applicationschema/cap-iacs-base#CropItemCodeValue> ;
                                                                                                                rdfs:label "Other industrial crops"@en ;
                                                                                                                <http://www.w3.org/2004/02/skos/core#definition> """-- Definition --
||Other industrial crops.
-- Description --
Cereals and main crops - C
NOTE. Initial value:C1570"""@en ;
                                                                                                                <http://www.w3.org/2004/02/skos/core#inScheme> :CropItemCodeValue .


###  http://lpis.ec.europa.eu/registry/applicationschema/cap-iacs-base/code#CropItemCodeValue/otherIndustrialCropsNec
<http://lpis.ec.europa.eu/registry/applicationschema/cap-iacs-base/code#CropItemCodeValue/otherIndustrialCropsNec> rdf:type owl:NamedIndividual ,
                                                                                                                            <http://lpis.ec.europa.eu/registry/applicationschema/cap-iacs-base#CropItemCodeValue> ;
                                                                                                                   rdfs:label "Other industrial crops n.e.c."@en ;
                                                                                                                   <http://www.w3.org/2004/02/skos/core#definition> """-- Definition --
|||Other industrial crops n.e.c.
-- Description --
Cereals and main crops - C
NOTE. Initial value:C1589"""@en ;
                                                                                                                   <http://www.w3.org/2004/02/skos/core#inScheme> :CropItemCodeValue .


###  http://lpis.ec.europa.eu/registry/applicationschema/cap-iacs-base/code#CropItemCodeValue/otherLeafyOrStalkedVegetablesNec
<http://lpis.ec.europa.eu/registry/applicationschema/cap-iacs-base/code#CropItemCodeValue/otherLeafyOrStalkedVegetablesNec> rdf:type owl:NamedIndividual ,
                                                                                                                                     <http://lpis.ec.europa.eu/registry/applicationschema/cap-iacs-base#CropItemCodeValue> ;
                                                                                                                            rdfs:label "Other leafy or stalked vegetables n.e.c."@en ;
                                                                                                                            <http://www.w3.org/2004/02/skos/core#definition> """-- Definition --
|||Other leafy or stalked vegetables n.e.c.
-- Description --
Cereals and main crops - C
NOTE. Initial value:C1725"""@en ;
                                                                                                                            <http://www.w3.org/2004/02/skos/core#inScheme> :CropItemCodeValue .


###  http://lpis.ec.europa.eu/registry/applicationschema/cap-iacs-base/code#CropItemCodeValue/otherLeguminousPlantsNec
<http://lpis.ec.europa.eu/registry/applicationschema/cap-iacs-base/code#CropItemCodeValue/otherLeguminousPlantsNec> rdf:type owl:NamedIndividual ,
                                                                                                                             <http://lpis.ec.europa.eu/registry/applicationschema/cap-iacs-base#CropItemCodeValue> ;
                                                                                                                    rdfs:label "Other leguminous plants n.e.c."@en ;
                                                                                                                    <http://www.w3.org/2004/02/skos/core#definition> """-- Definition --
|||Other leguminous plants n.e.c.
-- Description --
Cereals and main crops - C
NOTE. Initial value:C2673"""@en ;
                                                                                                                    <http://www.w3.org/2004/02/skos/core#inScheme> :CropItemCodeValue .


###  http://lpis.ec.europa.eu/registry/applicationschema/cap-iacs-base/code#CropItemCodeValue/otherNutsNec
<http://lpis.ec.europa.eu/registry/applicationschema/cap-iacs-base/code#CropItemCodeValue/otherNutsNec> rdf:type owl:NamedIndividual ,
                                                                                                                 <http://lpis.ec.europa.eu/registry/applicationschema/cap-iacs-base#CropItemCodeValue> ;
                                                                                                        rdfs:label "Other nuts n.e.c."@en ;
                                                                                                        <http://www.w3.org/2004/02/skos/core#definition> """-- Definition --
|||Other nuts n.e.c.
-- Description --
Cereals and main crops - C
NOTE. Initial value:C2240"""@en ;
                                                                                                        <http://www.w3.org/2004/02/skos/core#inScheme> :CropItemCodeValue .


###  http://lpis.ec.europa.eu/registry/applicationschema/cap-iacs-base/code#CropItemCodeValue/otherOilSeedCropsNec
<http://lpis.ec.europa.eu/registry/applicationschema/cap-iacs-base/code#CropItemCodeValue/otherOilSeedCropsNec> rdf:type owl:NamedIndividual ,
                                                                                                                         <http://lpis.ec.europa.eu/registry/applicationschema/cap-iacs-base#CropItemCodeValue> ;
                                                                                                                rdfs:label "Other oil seed crops n.e.c. "@en ;
                                                                                                                <http://www.w3.org/2004/02/skos/core#definition> """-- Definition --
|||Other oil seed crops n.e.c. 
-- Description --
Cereals and main crops - C
NOTE. Initial value:C1480"""@en ;
                                                                                                                <http://www.w3.org/2004/02/skos/core#inScheme> :CropItemCodeValue .


###  http://lpis.ec.europa.eu/registry/applicationschema/cap-iacs-base/code#CropItemCodeValue/otherPermanentCrops
<http://lpis.ec.europa.eu/registry/applicationschema/cap-iacs-base/code#CropItemCodeValue/otherPermanentCrops> rdf:type owl:NamedIndividual ,
                                                                                                                        <http://lpis.ec.europa.eu/registry/applicationschema/cap-iacs-base#CropItemCodeValue> ;
                                                                                                               rdfs:label "Other permanent crops"@en ;
                                                                                                               <http://www.w3.org/2004/02/skos/core#definition> """-- Definition --
|||Other permanent crops.
-- Description --
Land use of Agriculture Area in Use -L
NOTE. Initial value:L2980"""@en ;
                                                                                                               <http://www.w3.org/2004/02/skos/core#inScheme> :CropItemCodeValue .


###  http://lpis.ec.europa.eu/registry/applicationschema/cap-iacs-base/code#CropItemCodeValue/otherPotatoes
<http://lpis.ec.europa.eu/registry/applicationschema/cap-iacs-base/code#CropItemCodeValue/otherPotatoes> rdf:type owl:NamedIndividual ,
                                                                                                                  <http://lpis.ec.europa.eu/registry/applicationschema/cap-iacs-base#CropItemCodeValue> ;
                                                                                                         rdfs:label "Other potatoes"@en ;
                                                                                                         <http://www.w3.org/2004/02/skos/core#definition> """-- Definition --
|||Other potatoes.
-- Description --
Cereals and main crops - C
NOTE. Initial value:C1363"""@en ;
                                                                                                         <http://www.w3.org/2004/02/skos/core#inScheme> :CropItemCodeValue .


###  http://lpis.ec.europa.eu/registry/applicationschema/cap-iacs-base/code#CropItemCodeValue/otherPulsesNec
<http://lpis.ec.europa.eu/registry/applicationschema/cap-iacs-base/code#CropItemCodeValue/otherPulsesNec> rdf:type owl:NamedIndividual ,
                                                                                                                   <http://lpis.ec.europa.eu/registry/applicationschema/cap-iacs-base#CropItemCodeValue> ;
                                                                                                          rdfs:label "Other pulses n.e.c."@en ;
                                                                                                          <http://www.w3.org/2004/02/skos/core#definition> """-- Definition --
|||Other pulses n.e.c.
-- Description --
Cereals and main crops - C
NOTE. Initial value:C1905"""@en ;
                                                                                                          <http://www.w3.org/2004/02/skos/core#inScheme> :CropItemCodeValue .


###  http://lpis.ec.europa.eu/registry/applicationschema/cap-iacs-base/code#CropItemCodeValue/otherRootAndTuberVegetablesNec
<http://lpis.ec.europa.eu/registry/applicationschema/cap-iacs-base/code#CropItemCodeValue/otherRootAndTuberVegetablesNec> rdf:type owl:NamedIndividual ,
                                                                                                                                   <http://lpis.ec.europa.eu/registry/applicationschema/cap-iacs-base#CropItemCodeValue> ;
                                                                                                                          rdfs:label "Other root and tuber vegetables n.e.c."@en ;
                                                                                                                          <http://www.w3.org/2004/02/skos/core#definition> """-- Definition --
|||Other root and tuber vegetables n.e.c.
-- Description --
Cereals and main crops - C
NOTE. Initial value:C1884"""@en ;
                                                                                                                          <http://www.w3.org/2004/02/skos/core#inScheme> :CropItemCodeValue .


###  http://lpis.ec.europa.eu/registry/applicationschema/cap-iacs-base/code#CropItemCodeValue/otherRootCropsNec
<http://lpis.ec.europa.eu/registry/applicationschema/cap-iacs-base/code#CropItemCodeValue/otherRootCropsNec> rdf:type owl:NamedIndividual ,
                                                                                                                      <http://lpis.ec.europa.eu/registry/applicationschema/cap-iacs-base#CropItemCodeValue> ;
                                                                                                             rdfs:label "Other root crops n.e.c. "@en ;
                                                                                                             <http://www.w3.org/2004/02/skos/core#definition> """-- Definition --
||Other root crops n.e.c. 
-- Description --
Cereals and main crops - C
NOTE. Initial value:C1380"""@en ;
                                                                                                             <http://www.w3.org/2004/02/skos/core#inScheme> :CropItemCodeValue .


###  http://lpis.ec.europa.eu/registry/applicationschema/cap-iacs-base/code#CropItemCodeValue/otherRootCropsNecL1380
<http://lpis.ec.europa.eu/registry/applicationschema/cap-iacs-base/code#CropItemCodeValue/otherRootCropsNecL1380> rdf:type owl:NamedIndividual ,
                                                                                                                           <http://lpis.ec.europa.eu/registry/applicationschema/cap-iacs-base#CropItemCodeValue> ;
                                                                                                                  rdfs:label "Other root crops n.e.c. L1380"@en ;
                                                                                                                  <http://www.w3.org/2004/02/skos/core#definition> """-- Definition --
||||Other root crops n.e.c. L1380.
-- Description --
Land use of Agriculture Area in Use -L
NOTE. Initial value:L1380"""@en ;
                                                                                                                  <http://www.w3.org/2004/02/skos/core#inScheme> :CropItemCodeValue .


###  http://lpis.ec.europa.eu/registry/applicationschema/cap-iacs-base/code#CropItemCodeValue/otherStoneFruitsNec
<http://lpis.ec.europa.eu/registry/applicationschema/cap-iacs-base/code#CropItemCodeValue/otherStoneFruitsNec> rdf:type owl:NamedIndividual ,
                                                                                                                        <http://lpis.ec.europa.eu/registry/applicationschema/cap-iacs-base#CropItemCodeValue> ;
                                                                                                               rdfs:label "Other stone fruits n.e.c."@en ;
                                                                                                               <http://www.w3.org/2004/02/skos/core#definition> """-- Definition --
|||Other stone fruits n.e.c.
-- Description --
Cereals and main crops - C
NOTE. Initial value:C2229"""@en ;
                                                                                                               <http://www.w3.org/2004/02/skos/core#inScheme> :CropItemCodeValue .


###  http://lpis.ec.europa.eu/registry/applicationschema/cap-iacs-base/code#CropItemCodeValue/otherUtilisedAgriculturalArea
<http://lpis.ec.europa.eu/registry/applicationschema/cap-iacs-base/code#CropItemCodeValue/otherUtilisedAgriculturalArea> rdf:type owl:NamedIndividual ,
                                                                                                                                  <http://lpis.ec.europa.eu/registry/applicationschema/cap-iacs-base#CropItemCodeValue> ;
                                                                                                                         rdfs:label "Other utilised agricultural area"@en ;
                                                                                                                         <http://www.w3.org/2004/02/skos/core#definition> """-- Definition --
||Other utilised agricultural area.
-- Description --
Land use of Agriculture Area in Use -L
NOTE. Initial value:L2990"""@en ;
                                                                                                                         <http://www.w3.org/2004/02/skos/core#inScheme> :CropItemCodeValue .


###  http://lpis.ec.europa.eu/registry/applicationschema/cap-iacs-base/code#CropItemCodeValue/otherVegetablesCultivatedForFruitNec
<http://lpis.ec.europa.eu/registry/applicationschema/cap-iacs-base/code#CropItemCodeValue/otherVegetablesCultivatedForFruitNec> rdf:type owl:NamedIndividual ,
                                                                                                                                         <http://lpis.ec.europa.eu/registry/applicationschema/cap-iacs-base#CropItemCodeValue> ;
                                                                                                                                rdfs:label "Other vegetables cultivated for fruit n.e.c."@en ;
                                                                                                                                <http://www.w3.org/2004/02/skos/core#definition> """-- Definition --
|||Other vegetables cultivated for fruit n.e.c.
-- Description --
Cereals and main crops - C
NOTE. Initial value:C1799"""@en ;
                                                                                                                                <http://www.w3.org/2004/02/skos/core#inScheme> :CropItemCodeValue .


###  http://lpis.ec.europa.eu/registry/applicationschema/cap-iacs-base/code#CropItemCodeValue/peaches
<http://lpis.ec.europa.eu/registry/applicationschema/cap-iacs-base/code#CropItemCodeValue/peaches> rdf:type owl:NamedIndividual ,
                                                                                                            <http://lpis.ec.europa.eu/registry/applicationschema/cap-iacs-base#CropItemCodeValue> ;
                                                                                                   rdfs:label "Peaches"@en ;
                                                                                                   <http://www.w3.org/2004/02/skos/core#definition> """-- Definition --
|||Peaches.
-- Description --
Cereals and main crops - C
NOTE. Initial value:C2180"""@en ;
                                                                                                   <http://www.w3.org/2004/02/skos/core#inScheme> :CropItemCodeValue .


###  http://lpis.ec.europa.eu/registry/applicationschema/cap-iacs-base/code#CropItemCodeValue/pears
<http://lpis.ec.europa.eu/registry/applicationschema/cap-iacs-base/code#CropItemCodeValue/pears> rdf:type owl:NamedIndividual ,
                                                                                                          <http://lpis.ec.europa.eu/registry/applicationschema/cap-iacs-base#CropItemCodeValue> ;
                                                                                                 rdfs:label "Pears"@en ;
                                                                                                 <http://www.w3.org/2004/02/skos/core#definition> """-- Definition --
||Pears.
-- Description --
Cereals and main crops - C
NOTE. Initial value:C2095"""@en ;
                                                                                                 <http://www.w3.org/2004/02/skos/core#inScheme> :CropItemCodeValue .


###  http://lpis.ec.europa.eu/registry/applicationschema/cap-iacs-base/code#CropItemCodeValue/pearsForFreshConsumption
<http://lpis.ec.europa.eu/registry/applicationschema/cap-iacs-base/code#CropItemCodeValue/pearsForFreshConsumption> rdf:type owl:NamedIndividual ,
                                                                                                                             <http://lpis.ec.europa.eu/registry/applicationschema/cap-iacs-base#CropItemCodeValue> ;
                                                                                                                    rdfs:label "Pears for fresh consumption"@en ;
                                                                                                                    <http://www.w3.org/2004/02/skos/core#definition> """-- Definition --
|||Pears for fresh consumption.
-- Description --
Cereals and main crops - C
NOTE. Initial value:C2130"""@en ;
                                                                                                                    <http://www.w3.org/2004/02/skos/core#inScheme> :CropItemCodeValue .


###  http://lpis.ec.europa.eu/registry/applicationschema/cap-iacs-base/code#CropItemCodeValue/peas
<http://lpis.ec.europa.eu/registry/applicationschema/cap-iacs-base/code#CropItemCodeValue/peas> rdf:type owl:NamedIndividual ,
                                                                                                         <http://lpis.ec.europa.eu/registry/applicationschema/cap-iacs-base#CropItemCodeValue> ;
                                                                                                rdfs:label "Peas"@en ;
                                                                                                <http://www.w3.org/2004/02/skos/core#definition> """-- Definition --
|||Peas.
-- Description --
Cereals and main crops - C
NOTE. Initial value:C1890"""@en ;
                                                                                                <http://www.w3.org/2004/02/skos/core#inScheme> :CropItemCodeValue .


###  http://lpis.ec.europa.eu/registry/applicationschema/cap-iacs-base/code#CropItemCodeValue/permanentCrops
<http://lpis.ec.europa.eu/registry/applicationschema/cap-iacs-base/code#CropItemCodeValue/permanentCrops> rdf:type owl:NamedIndividual ,
                                                                                                                   <http://lpis.ec.europa.eu/registry/applicationschema/cap-iacs-base#CropItemCodeValue> ;
                                                                                                          rdfs:label "Permanent crops"@en ;
                                                                                                          <http://www.w3.org/2004/02/skos/core#definition> """-- Definition --
|Permanent crops.
-- Description --
Cereals and main crops - C
NOTE. Initial value:C2007"""@en ;
                                                                                                          <http://www.w3.org/2004/02/skos/core#inScheme> :CropItemCodeValue .


###  http://lpis.ec.europa.eu/registry/applicationschema/cap-iacs-base/code#CropItemCodeValue/permanentCropsL0003
<http://lpis.ec.europa.eu/registry/applicationschema/cap-iacs-base/code#CropItemCodeValue/permanentCropsL0003> rdf:type owl:NamedIndividual ,
                                                                                                                        <http://lpis.ec.europa.eu/registry/applicationschema/cap-iacs-base#CropItemCodeValue> ;
                                                                                                               rdfs:label "Permanent crops L0003"@en ;
                                                                                                               <http://www.w3.org/2004/02/skos/core#definition> """-- Definition --
||Permanent crops L0003.
-- Description --
Land use of Agriculture Area in Use -L
NOTE. Initial value:L0003"""@en ;
                                                                                                               <http://www.w3.org/2004/02/skos/core#inScheme> :CropItemCodeValue .


###  http://lpis.ec.europa.eu/registry/applicationschema/cap-iacs-base/code#CropItemCodeValue/permanentCropsUnderGlassOrHighAccessibleCover
<http://lpis.ec.europa.eu/registry/applicationschema/cap-iacs-base/code#CropItemCodeValue/permanentCropsUnderGlassOrHighAccessibleCover> rdf:type owl:NamedIndividual ,
                                                                                                                                                  <http://lpis.ec.europa.eu/registry/applicationschema/cap-iacs-base#CropItemCodeValue> ;
                                                                                                                                         rdfs:label "Permanent crops under glass or high accessible cover"@en ;
                                                                                                                                         <http://www.w3.org/2004/02/skos/core#definition> """-- Definition --
Permanent crops under glass or high accessible cover.
-- Description --
Land use of Agriculture Area in Use -L. Special aggregates
NOTE. Initial value:L1114"""@en ;
                                                                                                                                         <http://www.w3.org/2004/02/skos/core#inScheme> :CropItemCodeValue .


###  http://lpis.ec.europa.eu/registry/applicationschema/cap-iacs-base/code#CropItemCodeValue/permanentGrassland
<http://lpis.ec.europa.eu/registry/applicationschema/cap-iacs-base/code#CropItemCodeValue/permanentGrassland> rdf:type owl:NamedIndividual ,
                                                                                                                       <http://lpis.ec.europa.eu/registry/applicationschema/cap-iacs-base#CropItemCodeValue> ;
                                                                                                              rdfs:label "Permanent grassland"@en ;
                                                                                                              <http://www.w3.org/2004/02/skos/core#definition> """-- Definition --
||Permanent grassland.
-- Description --
Land use of Agriculture Area in Use -L
NOTE. Initial value:L0002"""@en ;
                                                                                                              <http://www.w3.org/2004/02/skos/core#inScheme> :CropItemCodeValue .


###  http://lpis.ec.europa.eu/registry/applicationschema/cap-iacs-base/code#CropItemCodeValue/permanentGrasslandPasturesAndMeadows
<http://lpis.ec.europa.eu/registry/applicationschema/cap-iacs-base/code#CropItemCodeValue/permanentGrasslandPasturesAndMeadows> rdf:type owl:NamedIndividual ,
                                                                                                                                         <http://lpis.ec.europa.eu/registry/applicationschema/cap-iacs-base#CropItemCodeValue> ;
                                                                                                                                rdfs:label "Permanent grassland (pastures and meadows)"@en ;
                                                                                                                                <http://www.w3.org/2004/02/skos/core#definition> """-- Definition --
|Permanent grassland (pastures and meadows).
-- Description --
Cereals and main crops - C
NOTE. Initial value:C0002"""@en ;
                                                                                                                                <http://www.w3.org/2004/02/skos/core#inScheme> :CropItemCodeValue .


###  http://lpis.ec.europa.eu/registry/applicationschema/cap-iacs-base/code#CropItemCodeValue/plantsHarvestedGreenC2610
<http://lpis.ec.europa.eu/registry/applicationschema/cap-iacs-base/code#CropItemCodeValue/plantsHarvestedGreenC2610> rdf:type owl:NamedIndividual ,
                                                                                                                              <http://lpis.ec.europa.eu/registry/applicationschema/cap-iacs-base#CropItemCodeValue> ;
                                                                                                                     rdfs:label "Plants harvested green C2610 "@en ;
                                                                                                                     <http://www.w3.org/2004/02/skos/core#definition> """-- Definition --
|Plants harvested green C2610.
-- Description --
Cereals and main crops - C
NOTE. Initial value:C2610"""@en ;
                                                                                                                     <http://www.w3.org/2004/02/skos/core#inScheme> :CropItemCodeValue .


###  http://lpis.ec.europa.eu/registry/applicationschema/cap-iacs-base/code#CropItemCodeValue/plantsHarvestedGreenGrownOnArableLand
<http://lpis.ec.europa.eu/registry/applicationschema/cap-iacs-base/code#CropItemCodeValue/plantsHarvestedGreenGrownOnArableLand> rdf:type owl:NamedIndividual ,
                                                                                                                                          <http://lpis.ec.europa.eu/registry/applicationschema/cap-iacs-base#CropItemCodeValue> ;
                                                                                                                                 rdfs:label "Plants harvested green (grown on arable land)"@en ;
                                                                                                                                 <http://www.w3.org/2004/02/skos/core#definition> """-- Definition --
|||Plants harvested green (grown on arable land).
-- Description --
Land use of Agriculture Area in Use -L
NOTE. Initial value:L2610"""@en ;
                                                                                                                                 <http://www.w3.org/2004/02/skos/core#inScheme> :CropItemCodeValue .


###  http://lpis.ec.europa.eu/registry/applicationschema/cap-iacs-base/code#CropItemCodeValue/plums
<http://lpis.ec.europa.eu/registry/applicationschema/cap-iacs-base/code#CropItemCodeValue/plums> rdf:type owl:NamedIndividual ,
                                                                                                          <http://lpis.ec.europa.eu/registry/applicationschema/cap-iacs-base#CropItemCodeValue> ;
                                                                                                 rdfs:label "Plums"@en ;
                                                                                                 <http://www.w3.org/2004/02/skos/core#definition> """-- Definition --
|||Plums.
-- Description --
Cereals and main crops - C
NOTE. Initial value:C2210"""@en ;
                                                                                                 <http://www.w3.org/2004/02/skos/core#inScheme> :CropItemCodeValue .


###  http://lpis.ec.europa.eu/registry/applicationschema/cap-iacs-base/code#CropItemCodeValue/pomelosAndGrapefruitC2380
<http://lpis.ec.europa.eu/registry/applicationschema/cap-iacs-base/code#CropItemCodeValue/pomelosAndGrapefruitC2380> rdf:type owl:NamedIndividual ,
                                                                                                                              <http://lpis.ec.europa.eu/registry/applicationschema/cap-iacs-base#CropItemCodeValue> ;
                                                                                                                     rdfs:label "Pomelos and grapefruit C2380"@en ;
                                                                                                                     <http://www.w3.org/2004/02/skos/core#definition> """-- Definition --
|||Pomelos and grapefruit C2380.
-- Description --
Cereals and main crops - C
NOTE. Initial value:C2380"""@en ;
                                                                                                                     <http://www.w3.org/2004/02/skos/core#inScheme> :CropItemCodeValue .


###  http://lpis.ec.europa.eu/registry/applicationschema/cap-iacs-base/code#CropItemCodeValue/potatoesIncludingEarlyPotatoesAndSeedPotatoes
<http://lpis.ec.europa.eu/registry/applicationschema/cap-iacs-base/code#CropItemCodeValue/potatoesIncludingEarlyPotatoesAndSeedPotatoes> rdf:type owl:NamedIndividual ,
                                                                                                                                                  <http://lpis.ec.europa.eu/registry/applicationschema/cap-iacs-base#CropItemCodeValue> ;
                                                                                                                                         rdfs:label "Potatoes (including early potatoes and seed potatoes)"@en ;
                                                                                                                                         <http://www.w3.org/2004/02/skos/core#definition> """-- Definition --
||Potatoes (including early potatoes and seed potatoes).
-- Description --
Cereals and main crops - C
NOTE. Initial value:C1360"""@en ;
                                                                                                                                         <http://www.w3.org/2004/02/skos/core#inScheme> :CropItemCodeValue .


###  http://lpis.ec.europa.eu/registry/applicationschema/cap-iacs-base/code#CropItemCodeValue/potatoesIncludingEarlyPotatoesAndSeedPotatoesL1360
<http://lpis.ec.europa.eu/registry/applicationschema/cap-iacs-base/code#CropItemCodeValue/potatoesIncludingEarlyPotatoesAndSeedPotatoesL1360> rdf:type owl:NamedIndividual ,
                                                                                                                                                       <http://lpis.ec.europa.eu/registry/applicationschema/cap-iacs-base#CropItemCodeValue> ;
                                                                                                                                              rdfs:label "Potatoes (including early potatoes and seed potatoes) L1360"@en ;
                                                                                                                                              <http://www.w3.org/2004/02/skos/core#definition> """-- Definition --
||||Potatoes (including early potatoes and seed potatoes) L1360.
-- Description --
Land use of Agriculture Area in Use -L
NOTE. Initial value:L1360"""@en ;
                                                                                                                                              <http://www.w3.org/2004/02/skos/core#inScheme> :CropItemCodeValue .


###  http://lpis.ec.europa.eu/registry/applicationschema/cap-iacs-base/code#CropItemCodeValue/pulses
<http://lpis.ec.europa.eu/registry/applicationschema/cap-iacs-base/code#CropItemCodeValue/pulses> rdf:type owl:NamedIndividual ,
                                                                                                           <http://lpis.ec.europa.eu/registry/applicationschema/cap-iacs-base#CropItemCodeValue> ;
                                                                                                  rdfs:label "Pulses"@en ;
                                                                                                  <http://www.w3.org/2004/02/skos/core#definition> """-- Definition --
||Pulses.
-- Description --
Cereals and main crops - C
NOTE. Initial value:C1885"""@en ;
                                                                                                  <http://www.w3.org/2004/02/skos/core#inScheme> :CropItemCodeValue .


###  http://lpis.ec.europa.eu/registry/applicationschema/cap-iacs-base/code#CropItemCodeValue/quinces
<http://lpis.ec.europa.eu/registry/applicationschema/cap-iacs-base/code#CropItemCodeValue/quinces> rdf:type owl:NamedIndividual ,
                                                                                                            <http://lpis.ec.europa.eu/registry/applicationschema/cap-iacs-base#CropItemCodeValue> ;
                                                                                                   rdfs:label "Quinces"@en ;
                                                                                                   <http://www.w3.org/2004/02/skos/core#definition> """-- Definition --
|||Quinces.
-- Description --
Cereals and main crops - C
NOTE. Initial value:C2252"""@en ;
                                                                                                   <http://www.w3.org/2004/02/skos/core#inScheme> :CropItemCodeValue .


###  http://lpis.ec.europa.eu/registry/applicationschema/cap-iacs-base/code#CropItemCodeValue/radishes
<http://lpis.ec.europa.eu/registry/applicationschema/cap-iacs-base/code#CropItemCodeValue/radishes> rdf:type owl:NamedIndividual ,
                                                                                                             <http://lpis.ec.europa.eu/registry/applicationschema/cap-iacs-base#CropItemCodeValue> ;
                                                                                                    rdfs:label "Radishes"@en ;
                                                                                                    <http://www.w3.org/2004/02/skos/core#definition> """-- Definition --
|||Radishes.
-- Description --
Cereals and main crops - C
NOTE. Initial value:C1877"""@en ;
                                                                                                    <http://www.w3.org/2004/02/skos/core#inScheme> :CropItemCodeValue .


###  http://lpis.ec.europa.eu/registry/applicationschema/cap-iacs-base/code#CropItemCodeValue/rape
<http://lpis.ec.europa.eu/registry/applicationschema/cap-iacs-base/code#CropItemCodeValue/rape> rdf:type owl:NamedIndividual ,
                                                                                                         <http://lpis.ec.europa.eu/registry/applicationschema/cap-iacs-base#CropItemCodeValue> ;
                                                                                                rdfs:label "Rape"@en ;
                                                                                                <http://www.w3.org/2004/02/skos/core#definition> """-- Definition --
|||||Rape.
-- Description --
Cereals and main crops - C
NOTE. Initial value:C1430"""@en ;
                                                                                                <http://www.w3.org/2004/02/skos/core#inScheme> :CropItemCodeValue .


###  http://lpis.ec.europa.eu/registry/applicationschema/cap-iacs-base/code#CropItemCodeValue/rapeAndTurnipRape
<http://lpis.ec.europa.eu/registry/applicationschema/cap-iacs-base/code#CropItemCodeValue/rapeAndTurnipRape> rdf:type owl:NamedIndividual ,
                                                                                                                      <http://lpis.ec.europa.eu/registry/applicationschema/cap-iacs-base#CropItemCodeValue> ;
                                                                                                             rdfs:label "Rape and turnip rape"@en ;
                                                                                                             <http://www.w3.org/2004/02/skos/core#definition> """-- Definition --
||||Rape and turnip rape.
-- Description --
Cereals and main crops - C
NOTE. Initial value:C1420"""@en ;
                                                                                                             <http://www.w3.org/2004/02/skos/core#inScheme> :CropItemCodeValue .


###  http://lpis.ec.europa.eu/registry/applicationschema/cap-iacs-base/code#CropItemCodeValue/raspberries
<http://lpis.ec.europa.eu/registry/applicationschema/cap-iacs-base/code#CropItemCodeValue/raspberries> rdf:type owl:NamedIndividual ,
                                                                                                                <http://lpis.ec.europa.eu/registry/applicationschema/cap-iacs-base#CropItemCodeValue> ;
                                                                                                       rdfs:label "Raspberries"@en ;
                                                                                                       <http://www.w3.org/2004/02/skos/core#definition> """-- Definition --
|||Raspberries.
-- Description --
Cereals and main crops - C
NOTE. Initial value:C2278"""@en ;
                                                                                                       <http://www.w3.org/2004/02/skos/core#inScheme> :CropItemCodeValue .


###  http://lpis.ec.europa.eu/registry/applicationschema/cap-iacs-base/code#CropItemCodeValue/redCurrants
<http://lpis.ec.europa.eu/registry/applicationschema/cap-iacs-base/code#CropItemCodeValue/redCurrants> rdf:type owl:NamedIndividual ,
                                                                                                                <http://lpis.ec.europa.eu/registry/applicationschema/cap-iacs-base#CropItemCodeValue> ;
                                                                                                       rdfs:label "Red currants"@en ;
                                                                                                       <http://www.w3.org/2004/02/skos/core#definition> """-- Definition --
||||Red currants.
-- Description --
Cereals and main crops - C
NOTE. Initial value:C2275"""@en ;
                                                                                                       <http://www.w3.org/2004/02/skos/core#inScheme> :CropItemCodeValue .


###  http://lpis.ec.europa.eu/registry/applicationschema/cap-iacs-base/code#CropItemCodeValue/redPepperCapsicum
<http://lpis.ec.europa.eu/registry/applicationschema/cap-iacs-base/code#CropItemCodeValue/redPepperCapsicum> rdf:type owl:NamedIndividual ,
                                                                                                                      <http://lpis.ec.europa.eu/registry/applicationschema/cap-iacs-base#CropItemCodeValue> ;
                                                                                                             rdfs:label "Red pepper, capsicum"@en ;
                                                                                                             <http://www.w3.org/2004/02/skos/core#definition> """-- Definition --
|||Red pepper, capsicum.
-- Description --
Cereals and main crops - C
NOTE. Initial value:C1790"""@en ;
                                                                                                             <http://www.w3.org/2004/02/skos/core#inScheme> :CropItemCodeValue .


###  http://lpis.ec.europa.eu/registry/applicationschema/cap-iacs-base/code#CropItemCodeValue/redPepperCapsicumUnderGlassOrHighAccessibleCoverC1791
<http://lpis.ec.europa.eu/registry/applicationschema/cap-iacs-base/code#CropItemCodeValue/redPepperCapsicumUnderGlassOrHighAccessibleCoverC1791> rdf:type owl:NamedIndividual ,
                                                                                                                                                          <http://lpis.ec.europa.eu/registry/applicationschema/cap-iacs-base#CropItemCodeValue> ;
                                                                                                                                                 rdfs:label "Red pepper, capsicum under glass or high accessible cover C1791"@en ;
                                                                                                                                                 <http://www.w3.org/2004/02/skos/core#definition> """-- Definition --
||||Red pepper, capsicum under glass or high accessible cover C1791.
-- Description --
Cereals and main crops - C
NOTE. Initial value:C1791"""@en ;
                                                                                                                                                 <http://www.w3.org/2004/02/skos/core#inScheme> :CropItemCodeValue .


###  http://lpis.ec.europa.eu/registry/applicationschema/cap-iacs-base/code#CropItemCodeValue/rice
<http://lpis.ec.europa.eu/registry/applicationschema/cap-iacs-base/code#CropItemCodeValue/rice> rdf:type owl:NamedIndividual ,
                                                                                                         <http://lpis.ec.europa.eu/registry/applicationschema/cap-iacs-base#CropItemCodeValue> ;
                                                                                                rdfs:label "Rice "@en ;
                                                                                                <http://www.w3.org/2004/02/skos/core#definition> """-- Definition --
||Rice.
-- Description --
Cereals and main crops - C
NOTE. Initial value:C1250"""@en ;
                                                                                                <http://www.w3.org/2004/02/skos/core#inScheme> :CropItemCodeValue .


###  http://lpis.ec.europa.eu/registry/applicationschema/cap-iacs-base/code#CropItemCodeValue/riceIndica
<http://lpis.ec.europa.eu/registry/applicationschema/cap-iacs-base/code#CropItemCodeValue/riceIndica> rdf:type owl:NamedIndividual ,
                                                                                                               <http://lpis.ec.europa.eu/registry/applicationschema/cap-iacs-base#CropItemCodeValue> ;
                                                                                                      rdfs:label "Rice Indica "@en ;
                                                                                                      <http://www.w3.org/2004/02/skos/core#definition> """-- Definition --
|||Rice Indica.
-- Description --
Cereals and main crops - C
NOTE. Initial value:C1251"""@en ;
                                                                                                      <http://www.w3.org/2004/02/skos/core#inScheme> :CropItemCodeValue .


###  http://lpis.ec.europa.eu/registry/applicationschema/cap-iacs-base/code#CropItemCodeValue/riceJaponica
<http://lpis.ec.europa.eu/registry/applicationschema/cap-iacs-base/code#CropItemCodeValue/riceJaponica> rdf:type owl:NamedIndividual ,
                                                                                                                 <http://lpis.ec.europa.eu/registry/applicationschema/cap-iacs-base#CropItemCodeValue> ;
                                                                                                        rdfs:label "Rice Japonica"@en ;
                                                                                                        <http://www.w3.org/2004/02/skos/core#definition> """-- Definition --
|||Rice Japonica.
-- Description --
Cereals and main crops - C
NOTE. Initial value:C1252"""@en ;
                                                                                                        <http://www.w3.org/2004/02/skos/core#inScheme> :CropItemCodeValue .


###  http://lpis.ec.europa.eu/registry/applicationschema/cap-iacs-base/code#CropItemCodeValue/riceOp
<http://lpis.ec.europa.eu/registry/applicationschema/cap-iacs-base/code#CropItemCodeValue/riceOp> rdf:type owl:NamedIndividual ,
                                                                                                           <http://lpis.ec.europa.eu/registry/applicationschema/cap-iacs-base#CropItemCodeValue> ;
                                                                                                  rdfs:label "Rice Op"@en ;
                                                                                                  <http://www.w3.org/2004/02/skos/core#definition> """-- Definition --
|||Rice Op.
-- Description --
Land use of Agriculture Area in Use -L
NOTE. Initial value:L1250"""@en ;
                                                                                                  <http://www.w3.org/2004/02/skos/core#inScheme> :CropItemCodeValue .


###  http://lpis.ec.europa.eu/registry/applicationschema/cap-iacs-base/code#CropItemCodeValue/rootAndTuberVegetables
<http://lpis.ec.europa.eu/registry/applicationschema/cap-iacs-base/code#CropItemCodeValue/rootAndTuberVegetables> rdf:type owl:NamedIndividual ,
                                                                                                                           <http://lpis.ec.europa.eu/registry/applicationschema/cap-iacs-base#CropItemCodeValue> ;
                                                                                                                  rdfs:label "Root and tuber vegetables"@en ;
                                                                                                                  <http://www.w3.org/2004/02/skos/core#definition> """-- Definition --
||Root and tuber vegetables.
-- Description --
Cereals and main crops - C
NOTE. Initial value:C1800"""@en ;
                                                                                                                  <http://www.w3.org/2004/02/skos/core#inScheme> :CropItemCodeValue .


###  http://lpis.ec.europa.eu/registry/applicationschema/cap-iacs-base/code#CropItemCodeValue/rootCrops
<http://lpis.ec.europa.eu/registry/applicationschema/cap-iacs-base/code#CropItemCodeValue/rootCrops> rdf:type owl:NamedIndividual ,
                                                                                                              <http://lpis.ec.europa.eu/registry/applicationschema/cap-iacs-base#CropItemCodeValue> ;
                                                                                                     rdfs:label "Root crops"@en ;
                                                                                                     <http://www.w3.org/2004/02/skos/core#definition> """-- Definition --
|Root crops.
-- Description --
Cereals and main crops - C
NOTE. Initial value:C1350"""@en ;
                                                                                                     <http://www.w3.org/2004/02/skos/core#inScheme> :CropItemCodeValue .


###  http://lpis.ec.europa.eu/registry/applicationschema/cap-iacs-base/code#CropItemCodeValue/rootCropsL1350
<http://lpis.ec.europa.eu/registry/applicationschema/cap-iacs-base/code#CropItemCodeValue/rootCropsL1350> rdf:type owl:NamedIndividual ,
                                                                                                                   <http://lpis.ec.europa.eu/registry/applicationschema/cap-iacs-base#CropItemCodeValue> ;
                                                                                                          rdfs:label "Root crops L1350"@en ;
                                                                                                          <http://www.w3.org/2004/02/skos/core#definition> """-- Definition --
|||Root crops L1350.
-- Description --
Land use of Agriculture Area in Use -L
NOTE. Initial value:L1350"""@en ;
                                                                                                          <http://www.w3.org/2004/02/skos/core#inScheme> :CropItemCodeValue .


###  http://lpis.ec.europa.eu/registry/applicationschema/cap-iacs-base/code#CropItemCodeValue/rye
<http://lpis.ec.europa.eu/registry/applicationschema/cap-iacs-base/code#CropItemCodeValue/rye> rdf:type owl:NamedIndividual ,
                                                                                                        <http://lpis.ec.europa.eu/registry/applicationschema/cap-iacs-base#CropItemCodeValue> ;
                                                                                               rdfs:label "Rye"@en ;
                                                                                               <http://www.w3.org/2004/02/skos/core#definition> """-- Definition --
||||Rye.
-- Description --
Cereals and main crops - C
NOTE. Initial value:C1150"""@en ;
                                                                                               <http://www.w3.org/2004/02/skos/core#inScheme> :CropItemCodeValue .


###  http://lpis.ec.europa.eu/registry/applicationschema/cap-iacs-base/code#CropItemCodeValue/ryeAndMaslin
<http://lpis.ec.europa.eu/registry/applicationschema/cap-iacs-base/code#CropItemCodeValue/ryeAndMaslin> rdf:type owl:NamedIndividual ,
                                                                                                                 <http://lpis.ec.europa.eu/registry/applicationschema/cap-iacs-base#CropItemCodeValue> ;
                                                                                                        rdfs:label "Rye and maslin"@en ;
                                                                                                        <http://www.w3.org/2004/02/skos/core#definition> """-- Definition --
|||Rye and maslin.
-- Description --
Cereals and main crops - C
NOTE. Initial value:C1140"""@en ;
                                                                                                        <http://www.w3.org/2004/02/skos/core#inScheme> :CropItemCodeValue .


###  http://lpis.ec.europa.eu/registry/applicationschema/cap-iacs-base/code#CropItemCodeValue/salsifyAndScorzonera
<http://lpis.ec.europa.eu/registry/applicationschema/cap-iacs-base/code#CropItemCodeValue/salsifyAndScorzonera> rdf:type owl:NamedIndividual ,
                                                                                                                         <http://lpis.ec.europa.eu/registry/applicationschema/cap-iacs-base#CropItemCodeValue> ;
                                                                                                                rdfs:label "Salsify and scorzonera"@en ;
                                                                                                                <http://www.w3.org/2004/02/skos/core#definition> """-- Definition --
|||Salsify and scorzonera.
-- Description --
Cereals and main crops - C
NOTE. Initial value:C1870"""@en ;
                                                                                                                <http://www.w3.org/2004/02/skos/core#inScheme> :CropItemCodeValue .


###  http://lpis.ec.europa.eu/registry/applicationschema/cap-iacs-base/code#CropItemCodeValue/satsumas
<http://lpis.ec.europa.eu/registry/applicationschema/cap-iacs-base/code#CropItemCodeValue/satsumas> rdf:type owl:NamedIndividual ,
                                                                                                             <http://lpis.ec.europa.eu/registry/applicationschema/cap-iacs-base#CropItemCodeValue> ;
                                                                                                    rdfs:label "Satsumas"@en ;
                                                                                                    <http://www.w3.org/2004/02/skos/core#definition> """-- Definition --
||||Satsumas.
-- Description --
Cereals and main crops - C
NOTE. Initial value:C2352"""@en ;
                                                                                                    <http://www.w3.org/2004/02/skos/core#inScheme> :CropItemCodeValue .


###  http://lpis.ec.europa.eu/registry/applicationschema/cap-iacs-base/code#CropItemCodeValue/seedsAndSeedlings
<http://lpis.ec.europa.eu/registry/applicationschema/cap-iacs-base/code#CropItemCodeValue/seedsAndSeedlings> rdf:type owl:NamedIndividual ,
                                                                                                                      <http://lpis.ec.europa.eu/registry/applicationschema/cap-iacs-base#CropItemCodeValue> ;
                                                                                                             rdfs:label "Seeds and seedlings"@en ;
                                                                                                             <http://www.w3.org/2004/02/skos/core#definition> """-- Definition --
|||Seeds and seedlings.
-- Description --
Land use of Agriculture Area in Use -L
NOTE. Initial value:L3310"""@en ;
                                                                                                             <http://www.w3.org/2004/02/skos/core#inScheme> :CropItemCodeValue .


###  http://lpis.ec.europa.eu/registry/applicationschema/cap-iacs-base/code#CropItemCodeValue/shallots
<http://lpis.ec.europa.eu/registry/applicationschema/cap-iacs-base/code#CropItemCodeValue/shallots> rdf:type owl:NamedIndividual ,
                                                                                                             <http://lpis.ec.europa.eu/registry/applicationschema/cap-iacs-base#CropItemCodeValue> ;
                                                                                                    rdfs:label "Shallots"@en ;
                                                                                                    <http://www.w3.org/2004/02/skos/core#definition> """-- Definition --
|||Shallots.
-- Description --
Cereals and main crops - C
NOTE. Initial value:C1855"""@en ;
                                                                                                    <http://www.w3.org/2004/02/skos/core#inScheme> :CropItemCodeValue .


###  http://lpis.ec.europa.eu/registry/applicationschema/cap-iacs-base/code#CropItemCodeValue/smallCitrusFruits
<http://lpis.ec.europa.eu/registry/applicationschema/cap-iacs-base/code#CropItemCodeValue/smallCitrusFruits> rdf:type owl:NamedIndividual ,
                                                                                                                      <http://lpis.ec.europa.eu/registry/applicationschema/cap-iacs-base#CropItemCodeValue> ;
                                                                                                             rdfs:label "Small citrus fruits"@en ;
                                                                                                             <http://www.w3.org/2004/02/skos/core#definition> """-- Definition --
|||Small citrus fruits.
-- Description --
Cereals and main crops - C
NOTE. Initial value:C2340"""@en ;
                                                                                                             <http://www.w3.org/2004/02/skos/core#inScheme> :CropItemCodeValue .


###  http://lpis.ec.europa.eu/registry/applicationschema/cap-iacs-base/code#CropItemCodeValue/sorghum
<http://lpis.ec.europa.eu/registry/applicationschema/cap-iacs-base/code#CropItemCodeValue/sorghum> rdf:type owl:NamedIndividual ,
                                                                                                            <http://lpis.ec.europa.eu/registry/applicationschema/cap-iacs-base#CropItemCodeValue> ;
                                                                                                   rdfs:label "Sorghum "@en ;
                                                                                                   <http://www.w3.org/2004/02/skos/core#definition> """-- Definition --
|||Sorghum.
-- Description --
Cereals and main crops - C
NOTE. Initial value:C1211"""@en ;
                                                                                                   <http://www.w3.org/2004/02/skos/core#inScheme> :CropItemCodeValue .


###  http://lpis.ec.europa.eu/registry/applicationschema/cap-iacs-base/code#CropItemCodeValue/sourCherries
<http://lpis.ec.europa.eu/registry/applicationschema/cap-iacs-base/code#CropItemCodeValue/sourCherries> rdf:type owl:NamedIndividual ,
                                                                                                                 <http://lpis.ec.europa.eu/registry/applicationschema/cap-iacs-base#CropItemCodeValue> ;
                                                                                                        rdfs:label "Sour cherries"@en ;
                                                                                                        <http://www.w3.org/2004/02/skos/core#definition> """-- Definition --
||||Sour cherries.
-- Description --
Cereals and main crops - C
NOTE. Initial value:C2201"""@en ;
                                                                                                        <http://www.w3.org/2004/02/skos/core#inScheme> :CropItemCodeValue .


###  http://lpis.ec.europa.eu/registry/applicationschema/cap-iacs-base/code#CropItemCodeValue/soya
<http://lpis.ec.europa.eu/registry/applicationschema/cap-iacs-base/code#CropItemCodeValue/soya> rdf:type owl:NamedIndividual ,
                                                                                                         <http://lpis.ec.europa.eu/registry/applicationschema/cap-iacs-base#CropItemCodeValue> ;
                                                                                                rdfs:label "Soya "@en ;
                                                                                                <http://www.w3.org/2004/02/skos/core#definition> """-- Definition --
||||Soya.
-- Description --
Cereals and main crops - C
NOTE. Initial value:C1470"""@en ;
                                                                                                <http://www.w3.org/2004/02/skos/core#inScheme> :CropItemCodeValue .


###  http://lpis.ec.europa.eu/registry/applicationschema/cap-iacs-base/code#CropItemCodeValue/spinach
<http://lpis.ec.europa.eu/registry/applicationschema/cap-iacs-base/code#CropItemCodeValue/spinach> rdf:type owl:NamedIndividual ,
                                                                                                            <http://lpis.ec.europa.eu/registry/applicationschema/cap-iacs-base#CropItemCodeValue> ;
                                                                                                   rdfs:label "Spinach"@en ;
                                                                                                   <http://www.w3.org/2004/02/skos/core#definition> """-- Definition --
|||Spinach.
-- Description --
Cereals and main crops - C
NOTE. Initial value:C1690"""@en ;
                                                                                                   <http://www.w3.org/2004/02/skos/core#inScheme> :CropItemCodeValue .


###  http://lpis.ec.europa.eu/registry/applicationschema/cap-iacs-base/code#CropItemCodeValue/springBarley
<http://lpis.ec.europa.eu/registry/applicationschema/cap-iacs-base/code#CropItemCodeValue/springBarley> rdf:type owl:NamedIndividual ,
                                                                                                                 <http://lpis.ec.europa.eu/registry/applicationschema/cap-iacs-base#CropItemCodeValue> ;
                                                                                                        rdfs:label "Spring barley"@en ;
                                                                                                        <http://www.w3.org/2004/02/skos/core#definition> """-- Definition --
||||Spring barley.
-- Description --
Cereals and main crops - C
NOTE. Initial value:C1164"""@en ;
                                                                                                        <http://www.w3.org/2004/02/skos/core#inScheme> :CropItemCodeValue .


###  http://lpis.ec.europa.eu/registry/applicationschema/cap-iacs-base/code#CropItemCodeValue/springDurumWheat
<http://lpis.ec.europa.eu/registry/applicationschema/cap-iacs-base/code#CropItemCodeValue/springDurumWheat> rdf:type owl:NamedIndividual ,
                                                                                                                     <http://lpis.ec.europa.eu/registry/applicationschema/cap-iacs-base#CropItemCodeValue> ;
                                                                                                            rdfs:label "Spring durum wheat"@en ;
                                                                                                            <http://www.w3.org/2004/02/skos/core#definition> """-- Definition --
|||||Spring durum wheat.
-- Description --
Cereals and main crops - C
NOTE. Initial value:C1134"""@en ;
                                                                                                            <http://www.w3.org/2004/02/skos/core#inScheme> :CropItemCodeValue .


###  http://lpis.ec.europa.eu/registry/applicationschema/cap-iacs-base/code#CropItemCodeValue/springRape
<http://lpis.ec.europa.eu/registry/applicationschema/cap-iacs-base/code#CropItemCodeValue/springRape> rdf:type owl:NamedIndividual ,
                                                                                                               <http://lpis.ec.europa.eu/registry/applicationschema/cap-iacs-base#CropItemCodeValue> ;
                                                                                                      rdfs:label "Spring rape"@en ;
                                                                                                      <http://www.w3.org/2004/02/skos/core#definition> """-- Definition --
||||||Spring rape.
-- Description --
Cereals and main crops - C
NOTE. Initial value:C1432"""@en ;
                                                                                                      <http://www.w3.org/2004/02/skos/core#inScheme> :CropItemCodeValue .


###  http://lpis.ec.europa.eu/registry/applicationschema/cap-iacs-base/code#CropItemCodeValue/springRye
<http://lpis.ec.europa.eu/registry/applicationschema/cap-iacs-base/code#CropItemCodeValue/springRye> rdf:type owl:NamedIndividual ,
                                                                                                              <http://lpis.ec.europa.eu/registry/applicationschema/cap-iacs-base#CropItemCodeValue> ;
                                                                                                     rdfs:label "Spring rye"@en ;
                                                                                                     <http://www.w3.org/2004/02/skos/core#definition> """-- Definition --
|||||Spring rye.
-- Description --
Cereals and main crops - C
NOTE. Initial value:C1152"""@en ;
                                                                                                     <http://www.w3.org/2004/02/skos/core#inScheme> :CropItemCodeValue .


###  http://lpis.ec.europa.eu/registry/applicationschema/cap-iacs-base/code#CropItemCodeValue/stoneFruits
<http://lpis.ec.europa.eu/registry/applicationschema/cap-iacs-base/code#CropItemCodeValue/stoneFruits> rdf:type owl:NamedIndividual ,
                                                                                                                <http://lpis.ec.europa.eu/registry/applicationschema/cap-iacs-base#CropItemCodeValue> ;
                                                                                                       rdfs:label "Stone fruits"@en ;
                                                                                                       <http://www.w3.org/2004/02/skos/core#definition> """-- Definition --
||Stone fruits.
-- Description --
Cereals and main crops - C
NOTE. Initial value:C2170"""@en ;
                                                                                                       <http://www.w3.org/2004/02/skos/core#inScheme> :CropItemCodeValue .


###  http://lpis.ec.europa.eu/registry/applicationschema/cap-iacs-base/code#CropItemCodeValue/strawberries
<http://lpis.ec.europa.eu/registry/applicationschema/cap-iacs-base/code#CropItemCodeValue/strawberries> rdf:type owl:NamedIndividual ,
                                                                                                                 <http://lpis.ec.europa.eu/registry/applicationschema/cap-iacs-base#CropItemCodeValue> ;
                                                                                                        rdfs:label "Strawberries"@en ;
                                                                                                        <http://www.w3.org/2004/02/skos/core#definition> """-- Definition --
||Strawberries.
-- Description --
Cereals and main crops - C
NOTE. Initial value:C2260"""@en ;
                                                                                                        <http://www.w3.org/2004/02/skos/core#inScheme> :CropItemCodeValue .


###  http://lpis.ec.europa.eu/registry/applicationschema/cap-iacs-base/code#CropItemCodeValue/strawberriesUnderGlassOrHighAccessibleCoverC2261
<http://lpis.ec.europa.eu/registry/applicationschema/cap-iacs-base/code#CropItemCodeValue/strawberriesUnderGlassOrHighAccessibleCoverC2261> rdf:type owl:NamedIndividual ,
                                                                                                                                                     <http://lpis.ec.europa.eu/registry/applicationschema/cap-iacs-base#CropItemCodeValue> ;
                                                                                                                                            rdfs:label "Strawberries under glass or high accessible cover C2261 "@en ;
                                                                                                                                            <http://www.w3.org/2004/02/skos/core#definition> """-- Definition --
|||Strawberries under glass or high accessible cover C2261.
-- Description --
Cereals and main crops - C
NOTE. Initial value:C2261"""@en ;
                                                                                                                                            <http://www.w3.org/2004/02/skos/core#inScheme> :CropItemCodeValue .


###  http://lpis.ec.europa.eu/registry/applicationschema/cap-iacs-base/code#CropItemCodeValue/sugarBeetExcludingSeed
<http://lpis.ec.europa.eu/registry/applicationschema/cap-iacs-base/code#CropItemCodeValue/sugarBeetExcludingSeed> rdf:type owl:NamedIndividual ,
                                                                                                                           <http://lpis.ec.europa.eu/registry/applicationschema/cap-iacs-base#CropItemCodeValue> ;
                                                                                                                  rdfs:label "Sugar beet (excluding seed)"@en ;
                                                                                                                  <http://www.w3.org/2004/02/skos/core#definition> """-- Definition --
||Sugar beet (excluding seed).
-- Description --
Cereals and main crops - C
NOTE. Initial value:C1370"""@en ;
                                                                                                                  <http://www.w3.org/2004/02/skos/core#inScheme> :CropItemCodeValue .


###  http://lpis.ec.europa.eu/registry/applicationschema/cap-iacs-base/code#CropItemCodeValue/sugarBeetExcludingSeedL1370
<http://lpis.ec.europa.eu/registry/applicationschema/cap-iacs-base/code#CropItemCodeValue/sugarBeetExcludingSeedL1370> rdf:type owl:NamedIndividual ,
                                                                                                                                <http://lpis.ec.europa.eu/registry/applicationschema/cap-iacs-base#CropItemCodeValue> ;
                                                                                                                       rdfs:label "Sugar beet (excluding seed) L1370"@en ;
                                                                                                                       <http://www.w3.org/2004/02/skos/core#definition> """-- Definition --
||||Sugar beet (excluding seed) L1370.
-- Description --
Land use of Agriculture Area in Use -L
NOTE. Initial value:L1370"""@en ;
                                                                                                                       <http://www.w3.org/2004/02/skos/core#inScheme> :CropItemCodeValue .


###  http://lpis.ec.europa.eu/registry/applicationschema/cap-iacs-base/code#CropItemCodeValue/sunflowerSeed
<http://lpis.ec.europa.eu/registry/applicationschema/cap-iacs-base/code#CropItemCodeValue/sunflowerSeed> rdf:type owl:NamedIndividual ,
                                                                                                                  <http://lpis.ec.europa.eu/registry/applicationschema/cap-iacs-base#CropItemCodeValue> ;
                                                                                                         rdfs:label "Sunflower seed "@en ;
                                                                                                         <http://www.w3.org/2004/02/skos/core#definition> """-- Definition --
||||Sunflower seed.
-- Description --
Cereals and main crops - C
NOTE. Initial value:C1450"""@en ;
                                                                                                         <http://www.w3.org/2004/02/skos/core#inScheme> :CropItemCodeValue .


###  http://lpis.ec.europa.eu/registry/applicationschema/cap-iacs-base/code#CropItemCodeValue/sweetLupinsC1343
<http://lpis.ec.europa.eu/registry/applicationschema/cap-iacs-base/code#CropItemCodeValue/sweetLupinsC1343> rdf:type owl:NamedIndividual ,
                                                                                                                     <http://lpis.ec.europa.eu/registry/applicationschema/cap-iacs-base#CropItemCodeValue> ;
                                                                                                            rdfs:label "Sweet lupins C1343"@en ;
                                                                                                            <http://www.w3.org/2004/02/skos/core#definition> """-- Definition --
||Sweet lupins C1343.
-- Description --
Cereals and main crops - C
NOTE. Initial value:C1343"""@en ;
                                                                                                            <http://www.w3.org/2004/02/skos/core#inScheme> :CropItemCodeValue .


###  http://lpis.ec.europa.eu/registry/applicationschema/cap-iacs-base/code#CropItemCodeValue/temporaryGrassesAndGrazing
<http://lpis.ec.europa.eu/registry/applicationschema/cap-iacs-base/code#CropItemCodeValue/temporaryGrassesAndGrazing> rdf:type owl:NamedIndividual ,
                                                                                                                               <http://lpis.ec.europa.eu/registry/applicationschema/cap-iacs-base#CropItemCodeValue> ;
                                                                                                                      rdfs:label "Temporary grasses and grazing "@en ;
                                                                                                                      <http://www.w3.org/2004/02/skos/core#definition> """-- Definition --
||Temporary grasses and grazing.
-- Description --
Cereals and main crops - C
NOTE. Initial value:C2680"""@en ;
                                                                                                                      <http://www.w3.org/2004/02/skos/core#inScheme> :CropItemCodeValue .


###  http://lpis.ec.europa.eu/registry/applicationschema/cap-iacs-base/code#CropItemCodeValue/tobacco
<http://lpis.ec.europa.eu/registry/applicationschema/cap-iacs-base/code#CropItemCodeValue/tobacco> rdf:type owl:NamedIndividual ,
                                                                                                            <http://lpis.ec.europa.eu/registry/applicationschema/cap-iacs-base#CropItemCodeValue> ;
                                                                                                   rdfs:label "Tobacco"@en ;
                                                                                                   <http://www.w3.org/2004/02/skos/core#definition> """-- Definition --
||Tobacco.
-- Description --
Cereals and main crops - C
NOTE. Initial value:C1550"""@en ;
                                                                                                   <http://www.w3.org/2004/02/skos/core#inScheme> :CropItemCodeValue .


###  http://lpis.ec.europa.eu/registry/applicationschema/cap-iacs-base/code#CropItemCodeValue/tomatoes
<http://lpis.ec.europa.eu/registry/applicationschema/cap-iacs-base/code#CropItemCodeValue/tomatoes> rdf:type owl:NamedIndividual ,
                                                                                                             <http://lpis.ec.europa.eu/registry/applicationschema/cap-iacs-base#CropItemCodeValue> ;
                                                                                                    rdfs:label "Tomatoes"@en ;
                                                                                                    <http://www.w3.org/2004/02/skos/core#definition> """-- Definition --
|||Tomatoes.
-- Description --
Cereals and main crops - C
NOTE. Initial value:C1750"""@en ;
                                                                                                    <http://www.w3.org/2004/02/skos/core#inScheme> :CropItemCodeValue .


###  http://lpis.ec.europa.eu/registry/applicationschema/cap-iacs-base/code#CropItemCodeValue/tomatoesForFreshConsumption
<http://lpis.ec.europa.eu/registry/applicationschema/cap-iacs-base/code#CropItemCodeValue/tomatoesForFreshConsumption> rdf:type owl:NamedIndividual ,
                                                                                                                                <http://lpis.ec.europa.eu/registry/applicationschema/cap-iacs-base#CropItemCodeValue> ;
                                                                                                                       rdfs:label "Tomatoes for fresh consumption"@en ;
                                                                                                                       <http://www.w3.org/2004/02/skos/core#definition> """-- Definition --
||||Tomatoes for fresh consumption.
-- Description --
Cereals and main crops - C
NOTE. Initial value:C1751"""@en ;
                                                                                                                       <http://www.w3.org/2004/02/skos/core#inScheme> :CropItemCodeValue .


###  http://lpis.ec.europa.eu/registry/applicationschema/cap-iacs-base/code#CropItemCodeValue/tomatoesForFreshConsumptionUnderGlassOrHighAccessibleCover
<http://lpis.ec.europa.eu/registry/applicationschema/cap-iacs-base/code#CropItemCodeValue/tomatoesForFreshConsumptionUnderGlassOrHighAccessibleCover> rdf:type owl:NamedIndividual ,
                                                                                                                                                               <http://lpis.ec.europa.eu/registry/applicationschema/cap-iacs-base#CropItemCodeValue> ;
                                                                                                                                                      rdfs:label "Tomatoes for fresh consumption under glass or high accessible cover"@en ;
                                                                                                                                                      <http://www.w3.org/2004/02/skos/core#definition> """-- Definition --
|||||Tomatoes for fresh consumption under glass or high accessible cover.
-- Description --
Cereals and main crops - C
NOTE. Initial value:C1752"""@en ;
                                                                                                                                                      <http://www.w3.org/2004/02/skos/core#inScheme> :CropItemCodeValue .


###  http://lpis.ec.europa.eu/registry/applicationschema/cap-iacs-base/code#CropItemCodeValue/triticale
<http://lpis.ec.europa.eu/registry/applicationschema/cap-iacs-base/code#CropItemCodeValue/triticale> rdf:type owl:NamedIndividual ,
                                                                                                              <http://lpis.ec.europa.eu/registry/applicationschema/cap-iacs-base#CropItemCodeValue> ;
                                                                                                     rdfs:label "Triticale"@en ;
                                                                                                     <http://www.w3.org/2004/02/skos/core#definition> """-- Definition --
|||Triticale.
-- Description --
Cereals and main crops - C
NOTE. Initial value:C1212"""@en ;
                                                                                                     <http://www.w3.org/2004/02/skos/core#inScheme> :CropItemCodeValue .


###  http://lpis.ec.europa.eu/registry/applicationschema/cap-iacs-base/code#CropItemCodeValue/turnipRape
<http://lpis.ec.europa.eu/registry/applicationschema/cap-iacs-base/code#CropItemCodeValue/turnipRape> rdf:type owl:NamedIndividual ,
                                                                                                               <http://lpis.ec.europa.eu/registry/applicationschema/cap-iacs-base#CropItemCodeValue> ;
                                                                                                      rdfs:label "Turnip rape"@en ;
                                                                                                      <http://www.w3.org/2004/02/skos/core#definition> """-- Definition --
|||||Turnip rape.
-- Description --
Cereals and main crops - C
NOTE. Initial value:C1440"""@en ;
                                                                                                      <http://www.w3.org/2004/02/skos/core#inScheme> :CropItemCodeValue .


###  http://lpis.ec.europa.eu/registry/applicationschema/cap-iacs-base/code#CropItemCodeValue/turnips
<http://lpis.ec.europa.eu/registry/applicationschema/cap-iacs-base/code#CropItemCodeValue/turnips> rdf:type owl:NamedIndividual ,
                                                                                                            <http://lpis.ec.europa.eu/registry/applicationschema/cap-iacs-base#CropItemCodeValue> ;
                                                                                                   rdfs:label "Turnips"@en ;
                                                                                                   <http://www.w3.org/2004/02/skos/core#definition> """-- Definition --
|||Turnips.
-- Description --
Cereals and main crops - C
NOTE. Initial value:C1820"""@en ;
                                                                                                   <http://www.w3.org/2004/02/skos/core#inScheme> :CropItemCodeValue .


###  http://lpis.ec.europa.eu/registry/applicationschema/cap-iacs-base/code#CropItemCodeValue/utilisedAgriculturalAreaUAA
<http://lpis.ec.europa.eu/registry/applicationschema/cap-iacs-base/code#CropItemCodeValue/utilisedAgriculturalAreaUAA> rdf:type owl:NamedIndividual ,
                                                                                                                                <http://lpis.ec.europa.eu/registry/applicationschema/cap-iacs-base#CropItemCodeValue> ;
                                                                                                                       rdfs:label "Utilised agricultural area (UAA)"@en ;
                                                                                                                       <http://www.w3.org/2004/02/skos/core#definition> """-- Definition --
|Utilised agricultural area (UAA).
-- Description --
Land use of Agriculture Area in Use -L
NOTE. Initial value:L0005"""@en ;
                                                                                                                       <http://www.w3.org/2004/02/skos/core#inScheme> :CropItemCodeValue .


###  http://lpis.ec.europa.eu/registry/applicationschema/cap-iacs-base/code#CropItemCodeValue/vegetablesCultivatedForFruit
<http://lpis.ec.europa.eu/registry/applicationschema/cap-iacs-base/code#CropItemCodeValue/vegetablesCultivatedForFruit> rdf:type owl:NamedIndividual ,
                                                                                                                                 <http://lpis.ec.europa.eu/registry/applicationschema/cap-iacs-base#CropItemCodeValue> ;
                                                                                                                        rdfs:label "Vegetables cultivated for fruit"@en ;
                                                                                                                        <http://www.w3.org/2004/02/skos/core#definition> """-- Definition --
||Vegetables cultivated for fruit.
-- Description --
Cereals and main crops - C
NOTE. Initial value:C1740"""@en ;
                                                                                                                        <http://www.w3.org/2004/02/skos/core#inScheme> :CropItemCodeValue .


###  http://lpis.ec.europa.eu/registry/applicationschema/cap-iacs-base/code#CropItemCodeValue/vegetablesFromKitchenGardensC2992
<http://lpis.ec.europa.eu/registry/applicationschema/cap-iacs-base/code#CropItemCodeValue/vegetablesFromKitchenGardensC2992> rdf:type owl:NamedIndividual ,
                                                                                                                                      <http://lpis.ec.europa.eu/registry/applicationschema/cap-iacs-base#CropItemCodeValue> ;
                                                                                                                             rdfs:label "Vegetables from kitchen gardens C2992"@en ;
                                                                                                                             <http://www.w3.org/2004/02/skos/core#definition> """-- Definition --
Vegetables from kitchen gardens C2992.
-- Description --
Cereals and main crops - C
NOTE. Initial value:C2992"""@en ;
                                                                                                                             <http://www.w3.org/2004/02/skos/core#inScheme> :CropItemCodeValue .


###  http://lpis.ec.europa.eu/registry/applicationschema/cap-iacs-base/code#CropItemCodeValue/vegetablesMelonsAndStrawberries
<http://lpis.ec.europa.eu/registry/applicationschema/cap-iacs-base/code#CropItemCodeValue/vegetablesMelonsAndStrawberries> rdf:type owl:NamedIndividual ,
                                                                                                                                    <http://lpis.ec.europa.eu/registry/applicationschema/cap-iacs-base#CropItemCodeValue> ;
                                                                                                                           rdfs:label "Vegetables, melons and strawberries"@en ;
                                                                                                                           <http://www.w3.org/2004/02/skos/core#definition> """-- Definition --
|||Vegetables, melons and strawberries.
-- Description --
Land use of Agriculture Area in Use -L
NOTE. Initial value:L1600"""@en ;
                                                                                                                           <http://www.w3.org/2004/02/skos/core#inScheme> :CropItemCodeValue .


###  http://lpis.ec.europa.eu/registry/applicationschema/cap-iacs-base/code#CropItemCodeValue/vegetablesMelonsAndStrawberriesExcludingKitchenGardens
<http://lpis.ec.europa.eu/registry/applicationschema/cap-iacs-base/code#CropItemCodeValue/vegetablesMelonsAndStrawberriesExcludingKitchenGardens> rdf:type owl:NamedIndividual ,
                                                                                                                                                           <http://lpis.ec.europa.eu/registry/applicationschema/cap-iacs-base#CropItemCodeValue> ;
                                                                                                                                                  rdfs:label "Vegetables, melons and strawberries (excluding kitchen gardens)"@en ;
                                                                                                                                                  <http://www.w3.org/2004/02/skos/core#definition> """-- Definition --
|Vegetables, melons and strawberries (excluding kitchen gardens).
-- Description --
Cereals and main crops - C
NOTE. Initial value:C1600"""@en ;
                                                                                                                                                  <http://www.w3.org/2004/02/skos/core#inScheme> :CropItemCodeValue .


###  http://lpis.ec.europa.eu/registry/applicationschema/cap-iacs-base/code#CropItemCodeValue/vegetablesMelonsAndStrawberriesUnderGlassHighAccessibleCover
<http://lpis.ec.europa.eu/registry/applicationschema/cap-iacs-base/code#CropItemCodeValue/vegetablesMelonsAndStrawberriesUnderGlassHighAccessibleCover> rdf:type owl:NamedIndividual ,
                                                                                                                                                                 <http://lpis.ec.europa.eu/registry/applicationschema/cap-iacs-base#CropItemCodeValue> ;
                                                                                                                                                        rdfs:label "Vegetables, melons and strawberries under glass high accessible cover"@en ;
                                                                                                                                                        <http://www.w3.org/2004/02/skos/core#definition> """-- Definition --
Vegetables, melons and strawberries under glass high accessible cover.
-- Description --
Land use of Agriculture Area in Use -L. Special aggregates
NOTE. Initial value:L1112"""@en ;
                                                                                                                                                        <http://www.w3.org/2004/02/skos/core#inScheme> :CropItemCodeValue .


###  http://lpis.ec.europa.eu/registry/applicationschema/cap-iacs-base/code#CropItemCodeValue/vineyards
<http://lpis.ec.europa.eu/registry/applicationschema/cap-iacs-base/code#CropItemCodeValue/vineyards> rdf:type owl:NamedIndividual ,
                                                                                                              <http://lpis.ec.europa.eu/registry/applicationschema/cap-iacs-base#CropItemCodeValue> ;
                                                                                                     rdfs:label "Vineyards"@en ;
                                                                                                     <http://www.w3.org/2004/02/skos/core#definition> """-- Definition --
|||Vineyards.
-- Description --
Land use of Agriculture Area in Use -L
NOTE. Initial value:L2410"""@en ;
                                                                                                     <http://www.w3.org/2004/02/skos/core#inScheme> :CropItemCodeValue .


###  http://lpis.ec.europa.eu/registry/applicationschema/cap-iacs-base/code#CropItemCodeValue/vineyardsC2410
<http://lpis.ec.europa.eu/registry/applicationschema/cap-iacs-base/code#CropItemCodeValue/vineyardsC2410> rdf:type owl:NamedIndividual ,
                                                                                                                   <http://lpis.ec.europa.eu/registry/applicationschema/cap-iacs-base#CropItemCodeValue> ;
                                                                                                          rdfs:label "Vineyards C2410"@en ;
                                                                                                          <http://www.w3.org/2004/02/skos/core#definition> """-- Definition --
||Vineyards C2410.
-- Description --
Cereals and main crops - C
NOTE. Initial value:C2410"""@en ;
                                                                                                          <http://www.w3.org/2004/02/skos/core#inScheme> :CropItemCodeValue .


###  http://lpis.ec.europa.eu/registry/applicationschema/cap-iacs-base/code#CropItemCodeValue/vineyardsForOtherGrapeProductionNec
<http://lpis.ec.europa.eu/registry/applicationschema/cap-iacs-base/code#CropItemCodeValue/vineyardsForOtherGrapeProductionNec> rdf:type owl:NamedIndividual ,
                                                                                                                                        <http://lpis.ec.europa.eu/registry/applicationschema/cap-iacs-base#CropItemCodeValue> ;
                                                                                                                               rdfs:label "Vineyards for other grape production n.e.c."@en ;
                                                                                                                               <http://www.w3.org/2004/02/skos/core#definition> """-- Definition --
|||Vineyards for other grape production n.e.c.
-- Description --
Cereals and main crops - C
NOTE. Initial value:C2445"""@en ;
                                                                                                                               <http://www.w3.org/2004/02/skos/core#inScheme> :CropItemCodeValue .


###  http://lpis.ec.europa.eu/registry/applicationschema/cap-iacs-base/code#CropItemCodeValue/vineyardsForOtherWines
<http://lpis.ec.europa.eu/registry/applicationschema/cap-iacs-base/code#CropItemCodeValue/vineyardsForOtherWines> rdf:type owl:NamedIndividual ,
                                                                                                                           <http://lpis.ec.europa.eu/registry/applicationschema/cap-iacs-base#CropItemCodeValue> ;
                                                                                                                  rdfs:label "Vineyards for other wines"@en ;
                                                                                                                  <http://www.w3.org/2004/02/skos/core#definition> """-- Definition --
||||Vineyards for other wines.
-- Description --
Cereals and main crops - C
NOTE. Initial value:C2443"""@en ;
                                                                                                                  <http://www.w3.org/2004/02/skos/core#inScheme> :CropItemCodeValue .


###  http://lpis.ec.europa.eu/registry/applicationschema/cap-iacs-base/code#CropItemCodeValue/vineyardsForRaisins
<http://lpis.ec.europa.eu/registry/applicationschema/cap-iacs-base/code#CropItemCodeValue/vineyardsForRaisins> rdf:type owl:NamedIndividual ,
                                                                                                                        <http://lpis.ec.europa.eu/registry/applicationschema/cap-iacs-base#CropItemCodeValue> ;
                                                                                                               rdfs:label "Vineyards for raisins"@en ;
                                                                                                               <http://www.w3.org/2004/02/skos/core#definition> """-- Definition --
|||Vineyards for raisins.
-- Description --
Cereals and main crops - C
NOTE. Initial value:C2416"""@en ;
                                                                                                               <http://www.w3.org/2004/02/skos/core#inScheme> :CropItemCodeValue .


###  http://lpis.ec.europa.eu/registry/applicationschema/cap-iacs-base/code#CropItemCodeValue/vineyardsForTableGrapes
<http://lpis.ec.europa.eu/registry/applicationschema/cap-iacs-base/code#CropItemCodeValue/vineyardsForTableGrapes> rdf:type owl:NamedIndividual ,
                                                                                                                            <http://lpis.ec.europa.eu/registry/applicationschema/cap-iacs-base#CropItemCodeValue> ;
                                                                                                                   rdfs:label "Vineyards for table grapes"@en ;
                                                                                                                   <http://www.w3.org/2004/02/skos/core#definition> """-- Definition --
|||Vineyards for table grapes.
-- Description --
Cereals and main crops - C
NOTE. Initial value:C2420"""@en ;
                                                                                                                   <http://www.w3.org/2004/02/skos/core#inScheme> :CropItemCodeValue .


###  http://lpis.ec.europa.eu/registry/applicationschema/cap-iacs-base/code#CropItemCodeValue/vineyardsForWine
<http://lpis.ec.europa.eu/registry/applicationschema/cap-iacs-base/code#CropItemCodeValue/vineyardsForWine> rdf:type owl:NamedIndividual ,
                                                                                                                     <http://lpis.ec.europa.eu/registry/applicationschema/cap-iacs-base#CropItemCodeValue> ;
                                                                                                            rdfs:label "Vineyards for wine"@en ;
                                                                                                            <http://www.w3.org/2004/02/skos/core#definition> """-- Definition --
|||Vineyards for wine.
-- Description --
Cereals and main crops - C
NOTE. Initial value:C2440"""@en ;
                                                                                                            <http://www.w3.org/2004/02/skos/core#inScheme> :CropItemCodeValue .


###  http://lpis.ec.europa.eu/registry/applicationschema/cap-iacs-base/code#CropItemCodeValue/vineyardsForWinesWithProtectedDesignationOfOriginPDO
<http://lpis.ec.europa.eu/registry/applicationschema/cap-iacs-base/code#CropItemCodeValue/vineyardsForWinesWithProtectedDesignationOfOriginPDO> rdf:type owl:NamedIndividual ,
                                                                                                                                                         <http://lpis.ec.europa.eu/registry/applicationschema/cap-iacs-base#CropItemCodeValue> ;
                                                                                                                                                rdfs:label "Vineyards for wines with protected designation of origin (PDO)"@en ;
                                                                                                                                                <http://www.w3.org/2004/02/skos/core#definition> """-- Definition --
||||Vineyards for wines with protected designation of origin (PDO).
-- Description --
Cereals and main crops - C
NOTE. Initial value:C2441"""@en ;
                                                                                                                                                <http://www.w3.org/2004/02/skos/core#inScheme> :CropItemCodeValue .


###  http://lpis.ec.europa.eu/registry/applicationschema/cap-iacs-base/code#CropItemCodeValue/vineyardsForWinesWithProtectedGeographicalIndicationPGI
<http://lpis.ec.europa.eu/registry/applicationschema/cap-iacs-base/code#CropItemCodeValue/vineyardsForWinesWithProtectedGeographicalIndicationPGI> rdf:type owl:NamedIndividual ,
                                                                                                                                                            <http://lpis.ec.europa.eu/registry/applicationschema/cap-iacs-base#CropItemCodeValue> ;
                                                                                                                                                   rdfs:label "Vineyards for wines with protected geographical indication (PGI)"@en ;
                                                                                                                                                   <http://www.w3.org/2004/02/skos/core#definition> """-- Definition --
||||Vineyards for wines with protected geographical indication (PGI).
-- Description --
Cereals and main crops - C
NOTE. Initial value:C2442"""@en ;
                                                                                                                                                   <http://www.w3.org/2004/02/skos/core#inScheme> :CropItemCodeValue .


###  http://lpis.ec.europa.eu/registry/applicationschema/cap-iacs-base/code#CropItemCodeValue/walnuts
<http://lpis.ec.europa.eu/registry/applicationschema/cap-iacs-base/code#CropItemCodeValue/walnuts> rdf:type owl:NamedIndividual ,
                                                                                                            <http://lpis.ec.europa.eu/registry/applicationschema/cap-iacs-base#CropItemCodeValue> ;
                                                                                                   rdfs:label "Walnuts"@en ;
                                                                                                   <http://www.w3.org/2004/02/skos/core#definition> """-- Definition --
|||Walnuts.
-- Description --
Cereals and main crops - C
NOTE. Initial value:C2231"""@en ;
                                                                                                   <http://www.w3.org/2004/02/skos/core#inScheme> :CropItemCodeValue .


###  http://lpis.ec.europa.eu/registry/applicationschema/cap-iacs-base/code#CropItemCodeValue/watermelons
<http://lpis.ec.europa.eu/registry/applicationschema/cap-iacs-base/code#CropItemCodeValue/watermelons> rdf:type owl:NamedIndividual ,
                                                                                                                <http://lpis.ec.europa.eu/registry/applicationschema/cap-iacs-base#CropItemCodeValue> ;
                                                                                                       rdfs:label "Watermelons"@en ;
                                                                                                       <http://www.w3.org/2004/02/skos/core#definition> """-- Definition --
||Watermelons.
-- Description --
Cereals and main crops - C
NOTE. Initial value:C1777"""@en ;
                                                                                                       <http://www.w3.org/2004/02/skos/core#inScheme> :CropItemCodeValue .


###  http://lpis.ec.europa.eu/registry/applicationschema/cap-iacs-base/code#CropItemCodeValue/weavingPlants
<http://lpis.ec.europa.eu/registry/applicationschema/cap-iacs-base/code#CropItemCodeValue/weavingPlants> rdf:type owl:NamedIndividual ,
                                                                                                                  <http://lpis.ec.europa.eu/registry/applicationschema/cap-iacs-base#CropItemCodeValue> ;
                                                                                                         rdfs:label "Weaving plants"@en ;
                                                                                                         <http://www.w3.org/2004/02/skos/core#definition> """-- Definition --
|||Weaving plants.
-- Description --
Land use of Agriculture Area in Use -L
NOTE. Initial value:L2960"""@en ;
                                                                                                         <http://www.w3.org/2004/02/skos/core#inScheme> :CropItemCodeValue .


###  http://lpis.ec.europa.eu/registry/applicationschema/cap-iacs-base/code#CropItemCodeValue/wheatIncludingSpelt
<http://lpis.ec.europa.eu/registry/applicationschema/cap-iacs-base/code#CropItemCodeValue/wheatIncludingSpelt> rdf:type owl:NamedIndividual ,
                                                                                                                        <http://lpis.ec.europa.eu/registry/applicationschema/cap-iacs-base#CropItemCodeValue> ;
                                                                                                               rdfs:label "Wheat (including spelt)"@en ;
                                                                                                               <http://www.w3.org/2004/02/skos/core#definition> """-- Definition --
|||Wheat (including spelt).
-- Description --
Cereals and main crops - C
NOTE. Initial value:C1100"""@en ;
                                                                                                               <http://www.w3.org/2004/02/skos/core#inScheme> :CropItemCodeValue .


###  http://lpis.ec.europa.eu/registry/applicationschema/cap-iacs-base/code#CropItemCodeValue/winterBarley
<http://lpis.ec.europa.eu/registry/applicationschema/cap-iacs-base/code#CropItemCodeValue/winterBarley> rdf:type owl:NamedIndividual ,
                                                                                                                 <http://lpis.ec.europa.eu/registry/applicationschema/cap-iacs-base#CropItemCodeValue> ;
                                                                                                        rdfs:label "Winter barley"@en ;
                                                                                                        <http://www.w3.org/2004/02/skos/core#definition> """-- Definition --
||||Winter barley.
-- Description --
Cereals and main crops - C
NOTE. Initial value:C1163"""@en ;
                                                                                                        <http://www.w3.org/2004/02/skos/core#inScheme> :CropItemCodeValue .


###  http://lpis.ec.europa.eu/registry/applicationschema/cap-iacs-base/code#CropItemCodeValue/winterDurumWheat
<http://lpis.ec.europa.eu/registry/applicationschema/cap-iacs-base/code#CropItemCodeValue/winterDurumWheat> rdf:type owl:NamedIndividual ,
                                                                                                                     <http://lpis.ec.europa.eu/registry/applicationschema/cap-iacs-base#CropItemCodeValue> ;
                                                                                                            rdfs:label "Winter durum wheat"@en ;
                                                                                                            <http://www.w3.org/2004/02/skos/core#definition> """-- Definition --
|||||Winter durum wheat.
-- Description --
Cereals and main crops - C
NOTE. Initial value:C1133"""@en ;
                                                                                                            <http://www.w3.org/2004/02/skos/core#inScheme> :CropItemCodeValue .


###  http://lpis.ec.europa.eu/registry/applicationschema/cap-iacs-base/code#CropItemCodeValue/winterRape
<http://lpis.ec.europa.eu/registry/applicationschema/cap-iacs-base/code#CropItemCodeValue/winterRape> rdf:type owl:NamedIndividual ,
                                                                                                               <http://lpis.ec.europa.eu/registry/applicationschema/cap-iacs-base#CropItemCodeValue> ;
                                                                                                      rdfs:label "Winter rape"@en ;
                                                                                                      <http://www.w3.org/2004/02/skos/core#definition> """-- Definition --
||||||Winter rape.
-- Description --
Cereals and main crops - C
NOTE. Initial value:C1431"""@en ;
                                                                                                      <http://www.w3.org/2004/02/skos/core#inScheme> :CropItemCodeValue .


###  http://lpis.ec.europa.eu/registry/applicationschema/cap-iacs-base/code#CropItemCodeValue/winterRye
<http://lpis.ec.europa.eu/registry/applicationschema/cap-iacs-base/code#CropItemCodeValue/winterRye> rdf:type owl:NamedIndividual ,
                                                                                                              <http://lpis.ec.europa.eu/registry/applicationschema/cap-iacs-base#CropItemCodeValue> ;
                                                                                                     rdfs:label "Winter rye"@en ;
                                                                                                     <http://www.w3.org/2004/02/skos/core#definition> """-- Definition --
|||||Winter rye.
-- Description --
Cereals and main crops - C
NOTE. Initial value:C1151"""@en ;
                                                                                                     <http://www.w3.org/2004/02/skos/core#inScheme> :CropItemCodeValue .


###  http://lpis.ec.europa.eu/registry/applicationschema/cap-iacs-base/code#CropItemCodeValue/winterTriticale
<http://lpis.ec.europa.eu/registry/applicationschema/cap-iacs-base/code#CropItemCodeValue/winterTriticale> rdf:type owl:NamedIndividual ,
                                                                                                                    <http://lpis.ec.europa.eu/registry/applicationschema/cap-iacs-base#CropItemCodeValue> ;
                                                                                                           rdfs:label "Winter triticale"@en ;
                                                                                                           <http://www.w3.org/2004/02/skos/core#definition> """-- Definition --
||||Winter triticale.
-- Description --
Cereals and main crops - C
NOTE. Initial value:C1213"""@en ;
                                                                                                           <http://www.w3.org/2004/02/skos/core#inScheme> :CropItemCodeValue .


###  http://lpis.ec.europa.eu/registry/applicationschema/cap-iacs-base/code#CropItemCodeValue/yellowLemons
<http://lpis.ec.europa.eu/registry/applicationschema/cap-iacs-base/code#CropItemCodeValue/yellowLemons> rdf:type owl:NamedIndividual ,
                                                                                                                 <http://lpis.ec.europa.eu/registry/applicationschema/cap-iacs-base#CropItemCodeValue> ;
                                                                                                        rdfs:label "Yellow lemons"@en ;
                                                                                                        <http://www.w3.org/2004/02/skos/core#definition> """-- Definition --
||||Yellow lemons.
-- Description --
Cereals and main crops - C
NOTE. Initial value:C2371"""@en ;
                                                                                                        <http://www.w3.org/2004/02/skos/core#inScheme> :CropItemCodeValue .


###  http://lpis.ec.europa.eu/registry/applicationschema/cap-iacs-base/code#CrossComplianceRuleValue/animalWelfareAnimalWelfareSmr11
<http://lpis.ec.europa.eu/registry/applicationschema/cap-iacs-base/code#CrossComplianceRuleValue/animalWelfareAnimalWelfareSmr11> rdf:type owl:NamedIndividual ,
                                                                                                                                           <http://lpis.ec.europa.eu/registry/applicationschema/cap-iacs-base#CrossComplianceRuleValue> ;
                                                                                                                                  rdfs:label "Animal welfare - Animal welfare SMR11"@en ;
                                                                                                                                  <http://www.w3.org/2004/02/skos/core#definition> """-- Definition --
Animal welfare - Animal welfare SMR11.
-- Description --
Council Directive 2008/119/EC of 18 December 2008 laying down minimum standards for the protection of calves (OJ L 10, 15.1.2009, p. 7) . Articles 3 and 4.
NOTE. Initial value:SMR11"""@en ;
                                                                                                                                  <http://www.w3.org/2004/02/skos/core#inScheme> :CrossComplianceRuleValue .


###  http://lpis.ec.europa.eu/registry/applicationschema/cap-iacs-base/code#CrossComplianceRuleValue/animalWelfareAnimalWelfareSmr12
<http://lpis.ec.europa.eu/registry/applicationschema/cap-iacs-base/code#CrossComplianceRuleValue/animalWelfareAnimalWelfareSmr12> rdf:type owl:NamedIndividual ,
                                                                                                                                           <http://lpis.ec.europa.eu/registry/applicationschema/cap-iacs-base#CrossComplianceRuleValue> ;
                                                                                                                                  rdfs:label "Animal welfare - Animal welfare SMR12"@en ;
                                                                                                                                  <http://www.w3.org/2004/02/skos/core#definition> """-- Definition --
Animal welfare - Animal welfare SMR12.
-- Description --
Council Directive 2008/120/EC of 18 December 2008 laying down minimum standards for the protection of pigs (OJ L 47, 18.2.2009, p. 5). Article 3 and Article 4.
NOTE. Initial value:SMR12"""@en ;
                                                                                                                                  <http://www.w3.org/2004/02/skos/core#inScheme> :CrossComplianceRuleValue .


###  http://lpis.ec.europa.eu/registry/applicationschema/cap-iacs-base/code#CrossComplianceRuleValue/animalWelfareAnimalWelfareSmr13
<http://lpis.ec.europa.eu/registry/applicationschema/cap-iacs-base/code#CrossComplianceRuleValue/animalWelfareAnimalWelfareSmr13> rdf:type owl:NamedIndividual ,
                                                                                                                                           <http://lpis.ec.europa.eu/registry/applicationschema/cap-iacs-base#CrossComplianceRuleValue> ;
                                                                                                                                  rdfs:label "Animal welfare - Animal welfare SMR13"@en ;
                                                                                                                                  <http://www.w3.org/2004/02/skos/core#definition> """-- Definition --
Animal welfare - Animal welfare SMR13.
-- Description --
Council Directive 98/58/EC of 20 July 1998 concerning the protection of animals kept for farming purposes (OJ L 221, 8.8.1998, p. 23) . Article 4 .
NOTE. Initial value:SMR13"""@en ;
                                                                                                                                  <http://www.w3.org/2004/02/skos/core#inScheme> :CrossComplianceRuleValue .


###  http://lpis.ec.europa.eu/registry/applicationschema/cap-iacs-base/code#CrossComplianceRuleValue/environmentClimateChangeGoodAgriculturalConditionOfLandBiodiversitySmr2
<http://lpis.ec.europa.eu/registry/applicationschema/cap-iacs-base/code#CrossComplianceRuleValue/environmentClimateChangeGoodAgriculturalConditionOfLandBiodiversitySmr2> rdf:type owl:NamedIndividual ,
                                                                                                                                                                                   <http://lpis.ec.europa.eu/registry/applicationschema/cap-iacs-base#CrossComplianceRuleValue> ;
                                                                                                                                                                          rdfs:label "Environment, climate change, good agricultural condition of land  - Biodiversity SMR2"@en ;
                                                                                                                                                                          <http://www.w3.org/2004/02/skos/core#definition> """-- Definition --
Environment, climate change, good agricultural condition of land  - Biodiversity SMR2.
-- Description --
Directive 2009/147/EC of the European Parliament and of the Council of 30 November 2009 on the conservation of wild birds (OJ L 20, 26.1.2010, p. 7). Article 3(1), Article 3(2)(b), Article 4(1), (2) and (4).
NOTE. Initial value:SMR2"""@en ;
                                                                                                                                                                          <http://www.w3.org/2004/02/skos/core#inScheme> :CrossComplianceRuleValue .


###  http://lpis.ec.europa.eu/registry/applicationschema/cap-iacs-base/code#CrossComplianceRuleValue/environmentClimateChangeGoodAgriculturalConditionOfLandBiodiversitySmr3
<http://lpis.ec.europa.eu/registry/applicationschema/cap-iacs-base/code#CrossComplianceRuleValue/environmentClimateChangeGoodAgriculturalConditionOfLandBiodiversitySmr3> rdf:type owl:NamedIndividual ,
                                                                                                                                                                                   <http://lpis.ec.europa.eu/registry/applicationschema/cap-iacs-base#CrossComplianceRuleValue> ;
                                                                                                                                                                          rdfs:label "Environment, climate change, good agricultural condition of land  - Biodiversity SMR3"@en ;
                                                                                                                                                                          <http://www.w3.org/2004/02/skos/core#definition> """-- Definition --
Environment, climate change, good agricultural condition of land  - Biodiversity SMR3.
-- Description --
Council Directive 92/43/EEC of 21 May 1992 on the conservation of natural habitats and of wild flora and fauna (OJ L 206, 22.7.1992, p. 7) . Article 6(1) and (2).
NOTE. Initial value:SMR3"""@en ;
                                                                                                                                                                          <http://www.w3.org/2004/02/skos/core#inScheme> :CrossComplianceRuleValue .


###  http://lpis.ec.europa.eu/registry/applicationschema/cap-iacs-base/code#CrossComplianceRuleValue/environmentClimateChangeGoodAgriculturalConditionOfLandLandscapeMinimumLevelOfMaintenanceGaec7
<http://lpis.ec.europa.eu/registry/applicationschema/cap-iacs-base/code#CrossComplianceRuleValue/environmentClimateChangeGoodAgriculturalConditionOfLandLandscapeMinimumLevelOfMaintenanceGaec7> rdf:type owl:NamedIndividual ,
                                                                                                                                                                                                          <http://lpis.ec.europa.eu/registry/applicationschema/cap-iacs-base#CrossComplianceRuleValue> ;
                                                                                                                                                                                                 rdfs:label "Environment, climate change, good agricultural condition of land  - Landscape, minimum level of maintenance GAEC7"@en ;
                                                                                                                                                                                                 <http://www.w3.org/2004/02/skos/core#definition> """-- Definition --
Environment, climate change, good agricultural condition of land  - Landscape, minimum level of maintenance GAEC7.
-- Description --
Retention of landscape features, including where appropriate, hedges, ponds, ditches, trees in line, in group or isolated, field margins and terraces, and including a ban on cutting hedges and trees during the bird breeding and rearing season and, as an option, measures for avoiding invasive plant species. 
NOTE. Initial value:GAEC7."""@en ;
                                                                                                                                                                                                 <http://www.w3.org/2004/02/skos/core#inScheme> :CrossComplianceRuleValue .


###  http://lpis.ec.europa.eu/registry/applicationschema/cap-iacs-base/code#CrossComplianceRuleValue/environmentClimateChangeGoodAgriculturalConditionOfLandSoilAndCarbonStockGaec4
<http://lpis.ec.europa.eu/registry/applicationschema/cap-iacs-base/code#CrossComplianceRuleValue/environmentClimateChangeGoodAgriculturalConditionOfLandSoilAndCarbonStockGaec4> rdf:type owl:NamedIndividual ,
                                                                                                                                                                                          <http://lpis.ec.europa.eu/registry/applicationschema/cap-iacs-base#CrossComplianceRuleValue> ;
                                                                                                                                                                                 rdfs:label "Environment, climate change, good agricultural condition of land  - Soil and carbon stock  GAEC4"@en ;
                                                                                                                                                                                 <http://www.w3.org/2004/02/skos/core#definition> """-- Definition --
Environment, climate change, good agricultural condition of land  - Soil and carbon stock  GAEC4.
-- Description --
Minimum soil cover. 
NOTE. Initial value:GAEC4"""@en ;
                                                                                                                                                                                 <http://www.w3.org/2004/02/skos/core#inScheme> :CrossComplianceRuleValue .


###  http://lpis.ec.europa.eu/registry/applicationschema/cap-iacs-base/code#CrossComplianceRuleValue/environmentClimateChangeGoodAgriculturalConditionOfLandSoilAndCarbonStockGaec5
<http://lpis.ec.europa.eu/registry/applicationschema/cap-iacs-base/code#CrossComplianceRuleValue/environmentClimateChangeGoodAgriculturalConditionOfLandSoilAndCarbonStockGaec5> rdf:type owl:NamedIndividual ,
                                                                                                                                                                                          <http://lpis.ec.europa.eu/registry/applicationschema/cap-iacs-base#CrossComplianceRuleValue> ;
                                                                                                                                                                                 rdfs:label "Environment, climate change, good agricultural condition of land  - Soil and carbon stock  GAEC5"@en ;
                                                                                                                                                                                 <http://www.w3.org/2004/02/skos/core#definition> """-- Definition --
Environment, climate change, good agricultural condition of land  - Soil and carbon stock  GAEC5.
-- Description --
Minimum land management reflecting site specific conditions to limit erosion. 
NOTE. Initial value:GAEC5"""@en ;
                                                                                                                                                                                 <http://www.w3.org/2004/02/skos/core#inScheme> :CrossComplianceRuleValue .


###  http://lpis.ec.europa.eu/registry/applicationschema/cap-iacs-base/code#CrossComplianceRuleValue/environmentClimateChangeGoodAgriculturalConditionOfLandSoilAndCarbonStockGaec6
<http://lpis.ec.europa.eu/registry/applicationschema/cap-iacs-base/code#CrossComplianceRuleValue/environmentClimateChangeGoodAgriculturalConditionOfLandSoilAndCarbonStockGaec6> rdf:type owl:NamedIndividual ,
                                                                                                                                                                                          <http://lpis.ec.europa.eu/registry/applicationschema/cap-iacs-base#CrossComplianceRuleValue> ;
                                                                                                                                                                                 rdfs:label "Environment, climate change, good agricultural condition of land  - Soil and carbon stock  GAEC6"@en ;
                                                                                                                                                                                 <http://www.w3.org/2004/02/skos/core#definition> """-- Definition --
Environment, climate change, good agricultural condition of land  - Soil and carbon stock  GAEC6.
-- Description --
Maintenance of soil organic matter level through appropriate practices including ban on burning arable stubble, except for plant health reasons.. The requirement can be limited to a general ban on burning arable stubble, but a Member State may decide to prescribe further requirements.
NOTE. Initial value:GAEC6"""@en ;
                                                                                                                                                                                 <http://www.w3.org/2004/02/skos/core#inScheme> :CrossComplianceRuleValue .


###  http://lpis.ec.europa.eu/registry/applicationschema/cap-iacs-base/code#CrossComplianceRuleValue/environmentClimateChangeGoodAgriculturalConditionOfLandWaterGaec1
<http://lpis.ec.europa.eu/registry/applicationschema/cap-iacs-base/code#CrossComplianceRuleValue/environmentClimateChangeGoodAgriculturalConditionOfLandWaterGaec1> rdf:type owl:NamedIndividual ,
                                                                                                                                                                             <http://lpis.ec.europa.eu/registry/applicationschema/cap-iacs-base#CrossComplianceRuleValue> ;
                                                                                                                                                                    rdfs:label "Environment, climate change, good agricultural condition of land  - Water GAEC1"@en ;
                                                                                                                                                                    <http://www.w3.org/2004/02/skos/core#definition> """-- Definition --
Environment, climate change, good agricultural condition of land  - Water GAEC1.
-- Description --
Establishment of buffer strips along water courses. The GAEC buffer strips must respect, both within and outside vulnerable zones designated pursuant to Article 3(2) of Directive 91/676/EEC, at least the requirements relating to the conditions for land application of fertiliser near water courses, referred to in point A.4 of Annex II to Directive 91/676/EEC to be applied in accordance with the action programmes of Member States established under Article 5(4) of Directive 91/676/EEC.
NOTE. Initial value:GAEC1"""@en ;
                                                                                                                                                                    <http://www.w3.org/2004/02/skos/core#inScheme> :CrossComplianceRuleValue .


###  http://lpis.ec.europa.eu/registry/applicationschema/cap-iacs-base/code#CrossComplianceRuleValue/environmentClimateChangeGoodAgriculturalConditionOfLandWaterGaec2
<http://lpis.ec.europa.eu/registry/applicationschema/cap-iacs-base/code#CrossComplianceRuleValue/environmentClimateChangeGoodAgriculturalConditionOfLandWaterGaec2> rdf:type owl:NamedIndividual ,
                                                                                                                                                                             <http://lpis.ec.europa.eu/registry/applicationschema/cap-iacs-base#CrossComplianceRuleValue> ;
                                                                                                                                                                    rdfs:label "Environment, climate change, good agricultural condition of land  - Water GAEC2"@en ;
                                                                                                                                                                    <http://www.w3.org/2004/02/skos/core#definition> """-- Definition --
Environment, climate change, good agricultural condition of land  - Water GAEC2.
-- Description --
Where use of water for irrigation is subject to authorisation, compliance with authorisation procedures. 
NOTE. Initial value:GAEC2"""@en ;
                                                                                                                                                                    <http://www.w3.org/2004/02/skos/core#inScheme> :CrossComplianceRuleValue .


###  http://lpis.ec.europa.eu/registry/applicationschema/cap-iacs-base/code#CrossComplianceRuleValue/environmentClimateChangeGoodAgriculturalConditionOfLandWaterGaec3
<http://lpis.ec.europa.eu/registry/applicationschema/cap-iacs-base/code#CrossComplianceRuleValue/environmentClimateChangeGoodAgriculturalConditionOfLandWaterGaec3> rdf:type owl:NamedIndividual ,
                                                                                                                                                                             <http://lpis.ec.europa.eu/registry/applicationschema/cap-iacs-base#CrossComplianceRuleValue> ;
                                                                                                                                                                    rdfs:label "Environment, climate change, good agricultural condition of land  - Water GAEC3"@en ;
                                                                                                                                                                    <http://www.w3.org/2004/02/skos/core#definition> """-- Definition --
Environment, climate change, good agricultural condition of land  - Water GAEC3.
-- Description --
Protection of ground water against pollution: prohibition of direct discharge into groundwater and measures to prevent indirect pollution of groundwater through discharge on the ground and percolation through the soil of dangerous substances, as listed in the Annex to Directive 80/68/EEC in its version in force on the last day of its validity, as far as it relates to agricultural activity. 
NOTE. Initial value:GAEC3"""@en ;
                                                                                                                                                                    <http://www.w3.org/2004/02/skos/core#inScheme> :CrossComplianceRuleValue .


###  http://lpis.ec.europa.eu/registry/applicationschema/cap-iacs-base/code#CrossComplianceRuleValue/environmentClimateChangeGoodAgriculturalConditionOfLandWaterSmr1
<http://lpis.ec.europa.eu/registry/applicationschema/cap-iacs-base/code#CrossComplianceRuleValue/environmentClimateChangeGoodAgriculturalConditionOfLandWaterSmr1> rdf:type owl:NamedIndividual ,
                                                                                                                                                                            <http://lpis.ec.europa.eu/registry/applicationschema/cap-iacs-base#CrossComplianceRuleValue> ;
                                                                                                                                                                   rdfs:label "Environment, climate change, good agricultural condition of land  - Water SMR1"@en ;
                                                                                                                                                                   <http://www.w3.org/2004/02/skos/core#definition> """-- Definition --
Environment, climate change, good agricultural condition of land  - Water SMR1.
-- Description --
Council Directive 91/676/EEC of 12 December 1991 concerning the protection of waters against pollution caused by nitrates from agricultural sources (OJ L 375, 31.12.1991, p. 1) . Articles 4 and 5.
NOTE. Initial value:SMR1"""@en ;
                                                                                                                                                                   <http://www.w3.org/2004/02/skos/core#inScheme> :CrossComplianceRuleValue .


###  http://lpis.ec.europa.eu/registry/applicationschema/cap-iacs-base/code#CrossComplianceRuleValue/publicHealthAnimalHealthAndPlantHealthAnimalDiseasesSmr9
<http://lpis.ec.europa.eu/registry/applicationschema/cap-iacs-base/code#CrossComplianceRuleValue/publicHealthAnimalHealthAndPlantHealthAnimalDiseasesSmr9> rdf:type owl:NamedIndividual ,
                                                                                                                                                                    <http://lpis.ec.europa.eu/registry/applicationschema/cap-iacs-base#CrossComplianceRuleValue> ;
                                                                                                                                                           rdfs:label "Public health, animal health and plant health  - Animal diseases SMR9"@en ;
                                                                                                                                                           <http://www.w3.org/2004/02/skos/core#definition> """-- Definition --
Public health, animal health and plant health  - Animal diseases SMR9.
-- Description --
Regulation (EC) No 999/2001 of the European Parliament and of the Council of 22 May 2001 laying down rules for the prevention, control and eradication of certain transmissible spongiform encephalopathies (OJ L 147, 31.5.2001, p. 1). Articles 7, 11, 12, 13 and 15.
NOTE. Initial value:SMR9"""@en ;
                                                                                                                                                           <http://www.w3.org/2004/02/skos/core#inScheme> :CrossComplianceRuleValue .


###  http://lpis.ec.europa.eu/registry/applicationschema/cap-iacs-base/code#CrossComplianceRuleValue/publicHealthAnimalHealthAndPlantHealthFoodSafetySmr4
<http://lpis.ec.europa.eu/registry/applicationschema/cap-iacs-base/code#CrossComplianceRuleValue/publicHealthAnimalHealthAndPlantHealthFoodSafetySmr4> rdf:type owl:NamedIndividual ,
                                                                                                                                                                <http://lpis.ec.europa.eu/registry/applicationschema/cap-iacs-base#CrossComplianceRuleValue> ;
                                                                                                                                                       rdfs:label "Public health, animal health and plant health  - Food safety SMR4"@en ;
                                                                                                                                                       <http://www.w3.org/2004/02/skos/core#definition> """-- Definition --
Public health, animal health and plant health  - Food safety SMR4.
-- Description --
Regulation (EC) No 178/2002 of the European Parliament and of the Council of 28 January 2002 laying down the general principles and requirements of food law, establishing the European Food Safety Authority and laying down procedures in matters of food safety (OJ L 31, 1.2.2002, p. 1). Articles 14 and 15, Article 17(1) [3] and Articles 18, 19 and 20 [3] As implemented in particular by:- Article 14 of Regulation (EC) No 470/2009 and the Annex of Regulation (EC) No 37/2010,- Regulation (EC) No 852/2004: Article 4(1) and Annex I part A (II 4 (g, h, j), 5 (f, h), 6; III 8 (a, b, d, e), 9 (a, c)),- Regulation (EC) No 853/2004: Article 3(1) and Annex III Section IX Chapter 1 (I-1 b, c, d, e; I-2 a (i, ii, iii), b (i, ii), c; I-3; I-4; I-5; II-A 1, 2, 3, 4; II-B 1(a, d), 2, 4 (a, b)), Annex III Section X Chapter 1(1),- Regulation (EC) No 183/2005: Article 5(1) and Annex I, part A (I-4 e, g; II-2 a, b, e), Article 5(5) and Annex III (1, 2), Article 5(6), and- Regulation (EC) No 396/2005: Article 18.
NOTE. Initial value:SMR4"""@en ;
                                                                                                                                                       <http://www.w3.org/2004/02/skos/core#inScheme> :CrossComplianceRuleValue .


###  http://lpis.ec.europa.eu/registry/applicationschema/cap-iacs-base/code#CrossComplianceRuleValue/publicHealthAnimalHealthAndPlantHealthFoodSafetySmr5
<http://lpis.ec.europa.eu/registry/applicationschema/cap-iacs-base/code#CrossComplianceRuleValue/publicHealthAnimalHealthAndPlantHealthFoodSafetySmr5> rdf:type owl:NamedIndividual ,
                                                                                                                                                                <http://lpis.ec.europa.eu/registry/applicationschema/cap-iacs-base#CrossComplianceRuleValue> ;
                                                                                                                                                       rdfs:label "Public health, animal health and plant health  - Food safety SMR5"@en ;
                                                                                                                                                       <http://www.w3.org/2004/02/skos/core#definition> """-- Definition --
Public health, animal health and plant health  - Food safety SMR5.
-- Description --
Council Directive 96/22/EC of 29 April 1996 concerning the prohibition on the use in stockfarming of certain substances having a hormonal or thyrostatic action and beta-agonists, and repealing Directives 81/602/EEC, 88/146/EEC and 88/299/EEC (OJ L 125, 23.5.1996, p. 3). Article 3(a), (b), (d) and (e) and Articles 4, 5 and 7.
NOTE. Initial value:SMR5"""@en ;
                                                                                                                                                       <http://www.w3.org/2004/02/skos/core#inScheme> :CrossComplianceRuleValue .


###  http://lpis.ec.europa.eu/registry/applicationschema/cap-iacs-base/code#CrossComplianceRuleValue/publicHealthAnimalHealthAndPlantHealthIdentificationAndRegistrationOfAnimalsSmr6
<http://lpis.ec.europa.eu/registry/applicationschema/cap-iacs-base/code#CrossComplianceRuleValue/publicHealthAnimalHealthAndPlantHealthIdentificationAndRegistrationOfAnimalsSmr6> rdf:type owl:NamedIndividual ,
                                                                                                                                                                                            <http://lpis.ec.europa.eu/registry/applicationschema/cap-iacs-base#CrossComplianceRuleValue> ;
                                                                                                                                                                                   rdfs:label "Public health, animal health and plant health  - Identification and registration of animals SMR6"@en ;
                                                                                                                                                                                   <http://www.w3.org/2004/02/skos/core#definition> """-- Definition --
Public health, animal health and plant health  - Identification and registration of animals SMR6.
-- Description --
Council Directive 2008/71/EC of 15 July 2008 on identification and registration of pigs (OJ L 213, 8.8.2005, p. 31). Articles 3, 4 and 5.
NOTE. Initial value:SMR6"""@en ;
                                                                                                                                                                                   <http://www.w3.org/2004/02/skos/core#inScheme> :CrossComplianceRuleValue .


###  http://lpis.ec.europa.eu/registry/applicationschema/cap-iacs-base/code#CrossComplianceRuleValue/publicHealthAnimalHealthAndPlantHealthIdentificationAndRegistrationOfAnimalsSmr7
<http://lpis.ec.europa.eu/registry/applicationschema/cap-iacs-base/code#CrossComplianceRuleValue/publicHealthAnimalHealthAndPlantHealthIdentificationAndRegistrationOfAnimalsSmr7> rdf:type owl:NamedIndividual ,
                                                                                                                                                                                            <http://lpis.ec.europa.eu/registry/applicationschema/cap-iacs-base#CrossComplianceRuleValue> ;
                                                                                                                                                                                   rdfs:label "Public health, animal health and plant health  - Identification and registration of animals SMR7"@en ;
                                                                                                                                                                                   <http://www.w3.org/2004/02/skos/core#definition> """-- Definition --
Public health, animal health and plant health  - Identification and registration of animals SMR7.
-- Description --
Regulation (EC) No 1760/2000 of the European Parliament and of the Council of 17 July 2000 establishing a system for the identification and registration of bovine animals and regarding the labelling of beef and beef products and repealing Council Regulation (EC) No 820/97(OJ L 204, 11.8.2000, p. 1) . Articles 4 and 7.
NOTE. Initial value:SMR7"""@en ;
                                                                                                                                                                                   <http://www.w3.org/2004/02/skos/core#inScheme> :CrossComplianceRuleValue .


###  http://lpis.ec.europa.eu/registry/applicationschema/cap-iacs-base/code#CrossComplianceRuleValue/publicHealthAnimalHealthAndPlantHealthIdentificationAndRegistrationOfAnimalsSmr8
<http://lpis.ec.europa.eu/registry/applicationschema/cap-iacs-base/code#CrossComplianceRuleValue/publicHealthAnimalHealthAndPlantHealthIdentificationAndRegistrationOfAnimalsSmr8> rdf:type owl:NamedIndividual ,
                                                                                                                                                                                            <http://lpis.ec.europa.eu/registry/applicationschema/cap-iacs-base#CrossComplianceRuleValue> ;
                                                                                                                                                                                   rdfs:label "Public health, animal health and plant health  - Identification and registration of animals SMR8"@en ;
                                                                                                                                                                                   <http://www.w3.org/2004/02/skos/core#definition> """-- Definition --
Public health, animal health and plant health  - Identification and registration of animals SMR8.
-- Description --
Council Regulation (EC) No 21/2004 of 17 December 2003 establishing a system for the identification and registration of ovine and caprine animals and amending Regulation (EC) No 1782/2003 and Directives 92/102/EEC and 64/432/EEC (OJ L 5, 9.1.2004, p. 8). Articles 3, 4 and 5.
NOTE. Initial value:SMR8"""@en ;
                                                                                                                                                                                   <http://www.w3.org/2004/02/skos/core#inScheme> :CrossComplianceRuleValue .


###  http://lpis.ec.europa.eu/registry/applicationschema/cap-iacs-base/code#CrossComplianceRuleValue/publicHealthAnimalHealthAndPlantHealthPlantProtectionProductsSmr10
<http://lpis.ec.europa.eu/registry/applicationschema/cap-iacs-base/code#CrossComplianceRuleValue/publicHealthAnimalHealthAndPlantHealthPlantProtectionProductsSmr10> rdf:type owl:NamedIndividual ,
                                                                                                                                                                              <http://lpis.ec.europa.eu/registry/applicationschema/cap-iacs-base#CrossComplianceRuleValue> ;
                                                                                                                                                                     rdfs:label "Public health, animal health and plant health  - Plant protection products SMR10"@en ;
                                                                                                                                                                     <http://www.w3.org/2004/02/skos/core#definition> """-- Definition --
Public health, animal health and plant health  - Plant protection products SMR10
-- Description --
Regulation (EC) No 1107/2009 of the European Parliament and of the Council of 21 October 2009 concerning the placing of plant protection products on the market and repealing Council Directives 79/117/EEC and 91/414/EEC (OJ L 309, 24.11.2009, p. 1). Article 55, first and second sentence.
NOTE. Initial value:SMR10"""@en ;
                                                                                                                                                                     <http://www.w3.org/2004/02/skos/core#inScheme> :CrossComplianceRuleValue .


###  http://lpis.ec.europa.eu/registry/applicationschema/cap-iacs-base/code#FarmStructureSurveyNumberValue/arableLand
<http://lpis.ec.europa.eu/registry/applicationschema/cap-iacs-base/code#FarmStructureSurveyNumberValue/arableLand> rdf:type owl:NamedIndividual ,
                                                                                                                            <http://lpis.ec.europa.eu/registry/applicationschema/cap-iacs-base#FarmStructureSurveyNumberValue> ;
                                                                                                                   rdfs:label "Arable land"@en ;
                                                                                                                   <http://www.w3.org/2004/02/skos/core#definition> """-- Definition --
Arable land.
-- Description --
Land worked (ploughed or tilled) regularly, generally under a system of crop rotation.
Crop rotation is the practice of alternating annual crops grown on a specific field in a planned pattern or sequence in successive crop years so that crops of the same species are not grown without interruption on the same field. Normally the crops are changed annually, but they can also be multiannual. To distinguish arable land from permanent crops or permanent grassland, a threshold of five years is used. This means that if a plot is used for the same crop for five years or more, without in the meantime removing the preceding crop and establishing a new one, it is not considered arable land.
NOTE. Initial value:2.01"""@en ;
                                                                                                                   <http://www.w3.org/2004/02/skos/core#inScheme> :FarmStructureSurveyNumberValue .


###  http://lpis.ec.europa.eu/registry/applicationschema/cap-iacs-base/code#FarmStructureSurveyNumberValue/arableLandSeedAndSeedlings
<http://lpis.ec.europa.eu/registry/applicationschema/cap-iacs-base/code#FarmStructureSurveyNumberValue/arableLandSeedAndSeedlings> rdf:type owl:NamedIndividual ,
                                                                                                                                            <http://lpis.ec.europa.eu/registry/applicationschema/cap-iacs-base#FarmStructureSurveyNumberValue> ;
                                                                                                                                   rdfs:label "Arable land seed and seedlings"@en ;
                                                                                                                                   <http://www.w3.org/2004/02/skos/core#definition> """-- Definition --
Arable land seed and seedlings.
-- Description --
Areas producing seeds and seedlings for sale, excluding cereals, rice, pulses, potatoes and oil seeds.
NOTE. Initial value:2.01.10"""@en ;
                                                                                                                                   <http://www.w3.org/2004/02/skos/core#inScheme> :FarmStructureSurveyNumberValue .


###  http://lpis.ec.europa.eu/registry/applicationschema/cap-iacs-base/code#FarmStructureSurveyNumberValue/aromaticPlantsMedicinalAndCulinaryPlants
<http://lpis.ec.europa.eu/registry/applicationschema/cap-iacs-base/code#FarmStructureSurveyNumberValue/aromaticPlantsMedicinalAndCulinaryPlants> rdf:type owl:NamedIndividual ,
                                                                                                                                                          <http://lpis.ec.europa.eu/registry/applicationschema/cap-iacs-base#FarmStructureSurveyNumberValue> ;
                                                                                                                                                 rdfs:label "Aromatic plants, medicinal and culinary plants"@en ;
                                                                                                                                                 <http://www.w3.org/2004/02/skos/core#definition> """-- Definition --
Aromatic plants, medicinal and culinary plants.
-- Description --
Plants or parts of plants for pharmaceutical purposes, perfume manufacture or human consumption.
Culinary plants are distinguished from vegetables in that they are used in small amounts and provide flavour rather than substance to food.
NOTE. Initial value:2.01.06.12"""@en ;
                                                                                                                                                 <http://www.w3.org/2004/02/skos/core#inScheme> :FarmStructureSurveyNumberValue .


###  http://lpis.ec.europa.eu/registry/applicationschema/cap-iacs-base/code#FarmStructureSurveyNumberValue/barley
<http://lpis.ec.europa.eu/registry/applicationschema/cap-iacs-base/code#FarmStructureSurveyNumberValue/barley> rdf:type owl:NamedIndividual ,
                                                                                                                        <http://lpis.ec.europa.eu/registry/applicationschema/cap-iacs-base#FarmStructureSurveyNumberValue> ;
                                                                                                               rdfs:label "Barley"@en ;
                                                                                                               <http://www.w3.org/2004/02/skos/core#definition> """-- Definition --
Barley.
-- Description --
Hordeum vulgare L.
NOTE. Initial value:2.01.01.04"""@en ;
                                                                                                               <http://www.w3.org/2004/02/skos/core#inScheme> :FarmStructureSurveyNumberValue .


###  http://lpis.ec.europa.eu/registry/applicationschema/cap-iacs-base/code#FarmStructureSurveyNumberValue/berrySpecies
<http://lpis.ec.europa.eu/registry/applicationschema/cap-iacs-base/code#FarmStructureSurveyNumberValue/berrySpecies> rdf:type owl:NamedIndividual ,
                                                                                                                              <http://lpis.ec.europa.eu/registry/applicationschema/cap-iacs-base#FarmStructureSurveyNumberValue> ;
                                                                                                                     rdfs:label "Berry species"@en ;
                                                                                                                     <http://www.w3.org/2004/02/skos/core#definition> """-- Definition --
Berry species.
-- Description --
Berry plantations which are traditionally cropped both in temperate and subtropical climates for producing berries.
NOTE. Initial value:2.04.01.02"""@en ;
                                                                                                                     <http://www.w3.org/2004/02/skos/core#inScheme> :FarmStructureSurveyNumberValue .


###  http://lpis.ec.europa.eu/registry/applicationschema/cap-iacs-base/code#FarmStructureSurveyNumberValue/cerealsForTheProductionOfGrainIncludingSeed
<http://lpis.ec.europa.eu/registry/applicationschema/cap-iacs-base/code#FarmStructureSurveyNumberValue/cerealsForTheProductionOfGrainIncludingSeed> rdf:type owl:NamedIndividual ,
                                                                                                                                                             <http://lpis.ec.europa.eu/registry/applicationschema/cap-iacs-base#FarmStructureSurveyNumberValue> ;
                                                                                                                                                    rdfs:label "Cereals for the production of grain (including seed)"@en ;
                                                                                                                                                    <http://www.w3.org/2004/02/skos/core#definition> """-- Definition --
Cereals for the production of grain (including seed).
-- Description --
All areas of cereals harvested dry for grain, regardless of use, shall be recorded here (including cereals used for renewable energy production).
NOTE. Initial value:2.01.01"""@en ;
                                                                                                                                                    <http://www.w3.org/2004/02/skos/core#inScheme> :FarmStructureSurveyNumberValue .


###  http://lpis.ec.europa.eu/registry/applicationschema/cap-iacs-base/code#FarmStructureSurveyNumberValue/citrusPlantations
<http://lpis.ec.europa.eu/registry/applicationschema/cap-iacs-base/code#FarmStructureSurveyNumberValue/citrusPlantations> rdf:type owl:NamedIndividual ,
                                                                                                                                   <http://lpis.ec.europa.eu/registry/applicationschema/cap-iacs-base#FarmStructureSurveyNumberValue> ;
                                                                                                                          rdfs:label "Citrus plantations"@en ;
                                                                                                                          <http://www.w3.org/2004/02/skos/core#definition> """-- Definition --
Citrus plantations.
-- Description --
Plantations of Citrus spp.
NOTE. Initial value:2.04.02"""@en ;
                                                                                                                          <http://www.w3.org/2004/02/skos/core#inScheme> :FarmStructureSurveyNumberValue .


###  http://lpis.ec.europa.eu/registry/applicationschema/cap-iacs-base/code#FarmStructureSurveyNumberValue/commonWheatAndSpelt
<http://lpis.ec.europa.eu/registry/applicationschema/cap-iacs-base/code#FarmStructureSurveyNumberValue/commonWheatAndSpelt> rdf:type owl:NamedIndividual ,
                                                                                                                                     <http://lpis.ec.europa.eu/registry/applicationschema/cap-iacs-base#FarmStructureSurveyNumberValue> ;
                                                                                                                            rdfs:label "Common wheat and spelt"@en ;
                                                                                                                            <http://www.w3.org/2004/02/skos/core#definition> """-- Definition --
Common wheat and spelt.
-- Description --
Triticum aestivum L. emend. Fiori et Paol., Triticum spelta L. and Triticum monococcum L.
NOTE. Initial value:2.01.01.01"""@en ;
                                                                                                                            <http://www.w3.org/2004/02/skos/core#inScheme> :FarmStructureSurveyNumberValue .


###  http://lpis.ec.europa.eu/registry/applicationschema/cap-iacs-base/code#FarmStructureSurveyNumberValue/cotton
<http://lpis.ec.europa.eu/registry/applicationschema/cap-iacs-base/code#FarmStructureSurveyNumberValue/cotton> rdf:type owl:NamedIndividual ,
                                                                                                                        <http://lpis.ec.europa.eu/registry/applicationschema/cap-iacs-base#FarmStructureSurveyNumberValue> ;
                                                                                                               rdfs:label "Cotton"@en ;
                                                                                                               <http://www.w3.org/2004/02/skos/core#definition> """-- Definition --
Cotton.
-- Description --
Gossypium spp., harvested for fibre as well as for oil-seeds.
NOTE. Initial value:2.01.06.03"""@en ;
                                                                                                               <http://www.w3.org/2004/02/skos/core#inScheme> :FarmStructureSurveyNumberValue .


###  http://lpis.ec.europa.eu/registry/applicationschema/cap-iacs-base/code#FarmStructureSurveyNumberValue/driedPulsesAndProteinCropsForTheProductionOfGrain
<http://lpis.ec.europa.eu/registry/applicationschema/cap-iacs-base/code#FarmStructureSurveyNumberValue/driedPulsesAndProteinCropsForTheProductionOfGrain> rdf:type owl:NamedIndividual ,
                                                                                                                                                                   <http://lpis.ec.europa.eu/registry/applicationschema/cap-iacs-base#FarmStructureSurveyNumberValue> ;
                                                                                                                                                          rdfs:label "Dried pulses and protein crops for the production of grain"@en ;
                                                                                                                                                          <http://www.w3.org/2004/02/skos/core#definition> """-- Definition --
Dried pulses and protein crops for the production of grain.
-- Description --
Dried pulses and protein crops for the production of grain (including seed and mixtures of cereals and pulses)
Crops sown and harvested mainly for their protein content.
All areas of dried pulses and protein crops harvested dry for grain, regardless of use, shall be recorded here (including crops used for renewable energy production).
NOTE. Initial value:2.01.02"""@en ;
                                                                                                                                                          <http://www.w3.org/2004/02/skos/core#inScheme> :FarmStructureSurveyNumberValue .


###  http://lpis.ec.europa.eu/registry/applicationschema/cap-iacs-base/code#FarmStructureSurveyNumberValue/durumWheat
<http://lpis.ec.europa.eu/registry/applicationschema/cap-iacs-base/code#FarmStructureSurveyNumberValue/durumWheat> rdf:type owl:NamedIndividual ,
                                                                                                                            <http://lpis.ec.europa.eu/registry/applicationschema/cap-iacs-base#FarmStructureSurveyNumberValue> ;
                                                                                                                   rdfs:label "Durum wheat"@en ;
                                                                                                                   <http://www.w3.org/2004/02/skos/core#definition> """-- Definition --
Durum wheat.
-- Description --
Triticum durum Desf.
NOTE. Initial value:2.01.01.02"""@en ;
                                                                                                                   <http://www.w3.org/2004/02/skos/core#inScheme> :FarmStructureSurveyNumberValue .


###  http://lpis.ec.europa.eu/registry/applicationschema/cap-iacs-base/code#FarmStructureSurveyNumberValue/energyCropsForTheProductionOfBiofuelsOrOtherRenewableEnergy
<http://lpis.ec.europa.eu/registry/applicationschema/cap-iacs-base/code#FarmStructureSurveyNumberValue/energyCropsForTheProductionOfBiofuelsOrOtherRenewableEnergy> rdf:type owl:NamedIndividual ,
                                                                                                                                                                             <http://lpis.ec.europa.eu/registry/applicationschema/cap-iacs-base#FarmStructureSurveyNumberValue> ;
                                                                                                                                                                    rdfs:label "Energy crops (for the production of biofuels or other renewable energy)"@en ;
                                                                                                                                                                    <http://www.w3.org/2004/02/skos/core#definition> """-- Definition --
Energy crops (for the production of biofuels or other renewable energy).
-- Description --
The production area of energy crops benefiting from the following support schemes under Regulation (EC) No 1782/2003: the specific aid for energy crops (Article 88), the payment linked to set-aside entitlement when production takes place on set-aside area (Article 55 or 56).
Other areas used for the production of energy crops (notably benefiting of the payment linked to‘normal’ entitlement under the Single Payment Scheme or the Simplified Area Payment Scheme) are not covered.
NOTE. Initial value:2.06.03"""@en ;
                                                                                                                                                                    <http://www.w3.org/2004/02/skos/core#inScheme> :FarmStructureSurveyNumberValue .


###  http://lpis.ec.europa.eu/registry/applicationschema/cap-iacs-base/code#FarmStructureSurveyNumberValue/fallowLand
<http://lpis.ec.europa.eu/registry/applicationschema/cap-iacs-base/code#FarmStructureSurveyNumberValue/fallowLand> rdf:type owl:NamedIndividual ,
                                                                                                                            <http://lpis.ec.europa.eu/registry/applicationschema/cap-iacs-base#FarmStructureSurveyNumberValue> ;
                                                                                                                   rdfs:label "Fallow land"@en ;
                                                                                                                   <http://www.w3.org/2004/02/skos/core#definition> """-- Definition --
Fallow land.
-- Description --
All arable land included in the crop rotation system, whether worked or not, but with no intention to produce a harvest for the duration of a crop year.
The essential characteristic of fallow land is that it is left to recover, normally for the whole of a crop year.
Fallow land may be:
1. bare land bearing no crops at all;
2. land with spontaneous natural growth, which may be used as feed or ploughed in;
3. land sown exclusively for the production of green manure (green fallow).
All areas of arable land maintained in good agricultural and environmental conditions as set out in Article 5 of the Council Regulation (EC) No 1782/2003(1)
OJ L 270, 21.10.2003, p. 1. (1) or, where applicable, in the most recent legislation, regardless of whether they are part of the crop rotation or not, are included.
NOTE. Initial value:2.01.12"""@en ;
                                                                                                                   <http://www.w3.org/2004/02/skos/core#inScheme> :FarmStructureSurveyNumberValue .


###  http://lpis.ec.europa.eu/registry/applicationschema/cap-iacs-base/code#FarmStructureSurveyNumberValue/fallowLandSubjectToThePaymentOfSubsidiesWithNoEconomicUse
<http://lpis.ec.europa.eu/registry/applicationschema/cap-iacs-base/code#FarmStructureSurveyNumberValue/fallowLandSubjectToThePaymentOfSubsidiesWithNoEconomicUse> rdf:type owl:NamedIndividual ,
                                                                                                                                                                           <http://lpis.ec.europa.eu/registry/applicationschema/cap-iacs-base#FarmStructureSurveyNumberValue> ;
                                                                                                                                                                  rdfs:label "Fallow land subject to the payment of subsidies, with no economic use"@en ;
                                                                                                                                                                  <http://www.w3.org/2004/02/skos/core#definition> """-- Definition --
Fallow land subject to the payment of subsidies, with no economic use.
-- Description --
Fallow land for which the holding is entitled to financial aid.
NOTE. Initial value:2.01.12.02"""@en ;
                                                                                                                                                                  <http://www.w3.org/2004/02/skos/core#inScheme> :FarmStructureSurveyNumberValue .


###  http://lpis.ec.europa.eu/registry/applicationschema/cap-iacs-base/code#FarmStructureSurveyNumberValue/flax
<http://lpis.ec.europa.eu/registry/applicationschema/cap-iacs-base/code#FarmStructureSurveyNumberValue/flax> rdf:type owl:NamedIndividual ,
                                                                                                                      <http://lpis.ec.europa.eu/registry/applicationschema/cap-iacs-base#FarmStructureSurveyNumberValue> ;
                                                                                                             rdfs:label "Flax"@en ;
                                                                                                             <http://www.w3.org/2004/02/skos/core#definition> """-- Definition --
Flax.
-- Description --
Linum usitatissimum L., varieties grown mainly for producing fibre.
NOTE. Initial value:2.01.06.09"""@en ;
                                                                                                             <http://www.w3.org/2004/02/skos/core#inScheme> :FarmStructureSurveyNumberValue .


###  http://lpis.ec.europa.eu/registry/applicationschema/cap-iacs-base/code#FarmStructureSurveyNumberValue/flowersAndOrnamentalPlantsExcludingNurseries
<http://lpis.ec.europa.eu/registry/applicationschema/cap-iacs-base/code#FarmStructureSurveyNumberValue/flowersAndOrnamentalPlantsExcludingNurseries> rdf:type owl:NamedIndividual ,
                                                                                                                                                              <http://lpis.ec.europa.eu/registry/applicationschema/cap-iacs-base#FarmStructureSurveyNumberValue> ;
                                                                                                                                                     rdfs:label "Flowers and ornamental plants (excluding nurseries)"@en ;
                                                                                                                                                     <http://www.w3.org/2004/02/skos/core#definition> """-- Definition --
Flowers and ornamental plants (excluding nurseries).
-- Description --
Flowers and ornamental plants (excluding nurseries).
NOTE. Initial value:2.01.08"""@en ;
                                                                                                                                                     <http://www.w3.org/2004/02/skos/core#inScheme> :FarmStructureSurveyNumberValue .


###  http://lpis.ec.europa.eu/registry/applicationschema/cap-iacs-base/code#FarmStructureSurveyNumberValue/fodderRootsAndBrassicasExcludingSeed
<http://lpis.ec.europa.eu/registry/applicationschema/cap-iacs-base/code#FarmStructureSurveyNumberValue/fodderRootsAndBrassicasExcludingSeed> rdf:type owl:NamedIndividual ,
                                                                                                                                                      <http://lpis.ec.europa.eu/registry/applicationschema/cap-iacs-base#FarmStructureSurveyNumberValue> ;
                                                                                                                                             rdfs:label "Fodder roots and brassicas (excluding seed)"@en ;
                                                                                                                                             <http://www.w3.org/2004/02/skos/core#definition> """-- Definition --
Fodder roots and brassicas (excluding seed)
-- Description --
Fodder beet (Beta vulgaris L.) and plants of the Brassicae family harvested mainly for animal feed, regardless whether it is the root or the stem, and other plants cultivated mainly for their roots for fodder, not mentioned elsewhere.
NOTE. Initial value:2.01.05"""@en ;
                                                                                                                                             <http://www.w3.org/2004/02/skos/core#inScheme> :FarmStructureSurveyNumberValue .


###  http://lpis.ec.europa.eu/registry/applicationschema/cap-iacs-base/code#FarmStructureSurveyNumberValue/freshVegetablesMelonsAndStrawberriesOfWhich
<http://lpis.ec.europa.eu/registry/applicationschema/cap-iacs-base/code#FarmStructureSurveyNumberValue/freshVegetablesMelonsAndStrawberriesOfWhich> rdf:type owl:NamedIndividual ,
                                                                                                                                                             <http://lpis.ec.europa.eu/registry/applicationschema/cap-iacs-base#FarmStructureSurveyNumberValue> ;
                                                                                                                                                    rdfs:label "Fresh vegetables, melons and strawberries of which:"@en ;
                                                                                                                                                    <http://www.w3.org/2004/02/skos/core#definition> """-- Definition --
Fresh vegetables, melons and strawberries of which:
-- Description --
Fresh vegetables, melons and strawberries of which:
NOTE. Initial value:2.01.07"""@en ;
                                                                                                                                                    <http://www.w3.org/2004/02/skos/core#inScheme> :FarmStructureSurveyNumberValue .


###  http://lpis.ec.europa.eu/registry/applicationschema/cap-iacs-base/code#FarmStructureSurveyNumberValue/fruitAndBerryPlantations
<http://lpis.ec.europa.eu/registry/applicationschema/cap-iacs-base/code#FarmStructureSurveyNumberValue/fruitAndBerryPlantations> rdf:type owl:NamedIndividual ,
                                                                                                                                          <http://lpis.ec.europa.eu/registry/applicationschema/cap-iacs-base#FarmStructureSurveyNumberValue> ;
                                                                                                                                 rdfs:label "Fruit and berry plantations"@en ;
                                                                                                                                 <http://www.w3.org/2004/02/skos/core#definition> """-- Definition --
Fruit and berry plantations.
-- Description --
Areas containing trees, bushes and perennial berry plants other than strawberries for the production of fruit. Orchards may be of the continuous type with minimum spacing between trees or of the non-continuous type with wide spacing.
NOTE. Initial value:2.04.01"""@en ;
                                                                                                                                 <http://www.w3.org/2004/02/skos/core#inScheme> :FarmStructureSurveyNumberValue .


###  http://lpis.ec.europa.eu/registry/applicationschema/cap-iacs-base/code#FarmStructureSurveyNumberValue/fruitSpeciesOfWhich
<http://lpis.ec.europa.eu/registry/applicationschema/cap-iacs-base/code#FarmStructureSurveyNumberValue/fruitSpeciesOfWhich> rdf:type owl:NamedIndividual ,
                                                                                                                                     <http://lpis.ec.europa.eu/registry/applicationschema/cap-iacs-base#FarmStructureSurveyNumberValue> ;
                                                                                                                            rdfs:label "Fruit species, of which:"@en ;
                                                                                                                            <http://www.w3.org/2004/02/skos/core#definition> """-- Definition --
Fruit species, of which:
-- Description --
Fruit species, of which:
NOTE. Initial value:2.04.01.01"""@en ;
                                                                                                                            <http://www.w3.org/2004/02/skos/core#inScheme> :FarmStructureSurveyNumberValue .


###  http://lpis.ec.europa.eu/registry/applicationschema/cap-iacs-base/code#FarmStructureSurveyNumberValue/fruitSpeciesOfWhichFruitOfSubtropicalClimateZones
<http://lpis.ec.europa.eu/registry/applicationschema/cap-iacs-base/code#FarmStructureSurveyNumberValue/fruitSpeciesOfWhichFruitOfSubtropicalClimateZones> rdf:type owl:NamedIndividual ,
                                                                                                                                                                   <http://lpis.ec.europa.eu/registry/applicationschema/cap-iacs-base#FarmStructureSurveyNumberValue> ;
                                                                                                                                                          rdfs:label "Fruit species, of which: Fruit of subtropical climate zones"@en ;
                                                                                                                                                          <http://www.w3.org/2004/02/skos/core#definition> """-- Definition --
Fruit species, of which: Fruit of subtropical climate zones.
-- Description --
Fruit tree plantations which are traditionally cropped in subtropical climates for producing fruits.
NOTE. Initial value:2.04.01.01.02"""@en ;
                                                                                                                                                          <http://www.w3.org/2004/02/skos/core#inScheme> :FarmStructureSurveyNumberValue .


###  http://lpis.ec.europa.eu/registry/applicationschema/cap-iacs-base/code#FarmStructureSurveyNumberValue/fruitSpeciesOfWhichFruitOfTemperateClimateZones
<http://lpis.ec.europa.eu/registry/applicationschema/cap-iacs-base/code#FarmStructureSurveyNumberValue/fruitSpeciesOfWhichFruitOfTemperateClimateZones> rdf:type owl:NamedIndividual ,
                                                                                                                                                                 <http://lpis.ec.europa.eu/registry/applicationschema/cap-iacs-base#FarmStructureSurveyNumberValue> ;
                                                                                                                                                        rdfs:label "Fruit species, of which: Fruit of temperate climate zones"@en ;
                                                                                                                                                        <http://www.w3.org/2004/02/skos/core#definition> """-- Definition --
Fruit species, of which: Fruit of temperate climate zones.
-- Description --
Fruit tree plantations which are traditionally cropped in temperate climates for producing fruits.
NOTE. Initial value:2.04.01.01.01"""@en ;
                                                                                                                                                        <http://www.w3.org/2004/02/skos/core#inScheme> :FarmStructureSurveyNumberValue .


###  http://lpis.ec.europa.eu/registry/applicationschema/cap-iacs-base/code#FarmStructureSurveyNumberValue/geneticallyModifiedCrops
<http://lpis.ec.europa.eu/registry/applicationschema/cap-iacs-base/code#FarmStructureSurveyNumberValue/geneticallyModifiedCrops> rdf:type owl:NamedIndividual ,
                                                                                                                                          <http://lpis.ec.europa.eu/registry/applicationschema/cap-iacs-base#FarmStructureSurveyNumberValue> ;
                                                                                                                                 rdfs:label "Genetically modified crops"@en ;
                                                                                                                                 <http://www.w3.org/2004/02/skos/core#definition> """-- Definition --
Genetically modified crops.
-- Description --
‘Genetically modified crops (GMC)’ mean any organism as defined in Article 2 of Council Directive 2001/18/EC(1) OJ L 106, 17.4.2001, p. 1. (1) or, where applicable, the most recent legislation.
NOTE. Initial value:2.06.04"""@en ;
                                                                                                                                 <http://www.w3.org/2004/02/skos/core#inScheme> :FarmStructureSurveyNumberValue .


###  http://lpis.ec.europa.eu/registry/applicationschema/cap-iacs-base/code#FarmStructureSurveyNumberValue/grainMaize
<http://lpis.ec.europa.eu/registry/applicationschema/cap-iacs-base/code#FarmStructureSurveyNumberValue/grainMaize> rdf:type owl:NamedIndividual ,
                                                                                                                            <http://lpis.ec.europa.eu/registry/applicationschema/cap-iacs-base#FarmStructureSurveyNumberValue> ;
                                                                                                                   rdfs:label "Grain maize"@en ;
                                                                                                                   <http://www.w3.org/2004/02/skos/core#definition> """-- Definition --
Grain maize.
-- Description --
Maize (Zea mays L.) harvested for grain.
NOTE. Initial value:2.01.01.06"""@en ;
                                                                                                                   <http://www.w3.org/2004/02/skos/core#inScheme> :FarmStructureSurveyNumberValue .


###  http://lpis.ec.europa.eu/registry/applicationschema/cap-iacs-base/code#FarmStructureSurveyNumberValue/greenMaize
<http://lpis.ec.europa.eu/registry/applicationschema/cap-iacs-base/code#FarmStructureSurveyNumberValue/greenMaize> rdf:type owl:NamedIndividual ,
                                                                                                                            <http://lpis.ec.europa.eu/registry/applicationschema/cap-iacs-base#FarmStructureSurveyNumberValue> ;
                                                                                                                   rdfs:label "Green maize"@en ;
                                                                                                                   <http://www.w3.org/2004/02/skos/core#definition> """-- Definition --
Green maize.
-- Description --
All forms of maize (Zea mays L.) grown mainly for silage, which is not harvested for grain (whole cob, parts of or whole plant).
This includes green maize directly consumed by animals (without silage) and whole cobs (grain, rachis, husk) harvested for feedstuff or silage as well as for renewable energy production.
NOTE. Initial value:2.01.09.02.01"""@en ;
                                                                                                                   <http://www.w3.org/2004/02/skos/core#inScheme> :FarmStructureSurveyNumberValue .


###  http://lpis.ec.europa.eu/registry/applicationschema/cap-iacs-base/code#FarmStructureSurveyNumberValue/hemp
<http://lpis.ec.europa.eu/registry/applicationschema/cap-iacs-base/code#FarmStructureSurveyNumberValue/hemp> rdf:type owl:NamedIndividual ,
                                                                                                                      <http://lpis.ec.europa.eu/registry/applicationschema/cap-iacs-base#FarmStructureSurveyNumberValue> ;
                                                                                                             rdfs:label "Hemp"@en ;
                                                                                                             <http://www.w3.org/2004/02/skos/core#definition> """-- Definition --
Hemp.
-- Description --
Cannabis sativa L.
NOTE. Initial value:2.01.06.10"""@en ;
                                                                                                             <http://www.w3.org/2004/02/skos/core#inScheme> :FarmStructureSurveyNumberValue .


###  http://lpis.ec.europa.eu/registry/applicationschema/cap-iacs-base/code#FarmStructureSurveyNumberValue/hops
<http://lpis.ec.europa.eu/registry/applicationschema/cap-iacs-base/code#FarmStructureSurveyNumberValue/hops> rdf:type owl:NamedIndividual ,
                                                                                                                      <http://lpis.ec.europa.eu/registry/applicationschema/cap-iacs-base#FarmStructureSurveyNumberValue> ;
                                                                                                             rdfs:label "Hops"@en ;
                                                                                                             <http://www.w3.org/2004/02/skos/core#definition> """-- Definition --
Hops.
-- Description --
Humulus lupulus L.
NOTE. Initial value:2.01.06.02"""@en ;
                                                                                                             <http://www.w3.org/2004/02/skos/core#inScheme> :FarmStructureSurveyNumberValue .


###  http://lpis.ec.europa.eu/registry/applicationschema/cap-iacs-base/code#FarmStructureSurveyNumberValue/industrialCrops
<http://lpis.ec.europa.eu/registry/applicationschema/cap-iacs-base/code#FarmStructureSurveyNumberValue/industrialCrops> rdf:type owl:NamedIndividual ,
                                                                                                                                 <http://lpis.ec.europa.eu/registry/applicationschema/cap-iacs-base#FarmStructureSurveyNumberValue> ;
                                                                                                                        rdfs:label "Industrial crops"@en ;
                                                                                                                        <http://www.w3.org/2004/02/skos/core#definition> """-- Definition --
Industrial crops.
-- Description --
Crops that are normally not sold directly for consumption because they need to be industrially processed prior to final use.
All harvested areas of industrial crops, regardless of use, shall be recorded here (including crops used for renewable energy production).
NOTE. Initial value:2.01.06"""@en ;
                                                                                                                        <http://www.w3.org/2004/02/skos/core#inScheme> :FarmStructureSurveyNumberValue .


###  http://lpis.ec.europa.eu/registry/applicationschema/cap-iacs-base/code#FarmStructureSurveyNumberValue/irrigatedArea
<http://lpis.ec.europa.eu/registry/applicationschema/cap-iacs-base/code#FarmStructureSurveyNumberValue/irrigatedArea> rdf:type owl:NamedIndividual ,
                                                                                                                               <http://lpis.ec.europa.eu/registry/applicationschema/cap-iacs-base#FarmStructureSurveyNumberValue> ;
                                                                                                                      rdfs:label "Irrigated area"@en ;
                                                                                                                      <http://www.w3.org/2004/02/skos/core#definition> """-- Definition --
Irrigated area.
-- Description --
Irrigated area.
NOTE. Initial value:2.06.02"""@en ;
                                                                                                                      <http://www.w3.org/2004/02/skos/core#inScheme> :FarmStructureSurveyNumberValue .


###  http://lpis.ec.europa.eu/registry/applicationschema/cap-iacs-base/code#FarmStructureSurveyNumberValue/kitchenGardens
<http://lpis.ec.europa.eu/registry/applicationschema/cap-iacs-base/code#FarmStructureSurveyNumberValue/kitchenGardens> rdf:type owl:NamedIndividual ,
                                                                                                                                <http://lpis.ec.europa.eu/registry/applicationschema/cap-iacs-base#FarmStructureSurveyNumberValue> ;
                                                                                                                       rdfs:label "Kitchen gardens"@en ;
                                                                                                                       <http://www.w3.org/2004/02/skos/core#definition> """-- Definition --
Kitchen gardens.
-- Description --
Areas devoted to the cultivation of agricultural products intended for self-consumption by the holder and his household, normally separated off from the rest of the agricultural land, and recognisable as kitchen gardens.
Only occasional surplus products coming from this area are sold off from the holding. All areas from which products are consistently sold on the market belong under other items, even if part of the production is consumed by the holder and his household.
NOTE. Initial value:2.02"""@en ;
                                                                                                                       <http://www.w3.org/2004/02/skos/core#inScheme> :FarmStructureSurveyNumberValue .


###  http://lpis.ec.europa.eu/registry/applicationschema/cap-iacs-base/code#FarmStructureSurveyNumberValue/lallowLandWithoutAnySubsidies
<http://lpis.ec.europa.eu/registry/applicationschema/cap-iacs-base/code#FarmStructureSurveyNumberValue/lallowLandWithoutAnySubsidies> rdf:type owl:NamedIndividual ,
                                                                                                                                               <http://lpis.ec.europa.eu/registry/applicationschema/cap-iacs-base#FarmStructureSurveyNumberValue> ;
                                                                                                                                      rdfs:label "Fallow land without any subsidies"@en ;
                                                                                                                                      <http://www.w3.org/2004/02/skos/core#definition> """-- Definition --
Fallow land without any subsidies.
-- Description --
Fallow land for which no financial aid or subsidy is paid.
NOTE. Initial value:2.01.12.01"""@en ;
                                                                                                                                      <http://www.w3.org/2004/02/skos/core#inScheme> :FarmStructureSurveyNumberValue .


###  http://lpis.ec.europa.eu/registry/applicationschema/cap-iacs-base/code#FarmStructureSurveyNumberValue/leguminousPlants
<http://lpis.ec.europa.eu/registry/applicationschema/cap-iacs-base/code#FarmStructureSurveyNumberValue/leguminousPlants> rdf:type owl:NamedIndividual ,
                                                                                                                                  <http://lpis.ec.europa.eu/registry/applicationschema/cap-iacs-base#FarmStructureSurveyNumberValue> ;
                                                                                                                         rdfs:label "Leguminous plants"@en ;
                                                                                                                         <http://www.w3.org/2004/02/skos/core#definition> """-- Definition --
Leguminous plants.
-- Description --
Leguminous plants grown and harvested green as the whole plant mainly for forage.
Mixtures of predominantly leguminous (normally > 80 %) forage crops and grass plants, harvested green or as dried hay are included here.
NOTE. Initial value:2.01.09.02.02"""@en ;
                                                                                                                         <http://www.w3.org/2004/02/skos/core#inScheme> :FarmStructureSurveyNumberValue .


###  http://lpis.ec.europa.eu/registry/applicationschema/cap-iacs-base/code#FarmStructureSurveyNumberValue/linseedOilFlax
<http://lpis.ec.europa.eu/registry/applicationschema/cap-iacs-base/code#FarmStructureSurveyNumberValue/linseedOilFlax> rdf:type owl:NamedIndividual ,
                                                                                                                                <http://lpis.ec.europa.eu/registry/applicationschema/cap-iacs-base#FarmStructureSurveyNumberValue> ;
                                                                                                                       rdfs:label "Linseed (oil flax)"@en ;
                                                                                                                       <http://www.w3.org/2004/02/skos/core#definition> """-- Definition --
Linseed (oil flax).
-- Description --
Linum usitatissimum L., varieties grown mainly for producing oil, harvested as dry grains.
NOTE. Initial value:2.01.06.07"""@en ;
                                                                                                                       <http://www.w3.org/2004/02/skos/core#inScheme> :FarmStructureSurveyNumberValue .


###  http://lpis.ec.europa.eu/registry/applicationschema/cap-iacs-base/code#FarmStructureSurveyNumberValue/marketGardening
<http://lpis.ec.europa.eu/registry/applicationschema/cap-iacs-base/code#FarmStructureSurveyNumberValue/marketGardening> rdf:type owl:NamedIndividual ,
                                                                                                                                 <http://lpis.ec.europa.eu/registry/applicationschema/cap-iacs-base#FarmStructureSurveyNumberValue> ;
                                                                                                                        rdfs:label "Market gardening"@en ;
                                                                                                                        <http://www.w3.org/2004/02/skos/core#definition> """-- Definition --
Market gardening.
-- Description --
Fresh vegetables, melons and strawberries grown on arable land in rotation with other horticultural crops.
NOTE. Initial value:2.01.07.01.02"""@en ;
                                                                                                                        <http://www.w3.org/2004/02/skos/core#inScheme> :FarmStructureSurveyNumberValue .


###  http://lpis.ec.europa.eu/registry/applicationschema/cap-iacs-base/code#FarmStructureSurveyNumberValue/mushrooms
<http://lpis.ec.europa.eu/registry/applicationschema/cap-iacs-base/code#FarmStructureSurveyNumberValue/mushrooms> rdf:type owl:NamedIndividual ,
                                                                                                                           <http://lpis.ec.europa.eu/registry/applicationschema/cap-iacs-base#FarmStructureSurveyNumberValue> ;
                                                                                                                  rdfs:label "Mushrooms"@en ;
                                                                                                                  <http://www.w3.org/2004/02/skos/core#definition> """-- Definition --
Mushrooms.
-- Description --
Cultivated mushrooms grown in buildings which have been specially erected or adapted for growing mushrooms, as well as in underground premises, caves and cellars.
NOTE. Initial value:2.06.01"""@en ;
                                                                                                                  <http://www.w3.org/2004/02/skos/core#inScheme> :FarmStructureSurveyNumberValue .


###  http://lpis.ec.europa.eu/registry/applicationschema/cap-iacs-base/code#FarmStructureSurveyNumberValue/mushroomsIrrigatedAreaEnergyCropsAndGeneticallyModifiedCrops
<http://lpis.ec.europa.eu/registry/applicationschema/cap-iacs-base/code#FarmStructureSurveyNumberValue/mushroomsIrrigatedAreaEnergyCropsAndGeneticallyModifiedCrops> rdf:type owl:NamedIndividual ,
                                                                                                                                                                              <http://lpis.ec.europa.eu/registry/applicationschema/cap-iacs-base#FarmStructureSurveyNumberValue> ;
                                                                                                                                                                     rdfs:label "Mushrooms, irrigated area, energy crops and genetically modified crops"@en ;
                                                                                                                                                                     <http://www.w3.org/2004/02/skos/core#definition> """-- Definition --
Mushrooms, irrigated area, energy crops and genetically modified crops.
-- Description --
Mushrooms, irrigated area, energy crops and genetically modified crops.
NOTE. Initial value:2.06"""@en ;
                                                                                                                                                                     <http://www.w3.org/2004/02/skos/core#inScheme> :FarmStructureSurveyNumberValue .


###  http://lpis.ec.europa.eu/registry/applicationschema/cap-iacs-base/code#FarmStructureSurveyNumberValue/normallyProducingOlivesForOilProduction
<http://lpis.ec.europa.eu/registry/applicationschema/cap-iacs-base/code#FarmStructureSurveyNumberValue/normallyProducingOlivesForOilProduction> rdf:type owl:NamedIndividual ,
                                                                                                                                                         <http://lpis.ec.europa.eu/registry/applicationschema/cap-iacs-base#FarmStructureSurveyNumberValue> ;
                                                                                                                                                rdfs:label "Normally producing olives for oil production"@en ;
                                                                                                                                                <http://www.w3.org/2004/02/skos/core#definition> """-- Definition --
Normally producing olives for oil production.
-- Description --
Plantations of varieties normally grown for producing olive oil.
NOTE. Initial value:2.04.03.02"""@en ;
                                                                                                                                                <http://www.w3.org/2004/02/skos/core#inScheme> :FarmStructureSurveyNumberValue .


###  http://lpis.ec.europa.eu/registry/applicationschema/cap-iacs-base/code#FarmStructureSurveyNumberValue/normallyProducingTableOlives
<http://lpis.ec.europa.eu/registry/applicationschema/cap-iacs-base/code#FarmStructureSurveyNumberValue/normallyProducingTableOlives> rdf:type owl:NamedIndividual ,
                                                                                                                                              <http://lpis.ec.europa.eu/registry/applicationschema/cap-iacs-base#FarmStructureSurveyNumberValue> ;
                                                                                                                                     rdfs:label "Normally producing table olives"@en ;
                                                                                                                                     <http://www.w3.org/2004/02/skos/core#definition> """-- Definition --
Normally producing table olives.
-- Description --
Plantations of varieties normally grown for producing table olives.
NOTE. Initial value:2.04.03.01"""@en ;
                                                                                                                                     <http://www.w3.org/2004/02/skos/core#inScheme> :FarmStructureSurveyNumberValue .


###  http://lpis.ec.europa.eu/registry/applicationschema/cap-iacs-base/code#FarmStructureSurveyNumberValue/nurseries
<http://lpis.ec.europa.eu/registry/applicationschema/cap-iacs-base/code#FarmStructureSurveyNumberValue/nurseries> rdf:type owl:NamedIndividual ,
                                                                                                                           <http://lpis.ec.europa.eu/registry/applicationschema/cap-iacs-base#FarmStructureSurveyNumberValue> ;
                                                                                                                  rdfs:label "Nurseries"@en ;
                                                                                                                  <http://www.w3.org/2004/02/skos/core#definition> """-- Definition --
Nurseries.
-- Description --
Areas of young ligneous (woody) plants grown in the open air for subsequent transplantation:
(a) vine and root-stock nurseries;
(b) fruit tree and berries nurseries;
(c) ornamental nurseries;
(d) commercial nurseries of forest trees (excluding those for the holding’s own requirements grown within woodland);
(e) trees and bushes for planting in gardens, parks, at the roadside and on embankments (e.g. hedgerow plants, rose trees and other ornamental bushes, ornamental conifers), including in all cases their stocks and young seedlings.
NOTE. Initial value:2.04.05"""@en ;
                                                                                                                  <http://www.w3.org/2004/02/skos/core#inScheme> :FarmStructureSurveyNumberValue .


###  http://lpis.ec.europa.eu/registry/applicationschema/cap-iacs-base/code#FarmStructureSurveyNumberValue/nuts
<http://lpis.ec.europa.eu/registry/applicationschema/cap-iacs-base/code#FarmStructureSurveyNumberValue/nuts> rdf:type owl:NamedIndividual ,
                                                                                                                      <http://lpis.ec.europa.eu/registry/applicationschema/cap-iacs-base#FarmStructureSurveyNumberValue> ;
                                                                                                             rdfs:label "Nuts"@en ;
                                                                                                             <http://www.w3.org/2004/02/skos/core#definition> """-- Definition --
Nuts.
-- Description --
Nut tree plantations which are traditionally cropped in temperate and subtropical climates.
NOTE. Initial value:2.04.01.03"""@en ;
                                                                                                             <http://www.w3.org/2004/02/skos/core#inScheme> :FarmStructureSurveyNumberValue .


###  http://lpis.ec.europa.eu/registry/applicationschema/cap-iacs-base/code#FarmStructureSurveyNumberValue/oats
<http://lpis.ec.europa.eu/registry/applicationschema/cap-iacs-base/code#FarmStructureSurveyNumberValue/oats> rdf:type owl:NamedIndividual ,
                                                                                                                      <http://lpis.ec.europa.eu/registry/applicationschema/cap-iacs-base#FarmStructureSurveyNumberValue> ;
                                                                                                             rdfs:label "Oats"@en ;
                                                                                                             <http://www.w3.org/2004/02/skos/core#definition> """-- Definition --
Oats.
-- Description --
Avena sativa L., including mixtures of oats and other cereals sown in the spring.
NOTE. Initial value:2.01.01.05"""@en ;
                                                                                                             <http://www.w3.org/2004/02/skos/core#inScheme> :FarmStructureSurveyNumberValue .


###  http://lpis.ec.europa.eu/registry/applicationschema/cap-iacs-base/code#FarmStructureSurveyNumberValue/ofWhichChristmasTrees
<http://lpis.ec.europa.eu/registry/applicationschema/cap-iacs-base/code#FarmStructureSurveyNumberValue/ofWhichChristmasTrees> rdf:type owl:NamedIndividual ,
                                                                                                                                       <http://lpis.ec.europa.eu/registry/applicationschema/cap-iacs-base#FarmStructureSurveyNumberValue> ;
                                                                                                                              rdfs:label "of which Christmas trees(1)"@en ;
                                                                                                                              <http://www.w3.org/2004/02/skos/core#definition> """-- Definition --
of which Christmas trees(1).
-- Description --
Not to be provided in 2010. (1)
Trees planted for commercial purposes as Christmas trees on the utilised agricultural area.
NOTE. Initial value:2.04.06.01"""@en ;
                                                                                                                              <http://www.w3.org/2004/02/skos/core#inScheme> :FarmStructureSurveyNumberValue .


###  http://lpis.ec.europa.eu/registry/applicationschema/cap-iacs-base/code#FarmStructureSurveyNumberValue/ofWhichOnSetAsideArea
<http://lpis.ec.europa.eu/registry/applicationschema/cap-iacs-base/code#FarmStructureSurveyNumberValue/ofWhichOnSetAsideArea> rdf:type owl:NamedIndividual ,
                                                                                                                                       <http://lpis.ec.europa.eu/registry/applicationschema/cap-iacs-base#FarmStructureSurveyNumberValue> ;
                                                                                                                              rdfs:label "of which on set-aside area"@en ;
                                                                                                                              <http://www.w3.org/2004/02/skos/core#definition> """-- Definition --
of which on set-aside area.
-- Description --
The production area of energy crops benefiting of the payment linked to set-aside entitlement when production takes place on set-aside area (Council Regulation (EC) No 1782/2003, Article 55 or 56).
NOTE. Initial value:2.06.03.01"""@en ;
                                                                                                                              <http://www.w3.org/2004/02/skos/core#inScheme> :FarmStructureSurveyNumberValue .


###  http://lpis.ec.europa.eu/registry/applicationschema/cap-iacs-base/code#FarmStructureSurveyNumberValue/ofWhichPeasFieldBeansAndSweetLupins
<http://lpis.ec.europa.eu/registry/applicationschema/cap-iacs-base/code#FarmStructureSurveyNumberValue/ofWhichPeasFieldBeansAndSweetLupins> rdf:type owl:NamedIndividual ,
                                                                                                                                                     <http://lpis.ec.europa.eu/registry/applicationschema/cap-iacs-base#FarmStructureSurveyNumberValue> ;
                                                                                                                                            rdfs:label "of which peas, field beans and sweet lupins"@en ;
                                                                                                                                            <http://www.w3.org/2004/02/skos/core#definition> """-- Definition --
of which peas, field beans and sweet lupins.
-- Description --
Pisum sativum L., Vicia faba L., Lupinus spp., sown in pure crops, harvested dry for grain.
NOTE. Initial value:2.01.02.01"""@en ;
                                                                                                                                            <http://www.w3.org/2004/02/skos/core#inScheme> :FarmStructureSurveyNumberValue .


###  http://lpis.ec.europa.eu/registry/applicationschema/cap-iacs-base/code#FarmStructureSurveyNumberValue/ofWhichShortRotationCoppices
<http://lpis.ec.europa.eu/registry/applicationschema/cap-iacs-base/code#FarmStructureSurveyNumberValue/ofWhichShortRotationCoppices> rdf:type owl:NamedIndividual ,
                                                                                                                                              <http://lpis.ec.europa.eu/registry/applicationschema/cap-iacs-base#FarmStructureSurveyNumberValue> ;
                                                                                                                                     rdfs:label "of which short rotation coppices"@en ;
                                                                                                                                     <http://www.w3.org/2004/02/skos/core#definition> """-- Definition --
of which short rotation coppices.
-- Description --
Wooded areas managed for growing wooded plants, where the rotation period is 20 years or less.
The rotation period is the time between the first sowing/planting of the trees and the harvest of the final product, where harvesting does not include normal management actions like thinning.
NOTE. Initial value:2.05.02.01"""@en ;
                                                                                                                                     <http://www.w3.org/2004/02/skos/core#inScheme> :FarmStructureSurveyNumberValue .


###  http://lpis.ec.europa.eu/registry/applicationschema/cap-iacs-base/code#FarmStructureSurveyNumberValue/olivePlantations
<http://lpis.ec.europa.eu/registry/applicationschema/cap-iacs-base/code#FarmStructureSurveyNumberValue/olivePlantations> rdf:type owl:NamedIndividual ,
                                                                                                                                  <http://lpis.ec.europa.eu/registry/applicationschema/cap-iacs-base#FarmStructureSurveyNumberValue> ;
                                                                                                                         rdfs:label "Olive plantations"@en ;
                                                                                                                         <http://www.w3.org/2004/02/skos/core#definition> """-- Definition --
Olive plantations.
-- Description --
Plantations of Olea europea L.
NOTE. Initial value:2.04.03"""@en ;
                                                                                                                         <http://www.w3.org/2004/02/skos/core#inScheme> :FarmStructureSurveyNumberValue .


###  http://lpis.ec.europa.eu/registry/applicationschema/cap-iacs-base/code#FarmStructureSurveyNumberValue/openField
<http://lpis.ec.europa.eu/registry/applicationschema/cap-iacs-base/code#FarmStructureSurveyNumberValue/openField> rdf:type owl:NamedIndividual ,
                                                                                                                           <http://lpis.ec.europa.eu/registry/applicationschema/cap-iacs-base#FarmStructureSurveyNumberValue> ;
                                                                                                                  rdfs:label "Open field"@en ;
                                                                                                                  <http://www.w3.org/2004/02/skos/core#definition> """-- Definition --
Open field.
-- Description --
Fresh vegetables, melons and strawberries grown on arable land in rotation with other agricultural crops.
NOTE. Initial value:2.01.07.01.01"""@en ;
                                                                                                                  <http://www.w3.org/2004/02/skos/core#inScheme> :FarmStructureSurveyNumberValue .


###  http://lpis.ec.europa.eu/registry/applicationschema/cap-iacs-base/code#FarmStructureSurveyNumberValue/otherArableLandCrops
<http://lpis.ec.europa.eu/registry/applicationschema/cap-iacs-base/code#FarmStructureSurveyNumberValue/otherArableLandCrops> rdf:type owl:NamedIndividual ,
                                                                                                                                      <http://lpis.ec.europa.eu/registry/applicationschema/cap-iacs-base#FarmStructureSurveyNumberValue> ;
                                                                                                                             rdfs:label "Other arable land crops"@en ;
                                                                                                                             <http://www.w3.org/2004/02/skos/core#definition> """-- Definition --
Other arable land crops.
-- Description --
Arable crops not included elsewhere.
NOTE. Initial value:2.01.11"""@en ;
                                                                                                                             <http://www.w3.org/2004/02/skos/core#inScheme> :FarmStructureSurveyNumberValue .


###  http://lpis.ec.europa.eu/registry/applicationschema/cap-iacs-base/code#FarmStructureSurveyNumberValue/otherCerealsForTheProductionOfGrain
<http://lpis.ec.europa.eu/registry/applicationschema/cap-iacs-base/code#FarmStructureSurveyNumberValue/otherCerealsForTheProductionOfGrain> rdf:type owl:NamedIndividual ,
                                                                                                                                                     <http://lpis.ec.europa.eu/registry/applicationschema/cap-iacs-base#FarmStructureSurveyNumberValue> ;
                                                                                                                                            rdfs:label "Other cereals for the production of grain"@en ;
                                                                                                                                            <http://www.w3.org/2004/02/skos/core#definition> """-- Definition --
Other cereals for the production of grain.
-- Description --
Cereals sown in pure crops, harvested dry for grain, and that are not recorded elsewhere under the previous items.
NOTE. Initial value:2.01.01.99"""@en ;
                                                                                                                                            <http://www.w3.org/2004/02/skos/core#inScheme> :FarmStructureSurveyNumberValue .


###  http://lpis.ec.europa.eu/registry/applicationschema/cap-iacs-base/code#FarmStructureSurveyNumberValue/otherFibreCrops
<http://lpis.ec.europa.eu/registry/applicationschema/cap-iacs-base/code#FarmStructureSurveyNumberValue/otherFibreCrops> rdf:type owl:NamedIndividual ,
                                                                                                                                 <http://lpis.ec.europa.eu/registry/applicationschema/cap-iacs-base#FarmStructureSurveyNumberValue> ;
                                                                                                                        rdfs:label "Other fibre crops"@en ;
                                                                                                                        <http://www.w3.org/2004/02/skos/core#definition> """-- Definition --
Other fibre crops.
-- Description --
Other plants grown mainly for their fibre content, not mentioned elsewhere.
NOTE. Initial value:2.01.06.11"""@en ;
                                                                                                                        <http://www.w3.org/2004/02/skos/core#inScheme> :FarmStructureSurveyNumberValue .


###  http://lpis.ec.europa.eu/registry/applicationschema/cap-iacs-base/code#FarmStructureSurveyNumberValue/otherIndustrialCropsNotMentionedElsewhere
<http://lpis.ec.europa.eu/registry/applicationschema/cap-iacs-base/code#FarmStructureSurveyNumberValue/otherIndustrialCropsNotMentionedElsewhere> rdf:type owl:NamedIndividual ,
                                                                                                                                                           <http://lpis.ec.europa.eu/registry/applicationschema/cap-iacs-base#FarmStructureSurveyNumberValue> ;
                                                                                                                                                  rdfs:label "Other industrial crops not mentioned elsewhere"@en ;
                                                                                                                                                  <http://www.w3.org/2004/02/skos/core#definition> """-- Definition --
Other industrial crops not mentioned elsewhere.
-- Description --
Other industrial crops that have not been mentioned elsewhere.
Areas of crops used exclusively for renewable energy production are included.
NOTE. Initial value:2.01.06.99"""@en ;
                                                                                                                                                  <http://www.w3.org/2004/02/skos/core#inScheme> :FarmStructureSurveyNumberValue .


###  http://lpis.ec.europa.eu/registry/applicationschema/cap-iacs-base/code#FarmStructureSurveyNumberValue/otherLand
<http://lpis.ec.europa.eu/registry/applicationschema/cap-iacs-base/code#FarmStructureSurveyNumberValue/otherLand> rdf:type owl:NamedIndividual ,
                                                                                                                           <http://lpis.ec.europa.eu/registry/applicationschema/cap-iacs-base#FarmStructureSurveyNumberValue> ;
                                                                                                                  rdfs:label "Other land"@en ;
                                                                                                                  <http://www.w3.org/2004/02/skos/core#definition> """-- Definition --
Other land.
-- Description --
‘Other land’ includes unutilised agricultural land (agricultural land which is no longer farmed, for economic, social or other reasons, and which is not used in the crop rotation system), wooded area and other land occupied by buildings, farmyards, tracks, ponds, quarries, infertile land, rock, etc.
NOTE. Initial value:2.05"""@en ;
                                                                                                                  <http://www.w3.org/2004/02/skos/core#inScheme> :FarmStructureSurveyNumberValue .


###  http://lpis.ec.europa.eu/registry/applicationschema/cap-iacs-base/code#FarmStructureSurveyNumberValue/otherLandLandOccupiedByBuildingsFarmyardsTracksPondsQuarriesInfertileLandRockEtc
<http://lpis.ec.europa.eu/registry/applicationschema/cap-iacs-base/code#FarmStructureSurveyNumberValue/otherLandLandOccupiedByBuildingsFarmyardsTracksPondsQuarriesInfertileLandRockEtc> rdf:type owl:NamedIndividual ,
                                                                                                                                                                                                  <http://lpis.ec.europa.eu/registry/applicationschema/cap-iacs-base#FarmStructureSurveyNumberValue> ;
                                                                                                                                                                                         rdfs:label "Other land (land occupied by buildings, farmyards, tracks, ponds, quarries, infertile land, rock, etc.)"@en ;
                                                                                                                                                                                         <http://www.w3.org/2004/02/skos/core#definition> """-- Definition --
Other land (land occupied by buildings, farmyards, tracks, ponds, quarries, infertile land, rock, etc.)
-- Description --
All those parts of the total area belonging to the agricultural holding which constitute neither utilised agricultural area, unutilised agricultural area nor wooded area.
NOTE. Initial value:2.05.03"""@en ;
                                                                                                                                                                                         <http://www.w3.org/2004/02/skos/core#inScheme> :FarmStructureSurveyNumberValue .


###  http://lpis.ec.europa.eu/registry/applicationschema/cap-iacs-base/code#FarmStructureSurveyNumberValue/otherOilSeedCrops
<http://lpis.ec.europa.eu/registry/applicationschema/cap-iacs-base/code#FarmStructureSurveyNumberValue/otherOilSeedCrops> rdf:type owl:NamedIndividual ,
                                                                                                                                   <http://lpis.ec.europa.eu/registry/applicationschema/cap-iacs-base#FarmStructureSurveyNumberValue> ;
                                                                                                                          rdfs:label "Other oil seed crops"@en ;
                                                                                                                          <http://www.w3.org/2004/02/skos/core#definition> """-- Definition --
Other oil seed crops.
-- Description --
Other crops grown mainly for their oil content, harvested as dry grains, which are not mentioned elsewhere.
NOTE. Initial value:2.01.06.08"""@en ;
                                                                                                                          <http://www.w3.org/2004/02/skos/core#inScheme> :FarmStructureSurveyNumberValue .


###  http://lpis.ec.europa.eu/registry/applicationschema/cap-iacs-base/code#FarmStructureSurveyNumberValue/otherPermanentCrops
<http://lpis.ec.europa.eu/registry/applicationschema/cap-iacs-base/code#FarmStructureSurveyNumberValue/otherPermanentCrops> rdf:type owl:NamedIndividual ,
                                                                                                                                     <http://lpis.ec.europa.eu/registry/applicationschema/cap-iacs-base#FarmStructureSurveyNumberValue> ;
                                                                                                                            rdfs:label "Other permanent crops"@en ;
                                                                                                                            <http://www.w3.org/2004/02/skos/core#definition> """-- Definition --
Other permanent crops.
-- Description --
Open-air permanent crops other than those under the previous heading and in particular those used for plaiting or weaving, harvested generally every year.
NOTE. Initial value:2.04.06"""@en ;
                                                                                                                            <http://www.w3.org/2004/02/skos/core#inScheme> :FarmStructureSurveyNumberValue .


###  http://lpis.ec.europa.eu/registry/applicationschema/cap-iacs-base/code#FarmStructureSurveyNumberValue/otherPlantsHarvestedGreen
<http://lpis.ec.europa.eu/registry/applicationschema/cap-iacs-base/code#FarmStructureSurveyNumberValue/otherPlantsHarvestedGreen> rdf:type owl:NamedIndividual ,
                                                                                                                                           <http://lpis.ec.europa.eu/registry/applicationschema/cap-iacs-base#FarmStructureSurveyNumberValue> ;
                                                                                                                                  rdfs:label "Other plants harvested green"@en ;
                                                                                                                                  <http://www.w3.org/2004/02/skos/core#definition> """-- Definition --
Other plants harvested green.
-- Description --
Other annual or multiannual (less than five years) fodder crops.
NOTE. Initial value:2.01.09.02"""@en ;
                                                                                                                                  <http://www.w3.org/2004/02/skos/core#inScheme> :FarmStructureSurveyNumberValue .


###  http://lpis.ec.europa.eu/registry/applicationschema/cap-iacs-base/code#FarmStructureSurveyNumberValue/otherPlantsHarvestedGreenNotMentionedElsewhere
<http://lpis.ec.europa.eu/registry/applicationschema/cap-iacs-base/code#FarmStructureSurveyNumberValue/otherPlantsHarvestedGreenNotMentionedElsewhere> rdf:type owl:NamedIndividual ,
                                                                                                                                                                <http://lpis.ec.europa.eu/registry/applicationschema/cap-iacs-base#FarmStructureSurveyNumberValue> ;
                                                                                                                                                       rdfs:label "Other plants harvested green not mentioned elsewhere"@en ;
                                                                                                                                                       <http://www.w3.org/2004/02/skos/core#definition> """-- Definition --
Other plants harvested green not mentioned elsewhere.
-- Description --
Other arable crops intended mainly for animal fodder, harvested green, not mentioned elsewhere.
NOTE. Initial value:2.01.09.02.99"""@en ;
                                                                                                                                                       <http://www.w3.org/2004/02/skos/core#inScheme> :FarmStructureSurveyNumberValue .


###  http://lpis.ec.europa.eu/registry/applicationschema/cap-iacs-base/code#FarmStructureSurveyNumberValue/otherWines
<http://lpis.ec.europa.eu/registry/applicationschema/cap-iacs-base/code#FarmStructureSurveyNumberValue/otherWines> rdf:type owl:NamedIndividual ,
                                                                                                                            <http://lpis.ec.europa.eu/registry/applicationschema/cap-iacs-base#FarmStructureSurveyNumberValue> ;
                                                                                                                   rdfs:label "Other wines"@en ;
                                                                                                                   <http://www.w3.org/2004/02/skos/core#definition> """-- Definition --
Other wines.
-- Description --
Grape varieties normally grown for the production of wines other than PDO and PGI wines.
NOTE. Initial value:2.04.04.02"""@en ;
                                                                                                                   <http://www.w3.org/2004/02/skos/core#inScheme> :FarmStructureSurveyNumberValue .


###  http://lpis.ec.europa.eu/registry/applicationschema/cap-iacs-base/code#FarmStructureSurveyNumberValue/outdoorOrUnderLowNotAccessibleProtectiveCover
<http://lpis.ec.europa.eu/registry/applicationschema/cap-iacs-base/code#FarmStructureSurveyNumberValue/outdoorOrUnderLowNotAccessibleProtectiveCover> rdf:type owl:NamedIndividual ,
                                                                                                                                                               <http://lpis.ec.europa.eu/registry/applicationschema/cap-iacs-base#FarmStructureSurveyNumberValue> ;
                                                                                                                                                      rdfs:label "Outdoor or under low (not accessible) protective cover"@en ;
                                                                                                                                                      <http://www.w3.org/2004/02/skos/core#definition> """-- Definition --
Outdoor or under low (not accessible) protective cover.
-- Description --
Fresh vegetables, melons and strawberries, outdoor or under low (non-accessible) cover.
NOTE. Initial value:2.01.07.01"""@en ;
                                                                                                                                                      <http://www.w3.org/2004/02/skos/core#inScheme> :FarmStructureSurveyNumberValue .


###  http://lpis.ec.europa.eu/registry/applicationschema/cap-iacs-base/code#FarmStructureSurveyNumberValue/pastureAndMeadowExcludingRoughGrazings
<http://lpis.ec.europa.eu/registry/applicationschema/cap-iacs-base/code#FarmStructureSurveyNumberValue/pastureAndMeadowExcludingRoughGrazings> rdf:type owl:NamedIndividual ,
                                                                                                                                                        <http://lpis.ec.europa.eu/registry/applicationschema/cap-iacs-base#FarmStructureSurveyNumberValue> ;
                                                                                                                                               rdfs:label "Pasture and meadow, excluding rough grazings"@en ;
                                                                                                                                               <http://www.w3.org/2004/02/skos/core#definition> """-- Definition --
Pasture and meadow, excluding rough grazings.
-- Description --
Permanent pasture on good or medium quality soils. These areas can normally be used for intensive grazing.
NOTE. Initial value:2.03.01"""@en ;
                                                                                                                                               <http://www.w3.org/2004/02/skos/core#inScheme> :FarmStructureSurveyNumberValue .


###  http://lpis.ec.europa.eu/registry/applicationschema/cap-iacs-base/code#FarmStructureSurveyNumberValue/permanentCrops
<http://lpis.ec.europa.eu/registry/applicationschema/cap-iacs-base/code#FarmStructureSurveyNumberValue/permanentCrops> rdf:type owl:NamedIndividual ,
                                                                                                                                <http://lpis.ec.europa.eu/registry/applicationschema/cap-iacs-base#FarmStructureSurveyNumberValue> ;
                                                                                                                       rdfs:label "Permanent crops"@en ;
                                                                                                                       <http://www.w3.org/2004/02/skos/core#definition> """-- Definition --
Permanent crops.
-- Description --
Crops not grown in rotation, other than permanent grassland, which occupy the soil for a long period and yield crops over several years.
NOTE. Initial value:2.04"""@en ;
                                                                                                                       <http://www.w3.org/2004/02/skos/core#inScheme> :FarmStructureSurveyNumberValue .


###  http://lpis.ec.europa.eu/registry/applicationschema/cap-iacs-base/code#FarmStructureSurveyNumberValue/permanentCropsUnderGlass
<http://lpis.ec.europa.eu/registry/applicationschema/cap-iacs-base/code#FarmStructureSurveyNumberValue/permanentCropsUnderGlass> rdf:type owl:NamedIndividual ,
                                                                                                                                          <http://lpis.ec.europa.eu/registry/applicationschema/cap-iacs-base#FarmStructureSurveyNumberValue> ;
                                                                                                                                 rdfs:label "Permanent crops under glass"@en ;
                                                                                                                                 <http://www.w3.org/2004/02/skos/core#definition> """-- Definition --
Permanent crops under glass.
-- Description --
Permanent crops under glass.
NOTE. Initial value:2.04.07"""@en ;
                                                                                                                                 <http://www.w3.org/2004/02/skos/core#inScheme> :FarmStructureSurveyNumberValue .


###  http://lpis.ec.europa.eu/registry/applicationschema/cap-iacs-base/code#FarmStructureSurveyNumberValue/permanentGrassland
<http://lpis.ec.europa.eu/registry/applicationschema/cap-iacs-base/code#FarmStructureSurveyNumberValue/permanentGrassland> rdf:type owl:NamedIndividual ,
                                                                                                                                    <http://lpis.ec.europa.eu/registry/applicationschema/cap-iacs-base#FarmStructureSurveyNumberValue> ;
                                                                                                                           rdfs:label "Permanent grassland"@en ;
                                                                                                                           <http://www.w3.org/2004/02/skos/core#definition> """-- Definition --
Permanent grassland.
-- Description --
Land used permanently (for five years or more) to grow herbaceous forage crops, through cultivation (sown) or naturally (self-seeded), and that is not included in the crop rotation on the holding.
The land can be used for grazing or mown for silage, hay or used for renewable energy production.
NOTE. Initial value:2.03"""@en ;
                                                                                                                           <http://www.w3.org/2004/02/skos/core#inScheme> :FarmStructureSurveyNumberValue .


###  http://lpis.ec.europa.eu/registry/applicationschema/cap-iacs-base/code#FarmStructureSurveyNumberValue/permanentGrasslandNoLongerUsedForProductionPurposesAndEligibleForThePaymentOfSubsidies
<http://lpis.ec.europa.eu/registry/applicationschema/cap-iacs-base/code#FarmStructureSurveyNumberValue/permanentGrasslandNoLongerUsedForProductionPurposesAndEligibleForThePaymentOfSubsidies> rdf:type owl:NamedIndividual ,
                                                                                                                                                                                                        <http://lpis.ec.europa.eu/registry/applicationschema/cap-iacs-base#FarmStructureSurveyNumberValue> ;
                                                                                                                                                                                               rdfs:label "Permanent grassland no longer used for production purposes and eligible for the payment of subsidies"@en ;
                                                                                                                                                                                               <http://www.w3.org/2004/02/skos/core#definition> """-- Definition --
Permanent grassland no longer used for production purposes and eligible for the payment of subsidies.
-- Description --
Areas of permanent grassland and meadows no longer used for production purposes which, in line with Regulation (EC) No 1782/2003 or, where applicable, the most recent legislation, are maintained in good agricultural and environmental condition and are eligible for financial support.
NOTE. Initial value:2.03.03"""@en ;
                                                                                                                                                                                               <http://www.w3.org/2004/02/skos/core#inScheme> :FarmStructureSurveyNumberValue .


###  http://lpis.ec.europa.eu/registry/applicationschema/cap-iacs-base/code#FarmStructureSurveyNumberValue/plantsHarvestedGreen
<http://lpis.ec.europa.eu/registry/applicationschema/cap-iacs-base/code#FarmStructureSurveyNumberValue/plantsHarvestedGreen> rdf:type owl:NamedIndividual ,
                                                                                                                                      <http://lpis.ec.europa.eu/registry/applicationschema/cap-iacs-base#FarmStructureSurveyNumberValue> ;
                                                                                                                             rdfs:label "Plants harvested green"@en ;
                                                                                                                             <http://www.w3.org/2004/02/skos/core#definition> """-- Definition --
Plants harvested green.
-- Description --
All ‘green’ arable crops intended mainly for animal feed, grown in rotation with other crops and occupying the same parcel for less than five years (annual or multiannual fodder crops).
Green crops used for renewable energy production are included.
Crops not used on the holding but sold, either for direct use on other agricultural holdings or to industry, are included.
NOTE. Initial value:2.01.09"""@en ;
                                                                                                                             <http://www.w3.org/2004/02/skos/core#inScheme> :FarmStructureSurveyNumberValue .


###  http://lpis.ec.europa.eu/registry/applicationschema/cap-iacs-base/code#FarmStructureSurveyNumberValue/potatoesIncludingEarlyPotatoesAndSeedPotatoes
<http://lpis.ec.europa.eu/registry/applicationschema/cap-iacs-base/code#FarmStructureSurveyNumberValue/potatoesIncludingEarlyPotatoesAndSeedPotatoes> rdf:type owl:NamedIndividual ,
                                                                                                                                                               <http://lpis.ec.europa.eu/registry/applicationschema/cap-iacs-base#FarmStructureSurveyNumberValue> ;
                                                                                                                                                      rdfs:label "Potatoes (including early potatoes and seed potatoes)"@en ;
                                                                                                                                                      <http://www.w3.org/2004/02/skos/core#definition> """-- Definition --
Potatoes (including early potatoes and seed potatoes).
-- Description --
Solanum tuberosum L.
NOTE. Initial value:2.01.03"""@en ;
                                                                                                                                                      <http://www.w3.org/2004/02/skos/core#inScheme> :FarmStructureSurveyNumberValue .


###  http://lpis.ec.europa.eu/registry/applicationschema/cap-iacs-base/code#FarmStructureSurveyNumberValue/qualityWine
<http://lpis.ec.europa.eu/registry/applicationschema/cap-iacs-base/code#FarmStructureSurveyNumberValue/qualityWine> rdf:type owl:NamedIndividual ,
                                                                                                                             <http://lpis.ec.europa.eu/registry/applicationschema/cap-iacs-base#FarmStructureSurveyNumberValue> ;
                                                                                                                    rdfs:label "Quality wine"@en ;
                                                                                                                    <http://www.w3.org/2004/02/skos/core#definition> """-- Definition --
Quality wine.
-- Description --
Grape varieties normally grown for the production of wines with a protected designation of origin (PDO) which comply with the requirements (i) of Council Regulation (EC) No 479/2008(1)
OJ L 148, 6.6.2008, p. 1. (1) or, where applicable, the most recent legislation; and (ii) the corresponding national rules.
Grape varieties normally grown for the production of wines with a protected geographical indication (PGI) which comply with the requirements (i) of Regulation (EC) No 479/2008 or, where applicable, the most recent legislation; and (ii) the corresponding national rules.
NOTE. Initial value:2.04.04.01"""@en ;
                                                                                                                    <http://www.w3.org/2004/02/skos/core#inScheme> :FarmStructureSurveyNumberValue .


###  http://lpis.ec.europa.eu/registry/applicationschema/cap-iacs-base/code#FarmStructureSurveyNumberValue/raisins
<http://lpis.ec.europa.eu/registry/applicationschema/cap-iacs-base/code#FarmStructureSurveyNumberValue/raisins> rdf:type owl:NamedIndividual ,
                                                                                                                         <http://lpis.ec.europa.eu/registry/applicationschema/cap-iacs-base#FarmStructureSurveyNumberValue> ;
                                                                                                                rdfs:label "Raisins"@en ;
                                                                                                                <http://www.w3.org/2004/02/skos/core#definition> """-- Definition --
Raisins.
-- Description --
Grape varieties normally grown for the production of raisins.
NOTE. Initial value:2.04.04.04"""@en ;
                                                                                                                <http://www.w3.org/2004/02/skos/core#inScheme> :FarmStructureSurveyNumberValue .


###  http://lpis.ec.europa.eu/registry/applicationschema/cap-iacs-base/code#FarmStructureSurveyNumberValue/rapeAndTurnipRape
<http://lpis.ec.europa.eu/registry/applicationschema/cap-iacs-base/code#FarmStructureSurveyNumberValue/rapeAndTurnipRape> rdf:type owl:NamedIndividual ,
                                                                                                                                   <http://lpis.ec.europa.eu/registry/applicationschema/cap-iacs-base#FarmStructureSurveyNumberValue> ;
                                                                                                                          rdfs:label "Rape and turnip rape"@en ;
                                                                                                                          <http://www.w3.org/2004/02/skos/core#definition> """-- Definition --
Rape and turnip rape.
-- Description --
Brassica napus L. (partim) and Brassica rapa L. var. sylvestris (Lam.) Briggs, grown for the production of oil, harvested as dry grains.
NOTE. Initial value:2.01.06.04"""@en ;
                                                                                                                          <http://www.w3.org/2004/02/skos/core#inScheme> :FarmStructureSurveyNumberValue .


###  http://lpis.ec.europa.eu/registry/applicationschema/cap-iacs-base/code#FarmStructureSurveyNumberValue/rice
<http://lpis.ec.europa.eu/registry/applicationschema/cap-iacs-base/code#FarmStructureSurveyNumberValue/rice> rdf:type owl:NamedIndividual ,
                                                                                                                      <http://lpis.ec.europa.eu/registry/applicationschema/cap-iacs-base#FarmStructureSurveyNumberValue> ;
                                                                                                             rdfs:label "Rice"@en ;
                                                                                                             <http://www.w3.org/2004/02/skos/core#definition> """-- Definition --
Rice.
-- Description --
Oryza sativa L.
NOTE. Initial value:2.01.01.07"""@en ;
                                                                                                             <http://www.w3.org/2004/02/skos/core#inScheme> :FarmStructureSurveyNumberValue .


###  http://lpis.ec.europa.eu/registry/applicationschema/cap-iacs-base/code#FarmStructureSurveyNumberValue/roughGrazings
<http://lpis.ec.europa.eu/registry/applicationschema/cap-iacs-base/code#FarmStructureSurveyNumberValue/roughGrazings> rdf:type owl:NamedIndividual ,
                                                                                                                               <http://lpis.ec.europa.eu/registry/applicationschema/cap-iacs-base#FarmStructureSurveyNumberValue> ;
                                                                                                                      rdfs:label "Rough grazings"@en ;
                                                                                                                      <http://www.w3.org/2004/02/skos/core#definition> """-- Definition --
Rough grazings.
-- Description --
Low yielding permanent grassland, usually on low quality soil, for example on hilly land and at high altitudes, usually unimproved by fertiliser, cultivation, reseeding or drainage.
These areas can normally be used only for extensive grazing and are not normally mown or are mown in an extensive manner; they cannot support a large density of animals.
NOTE. Initial value:2.03.02"""@en ;
                                                                                                                      <http://www.w3.org/2004/02/skos/core#inScheme> :FarmStructureSurveyNumberValue .


###  http://lpis.ec.europa.eu/registry/applicationschema/cap-iacs-base/code#FarmStructureSurveyNumberValue/rye
<http://lpis.ec.europa.eu/registry/applicationschema/cap-iacs-base/code#FarmStructureSurveyNumberValue/rye> rdf:type owl:NamedIndividual ,
                                                                                                                     <http://lpis.ec.europa.eu/registry/applicationschema/cap-iacs-base#FarmStructureSurveyNumberValue> ;
                                                                                                            rdfs:label "Rye"@en ;
                                                                                                            <http://www.w3.org/2004/02/skos/core#definition> """-- Definition --
Rye.
-- Description --
Secale cereale L., including mixtures of rye and other cereals sown in the autumn (maslin).
NOTE. Initial value:2.01.01.03"""@en ;
                                                                                                            <http://www.w3.org/2004/02/skos/core#inScheme> :FarmStructureSurveyNumberValue .


###  http://lpis.ec.europa.eu/registry/applicationschema/cap-iacs-base/code#FarmStructureSurveyNumberValue/soya
<http://lpis.ec.europa.eu/registry/applicationschema/cap-iacs-base/code#FarmStructureSurveyNumberValue/soya> rdf:type owl:NamedIndividual ,
                                                                                                                      <http://lpis.ec.europa.eu/registry/applicationschema/cap-iacs-base#FarmStructureSurveyNumberValue> ;
                                                                                                             rdfs:label "Soya"@en ;
                                                                                                             <http://www.w3.org/2004/02/skos/core#definition> """-- Definition --
Soya.
-- Description --
Glycine max L. Merril, harvested as dry grains.
NOTE. Initial value:2.01.06.06"""@en ;
                                                                                                             <http://www.w3.org/2004/02/skos/core#inScheme> :FarmStructureSurveyNumberValue .


###  http://lpis.ec.europa.eu/registry/applicationschema/cap-iacs-base/code#FarmStructureSurveyNumberValue/sugarBeetExcludingSeed
<http://lpis.ec.europa.eu/registry/applicationschema/cap-iacs-base/code#FarmStructureSurveyNumberValue/sugarBeetExcludingSeed> rdf:type owl:NamedIndividual ,
                                                                                                                                        <http://lpis.ec.europa.eu/registry/applicationschema/cap-iacs-base#FarmStructureSurveyNumberValue> ;
                                                                                                                               rdfs:label "Sugar beet (excluding seed)"@en ;
                                                                                                                               <http://www.w3.org/2004/02/skos/core#definition> """-- Definition --
Sugar beet (excluding seed).
-- Description --
Beta vulgaris L. intended for the sugar industry and alcohol production (including energy production).
NOTE. Initial value:2.01.04"""@en ;
                                                                                                                               <http://www.w3.org/2004/02/skos/core#inScheme> :FarmStructureSurveyNumberValue .


###  http://lpis.ec.europa.eu/registry/applicationschema/cap-iacs-base/code#FarmStructureSurveyNumberValue/sunflower
<http://lpis.ec.europa.eu/registry/applicationschema/cap-iacs-base/code#FarmStructureSurveyNumberValue/sunflower> rdf:type owl:NamedIndividual ,
                                                                                                                           <http://lpis.ec.europa.eu/registry/applicationschema/cap-iacs-base#FarmStructureSurveyNumberValue> ;
                                                                                                                  rdfs:label "Sunflower"@en ;
                                                                                                                  <http://www.w3.org/2004/02/skos/core#definition> """-- Definition --
Sunflower.
-- Description --
Helianthus annuus L., harvested as dry grains.
NOTE. Initial value:2.01.06.05"""@en ;
                                                                                                                  <http://www.w3.org/2004/02/skos/core#inScheme> :FarmStructureSurveyNumberValue .


###  http://lpis.ec.europa.eu/registry/applicationschema/cap-iacs-base/code#FarmStructureSurveyNumberValue/tableGrapes
<http://lpis.ec.europa.eu/registry/applicationschema/cap-iacs-base/code#FarmStructureSurveyNumberValue/tableGrapes> rdf:type owl:NamedIndividual ,
                                                                                                                             <http://lpis.ec.europa.eu/registry/applicationschema/cap-iacs-base#FarmStructureSurveyNumberValue> ;
                                                                                                                    rdfs:label "Table grapes"@en ;
                                                                                                                    <http://www.w3.org/2004/02/skos/core#definition> """-- Definition --
Table grapes.
-- Description --
Grape varieties normally grown for the production of fresh grapes.
NOTE. Initial value:2.04.04.03"""@en ;
                                                                                                                    <http://www.w3.org/2004/02/skos/core#inScheme> :FarmStructureSurveyNumberValue .


###  http://lpis.ec.europa.eu/registry/applicationschema/cap-iacs-base/code#FarmStructureSurveyNumberValue/temporaryGrass
<http://lpis.ec.europa.eu/registry/applicationschema/cap-iacs-base/code#FarmStructureSurveyNumberValue/temporaryGrass> rdf:type owl:NamedIndividual ,
                                                                                                                                <http://lpis.ec.europa.eu/registry/applicationschema/cap-iacs-base#FarmStructureSurveyNumberValue> ;
                                                                                                                       rdfs:label "Temporary grass"@en ;
                                                                                                                       <http://www.w3.org/2004/02/skos/core#definition> """-- Definition --
Temporary grass.
-- Description --
Grass plants for grazing, hay or silage included as a part of a normal crop rotation, lasting at least one crop year and less than five years, sown with grass or grass mixtures. The areas are broken up by ploughing or other tilling or the plants are destroyed by other means such as by herbicides before they are sown again.
Mixtures of predominantly grass plants and other forage crops (usually leguminous), grazed, harvested green or as dried hay are included here.
NOTE. Initial value:2.01.09.01"""@en ;
                                                                                                                       <http://www.w3.org/2004/02/skos/core#inScheme> :FarmStructureSurveyNumberValue .


###  http://lpis.ec.europa.eu/registry/applicationschema/cap-iacs-base/code#FarmStructureSurveyNumberValue/tobacco
<http://lpis.ec.europa.eu/registry/applicationschema/cap-iacs-base/code#FarmStructureSurveyNumberValue/tobacco> rdf:type owl:NamedIndividual ,
                                                                                                                         <http://lpis.ec.europa.eu/registry/applicationschema/cap-iacs-base#FarmStructureSurveyNumberValue> ;
                                                                                                                rdfs:label "Tobacco"@en ;
                                                                                                                <http://www.w3.org/2004/02/skos/core#definition> """-- Definition --
Tobacco
-- Description --
Nicotiana tabacum L.
NOTE. Initial value:2.01.06.01"""@en ;
                                                                                                                <http://www.w3.org/2004/02/skos/core#inScheme> :FarmStructureSurveyNumberValue .


###  http://lpis.ec.europa.eu/registry/applicationschema/cap-iacs-base/code#FarmStructureSurveyNumberValue/totalCultivatedAreaIrrigatedAtLeastOnceDuringThePrevious12Months
<http://lpis.ec.europa.eu/registry/applicationschema/cap-iacs-base/code#FarmStructureSurveyNumberValue/totalCultivatedAreaIrrigatedAtLeastOnceDuringThePrevious12Months> rdf:type owl:NamedIndividual ,
                                                                                                                                                                                  <http://lpis.ec.europa.eu/registry/applicationschema/cap-iacs-base#FarmStructureSurveyNumberValue> ;
                                                                                                                                                                         rdfs:label "Total cultivated area irrigated at least once during the previous 12 months"@en ;
                                                                                                                                                                         <http://www.w3.org/2004/02/skos/core#definition> """-- Definition --
Total cultivated area irrigated at least once during the previous 12 months.
-- Description --
Area of crops which have actually been irrigated at least once during the 12 months prior to the reference day of the survey.
NOTE. Initial value:2.06.02.02"""@en ;
                                                                                                                                                                         <http://www.w3.org/2004/02/skos/core#inScheme> :FarmStructureSurveyNumberValue .


###  http://lpis.ec.europa.eu/registry/applicationschema/cap-iacs-base/code#FarmStructureSurveyNumberValue/totalIrrigableArea
<http://lpis.ec.europa.eu/registry/applicationschema/cap-iacs-base/code#FarmStructureSurveyNumberValue/totalIrrigableArea> rdf:type owl:NamedIndividual ,
                                                                                                                                    <http://lpis.ec.europa.eu/registry/applicationschema/cap-iacs-base#FarmStructureSurveyNumberValue> ;
                                                                                                                           rdfs:label "Total irrigable area"@en ;
                                                                                                                           <http://www.w3.org/2004/02/skos/core#definition> """-- Definition --
Total irrigable area.
-- Description --
Total maximum utilised agricultural area which could be irrigated in the reference year using the equipment and the quantity of water normally available on the holding.
NOTE. Initial value:2.06.02.01"""@en ;
                                                                                                                           <http://www.w3.org/2004/02/skos/core#inScheme> :FarmStructureSurveyNumberValue .


###  http://lpis.ec.europa.eu/registry/applicationschema/cap-iacs-base/code#FarmStructureSurveyNumberValue/underGlassOrOtherAccessibleProtectiveCover
<http://lpis.ec.europa.eu/registry/applicationschema/cap-iacs-base/code#FarmStructureSurveyNumberValue/underGlassOrOtherAccessibleProtectiveCover> rdf:type owl:NamedIndividual ,
                                                                                                                                                            <http://lpis.ec.europa.eu/registry/applicationschema/cap-iacs-base#FarmStructureSurveyNumberValue> ;
                                                                                                                                                   rdfs:label "Under glass or other (accessible) protective cover"@en ;
                                                                                                                                                   <http://www.w3.org/2004/02/skos/core#definition> """-- Definition --
Under glass or other (accessible) protective cover.
-- Description --
Crops, which for the whole of their period of growth or for the predominant part of it are covered by greenhouses or fixed or mobile high cover (glass or rigid or flexible plastic).
NOTE. Initial value:2.01.07.02"""@en ;
                                                                                                                                                   <http://www.w3.org/2004/02/skos/core#inScheme> :FarmStructureSurveyNumberValue .


###  http://lpis.ec.europa.eu/registry/applicationschema/cap-iacs-base/code#FarmStructureSurveyNumberValue/underGlassOrOtherAccessibleProtectiveCoverFlowers
<http://lpis.ec.europa.eu/registry/applicationschema/cap-iacs-base/code#FarmStructureSurveyNumberValue/underGlassOrOtherAccessibleProtectiveCoverFlowers> rdf:type owl:NamedIndividual ,
                                                                                                                                                                   <http://lpis.ec.europa.eu/registry/applicationschema/cap-iacs-base#FarmStructureSurveyNumberValue> ;
                                                                                                                                                          rdfs:label "Under glass or other (accessible)  protective cover"@en ;
                                                                                                                                                          <http://www.w3.org/2004/02/skos/core#definition> """-- Definition --
Under glass or other (accessible)  protective cover.
-- Description --
Flowers and ornamental plants (excluding nurseries), which for the whole of their period of growth or for the predominant part of it are covered by greenhouses or fixed or mobile high cover (glass or rigid or flexible plastic).
NOTE. Initial value:2.01.08.02"""@en ;
                                                                                                                                                          <http://www.w3.org/2004/02/skos/core#inScheme> :FarmStructureSurveyNumberValue .


###  http://lpis.ec.europa.eu/registry/applicationschema/cap-iacs-base/code#FarmStructureSurveyNumberValue/unutilisedAgriculturalLand
<http://lpis.ec.europa.eu/registry/applicationschema/cap-iacs-base/code#FarmStructureSurveyNumberValue/unutilisedAgriculturalLand> rdf:type owl:NamedIndividual ,
                                                                                                                                            <http://lpis.ec.europa.eu/registry/applicationschema/cap-iacs-base#FarmStructureSurveyNumberValue> ;
                                                                                                                                   rdfs:label "Unutilised agricultural land"@en ;
                                                                                                                                   <http://www.w3.org/2004/02/skos/core#definition> """-- Definition --
Unutilised agricultural land.
-- Description --
Area previously used as an agricultural area and, during the reference year of the survey, no longer worked for economic, social or other reasons and which is not used in the crop rotation system, i.e. land where no agricultural use is intended.
This land could be brought back into cultivation using the resources normally available on an agricultural holding.
NOTE. Initial value:2.05.01"""@en ;
                                                                                                                                   <http://www.w3.org/2004/02/skos/core#inScheme> :FarmStructureSurveyNumberValue .


###  http://lpis.ec.europa.eu/registry/applicationschema/cap-iacs-base/code#FarmStructureSurveyNumberValue/vineyardsOfWhichNormallyProducing
<http://lpis.ec.europa.eu/registry/applicationschema/cap-iacs-base/code#FarmStructureSurveyNumberValue/vineyardsOfWhichNormallyProducing> rdf:type owl:NamedIndividual ,
                                                                                                                                                   <http://lpis.ec.europa.eu/registry/applicationschema/cap-iacs-base#FarmStructureSurveyNumberValue> ;
                                                                                                                                          rdfs:label "Vineyards, of which normally producing:"@en ;
                                                                                                                                          <http://www.w3.org/2004/02/skos/core#definition> """-- Definition --
Vineyards, of which normally producing:
-- Description --
Plantations of Vitis vinifera L.
NOTE. Initial value:2.04.04"""@en ;
                                                                                                                                          <http://www.w3.org/2004/02/skos/core#inScheme> :FarmStructureSurveyNumberValue .


###  http://lpis.ec.europa.eu/registry/applicationschema/cap-iacs-base/code#FarmStructureSurveyNumberValue/woodedArea
<http://lpis.ec.europa.eu/registry/applicationschema/cap-iacs-base/code#FarmStructureSurveyNumberValue/woodedArea> rdf:type owl:NamedIndividual ,
                                                                                                                            <http://lpis.ec.europa.eu/registry/applicationschema/cap-iacs-base#FarmStructureSurveyNumberValue> ;
                                                                                                                   rdfs:label "Wooded area"@en ;
                                                                                                                   <http://www.w3.org/2004/02/skos/core#definition> """-- Definition --
Wooded area.
-- Description --
Areas covered with trees or forest shrubs, including poplar plantations inside or outside woods and forest-tree nurseries grown in woodland for the holding’s own requirements, as well as forest facilities (forest roads, storage depots for timber, etc.).
NOTE. Initial value:2.05.02"""@en ;
                                                                                                                   <http://www.w3.org/2004/02/skos/core#inScheme> :FarmStructureSurveyNumberValue .


###  http://lpis.ec.europa.eu/registry/applicationschema/cap-iacs-base/code#MonthValue/april
<http://lpis.ec.europa.eu/registry/applicationschema/cap-iacs-base/code#MonthValue/april> rdf:type owl:NamedIndividual ,
                                                                                                   <http://lpis.ec.europa.eu/registry/applicationschema/cap-iacs-base#MonthValue> ;
                                                                                          rdfs:label "April"@en ;
                                                                                          <http://www.w3.org/2004/02/skos/core#definition> """-- Definition --
April.
-- Description --
Item description."""@en ;
                                                                                          <http://www.w3.org/2004/02/skos/core#inScheme> :MonthValue .


###  http://lpis.ec.europa.eu/registry/applicationschema/cap-iacs-base/code#MonthValue/august
<http://lpis.ec.europa.eu/registry/applicationschema/cap-iacs-base/code#MonthValue/august> rdf:type owl:NamedIndividual ,
                                                                                                    <http://lpis.ec.europa.eu/registry/applicationschema/cap-iacs-base#MonthValue> ;
                                                                                           rdfs:label "August"@en ;
                                                                                           <http://www.w3.org/2004/02/skos/core#definition> """-- Definition --
August.
-- Description --
Item description."""@en ;
                                                                                           <http://www.w3.org/2004/02/skos/core#inScheme> :MonthValue .


###  http://lpis.ec.europa.eu/registry/applicationschema/cap-iacs-base/code#MonthValue/december
<http://lpis.ec.europa.eu/registry/applicationschema/cap-iacs-base/code#MonthValue/december> rdf:type owl:NamedIndividual ,
                                                                                                      <http://lpis.ec.europa.eu/registry/applicationschema/cap-iacs-base#MonthValue> ;
                                                                                             rdfs:label "December"@en ;
                                                                                             <http://www.w3.org/2004/02/skos/core#definition> """-- Definition --
December.
-- Description --
Item description."""@en ;
                                                                                             <http://www.w3.org/2004/02/skos/core#inScheme> :MonthValue .


###  http://lpis.ec.europa.eu/registry/applicationschema/cap-iacs-base/code#MonthValue/february
<http://lpis.ec.europa.eu/registry/applicationschema/cap-iacs-base/code#MonthValue/february> rdf:type owl:NamedIndividual ,
                                                                                                      <http://lpis.ec.europa.eu/registry/applicationschema/cap-iacs-base#MonthValue> ;
                                                                                             rdfs:label "February"@en ;
                                                                                             <http://www.w3.org/2004/02/skos/core#definition> """-- Definition --
February.
-- Description --
Item description."""@en ;
                                                                                             <http://www.w3.org/2004/02/skos/core#inScheme> :MonthValue .


###  http://lpis.ec.europa.eu/registry/applicationschema/cap-iacs-base/code#MonthValue/january
<http://lpis.ec.europa.eu/registry/applicationschema/cap-iacs-base/code#MonthValue/january> rdf:type owl:NamedIndividual ,
                                                                                                     <http://lpis.ec.europa.eu/registry/applicationschema/cap-iacs-base#MonthValue> ;
                                                                                            rdfs:label "January"@en ;
                                                                                            <http://www.w3.org/2004/02/skos/core#definition> """-- Definition --
January.
-- Description --
Item description."""@en ;
                                                                                            <http://www.w3.org/2004/02/skos/core#inScheme> :MonthValue .


###  http://lpis.ec.europa.eu/registry/applicationschema/cap-iacs-base/code#MonthValue/july
<http://lpis.ec.europa.eu/registry/applicationschema/cap-iacs-base/code#MonthValue/july> rdf:type owl:NamedIndividual ,
                                                                                                  <http://lpis.ec.europa.eu/registry/applicationschema/cap-iacs-base#MonthValue> ;
                                                                                         rdfs:label "July"@en ;
                                                                                         <http://www.w3.org/2004/02/skos/core#definition> """-- Definition --
July.
-- Description --
Item description."""@en ;
                                                                                         <http://www.w3.org/2004/02/skos/core#inScheme> :MonthValue .


###  http://lpis.ec.europa.eu/registry/applicationschema/cap-iacs-base/code#MonthValue/june
<http://lpis.ec.europa.eu/registry/applicationschema/cap-iacs-base/code#MonthValue/june> rdf:type owl:NamedIndividual ,
                                                                                                  <http://lpis.ec.europa.eu/registry/applicationschema/cap-iacs-base#MonthValue> ;
                                                                                         rdfs:label "June"@en ;
                                                                                         <http://www.w3.org/2004/02/skos/core#definition> """-- Definition --
June.
-- Description --
Item description."""@en ;
                                                                                         <http://www.w3.org/2004/02/skos/core#inScheme> :MonthValue .


###  http://lpis.ec.europa.eu/registry/applicationschema/cap-iacs-base/code#MonthValue/march
<http://lpis.ec.europa.eu/registry/applicationschema/cap-iacs-base/code#MonthValue/march> rdf:type owl:NamedIndividual ,
                                                                                                   <http://lpis.ec.europa.eu/registry/applicationschema/cap-iacs-base#MonthValue> ;
                                                                                          rdfs:label "March"@en ;
                                                                                          <http://www.w3.org/2004/02/skos/core#definition> """-- Definition --
March.
-- Description --
Item description."""@en ;
                                                                                          <http://www.w3.org/2004/02/skos/core#inScheme> :MonthValue .


###  http://lpis.ec.europa.eu/registry/applicationschema/cap-iacs-base/code#MonthValue/may
<http://lpis.ec.europa.eu/registry/applicationschema/cap-iacs-base/code#MonthValue/may> rdf:type owl:NamedIndividual ,
                                                                                                 <http://lpis.ec.europa.eu/registry/applicationschema/cap-iacs-base#MonthValue> ;
                                                                                        rdfs:label "May"@en ;
                                                                                        <http://www.w3.org/2004/02/skos/core#definition> """-- Definition --
May.
-- Description --
Item description."""@en ;
                                                                                        <http://www.w3.org/2004/02/skos/core#inScheme> :MonthValue .


###  http://lpis.ec.europa.eu/registry/applicationschema/cap-iacs-base/code#MonthValue/november
<http://lpis.ec.europa.eu/registry/applicationschema/cap-iacs-base/code#MonthValue/november> rdf:type owl:NamedIndividual ,
                                                                                                      <http://lpis.ec.europa.eu/registry/applicationschema/cap-iacs-base#MonthValue> ;
                                                                                             rdfs:label "November"@en ;
                                                                                             <http://www.w3.org/2004/02/skos/core#definition> """-- Definition --
November.
-- Description --
Item description."""@en ;
                                                                                             <http://www.w3.org/2004/02/skos/core#inScheme> :MonthValue .


###  http://lpis.ec.europa.eu/registry/applicationschema/cap-iacs-base/code#MonthValue/october
<http://lpis.ec.europa.eu/registry/applicationschema/cap-iacs-base/code#MonthValue/october> rdf:type owl:NamedIndividual ,
                                                                                                     <http://lpis.ec.europa.eu/registry/applicationschema/cap-iacs-base#MonthValue> ;
                                                                                            rdfs:label "October"@en ;
                                                                                            <http://www.w3.org/2004/02/skos/core#definition> """-- Definition --
October.
-- Description --
Item description."""@en ;
                                                                                            <http://www.w3.org/2004/02/skos/core#inScheme> :MonthValue .


###  http://lpis.ec.europa.eu/registry/applicationschema/cap-iacs-base/code#MonthValue/september
<http://lpis.ec.europa.eu/registry/applicationschema/cap-iacs-base/code#MonthValue/september> rdf:type owl:NamedIndividual ,
                                                                                                       <http://lpis.ec.europa.eu/registry/applicationschema/cap-iacs-base#MonthValue> ;
                                                                                              rdfs:label "September"@en ;
                                                                                              <http://www.w3.org/2004/02/skos/core#definition> """-- Definition --
September.
-- Description --
Item description."""@en ;
                                                                                              <http://www.w3.org/2004/02/skos/core#inScheme> :MonthValue .


###  http://lpis.ec.europa.eu/registry/applicationschema/cap-iacs-base/code#NotificationGroupValue/notificationOnTheResultsOfOtsc
<http://lpis.ec.europa.eu/registry/applicationschema/cap-iacs-base/code#NotificationGroupValue/notificationOnTheResultsOfOtsc> rdf:type owl:NamedIndividual ,
                                                                                                                                        <http://lpis.ec.europa.eu/registry/applicationschema/cap-iacs-base#NotificationGroupValue> ;
                                                                                                                               rdfs:label "Notifications concerning complementary national direct payments (BG and RO only)"@en ;
                                                                                                                               <http://www.w3.org/2004/02/skos/core#definition> """Notification on the results of OTSC

Each year, by 15 July, for all direct payment schemes, rural development measures and technical assistance and support schemes in the wine sector Member States shall notify the Commission of the control data and control statistics covering results of administrative, on-the-spot checks and ex post checks [Art. 9(1)(a) of R 809/2014]."""@en ;
                                                                                                                               <http://www.w3.org/2004/02/skos/core#inScheme> :NotificationGroupValue .


###  http://lpis.ec.europa.eu/registry/applicationschema/cap-iacs-base/code#NotificationGroupValue/notificationsConcerningAdjustmentRateForAGroupAtTheLevelOfItsMembers
<http://lpis.ec.europa.eu/registry/applicationschema/cap-iacs-base/code#NotificationGroupValue/notificationsConcerningAdjustmentRateForAGroupAtTheLevelOfItsMembers> rdf:type owl:NamedIndividual ,
                                                                                                                                                                              <http://lpis.ec.europa.eu/registry/applicationschema/cap-iacs-base#NotificationGroupValue> ;
                                                                                                                                                                     rdfs:label "Notifications concerning adjustment rate for a group at the level of its members"@en ;
                                                                                                                                                                     <http://www.w3.org/2004/02/skos/core#definition> """-- Definition --
Notifications concerning adjustment rate for a group at the level of its members
-- Description --
NOTE.71"""@en ;
                                                                                                                                                                     <http://www.w3.org/2004/02/skos/core#inScheme> :NotificationGroupValue .


###  http://lpis.ec.europa.eu/registry/applicationschema/cap-iacs-base/code#NotificationGroupValue/notificationsConcerningAnyAdditionalDetailsToBeProvidedOnRequest
<http://lpis.ec.europa.eu/registry/applicationschema/cap-iacs-base/code#NotificationGroupValue/notificationsConcerningAnyAdditionalDetailsToBeProvidedOnRequest> rdf:type owl:NamedIndividual ,
                                                                                                                                                                          <http://lpis.ec.europa.eu/registry/applicationschema/cap-iacs-base#NotificationGroupValue> ;
                                                                                                                                                                 rdfs:label "Notifications concerning any additional details to be provided on request"@en ;
                                                                                                                                                                 <http://www.w3.org/2004/02/skos/core#definition> """-- Definition --
Notifications concerning any additional details to be provided on request.
-- Description --
NOTE.721"""@en ;
                                                                                                                                                                 <http://www.w3.org/2004/02/skos/core#inScheme> :NotificationGroupValue .


###  http://lpis.ec.europa.eu/registry/applicationschema/cap-iacs-base/code#NotificationGroupValue/notificationsConcerningApplicationOfLinearReductions
<http://lpis.ec.europa.eu/registry/applicationschema/cap-iacs-base/code#NotificationGroupValue/notificationsConcerningApplicationOfLinearReductions> rdf:type owl:NamedIndividual ,
                                                                                                                                                              <http://lpis.ec.europa.eu/registry/applicationschema/cap-iacs-base#NotificationGroupValue> ;
                                                                                                                                                     rdfs:label "Notifications concerning application of linear reductions"@en ;
                                                                                                                                                     <http://www.w3.org/2004/02/skos/core#definition> """-- Definition --
Notifications concerning application of linear reductions.
-- Description --
NOTE.72"""@en ;
                                                                                                                                                     <http://www.w3.org/2004/02/skos/core#inScheme> :NotificationGroupValue .


###  http://lpis.ec.europa.eu/registry/applicationschema/cap-iacs-base/code#NotificationGroupValue/notificationsConcerningComplementaryNationalDirectPaymentsBgRo
<http://lpis.ec.europa.eu/registry/applicationschema/cap-iacs-base/code#NotificationGroupValue/notificationsConcerningComplementaryNationalDirectPaymentsBgRo> rdf:type owl:NamedIndividual ,
                                                                                                                                                                        <http://lpis.ec.europa.eu/registry/applicationschema/cap-iacs-base#NotificationGroupValue> ;
                                                                                                                                                               rdfs:label "Notifications concerning complementary national direct payments (BG and RO only)"@en ;
                                                                                                                                                               <http://www.w3.org/2004/02/skos/core#definition> """-- Definition --
Notifications concerning complementary national direct payments (BG and RO only).
-- Description --
NOTE.73"""@en ;
                                                                                                                                                               <http://www.w3.org/2004/02/skos/core#inScheme> :NotificationGroupValue .


###  http://lpis.ec.europa.eu/registry/applicationschema/cap-iacs-base/code#NotificationGroupValue/notificationsConcerningTheMinimumRequirementsForReceivingDirectPayments
<http://lpis.ec.europa.eu/registry/applicationschema/cap-iacs-base/code#NotificationGroupValue/notificationsConcerningTheMinimumRequirementsForReceivingDirectPayments> rdf:type owl:NamedIndividual ,
                                                                                                                                                                                 <http://lpis.ec.europa.eu/registry/applicationschema/cap-iacs-base#NotificationGroupValue> ;
                                                                                                                                                                        rdfs:label "Notifications concerning the minimum requirements for receiving direct payments"@en ;
                                                                                                                                                                        <http://www.w3.org/2004/02/skos/core#definition> """-- Definition --
Notifications concerning the minimum requirements for receiving direct payments.
-- Description --
NOTE.67"""@en ;
                                                                                                                                                                        <http://www.w3.org/2004/02/skos/core#inScheme> :NotificationGroupValue .


###  http://lpis.ec.europa.eu/registry/applicationschema/cap-iacs-base/code#NotificationGroupValue/notificationsConcerningThePaymentForAreasWithNaturalConstraints
<http://lpis.ec.europa.eu/registry/applicationschema/cap-iacs-base/code#NotificationGroupValue/notificationsConcerningThePaymentForAreasWithNaturalConstraints> rdf:type owl:NamedIndividual ,
                                                                                                                                                                         <http://lpis.ec.europa.eu/registry/applicationschema/cap-iacs-base#NotificationGroupValue> ;
                                                                                                                                                                rdfs:label "Notifications concerning the payment for areas with natural constraints"@en ;
                                                                                                                                                                <http://www.w3.org/2004/02/skos/core#definition> """-- Definition --
Notifications concerning the payment for areas with natural constraints.
-- Description --
NOTE.69"""@en ;
                                                                                                                                                                <http://www.w3.org/2004/02/skos/core#inScheme> :NotificationGroupValue .


###  http://lpis.ec.europa.eu/registry/applicationschema/cap-iacs-base/code#NotificationGroupValue/notificationsConcerningThePriorApprovaSystemForHempCultivation
<http://lpis.ec.europa.eu/registry/applicationschema/cap-iacs-base/code#NotificationGroupValue/notificationsConcerningThePriorApprovaSystemForHempCultivation> rdf:type owl:NamedIndividual ,
                                                                                                                                                                        <http://lpis.ec.europa.eu/registry/applicationschema/cap-iacs-base#NotificationGroupValue> ;
                                                                                                                                                               rdfs:label "Notifications concerning the small farmers scheme"@en ;
                                                                                                                                                               <http://www.w3.org/2004/02/skos/core#definition> "Notifications concerning the prior approval system for hemp cultivation"@en ;
                                                                                                                                                               <http://www.w3.org/2004/02/skos/core#inScheme> :NotificationGroupValue .


###  http://lpis.ec.europa.eu/registry/applicationschema/cap-iacs-base/code#NotificationGroupValue/notificationsConcerningTheRedistributivePayment
<http://lpis.ec.europa.eu/registry/applicationschema/cap-iacs-base/code#NotificationGroupValue/notificationsConcerningTheRedistributivePayment> rdf:type owl:NamedIndividual ,
                                                                                                                                                         <http://lpis.ec.europa.eu/registry/applicationschema/cap-iacs-base#NotificationGroupValue> ;
                                                                                                                                                rdfs:label "Notifications concerning the redistributive payment"@en ;
                                                                                                                                                <http://www.w3.org/2004/02/skos/core#definition> """-- Definition --
Notifications concerning the redistributive payment.
-- Description --
NOTE.68"""@en ;
                                                                                                                                                <http://www.w3.org/2004/02/skos/core#inScheme> :NotificationGroupValue .


###  http://lpis.ec.europa.eu/registry/applicationschema/cap-iacs-base/code#NotificationGroupValue/notificationsConcerningTheSmallFarmersScheme
<http://lpis.ec.europa.eu/registry/applicationschema/cap-iacs-base/code#NotificationGroupValue/notificationsConcerningTheSmallFarmersScheme> rdf:type owl:NamedIndividual ,
                                                                                                                                                      <http://lpis.ec.europa.eu/registry/applicationschema/cap-iacs-base#NotificationGroupValue> ;
                                                                                                                                             rdfs:label "Notifications concerning the small farmers scheme"@en ;
                                                                                                                                             <http://www.w3.org/2004/02/skos/core#definition> """-- Definition --
Notifications concerning the small farmers scheme.
-- Description --
NOTE.70"""@en ;
                                                                                                                                             <http://www.w3.org/2004/02/skos/core#inScheme> :NotificationGroupValue .


###  http://lpis.ec.europa.eu/registry/applicationschema/cap-iacs-base/code#NotificationGroupValue/notificationsConcerningTheValueOfPaymentEntitlementsSpsAndConvergence
<http://lpis.ec.europa.eu/registry/applicationschema/cap-iacs-base/code#NotificationGroupValue/notificationsConcerningTheValueOfPaymentEntitlementsSpsAndConvergence> rdf:type owl:NamedIndividual ,
                                                                                                                                                                               <http://lpis.ec.europa.eu/registry/applicationschema/cap-iacs-base#NotificationGroupValue> ;
                                                                                                                                                                      rdfs:label "Notifications concerning the value of payment entitlements (SPS) and convergence"@en ;
                                                                                                                                                                      <http://www.w3.org/2004/02/skos/core#definition> """-- Definition --
Notifications concerning the value of payment entitlements (SPS) and convergence.
-- Description --
NOTE.76"""@en ;
                                                                                                                                                                      <http://www.w3.org/2004/02/skos/core#inScheme> :NotificationGroupValue .


###  http://lpis.ec.europa.eu/registry/applicationschema/cap-iacs-base/code#NotificationGroupValue/notificationsRelatingDecisionsToReviewOfPreviousNotifications
<http://lpis.ec.europa.eu/registry/applicationschema/cap-iacs-base/code#NotificationGroupValue/notificationsRelatingDecisionsToReviewOfPreviousNotifications> rdf:type owl:NamedIndividual ,
                                                                                                                                                                       <http://lpis.ec.europa.eu/registry/applicationschema/cap-iacs-base#NotificationGroupValue> ;
                                                                                                                                                              rdfs:label "Notifications relating decisions to review of previous notifications"@en ;
                                                                                                                                                              <http://www.w3.org/2004/02/skos/core#definition> """-- Definition --
Notifications relating decisions to review of previous notifications.
-- Description --
NOTE.75"""@en ;
                                                                                                                                                              <http://www.w3.org/2004/02/skos/core#inScheme> :NotificationGroupValue .


###  http://lpis.ec.europa.eu/registry/applicationschema/cap-iacs-base/code#NotificationGroupValue/notificationsRelatingToDefinitionsAndRelatedProvisions
<http://lpis.ec.europa.eu/registry/applicationschema/cap-iacs-base/code#NotificationGroupValue/notificationsRelatingToDefinitionsAndRelatedProvisions> rdf:type owl:NamedIndividual ,
                                                                                                                                                                <http://lpis.ec.europa.eu/registry/applicationschema/cap-iacs-base#NotificationGroupValue> ;
                                                                                                                                                       rdfs:label "Notifications relating to definitions and related provisions"@en ;
                                                                                                                                                       <http://www.w3.org/2004/02/skos/core#definition> """-- Definition --
Notifications relating to definitions and related provisions.
-- Description --
NOTE.61"""@en ;
                                                                                                                                                       <http://www.w3.org/2004/02/skos/core#inScheme> :NotificationGroupValue .


###  http://lpis.ec.europa.eu/registry/applicationschema/cap-iacs-base/code#NotificationGroupValue/notificationsRelatingToGreening
<http://lpis.ec.europa.eu/registry/applicationschema/cap-iacs-base/code#NotificationGroupValue/notificationsRelatingToGreening> rdf:type owl:NamedIndividual ,
                                                                                                                                         <http://lpis.ec.europa.eu/registry/applicationschema/cap-iacs-base#NotificationGroupValue> ;
                                                                                                                                rdfs:label "Notifications relating to greening"@en ;
                                                                                                                                <http://www.w3.org/2004/02/skos/core#definition> """-- Definition --
Notifications relating to greening.
-- Description --
NOTE.64"""@en ;
                                                                                                                                <http://www.w3.org/2004/02/skos/core#inScheme> :NotificationGroupValue .


###  http://lpis.ec.europa.eu/registry/applicationschema/cap-iacs-base/code#NotificationGroupValue/notificationsRelatingToSapsDecisionsOnTransitionalNationalAid
<http://lpis.ec.europa.eu/registry/applicationschema/cap-iacs-base/code#NotificationGroupValue/notificationsRelatingToSapsDecisionsOnTransitionalNationalAid> rdf:type owl:NamedIndividual ,
                                                                                                                                                                       <http://lpis.ec.europa.eu/registry/applicationschema/cap-iacs-base#NotificationGroupValue> ;
                                                                                                                                                              rdfs:label "Notifications relating to SAPS decisions on transitional national aid"@en ;
                                                                                                                                                              <http://www.w3.org/2004/02/skos/core#definition> """-- Definition --
Notifications relating to SAPS decisions on transitional national aid.
-- Description --
NOTE.74"""@en ;
                                                                                                                                                              <http://www.w3.org/2004/02/skos/core#inScheme> :NotificationGroupValue .


###  http://lpis.ec.europa.eu/registry/applicationschema/cap-iacs-base/code#NotificationGroupValue/notificationsRelatingToTheAccreditedPayingAgenciesAndCoordinatingBodies
<http://lpis.ec.europa.eu/registry/applicationschema/cap-iacs-base/code#NotificationGroupValue/notificationsRelatingToTheAccreditedPayingAgenciesAndCoordinatingBodies> rdf:type owl:NamedIndividual ,
                                                                                                                                                                                 <http://lpis.ec.europa.eu/registry/applicationschema/cap-iacs-base#NotificationGroupValue> ;
                                                                                                                                                                        rdfs:label "Notifications relating to the accredited paying agencies and coordinating bodies"@en ;
                                                                                                                                                                        <http://www.w3.org/2004/02/skos/core#definition> """-- Definition --
Notifications relating to the accredited paying agencies and coordinating bodies.
-- Description --
In addition to the provisions laid down in the sectoral Regulations, Member States shall send to the Commission the information, declarations and documents: for accredited paying agencies and accredited coordinating bodies
(a)(i) their accreditation document;
(a)(ii) their function (accredited paying agency or accredited coordinating body);
(a)(iii) where relevant, the withdrawal of their accreditation.
NOTE.1011a"""@en ;
                                                                                                                                                                        <http://www.w3.org/2004/02/skos/core#inScheme> :NotificationGroupValue .


###  http://lpis.ec.europa.eu/registry/applicationschema/cap-iacs-base/code#NotificationGroupValue/notificationsRelatingToTheApplicationOfTheIntegratedSystem
<http://lpis.ec.europa.eu/registry/applicationschema/cap-iacs-base/code#NotificationGroupValue/notificationsRelatingToTheApplicationOfTheIntegratedSystem> rdf:type owl:NamedIndividual ,
                                                                                                                                                                    <http://lpis.ec.europa.eu/registry/applicationschema/cap-iacs-base#NotificationGroupValue> ;
                                                                                                                                                           rdfs:label "Notifications relating to the application of the integrated system"@en ;
                                                                                                                                                           <http://www.w3.org/2004/02/skos/core#definition> """-- Definition --
Notifications relating to the the application of the integrated system.
-- Description --
Member State shall inform the Commission regularly of the application of the integrated system referred to in Chapter II of Title V. The Commission shall organize exchanges of views on this subject with the Member States.
NOTE.1023"""@en ;
                                                                                                                                                           <http://www.w3.org/2004/02/skos/core#inScheme> :NotificationGroupValue .


###  http://lpis.ec.europa.eu/registry/applicationschema/cap-iacs-base/code#NotificationGroupValue/notificationsRelatingToTheBasicPayment
<http://lpis.ec.europa.eu/registry/applicationschema/cap-iacs-base/code#NotificationGroupValue/notificationsRelatingToTheBasicPayment> rdf:type owl:NamedIndividual ,
                                                                                                                                                <http://lpis.ec.europa.eu/registry/applicationschema/cap-iacs-base#NotificationGroupValue> ;
                                                                                                                                       rdfs:label "Notifications relating to the basic payment"@en ;
                                                                                                                                       <http://www.w3.org/2004/02/skos/core#definition> """-- Definition --
Notifications relating to the basic payment.
-- Description --
NOTE.63"""@en ;
                                                                                                                                       <http://www.w3.org/2004/02/skos/core#inScheme> :NotificationGroupValue .


###  http://lpis.ec.europa.eu/registry/applicationschema/cap-iacs-base/code#NotificationGroupValue/notificationsRelatingToTheCertificationBodies
<http://lpis.ec.europa.eu/registry/applicationschema/cap-iacs-base/code#NotificationGroupValue/notificationsRelatingToTheCertificationBodies> rdf:type owl:NamedIndividual ,
                                                                                                                                                       <http://lpis.ec.europa.eu/registry/applicationschema/cap-iacs-base#NotificationGroupValue> ;
                                                                                                                                              rdfs:label "Notifications relating to the certification bodies"@en ;
                                                                                                                                              <http://www.w3.org/2004/02/skos/core#definition> """-- Definition --
Notifications relating to the certification bodies.
-- Description --
In addition to the provisions laid down in the sectoral Regulations, Member States shall send to the Commission the information, declarations and documents:  for certification bodies:
(b)(i) their name;
(b)(ii) their address,
NOTE.1011b"""@en ;
                                                                                                                                              <http://www.w3.org/2004/02/skos/core#inScheme> :NotificationGroupValue .


###  http://lpis.ec.europa.eu/registry/applicationschema/cap-iacs-base/code#NotificationGroupValue/notificationsRelatingToTheFinancialAdjustmentsMadeByMemberStatesInConnectionWithRuralDevelopment
<http://lpis.ec.europa.eu/registry/applicationschema/cap-iacs-base/code#NotificationGroupValue/notificationsRelatingToTheFinancialAdjustmentsMadeByMemberStatesInConnectionWithRuralDevelopment> rdf:type owl:NamedIndividual ,
                                                                                                                                                                                                          <http://lpis.ec.europa.eu/registry/applicationschema/cap-iacs-base#NotificationGroupValue> ;
                                                                                                                                                                                                 rdfs:label "Notifications relating to the financial adjustments made by Member States in connection with rural development"@en ;
                                                                                                                                                                                                 <http://www.w3.org/2004/02/skos/core#definition> """-- Definition --
Notifications relating to the financial adjustments made by Member States in connection with rural development.
-- Description --
NOTE.104"""@en ;
                                                                                                                                                                                                 <http://www.w3.org/2004/02/skos/core#inScheme> :NotificationGroupValue .


###  http://lpis.ec.europa.eu/registry/applicationschema/cap-iacs-base/code#NotificationGroupValue/notificationsRelatingToTheImplementationOfGaecAndFas
<http://lpis.ec.europa.eu/registry/applicationschema/cap-iacs-base/code#NotificationGroupValue/notificationsRelatingToTheImplementationOfGaecAndFas> rdf:type owl:NamedIndividual ,
                                                                                                                                                              <http://lpis.ec.europa.eu/registry/applicationschema/cap-iacs-base#NotificationGroupValue> ;
                                                                                                                                                     rdfs:label "Notifications relating to the implementation of GAEC and FAS"@en ;
                                                                                                                                                     <http://www.w3.org/2004/02/skos/core#definition> """-- Definition --
Notifications relating to the implementation of GAEC and FAS.
-- Description --
Member States shall inform the Commission in detail of the measures taken to implement the good agricultural and environmental condition referred to in Article 94 and the details of the farm advisory system referred to in Title 
III.
NOTE.1012"""@en ;
                                                                                                                                                     <http://www.w3.org/2004/02/skos/core#inScheme> :NotificationGroupValue .


###  http://lpis.ec.europa.eu/registry/applicationschema/cap-iacs-base/code#NotificationGroupValue/notificationsRelatingToTheMeasuresRelatedToOperationsFinancedByTheFunds
<http://lpis.ec.europa.eu/registry/applicationschema/cap-iacs-base/code#NotificationGroupValue/notificationsRelatingToTheMeasuresRelatedToOperationsFinancedByTheFunds> rdf:type owl:NamedIndividual ,
                                                                                                                                                                                 <http://lpis.ec.europa.eu/registry/applicationschema/cap-iacs-base#NotificationGroupValue> ;
                                                                                                                                                                        rdfs:label "Notifications relating to the  measures related to operations financed by the Funds"@en ;
                                                                                                                                                                        <http://www.w3.org/2004/02/skos/core#definition> """-- Definition --
Notifications relating to the  measures related to operations financed by the Funds.
-- Description --
In addition to the provisions laid down in the sectoral Regulations, Member States shall send to the Commission the information, declarations and documents:  for measures relating to operations financed by the Funds:
(c)(i) declarations of expenditure, which also act as payment requests, signed by the accredited paying agency or the accredited coordinating body and accompanied by the requisite information;
(c)(ii) estimates of their financial requirements, with regard to the EAGF and, with regard to the EAFRD, an update of estimated declarations of expenditure which will be submitted during the year and estimated declarations of 
expenditure in respect of the following financial year;
(c)(iii) the management declaration and the annual accounts of the accredited paying agencies;
(c)(iv) an annual summary of the results of all available audits and checks carried out in accordance with the schedule and detailed provisions laid down in the sector specific rules.
The annual accounts of accredited paying agencies relating to EAFRD expenditure shall be submitted at the level of each programme.
NOTE.1011c"""@en ;
                                                                                                                                                                        <http://www.w3.org/2004/02/skos/core#inScheme> :NotificationGroupValue .


###  http://lpis.ec.europa.eu/registry/applicationschema/cap-iacs-base/code#NotificationGroupValue/notificationsRelatingToThePaymentForYoungFarmers
<http://lpis.ec.europa.eu/registry/applicationschema/cap-iacs-base/code#NotificationGroupValue/notificationsRelatingToThePaymentForYoungFarmers> rdf:type owl:NamedIndividual ,
                                                                                                                                                          <http://lpis.ec.europa.eu/registry/applicationschema/cap-iacs-base#NotificationGroupValue> ;
                                                                                                                                                 rdfs:label "Notifications relating to the payment for young farmers"@en ;
                                                                                                                                                 <http://www.w3.org/2004/02/skos/core#definition> """-- Definition --
Notifications relating to the payment for young farmers.
-- Description --
NOTE.65"""@en ;
                                                                                                                                                 <http://www.w3.org/2004/02/skos/core#inScheme> :NotificationGroupValue .


###  http://lpis.ec.europa.eu/registry/applicationschema/cap-iacs-base/code#NotificationGroupValue/notificationsRelatingToTheReductionCoefficient
<http://lpis.ec.europa.eu/registry/applicationschema/cap-iacs-base/code#NotificationGroupValue/notificationsRelatingToTheReductionCoefficient> rdf:type owl:NamedIndividual ,
                                                                                                                                                        <http://lpis.ec.europa.eu/registry/applicationschema/cap-iacs-base#NotificationGroupValue> ;
                                                                                                                                               rdfs:label "Notifications relating to the reduction coefficient"@en ;
                                                                                                                                               <http://www.w3.org/2004/02/skos/core#definition> """-- Definition --
Notifications relating to the reduction coefficient.
-- Description --
NOTE.62"""@en ;
                                                                                                                                               <http://www.w3.org/2004/02/skos/core#inScheme> :NotificationGroupValue .


###  http://lpis.ec.europa.eu/registry/applicationschema/cap-iacs-base/code#NotificationGroupValue/notificationsRelatingToTheVoluntaryCoupledSupport
<http://lpis.ec.europa.eu/registry/applicationschema/cap-iacs-base/code#NotificationGroupValue/notificationsRelatingToTheVoluntaryCoupledSupport> rdf:type owl:NamedIndividual ,
                                                                                                                                                           <http://lpis.ec.europa.eu/registry/applicationschema/cap-iacs-base#NotificationGroupValue> ;
                                                                                                                                                  rdfs:label "Notifications relating to the voluntary coupled support"@en ;
                                                                                                                                                  <http://www.w3.org/2004/02/skos/core#definition> """-- Definition --
Notifications relating to the voluntary coupled support.
-- Description --
NOTE.66"""@en ;
                                                                                                                                                  <http://www.w3.org/2004/02/skos/core#inScheme> :NotificationGroupValue .


###  http://lpis.ec.europa.eu/registry/applicationschema/cap-iacs-base/code#OrdinalNumberValue/first
<http://lpis.ec.europa.eu/registry/applicationschema/cap-iacs-base/code#OrdinalNumberValue/first> rdf:type owl:NamedIndividual ,
                                                                                                           <http://lpis.ec.europa.eu/registry/applicationschema/cap-iacs-base#OrdinalNumberValue> ;
                                                                                                  rdfs:label "First"@en ;
                                                                                                  <http://www.w3.org/2004/02/skos/core#definition> """-- Definition --
First.
-- Description --
Item description."""@en ;
                                                                                                  <http://www.w3.org/2004/02/skos/core#inScheme> :OrdinalNumberValue .


###  http://lpis.ec.europa.eu/registry/applicationschema/cap-iacs-base/code#OrdinalNumberValue/fourth
<http://lpis.ec.europa.eu/registry/applicationschema/cap-iacs-base/code#OrdinalNumberValue/fourth> rdf:type owl:NamedIndividual ,
                                                                                                            <http://lpis.ec.europa.eu/registry/applicationschema/cap-iacs-base#OrdinalNumberValue> ;
                                                                                                   rdfs:label "Fourth"@en ;
                                                                                                   <http://www.w3.org/2004/02/skos/core#definition> """-- Definition --
Fourth.
-- Description --
Item description."""@en ;
                                                                                                   <http://www.w3.org/2004/02/skos/core#inScheme> :OrdinalNumberValue .


###  http://lpis.ec.europa.eu/registry/applicationschema/cap-iacs-base/code#OrdinalNumberValue/last
<http://lpis.ec.europa.eu/registry/applicationschema/cap-iacs-base/code#OrdinalNumberValue/last> rdf:type owl:NamedIndividual ,
                                                                                                          <http://lpis.ec.europa.eu/registry/applicationschema/cap-iacs-base#OrdinalNumberValue> ;
                                                                                                 rdfs:label "Last"@en ;
                                                                                                 <http://www.w3.org/2004/02/skos/core#definition> """-- Definition --
Last.
-- Description --
Item description."""@en ;
                                                                                                 <http://www.w3.org/2004/02/skos/core#inScheme> :OrdinalNumberValue .


###  http://lpis.ec.europa.eu/registry/applicationschema/cap-iacs-base/code#OrdinalNumberValue/second
<http://lpis.ec.europa.eu/registry/applicationschema/cap-iacs-base/code#OrdinalNumberValue/second> rdf:type owl:NamedIndividual ,
                                                                                                            <http://lpis.ec.europa.eu/registry/applicationschema/cap-iacs-base#OrdinalNumberValue> ;
                                                                                                   rdfs:label "Second"@en ;
                                                                                                   <http://www.w3.org/2004/02/skos/core#definition> """-- Definition --
Second.
-- Description --
Item description."""@en ;
                                                                                                   <http://www.w3.org/2004/02/skos/core#inScheme> :OrdinalNumberValue .


###  http://lpis.ec.europa.eu/registry/applicationschema/cap-iacs-base/code#OrdinalNumberValue/third
<http://lpis.ec.europa.eu/registry/applicationschema/cap-iacs-base/code#OrdinalNumberValue/third> rdf:type owl:NamedIndividual ,
                                                                                                           <http://lpis.ec.europa.eu/registry/applicationschema/cap-iacs-base#OrdinalNumberValue> ;
                                                                                                  rdfs:label "Third"@en ;
                                                                                                  <http://www.w3.org/2004/02/skos/core#definition> """-- Definition --
Third.
-- Description --
Item description."""@en ;
                                                                                                  <http://www.w3.org/2004/02/skos/core#inScheme> :OrdinalNumberValue .


###  http://lpis.ec.europa.eu/registry/applicationschema/cap-iacs-base/code#RecurenceValue/daily
<http://lpis.ec.europa.eu/registry/applicationschema/cap-iacs-base/code#RecurenceValue/daily> rdf:type owl:NamedIndividual ,
                                                                                                       <http://lpis.ec.europa.eu/registry/applicationschema/cap-iacs-base#RecurenceValue> ;
                                                                                              rdfs:label "Daily recurrence"@en ;
                                                                                              <http://www.w3.org/2004/02/skos/core#definition> """-- Definition --
Daily recurrence.
-- Description --
Item description."""@en ;
                                                                                              <http://www.w3.org/2004/02/skos/core#inScheme> :RecurenceValue .


###  http://lpis.ec.europa.eu/registry/applicationschema/cap-iacs-base/code#RecurenceValue/monthly
<http://lpis.ec.europa.eu/registry/applicationschema/cap-iacs-base/code#RecurenceValue/monthly> rdf:type owl:NamedIndividual ,
                                                                                                         <http://lpis.ec.europa.eu/registry/applicationschema/cap-iacs-base#RecurenceValue> ;
                                                                                                rdfs:label "Monthly recurrence"@en ;
                                                                                                <http://www.w3.org/2004/02/skos/core#definition> """-- Definition --
Monthly recurrence.
-- Description --
Item description."""@en ;
                                                                                                <http://www.w3.org/2004/02/skos/core#inScheme> :RecurenceValue .


###  http://lpis.ec.europa.eu/registry/applicationschema/cap-iacs-base/code#RecurenceValue/noRecurrence
<http://lpis.ec.europa.eu/registry/applicationschema/cap-iacs-base/code#RecurenceValue/noRecurrence> rdf:type owl:NamedIndividual ,
                                                                                                              <http://lpis.ec.europa.eu/registry/applicationschema/cap-iacs-base#RecurenceValue> ;
                                                                                                     rdfs:label "No recurrence"@en ;
                                                                                                     <http://www.w3.org/2004/02/skos/core#definition> """-- Definition --
No recurrence.
-- Description --
Item description."""@en ;
                                                                                                     <http://www.w3.org/2004/02/skos/core#inScheme> :RecurenceValue .


###  http://lpis.ec.europa.eu/registry/applicationschema/cap-iacs-base/code#RecurenceValue/weekly
<http://lpis.ec.europa.eu/registry/applicationschema/cap-iacs-base/code#RecurenceValue/weekly> rdf:type owl:NamedIndividual ,
                                                                                                        <http://lpis.ec.europa.eu/registry/applicationschema/cap-iacs-base#RecurenceValue> ;
                                                                                               rdfs:label "Weekly recurrence"@en ;
                                                                                               <http://www.w3.org/2004/02/skos/core#definition> """-- Definition --
Weekly recurrence.
-- Description --
Item description."""@en ;
                                                                                               <http://www.w3.org/2004/02/skos/core#inScheme> :RecurenceValue .


###  http://lpis.ec.europa.eu/registry/applicationschema/cap-iacs-base/code#RecurenceValue/yearly
<http://lpis.ec.europa.eu/registry/applicationschema/cap-iacs-base/code#RecurenceValue/yearly> rdf:type owl:NamedIndividual ,
                                                                                                        <http://lpis.ec.europa.eu/registry/applicationschema/cap-iacs-base#RecurenceValue> ;
                                                                                               rdfs:label "Yearly recurrence"@en ;
                                                                                               <http://www.w3.org/2004/02/skos/core#definition> """-- Definition --
Yearly recurrence.
-- Description --
Item description."""@en ;
                                                                                               <http://www.w3.org/2004/02/skos/core#inScheme> :RecurenceValue .


###  http://lpis.ec.europa.eu/registry/applicationschema/cap-iacs-base/code#SpecieCodeValue/agrostisCaninaLVelvetBent
<http://lpis.ec.europa.eu/registry/applicationschema/cap-iacs-base/code#SpecieCodeValue/agrostisCaninaLVelvetBent> rdf:type owl:NamedIndividual ,
                                                                                                                            <http://lpis.ec.europa.eu/registry/applicationschema/cap-iacs-base#SpecieCodeValue> ;
                                                                                                                   rdfs:label "Agrostis canina L. Velvet bent"@en ;
                                                                                                                   <http://www.w3.org/2004/02/skos/core#definition> """-- Definition --
Agrostis canina L. Velvet bent.
-- Description --
List of agricultural species -A
II. Fodder plants
NOTE. Initial value: A - 3."""@en ;
                                                                                                                   <http://www.w3.org/2004/02/skos/core#inScheme> :SpecieCodeValue .


###  http://lpis.ec.europa.eu/registry/applicationschema/cap-iacs-base/code#SpecieCodeValue/agrostisCapillarisLBrownTop
<http://lpis.ec.europa.eu/registry/applicationschema/cap-iacs-base/code#SpecieCodeValue/agrostisCapillarisLBrownTop> rdf:type owl:NamedIndividual ,
                                                                                                                              <http://lpis.ec.europa.eu/registry/applicationschema/cap-iacs-base#SpecieCodeValue> ;
                                                                                                                     rdfs:label "Agrostis capillaris L. Brown top"@en ;
                                                                                                                     <http://www.w3.org/2004/02/skos/core#definition> """-- Definition --
Agrostis capillaris L. Brown top.
-- Description --
List of agricultural species -A
II. Fodder plants
NOTE. Initial value: A - 6."""@en ;
                                                                                                                     <http://www.w3.org/2004/02/skos/core#inScheme> :SpecieCodeValue .


###  http://lpis.ec.europa.eu/registry/applicationschema/cap-iacs-base/code#SpecieCodeValue/agrostisGiganteaLRedTop
<http://lpis.ec.europa.eu/registry/applicationschema/cap-iacs-base/code#SpecieCodeValue/agrostisGiganteaLRedTop> rdf:type owl:NamedIndividual ,
                                                                                                                          <http://lpis.ec.europa.eu/registry/applicationschema/cap-iacs-base#SpecieCodeValue> ;
                                                                                                                 rdfs:label "Agrostis gigantea L. Red top"@en ;
                                                                                                                 <http://www.w3.org/2004/02/skos/core#definition> """-- Definition --
Agrostis gigantea L. Red top.
-- Description --
List of agricultural species -A
II. Fodder plants
NOTE. Initial value: A - 4."""@en ;
                                                                                                                 <http://www.w3.org/2004/02/skos/core#inScheme> :SpecieCodeValue .


###  http://lpis.ec.europa.eu/registry/applicationschema/cap-iacs-base/code#SpecieCodeValue/agrostisStoloniferaLCreepingBent
<http://lpis.ec.europa.eu/registry/applicationschema/cap-iacs-base/code#SpecieCodeValue/agrostisStoloniferaLCreepingBent> rdf:type owl:NamedIndividual ,
                                                                                                                                   <http://lpis.ec.europa.eu/registry/applicationschema/cap-iacs-base#SpecieCodeValue> ;
                                                                                                                          rdfs:label "Agrostis stolonifera L. Creeping bent"@en ;
                                                                                                                          <http://www.w3.org/2004/02/skos/core#definition> """-- Definition --
Agrostis stolonifera L. Creeping bent.
-- Description --
List of agricultural species -A
II. Fodder plants
NOTE. Initial value: A - 5."""@en ;
                                                                                                                          <http://www.w3.org/2004/02/skos/core#inScheme> :SpecieCodeValue .


###  http://lpis.ec.europa.eu/registry/applicationschema/cap-iacs-base/code#SpecieCodeValue/alliumCepaLAggregatumGroupShallot
<http://lpis.ec.europa.eu/registry/applicationschema/cap-iacs-base/code#SpecieCodeValue/alliumCepaLAggregatumGroupShallot> rdf:type owl:NamedIndividual ,
                                                                                                                                    <http://lpis.ec.europa.eu/registry/applicationschema/cap-iacs-base#SpecieCodeValue> ;
                                                                                                                           rdfs:label "Allium cepa L. Aggregatum group - Shallot"@en ;
                                                                                                                           <http://www.w3.org/2004/02/skos/core#definition> """-- Definition --
Allium cepa L. Aggregatum group - Shallot.
-- Description --
List of vegetable specie -H
NOTE. Initial value: H - 1.1"""@en ;
                                                                                                                           <http://www.w3.org/2004/02/skos/core#inScheme> :SpecieCodeValue .


###  http://lpis.ec.europa.eu/registry/applicationschema/cap-iacs-base/code#SpecieCodeValue/alliumCepaLCepaGroupOnionEchalion
<http://lpis.ec.europa.eu/registry/applicationschema/cap-iacs-base/code#SpecieCodeValue/alliumCepaLCepaGroupOnionEchalion> rdf:type owl:NamedIndividual ,
                                                                                                                                    <http://lpis.ec.europa.eu/registry/applicationschema/cap-iacs-base#SpecieCodeValue> ;
                                                                                                                           rdfs:label "Allium cepa L. Cepa group - Onion, Echalion"@en ;
                                                                                                                           <http://www.w3.org/2004/02/skos/core#definition> """-- Definition --
Allium cepa L. Cepa group - Onion, Echalion.
-- Description --
List of vegetable specie -H
NOTE. Initial value: H - 1.2"""@en ;
                                                                                                                           <http://www.w3.org/2004/02/skos/core#inScheme> :SpecieCodeValue .


###  http://lpis.ec.europa.eu/registry/applicationschema/cap-iacs-base/code#SpecieCodeValue/alliumFistulosumLJapaneseBunchingOnionWelshOnion
<http://lpis.ec.europa.eu/registry/applicationschema/cap-iacs-base/code#SpecieCodeValue/alliumFistulosumLJapaneseBunchingOnionWelshOnion> rdf:type owl:NamedIndividual ,
                                                                                                                                                   <http://lpis.ec.europa.eu/registry/applicationschema/cap-iacs-base#SpecieCodeValue> ;
                                                                                                                                          rdfs:label "Allium fistulosum L. Japanese bunching onion / Welsh onion"@en ;
                                                                                                                                          <http://www.w3.org/2004/02/skos/core#definition> """-- Definition --
Allium fistulosum L. Japanese bunching onion / Welsh onion.
-- Description --
List of vegetable specie -H
NOTE. Initial value: H - 2."""@en ;
                                                                                                                                          <http://www.w3.org/2004/02/skos/core#inScheme> :SpecieCodeValue .


###  http://lpis.ec.europa.eu/registry/applicationschema/cap-iacs-base/code#SpecieCodeValue/alliumPorrumLLeek
<http://lpis.ec.europa.eu/registry/applicationschema/cap-iacs-base/code#SpecieCodeValue/alliumPorrumLLeek> rdf:type owl:NamedIndividual ,
                                                                                                                    <http://lpis.ec.europa.eu/registry/applicationschema/cap-iacs-base#SpecieCodeValue> ;
                                                                                                           rdfs:label "Allium porrum L. Leek"@en ;
                                                                                                           <http://www.w3.org/2004/02/skos/core#definition> """-- Definition --
Allium porrum L. Leek.
-- Description --
List of vegetable specie -H
NOTE. Initial value: H - 3."""@en ;
                                                                                                           <http://www.w3.org/2004/02/skos/core#inScheme> :SpecieCodeValue .


###  http://lpis.ec.europa.eu/registry/applicationschema/cap-iacs-base/code#SpecieCodeValue/alliumSativumLGarlic
<http://lpis.ec.europa.eu/registry/applicationschema/cap-iacs-base/code#SpecieCodeValue/alliumSativumLGarlic> rdf:type owl:NamedIndividual ,
                                                                                                                       <http://lpis.ec.europa.eu/registry/applicationschema/cap-iacs-base#SpecieCodeValue> ;
                                                                                                              rdfs:label "Allium sativum L. Garlic"@en ;
                                                                                                              <http://www.w3.org/2004/02/skos/core#definition> """-- Definition --
Allium sativum L. Garlic.
-- Description --
List of vegetable specie -H
NOTE. Initial value: H - 4."""@en ;
                                                                                                              <http://www.w3.org/2004/02/skos/core#inScheme> :SpecieCodeValue .


###  http://lpis.ec.europa.eu/registry/applicationschema/cap-iacs-base/code#SpecieCodeValue/alliumSchoenoprasumLChives
<http://lpis.ec.europa.eu/registry/applicationschema/cap-iacs-base/code#SpecieCodeValue/alliumSchoenoprasumLChives> rdf:type owl:NamedIndividual ,
                                                                                                                             <http://lpis.ec.europa.eu/registry/applicationschema/cap-iacs-base#SpecieCodeValue> ;
                                                                                                                    rdfs:label "Allium schoenoprasum L. Chives"@en ;
                                                                                                                    <http://www.w3.org/2004/02/skos/core#definition> """-- Definition --
Allium schoenoprasum L. Chives.
-- Description --
List of vegetable specie -H
NOTE. Initial value: H - 5."""@en ;
                                                                                                                    <http://www.w3.org/2004/02/skos/core#inScheme> :SpecieCodeValue .


###  http://lpis.ec.europa.eu/registry/applicationschema/cap-iacs-base/code#SpecieCodeValue/alopecurusPratensisLMeadowFoxtail
<http://lpis.ec.europa.eu/registry/applicationschema/cap-iacs-base/code#SpecieCodeValue/alopecurusPratensisLMeadowFoxtail> rdf:type owl:NamedIndividual ,
                                                                                                                                    <http://lpis.ec.europa.eu/registry/applicationschema/cap-iacs-base#SpecieCodeValue> ;
                                                                                                                           rdfs:label "Alopecurus pratensis L. Meadow foxtail "@en ;
                                                                                                                           <http://www.w3.org/2004/02/skos/core#definition> """-- Definition --
Alopecurus pratensis L. Meadow foxtail.
-- Description --
List of agricultural species -A
II. Fodder plants
NOTE. Initial value: A - 7."""@en ;
                                                                                                                           <http://www.w3.org/2004/02/skos/core#inScheme> :SpecieCodeValue .


###  http://lpis.ec.europa.eu/registry/applicationschema/cap-iacs-base/code#SpecieCodeValue/anthriscusCerefoliumLHoffmChervil
<http://lpis.ec.europa.eu/registry/applicationschema/cap-iacs-base/code#SpecieCodeValue/anthriscusCerefoliumLHoffmChervil> rdf:type owl:NamedIndividual ,
                                                                                                                                    <http://lpis.ec.europa.eu/registry/applicationschema/cap-iacs-base#SpecieCodeValue> ;
                                                                                                                           rdfs:label "Anthriscus cerefolium (L.) Hoffm. Chervil"@en ;
                                                                                                                           <http://www.w3.org/2004/02/skos/core#definition> """-- Definition --
Anthriscus cerefolium (L.) Hoffm. Chervil.
-- Description --
List of vegetable specie -H
NOTE. Initial value: H - 6."""@en ;
                                                                                                                           <http://www.w3.org/2004/02/skos/core#inScheme> :SpecieCodeValue .


###  http://lpis.ec.europa.eu/registry/applicationschema/cap-iacs-base/code#SpecieCodeValue/apiumGraveolensLCeleriac
<http://lpis.ec.europa.eu/registry/applicationschema/cap-iacs-base/code#SpecieCodeValue/apiumGraveolensLCeleriac> rdf:type owl:NamedIndividual ,
                                                                                                                           <http://lpis.ec.europa.eu/registry/applicationschema/cap-iacs-base#SpecieCodeValue> ;
                                                                                                                  rdfs:label "Apium graveolens L. Celeriac"@en ;
                                                                                                                  <http://www.w3.org/2004/02/skos/core#definition> """-- Definition --
Apium graveolens L. Celeriac.
-- Description --
List of vegetable specie -H
NOTE. Initial value: H - 7.2"""@en ;
                                                                                                                  <http://www.w3.org/2004/02/skos/core#inScheme> :SpecieCodeValue .


###  http://lpis.ec.europa.eu/registry/applicationschema/cap-iacs-base/code#SpecieCodeValue/apiumGraveolensLCelery
<http://lpis.ec.europa.eu/registry/applicationschema/cap-iacs-base/code#SpecieCodeValue/apiumGraveolensLCelery> rdf:type owl:NamedIndividual ,
                                                                                                                         <http://lpis.ec.europa.eu/registry/applicationschema/cap-iacs-base#SpecieCodeValue> ;
                                                                                                                rdfs:label "Apium graveolens L. Celery"@en ;
                                                                                                                <http://www.w3.org/2004/02/skos/core#definition> """-- Definition --
Apium graveolens L. Celery.
-- Description --
List of vegetable specie -H
NOTE. Initial value: H - 7.1"""@en ;
                                                                                                                <http://www.w3.org/2004/02/skos/core#inScheme> :SpecieCodeValue .


###  http://lpis.ec.europa.eu/registry/applicationschema/cap-iacs-base/code#SpecieCodeValue/arachisHypogeaLGroundnutPeanut
<http://lpis.ec.europa.eu/registry/applicationschema/cap-iacs-base/code#SpecieCodeValue/arachisHypogeaLGroundnutPeanut> rdf:type owl:NamedIndividual ,
                                                                                                                                 <http://lpis.ec.europa.eu/registry/applicationschema/cap-iacs-base#SpecieCodeValue> ;
                                                                                                                        rdfs:label "Arachis hypogea L. Groundnut/Peanut"@en ;
                                                                                                                        <http://www.w3.org/2004/02/skos/core#definition> """-- Definition --
Arachis hypogea L. Groundnut/Peanut.
-- Description --
List of agricultural species -A
III. Oil and fibre plants
NOTE. Initial value: A - 58."""@en ;
                                                                                                                        <http://www.w3.org/2004/02/skos/core#inScheme> :SpecieCodeValue .


###  http://lpis.ec.europa.eu/registry/applicationschema/cap-iacs-base/code#SpecieCodeValue/arrhenatherumElatiusLTallOatgrass
<http://lpis.ec.europa.eu/registry/applicationschema/cap-iacs-base/code#SpecieCodeValue/arrhenatherumElatiusLTallOatgrass> rdf:type owl:NamedIndividual ,
                                                                                                                                    <http://lpis.ec.europa.eu/registry/applicationschema/cap-iacs-base#SpecieCodeValue> ;
                                                                                                                           rdfs:label "Arrhenatherum elatius L. Tall oatgrass "@en ;
                                                                                                                           <http://www.w3.org/2004/02/skos/core#definition> """-- Definition --
Arrhenatherum elatius L. Tall oatgrass.
-- Description --
List of agricultural species -A
II. Fodder plants
NOTE. Initial value: A - 8."""@en ;
                                                                                                                           <http://www.w3.org/2004/02/skos/core#inScheme> :SpecieCodeValue .


###  http://lpis.ec.europa.eu/registry/applicationschema/cap-iacs-base/code#SpecieCodeValue/asparagusOfficinalisLAsparagus
<http://lpis.ec.europa.eu/registry/applicationschema/cap-iacs-base/code#SpecieCodeValue/asparagusOfficinalisLAsparagus> rdf:type owl:NamedIndividual ,
                                                                                                                                 <http://lpis.ec.europa.eu/registry/applicationschema/cap-iacs-base#SpecieCodeValue> ;
                                                                                                                        rdfs:label "Asparagus officinalis L. Asparagus"@en ;
                                                                                                                        <http://www.w3.org/2004/02/skos/core#definition> """-- Definition --
Asparagus officinalis L. Asparagus.
-- Description --
List of vegetable specie -H
NOTE. Initial value: H - 8."""@en ;
                                                                                                                        <http://www.w3.org/2004/02/skos/core#inScheme> :SpecieCodeValue .


###  http://lpis.ec.europa.eu/registry/applicationschema/cap-iacs-base/code#SpecieCodeValue/avenaNudaLSmallNakedOatHullessOat
<http://lpis.ec.europa.eu/registry/applicationschema/cap-iacs-base/code#SpecieCodeValue/avenaNudaLSmallNakedOatHullessOat> rdf:type owl:NamedIndividual ,
                                                                                                                                    <http://lpis.ec.europa.eu/registry/applicationschema/cap-iacs-base#SpecieCodeValue> ;
                                                                                                                           rdfs:label "Avena nuda L. Small naked oat / Hulless oat "@en ;
                                                                                                                           <http://www.w3.org/2004/02/skos/core#definition> """-- Definition --
Avena nuda L. Small naked oat / Hulless oat.
-- Description --
List of agricultural species -A   
IV. Cereals
NOTE. Initial value: A - 72."""@en ;
                                                                                                                           <http://www.w3.org/2004/02/skos/core#inScheme> :SpecieCodeValue .


###  http://lpis.ec.europa.eu/registry/applicationschema/cap-iacs-base/code#SpecieCodeValue/avenaSativaLIncludingAByzantinaKKochOatAndRedOat
<http://lpis.ec.europa.eu/registry/applicationschema/cap-iacs-base/code#SpecieCodeValue/avenaSativaLIncludingAByzantinaKKochOatAndRedOat> rdf:type owl:NamedIndividual ,
                                                                                                                                                   <http://lpis.ec.europa.eu/registry/applicationschema/cap-iacs-base#SpecieCodeValue> ;
                                                                                                                                          rdfs:label "Avena sativa L. (including A. byzantina K. Koch) Oat and Red oat"@en ;
                                                                                                                                          <http://www.w3.org/2004/02/skos/core#definition> """-- Definition --
Avena sativa L. (including A. byzantina K. Koch) Oat and Red oat.
-- Description --
List of agricultural species -A   
IV. Cereals
NOTE. Initial value: A - 73."""@en ;
                                                                                                                                          <http://www.w3.org/2004/02/skos/core#inScheme> :SpecieCodeValue .


###  http://lpis.ec.europa.eu/registry/applicationschema/cap-iacs-base/code#SpecieCodeValue/avenaStrigosaSchrebLBlackOatBristle
<http://lpis.ec.europa.eu/registry/applicationschema/cap-iacs-base/code#SpecieCodeValue/avenaStrigosaSchrebLBlackOatBristle> rdf:type owl:NamedIndividual ,
                                                                                                                                      <http://lpis.ec.europa.eu/registry/applicationschema/cap-iacs-base#SpecieCodeValue> ;
                                                                                                                             rdfs:label "Avena strigosa Schreb. L. Black oat / Bristle"@en ;
                                                                                                                             <http://www.w3.org/2004/02/skos/core#definition> """-- Definition --
Avena strigosa Schreb. L. Black oat / Bristle.
-- Description --
List of agricultural species -A   
IV. Cereals
NOTE. Initial value: A - 74."""@en ;
                                                                                                                             <http://www.w3.org/2004/02/skos/core#inScheme> :SpecieCodeValue .


###  http://lpis.ec.europa.eu/registry/applicationschema/cap-iacs-base/code#SpecieCodeValue/betaVulgarisLBeetrootIncludingCheltenhamBeet
<http://lpis.ec.europa.eu/registry/applicationschema/cap-iacs-base/code#SpecieCodeValue/betaVulgarisLBeetrootIncludingCheltenhamBeet> rdf:type owl:NamedIndividual ,
                                                                                                                                               <http://lpis.ec.europa.eu/registry/applicationschema/cap-iacs-base#SpecieCodeValue> ;
                                                                                                                                      rdfs:label "Beta vulgaris L. Beetroot, including Cheltenham beet"@en ;
                                                                                                                                      <http://www.w3.org/2004/02/skos/core#definition> """-- Definition --
Beta vulgaris L. Beetroot, including Cheltenham beet.
-- Description --
List of vegetable specie -H
NOTE. Initial value: H - 9.1"""@en ;
                                                                                                                                      <http://www.w3.org/2004/02/skos/core#inScheme> :SpecieCodeValue .


###  http://lpis.ec.europa.eu/registry/applicationschema/cap-iacs-base/code#SpecieCodeValue/betaVulgarisLFodderBeet
<http://lpis.ec.europa.eu/registry/applicationschema/cap-iacs-base/code#SpecieCodeValue/betaVulgarisLFodderBeet> rdf:type owl:NamedIndividual ,
                                                                                                                          <http://lpis.ec.europa.eu/registry/applicationschema/cap-iacs-base#SpecieCodeValue> ;
                                                                                                                 rdfs:label "Beta vulgaris L. Fodder beet "@en ;
                                                                                                                 <http://www.w3.org/2004/02/skos/core#definition> """-- Definition --
Beta vulgaris L. Fodder beet.
-- Description --
List of agricultural species -A
I. Beet
NOTE. Initial value: A - 2."""@en ;
                                                                                                                 <http://www.w3.org/2004/02/skos/core#inScheme> :SpecieCodeValue .


###  http://lpis.ec.europa.eu/registry/applicationschema/cap-iacs-base/code#SpecieCodeValue/betaVulgarisLSpinachBeetOrChard
<http://lpis.ec.europa.eu/registry/applicationschema/cap-iacs-base/code#SpecieCodeValue/betaVulgarisLSpinachBeetOrChard> rdf:type owl:NamedIndividual ,
                                                                                                                                  <http://lpis.ec.europa.eu/registry/applicationschema/cap-iacs-base#SpecieCodeValue> ;
                                                                                                                         rdfs:label "Beta vulgaris L. Spinach beet or Chard"@en ;
                                                                                                                         <http://www.w3.org/2004/02/skos/core#definition> """-- Definition --
Beta vulgaris L. Spinach beet or Chard.
-- Description --
List of vegetable specie -H
NOTE. Initial value: H - 9.2"""@en ;
                                                                                                                         <http://www.w3.org/2004/02/skos/core#inScheme> :SpecieCodeValue .


###  http://lpis.ec.europa.eu/registry/applicationschema/cap-iacs-base/code#SpecieCodeValue/betaVulgarisLSugarBeet
<http://lpis.ec.europa.eu/registry/applicationschema/cap-iacs-base/code#SpecieCodeValue/betaVulgarisLSugarBeet> rdf:type owl:NamedIndividual ,
                                                                                                                         <http://lpis.ec.europa.eu/registry/applicationschema/cap-iacs-base#SpecieCodeValue> ;
                                                                                                                rdfs:label "Beta vulgaris L. Sugar beet"@en ;
                                                                                                                <http://www.w3.org/2004/02/skos/core#definition> """-- Definition --
Beta vulgaris L. Sugar beet.
-- Description --
List of agricultural species -A
I. Beet
NOTE. Initial value: A - 1."""@en ;
                                                                                                                <http://www.w3.org/2004/02/skos/core#inScheme> :SpecieCodeValue .


###  http://lpis.ec.europa.eu/registry/applicationschema/cap-iacs-base/code#SpecieCodeValue/brassicaJunceaLBrownMustard
<http://lpis.ec.europa.eu/registry/applicationschema/cap-iacs-base/code#SpecieCodeValue/brassicaJunceaLBrownMustard> rdf:type owl:NamedIndividual ,
                                                                                                                              <http://lpis.ec.europa.eu/registry/applicationschema/cap-iacs-base#SpecieCodeValue> ;
                                                                                                                     rdfs:label "Brassica juncea L. Brown mustard "@en ;
                                                                                                                     <http://www.w3.org/2004/02/skos/core#definition> """-- Definition --
Brassica juncea L. Brown mustard.
-- Description --
List of agricultural species -A
III. Oil and fibre plants
NOTE. Initial value: A - 60."""@en ;
                                                                                                                     <http://www.w3.org/2004/02/skos/core#inScheme> :SpecieCodeValue .


###  http://lpis.ec.europa.eu/registry/applicationschema/cap-iacs-base/code#SpecieCodeValue/brassicaNapusLPartimSwedeRape
<http://lpis.ec.europa.eu/registry/applicationschema/cap-iacs-base/code#SpecieCodeValue/brassicaNapusLPartimSwedeRape> rdf:type owl:NamedIndividual ,
                                                                                                                                <http://lpis.ec.europa.eu/registry/applicationschema/cap-iacs-base#SpecieCodeValue> ;
                                                                                                                       rdfs:label "Brassica napus L. (partim) Swede rape "@en ;
                                                                                                                       <http://www.w3.org/2004/02/skos/core#definition> """-- Definition --
Brassica napus L. (partim) Swede rape.
-- Description --
List of agricultural species -A
III. Oil and fibre plants
NOTE. Initial value: A - 61."""@en ;
                                                                                                                       <http://www.w3.org/2004/02/skos/core#inScheme> :SpecieCodeValue .


###  http://lpis.ec.europa.eu/registry/applicationschema/cap-iacs-base/code#SpecieCodeValue/brassicaNapusLSwede
<http://lpis.ec.europa.eu/registry/applicationschema/cap-iacs-base/code#SpecieCodeValue/brassicaNapusLSwede> rdf:type owl:NamedIndividual ,
                                                                                                                      <http://lpis.ec.europa.eu/registry/applicationschema/cap-iacs-base#SpecieCodeValue> ;
                                                                                                             rdfs:label "Brassica napus L. Swede "@en ;
                                                                                                             <http://www.w3.org/2004/02/skos/core#definition> """-- Definition --
Brassica napus L. Swede.
-- Description --
List of agricultural species -A
II. Fodder plants
NOTE. Initial value: A - 54."""@en ;
                                                                                                             <http://www.w3.org/2004/02/skos/core#inScheme> :SpecieCodeValue .


###  http://lpis.ec.europa.eu/registry/applicationschema/cap-iacs-base/code#SpecieCodeValue/brassicaNigraLBlackMustard
<http://lpis.ec.europa.eu/registry/applicationschema/cap-iacs-base/code#SpecieCodeValue/brassicaNigraLBlackMustard> rdf:type owl:NamedIndividual ,
                                                                                                                             <http://lpis.ec.europa.eu/registry/applicationschema/cap-iacs-base#SpecieCodeValue> ;
                                                                                                                    rdfs:label "Brassica nigra L. Black mustard "@en ;
                                                                                                                    <http://www.w3.org/2004/02/skos/core#definition> """-- Definition --
Brassica nigra L. Black mustard.
-- Description --
List of agricultural species -A
III. Oil and fibre plants
NOTE. Initial value: A - 62."""@en ;
                                                                                                                    <http://www.w3.org/2004/02/skos/core#inScheme> :SpecieCodeValue .


###  http://lpis.ec.europa.eu/registry/applicationschema/cap-iacs-base/code#SpecieCodeValue/brassicaOleraceaLBrusselsSprouts
<http://lpis.ec.europa.eu/registry/applicationschema/cap-iacs-base/code#SpecieCodeValue/brassicaOleraceaLBrusselsSprouts> rdf:type owl:NamedIndividual ,
                                                                                                                                   <http://lpis.ec.europa.eu/registry/applicationschema/cap-iacs-base#SpecieCodeValue> ;
                                                                                                                          rdfs:label "Brassica oleracea L. Brussels sprouts"@en ;
                                                                                                                          <http://www.w3.org/2004/02/skos/core#definition> """-- Definition --
Brassica oleracea L. Brussels sprouts.
-- Description --
List of vegetable specie -H
NOTE. Initial value: H - 10.4"""@en ;
                                                                                                                          <http://www.w3.org/2004/02/skos/core#inScheme> :SpecieCodeValue .


###  http://lpis.ec.europa.eu/registry/applicationschema/cap-iacs-base/code#SpecieCodeValue/brassicaOleraceaLCauliflower
<http://lpis.ec.europa.eu/registry/applicationschema/cap-iacs-base/code#SpecieCodeValue/brassicaOleraceaLCauliflower> rdf:type owl:NamedIndividual ,
                                                                                                                               <http://lpis.ec.europa.eu/registry/applicationschema/cap-iacs-base#SpecieCodeValue> ;
                                                                                                                      rdfs:label "Brassica oleracea L. Cauliflower"@en ;
                                                                                                                      <http://www.w3.org/2004/02/skos/core#definition> """-- Definition --
Brassica oleracea L. Cauliflower.
-- Description --
List of vegetable specie -H
NOTE. Initial value: H - 10.2"""@en ;
                                                                                                                      <http://www.w3.org/2004/02/skos/core#inScheme> :SpecieCodeValue .


###  http://lpis.ec.europa.eu/registry/applicationschema/cap-iacs-base/code#SpecieCodeValue/brassicaOleraceaLCurlyKale
<http://lpis.ec.europa.eu/registry/applicationschema/cap-iacs-base/code#SpecieCodeValue/brassicaOleraceaLCurlyKale> rdf:type owl:NamedIndividual ,
                                                                                                                             <http://lpis.ec.europa.eu/registry/applicationschema/cap-iacs-base#SpecieCodeValue> ;
                                                                                                                    rdfs:label "Brassica oleracea L. Curly kale"@en ;
                                                                                                                    <http://www.w3.org/2004/02/skos/core#definition> """-- Definition --
Brassica oleracea L. Curly kale.
-- Description --
List of vegetable specie -H
NOTE. Initial value: H - 10.1"""@en ;
                                                                                                                    <http://www.w3.org/2004/02/skos/core#inScheme> :SpecieCodeValue .


###  http://lpis.ec.europa.eu/registry/applicationschema/cap-iacs-base/code#SpecieCodeValue/brassicaOleraceaLFodderKale
<http://lpis.ec.europa.eu/registry/applicationschema/cap-iacs-base/code#SpecieCodeValue/brassicaOleraceaLFodderKale> rdf:type owl:NamedIndividual ,
                                                                                                                              <http://lpis.ec.europa.eu/registry/applicationschema/cap-iacs-base#SpecieCodeValue> ;
                                                                                                                     rdfs:label "Brassica oleracea L. Fodder kale "@en ;
                                                                                                                     <http://www.w3.org/2004/02/skos/core#definition> """-- Definition --
Brassica oleracea L. Fodder kale.
-- Description --
List of agricultural species -A
II. Fodder plants
NOTE. Initial value: A - 55."""@en ;
                                                                                                                     <http://www.w3.org/2004/02/skos/core#inScheme> :SpecieCodeValue .


###  http://lpis.ec.europa.eu/registry/applicationschema/cap-iacs-base/code#SpecieCodeValue/brassicaOleraceaLKohlrabi
<http://lpis.ec.europa.eu/registry/applicationschema/cap-iacs-base/code#SpecieCodeValue/brassicaOleraceaLKohlrabi> rdf:type owl:NamedIndividual ,
                                                                                                                            <http://lpis.ec.europa.eu/registry/applicationschema/cap-iacs-base#SpecieCodeValue> ;
                                                                                                                   rdfs:label "Brassica oleracea L. Kohlrabi "@en ;
                                                                                                                   <http://www.w3.org/2004/02/skos/core#definition> """-- Definition --
Brassica oleracea L. Kohlrabi.
-- Description --
List of vegetable specie -H
NOTE. Initial value: H - 10.8"""@en ;
                                                                                                                   <http://www.w3.org/2004/02/skos/core#inScheme> :SpecieCodeValue .


###  http://lpis.ec.europa.eu/registry/applicationschema/cap-iacs-base/code#SpecieCodeValue/brassicaOleraceaLRedCabbage
<http://lpis.ec.europa.eu/registry/applicationschema/cap-iacs-base/code#SpecieCodeValue/brassicaOleraceaLRedCabbage> rdf:type owl:NamedIndividual ,
                                                                                                                              <http://lpis.ec.europa.eu/registry/applicationschema/cap-iacs-base#SpecieCodeValue> ;
                                                                                                                     rdfs:label "Brassica oleracea L. Red cabbage"@en ;
                                                                                                                     <http://www.w3.org/2004/02/skos/core#definition> """-- Definition --
Brassica oleracea L. Red cabbage.
-- Description --
List of vegetable specie -H
NOTE. Initial value: H - 10.7"""@en ;
                                                                                                                     <http://www.w3.org/2004/02/skos/core#inScheme> :SpecieCodeValue .


###  http://lpis.ec.europa.eu/registry/applicationschema/cap-iacs-base/code#SpecieCodeValue/brassicaOleraceaLSavoyCabbage
<http://lpis.ec.europa.eu/registry/applicationschema/cap-iacs-base/code#SpecieCodeValue/brassicaOleraceaLSavoyCabbage> rdf:type owl:NamedIndividual ,
                                                                                                                                <http://lpis.ec.europa.eu/registry/applicationschema/cap-iacs-base#SpecieCodeValue> ;
                                                                                                                       rdfs:label "Brassica oleracea L. Savoy cabbage"@en ;
                                                                                                                       <http://www.w3.org/2004/02/skos/core#definition> """-- Definition --
Brassica oleracea L. Savoy cabbage.
-- Description --
List of vegetable specie -H
NOTE. Initial value: H - 10.5"""@en ;
                                                                                                                       <http://www.w3.org/2004/02/skos/core#inScheme> :SpecieCodeValue .


###  http://lpis.ec.europa.eu/registry/applicationschema/cap-iacs-base/code#SpecieCodeValue/brassicaOleraceaLSproutingBroccoliCalabrese
<http://lpis.ec.europa.eu/registry/applicationschema/cap-iacs-base/code#SpecieCodeValue/brassicaOleraceaLSproutingBroccoliCalabrese> rdf:type owl:NamedIndividual ,
                                                                                                                                              <http://lpis.ec.europa.eu/registry/applicationschema/cap-iacs-base#SpecieCodeValue> ;
                                                                                                                                     rdfs:label "Brassica oleracea L. Sprouting broccoli / Calabrese"@en ;
                                                                                                                                     <http://www.w3.org/2004/02/skos/core#definition> """-- Definition --
Brassica oleracea L. Sprouting broccoli / Calabrese.
-- Description --
List of vegetable specie -H
NOTE. Initial value: H - 10.3"""@en ;
                                                                                                                                     <http://www.w3.org/2004/02/skos/core#inScheme> :SpecieCodeValue .


###  http://lpis.ec.europa.eu/registry/applicationschema/cap-iacs-base/code#SpecieCodeValue/brassicaOleraceaLWhiteCabbage
<http://lpis.ec.europa.eu/registry/applicationschema/cap-iacs-base/code#SpecieCodeValue/brassicaOleraceaLWhiteCabbage> rdf:type owl:NamedIndividual ,
                                                                                                                                <http://lpis.ec.europa.eu/registry/applicationschema/cap-iacs-base#SpecieCodeValue> ;
                                                                                                                       rdfs:label "Brassica oleracea L. White cabbage"@en ;
                                                                                                                       <http://www.w3.org/2004/02/skos/core#definition> """-- Definition --
Brassica oleracea L. White cabbage.
-- Description --
List of vegetable specie -H
NOTE. Initial value: H - 10.6"""@en ;
                                                                                                                       <http://www.w3.org/2004/02/skos/core#inScheme> :SpecieCodeValue .


###  http://lpis.ec.europa.eu/registry/applicationschema/cap-iacs-base/code#SpecieCodeValue/brassicaRapaLChineseCabbage
<http://lpis.ec.europa.eu/registry/applicationschema/cap-iacs-base/code#SpecieCodeValue/brassicaRapaLChineseCabbage> rdf:type owl:NamedIndividual ,
                                                                                                                              <http://lpis.ec.europa.eu/registry/applicationschema/cap-iacs-base#SpecieCodeValue> ;
                                                                                                                     rdfs:label "Brassica rapa L. Chinese cabbage"@en ;
                                                                                                                     <http://www.w3.org/2004/02/skos/core#definition> """-- Definition --
Brassica rapa L. Chinese cabbage.
-- Description --
List of vegetable specie -H
NOTE. Initial value: H - 11.1"""@en ;
                                                                                                                     <http://www.w3.org/2004/02/skos/core#inScheme> :SpecieCodeValue .


###  http://lpis.ec.europa.eu/registry/applicationschema/cap-iacs-base/code#SpecieCodeValue/brassicaRapaLTurnip
<http://lpis.ec.europa.eu/registry/applicationschema/cap-iacs-base/code#SpecieCodeValue/brassicaRapaLTurnip> rdf:type owl:NamedIndividual ,
                                                                                                                      <http://lpis.ec.europa.eu/registry/applicationschema/cap-iacs-base#SpecieCodeValue> ;
                                                                                                             rdfs:label "Brassica rapa L. Turnip"@en ;
                                                                                                             <http://www.w3.org/2004/02/skos/core#definition> """-- Definition --
Brassica rapa L. Turnip.
-- Description --
List of vegetable specie -H
NOTE. Initial value: H - 11.2"""@en ;
                                                                                                             <http://www.w3.org/2004/02/skos/core#inScheme> :SpecieCodeValue .


###  http://lpis.ec.europa.eu/registry/applicationschema/cap-iacs-base/code#SpecieCodeValue/brassicaRapaLVarSilvestrisLamBriggsTurnipRape
<http://lpis.ec.europa.eu/registry/applicationschema/cap-iacs-base/code#SpecieCodeValue/brassicaRapaLVarSilvestrisLamBriggsTurnipRape> rdf:type owl:NamedIndividual ,
                                                                                                                                                <http://lpis.ec.europa.eu/registry/applicationschema/cap-iacs-base#SpecieCodeValue> ;
                                                                                                                                       rdfs:label "Brassica rapa L. var. silvestris (Lam.) Briggs Turnip rape "@en ;
                                                                                                                                       <http://www.w3.org/2004/02/skos/core#definition> """-- Definition --
Brassica rapa L. var. silvestris (Lam.) Briggs Turnip rape.
-- Description --
List of agricultural species -A
III. Oil and fibre plants
NOTE. Initial value: A - 59."""@en ;
                                                                                                                                       <http://www.w3.org/2004/02/skos/core#inScheme> :SpecieCodeValue .


###  http://lpis.ec.europa.eu/registry/applicationschema/cap-iacs-base/code#SpecieCodeValue/bromusCatharticusLRescueGrass
<http://lpis.ec.europa.eu/registry/applicationschema/cap-iacs-base/code#SpecieCodeValue/bromusCatharticusLRescueGrass> rdf:type owl:NamedIndividual ,
                                                                                                                                <http://lpis.ec.europa.eu/registry/applicationschema/cap-iacs-base#SpecieCodeValue> ;
                                                                                                                       rdfs:label "Bromus catharticus L. Rescue grass"@en ;
                                                                                                                       <http://www.w3.org/2004/02/skos/core#definition> """-- Definition --
Bromus catharticus L. Rescue grass.
-- Description --
List of agricultural species -A
II. Fodder plants
NOTE. Initial value: A - 9."""@en ;
                                                                                                                       <http://www.w3.org/2004/02/skos/core#inScheme> :SpecieCodeValue .


###  http://lpis.ec.europa.eu/registry/applicationschema/cap-iacs-base/code#SpecieCodeValue/bromusSitchensisLAlaskaBromeGrass
<http://lpis.ec.europa.eu/registry/applicationschema/cap-iacs-base/code#SpecieCodeValue/bromusSitchensisLAlaskaBromeGrass> rdf:type owl:NamedIndividual ,
                                                                                                                                    <http://lpis.ec.europa.eu/registry/applicationschema/cap-iacs-base#SpecieCodeValue> ;
                                                                                                                           rdfs:label "Bromus sitchensis L. Alaska brome-grass"@en ;
                                                                                                                           <http://www.w3.org/2004/02/skos/core#definition> """-- Definition --
Bromus sitchensis L. Alaska brome-grass.
-- Description --
List of agricultural species -A
II. Fodder plants
NOTE. Initial value: A - 10."""@en ;
                                                                                                                           <http://www.w3.org/2004/02/skos/core#inScheme> :SpecieCodeValue .


###  http://lpis.ec.europa.eu/registry/applicationschema/cap-iacs-base/code#SpecieCodeValue/cannabisSativaLHemp
<http://lpis.ec.europa.eu/registry/applicationschema/cap-iacs-base/code#SpecieCodeValue/cannabisSativaLHemp> rdf:type owl:NamedIndividual ,
                                                                                                                      <http://lpis.ec.europa.eu/registry/applicationschema/cap-iacs-base#SpecieCodeValue> ;
                                                                                                             rdfs:label "Cannabis sativa L. Hemp "@en ;
                                                                                                             <http://www.w3.org/2004/02/skos/core#definition> """-- Definition --
Cannabis sativa L. Hemp.
-- Description --
List of agricultural species -A
III. Oil and fibre plants
NOTE. Initial value: A - 63."""@en ;
                                                                                                             <http://www.w3.org/2004/02/skos/core#inScheme> :SpecieCodeValue .


###  http://lpis.ec.europa.eu/registry/applicationschema/cap-iacs-base/code#SpecieCodeValue/capsicumAnnuumLChiliPepper
<http://lpis.ec.europa.eu/registry/applicationschema/cap-iacs-base/code#SpecieCodeValue/capsicumAnnuumLChiliPepper> rdf:type owl:NamedIndividual ,
                                                                                                                             <http://lpis.ec.europa.eu/registry/applicationschema/cap-iacs-base#SpecieCodeValue> ;
                                                                                                                    rdfs:label "Capsicum annuum L. Chili, Pepper "@en ;
                                                                                                                    <http://www.w3.org/2004/02/skos/core#definition> """-- Definition --
Capsicum annuum L. Chili, Pepper.
-- Description --
List of vegetable specie -H
NOTE. Initial value: H - 12."""@en ;
                                                                                                                    <http://www.w3.org/2004/02/skos/core#inScheme> :SpecieCodeValue .


###  http://lpis.ec.europa.eu/registry/applicationschema/cap-iacs-base/code#SpecieCodeValue/carthamusTinctoriusLSafflower
<http://lpis.ec.europa.eu/registry/applicationschema/cap-iacs-base/code#SpecieCodeValue/carthamusTinctoriusLSafflower> rdf:type owl:NamedIndividual ,
                                                                                                                                <http://lpis.ec.europa.eu/registry/applicationschema/cap-iacs-base#SpecieCodeValue> ;
                                                                                                                       rdfs:label "Carthamus tinctorius L. Safflower"@en ;
                                                                                                                       <http://www.w3.org/2004/02/skos/core#definition> """-- Definition --
Carthamus tinctorius L. Safflower.
-- Description --
List of agricultural species -A
III. Oil and fibre plants
NOTE. Initial value: A - 64."""@en ;
                                                                                                                       <http://www.w3.org/2004/02/skos/core#inScheme> :SpecieCodeValue .


###  http://lpis.ec.europa.eu/registry/applicationschema/cap-iacs-base/code#SpecieCodeValue/carumCarviLCaraway
<http://lpis.ec.europa.eu/registry/applicationschema/cap-iacs-base/code#SpecieCodeValue/carumCarviLCaraway> rdf:type owl:NamedIndividual ,
                                                                                                                     <http://lpis.ec.europa.eu/registry/applicationschema/cap-iacs-base#SpecieCodeValue> ;
                                                                                                            rdfs:label "Carum carvi L. Caraway"@en ;
                                                                                                            <http://www.w3.org/2004/02/skos/core#definition> """-- Definition --
Carum carvi L. Caraway.
-- Description --
List of agricultural species -A
III. Oil and fibre plants
NOTE. Initial value: A - 65."""@en ;
                                                                                                            <http://www.w3.org/2004/02/skos/core#inScheme> :SpecieCodeValue .


###  http://lpis.ec.europa.eu/registry/applicationschema/cap-iacs-base/code#SpecieCodeValue/cichoriumEndiviaLCurledLeavedEndive
<http://lpis.ec.europa.eu/registry/applicationschema/cap-iacs-base/code#SpecieCodeValue/cichoriumEndiviaLCurledLeavedEndive> rdf:type owl:NamedIndividual ,
                                                                                                                                      <http://lpis.ec.europa.eu/registry/applicationschema/cap-iacs-base#SpecieCodeValue> ;
                                                                                                                             rdfs:label "Cichorium endivia L. Curled-leaved endive"@en ;
                                                                                                                             <http://www.w3.org/2004/02/skos/core#definition> """-- Definition --
Cichorium endivia L. Curled-leaved endive.
-- Description --
List of vegetable specie -H
NOTE. Initial value: H - 13.1"""@en ;
                                                                                                                             <http://www.w3.org/2004/02/skos/core#inScheme> :SpecieCodeValue .


###  http://lpis.ec.europa.eu/registry/applicationschema/cap-iacs-base/code#SpecieCodeValue/cichoriumEndiviaLPlainLeavedEndive
<http://lpis.ec.europa.eu/registry/applicationschema/cap-iacs-base/code#SpecieCodeValue/cichoriumEndiviaLPlainLeavedEndive> rdf:type owl:NamedIndividual ,
                                                                                                                                     <http://lpis.ec.europa.eu/registry/applicationschema/cap-iacs-base#SpecieCodeValue> ;
                                                                                                                            rdfs:label "Cichorium endivia L. Plain-leaved endive"@en ;
                                                                                                                            <http://www.w3.org/2004/02/skos/core#definition> """-- Definition --
Cichorium endivia L. Plain-leaved endive.
-- Description --
List of vegetable specie -H
NOTE. Initial value: H - 13.2"""@en ;
                                                                                                                            <http://www.w3.org/2004/02/skos/core#inScheme> :SpecieCodeValue .


###  http://lpis.ec.europa.eu/registry/applicationschema/cap-iacs-base/code#SpecieCodeValue/cichoriumIntybusLIndustrialChicory
<http://lpis.ec.europa.eu/registry/applicationschema/cap-iacs-base/code#SpecieCodeValue/cichoriumIntybusLIndustrialChicory> rdf:type owl:NamedIndividual ,
                                                                                                                                     <http://lpis.ec.europa.eu/registry/applicationschema/cap-iacs-base#SpecieCodeValue> ;
                                                                                                                            rdfs:label "Cichorium intybus L. Industrial chicory"@en ;
                                                                                                                            <http://www.w3.org/2004/02/skos/core#definition> """-- Definition --
Cichorium intybus L. Industrial chicory.
-- Description --
List of vegetable specie -H
NOTE. Initial value: H - 14.3"""@en ;
                                                                                                                            <http://www.w3.org/2004/02/skos/core#inScheme> :SpecieCodeValue .


###  http://lpis.ec.europa.eu/registry/applicationschema/cap-iacs-base/code#SpecieCodeValue/cichoriumIntybusLLargeLeavedChicoryItalianChicory
<http://lpis.ec.europa.eu/registry/applicationschema/cap-iacs-base/code#SpecieCodeValue/cichoriumIntybusLLargeLeavedChicoryItalianChicory> rdf:type owl:NamedIndividual ,
                                                                                                                                                    <http://lpis.ec.europa.eu/registry/applicationschema/cap-iacs-base#SpecieCodeValue> ;
                                                                                                                                           rdfs:label "Cichorium intybus L. Large-leaved chicory / Italian chicory"@en ;
                                                                                                                                           <http://www.w3.org/2004/02/skos/core#definition> """-- Definition --
Cichorium intybus L. Large-leaved chicory / Italian chicory.
-- Description --
List of vegetable specie -H
NOTE. Initial value: H - 14.2"""@en ;
                                                                                                                                           <http://www.w3.org/2004/02/skos/core#inScheme> :SpecieCodeValue .


###  http://lpis.ec.europa.eu/registry/applicationschema/cap-iacs-base/code#SpecieCodeValue/cichoriumIntybusLWitloofChicory
<http://lpis.ec.europa.eu/registry/applicationschema/cap-iacs-base/code#SpecieCodeValue/cichoriumIntybusLWitloofChicory> rdf:type owl:NamedIndividual ,
                                                                                                                                  <http://lpis.ec.europa.eu/registry/applicationschema/cap-iacs-base#SpecieCodeValue> ;
                                                                                                                         rdfs:label "Cichorium intybus L. Witloof chicory"@en ;
                                                                                                                         <http://www.w3.org/2004/02/skos/core#definition> """-- Definition --
Cichorium intybus L. Witloof chicory.
-- Description --
List of vegetable specie -H
NOTE. Initial value: H - 14.1"""@en ;
                                                                                                                         <http://www.w3.org/2004/02/skos/core#inScheme> :SpecieCodeValue .


###  http://lpis.ec.europa.eu/registry/applicationschema/cap-iacs-base/code#SpecieCodeValue/citrullusLanatusThunbMatsumEtNakaiWatermelon
<http://lpis.ec.europa.eu/registry/applicationschema/cap-iacs-base/code#SpecieCodeValue/citrullusLanatusThunbMatsumEtNakaiWatermelon> rdf:type owl:NamedIndividual ,
                                                                                                                                               <http://lpis.ec.europa.eu/registry/applicationschema/cap-iacs-base#SpecieCodeValue> ;
                                                                                                                                      rdfs:label "Citrullus lanatus (Thunb.) Matsum. et Nakai Watermelon"@en ;
                                                                                                                                      <http://www.w3.org/2004/02/skos/core#definition> """-- Definition --
Citrullus lanatus (Thunb.) Matsum. et Nakai Watermelon.
-- Description --
List of vegetable specie -H
NOTE. Initial value: H - 15."""@en ;
                                                                                                                                      <http://www.w3.org/2004/02/skos/core#inScheme> :SpecieCodeValue .


###  http://lpis.ec.europa.eu/registry/applicationschema/cap-iacs-base/code#SpecieCodeValue/cucumisMeloLMelon
<http://lpis.ec.europa.eu/registry/applicationschema/cap-iacs-base/code#SpecieCodeValue/cucumisMeloLMelon> rdf:type owl:NamedIndividual ,
                                                                                                                    <http://lpis.ec.europa.eu/registry/applicationschema/cap-iacs-base#SpecieCodeValue> ;
                                                                                                           rdfs:label "Cucumis melo L. Melon"@en ;
                                                                                                           <http://www.w3.org/2004/02/skos/core#definition> """-- Definition --
Cucumis melo L. Melon.
-- Description --
List of vegetable specie -H
NOTE. Initial value: H - 16."""@en ;
                                                                                                           <http://www.w3.org/2004/02/skos/core#inScheme> :SpecieCodeValue .


###  http://lpis.ec.europa.eu/registry/applicationschema/cap-iacs-base/code#SpecieCodeValue/cucumisSativusLCucumber
<http://lpis.ec.europa.eu/registry/applicationschema/cap-iacs-base/code#SpecieCodeValue/cucumisSativusLCucumber> rdf:type owl:NamedIndividual ,
                                                                                                                          <http://lpis.ec.europa.eu/registry/applicationschema/cap-iacs-base#SpecieCodeValue> ;
                                                                                                                 rdfs:label "Cucumis sativus L. Cucumber"@en ;
                                                                                                                 <http://www.w3.org/2004/02/skos/core#definition> """-- Definition --
Cucumis sativus L. Cucumber.
-- Description --
List of vegetable specie -H
NOTE. Initial value: H - 17.1"""@en ;
                                                                                                                 <http://www.w3.org/2004/02/skos/core#inScheme> :SpecieCodeValue .


###  http://lpis.ec.europa.eu/registry/applicationschema/cap-iacs-base/code#SpecieCodeValue/cucumisSativusLGherkin
<http://lpis.ec.europa.eu/registry/applicationschema/cap-iacs-base/code#SpecieCodeValue/cucumisSativusLGherkin> rdf:type owl:NamedIndividual ,
                                                                                                                         <http://lpis.ec.europa.eu/registry/applicationschema/cap-iacs-base#SpecieCodeValue> ;
                                                                                                                rdfs:label "Cucumis sativus L. Gherkin"@en ;
                                                                                                                <http://www.w3.org/2004/02/skos/core#definition> """-- Definition --
Cucumis sativus L. Gherkin.
-- Description --
List of vegetable specie -H
NOTE. Initial value: H - 17.2"""@en ;
                                                                                                                <http://www.w3.org/2004/02/skos/core#inScheme> :SpecieCodeValue .


###  http://lpis.ec.europa.eu/registry/applicationschema/cap-iacs-base/code#SpecieCodeValue/cucurbitaFicifoliaBouche
<http://lpis.ec.europa.eu/registry/applicationschema/cap-iacs-base/code#SpecieCodeValue/cucurbitaFicifoliaBouche> rdf:type owl:NamedIndividual ,
                                                                                                                           <http://lpis.ec.europa.eu/registry/applicationschema/cap-iacs-base#SpecieCodeValue> ;
                                                                                                                  rdfs:label "Cucurbita ficifolia Bouché"@en ;
                                                                                                                  <http://www.w3.org/2004/02/skos/core#definition> """-- Definition --
Cucurbita ficifolia Bouché.
-- Description --
List of vegetable specie -H
NOTE. Initial value: H - 37.1"""@en ;
                                                                                                                  <http://www.w3.org/2004/02/skos/core#inScheme> :SpecieCodeValue .


###  http://lpis.ec.europa.eu/registry/applicationschema/cap-iacs-base/code#SpecieCodeValue/cucurbitaMaximaDuchesneGourd
<http://lpis.ec.europa.eu/registry/applicationschema/cap-iacs-base/code#SpecieCodeValue/cucurbitaMaximaDuchesneGourd> rdf:type owl:NamedIndividual ,
                                                                                                                               <http://lpis.ec.europa.eu/registry/applicationschema/cap-iacs-base#SpecieCodeValue> ;
                                                                                                                      rdfs:label "Cucurbita Maxima Duchesne Gourd"@en ;
                                                                                                                      <http://www.w3.org/2004/02/skos/core#definition> """-- Definition --
Cucurbita Maxima Duchesne Gourd.
-- Description --
List of vegetable specie -H
NOTE. Initial value: H - 18."""@en ;
                                                                                                                      <http://www.w3.org/2004/02/skos/core#inScheme> :SpecieCodeValue .


###  http://lpis.ec.europa.eu/registry/applicationschema/cap-iacs-base/code#SpecieCodeValue/cucurbitaMaximaDuchxCMoschataDuch
<http://lpis.ec.europa.eu/registry/applicationschema/cap-iacs-base/code#SpecieCodeValue/cucurbitaMaximaDuchxCMoschataDuch> rdf:type owl:NamedIndividual ,
                                                                                                                                    <http://lpis.ec.europa.eu/registry/applicationschema/cap-iacs-base#SpecieCodeValue> ;
                                                                                                                           rdfs:label "Cucurbita maxima Duch. x C. moschata Duch."@en ;
                                                                                                                           <http://www.w3.org/2004/02/skos/core#definition> """-- Definition --
Cucurbita maxima Duch. x C. moschata Duch.
-- Description --
List of vegetable specie -H
NOTE. Initial value: H - 37.2"""@en ;
                                                                                                                           <http://www.w3.org/2004/02/skos/core#inScheme> :SpecieCodeValue .


###  http://lpis.ec.europa.eu/registry/applicationschema/cap-iacs-base/code#SpecieCodeValue/cucurbitaMoschata
<http://lpis.ec.europa.eu/registry/applicationschema/cap-iacs-base/code#SpecieCodeValue/cucurbitaMoschata> rdf:type owl:NamedIndividual ,
                                                                                                                    <http://lpis.ec.europa.eu/registry/applicationschema/cap-iacs-base#SpecieCodeValue> ;
                                                                                                           rdfs:label "Cucurbita moschata"@en ;
                                                                                                           <http://www.w3.org/2004/02/skos/core#definition> """-- Definition --
Cucurbita moschata.
-- Description --
List of vegetable specie -H
NOTE. Initial value: H - 37.7"""@en ;
                                                                                                           <http://www.w3.org/2004/02/skos/core#inScheme> :SpecieCodeValue .


###  http://lpis.ec.europa.eu/registry/applicationschema/cap-iacs-base/code#SpecieCodeValue/cucurbitaPepoLMarrowOrCourgette
<http://lpis.ec.europa.eu/registry/applicationschema/cap-iacs-base/code#SpecieCodeValue/cucurbitaPepoLMarrowOrCourgette> rdf:type owl:NamedIndividual ,
                                                                                                                                  <http://lpis.ec.europa.eu/registry/applicationschema/cap-iacs-base#SpecieCodeValue> ;
                                                                                                                         rdfs:label "Cucurbita pepo L. Marrow or Courgette"@en ;
                                                                                                                         <http://www.w3.org/2004/02/skos/core#definition> """-- Definition --
Cucurbita pepo L. Marrow or Courgette.
-- Description --
List of vegetable specie -H
NOTE. Initial value: H - 19."""@en ;
                                                                                                                         <http://www.w3.org/2004/02/skos/core#inScheme> :SpecieCodeValue .


###  http://lpis.ec.europa.eu/registry/applicationschema/cap-iacs-base/code#SpecieCodeValue/cynaraCardunculusLCardoon
<http://lpis.ec.europa.eu/registry/applicationschema/cap-iacs-base/code#SpecieCodeValue/cynaraCardunculusLCardoon> rdf:type owl:NamedIndividual ,
                                                                                                                            <http://lpis.ec.europa.eu/registry/applicationschema/cap-iacs-base#SpecieCodeValue> ;
                                                                                                                   rdfs:label "Cynara cardunculus L. Cardoon"@en ;
                                                                                                                   <http://www.w3.org/2004/02/skos/core#definition> """-- Definition --
Cynara cardunculus L. Cardoon.
-- Description --
List of vegetable specie -H
NOTE. Initial value: H - 20.2"""@en ;
                                                                                                                   <http://www.w3.org/2004/02/skos/core#inScheme> :SpecieCodeValue .


###  http://lpis.ec.europa.eu/registry/applicationschema/cap-iacs-base/code#SpecieCodeValue/cynaraCardunculusLGlobeArtichoke
<http://lpis.ec.europa.eu/registry/applicationschema/cap-iacs-base/code#SpecieCodeValue/cynaraCardunculusLGlobeArtichoke> rdf:type owl:NamedIndividual ,
                                                                                                                                   <http://lpis.ec.europa.eu/registry/applicationschema/cap-iacs-base#SpecieCodeValue> ;
                                                                                                                          rdfs:label "Cynara cardunculus L. Globe artichoke"@en ;
                                                                                                                          <http://www.w3.org/2004/02/skos/core#definition> """-- Definition --
Cynara cardunculus L. Globe artichoke.
-- Description --
List of vegetable specie -H
NOTE. Initial value: H - 20.1"""@en ;
                                                                                                                          <http://www.w3.org/2004/02/skos/core#inScheme> :SpecieCodeValue .


###  http://lpis.ec.europa.eu/registry/applicationschema/cap-iacs-base/code#SpecieCodeValue/cynodonDactylonLBermudaGrass
<http://lpis.ec.europa.eu/registry/applicationschema/cap-iacs-base/code#SpecieCodeValue/cynodonDactylonLBermudaGrass> rdf:type owl:NamedIndividual ,
                                                                                                                               <http://lpis.ec.europa.eu/registry/applicationschema/cap-iacs-base#SpecieCodeValue> ;
                                                                                                                      rdfs:label "Cynodon dactylon L. Bermuda grass"@en ;
                                                                                                                      <http://www.w3.org/2004/02/skos/core#definition> """-- Definition --
Cynodon dactylon L. Bermuda grass.
-- Description --
List of agricultural species -A
II. Fodder plants
NOTE. Initial value: A - 11."""@en ;
                                                                                                                      <http://www.w3.org/2004/02/skos/core#inScheme> :SpecieCodeValue .


###  http://lpis.ec.europa.eu/registry/applicationschema/cap-iacs-base/code#SpecieCodeValue/dactylisGlomerataLCocksfoot
<http://lpis.ec.europa.eu/registry/applicationschema/cap-iacs-base/code#SpecieCodeValue/dactylisGlomerataLCocksfoot> rdf:type owl:NamedIndividual ,
                                                                                                                              <http://lpis.ec.europa.eu/registry/applicationschema/cap-iacs-base#SpecieCodeValue> ;
                                                                                                                     rdfs:label "Dactylis glomerata L. Cocksfoot "@en ;
                                                                                                                     <http://www.w3.org/2004/02/skos/core#definition> """-- Definition --
Dactylis glomerata L. Cocksfoot.
-- Description --
List of agricultural species -A
II. Fodder plants
NOTE. Initial value: A - 12."""@en ;
                                                                                                                     <http://www.w3.org/2004/02/skos/core#inScheme> :SpecieCodeValue .


###  http://lpis.ec.europa.eu/registry/applicationschema/cap-iacs-base/code#SpecieCodeValue/daucusCarotaLCarrot
<http://lpis.ec.europa.eu/registry/applicationschema/cap-iacs-base/code#SpecieCodeValue/daucusCarotaLCarrot> rdf:type owl:NamedIndividual ,
                                                                                                                      <http://lpis.ec.europa.eu/registry/applicationschema/cap-iacs-base#SpecieCodeValue> ;
                                                                                                             rdfs:label "Daucus carota L. Carrot"@en ;
                                                                                                             <http://www.w3.org/2004/02/skos/core#definition> """-- Definition --
Daucus carota L. Carrot.
-- Description --
List of vegetable specie -H
NOTE. Initial value: H - 21.1"""@en ;
                                                                                                             <http://www.w3.org/2004/02/skos/core#inScheme> :SpecieCodeValue .


###  http://lpis.ec.europa.eu/registry/applicationschema/cap-iacs-base/code#SpecieCodeValue/daucusCarotaLFodderCarrot
<http://lpis.ec.europa.eu/registry/applicationschema/cap-iacs-base/code#SpecieCodeValue/daucusCarotaLFodderCarrot> rdf:type owl:NamedIndividual ,
                                                                                                                            <http://lpis.ec.europa.eu/registry/applicationschema/cap-iacs-base#SpecieCodeValue> ;
                                                                                                                   rdfs:label "Daucus carota L. Fodder carrot"@en ;
                                                                                                                   <http://www.w3.org/2004/02/skos/core#definition> """-- Definition --
Daucus carota L. Fodder carrot.
-- Description --
List of vegetable specie -H
NOTE. Initial value: H - 21.2"""@en ;
                                                                                                                   <http://www.w3.org/2004/02/skos/core#inScheme> :SpecieCodeValue .


###  http://lpis.ec.europa.eu/registry/applicationschema/cap-iacs-base/code#SpecieCodeValue/festucaArundinaceaSchreberTallFescue
<http://lpis.ec.europa.eu/registry/applicationschema/cap-iacs-base/code#SpecieCodeValue/festucaArundinaceaSchreberTallFescue> rdf:type owl:NamedIndividual ,
                                                                                                                                       <http://lpis.ec.europa.eu/registry/applicationschema/cap-iacs-base#SpecieCodeValue> ;
                                                                                                                              rdfs:label "Festuca arundinacea Schreber Tall fescue"@en ;
                                                                                                                              <http://www.w3.org/2004/02/skos/core#definition> """-- Definition --
Festuca arundinacea Schreber Tall fescue.
-- Description --
List of agricultural species -A
II. Fodder plants
NOTE. Initial value: A - 13."""@en ;
                                                                                                                              <http://www.w3.org/2004/02/skos/core#inScheme> :SpecieCodeValue .


###  http://lpis.ec.europa.eu/registry/applicationschema/cap-iacs-base/code#SpecieCodeValue/festucaFiliformisLFineLeavedSheeps
<http://lpis.ec.europa.eu/registry/applicationschema/cap-iacs-base/code#SpecieCodeValue/festucaFiliformisLFineLeavedSheeps> rdf:type owl:NamedIndividual ,
                                                                                                                                     <http://lpis.ec.europa.eu/registry/applicationschema/cap-iacs-base#SpecieCodeValue> ;
                                                                                                                            rdfs:label "Festuca filiformis L. Fine leaved sheep's"@en ;
                                                                                                                            <http://www.w3.org/2004/02/skos/core#definition> """-- Definition --
Festuca filiformis L. Fine leaved sheep's.
-- Description --
List of agricultural species -A
II. Fodder plants
NOTE. Initial value: A - 14."""@en ;
                                                                                                                            <http://www.w3.org/2004/02/skos/core#inScheme> :SpecieCodeValue .


###  http://lpis.ec.europa.eu/registry/applicationschema/cap-iacs-base/code#SpecieCodeValue/festucaOvinaLSheepsFescue
<http://lpis.ec.europa.eu/registry/applicationschema/cap-iacs-base/code#SpecieCodeValue/festucaOvinaLSheepsFescue> rdf:type owl:NamedIndividual ,
                                                                                                                            <http://lpis.ec.europa.eu/registry/applicationschema/cap-iacs-base#SpecieCodeValue> ;
                                                                                                                   rdfs:label "Festuca ovina L. Sheep's fescue"@en ;
                                                                                                                   <http://www.w3.org/2004/02/skos/core#definition> """-- Definition --
Festuca ovina L. Sheep's fescue.
-- Description --
List of agricultural species -A
II. Fodder plants
NOTE. Initial value: A - 15."""@en ;
                                                                                                                   <http://www.w3.org/2004/02/skos/core#inScheme> :SpecieCodeValue .


###  http://lpis.ec.europa.eu/registry/applicationschema/cap-iacs-base/code#SpecieCodeValue/festucaPratensisHudsMeadowFescue
<http://lpis.ec.europa.eu/registry/applicationschema/cap-iacs-base/code#SpecieCodeValue/festucaPratensisHudsMeadowFescue> rdf:type owl:NamedIndividual ,
                                                                                                                                   <http://lpis.ec.europa.eu/registry/applicationschema/cap-iacs-base#SpecieCodeValue> ;
                                                                                                                          rdfs:label "Festuca pratensis Huds. Meadow fescue   "@en ;
                                                                                                                          <http://www.w3.org/2004/02/skos/core#definition> """-- Definition --
Festuca pratensis Huds. Meadow fescue.
-- Description --
List of agricultural species -A
II. Fodder plants
NOTE. Initial value: A - 16."""@en ;
                                                                                                                          <http://www.w3.org/2004/02/skos/core#inScheme> :SpecieCodeValue .


###  http://lpis.ec.europa.eu/registry/applicationschema/cap-iacs-base/code#SpecieCodeValue/festucaRubraLRedFescue
<http://lpis.ec.europa.eu/registry/applicationschema/cap-iacs-base/code#SpecieCodeValue/festucaRubraLRedFescue> rdf:type owl:NamedIndividual ,
                                                                                                                         <http://lpis.ec.europa.eu/registry/applicationschema/cap-iacs-base#SpecieCodeValue> ;
                                                                                                                rdfs:label "Festuca rubra L. Red fescue"@en ;
                                                                                                                <http://www.w3.org/2004/02/skos/core#definition> """-- Definition --
Festuca rubra L. Red fescue.
-- Description --
List of agricultural species -A
II. Fodder plants
NOTE. Initial value: A - 17."""@en ;
                                                                                                                <http://www.w3.org/2004/02/skos/core#inScheme> :SpecieCodeValue .


###  http://lpis.ec.europa.eu/registry/applicationschema/cap-iacs-base/code#SpecieCodeValue/festucaTrachyphyllaHackKrajinaHardFescue
<http://lpis.ec.europa.eu/registry/applicationschema/cap-iacs-base/code#SpecieCodeValue/festucaTrachyphyllaHackKrajinaHardFescue> rdf:type owl:NamedIndividual ,
                                                                                                                                           <http://lpis.ec.europa.eu/registry/applicationschema/cap-iacs-base#SpecieCodeValue> ;
                                                                                                                                  rdfs:label "Festuca trachyphylla (Hack.) Krajina Hard fescue "@en ;
                                                                                                                                  <http://www.w3.org/2004/02/skos/core#definition> """-- Definition --
Festuca trachyphylla (Hack.) Krajina Hard fescue.
-- Description --
List of agricultural species -A
II. Fodder plants
NOTE. Initial value: A - 18."""@en ;
                                                                                                                                  <http://www.w3.org/2004/02/skos/core#inScheme> :SpecieCodeValue .


###  http://lpis.ec.europa.eu/registry/applicationschema/cap-iacs-base/code#SpecieCodeValue/foeniculumVulgareMillFennel
<http://lpis.ec.europa.eu/registry/applicationschema/cap-iacs-base/code#SpecieCodeValue/foeniculumVulgareMillFennel> rdf:type owl:NamedIndividual ,
                                                                                                                              <http://lpis.ec.europa.eu/registry/applicationschema/cap-iacs-base#SpecieCodeValue> ;
                                                                                                                     rdfs:label "Foeniculum vulgare Mill. Fennel"@en ;
                                                                                                                     <http://www.w3.org/2004/02/skos/core#definition> """-- Definition --
Foeniculum vulgare Mill. Fennel.
-- Description --
List of vegetable specie -H
NOTE. Initial value: H - 22."""@en ;
                                                                                                                     <http://www.w3.org/2004/02/skos/core#inScheme> :SpecieCodeValue .


###  http://lpis.ec.europa.eu/registry/applicationschema/cap-iacs-base/code#SpecieCodeValue/galegaOrientalisLFodderGalega
<http://lpis.ec.europa.eu/registry/applicationschema/cap-iacs-base/code#SpecieCodeValue/galegaOrientalisLFodderGalega> rdf:type owl:NamedIndividual ,
                                                                                                                                <http://lpis.ec.europa.eu/registry/applicationschema/cap-iacs-base#SpecieCodeValue> ;
                                                                                                                       rdfs:label "Galega orientalis L. Fodder galega"@en ;
                                                                                                                       <http://www.w3.org/2004/02/skos/core#definition> """-- Definition --
Galega orientalis L. Fodder galega
-- Description --
List of agricultural species -A
II. Fodder plants
NOTE. Initial value: A - 32."""@en ;
                                                                                                                       <http://www.w3.org/2004/02/skos/core#inScheme> :SpecieCodeValue .


###  http://lpis.ec.europa.eu/registry/applicationschema/cap-iacs-base/code#SpecieCodeValue/gossypiumSppCotton
<http://lpis.ec.europa.eu/registry/applicationschema/cap-iacs-base/code#SpecieCodeValue/gossypiumSppCotton> rdf:type owl:NamedIndividual ,
                                                                                                                     <http://lpis.ec.europa.eu/registry/applicationschema/cap-iacs-base#SpecieCodeValue> ;
                                                                                                            rdfs:label "Gossypium spp. Cotton "@en ;
                                                                                                            <http://www.w3.org/2004/02/skos/core#definition> """-- Definition --
Gossypium spp. Cotton.
-- Description --
List of agricultural species -A
III. Oil and fibre plants
NOTE. Initial value: A - 66."""@en ;
                                                                                                            <http://www.w3.org/2004/02/skos/core#inScheme> :SpecieCodeValue .


###  http://lpis.ec.europa.eu/registry/applicationschema/cap-iacs-base/code#SpecieCodeValue/hedysarumCoronariumLSulla
<http://lpis.ec.europa.eu/registry/applicationschema/cap-iacs-base/code#SpecieCodeValue/hedysarumCoronariumLSulla> rdf:type owl:NamedIndividual ,
                                                                                                                            <http://lpis.ec.europa.eu/registry/applicationschema/cap-iacs-base#SpecieCodeValue> ;
                                                                                                                   rdfs:label "Hedysarum coronarium L. Sulla "@en ;
                                                                                                                   <http://www.w3.org/2004/02/skos/core#definition> """-- Definition --
Hedysarum coronarium L. Sulla
-- Description --
List of agricultural species -A
II. Fodder plants
NOTE. Initial value: A - 33."""@en ;
                                                                                                                   <http://www.w3.org/2004/02/skos/core#inScheme> :SpecieCodeValue .


###  http://lpis.ec.europa.eu/registry/applicationschema/cap-iacs-base/code#SpecieCodeValue/helianthusAnnuusLSunflower
<http://lpis.ec.europa.eu/registry/applicationschema/cap-iacs-base/code#SpecieCodeValue/helianthusAnnuusLSunflower> rdf:type owl:NamedIndividual ,
                                                                                                                             <http://lpis.ec.europa.eu/registry/applicationschema/cap-iacs-base#SpecieCodeValue> ;
                                                                                                                    rdfs:label "Helianthus annuus L. Sunflower "@en ;
                                                                                                                    <http://www.w3.org/2004/02/skos/core#definition> """-- Definition --
Helianthus annuus L. Sunflower.
-- Description --
List of agricultural species -A
III. Oil and fibre plants
NOTE. Initial value: A - 67."""@en ;
                                                                                                                    <http://www.w3.org/2004/02/skos/core#inScheme> :SpecieCodeValue .


###  http://lpis.ec.europa.eu/registry/applicationschema/cap-iacs-base/code#SpecieCodeValue/hordeumVulgareLBarley2RowBarley
<http://lpis.ec.europa.eu/registry/applicationschema/cap-iacs-base/code#SpecieCodeValue/hordeumVulgareLBarley2RowBarley> rdf:type owl:NamedIndividual ,
                                                                                                                                  <http://lpis.ec.europa.eu/registry/applicationschema/cap-iacs-base#SpecieCodeValue> ;
                                                                                                                         rdfs:label "Hordeum vulgare L. Barley 2-row barley "@en ;
                                                                                                                         <http://www.w3.org/2004/02/skos/core#definition> """-- Definition --
Hordeum vulgare L. Barley 2-row barley 
-- Description --
List of agricultural species -A   
IV. Cereals
NOTE. Initial value: A - 75.1"""@en ;
                                                                                                                         <http://www.w3.org/2004/02/skos/core#inScheme> :SpecieCodeValue .


###  http://lpis.ec.europa.eu/registry/applicationschema/cap-iacs-base/code#SpecieCodeValue/hordeumVulgareLBarley6RowBarley
<http://lpis.ec.europa.eu/registry/applicationschema/cap-iacs-base/code#SpecieCodeValue/hordeumVulgareLBarley6RowBarley> rdf:type owl:NamedIndividual ,
                                                                                                                                  <http://lpis.ec.europa.eu/registry/applicationschema/cap-iacs-base#SpecieCodeValue> ;
                                                                                                                         rdfs:label "Hordeum vulgare L. Barley 6-row barley "@en ;
                                                                                                                         <http://www.w3.org/2004/02/skos/core#definition> """-- Definition --
Hordeum vulgare L. Barley 6-row barley.
-- Description --
List of agricultural species -A   
IV. Cereals
NOTE. Initial value: A - 75.2"""@en ;
                                                                                                                         <http://www.w3.org/2004/02/skos/core#inScheme> :SpecieCodeValue .


###  http://lpis.ec.europa.eu/registry/applicationschema/cap-iacs-base/code#SpecieCodeValue/lactucaSativaLLettuce
<http://lpis.ec.europa.eu/registry/applicationschema/cap-iacs-base/code#SpecieCodeValue/lactucaSativaLLettuce> rdf:type owl:NamedIndividual ,
                                                                                                                        <http://lpis.ec.europa.eu/registry/applicationschema/cap-iacs-base#SpecieCodeValue> ;
                                                                                                               rdfs:label "Lactuca sativa L. Lettuce"@en ;
                                                                                                               <http://www.w3.org/2004/02/skos/core#definition> """-- Definition --
Lactuca sativa L. Lettuce.
-- Description --
List of vegetable specie -H
NOTE. Initial value: H - 23."""@en ;
                                                                                                               <http://www.w3.org/2004/02/skos/core#inScheme> :SpecieCodeValue .


###  http://lpis.ec.europa.eu/registry/applicationschema/cap-iacs-base/code#SpecieCodeValue/lagenariaSicerariaMolStandl
<http://lpis.ec.europa.eu/registry/applicationschema/cap-iacs-base/code#SpecieCodeValue/lagenariaSicerariaMolStandl> rdf:type owl:NamedIndividual ,
                                                                                                                              <http://lpis.ec.europa.eu/registry/applicationschema/cap-iacs-base#SpecieCodeValue> ;
                                                                                                                     rdfs:label "Lagenaria siceraria (Mol.) Standl."@en ;
                                                                                                                     <http://www.w3.org/2004/02/skos/core#definition> """-- Definition --
Lagenaria siceraria (Mol.) Standl.
-- Description --
List of vegetable specie -H
NOTE. Initial value: H - 37.3"""@en ;
                                                                                                                     <http://www.w3.org/2004/02/skos/core#inScheme> :SpecieCodeValue .


###  http://lpis.ec.europa.eu/registry/applicationschema/cap-iacs-base/code#SpecieCodeValue/linumUsitatissimumLFlaxLinseed
<http://lpis.ec.europa.eu/registry/applicationschema/cap-iacs-base/code#SpecieCodeValue/linumUsitatissimumLFlaxLinseed> rdf:type owl:NamedIndividual ,
                                                                                                                                 <http://lpis.ec.europa.eu/registry/applicationschema/cap-iacs-base#SpecieCodeValue> ;
                                                                                                                        rdfs:label "Linum usitatissimum L. Flax, Linseed "@en ;
                                                                                                                        <http://www.w3.org/2004/02/skos/core#definition> """-- Definition --
Linum usitatissimum L. Flax, Linseed.
-- Description --
List of agricultural species -A
III. Oil and fibre plants
NOTE. Initial value: A - 68."""@en ;
                                                                                                                        <http://www.w3.org/2004/02/skos/core#inScheme> :SpecieCodeValue .


###  http://lpis.ec.europa.eu/registry/applicationschema/cap-iacs-base/code#SpecieCodeValue/loliumPerenneLPerennialRyegrass
<http://lpis.ec.europa.eu/registry/applicationschema/cap-iacs-base/code#SpecieCodeValue/loliumPerenneLPerennialRyegrass> rdf:type owl:NamedIndividual ,
                                                                                                                                  <http://lpis.ec.europa.eu/registry/applicationschema/cap-iacs-base#SpecieCodeValue> ;
                                                                                                                         rdfs:label "Lolium perenne L. Perennial ryegrass"@en ;
                                                                                                                         <http://www.w3.org/2004/02/skos/core#definition> """-- Definition --
Lolium perenne L. Perennial ryegrass.
-- Description --
List of agricultural species -A
II. Fodder plants
NOTE. Initial value: A - 21."""@en ;
                                                                                                                         <http://www.w3.org/2004/02/skos/core#inScheme> :SpecieCodeValue .


###  http://lpis.ec.europa.eu/registry/applicationschema/cap-iacs-base/code#SpecieCodeValue/lotusCorniculatusLBirdsfootTrefoil
<http://lpis.ec.europa.eu/registry/applicationschema/cap-iacs-base/code#SpecieCodeValue/lotusCorniculatusLBirdsfootTrefoil> rdf:type owl:NamedIndividual ,
                                                                                                                                     <http://lpis.ec.europa.eu/registry/applicationschema/cap-iacs-base#SpecieCodeValue> ;
                                                                                                                            rdfs:label "Lotus corniculatus L. Birdsfoot trefoil"@en ;
                                                                                                                            <http://www.w3.org/2004/02/skos/core#definition> """-- Definition --
Lotus corniculatus L. Birdsfoot trefoil
-- Description --
List of agricultural species -A
II. Fodder plants
NOTE. Initial value: A - 34."""@en ;
                                                                                                                            <http://www.w3.org/2004/02/skos/core#inScheme> :SpecieCodeValue .


###  http://lpis.ec.europa.eu/registry/applicationschema/cap-iacs-base/code#SpecieCodeValue/lupinusAlbusLWhiteLupin
<http://lpis.ec.europa.eu/registry/applicationschema/cap-iacs-base/code#SpecieCodeValue/lupinusAlbusLWhiteLupin> rdf:type owl:NamedIndividual ,
                                                                                                                          <http://lpis.ec.europa.eu/registry/applicationschema/cap-iacs-base#SpecieCodeValue> ;
                                                                                                                 rdfs:label "Lupinus albus L. White lupin"@en ;
                                                                                                                 <http://www.w3.org/2004/02/skos/core#definition> """-- Definition --
Lupinus albus L. White lupin.
-- Description --
List of agricultural species -A
II. Fodder plants
NOTE. Initial value: A - 35."""@en ;
                                                                                                                 <http://www.w3.org/2004/02/skos/core#inScheme> :SpecieCodeValue .


###  http://lpis.ec.europa.eu/registry/applicationschema/cap-iacs-base/code#SpecieCodeValue/lupinusAngustifoliusLNarrowLeavedLupin
<http://lpis.ec.europa.eu/registry/applicationschema/cap-iacs-base/code#SpecieCodeValue/lupinusAngustifoliusLNarrowLeavedLupin> rdf:type owl:NamedIndividual ,
                                                                                                                                         <http://lpis.ec.europa.eu/registry/applicationschema/cap-iacs-base#SpecieCodeValue> ;
                                                                                                                                rdfs:label "Lupinus angustifolius L. Narrow leaved lupin"@en ;
                                                                                                                                <http://www.w3.org/2004/02/skos/core#definition> """-- Definition --
Lupinus angustifolius L. Narrow leaved lupin.
-- Description --
List of agricultural species -A
II. Fodder plants
NOTE. Initial value: A - 36."""@en ;
                                                                                                                                <http://www.w3.org/2004/02/skos/core#inScheme> :SpecieCodeValue .


###  http://lpis.ec.europa.eu/registry/applicationschema/cap-iacs-base/code#SpecieCodeValue/lupinusLuteusLYellowLupin
<http://lpis.ec.europa.eu/registry/applicationschema/cap-iacs-base/code#SpecieCodeValue/lupinusLuteusLYellowLupin> rdf:type owl:NamedIndividual ,
                                                                                                                            <http://lpis.ec.europa.eu/registry/applicationschema/cap-iacs-base#SpecieCodeValue> ;
                                                                                                                   rdfs:label "Lupinus luteus L. Yellow lupin"@en ;
                                                                                                                   <http://www.w3.org/2004/02/skos/core#definition> """-- Definition --
Lupinus luteus L. Yellow lupin.
-- Description --
List of agricultural species -A
II. Fodder plants
NOTE. Initial value: A - 37."""@en ;
                                                                                                                   <http://www.w3.org/2004/02/skos/core#inScheme> :SpecieCodeValue .


###  http://lpis.ec.europa.eu/registry/applicationschema/cap-iacs-base/code#SpecieCodeValue/lycopersiconEsculentumLxLPimpinellifolium
<http://lpis.ec.europa.eu/registry/applicationschema/cap-iacs-base/code#SpecieCodeValue/lycopersiconEsculentumLxLPimpinellifolium> rdf:type owl:NamedIndividual ,
                                                                                                                                            <http://lpis.ec.europa.eu/registry/applicationschema/cap-iacs-base#SpecieCodeValue> ;
                                                                                                                                   rdfs:label "Lycopersicon esculentum L. x L. pimpinellifolium"@en ;
                                                                                                                                   <http://www.w3.org/2004/02/skos/core#definition> """-- Definition --
Lycopersicon esculentum L. x L. pimpinellifolium.
-- Description --
List of vegetable specie -H
NOTE. Initial value: H - 37.5"""@en ;
                                                                                                                                   <http://www.w3.org/2004/02/skos/core#inScheme> :SpecieCodeValue .


###  http://lpis.ec.europa.eu/registry/applicationschema/cap-iacs-base/code#SpecieCodeValue/lycopersiconEsculentumLxSHabrochaite
<http://lpis.ec.europa.eu/registry/applicationschema/cap-iacs-base/code#SpecieCodeValue/lycopersiconEsculentumLxSHabrochaite> rdf:type owl:NamedIndividual ,
                                                                                                                                       <http://lpis.ec.europa.eu/registry/applicationschema/cap-iacs-base#SpecieCodeValue> ;
                                                                                                                              rdfs:label "Lycopersicon esculentum L. x S. habrochaites"@en ;
                                                                                                                              <http://www.w3.org/2004/02/skos/core#definition> """-- Definition --
Lycopersicon esculentum L. x S. habrochaites.
-- Description --
List of vegetable specie -H
NOTE. Initial value: H - 37.4"""@en ;
                                                                                                                              <http://www.w3.org/2004/02/skos/core#inScheme> :SpecieCodeValue .


###  http://lpis.ec.europa.eu/registry/applicationschema/cap-iacs-base/code#SpecieCodeValue/lycopersiconEsculentumMillTomato
<http://lpis.ec.europa.eu/registry/applicationschema/cap-iacs-base/code#SpecieCodeValue/lycopersiconEsculentumMillTomato> rdf:type owl:NamedIndividual ,
                                                                                                                                   <http://lpis.ec.europa.eu/registry/applicationschema/cap-iacs-base#SpecieCodeValue> ;
                                                                                                                          rdfs:label "Lycopersicon esculentum Mill. Tomato"@en ;
                                                                                                                          <http://www.w3.org/2004/02/skos/core#definition> """-- Definition --
Lycopersicon esculentum Mill. Tomato.
-- Description --
List of vegetable specie -H
NOTE. Initial value: H - 24."""@en ;
                                                                                                                          <http://www.w3.org/2004/02/skos/core#inScheme> :SpecieCodeValue .


###  http://lpis.ec.europa.eu/registry/applicationschema/cap-iacs-base/code#SpecieCodeValue/medicagoLupulinaLTrefoil
<http://lpis.ec.europa.eu/registry/applicationschema/cap-iacs-base/code#SpecieCodeValue/medicagoLupulinaLTrefoil> rdf:type owl:NamedIndividual ,
                                                                                                                           <http://lpis.ec.europa.eu/registry/applicationschema/cap-iacs-base#SpecieCodeValue> ;
                                                                                                                  rdfs:label "Medicago lupulina L. Trefoil"@en ;
                                                                                                                  <http://www.w3.org/2004/02/skos/core#definition> """-- Definition --
Medicago lupulina L. Trefoil.
-- Description --
List of agricultural species -A
II. Fodder plants
NOTE. Initial value: A - 38."""@en ;
                                                                                                                  <http://www.w3.org/2004/02/skos/core#inScheme> :SpecieCodeValue .


###  http://lpis.ec.europa.eu/registry/applicationschema/cap-iacs-base/code#SpecieCodeValue/medicagoSativaLLucerne
<http://lpis.ec.europa.eu/registry/applicationschema/cap-iacs-base/code#SpecieCodeValue/medicagoSativaLLucerne> rdf:type owl:NamedIndividual ,
                                                                                                                         <http://lpis.ec.europa.eu/registry/applicationschema/cap-iacs-base#SpecieCodeValue> ;
                                                                                                                rdfs:label "Medicago sativa L. Lucerne "@en ;
                                                                                                                <http://www.w3.org/2004/02/skos/core#definition> """-- Definition --
Medicago sativa L. Lucerne.
-- Description --
List of agricultural species -A
II. Fodder plants
NOTE. Initial value: A - 39."""@en ;
                                                                                                                <http://www.w3.org/2004/02/skos/core#inScheme> :SpecieCodeValue .


###  http://lpis.ec.europa.eu/registry/applicationschema/cap-iacs-base/code#SpecieCodeValue/onobrychisViciifoliaScopSainfoin
<http://lpis.ec.europa.eu/registry/applicationschema/cap-iacs-base/code#SpecieCodeValue/onobrychisViciifoliaScopSainfoin> rdf:type owl:NamedIndividual ,
                                                                                                                                   <http://lpis.ec.europa.eu/registry/applicationschema/cap-iacs-base#SpecieCodeValue> ;
                                                                                                                          rdfs:label "Onobrychis viciifolia Scop. Sainfoin"@en ;
                                                                                                                          <http://www.w3.org/2004/02/skos/core#definition> """-- Definition --
Onobrychis viciifolia Scop. Sainfoin.
-- Description --
List of agricultural species -A
II. Fodder plants
NOTE. Initial value: A - 41."""@en ;
                                                                                                                          <http://www.w3.org/2004/02/skos/core#inScheme> :SpecieCodeValue .


###  http://lpis.ec.europa.eu/registry/applicationschema/cap-iacs-base/code#SpecieCodeValue/oryzaSativaLRice
<http://lpis.ec.europa.eu/registry/applicationschema/cap-iacs-base/code#SpecieCodeValue/oryzaSativaLRice> rdf:type owl:NamedIndividual ,
                                                                                                                   <http://lpis.ec.europa.eu/registry/applicationschema/cap-iacs-base#SpecieCodeValue> ;
                                                                                                          rdfs:label "Oryza sativa L. Rice "@en ;
                                                                                                          <http://www.w3.org/2004/02/skos/core#definition> """-- Definition --
Oryza sativa L. Rice.
-- Description --
List of agricultural species -A   
IV. Cereals
NOTE. Initial value: A - 76."""@en ;
                                                                                                          <http://www.w3.org/2004/02/skos/core#inScheme> :SpecieCodeValue .


###  http://lpis.ec.europa.eu/registry/applicationschema/cap-iacs-base/code#SpecieCodeValue/papaverSomniferumLPoppy
<http://lpis.ec.europa.eu/registry/applicationschema/cap-iacs-base/code#SpecieCodeValue/papaverSomniferumLPoppy> rdf:type owl:NamedIndividual ,
                                                                                                                          <http://lpis.ec.europa.eu/registry/applicationschema/cap-iacs-base#SpecieCodeValue> ;
                                                                                                                 rdfs:label "Papaver somniferum L. Poppy"@en ;
                                                                                                                 <http://www.w3.org/2004/02/skos/core#definition> """-- Definition --
Papaver somniferum L. Poppy.
-- Description --
List of agricultural species -A
III. Oil and fibre plants
NOTE. Initial value: A - 69."""@en ;
                                                                                                                 <http://www.w3.org/2004/02/skos/core#inScheme> :SpecieCodeValue .


###  http://lpis.ec.europa.eu/registry/applicationschema/cap-iacs-base/code#SpecieCodeValue/petroselinumCrispumMillNymanExAWHillParsley
<http://lpis.ec.europa.eu/registry/applicationschema/cap-iacs-base/code#SpecieCodeValue/petroselinumCrispumMillNymanExAWHillParsley> rdf:type owl:NamedIndividual ,
                                                                                                                                              <http://lpis.ec.europa.eu/registry/applicationschema/cap-iacs-base#SpecieCodeValue> ;
                                                                                                                                     rdfs:label "Petroselinum crispum (Mill.) Nyman ex A. W. Hill Parsley"@en ;
                                                                                                                                     <http://www.w3.org/2004/02/skos/core#definition> """-- Definition --
Petroselinum crispum (Mill.) Nyman ex A. W. Hill Parsley.
-- Description --
List of vegetable specie -H
NOTE. Initial value: H - 25."""@en ;
                                                                                                                                     <http://www.w3.org/2004/02/skos/core#inScheme> :SpecieCodeValue .


###  http://lpis.ec.europa.eu/registry/applicationschema/cap-iacs-base/code#SpecieCodeValue/phaceliaTanacetifoliaLCaliforniaBluebell
<http://lpis.ec.europa.eu/registry/applicationschema/cap-iacs-base/code#SpecieCodeValue/phaceliaTanacetifoliaLCaliforniaBluebell> rdf:type owl:NamedIndividual ,
                                                                                                                                           <http://lpis.ec.europa.eu/registry/applicationschema/cap-iacs-base#SpecieCodeValue> ;
                                                                                                                                  rdfs:label "Phacelia tanacetifolia L. California bluebell "@en ;
                                                                                                                                  <http://www.w3.org/2004/02/skos/core#definition> """-- Definition --
Phacelia tanacetifolia L. California bluebell.
-- Description --
List of agricultural species -A
II. Fodder plants
NOTE. Initial value: A - 56."""@en ;
                                                                                                                                  <http://www.w3.org/2004/02/skos/core#inScheme> :SpecieCodeValue .


###  http://lpis.ec.europa.eu/registry/applicationschema/cap-iacs-base/code#SpecieCodeValue/phalarisAquaticaLHardingGrassPhalaris
<http://lpis.ec.europa.eu/registry/applicationschema/cap-iacs-base/code#SpecieCodeValue/phalarisAquaticaLHardingGrassPhalaris> rdf:type owl:NamedIndividual ,
                                                                                                                                        <http://lpis.ec.europa.eu/registry/applicationschema/cap-iacs-base#SpecieCodeValue> ;
                                                                                                                               rdfs:label "Phalaris aquatica L. Harding grass/Phalaris"@en ;
                                                                                                                               <http://www.w3.org/2004/02/skos/core#definition> """-- Definition --
Phalaris aquatica L. Harding grass/Phalaris.
-- Description --
List of agricultural species -A
II. Fodder plants
NOTE. Initial value: A - 23."""@en ;
                                                                                                                               <http://www.w3.org/2004/02/skos/core#inScheme> :SpecieCodeValue .


###  http://lpis.ec.europa.eu/registry/applicationschema/cap-iacs-base/code#SpecieCodeValue/phalarisCanariensisLCanaryGrass
<http://lpis.ec.europa.eu/registry/applicationschema/cap-iacs-base/code#SpecieCodeValue/phalarisCanariensisLCanaryGrass> rdf:type owl:NamedIndividual ,
                                                                                                                                  <http://lpis.ec.europa.eu/registry/applicationschema/cap-iacs-base#SpecieCodeValue> ;
                                                                                                                         rdfs:label "Phalaris canariensis L. Canary grass"@en ;
                                                                                                                         <http://www.w3.org/2004/02/skos/core#definition> """-- Definition --
Phalaris canariensis L. Canary grass.
-- Description --
List of agricultural species -A   
IV. Cereals
NOTE. Initial value: A - 77."""@en ;
                                                                                                                         <http://www.w3.org/2004/02/skos/core#inScheme> :SpecieCodeValue .


###  http://lpis.ec.europa.eu/registry/applicationschema/cap-iacs-base/code#SpecieCodeValue/phaseolusCoccineusLRunnerBean
<http://lpis.ec.europa.eu/registry/applicationschema/cap-iacs-base/code#SpecieCodeValue/phaseolusCoccineusLRunnerBean> rdf:type owl:NamedIndividual ,
                                                                                                                                <http://lpis.ec.europa.eu/registry/applicationschema/cap-iacs-base#SpecieCodeValue> ;
                                                                                                                       rdfs:label "Phaseolus coccineus L. Runner bean"@en ;
                                                                                                                       <http://www.w3.org/2004/02/skos/core#definition> """-- Definition --
Phaseolus coccineus L. Runner bean.
-- Description --
List of vegetable specie -H
NOTE. Initial value: H - 26."""@en ;
                                                                                                                       <http://www.w3.org/2004/02/skos/core#inScheme> :SpecieCodeValue .


###  http://lpis.ec.europa.eu/registry/applicationschema/cap-iacs-base/code#SpecieCodeValue/phaseolusVulgarisLClimbingFrenchBean
<http://lpis.ec.europa.eu/registry/applicationschema/cap-iacs-base/code#SpecieCodeValue/phaseolusVulgarisLClimbingFrenchBean> rdf:type owl:NamedIndividual ,
                                                                                                                                       <http://lpis.ec.europa.eu/registry/applicationschema/cap-iacs-base#SpecieCodeValue> ;
                                                                                                                              rdfs:label "Phaseolus vulgaris L. Climbing French bean"@en ;
                                                                                                                              <http://www.w3.org/2004/02/skos/core#definition> """-- Definition --
Phaseolus vulgaris L. Climbing French bean.
-- Description --
List of vegetable specie -H
NOTE. Initial value: H - 27.2"""@en ;
                                                                                                                              <http://www.w3.org/2004/02/skos/core#inScheme> :SpecieCodeValue .


###  http://lpis.ec.europa.eu/registry/applicationschema/cap-iacs-base/code#SpecieCodeValue/phaseolusVulgarisLDwarfFrenchBean
<http://lpis.ec.europa.eu/registry/applicationschema/cap-iacs-base/code#SpecieCodeValue/phaseolusVulgarisLDwarfFrenchBean> rdf:type owl:NamedIndividual ,
                                                                                                                                    <http://lpis.ec.europa.eu/registry/applicationschema/cap-iacs-base#SpecieCodeValue> ;
                                                                                                                           rdfs:label "Phaseolus vulgaris L. Dwarf French bean"@en ;
                                                                                                                           <http://www.w3.org/2004/02/skos/core#definition> """-- Definition --
Phaseolus vulgaris L. Dwarf French bean.
-- Description --
List of vegetable specie -H
NOTE. Initial value: H - 27.1"""@en ;
                                                                                                                           <http://www.w3.org/2004/02/skos/core#inScheme> :SpecieCodeValue .


###  http://lpis.ec.europa.eu/registry/applicationschema/cap-iacs-base/code#SpecieCodeValue/phleumNodosumLSmallTimothy
<http://lpis.ec.europa.eu/registry/applicationschema/cap-iacs-base/code#SpecieCodeValue/phleumNodosumLSmallTimothy> rdf:type owl:NamedIndividual ,
                                                                                                                             <http://lpis.ec.europa.eu/registry/applicationschema/cap-iacs-base#SpecieCodeValue> ;
                                                                                                                    rdfs:label "Phleum nodosum L. Small timothy"@en ;
                                                                                                                    <http://www.w3.org/2004/02/skos/core#definition> """-- Definition --
Phleum nodosum L. Small timothy.
-- Description --
List of agricultural species -A
II. Fodder plants
NOTE. Initial value: A - 24."""@en ;
                                                                                                                    <http://www.w3.org/2004/02/skos/core#inScheme> :SpecieCodeValue .


###  http://lpis.ec.europa.eu/registry/applicationschema/cap-iacs-base/code#SpecieCodeValue/phleumPratenseLTimothy
<http://lpis.ec.europa.eu/registry/applicationschema/cap-iacs-base/code#SpecieCodeValue/phleumPratenseLTimothy> rdf:type owl:NamedIndividual ,
                                                                                                                         <http://lpis.ec.europa.eu/registry/applicationschema/cap-iacs-base#SpecieCodeValue> ;
                                                                                                                rdfs:label "Phleum pratense L. Timothy "@en ;
                                                                                                                <http://www.w3.org/2004/02/skos/core#definition> """-- Definition --
Phleum pratense L. Timothy.
-- Description --
List of agricultural species -A
II. Fodder plants
NOTE. Initial value: A - 25."""@en ;
                                                                                                                <http://www.w3.org/2004/02/skos/core#inScheme> :SpecieCodeValue .


###  http://lpis.ec.europa.eu/registry/applicationschema/cap-iacs-base/code#SpecieCodeValue/pisumSativumLPartimFieldPea
<http://lpis.ec.europa.eu/registry/applicationschema/cap-iacs-base/code#SpecieCodeValue/pisumSativumLPartimFieldPea> rdf:type owl:NamedIndividual ,
                                                                                                                              <http://lpis.ec.europa.eu/registry/applicationschema/cap-iacs-base#SpecieCodeValue> ;
                                                                                                                     rdfs:label "Pisum sativum L. (Partim) Field pea"@en ;
                                                                                                                     <http://www.w3.org/2004/02/skos/core#definition> """-- Definition --
Pisum sativum L. (Partim) Field pea.
-- Description --
List of agricultural species -A
II. Fodder plants
NOTE. Initial value: A - 42."""@en ;
                                                                                                                     <http://www.w3.org/2004/02/skos/core#inScheme> :SpecieCodeValue .


###  http://lpis.ec.europa.eu/registry/applicationschema/cap-iacs-base/code#SpecieCodeValue/pisumSativumLPartimRoundPea
<http://lpis.ec.europa.eu/registry/applicationschema/cap-iacs-base/code#SpecieCodeValue/pisumSativumLPartimRoundPea> rdf:type owl:NamedIndividual ,
                                                                                                                              <http://lpis.ec.europa.eu/registry/applicationschema/cap-iacs-base#SpecieCodeValue> ;
                                                                                                                     rdfs:label "Pisum sativum L. (partim) Round pea"@en ;
                                                                                                                     <http://www.w3.org/2004/02/skos/core#definition> """-- Definition --
Pisum sativum L. (partim) Round pea.
-- Description --
List of vegetable specie -H
NOTE. Initial value: H - 28.2"""@en ;
                                                                                                                     <http://www.w3.org/2004/02/skos/core#inScheme> :SpecieCodeValue .


###  http://lpis.ec.europa.eu/registry/applicationschema/cap-iacs-base/code#SpecieCodeValue/pisumSativumLPartimSugarPea
<http://lpis.ec.europa.eu/registry/applicationschema/cap-iacs-base/code#SpecieCodeValue/pisumSativumLPartimSugarPea> rdf:type owl:NamedIndividual ,
                                                                                                                              <http://lpis.ec.europa.eu/registry/applicationschema/cap-iacs-base#SpecieCodeValue> ;
                                                                                                                     rdfs:label "Pisum sativum L. (partim) Sugar pea"@en ;
                                                                                                                     <http://www.w3.org/2004/02/skos/core#definition> """-- Definition --
Pisum sativum L. (partim) Sugar pea.
-- Description --
List of vegetable specie -H
NOTE. Initial value:H - 28.3"""@en ;
                                                                                                                     <http://www.w3.org/2004/02/skos/core#inScheme> :SpecieCodeValue .


###  http://lpis.ec.europa.eu/registry/applicationschema/cap-iacs-base/code#SpecieCodeValue/pisumSativumLPartimWrinkledPea
<http://lpis.ec.europa.eu/registry/applicationschema/cap-iacs-base/code#SpecieCodeValue/pisumSativumLPartimWrinkledPea> rdf:type owl:NamedIndividual ,
                                                                                                                                 <http://lpis.ec.europa.eu/registry/applicationschema/cap-iacs-base#SpecieCodeValue> ;
                                                                                                                        rdfs:label "Pisum sativum L. (partim) Wrinkled pea"@en ;
                                                                                                                        <http://www.w3.org/2004/02/skos/core#definition> """-- Definition --
Pisum sativum L. (partim) Wrinkled pea.
-- Description --
List of vegetable specie -H
NOTE. Initial value: H - 28.1"""@en ;
                                                                                                                        <http://www.w3.org/2004/02/skos/core#inScheme> :SpecieCodeValue .


###  http://lpis.ec.europa.eu/registry/applicationschema/cap-iacs-base/code#SpecieCodeValue/poaAnnuaLAnnualMeadowgrass
<http://lpis.ec.europa.eu/registry/applicationschema/cap-iacs-base/code#SpecieCodeValue/poaAnnuaLAnnualMeadowgrass> rdf:type owl:NamedIndividual ,
                                                                                                                             <http://lpis.ec.europa.eu/registry/applicationschema/cap-iacs-base#SpecieCodeValue> ;
                                                                                                                    rdfs:label "Poa annua L. Annual meadowgrass"@en ;
                                                                                                                    <http://www.w3.org/2004/02/skos/core#definition> """-- Definition --
Poa annua L. Annual meadowgrass.
-- Description --
List of agricultural species -A
II. Fodder plants
NOTE. Initial value: A - 26."""@en ;
                                                                                                                    <http://www.w3.org/2004/02/skos/core#inScheme> :SpecieCodeValue .


###  http://lpis.ec.europa.eu/registry/applicationschema/cap-iacs-base/code#SpecieCodeValue/poaNemoralisLWoodMeadowgrass
<http://lpis.ec.europa.eu/registry/applicationschema/cap-iacs-base/code#SpecieCodeValue/poaNemoralisLWoodMeadowgrass> rdf:type owl:NamedIndividual ,
                                                                                                                               <http://lpis.ec.europa.eu/registry/applicationschema/cap-iacs-base#SpecieCodeValue> ;
                                                                                                                      rdfs:label "Poa nemoralis L.Wood meadowgrass"@en ;
                                                                                                                      <http://www.w3.org/2004/02/skos/core#definition> """-- Definition --
Poa nemoralis L.Wood meadowgrass
-- Description --
List of agricultural species -A
II. Fodder plants
NOTE. Initial value: A - 27."""@en ;
                                                                                                                      <http://www.w3.org/2004/02/skos/core#inScheme> :SpecieCodeValue .


###  http://lpis.ec.europa.eu/registry/applicationschema/cap-iacs-base/code#SpecieCodeValue/poaPalustrisLSwampMeadowgras
<http://lpis.ec.europa.eu/registry/applicationschema/cap-iacs-base/code#SpecieCodeValue/poaPalustrisLSwampMeadowgras> rdf:type owl:NamedIndividual ,
                                                                                                                               <http://lpis.ec.europa.eu/registry/applicationschema/cap-iacs-base#SpecieCodeValue> ;
                                                                                                                      rdfs:label "Poa palustris L. Swamp meadowgras"@en ;
                                                                                                                      <http://www.w3.org/2004/02/skos/core#definition> """-- Definition --
Poa palustris L. Swamp meadowgras.
-- Description --
List of agricultural species -A
II. Fodder plants
NOTE. Initial value: A - 28."""@en ;
                                                                                                                      <http://www.w3.org/2004/02/skos/core#inScheme> :SpecieCodeValue .


###  http://lpis.ec.europa.eu/registry/applicationschema/cap-iacs-base/code#SpecieCodeValue/poaPratensisLSmoothStalkedMeadowgrass
<http://lpis.ec.europa.eu/registry/applicationschema/cap-iacs-base/code#SpecieCodeValue/poaPratensisLSmoothStalkedMeadowgrass> rdf:type owl:NamedIndividual ,
                                                                                                                                        <http://lpis.ec.europa.eu/registry/applicationschema/cap-iacs-base#SpecieCodeValue> ;
                                                                                                                               rdfs:label "Poa pratensis L. Smooth-stalked meadowgrass"@en ;
                                                                                                                               <http://www.w3.org/2004/02/skos/core#definition> """-- Definition --
Poa pratensis L. Smooth-stalked meadowgrass.
-- Description --
List of agricultural species -A
II. Fodder plants
NOTE. Initial value: A - 29."""@en ;
                                                                                                                               <http://www.w3.org/2004/02/skos/core#inScheme> :SpecieCodeValue .


###  http://lpis.ec.europa.eu/registry/applicationschema/cap-iacs-base/code#SpecieCodeValue/poaTrivialisLRoughStalkedMeadowgrass
<http://lpis.ec.europa.eu/registry/applicationschema/cap-iacs-base/code#SpecieCodeValue/poaTrivialisLRoughStalkedMeadowgrass> rdf:type owl:NamedIndividual ,
                                                                                                                                       <http://lpis.ec.europa.eu/registry/applicationschema/cap-iacs-base#SpecieCodeValue> ;
                                                                                                                              rdfs:label "Poa trivialis L. Rough-stalked meadowgrass"@en ;
                                                                                                                              <http://www.w3.org/2004/02/skos/core#definition> """-- Definition --
Poa trivialis L. Rough-stalked meadowgrass.
-- Description --
List of agricultural species -A
II. Fodder plants
NOTE. Initial value: A - 30."""@en ;
                                                                                                                              <http://www.w3.org/2004/02/skos/core#inScheme> :SpecieCodeValue .


###  http://lpis.ec.europa.eu/registry/applicationschema/cap-iacs-base/code#SpecieCodeValue/raphanusSativusLBlackRadish
<http://lpis.ec.europa.eu/registry/applicationschema/cap-iacs-base/code#SpecieCodeValue/raphanusSativusLBlackRadish> rdf:type owl:NamedIndividual ,
                                                                                                                              <http://lpis.ec.europa.eu/registry/applicationschema/cap-iacs-base#SpecieCodeValue> ;
                                                                                                                     rdfs:label "Raphanus sativus L. Black radish"@en ;
                                                                                                                     <http://www.w3.org/2004/02/skos/core#definition> """-- Definition --
Raphanus sativus L. Black radish.
-- Description --
List of vegetable specie -H
NOTE. Initial value: H - 29.2"""@en ;
                                                                                                                     <http://www.w3.org/2004/02/skos/core#inScheme> :SpecieCodeValue .


###  http://lpis.ec.europa.eu/registry/applicationschema/cap-iacs-base/code#SpecieCodeValue/raphanusSativusLRadish
<http://lpis.ec.europa.eu/registry/applicationschema/cap-iacs-base/code#SpecieCodeValue/raphanusSativusLRadish> rdf:type owl:NamedIndividual ,
                                                                                                                         <http://lpis.ec.europa.eu/registry/applicationschema/cap-iacs-base#SpecieCodeValue> ;
                                                                                                                rdfs:label "Raphanus sativus L. Radish"@en ;
                                                                                                                <http://www.w3.org/2004/02/skos/core#definition> """-- Definition --
Raphanus sativus L. Radish.
-- Description --
List of vegetable specie -H
NOTE. Initial value: H - 29.1"""@en ;
                                                                                                                <http://www.w3.org/2004/02/skos/core#inScheme> :SpecieCodeValue .


###  http://lpis.ec.europa.eu/registry/applicationschema/cap-iacs-base/code#SpecieCodeValue/raphanusSativusLVarOleiformisPersFodderRadish
<http://lpis.ec.europa.eu/registry/applicationschema/cap-iacs-base/code#SpecieCodeValue/raphanusSativusLVarOleiformisPersFodderRadish> rdf:type owl:NamedIndividual ,
                                                                                                                                                <http://lpis.ec.europa.eu/registry/applicationschema/cap-iacs-base#SpecieCodeValue> ;
                                                                                                                                       rdfs:label "Raphanus sativus L. var. oleiformis Pers. Fodder radish"@en ;
                                                                                                                                       <http://www.w3.org/2004/02/skos/core#definition> """-- Definition --
Raphanus sativus L. var. oleiformis Pers. Fodder radish.
-- Description --
List of agricultural species -A
II. Fodder plants
NOTE. Initial value: A - 57."""@en ;
                                                                                                                                       <http://www.w3.org/2004/02/skos/core#inScheme> :SpecieCodeValue .


###  http://lpis.ec.europa.eu/registry/applicationschema/cap-iacs-base/code#SpecieCodeValue/rheumRhabarbarumLRhubarb
<http://lpis.ec.europa.eu/registry/applicationschema/cap-iacs-base/code#SpecieCodeValue/rheumRhabarbarumLRhubarb> rdf:type owl:NamedIndividual ,
                                                                                                                           <http://lpis.ec.europa.eu/registry/applicationschema/cap-iacs-base#SpecieCodeValue> ;
                                                                                                                  rdfs:label "Rheum rhabarbarum L. Rhubarb"@en ;
                                                                                                                  <http://www.w3.org/2004/02/skos/core#definition> """-- Definition --
Rheum rhabarbarum L. Rhubarb.
-- Description --
List of vegetable specie -H
NOTE. Initial value: H - 30."""@en ;
                                                                                                                  <http://www.w3.org/2004/02/skos/core#inScheme> :SpecieCodeValue .


###  http://lpis.ec.europa.eu/registry/applicationschema/cap-iacs-base/code#SpecieCodeValue/scorzoneraHispanicaLScorzoneraBlackSalsify
<http://lpis.ec.europa.eu/registry/applicationschema/cap-iacs-base/code#SpecieCodeValue/scorzoneraHispanicaLScorzoneraBlackSalsify> rdf:type owl:NamedIndividual ,
                                                                                                                                             <http://lpis.ec.europa.eu/registry/applicationschema/cap-iacs-base#SpecieCodeValue> ;
                                                                                                                                    rdfs:label "Scorzonera hispanica L. Scorzonera / Black salsify"@en ;
                                                                                                                                    <http://www.w3.org/2004/02/skos/core#definition> """-- Definition --
Scorzonera hispanica L. Scorzonera / Black salsify.
-- Description --
List of vegetable specie -H
NOTE. Initial value: H - 31."""@en ;
                                                                                                                                    <http://www.w3.org/2004/02/skos/core#inScheme> :SpecieCodeValue .


###  http://lpis.ec.europa.eu/registry/applicationschema/cap-iacs-base/code#SpecieCodeValue/secaleCerealeLRye
<http://lpis.ec.europa.eu/registry/applicationschema/cap-iacs-base/code#SpecieCodeValue/secaleCerealeLRye> rdf:type owl:NamedIndividual ,
                                                                                                                    <http://lpis.ec.europa.eu/registry/applicationschema/cap-iacs-base#SpecieCodeValue> ;
                                                                                                           rdfs:label "Secale cereale L. Rye   "@en ;
                                                                                                           <http://www.w3.org/2004/02/skos/core#definition> """-- Definition --
Secale cereale L. Rye.
-- Description --
List of agricultural species -A   
IV. Cereals
NOTE. Initial value: A - 78."""@en ;
                                                                                                           <http://www.w3.org/2004/02/skos/core#inScheme> :SpecieCodeValue .


###  http://lpis.ec.europa.eu/registry/applicationschema/cap-iacs-base/code#SpecieCodeValue/sicyosAngulatus
<http://lpis.ec.europa.eu/registry/applicationschema/cap-iacs-base/code#SpecieCodeValue/sicyosAngulatus> rdf:type owl:NamedIndividual ,
                                                                                                                  <http://lpis.ec.europa.eu/registry/applicationschema/cap-iacs-base#SpecieCodeValue> ;
                                                                                                         rdfs:label "Sicyos angulatus"@en ;
                                                                                                         <http://www.w3.org/2004/02/skos/core#definition> """-- Definition --
Sicyos angulatus.
-- Description --
List of vegetable specie -H
NOTE. Initial value: H - 37.6"""@en ;
                                                                                                         <http://www.w3.org/2004/02/skos/core#inScheme> :SpecieCodeValue .


###  http://lpis.ec.europa.eu/registry/applicationschema/cap-iacs-base/code#SpecieCodeValue/sinapisAlbaLWhiteMustard
<http://lpis.ec.europa.eu/registry/applicationschema/cap-iacs-base/code#SpecieCodeValue/sinapisAlbaLWhiteMustard> rdf:type owl:NamedIndividual ,
                                                                                                                           <http://lpis.ec.europa.eu/registry/applicationschema/cap-iacs-base#SpecieCodeValue> ;
                                                                                                                  rdfs:label "Sinapis alba L. White mustard"@en ;
                                                                                                                  <http://www.w3.org/2004/02/skos/core#definition> """-- Definition --
Sinapis alba L. White mustard.
-- Description --
List of agricultural species -A
III. Oil and fibre plants
NOTE. Initial value: A - 70."""@en ;
                                                                                                                  <http://www.w3.org/2004/02/skos/core#inScheme> :SpecieCodeValue .


###  http://lpis.ec.europa.eu/registry/applicationschema/cap-iacs-base/code#SpecieCodeValue/slycineMaxLMerrillSoyaBean
<http://lpis.ec.europa.eu/registry/applicationschema/cap-iacs-base/code#SpecieCodeValue/slycineMaxLMerrillSoyaBean> rdf:type owl:NamedIndividual ,
                                                                                                                             <http://lpis.ec.europa.eu/registry/applicationschema/cap-iacs-base#SpecieCodeValue> ;
                                                                                                                    rdfs:label "Glycine max (L.) Merrill Soya bean  "@en ;
                                                                                                                    <http://www.w3.org/2004/02/skos/core#definition> """-- Definition --
Glycine max (L.) Merrill Soya bean.
-- Description --
List of agricultural species -A
III. Oil and fibre plants
NOTE. Initial value: A - 71."""@en ;
                                                                                                                    <http://www.w3.org/2004/02/skos/core#inScheme> :SpecieCodeValue .


###  http://lpis.ec.europa.eu/registry/applicationschema/cap-iacs-base/code#SpecieCodeValue/solanumMelongenaLAubergineEggPlant
<http://lpis.ec.europa.eu/registry/applicationschema/cap-iacs-base/code#SpecieCodeValue/solanumMelongenaLAubergineEggPlant> rdf:type owl:NamedIndividual ,
                                                                                                                                     <http://lpis.ec.europa.eu/registry/applicationschema/cap-iacs-base#SpecieCodeValue> ;
                                                                                                                            rdfs:label "Solanum melongena L. Aubergine / Egg plant"@en ;
                                                                                                                            <http://www.w3.org/2004/02/skos/core#definition> """-- Definition --
Solanum melongena L. Aubergine / Egg plant.
-- Description --
List of vegetable specie -H
NOTE. Initial value: H - 32."""@en ;
                                                                                                                            <http://www.w3.org/2004/02/skos/core#inScheme> :SpecieCodeValue .


###  http://lpis.ec.europa.eu/registry/applicationschema/cap-iacs-base/code#SpecieCodeValue/solanumTorvumSw
<http://lpis.ec.europa.eu/registry/applicationschema/cap-iacs-base/code#SpecieCodeValue/solanumTorvumSw> rdf:type owl:NamedIndividual ,
                                                                                                                  <http://lpis.ec.europa.eu/registry/applicationschema/cap-iacs-base#SpecieCodeValue> ;
                                                                                                         rdfs:label "Solanum torvum Sw."@en ;
                                                                                                         <http://www.w3.org/2004/02/skos/core#definition> """-- Definition --
Solanum torvum Sw.
-- Description --
List of vegetable specie -H
NOTE. Initial value: H - 37.8"""@en ;
                                                                                                         <http://www.w3.org/2004/02/skos/core#inScheme> :SpecieCodeValue .


###  http://lpis.ec.europa.eu/registry/applicationschema/cap-iacs-base/code#SpecieCodeValue/solanumTuberosumLPotato
<http://lpis.ec.europa.eu/registry/applicationschema/cap-iacs-base/code#SpecieCodeValue/solanumTuberosumLPotato> rdf:type owl:NamedIndividual ,
                                                                                                                          <http://lpis.ec.europa.eu/registry/applicationschema/cap-iacs-base#SpecieCodeValue> ;
                                                                                                                 rdfs:label "Solanum tuberosum L. Potato"@en ;
                                                                                                                 <http://www.w3.org/2004/02/skos/core#definition> """-- Definition --
Solanum tuberosum L. Potato.
-- Description --
List of agricultural species -A   
V. Potatoes
NOTE. Initial value: A - 87."""@en ;
                                                                                                                 <http://www.w3.org/2004/02/skos/core#inScheme> :SpecieCodeValue .


###  http://lpis.ec.europa.eu/registry/applicationschema/cap-iacs-base/code#SpecieCodeValue/sorghumBicolorLMoenchSorghum
<http://lpis.ec.europa.eu/registry/applicationschema/cap-iacs-base/code#SpecieCodeValue/sorghumBicolorLMoenchSorghum> rdf:type owl:NamedIndividual ,
                                                                                                                               <http://lpis.ec.europa.eu/registry/applicationschema/cap-iacs-base#SpecieCodeValue> ;
                                                                                                                      rdfs:label "Sorghum bicolor (L.) Moench Sorghum "@en ;
                                                                                                                      <http://www.w3.org/2004/02/skos/core#definition> """-- Definition --
Sorghum bicolor (L.) Moench Sorghum.
-- Description --
List of agricultural species -A   
IV. Cereals
NOTE. Initial value: A - 79."""@en ;
                                                                                                                      <http://www.w3.org/2004/02/skos/core#inScheme> :SpecieCodeValue .


###  http://lpis.ec.europa.eu/registry/applicationschema/cap-iacs-base/code#SpecieCodeValue/sorghumSudanenseLSudanGrass
<http://lpis.ec.europa.eu/registry/applicationschema/cap-iacs-base/code#SpecieCodeValue/sorghumSudanenseLSudanGrass> rdf:type owl:NamedIndividual ,
                                                                                                                              <http://lpis.ec.europa.eu/registry/applicationschema/cap-iacs-base#SpecieCodeValue> ;
                                                                                                                     rdfs:label "Sorghum sudanense L. Sudan grass "@en ;
                                                                                                                     <http://www.w3.org/2004/02/skos/core#definition> """-- Definition --
Sorghum sudanense L. Sudan grass.
-- Description --
List of agricultural species -A   
IV. Cereals
NOTE. Initial value: A - 80."""@en ;
                                                                                                                     <http://www.w3.org/2004/02/skos/core#inScheme> :SpecieCodeValue .


###  http://lpis.ec.europa.eu/registry/applicationschema/cap-iacs-base/code#SpecieCodeValue/spinaciaOleraceaLSpinach
<http://lpis.ec.europa.eu/registry/applicationschema/cap-iacs-base/code#SpecieCodeValue/spinaciaOleraceaLSpinach> rdf:type owl:NamedIndividual ,
                                                                                                                           <http://lpis.ec.europa.eu/registry/applicationschema/cap-iacs-base#SpecieCodeValue> ;
                                                                                                                  rdfs:label "Spinacia oleracea L. Spinach"@en ;
                                                                                                                  <http://www.w3.org/2004/02/skos/core#definition> """-- Definition --
Spinacia oleracea L. Spinach.
-- Description --
List of vegetable specie -H
NOTE. Initial value: H - 33."""@en ;
                                                                                                                  <http://www.w3.org/2004/02/skos/core#inScheme> :SpecieCodeValue .


###  http://lpis.ec.europa.eu/registry/applicationschema/cap-iacs-base/code#SpecieCodeValue/sspAlternativum
<http://lpis.ec.europa.eu/registry/applicationschema/cap-iacs-base/code#SpecieCodeValue/sspAlternativum> rdf:type owl:NamedIndividual ,
                                                                                                                  <http://lpis.ec.europa.eu/registry/applicationschema/cap-iacs-base#SpecieCodeValue> ;
                                                                                                         rdfs:label "Ssp. alternativum"@en ;
                                                                                                         <http://www.w3.org/2004/02/skos/core#definition> """-- Definition --
Lolium multiflorum Lam. Italian ryegrass (including Westerwold ryegrass) Ssp. alternativum. 
-- Description --
List of agricultural species -A
II. Fodder plants
NOTE. Initial value: A - 20.1"""@en ;
                                                                                                         <http://www.w3.org/2004/02/skos/core#inScheme> :SpecieCodeValue .


###  http://lpis.ec.europa.eu/registry/applicationschema/cap-iacs-base/code#SpecieCodeValue/sspNonAlternativum
<http://lpis.ec.europa.eu/registry/applicationschema/cap-iacs-base/code#SpecieCodeValue/sspNonAlternativum> rdf:type owl:NamedIndividual ,
                                                                                                                     <http://lpis.ec.europa.eu/registry/applicationschema/cap-iacs-base#SpecieCodeValue> ;
                                                                                                            rdfs:label "Ssp. non alternativum"@en ;
                                                                                                            <http://www.w3.org/2004/02/skos/core#definition> """-- Definition --
Lolium multiflorum Lam. Italian ryegrass (including Westerwold ryegrass) Ssp. non alternativum.
-- Description --
NOTE. Initial value: A - 20.2"""@en ;
                                                                                                            <http://www.w3.org/2004/02/skos/core#inScheme> :SpecieCodeValue .


###  http://lpis.ec.europa.eu/registry/applicationschema/cap-iacs-base/code#SpecieCodeValue/trifoliumAlexandrinumLBerseemEgyptian
<http://lpis.ec.europa.eu/registry/applicationschema/cap-iacs-base/code#SpecieCodeValue/trifoliumAlexandrinumLBerseemEgyptian> rdf:type owl:NamedIndividual ,
                                                                                                                                        <http://lpis.ec.europa.eu/registry/applicationschema/cap-iacs-base#SpecieCodeValue> ;
                                                                                                                               rdfs:label "Trifolium alexandrinum L. Berseem/Egyptian"@en ;
                                                                                                                               <http://www.w3.org/2004/02/skos/core#definition> """-- Definition --
Trifolium alexandrinum L. Berseem/Egyptian.
-- Description --
List of agricultural species -A
II. Fodder plants
NOTE. Initial value: A - 43."""@en ;
                                                                                                                               <http://www.w3.org/2004/02/skos/core#inScheme> :SpecieCodeValue .


###  http://lpis.ec.europa.eu/registry/applicationschema/cap-iacs-base/code#SpecieCodeValue/trifoliumIncarnatumLCrimsonClover
<http://lpis.ec.europa.eu/registry/applicationschema/cap-iacs-base/code#SpecieCodeValue/trifoliumIncarnatumLCrimsonClover> rdf:type owl:NamedIndividual ,
                                                                                                                                    <http://lpis.ec.europa.eu/registry/applicationschema/cap-iacs-base#SpecieCodeValue> ;
                                                                                                                           rdfs:label "Trifolium incarnatum L. Crimson clover"@en ;
                                                                                                                           <http://www.w3.org/2004/02/skos/core#definition> """-- Definition --
Trifolium incarnatum L. Crimson clover.
-- Description --
List of agricultural species -A
II. Fodder plants
NOTE. Initial value: A - 45."""@en ;
                                                                                                                           <http://www.w3.org/2004/02/skos/core#inScheme> :SpecieCodeValue .


###  http://lpis.ec.europa.eu/registry/applicationschema/cap-iacs-base/code#SpecieCodeValue/trifoliumPratenseLRedClover
<http://lpis.ec.europa.eu/registry/applicationschema/cap-iacs-base/code#SpecieCodeValue/trifoliumPratenseLRedClover> rdf:type owl:NamedIndividual ,
                                                                                                                              <http://lpis.ec.europa.eu/registry/applicationschema/cap-iacs-base#SpecieCodeValue> ;
                                                                                                                     rdfs:label "Trifolium pratense L. Red clover"@en ;
                                                                                                                     <http://www.w3.org/2004/02/skos/core#definition> """-- Definition --
Trifolium pratense L. Red clover.
-- Description --
List of agricultural species -A
II. Fodder plants
NOTE. Initial value: A - 46."""@en ;
                                                                                                                     <http://www.w3.org/2004/02/skos/core#inScheme> :SpecieCodeValue .


###  http://lpis.ec.europa.eu/registry/applicationschema/cap-iacs-base/code#SpecieCodeValue/trifoliumRepensLWhiteClover
<http://lpis.ec.europa.eu/registry/applicationschema/cap-iacs-base/code#SpecieCodeValue/trifoliumRepensLWhiteClover> rdf:type owl:NamedIndividual ,
                                                                                                                              <http://lpis.ec.europa.eu/registry/applicationschema/cap-iacs-base#SpecieCodeValue> ;
                                                                                                                     rdfs:label "Trifolium repens L. White clover"@en ;
                                                                                                                     <http://www.w3.org/2004/02/skos/core#definition> """-- Definition --
Trifolium repens L. White clover.
-- Description --
List of agricultural species -A
II. Fodder plants
NOTE. Initial value: A - 47."""@en ;
                                                                                                                     <http://www.w3.org/2004/02/skos/core#inScheme> :SpecieCodeValue .


###  http://lpis.ec.europa.eu/registry/applicationschema/cap-iacs-base/code#SpecieCodeValue/trifoliumResupinatumLPersianClover
<http://lpis.ec.europa.eu/registry/applicationschema/cap-iacs-base/code#SpecieCodeValue/trifoliumResupinatumLPersianClover> rdf:type owl:NamedIndividual ,
                                                                                                                                     <http://lpis.ec.europa.eu/registry/applicationschema/cap-iacs-base#SpecieCodeValue> ;
                                                                                                                            rdfs:label "Trifolium resupinatum L. Persian clover"@en ;
                                                                                                                            <http://www.w3.org/2004/02/skos/core#definition> """-- Definition --
Trifolium resupinatum L. Persian clover.
-- Description --
List of agricultural species -A
II. Fodder plants
NOTE. Initial value: A - 48."""@en ;
                                                                                                                            <http://www.w3.org/2004/02/skos/core#inScheme> :SpecieCodeValue .


###  http://lpis.ec.europa.eu/registry/applicationschema/cap-iacs-base/code#SpecieCodeValue/trifotiumHybridumLAlsikeClover
<http://lpis.ec.europa.eu/registry/applicationschema/cap-iacs-base/code#SpecieCodeValue/trifotiumHybridumLAlsikeClover> rdf:type owl:NamedIndividual ,
                                                                                                                                 <http://lpis.ec.europa.eu/registry/applicationschema/cap-iacs-base#SpecieCodeValue> ;
                                                                                                                        rdfs:label "Trifolium hybridum L. Alsike clover"@en ;
                                                                                                                        <http://www.w3.org/2004/02/skos/core#definition> """-- Definition --
Trifolium hybridum L. Alsike clover.
-- Description --
List of agricultural species -A
II. Fodder plants
NOTE. Initial value: A - 44."""@en ;
                                                                                                                        <http://www.w3.org/2004/02/skos/core#inScheme> :SpecieCodeValue .


###  http://lpis.ec.europa.eu/registry/applicationschema/cap-iacs-base/code#SpecieCodeValue/trigonellaFoenumGraecumLFenugreek
<http://lpis.ec.europa.eu/registry/applicationschema/cap-iacs-base/code#SpecieCodeValue/trigonellaFoenumGraecumLFenugreek> rdf:type owl:NamedIndividual ,
                                                                                                                                    <http://lpis.ec.europa.eu/registry/applicationschema/cap-iacs-base#SpecieCodeValue> ;
                                                                                                                           rdfs:label "Trigonella foenum-graecum L. Fenugreek   "@en ;
                                                                                                                           <http://www.w3.org/2004/02/skos/core#definition> """-- Definition --
Trigonella foenum-graecum L. Fenugreek.
-- Description --
List of agricultural species -A
II. Fodder plants
NOTE. Initial value: A - 49."""@en ;
                                                                                                                           <http://www.w3.org/2004/02/skos/core#inScheme> :SpecieCodeValue .


###  http://lpis.ec.europa.eu/registry/applicationschema/cap-iacs-base/code#SpecieCodeValue/trisetumFlavescensLGoldenOatgrass
<http://lpis.ec.europa.eu/registry/applicationschema/cap-iacs-base/code#SpecieCodeValue/trisetumFlavescensLGoldenOatgrass> rdf:type owl:NamedIndividual ,
                                                                                                                                    <http://lpis.ec.europa.eu/registry/applicationschema/cap-iacs-base#SpecieCodeValue> ;
                                                                                                                           rdfs:label "Trisetum flavescens L. Golden oatgrass"@en ;
                                                                                                                           <http://www.w3.org/2004/02/skos/core#definition> """-- Definition --
Trisetum flavescens L. Golden oatgrass
-- Description --
List of agricultural species -A
II. Fodder plants
NOTE. Initial value: A - 31."""@en ;
                                                                                                                           <http://www.w3.org/2004/02/skos/core#inScheme> :SpecieCodeValue .


###  http://lpis.ec.europa.eu/registry/applicationschema/cap-iacs-base/code#SpecieCodeValue/triticumAestivumLWheat
<http://lpis.ec.europa.eu/registry/applicationschema/cap-iacs-base/code#SpecieCodeValue/triticumAestivumLWheat> rdf:type owl:NamedIndividual ,
                                                                                                                         <http://lpis.ec.europa.eu/registry/applicationschema/cap-iacs-base#SpecieCodeValue> ;
                                                                                                                rdfs:label "Triticum aestivum L. Wheat"@en ;
                                                                                                                <http://www.w3.org/2004/02/skos/core#definition> """-- Definition --
Triticum aestivum L. Wheat.
-- Description --
List of agricultural species -A   
IV. Cereals
NOTE. Initial value: A - 83."""@en ;
                                                                                                                <http://www.w3.org/2004/02/skos/core#inScheme> :SpecieCodeValue .


###  http://lpis.ec.europa.eu/registry/applicationschema/cap-iacs-base/code#SpecieCodeValue/triticumDurumDesfDurumWheat
<http://lpis.ec.europa.eu/registry/applicationschema/cap-iacs-base/code#SpecieCodeValue/triticumDurumDesfDurumWheat> rdf:type owl:NamedIndividual ,
                                                                                                                              <http://lpis.ec.europa.eu/registry/applicationschema/cap-iacs-base#SpecieCodeValue> ;
                                                                                                                     rdfs:label "Triticum durum Desf. Durum wheat "@en ;
                                                                                                                     <http://www.w3.org/2004/02/skos/core#definition> """-- Definition --
Triticum durum Desf. Durum wheat.
-- Description --
List of agricultural species -A   
IV. Cereals
NOTE. Initial value: A - 84."""@en ;
                                                                                                                     <http://www.w3.org/2004/02/skos/core#inScheme> :SpecieCodeValue .


###  http://lpis.ec.europa.eu/registry/applicationschema/cap-iacs-base/code#SpecieCodeValue/triticumSpeltaLSpeltWheat
<http://lpis.ec.europa.eu/registry/applicationschema/cap-iacs-base/code#SpecieCodeValue/triticumSpeltaLSpeltWheat> rdf:type owl:NamedIndividual ,
                                                                                                                            <http://lpis.ec.europa.eu/registry/applicationschema/cap-iacs-base#SpecieCodeValue> ;
                                                                                                                   rdfs:label "Triticum spelta L. Spelt wheat  "@en ;
                                                                                                                   <http://www.w3.org/2004/02/skos/core#definition> """-- Definition --
Triticum spelta L. Spelt wheat.
-- Description --
List of agricultural species -A   
IV. Cereals
NOTE. Initial value: A - 85."""@en ;
                                                                                                                   <http://www.w3.org/2004/02/skos/core#inScheme> :SpecieCodeValue .


###  http://lpis.ec.europa.eu/registry/applicationschema/cap-iacs-base/code#SpecieCodeValue/valerianellaLocustaLLaterrCornSaladLambsLettuce
<http://lpis.ec.europa.eu/registry/applicationschema/cap-iacs-base/code#SpecieCodeValue/valerianellaLocustaLLaterrCornSaladLambsLettuce> rdf:type owl:NamedIndividual ,
                                                                                                                                                  <http://lpis.ec.europa.eu/registry/applicationschema/cap-iacs-base#SpecieCodeValue> ;
                                                                                                                                         rdfs:label "Valerianella locusta (L.) Laterr. Corn salad / Lamb's lettuce"@en ;
                                                                                                                                         <http://www.w3.org/2004/02/skos/core#definition> """-- Definition --
Valerianella locusta (L.) Laterr. Corn salad / Lamb's lettuce.
-- Description --
List of vegetable specie -H
NOTE. Initial value: H - 34."""@en ;
                                                                                                                                         <http://www.w3.org/2004/02/skos/core#inScheme> :SpecieCodeValue .


###  http://lpis.ec.europa.eu/registry/applicationschema/cap-iacs-base/code#SpecieCodeValue/viciaFabaLPartimBroadBean
<http://lpis.ec.europa.eu/registry/applicationschema/cap-iacs-base/code#SpecieCodeValue/viciaFabaLPartimBroadBean> rdf:type owl:NamedIndividual ,
                                                                                                                            <http://lpis.ec.europa.eu/registry/applicationschema/cap-iacs-base#SpecieCodeValue> ;
                                                                                                                   rdfs:label "Vicia faba L. (partim) Broad bean"@en ;
                                                                                                                   <http://www.w3.org/2004/02/skos/core#definition> """-- Definition --
Vicia faba L. (partim) Broad bean.
-- Description --
List of vegetable specie -H
NOTE. Initial value: H - 35."""@en ;
                                                                                                                   <http://www.w3.org/2004/02/skos/core#inScheme> :SpecieCodeValue .


###  http://lpis.ec.europa.eu/registry/applicationschema/cap-iacs-base/code#SpecieCodeValue/viciaFabaLPartimFieldBean
<http://lpis.ec.europa.eu/registry/applicationschema/cap-iacs-base/code#SpecieCodeValue/viciaFabaLPartimFieldBean> rdf:type owl:NamedIndividual ,
                                                                                                                            <http://lpis.ec.europa.eu/registry/applicationschema/cap-iacs-base#SpecieCodeValue> ;
                                                                                                                   rdfs:label "Vicia faba L. (Partim) Field bean"@en ;
                                                                                                                   <http://www.w3.org/2004/02/skos/core#definition> """-- Definition --
Vicia faba L. (Partim) Field bean.
-- Description --
List of agricultural species -A
II. Fodder plants
NOTE. Initial value: A - 50."""@en ;
                                                                                                                   <http://www.w3.org/2004/02/skos/core#inScheme> :SpecieCodeValue .


###  http://lpis.ec.europa.eu/registry/applicationschema/cap-iacs-base/code#SpecieCodeValue/viciaPannonicaLHungarianVetch
<http://lpis.ec.europa.eu/registry/applicationschema/cap-iacs-base/code#SpecieCodeValue/viciaPannonicaLHungarianVetch> rdf:type owl:NamedIndividual ,
                                                                                                                                <http://lpis.ec.europa.eu/registry/applicationschema/cap-iacs-base#SpecieCodeValue> ;
                                                                                                                       rdfs:label "Vicia pannonica L. Hungarian vetch "@en ;
                                                                                                                       <http://www.w3.org/2004/02/skos/core#definition> """-- Definition --
Vicia pannonica L. Hungarian vetch.
-- Description --
List of agricultural species -A
II. Fodder plants
NOTE. Initial value: A - 51."""@en ;
                                                                                                                       <http://www.w3.org/2004/02/skos/core#inScheme> :SpecieCodeValue .


###  http://lpis.ec.europa.eu/registry/applicationschema/cap-iacs-base/code#SpecieCodeValue/viciaSativaLCommonVetch
<http://lpis.ec.europa.eu/registry/applicationschema/cap-iacs-base/code#SpecieCodeValue/viciaSativaLCommonVetch> rdf:type owl:NamedIndividual ,
                                                                                                                          <http://lpis.ec.europa.eu/registry/applicationschema/cap-iacs-base#SpecieCodeValue> ;
                                                                                                                 rdfs:label "Vicia sativa L. Common vetch "@en ;
                                                                                                                 <http://www.w3.org/2004/02/skos/core#definition> """-- Definition --
Vicia sativa L. Common vetch.
-- Description --
List of agricultural species -A
II. Fodder plants
NOTE. Initial value: A - 52."""@en ;
                                                                                                                 <http://www.w3.org/2004/02/skos/core#inScheme> :SpecieCodeValue .


###  http://lpis.ec.europa.eu/registry/applicationschema/cap-iacs-base/code#SpecieCodeValue/viciaVillosaRothHairyVetch
<http://lpis.ec.europa.eu/registry/applicationschema/cap-iacs-base/code#SpecieCodeValue/viciaVillosaRothHairyVetch> rdf:type owl:NamedIndividual ,
                                                                                                                             <http://lpis.ec.europa.eu/registry/applicationschema/cap-iacs-base#SpecieCodeValue> ;
                                                                                                                    rdfs:label "Vicia villosa Roth. Hairy vetch"@en ;
                                                                                                                    <http://www.w3.org/2004/02/skos/core#definition> """-- Definition --
Vicia villosa Roth. Hairy vetch.
-- Description --
List of agricultural species -A
II. Fodder plants
NOTE. Initial value: A - 53."""@en ;
                                                                                                                    <http://www.w3.org/2004/02/skos/core#inScheme> :SpecieCodeValue .


###  http://lpis.ec.europa.eu/registry/applicationschema/cap-iacs-base/code#SpecieCodeValue/zeaMaysLMaize
<http://lpis.ec.europa.eu/registry/applicationschema/cap-iacs-base/code#SpecieCodeValue/zeaMaysLMaize> rdf:type owl:NamedIndividual ,
                                                                                                                <http://lpis.ec.europa.eu/registry/applicationschema/cap-iacs-base#SpecieCodeValue> ;
                                                                                                       rdfs:label "Zea mays L. Maize  "@en ;
                                                                                                       <http://www.w3.org/2004/02/skos/core#definition> """-- Definition --
Zea mays L. Maize.
-- Description --
List of agricultural species -A   
IV. Cereals
NOTE. Initial value: A - 86."""@en ;
                                                                                                       <http://www.w3.org/2004/02/skos/core#inScheme> :SpecieCodeValue .


###  http://lpis.ec.europa.eu/registry/applicationschema/cap-iacs-base/code#SpecieCodeValue/zeaMaysLPopcorn
<http://lpis.ec.europa.eu/registry/applicationschema/cap-iacs-base/code#SpecieCodeValue/zeaMaysLPopcorn> rdf:type owl:NamedIndividual ,
                                                                                                                  <http://lpis.ec.europa.eu/registry/applicationschema/cap-iacs-base#SpecieCodeValue> ;
                                                                                                         rdfs:label "Zea mays L. Popcorn"@en ;
                                                                                                         <http://www.w3.org/2004/02/skos/core#definition> """-- Definition --
Zea mays L. Popcorn.
-- Description --
List of vegetable specie -H
NOTE. Initial value: H - 36.2"""@en ;
                                                                                                         <http://www.w3.org/2004/02/skos/core#inScheme> :SpecieCodeValue .


###  http://lpis.ec.europa.eu/registry/applicationschema/cap-iacs-base/code#SpecieCodeValue/zeaMaysLSweetCorn
<http://lpis.ec.europa.eu/registry/applicationschema/cap-iacs-base/code#SpecieCodeValue/zeaMaysLSweetCorn> rdf:type owl:NamedIndividual ,
                                                                                                                    <http://lpis.ec.europa.eu/registry/applicationschema/cap-iacs-base#SpecieCodeValue> ;
                                                                                                           rdfs:label "Zea mays L. Sweet corn"@en ;
                                                                                                           <http://www.w3.org/2004/02/skos/core#definition> """-- Definition --
Zea mays L. Sweet corn.
-- Description --
List of vegetable specie -H
NOTE. Initial value: H - 36.1"""@en ;
                                                                                                           <http://www.w3.org/2004/02/skos/core#inScheme> :SpecieCodeValue .


###  http://lpis.ec.europa.eu/registry/applicationschema/cap-iacs-base/code#SpecieCodeValue/lolium×BoucheanumKunthHybridRyegrass
<http://lpis.ec.europa.eu/registry/applicationschema/cap-iacs-base/code#SpecieCodeValue/lolium×BoucheanumKunthHybridRyegrass> rdf:type owl:NamedIndividual ,
                                                                                                                                       <http://lpis.ec.europa.eu/registry/applicationschema/cap-iacs-base#SpecieCodeValue> ;
                                                                                                                              rdfs:label "Lolium × boucheanum Kunth Hybrid ryegrass "@en ;
                                                                                                                              <http://www.w3.org/2004/02/skos/core#definition> """-- Definition --
Lolium × boucheanum Kunth Hybrid ryegrass.
-- Description --
List of agricultural species -A
II. Fodder plants
NOTE. Initial value: A - 22."""@en ;
                                                                                                                              <http://www.w3.org/2004/02/skos/core#inScheme> :SpecieCodeValue .


###  http://lpis.ec.europa.eu/registry/applicationschema/cap-iacs-base/code#SpecieCodeValue/medicago×VariaLSandLucerne
<http://lpis.ec.europa.eu/registry/applicationschema/cap-iacs-base/code#SpecieCodeValue/medicago×VariaLSandLucerne> rdf:type owl:NamedIndividual ,
                                                                                                                             <http://lpis.ec.europa.eu/registry/applicationschema/cap-iacs-base#SpecieCodeValue> ;
                                                                                                                    rdfs:label "Medicago × varia L. Sand lucerne"@en ;
                                                                                                                    <http://www.w3.org/2004/02/skos/core#definition> """-- Definition --
Medicago × varia L. Sand lucerne.
-- Description --
List of agricultural species -A
II. Fodder plants
NOTE. Initial value:A - 40."""@en ;
                                                                                                                    <http://www.w3.org/2004/02/skos/core#inScheme> :SpecieCodeValue .


###  http://lpis.ec.europa.eu/registry/applicationschema/cap-iacs-base/code#SpecieCodeValue/sorghumBicolorLMoench×SorghumSudanensePiperStapfHybrids
<http://lpis.ec.europa.eu/registry/applicationschema/cap-iacs-base/code#SpecieCodeValue/sorghumBicolorLMoench×SorghumSudanensePiperStapfHybrids> rdf:type owl:NamedIndividual ,
                                                                                                                                                          <http://lpis.ec.europa.eu/registry/applicationschema/cap-iacs-base#SpecieCodeValue> ;
                                                                                                                                                 rdfs:label "Sorghum bicolor (L.) Moench × Sorghum sudanense (Piper) Stapf. Hybrids"@en ;
                                                                                                                                                 <http://www.w3.org/2004/02/skos/core#definition> """-- Definition --
Sorghum bicolor (L.) Moench × Sorghum sudanense (Piper) Stapf. Hybrids resulting from the crossing of Sorghum bicolor and Sorghum sudanense.
-- Description --
List of agricultural species -A   
IV. Cereals
NOTE. Initial value: A - 81."""@en ;
                                                                                                                                                 <http://www.w3.org/2004/02/skos/core#inScheme> :SpecieCodeValue .


###  http://lpis.ec.europa.eu/registry/applicationschema/cap-iacs-base/code#SpecieCodeValue/×FestuloliumAschEtGraebnHybrids
<http://lpis.ec.europa.eu/registry/applicationschema/cap-iacs-base/code#SpecieCodeValue/×FestuloliumAschEtGraebnHybrids> rdf:type owl:NamedIndividual ,
                                                                                                                                  <http://lpis.ec.europa.eu/registry/applicationschema/cap-iacs-base#SpecieCodeValue> ;
                                                                                                                         rdfs:label "×Festulolium Asch. et Graebn. Hybrids"@en ;
                                                                                                                         <http://www.w3.org/2004/02/skos/core#definition> """-- Definition --
×Festulolium Asch. et Graebn. Hybrids resulting from the crossing of a species of the genus Festuca with a species of the genus Lolium.
-- Description --
List of agricultural species -A
II. Fodder plants
NOTE. Initial value: A - 19."""@en ;
                                                                                                                         <http://www.w3.org/2004/02/skos/core#inScheme> :SpecieCodeValue .


###  http://lpis.ec.europa.eu/registry/applicationschema/cap-iacs-base/code#SpecieCodeValue/×TriticosecaleWittmExACamusHybrids
<http://lpis.ec.europa.eu/registry/applicationschema/cap-iacs-base/code#SpecieCodeValue/×TriticosecaleWittmExACamusHybrids> rdf:type owl:NamedIndividual ,
                                                                                                                                     <http://lpis.ec.europa.eu/registry/applicationschema/cap-iacs-base#SpecieCodeValue> ;
                                                                                                                            rdfs:label "×Triticosecale Wittm. ex A. Camus Hybrids"@en ;
                                                                                                                            <http://www.w3.org/2004/02/skos/core#definition> """-- Definition --
×Triticosecale Wittm. ex A. Camus Hybrids resulting from the crossing of a species of the genus Triticum and a species of the genus Secale.
-- Description --
List of agricultural species -A   
IV. Cereals
NOTE. Initial value: A - 82."""@en ;
                                                                                                                            <http://www.w3.org/2004/02/skos/core#inScheme> :SpecieCodeValue .


###  http://lpis.ec.europa.eu/registry/applicationschema/cap-iacs-base/code#StatusOfAnomalyValue/archived
<http://lpis.ec.europa.eu/registry/applicationschema/cap-iacs-base/code#StatusOfAnomalyValue/archived> rdf:type owl:NamedIndividual ,
                                                                                                                <http://lpis.ec.europa.eu/registry/applicationschema/cap-iacs-base#StatusOfAnomalyValue> ;
                                                                                                       rdfs:label "Closed"@en ;
                                                                                                       <http://www.w3.org/2004/02/skos/core#definition> """--Name--
Archived

-- Definition --
Status of anomaly as soon as it has been resolved.

--Description--
Anomalies are archived for historic reference."""@en ;
                                                                                                       <http://www.w3.org/2004/02/skos/core#inScheme> :StatusOfAnomalyValue .


###  http://lpis.ec.europa.eu/registry/applicationschema/cap-iacs-base/code#StatusOfAnomalyValue/inProgress
<http://lpis.ec.europa.eu/registry/applicationschema/cap-iacs-base/code#StatusOfAnomalyValue/inProgress> rdf:type owl:NamedIndividual ,
                                                                                                                  <http://lpis.ec.europa.eu/registry/applicationschema/cap-iacs-base#StatusOfAnomalyValue> ;
                                                                                                         rdfs:label "In progress"@en ;
                                                                                                         <http://www.w3.org/2004/02/skos/core#definition> """--Name--
In progress

-- Definition --
Status of the anomaly as soon as its processing has started or has been flagged for later resolution."""@en ;
                                                                                                         <http://www.w3.org/2004/02/skos/core#inScheme> :StatusOfAnomalyValue .


###  http://lpis.ec.europa.eu/registry/applicationschema/cap-iacs-base/code#StatusOfAnomalyValue/open
<http://lpis.ec.europa.eu/registry/applicationschema/cap-iacs-base/code#StatusOfAnomalyValue/open> rdf:type owl:NamedIndividual ,
                                                                                                            <http://lpis.ec.europa.eu/registry/applicationschema/cap-iacs-base#StatusOfAnomalyValue> ;
                                                                                                   rdfs:label "Open"@en ;
                                                                                                   <http://www.w3.org/2004/02/skos/core#definition> """--Name--
Open

-- Definition --
Status of anomaly after recording it in the information system."""@en ;
                                                                                                   <http://www.w3.org/2004/02/skos/core#inScheme> :StatusOfAnomalyValue .


###  http://lpis.ec.europa.eu/registry/applicationschema/cap-iacs-base/code#StatusOfIssueValue/archived
<http://lpis.ec.europa.eu/registry/applicationschema/cap-iacs-base/code#StatusOfIssueValue/archived> rdf:type owl:NamedIndividual ,
                                                                                                              <http://lpis.ec.europa.eu/registry/applicationschema/cap-iacs-base#StatusOfIssueValue> ;
                                                                                                     rdfs:label "Closed"@en ;
                                                                                                     <http://www.w3.org/2004/02/skos/core#definition> """--Name--
Archived

-- Definition --
Status of issue as soon as it has been resolved.

--Description--
Issues are archived for historic reference."""@en ;
                                                                                                     <http://www.w3.org/2004/02/skos/core#inScheme> :StatusOfIssueValue .


###  http://lpis.ec.europa.eu/registry/applicationschema/cap-iacs-base/code#StatusOfIssueValue/inProgress
<http://lpis.ec.europa.eu/registry/applicationschema/cap-iacs-base/code#StatusOfIssueValue/inProgress> rdf:type owl:NamedIndividual ,
                                                                                                                <http://lpis.ec.europa.eu/registry/applicationschema/cap-iacs-base#StatusOfIssueValue> ;
                                                                                                       rdfs:label "In progress"@en ;
                                                                                                       <http://www.w3.org/2004/02/skos/core#definition> """--Name--
In progress

-- Definition --
Status of the issue as soon as its processing has started or has been flagged for later resolution."""@en ;
                                                                                                       <http://www.w3.org/2004/02/skos/core#inScheme> :StatusOfIssueValue .


###  http://lpis.ec.europa.eu/registry/applicationschema/cap-iacs-base/code#StatusOfIssueValue/open
<http://lpis.ec.europa.eu/registry/applicationschema/cap-iacs-base/code#StatusOfIssueValue/open> rdf:type owl:NamedIndividual ,
                                                                                                          <http://lpis.ec.europa.eu/registry/applicationschema/cap-iacs-base#StatusOfIssueValue> ;
                                                                                                 rdfs:label "Open"@en ;
                                                                                                 <http://www.w3.org/2004/02/skos/core#definition> """--Name--
Open

-- Definition --
Status of issue after recording it in the information system."""@en ;
                                                                                                 <http://www.w3.org/2004/02/skos/core#inScheme> :StatusOfIssueValue .


###  http://lpis.ec.europa.eu/registry/applicationschema/cap-iacs-base/code#StatusValue/approved
<http://lpis.ec.europa.eu/registry/applicationschema/cap-iacs-base/code#StatusValue/approved> rdf:type owl:NamedIndividual ,
                                                                                                       <http://lpis.ec.europa.eu/registry/applicationschema/cap-iacs-base#StatusValue> ;
                                                                                              rdfs:label "Approved, valid, archival"@en ;
                                                                                              <http://www.w3.org/2004/02/skos/core#definition> """-- Definition --
Approved,

--Definition--
Status of an object according to the state machine diagram.

-- Description --
Status of the targeted schema / data object after final controls (consistency with IACS  and local rules)."""@en ;
                                                                                              <http://www.w3.org/2004/02/skos/core#inScheme> :StatusValue .


###  http://lpis.ec.europa.eu/registry/applicationschema/cap-iacs-base/code#StatusValue/archived
<http://lpis.ec.europa.eu/registry/applicationschema/cap-iacs-base/code#StatusValue/archived> rdf:type owl:NamedIndividual ,
                                                                                                       <http://lpis.ec.europa.eu/registry/applicationschema/cap-iacs-base#StatusValue> ;
                                                                                              <http://www.w3.org/2004/02/skos/core#definition> """--Name--
Archived

--Definition--
Status of an object according to the state machine diagram.

-- Description--
Final state of an object after its depreciation (retirement).
Such object is no more in use; its life cycle has been completed.

NOTE 1. FeatureLevelMetadata.endLifespanVersion<>Null

NOTE 2. NOTE 2: If applied, FeatureLevelMetadata.validTo<>Null"""@en ;
                                                                                              <http://www.w3.org/2004/02/skos/core#inScheme> :StatusValue .


###  http://lpis.ec.europa.eu/registry/applicationschema/cap-iacs-base/code#StatusValue/inProgress
<http://lpis.ec.europa.eu/registry/applicationschema/cap-iacs-base/code#StatusValue/inProgress> rdf:type owl:NamedIndividual ,
                                                                                                         <http://lpis.ec.europa.eu/registry/applicationschema/cap-iacs-base#StatusValue> ;
                                                                                                rdfs:label "Under construction"@en ;
                                                                                                <http://www.w3.org/2004/02/skos/core#definition> """-- Name--
In progress

--Definition--
Status of an object according to the state machine diagram.

-- Description --
The value shall be assigned when processing of the issue/anomaly has been started. The value is applicable to
- the issue/anomaly that reported the change request
- the object (schema element or data) that is subject of the change request.

EXAMPLE 1. Schema element objects are:
- the entire application schema,
- feature and data types
- attributes, association roles,
- constraints
- value types (etc).

EXAMPLE 2. Data objects are specific instances of a feature or data types (e.g. RP, farmer, anomaly, payment. The change may be applied to 
- the instance as a whole (depreciation of an obsolete instance or introduction of a new instance),
- a specific value (attribute) of an instance.

NOTE: Rules for depreciation are defined by internal business rules of the MS/Region"""@en ;
                                                                                                <http://www.w3.org/2004/02/skos/core#inScheme> :StatusValue .


###  http://lpis.ec.europa.eu/registry/applicationschema/cap-iacs-base/code#StatusValue/open
<http://lpis.ec.europa.eu/registry/applicationschema/cap-iacs-base/code#StatusValue/open> rdf:type owl:NamedIndividual ,
                                                                                                   <http://lpis.ec.europa.eu/registry/applicationschema/cap-iacs-base#StatusValue> ;
                                                                                          rdfs:label "Registered"@en ;
                                                                                          <http://www.w3.org/2004/02/skos/core#definition> """--Name--
Open

--Definition--
Status of an object according to the state machine diagram.

--Description --
This status is applicable to UpgradeIssue and Anomaly feature types only. The value is assigned in the moment when an instance of these feature types is introduced in the information system."""@en ;
                                                                                          <http://www.w3.org/2004/02/skos/core#inScheme> :StatusValue .


###  http://lpis.ec.europa.eu/registry/applicationschema/cap-iacs-base/code#StatusValue/rejected
<http://lpis.ec.europa.eu/registry/applicationschema/cap-iacs-base/code#StatusValue/rejected> rdf:type owl:NamedIndividual ,
                                                                                                       <http://lpis.ec.europa.eu/registry/applicationschema/cap-iacs-base#StatusValue> ;
                                                                                              rdfs:label "Rejected, not valid, archival"@en ;
                                                                                              <http://www.w3.org/2004/02/skos/core#definition> """-- Name--
Rejected

--Definition--
Status of an object according to the state machine diagram.

-- Description --
Status of the change request after the negative outcome of the preliminary evaluation or the cross-check. It also means that no modification to the existing information can be executed.

NOTE: For transparency, the rejected change requests shall be archived."""@en ;
                                                                                              <http://www.w3.org/2004/02/skos/core#inScheme> :StatusValue .


###  http://lpis.ec.europa.eu/registry/applicationschema/cap-iacs-base/code#StatusValue/underApproval
<http://lpis.ec.europa.eu/registry/applicationschema/cap-iacs-base/code#StatusValue/underApproval> rdf:type owl:NamedIndividual ,
                                                                                                            <http://lpis.ec.europa.eu/registry/applicationschema/cap-iacs-base#StatusValue> ;
                                                                                                   rdfs:label "Under aprooval"@en ;
                                                                                                   <http://www.w3.org/2004/02/skos/core#definition> """-- Name--
Under approval

--Definition--
Status of an object according to the state machine diagram.

-- Description --
Based on the outcome of cross checks the change request is approved. The object is waiting for finalisation."""@en ;
                                                                                                   <http://www.w3.org/2004/02/skos/core#inScheme> :StatusValue .


###  http://lpis.ec.europa.eu/registry/applicationschema/cap-iacs-base/code#StatusValue/underCrossCheck
<http://lpis.ec.europa.eu/registry/applicationschema/cap-iacs-base/code#StatusValue/underCrossCheck> rdf:type owl:NamedIndividual ,
                                                                                                              <http://lpis.ec.europa.eu/registry/applicationschema/cap-iacs-base#StatusValue> ;
                                                                                                     rdfs:label "Under construction"@en ;
                                                                                                     <http://www.w3.org/2004/02/skos/core#definition> """-- Name--
Under cross-check

--Definition--
Status of an object according to the state machine diagram.

-- Description --
Whenever a transaction in the information system is performed, the system shall be checked for integrity of the schema and the consistency of data. 

NOTE 1. Cross checks are also the tools to find further issues/anomalies. When a new upgrade issue/anomaly is found, the \"open\" value shall be assigned and the full life cycle assessment of the object has to be performed."""@en ;
                                                                                                     <http://www.w3.org/2004/02/skos/core#inScheme> :StatusValue .


###  http://lpis.ec.europa.eu/registry/applicationschema/cap-iacs-base/code#StatusValue/underEvaluation
<http://lpis.ec.europa.eu/registry/applicationschema/cap-iacs-base/code#StatusValue/underEvaluation> rdf:type owl:NamedIndividual ,
                                                                                                              <http://lpis.ec.europa.eu/registry/applicationschema/cap-iacs-base#StatusValue> ;
                                                                                                     rdfs:label "Under evaluation"@en ;
                                                                                                     <http://www.w3.org/2004/02/skos/core#definition> """-- Name--
Under evaluation

--Definition--
Status of an object according to the state machine diagram.

-- Description --
Preliminary assessment about the impact of the Upgrade issue or the anomaly. This value should be assigned in the phase when
- supporting evidences are collected  and/or
- checks for issue/anomaly duplicates are performed.  
The assessment may conclude that no modification to the existing data is needed, or that the reported change request has to be further processed."""@en ;
                                                                                                     <http://www.w3.org/2004/02/skos/core#inScheme> :StatusValue .


###  http://lpis.ec.europa.eu/registry/applicationschema/cap-iacs-base/code#StatusValue/valid
<http://lpis.ec.europa.eu/registry/applicationschema/cap-iacs-base/code#StatusValue/valid> rdf:type owl:NamedIndividual ,
                                                                                                    <http://lpis.ec.europa.eu/registry/applicationschema/cap-iacs-base#StatusValue> ;
                                                                                           <http://www.w3.org/2004/02/skos/core#definition> """-- Name--
Valid

--Definition--
Status of an object according to the state machine diagram.

-- Description --
The most current state of the object that shall be used by the users. 

NOTE 1: It is a current object whose life-cycle has not ended.
FeatureLevelMetadata.endLifespanVersion=Null

NOTE 2: If applied, FeatureLevelMetadata.validTo=Null"""@en ;
                                                                                           <http://www.w3.org/2004/02/skos/core#inScheme> :StatusValue .


###  http://lpis.ec.europa.eu/registry/applicationschema/cap-iacs-base/code#SupportSchemeTypeValue/aegeanIslands
<http://lpis.ec.europa.eu/registry/applicationschema/cap-iacs-base/code#SupportSchemeTypeValue/aegeanIslands> rdf:type owl:NamedIndividual ,
                                                                                                                       <http://lpis.ec.europa.eu/registry/applicationschema/cap-iacs-base#SupportSchemeTypeValue> ;
                                                                                                              rdfs:label "Aegean islands"@en ;
                                                                                                              <http://www.w3.org/2004/02/skos/core#definition> """Aegean islands

Chapter IV of Regulation (EU) No 229/2013 / Direct payments under measures established in the programmes: Specific measures in favour of the smaller Aegean islands."""@en ;
                                                                                                              <http://www.w3.org/2004/02/skos/core#inScheme> :SupportSchemeTypeValue .


###  http://lpis.ec.europa.eu/registry/applicationschema/cap-iacs-base/code#SupportSchemeTypeValue/basicPaymentScheme
<http://lpis.ec.europa.eu/registry/applicationschema/cap-iacs-base/code#SupportSchemeTypeValue/basicPaymentScheme> rdf:type owl:NamedIndividual ,
                                                                                                                            <http://lpis.ec.europa.eu/registry/applicationschema/cap-iacs-base#SupportSchemeTypeValue> ;
                                                                                                                   rdfs:label "Basic payment scheme"@en ;
                                                                                                                   <http://www.w3.org/2004/02/skos/core#definition> """Basic payment scheme

Basic payment scheme - BPS as described in Title III, Chapter 1, Sections 1, 2, 3 and 5 of Regulation (EU) 1307/2013.

Decoupled payment that is based on entitlements."""@en ;
                                                                                                                   <http://www.w3.org/2004/02/skos/core#inScheme> :SupportSchemeTypeValue .


###  http://lpis.ec.europa.eu/registry/applicationschema/cap-iacs-base/code#SupportSchemeTypeValue/cropSpecificPaymentForCotton
<http://lpis.ec.europa.eu/registry/applicationschema/cap-iacs-base/code#SupportSchemeTypeValue/cropSpecificPaymentForCotton> rdf:type owl:NamedIndividual ,
                                                                                                                                      <http://lpis.ec.europa.eu/registry/applicationschema/cap-iacs-base#SupportSchemeTypeValue> ;
                                                                                                                             rdfs:label "Crop-specific payment for cotton"@en ;
                                                                                                                             <http://www.w3.org/2004/02/skos/core#definition> """Crop-specific payment for cotton

Aid shall be granted to farmers producing cotton falling within CN code 5201 00 under the conditions laid down in this Chapter.

Title IV, Chapter 2 of 1307/2013 Regulation / Area payment."""@en ;
                                                                                                                             <http://www.w3.org/2004/02/skos/core#inScheme> :SupportSchemeTypeValue .


###  http://lpis.ec.europa.eu/registry/applicationschema/cap-iacs-base/code#SupportSchemeTypeValue/paymentForAgriculturalPracticesBeneficialForTheClimateAndTheEnvironment
<http://lpis.ec.europa.eu/registry/applicationschema/cap-iacs-base/code#SupportSchemeTypeValue/paymentForAgriculturalPracticesBeneficialForTheClimateAndTheEnvironment> rdf:type owl:NamedIndividual ,
                                                                                                                                                                                 <http://lpis.ec.europa.eu/registry/applicationschema/cap-iacs-base#SupportSchemeTypeValue> ;
                                                                                                                                                                        rdfs:label "Payment for agricultural practices beneficial for the climate and the environment"@en ;
                                                                                                                                                                        <http://www.w3.org/2004/02/skos/core#definition> """Payment for agricultural practices beneficial for the climate and the environment 

Farmers entitled to a payment under the basic payment scheme or the single area payment scheme shall observe, on all their eligible hectares within the meaning of Article 32(2) to (5), the agricultural practices beneficial for the climate and the environment referred to in paragraph 2 of this Article or the equivalent practices referred to in paragraph 3 of this Article.

According to Title III, Chapter 3 of 1307/2013 Regulation  it is a decoupled payment. Also known as the Green Payment."""@en ;
                                                                                                                                                                        <http://www.w3.org/2004/02/skos/core#inScheme> :SupportSchemeTypeValue .


###  http://lpis.ec.europa.eu/registry/applicationschema/cap-iacs-base/code#SupportSchemeTypeValue/paymentForAreasWithNaturalConstraints
<http://lpis.ec.europa.eu/registry/applicationschema/cap-iacs-base/code#SupportSchemeTypeValue/paymentForAreasWithNaturalConstraints> rdf:type owl:NamedIndividual ,
                                                                                                                                               <http://lpis.ec.europa.eu/registry/applicationschema/cap-iacs-base#SupportSchemeTypeValue> ;
                                                                                                                                      rdfs:label "Payment for areas with natural constraints"@en ;
                                                                                                                                      <http://www.w3.org/2004/02/skos/core#definition> """Payment for areas with natural constraints

Payment to farmers who are entitled to BPS/SAPS and whose holdings are fully or partly situated in areas with natural constraints designated by Member States in accordance with Article 32(1) of Regulation (EU) No 1305/2013. 

NOTE
Rules in Title III, Chapter 4 of R 1307/2013"""@en ;
                                                                                                                                      <http://www.w3.org/2004/02/skos/core#inScheme> :SupportSchemeTypeValue .


###  http://lpis.ec.europa.eu/registry/applicationschema/cap-iacs-base/code#SupportSchemeTypeValue/paymentForYoungFarmers
<http://lpis.ec.europa.eu/registry/applicationschema/cap-iacs-base/code#SupportSchemeTypeValue/paymentForYoungFarmers> rdf:type owl:NamedIndividual ,
                                                                                                                                <http://lpis.ec.europa.eu/registry/applicationschema/cap-iacs-base#SupportSchemeTypeValue> ;
                                                                                                                       rdfs:label "Payment for young farmers"@en ;
                                                                                                                       <http://www.w3.org/2004/02/skos/core#definition> """Payment for young farmers

Member States shall grant an annual payment to young farmers who are entitled to a payment under the basic payment scheme or the single area payment scheme referred to in Chapter 1.

According to Title III, Chapter 5 of 1307/2013 Regulation it is a decoupled payment."""@en ;
                                                                                                                       <http://www.w3.org/2004/02/skos/core#inScheme> :SupportSchemeTypeValue .


###  http://lpis.ec.europa.eu/registry/applicationschema/cap-iacs-base/code#SupportSchemeTypeValue/posei
<http://lpis.ec.europa.eu/registry/applicationschema/cap-iacs-base/code#SupportSchemeTypeValue/posei> rdf:type owl:NamedIndividual ,
                                                                                                               <http://lpis.ec.europa.eu/registry/applicationschema/cap-iacs-base#SupportSchemeTypeValue> ;
                                                                                                      rdfs:label "Posei"@en ;
                                                                                                      <http://www.w3.org/2004/02/skos/core#definition> """POSEI

Chapter IV of Regulation (EU) No 228/2013 / Direct payments under measures established in the programmes.

NOTE
In full: \"Programme d'Options Spécifiques à l'Éloignement et l'Insularité\"."""@en ;
                                                                                                      <http://www.w3.org/2004/02/skos/core#inScheme> :SupportSchemeTypeValue .


###  http://lpis.ec.europa.eu/registry/applicationschema/cap-iacs-base/code#SupportSchemeTypeValue/redistributivePayment
<http://lpis.ec.europa.eu/registry/applicationschema/cap-iacs-base/code#SupportSchemeTypeValue/redistributivePayment> rdf:type owl:NamedIndividual ,
                                                                                                                               <http://lpis.ec.europa.eu/registry/applicationschema/cap-iacs-base#SupportSchemeTypeValue> ;
                                                                                                                      rdfs:label "Redistributive payment "@en ;
                                                                                                                      <http://www.w3.org/2004/02/skos/core#definition> """Redistributive payment

Conditional payment scheme decided by MS to grant an annual payment to farmers who are entitled to a payment under the basic payment scheme or under the single area payment scheme.

Art. 4 of Title III, Chapter 2 of R 1307/2013 sets the calculation method:
It shall be calculated 
	- each year by Member States
	- by multiplying a figure to be set by the Member State, which shall not be higher than 65 % of the national or regional average payment per hectare, by the number of payment entitlements or by the number of eligible hectares. 
The number of such payment entitlements or hectares shall not exceed a maximum to be set by Member States which shall not be higher than 30 hectares or the average size of agricultural holdings set out in Annex VIII if that average size exceeds 30 hectares in the Member State concerned.

NOTE
MS may establish a graduation in the number of hectares that is equally applied to every farmer.
-- Description --
Regulation / Decoupled payment."""@en ;
                                                                                                                      <http://www.w3.org/2004/02/skos/core#inScheme> :SupportSchemeTypeValue .


###  http://lpis.ec.europa.eu/registry/applicationschema/cap-iacs-base/code#SupportSchemeTypeValue/singleAreaPaymentScheme
<http://lpis.ec.europa.eu/registry/applicationschema/cap-iacs-base/code#SupportSchemeTypeValue/singleAreaPaymentScheme> rdf:type owl:NamedIndividual ,
                                                                                                                                 <http://lpis.ec.europa.eu/registry/applicationschema/cap-iacs-base#SupportSchemeTypeValue> ;
                                                                                                                        rdfs:label "Single area payment scheme"@en ;
                                                                                                                        <http://www.w3.org/2004/02/skos/core#definition> """Single area payment scheme 

Payment scheme based on the single area payment granted on an annual basis for each eligible hectare declared by the farmer in accordance with point (a) of the first subparagraph of Article 72(1) of Regulation (EU) No 1306/2013.

As described in Article 36 of 1307/2013 Regulation  it is a decoupled payment based on utilised land."""@en ;
                                                                                                                        <http://www.w3.org/2004/02/skos/core#inScheme> :SupportSchemeTypeValue .


###  http://lpis.ec.europa.eu/registry/applicationschema/cap-iacs-base/code#SupportSchemeTypeValue/smallFarmersScheme
<http://lpis.ec.europa.eu/registry/applicationschema/cap-iacs-base/code#SupportSchemeTypeValue/smallFarmersScheme> rdf:type owl:NamedIndividual ,
                                                                                                                            <http://lpis.ec.europa.eu/registry/applicationschema/cap-iacs-base#SupportSchemeTypeValue> ;
                                                                                                                   rdfs:label "Small farmers scheme"@en ;
                                                                                                                   <http://www.w3.org/2004/02/skos/core#definition> """Small farmers scheme

Member States may establish a scheme for small farmers in accordance with the conditions laid down in this Title.

According to Title V of 1307/2013 Regulation it is a decoupled payment."""@en ;
                                                                                                                   <http://www.w3.org/2004/02/skos/core#inScheme> :SupportSchemeTypeValue .


###  http://lpis.ec.europa.eu/registry/applicationschema/cap-iacs-base/code#SupportSchemeTypeValue/voluntaryCoupledSupport
<http://lpis.ec.europa.eu/registry/applicationschema/cap-iacs-base/code#SupportSchemeTypeValue/voluntaryCoupledSupport> rdf:type owl:NamedIndividual ,
                                                                                                                                 <http://lpis.ec.europa.eu/registry/applicationschema/cap-iacs-base#SupportSchemeTypeValue> ;
                                                                                                                        rdfs:label "Voluntary coupled support"@en ;
                                                                                                                        <http://www.w3.org/2004/02/skos/core#definition> """Voluntary coupled support

Member States may grant coupled support to farmers  for
	- cereals, 
	- oilseeds, 
	- protein crops, 
	- grain legumes, 
	- flax, 
	- hemp, 
	- rice, 
	- nuts, 
	- starch potato, 
	- milk and milk products, 
	- seeds, 
	- sheepmeat and goatmeat, 
	- beef and veal, 
	- olive oil, 
	- silkworms, 
	- dried fodder, 
	- hops, 
	- sugar beet, 
	- cane and chicory, 
	- fruit and vegetables and 
	- short rotation coppice.

NOTE
Details in Title IV, Chapter 1 of R 1307/2013."""@en ;
                                                                                                                        <http://www.w3.org/2004/02/skos/core#inScheme> :SupportSchemeTypeValue .


###  http://lpis.ec.europa.eu/registry/applicationschema/cap-iacs-base/code#TestTypeValue/basic
<http://lpis.ec.europa.eu/registry/applicationschema/cap-iacs-base/code#TestTypeValue/basic> rdf:type owl:NamedIndividual ,
                                                                                                      <http://lpis.ec.europa.eu/registry/applicationschema/cap-iacs-base#TestTypeValue> ;
                                                                                             rdfs:label "Basic test"@en ;
                                                                                             <http://www.w3.org/2004/02/skos/core#definition> """--Name--
Basic

-- Definition --
Basic test .

-- Description --
Basic tests (BT) provide limited testing of IUT in order to establish whether or not it is appropriate to perform more thorough testing. They may be used to determine the degree of conformance prior to deciding whether or not to proceed with thorough capability testing. Basic tests are simple capability tests. Conformance clauses should identify those test cases that may be used as a basic test.

NOTE1. BT shall be used to for detecting obvious cases of non-conformity.

NOTE2. BT shall be used as a preliminary step in order to decide whether or not to run capability tests."""@en ;
                                                                                             <http://www.w3.org/2004/02/skos/core#inScheme> :TestTypeValue .


###  http://lpis.ec.europa.eu/registry/applicationschema/cap-iacs-base/code#TestTypeValue/capability
<http://lpis.ec.europa.eu/registry/applicationschema/cap-iacs-base/code#TestTypeValue/capability> rdf:type owl:NamedIndividual ,
                                                                                                           <http://lpis.ec.europa.eu/registry/applicationschema/cap-iacs-base#TestTypeValue> ;
                                                                                                  rdfs:label "Capability test"@en ;
                                                                                                  <http://www.w3.org/2004/02/skos/core#definition> """--Name--
Capability

-- Definition --
Capability test.

-- Description --
Capability tests (CT), should investigate an implementation as thoroughly as it is practical over the full range of conformance requirements specified in a standard/legal act. Capability tests should be provided to check the mandatory capabilities and those optional capabilities that are identified in the ICS as being supported by the IUT.

NOTE 1. CT shall be used to check that the capabilities of the IUT are consistent with the conformance requirements, that is, to determine whether or not an implementation conforms.

NOTE 2. CT shall be used to investigate causes of failure."""@en ;
                                                                                                  <http://www.w3.org/2004/02/skos/core#inScheme> :TestTypeValue .


###  http://lpis.ec.europa.eu/registry/applicationschema/cap-iacs-base/code#TestVerdictValue/fail
<http://lpis.ec.europa.eu/registry/applicationschema/cap-iacs-base/code#TestVerdictValue/fail> rdf:type owl:NamedIndividual ,
                                                                                                        <http://lpis.ec.europa.eu/registry/applicationschema/cap-iacs-base#TestVerdictValue> ;
                                                                                               rdfs:label "Fail verdict"@en ;
                                                                                               <http://www.w3.org/2004/02/skos/core#definition> """--Name--
Fail

-- Definition --
Fail verdict to indicate that SUT does not fulfil the requirements.

-- Description --
Test verdict of non-conformance . Failure to fulfil one or more requirements specified."""@en ;
                                                                                               <http://www.w3.org/2004/02/skos/core#inScheme> :TestVerdictValue .


###  http://lpis.ec.europa.eu/registry/applicationschema/cap-iacs-base/code#TestVerdictValue/inconclusive
<http://lpis.ec.europa.eu/registry/applicationschema/cap-iacs-base/code#TestVerdictValue/inconclusive> rdf:type owl:NamedIndividual ,
                                                                                                                <http://lpis.ec.europa.eu/registry/applicationschema/cap-iacs-base#TestVerdictValue> ;
                                                                                                       rdfs:label "Inconclusive verdict"@en ;
                                                                                                       <http://www.w3.org/2004/02/skos/core#definition> """--Name--
Inconclusive

-- Definition --
A value “inconclusive” indicates that the testing process has not yet yield a verdict.


-- Description --
Neither fail nor pass verdict can be assigned based on the test."""@en ;
                                                                                                       <http://www.w3.org/2004/02/skos/core#inScheme> :TestVerdictValue .


###  http://lpis.ec.europa.eu/registry/applicationschema/cap-iacs-base/code#TestVerdictValue/pass
<http://lpis.ec.europa.eu/registry/applicationschema/cap-iacs-base/code#TestVerdictValue/pass> rdf:type owl:NamedIndividual ,
                                                                                                        <http://lpis.ec.europa.eu/registry/applicationschema/cap-iacs-base#TestVerdictValue> ;
                                                                                               rdfs:label "Pas verdict"@en ;
                                                                                               <http://www.w3.org/2004/02/skos/core#definition> """--Name--
Pass

-- Definition --
Pass verdict to indicate that the tested requirements are fulfilled.

-- Description --
Test verdict of conformance."""@en ;
                                                                                               <http://www.w3.org/2004/02/skos/core#inScheme> :TestVerdictValue .


###  http://lpis.ec.europa.eu/registry/applicationschema/cap-iacs-base/code#TestingTypeValue/automated
<http://lpis.ec.europa.eu/registry/applicationschema/cap-iacs-base/code#TestingTypeValue/automated> rdf:type owl:NamedIndividual ,
                                                                                                             <http://lpis.ec.europa.eu/registry/applicationschema/cap-iacs-base#TestingTypeValue> ;
                                                                                                    rdfs:label "Automated testing"@en ;
                                                                                                    <http://www.w3.org/2004/02/skos/core#definition> """--Name--
Automated

-- Definition --
Automated test.

-- Description --
Automated testing may implement the required tests as a software system using either verification testing or falsification testing."""@en ;
                                                                                                    <http://www.w3.org/2004/02/skos/core#inScheme> :TestingTypeValue .


###  http://lpis.ec.europa.eu/registry/applicationschema/cap-iacs-base/code#TestingTypeValue/manual
<http://lpis.ec.europa.eu/registry/applicationschema/cap-iacs-base/code#TestingTypeValue/manual> rdf:type owl:NamedIndividual ,
                                                                                                          <http://lpis.ec.europa.eu/registry/applicationschema/cap-iacs-base#TestingTypeValue> ;
                                                                                                 rdfs:label "Manual testing"@en ;
                                                                                                 <http://www.w3.org/2004/02/skos/core#definition> """--Name--
Manual

-- Definition --
Manual testing.

-- Description --
Manual testing may be required when automated testing is too complex and/or human judgement is required. Manual testing should be used only for those standards where automatic testing is not viable."""@en ;
                                                                                                 <http://www.w3.org/2004/02/skos/core#inScheme> :TestingTypeValue .


###  http://lpis.ec.europa.eu/registry/applicationschema/cap-iacs-base/code#VarietalNameValue/abelia
<http://lpis.ec.europa.eu/registry/applicationschema/cap-iacs-base/code#VarietalNameValue/abelia> rdf:type owl:NamedIndividual ,
                                                                                                           <http://lpis.ec.europa.eu/registry/applicationschema/cap-iacs-base#VarietalNameValue> ;
                                                                                                  rdfs:label "H - 1.2  Abelia"@en ;
                                                                                                  <http://www.w3.org/2004/02/skos/core#definition> """-- Definition --
H - 1.2  Abelia
-- Description --
H - 1.2 Allium cepa L. Cepa group - Onion, Echalion /  Abelia.
NOTE. Initial value: Abelia
NOTE. MS - NL (Netherlands)."""@en ;
                                                                                                  <http://www.w3.org/2004/02/skos/core#inScheme> :VarietalNameValue .


###  http://lpis.ec.europa.eu/registry/applicationschema/cap-iacs-base/code#VarietalNameValue/accent
<http://lpis.ec.europa.eu/registry/applicationschema/cap-iacs-base/code#VarietalNameValue/accent> rdf:type owl:NamedIndividual ,
                                                                                                           <http://lpis.ec.europa.eu/registry/applicationschema/cap-iacs-base#VarietalNameValue> ;
                                                                                                  rdfs:label "H - 1.2  Accent"@en ;
                                                                                                  <http://www.w3.org/2004/02/skos/core#definition> """-- Definition --
H - 1.2  Accent
-- Description --
H - 1.2 Allium cepa L. Cepa group - Onion, Echalion /  Accent.
NOTE. Initial value: Accent
NOTE. MS - NL (Netherlands)."""@en ;
                                                                                                  <http://www.w3.org/2004/02/skos/core#inScheme> :VarietalNameValue .


###  http://lpis.ec.europa.eu/registry/applicationschema/cap-iacs-base/code#VarietalNameValue/adonis
<http://lpis.ec.europa.eu/registry/applicationschema/cap-iacs-base/code#VarietalNameValue/adonis> rdf:type owl:NamedIndividual ,
                                                                                                           <http://lpis.ec.europa.eu/registry/applicationschema/cap-iacs-base#VarietalNameValue> ;
                                                                                                  rdfs:label "H - 1.2  Adonis"@en ;
                                                                                                  <http://www.w3.org/2004/02/skos/core#definition> """-- Definition --
H - 1.2  Adonis
-- Description --
H - 1.2 Allium cepa L. Cepa group - Onion, Echalion /  Adonis.
NOTE. Initial value: Adonis
NOTE. MS - NL (Netherlands)."""@en ;
                                                                                                  <http://www.w3.org/2004/02/skos/core#inScheme> :VarietalNameValue .


###  http://lpis.ec.europa.eu/registry/applicationschema/cap-iacs-base/code#VarietalNameValue/ambition
<http://lpis.ec.europa.eu/registry/applicationschema/cap-iacs-base/code#VarietalNameValue/ambition> rdf:type owl:NamedIndividual ,
                                                                                                             <http://lpis.ec.europa.eu/registry/applicationschema/cap-iacs-base#VarietalNameValue> ;
                                                                                                    rdfs:label "H - 1.1  Ambition"@en ;
                                                                                                    <http://www.w3.org/2004/02/skos/core#definition> """-- Definition --
H - 1.1  Ambition
-- Description --
H - 1.1 Allium cepa L. Aggregatum group - Shallot /  Ambition.
NOTE. Initial value: Ambition
NOTE. MS - NL (Netherlands)."""@en ;
                                                                                                    <http://www.w3.org/2004/02/skos/core#inScheme> :VarietalNameValue .


###  http://lpis.ec.europa.eu/registry/applicationschema/cap-iacs-base/code#VarietalNameValue/armador
<http://lpis.ec.europa.eu/registry/applicationschema/cap-iacs-base/code#VarietalNameValue/armador> rdf:type owl:NamedIndividual ,
                                                                                                            <http://lpis.ec.europa.eu/registry/applicationschema/cap-iacs-base#VarietalNameValue> ;
                                                                                                   rdfs:label "H - 1.1  Armador"@en ;
                                                                                                   <http://www.w3.org/2004/02/skos/core#definition> """-- Definition --
H - 1.1  Armador
-- Description --
H - 1.1 Allium cepa L. Aggregatum group - Shallot /  Armador.
NOTE. Initial value: Armador
NOTE. MS - NL (Netherlands)."""@en ;
                                                                                                   <http://www.w3.org/2004/02/skos/core#inScheme> :VarietalNameValue .


###  http://lpis.ec.europa.eu/registry/applicationschema/cap-iacs-base/code#VarietalNameValue/biztro
<http://lpis.ec.europa.eu/registry/applicationschema/cap-iacs-base/code#VarietalNameValue/biztro> rdf:type owl:NamedIndividual ,
                                                                                                           <http://lpis.ec.europa.eu/registry/applicationschema/cap-iacs-base#VarietalNameValue> ;
                                                                                                  rdfs:label "H - 1.1  Biztro"@en ;
                                                                                                  <http://www.w3.org/2004/02/skos/core#definition> """-- Definition --
H - 1.1  Biztro
-- Description --
H - 1.1 Allium cepa L. Aggregatum group - Shallot /  Biztro.
NOTE. Initial value: Biztro
NOTE. MS - NL (Netherlands)."""@en ;
                                                                                                  <http://www.w3.org/2004/02/skos/core#inScheme> :VarietalNameValue .


###  http://lpis.ec.europa.eu/registry/applicationschema/cap-iacs-base/code#WeekdayValue/friday
<http://lpis.ec.europa.eu/registry/applicationschema/cap-iacs-base/code#WeekdayValue/friday> rdf:type owl:NamedIndividual ,
                                                                                                      <http://lpis.ec.europa.eu/registry/applicationschema/cap-iacs-base#WeekdayValue> ;
                                                                                             rdfs:label "Friday"@en ;
                                                                                             <http://www.w3.org/2004/02/skos/core#definition> """-- Definition --
Friday.
-- Description --
Item description."""@en ;
                                                                                             <http://www.w3.org/2004/02/skos/core#inScheme> :WeekdayValue .


###  http://lpis.ec.europa.eu/registry/applicationschema/cap-iacs-base/code#WeekdayValue/monday
<http://lpis.ec.europa.eu/registry/applicationschema/cap-iacs-base/code#WeekdayValue/monday> rdf:type owl:NamedIndividual ,
                                                                                                      <http://lpis.ec.europa.eu/registry/applicationschema/cap-iacs-base#WeekdayValue> ;
                                                                                             rdfs:label "Monday"@en ;
                                                                                             <http://www.w3.org/2004/02/skos/core#definition> """-- Definition --
Monday.
-- Description --
Item description."""@en ;
                                                                                             <http://www.w3.org/2004/02/skos/core#inScheme> :WeekdayValue .


###  http://lpis.ec.europa.eu/registry/applicationschema/cap-iacs-base/code#WeekdayValue/saturday
<http://lpis.ec.europa.eu/registry/applicationschema/cap-iacs-base/code#WeekdayValue/saturday> rdf:type owl:NamedIndividual ,
                                                                                                        <http://lpis.ec.europa.eu/registry/applicationschema/cap-iacs-base#WeekdayValue> ;
                                                                                               rdfs:label "Saturday"@en ;
                                                                                               <http://www.w3.org/2004/02/skos/core#definition> """-- Definition --
Saturday.
-- Description --
Item description."""@en ;
                                                                                               <http://www.w3.org/2004/02/skos/core#inScheme> :WeekdayValue .


###  http://lpis.ec.europa.eu/registry/applicationschema/cap-iacs-base/code#WeekdayValue/sunday
<http://lpis.ec.europa.eu/registry/applicationschema/cap-iacs-base/code#WeekdayValue/sunday> rdf:type owl:NamedIndividual ,
                                                                                                      <http://lpis.ec.europa.eu/registry/applicationschema/cap-iacs-base#WeekdayValue> ;
                                                                                             rdfs:label "Sunday"@en ;
                                                                                             <http://www.w3.org/2004/02/skos/core#definition> """-- Definition --
Sunday.
-- Description --
Item description."""@en ;
                                                                                             <http://www.w3.org/2004/02/skos/core#inScheme> :WeekdayValue .


###  http://lpis.ec.europa.eu/registry/applicationschema/cap-iacs-base/code#WeekdayValue/thursday
<http://lpis.ec.europa.eu/registry/applicationschema/cap-iacs-base/code#WeekdayValue/thursday> rdf:type owl:NamedIndividual ,
                                                                                                        <http://lpis.ec.europa.eu/registry/applicationschema/cap-iacs-base#WeekdayValue> ;
                                                                                               rdfs:label "Thursday"@en ;
                                                                                               <http://www.w3.org/2004/02/skos/core#definition> """-- Definition --
Thursday.
-- Description --
Item description."""@en ;
                                                                                               <http://www.w3.org/2004/02/skos/core#inScheme> :WeekdayValue .


###  http://lpis.ec.europa.eu/registry/applicationschema/cap-iacs-base/code#WeekdayValue/tuesday
<http://lpis.ec.europa.eu/registry/applicationschema/cap-iacs-base/code#WeekdayValue/tuesday> rdf:type owl:NamedIndividual ,
                                                                                                       <http://lpis.ec.europa.eu/registry/applicationschema/cap-iacs-base#WeekdayValue> ;
                                                                                              rdfs:label "Tuesday"@en ;
                                                                                              <http://www.w3.org/2004/02/skos/core#definition> """-- Definition --
Tuesday.
-- Description --
Item description."""@en ;
                                                                                              <http://www.w3.org/2004/02/skos/core#inScheme> :WeekdayValue .


###  http://lpis.ec.europa.eu/registry/applicationschema/cap-iacs-base/code#WeekdayValue/wednesday
<http://lpis.ec.europa.eu/registry/applicationschema/cap-iacs-base/code#WeekdayValue/wednesday> rdf:type owl:NamedIndividual ,
                                                                                                         <http://lpis.ec.europa.eu/registry/applicationschema/cap-iacs-base#WeekdayValue> ;
                                                                                                rdfs:label "Wednesday"@en ;
                                                                                                <http://www.w3.org/2004/02/skos/core#definition> """-- Definition --
Wednesday.
-- Description --
Item description."""@en ;
                                                                                                <http://www.w3.org/2004/02/skos/core#inScheme> :WeekdayValue .


###  Generated by the OWL API (version 5.1.18) https://github.com/owlcs/owlapi/
