@prefix : <http://lpis.ec.europa.eu/registry/applicationschema/cap-iacs-parcel/code#> .
@prefix owl: <http://www.w3.org/2002/07/owl#> .
@prefix rdf: <http://www.w3.org/1999/02/22-rdf-syntax-ns#> .
@prefix xml: <http://www.w3.org/XML/1998/namespace> .
@prefix xsd: <http://www.w3.org/2001/XMLSchema#> .
@prefix rdfs: <http://www.w3.org/2000/01/rdf-schema#> .
@base <http://lpis.ec.europa.eu/registry/applicationschema/cap-iacs-parcel/code#> .

<http://lpis.ec.europa.eu/registry/applicationschema/cap-iacs-parcel/code> rdf:type owl:Ontology ;
                                                                            owl:versionIRI <http://lpis.ec.europa.eu/registry/applicationschema/cap-iacs-base/code/3.0> ;
                                                                            <http://purl.org/dc/terms/creator> _:genid1 ;
                                                                            <http://purl.org/dc/terms/description> "Ontology of the identification system for agricultural parcels code lists used in IACS, generated from the transformation of the corresponding JRC application schema"@en ;
                                                                            <http://purl.org/dc/terms/rights> "This ontology is distributed under Creative Commons Attribution 4.0 License - http://creativecommons.org/licenses/by/4.0"@en ;
                                                                            <http://purl.org/dc/terms/source> "JRC IACS application schema. https://doi.org/10.1016/j.landusepol.2016.05.023"@en ;
                                                                            <http://purl.org/dc/terms/title> "JRC IACS - Identification System for Agricultural Parcels Code Lists"@en ;
                                                                            rdfs:label "Identification system for agricultural parcels code lists"@en ;
                                                                            owl:versionInfo "3.0" .

_:genid1 <http://schema.org/affiliation> [ <http://xmlns.com/foaf/0.1/name> "PSNC"
                                          ] ;
          rdfs:seeAlso <http://orcid.org/0000-0003-4289-4922> ;
          <http://xmlns.com/foaf/0.1/name> "Raul Palma" .

#################################################################
#    Annotation properties
#################################################################

###  http://purl.org/dc/terms/creator
<http://purl.org/dc/terms/creator> rdf:type owl:AnnotationProperty .


###  http://purl.org/dc/terms/description
<http://purl.org/dc/terms/description> rdf:type owl:AnnotationProperty .


###  http://purl.org/dc/terms/isFormatOf
<http://purl.org/dc/terms/isFormatOf> rdf:type owl:AnnotationProperty .


###  http://purl.org/dc/terms/rights
<http://purl.org/dc/terms/rights> rdf:type owl:AnnotationProperty .


###  http://purl.org/dc/terms/source
<http://purl.org/dc/terms/source> rdf:type owl:AnnotationProperty .


###  http://purl.org/dc/terms/title
<http://purl.org/dc/terms/title> rdf:type owl:AnnotationProperty .


###  http://schema.org/affiliation
<http://schema.org/affiliation> rdf:type owl:AnnotationProperty .


###  http://www.w3.org/2004/02/skos/core#definition
<http://www.w3.org/2004/02/skos/core#definition> rdf:type owl:AnnotationProperty .


###  http://www.w3.org/2004/02/skos/core#inScheme
<http://www.w3.org/2004/02/skos/core#inScheme> rdf:type owl:AnnotationProperty .


###  http://xmlns.com/foaf/0.1/name
<http://xmlns.com/foaf/0.1/name> rdf:type owl:AnnotationProperty .


#################################################################
#    Classes
#################################################################

###  http://lpis.ec.europa.eu/registry/applicationschema/cap-iacs-parcel#AcceptanceNumberValue
<http://lpis.ec.europa.eu/registry/applicationschema/cap-iacs-parcel#AcceptanceNumberValue> rdf:type owl:Class .


###  http://lpis.ec.europa.eu/registry/applicationschema/cap-iacs-parcel#AgriculturalAreaTypeValue
<http://lpis.ec.europa.eu/registry/applicationschema/cap-iacs-parcel#AgriculturalAreaTypeValue> rdf:type owl:Class .


###  http://lpis.ec.europa.eu/registry/applicationschema/cap-iacs-parcel#ContaminationTypeValue
<http://lpis.ec.europa.eu/registry/applicationschema/cap-iacs-parcel#ContaminationTypeValue> rdf:type owl:Class .


###  http://lpis.ec.europa.eu/registry/applicationschema/cap-iacs-parcel#CriticalDefectTypeEfaValue
<http://lpis.ec.europa.eu/registry/applicationschema/cap-iacs-parcel#CriticalDefectTypeEfaValue> rdf:type owl:Class .


###  http://lpis.ec.europa.eu/registry/applicationschema/cap-iacs-parcel#CriticalDefectTypeValue
<http://lpis.ec.europa.eu/registry/applicationschema/cap-iacs-parcel#CriticalDefectTypeValue> rdf:type owl:Class .


###  http://lpis.ec.europa.eu/registry/applicationschema/cap-iacs-parcel#DataQualityMeasureNameValue
<http://lpis.ec.europa.eu/registry/applicationschema/cap-iacs-parcel#DataQualityMeasureNameValue> rdf:type owl:Class .


###  http://lpis.ec.europa.eu/registry/applicationschema/cap-iacs-parcel#DataQualityMeasureTypeEfaValue
<http://lpis.ec.europa.eu/registry/applicationschema/cap-iacs-parcel#DataQualityMeasureTypeEfaValue> rdf:type owl:Class .


###  http://lpis.ec.europa.eu/registry/applicationschema/cap-iacs-parcel#DataQualityMeasureTypeEtsValue
<http://lpis.ec.europa.eu/registry/applicationschema/cap-iacs-parcel#DataQualityMeasureTypeEtsValue> rdf:type owl:Class .


###  http://lpis.ec.europa.eu/registry/applicationschema/cap-iacs-parcel#DataQualityMeasureTypeIuiCcValue
<http://lpis.ec.europa.eu/registry/applicationschema/cap-iacs-parcel#DataQualityMeasureTypeIuiCcValue> rdf:type owl:Class .


###  http://lpis.ec.europa.eu/registry/applicationschema/cap-iacs-parcel#DataQualityMeasureTypeIuiEfaValue
<http://lpis.ec.europa.eu/registry/applicationschema/cap-iacs-parcel#DataQualityMeasureTypeIuiEfaValue> rdf:type owl:Class .


###  http://lpis.ec.europa.eu/registry/applicationschema/cap-iacs-parcel#DataQualityMeasureTypeIuiValue
<http://lpis.ec.europa.eu/registry/applicationschema/cap-iacs-parcel#DataQualityMeasureTypeIuiValue> rdf:type owl:Class .


###  http://lpis.ec.europa.eu/registry/applicationschema/cap-iacs-parcel#DataQualityMeasureValueStructureValue
<http://lpis.ec.europa.eu/registry/applicationschema/cap-iacs-parcel#DataQualityMeasureValueStructureValue> rdf:type owl:Class .


###  http://lpis.ec.europa.eu/registry/applicationschema/cap-iacs-parcel#EcologicalFocusAreaEquivalentPracticeTypeValue
<http://lpis.ec.europa.eu/registry/applicationschema/cap-iacs-parcel#EcologicalFocusAreaEquivalentPracticeTypeValue> rdf:type owl:Class .


###  http://lpis.ec.europa.eu/registry/applicationschema/cap-iacs-parcel#EcologicalFocusAreaTypeValue
<http://lpis.ec.europa.eu/registry/applicationschema/cap-iacs-parcel#EcologicalFocusAreaTypeValue> rdf:type owl:Class .


###  http://lpis.ec.europa.eu/registry/applicationschema/cap-iacs-parcel#HomogeneityTypeValue
<http://lpis.ec.europa.eu/registry/applicationschema/cap-iacs-parcel#HomogeneityTypeValue> rdf:type owl:Class .


###  http://lpis.ec.europa.eu/registry/applicationschema/cap-iacs-parcel#InspectionMethodValue
<http://lpis.ec.europa.eu/registry/applicationschema/cap-iacs-parcel#InspectionMethodValue> rdf:type owl:Class .


###  http://lpis.ec.europa.eu/registry/applicationschema/cap-iacs-parcel#LandscapeFeatureValueType
<http://lpis.ec.europa.eu/registry/applicationschema/cap-iacs-parcel#LandscapeFeatureValueType> rdf:type owl:Class .


###  http://lpis.ec.europa.eu/registry/applicationschema/cap-iacs-parcel#LimitingQualityValue
<http://lpis.ec.europa.eu/registry/applicationschema/cap-iacs-parcel#LimitingQualityValue> rdf:type owl:Class .


###  http://lpis.ec.europa.eu/registry/applicationschema/cap-iacs-parcel#LotSizeValue
<http://lpis.ec.europa.eu/registry/applicationschema/cap-iacs-parcel#LotSizeValue> rdf:type owl:Class .


###  http://lpis.ec.europa.eu/registry/applicationschema/cap-iacs-parcel#ProRataCategoryValue
<http://lpis.ec.europa.eu/registry/applicationschema/cap-iacs-parcel#ProRataCategoryValue> rdf:type owl:Class .


###  http://lpis.ec.europa.eu/registry/applicationschema/cap-iacs-parcel#SampleSizeValue
<http://lpis.ec.europa.eu/registry/applicationschema/cap-iacs-parcel#SampleSizeValue> rdf:type owl:Class .


###  http://lpis.ec.europa.eu/registry/applicationschema/cap-iacs-parcel#SkippingReasonTypeValue
<http://lpis.ec.europa.eu/registry/applicationschema/cap-iacs-parcel#SkippingReasonTypeValue> rdf:type owl:Class .


###  http://lpis.ec.europa.eu/registry/applicationschema/cap-iacs-parcel#TechnicalReasonValue
<http://lpis.ec.europa.eu/registry/applicationschema/cap-iacs-parcel#TechnicalReasonValue> rdf:type owl:Class .


###  http://lpis.ec.europa.eu/registry/applicationschema/cap-iacs-parcel#TestTypeMtsValue
<http://lpis.ec.europa.eu/registry/applicationschema/cap-iacs-parcel#TestTypeMtsValue> rdf:type owl:Class .


###  http://www.w3.org/2004/02/skos/core#ConceptScheme
<http://www.w3.org/2004/02/skos/core#ConceptScheme> rdf:type owl:Class .


#################################################################
#    Individuals
#################################################################

###  http://lpis.ec.europa.eu/registry/applicationschema/cap-iacs-parcel/code#AcceptanceNumberValue
:AcceptanceNumberValue rdf:type owl:NamedIndividual ,
                                <http://www.w3.org/2004/02/skos/core#ConceptScheme> ;
                       <http://purl.org/dc/terms/isFormatOf> <http://lpis.ec.europa.eu/registry/applicationschema/cap-iacs-parcel#AcceptanceNumberValue> ;
                       rdfs:label "List of possible acceptance values"@en ;
                       <http://www.w3.org/2004/02/skos/core#definition> """--Name--
Acceptance number value

-- Definition --
List of possible acceptance values.

-- Description --
Acceptance values are selected based on the sample size and the limiting quality values defined in ISO 2859-2:1985 Sampling procedures for inspection by attributes, Part 2: Sampling plans indexed by limiting quality (LQ) for isolated lot inspection."""@en .


###  http://lpis.ec.europa.eu/registry/applicationschema/cap-iacs-parcel/code#AgriculturalAreaTypeValue
:AgriculturalAreaTypeValue rdf:type owl:NamedIndividual ,
                                    <http://www.w3.org/2004/02/skos/core#ConceptScheme> ;
                           <http://purl.org/dc/terms/isFormatOf> <http://lpis.ec.europa.eu/registry/applicationschema/cap-iacs-parcel#AgriculturalAreaTypeValue> ;
                           rdfs:label "List of agricultural area type values"@en ;
                           <http://www.w3.org/2004/02/skos/core#definition> """--Name--
Agricultural area type value

-- Definition --
Types of agricultural area.

-- Description --
List of agricultural area type values.  QAF: Eligibility profile value.

NOTE 1:  According to DSCG/2014/33  arableLand, permanentCrop and permanetGrassland are the minimum level of details of land cover types needed for distinction of agricultural area.

NOTE 2:  sensitivePermanetGrassland type to be protected under greening  is required by Art.5(2)(d) of Regulation (EU) No 640/2014.

NOTE 3: This code list can be extended with narrower categories replacing the listed broader code list values. 

 

NOTE 4: For the purposes of ETS MS/Region may use the same code list applied in IACS, or a generalised one. For the purposes of ETS the generalised code list is sufficient.
When detailed  (crop level) agricultural area types are used, in course of MTS the mapping to the general categories listed in the LCM has to be given.

EXAMPLE: Sensitive permanent grassland may be replaced by any sub-category (narrower value) referred to in Art. 41 of (EU) R 639/2014."""@en .


###  http://lpis.ec.europa.eu/registry/applicationschema/cap-iacs-parcel/code#ContaminationTypeValue
:ContaminationTypeValue rdf:type owl:NamedIndividual ,
                                 <http://www.w3.org/2004/02/skos/core#ConceptScheme> ;
                        <http://purl.org/dc/terms/isFormatOf> <http://lpis.ec.europa.eu/registry/applicationschema/cap-iacs-parcel#ContaminationTypeValue> ;
                        rdfs:label "Contamination type value list"@en ;
                        <http://www.w3.org/2004/02/skos/core#definition> """--Name--
Contamination type value

-- Definition --
List of contamination type values.

-- Description --
NOTE: the code list is centrally managed by the Commission services and cannot be extended by MS/Regions."""@en .


###  http://lpis.ec.europa.eu/registry/applicationschema/cap-iacs-parcel/code#CriticalDefectTypeEfaValue
:CriticalDefectTypeEfaValue rdf:type owl:NamedIndividual ,
                                     <http://www.w3.org/2004/02/skos/core#ConceptScheme> ;
                            <http://purl.org/dc/terms/isFormatOf> <http://lpis.ec.europa.eu/registry/applicationschema/cap-iacs-parcel#CriticalDefectTypeEfaValue> ;
                            rdfs:label "Critical defect type value"@en ;
                            <http://www.w3.org/2004/02/skos/core#definition> """--Name--
EFA critical defect type

-- Definition --
This is a placeholder only; currently not to be implemented.

-- Description --
List of error types leading to obstruction of usability of the item under inspection (critical defect)."""@en .


###  http://lpis.ec.europa.eu/registry/applicationschema/cap-iacs-parcel/code#CriticalDefectTypeValue
:CriticalDefectTypeValue rdf:type owl:NamedIndividual ,
                                  <http://www.w3.org/2004/02/skos/core#ConceptScheme> ;
                         <http://purl.org/dc/terms/isFormatOf> <http://lpis.ec.europa.eu/registry/applicationschema/cap-iacs-parcel#CriticalDefectTypeValue> ;
                         rdfs:label "Critical defect type value"@en ;
                         <http://www.w3.org/2004/02/skos/core#definition> """--Name--
Critical defect type value

-- Definition --
List of critical defect type values.

-- Description --
List of error types leading to obstruction of usability of the item under inspection (critical defect)."""@en .


###  http://lpis.ec.europa.eu/registry/applicationschema/cap-iacs-parcel/code#DataQualityMeasureNameValue
:DataQualityMeasureNameValue rdf:type owl:NamedIndividual ,
                                      <http://www.w3.org/2004/02/skos/core#ConceptScheme> ;
                             <http://purl.org/dc/terms/isFormatOf> <http://lpis.ec.europa.eu/registry/applicationschema/cap-iacs-parcel#DataQualityMeasureNameValue> ;
                             rdfs:label "ETS data quality measure name list"@en ;
                             <http://www.w3.org/2004/02/skos/core#definition> """--Name--
Data quality measure name value

-- Definition --
Data quality measures applicable for LPIS quality assessment process.

-- Description --
This is the unified code list of all DQM applied at item and sample level."""@en .


###  http://lpis.ec.europa.eu/registry/applicationschema/cap-iacs-parcel/code#DataQualityMeasureTypeEfaValue
:DataQualityMeasureTypeEfaValue rdf:type owl:NamedIndividual ,
                                         <http://www.w3.org/2004/02/skos/core#ConceptScheme> ;
                                <http://purl.org/dc/terms/isFormatOf> <http://lpis.ec.europa.eu/registry/applicationschema/cap-iacs-parcel#DataQualityMeasureTypeEfaValue> ;
                                rdfs:label "EFA data quality measure type list"@en ;
                                <http://www.w3.org/2004/02/skos/core#definition> """--Name--
Data quality measure types applicable to the EFA inspection sample

-- Definition --
This is a placeholder only; currently not to be implemented.

-- Description --
Data quality measure type list for EFA sample. 
NOTE. Full description of each value must be provided in DQM_Measure."""@en .


###  http://lpis.ec.europa.eu/registry/applicationschema/cap-iacs-parcel/code#DataQualityMeasureTypeEtsValue
:DataQualityMeasureTypeEtsValue rdf:type owl:NamedIndividual ,
                                         <http://www.w3.org/2004/02/skos/core#ConceptScheme> ;
                                <http://purl.org/dc/terms/isFormatOf> <http://lpis.ec.europa.eu/registry/applicationschema/cap-iacs-parcel#DataQualityMeasureTypeEtsValue> ;
                                rdfs:label "DTS data quality measure type list"@en ;
                                <http://www.w3.org/2004/02/skos/core#definition> """--Name--
Data quality measure types applicable for ETS sample

-- Definition --
Data quality measures applicable for LPIS quality assessment process at sample level.

--Description--
By exclusion of misclassification  matrix the elements of the code list are user defined data quality measures to assess quality of the ETS sample. Misclassification matrix comes directly from ISO 19157:2013."""@en .


###  http://lpis.ec.europa.eu/registry/applicationschema/cap-iacs-parcel/code#DataQualityMeasureTypeIuiCcValue
:DataQualityMeasureTypeIuiCcValue rdf:type owl:NamedIndividual ,
                                           <http://www.w3.org/2004/02/skos/core#ConceptScheme> ;
                                  <http://purl.org/dc/terms/isFormatOf> <http://lpis.ec.europa.eu/registry/applicationschema/cap-iacs-parcel#DataQualityMeasureTypeIuiCcValue> ;
                                  rdfs:label "IUI CC data quality measure type list"@en ;
                                  <http://www.w3.org/2004/02/skos/core#definition> """--Name--
Classification Correctness DQM value

-- Definition --
Data quality measure describing the correctness of classification of the feature type.

-- Description --
The classification shall be performed according to the types defined in the eligibility profile. This DQM is applicable for evaluating the classification correctness of agricultural land(s) and the landscape feature(s) present in the item under inspection.  

NOTE: This is a new quality measure from ETS v 6.0 on."""@en .


###  http://lpis.ec.europa.eu/registry/applicationschema/cap-iacs-parcel/code#DataQualityMeasureTypeIuiEfaValue
:DataQualityMeasureTypeIuiEfaValue rdf:type owl:NamedIndividual ,
                                            <http://www.w3.org/2004/02/skos/core#ConceptScheme> ;
                                   <http://purl.org/dc/terms/isFormatOf> <http://lpis.ec.europa.eu/registry/applicationschema/cap-iacs-parcel#DataQualityMeasureTypeIuiEfaValue> ;
                                   rdfs:label "IUI EFA data quality measure type list"@en ;
                                   <http://www.w3.org/2004/02/skos/core#definition> """--Name--
Data quality measure types applicable to EFA items

-- Definition --
This is a placeholder only; currently not to be implemented.

-- Description --
Data quality measure type list for items under inspection.
NOTE. Full description of each value must be provided in DQM_Measure."""@en .


###  http://lpis.ec.europa.eu/registry/applicationschema/cap-iacs-parcel/code#DataQualityMeasureTypeIuiValue
:DataQualityMeasureTypeIuiValue rdf:type owl:NamedIndividual ,
                                         <http://www.w3.org/2004/02/skos/core#ConceptScheme> ;
                                <http://purl.org/dc/terms/isFormatOf> <http://lpis.ec.europa.eu/registry/applicationschema/cap-iacs-parcel#DataQualityMeasureTypeIuiValue> ;
                                rdfs:label "IUI data quality measure type list"@en ;
                                <http://www.w3.org/2004/02/skos/core#definition> """--Name--
Data quality measure types applicable to items under inspection

-- Definition --
List of data quality measure types applicable for inspecting items of reference parcels.

-- Description --
These user defined data quality measures are used to assess the quality of reference parcels in terms of area measurement accuracy and thematic classification correctness."""@en .


###  http://lpis.ec.europa.eu/registry/applicationschema/cap-iacs-parcel/code#DataQualityMeasureValueStructureValue
:DataQualityMeasureValueStructureValue rdf:type owl:NamedIndividual ,
                                                <http://www.w3.org/2004/02/skos/core#ConceptScheme> ;
                                       <http://purl.org/dc/terms/isFormatOf> <http://lpis.ec.europa.eu/registry/applicationschema/cap-iacs-parcel#DataQualityMeasureValueStructureValue> ;
                                       rdfs:label "Data quality measure value structure value list"@en ;
                                       <http://www.w3.org/2004/02/skos/core#definition> """--Name--
Data quality Measure value structure

--Definition--
Structure used for presenting multiple values of DQ results.

--Description--
A result may consist of multiple values. In such cases, the result shall be structured using the value structure as given in C.3.3 of ISO 19157:2013. 

EXAMPLE: The results for misclassification shall be given as a matrix."""@en .


###  http://lpis.ec.europa.eu/registry/applicationschema/cap-iacs-parcel/code#EcologicalFocusAreaEquivalentPracticeTypeValue
:EcologicalFocusAreaEquivalentPracticeTypeValue rdf:type owl:NamedIndividual ,
                                                         <http://www.w3.org/2004/02/skos/core#ConceptScheme> ;
                                                <http://purl.org/dc/terms/isFormatOf> <http://lpis.ec.europa.eu/registry/applicationschema/cap-iacs-parcel#EcologicalFocusAreaEquivalentPracticeTypeValue> ;
                                                rdfs:label "List of EFA equivalent practices"@en ;
                                                <http://www.w3.org/2004/02/skos/core#definition> """--Name--
EFA equivalent practice type

-- Definition --
Equivalent practices with EFAs which are listed  in print III of Annex IX of Regulation (EU) No 1307/2013.

-- Description --
The specific AECM reason has to be linked to the EFA type."""@en .


###  http://lpis.ec.europa.eu/registry/applicationschema/cap-iacs-parcel/code#EcologicalFocusAreaTypeValue
:EcologicalFocusAreaTypeValue rdf:type owl:NamedIndividual ,
                                       <http://www.w3.org/2004/02/skos/core#ConceptScheme> ;
                              <http://purl.org/dc/terms/isFormatOf> <http://lpis.ec.europa.eu/registry/applicationschema/cap-iacs-parcel#EcologicalFocusAreaTypeValue> ;
                              rdfs:label "List of ecological focuse areas"@en ;
                              <http://www.w3.org/2004/02/skos/core#definition> """--Name--
Ecological focus area type value

-- Definition --
Types of EFA as listed in Art. 46(2) of (EU) R 1307/2013.

-- Description --
MS shall decide that one or more values of this code list  are considered to be ecological focus area.

NOTE 1: Member States may decide to limit the selection of landscape features to those under GAEC 7, SMR 2 or SMR 3  as referred to in Annex II to Regulation (EU) No 640/2013 and/or to one or more of those listed in point (a) to (h) of the first subparagraph, where duly justified. Should it be the case, the code list of EFA types have to be modifie accordingly.

NOTE 2: The extension of this code list shall be documented in the eligibility profile of the MS/region. It is recommended to use  a register / registry service to publish the extended values and their definitions.

NOTE 3: Landscape features shall be:
-at the disposal of the farmer;
-shall be those that are protected under GAEC 7, SMR 2 or SMR 3 as referred to in Annex II to Regulation (EU) No 640/2014."""@en .


###  http://lpis.ec.europa.eu/registry/applicationschema/cap-iacs-parcel/code#HomogeneityTypeValue
:HomogeneityTypeValue rdf:type owl:NamedIndividual ,
                               <http://www.w3.org/2004/02/skos/core#ConceptScheme> ;
                      <http://purl.org/dc/terms/isFormatOf> <http://lpis.ec.europa.eu/registry/applicationschema/cap-iacs-parcel#HomogeneityTypeValue> ;
                      rdfs:label "List of homogeneity type"@en ;
                      <http://www.w3.org/2004/02/skos/core#definition> """--Name--
Homogeneity type value

-- Definition --
Code list of homogeneity types for single and homogenous geographical areas with similar agricultural and environmental conditions as referred to Art. 46(1) of (EU) R 639/2014.

-- Description --
It is a code list managed by the Commission Services, therefore is not extensible by the MS/regions."""@en .


###  http://lpis.ec.europa.eu/registry/applicationschema/cap-iacs-parcel/code#InspectionMethodValue
:InspectionMethodValue rdf:type owl:NamedIndividual ,
                                <http://www.w3.org/2004/02/skos/core#ConceptScheme> ;
                       <http://purl.org/dc/terms/isFormatOf> <http://lpis.ec.europa.eu/registry/applicationschema/cap-iacs-parcel#InspectionMethodValue> ;
                       rdfs:label "List of inspection methods"@en ;
                       <http://www.w3.org/2004/02/skos/core#definition> """--Name--
Inspection method  value

-- Definition --
Data collection methods applicable for LPISQA.

-- Description --
MS/Regions shall chose on of the following methods:
- field survey,
- computer assisted photo interpretation (CAPI)
- combined CAPI and field measurements."""@en .


###  http://lpis.ec.europa.eu/registry/applicationschema/cap-iacs-parcel/code#LandscapeFeatureValueType
:LandscapeFeatureValueType rdf:type owl:NamedIndividual ,
                                    <http://www.w3.org/2004/02/skos/core#ConceptScheme> ;
                           <http://purl.org/dc/terms/isFormatOf> <http://lpis.ec.europa.eu/registry/applicationschema/cap-iacs-parcel#LandscapeFeatureValueType> ;
                           rdfs:label "List of landscape features"@en ;
                           <http://www.w3.org/2004/02/skos/core#definition> """--Name--
Landscape feature value type

-- Definition --
Types of landscape features.

-- Description --
MS shall decide that one or more values of this code list  are considered to be landscape feature. The code list can be extended."""@en .


###  http://lpis.ec.europa.eu/registry/applicationschema/cap-iacs-parcel/code#LimitingQualityValue
:LimitingQualityValue rdf:type owl:NamedIndividual ,
                               <http://www.w3.org/2004/02/skos/core#ConceptScheme> ;
                      <http://purl.org/dc/terms/isFormatOf> <http://lpis.ec.europa.eu/registry/applicationschema/cap-iacs-parcel#LimitingQualityValue> ;
                      rdfs:label "List of possible limiting quality values"@en ;
                      <http://www.w3.org/2004/02/skos/core#definition> """--Name--
Limiting quality value

-- Definition --
List of limiting quality values applicable in LPISQA.

-- Description --
Limiting quality values are defined by ISO 2859-2:1985."""@en .


###  http://lpis.ec.europa.eu/registry/applicationschema/cap-iacs-parcel/code#LotSizeValue
:LotSizeValue rdf:type owl:NamedIndividual ,
                       <http://www.w3.org/2004/02/skos/core#ConceptScheme> ;
              <http://purl.org/dc/terms/isFormatOf> <http://lpis.ec.europa.eu/registry/applicationschema/cap-iacs-parcel#LotSizeValue> ;
              rdfs:label "List of possible lot size range values"@en ;
              <http://www.w3.org/2004/02/skos/core#definition> """--Name--
Lot size value

-- Definition --
List of possible lot size range values. according to ISO 2859-2:1985.

-- Description --
The ranges are defined in ISO 2859-2:1985 Sampling procedures for inspection by attributes, Part 2: Sampling plans indexed by limiting quality (LQ) for isolated lot inspection."""@en .


###  http://lpis.ec.europa.eu/registry/applicationschema/cap-iacs-parcel/code#ProRataCategoryValue
:ProRataCategoryValue rdf:type owl:NamedIndividual ,
                               <http://www.w3.org/2004/02/skos/core#ConceptScheme> ;
                      <http://purl.org/dc/terms/isFormatOf> <http://lpis.ec.europa.eu/registry/applicationschema/cap-iacs-parcel#ProRataCategoryValue> ;
                      rdfs:label "List of pro rata category values"@en ;
                      <http://www.w3.org/2004/02/skos/core#definition> """--Name--
Pro-rata category value

-- Definition --
Pro rata categories represent groups of land cover classes that share an eligibility rate.

-- Description --
Categories are predefined by MS/Regions. The code list can be extended."""@en .


###  http://lpis.ec.europa.eu/registry/applicationschema/cap-iacs-parcel/code#SampleSizeValue
:SampleSizeValue rdf:type owl:NamedIndividual ,
                          <http://www.w3.org/2004/02/skos/core#ConceptScheme> ;
                 <http://purl.org/dc/terms/isFormatOf> <http://lpis.ec.europa.eu/registry/applicationschema/cap-iacs-parcel#SampleSizeValue> ;
                 rdfs:label "List of possible sample size values"@en ;
                 <http://www.w3.org/2004/02/skos/core#definition> """--Name--
Sample size value

-- Definition --
List of sample size values applicable for LPISQA.

-- Description --
The sample size is selected as function of the lot size and the limiting quality defined in  ISO 2859-2:1985 (Sampling procedures for inspection by attributes, Part 2: Sampling plans indexed by limiting quality (LQ) for isolated lot inspection)."""@en .


###  http://lpis.ec.europa.eu/registry/applicationschema/cap-iacs-parcel/code#SkippingReasonTypeValue
:SkippingReasonTypeValue rdf:type owl:NamedIndividual ,
                                  <http://www.w3.org/2004/02/skos/core#ConceptScheme> ;
                         <http://purl.org/dc/terms/isFormatOf> <http://lpis.ec.europa.eu/registry/applicationschema/cap-iacs-parcel#SkippingReasonTypeValue> ;
                         rdfs:label "Skipping reason type value"@en ;
                         <http://www.w3.org/2004/02/skos/core#definition> """--Name--
Skipping reason value type

-- Definition --
List  of reasons that do not allow the inspection of a given item under inspection.

-- Description --
Objective reasons for skipping  an item under inspection.

NOTE: This code list is managed by DG JRC. MS/Regions are not allowed to extend it."""@en .


###  http://lpis.ec.europa.eu/registry/applicationschema/cap-iacs-parcel/code#TechnicalReasonValue
:TechnicalReasonValue rdf:type owl:NamedIndividual ,
                               <http://www.w3.org/2004/02/skos/core#ConceptScheme> ;
                      <http://purl.org/dc/terms/isFormatOf> <http://lpis.ec.europa.eu/registry/applicationschema/cap-iacs-parcel#TechnicalReasonValue> ;
                      rdfs:label "List of possible technical reason values"@en ;
                      <http://www.w3.org/2004/02/skos/core#definition> """--Name--
Technical reason value

--Definition --
List of the technical reasons.

--Description--
List of the causes leading to non-conformance of items under inspection."""@en .


###  http://lpis.ec.europa.eu/registry/applicationschema/cap-iacs-parcel/code#TestTypeMtsValue
:TestTypeMtsValue rdf:type owl:NamedIndividual ,
                           <http://www.w3.org/2004/02/skos/core#ConceptScheme> ;
                  <http://purl.org/dc/terms/isFormatOf> <http://lpis.ec.europa.eu/registry/applicationschema/cap-iacs-parcel#TestTypeMtsValue> ;
                  rdfs:label "MTS test type value list"@en ;
                  <http://www.w3.org/2004/02/skos/core#definition> """--Name--
MTS  test type values

--Definition--
Abstract test cases applicable in model based testing for LPISQA.

--Description--
These abstract test cases are applicable for conformance testing of the eligibility profile in general. They should  be further specified  in the executable test cases according to the implementation choices of the MS/Regions."""@en .


###  http://lpis.ec.europa.eu/registry/applicationschema/cap-iacs-parcel/code#AcceptanceNumberValue/10
<http://lpis.ec.europa.eu/registry/applicationschema/cap-iacs-parcel/code#AcceptanceNumberValue/10> rdf:type owl:NamedIndividual ,
                                                                                                             <http://lpis.ec.europa.eu/registry/applicationschema/cap-iacs-parcel#AcceptanceNumberValue> ;
                                                                                                    rdfs:label "10"@en ;
                                                                                                    <http://www.w3.org/2004/02/skos/core#definition> """--Name--
10

-- Definition --
Acceptance number value 10.

-- Description --
ISO2859-2: Sampling procedures for inspection by attributes, Part 2: Sampling plans indexed by limiting quality (LQ) for isolated lot inspection."""@en ;
                                                                                                    <http://www.w3.org/2004/02/skos/core#inScheme> :AcceptanceNumberValue .


###  http://lpis.ec.europa.eu/registry/applicationschema/cap-iacs-parcel/code#AcceptanceNumberValue/18
<http://lpis.ec.europa.eu/registry/applicationschema/cap-iacs-parcel/code#AcceptanceNumberValue/18> rdf:type owl:NamedIndividual ,
                                                                                                             <http://lpis.ec.europa.eu/registry/applicationschema/cap-iacs-parcel#AcceptanceNumberValue> ;
                                                                                                    rdfs:label "18"@en ;
                                                                                                    <http://www.w3.org/2004/02/skos/core#definition> """--Name--
18

-- Definition --
Acceptance number value 18.

-- Description --
Value defined in ISO 2859-2:1985."""@en ;
                                                                                                    <http://www.w3.org/2004/02/skos/core#inScheme> :AcceptanceNumberValue .


###  http://lpis.ec.europa.eu/registry/applicationschema/cap-iacs-parcel/code#AcceptanceNumberValue/5
<http://lpis.ec.europa.eu/registry/applicationschema/cap-iacs-parcel/code#AcceptanceNumberValue/5> rdf:type owl:NamedIndividual ,
                                                                                                            <http://lpis.ec.europa.eu/registry/applicationschema/cap-iacs-parcel#AcceptanceNumberValue> ;
                                                                                                   rdfs:label "5"@en ;
                                                                                                   <http://www.w3.org/2004/02/skos/core#definition> """--Name--
5

-- Definition --
Acceptance number value 5.

-- Description --
Value defined in ISO 2859-2:1985."""@en ;
                                                                                                   <http://www.w3.org/2004/02/skos/core#inScheme> :AcceptanceNumberValue .


###  http://lpis.ec.europa.eu/registry/applicationschema/cap-iacs-parcel/code#AgriculturalAreaTypeValue/arableLand
<http://lpis.ec.europa.eu/registry/applicationschema/cap-iacs-parcel/code#AgriculturalAreaTypeValue/arableLand> rdf:type owl:NamedIndividual ,
                                                                                                                         <http://lpis.ec.europa.eu/registry/applicationschema/cap-iacs-parcel#AgriculturalAreaTypeValue> ;
                                                                                                                rdfs:label "Arable land"@en ;
                                                                                                                <http://www.w3.org/2004/02/skos/core#definition> """--Name--
Arable land

-- Definition --
Land cultivated for crop production or areas available for crop production but lying fallow, including areas set aside in accordance with Articles 22, 23 and 24 of Regulation (EC) No 1257/1999, with Article 39 of Regulation (EC) No 1698/2005 and with Article 28 of Regulation (EU) No 1305/2013, irrespective of whether or not that land is under greenhouses or under fixed or mobile cover."""@en ;
                                                                                                                <http://www.w3.org/2004/02/skos/core#inScheme> :AgriculturalAreaTypeValue .


###  http://lpis.ec.europa.eu/registry/applicationschema/cap-iacs-parcel/code#AgriculturalAreaTypeValue/permanentCrop
<http://lpis.ec.europa.eu/registry/applicationschema/cap-iacs-parcel/code#AgriculturalAreaTypeValue/permanentCrop> rdf:type owl:NamedIndividual ,
                                                                                                                            <http://lpis.ec.europa.eu/registry/applicationschema/cap-iacs-parcel#AgriculturalAreaTypeValue> ;
                                                                                                                   rdfs:label "Permanent crop"@en ;
                                                                                                                   <http://www.w3.org/2004/02/skos/core#definition> """--Name--
Permanent crop

-- Definition --
Non-rotational crops other than permanent grassland and permanent pasture that occupy the land for five years or more and yield repeated harvests, including nurseries and short rotation coppice. [Art. 4 (1)(g) of (EU) R No 1307/2013]."""@en ;
                                                                                                                   <http://www.w3.org/2004/02/skos/core#inScheme> :AgriculturalAreaTypeValue .


###  http://lpis.ec.europa.eu/registry/applicationschema/cap-iacs-parcel/code#AgriculturalAreaTypeValue/permanentGrassland
<http://lpis.ec.europa.eu/registry/applicationschema/cap-iacs-parcel/code#AgriculturalAreaTypeValue/permanentGrassland> rdf:type owl:NamedIndividual ,
                                                                                                                                 <http://lpis.ec.europa.eu/registry/applicationschema/cap-iacs-parcel#AgriculturalAreaTypeValue> ;
                                                                                                                        rdfs:label "Permanent grassland"@en ;
                                                                                                                        <http://www.w3.org/2004/02/skos/core#definition> """--Name--
Permanent grassland

-- Definition --
Permanent grassland and permanent pasture (together referred to as \"permanent grassland\") means land used to grow grasses or other herbaceous forage naturally (self-seeded) or through cultivation (sown) and that has not been included in the crop rotation of the holding for five years or more; it may include other species such as shrubs and/or trees which can be grazed provided that the grasses and other herbaceous forage remain predominant as well as, where Member States so decide, land which can be grazed and which forms part of established local practices where grasses and other herbaceous forage are traditionally not predominant in grazing areas. [Art. 4(1)(g) 0f (EU) R No 1307/2013]."""@en ;
                                                                                                                        <http://www.w3.org/2004/02/skos/core#inScheme> :AgriculturalAreaTypeValue .


###  http://lpis.ec.europa.eu/registry/applicationschema/cap-iacs-parcel/code#AgriculturalAreaTypeValue/permanentGrasslandElp
<http://lpis.ec.europa.eu/registry/applicationschema/cap-iacs-parcel/code#AgriculturalAreaTypeValue/permanentGrasslandElp> rdf:type owl:NamedIndividual ,
                                                                                                                                    <http://lpis.ec.europa.eu/registry/applicationschema/cap-iacs-parcel#AgriculturalAreaTypeValue> ;
                                                                                                                           rdfs:label "Permanent grassland established under local practices"@en ;
                                                                                                                           <http://www.w3.org/2004/02/skos/core#definition> """--Name--
Permanent grassland under established  local practices

-- Definition --
Permanent grassland under established local practices as referred to in Art.4(1)(h) of R (EU) No 1307/2013. 

-- Description --
Land which can be grazed and which forms part of established local practices where grasses and other herbaceous forage are traditionally not predominant in grazing areas.

NOTE: According to DSCG/2014/33  these areas should be added and identified in LPIS."""@en ;
                                                                                                                           <http://www.w3.org/2004/02/skos/core#inScheme> :AgriculturalAreaTypeValue .


###  http://lpis.ec.europa.eu/registry/applicationschema/cap-iacs-parcel/code#AgriculturalAreaTypeValue/permanentGrasslandSensitive
<http://lpis.ec.europa.eu/registry/applicationschema/cap-iacs-parcel/code#AgriculturalAreaTypeValue/permanentGrasslandSensitive> rdf:type owl:NamedIndividual ,
                                                                                                                                          <http://lpis.ec.europa.eu/registry/applicationschema/cap-iacs-parcel#AgriculturalAreaTypeValue> ;
                                                                                                                                 rdfs:label "Permanent grassland sensitive"@en ;
                                                                                                                                 <http://www.w3.org/2004/02/skos/core#definition> """--Name--
Sensitive permanent grassland

-- Definition --
Permanent grassland designated as sensitive as referred to in Art. 41 of (EU) R 639/2014.

-- Description --
Sensitiveness may be designated on the basis of:
- covering organic soils with a high percentage of organic carbon, such as peat land or wetlands;
- hosting habitats listed in Annex I to Directive 92/43/EEC or protected under national legislation;
- hosting plant species listed in Annex II to Directive 92/43/EEC or protected under national legislation;
- being of significant importance for wild bird species listed in Annex I to Directive 2009/147/EC;
- being of significant importance for wild animal species protected under Directive 92/43/EEC or protected under national legislation;
- covering permanent grassland of high nature value as defined by objective criteria to be established by the MS;
- covering soils with a high risk of erosion;
- being located in a sensitive area designated within the river basin management plans pursuant to Directive 2000/60/EC;
- the decision of the MS;
- re-conversion as referred to in Art. 42 of (EU) R 639/2014.

NOTE: This type includes grasslands covered by Directives 92/43/EEC or 2009/147/EC, including in peat and wetlands situated in these areas [Art. 45(1) of (EU) R 1307/2013."""@en ;
                                                                                                                                 <http://www.w3.org/2004/02/skos/core#inScheme> :AgriculturalAreaTypeValue .


###  http://lpis.ec.europa.eu/registry/applicationschema/cap-iacs-parcel/code#ContaminationTypeValue/artificialSealedSurface
<http://lpis.ec.europa.eu/registry/applicationschema/cap-iacs-parcel/code#ContaminationTypeValue/artificialSealedSurface> rdf:type owl:NamedIndividual ,
                                                                                                                                   <http://lpis.ec.europa.eu/registry/applicationschema/cap-iacs-parcel#ContaminationTypeValue> ;
                                                                                                                          rdfs:label "Artificial sealed surface"@en ;
                                                                                                                          <http://www.w3.org/2004/02/skos/core#definition> """--Name--
Artificial sealed surface

-- Definition --
Sealed surface of man-made origin.

-- Description --
Any artificial surface such as roads, houses, other constructions."""@en ;
                                                                                                                          <http://www.w3.org/2004/02/skos/core#inScheme> :ContaminationTypeValue .


###  http://lpis.ec.europa.eu/registry/applicationschema/cap-iacs-parcel/code#ContaminationTypeValue/crosscuttingNonAgriculturalLc
<http://lpis.ec.europa.eu/registry/applicationschema/cap-iacs-parcel/code#ContaminationTypeValue/crosscuttingNonAgriculturalLc> rdf:type owl:NamedIndividual ,
                                                                                                                                         <http://lpis.ec.europa.eu/registry/applicationschema/cap-iacs-parcel#ContaminationTypeValue> ;
                                                                                                                                rdfs:label "Crosscutting non agricultural land cover"@en ;
                                                                                                                                <http://www.w3.org/2004/02/skos/core#definition> """--Name--
Cross cutting non-agricultural land

-- Definition --
Ineligible land cover type crosscutting the item under inspection.

-- Description --
Ineligible LC type (e.g. road, a water body, etc.) that causes discontinuity of agricultural land within a reference parcel.

NOTE: This value is applicable in LPIS that follow the cadastral parcel or topographic block design."""@en ;
                                                                                                                                <http://www.w3.org/2004/02/skos/core#inScheme> :ContaminationTypeValue .


###  http://lpis.ec.europa.eu/registry/applicationschema/cap-iacs-parcel/code#CriticalDefectTypeEfaValue/invalidConversionParameter
<http://lpis.ec.europa.eu/registry/applicationschema/cap-iacs-parcel/code#CriticalDefectTypeEfaValue/invalidConversionParameter> rdf:type owl:NamedIndividual ,
                                                                                                                                          <http://lpis.ec.europa.eu/registry/applicationschema/cap-iacs-parcel#CriticalDefectTypeEfaValue> ;
                                                                                                                                 rdfs:label "Invalid conversion parameter"@en ;
                                                                                                                                 <http://www.w3.org/2004/02/skos/core#definition> """--Name--
Invalid conversion parameter

-- Definition --
This is a placeholder only; currently not to be implemented.

-- Description --
Error in selection of the conversion parameter."""@en ;
                                                                                                                                 <http://www.w3.org/2004/02/skos/core#inScheme> :CriticalDefectTypeEfaValue .


###  http://lpis.ec.europa.eu/registry/applicationschema/cap-iacs-parcel/code#CriticalDefectTypeEfaValue/invalidGeometry
<http://lpis.ec.europa.eu/registry/applicationschema/cap-iacs-parcel/code#CriticalDefectTypeEfaValue/invalidGeometry> rdf:type owl:NamedIndividual ,
                                                                                                                               <http://lpis.ec.europa.eu/registry/applicationschema/cap-iacs-parcel#CriticalDefectTypeEfaValue> ;
                                                                                                                      rdfs:label "Invalid geometry"@en ;
                                                                                                                      <http://www.w3.org/2004/02/skos/core#definition> """--Name--
Invalid geometry

-- Definition --
This is a placeholder only; currently not to be implemented.

-- Description --
Other geometry than the choice of the MS/Region has been used."""@en ;
                                                                                                                      <http://www.w3.org/2004/02/skos/core#inScheme> :CriticalDefectTypeEfaValue .


###  http://lpis.ec.europa.eu/registry/applicationschema/cap-iacs-parcel/code#CriticalDefectTypeEfaValue/invalidWeightingParameter
<http://lpis.ec.europa.eu/registry/applicationschema/cap-iacs-parcel/code#CriticalDefectTypeEfaValue/invalidWeightingParameter> rdf:type owl:NamedIndividual ,
                                                                                                                                         <http://lpis.ec.europa.eu/registry/applicationschema/cap-iacs-parcel#CriticalDefectTypeEfaValue> ;
                                                                                                                                rdfs:label "Invalid weighting parameter"@en ;
                                                                                                                                <http://www.w3.org/2004/02/skos/core#definition> """--Name--
Invalid weighting parameter

-- Definition --
This is a placeholder only; currently not to be implemented.

-- Description --
Error in selecting the weighting parameter."""@en ;
                                                                                                                                <http://www.w3.org/2004/02/skos/core#inScheme> :CriticalDefectTypeEfaValue .


###  http://lpis.ec.europa.eu/registry/applicationschema/cap-iacs-parcel/code#CriticalDefectTypeEfaValue/notConnectedToArable
<http://lpis.ec.europa.eu/registry/applicationschema/cap-iacs-parcel/code#CriticalDefectTypeEfaValue/notConnectedToArable> rdf:type owl:NamedIndividual ,
                                                                                                                                    <http://lpis.ec.europa.eu/registry/applicationschema/cap-iacs-parcel#CriticalDefectTypeEfaValue> ;
                                                                                                                           rdfs:label "Not connected to arable land"@en ;
                                                                                                                           <http://www.w3.org/2004/02/skos/core#definition> """--Name--
Not connected to arable land

-- Definition --
This is a placeholder only; currently not to be implemented.

--Description --
Not connected to arable land."""@en ;
                                                                                                                           <http://www.w3.org/2004/02/skos/core#inScheme> :CriticalDefectTypeEfaValue .


###  http://lpis.ec.europa.eu/registry/applicationschema/cap-iacs-parcel/code#CriticalDefectTypeEfaValue/totalAbsanceOfEligibleTypes
<http://lpis.ec.europa.eu/registry/applicationschema/cap-iacs-parcel/code#CriticalDefectTypeEfaValue/totalAbsanceOfEligibleTypes> rdf:type owl:NamedIndividual ,
                                                                                                                                           <http://lpis.ec.europa.eu/registry/applicationschema/cap-iacs-parcel#CriticalDefectTypeEfaValue> ;
                                                                                                                                  rdfs:label "Total absance of eligible types"@en ;
                                                                                                                                  <http://www.w3.org/2004/02/skos/core#definition> """--Name--
Total absence of eligible types

-- Definition --
This is a placeholder only; currently not to be implemented.

-- Description --
Total absence of eligible types."""@en ;
                                                                                                                                  <http://www.w3.org/2004/02/skos/core#inScheme> :CriticalDefectTypeEfaValue .


###  http://lpis.ec.europa.eu/registry/applicationschema/cap-iacs-parcel/code#CriticalDefectTypeValue/incompleteBlock
<http://lpis.ec.europa.eu/registry/applicationschema/cap-iacs-parcel/code#CriticalDefectTypeValue/incompleteBlock> rdf:type owl:NamedIndividual ,
                                                                                                                            <http://lpis.ec.europa.eu/registry/applicationschema/cap-iacs-parcel#CriticalDefectTypeValue> ;
                                                                                                                   rdfs:label "Incomplete block"@en ;
                                                                                                                   <http://www.w3.org/2004/02/skos/core#definition> """--Name--
Incomplete block

-- Definition --
Production block, where Land use / land cover counter-indicates the presence of a true stable physical boundary of the block. [Wikicap]

-- Description --
NOTE:  This types is applicable for physical and topographic block systems only."""@en ;
                                                                                                                   <http://www.w3.org/2004/02/skos/core#inScheme> :CriticalDefectTypeValue .


###  http://lpis.ec.europa.eu/registry/applicationschema/cap-iacs-parcel/code#CriticalDefectTypeValue/invalidCommonRpBoundary
<http://lpis.ec.europa.eu/registry/applicationschema/cap-iacs-parcel/code#CriticalDefectTypeValue/invalidCommonRpBoundary> rdf:type owl:NamedIndividual ,
                                                                                                                                    <http://lpis.ec.europa.eu/registry/applicationschema/cap-iacs-parcel#CriticalDefectTypeValue> ;
                                                                                                                           rdfs:label "Invalid common reference parcel boundary"@en ;
                                                                                                                           <http://www.w3.org/2004/02/skos/core#definition> """--Name--
Invalid common RP boundary

-- Definition --
Location of common boundaries that cannot be derived from surrounding land cover / land use elements. [Wikicap] 

-- Description --
NOTE:  This types is applicable for physical and topographic block systems only."""@en ;
                                                                                                                           <http://www.w3.org/2004/02/skos/core#inScheme> :CriticalDefectTypeValue .


###  http://lpis.ec.europa.eu/registry/applicationschema/cap-iacs-parcel/code#CriticalDefectTypeValue/invalidRpPerimeter
<http://lpis.ec.europa.eu/registry/applicationschema/cap-iacs-parcel/code#CriticalDefectTypeValue/invalidRpPerimeter> rdf:type owl:NamedIndividual ,
                                                                                                                               <http://lpis.ec.europa.eu/registry/applicationschema/cap-iacs-parcel#CriticalDefectTypeValue> ;
                                                                                                                      rdfs:label "Invalid RP perimeter"@en ;
                                                                                                                      <http://www.w3.org/2004/02/skos/core#definition> """--Name--
Invalid RP perimeter

-- Definition --
Spatial representation on RP boundary which does not correspond to the observable ground truth.

-- Description --
RP with invalid perimeter is represented by a completely virtual polygon geometry that crosses through both agricultural land and non-agricultural land covers.

NOTE: It is applicable only for reference parcels that cannot be measured."""@en ;
                                                                                                                      <http://www.w3.org/2004/02/skos/core#inScheme> :CriticalDefectTypeValue .


###  http://lpis.ec.europa.eu/registry/applicationschema/cap-iacs-parcel/code#CriticalDefectTypeValue/multiParcel
<http://lpis.ec.europa.eu/registry/applicationschema/cap-iacs-parcel/code#CriticalDefectTypeValue/multiParcel> rdf:type owl:NamedIndividual ,
                                                                                                                        <http://lpis.ec.europa.eu/registry/applicationschema/cap-iacs-parcel#CriticalDefectTypeValue> ;
                                                                                                               rdfs:label "Multi-parcel"@en ;
                                                                                                               <http://www.w3.org/2004/02/skos/core#definition> """--Name--
Multi-parcel

-- Definition --
Multi-parcel is a block that amalgamates ten or more clearly distinct parcels.

-- Description --
According to the internal rules of the given LPIS the contained units of agriculture land should have been processed separately.

NOTE: This value is applicable to production and topographic blocks only."""@en ;
                                                                                                               <http://www.w3.org/2004/02/skos/core#inScheme> :CriticalDefectTypeValue .


###  http://lpis.ec.europa.eu/registry/applicationschema/cap-iacs-parcel/code#CriticalDefectTypeValue/multiSurface
<http://lpis.ec.europa.eu/registry/applicationschema/cap-iacs-parcel/code#CriticalDefectTypeValue/multiSurface> rdf:type owl:NamedIndividual ,
                                                                                                                         <http://lpis.ec.europa.eu/registry/applicationschema/cap-iacs-parcel#CriticalDefectTypeValue> ;
                                                                                                                rdfs:label "Multi-surface"@en ;
                                                                                                                <http://www.w3.org/2004/02/skos/core#definition> """--Name--
Multi-surface

-- Definition --
Invalid geometry type (multi -surface, GM_Multisurface) for an inspected item.

-- Description --
The parcel that carries one identifier consists of two or more disjoint surface units.

NOTE 1: This value is not applicable, when the parcel aggregation methodology is used.

NOTE 2: Previous name was multiPolygon."""@en ;
                                                                                                                <http://www.w3.org/2004/02/skos/core#inScheme> :CriticalDefectTypeValue .


###  http://lpis.ec.europa.eu/registry/applicationschema/cap-iacs-parcel/code#CriticalDefectTypeValue/totalAbsenceOfAgriculturalLand
<http://lpis.ec.europa.eu/registry/applicationschema/cap-iacs-parcel/code#CriticalDefectTypeValue/totalAbsenceOfAgriculturalLand> rdf:type owl:NamedIndividual ,
                                                                                                                                           <http://lpis.ec.europa.eu/registry/applicationschema/cap-iacs-parcel#CriticalDefectTypeValue> ;
                                                                                                                                  rdfs:label "Total absence of agricultural land"@en ;
                                                                                                                                  <http://www.w3.org/2004/02/skos/core#definition> """--Name--
Total absence of agricultural land

-- Definition --
Item under inspection with total absence of agricultural land.

--Description --
Item under inspection, which does not contain any instance of agricultural land cover type listed in the eligibility profile.

NOTE: Stand-alone eligible landscape feature (without agricultural land) within the item of inspection does not vindicate critical defect."""@en ;
                                                                                                                                  <http://www.w3.org/2004/02/skos/core#inScheme> :CriticalDefectTypeValue .


###  http://lpis.ec.europa.eu/registry/applicationschema/cap-iacs-parcel/code#DataQualityMeasureNameValue/areaConformance
<http://lpis.ec.europa.eu/registry/applicationschema/cap-iacs-parcel/code#DataQualityMeasureNameValue/areaConformance> rdf:type owl:NamedIndividual ,
                                                                                                                                <http://lpis.ec.europa.eu/registry/applicationschema/cap-iacs-parcel#DataQualityMeasureNameValue> ;
                                                                                                                       rdfs:label "I_ACON"@en ;
                                                                                                                       <http://www.w3.org/2004/02/skos/core#definition> """-- Description --
For definition and description see the corresponding value in DataQualityMeasureTypeIuiValue code list."""@en ;
                                                                                                                       <http://www.w3.org/2004/02/skos/core#inScheme> :DataQualityMeasureNameValue .


###  http://lpis.ec.europa.eu/registry/applicationschema/cap-iacs-parcel/code#DataQualityMeasureNameValue/areaCorrectnessDistribution
<http://lpis.ec.europa.eu/registry/applicationschema/cap-iacs-parcel/code#DataQualityMeasureNameValue/areaCorrectnessDistribution> rdf:type owl:NamedIndividual ,
                                                                                                                                            <http://lpis.ec.europa.eu/registry/applicationschema/cap-iacs-parcel#DataQualityMeasureNameValue> ;
                                                                                                                                   rdfs:label "L_ACD"@en ;
                                                                                                                                   <http://www.w3.org/2004/02/skos/core#definition> """-- Description --
For definition and description see the corresponding value in DataQualityMeasureTypeEtsValue code list."""@en ;
                                                                                                                                   <http://www.w3.org/2004/02/skos/core#inScheme> :DataQualityMeasureNameValue .


###  http://lpis.ec.europa.eu/registry/applicationschema/cap-iacs-parcel/code#DataQualityMeasureNameValue/areaDifferenceCorrectness
<http://lpis.ec.europa.eu/registry/applicationschema/cap-iacs-parcel/code#DataQualityMeasureNameValue/areaDifferenceCorrectness> rdf:type owl:NamedIndividual ,
                                                                                                                                          <http://lpis.ec.europa.eu/registry/applicationschema/cap-iacs-parcel#DataQualityMeasureNameValue> ;
                                                                                                                                 rdfs:label "I_ADC"@en ;
                                                                                                                                 <http://www.w3.org/2004/02/skos/core#definition> """-- Description --
For definition and description see the corresponding value in DataQualityMeasureTypeIuiValue code list."""@en ;
                                                                                                                                 <http://www.w3.org/2004/02/skos/core#inScheme> :DataQualityMeasureNameValue .


###  http://lpis.ec.europa.eu/registry/applicationschema/cap-iacs-parcel/code#DataQualityMeasureNameValue/classificationCorrectness
<http://lpis.ec.europa.eu/registry/applicationschema/cap-iacs-parcel/code#DataQualityMeasureNameValue/classificationCorrectness> rdf:type owl:NamedIndividual ,
                                                                                                                                          <http://lpis.ec.europa.eu/registry/applicationschema/cap-iacs-parcel#DataQualityMeasureNameValue> ;
                                                                                                                                 rdfs:label "I_CC"@en ;
                                                                                                                                 <http://www.w3.org/2004/02/skos/core#definition> """-- Description --
For definition and description see the corresponding value in DataQualityMeasureTypeIuiValue code list."""@en ;
                                                                                                                                 <http://www.w3.org/2004/02/skos/core#inScheme> :DataQualityMeasureNameValue .


###  http://lpis.ec.europa.eu/registry/applicationschema/cap-iacs-parcel/code#DataQualityMeasureNameValue/conformityClass1
<http://lpis.ec.europa.eu/registry/applicationschema/cap-iacs-parcel/code#DataQualityMeasureNameValue/conformityClass1> rdf:type owl:NamedIndividual ,
                                                                                                                                 <http://lpis.ec.europa.eu/registry/applicationschema/cap-iacs-parcel#DataQualityMeasureNameValue> ;
                                                                                                                        rdfs:label "L_CLASS1"@en ;
                                                                                                                        <http://www.w3.org/2004/02/skos/core#definition> """-- Description --
For definition and description see the corresponding value in DataQualityMeasureTypeEtsValue code list."""@en ;
                                                                                                                        <http://www.w3.org/2004/02/skos/core#inScheme> :DataQualityMeasureNameValue .


###  http://lpis.ec.europa.eu/registry/applicationschema/cap-iacs-parcel/code#DataQualityMeasureNameValue/conformityClass2
<http://lpis.ec.europa.eu/registry/applicationschema/cap-iacs-parcel/code#DataQualityMeasureNameValue/conformityClass2> rdf:type owl:NamedIndividual ,
                                                                                                                                 <http://lpis.ec.europa.eu/registry/applicationschema/cap-iacs-parcel#DataQualityMeasureNameValue> ;
                                                                                                                        rdfs:label "L_CLASS2"@en ;
                                                                                                                        <http://www.w3.org/2004/02/skos/core#definition> """-- Description --
For definition and description see the corresponding value in DataQualoityMeasureTypeEtsValue code list."""@en ;
                                                                                                                        <http://www.w3.org/2004/02/skos/core#inScheme> :DataQualityMeasureNameValue .


###  http://lpis.ec.europa.eu/registry/applicationschema/cap-iacs-parcel/code#DataQualityMeasureNameValue/cummulativeRateOfMissedUpdates
<http://lpis.ec.europa.eu/registry/applicationschema/cap-iacs-parcel/code#DataQualityMeasureNameValue/cummulativeRateOfMissedUpdates> rdf:type owl:NamedIndividual ,
                                                                                                                                               <http://lpis.ec.europa.eu/registry/applicationschema/cap-iacs-parcel#DataQualityMeasureNameValue> ;
                                                                                                                                      rdfs:label "L_CRMU"@en ;
                                                                                                                                      <http://www.w3.org/2004/02/skos/core#definition> """-- Description --
For definition and description see the corresponding value in DataQualityMeasureTypeEtsValue code list."""@en ;
                                                                                                                                      <http://www.w3.org/2004/02/skos/core#inScheme> :DataQualityMeasureNameValue .


###  http://lpis.ec.europa.eu/registry/applicationschema/cap-iacs-parcel/code#DataQualityMeasureNameValue/itemConformance
<http://lpis.ec.europa.eu/registry/applicationschema/cap-iacs-parcel/code#DataQualityMeasureNameValue/itemConformance> rdf:type owl:NamedIndividual ,
                                                                                                                                <http://lpis.ec.europa.eu/registry/applicationschema/cap-iacs-parcel#DataQualityMeasureNameValue> ;
                                                                                                                       rdfs:label "I_CON"@en ;
                                                                                                                       <http://www.w3.org/2004/02/skos/core#definition> """-- Description --
For definition and description see the corresponding value in DataQualityMeasureTypeIuiValue code list."""@en ;
                                                                                                                       <http://www.w3.org/2004/02/skos/core#inScheme> :DataQualityMeasureNameValue .


###  http://lpis.ec.europa.eu/registry/applicationschema/cap-iacs-parcel/code#DataQualityMeasureNameValue/itemCriticalDefectConformance
<http://lpis.ec.europa.eu/registry/applicationschema/cap-iacs-parcel/code#DataQualityMeasureNameValue/itemCriticalDefectConformance> rdf:type owl:NamedIndividual ,
                                                                                                                                              <http://lpis.ec.europa.eu/registry/applicationschema/cap-iacs-parcel#DataQualityMeasureNameValue> ;
                                                                                                                                     rdfs:label "I_CDCON"@en ;
                                                                                                                                     <http://www.w3.org/2004/02/skos/core#definition> """-- Description --
For definition and description see the corresponding value in DataQualityMeasureTypeIuiValue code list."""@en ;
                                                                                                                                     <http://www.w3.org/2004/02/skos/core#inScheme> :DataQualityMeasureNameValue .


###  http://lpis.ec.europa.eu/registry/applicationschema/cap-iacs-parcel/code#DataQualityMeasureNameValue/lpisAreaOverestimates
<http://lpis.ec.europa.eu/registry/applicationschema/cap-iacs-parcel/code#DataQualityMeasureNameValue/lpisAreaOverestimates> rdf:type owl:NamedIndividual ,
                                                                                                                                      <http://lpis.ec.europa.eu/registry/applicationschema/cap-iacs-parcel#DataQualityMeasureNameValue> ;
                                                                                                                             rdfs:label "L_AOE"@en ;
                                                                                                                             <http://www.w3.org/2004/02/skos/core#definition> """-- Description --
For definition and description see the corresponding value in DataQualityMeasureTypeEtsValue code list."""@en ;
                                                                                                                             <http://www.w3.org/2004/02/skos/core#inScheme> :DataQualityMeasureNameValue .


###  http://lpis.ec.europa.eu/registry/applicationschema/cap-iacs-parcel/code#DataQualityMeasureNameValue/lpisAreaPrecisionConformance
<http://lpis.ec.europa.eu/registry/applicationschema/cap-iacs-parcel/code#DataQualityMeasureNameValue/lpisAreaPrecisionConformance> rdf:type owl:NamedIndividual ,
                                                                                                                                             <http://lpis.ec.europa.eu/registry/applicationschema/cap-iacs-parcel#DataQualityMeasureNameValue> ;
                                                                                                                                    rdfs:label "L_APCON"@en ;
                                                                                                                                    <http://www.w3.org/2004/02/skos/core#definition> """-- Description --
For definition and description see the corresponding value in DataQualityMeasureTypeEtsValue code list."""@en ;
                                                                                                                                    <http://www.w3.org/2004/02/skos/core#inScheme> :DataQualityMeasureNameValue .


###  http://lpis.ec.europa.eu/registry/applicationschema/cap-iacs-parcel/code#DataQualityMeasureNameValue/lpisAreaUnderestimates
<http://lpis.ec.europa.eu/registry/applicationschema/cap-iacs-parcel/code#DataQualityMeasureNameValue/lpisAreaUnderestimates> rdf:type owl:NamedIndividual ,
                                                                                                                                       <http://lpis.ec.europa.eu/registry/applicationschema/cap-iacs-parcel#DataQualityMeasureNameValue> ;
                                                                                                                              rdfs:label "L_AUE"@en ;
                                                                                                                              <http://www.w3.org/2004/02/skos/core#definition> """-- Description --
For definition and description see the corresponding value in DataQualityMeasureTypeEtsValue code list."""@en ;
                                                                                                                              <http://www.w3.org/2004/02/skos/core#inScheme> :DataQualityMeasureNameValue .


###  http://lpis.ec.europa.eu/registry/applicationschema/cap-iacs-parcel/code#DataQualityMeasureNameValue/lpisCriticalDefectConfromance
<http://lpis.ec.europa.eu/registry/applicationschema/cap-iacs-parcel/code#DataQualityMeasureNameValue/lpisCriticalDefectConfromance> rdf:type owl:NamedIndividual ,
                                                                                                                                              <http://lpis.ec.europa.eu/registry/applicationschema/cap-iacs-parcel#DataQualityMeasureNameValue> ;
                                                                                                                                     rdfs:label "L_CDCON"@en ;
                                                                                                                                     <http://www.w3.org/2004/02/skos/core#definition> """-- Description --
For definition and description see the corresponding value in DataQualityMeasureTypeEtsValue code list."""@en ;
                                                                                                                                     <http://www.w3.org/2004/02/skos/core#inScheme> :DataQualityMeasureNameValue .


###  http://lpis.ec.europa.eu/registry/applicationschema/cap-iacs-parcel/code#DataQualityMeasureNameValue/lpisItemConformance
<http://lpis.ec.europa.eu/registry/applicationschema/cap-iacs-parcel/code#DataQualityMeasureNameValue/lpisItemConformance> rdf:type owl:NamedIndividual ,
                                                                                                                                    <http://lpis.ec.europa.eu/registry/applicationschema/cap-iacs-parcel#DataQualityMeasureNameValue> ;
                                                                                                                           rdfs:label "L_ICON"@en ;
                                                                                                                           <http://www.w3.org/2004/02/skos/core#definition> """-- Description --
For definition and description see the corresponding value in DataQualityMeasureTypeEtsValue code list."""@en ;
                                                                                                                           <http://www.w3.org/2004/02/skos/core#inScheme> :DataQualityMeasureNameValue .


###  http://lpis.ec.europa.eu/registry/applicationschema/cap-iacs-parcel/code#DataQualityMeasureNameValue/lpisRelativeAreaConformance
<http://lpis.ec.europa.eu/registry/applicationschema/cap-iacs-parcel/code#DataQualityMeasureNameValue/lpisRelativeAreaConformance> rdf:type owl:NamedIndividual ,
                                                                                                                                            <http://lpis.ec.europa.eu/registry/applicationschema/cap-iacs-parcel#DataQualityMeasureNameValue> ;
                                                                                                                                   rdfs:label "L_RACON"@en ;
                                                                                                                                   <http://www.w3.org/2004/02/skos/core#definition> """-- Description --
For definition and description see the corresponding value in DataQualoityMeasureTypeEtsValue code list."""@en ;
                                                                                                                                   <http://www.w3.org/2004/02/skos/core#inScheme> :DataQualityMeasureNameValue .


###  http://lpis.ec.europa.eu/registry/applicationschema/cap-iacs-parcel/code#DataQualityMeasureNameValue/lpisRelativeAreaCorrectness
<http://lpis.ec.europa.eu/registry/applicationschema/cap-iacs-parcel/code#DataQualityMeasureNameValue/lpisRelativeAreaCorrectness> rdf:type owl:NamedIndividual ,
                                                                                                                                            <http://lpis.ec.europa.eu/registry/applicationschema/cap-iacs-parcel#DataQualityMeasureNameValue> ;
                                                                                                                                   rdfs:label "L_RAC"@en ;
                                                                                                                                   <http://www.w3.org/2004/02/skos/core#definition> """-- Description --
For definition and description see the corresponding value in DataQualityMeasureTypeEtsValue code list."""@en ;
                                                                                                                                   <http://www.w3.org/2004/02/skos/core#inScheme> :DataQualityMeasureNameValue .


###  http://lpis.ec.europa.eu/registry/applicationschema/cap-iacs-parcel/code#DataQualityMeasureNameValue/misclassificationMatrix
<http://lpis.ec.europa.eu/registry/applicationschema/cap-iacs-parcel/code#DataQualityMeasureNameValue/misclassificationMatrix> rdf:type owl:NamedIndividual ,
                                                                                                                                        <http://lpis.ec.europa.eu/registry/applicationschema/cap-iacs-parcel#DataQualityMeasureNameValue> ;
                                                                                                                               rdfs:label "L_MCM"@en ;
                                                                                                                               <http://www.w3.org/2004/02/skos/core#definition> """-- Description --
For definition and description see the corresponding value in DataQualoityMeasureTypeEtsValue code list."""@en ;
                                                                                                                               <http://www.w3.org/2004/02/skos/core#inScheme> :DataQualityMeasureNameValue .


###  http://lpis.ec.europa.eu/registry/applicationschema/cap-iacs-parcel/code#DataQualityMeasureNameValue/numberOfAreaNonConformingItems
<http://lpis.ec.europa.eu/registry/applicationschema/cap-iacs-parcel/code#DataQualityMeasureNameValue/numberOfAreaNonConformingItems> rdf:type owl:NamedIndividual ,
                                                                                                                                               <http://lpis.ec.europa.eu/registry/applicationschema/cap-iacs-parcel#DataQualityMeasureNameValue> ;
                                                                                                                                      rdfs:label "L_NANC_A"@en ;
                                                                                                                                      <http://www.w3.org/2004/02/skos/core#definition> """-- Description --
For definition and description see the corresponding value in DataQualityMeasureTypeEtsValue code list."""@en ;
                                                                                                                                      <http://www.w3.org/2004/02/skos/core#inScheme> :DataQualityMeasureNameValue .


###  http://lpis.ec.europa.eu/registry/applicationschema/cap-iacs-parcel/code#DataQualityMeasureNameValue/numberOfCriticalDefects
<http://lpis.ec.europa.eu/registry/applicationschema/cap-iacs-parcel/code#DataQualityMeasureNameValue/numberOfCriticalDefects> rdf:type owl:NamedIndividual ,
                                                                                                                                        <http://lpis.ec.europa.eu/registry/applicationschema/cap-iacs-parcel#DataQualityMeasureNameValue> ;
                                                                                                                               rdfs:label "L_NCD"@en ;
                                                                                                                               <http://www.w3.org/2004/02/skos/core#definition> """-- Description --
For definition and description see the corresponding value in DataQualityMeasureTypeEtsValue code list."""@en ;
                                                                                                                               <http://www.w3.org/2004/02/skos/core#inScheme> :DataQualityMeasureNameValue .


###  http://lpis.ec.europa.eu/registry/applicationschema/cap-iacs-parcel/code#DataQualityMeasureNameValue/numberOfLargeAreaNonConformingItems
<http://lpis.ec.europa.eu/registry/applicationschema/cap-iacs-parcel/code#DataQualityMeasureNameValue/numberOfLargeAreaNonConformingItems> rdf:type owl:NamedIndividual ,
                                                                                                                                                    <http://lpis.ec.europa.eu/registry/applicationschema/cap-iacs-parcel#DataQualityMeasureNameValue> ;
                                                                                                                                           rdfs:label "L_NANC_B"@en ;
                                                                                                                                           <http://www.w3.org/2004/02/skos/core#definition> """-- Description --
For definition and description see the corresponding value in DataQualityMeasureTypeEtsValue code list."""@en ;
                                                                                                                                           <http://www.w3.org/2004/02/skos/core#inScheme> :DataQualityMeasureNameValue .


###  http://lpis.ec.europa.eu/registry/applicationschema/cap-iacs-parcel/code#DataQualityMeasureNameValue/relativeAreaCorrectness
<http://lpis.ec.europa.eu/registry/applicationschema/cap-iacs-parcel/code#DataQualityMeasureNameValue/relativeAreaCorrectness> rdf:type owl:NamedIndividual ,
                                                                                                                                        <http://lpis.ec.europa.eu/registry/applicationschema/cap-iacs-parcel#DataQualityMeasureNameValue> ;
                                                                                                                               rdfs:label "I_RAC"@en ;
                                                                                                                               <http://www.w3.org/2004/02/skos/core#definition> """-- Description --
For definition and description see the corresponding value in DataQualityMeasureTypeIuiValue code list."""@en ;
                                                                                                                               <http://www.w3.org/2004/02/skos/core#inScheme> :DataQualityMeasureNameValue .


###  http://lpis.ec.europa.eu/registry/applicationschema/cap-iacs-parcel/code#DataQualityMeasureTypeEfaValue/areaCorrectnessDistribution
<http://lpis.ec.europa.eu/registry/applicationschema/cap-iacs-parcel/code#DataQualityMeasureTypeEfaValue/areaCorrectnessDistribution> rdf:type owl:NamedIndividual ,
                                                                                                                                               <http://lpis.ec.europa.eu/registry/applicationschema/cap-iacs-parcel#DataQualityMeasureTypeEfaValue> ;
                                                                                                                                      rdfs:label "Area correctness distribution"@en ;
                                                                                                                                      <http://www.w3.org/2004/02/skos/core#definition> """--Name--

-- Definition --
This is a placeholder only; currently not to be implemented.
Statistical distribution of  relative area correctness  values.

-- Description --
the population of relativeAreaCorrectness values defined for the following intervals: [-50%,<], [-50,-20%], [-20,-12%], [-12,-8%;], [-8,-4%,], [-4,-2%], [-2, 0%], [0, 2%], [2, 4%], [4, 8%], [8, 12%], [12, 20%], [20, 50%], [<50%]
NOTE. DQM_Measure.DQM_ValueStructure=Table"""@en ;
                                                                                                                                      <http://www.w3.org/2004/02/skos/core#inScheme> :DataQualityMeasureTypeEfaValue .


###  http://lpis.ec.europa.eu/registry/applicationschema/cap-iacs-parcel/code#DataQualityMeasureTypeEfaValue/cummulativeNumberOfMissedUpdates
<http://lpis.ec.europa.eu/registry/applicationschema/cap-iacs-parcel/code#DataQualityMeasureTypeEfaValue/cummulativeNumberOfMissedUpdates> rdf:type owl:NamedIndividual ,
                                                                                                                                                    <http://lpis.ec.europa.eu/registry/applicationschema/cap-iacs-parcel#DataQualityMeasureTypeEfaValue> ;
                                                                                                                                           rdfs:label "Cummulative number of missed updates"@en ;
                                                                                                                                           <http://www.w3.org/2004/02/skos/core#definition> """--Name--
Cumulative number of missed updates

-- Definition --
This is a placeholder only; currently not to be implemented.

Rate of undetected anomalies (changes of the land) since the last update of EFA.

-- Description --
Ratio of the abundance of missedUpdates to the number of inspected items calculated for each year and summed up starting from the year of last update."""@en ;
                                                                                                                                           <http://www.w3.org/2004/02/skos/core#inScheme> :DataQualityMeasureTypeEfaValue .


###  http://lpis.ec.europa.eu/registry/applicationschema/cap-iacs-parcel/code#DataQualityMeasureTypeEfaValue/numberOfAreaNonConformity
<http://lpis.ec.europa.eu/registry/applicationschema/cap-iacs-parcel/code#DataQualityMeasureTypeEfaValue/numberOfAreaNonConformity> rdf:type owl:NamedIndividual ,
                                                                                                                                             <http://lpis.ec.europa.eu/registry/applicationschema/cap-iacs-parcel#DataQualityMeasureTypeEfaValue> ;
                                                                                                                                    rdfs:label "Number of area non-conformity"@en ;
                                                                                                                                    <http://www.w3.org/2004/02/skos/core#definition> """--Name--
Number of area non-conformities

-- Definition --
This is a placeholder only; currently not to be implemented.

Number of non conforming inspected items within the ETS sample.

-- Description --
Count of items with itemConformance=FALSE value."""@en ;
                                                                                                                                    <http://www.w3.org/2004/02/skos/core#inScheme> :DataQualityMeasureTypeEfaValue .


###  http://lpis.ec.europa.eu/registry/applicationschema/cap-iacs-parcel/code#DataQualityMeasureTypeEfaValue/numberOfCriticalDefects
<http://lpis.ec.europa.eu/registry/applicationschema/cap-iacs-parcel/code#DataQualityMeasureTypeEfaValue/numberOfCriticalDefects> rdf:type owl:NamedIndividual ,
                                                                                                                                           <http://lpis.ec.europa.eu/registry/applicationschema/cap-iacs-parcel#DataQualityMeasureTypeEfaValue> ;
                                                                                                                                  rdfs:label "Number of critical defects"@en ;
                                                                                                                                  <http://www.w3.org/2004/02/skos/core#definition> """--Name--
Number of critical defects

-- Definition --
This is a placeholder only; currently not to be implemented.

Number of all critical defects found in course of inspection.

--Description --
The scope of this data quality measure is the critical defect property occurring  in course of inspection."""@en ;
                                                                                                                                  <http://www.w3.org/2004/02/skos/core#inScheme> :DataQualityMeasureTypeEfaValue .


###  http://lpis.ec.europa.eu/registry/applicationschema/cap-iacs-parcel/code#DataQualityMeasureTypeEfaValue/numberOfErroneousProcessing
<http://lpis.ec.europa.eu/registry/applicationschema/cap-iacs-parcel/code#DataQualityMeasureTypeEfaValue/numberOfErroneousProcessing> rdf:type owl:NamedIndividual ,
                                                                                                                                               <http://lpis.ec.europa.eu/registry/applicationschema/cap-iacs-parcel#DataQualityMeasureTypeEfaValue> ;
                                                                                                                                      rdfs:label "Number of erroneous processing "@en ;
                                                                                                                                      <http://www.w3.org/2004/02/skos/core#definition> """--Name--
Number of erroneous processing

-- Definition --
This is a placeholder only; currently not to be implemented.

Abundance of processing errors within the sample as technical cause for critical defects and non conformances.

--Description --
Occurrences of processingErrors value assigned to the items under inspection  within the sample."""@en ;
                                                                                                                                      <http://www.w3.org/2004/02/skos/core#inScheme> :DataQualityMeasureTypeEfaValue .


###  http://lpis.ec.europa.eu/registry/applicationschema/cap-iacs-parcel/code#DataQualityMeasureTypeEfaValue/numberOfIncompatibleDesign
<http://lpis.ec.europa.eu/registry/applicationschema/cap-iacs-parcel/code#DataQualityMeasureTypeEfaValue/numberOfIncompatibleDesign> rdf:type owl:NamedIndividual ,
                                                                                                                                              <http://lpis.ec.europa.eu/registry/applicationschema/cap-iacs-parcel#DataQualityMeasureTypeEfaValue> ;
                                                                                                                                     rdfs:label "Number of incompatible design"@en ;
                                                                                                                                     <http://www.w3.org/2004/02/skos/core#definition> """--Name--
Number of incompatible design

-- Definition --
This is a placeholder only; currently not to be implemented.

Abundance of incompatible design instances within the sample as technical cause for critical defects and non conformances.

--Description --
Occurrences of incompatibelDesign value assigned to the items under inspection within the sample."""@en ;
                                                                                                                                     <http://www.w3.org/2004/02/skos/core#inScheme> :DataQualityMeasureTypeEfaValue .


###  http://lpis.ec.europa.eu/registry/applicationschema/cap-iacs-parcel/code#DataQualityMeasureTypeEfaValue/numberOfIncompleteProcessing
<http://lpis.ec.europa.eu/registry/applicationschema/cap-iacs-parcel/code#DataQualityMeasureTypeEfaValue/numberOfIncompleteProcessing> rdf:type owl:NamedIndividual ,
                                                                                                                                                <http://lpis.ec.europa.eu/registry/applicationschema/cap-iacs-parcel#DataQualityMeasureTypeEfaValue> ;
                                                                                                                                       rdfs:label "Number of incomplete processing"@en ;
                                                                                                                                       <http://www.w3.org/2004/02/skos/core#definition> """--Name--
Number of incomplete processing

-- Definition --
This is a placeholder only; currently not to be implemented.

Abundance of incomplete processing instances within the sample as technical cause for critical defects and non conformances.

--Description --
Occurrences of incompleteProcessing value assigned to the items under inspection within the sample."""@en ;
                                                                                                                                       <http://www.w3.org/2004/02/skos/core#inScheme> :DataQualityMeasureTypeEfaValue .


###  http://lpis.ec.europa.eu/registry/applicationschema/cap-iacs-parcel/code#DataQualityMeasureTypeEfaValue/numberOfMissedUpdate
<http://lpis.ec.europa.eu/registry/applicationschema/cap-iacs-parcel/code#DataQualityMeasureTypeEfaValue/numberOfMissedUpdate> rdf:type owl:NamedIndividual ,
                                                                                                                                        <http://lpis.ec.europa.eu/registry/applicationschema/cap-iacs-parcel#DataQualityMeasureTypeEfaValue> ;
                                                                                                                               rdfs:label "Number of missed updates"@en ;
                                                                                                                               <http://www.w3.org/2004/02/skos/core#definition> """--Name--
Number of missed updates

-- Definition --
This is a placeholder only; currently not to be implemented.

Abundance of missed updates within the sample as technical cause for critical defects and non conformances.

--Description --
Occurrences of missedUpdate value assigned to the items under inspection within the sample."""@en ;
                                                                                                                               <http://www.w3.org/2004/02/skos/core#inScheme> :DataQualityMeasureTypeEfaValue .


###  http://lpis.ec.europa.eu/registry/applicationschema/cap-iacs-parcel/code#DataQualityMeasureTypeEfaValue/numberOfMissedUpgrades
<http://lpis.ec.europa.eu/registry/applicationschema/cap-iacs-parcel/code#DataQualityMeasureTypeEfaValue/numberOfMissedUpgrades> rdf:type owl:NamedIndividual ,
                                                                                                                                          <http://lpis.ec.europa.eu/registry/applicationschema/cap-iacs-parcel#DataQualityMeasureTypeEfaValue> ;
                                                                                                                                 rdfs:label "Number of missed upgrades"@en ;
                                                                                                                                 <http://www.w3.org/2004/02/skos/core#definition> """--Name--
Number of Missed upgrades

-- Definition --
This is a placeholder only; currently not to be implemented.

Abundance of missed upgrades within the sample as technical cause for critical defects and non conformances.

--Description --
Occurrences of missedUpgrade value assigned to the items under inspection within the sample."""@en ;
                                                                                                                                 <http://www.w3.org/2004/02/skos/core#inScheme> :DataQualityMeasureTypeEfaValue .


###  http://lpis.ec.europa.eu/registry/applicationschema/cap-iacs-parcel/code#DataQualityMeasureTypeEfaValue/relativeAreaCorrectness
<http://lpis.ec.europa.eu/registry/applicationschema/cap-iacs-parcel/code#DataQualityMeasureTypeEfaValue/relativeAreaCorrectness> rdf:type owl:NamedIndividual ,
                                                                                                                                           <http://lpis.ec.europa.eu/registry/applicationschema/cap-iacs-parcel#DataQualityMeasureTypeEfaValue> ;
                                                                                                                                  rdfs:label "Relative area correctness"@en ;
                                                                                                                                  <http://www.w3.org/2004/02/skos/core#definition> """--Name--
EFA relative  area correctness

--Definition --
This is a placeholder only; currently not to be implemented.

Ratio of the total area  observed  in course of EFA to the sum of EFA areas of  the corresponding  items. 

-- Description --
The ratio shall be expressed in percentages."""@en ;
                                                                                                                                  <http://www.w3.org/2004/02/skos/core#inScheme> :DataQualityMeasureTypeEfaValue .


###  http://lpis.ec.europa.eu/registry/applicationschema/cap-iacs-parcel/code#DataQualityMeasureTypeEtsValue/areaCorrectnessDistribution
<http://lpis.ec.europa.eu/registry/applicationschema/cap-iacs-parcel/code#DataQualityMeasureTypeEtsValue/areaCorrectnessDistribution> rdf:type owl:NamedIndividual ,
                                                                                                                                               <http://lpis.ec.europa.eu/registry/applicationschema/cap-iacs-parcel#DataQualityMeasureTypeEtsValue> ;
                                                                                                                                      rdfs:label "QE2b"@en ;
                                                                                                                                      <http://www.w3.org/2004/02/skos/core#definition> """--Name--
Area correctness distribution

-- Definition --
Statistical distribution of relative area correctness values.

-- Description --
The population of relativeAreaCorrectness values defined for the following intervals: 
- [-50%,<], (-50,-20%], (-20,-12%], (-12,-8%;], (-8,-4%,], (-4,-2%],  (-2, 0%], (0, 2%], (2, 4%], (4, 8%], (8, 12%], (12, 20%], (20, 50%], (<50%]

Measure identifier: L_ACD
Name: Area correctness distribution
Alias: QE2b
Element name: Relatives or internal accuracy
Value type: Measure
Value Structure: sequence (table)

NOTE 1: Previously named as  10203 LPIS_RP_SEA

NOTE 2: DQM_Measure.DQM_ValueStructure=Sequence (previously was Table)."""@en ;
                                                                                                                                      <http://www.w3.org/2004/02/skos/core#inScheme> :DataQualityMeasureTypeEtsValue .


###  http://lpis.ec.europa.eu/registry/applicationschema/cap-iacs-parcel/code#DataQualityMeasureTypeEtsValue/conformityClass1
<http://lpis.ec.europa.eu/registry/applicationschema/cap-iacs-parcel/code#DataQualityMeasureTypeEtsValue/conformityClass1> rdf:type owl:NamedIndividual ,
                                                                                                                                    <http://lpis.ec.europa.eu/registry/applicationschema/cap-iacs-parcel#DataQualityMeasureTypeEtsValue> ;
                                                                                                                           rdfs:label "First conformance class"@en ;
                                                                                                                           <http://www.w3.org/2004/02/skos/core#definition> """--Name--
Conformity to class 1

-- Definition --
Conformance class as defined in Article 6 (1) of EU 640/2014.

-- Description --
It is the aggregated quality measure of the conformance results of QE1, QE2, and QE3.  In order to pass, each composing element shall be conforming.

Measure identifier: L_CLASS1
Name: Conformity with class 1
Alias: First conformance class
Element name: Conceptual consistency
Basic measure: Error indicator
Value type: Boolean
Value Structure: n.a."""@en ;
                                                                                                                           <http://www.w3.org/2004/02/skos/core#inScheme> :DataQualityMeasureTypeEtsValue .


###  http://lpis.ec.europa.eu/registry/applicationschema/cap-iacs-parcel/code#DataQualityMeasureTypeEtsValue/conformityClass2
<http://lpis.ec.europa.eu/registry/applicationschema/cap-iacs-parcel/code#DataQualityMeasureTypeEtsValue/conformityClass2> rdf:type owl:NamedIndividual ,
                                                                                                                                    <http://lpis.ec.europa.eu/registry/applicationschema/cap-iacs-parcel#DataQualityMeasureTypeEtsValue> ;
                                                                                                                           rdfs:label "Second Conformnace Class"@en ;
                                                                                                                           <http://www.w3.org/2004/02/skos/core#definition> """--Name--
Conformity to class 2

-- Definition --
Conformance class as defined in Article 6 (1) of EU 640/2014.

-- Description --
It is the aggregated quality measure of the conformance results of QE4, QE5 and QE6.  In order to pass, each composing element must pass the test.
Since at the moment no conformance for QE4 and QE5 are defined, the value of this element coincides with the values of QE6.

Measure identifier: L_CLASS2
Name: Conformity with class 2
Alias: Second conformance class
Element name: Conceptual consistency
Basic measure: Error indicator
Value type: Boolean
Value Structure: n.a."""@en ;
                                                                                                                           <http://www.w3.org/2004/02/skos/core#inScheme> :DataQualityMeasureTypeEtsValue .


###  http://lpis.ec.europa.eu/registry/applicationschema/cap-iacs-parcel/code#DataQualityMeasureTypeEtsValue/cumulativeRateOfMissedUpdates
<http://lpis.ec.europa.eu/registry/applicationschema/cap-iacs-parcel/code#DataQualityMeasureTypeEtsValue/cumulativeRateOfMissedUpdates> rdf:type owl:NamedIndividual ,
                                                                                                                                                 <http://lpis.ec.europa.eu/registry/applicationschema/cap-iacs-parcel#DataQualityMeasureTypeEtsValue> ;
                                                                                                                                        rdfs:label "10207 LPIS_RP_CMC"@en ;
                                                                                                                                        <http://www.w3.org/2004/02/skos/core#definition> """--Name--
Cumulative rate of missed updates

-- Definition --
Rate of undetected anomalies (changes of the land) since the last update of LPIS.

-- Description --
Ratio of the abundance of missedUpdates to the number of inspected items calculated for each year and summed up starting from the year of last update (refresh).

Measure identifier: L_CRMU
Name: Cumulative rate of missed updates
Alias:  Missed updated accumulation
Element name: Non-quantitative attribute correctness
Basic measure: Error rate
Value type: Real. The value shall be expressed in %.
Value Structure: n.a.

NOTE. Previouslynamed QE6, 10207 LPIS_RP_CMC"""@en ;
                                                                                                                                        <http://www.w3.org/2004/02/skos/core#inScheme> :DataQualityMeasureTypeEtsValue .


###  http://lpis.ec.europa.eu/registry/applicationschema/cap-iacs-parcel/code#DataQualityMeasureTypeEtsValue/lpisAreaAccuracyConformance
<http://lpis.ec.europa.eu/registry/applicationschema/cap-iacs-parcel/code#DataQualityMeasureTypeEtsValue/lpisAreaAccuracyConformance> rdf:type owl:NamedIndividual ,
                                                                                                                                               <http://lpis.ec.europa.eu/registry/applicationschema/cap-iacs-parcel#DataQualityMeasureTypeEtsValue> ;
                                                                                                                                      rdfs:label "QE1 confromance"@en ;
                                                                                                                                      <http://www.w3.org/2004/02/skos/core#definition> """--Name--
LPIS area accuracy conformance

-- Definition --
Assessment of correct quantification of the maximum eligible area according to EU 640/2014 Art. 6.1(a). 

-- Description --
Conformance statement on area quantification. The threshold is +/- 2%.

Measure identifier: L_RACON
Name: LPIS area accuracy correctness
Alias: QE1 conformance
Element name: Conceptual consistency
Basic measure: Error indicator
Value type: Boolean
Value Structure: n.a.

NOTE. Previously named: QE 1A"""@en ;
                                                                                                                                      <http://www.w3.org/2004/02/skos/core#inScheme> :DataQualityMeasureTypeEtsValue .


###  http://lpis.ec.europa.eu/registry/applicationschema/cap-iacs-parcel/code#DataQualityMeasureTypeEtsValue/lpisAreaOverestimates
<http://lpis.ec.europa.eu/registry/applicationschema/cap-iacs-parcel/code#DataQualityMeasureTypeEtsValue/lpisAreaOverestimates> rdf:type owl:NamedIndividual ,
                                                                                                                                         <http://lpis.ec.europa.eu/registry/applicationschema/cap-iacs-parcel#DataQualityMeasureTypeEtsValue> ;
                                                                                                                                rdfs:label "LPIS lower interval boundary"@en ;
                                                                                                                                <http://www.w3.org/2004/02/skos/core#definition> """--Name--
LPIS area overestimates

-- Definition --
One-sided probability boundary of the rate of the eligible hectares that indicate overestimations found in respect to the total number of eligible hectares currently recorded in the LPIS.

--Description --
Technical definition: Lower Interval Boundary (LIB)
Calculation method: LIB=OER-1,6449xOERxstdev(OER)

Measure identifier: L_AOE
Name: LPIS area overestimates
Alias: LPIS lower interval boundary
Element name: Quantitative attribute accuracy
Basic measure: LE 98
Value type: Measure
Value Structure: n.a.

NOTE. Previously it was known as part of 10201_2 LPIS_RP_MEA_B"""@en ;
                                                                                                                                <http://www.w3.org/2004/02/skos/core#inScheme> :DataQualityMeasureTypeEtsValue .


###  http://lpis.ec.europa.eu/registry/applicationschema/cap-iacs-parcel/code#DataQualityMeasureTypeEtsValue/lpisAreaPrecisionConformance
<http://lpis.ec.europa.eu/registry/applicationschema/cap-iacs-parcel/code#DataQualityMeasureTypeEtsValue/lpisAreaPrecisionConformance> rdf:type owl:NamedIndividual ,
                                                                                                                                                <http://lpis.ec.europa.eu/registry/applicationschema/cap-iacs-parcel#DataQualityMeasureTypeEtsValue> ;
                                                                                                                                       rdfs:label "Over- and underestimate conformance"@en ;
                                                                                                                                       <http://www.w3.org/2004/02/skos/core#definition> """--Name--
LPIS area precision conformance

-- Definition --
Assessment of the severity of area under-and overestimates as required by Eu 640/2014 Art. 6.1(b).

-- Description --
Conformance statement on the severity of area under and overestimates.
Conformity thresholds: LIB>=-2%, UIB<=2%.

Measure identifier: L_APCON
Name: LPIS area precision conformance
Alias:  LPIS area over- and underestimate conformance
Element name: Conceptual consistency
Basic measure: Error indicator
Value type: Boolean
Value Structure: n.a.

NOTE. Previously known as part of QE1B or 10201_2 LPIS_RP_MEA_B"""@en ;
                                                                                                                                       <http://www.w3.org/2004/02/skos/core#inScheme> :DataQualityMeasureTypeEtsValue .


###  http://lpis.ec.europa.eu/registry/applicationschema/cap-iacs-parcel/code#DataQualityMeasureTypeEtsValue/lpisAreaUnderestimates
<http://lpis.ec.europa.eu/registry/applicationschema/cap-iacs-parcel/code#DataQualityMeasureTypeEtsValue/lpisAreaUnderestimates> rdf:type owl:NamedIndividual ,
                                                                                                                                          <http://lpis.ec.europa.eu/registry/applicationschema/cap-iacs-parcel#DataQualityMeasureTypeEtsValue> ;
                                                                                                                                 rdfs:label "LPIS upper interval boundary"@en ;
                                                                                                                                 <http://www.w3.org/2004/02/skos/core#definition> """--Name--
LPIS area underestimates

-- Definition --
One-sided probability boundary of the rate if the eligible hectares that indicate underestimation found in respect to the total number of eligible hectares currently recorded in the LPIS . 

-- Description --
Technical definition: Upper Interval Boundary
Calculation method: UIB=UER-1,6449xUERxstdev(UER)

Measure identifier: L_AUE
Name: LPIS area underestimates
Alias: LPIS upper interval boundary
Element name: Quantitative attribute accuracy
Definition: LE98
Value type: Measure
Value Structure: n.a.

NOTE. Previously named as 10201_2 LPIS_RP_MEA_B"""@en ;
                                                                                                                                 <http://www.w3.org/2004/02/skos/core#inScheme> :DataQualityMeasureTypeEtsValue .


###  http://lpis.ec.europa.eu/registry/applicationschema/cap-iacs-parcel/code#DataQualityMeasureTypeEtsValue/lpisCriticalDefectConformance
<http://lpis.ec.europa.eu/registry/applicationschema/cap-iacs-parcel/code#DataQualityMeasureTypeEtsValue/lpisCriticalDefectConformance> rdf:type owl:NamedIndividual ,
                                                                                                                                                 <http://lpis.ec.europa.eu/registry/applicationschema/cap-iacs-parcel#DataQualityMeasureTypeEtsValue> ;
                                                                                                                                        rdfs:label "QE3"@en ;
                                                                                                                                        <http://www.w3.org/2004/02/skos/core#definition> """--Name--
LPIS critical defect conformance

-- Definition --
Achievement of the acceptance number prescribed for critical defects for the given lot. 

-- Description --
For conformance the number of critical defects shall not exceed the value of criticalDefectAcceptanceNumber selected in function of the lot size and LQ=2,0.

Measure identifier: L_CDCON
Name: LPIS critical defect conformance
Alias: QE3
Element name: Conceptual consistency
Basic measure: Error indicator
Value type: Boolean
Value Structure: n.a.

NOTE. Previously named QE4,10205 LPIS_RP_CRA."""@en ;
                                                                                                                                        <http://www.w3.org/2004/02/skos/core#inScheme> :DataQualityMeasureTypeEtsValue .


###  http://lpis.ec.europa.eu/registry/applicationschema/cap-iacs-parcel/code#DataQualityMeasureTypeEtsValue/lpisItemConformance
<http://lpis.ec.europa.eu/registry/applicationschema/cap-iacs-parcel/code#DataQualityMeasureTypeEtsValue/lpisItemConformance> rdf:type owl:NamedIndividual ,
                                                                                                                                       <http://lpis.ec.europa.eu/registry/applicationschema/cap-iacs-parcel#DataQualityMeasureTypeEtsValue> ;
                                                                                                                              rdfs:label "QE2a"@en ;
                                                                                                                              <http://www.w3.org/2004/02/skos/core#definition> """--Name--
LPIS item conformnace

-- Definition --
Achievement of the value of the acceptance number prescribed for the area based quality measures.

-- Description --
Conformance statement whether the number of non-conforming item has exceeded the acceptance number.
  
Measure identifier: L_ICON
Name: LPIS item conformance
Alias: QE2a
Element name: Conceptual consistency
Basic measure: Error indicator
Value type: Boolean
Value Structure: n.a.

NOTE. Previously known as number of non-conforming reference parcels in LPIS, or 10202 LPIS_RP_NEA"""@en ;
                                                                                                                              <http://www.w3.org/2004/02/skos/core#inScheme> :DataQualityMeasureTypeEtsValue .


###  http://lpis.ec.europa.eu/registry/applicationschema/cap-iacs-parcel/code#DataQualityMeasureTypeEtsValue/lpisRelativeAreaCorrectness
<http://lpis.ec.europa.eu/registry/applicationschema/cap-iacs-parcel/code#DataQualityMeasureTypeEtsValue/lpisRelativeAreaCorrectness> rdf:type owl:NamedIndividual ,
                                                                                                                                               <http://lpis.ec.europa.eu/registry/applicationschema/cap-iacs-parcel#DataQualityMeasureTypeEtsValue> ;
                                                                                                                                      rdfs:label "LPIS maximum eligible area correctness"@en ;
                                                                                                                                      <http://www.w3.org/2004/02/skos/core#definition> """--Name--
LPIS relative area correctness

--Definition --
Ratio of the total observed area in course of ETS to the sum of reference area of the corresponding parcels.

-- Description --
Measure identifier: L_RAC
Name: LPIS relative area correctness
Alias: LPIS maximum eligible area correctness
Element name: Relative or internal accuracy
Basic measure: Error rate
Value type: Measure. The ratio shall be expressed in percentages.
Value Structure: n.a.

NOTE. Previously named: 10201 LPIS_RP_MEA"""@en ;
                                                                                                                                      <http://www.w3.org/2004/02/skos/core#inScheme> :DataQualityMeasureTypeEtsValue .


###  http://lpis.ec.europa.eu/registry/applicationschema/cap-iacs-parcel/code#DataQualityMeasureTypeEtsValue/misclassificationMatrix
<http://lpis.ec.europa.eu/registry/applicationschema/cap-iacs-parcel/code#DataQualityMeasureTypeEtsValue/misclassificationMatrix> rdf:type owl:NamedIndividual ,
                                                                                                                                           <http://lpis.ec.europa.eu/registry/applicationschema/cap-iacs-parcel#DataQualityMeasureTypeEtsValue> ;
                                                                                                                                  rdfs:label "Misclassification matrix"@en ;
                                                                                                                                  <http://www.w3.org/2004/02/skos/core#definition> """--Name--
Misclassification matrix

-- Definition --
Misclassification matrix comparing the assignment of LC types registered in LPIS to the LC types observed in course of inspection.

-- Description --
All land cover types (both agricultural land and landscape feature) enter in the evaluation process. 

Measure identifier: L_MCM
Name: LPIS misclassification matrix
Alias: LC confusion matrix
Element name: Classification correctness
Basic measure: n.a.
Value type: Measure
Value Structure:  Matrix

NOTE 1: Classifying one pro-rata grassland type to another pro-rata class is considered as a misclassification instance.

NOTE 2: This is an indicative measure for self-evaluation, which is not required by regulation EU 640/2014.

NOTE 3: This is a DQM directly taken from IOS 19157:2013 (see table D.65)."""@en ;
                                                                                                                                  <http://www.w3.org/2004/02/skos/core#inScheme> :DataQualityMeasureTypeEtsValue .


###  http://lpis.ec.europa.eu/registry/applicationschema/cap-iacs-parcel/code#DataQualityMeasureTypeEtsValue/numberOfAreaNonConformingItems
<http://lpis.ec.europa.eu/registry/applicationschema/cap-iacs-parcel/code#DataQualityMeasureTypeEtsValue/numberOfAreaNonConformingItems> rdf:type owl:NamedIndividual ,
                                                                                                                                                  <http://lpis.ec.europa.eu/registry/applicationschema/cap-iacs-parcel#DataQualityMeasureTypeEtsValue> ;
                                                                                                                                         rdfs:label "Number of area non-conforming items"@en ;
                                                                                                                                         <http://www.w3.org/2004/02/skos/core#definition> """--Name--
Number of area non-conformities

-- Definition --
Number of area non-conforming inspected items (N1) within the ETS sample.

-- Description --
Count of items with itemConformance (area)=FALSE value.  

Measure identifier: L_NANC_A
Name: Number of area non-conforming items
Alias: Item area non conformity number
Element name: Conceptual consistency
Basic measure: Error count
Value type: Number
Value Structure: n.a."""@en ;
                                                                                                                                         <http://www.w3.org/2004/02/skos/core#inScheme> :DataQualityMeasureTypeEtsValue .


###  http://lpis.ec.europa.eu/registry/applicationschema/cap-iacs-parcel/code#DataQualityMeasureTypeEtsValue/numberOfCriticalDefects
<http://lpis.ec.europa.eu/registry/applicationschema/cap-iacs-parcel/code#DataQualityMeasureTypeEtsValue/numberOfCriticalDefects> rdf:type owl:NamedIndividual ,
                                                                                                                                           <http://lpis.ec.europa.eu/registry/applicationschema/cap-iacs-parcel#DataQualityMeasureTypeEtsValue> ;
                                                                                                                                  rdfs:label "LPIS Critical Defects"@en ;
                                                                                                                                  <http://www.w3.org/2004/02/skos/core#definition> """--Name--
Number of critical defects

-- Definition --
Number of all critical defects (M) found in course of inspection.

--Description --
The scope of this data quality measure is the critical defect property (instances of critical defects) occurring  in course of inspection,

Measure identifier: L_NCD
Name: LPIS number of critical defects
Alias: LPIS critical defects
Element name: Conceptual consistency
Basic measure: Error count
Value type: Number
Value Structure: n.a.

NOTE. Previously named as 10205 LPIS_RP_CRA"""@en ;
                                                                                                                                  <http://www.w3.org/2004/02/skos/core#inScheme> :DataQualityMeasureTypeEtsValue .


###  http://lpis.ec.europa.eu/registry/applicationschema/cap-iacs-parcel/code#DataQualityMeasureTypeEtsValue/numberOfLargeAreaNonConformingItems
<http://lpis.ec.europa.eu/registry/applicationschema/cap-iacs-parcel/code#DataQualityMeasureTypeEtsValue/numberOfLargeAreaNonConformingItems> rdf:type owl:NamedIndividual ,
                                                                                                                                                       <http://lpis.ec.europa.eu/registry/applicationschema/cap-iacs-parcel#DataQualityMeasureTypeEtsValue> ;
                                                                                                                                              rdfs:label "Number of area >0,1 ha non-conforming items"@en ;
                                                                                                                                              <http://www.w3.org/2004/02/skos/core#definition> """--Name--
Number of large area non-conformities

-- Definition --
Number of non-conforming inspected items (N2) with area >0,1 ha within the ETS sample.

-- Description --
Count of items with itemConformance (area)=FALSE value. 
  
Measure identifier: L_NANC_B
Name: Number of area non-conforming items
Alias: Item area non conformity number
Element name: Conceptual consistency
Basic measure: Error count
Value type: Number
Value Structure: n.a."""@en ;
                                                                                                                                              <http://www.w3.org/2004/02/skos/core#inScheme> :DataQualityMeasureTypeEtsValue .


###  http://lpis.ec.europa.eu/registry/applicationschema/cap-iacs-parcel/code#DataQualityMeasureTypeIuiCcValue/classificationCorrectness
<http://lpis.ec.europa.eu/registry/applicationschema/cap-iacs-parcel/code#DataQualityMeasureTypeIuiCcValue/classificationCorrectness> rdf:type owl:NamedIndividual ,
                                                                                                                                               <http://lpis.ec.europa.eu/registry/applicationschema/cap-iacs-parcel#DataQualityMeasureTypeIuiCcValue> ;
                                                                                                                                      rdfs:label "Classification correctness"@en ;
                                                                                                                                      <http://www.w3.org/2004/02/skos/core#definition> """--Name--
Classification correctness

-- Definition --
Thematic classification correctness as defined in ISO 19157:2013.

-- Description --
Thematic classification correctness applied to the land cover class.

EXAMPLE:  A MS has defined Hedge landscape feature and Line of trees landscape feature. Attributing an instance of hedge to line of trees class is a classification error.

NOTE 1. The correct classification and quantification of the land cover types (arable/PC) is directly used for assessing the exemption for the green payments (EFA, crop diversification)

NOTE 2. The correct classification of the grassland is relevant because it acts as a threshold fors crop diversification. Certain types of grassland (pro-rata or not) are subject to specific requirements and therefore need to be distinguished (thus recorded).  In general, such detailed inspection triggers a better understanding of the pro-rata behaviour in the LPIS.
NOTE 3. Each pro-rata type shall be regarded as a separate land cover class For example permanent grassland of 50% is one class, and permanent grassland  90%  is another class. Therefore classifying an instance of permanent grassland of 50% to class permanent grassland  90%  a  is a classification error (like in the example above with the hedge and line of trees)."""@en ;
                                                                                                                                      <http://www.w3.org/2004/02/skos/core#inScheme> :DataQualityMeasureTypeIuiCcValue .


###  http://lpis.ec.europa.eu/registry/applicationschema/cap-iacs-parcel/code#DataQualityMeasureTypeIuiEfaValue/efaClassificationCorrectness
<http://lpis.ec.europa.eu/registry/applicationschema/cap-iacs-parcel/code#DataQualityMeasureTypeIuiEfaValue/efaClassificationCorrectness> rdf:type owl:NamedIndividual ,
                                                                                                                                                   <http://lpis.ec.europa.eu/registry/applicationschema/cap-iacs-parcel#DataQualityMeasureTypeIuiEfaValue> ;
                                                                                                                                          rdfs:label "EFA classification correctness"@en ;
                                                                                                                                          <http://www.w3.org/2004/02/skos/core#definition> """--Name--
EFA classification correctness

- Definition --
This is a placeholder only; currently not to be implemented.

Thematic classification correctness. The assignment of an item to a certain class can either be correct or incorrect. [ISO 19157].

-- Description --
Thematic classification correctness applied to the EFA.
NOTE. Must have separate DQM_Measure description."""@en ;
                                                                                                                                          <http://www.w3.org/2004/02/skos/core#inScheme> :DataQualityMeasureTypeIuiEfaValue .


###  http://lpis.ec.europa.eu/registry/applicationschema/cap-iacs-parcel/code#DataQualityMeasureTypeIuiEfaValue/efaRelativeAreaConformance
<http://lpis.ec.europa.eu/registry/applicationschema/cap-iacs-parcel/code#DataQualityMeasureTypeIuiEfaValue/efaRelativeAreaConformance> rdf:type owl:NamedIndividual ,
                                                                                                                                                 <http://lpis.ec.europa.eu/registry/applicationschema/cap-iacs-parcel#DataQualityMeasureTypeIuiEfaValue> ;
                                                                                                                                        rdfs:label "EFA relative area conformance"@en ;
                                                                                                                                        <http://www.w3.org/2004/02/skos/core#definition> """--Name--
EFA relative area correctness

-- Definition --
This is a placeholder only; currently not to be implemented.

Conformance statement applicable on the value of relative area correctness.

-- Description --
The conformance thresholds are area dependent.
NOTE. Must have separate DQM_Measure description."""@en ;
                                                                                                                                        <http://www.w3.org/2004/02/skos/core#inScheme> :DataQualityMeasureTypeIuiEfaValue .


###  http://lpis.ec.europa.eu/registry/applicationschema/cap-iacs-parcel/code#DataQualityMeasureTypeIuiValue/areaConformance
<http://lpis.ec.europa.eu/registry/applicationschema/cap-iacs-parcel/code#DataQualityMeasureTypeIuiValue/areaConformance> rdf:type owl:NamedIndividual ,
                                                                                                                                   <http://lpis.ec.europa.eu/registry/applicationschema/cap-iacs-parcel#DataQualityMeasureTypeIuiValue> ;
                                                                                                                          rdfs:label "Area conformance"@en ;
                                                                                                                          <http://www.w3.org/2004/02/skos/core#definition> """--Name--
Area conformance

--Definition --
Conformance statement based on the value of relative area correctness. 

-- Description --
The conformance thresholds are area dependent:
- area >5000 sq.m. : 97,00% - 103,00% conforming;
- 2000 sq.m.<area<5000 sq.m.: 95% - 105% conforming;
- area<2000 sq.m.: 93%-107% conforming.

Measure identifier: I_ACON
Name: Item area conformance
Alias: Parcel area conformance
Element name: Domain consistency
Basic measure: Error indicator
Value type: Boolean
Value Structure: n.a.

NOTE. Previously  it was part of RP conformance - code list for conformance level."""@en ;
                                                                                                                          <http://www.w3.org/2004/02/skos/core#inScheme> :DataQualityMeasureTypeIuiValue .


###  http://lpis.ec.europa.eu/registry/applicationschema/cap-iacs-parcel/code#DataQualityMeasureTypeIuiValue/areaDifferenceCorrectness
<http://lpis.ec.europa.eu/registry/applicationschema/cap-iacs-parcel/code#DataQualityMeasureTypeIuiValue/areaDifferenceCorrectness> rdf:type owl:NamedIndividual ,
                                                                                                                                             <http://lpis.ec.europa.eu/registry/applicationschema/cap-iacs-parcel#DataQualityMeasureTypeIuiValue> ;
                                                                                                                                    rdfs:label "Area difference correctness"@en ;
                                                                                                                                    <http://www.w3.org/2004/02/skos/core#definition> """--Name--
Area difference correctness

-- Definition --
Difference between eligible recorded area and observed area.

-- Description --
Measure identifier: I_ADC
Name: Area difference correctness
Alias: Area difference accuracy
Element name: Relative  or internal accuracy
Value type: Measure
Value Structure: n.a.

NOTE 1: This measure is applicable for parcels >10000 sq.m.

NOTE 2: Previously named: RP conformance (area purity) v2, 10102 RP_CNF."""@en ;
                                                                                                                                    <http://www.w3.org/2004/02/skos/core#inScheme> :DataQualityMeasureTypeIuiValue .


###  http://lpis.ec.europa.eu/registry/applicationschema/cap-iacs-parcel/code#DataQualityMeasureTypeIuiValue/itemConformance
<http://lpis.ec.europa.eu/registry/applicationschema/cap-iacs-parcel/code#DataQualityMeasureTypeIuiValue/itemConformance> rdf:type owl:NamedIndividual ,
                                                                                                                                   <http://lpis.ec.europa.eu/registry/applicationschema/cap-iacs-parcel#DataQualityMeasureTypeIuiValue> ;
                                                                                                                          rdfs:label "Parcel conformance"@en ;
                                                                                                                          <http://www.w3.org/2004/02/skos/core#definition> """--Name--
Item conformance

-- Definition --
Conformance statement on the item under inspection.

-- Description --
The item under inspection is conforming when no associated feature type is misclassified, it is contamination free or the contaminations found are waivered, and it is conforming in terms of area. The values of classificationCorrectness, waivered and areaConformance shall be true.
NOTE: since the conformance in term of critical defect is evaluated separately, the scope of this measure does not contain critical defects. 

Measure identifier: I_CON
Name: Item conformance
Alias: Parcel conformance
Element name: Domain consistency
Basic measure: Error indicator
Value type: Boolean
Value Structure: n.a."""@en ;
                                                                                                                          <http://www.w3.org/2004/02/skos/core#inScheme> :DataQualityMeasureTypeIuiValue .


###  http://lpis.ec.europa.eu/registry/applicationschema/cap-iacs-parcel/code#DataQualityMeasureTypeIuiValue/itemContaminationConformance
<http://lpis.ec.europa.eu/registry/applicationschema/cap-iacs-parcel/code#DataQualityMeasureTypeIuiValue/itemContaminationConformance> rdf:type owl:NamedIndividual ,
                                                                                                                                                <http://lpis.ec.europa.eu/registry/applicationschema/cap-iacs-parcel#DataQualityMeasureTypeIuiValue> ;
                                                                                                                                       rdfs:label "Contamination conformance"@en ;
                                                                                                                                       <http://www.w3.org/2004/02/skos/core#definition> """--Name--
Item contamination conformance

-- Definition --
Conformance statement on the value of contaminations.

-- Description --
The item is conforming when t is contamination free, or the contaminations found are waivered. 

Measure identifier: I_CCON
Name: Item contamination conformance
Alias: Parcel contamination conformance
Element name: Domain consistency
Basic measure: Error indicator
Value type: Boolean
Value Structure: n.a."""@en ;
                                                                                                                                       <http://www.w3.org/2004/02/skos/core#inScheme> :DataQualityMeasureTypeIuiValue .


###  http://lpis.ec.europa.eu/registry/applicationschema/cap-iacs-parcel/code#DataQualityMeasureTypeIuiValue/itemCriticalDefectConformance
<http://lpis.ec.europa.eu/registry/applicationschema/cap-iacs-parcel/code#DataQualityMeasureTypeIuiValue/itemCriticalDefectConformance> rdf:type owl:NamedIndividual ,
                                                                                                                                                 <http://lpis.ec.europa.eu/registry/applicationschema/cap-iacs-parcel#DataQualityMeasureTypeIuiValue> ;
                                                                                                                                        rdfs:label "Critical defect conformance"@en ;
                                                                                                                                        <http://www.w3.org/2004/02/skos/core#definition> """--Name--
Critical defect conformance

--Definition --
Conformance statement based on the detection of critical defect conditions.

-- Description --
The item under inspection is conforming when no critical defect occurs (i.e. the multiplicity of the association role from ItemUnderInspection to CriticalDefect is zero).

Measure identifier: I_CDCON
Name: Item critical defect conformance
Alias: Critical defect conformance
Element name: Domain consistency
Value type: Boolean
Value Structure: n.a."""@en ;
                                                                                                                                        <http://www.w3.org/2004/02/skos/core#inScheme> :DataQualityMeasureTypeIuiValue .


###  http://lpis.ec.europa.eu/registry/applicationschema/cap-iacs-parcel/code#DataQualityMeasureTypeIuiValue/relativeAreaCorrectness
<http://lpis.ec.europa.eu/registry/applicationschema/cap-iacs-parcel/code#DataQualityMeasureTypeIuiValue/relativeAreaCorrectness> rdf:type owl:NamedIndividual ,
                                                                                                                                           <http://lpis.ec.europa.eu/registry/applicationschema/cap-iacs-parcel#DataQualityMeasureTypeIuiValue> ;
                                                                                                                                  rdfs:label "Relative area correctness"@en ;
                                                                                                                                  <http://www.w3.org/2004/02/skos/core#definition> """--Name--
Relative area correctness

-- Definition --
Ability of the reference area to quantify the area of all eligible land cover types present in the inspected item. 

-- Description --
Measure identifier: I_RAC
Name: Relative area correctness
Alias: Relative area accuracy
Element name: Relative or internal accuracy
Basic measure: Error rate
Value type: Measure. Result output shall be provided in %.
Value Structure: n.a.

NOTE. Previously named: 10101 RP_MEA."""@en ;
                                                                                                                                  <http://www.w3.org/2004/02/skos/core#inScheme> :DataQualityMeasureTypeIuiValue .


###  http://lpis.ec.europa.eu/registry/applicationschema/cap-iacs-parcel/code#DataQualityMeasureValueStructureValue/bag
<http://lpis.ec.europa.eu/registry/applicationschema/cap-iacs-parcel/code#DataQualityMeasureValueStructureValue/bag> rdf:type owl:NamedIndividual ,
                                                                                                                              <http://lpis.ec.europa.eu/registry/applicationschema/cap-iacs-parcel#DataQualityMeasureValueStructureValue> ;
                                                                                                                     rdfs:label "Bag"@en ;
                                                                                                                     <http://www.w3.org/2004/02/skos/core#definition> """--Name--
Bag

--Definition--
Finite, unordered collection of related items (objects or values) that may be repeated (ISO 19107:2003).

--Description--
NOTE: Currently, this type is not being used in LPISQA."""@en ;
                                                                                                                     <http://www.w3.org/2004/02/skos/core#inScheme> :DataQualityMeasureValueStructureValue .


###  http://lpis.ec.europa.eu/registry/applicationschema/cap-iacs-parcel/code#DataQualityMeasureValueStructureValue/coverage
<http://lpis.ec.europa.eu/registry/applicationschema/cap-iacs-parcel/code#DataQualityMeasureValueStructureValue/coverage> rdf:type owl:NamedIndividual ,
                                                                                                                                   <http://lpis.ec.europa.eu/registry/applicationschema/cap-iacs-parcel#DataQualityMeasureValueStructureValue> ;
                                                                                                                          rdfs:label "Coverage"@en ;
                                                                                                                          <http://www.w3.org/2004/02/skos/core#definition> """--Name--
Coverage

--Definition--
Feature that acts as a function to return values from its range for any direct position within its spatial, temporal or spatiotemporal domain (ISO 19123:2005).

--Description--
NOTE: Currently, this type is not being used in LPISQA."""@en ;
                                                                                                                          <http://www.w3.org/2004/02/skos/core#inScheme> :DataQualityMeasureValueStructureValue .


###  http://lpis.ec.europa.eu/registry/applicationschema/cap-iacs-parcel/code#DataQualityMeasureValueStructureValue/matrix
<http://lpis.ec.europa.eu/registry/applicationschema/cap-iacs-parcel/code#DataQualityMeasureValueStructureValue/matrix> rdf:type owl:NamedIndividual ,
                                                                                                                                 <http://lpis.ec.europa.eu/registry/applicationschema/cap-iacs-parcel#DataQualityMeasureValueStructureValue> ;
                                                                                                                        rdfs:label "Matrix"@en ;
                                                                                                                        <http://www.w3.org/2004/02/skos/core#definition> """--Name--
Matrix

--Definition--
Rectangular array of numbers (ISO/TS 19129:2009).

--Description--
This structure is used to provide the misclassification matrix DQM."""@en ;
                                                                                                                        <http://www.w3.org/2004/02/skos/core#inScheme> :DataQualityMeasureValueStructureValue .


###  http://lpis.ec.europa.eu/registry/applicationschema/cap-iacs-parcel/code#DataQualityMeasureValueStructureValue/sequence
<http://lpis.ec.europa.eu/registry/applicationschema/cap-iacs-parcel/code#DataQualityMeasureValueStructureValue/sequence> rdf:type owl:NamedIndividual ,
                                                                                                                                   <http://lpis.ec.europa.eu/registry/applicationschema/cap-iacs-parcel#DataQualityMeasureValueStructureValue> ;
                                                                                                                          rdfs:label "Sequence"@en ;
                                                                                                                          <http://www.w3.org/2004/02/skos/core#definition> """--Name--
Sequence

--Definition--
Finite, ordered collection of related items (objects or values) that may be repeated (ISO 19107:2003).

--Description--
This structure can be used for providing QE2b values."""@en ;
                                                                                                                          <http://www.w3.org/2004/02/skos/core#inScheme> :DataQualityMeasureValueStructureValue .


###  http://lpis.ec.europa.eu/registry/applicationschema/cap-iacs-parcel/code#DataQualityMeasureValueStructureValue/set
<http://lpis.ec.europa.eu/registry/applicationschema/cap-iacs-parcel/code#DataQualityMeasureValueStructureValue/set> rdf:type owl:NamedIndividual ,
                                                                                                                              <http://lpis.ec.europa.eu/registry/applicationschema/cap-iacs-parcel#DataQualityMeasureValueStructureValue> ;
                                                                                                                     rdfs:label "Set"@en ;
                                                                                                                     <http://www.w3.org/2004/02/skos/core#definition> """--Name--
Set

--Definition--
Unordered collection of related items (objects or values) with no repetition (ISO 19107:2003).

--Description--
NOTE: Currently, this type is not being used in LPISQA."""@en ;
                                                                                                                     <http://www.w3.org/2004/02/skos/core#inScheme> :DataQualityMeasureValueStructureValue .


###  http://lpis.ec.europa.eu/registry/applicationschema/cap-iacs-parcel/code#DataQualityMeasureValueStructureValue/table
<http://lpis.ec.europa.eu/registry/applicationschema/cap-iacs-parcel/code#DataQualityMeasureValueStructureValue/table> rdf:type owl:NamedIndividual ,
                                                                                                                                <http://lpis.ec.europa.eu/registry/applicationschema/cap-iacs-parcel#DataQualityMeasureValueStructureValue> ;
                                                                                                                       rdfs:label "Table"@en ;
                                                                                                                       <http://www.w3.org/2004/02/skos/core#definition> """--Name--
Table

--Definition--
An arrangement of data in which each item may be identified by means of arguments or keys (ISO/IEC 2382-4:1999).

-Description--
This structure can be used for providing QE2b values."""@en ;
                                                                                                                       <http://www.w3.org/2004/02/skos/core#inScheme> :DataQualityMeasureValueStructureValue .


###  http://lpis.ec.europa.eu/registry/applicationschema/cap-iacs-parcel/code#EcologicalFocusAreaEquivalentPracticeTypeValue/bufferZonesForHighNatureValueAreasNatura2000OrSimilar
<http://lpis.ec.europa.eu/registry/applicationschema/cap-iacs-parcel/code#EcologicalFocusAreaEquivalentPracticeTypeValue/bufferZonesForHighNatureValueAreasNatura2000OrSimilar> rdf:type owl:NamedIndividual ,
                                                                                                                                                                                         <http://lpis.ec.europa.eu/registry/applicationschema/cap-iacs-parcel#EcologicalFocusAreaEquivalentPracticeTypeValue> ;
                                                                                                                                                                                rdfs:label "Buffer zones for high nature value areas ( Natura 2000 or similar)"@en ;
                                                                                                                                                                                <http://www.w3.org/2004/02/skos/core#definition> """--Name--
Buffer zones for high nature value areas

-- Definition --
Value listed in print III of Annex IX of Regulation (EU) No 1307/2013.

-- Description --
Natura 2000 or similar."""@en ;
                                                                                                                                                                                <http://www.w3.org/2004/02/skos/core#inScheme> :EcologicalFocusAreaEquivalentPracticeTypeValue .


###  http://lpis.ec.europa.eu/registry/applicationschema/cap-iacs-parcel/code#EcologicalFocusAreaEquivalentPracticeTypeValue/conversionOfArableLandIntoPermanentGrasslandExtensivelyUsed
<http://lpis.ec.europa.eu/registry/applicationschema/cap-iacs-parcel/code#EcologicalFocusAreaEquivalentPracticeTypeValue/conversionOfArableLandIntoPermanentGrasslandExtensivelyUsed> rdf:type owl:NamedIndividual ,
                                                                                                                                                                                               <http://lpis.ec.europa.eu/registry/applicationschema/cap-iacs-parcel#EcologicalFocusAreaEquivalentPracticeTypeValue> ;
                                                                                                                                                                                      rdfs:label "Conversion of arable land into permanent grassland extensively used"@en ;
                                                                                                                                                                                      <http://www.w3.org/2004/02/skos/core#definition> """--Name--
Conversion of arable land into extensively used permanent grassland

-- Definition --
Value listed in print III of Annex IX of Regulation (EU) No 1307/2013.

-- Description --
Item description."""@en ;
                                                                                                                                                                                      <http://www.w3.org/2004/02/skos/core#inScheme> :EcologicalFocusAreaEquivalentPracticeTypeValue .


###  http://lpis.ec.europa.eu/registry/applicationschema/cap-iacs-parcel/code#EcologicalFocusAreaEquivalentPracticeTypeValue/ecologicalSetAside
<http://lpis.ec.europa.eu/registry/applicationschema/cap-iacs-parcel/code#EcologicalFocusAreaEquivalentPracticeTypeValue/ecologicalSetAside> rdf:type owl:NamedIndividual ,
                                                                                                                                                      <http://lpis.ec.europa.eu/registry/applicationschema/cap-iacs-parcel#EcologicalFocusAreaEquivalentPracticeTypeValue> ;
                                                                                                                                             rdfs:label "Ecological set-aside"@en ;
                                                                                                                                             <http://www.w3.org/2004/02/skos/core#definition> """--Name--
Ecological set aside

-- Definition --
Value listed in print III of Annex IX of Regulation (EU) No 1307/2013.


-- Description --
Item description."""@en ;
                                                                                                                                             <http://www.w3.org/2004/02/skos/core#inScheme> :EcologicalFocusAreaEquivalentPracticeTypeValue .


###  http://lpis.ec.europa.eu/registry/applicationschema/cap-iacs-parcel/code#EcologicalFocusAreaEquivalentPracticeTypeValue/keepingArablePeatyOrWetSoilsUnderGrass
<http://lpis.ec.europa.eu/registry/applicationschema/cap-iacs-parcel/code#EcologicalFocusAreaEquivalentPracticeTypeValue/keepingArablePeatyOrWetSoilsUnderGrass> rdf:type owl:NamedIndividual ,
                                                                                                                                                                          <http://lpis.ec.europa.eu/registry/applicationschema/cap-iacs-parcel#EcologicalFocusAreaEquivalentPracticeTypeValue> ;
                                                                                                                                                                 rdfs:label "Keeping arable peaty or wet soils under grass"@en ;
                                                                                                                                                                 <http://www.w3.org/2004/02/skos/core#definition> """--Name--
Keeping arable peaty or wet soils under grass

-- Definition --
Value listed in print III of Annex IX of Regulation (EU) No 1307/2013.

-- Description --
Item description."""@en ;
                                                                                                                                                                 <http://www.w3.org/2004/02/skos/core#inScheme> :EcologicalFocusAreaEquivalentPracticeTypeValue .


###  http://lpis.ec.europa.eu/registry/applicationschema/cap-iacs-parcel/code#EcologicalFocusAreaEquivalentPracticeTypeValue/managementOfLandscapeFeatures
<http://lpis.ec.europa.eu/registry/applicationschema/cap-iacs-parcel/code#EcologicalFocusAreaEquivalentPracticeTypeValue/managementOfLandscapeFeatures> rdf:type owl:NamedIndividual ,
                                                                                                                                                                 <http://lpis.ec.europa.eu/registry/applicationschema/cap-iacs-parcel#EcologicalFocusAreaEquivalentPracticeTypeValue> ;
                                                                                                                                                        rdfs:label "Management of landscape features"@en ;
                                                                                                                                                        <http://www.w3.org/2004/02/skos/core#definition> """--Name--
Management of landscape features

-- Definition --
Value listed in print III of Annex IX of Regulation (EU) No 1307/2013.

-- Description --
Item description."""@en ;
                                                                                                                                                        <http://www.w3.org/2004/02/skos/core#inScheme> :EcologicalFocusAreaEquivalentPracticeTypeValue .


###  http://lpis.ec.europa.eu/registry/applicationschema/cap-iacs-parcel/code#EcologicalFocusAreaEquivalentPracticeTypeValue/patchesManagedForWildlifeOrSpecificFauna
<http://lpis.ec.europa.eu/registry/applicationschema/cap-iacs-parcel/code#EcologicalFocusAreaEquivalentPracticeTypeValue/patchesManagedForWildlifeOrSpecificFauna> rdf:type owl:NamedIndividual ,
                                                                                                                                                                            <http://lpis.ec.europa.eu/registry/applicationschema/cap-iacs-parcel#EcologicalFocusAreaEquivalentPracticeTypeValue> ;
                                                                                                                                                                   rdfs:label "Patches managed for wildlife or specific fauna"@en ;
                                                                                                                                                                   <http://www.w3.org/2004/02/skos/core#definition> """--Name--
Patches managed for wildlife or specific fauna

-- Definition --
Value listed in print III of Annex IX of Regulation (EU) No 1307/2013.

-- Description --
Item description."""@en ;
                                                                                                                                                                   <http://www.w3.org/2004/02/skos/core#inScheme> :EcologicalFocusAreaEquivalentPracticeTypeValue .


###  http://lpis.ec.europa.eu/registry/applicationschema/cap-iacs-parcel/code#EcologicalFocusAreaEquivalentPracticeTypeValue/productionOnArableLandWithoutFertilizersOrPlantProtection
<http://lpis.ec.europa.eu/registry/applicationschema/cap-iacs-parcel/code#EcologicalFocusAreaEquivalentPracticeTypeValue/productionOnArableLandWithoutFertilizersOrPlantProtection> rdf:type owl:NamedIndividual ,
                                                                                                                                                                                             <http://lpis.ec.europa.eu/registry/applicationschema/cap-iacs-parcel#EcologicalFocusAreaEquivalentPracticeTypeValue> ;
                                                                                                                                                                                    rdfs:label "Production on arable land without fertilizers or plant protection products (for 2 years with different crops)"@en ;
                                                                                                                                                                                    <http://www.w3.org/2004/02/skos/core#definition> """--Name--
Production on arable land without fertilizers of plant protection

-- Definition --
Value listed in print III of Annex IX of Regulation (EU) No 1307/2013.

-- Description --
Item description."""@en ;
                                                                                                                                                                                    <http://www.w3.org/2004/02/skos/core#inScheme> :EcologicalFocusAreaEquivalentPracticeTypeValue .


###  http://lpis.ec.europa.eu/registry/applicationschema/cap-iacs-parcel/code#EcologicalFocusAreaEquivalentPracticeTypeValue/uncultivatedBufferStripsAndFieldMargins
<http://lpis.ec.europa.eu/registry/applicationschema/cap-iacs-parcel/code#EcologicalFocusAreaEquivalentPracticeTypeValue/uncultivatedBufferStripsAndFieldMargins> rdf:type owl:NamedIndividual ,
                                                                                                                                                                           <http://lpis.ec.europa.eu/registry/applicationschema/cap-iacs-parcel#EcologicalFocusAreaEquivalentPracticeTypeValue> ;
                                                                                                                                                                  rdfs:label "Uncultivated buffer strips and field margins"@en ;
                                                                                                                                                                  <http://www.w3.org/2004/02/skos/core#definition> """--Name--
Uncultivated buffer strips and field margins

-- Definition --
Value listed in print III of Annex IX of Regulation (EU) No 1307/2013.

-- Description --
Item description."""@en ;
                                                                                                                                                                  <http://www.w3.org/2004/02/skos/core#inScheme> :EcologicalFocusAreaEquivalentPracticeTypeValue .


###  http://lpis.ec.europa.eu/registry/applicationschema/cap-iacs-parcel/code#EcologicalFocusAreaTypeValue/afforestedAreas
<http://lpis.ec.europa.eu/registry/applicationschema/cap-iacs-parcel/code#EcologicalFocusAreaTypeValue/afforestedAreas> rdf:type owl:NamedIndividual ,
                                                                                                                                 <http://lpis.ec.europa.eu/registry/applicationschema/cap-iacs-parcel#EcologicalFocusAreaTypeValue> ;
                                                                                                                        rdfs:label "Afforested areas"@en ;
                                                                                                                        <http://www.w3.org/2004/02/skos/core#definition> """--Name--
Afforested areas

-- Definition --
Ecological focus area type as defined by Art. 46(2) of (EU) R 1307/2013.

-- Description --
Afforested areas referred to in point (b)(ii) of Article 32(2) of (EU) R 1307/2013."""@en ;
                                                                                                                        <http://www.w3.org/2004/02/skos/core#inScheme> :EcologicalFocusAreaTypeValue .


###  http://lpis.ec.europa.eu/registry/applicationschema/cap-iacs-parcel/code#EcologicalFocusAreaTypeValue/areasWithCatchCropsOrGreenCover
<http://lpis.ec.europa.eu/registry/applicationschema/cap-iacs-parcel/code#EcologicalFocusAreaTypeValue/areasWithCatchCropsOrGreenCover> rdf:type owl:NamedIndividual ,
                                                                                                                                                 <http://lpis.ec.europa.eu/registry/applicationschema/cap-iacs-parcel#EcologicalFocusAreaTypeValue> ;
                                                                                                                                        rdfs:label "Areas with catch crops or green cover"@en ;
                                                                                                                                        <http://www.w3.org/2004/02/skos/core#definition> """--Name--
Areas with Catch crops or green cover

-- Definition --
Ecological focus area type as defined by Art. 46(2) of (EU) R 1307/2013.

-- Description --
Areas with catch crops or green cover established by the planting and germination of seeds, subject to the application of weighting factors referred to in paragraph 3 of this Article.

Areas under catch crops or green cover shall include:
- areas established pursuant to the requirements under SMR 1;
- other areas  on the condition that they were established by sowing a mixture of crop species or by under-sowing grass in the main crop. 

NOTE: MS shall establish set up specific rules, including the list of mixtures of crop species to be used and the period for the sowing  and may establish additional conditions notably with regard to production methods. The period to be set by Member States shall not extend after 1 October."""@en ;
                                                                                                                                        <http://www.w3.org/2004/02/skos/core#inScheme> :EcologicalFocusAreaTypeValue .


###  http://lpis.ec.europa.eu/registry/applicationschema/cap-iacs-parcel/code#EcologicalFocusAreaTypeValue/areasWithNitrogenFixingCrops
<http://lpis.ec.europa.eu/registry/applicationschema/cap-iacs-parcel/code#EcologicalFocusAreaTypeValue/areasWithNitrogenFixingCrops> rdf:type owl:NamedIndividual ,
                                                                                                                                              <http://lpis.ec.europa.eu/registry/applicationschema/cap-iacs-parcel#EcologicalFocusAreaTypeValue> ;
                                                                                                                                     rdfs:label "Areas with nitrogen fixing crops"@en ;
                                                                                                                                     <http://www.w3.org/2004/02/skos/core#definition> """--Name--
Areas with nitrogen fixing crop

-- Definition --
Ecological focus area type as defined by Art. 46(2) of (EU) R 1307/2013.

-- Description --
Areas with nitrogen fixing crops.

NOTE: A list of nitrogen-fixing crops shall be established by the MS [Art. 45(10) (EU) R No 637/2014]."""@en ;
                                                                                                                                     <http://www.w3.org/2004/02/skos/core#inScheme> :EcologicalFocusAreaTypeValue .


###  http://lpis.ec.europa.eu/registry/applicationschema/cap-iacs-parcel/code#EcologicalFocusAreaTypeValue/areasWithShortRotationCoppice
<http://lpis.ec.europa.eu/registry/applicationschema/cap-iacs-parcel/code#EcologicalFocusAreaTypeValue/areasWithShortRotationCoppice> rdf:type owl:NamedIndividual ,
                                                                                                                                               <http://lpis.ec.europa.eu/registry/applicationschema/cap-iacs-parcel#EcologicalFocusAreaTypeValue> ;
                                                                                                                                      rdfs:label "Areas with short rotation coppice"@en ;
                                                                                                                                      <http://www.w3.org/2004/02/skos/core#definition> """--Name--
Areas with short rotation coppice

-- Definition --
Ecological focus area type as defined by Art. 46(2) of (EU) R 1307/2013.

-- Description --
Areas with short rotation coppice  with no use of mineral fertiliser and/or plant protection products.

NOTE:  MS shall establish:
- a list of species that can be used for this purpose, by selecting from the list established pursuant to Article 4(2)(c) of R (EU) No 1307/2013;
- the requirements as regards the use of mineral fertilisers and plant protection products, keeping in mind the objective of this particular form of ecological focus areas in particular to safeguard and improve biodiversity."""@en ;
                                                                                                                                      <http://www.w3.org/2004/02/skos/core#inScheme> :EcologicalFocusAreaTypeValue .


###  http://lpis.ec.europa.eu/registry/applicationschema/cap-iacs-parcel/code#EcologicalFocusAreaTypeValue/bufferStrips
<http://lpis.ec.europa.eu/registry/applicationschema/cap-iacs-parcel/code#EcologicalFocusAreaTypeValue/bufferStrips> rdf:type owl:NamedIndividual ,
                                                                                                                              <http://lpis.ec.europa.eu/registry/applicationschema/cap-iacs-parcel#EcologicalFocusAreaTypeValue> ;
                                                                                                                     rdfs:label "Buffer strips"@en ;
                                                                                                                     <http://www.w3.org/2004/02/skos/core#definition> """--Name--
Buffer strips

-- Definition --
Ecological focus area type as defined by Art. 46(2) of (EU) R 1307/2013.

-- Description --
Buffer strips, including buffer strips covered by permanent grassland, provided that these are distinct from adjacent eligible agricultural area [Art. 46(2) (d) of (EU) R 1307/2013].

NOTE 1: Buffer strips shall include the buffer strips:
- along water courses required under GAEC 1, SMR 1 or SMR 10 as referred to in Annex II to Regulation (EU) No 640/2014;
- other buffer strips defined by MS. minimum width that shall not be below 1 meter.

NOTE 2: Buffer strips shall be located on or adjacent to an arable field with their long edges parallel to the edge of a water course or water body.

NOTE 3:  Along water courses, buffer strips may include strips with riparian vegetation with a width of up to 10 meters with no agricultural production. (By way of derogation MS may allow grazing or cutting, provided that the buffer strip remains distinguishable from adjacent agricultural land)."""@en ;
                                                                                                                     <http://www.w3.org/2004/02/skos/core#inScheme> :EcologicalFocusAreaTypeValue .


###  http://lpis.ec.europa.eu/registry/applicationschema/cap-iacs-parcel/code#EcologicalFocusAreaTypeValue/hectaresOfArgoForestry
<http://lpis.ec.europa.eu/registry/applicationschema/cap-iacs-parcel/code#EcologicalFocusAreaTypeValue/hectaresOfArgoForestry> rdf:type owl:NamedIndividual ,
                                                                                                                                        <http://lpis.ec.europa.eu/registry/applicationschema/cap-iacs-parcel#EcologicalFocusAreaTypeValue> ;
                                                                                                                               rdfs:label "Hectares of agro-forestry"@en ;
                                                                                                                               <http://www.w3.org/2004/02/skos/core#definition> """--Name--
Hectares of agro-forestry

-- Definition --
Ecological focus area type as defined by Art. 46(2) of (EU) R 1307/2013

-- Description --
Hectares of agro-forestry
- are those that receive, or have received, support under Article 44 of Regulation (EC) No 1698/2005 and/or Article 23 of Regulation (EU) No 1305/2013
- shall be arable land eligible for the basic payment scheme or the single area payment scheme  for which support under Article 44 of Regulation (EC) No 1698/2005 or Article 23 of Regulation (EU) No 1305/2013 was or is granted."""@en ;
                                                                                                                               <http://www.w3.org/2004/02/skos/core#inScheme> :EcologicalFocusAreaTypeValue .


###  http://lpis.ec.europa.eu/registry/applicationschema/cap-iacs-parcel/code#EcologicalFocusAreaTypeValue/landLyingFallow
<http://lpis.ec.europa.eu/registry/applicationschema/cap-iacs-parcel/code#EcologicalFocusAreaTypeValue/landLyingFallow> rdf:type owl:NamedIndividual ,
                                                                                                                                 <http://lpis.ec.europa.eu/registry/applicationschema/cap-iacs-parcel#EcologicalFocusAreaTypeValue> ;
                                                                                                                        rdfs:label "Land lying fallow"@en ;
                                                                                                                        <http://www.w3.org/2004/02/skos/core#definition> """--Name--
Land laying fallow

-- Definition --
Land laying fallow for application of ecological focus area type selected under Art. 46(2) of (EU) R 1307/2013.

-- Description --
On land lying fallow there shall be no agricultural production. By way of derogation from Article 4(1)(h) of ( EU) R No 639/2014, land lying fallow for the purpose of fulfilling the ecological focus area  for more than five years shall remain arable land."""@en ;
                                                                                                                        <http://www.w3.org/2004/02/skos/core#inScheme> :EcologicalFocusAreaTypeValue .


###  http://lpis.ec.europa.eu/registry/applicationschema/cap-iacs-parcel/code#EcologicalFocusAreaTypeValue/landscapeFeatureDitches
<http://lpis.ec.europa.eu/registry/applicationschema/cap-iacs-parcel/code#EcologicalFocusAreaTypeValue/landscapeFeatureDitches> rdf:type owl:NamedIndividual ,
                                                                                                                                         <http://lpis.ec.europa.eu/registry/applicationschema/cap-iacs-parcel#EcologicalFocusAreaTypeValue> ;
                                                                                                                                rdfs:label "Landscape feature, ditches"@en ;
                                                                                                                                <http://www.w3.org/2004/02/skos/core#definition> """--Name--
LF ditches

-- Definition --
Ecological focus area type as defined by Art. 46(2) of (EU) R 1307/2013.

-- Description --
Landscape feature, ditches with a maximum width of 6 meters, including open watercourses for the purpose of irrigation or drainage. Channels with walls of concrete shall not be considered ecological focus area.   [Art. 45(3)(g) of (EU) R No  639/2014].

NOTE : When this type of LF is protected under SMR 3, MS may specify other width based on  national requirements."""@en ;
                                                                                                                                <http://www.w3.org/2004/02/skos/core#inScheme> :EcologicalFocusAreaTypeValue .


###  http://lpis.ec.europa.eu/registry/applicationschema/cap-iacs-parcel/code#EcologicalFocusAreaTypeValue/landscapeFeatureFieldMargin
<http://lpis.ec.europa.eu/registry/applicationschema/cap-iacs-parcel/code#EcologicalFocusAreaTypeValue/landscapeFeatureFieldMargin> rdf:type owl:NamedIndividual ,
                                                                                                                                             <http://lpis.ec.europa.eu/registry/applicationschema/cap-iacs-parcel#EcologicalFocusAreaTypeValue> ;
                                                                                                                                    rdfs:label "Landscape feature, field margin"@en ;
                                                                                                                                    <http://www.w3.org/2004/02/skos/core#definition> """--Name--
LF field margine

-- Definition --
Ecological focus area type as defined by Art. 46(2) of (EU) R 1307/2013.

-- Description --
Landscape feature, field margin with a width between 1 and 20 meters, on which there shall be no agricultural production.   [Art. 45(3)(e) of (EU) R No  639/2014].

NOTE1:  MS may establish a lower maximum width.

NOTE 2: When this type of LF is protected under SMR 3, MS may specify other width based on  national requirements."""@en ;
                                                                                                                                    <http://www.w3.org/2004/02/skos/core#inScheme> :EcologicalFocusAreaTypeValue .


###  http://lpis.ec.europa.eu/registry/applicationschema/cap-iacs-parcel/code#EcologicalFocusAreaTypeValue/landscapeFeatureGroupOfTrees
<http://lpis.ec.europa.eu/registry/applicationschema/cap-iacs-parcel/code#EcologicalFocusAreaTypeValue/landscapeFeatureGroupOfTrees> rdf:type owl:NamedIndividual ,
                                                                                                                                              <http://lpis.ec.europa.eu/registry/applicationschema/cap-iacs-parcel#EcologicalFocusAreaTypeValue> ;
                                                                                                                                     rdfs:label "Landscape feature, group of trees/Field copses"@en ;
                                                                                                                                     <http://www.w3.org/2004/02/skos/core#definition> """--Name--
LF Group of trees

-- Definition --
Ecological focus area type as defined by Art. 46(2) of (EU) R 1307/2013.

-- Description --
Landscape feature, group of trees, where trees are connected by overlapping crown cover, and field copses of maximum 0.3 ha in both cases.   [Art. 45(3)(d) of (EU) R No 639/2014]."""@en ;
                                                                                                                                     <http://www.w3.org/2004/02/skos/core#inScheme> :EcologicalFocusAreaTypeValue .


###  http://lpis.ec.europa.eu/registry/applicationschema/cap-iacs-parcel/code#EcologicalFocusAreaTypeValue/landscapeFeatureIsolatedTree
<http://lpis.ec.europa.eu/registry/applicationschema/cap-iacs-parcel/code#EcologicalFocusAreaTypeValue/landscapeFeatureIsolatedTree> rdf:type owl:NamedIndividual ,
                                                                                                                                              <http://lpis.ec.europa.eu/registry/applicationschema/cap-iacs-parcel#EcologicalFocusAreaTypeValue> ;
                                                                                                                                     rdfs:label "Landscape feature, isolated tree"@en ;
                                                                                                                                     <http://www.w3.org/2004/02/skos/core#definition> """--Name--
LF isolated tree

-- Definition --
Ecological focus area type as defined by Art. 46(2) of (EU) R 1307/2013.

-- Description --
Landscape feature, isolated tree with a crown diameter of minimum 4 meters.  [Art. 45(3)(b) of (EU) R No 639/2014].

NOTE 1: Member States may include trees recognised by them as valuable landscape features with a crown diameter below 4 meters.

NOTE 2: When stable in time, this LF needs to be identified in the LPIS in view of checking their retention during OTSC. This identification of cross compliance Landscape Features can be done e.g. by alpha-numerical information (or by delineation) associated to the parcel."""@en ;
                                                                                                                                     <http://www.w3.org/2004/02/skos/core#inScheme> :EcologicalFocusAreaTypeValue .


###  http://lpis.ec.europa.eu/registry/applicationschema/cap-iacs-parcel/code#EcologicalFocusAreaTypeValue/landscapeFeatureOtherProtectedByGaecSmr
<http://lpis.ec.europa.eu/registry/applicationschema/cap-iacs-parcel/code#EcologicalFocusAreaTypeValue/landscapeFeatureOtherProtectedByGaecSmr> rdf:type owl:NamedIndividual ,
                                                                                                                                                         <http://lpis.ec.europa.eu/registry/applicationschema/cap-iacs-parcel#EcologicalFocusAreaTypeValue> ;
                                                                                                                                                rdfs:label "Landscape feature, other features not listed in this code list but protected under GAEC7, SMR 2 or SMR 3"@en ;
                                                                                                                                                <http://www.w3.org/2004/02/skos/core#definition> """--Name--
Other LF protected by GAEC or SMR.

-- Definition --
Ecological focus area type as defined by Art. 46(2) of (EU) R 1307/2013.

-- Description --
Landscape feature, other features not listed in this code list but protected under GAEC7, SMR 2 or SMR 3.   [Art. 45(3)(a) of (EU) R No  639/2014].

NOTE 3: When this type of LF is protected under GAEC 7 SMR 2 and SMR  3, MS may specify other width based on  national requirements [DSCG/2014/31]."""@en ;
                                                                                                                                                <http://www.w3.org/2004/02/skos/core#inScheme> :EcologicalFocusAreaTypeValue .


###  http://lpis.ec.europa.eu/registry/applicationschema/cap-iacs-parcel/code#EcologicalFocusAreaTypeValue/landscapeFeaturePonds
<http://lpis.ec.europa.eu/registry/applicationschema/cap-iacs-parcel/code#EcologicalFocusAreaTypeValue/landscapeFeaturePonds> rdf:type owl:NamedIndividual ,
                                                                                                                                       <http://lpis.ec.europa.eu/registry/applicationschema/cap-iacs-parcel#EcologicalFocusAreaTypeValue> ;
                                                                                                                              rdfs:label "Landscape feature, ponds"@en ;
                                                                                                                              <http://www.w3.org/2004/02/skos/core#definition> """--Name--
LF ponds

-- Definition --
Ecological focus area type as defined by Art. 46(2) of (EU) R 1307/2013.

-- Description --
Landscape feature, ponds of up to a maximum of 0.1 ha. Reservoirs made of concrete or plastic shall not be considered ecological focus area;   [Art. 45(3)(f) of (EU) R No 639/2014].

NOTE 1: MS may set a minimum size for ponds and they may decide that a strip with riparian vegetation along the water with a width of up to 10 meters is included in the size of the pond. They may establish criteria to ensure that ponds are of natural value, taking into account the role that natural ponds play for wildlife the conservation of habitats and species.

NOTE 2: When this type of LF is protected under GAEC 7 MS may specify other area  for ponds based on national requirements."""@en ;
                                                                                                                              <http://www.w3.org/2004/02/skos/core#inScheme> :EcologicalFocusAreaTypeValue .


###  http://lpis.ec.europa.eu/registry/applicationschema/cap-iacs-parcel/code#EcologicalFocusAreaTypeValue/landscapeFeatureTraditionalStoneWalls
<http://lpis.ec.europa.eu/registry/applicationschema/cap-iacs-parcel/code#EcologicalFocusAreaTypeValue/landscapeFeatureTraditionalStoneWalls> rdf:type owl:NamedIndividual ,
                                                                                                                                                       <http://lpis.ec.europa.eu/registry/applicationschema/cap-iacs-parcel#EcologicalFocusAreaTypeValue> ;
                                                                                                                                              rdfs:label "Landscape feature traditional stone walls"@en ;
                                                                                                                                              <http://www.w3.org/2004/02/skos/core#definition> """--Name--
LF traditional walls

-- Definition --
Ecological focus area type as defined by Art. 46(2) of (EU) R 1307/2013.

-- Description --
Landscape feature traditional stone walls.   [Art. 45(3)(a) of (EU) R No  639/2014].

NOTE: Member States shall establish minimum criteria based on national or regional specificities, including limits to the dimensions of height and width.

NOTE 2: When this type of LF is protected under SMR 3, MS may specify other width based on  national requirements."""@en ;
                                                                                                                                              <http://www.w3.org/2004/02/skos/core#inScheme> :EcologicalFocusAreaTypeValue .


###  http://lpis.ec.europa.eu/registry/applicationschema/cap-iacs-parcel/code#EcologicalFocusAreaTypeValue/landscapeFeatureTreesInLine
<http://lpis.ec.europa.eu/registry/applicationschema/cap-iacs-parcel/code#EcologicalFocusAreaTypeValue/landscapeFeatureTreesInLine> rdf:type owl:NamedIndividual ,
                                                                                                                                             <http://lpis.ec.europa.eu/registry/applicationschema/cap-iacs-parcel#EcologicalFocusAreaTypeValue> ;
                                                                                                                                    rdfs:label "Landscape feature, trees in line"@en ;
                                                                                                                                    <http://www.w3.org/2004/02/skos/core#definition> """--Name--
LF trees in line

-- Definition --
Ecological focus area type as defined by Art. 46(2) of (EU) R 1307/2013.

-- Description --
Landscape feature, trees in line  trees in line with a crown diameter of minimum 4 meters. The space between the crowns shall not exceed 5 meters. [Art. 45(3)(c) of (EU) R No  639/2014].

NOTE 1: Member States may include trees recognised by them as valuable landscape features with a crown diameter below 4 meters.

NOTE 2: When this type of LF is protected under GAEC 7, SMR 3, MS may specify other width based on national requirements."""@en ;
                                                                                                                                    <http://www.w3.org/2004/02/skos/core#inScheme> :EcologicalFocusAreaTypeValue .


###  http://lpis.ec.europa.eu/registry/applicationschema/cap-iacs-parcel/code#EcologicalFocusAreaTypeValue/landscapeFeaturesHedgesWoodedStrips
<http://lpis.ec.europa.eu/registry/applicationschema/cap-iacs-parcel/code#EcologicalFocusAreaTypeValue/landscapeFeaturesHedgesWoodedStrips> rdf:type owl:NamedIndividual ,
                                                                                                                                                     <http://lpis.ec.europa.eu/registry/applicationschema/cap-iacs-parcel#EcologicalFocusAreaTypeValue> ;
                                                                                                                                            rdfs:label "Landscape features: Hedges/wooded strips"@en ;
                                                                                                                                            <http://www.w3.org/2004/02/skos/core#definition> """--Name--
LF hedges and wooded strips

-- Definition --
Ecological focus area type as defined by Art. 46(2) of (EU) R 1307/2013

-- Description --
Landscape features: Hedges/wooded strips with a width of up to 10 meters [Art. 45(3)(a) of (EU) R No 639/2014]

NOTE 1: When  such LF are protected under GAEC 7, SMR 2 and SMR 3, MS may specify other width based on national requirements.

NOTE 2: This LF, when stable in time, need to be identified in the LPIS in view of checking their retention during OTSC. This identification of cross compliance Landscape Features can be done e.g. by alpha-numerical information (or by delineation) associated to the parcel."""@en ;
                                                                                                                                            <http://www.w3.org/2004/02/skos/core#inScheme> :EcologicalFocusAreaTypeValue .


###  http://lpis.ec.europa.eu/registry/applicationschema/cap-iacs-parcel/code#EcologicalFocusAreaTypeValue/stripsOfEligibleHectaresAlongForestEdgesWithProduction
<http://lpis.ec.europa.eu/registry/applicationschema/cap-iacs-parcel/code#EcologicalFocusAreaTypeValue/stripsOfEligibleHectaresAlongForestEdgesWithProduction> rdf:type owl:NamedIndividual ,
                                                                                                                                                                        <http://lpis.ec.europa.eu/registry/applicationschema/cap-iacs-parcel#EcologicalFocusAreaTypeValue> ;
                                                                                                                                                               rdfs:label "Strips of eligible hectares along forest edges with production"@en ;
                                                                                                                                                               <http://www.w3.org/2004/02/skos/core#definition> """--Name--
Strips of eligible hectares with production

-- Definition --
Ecological focus area type as defined by Art. 46(2) of (EU) R 1307/2013

-- Description --
Strips of eligible hectares along forest edges with production.

NOTE: width shall be defined by the MS within the limits
- minimum shall not be below 1 meter
- maximum width shall be 10 meters."""@en ;
                                                                                                                                                               <http://www.w3.org/2004/02/skos/core#inScheme> :EcologicalFocusAreaTypeValue .


###  http://lpis.ec.europa.eu/registry/applicationschema/cap-iacs-parcel/code#EcologicalFocusAreaTypeValue/stripsOfEligibleHectaresAlongForestEdgesWithoutProduction
<http://lpis.ec.europa.eu/registry/applicationschema/cap-iacs-parcel/code#EcologicalFocusAreaTypeValue/stripsOfEligibleHectaresAlongForestEdgesWithoutProduction> rdf:type owl:NamedIndividual ,
                                                                                                                                                                           <http://lpis.ec.europa.eu/registry/applicationschema/cap-iacs-parcel#EcologicalFocusAreaTypeValue> ;
                                                                                                                                                                  rdfs:label "Strips of eligible hectares along forest edges without production"@en ;
                                                                                                                                                                  <http://www.w3.org/2004/02/skos/core#definition> """--Name--
Strips of eligible hectares without production

-- Definition --
Ecological focus area type as defined by Art. 46(2) of (EU) R 1307/2013

-- Description --
Strips of eligible hectares along forest edges without production. 

NOTE 1: by way of derogation from the no production requirement, grazing or cutting may be allowed, provided the strip remains distinguishable from adjacent agricultural land. 

NOTE 2: width shall be defined by the MS within the limits
- minimum shall not be below 1 meter
- maximum width shall be 10 meters."""@en ;
                                                                                                                                                                  <http://www.w3.org/2004/02/skos/core#inScheme> :EcologicalFocusAreaTypeValue .


###  http://lpis.ec.europa.eu/registry/applicationschema/cap-iacs-parcel/code#EcologicalFocusAreaTypeValue/terraces
<http://lpis.ec.europa.eu/registry/applicationschema/cap-iacs-parcel/code#EcologicalFocusAreaTypeValue/terraces> rdf:type owl:NamedIndividual ,
                                                                                                                          <http://lpis.ec.europa.eu/registry/applicationschema/cap-iacs-parcel#EcologicalFocusAreaTypeValue> ;
                                                                                                                 rdfs:label "Terraces"@en ;
                                                                                                                 <http://www.w3.org/2004/02/skos/core#definition> """--Name--
Terraces

-- Definition --
Ecological focus area type as defined by Art. 46(2) of (EU) R 1307/2013

-- Description --
Terraces shall be terraces that:
-are protected under GAEC 7 as referred to in Annex II to Regulation (EU) No 640/2014;
-other terraces established based on criteria defined by MS. 
Criteria may include minimum height based on national or regional specificities."""@en ;
                                                                                                                 <http://www.w3.org/2004/02/skos/core#inScheme> :EcologicalFocusAreaTypeValue .


###  http://lpis.ec.europa.eu/registry/applicationschema/cap-iacs-parcel/code#HomogeneityTypeValue/elevation
<http://lpis.ec.europa.eu/registry/applicationschema/cap-iacs-parcel/code#HomogeneityTypeValue/elevation> rdf:type owl:NamedIndividual ,
                                                                                                                   <http://lpis.ec.europa.eu/registry/applicationschema/cap-iacs-parcel#HomogeneityTypeValue> ;
                                                                                                          rdfs:label "Elevation"@en ;
                                                                                                          <http://www.w3.org/2004/02/skos/core#definition> """--Name--
Elevation

-- Definition --
Homogeneity criteria established on elevation values.

-- Description --
Criteria that can be derived using digital elevation models for land surface.

NOTE: the criteria have to be documented in the eligibility profile of the MS/regions, or have to be described in a document dully cited or inserted in the information system."""@en ;
                                                                                                          <http://www.w3.org/2004/02/skos/core#inScheme> :HomogeneityTypeValue .


###  http://lpis.ec.europa.eu/registry/applicationschema/cap-iacs-parcel/code#HomogeneityTypeValue/naturalArea
<http://lpis.ec.europa.eu/registry/applicationschema/cap-iacs-parcel/code#HomogeneityTypeValue/naturalArea> rdf:type owl:NamedIndividual ,
                                                                                                                     <http://lpis.ec.europa.eu/registry/applicationschema/cap-iacs-parcel#HomogeneityTypeValue> ;
                                                                                                            rdfs:label "Natural area"@en ;
                                                                                                            <http://www.w3.org/2004/02/skos/core#definition> """--Name--
Natural area

-- Definition --
Natural area type according to objective criteria

-- Description --
Natural area types shall be defined based on objective criteria, for example:
-bio-geographical regions,
-habitats and biotopes,
-species distribution,
-climate zones,
-homogeneous geology,
-natural risk zones,
-protected sites (Natura 2000),
-river basin management, etc.

NOTE: the applicable values of natural area hall be documented in the eligibility profile of the MS/regions, and have to be described in a document dully cited or inserted in the information system.

EXAMPLE:  http://inspire.ec.europa.eu/applicationschema/ provides the list of INSPIRE  data themes (applications schemas) that may be used for selecting homogeneity criteria."""@en ;
                                                                                                            <http://www.w3.org/2004/02/skos/core#inScheme> :HomogeneityTypeValue .


###  http://lpis.ec.europa.eu/registry/applicationschema/cap-iacs-parcel/code#HomogeneityTypeValue/semiNaturalArea
<http://lpis.ec.europa.eu/registry/applicationschema/cap-iacs-parcel/code#HomogeneityTypeValue/semiNaturalArea> rdf:type owl:NamedIndividual ,
                                                                                                                         <http://lpis.ec.europa.eu/registry/applicationschema/cap-iacs-parcel#HomogeneityTypeValue> ;
                                                                                                                rdfs:label "Semi-natural area"@en ;
                                                                                                                <http://www.w3.org/2004/02/skos/core#definition> """--Name--
Semi-natural area

-- Definition --
Semi natural area type according to objective criteria

-- Description --
Natural area types with human impact that further delimits homogeneity. 

NOTE: the applicable values of semi natural area hall be documented in the eligibility profile of the MS/regions, and have to be described in a document dully cited or inserted in the information system.

EXAMPLE:  http://inspire.ec.europa.eu/applicationschema/ provides the list of INSPIRE  data themes (applications schemas) that may be used for selecting homogeneity criteria."""@en ;
                                                                                                                <http://www.w3.org/2004/02/skos/core#inScheme> :HomogeneityTypeValue .


###  http://lpis.ec.europa.eu/registry/applicationschema/cap-iacs-parcel/code#HomogeneityTypeValue/soilType
<http://lpis.ec.europa.eu/registry/applicationschema/cap-iacs-parcel/code#HomogeneityTypeValue/soilType> rdf:type owl:NamedIndividual ,
                                                                                                                  <http://lpis.ec.europa.eu/registry/applicationschema/cap-iacs-parcel#HomogeneityTypeValue> ;
                                                                                                         rdfs:label "Soil type"@en ;
                                                                                                         <http://www.w3.org/2004/02/skos/core#definition> """--Name--
Soil type

-- Definition --
Soil type according to a well-established classification system.

-- Description --
The classification system shall be described or referred with a citation.

NOTE: the applicable values of soil type shall be documented in the eligibility profile of the MS/regions, or have to be described in a document dully cited or inserted in the information system.

EXAMPLE:  http://inspire.ec.europa.eu/codelist/ 
INSPIRE code list  registry comprising Soil data theme."""@en ;
                                                                                                         <http://www.w3.org/2004/02/skos/core#inScheme> :HomogeneityTypeValue .


###  http://lpis.ec.europa.eu/registry/applicationschema/cap-iacs-parcel/code#InspectionMethodValue/capi
<http://lpis.ec.europa.eu/registry/applicationschema/cap-iacs-parcel/code#InspectionMethodValue/capi> rdf:type owl:NamedIndividual ,
                                                                                                               <http://lpis.ec.europa.eu/registry/applicationschema/cap-iacs-parcel#InspectionMethodValue> ;
                                                                                                      rdfs:label "Computer assisted photo interpretation"@en ;
                                                                                                      <http://www.w3.org/2004/02/skos/core#definition> """--Name--
Computer assisted photo interpretation (CAPI)

-- Definition --
Computer assisted photo interpretation method of inspection.

-- Description --
All observations and measurements are performed on the basis of orthtoimagery using suitable GIS software."""@en ;
                                                                                                      <http://www.w3.org/2004/02/skos/core#inScheme> :InspectionMethodValue .


###  http://lpis.ec.europa.eu/registry/applicationschema/cap-iacs-parcel/code#InspectionMethodValue/combinedCapiAndFieldSurvey
<http://lpis.ec.europa.eu/registry/applicationschema/cap-iacs-parcel/code#InspectionMethodValue/combinedCapiAndFieldSurvey> rdf:type owl:NamedIndividual ,
                                                                                                                                     <http://lpis.ec.europa.eu/registry/applicationschema/cap-iacs-parcel#InspectionMethodValue> ;
                                                                                                                            rdfs:label "Combined CAPI and field survey"@en ;
                                                                                                                            <http://www.w3.org/2004/02/skos/core#definition> """--Name--
Combined CAPI and filed survey

-- Definition --
Combined method of inspection using CAPI and field survey.

-- Description --
The default inspection method is CAPI. In case when the measurement of the item is not feasible, or unambiguous classification of land cover is not possible, field visit shall be performed. Therefore there are three options: 
1. Combined CAPI supported by land cover detection and area measurement in the field,
2. Combined CAPI supported by land cover detection only in the field,
3. Combined CAPI supported by area measurement only in the field.

NOTE: At this method the \"False\" value of the feasibilityForMeasurement attribute of ETSItemUnderInspection feature type can be very rarely assigned, only if the measurement is not feasible in the field (force major)."""@en ;
                                                                                                                            <http://www.w3.org/2004/02/skos/core#inScheme> :InspectionMethodValue .


###  http://lpis.ec.europa.eu/registry/applicationschema/cap-iacs-parcel/code#InspectionMethodValue/fieldSurvey
<http://lpis.ec.europa.eu/registry/applicationschema/cap-iacs-parcel/code#InspectionMethodValue/fieldSurvey> rdf:type owl:NamedIndividual ,
                                                                                                                      <http://lpis.ec.europa.eu/registry/applicationschema/cap-iacs-parcel#InspectionMethodValue> ;
                                                                                                             rdfs:label "Field survey"@en ;
                                                                                                             <http://www.w3.org/2004/02/skos/core#definition> """--Name--
Field survey

-- Definition --
Observations and measurements necessary for inspection are performed exclusively in the field.

-- Description --
Measurements can be performed by any means listed in the common technical specifications (e.g. GNSS, total station, etc.)

NOTE: In ETS 5.3 the value used to be field inspection."""@en ;
                                                                                                             <http://www.w3.org/2004/02/skos/core#inScheme> :InspectionMethodValue .


###  http://lpis.ec.europa.eu/registry/applicationschema/cap-iacs-parcel/code#LandscapeFeatureValueType/landscapeFeatureDitches
<http://lpis.ec.europa.eu/registry/applicationschema/cap-iacs-parcel/code#LandscapeFeatureValueType/landscapeFeatureDitches> rdf:type owl:NamedIndividual ,
                                                                                                                                      <http://lpis.ec.europa.eu/registry/applicationschema/cap-iacs-parcel#LandscapeFeatureValueType> ;
                                                                                                                             rdfs:label "Landscape feature, ditches"@en ;
                                                                                                                             <http://www.w3.org/2004/02/skos/core#definition> """--Name--
Ditches

-- Definition --
Ditches in the agricultural area that are traditionally part of good agriculture cropping or utilization practices.

-- Description --
Ditches may become an EFA element when their width does not exceeds 6 meters. Ditches also include open watercourses for the purpose of irrigation or drainage. Channels with walls of concrete shall not be considered ecological focus area. [Art. 45(3)(g) of (EU) R No  639/2014].

NOTE : When this type of LF is protected under SMR 3, MS may specify other width based on  national requirements."""@en ;
                                                                                                                             <http://www.w3.org/2004/02/skos/core#inScheme> :LandscapeFeatureValueType .


###  http://lpis.ec.europa.eu/registry/applicationschema/cap-iacs-parcel/code#LandscapeFeatureValueType/landscapeFeatureFieldMargin
<http://lpis.ec.europa.eu/registry/applicationschema/cap-iacs-parcel/code#LandscapeFeatureValueType/landscapeFeatureFieldMargin> rdf:type owl:NamedIndividual ,
                                                                                                                                          <http://lpis.ec.europa.eu/registry/applicationschema/cap-iacs-parcel#LandscapeFeatureValueType> ;
                                                                                                                                 rdfs:label "Landscape feature, field margin"@en ;
                                                                                                                                 <http://www.w3.org/2004/02/skos/core#definition> """--Name--
Field margin

-- Definition --
Field margin in the agricultural area that is traditionally part of good agriculture cropping or utilization practices.

-- Description --
Field margin may become an EFA element when its width is between 1 and 20 meters. There shall be no agricultural production on it. [Art. 45(3)(e) of (EU) R No  639/2014].

NOTE 1. MS may establish a lower maximum width.

NOTE 2. When this type of LF is protected under SMR 3, MS may specify other width based on national requirements."""@en ;
                                                                                                                                 <http://www.w3.org/2004/02/skos/core#inScheme> :LandscapeFeatureValueType .


###  http://lpis.ec.europa.eu/registry/applicationschema/cap-iacs-parcel/code#LandscapeFeatureValueType/landscapeFeatureGroupOfTrees
<http://lpis.ec.europa.eu/registry/applicationschema/cap-iacs-parcel/code#LandscapeFeatureValueType/landscapeFeatureGroupOfTrees> rdf:type owl:NamedIndividual ,
                                                                                                                                           <http://lpis.ec.europa.eu/registry/applicationschema/cap-iacs-parcel#LandscapeFeatureValueType> ;
                                                                                                                                  rdfs:label "Landscape feature, group of trees/Field copses"@en ;
                                                                                                                                  <http://www.w3.org/2004/02/skos/core#definition> """--Name--
Group of trees

-- Definition --
Group of trees in the agricultural area that is traditionally part of good agriculture cropping or utilization practices 

-- Description --
Group of trees may become an EFA element where trees are connected by overlapping crown cover, and field copses of maximum 0.3 ha in both cases. [Art. 45(3)(d) of (EU) R No 639/2014]."""@en ;
                                                                                                                                  <http://www.w3.org/2004/02/skos/core#inScheme> :LandscapeFeatureValueType .


###  http://lpis.ec.europa.eu/registry/applicationschema/cap-iacs-parcel/code#LandscapeFeatureValueType/landscapeFeatureHedgesAndWoodedStrips
<http://lpis.ec.europa.eu/registry/applicationschema/cap-iacs-parcel/code#LandscapeFeatureValueType/landscapeFeatureHedgesAndWoodedStrips> rdf:type owl:NamedIndividual ,
                                                                                                                                                    <http://lpis.ec.europa.eu/registry/applicationschema/cap-iacs-parcel#LandscapeFeatureValueType> ;
                                                                                                                                           rdfs:label "Landscape features: Hedges/wooded strips"@en ;
                                                                                                                                           <http://www.w3.org/2004/02/skos/core#definition> """--Name--
Hedges and wooded strips

-- Definition --
Hedges and wooded strips in the agricultural area that are traditionally part of good agriculture cropping or utilization practices.

-- Description --
These LF may become EFA when their width does not exceed 10 meters. [Art. 45(3)(a) of (EU) R No 639/2014]

NOTE 1: When such LF are protected under GAEC 7, SMR 2 and SMR 3, MS may specify an other width based on national/regional requirements.

NOTE 2: This LF, when stable in time, need to be identified in the LPIS in view of checking their retention during OTSC. This identification of cross compliance Landscape Features can be done e.g. by alpha-numerical information (or by delineation) associated to the parcel."""@en ;
                                                                                                                                           <http://www.w3.org/2004/02/skos/core#inScheme> :LandscapeFeatureValueType .


###  http://lpis.ec.europa.eu/registry/applicationschema/cap-iacs-parcel/code#LandscapeFeatureValueType/landscapeFeatureIsolatedTree
<http://lpis.ec.europa.eu/registry/applicationschema/cap-iacs-parcel/code#LandscapeFeatureValueType/landscapeFeatureIsolatedTree> rdf:type owl:NamedIndividual ,
                                                                                                                                           <http://lpis.ec.europa.eu/registry/applicationschema/cap-iacs-parcel#LandscapeFeatureValueType> ;
                                                                                                                                  rdfs:label "Landscape feature, isolated tree"@en ;
                                                                                                                                  <http://www.w3.org/2004/02/skos/core#definition> """--Name--
Isolated tree

-- Definition --
Isolated tree in the agricultural area that is traditionally part of good agriculture cropping or utilization practices.

-- Description --
Such LF may become an EFA element when its crown diameter is of minimum 4 meters. [Art. 45(3)(b) of (EU) R No 639/2014].

NOTE 1: Member States may include trees designated by them as valuable landscape features with a crown diameter below 4 meters.

NOTE 2: When stable in time, this LF needs to be identified in the LPIS in view of checking their retention during OTSC. This identification of cross compliance Landscape Features can be done e.g. by alpha-numerical information (or by delineation) associated to the parcel"""@en ;
                                                                                                                                  <http://www.w3.org/2004/02/skos/core#inScheme> :LandscapeFeatureValueType .


###  http://lpis.ec.europa.eu/registry/applicationschema/cap-iacs-parcel/code#LandscapeFeatureValueType/landscapeFeatureOtherProtectedByGaecSmr
<http://lpis.ec.europa.eu/registry/applicationschema/cap-iacs-parcel/code#LandscapeFeatureValueType/landscapeFeatureOtherProtectedByGaecSmr> rdf:type owl:NamedIndividual ,
                                                                                                                                                      <http://lpis.ec.europa.eu/registry/applicationschema/cap-iacs-parcel#LandscapeFeatureValueType> ;
                                                                                                                                             rdfs:label "Landscape feature, other features not listed in this code list but protected under GAEC7, SMR 2 or SMR 3"@en ;
                                                                                                                                             <http://www.w3.org/2004/02/skos/core#definition> """--Name--
Other LF protected by GAEC or SMR.

-- Definition --
Other LF protected by GAEC or SMR in the agricultural area that are part of good agriculture cropping or utilization practices.

-- Description --
Landscape feature, other features not listed in this code list but protected under GAEC7, SMR 2 or SMR 3 may become an EFA eleemnt. [Art. 45(3)(a) of (EU) R No  639/2014].

NOTE. When this type of LF is protected under GAEC 7 SMR 2 and SMR 3, MS shall provide semanic description and specification of properties (e.g. width)."""@en ;
                                                                                                                                             <http://www.w3.org/2004/02/skos/core#inScheme> :LandscapeFeatureValueType .


###  http://lpis.ec.europa.eu/registry/applicationschema/cap-iacs-parcel/code#LandscapeFeatureValueType/landscapeFeaturePonds
<http://lpis.ec.europa.eu/registry/applicationschema/cap-iacs-parcel/code#LandscapeFeatureValueType/landscapeFeaturePonds> rdf:type owl:NamedIndividual ,
                                                                                                                                    <http://lpis.ec.europa.eu/registry/applicationschema/cap-iacs-parcel#LandscapeFeatureValueType> ;
                                                                                                                           rdfs:label "Landscape feature, ponds"@en ;
                                                                                                                           <http://www.w3.org/2004/02/skos/core#definition> """--Name--
Ponds

-- Definition --
Ponds in the agricultural area that are traditionally part of good agriculture cropping or utilization practices.

-- Description --
Ponds may become an EFA element when their area is up to a maximum of 0.1 ha. Reservoirs made of concrete or plastic shall not be considered ecological focus area;   [Art. 45(3)(f) of (EU) R No 639/2014].

NOTE 1: MS may set a minimum size for ponds and they may decide that a strip with riparian vegetation along the water with a width of up to 10 meters is included in the size of the pond. They may establish criteria to ensure that ponds are of natural value, taking into account the role that natural ponds play for wildlife the conservation of habitats and species.

NOTE 2: When this type of LF is protected under GAEC 7 MS may specify other area  for ponds based on national requirements."""@en ;
                                                                                                                           <http://www.w3.org/2004/02/skos/core#inScheme> :LandscapeFeatureValueType .


###  http://lpis.ec.europa.eu/registry/applicationschema/cap-iacs-parcel/code#LandscapeFeatureValueType/landscapeFeatureTraditionalStoneWalls
<http://lpis.ec.europa.eu/registry/applicationschema/cap-iacs-parcel/code#LandscapeFeatureValueType/landscapeFeatureTraditionalStoneWalls> rdf:type owl:NamedIndividual ,
                                                                                                                                                    <http://lpis.ec.europa.eu/registry/applicationschema/cap-iacs-parcel#LandscapeFeatureValueType> ;
                                                                                                                                           rdfs:label "Landscape feature traditional stone walls"@en ;
                                                                                                                                           <http://www.w3.org/2004/02/skos/core#definition> """---Name--
Traditional stone walls

-- Definition --
Traditional stone walls in the agricultural area that are part of good agriculture cropping or utilization practices.

-- Description --
Traditional stone walls may become and EFA element. [Art. 45(3)(a) of (EU) R No 639/2014].

NOTE 1. Member States shall establish minimum criteria based on national or regional specificities, including limits to the dimensions of height and width.

NOTE 2. When this type of LF is protected under SMR 3, MS may specify other width based on  national requirements."""@en ;
                                                                                                                                           <http://www.w3.org/2004/02/skos/core#inScheme> :LandscapeFeatureValueType .


###  http://lpis.ec.europa.eu/registry/applicationschema/cap-iacs-parcel/code#LandscapeFeatureValueType/landscapeFeatureTtreesInLine
<http://lpis.ec.europa.eu/registry/applicationschema/cap-iacs-parcel/code#LandscapeFeatureValueType/landscapeFeatureTtreesInLine> rdf:type owl:NamedIndividual ,
                                                                                                                                           <http://lpis.ec.europa.eu/registry/applicationschema/cap-iacs-parcel#LandscapeFeatureValueType> ;
                                                                                                                                  rdfs:label "Landscape feature, trees in line"@en ;
                                                                                                                                  <http://www.w3.org/2004/02/skos/core#definition> """--Name--
Trees in line

-- Definition --
Trees in line in the agricultural area that are traditionally part of good agriculture cropping or utilization practices 

-- Description --
They may become an EFA element when the crown diameter is minimum 4 meters. The space between the crowns shall not exceed 5 meters. [Art. 45(3)(c) of (EU) R No  639/2014].

NOTE 1: Member States may include trees recognised by them as valuable landscape features with a crown diameter below 4 meters.

NOTE 2: When this type of LF is protected under GAEC 7, SMR 3, MS may specify other width based on national requirements.."""@en ;
                                                                                                                                  <http://www.w3.org/2004/02/skos/core#inScheme> :LandscapeFeatureValueType .


###  http://lpis.ec.europa.eu/registry/applicationschema/cap-iacs-parcel/code#LimitingQualityValue/12.50
<http://lpis.ec.europa.eu/registry/applicationschema/cap-iacs-parcel/code#LimitingQualityValue/12.50> rdf:type owl:NamedIndividual ,
                                                                                                               <http://lpis.ec.europa.eu/registry/applicationschema/cap-iacs-parcel#LimitingQualityValue> ;
                                                                                                      rdfs:label "12.50"@en ;
                                                                                                      <http://www.w3.org/2004/02/skos/core#definition> """--Name--
12.50

-- Definition --
Limiting quality value LQ=12,50.

-- Description --
Value defined by ISO 2859-2:1985. This value is applicable for all assessments (area and contamination conformity, item conformity) by exclusion of critical defect conformity. It expresses and indexes a quality expectation of 5% error rate or better."""@en ;
                                                                                                      <http://www.w3.org/2004/02/skos/core#inScheme> :LimitingQualityValue .


###  http://lpis.ec.europa.eu/registry/applicationschema/cap-iacs-parcel/code#LimitingQualityValue/2.00
<http://lpis.ec.europa.eu/registry/applicationschema/cap-iacs-parcel/code#LimitingQualityValue/2.00> rdf:type owl:NamedIndividual ,
                                                                                                              <http://lpis.ec.europa.eu/registry/applicationschema/cap-iacs-parcel#LimitingQualityValue> ;
                                                                                                     rdfs:label "2.00"@en ;
                                                                                                     <http://www.w3.org/2004/02/skos/core#definition> """--Name--
2.00

-- Definition --
Limiting quality value LQ=2,0

-- Description --
Value defined by ISO 2859-2:1985. This value is applicable for assessment of critical defects. It expresses and indexes a quality expectation of 1% error rate or better."""@en ;
                                                                                                     <http://www.w3.org/2004/02/skos/core#inScheme> :LimitingQualityValue .


###  http://lpis.ec.europa.eu/registry/applicationschema/cap-iacs-parcel/code#LotSizeValue/150001to500000
<http://lpis.ec.europa.eu/registry/applicationschema/cap-iacs-parcel/code#LotSizeValue/150001to500000> rdf:type owl:NamedIndividual ,
                                                                                                                <http://lpis.ec.europa.eu/registry/applicationschema/cap-iacs-parcel#LotSizeValue> ;
                                                                                                       rdfs:label "From 150001 to 500000"@en ;
                                                                                                       <http://www.w3.org/2004/02/skos/core#definition> """--Name--
-- Definition --
Lot size range from 150001 to 500000.

-- Description --
Range category according to ISO 2859-2:1985."""@en ;
                                                                                                       <http://www.w3.org/2004/02/skos/core#inScheme> :LotSizeValue .


###  http://lpis.ec.europa.eu/registry/applicationschema/cap-iacs-parcel/code#LotSizeValue/35001to150000
<http://lpis.ec.europa.eu/registry/applicationschema/cap-iacs-parcel/code#LotSizeValue/35001to150000> rdf:type owl:NamedIndividual ,
                                                                                                               <http://lpis.ec.europa.eu/registry/applicationschema/cap-iacs-parcel#LotSizeValue> ;
                                                                                                      rdfs:label "From 35001 to 150000"@en ;
                                                                                                      <http://www.w3.org/2004/02/skos/core#definition> """--Name--
-- Definition --
Lot size range from 35001 to 150000.

-- Description --
Range category according to ISO 2859-2:1985."""@en ;
                                                                                                      <http://www.w3.org/2004/02/skos/core#inScheme> :LotSizeValue .


###  http://lpis.ec.europa.eu/registry/applicationschema/cap-iacs-parcel/code#LotSizeValue/500000+
<http://lpis.ec.europa.eu/registry/applicationschema/cap-iacs-parcel/code#LotSizeValue/500000+> rdf:type owl:NamedIndividual ,
                                                                                                         <http://lpis.ec.europa.eu/registry/applicationschema/cap-iacs-parcel#LotSizeValue> ;
                                                                                                rdfs:label "More then 500000"@en ;
                                                                                                <http://www.w3.org/2004/02/skos/core#definition> """--Name--
-- Definition --
Lot size range from 500000 up.

-- Description --
Range category according to ISO 2859-2:1985."""@en ;
                                                                                                <http://www.w3.org/2004/02/skos/core#inScheme> :LotSizeValue .


###  http://lpis.ec.europa.eu/registry/applicationschema/cap-iacs-parcel/code#ProRataCategoryValue/grassland50
<http://lpis.ec.europa.eu/registry/applicationschema/cap-iacs-parcel/code#ProRataCategoryValue/grassland50> rdf:type owl:NamedIndividual ,
                                                                                                                     <http://lpis.ec.europa.eu/registry/applicationschema/cap-iacs-parcel#ProRataCategoryValue> ;
                                                                                                            rdfs:label "Grassland 50 percent"@en ;
                                                                                                            <http://www.w3.org/2004/02/skos/core#definition> """--Name--
Grassland 50 percent

-- Definition --
Grassland  with 50 percent eligibility.

-- Description --
NOTE. If the rate of eligibility drops below 50%, a careful analysis of the standard deviation of the class RC assessment is due. Below 50% eligibility grasslands should only be in the eligibility profile when the class is very specific and if the scattering of its ineligible features produces a low standard deviation of the RC. Indeed, a 10% standard deviation on 45% eligibility indicates that nearly a quarter of the agricultural land is deemed uncertain."""@en ;
                                                                                                            <http://www.w3.org/2004/02/skos/core#inScheme> :ProRataCategoryValue .


###  http://lpis.ec.europa.eu/registry/applicationschema/cap-iacs-parcel/code#ProRataCategoryValue/grassland90
<http://lpis.ec.europa.eu/registry/applicationschema/cap-iacs-parcel/code#ProRataCategoryValue/grassland90> rdf:type owl:NamedIndividual ,
                                                                                                                     <http://lpis.ec.europa.eu/registry/applicationschema/cap-iacs-parcel#ProRataCategoryValue> ;
                                                                                                            rdfs:label "Grassland 90 percent"@en ;
                                                                                                            <http://www.w3.org/2004/02/skos/core#definition> """--Name--
Grassland 90 percent 

-- Definition --
Grassland with 90 percent eligibility.

-- Description --
NOTE. If eligibility is above 90% then full eligibility applies (no pro rata)."""@en ;
                                                                                                            <http://www.w3.org/2004/02/skos/core#inScheme> :ProRataCategoryValue .


###  http://lpis.ec.europa.eu/registry/applicationschema/cap-iacs-parcel/code#SampleSizeValue/1250
<http://lpis.ec.europa.eu/registry/applicationschema/cap-iacs-parcel/code#SampleSizeValue/1250> rdf:type owl:NamedIndividual ,
                                                                                                         <http://lpis.ec.europa.eu/registry/applicationschema/cap-iacs-parcel#SampleSizeValue> ;
                                                                                                rdfs:label "1250"@en ;
                                                                                                <http://www.w3.org/2004/02/skos/core#definition> """--Name--
1250

-- Definition --
Sample size applicable for LPIS inspection, when the lot size is bigger than 500000.

-- Description --
Sample population corresponding to LQ=2,0 from ISO 2859-2:1985."""@en ;
                                                                                                <http://www.w3.org/2004/02/skos/core#inScheme> :SampleSizeValue .


###  http://lpis.ec.europa.eu/registry/applicationschema/cap-iacs-parcel/code#SampleSizeValue/200
<http://lpis.ec.europa.eu/registry/applicationschema/cap-iacs-parcel/code#SampleSizeValue/200> rdf:type owl:NamedIndividual ,
                                                                                                        <http://lpis.ec.europa.eu/registry/applicationschema/cap-iacs-parcel#SampleSizeValue> ;
                                                                                               rdfs:label "200"@en ;
                                                                                               <http://www.w3.org/2004/02/skos/core#definition> """--Name--
200

-- Definition --
Sample size value (population) applicable in LPISQA for parcel measurements.

-- Description --
Value selected on the basis of lot size and LQ=12,5 from ISO 2859-2:1985"""@en ;
                                                                                               <http://www.w3.org/2004/02/skos/core#inScheme> :SampleSizeValue .


###  http://lpis.ec.europa.eu/registry/applicationschema/cap-iacs-parcel/code#SampleSizeValue/500
<http://lpis.ec.europa.eu/registry/applicationschema/cap-iacs-parcel/code#SampleSizeValue/500> rdf:type owl:NamedIndividual ,
                                                                                                        <http://lpis.ec.europa.eu/registry/applicationschema/cap-iacs-parcel#SampleSizeValue> ;
                                                                                               rdfs:label "500"@en ;
                                                                                               <http://www.w3.org/2004/02/skos/core#definition> """--Name--
500

-- Definition --
Sample size applicable for LPIS inspection, when the lot size is smaller than or equal to 150000.

-- Description --
Sample population corresponding to LQ=2,0 from ISO 2859-2:1985."""@en ;
                                                                                               <http://www.w3.org/2004/02/skos/core#inScheme> :SampleSizeValue .


###  http://lpis.ec.europa.eu/registry/applicationschema/cap-iacs-parcel/code#SampleSizeValue/800
<http://lpis.ec.europa.eu/registry/applicationschema/cap-iacs-parcel/code#SampleSizeValue/800> rdf:type owl:NamedIndividual ,
                                                                                                        <http://lpis.ec.europa.eu/registry/applicationschema/cap-iacs-parcel#SampleSizeValue> ;
                                                                                               rdfs:label "800"@en ;
                                                                                               <http://www.w3.org/2004/02/skos/core#definition> """--Name--
800

-- Definition --
Sample size applicable for LPIS inspection, when the lot size is bigger than 150000, but is smaller than or equal to 500000.

-- Description --
Sample population corresponding to LQ=2,0 from ISO 2859-2:1985."""@en ;
                                                                                               <http://www.w3.org/2004/02/skos/core#inScheme> :SampleSizeValue .


###  http://lpis.ec.europa.eu/registry/applicationschema/cap-iacs-parcel/code#SkippingReasonTypeValue/cloudsOrHaze
<http://lpis.ec.europa.eu/registry/applicationschema/cap-iacs-parcel/code#SkippingReasonTypeValue/cloudsOrHaze> rdf:type owl:NamedIndividual ,
                                                                                                                         <http://lpis.ec.europa.eu/registry/applicationschema/cap-iacs-parcel#SkippingReasonTypeValue> ;
                                                                                                                rdfs:label "Clouds or haze"@en ;
                                                                                                                <http://www.w3.org/2004/02/skos/core#definition> """--Name--
Clouds or haze

-- Definition --
Insufficient image quality due to meteorological conditions.

-- Description --
Parcel partially or fully covered by clouds or haze.

NOTE 1: When an MS/Region opts for pure field observations and measurements, this reason is incompatible with the this method. Therefore this value should be deleted from the eligibility profile.

NOTE 2: In DTS 5.3 the  value was: parcelIsPartiallyOrFullyCoveredByCloudsOrHaze. The coresponding recommended coded value was T4.

NOTE 3: With the introduction of dedicated LPIS QA image acquisition, applicability should become rare."""@en ;
                                                                                                                <http://www.w3.org/2004/02/skos/core#inScheme> :SkippingReasonTypeValue .


###  http://lpis.ec.europa.eu/registry/applicationschema/cap-iacs-parcel/code#SkippingReasonTypeValue/errorInScope
<http://lpis.ec.europa.eu/registry/applicationschema/cap-iacs-parcel/code#SkippingReasonTypeValue/errorInScope> rdf:type owl:NamedIndividual ,
                                                                                                                         <http://lpis.ec.europa.eu/registry/applicationschema/cap-iacs-parcel#SkippingReasonTypeValue> ;
                                                                                                                rdfs:label "Extra parcel due to error in the scope"@en ;
                                                                                                                <http://www.w3.org/2004/02/skos/core#definition> """--Name--
Error in scope

-- Definition --
Systematic error in the scope of the population that has not been discovered at the moment of submitting the LPIS population for sampling.

-- Description --
The population submitted is complete, but it contains extra parcels that are not subject to inspection due to an erroneous query that can be easily reproduced/verified.

NOTE: In DTS 5.3 the value was erroneousScopingS1. The corresponding coded value was S1."""@en ;
                                                                                                                <http://www.w3.org/2004/02/skos/core#inScheme> :SkippingReasonTypeValue .


###  http://lpis.ec.europa.eu/registry/applicationschema/cap-iacs-parcel/code#SkippingReasonTypeValue/forceMajeure
<http://lpis.ec.europa.eu/registry/applicationschema/cap-iacs-parcel/code#SkippingReasonTypeValue/forceMajeure> rdf:type owl:NamedIndividual ,
                                                                                                                         <http://lpis.ec.europa.eu/registry/applicationschema/cap-iacs-parcel#SkippingReasonTypeValue> ;
                                                                                                                rdfs:label "Force Majeure"@en ;
                                                                                                                <http://www.w3.org/2004/02/skos/core#definition> """--Name--
Force majeure

-- Definition --
Failure to inspect the item of inspection due to force majeure circumstances observed on the item of inspection. 

-- Description --
EXAMPLES of force majeure: flood,  snow cover, fires, landslides, other natural hazards.

NOTE: In DTS 5.3 the  value was forceMajeureCircumstancesObservedOnLuiF1. The coresponding coded value was F1."""@en ;
                                                                                                                <http://www.w3.org/2004/02/skos/core#inScheme> :SkippingReasonTypeValue .


###  http://lpis.ec.europa.eu/registry/applicationschema/cap-iacs-parcel/code#SkippingReasonTypeValue/inspectedInAggregation
<http://lpis.ec.europa.eu/registry/applicationschema/cap-iacs-parcel/code#SkippingReasonTypeValue/inspectedInAggregation> rdf:type owl:NamedIndividual ,
                                                                                                                                   <http://lpis.ec.europa.eu/registry/applicationschema/cap-iacs-parcel#SkippingReasonTypeValue> ;
                                                                                                                          rdfs:label "Parcel already Inspected in aggregation"@en ;
                                                                                                                          <http://www.w3.org/2004/02/skos/core#definition> """--Name--
Inspected in aggregation

-- Definition --
Parcel already Inspected as part of an aggregation item.

-- Description --
If pre selected parcel has previously entered in to an aggregation then this parcel shall not be inspected again.

NOTE. This value is applicable if only the parcel aggregation method has been adapted."""@en ;
                                                                                                                          <http://www.w3.org/2004/02/skos/core#inScheme> :SkippingReasonTypeValue .


###  http://lpis.ec.europa.eu/registry/applicationschema/cap-iacs-parcel/code#SkippingReasonTypeValue/insufficientImageQuality
<http://lpis.ec.europa.eu/registry/applicationschema/cap-iacs-parcel/code#SkippingReasonTypeValue/insufficientImageQuality> rdf:type owl:NamedIndividual ,
                                                                                                                                     <http://lpis.ec.europa.eu/registry/applicationschema/cap-iacs-parcel#SkippingReasonTypeValue> ;
                                                                                                                            rdfs:label "Impossible interpretation"@en ;
                                                                                                                            <http://www.w3.org/2004/02/skos/core#definition> """--Name--
Insufficient image quality

-- Definition --
Insufficient image quality obstructing the process of inspection bz the method of CAPI.

-- Description --
Interpretation of the inspected item is not possible with the given orthoimagery.

NOTE 1: When an MS/Region opts for pure field observations and measurements, this reason is incompatible with the this method. Therefore this value should be deleted from the eligibility profile.

NOTE 2: In DTS 5.3 the value wasluiInterpretationImpossibleWithGivenOrthoimageC4. The corresponding coded value was C4."""@en ;
                                                                                                                            <http://www.w3.org/2004/02/skos/core#inScheme> :SkippingReasonTypeValue .


###  http://lpis.ec.europa.eu/registry/applicationschema/cap-iacs-parcel/code#SkippingReasonTypeValue/missingGeometry
<http://lpis.ec.europa.eu/registry/applicationschema/cap-iacs-parcel/code#SkippingReasonTypeValue/missingGeometry> rdf:type owl:NamedIndividual ,
                                                                                                                            <http://lpis.ec.europa.eu/registry/applicationschema/cap-iacs-parcel#SkippingReasonTypeValue> ;
                                                                                                                   rdfs:label "Parcel geometry missing"@en ;
                                                                                                                   <http://www.w3.org/2004/02/skos/core#definition> """--Name--
Missing geometry

-- Definition --
Incomplete vector dataset that obstructs the inspection process.

-- Description --
Geometric representation of the item under is not available.

NOTE: In DTS 5.3 the  value was: parcelGeometryIsNotAvailable. The coresponding
recommended coded value was T5."""@en ;
                                                                                                                   <http://www.w3.org/2004/02/skos/core#inScheme> :SkippingReasonTypeValue .


###  http://lpis.ec.europa.eu/registry/applicationschema/cap-iacs-parcel/code#SkippingReasonTypeValue/missingImageCoverage
<http://lpis.ec.europa.eu/registry/applicationschema/cap-iacs-parcel/code#SkippingReasonTypeValue/missingImageCoverage> rdf:type owl:NamedIndividual ,
                                                                                                                                 <http://lpis.ec.europa.eu/registry/applicationschema/cap-iacs-parcel#SkippingReasonTypeValue> ;
                                                                                                                        rdfs:label "Parcel not covered by image"@en ;
                                                                                                                        <http://www.w3.org/2004/02/skos/core#definition> """--Name--
Missing image coverage

-- Definition --
Incomplete othroimagery coverage.

-- Description --
Parcel is partially or full not covered by orhtoimagery.

NOTE 1: When an MS/Region opts for pure field observations and measurements, this reason is incompatible with the this method. Therefore this value should be deleted from the eligibility profile.

NOTE 2: In DTS 5.3 the  value was: parcelIsPartiallyOrFullyNotCoveredByImage. The coresponding recommended coded value was T2.

NOTE 3: With the introduction of dedicated LPIS QA image acquisition, applicability should become rare."""@en ;
                                                                                                                        <http://www.w3.org/2004/02/skos/core#inScheme> :SkippingReasonTypeValue .


###  http://lpis.ec.europa.eu/registry/applicationschema/cap-iacs-parcel/code#SkippingReasonTypeValue/notPersistentIdentifier
<http://lpis.ec.europa.eu/registry/applicationschema/cap-iacs-parcel/code#SkippingReasonTypeValue/notPersistentIdentifier> rdf:type owl:NamedIndividual ,
                                                                                                                                    <http://lpis.ec.europa.eu/registry/applicationschema/cap-iacs-parcel#SkippingReasonTypeValue> ;
                                                                                                                           rdfs:label "Not persistent referenceParcelId"@en ;
                                                                                                                           <http://www.w3.org/2004/02/skos/core#definition> """--Name--
Not persistent identifier

-- Definition --
Unambiguous  identification of the item of inspection is impossible due to the discrepancy between the position of the reference parcel feature type and the reality observed on the imagery or terrain.

-- Description --
This problem is caused by re-using identifiers due to the unclear life cycle rules  of the feature type corresponding to the item under inspection (e.g. reference parcel). Transaction  like merging, splitting, or incorporating new agricultural land in an existing RP.

NOTE 1: It is recommended to assign a new unique identifier whenever  a major transaction takes place.

NOTE 2: In DTS 5.3 the  value was: referenceParcelIdFoundNotPersistentInLpisA3. The coresponding recommended coded value was A3."""@en ;
                                                                                                                           <http://www.w3.org/2004/02/skos/core#inScheme> :SkippingReasonTypeValue .


###  http://lpis.ec.europa.eu/registry/applicationschema/cap-iacs-parcel/code#TechnicalReasonValue/incompatibleDesign
<http://lpis.ec.europa.eu/registry/applicationschema/cap-iacs-parcel/code#TechnicalReasonValue/incompatibleDesign> rdf:type owl:NamedIndividual ,
                                                                                                                            <http://lpis.ec.europa.eu/registry/applicationschema/cap-iacs-parcel#TechnicalReasonValue> ;
                                                                                                                   rdfs:label "Incompatible design"@en ;
                                                                                                                   <http://www.w3.org/2004/02/skos/core#definition> """--Name--
Incompatible design

-- Definition --
Incompatible design.

-- Description --
None of the other causes can be assigned. Item under inspection does not follow the conceptual schema of the national/regional eligibility profile and/or the methodology for delineation. An instance classified to a feature type does not follow the semantics of the type."""@en ;
                                                                                                                   <http://www.w3.org/2004/02/skos/core#inScheme> :TechnicalReasonValue .


###  http://lpis.ec.europa.eu/registry/applicationschema/cap-iacs-parcel/code#TechnicalReasonValue/incompleteProcessing
<http://lpis.ec.europa.eu/registry/applicationschema/cap-iacs-parcel/code#TechnicalReasonValue/incompleteProcessing> rdf:type owl:NamedIndividual ,
                                                                                                                              <http://lpis.ec.europa.eu/registry/applicationschema/cap-iacs-parcel#TechnicalReasonValue> ;
                                                                                                                     rdfs:label "Incomplete processing"@en ;
                                                                                                                     <http://www.w3.org/2004/02/skos/core#definition> """--Name--
Incomplete processing

-- Definition --
Errors due to omitted information.

-- Description --
The completeness of data is not full because of missing items (attributes, values, features). Some steps of the standard workflow have been not been foreseen (at system level), or have been omitted at item level. In  both cases this non-conformity is manifested at instance level."""@en ;
                                                                                                                     <http://www.w3.org/2004/02/skos/core#inScheme> :TechnicalReasonValue .


###  http://lpis.ec.europa.eu/registry/applicationschema/cap-iacs-parcel/code#TechnicalReasonValue/missedUpdate
<http://lpis.ec.europa.eu/registry/applicationschema/cap-iacs-parcel/code#TechnicalReasonValue/missedUpdate> rdf:type owl:NamedIndividual ,
                                                                                                                      <http://lpis.ec.europa.eu/registry/applicationschema/cap-iacs-parcel#TechnicalReasonValue> ;
                                                                                                             rdfs:label "Missed update"@en ;
                                                                                                             <http://www.w3.org/2004/02/skos/core#definition> """--Name--
Missed update

-- Definition --
Missed update.

-- Description --
Changes of the underlying land (real world objects) that  have not been applied in the data. Data do not reflect the current state of real world objects. Non-conformity manifests at instance level."""@en ;
                                                                                                             <http://www.w3.org/2004/02/skos/core#inScheme> :TechnicalReasonValue .


###  http://lpis.ec.europa.eu/registry/applicationschema/cap-iacs-parcel/code#TechnicalReasonValue/missedUpgrade
<http://lpis.ec.europa.eu/registry/applicationschema/cap-iacs-parcel/code#TechnicalReasonValue/missedUpgrade> rdf:type owl:NamedIndividual ,
                                                                                                                       <http://lpis.ec.europa.eu/registry/applicationschema/cap-iacs-parcel#TechnicalReasonValue> ;
                                                                                                              rdfs:label "Missed upgrade"@en ;
                                                                                                              <http://www.w3.org/2004/02/skos/core#definition> """--Name--
Missed upgrade

-- Definition --
Missed upgrade.

-- Description --
Changes in the legal acts have not been introduced in the data model. Presentation of data does not follow the prescribed requirements / conceptual model and /or the current national / regional eligibility profile. This brings systematic error in the dataset. Non-conformity manifests at the level of the feature / data types (all instances belonging to the type concerned)."""@en ;
                                                                                                              <http://www.w3.org/2004/02/skos/core#inScheme> :TechnicalReasonValue .


###  http://lpis.ec.europa.eu/registry/applicationschema/cap-iacs-parcel/code#TechnicalReasonValue/processingError
<http://lpis.ec.europa.eu/registry/applicationschema/cap-iacs-parcel/code#TechnicalReasonValue/processingError> rdf:type owl:NamedIndividual ,
                                                                                                                         <http://lpis.ec.europa.eu/registry/applicationschema/cap-iacs-parcel#TechnicalReasonValue> ;
                                                                                                                rdfs:label "Processing error"@en ;
                                                                                                                <http://www.w3.org/2004/02/skos/core#definition> """--Name--
Processing error

-- Definition --
Errors due to the incorrectly applied data processing methodology.

-- Description --
Deviations from the true values because of the deviations from the processing methodology."""@en ;
                                                                                                                <http://www.w3.org/2004/02/skos/core#inScheme> :TechnicalReasonValue .


###  http://lpis.ec.europa.eu/registry/applicationschema/cap-iacs-parcel/code#TestTypeMtsValue/attributeAndAssociationCompleteness
<http://lpis.ec.europa.eu/registry/applicationschema/cap-iacs-parcel/code#TestTypeMtsValue/attributeAndAssociationCompleteness> rdf:type owl:NamedIndividual ,
                                                                                                                                         <http://lpis.ec.europa.eu/registry/applicationschema/cap-iacs-parcel#TestTypeMtsValue> ;
                                                                                                                                rdfs:label "Attribute and association"@en ;
                                                                                                                                <http://www.w3.org/2004/02/skos/core#definition> """--Name--
Attribute and association completeness

--Definition --
Completeness of the eligibility profile  in terms of attributes and associations  as compared to the LCM. Eventual omissions trigger fail verdict in the corresponding tests.

-- Description --
All attributes and association roles defined in the LCM are mandatory.  When feature types of the eligibility profile include more attributes than defined in the LCM, this does not influence conformity. However, the definition of these attributes should not semantically clash with the definitions of those, already defined in the LCM. Omitted attributes/association rules found in course of testing triggers fail verdict in this test.

NOTE 1. From semantic and UML points of view attributes and associations are equivalent. Both describe the properties of the related class (feature type, or data type).

NOTE 2. Zero (0) multiplicity describes a natural state (semantic property) of the attribute/association. Therefore it should not be interpreted as indicator of optional implementation.

NOTE 3. Zero (0) multiplicity of abstract only concepts (no corresponding tangible entities in the real world) means that within a smaller their use is not required. EXAMPLE: identifiers  may not be required for specific uses.

NOTE 4. This is a capability test case."""@en ;
                                                                                                                                <http://www.w3.org/2004/02/skos/core#inScheme> :TestTypeMtsValue .


###  http://lpis.ec.europa.eu/registry/applicationschema/cap-iacs-parcel/code#TestTypeMtsValue/encoding
<http://lpis.ec.europa.eu/registry/applicationschema/cap-iacs-parcel/code#TestTypeMtsValue/encoding> rdf:type owl:NamedIndividual ,
                                                                                                              <http://lpis.ec.europa.eu/registry/applicationschema/cap-iacs-parcel#TestTypeMtsValue> ;
                                                                                                     rdfs:label "Encoding"@en ;
                                                                                                     <http://www.w3.org/2004/02/skos/core#definition> """--Name--
Encoding

--Definition --
Encoding applicable for data exchange within LPISQA.

-- Description --
The xml/gml schema should follow the standard specified by DG JRC. 

NOTE. This is a capability test case."""@en ;
                                                                                                     <http://www.w3.org/2004/02/skos/core#inScheme> :TestTypeMtsValue .


###  http://lpis.ec.europa.eu/registry/applicationschema/cap-iacs-parcel/code#TestTypeMtsValue/extendedCodeList
<http://lpis.ec.europa.eu/registry/applicationschema/cap-iacs-parcel/code#TestTypeMtsValue/extendedCodeList> rdf:type owl:NamedIndividual ,
                                                                                                                      <http://lpis.ec.europa.eu/registry/applicationschema/cap-iacs-parcel#TestTypeMtsValue> ;
                                                                                                             rdfs:label "Extended code list"@en ;
                                                                                                             <http://www.w3.org/2004/02/skos/core#definition> """--Name--
Extended code list

-- Definition --
Semantic analysis of the  extended elements of the code lists managed by the authorities of the MS /regions.  

--Description --
A semantic comparison of the extended code list values have to establish the relation between the extended values and the values included in the LCM. 
When \"narrower\" extensions are allowed the new values can restrict the semantic meaning of a value within the same code list of the LCM. The mapping between the original and extended value shall be provided.
When \"any\" extension is allowed that extended values must avoid semantic clashes with the values already defined in the LCM .

NOTE 1. When \"any\" extension is allowed, \"narrower\" code list elements can be introduced too.

NOTE 2. When notification about the extension to the Commission applies, consistency between the schema and the notification shall be preserved. 

NOTE 3. This is a capability test case."""@en ;
                                                                                                             <http://www.w3.org/2004/02/skos/core#inScheme> :TestTypeMtsValue .


###  http://lpis.ec.europa.eu/registry/applicationschema/cap-iacs-parcel/code#TestTypeMtsValue/featureTypeCompleteness
<http://lpis.ec.europa.eu/registry/applicationschema/cap-iacs-parcel/code#TestTypeMtsValue/featureTypeCompleteness> rdf:type owl:NamedIndividual ,
                                                                                                                             <http://lpis.ec.europa.eu/registry/applicationschema/cap-iacs-parcel#TestTypeMtsValue> ;
                                                                                                                    rdfs:label "Feature type completeness"@en ;
                                                                                                                    <http://www.w3.org/2004/02/skos/core#definition> """--Name--
Feature type completeness

--Definition --
Completeness of the eligibility profile  in terms of feature types as compared to the LCM.

-- Description --
All feature type included in the LCM shall be present in the eligibility profile. No one to one relationship  between the corresponding feature types is required. However, rules for schema mapping shall be unambiguous. 

NOTE 1. As best practice, EC services recommend the following solutions:
- one to one mapping between the feature types of the eligibility profile and the LCM
- A feature type in the eligibility profile is a specialisation of a feature type in the LCM.

NOTE 2. This is a capability test case."""@en ;
                                                                                                                    <http://www.w3.org/2004/02/skos/core#inScheme> :TestTypeMtsValue .


###  http://lpis.ec.europa.eu/registry/applicationschema/cap-iacs-parcel/code#TestTypeMtsValue/multiplicity
<http://lpis.ec.europa.eu/registry/applicationschema/cap-iacs-parcel/code#TestTypeMtsValue/multiplicity> rdf:type owl:NamedIndividual ,
                                                                                                                  <http://lpis.ec.europa.eu/registry/applicationschema/cap-iacs-parcel#TestTypeMtsValue> ;
                                                                                                         rdfs:label "Multiplicity"@en ;
                                                                                                         <http://www.w3.org/2004/02/skos/core#definition> """--Name--
Multiplicity

--Definition --
Number of currencies of a property (attribute or association).

-- Description --
Number of occurrences shall be exactly those that is specified in the LCM;
- 0: no value appears for the property 
- 1: only one value can be provided
-1..*: one or more value may be provided

NOTE 1. Multiplicities for attributes are indicated after the value type in [brackets]. If No brackets appear the specified multiplicity is 1.

NOTE 2. Multiplicity for association appears at the ends of the connectors representing the association role. Multiplicity rules shall be read in the direction of navigability (direction of \"arrows\").

NOTE 3. This is a capability test case."""@en ;
                                                                                                         <http://www.w3.org/2004/02/skos/core#inScheme> :TestTypeMtsValue .


###  http://lpis.ec.europa.eu/registry/applicationschema/cap-iacs-parcel/code#TestTypeMtsValue/schemaDefinition
<http://lpis.ec.europa.eu/registry/applicationschema/cap-iacs-parcel/code#TestTypeMtsValue/schemaDefinition> rdf:type owl:NamedIndividual ,
                                                                                                                      <http://lpis.ec.europa.eu/registry/applicationschema/cap-iacs-parcel#TestTypeMtsValue> ;
                                                                                                             rdfs:label "Schema definition"@en ;
                                                                                                             <http://www.w3.org/2004/02/skos/core#definition> """--Name--
Schema definition test

--Definition--
Completeness of the documentation of the eligibility profile.

--Description--
All implementation choices (differences of the eligibility profile as compared to the LCM) shall be thoroughly  documented. In particular, extended code lists, and constraints  shall be clearly documented and communicated to various actors (OTSC inspectors, auditors, EC services).

NOTE: This is a basic test case."""@en ;
                                                                                                             <http://www.w3.org/2004/02/skos/core#inScheme> :TestTypeMtsValue .


###  http://lpis.ec.europa.eu/registry/applicationschema/cap-iacs-parcel/code#TestTypeMtsValue/schemaMapping
<http://lpis.ec.europa.eu/registry/applicationschema/cap-iacs-parcel/code#TestTypeMtsValue/schemaMapping> rdf:type owl:NamedIndividual ,
                                                                                                                   <http://lpis.ec.europa.eu/registry/applicationschema/cap-iacs-parcel#TestTypeMtsValue> ;
                                                                                                          rdfs:label "Schema mapping"@en ;
                                                                                                          <http://www.w3.org/2004/02/skos/core#definition> """--Name--
Schema mapping

-- Definition --
Definition of mapping rules  from the national / regional eligibility profile to the LCM.

-- Description-- 
The mapping rules shall be defined for all elements (feature types, code lists, enumerations)  rendering the elements of the source schema (eligibility profile) with the corresponding elements of the LCM. 

Each feature type of the national / regional eligibility profile can be mapped to one or more feature types of the LCM. This mapping rule has to be unambiguous.

NOTE . This is a basic test case."""@en ;
                                                                                                          <http://www.w3.org/2004/02/skos/core#inScheme> :TestTypeMtsValue .


###  http://lpis.ec.europa.eu/registry/applicationschema/cap-iacs-parcel/code#TestTypeMtsValue/valueAndConstraint
<http://lpis.ec.europa.eu/registry/applicationschema/cap-iacs-parcel/code#TestTypeMtsValue/valueAndConstraint> rdf:type owl:NamedIndividual ,
                                                                                                                        <http://lpis.ec.europa.eu/registry/applicationschema/cap-iacs-parcel#TestTypeMtsValue> ;
                                                                                                               rdfs:label "Value and constraint"@en ;
                                                                                                               <http://www.w3.org/2004/02/skos/core#definition> """--Name--
Value and constraint

--Definition --
Range or restricted range of values that a property can take.

-- Description --
Constraints are set on value type, values, and association rules in the LCM. Some of them are conditional.

NOTE 1. Unit of measure test is a specific constraint set in order to verify whether area values are expressed in the units specified in the LCM.

NOTE 2. This is a capability test case."""@en ;
                                                                                                               <http://www.w3.org/2004/02/skos/core#inScheme> :TestTypeMtsValue .


###  http://lpis.ec.europa.eu/registry/applicationschema/cap-iacs-parcel/code#TestTypeMtsValue/valueType
<http://lpis.ec.europa.eu/registry/applicationschema/cap-iacs-parcel/code#TestTypeMtsValue/valueType> rdf:type owl:NamedIndividual ,
                                                                                                               <http://lpis.ec.europa.eu/registry/applicationschema/cap-iacs-parcel#TestTypeMtsValue> ;
                                                                                                      rdfs:label "Value type"@en ;
                                                                                                      <http://www.w3.org/2004/02/skos/core#definition> """--Name--
Value type

--Definition --
Type of the value that a specific attribute can take.

-- Description --
Value types can be specified using one of the following methods:
- selecting types of from the conceptual schema language and reference schemas (standards, INSPIRE)
- Data type specified in reference schemas or in the LCM
- Enumeration
- Code list

NOTE 1. for extensible code lists other values than specified in it can be introduced in the eligibility profile. The extended values shall not have semantic clashes with those values, specified in the LCM. When extension with \"narrower\" values is allowed, the an new value should be a semantic restriction of the parent value. For example \"permanent crop\" can be extended with \"citrus tree\".

NOTE 2. This is a capability test case."""@en ;
                                                                                                      <http://www.w3.org/2004/02/skos/core#inScheme> :TestTypeMtsValue .


###  Generated by the OWL API (version 5.1.18) https://github.com/owlcs/owlapi/
