<?xml version="1.0"?>
<rdf:RDF xmlns="http://lpis.ec.europa.eu/registry/applicationschema/cap-parcel-ext#"
     xml:base="http://lpis.ec.europa.eu/registry/applicationschema/cap-parcel-ext"
     xmlns:dc="http://purl.org/dc/elements/1.1/"
     xmlns:owl="http://www.w3.org/2002/07/owl#"
     xmlns:rdf="http://www.w3.org/1999/02/22-rdf-syntax-ns#"
     xmlns:xml="http://www.w3.org/XML/1998/namespace"
     xmlns:xsd="http://www.w3.org/2001/XMLSchema#"
     xmlns:foaf="http://xmlns.com/foaf/0.1/"
     xmlns:rdfs="http://www.w3.org/2000/01/rdf-schema#"
     xmlns:skos="http://www.w3.org/2004/02/skos/core#"
     xmlns:terms="http://purl.org/dc/terms/"
     xmlns:schema="http://schema.org/">
    <owl:Ontology rdf:about="http://lpis.ec.europa.eu/registry/applicationschema/cap-parcel-ext">
        <owl:versionIRI rdf:resource="http://lpis.ec.europa.eu/registry/applicationschema/cap-parcel-ext/1.0"/>
        <owl:imports rdf:resource="https://raw.githubusercontent.com/rapw3k/cap-iacs/main/cap-iacs-parcel.ttl"/>
        <terms:creator rdf:resource="_:genid-nodeid-node1gq1ujd74x3"/>
        <terms:creator rdf:nodeID="genid1"/>
        <terms:creator rdf:nodeID="genid3"/>
        <terms:description xml:lang="en">Extension of the identification system for agricultural parcels Ontology used in IACS that includes former Reference Parcel subtypes : CadParcel, AgrParcel, FarBlock, PhyBlock, TopoBlock and MixedParcelType</terms:description>
        <terms:rights xml:lang="en">This ontology is distributed under Creative Commons Attribution 4.0 License - http://creativecommons.org/licenses/by/4.0</terms:rights>
        <terms:source xml:lang="en">JRC IACS application schema. https://doi.org/10.1016/j.landusepol.2016.05.023</terms:source>
        <terms:title xml:lang="en">JRC IACS Extension - Extension of the identification System for Agricultural Parcels Ontology</terms:title>
        <owl:versionInfo>1.0</owl:versionInfo>
    </owl:Ontology>
    <rdf:Description rdf:nodeID="genid1">
        <schema:affiliation>
            <rdf:Description>
                <foaf:name>PSNC</foaf:name>
            </rdf:Description>
        </schema:affiliation>
        <rdfs:seeAlso rdf:resource="http://orcid.org/0000-0003-4289-4922"/>
        <foaf:name>Raul Palma</foaf:name>
    </rdf:Description>
    <rdf:Description rdf:nodeID="genid3">
        <schema:affiliation>
            <rdf:Description>
                <foaf:name>PSNC</foaf:name>
            </rdf:Description>
        </schema:affiliation>
        <foaf:name>Bogusz Janiak</foaf:name>
    </rdf:Description>
    


    <!-- 
    ///////////////////////////////////////////////////////////////////////////////////////
    //
    // Classes
    //
    ///////////////////////////////////////////////////////////////////////////////////////
     -->


    


    <!-- http://lpis.ec.europa.eu/registry/applicationschema/cap-iacs-aid#AgriculturalParcel -->


    <rdf:Description rdf:about="http://lpis.ec.europa.eu/registry/applicationschema/cap-iacs-aid#AgriculturalParcel">
        <rdfs:subClassOf rdf:resource="http://lpis.ec.europa.eu/registry/applicationschema/cap-iacs-parcel#ReferenceParcel"/>
    </rdf:Description>
    


    <!-- http://lpis.ec.europa.eu/registry/applicationschema/cap-iacs-parcel#CadParcel -->


    <owl:Class rdf:about="http://lpis.ec.europa.eu/registry/applicationschema/cap-iacs-parcel#CadParcel">
        <rdfs:subClassOf rdf:resource="http://lpis.ec.europa.eu/registry/applicationschema/cap-iacs-parcel#ReferenceParcel"/>
        <rdfs:label xml:lang="en">Cadastral parcel</rdfs:label>
        <skos:definition xml:lang="en">Reference Parcel subtype that is not anymore a core element of current IACS model. Main Features: i) one or more farmers; ii) based on ownership; iii) one or more crop groups</skos:definition>
    </owl:Class>
    


    <!-- http://lpis.ec.europa.eu/registry/applicationschema/cap-iacs-parcel#FarBlock -->


    <owl:Class rdf:about="http://lpis.ec.europa.eu/registry/applicationschema/cap-iacs-parcel#FarBlock">
        <rdfs:subClassOf rdf:resource="http://lpis.ec.europa.eu/registry/applicationschema/cap-iacs-parcel#ReferenceParcel"/>
        <rdfs:label xml:lang="en">Farmer&apos;s block</rdfs:label>
        <skos:definition xml:lang="en">Reference Parcel subtype that is not anymore a core element of current IACS model. Main Features: i) single farmer; ii) one or more crop groups; iii) no natural boundaries</skos:definition>
    </owl:Class>
    


    <!-- http://lpis.ec.europa.eu/registry/applicationschema/cap-iacs-parcel#MixedParcel -->


    <owl:Class rdf:about="http://lpis.ec.europa.eu/registry/applicationschema/cap-iacs-parcel#MixedParcel">
        <rdfs:subClassOf rdf:resource="http://lpis.ec.europa.eu/registry/applicationschema/cap-iacs-parcel#ReferenceParcel"/>
        <rdfs:label xml:lang="en">Mixed parcel</rdfs:label>
        <skos:definition xml:lang="en">Reference Parcel subtype that is not anymore a core element of current IACS model. Mixed parcel type</skos:definition>
    </owl:Class>
    


    <!-- http://lpis.ec.europa.eu/registry/applicationschema/cap-iacs-parcel#PhyBlock -->


    <owl:Class rdf:about="http://lpis.ec.europa.eu/registry/applicationschema/cap-iacs-parcel#PhyBlock">
        <owl:equivalentClass rdf:resource="http://lpis.ec.europa.eu/registry/applicationschema/cap-iacs-parcel#TopoBlock"/>
        <rdfs:subClassOf rdf:resource="http://lpis.ec.europa.eu/registry/applicationschema/cap-iacs-parcel#ReferenceParcel"/>
        <rdfs:label xml:lang="en">Physical block</rdfs:label>
        <skos:definition xml:lang="en">Reference Parcel subtype that is not anymore a core element of current IACS model. Main Features: i) one or more farmers; ii) area bordered by certain features; iii) one or more crop groups</skos:definition>
    </owl:Class>
    


    <!-- http://lpis.ec.europa.eu/registry/applicationschema/cap-iacs-parcel#TopoBlock -->


    <owl:Class rdf:about="http://lpis.ec.europa.eu/registry/applicationschema/cap-iacs-parcel#TopoBlock">
        <rdfs:subClassOf rdf:resource="http://lpis.ec.europa.eu/registry/applicationschema/cap-iacs-parcel#ReferenceParcel"/>
        <rdfs:label xml:lang="en">Topographical block</rdfs:label>
        <skos:definition xml:lang="en">Reference Parcel subtype that is not anymore a core element of current IACS model. Main Features: i) one or more farmers; ii) area bordered by certain features; iii) one or more crop groups</skos:definition>
    </owl:Class>
</rdf:RDF>



<!-- Generated by the OWL API (version 5.1.18) https://github.com/owlcs/owlapi/ -->


